<?xml version="1.0"?>
<rdf:RDF xmlns="https://www.sisostds.org/ontologies/C2SIM/cwix2025#"
     xml:base="https://www.sisostds.org/ontologies/C2SIM/cwix2025"
     xmlns:owl="http://www.w3.org/2002/07/owl#"
     xmlns:rdf="http://www.w3.org/1999/02/22-rdf-syntax-ns#"
     xmlns:xml="http://www.w3.org/XML/1998/namespace"
     xmlns:xsd="http://www.w3.org/2001/XMLSchema#"
     xmlns:rdfs="http://www.w3.org/2000/01/rdf-schema#">
    <owl:Ontology rdf:about="https://www.sisostds.org/ontologies/C2SIM/cwix2025">
        <rdfs:comment>CWIX 2025 built on CWIX 2024 branch, based on version 1.0.1 SISO Standard, April 2022.</rdfs:comment>
        <rdfs:comment>Version 1.0.0 SISO Standard, May 2020</rdfs:comment>
        <owl:versionInfo>C2SIM Core Ontology version CWIX2025</owl:versionInfo>
        <owl:versionInfo>C2SIM Land Operations Extension v1.0.0</owl:versionInfo>
        <owl:versionInfo>C2SIM Standard Military Extension vCWIX-2024</owl:versionInfo>
    </owl:Ontology>
    


    <!-- 
    ///////////////////////////////////////////////////////////////////////////////////////
    //
    // Annotation properties
    //
    ///////////////////////////////////////////////////////////////////////////////////////
     -->

    


    <!-- http://www.w3.org/2002/07/owl#maxQualifiedCardinality -->

    <owl:AnnotationProperty rdf:about="http://www.w3.org/2002/07/owl#maxQualifiedCardinality"/>
    


    <!-- http://www.w3.org/2002/07/owl#minQualifiedCardinality -->

    <owl:AnnotationProperty rdf:about="http://www.w3.org/2002/07/owl#minQualifiedCardinality"/>
    


    <!-- http://www.w3.org/2002/07/owl#qualifiedCardinality -->

    <owl:AnnotationProperty rdf:about="http://www.w3.org/2002/07/owl#qualifiedCardinality"/>
    


    <!-- 
    ///////////////////////////////////////////////////////////////////////////////////////
    //
    // Datatypes
    //
    ///////////////////////////////////////////////////////////////////////////////////////
     -->

    


    <!-- http://www.sisostds.org/ontologies/C2SIM#IsoDateTimeBase -->

    <rdfs:Datatype rdf:about="http://www.sisostds.org/ontologies/C2SIM#IsoDateTimeBase">
        <owl:equivalentClass>
            <rdfs:Datatype>
                <owl:onDatatype rdf:resource="http://www.w3.org/2001/XMLSchema#string"/>
                <owl:withRestrictions rdf:parseType="Collection">
                    <rdf:Description>
                        <xsd:pattern>[0-9]{4}-[0-9]{2}-[0-9]{2}[T]{1}[0-9]{2}:[0-9]{2}:[0-9]{2}[Z]{1}</xsd:pattern>
                    </rdf:Description>
                </owl:withRestrictions>
            </rdfs:Datatype>
        </owl:equivalentClass>
    </rdfs:Datatype>
    


    <!-- http://www.sisostds.org/ontologies/C2SIM#IsoTimeDurationBase -->

    <rdfs:Datatype rdf:about="http://www.sisostds.org/ontologies/C2SIM#IsoTimeDurationBase">
        <rdfs:comment>Time duration in ISO format.</rdfs:comment>
        <owl:equivalentClass>
            <rdfs:Datatype>
                <owl:onDatatype rdf:resource="http://www.w3.org/2001/XMLSchema#string"/>
                <owl:withRestrictions rdf:parseType="Collection">
                    <rdf:Description>
                        <xsd:pattern>[P]{1}[0-9]{2}[Y]{1}[0-9]{2}[M]{1}[0-9]{2}[D]{1}T{1}[0-9]{2}[H]{1}[0-9]{2}[M]{1}[0-9]{2}[S]{1}</xsd:pattern>
                    </rdf:Description>
                </owl:withRestrictions>
            </rdfs:Datatype>
        </owl:equivalentClass>
    </rdfs:Datatype>
    


    <!-- http://www.sisostds.org/ontologies/C2SIM#UUIDBase -->

    <rdfs:Datatype rdf:about="http://www.sisostds.org/ontologies/C2SIM#UUIDBase">
        <owl:equivalentClass>
            <rdfs:Datatype>
                <owl:onDatatype rdf:resource="http://www.w3.org/2001/XMLSchema#string"/>
                <owl:withRestrictions rdf:parseType="Collection">
                    <rdf:Description>
                        <xsd:pattern>[0-9a-fA-F]{8}\-[0-9a-fA-F]{4}\-[0-9a-fA-F]{4}\-[0-9a-fA-F]{4}\-[0-9a-fA-F]{12}</xsd:pattern>
                    </rdf:Description>
                </owl:withRestrictions>
            </rdfs:Datatype>
        </owl:equivalentClass>
    </rdfs:Datatype>
    


    <!-- http://www.sisostds.org/ontologies/C2SIM#angle -->

    <rdfs:Datatype rdf:about="http://www.sisostds.org/ontologies/C2SIM#angle">
        <owl:equivalentClass>
            <rdfs:Datatype>
                <owl:onDatatype rdf:resource="http://www.w3.org/2001/XMLSchema#double"/>
                <owl:withRestrictions rdf:parseType="Collection">
                    <rdf:Description>
                        <xsd:minInclusive rdf:datatype="http://www.w3.org/2001/XMLSchema#double">-3.1415926</xsd:minInclusive>
                    </rdf:Description>
                    <rdf:Description>
                        <xsd:maxInclusive rdf:datatype="http://www.w3.org/2001/XMLSchema#double">3.1415926</xsd:maxInclusive>
                    </rdf:Description>
                </owl:withRestrictions>
            </rdfs:Datatype>
        </owl:equivalentClass>
    </rdfs:Datatype>
    


    <!-- http://www.sisostds.org/ontologies/C2SIM#entityTypeString -->

    <rdfs:Datatype rdf:about="http://www.sisostds.org/ontologies/C2SIM#entityTypeString">
        <rdfs:comment>A string, possibly with several separated fields that can each hold an enumeration, thus identifying a category at each level of a hierarchy.</rdfs:comment>
    </rdfs:Datatype>
    


    <!-- http://www.sisostds.org/ontologies/C2SIM#latitude -->

    <rdfs:Datatype rdf:about="http://www.sisostds.org/ontologies/C2SIM#latitude">
        <owl:equivalentClass>
            <rdfs:Datatype>
                <owl:onDatatype rdf:resource="http://www.w3.org/2001/XMLSchema#double"/>
                <owl:withRestrictions rdf:parseType="Collection">
                    <rdf:Description>
                        <xsd:minInclusive rdf:datatype="http://www.w3.org/2001/XMLSchema#double">-90.0</xsd:minInclusive>
                    </rdf:Description>
                    <rdf:Description>
                        <xsd:maxInclusive rdf:datatype="http://www.w3.org/2001/XMLSchema#double">90.0</xsd:maxInclusive>
                    </rdf:Description>
                </owl:withRestrictions>
            </rdfs:Datatype>
        </owl:equivalentClass>
    </rdfs:Datatype>
    


    <!-- http://www.sisostds.org/ontologies/C2SIM#longitude -->

    <rdfs:Datatype rdf:about="http://www.sisostds.org/ontologies/C2SIM#longitude">
        <owl:equivalentClass>
            <rdfs:Datatype>
                <owl:onDatatype rdf:resource="http://www.w3.org/2001/XMLSchema#double"/>
                <owl:withRestrictions rdf:parseType="Collection">
                    <rdf:Description>
                        <xsd:minInclusive rdf:datatype="http://www.w3.org/2001/XMLSchema#double">-180.0</xsd:minInclusive>
                    </rdf:Description>
                    <rdf:Description>
                        <xsd:maxInclusive rdf:datatype="http://www.w3.org/2001/XMLSchema#double">180.0</xsd:maxInclusive>
                    </rdf:Description>
                </owl:withRestrictions>
            </rdfs:Datatype>
        </owl:equivalentClass>
    </rdfs:Datatype>
    


    <!-- http://www.sisostds.org/ontologies/C2SIM#percentage -->

    <rdfs:Datatype rdf:about="http://www.sisostds.org/ontologies/C2SIM#percentage">
        <owl:equivalentClass>
            <rdfs:Datatype>
                <owl:onDatatype rdf:resource="http://www.w3.org/2001/XMLSchema#nonNegativeInteger"/>
                <owl:withRestrictions rdf:parseType="Collection">
                    <rdf:Description>
                        <xsd:maxInclusive rdf:datatype="http://www.w3.org/2001/XMLSchema#nonNegativeInteger">100</xsd:maxInclusive>
                    </rdf:Description>
                </owl:withRestrictions>
            </rdfs:Datatype>
        </owl:equivalentClass>
    </rdfs:Datatype>
    


    <!-- http://www.sisostds.org/ontologies/C2SIM#playbackRealtimeMultiple -->

    <rdfs:Datatype rdf:about="http://www.sisostds.org/ontologies/C2SIM#playbackRealtimeMultiple">
        <rdfs:comment>playbackRealtimeMultiple is a datatype for setting the simulation time to realtime multiplier for the rate of playing back recorded messages in a C2SIM coalition of systems. It is defined as a positive decimal type. For example, a value of 2.5 indicates playback of recorded messages at 2.5 times faster than realtime. A value of 0.5 indicates playback of recorded messages at half the realtime clock, or running half the speed of realtime.</rdfs:comment>
        <owl:equivalentClass>
            <rdfs:Datatype>
                <owl:onDatatype rdf:resource="http://www.w3.org/2001/XMLSchema#decimal"/>
                <owl:withRestrictions rdf:parseType="Collection">
                    <rdf:Description>
                        <xsd:minExclusive rdf:datatype="http://www.w3.org/2001/XMLSchema#decimal">0.0</xsd:minExclusive>
                    </rdf:Description>
                </owl:withRestrictions>
            </rdfs:Datatype>
        </owl:equivalentClass>
    </rdfs:Datatype>
    


    <!-- http://www.sisostds.org/ontologies/C2SIM#simulationRealtimeMultiple -->

    <rdfs:Datatype rdf:about="http://www.sisostds.org/ontologies/C2SIM#simulationRealtimeMultiple">
        <rdfs:comment>simulationRealtimeMultiple is a datatype for setting the simulation time to realtime multiplier. It is defined as a positive decimal type. For example, a value of 2.5 indicates a simulation is advancing the simulation time 2.5 times faster than realtime. A value of 0.5 indicates a simulation is advancing the simulation time at half the realtime clock, or running half the speed of realtime. For example, a slower rate is sometimes used to slow down a simulation to allow more time for human operator interaction.</rdfs:comment>
        <owl:equivalentClass>
            <rdfs:Datatype>
                <owl:onDatatype rdf:resource="http://www.w3.org/2001/XMLSchema#decimal"/>
                <owl:withRestrictions rdf:parseType="Collection">
                    <rdf:Description>
                        <xsd:minExclusive rdf:datatype="http://www.w3.org/2001/XMLSchema#decimal">0.0</xsd:minExclusive>
                    </rdf:Description>
                </owl:withRestrictions>
            </rdfs:Datatype>
        </owl:equivalentClass>
    </rdfs:Datatype>
    


    <!-- http://www.sisostds.org/ontologies/smx#SymbolIDCodeString -->

    <rdfs:Datatype rdf:about="http://www.sisostds.org/ontologies/smx#SymbolIDCodeString">
        <owl:equivalentClass>
            <rdfs:Datatype>
                <owl:onDatatype rdf:resource="http://www.w3.org/2001/XMLSchema#string"/>
                <owl:withRestrictions rdf:parseType="Collection">
                    <rdf:Description>
                        <xsd:pattern>[SGIWMO]{1}[PUAFNSHJKO\-]{1}[PAGMOSTUFVXLIZ\-]{1}[AP\-]{1}[A-Z\-]{6}[A-Z\-\*]{2}[\-]{2}[AECGNSX\-\*]{1}</xsd:pattern>
                    </rdf:Description>
                </owl:withRestrictions>
            </rdfs:Datatype>
        </owl:equivalentClass>
    </rdfs:Datatype>
    <owl:Axiom>
        <owl:annotatedSource rdf:resource="http://www.sisostds.org/ontologies/smx#SymbolIDCodeString"/>
        <owl:annotatedProperty rdf:resource="http://www.w3.org/2002/07/owl#equivalentClass"/>
        <owl:annotatedTarget>
            <rdfs:Datatype>
                <owl:onDatatype rdf:resource="http://www.w3.org/2001/XMLSchema#string"/>
                <owl:withRestrictions rdf:parseType="Collection">
                    <rdf:Description>
                        <xsd:pattern>[SGIWMO]{1}[PUAFNSHJKO\-]{1}[PAGMOSTUFVXLIZ\-]{1}[AP\-]{1}[A-Z\-]{6}[A-Z\-\*]{2}[\-]{2}[AECGNSX\-\*]{1}</xsd:pattern>
                    </rdf:Description>
                </owl:withRestrictions>
            </rdfs:Datatype>
        </owl:annotatedTarget>
        <rdfs:comment>This pattern permits the full range of symbols for units, including their affiliation (position 2), status (position 4) and country (positions 13-14), even though this information is either a dynamic attribute and not part of the basic type of an entity (e.g., position 2) or redundant with information specified elsewhere in the ontology (positions 13-14). C2SIM systems should ignore characters in these fields.</rdfs:comment>
    </owl:Axiom>
    


    <!-- 
    ///////////////////////////////////////////////////////////////////////////////////////
    //
    // Object Properties
    //
    ///////////////////////////////////////////////////////////////////////////////////////
     -->

    


    <!-- http://www.sisostds.org/ontologies/C2SIM#hasAbstractObject -->

    <owl:ObjectProperty rdf:about="http://www.sisostds.org/ontologies/C2SIM#hasAbstractObject">
        <rdfs:range rdf:resource="http://www.sisostds.org/ontologies/C2SIM#AbstractObject"/>
        <rdfs:comment>Reference to an AbstractObject class</rdfs:comment>
    </owl:ObjectProperty>
    


    <!-- http://www.sisostds.org/ontologies/C2SIM#hasAcknowledgeTypeCode -->

    <owl:ObjectProperty rdf:about="http://www.sisostds.org/ontologies/C2SIM#hasAcknowledgeTypeCode">
        <rdfs:subPropertyOf rdf:resource="http://www.sisostds.org/ontologies/C2SIM#hasCode"/>
        <rdfs:range rdf:resource="http://www.sisostds.org/ontologies/C2SIM#AcknowledgeTypeCode"/>
    </owl:ObjectProperty>
    


    <!-- http://www.sisostds.org/ontologies/C2SIM#hasAction -->

    <owl:ObjectProperty rdf:about="http://www.sisostds.org/ontologies/C2SIM#hasAction">
        <rdfs:range rdf:resource="http://www.sisostds.org/ontologies/C2SIM#Action"/>
        <rdfs:comment>A reference to an Action (an Event or Task).</rdfs:comment>
    </owl:ObjectProperty>
    


    <!-- http://www.sisostds.org/ontologies/C2SIM#hasActionCode -->

    <owl:ObjectProperty rdf:about="http://www.sisostds.org/ontologies/C2SIM#hasActionCode">
        <rdfs:subPropertyOf rdf:resource="http://www.sisostds.org/ontologies/C2SIM#hasCode"/>
        <rdfs:range rdf:resource="http://www.sisostds.org/ontologies/C2SIM#ActionCode"/>
    </owl:ObjectProperty>
    


    <!-- http://www.sisostds.org/ontologies/C2SIM#hasActionTemporalAssociationCode -->

    <owl:ObjectProperty rdf:about="http://www.sisostds.org/ontologies/C2SIM#hasActionTemporalAssociationCode">
        <rdfs:subPropertyOf rdf:resource="http://www.sisostds.org/ontologies/C2SIM#hasCode"/>
        <rdfs:range rdf:resource="http://www.sisostds.org/ontologies/C2SIM#ActionTemporalAssociationCode"/>
        <rdfs:comment>An enumerated list of specific temporal relationships, i.e. between two actions.</rdfs:comment>
    </owl:ObjectProperty>
    


    <!-- http://www.sisostds.org/ontologies/C2SIM#hasActionTemporalRelationship -->

    <owl:ObjectProperty rdf:about="http://www.sisostds.org/ontologies/C2SIM#hasActionTemporalRelationship">
        <rdfs:range rdf:resource="http://www.sisostds.org/ontologies/C2SIM#ActionTemporalRelationship"/>
        <rdfs:comment>A property of an Action (the subject) that is a temporal property, relating to another action (the object).</rdfs:comment>
    </owl:ObjectProperty>
    


    <!-- http://www.sisostds.org/ontologies/C2SIM#hasAllegianceRelationship -->

    <owl:ObjectProperty rdf:about="http://www.sisostds.org/ontologies/C2SIM#hasAllegianceRelationship">
        <rdfs:range rdf:resource="http://www.sisostds.org/ontologies/C2SIM#AllegianceRelationship"/>
        <rdfs:comment>Reference to a class showing allegiance relationship (friendly, hostile, neutral, or unknown) of an actor toward another actor.</rdfs:comment>
    </owl:ObjectProperty>
    


    <!-- http://www.sisostds.org/ontologies/C2SIM#hasAllegianceRelationshipCode -->

    <owl:ObjectProperty rdf:about="http://www.sisostds.org/ontologies/C2SIM#hasAllegianceRelationshipCode">
        <rdfs:subPropertyOf rdf:resource="http://www.sisostds.org/ontologies/C2SIM#hasCode"/>
        <rdfs:range rdf:resource="http://www.sisostds.org/ontologies/C2SIM#AllegianceRelationshipCode"/>
    </owl:ObjectProperty>
    


    <!-- http://www.sisostds.org/ontologies/C2SIM#hasAuthorizationHeader -->

    <owl:ObjectProperty rdf:about="http://www.sisostds.org/ontologies/C2SIM#hasAuthorizationHeader">
        <rdfs:subPropertyOf rdf:resource="http://www.w3.org/2002/07/owl#topObjectProperty"/>
        <rdfs:range rdf:resource="http://www.sisostds.org/ontologies/C2SIM#AuthorizationHeader"/>
        <rdfs:comment>The authentication header of a C2SIM header.</rdfs:comment>
    </owl:ObjectProperty>
    


    <!-- http://www.sisostds.org/ontologies/C2SIM#hasC2SIMHeader -->

    <owl:ObjectProperty rdf:about="http://www.sisostds.org/ontologies/C2SIM#hasC2SIMHeader">
        <rdfs:range rdf:resource="http://www.sisostds.org/ontologies/C2SIM#C2SIMHeader"/>
        <rdfs:comment>Reference to the C2SIM header class for a Message.</rdfs:comment>
    </owl:ObjectProperty>
    


    <!-- http://www.sisostds.org/ontologies/C2SIM#hasCode -->

    <owl:ObjectProperty rdf:about="http://www.sisostds.org/ontologies/C2SIM#hasCode">
        <rdfs:range rdf:resource="http://www.sisostds.org/ontologies/C2SIM#Code"/>
        <rdfs:comment>Provides value of some Code associated with a class.</rdfs:comment>
    </owl:ObjectProperty>
    


    <!-- http://www.sisostds.org/ontologies/C2SIM#hasCommunicativeActTypeCode -->

    <owl:ObjectProperty rdf:about="http://www.sisostds.org/ontologies/C2SIM#hasCommunicativeActTypeCode">
        <rdfs:subPropertyOf rdf:resource="http://www.sisostds.org/ontologies/C2SIM#hasCode"/>
        <rdfs:range rdf:resource="http://www.sisostds.org/ontologies/C2SIM#CommunicativeActTypeCode"/>
    </owl:ObjectProperty>
    


    <!-- http://www.sisostds.org/ontologies/C2SIM#hasCountryCode -->

    <owl:ObjectProperty rdf:about="http://www.sisostds.org/ontologies/C2SIM#hasCountryCode">
        <rdfs:subPropertyOf rdf:resource="http://www.sisostds.org/ontologies/C2SIM#hasOrganizationCode"/>
        <rdfs:range rdf:resource="http://www.sisostds.org/ontologies/C2SIM#CountryCode"/>
    </owl:ObjectProperty>
    


    <!-- http://www.sisostds.org/ontologies/C2SIM#hasCurrentState -->

    <owl:ObjectProperty rdf:about="http://www.sisostds.org/ontologies/C2SIM#hasCurrentState">
        <rdfs:subPropertyOf rdf:resource="http://www.sisostds.org/ontologies/C2SIM#hasEntityState"/>
        <rdfs:range rdf:resource="http://www.sisostds.org/ontologies/C2SIM#EntityState"/>
        <rdfs:comment>Provides value for the current state of an Entity.</rdfs:comment>
    </owl:ObjectProperty>
    


    <!-- http://www.sisostds.org/ontologies/C2SIM#hasDateTime -->

    <owl:ObjectProperty rdf:about="http://www.sisostds.org/ontologies/C2SIM#hasDateTime">
        <rdfs:subPropertyOf rdf:resource="http://www.sisostds.org/ontologies/C2SIM#hasTimeInstant"/>
        <rdfs:range rdf:resource="http://www.sisostds.org/ontologies/C2SIM#DateTime"/>
        <rdfs:comment>Provides a value for a Time Instant in ISO DateTime format</rdfs:comment>
    </owl:ObjectProperty>
    


    <!-- http://www.sisostds.org/ontologies/C2SIM#hasDelayTimeAmount -->

    <owl:ObjectProperty rdf:about="http://www.sisostds.org/ontologies/C2SIM#hasDelayTimeAmount">
        <rdfs:subPropertyOf rdf:resource="http://www.sisostds.org/ontologies/C2SIM#hasTemporalConcept"/>
        <rdfs:range rdf:resource="http://www.sisostds.org/ontologies/C2SIM#Duration"/>
        <rdfs:comment>Provides a value in ISO format for a time delay from some other referenced value</rdfs:comment>
    </owl:ObjectProperty>
    


    <!-- http://www.sisostds.org/ontologies/C2SIM#hasDesiredEffectCode -->

    <owl:ObjectProperty rdf:about="http://www.sisostds.org/ontologies/C2SIM#hasDesiredEffectCode">
        <rdfs:subPropertyOf rdf:resource="http://www.sisostds.org/ontologies/C2SIM#hasCode"/>
        <rdfs:range rdf:resource="http://www.sisostds.org/ontologies/C2SIM#DesiredEffectCode"/>
    </owl:ObjectProperty>
    


    <!-- http://www.sisostds.org/ontologies/C2SIM#hasDirectionOfMovement -->

    <owl:ObjectProperty rdf:about="http://www.sisostds.org/ontologies/C2SIM#hasDirectionOfMovement">
        <rdfs:range rdf:resource="http://www.sisostds.org/ontologies/C2SIM#Orientation"/>
        <rdfs:comment>Provides value for the geospatial direction in which an Entity is moving.</rdfs:comment>
    </owl:ObjectProperty>
    


    <!-- http://www.sisostds.org/ontologies/C2SIM#hasDuration -->

    <owl:ObjectProperty rdf:about="http://www.sisostds.org/ontologies/C2SIM#hasDuration">
        <rdfs:subPropertyOf rdf:resource="http://www.sisostds.org/ontologies/C2SIM#hasTemporalConcept"/>
        <rdfs:range rdf:resource="http://www.sisostds.org/ontologies/C2SIM#Duration"/>
        <rdfs:comment>Provides a value in ISO format for the duration of an Activity/task.</rdfs:comment>
    </owl:ObjectProperty>
    


    <!-- http://www.sisostds.org/ontologies/C2SIM#hasEndTime -->

    <owl:ObjectProperty rdf:about="http://www.sisostds.org/ontologies/C2SIM#hasEndTime">
        <rdfs:subPropertyOf rdf:resource="http://www.sisostds.org/ontologies/C2SIM#hasTimeInstant"/>
        <rdfs:range rdf:resource="http://www.sisostds.org/ontologies/C2SIM#TimeInstant"/>
        <rdfs:comment>The ending  Time Instant of any concept that exists over an interval of time. For example, the period of effectiveness of an Action/Task (C-BML)</rdfs:comment>
    </owl:ObjectProperty>
    


    <!-- http://www.sisostds.org/ontologies/C2SIM#hasEntity -->

    <owl:ObjectProperty rdf:about="http://www.sisostds.org/ontologies/C2SIM#hasEntity">
        <rdfs:range rdf:resource="http://www.sisostds.org/ontologies/C2SIM#Entity"/>
        <rdfs:comment>A generic relation to an instance of an Entity.</rdfs:comment>
    </owl:ObjectProperty>
    


    <!-- http://www.sisostds.org/ontologies/C2SIM#hasEntityDescriptor -->

    <owl:ObjectProperty rdf:about="http://www.sisostds.org/ontologies/C2SIM#hasEntityDescriptor">
        <rdfs:range rdf:resource="http://www.sisostds.org/ontologies/C2SIM#EntityDescriptor"/>
        <rdfs:comment>A generic relation to a descriptor for an Entity.</rdfs:comment>
    </owl:ObjectProperty>
    


    <!-- http://www.sisostds.org/ontologies/C2SIM#hasEntityHealthStatus -->

    <owl:ObjectProperty rdf:about="http://www.sisostds.org/ontologies/C2SIM#hasEntityHealthStatus">
        <rdfs:range rdf:resource="http://www.sisostds.org/ontologies/C2SIM#EntityHealthStatus"/>
        <rdfs:comment>Provide a HealthStatus value for an Entity.</rdfs:comment>
    </owl:ObjectProperty>
    


    <!-- http://www.sisostds.org/ontologies/C2SIM#hasEntityState -->

    <owl:ObjectProperty rdf:about="http://www.sisostds.org/ontologies/C2SIM#hasEntityState">
        <rdfs:range rdf:resource="http://www.sisostds.org/ontologies/C2SIM#EntityState"/>
        <rdfs:comment>Provides a reference to a class containing a value for the state of an Entity.</rdfs:comment>
    </owl:ObjectProperty>
    


    <!-- http://www.sisostds.org/ontologies/C2SIM#hasEthnicGroupCode -->

    <owl:ObjectProperty rdf:about="http://www.sisostds.org/ontologies/C2SIM#hasEthnicGroupCode">
        <rdfs:subPropertyOf rdf:resource="http://www.sisostds.org/ontologies/C2SIM#hasOrganizationCode"/>
        <rdfs:range rdf:resource="http://www.sisostds.org/ontologies/C2SIM#EthnicGroupCode"/>
    </owl:ObjectProperty>
    


    <!-- http://www.sisostds.org/ontologies/C2SIM#hasEventCode -->

    <owl:ObjectProperty rdf:about="http://www.sisostds.org/ontologies/C2SIM#hasEventCode">
        <rdfs:subPropertyOf rdf:resource="http://www.sisostds.org/ontologies/C2SIM#hasActionCode"/>
        <rdfs:range rdf:resource="http://www.sisostds.org/ontologies/C2SIM#EventCode"/>
    </owl:ObjectProperty>
    


    <!-- http://www.sisostds.org/ontologies/C2SIM#hasInitializationDataFile -->

    <owl:ObjectProperty rdf:about="http://www.sisostds.org/ontologies/C2SIM#hasInitializationDataFile">
        <rdfs:range rdf:resource="http://www.sisostds.org/ontologies/C2SIM#InitializationDataFile"/>
        <rdfs:comment>Provides an identifier for a file containing initialization data.</rdfs:comment>
    </owl:ObjectProperty>
    


    <!-- http://www.sisostds.org/ontologies/C2SIM#hasIssuedTime -->

    <owl:ObjectProperty rdf:about="http://www.sisostds.org/ontologies/C2SIM#hasIssuedTime">
        <rdfs:subPropertyOf rdf:resource="http://www.sisostds.org/ontologies/C2SIM#hasDateTime"/>
        <rdfs:range rdf:resource="http://www.sisostds.org/ontologies/C2SIM#DateTime"/>
        <rdfs:comment>Provides a value in ISO Date Time format for the time when an Order was issued.</rdfs:comment>
    </owl:ObjectProperty>
    


    <!-- http://www.sisostds.org/ontologies/C2SIM#hasLocation -->

    <owl:ObjectProperty rdf:about="http://www.sisostds.org/ontologies/C2SIM#hasLocation">
        <rdfs:range rdf:resource="http://www.sisostds.org/ontologies/C2SIM#Location"/>
        <rdfs:comment>Provides a geospatial Location for an Object.</rdfs:comment>
    </owl:ObjectProperty>
    


    <!-- http://www.sisostds.org/ontologies/C2SIM#hasMessageBody -->

    <owl:ObjectProperty rdf:about="http://www.sisostds.org/ontologies/C2SIM#hasMessageBody">
        <rdfs:range rdf:resource="http://www.sisostds.org/ontologies/C2SIM#MessageBody"/>
        <rdfs:comment>Reference to a Body class for a Message.</rdfs:comment>
    </owl:ObjectProperty>
    


    <!-- http://www.sisostds.org/ontologies/C2SIM#hasNamedEntityType -->

    <owl:ObjectProperty rdf:about="http://www.sisostds.org/ontologies/C2SIM#hasNamedEntityType">
        <rdfs:range rdf:resource="http://www.sisostds.org/ontologies/C2SIM#NamedEntityType"/>
        <rdfs:comment>Property to specify additional (and more specific) information about the type of an entity.</rdfs:comment>
    </owl:ObjectProperty>
    


    <!-- http://www.sisostds.org/ontologies/C2SIM#hasObjectDefinitions -->

    <owl:ObjectProperty rdf:about="http://www.sisostds.org/ontologies/C2SIM#hasObjectDefinitions">
        <rdfs:range rdf:resource="http://www.sisostds.org/ontologies/C2SIM#ObjectDefinitions"/>
        <rdfs:comment>Reference to classes defining one or more Objects</rdfs:comment>
    </owl:ObjectProperty>
    


    <!-- http://www.sisostds.org/ontologies/C2SIM#hasOperationalStatusCode -->

    <owl:ObjectProperty rdf:about="http://www.sisostds.org/ontologies/C2SIM#hasOperationalStatusCode">
        <rdfs:subPropertyOf rdf:resource="http://www.sisostds.org/ontologies/C2SIM#hasCode"/>
        <rdfs:range rdf:resource="http://www.sisostds.org/ontologies/C2SIM#OperationalStatusCode"/>
    </owl:ObjectProperty>
    


    <!-- http://www.sisostds.org/ontologies/C2SIM#hasOrganizationCode -->

    <owl:ObjectProperty rdf:about="http://www.sisostds.org/ontologies/C2SIM#hasOrganizationCode">
        <rdfs:subPropertyOf rdf:resource="http://www.sisostds.org/ontologies/C2SIM#hasCode"/>
        <rdfs:range rdf:resource="http://www.sisostds.org/ontologies/C2SIM#OrganizationCode"/>
    </owl:ObjectProperty>
    


    <!-- http://www.sisostds.org/ontologies/C2SIM#hasOrganizationTypeCode -->

    <owl:ObjectProperty rdf:about="http://www.sisostds.org/ontologies/C2SIM#hasOrganizationTypeCode">
        <rdfs:subPropertyOf rdf:resource="http://www.sisostds.org/ontologies/C2SIM#hasOrganizationCode"/>
        <rdfs:range rdf:resource="http://www.sisostds.org/ontologies/C2SIM#OrganizationTypeCode"/>
    </owl:ObjectProperty>
    


    <!-- http://www.sisostds.org/ontologies/C2SIM#hasOrientation -->

    <owl:ObjectProperty rdf:about="http://www.sisostds.org/ontologies/C2SIM#hasOrientation">
        <rdfs:range rdf:resource="http://www.sisostds.org/ontologies/C2SIM#Orientation"/>
        <rdfs:comment>Provide the geospatial orientation for an Entity.</rdfs:comment>
    </owl:ObjectProperty>
    


    <!-- http://www.sisostds.org/ontologies/C2SIM#hasPlaybackStatusCode -->

    <owl:ObjectProperty rdf:about="http://www.sisostds.org/ontologies/C2SIM#hasPlaybackStatusCode">
        <rdfs:subPropertyOf rdf:resource="http://www.sisostds.org/ontologies/C2SIM#hasCode"/>
        <rdfs:range rdf:resource="http://www.sisostds.org/ontologies/C2SIM#PlaybackStatusCode"/>
    </owl:ObjectProperty>
    


    <!-- http://www.sisostds.org/ontologies/C2SIM#hasRecordingStatusCode -->

    <owl:ObjectProperty rdf:about="http://www.sisostds.org/ontologies/C2SIM#hasRecordingStatusCode">
        <rdfs:subPropertyOf rdf:resource="http://www.sisostds.org/ontologies/C2SIM#hasCode"/>
        <rdfs:range rdf:resource="http://www.sisostds.org/ontologies/C2SIM#RecordingStatusCode"/>
    </owl:ObjectProperty>
    


    <!-- http://www.sisostds.org/ontologies/C2SIM#hasRefreshInitSelection -->

    <owl:ObjectProperty rdf:about="http://www.sisostds.org/ontologies/C2SIM#hasRefreshInitSelection">
        <rdfs:subPropertyOf rdf:resource="http://www.sisostds.org/ontologies/C2SIM#hasCode"/>
        <rdfs:range rdf:resource="http://www.sisostds.org/ontologies/C2SIM#RefreshInitSelection"/>
    </owl:ObjectProperty>
    


    <!-- http://www.sisostds.org/ontologies/C2SIM#hasReligionCode -->

    <owl:ObjectProperty rdf:about="http://www.sisostds.org/ontologies/C2SIM#hasReligionCode">
        <rdfs:subPropertyOf rdf:resource="http://www.sisostds.org/ontologies/C2SIM#hasOrganizationCode"/>
        <rdfs:range rdf:resource="http://www.sisostds.org/ontologies/C2SIM#ReligionCode"/>
    </owl:ObjectProperty>
    


    <!-- http://www.sisostds.org/ontologies/C2SIM#hasReportContent -->

    <owl:ObjectProperty rdf:about="http://www.sisostds.org/ontologies/C2SIM#hasReportContent">
        <rdfs:range rdf:resource="http://www.sisostds.org/ontologies/C2SIM#ReportContent"/>
        <rdfs:comment>Provides the information content for a ReportBody in a Message.</rdfs:comment>
    </owl:ObjectProperty>
    


    <!-- http://www.sisostds.org/ontologies/C2SIM#hasRequestContent -->

    <owl:ObjectProperty rdf:about="http://www.sisostds.org/ontologies/C2SIM#hasRequestContent">
        <rdfs:range rdf:resource="http://www.sisostds.org/ontologies/C2SIM#RequestContent"/>
    </owl:ObjectProperty>
    


    <!-- http://www.sisostds.org/ontologies/C2SIM#hasResource -->

    <owl:ObjectProperty rdf:about="http://www.sisostds.org/ontologies/C2SIM#hasResource">
        <rdfs:range rdf:resource="http://www.sisostds.org/ontologies/C2SIM#Resource"/>
        <rdfs:comment>Provides a reference to a Resource class associated with an Object.</rdfs:comment>
    </owl:ObjectProperty>
    


    <!-- http://www.sisostds.org/ontologies/C2SIM#hasSISOEntityType -->

    <owl:ObjectProperty rdf:about="http://www.sisostds.org/ontologies/C2SIM#hasSISOEntityType">
        <rdfs:range rdf:resource="http://www.sisostds.org/ontologies/C2SIM#SISOEntityType"/>
        <rdfs:comment>Provide a value for the SISO Entity Type of a C2SIM Entity or a C2SIM Resource.</rdfs:comment>
    </owl:ObjectProperty>
    


    <!-- http://www.sisostds.org/ontologies/C2SIM#hasScenarioSetting -->

    <owl:ObjectProperty rdf:about="http://www.sisostds.org/ontologies/C2SIM#hasScenarioSetting">
        <rdfs:range rdf:resource="http://www.sisostds.org/ontologies/C2SIM#ScenarioSetting"/>
        <rdfs:comment>Provides a reference to a ScenarioSetting class associated with initiatlization.</rdfs:comment>
    </owl:ObjectProperty>
    


    <!-- http://www.sisostds.org/ontologies/C2SIM#hasSecurityClassificationCode -->

    <owl:ObjectProperty rdf:about="http://www.sisostds.org/ontologies/C2SIM#hasSecurityClassificationCode">
        <rdfs:subPropertyOf rdf:resource="http://www.sisostds.org/ontologies/C2SIM#hasCode"/>
        <rdfs:range rdf:resource="http://www.sisostds.org/ontologies/C2SIM#SecurityClassificationCode"/>
    </owl:ObjectProperty>
    


    <!-- http://www.sisostds.org/ontologies/C2SIM#hasSendingTime -->

    <owl:ObjectProperty rdf:about="http://www.sisostds.org/ontologies/C2SIM#hasSendingTime">
        <rdfs:subPropertyOf rdf:resource="http://www.sisostds.org/ontologies/C2SIM#hasDateTime"/>
        <rdfs:range rdf:resource="http://www.sisostds.org/ontologies/C2SIM#DateTime"/>
        <rdfs:comment>The DateTime that the message is sent.</rdfs:comment>
    </owl:ObjectProperty>
    


    <!-- http://www.sisostds.org/ontologies/C2SIM#hasSpatialOffset -->

    <owl:ObjectProperty rdf:about="http://www.sisostds.org/ontologies/C2SIM#hasSpatialOffset">
        <rdfs:range rdf:resource="http://www.sisostds.org/ontologies/C2SIM#SpatialOffset"/>
        <rdfs:comment>Provides a value for SpatialOffset of a geospatial location.</rdfs:comment>
    </owl:ObjectProperty>
    


    <!-- http://www.sisostds.org/ontologies/C2SIM#hasStartTime -->

    <owl:ObjectProperty rdf:about="http://www.sisostds.org/ontologies/C2SIM#hasStartTime">
        <rdfs:subPropertyOf rdf:resource="http://www.sisostds.org/ontologies/C2SIM#hasTimeInstant"/>
        <rdfs:range rdf:resource="http://www.sisostds.org/ontologies/C2SIM#TimeInstant"/>
        <rdfs:comment>The beginning time instant of any concept that has a duration over a time interval. For example, the time at which an action/task is to begin (C-BML)</rdfs:comment>
    </owl:ObjectProperty>
    


    <!-- http://www.sisostds.org/ontologies/C2SIM#hasSystemEntityList -->

    <owl:ObjectProperty rdf:about="http://www.sisostds.org/ontologies/C2SIM#hasSystemEntityList">
        <rdfs:range rdf:resource="http://www.sisostds.org/ontologies/C2SIM#SystemEntityList"/>
        <rdfs:comment>Provides a reference to a SystemEntityList associated with an Initialziation Message.</rdfs:comment>
    </owl:ObjectProperty>
    


    <!-- http://www.sisostds.org/ontologies/C2SIM#hasTask -->

    <owl:ObjectProperty rdf:about="http://www.sisostds.org/ontologies/C2SIM#hasTask">
        <rdfs:subPropertyOf rdf:resource="http://www.sisostds.org/ontologies/C2SIM#hasAction"/>
        <rdfs:range rdf:resource="http://www.sisostds.org/ontologies/C2SIM#Task"/>
        <rdfs:comment>Reference to a Task object.</rdfs:comment>
    </owl:ObjectProperty>
    


    <!-- http://www.sisostds.org/ontologies/C2SIM#hasTaskActionCode -->

    <owl:ObjectProperty rdf:about="http://www.sisostds.org/ontologies/C2SIM#hasTaskActionCode">
        <rdfs:subPropertyOf rdf:resource="http://www.sisostds.org/ontologies/C2SIM#hasActionCode"/>
        <rdfs:range rdf:resource="http://www.sisostds.org/ontologies/C2SIM#TaskActionCode"/>
    </owl:ObjectProperty>
    


    <!-- http://www.sisostds.org/ontologies/C2SIM#hasTaskStatusCode -->

    <owl:ObjectProperty rdf:about="http://www.sisostds.org/ontologies/C2SIM#hasTaskStatusCode">
        <rdfs:subPropertyOf rdf:resource="http://www.sisostds.org/ontologies/C2SIM#hasCode"/>
        <rdfs:range rdf:resource="http://www.sisostds.org/ontologies/C2SIM#TaskStatusCode"/>
        <rdfs:comment>Property of having a task status code.</rdfs:comment>
    </owl:ObjectProperty>
    


    <!-- http://www.sisostds.org/ontologies/C2SIM#hasTemporalConcept -->

    <owl:ObjectProperty rdf:about="http://www.sisostds.org/ontologies/C2SIM#hasTemporalConcept">
        <rdfs:range rdf:resource="http://www.sisostds.org/ontologies/C2SIM#TemporalConcept"/>
        <rdfs:comment>Provides a value for a TemporalConcept associated with a Task or Activity.</rdfs:comment>
    </owl:ObjectProperty>
    


    <!-- http://www.sisostds.org/ontologies/C2SIM#hasTimeInstant -->

    <owl:ObjectProperty rdf:about="http://www.sisostds.org/ontologies/C2SIM#hasTimeInstant">
        <rdfs:subPropertyOf rdf:resource="http://www.sisostds.org/ontologies/C2SIM#hasTemporalConcept"/>
        <rdfs:range rdf:resource="http://www.sisostds.org/ontologies/C2SIM#TimeInstant"/>
        <rdfs:comment>The object is referenced to a specific instant in time, specified in one of the ways that time can be represented--for example DateTime, Simulation Time, or Relative Time.</rdfs:comment>
    </owl:ObjectProperty>
    


    <!-- http://www.sisostds.org/ontologies/C2SIM#hasTimeOfObservation -->

    <owl:ObjectProperty rdf:about="http://www.sisostds.org/ontologies/C2SIM#hasTimeOfObservation">
        <rdfs:subPropertyOf rdf:resource="http://www.sisostds.org/ontologies/C2SIM#hasTimeInstant"/>
        <rdfs:range rdf:resource="http://www.sisostds.org/ontologies/C2SIM#TimeInstant"/>
        <rdfs:comment>provides a time at which a reported Observation was made</rdfs:comment>
    </owl:ObjectProperty>
    


    <!-- http://www.sisostds.org/ontologies/C2SIM#hasTimeReferenceCode -->

    <owl:ObjectProperty rdf:about="http://www.sisostds.org/ontologies/C2SIM#hasTimeReferenceCode">
        <rdfs:subPropertyOf rdf:resource="http://www.sisostds.org/ontologies/C2SIM#hasTemporalConcept"/>
        <rdfs:range rdf:resource="http://www.sisostds.org/ontologies/C2SIM#TimeReferenceCode"/>
        <rdfs:comment>A code indicating whether the reference to an event time (in a RelativeTime object) refers to the beginning or end time of the event.</rdfs:comment>
    </owl:ObjectProperty>
    


    <!-- http://www.sisostds.org/ontologies/lox#hasEvent -->

    <owl:ObjectProperty rdf:about="http://www.sisostds.org/ontologies/lox#hasEvent">
        <rdfs:subPropertyOf rdf:resource="http://www.sisostds.org/ontologies/C2SIM#hasAction"/>
        <rdfs:range rdf:resource="http://www.sisostds.org/ontologies/C2SIM#Event"/>
        <rdfs:comment>An event referenced to this class.</rdfs:comment>
    </owl:ObjectProperty>
    


    <!-- http://www.sisostds.org/ontologies/lox#hasPlanPhase -->

    <owl:ObjectProperty rdf:about="http://www.sisostds.org/ontologies/lox#hasPlanPhase">
        <rdfs:range rdf:resource="http://www.sisostds.org/ontologies/lox#PlanPhase"/>
        <rdfs:comment>Reference to a particular phase of an LOX Plan</rdfs:comment>
    </owl:ObjectProperty>
    


    <!-- http://www.sisostds.org/ontologies/lox#hasPlanPhaseCompletionCondition -->

    <owl:ObjectProperty rdf:about="http://www.sisostds.org/ontologies/lox#hasPlanPhaseCompletionCondition">
        <rdfs:range rdf:resource="http://www.sisostds.org/ontologies/lox#PlanPhaseCompletionCondition"/>
        <rdfs:comment>Provides a condition for completion of a LOX PlanPhase.</rdfs:comment>
    </owl:ObjectProperty>
    


    <!-- http://www.sisostds.org/ontologies/lox#hasPlanPhaseTrigger -->

    <owl:ObjectProperty rdf:about="http://www.sisostds.org/ontologies/lox#hasPlanPhaseTrigger">
        <rdfs:range rdf:resource="http://www.sisostds.org/ontologies/lox#PlanPhaseTrigger"/>
        <rdfs:comment>Provides the condition that will trigger an LOX PlanPhase</rdfs:comment>
    </owl:ObjectProperty>
    


    <!-- http://www.sisostds.org/ontologies/lox#hasRuleOfEngagement -->

    <owl:ObjectProperty rdf:about="http://www.sisostds.org/ontologies/lox#hasRuleOfEngagement">
        <rdfs:range rdf:resource="http://www.sisostds.org/ontologies/lox#RuleOfEngagement"/>
        <rdfs:comment>Provides RulesOfEngagement for an LOX Task or Activity.</rdfs:comment>
    </owl:ObjectProperty>
    


    <!-- http://www.sisostds.org/ontologies/lox#hasSubPhase -->

    <owl:ObjectProperty rdf:about="http://www.sisostds.org/ontologies/lox#hasSubPhase">
        <rdfs:range rdf:resource="http://www.sisostds.org/ontologies/lox#PlanPhase"/>
        <rdfs:comment>Reference to SubPhase of an LOX PlanPhase</rdfs:comment>
    </owl:ObjectProperty>
    


    <!-- http://www.sisostds.org/ontologies/lox#hasTaskFunctionalAssociationCode -->

    <owl:ObjectProperty rdf:about="http://www.sisostds.org/ontologies/lox#hasTaskFunctionalAssociationCode">
        <rdfs:range rdf:resource="http://www.sisostds.org/ontologies/lox#TaskFunctionalAssociationCode"/>
        <rdfs:comment>Provides a JC3IEDM ActionFunctionalAssociateCode forn LOX Task.</rdfs:comment>
    </owl:ObjectProperty>
    


    <!-- http://www.sisostds.org/ontologies/lox#hasTaskFunctionalRelation -->

    <owl:ObjectProperty rdf:about="http://www.sisostds.org/ontologies/lox#hasTaskFunctionalRelation">
        <rdfs:range rdf:resource="http://www.sisostds.org/ontologies/lox#TaskFunctionalRelation"/>
        <rdfs:comment>Provides a JC3IEDM FunctionalRelation code for an LOX Task.</rdfs:comment>
    </owl:ObjectProperty>
    


    <!-- http://www.sisostds.org/ontologies/lox#hasWeaponROECode -->

    <owl:ObjectProperty rdf:about="http://www.sisostds.org/ontologies/lox#hasWeaponROECode">
        <rdfs:subPropertyOf rdf:resource="http://www.sisostds.org/ontologies/C2SIM#hasCode"/>
    </owl:ObjectProperty>
    


    <!-- http://www.sisostds.org/ontologies/smx#hasAPP6CSymbol -->

    <owl:ObjectProperty rdf:about="http://www.sisostds.org/ontologies/smx#hasAPP6CSymbol">
        <rdfs:subPropertyOf rdf:resource="http://www.w3.org/2002/07/owl#topObjectProperty"/>
        <rdfs:range rdf:resource="http://www.sisostds.org/ontologies/smx#APP6CSymbol"/>
        <rdfs:comment>Indicates the NATO APP-6-C tactical graphic symbol.</rdfs:comment>
    </owl:ObjectProperty>
    


    <!-- http://www.sisostds.org/ontologies/smx#hasCommandRelation -->

    <owl:ObjectProperty rdf:about="http://www.sisostds.org/ontologies/smx#hasCommandRelation">
        <rdfs:range rdf:resource="http://www.sisostds.org/ontologies/smx#CommandRelation"/>
        <rdfs:comment>Indicates a miltary unit&apos;s particular command relationship.</rdfs:comment>
    </owl:ObjectProperty>
    


    <!-- http://www.sisostds.org/ontologies/smx#hasCommandRelationCode -->

    <owl:ObjectProperty rdf:about="http://www.sisostds.org/ontologies/smx#hasCommandRelationCode">
        <rdfs:subPropertyOf rdf:resource="http://www.sisostds.org/ontologies/C2SIM#hasCode"/>
        <rdfs:range rdf:resource="http://www.sisostds.org/ontologies/smx#CommandRelationCode"/>
    </owl:ObjectProperty>
    


    <!-- http://www.sisostds.org/ontologies/smx#hasEchelonCode -->

    <owl:ObjectProperty rdf:about="http://www.sisostds.org/ontologies/smx#hasEchelonCode">
        <rdfs:subPropertyOf rdf:resource="http://www.sisostds.org/ontologies/C2SIM#hasCode"/>
        <rdfs:range rdf:resource="http://www.sisostds.org/ontologies/smx#EchelonCode"/>
    </owl:ObjectProperty>
    


    <!-- http://www.sisostds.org/ontologies/smx#hasForceSideRelation -->

    <owl:ObjectProperty rdf:about="http://www.sisostds.org/ontologies/smx#hasForceSideRelation">
        <rdfs:range rdf:resource="http://www.sisostds.org/ontologies/smx#ForceSideRelation"/>
        <rdfs:comment>Indicates the ForceSideRelation code for an Entity.</rdfs:comment>
    </owl:ObjectProperty>
    


    <!-- http://www.sisostds.org/ontologies/smx#hasHostilityStatusCode -->

    <owl:ObjectProperty rdf:about="http://www.sisostds.org/ontologies/smx#hasHostilityStatusCode">
        <rdfs:subPropertyOf rdf:resource="http://www.sisostds.org/ontologies/C2SIM#hasCode"/>
        <rdfs:range rdf:resource="http://www.sisostds.org/ontologies/smx#HostilityStatusCode"/>
    </owl:ObjectProperty>
    


    <!-- http://www.sisostds.org/ontologies/smx#hasMIPRequestCategoryCode -->

    <owl:ObjectProperty rdf:about="http://www.sisostds.org/ontologies/smx#hasMIPRequestCategoryCode">
        <rdfs:subPropertyOf rdf:resource="http://www.sisostds.org/ontologies/C2SIM#hasCode"/>
        <rdfs:range rdf:resource="http://www.sisostds.org/ontologies/smx#MIPRequestCategoryCode"/>
        <rdfs:comment>A request category from the Joint Consultation Command Control Information Exchange Data Model (JC3IEDM) developed by the Multilateral Interoperability Programme (MIP).</rdfs:comment>
    </owl:ObjectProperty>
    


    <!-- http://www.sisostds.org/ontologies/smx#hasObservation -->

    <owl:ObjectProperty rdf:about="http://www.sisostds.org/ontologies/smx#hasObservation">
        <rdfs:range rdf:resource="http://www.sisostds.org/ontologies/smx#Observation"/>
        <rdfs:comment>Indicates an Observation value associated with a class.</rdfs:comment>
    </owl:ObjectProperty>
    


    <!-- http://www.sisostds.org/ontologies/smx#hasOperationalStatus -->

    <owl:ObjectProperty rdf:about="http://www.sisostds.org/ontologies/smx#hasOperationalStatus">
        <rdfs:subPropertyOf rdf:resource="http://www.w3.org/2002/07/owl#topObjectProperty"/>
        <rdfs:range rdf:resource="http://www.sisostds.org/ontologies/C2SIM#OperationalStatus"/>
        <rdfs:comment>Indicates the level to which a military unit is prepared to carry out its combat functions, from a range of values.</rdfs:comment>
    </owl:ObjectProperty>
    


    <!-- http://www.sisostds.org/ontologies/smx#hasReinforcedReducedType -->

    <owl:ObjectProperty rdf:about="http://www.sisostds.org/ontologies/smx#hasReinforcedReducedType">
        <rdfs:range rdf:resource="http://www.sisostds.org/ontologies/smx#ReinforcedReducedType"/>
        <rdfs:comment>Indiates the current code for type of reiforcement or reduction of an ENtity.</rdfs:comment>
    </owl:ObjectProperty>
    


    <!-- 
    ///////////////////////////////////////////////////////////////////////////////////////
    //
    // Data properties
    //
    ///////////////////////////////////////////////////////////////////////////////////////
     -->

    


    <!-- http://www.sisostds.org/ontologies/C2SIM#hasAbstractObjectReference -->

    <owl:DatatypeProperty rdf:about="http://www.sisostds.org/ontologies/C2SIM#hasAbstractObjectReference">
        <rdfs:subPropertyOf rdf:resource="http://www.sisostds.org/ontologies/C2SIM#hasReference"/>
        <rdfs:range rdf:resource="http://www.sisostds.org/ontologies/C2SIM#UUIDBase"/>
        <rdfs:comment>The reference is to some abstract object.</rdfs:comment>
    </owl:DatatypeProperty>
    


    <!-- http://www.sisostds.org/ontologies/C2SIM#hasAbstractOrganizationReference -->

    <owl:DatatypeProperty rdf:about="http://www.sisostds.org/ontologies/C2SIM#hasAbstractOrganizationReference">
        <rdfs:subPropertyOf rdf:resource="http://www.sisostds.org/ontologies/C2SIM#hasAbstractObjectReference"/>
        <rdfs:range rdf:resource="http://www.sisostds.org/ontologies/C2SIM#UUIDBase"/>
        <rdfs:comment>The reference is to an abstract organization.</rdfs:comment>
    </owl:DatatypeProperty>
    


    <!-- http://www.sisostds.org/ontologies/C2SIM#hasActionReference -->

    <owl:DatatypeProperty rdf:about="http://www.sisostds.org/ontologies/C2SIM#hasActionReference">
        <rdfs:subPropertyOf rdf:resource="http://www.sisostds.org/ontologies/C2SIM#hasReference"/>
        <rdfs:range rdf:resource="http://www.sisostds.org/ontologies/C2SIM#UUIDBase"/>
        <rdfs:comment>The reference is to another class identifying an Action.</rdfs:comment>
    </owl:DatatypeProperty>
    


    <!-- http://www.sisostds.org/ontologies/C2SIM#hasActorReference -->

    <owl:DatatypeProperty rdf:about="http://www.sisostds.org/ontologies/C2SIM#hasActorReference">
        <rdfs:subPropertyOf rdf:resource="http://www.sisostds.org/ontologies/C2SIM#hasEntityReference"/>
        <rdfs:range rdf:resource="http://www.sisostds.org/ontologies/C2SIM#UUIDBase"/>
        <rdfs:comment>These references should be to objects of class Actor, or subclasses.</rdfs:comment>
    </owl:DatatypeProperty>
    


    <!-- http://www.sisostds.org/ontologies/C2SIM#hasAffectedEntity -->

    <owl:DatatypeProperty rdf:about="http://www.sisostds.org/ontologies/C2SIM#hasAffectedEntity">
        <rdfs:subPropertyOf rdf:resource="http://www.sisostds.org/ontologies/C2SIM#hasActorReference"/>
        <rdfs:range rdf:resource="http://www.sisostds.org/ontologies/C2SIM#UUIDBase"/>
        <rdfs:comment>The reference is to an instance of AffectedEntity.</rdfs:comment>
    </owl:DatatypeProperty>
    


    <!-- http://www.sisostds.org/ontologies/C2SIM#hasAltitude -->

    <owl:DatatypeProperty rdf:about="http://www.sisostds.org/ontologies/C2SIM#hasAltitude">
        <rdfs:subPropertyOf rdf:resource="http://www.sisostds.org/ontologies/C2SIM#hasSpatialMeasure"/>
        <rdfs:range rdf:resource="http://www.w3.org/2001/XMLSchema#double"/>
        <rdfs:comment>Property of geospatial data values that represent distance vertically above a surface.</rdfs:comment>
    </owl:DatatypeProperty>
    


    <!-- http://www.sisostds.org/ontologies/C2SIM#hasAltitudeAGL -->

    <owl:DatatypeProperty rdf:about="http://www.sisostds.org/ontologies/C2SIM#hasAltitudeAGL">
        <rdfs:subPropertyOf rdf:resource="http://www.sisostds.org/ontologies/C2SIM#hasAltitude"/>
        <rdfs:range rdf:resource="http://www.w3.org/2001/XMLSchema#double"/>
        <rdfs:comment>Property of geospatial data values that represent distance vertically above ground level in meters.</rdfs:comment>
    </owl:DatatypeProperty>
    


    <!-- http://www.sisostds.org/ontologies/C2SIM#hasAltitudeMSL -->

    <owl:DatatypeProperty rdf:about="http://www.sisostds.org/ontologies/C2SIM#hasAltitudeMSL">
        <rdfs:subPropertyOf rdf:resource="http://www.sisostds.org/ontologies/C2SIM#hasAltitude"/>
        <rdfs:range rdf:resource="http://www.w3.org/2001/XMLSchema#double"/>
        <rdfs:comment>Property of geospatial data values that represent distance vertically above mean sea level in meters.</rdfs:comment>
    </owl:DatatypeProperty>
    


    <!-- http://www.sisostds.org/ontologies/C2SIM#hasAngle -->

    <owl:DatatypeProperty rdf:about="http://www.sisostds.org/ontologies/C2SIM#hasAngle">
        <rdfs:subPropertyOf rdf:resource="http://www.sisostds.org/ontologies/C2SIM#hasSpatialMeasure"/>
        <rdfs:range rdf:resource="http://www.w3.org/2001/XMLSchema#double"/>
    </owl:DatatypeProperty>
    


    <!-- http://www.sisostds.org/ontologies/C2SIM#hasAuthorizationCredentials -->

    <owl:DatatypeProperty rdf:about="http://www.sisostds.org/ontologies/C2SIM#hasAuthorizationCredentials">
        <rdfs:range rdf:resource="http://www.w3.org/2001/XMLSchema#string"/>
        <rdfs:comment>The actual authentication tokens or encoded user credentials. The format and content depend on the authentication scheme (see property hasAuthorizationType).</rdfs:comment>
    </owl:DatatypeProperty>
    


    <!-- http://www.sisostds.org/ontologies/C2SIM#hasAuthorizationType -->

    <owl:DatatypeProperty rdf:about="http://www.sisostds.org/ontologies/C2SIM#hasAuthorizationType">
        <rdfs:range rdf:resource="http://www.w3.org/2001/XMLSchema#string"/>
        <rdfs:comment>The authentication scheme (or type), such as Basic, Bearer, Digest, etc. It indicates the method used for encoding or handling the credentials.</rdfs:comment>
    </owl:DatatypeProperty>
    


    <!-- http://www.sisostds.org/ontologies/C2SIM#hasComment -->

    <owl:DatatypeProperty rdf:about="http://www.sisostds.org/ontologies/C2SIM#hasComment">
        <rdfs:range rdf:resource="http://www.w3.org/2001/XMLSchema#string"/>
        <rdfs:comment>The class has descriptive information to allow human understanding of its function.</rdfs:comment>
    </owl:DatatypeProperty>
    


    <!-- http://www.sisostds.org/ontologies/C2SIM#hasCommunicationsNetwork -->

    <owl:DatatypeProperty rdf:about="http://www.sisostds.org/ontologies/C2SIM#hasCommunicationsNetwork">
        <rdfs:subPropertyOf rdf:resource="http://www.sisostds.org/ontologies/C2SIM#hasAbstractObjectReference"/>
        <rdfs:range rdf:resource="http://www.sisostds.org/ontologies/C2SIM#UUIDBase"/>
        <rdfs:comment>The reference is to a class identifying a communications network.</rdfs:comment>
    </owl:DatatypeProperty>
    


    <!-- http://www.sisostds.org/ontologies/C2SIM#hasConcreteEntityReference -->

    <owl:DatatypeProperty rdf:about="http://www.sisostds.org/ontologies/C2SIM#hasConcreteEntityReference">
        <rdfs:subPropertyOf rdf:resource="http://www.sisostds.org/ontologies/C2SIM#hasEntityReference"/>
        <rdfs:range rdf:resource="http://www.sisostds.org/ontologies/C2SIM#UUIDBase"/>
        <rdfs:comment>Property of a class that has a Concrete Entity.</rdfs:comment>
    </owl:DatatypeProperty>
    


    <!-- http://www.sisostds.org/ontologies/C2SIM#hasConversationID -->

    <owl:DatatypeProperty rdf:about="http://www.sisostds.org/ontologies/C2SIM#hasConversationID">
        <rdfs:subPropertyOf rdf:resource="http://www.sisostds.org/ontologies/C2SIM#hasMessagingDataProperty"/>
        <rdfs:range rdf:resource="http://www.sisostds.org/ontologies/C2SIM#UUIDBase"/>
        <rdfs:comment>FIPA identifer unique to a particular thread of messages for a particular sender.</rdfs:comment>
    </owl:DatatypeProperty>
    


    <!-- http://www.sisostds.org/ontologies/C2SIM#hasCoordinateValue -->

    <owl:DatatypeProperty rdf:about="http://www.sisostds.org/ontologies/C2SIM#hasCoordinateValue">
        <rdfs:comment>Instances of the class have data identifying their geospatial location.</rdfs:comment>
    </owl:DatatypeProperty>
    


    <!-- http://www.sisostds.org/ontologies/C2SIM#hasCurrentTask -->

    <owl:DatatypeProperty rdf:about="http://www.sisostds.org/ontologies/C2SIM#hasCurrentTask">
        <rdfs:subPropertyOf rdf:resource="http://www.sisostds.org/ontologies/C2SIM#hasTaskReference"/>
        <rdfs:range rdf:resource="http://www.sisostds.org/ontologies/C2SIM#UUIDBase"/>
        <rdfs:comment>The reference is to another class identifying a Task which is currently active.</rdfs:comment>
    </owl:DatatypeProperty>
    


    <!-- http://www.sisostds.org/ontologies/C2SIM#hasDISCategory -->

    <owl:DatatypeProperty rdf:about="http://www.sisostds.org/ontologies/C2SIM#hasDISCategory">
        <rdfs:subPropertyOf rdf:resource="http://www.sisostds.org/ontologies/C2SIM#hasDISCode"/>
        <rdfs:range rdf:resource="http://www.w3.org/2001/XMLSchema#byte"/>
        <rdfs:comment>Provides a Category Code from the DIS standard IEEE 1516-2010.</rdfs:comment>
    </owl:DatatypeProperty>
    


    <!-- http://www.sisostds.org/ontologies/C2SIM#hasDISCode -->

    <owl:DatatypeProperty rdf:about="http://www.sisostds.org/ontologies/C2SIM#hasDISCode">
        <rdfs:comment>Provides an entity type code from IEEE 1516-2010 Distributed Interactive Simulation.</rdfs:comment>
    </owl:DatatypeProperty>
    


    <!-- http://www.sisostds.org/ontologies/C2SIM#hasDISCountry -->

    <owl:DatatypeProperty rdf:about="http://www.sisostds.org/ontologies/C2SIM#hasDISCountry">
        <rdfs:subPropertyOf rdf:resource="http://www.sisostds.org/ontologies/C2SIM#hasDISCode"/>
        <rdfs:range rdf:resource="http://www.w3.org/2001/XMLSchema#integer"/>
        <rdfs:comment>Provides a Country Code from the DIS standard IEEE 1516-2010.</rdfs:comment>
    </owl:DatatypeProperty>
    


    <!-- http://www.sisostds.org/ontologies/C2SIM#hasDISDomain -->

    <owl:DatatypeProperty rdf:about="http://www.sisostds.org/ontologies/C2SIM#hasDISDomain">
        <rdfs:subPropertyOf rdf:resource="http://www.sisostds.org/ontologies/C2SIM#hasDISCode"/>
        <rdfs:range rdf:resource="http://www.w3.org/2001/XMLSchema#byte"/>
        <rdfs:comment>Provides a Domain Code from the DIS standard IEEE 1516-2010.</rdfs:comment>
    </owl:DatatypeProperty>
    


    <!-- http://www.sisostds.org/ontologies/C2SIM#hasDISExtra -->

    <owl:DatatypeProperty rdf:about="http://www.sisostds.org/ontologies/C2SIM#hasDISExtra">
        <rdfs:subPropertyOf rdf:resource="http://www.sisostds.org/ontologies/C2SIM#hasDISCode"/>
        <rdfs:range rdf:resource="http://www.w3.org/2001/XMLSchema#byte"/>
        <rdfs:comment>Provides an Extra Code from the DIS standard IEEE 1516-2010.</rdfs:comment>
    </owl:DatatypeProperty>
    


    <!-- http://www.sisostds.org/ontologies/C2SIM#hasDISKind -->

    <owl:DatatypeProperty rdf:about="http://www.sisostds.org/ontologies/C2SIM#hasDISKind">
        <rdfs:subPropertyOf rdf:resource="http://www.sisostds.org/ontologies/C2SIM#hasDISCode"/>
        <rdfs:range rdf:resource="http://www.w3.org/2001/XMLSchema#byte"/>
        <rdfs:comment>Provides a Kind Code from the DIS standard IEEE 1516-2010.</rdfs:comment>
    </owl:DatatypeProperty>
    


    <!-- http://www.sisostds.org/ontologies/C2SIM#hasDISSpecific -->

    <owl:DatatypeProperty rdf:about="http://www.sisostds.org/ontologies/C2SIM#hasDISSpecific">
        <rdfs:subPropertyOf rdf:resource="http://www.sisostds.org/ontologies/C2SIM#hasDISCode"/>
        <rdfs:range rdf:resource="http://www.w3.org/2001/XMLSchema#byte"/>
        <rdfs:comment>Provides a Specific Code from the DIS standard IEEE 1516-2010.</rdfs:comment>
    </owl:DatatypeProperty>
    


    <!-- http://www.sisostds.org/ontologies/C2SIM#hasDISSubCategory -->

    <owl:DatatypeProperty rdf:about="http://www.sisostds.org/ontologies/C2SIM#hasDISSubCategory">
        <rdfs:subPropertyOf rdf:resource="http://www.sisostds.org/ontologies/C2SIM#hasDISCode"/>
        <rdfs:range rdf:resource="http://www.w3.org/2001/XMLSchema#byte"/>
        <rdfs:comment>Provides a SubCategory Code from the DIS standard IEEE 1516-2010.</rdfs:comment>
    </owl:DatatypeProperty>
    


    <!-- http://www.sisostds.org/ontologies/C2SIM#hasDistance -->

    <owl:DatatypeProperty rdf:about="http://www.sisostds.org/ontologies/C2SIM#hasDistance">
        <rdfs:subPropertyOf rdf:resource="http://www.sisostds.org/ontologies/C2SIM#hasSpatialMeasure"/>
        <rdfs:range rdf:resource="http://www.w3.org/2001/XMLSchema#double"/>
        <rdfs:comment>Property of geospatial data value that represents an aspect of a distance.</rdfs:comment>
    </owl:DatatypeProperty>
    


    <!-- http://www.sisostds.org/ontologies/C2SIM#hasEast -->

    <owl:DatatypeProperty rdf:about="http://www.sisostds.org/ontologies/C2SIM#hasEast">
        <rdfs:subPropertyOf rdf:resource="http://www.sisostds.org/ontologies/C2SIM#hasCoordinateValue"/>
        <rdfs:range rdf:resource="http://www.w3.org/2001/XMLSchema#double"/>
        <rdfs:comment>Value for East coordinate is included.</rdfs:comment>
    </owl:DatatypeProperty>
    


    <!-- http://www.sisostds.org/ontologies/C2SIM#hasEntityReference -->

    <owl:DatatypeProperty rdf:about="http://www.sisostds.org/ontologies/C2SIM#hasEntityReference">
        <rdfs:subPropertyOf rdf:resource="http://www.sisostds.org/ontologies/C2SIM#hasReference"/>
        <rdfs:range rdf:resource="http://www.sisostds.org/ontologies/C2SIM#UUIDBase"/>
        <rdfs:comment>The reference is to an instance of an Entity.</rdfs:comment>
    </owl:DatatypeProperty>
    


    <!-- http://www.sisostds.org/ontologies/C2SIM#hasEntityTypeName -->

    <owl:DatatypeProperty rdf:about="http://www.sisostds.org/ontologies/C2SIM#hasEntityTypeName">
        <rdfs:range rdf:resource="http://www.w3.org/2001/XMLSchema#string"/>
        <rdfs:comment>Name of an NamedEntityType.</rdfs:comment>
    </owl:DatatypeProperty>
    


    <!-- http://www.sisostds.org/ontologies/C2SIM#hasEntityTypeNamespace -->

    <owl:DatatypeProperty rdf:about="http://www.sisostds.org/ontologies/C2SIM#hasEntityTypeNamespace">
        <rdfs:range rdf:resource="http://www.w3.org/2001/XMLSchema#string"/>
        <rdfs:comment>Namespace of an NamedEntityType.</rdfs:comment>
    </owl:DatatypeProperty>
    


    <!-- http://www.sisostds.org/ontologies/C2SIM#hasEventReference -->

    <owl:DatatypeProperty rdf:about="http://www.sisostds.org/ontologies/C2SIM#hasEventReference">
        <rdfs:subPropertyOf rdf:resource="http://www.sisostds.org/ontologies/C2SIM#hasActionReference"/>
        <rdfs:range rdf:resource="http://www.sisostds.org/ontologies/C2SIM#UUIDBase"/>
        <rdfs:comment>The reference is to another Action class identifying an Event.</rdfs:comment>
    </owl:DatatypeProperty>
    


    <!-- http://www.sisostds.org/ontologies/C2SIM#hasFileSize -->

    <owl:DatatypeProperty rdf:about="http://www.sisostds.org/ontologies/C2SIM#hasFileSize">
        <rdfs:range rdf:resource="http://www.w3.org/2001/XMLSchema#nonNegativeInteger"/>
        <rdfs:comment>File size in kilobytes (rounded to nearest integer).</rdfs:comment>
    </owl:DatatypeProperty>
    


    <!-- http://www.sisostds.org/ontologies/C2SIM#hasHeadingAngle -->

    <owl:DatatypeProperty rdf:about="http://www.sisostds.org/ontologies/C2SIM#hasHeadingAngle">
        <rdfs:subPropertyOf rdf:resource="http://www.sisostds.org/ontologies/C2SIM#hasAngle"/>
        <rdfs:range rdf:resource="http://www.w3.org/2001/XMLSchema#double"/>
        <rdfs:comment>Property of geospatial data value that represents heading direction in degrees where north is zero.</rdfs:comment>
    </owl:DatatypeProperty>
    


    <!-- http://www.sisostds.org/ontologies/C2SIM#hasHeight -->

    <owl:DatatypeProperty rdf:about="http://www.sisostds.org/ontologies/C2SIM#hasHeight">
        <rdfs:subPropertyOf rdf:resource="http://www.sisostds.org/ontologies/C2SIM#hasDistance"/>
        <rdfs:range rdf:resource="http://www.w3.org/2001/XMLSchema#double"/>
        <rdfs:comment>Property of geospatial data value that represents height aspect of a distance in meters.</rdfs:comment>
    </owl:DatatypeProperty>
    


    <!-- http://www.sisostds.org/ontologies/C2SIM#hasIntializationFileType -->

    <owl:DatatypeProperty rdf:about="http://www.sisostds.org/ontologies/C2SIM#hasIntializationFileType">
        <rdfs:range rdf:resource="http://www.w3.org/2001/XMLSchema#string"/>
        <rdfs:comment>Indicates initialization information is available in a named data file.</rdfs:comment>
    </owl:DatatypeProperty>
    


    <!-- http://www.sisostds.org/ontologies/C2SIM#hasIsoDateTime -->

    <owl:DatatypeProperty rdf:about="http://www.sisostds.org/ontologies/C2SIM#hasIsoDateTime">
        <rdfs:range rdf:resource="http://www.sisostds.org/ontologies/C2SIM#IsoDateTimeBase"/>
        <rdfs:comment>Instances of the class include identifying &quot;When&quot; information in ISO Date Time format.</rdfs:comment>
    </owl:DatatypeProperty>
    


    <!-- http://www.sisostds.org/ontologies/C2SIM#hasIsoTimeDuration -->

    <owl:DatatypeProperty rdf:about="http://www.sisostds.org/ontologies/C2SIM#hasIsoTimeDuration">
        <rdfs:range rdf:resource="http://www.sisostds.org/ontologies/C2SIM#IsoTimeDurationBase"/>
        <rdfs:comment>Instances of the class have a data value identifying the duration of its &quot;When&quot; in ISO Time format.</rdfs:comment>
    </owl:DatatypeProperty>
    


    <!-- http://www.sisostds.org/ontologies/C2SIM#hasLatitude -->

    <owl:DatatypeProperty rdf:about="http://www.sisostds.org/ontologies/C2SIM#hasLatitude">
        <rdfs:subPropertyOf rdf:resource="http://www.sisostds.org/ontologies/C2SIM#hasCoordinateValue"/>
        <rdfs:range rdf:resource="http://www.sisostds.org/ontologies/C2SIM#latitude"/>
        <rdfs:comment>Value for Latitude coordinate is included. This should have a range specified of -90 to +90 (degrees)</rdfs:comment>
    </owl:DatatypeProperty>
    


    <!-- http://www.sisostds.org/ontologies/C2SIM#hasLength -->

    <owl:DatatypeProperty rdf:about="http://www.sisostds.org/ontologies/C2SIM#hasLength">
        <rdfs:subPropertyOf rdf:resource="http://www.sisostds.org/ontologies/C2SIM#hasDistance"/>
        <rdfs:range rdf:resource="http://www.w3.org/2001/XMLSchema#double"/>
        <rdfs:comment>Property of geospatial data value that represents length aspect of a distance in meters.</rdfs:comment>
    </owl:DatatypeProperty>
    


    <!-- http://www.sisostds.org/ontologies/C2SIM#hasLongitude -->

    <owl:DatatypeProperty rdf:about="http://www.sisostds.org/ontologies/C2SIM#hasLongitude">
        <rdfs:subPropertyOf rdf:resource="http://www.sisostds.org/ontologies/C2SIM#hasCoordinateValue"/>
        <rdfs:range rdf:resource="http://www.sisostds.org/ontologies/C2SIM#longitude"/>
        <rdfs:comment>Value for Longitude coordinate is included. This should have a range specified of -180 to +180 (degrees)</rdfs:comment>
    </owl:DatatypeProperty>
    


    <!-- http://www.sisostds.org/ontologies/C2SIM#hasMapGraphicID -->

    <owl:DatatypeProperty rdf:about="http://www.sisostds.org/ontologies/C2SIM#hasMapGraphicID">
        <rdfs:subPropertyOf rdf:resource="http://www.sisostds.org/ontologies/C2SIM#hasConcreteEntityReference"/>
        <rdfs:range rdf:resource="http://www.sisostds.org/ontologies/C2SIM#UUIDBase"/>
        <rdfs:comment>Property of a class that has a Concrete Entity that is a Map Graphic.</rdfs:comment>
    </owl:DatatypeProperty>
    


    <!-- http://www.sisostds.org/ontologies/C2SIM#hasMarking -->

    <owl:DatatypeProperty rdf:about="http://www.sisostds.org/ontologies/C2SIM#hasMarking">
        <rdfs:range rdf:resource="http://www.w3.org/2001/XMLSchema#string"/>
        <rdfs:comment>Instances of the class include data for alphanumeric information used to identify the instance; typically this is visual identification by humans.</rdfs:comment>
    </owl:DatatypeProperty>
    


    <!-- http://www.sisostds.org/ontologies/C2SIM#hasMessageID -->

    <owl:DatatypeProperty rdf:about="http://www.sisostds.org/ontologies/C2SIM#hasMessageID">
        <rdfs:subPropertyOf rdf:resource="http://www.sisostds.org/ontologies/C2SIM#hasMessagingDataProperty"/>
        <rdfs:range rdf:resource="http://www.sisostds.org/ontologies/C2SIM#UUIDBase"/>
        <rdfs:comment>FIPA identifer unique to an individual message for a particular sender.</rdfs:comment>
    </owl:DatatypeProperty>
    


    <!-- http://www.sisostds.org/ontologies/C2SIM#hasMessagingDataProperty -->

    <owl:DatatypeProperty rdf:about="http://www.sisostds.org/ontologies/C2SIM#hasMessagingDataProperty">
        <rdfs:comment>These are properties of classes associated with C2SIM Messages.</rdfs:comment>
    </owl:DatatypeProperty>
    


    <!-- http://www.sisostds.org/ontologies/C2SIM#hasName -->

    <owl:DatatypeProperty rdf:about="http://www.sisostds.org/ontologies/C2SIM#hasName">
        <rdfs:range rdf:resource="http://www.w3.org/2001/XMLSchema#string"/>
        <rdfs:comment>An alphanumeric identifier that serves for humans to recognize the instance.</rdfs:comment>
    </owl:DatatypeProperty>
    


    <!-- http://www.sisostds.org/ontologies/C2SIM#hasNorth -->

    <owl:DatatypeProperty rdf:about="http://www.sisostds.org/ontologies/C2SIM#hasNorth">
        <rdfs:subPropertyOf rdf:resource="http://www.sisostds.org/ontologies/C2SIM#hasCoordinateValue"/>
        <rdfs:range rdf:resource="http://www.w3.org/2001/XMLSchema#double"/>
        <rdfs:comment>Value for North coordinate is included.</rdfs:comment>
    </owl:DatatypeProperty>
    


    <!-- http://www.sisostds.org/ontologies/C2SIM#hasOnHandQuantity -->

    <owl:DatatypeProperty rdf:about="http://www.sisostds.org/ontologies/C2SIM#hasOnHandQuantity">
        <rdfs:range rdf:resource="http://www.w3.org/2001/XMLSchema#double"/>
        <rdfs:comment>Number of specific resources that a Resource has available.</rdfs:comment>
    </owl:DatatypeProperty>
    


    <!-- http://www.sisostds.org/ontologies/C2SIM#hasOperationalQuantity -->

    <owl:DatatypeProperty rdf:about="http://www.sisostds.org/ontologies/C2SIM#hasOperationalQuantity">
        <rdfs:range rdf:resource="http://www.w3.org/2001/XMLSchema#double"/>
        <rdfs:comment>Number of specific resources that a Resource has available for operations.</rdfs:comment>
    </owl:DatatypeProperty>
    


    <!-- http://www.sisostds.org/ontologies/C2SIM#hasOrderID -->

    <owl:DatatypeProperty rdf:about="http://www.sisostds.org/ontologies/C2SIM#hasOrderID">
        <rdfs:subPropertyOf rdf:resource="http://www.sisostds.org/ontologies/C2SIM#hasMessagingDataProperty"/>
        <rdfs:range rdf:resource="http://www.sisostds.org/ontologies/C2SIM#UUIDBase"/>
        <rdfs:comment>FIPA identifer unique to an individual Order for a particular sender.</rdfs:comment>
    </owl:DatatypeProperty>
    


    <!-- http://www.sisostds.org/ontologies/C2SIM#hasPerformingEntity -->

    <owl:DatatypeProperty rdf:about="http://www.sisostds.org/ontologies/C2SIM#hasPerformingEntity">
        <rdfs:subPropertyOf rdf:resource="http://www.sisostds.org/ontologies/C2SIM#hasActorReference"/>
        <rdfs:range rdf:resource="http://www.sisostds.org/ontologies/C2SIM#UUIDBase"/>
        <rdfs:comment>The reference is to an instance of PerformingEntity.</rdfs:comment>
    </owl:DatatypeProperty>
    


    <!-- http://www.sisostds.org/ontologies/C2SIM#hasPhi -->

    <owl:DatatypeProperty rdf:about="http://www.sisostds.org/ontologies/C2SIM#hasPhi">
        <rdfs:subPropertyOf rdf:resource="http://www.sisostds.org/ontologies/C2SIM#hasAngle"/>
        <rdfs:range rdf:resource="http://www.w3.org/2001/XMLSchema#double"/>
        <rdfs:comment>Property of geospatial data value that represents Euler Angle Phi in radians.</rdfs:comment>
    </owl:DatatypeProperty>
    


    <!-- http://www.sisostds.org/ontologies/C2SIM#hasPlaybackPosition -->

    <owl:DatatypeProperty rdf:about="http://www.sisostds.org/ontologies/C2SIM#hasPlaybackPosition">
        <rdfs:range rdf:resource="http://www.w3.org/2001/XMLSchema#string"/>
        <rdfs:comment>Gives the string value of the position of the playback in the file of recorded messages from execution of a C2SIM coalition of systems.</rdfs:comment>
    </owl:DatatypeProperty>
    


    <!-- http://www.sisostds.org/ontologies/C2SIM#hasPlaybackRealtimeMultiple -->

    <owl:DatatypeProperty rdf:about="http://www.sisostds.org/ontologies/C2SIM#hasPlaybackRealtimeMultiple">
        <rdfs:range rdf:resource="http://www.sisostds.org/ontologies/C2SIM#playbackRealtimeMultiple"/>
        <rdfs:comment>Decimal rate indicating ratio of simulation time to real time for playback of recorded messages (e.g., value of 2.0 indicates messages are played back at 2:1 simulation time to realtime [i.e., faster than realtime]; 0.5 indicates message playback at half realtime [i.e., slower than realtime]).</rdfs:comment>
    </owl:DatatypeProperty>
    


    <!-- http://www.sisostds.org/ontologies/C2SIM#hasProtocol -->

    <owl:DatatypeProperty rdf:about="http://www.sisostds.org/ontologies/C2SIM#hasProtocol">
        <rdfs:range rdf:resource="http://www.w3.org/2001/XMLSchema#string"/>
        <rdfs:comment>Instances of the class have a code identifying a protocol applicable to that class.</rdfs:comment>
    </owl:DatatypeProperty>
    


    <!-- http://www.sisostds.org/ontologies/C2SIM#hasProtocolVersion -->

    <owl:DatatypeProperty rdf:about="http://www.sisostds.org/ontologies/C2SIM#hasProtocolVersion">
        <rdfs:range rdf:resource="http://www.w3.org/2001/XMLSchema#string"/>
        <rdfs:comment>Instances of the class have a version identifier associated with a protocol applicable to that class, which in turn is identified by property has Protocol.</rdfs:comment>
    </owl:DatatypeProperty>
    


    <!-- http://www.sisostds.org/ontologies/C2SIM#hasPsi -->

    <owl:DatatypeProperty rdf:about="http://www.sisostds.org/ontologies/C2SIM#hasPsi">
        <rdfs:subPropertyOf rdf:resource="http://www.sisostds.org/ontologies/C2SIM#hasAngle"/>
        <rdfs:range rdf:resource="http://www.w3.org/2001/XMLSchema#double"/>
        <rdfs:comment>Property of geospatial data value that represents Euler Angle Psi in radians.</rdfs:comment>
    </owl:DatatypeProperty>
    


    <!-- http://www.sisostds.org/ontologies/C2SIM#hasReference -->

    <owl:DatatypeProperty rdf:about="http://www.sisostds.org/ontologies/C2SIM#hasReference">
        <rdfs:range rdf:resource="http://www.sisostds.org/ontologies/C2SIM#UUIDBase"/>
        <rdfs:comment>Instances of the class have reference to instanced of another associated class.</rdfs:comment>
    </owl:DatatypeProperty>
    


    <!-- http://www.sisostds.org/ontologies/C2SIM#hasReplyToSystem -->

    <owl:DatatypeProperty rdf:about="http://www.sisostds.org/ontologies/C2SIM#hasReplyToSystem">
        <rdfs:subPropertyOf rdf:resource="http://www.sisostds.org/ontologies/C2SIM#hasMessagingDataProperty"/>
        <rdfs:range rdf:resource="http://www.w3.org/2001/XMLSchema#string"/>
        <rdfs:comment>Unique FIPA identifer of the system to which individual message reply is to be made.</rdfs:comment>
    </owl:DatatypeProperty>
    


    <!-- http://www.sisostds.org/ontologies/C2SIM#hasReportID -->

    <owl:DatatypeProperty rdf:about="http://www.sisostds.org/ontologies/C2SIM#hasReportID">
        <rdfs:subPropertyOf rdf:resource="http://www.sisostds.org/ontologies/C2SIM#hasMessagingDataProperty"/>
        <rdfs:range rdf:resource="http://www.sisostds.org/ontologies/C2SIM#UUIDBase"/>
    </owl:DatatypeProperty>
    


    <!-- http://www.sisostds.org/ontologies/C2SIM#hasReportingEntity -->

    <owl:DatatypeProperty rdf:about="http://www.sisostds.org/ontologies/C2SIM#hasReportingEntity">
        <rdfs:subPropertyOf rdf:resource="http://www.sisostds.org/ontologies/C2SIM#hasActorReference"/>
        <rdfs:range rdf:resource="http://www.sisostds.org/ontologies/C2SIM#UUIDBase"/>
        <rdfs:comment>The reference is to an instance of ReportingEntity.</rdfs:comment>
    </owl:DatatypeProperty>
    


    <!-- http://www.sisostds.org/ontologies/C2SIM#hasRequestingEntity -->

    <owl:DatatypeProperty rdf:about="http://www.sisostds.org/ontologies/C2SIM#hasRequestingEntity">
        <rdfs:subPropertyOf rdf:resource="http://www.sisostds.org/ontologies/C2SIM#hasActorReference"/>
        <rdfs:range rdf:resource="http://www.sisostds.org/ontologies/C2SIM#UUIDBase"/>
        <rdfs:comment>The reference is to an instance of RequestingEntity.</rdfs:comment>
    </owl:DatatypeProperty>
    


    <!-- http://www.sisostds.org/ontologies/C2SIM#hasRequiredOnHandQuantity -->

    <owl:DatatypeProperty rdf:about="http://www.sisostds.org/ontologies/C2SIM#hasRequiredOnHandQuantity">
        <rdfs:range rdf:resource="http://www.w3.org/2001/XMLSchema#double"/>
        <rdfs:comment>Required number of specific resources that a Resource must have available for operations.</rdfs:comment>
    </owl:DatatypeProperty>
    


    <!-- http://www.sisostds.org/ontologies/C2SIM#hasSimulationRealtimeMultiple -->

    <owl:DatatypeProperty rdf:about="http://www.sisostds.org/ontologies/C2SIM#hasSimulationRealtimeMultiple">
        <rdfs:range rdf:resource="http://www.sisostds.org/ontologies/C2SIM#simulationRealtimeMultiple"/>
        <rdfs:comment>Decimal rate indicating ratio of simulation time to real time (e.g., value of 2.0 indicates simulation is executing at 2:1 simulation time to realtime [i.e., faster than realtime]; 0.5 indicates simulation  is executing at half realtime [i.e., slower than realtime]).</rdfs:comment>
    </owl:DatatypeProperty>
    


    <!-- http://www.sisostds.org/ontologies/C2SIM#hasSpatialMeasure -->

    <owl:DatatypeProperty rdf:about="http://www.sisostds.org/ontologies/C2SIM#hasSpatialMeasure">
        <rdfs:comment>Properties that provide geospatial data values for instances of the class.</rdfs:comment>
    </owl:DatatypeProperty>
    


    <!-- http://www.sisostds.org/ontologies/C2SIM#hasSpeed -->

    <owl:DatatypeProperty rdf:about="http://www.sisostds.org/ontologies/C2SIM#hasSpeed">
        <rdfs:subPropertyOf rdf:resource="http://www.sisostds.org/ontologies/C2SIM#hasSpatialMeasure"/>
        <rdfs:range rdf:resource="http://www.w3.org/2001/XMLSchema#double"/>
        <rdfs:comment>Speed in meters/second.</rdfs:comment>
    </owl:DatatypeProperty>
    


    <!-- http://www.sisostds.org/ontologies/C2SIM#hasStrengthPercentage -->

    <owl:DatatypeProperty rdf:about="http://www.sisostds.org/ontologies/C2SIM#hasStrengthPercentage">
        <rdfs:subPropertyOf rdf:resource="http://www.w3.org/2002/07/owl#topDataProperty"/>
        <rdfs:range rdf:resource="http://www.sisostds.org/ontologies/C2SIM#percentage"/>
        <rdfs:comment>The HealthStatus includes a value for Strength Percentage as a fraction of expected maximum numerical strength; vlue should be in range 0 to 100.</rdfs:comment>
    </owl:DatatypeProperty>
    


    <!-- http://www.sisostds.org/ontologies/C2SIM#hasSubjectEntity -->

    <owl:DatatypeProperty rdf:about="http://www.sisostds.org/ontologies/C2SIM#hasSubjectEntity">
        <rdfs:subPropertyOf rdf:resource="http://www.sisostds.org/ontologies/C2SIM#hasActorReference"/>
        <rdfs:range rdf:resource="http://www.sisostds.org/ontologies/C2SIM#UUIDBase"/>
        <rdfs:comment>The reference is to an instance of SubjectEntity.</rdfs:comment>
    </owl:DatatypeProperty>
    


    <!-- http://www.sisostds.org/ontologies/C2SIM#hasSubordinate -->

    <owl:DatatypeProperty rdf:about="http://www.sisostds.org/ontologies/C2SIM#hasSubordinate">
        <rdfs:subPropertyOf rdf:resource="http://www.sisostds.org/ontologies/C2SIM#hasActorReference"/>
        <rdfs:range rdf:resource="http://www.sisostds.org/ontologies/C2SIM#UUIDBase"/>
        <rdfs:comment>The reference is to an instance of Entity that is subordinate for purposes of the class.</rdfs:comment>
    </owl:DatatypeProperty>
    


    <!-- http://www.sisostds.org/ontologies/C2SIM#hasSuperior -->

    <owl:DatatypeProperty rdf:about="http://www.sisostds.org/ontologies/C2SIM#hasSuperior">
        <rdfs:subPropertyOf rdf:resource="http://www.sisostds.org/ontologies/C2SIM#hasActorReference"/>
        <rdfs:range rdf:resource="http://www.sisostds.org/ontologies/C2SIM#UUIDBase"/>
        <rdfs:comment>The reference is to an instance of Entity that is superior (that is, has authority to provide direction) for purposes of the class.</rdfs:comment>
    </owl:DatatypeProperty>
    


    <!-- http://www.sisostds.org/ontologies/C2SIM#hasSystemName -->

    <owl:DatatypeProperty rdf:about="http://www.sisostds.org/ontologies/C2SIM#hasSystemName">
        <rdfs:subPropertyOf rdf:resource="http://www.sisostds.org/ontologies/C2SIM#hasName"/>
        <rdfs:range rdf:resource="http://www.w3.org/2001/XMLSchema#string"/>
        <rdfs:comment>Instances of the class have an alphanumeric name for a system implementing C2SIM, unique within the class, that also serve symbolically for humans to recognize the instance.</rdfs:comment>
    </owl:DatatypeProperty>
    


    <!-- http://www.sisostds.org/ontologies/C2SIM#hasTaskID -->

    <owl:DatatypeProperty rdf:about="http://www.sisostds.org/ontologies/C2SIM#hasTaskID">
        <rdfs:subPropertyOf rdf:resource="http://www.sisostds.org/ontologies/C2SIM#hasTaskReference"/>
        <rdfs:range rdf:resource="http://www.sisostds.org/ontologies/C2SIM#UUIDBase"/>
        <rdfs:comment>Reference UUID to a defined Task instance.</rdfs:comment>
    </owl:DatatypeProperty>
    


    <!-- http://www.sisostds.org/ontologies/C2SIM#hasTaskReference -->

    <owl:DatatypeProperty rdf:about="http://www.sisostds.org/ontologies/C2SIM#hasTaskReference">
        <rdfs:subPropertyOf rdf:resource="http://www.sisostds.org/ontologies/C2SIM#hasActionReference"/>
        <rdfs:range rdf:resource="http://www.sisostds.org/ontologies/C2SIM#UUIDBase"/>
        <rdfs:comment>The reference is to another class identifying a Task.</rdfs:comment>
    </owl:DatatypeProperty>
    


    <!-- http://www.sisostds.org/ontologies/C2SIM#hasTasker -->

    <owl:DatatypeProperty rdf:about="http://www.sisostds.org/ontologies/C2SIM#hasTasker">
        <rdfs:subPropertyOf rdf:resource="http://www.sisostds.org/ontologies/C2SIM#hasActorReference"/>
        <rdfs:range rdf:resource="http://www.sisostds.org/ontologies/C2SIM#UUIDBase"/>
        <rdfs:comment>Reference to the UUID of the entity ordering another entity to perform a task.</rdfs:comment>
    </owl:DatatypeProperty>
    


    <!-- http://www.sisostds.org/ontologies/C2SIM#hasTemporalAssociationWithAction -->

    <owl:DatatypeProperty rdf:about="http://www.sisostds.org/ontologies/C2SIM#hasTemporalAssociationWithAction">
        <rdfs:subPropertyOf rdf:resource="http://www.sisostds.org/ontologies/C2SIM#hasActionReference"/>
        <rdfs:range rdf:resource="http://www.sisostds.org/ontologies/C2SIM#UUIDBase"/>
        <rdfs:comment>The object action with which the subject action has a temporal association (relationship)</rdfs:comment>
    </owl:DatatypeProperty>
    


    <!-- http://www.sisostds.org/ontologies/C2SIM#hasTheta -->

    <owl:DatatypeProperty rdf:about="http://www.sisostds.org/ontologies/C2SIM#hasTheta">
        <rdfs:subPropertyOf rdf:resource="http://www.sisostds.org/ontologies/C2SIM#hasAngle"/>
        <rdfs:range rdf:resource="http://www.w3.org/2001/XMLSchema#double"/>
        <rdfs:comment>Property of geospatial data value that represents Euler Angle Theta in radians.</rdfs:comment>
    </owl:DatatypeProperty>
    


    <!-- http://www.sisostds.org/ontologies/C2SIM#hasTimeSincePlaybackStart -->

    <owl:DatatypeProperty rdf:about="http://www.sisostds.org/ontologies/C2SIM#hasTimeSincePlaybackStart">
        <rdfs:range rdf:resource="http://www.sisostds.org/ontologies/C2SIM#IsoTimeDurationBase"/>
        <rdfs:comment>Gives the time duration (isoTimeDurationBase) since the start time of the current playback; i.e., the message timestamp that the playback has reached. Used in reporting the status of a current playback of recorded C2SIM messages.</rdfs:comment>
    </owl:DatatypeProperty>
    


    <!-- http://www.sisostds.org/ontologies/C2SIM#hasUUID -->

    <owl:DatatypeProperty rdf:about="http://www.sisostds.org/ontologies/C2SIM#hasUUID">
        <rdfs:subPropertyOf rdf:resource="http://www.sisostds.org/ontologies/C2SIM#hasUniqueIdentifier"/>
        <rdfs:range rdf:resource="http://www.sisostds.org/ontologies/C2SIM#UUIDBase"/>
        <rdfs:comment>A unique identifier in UUID format.</rdfs:comment>
    </owl:DatatypeProperty>
    


    <!-- http://www.sisostds.org/ontologies/C2SIM#hasUniqueIdentifier -->

    <owl:DatatypeProperty rdf:about="http://www.sisostds.org/ontologies/C2SIM#hasUniqueIdentifier">
        <rdfs:comment>Property of a class for which all instances have a unique identifier.</rdfs:comment>
    </owl:DatatypeProperty>
    


    <!-- http://www.sisostds.org/ontologies/C2SIM#hasUp -->

    <owl:DatatypeProperty rdf:about="http://www.sisostds.org/ontologies/C2SIM#hasUp">
        <rdfs:subPropertyOf rdf:resource="http://www.sisostds.org/ontologies/C2SIM#hasCoordinateValue"/>
        <rdfs:range rdf:resource="http://www.w3.org/2001/XMLSchema#double"/>
        <rdfs:comment>Value for Up coordinate is included.</rdfs:comment>
    </owl:DatatypeProperty>
    


    <!-- http://www.sisostds.org/ontologies/C2SIM#hasVersion -->

    <owl:DatatypeProperty rdf:about="http://www.sisostds.org/ontologies/C2SIM#hasVersion">
        <rdfs:range rdf:resource="http://www.w3.org/2001/XMLSchema#string"/>
        <rdfs:comment>Property of a class for which all instances have a unique identifier that represents a version.</rdfs:comment>
    </owl:DatatypeProperty>
    


    <!-- http://www.sisostds.org/ontologies/C2SIM#hasWidth -->

    <owl:DatatypeProperty rdf:about="http://www.sisostds.org/ontologies/C2SIM#hasWidth">
        <rdfs:subPropertyOf rdf:resource="http://www.sisostds.org/ontologies/C2SIM#hasDistance"/>
        <rdfs:range rdf:resource="http://www.w3.org/2001/XMLSchema#double"/>
        <rdfs:comment>Property of geospatial data value that represents width aspect of a distance in meters.</rdfs:comment>
    </owl:DatatypeProperty>
    


    <!-- http://www.sisostds.org/ontologies/C2SIM#isAffiliatedWith -->

    <owl:DatatypeProperty rdf:about="http://www.sisostds.org/ontologies/C2SIM#isAffiliatedWith">
        <rdfs:subPropertyOf rdf:resource="http://www.sisostds.org/ontologies/C2SIM#hasAbstractOrganizationReference"/>
        <rdfs:range rdf:resource="http://www.sisostds.org/ontologies/C2SIM#UUIDBase"/>
        <rdfs:comment>Indicates an AbstractOrganization that the entity is affiliated with in some way.</rdfs:comment>
    </owl:DatatypeProperty>
    


    <!-- http://www.sisostds.org/ontologies/C2SIM#isFromSender -->

    <owl:DatatypeProperty rdf:about="http://www.sisostds.org/ontologies/C2SIM#isFromSender">
        <rdfs:subPropertyOf rdf:resource="http://www.sisostds.org/ontologies/C2SIM#hasActorReference"/>
        <rdfs:range rdf:resource="http://www.sisostds.org/ontologies/C2SIM#UUIDBase"/>
        <rdfs:comment>The reference is to an instance of Entity that sent associated information.</rdfs:comment>
    </owl:DatatypeProperty>
    


    <!-- http://www.sisostds.org/ontologies/C2SIM#isFromSendingSystem -->

    <owl:DatatypeProperty rdf:about="http://www.sisostds.org/ontologies/C2SIM#isFromSendingSystem">
        <rdfs:subPropertyOf rdf:resource="http://www.sisostds.org/ontologies/C2SIM#hasMessagingDataProperty"/>
        <rdfs:range rdf:resource="http://www.w3.org/2001/XMLSchema#string"/>
        <rdfs:comment>Unique FIPA identifer of the system from which individual message is sent.</rdfs:comment>
    </owl:DatatypeProperty>
    


    <!-- http://www.sisostds.org/ontologies/C2SIM#isInReplyToMessageID -->

    <owl:DatatypeProperty rdf:about="http://www.sisostds.org/ontologies/C2SIM#isInReplyToMessageID">
        <rdfs:subPropertyOf rdf:resource="http://www.sisostds.org/ontologies/C2SIM#hasMessagingDataProperty"/>
        <rdfs:range rdf:resource="http://www.sisostds.org/ontologies/C2SIM#UUIDBase"/>
        <rdfs:comment>Unique FIPA identifer of the message to be identified in a message reply.</rdfs:comment>
    </owl:DatatypeProperty>
    


    <!-- http://www.sisostds.org/ontologies/C2SIM#isToReceiver -->

    <owl:DatatypeProperty rdf:about="http://www.sisostds.org/ontologies/C2SIM#isToReceiver">
        <rdfs:subPropertyOf rdf:resource="http://www.sisostds.org/ontologies/C2SIM#hasActorReference"/>
        <rdfs:range rdf:resource="http://www.sisostds.org/ontologies/C2SIM#UUIDBase"/>
        <rdfs:comment>The reference is to an instance of Entity that intended to receive the associated information.</rdfs:comment>
    </owl:DatatypeProperty>
    


    <!-- http://www.sisostds.org/ontologies/C2SIM#isToReceivingSystem -->

    <owl:DatatypeProperty rdf:about="http://www.sisostds.org/ontologies/C2SIM#isToReceivingSystem">
        <rdfs:subPropertyOf rdf:resource="http://www.sisostds.org/ontologies/C2SIM#hasMessagingDataProperty"/>
        <rdfs:range rdf:resource="http://www.w3.org/2001/XMLSchema#string"/>
        <rdfs:comment>Unique FIPA identifer of the system to which individual message is sent.</rdfs:comment>
    </owl:DatatypeProperty>
    


    <!-- http://www.sisostds.org/ontologies/lox#hasFunctionalAssociationWithTask -->

    <owl:DatatypeProperty rdf:about="http://www.sisostds.org/ontologies/lox#hasFunctionalAssociationWithTask">
        <rdfs:subPropertyOf rdf:resource="http://www.sisostds.org/ontologies/C2SIM#hasTaskReference"/>
        <rdfs:range rdf:resource="http://www.sisostds.org/ontologies/C2SIM#UUIDBase"/>
        <rdfs:comment>This property identifies the UUID of a Maneuver Warfare Task that is the object of a JC3IEDM ActionFunctionalAssociation.</rdfs:comment>
    </owl:DatatypeProperty>
    


    <!-- http://www.sisostds.org/ontologies/lox#hasPlanPhaseReference -->

    <owl:DatatypeProperty rdf:about="http://www.sisostds.org/ontologies/lox#hasPlanPhaseReference">
        <rdfs:subPropertyOf rdf:resource="http://www.sisostds.org/ontologies/C2SIM#hasReference"/>
        <rdfs:range rdf:resource="http://www.sisostds.org/ontologies/C2SIM#UUIDBase"/>
        <rdfs:comment>A reference to a plan phase.</rdfs:comment>
    </owl:DatatypeProperty>
    


    <!-- http://www.sisostds.org/ontologies/lox#hasText -->

    <owl:DatatypeProperty rdf:about="http://www.sisostds.org/ontologies/lox#hasText">
        <rdfs:range rdf:resource="http://www.w3.org/2001/XMLSchema#string"/>
        <rdfs:comment>Provides a Text annotation as part on an Object.</rdfs:comment>
    </owl:DatatypeProperty>
    


    <!-- http://www.sisostds.org/ontologies/lox#hasTriggerPhase -->

    <owl:DatatypeProperty rdf:about="http://www.sisostds.org/ontologies/lox#hasTriggerPhase">
        <rdfs:range rdf:resource="http://www.sisostds.org/ontologies/C2SIM#UUIDBase"/>
        <rdfs:comment>Provides a phase to trigger another phase in an LOX Plan.</rdfs:comment>
    </owl:DatatypeProperty>
    


    <!-- http://www.sisostds.org/ontologies/lox#isToBeExecutedNow -->

    <owl:DatatypeProperty rdf:about="http://www.sisostds.org/ontologies/lox#isToBeExecutedNow">
        <rdfs:range rdf:resource="http://www.w3.org/2001/XMLSchema#boolean"/>
        <rdfs:comment>Indicates an LOX Task or Activity to be excuted at this time.</rdfs:comment>
    </owl:DatatypeProperty>
    


    <!-- http://www.sisostds.org/ontologies/smx#hasAPP6C-SIDC -->

    <owl:DatatypeProperty rdf:about="http://www.sisostds.org/ontologies/smx#hasAPP6C-SIDC">
        <rdfs:range rdf:resource="http://www.sisostds.org/ontologies/smx#SymbolIDCodeString"/>
        <rdfs:comment>Provides a SIDC (Symbol Identification Code) string associated with the NATO APP-6-C Tactical Graphics symbol.</rdfs:comment>
    </owl:DatatypeProperty>
    


    <!-- http://www.sisostds.org/ontologies/smx#hasConfidenceLevel -->

    <owl:DatatypeProperty rdf:about="http://www.sisostds.org/ontologies/smx#hasConfidenceLevel">
        <rdfs:range rdf:resource="http://www.w3.org/2001/XMLSchema#double"/>
        <rdfs:comment>Provides a confidence level associated with a class, from a range of values.</rdfs:comment>
    </owl:DatatypeProperty>
    


    <!-- http://www.sisostds.org/ontologies/smx#hasHigherFormation -->

    <owl:DatatypeProperty rdf:about="http://www.sisostds.org/ontologies/smx#hasHigherFormation">
        <rdfs:range rdf:resource="http://www.w3.org/2001/XMLSchema#string"/>
        <rdfs:comment>The higher formation information associated with a unit tactical graphic.</rdfs:comment>
    </owl:DatatypeProperty>
    


    <!-- http://www.sisostds.org/ontologies/smx#hasOtherSide -->

    <owl:DatatypeProperty rdf:about="http://www.sisostds.org/ontologies/smx#hasOtherSide">
        <rdfs:subPropertyOf rdf:resource="http://www.sisostds.org/ontologies/C2SIM#hasAbstractObjectReference"/>
        <rdfs:range rdf:resource="http://www.sisostds.org/ontologies/C2SIM#UUIDBase"/>
    </owl:DatatypeProperty>
    


    <!-- http://www.sisostds.org/ontologies/smx#hasOwner -->

    <owl:DatatypeProperty rdf:about="http://www.sisostds.org/ontologies/smx#hasOwner">
        <rdfs:subPropertyOf rdf:resource="http://www.sisostds.org/ontologies/C2SIM#hasAbstractObjectReference"/>
        <rdfs:range rdf:resource="http://www.sisostds.org/ontologies/C2SIM#UUIDBase"/>
        <rdfs:comment>Provides a reference to the Owner associated with a class.</rdfs:comment>
    </owl:DatatypeProperty>
    


    <!-- http://www.sisostds.org/ontologies/smx#hasSide -->

    <owl:DatatypeProperty rdf:about="http://www.sisostds.org/ontologies/smx#hasSide">
        <rdfs:subPropertyOf rdf:resource="http://www.sisostds.org/ontologies/C2SIM#hasAbstractObjectReference"/>
        <rdfs:range rdf:resource="http://www.sisostds.org/ontologies/C2SIM#UUIDBase"/>
        <rdfs:comment>Provides a reference to the ForceSide associated with a class.</rdfs:comment>
    </owl:DatatypeProperty>
    


    <!-- http://www.sisostds.org/ontologies/smx#hasSpecialC2HQ -->

    <owl:DatatypeProperty rdf:about="http://www.sisostds.org/ontologies/smx#hasSpecialC2HQ">
        <rdfs:range rdf:resource="http://www.w3.org/2001/XMLSchema#string"/>
        <rdfs:comment>Provides a reference to aSpecial Comamnd and Control Headquarter for a military Entity.</rdfs:comment>
    </owl:DatatypeProperty>
    


    <!-- http://www.sisostds.org/ontologies/smx#hasUncertaintyInterval -->

    <owl:DatatypeProperty rdf:about="http://www.sisostds.org/ontologies/smx#hasUncertaintyInterval">
        <rdfs:range rdf:resource="http://www.w3.org/2001/XMLSchema#double"/>
        <rdfs:comment>Provides a value of Uncertainty Interval for the quantity in a class.</rdfs:comment>
    </owl:DatatypeProperty>
    


    <!-- 
    ///////////////////////////////////////////////////////////////////////////////////////
    //
    // Classes
    //
    ///////////////////////////////////////////////////////////////////////////////////////
     -->

    


    <!-- http://www.sisostds.org/ontologies/C2SIM#AbstractObject -->

    <owl:Class rdf:about="http://www.sisostds.org/ontologies/C2SIM#AbstractObject">
        <rdfs:subClassOf rdf:resource="http://www.sisostds.org/ontologies/C2SIM#C2SIMContent"/>
        <rdfs:subClassOf>
            <owl:Restriction>
                <owl:onProperty rdf:resource="http://www.sisostds.org/ontologies/C2SIM#hasName"/>
                <owl:minQualifiedCardinality rdf:datatype="http://www.w3.org/2001/XMLSchema#nonNegativeInteger">0</owl:minQualifiedCardinality>
                <owl:onDataRange rdf:resource="http://www.w3.org/2001/XMLSchema#string"/>
            </owl:Restriction>
        </rdfs:subClassOf>
        <rdfs:subClassOf>
            <owl:Restriction>
                <owl:onProperty rdf:resource="http://www.sisostds.org/ontologies/C2SIM#hasUUID"/>
                <owl:qualifiedCardinality rdf:datatype="http://www.w3.org/2001/XMLSchema#nonNegativeInteger">1</owl:qualifiedCardinality>
                <owl:onDataRange rdf:resource="http://www.sisostds.org/ontologies/C2SIM#UUIDBase"/>
            </owl:Restriction>
        </rdfs:subClassOf>
        <rdfs:comment>An AbstractObject is an object in the system that does not have the full characteristics of an entity. For example, it does not have a location or an extent. It does however have a unique identifier.</rdfs:comment>
    </owl:Class>
    <owl:Axiom>
        <owl:annotatedSource rdf:resource="http://www.sisostds.org/ontologies/C2SIM#AbstractObject"/>
        <owl:annotatedProperty rdf:resource="http://www.w3.org/2000/01/rdf-schema#subClassOf"/>
        <owl:annotatedTarget>
            <owl:Restriction>
                <owl:onProperty rdf:resource="http://www.sisostds.org/ontologies/C2SIM#hasUUID"/>
                <owl:qualifiedCardinality rdf:datatype="http://www.w3.org/2001/XMLSchema#nonNegativeInteger">1</owl:qualifiedCardinality>
                <owl:onDataRange rdf:resource="http://www.sisostds.org/ontologies/C2SIM#UUIDBase"/>
            </owl:Restriction>
        </owl:annotatedTarget>
        <rdfs:comment>This is the unique identifier of an individual in this class.</rdfs:comment>
    </owl:Axiom>
    


    <!-- http://www.sisostds.org/ontologies/C2SIM#AbstractOrganization -->

    <owl:Class rdf:about="http://www.sisostds.org/ontologies/C2SIM#AbstractOrganization">
        <rdfs:subClassOf rdf:resource="http://www.sisostds.org/ontologies/C2SIM#AbstractObject"/>
        <rdfs:subClassOf>
            <owl:Restriction>
                <owl:onProperty rdf:resource="http://www.sisostds.org/ontologies/C2SIM#hasOrganizationTypeCode"/>
                <owl:qualifiedCardinality rdf:datatype="http://www.w3.org/2001/XMLSchema#nonNegativeInteger">1</owl:qualifiedCardinality>
                <owl:onClass rdf:resource="http://www.sisostds.org/ontologies/C2SIM#OrganizationTypeCode"/>
            </owl:Restriction>
        </rdfs:subClassOf>
        <rdfs:subClassOf>
            <owl:Restriction>
                <owl:onProperty rdf:resource="http://www.sisostds.org/ontologies/C2SIM#hasCountryCode"/>
                <owl:maxQualifiedCardinality rdf:datatype="http://www.w3.org/2001/XMLSchema#nonNegativeInteger">1</owl:maxQualifiedCardinality>
                <owl:onClass rdf:resource="http://www.sisostds.org/ontologies/C2SIM#CountryCode"/>
            </owl:Restriction>
        </rdfs:subClassOf>
        <rdfs:subClassOf>
            <owl:Restriction>
                <owl:onProperty rdf:resource="http://www.sisostds.org/ontologies/C2SIM#hasEthnicGroupCode"/>
                <owl:maxQualifiedCardinality rdf:datatype="http://www.w3.org/2001/XMLSchema#nonNegativeInteger">1</owl:maxQualifiedCardinality>
                <owl:onClass rdf:resource="http://www.sisostds.org/ontologies/C2SIM#EthnicGroupCode"/>
            </owl:Restriction>
        </rdfs:subClassOf>
        <rdfs:subClassOf>
            <owl:Restriction>
                <owl:onProperty rdf:resource="http://www.sisostds.org/ontologies/C2SIM#hasReligionCode"/>
                <owl:maxQualifiedCardinality rdf:datatype="http://www.w3.org/2001/XMLSchema#nonNegativeInteger">1</owl:maxQualifiedCardinality>
                <owl:onClass rdf:resource="http://www.sisostds.org/ontologies/C2SIM#ReligionCode"/>
            </owl:Restriction>
        </rdfs:subClassOf>
        <rdfs:comment>A group that an actor can be affiliated with. Does not perform any actions and does not have a specific location.
Subclasses of this class can be created for country, religion, etc. Each of these will have defined instances (one for each country, etc.)</rdfs:comment>
    </owl:Class>
    


    <!-- http://www.sisostds.org/ontologies/C2SIM#AcknowledgeTypeCode -->

    <owl:Class rdf:about="http://www.sisostds.org/ontologies/C2SIM#AcknowledgeTypeCode">
        <rdfs:subClassOf rdf:resource="http://www.sisostds.org/ontologies/C2SIM#MessageCode"/>
        <rdfs:comment>Enumeration of different types of acknowledgements.</rdfs:comment>
    </owl:Class>
    


    <!-- http://www.sisostds.org/ontologies/C2SIM#AcknowledgementBody -->

    <owl:Class rdf:about="http://www.sisostds.org/ontologies/C2SIM#AcknowledgementBody">
        <rdfs:subClassOf rdf:resource="http://www.sisostds.org/ontologies/C2SIM#DomainMessageBody"/>
        <rdfs:subClassOf>
            <owl:Restriction>
                <owl:onProperty rdf:resource="http://www.sisostds.org/ontologies/C2SIM#hasAcknowledgeTypeCode"/>
                <owl:qualifiedCardinality rdf:datatype="http://www.w3.org/2001/XMLSchema#nonNegativeInteger">1</owl:qualifiedCardinality>
                <owl:onClass rdf:resource="http://www.sisostds.org/ontologies/C2SIM#AcknowledgeTypeCode"/>
            </owl:Restriction>
        </rdfs:subClassOf>
        <rdfs:comment>An acknowledgement from one Actor to another that a message was received.</rdfs:comment>
    </owl:Class>
    


    <!-- http://www.sisostds.org/ontologies/C2SIM#Action -->

    <owl:Class rdf:about="http://www.sisostds.org/ontologies/C2SIM#Action">
        <rdfs:subClassOf rdf:resource="http://www.sisostds.org/ontologies/C2SIM#C2SIMContent"/>
        <rdfs:subClassOf>
            <owl:Restriction>
                <owl:onProperty rdf:resource="http://www.sisostds.org/ontologies/C2SIM#hasActionTemporalRelationship"/>
                <owl:minQualifiedCardinality rdf:datatype="http://www.w3.org/2001/XMLSchema#nonNegativeInteger">0</owl:minQualifiedCardinality>
                <owl:onClass rdf:resource="http://www.sisostds.org/ontologies/C2SIM#ActionTemporalRelationship"/>
            </owl:Restriction>
        </rdfs:subClassOf>
        <rdfs:subClassOf>
            <owl:Restriction>
                <owl:onProperty rdf:resource="http://www.sisostds.org/ontologies/C2SIM#hasLocation"/>
                <owl:minQualifiedCardinality rdf:datatype="http://www.w3.org/2001/XMLSchema#nonNegativeInteger">0</owl:minQualifiedCardinality>
                <owl:onClass rdf:resource="http://www.sisostds.org/ontologies/C2SIM#Location"/>
            </owl:Restriction>
        </rdfs:subClassOf>
        <rdfs:subClassOf>
            <owl:Restriction>
                <owl:onProperty rdf:resource="http://www.sisostds.org/ontologies/C2SIM#hasMapGraphicID"/>
                <owl:minQualifiedCardinality rdf:datatype="http://www.w3.org/2001/XMLSchema#nonNegativeInteger">0</owl:minQualifiedCardinality>
                <owl:onDataRange rdf:resource="http://www.sisostds.org/ontologies/C2SIM#UUIDBase"/>
            </owl:Restriction>
        </rdfs:subClassOf>
        <rdfs:subClassOf>
            <owl:Restriction>
                <owl:onProperty rdf:resource="http://www.sisostds.org/ontologies/C2SIM#hasUUID"/>
                <owl:qualifiedCardinality rdf:datatype="http://www.w3.org/2001/XMLSchema#nonNegativeInteger">1</owl:qualifiedCardinality>
                <owl:onDataRange rdf:resource="http://www.sisostds.org/ontologies/C2SIM#UUIDBase"/>
            </owl:Restriction>
        </rdfs:subClassOf>
        <rdfs:subClassOf>
            <owl:Restriction>
                <owl:onProperty rdf:resource="http://www.sisostds.org/ontologies/C2SIM#hasName"/>
                <owl:maxQualifiedCardinality rdf:datatype="http://www.w3.org/2001/XMLSchema#nonNegativeInteger">1</owl:maxQualifiedCardinality>
                <owl:onDataRange rdf:resource="http://www.w3.org/2001/XMLSchema#string"/>
            </owl:Restriction>
        </rdfs:subClassOf>
        <rdfs:comment>Any occurrence that occurs at a moment in time or over a period of time.</rdfs:comment>
    </owl:Class>
    <owl:Axiom>
        <owl:annotatedSource rdf:resource="http://www.sisostds.org/ontologies/C2SIM#Action"/>
        <owl:annotatedProperty rdf:resource="http://www.w3.org/2000/01/rdf-schema#subClassOf"/>
        <owl:annotatedTarget>
            <owl:Restriction>
                <owl:onProperty rdf:resource="http://www.sisostds.org/ontologies/C2SIM#hasLocation"/>
                <owl:minQualifiedCardinality rdf:datatype="http://www.w3.org/2001/XMLSchema#nonNegativeInteger">0</owl:minQualifiedCardinality>
                <owl:onClass rdf:resource="http://www.sisostds.org/ontologies/C2SIM#Location"/>
            </owl:Restriction>
        </owl:annotatedTarget>
        <rdfs:comment>The general location of the task, if that makes sense. Specification of multiple locations where events of the task take place is normally done with map graphics.</rdfs:comment>
    </owl:Axiom>
    <owl:Axiom>
        <owl:annotatedSource rdf:resource="http://www.sisostds.org/ontologies/C2SIM#Action"/>
        <owl:annotatedProperty rdf:resource="http://www.w3.org/2000/01/rdf-schema#subClassOf"/>
        <owl:annotatedTarget>
            <owl:Restriction>
                <owl:onProperty rdf:resource="http://www.sisostds.org/ontologies/C2SIM#hasMapGraphicID"/>
                <owl:minQualifiedCardinality rdf:datatype="http://www.w3.org/2001/XMLSchema#nonNegativeInteger">0</owl:minQualifiedCardinality>
                <owl:onDataRange rdf:resource="http://www.sisostds.org/ontologies/C2SIM#UUIDBase"/>
            </owl:Restriction>
        </owl:annotatedTarget>
        <rdfs:comment>This is a reference to a MapGraphic individual defined elsewhere.</rdfs:comment>
    </owl:Axiom>
    <owl:Axiom>
        <owl:annotatedSource rdf:resource="http://www.sisostds.org/ontologies/C2SIM#Action"/>
        <owl:annotatedProperty rdf:resource="http://www.w3.org/2000/01/rdf-schema#subClassOf"/>
        <owl:annotatedTarget>
            <owl:Restriction>
                <owl:onProperty rdf:resource="http://www.sisostds.org/ontologies/C2SIM#hasUUID"/>
                <owl:qualifiedCardinality rdf:datatype="http://www.w3.org/2001/XMLSchema#nonNegativeInteger">1</owl:qualifiedCardinality>
                <owl:onDataRange rdf:resource="http://www.sisostds.org/ontologies/C2SIM#UUIDBase"/>
            </owl:Restriction>
        </owl:annotatedTarget>
        <rdfs:comment>This is the unique identifier of an individual in this class.</rdfs:comment>
    </owl:Axiom>
    


    <!-- http://www.sisostds.org/ontologies/C2SIM#ActionCode -->

    <owl:Class rdf:about="http://www.sisostds.org/ontologies/C2SIM#ActionCode">
        <rdfs:subClassOf rdf:resource="http://www.sisostds.org/ontologies/C2SIM#Code"/>
        <rdfs:comment>An enumeration describing what the action is.</rdfs:comment>
    </owl:Class>
    


    <!-- http://www.sisostds.org/ontologies/C2SIM#ActionTemporalAssociationCode -->

    <owl:Class rdf:about="http://www.sisostds.org/ontologies/C2SIM#ActionTemporalAssociationCode">
        <rdfs:subClassOf rdf:resource="http://www.sisostds.org/ontologies/C2SIM#Code"/>
        <rdfs:comment>An enumeration describing the temporal relationship between two actions.</rdfs:comment>
    </owl:Class>
    


    <!-- http://www.sisostds.org/ontologies/C2SIM#ActionTemporalRelationship -->

    <owl:Class rdf:about="http://www.sisostds.org/ontologies/C2SIM#ActionTemporalRelationship">
        <rdfs:subClassOf rdf:resource="http://www.sisostds.org/ontologies/C2SIM#Relationship"/>
        <rdfs:subClassOf>
            <owl:Restriction>
                <owl:onProperty rdf:resource="http://www.sisostds.org/ontologies/C2SIM#hasActionTemporalAssociationCode"/>
                <owl:qualifiedCardinality rdf:datatype="http://www.w3.org/2001/XMLSchema#nonNegativeInteger">1</owl:qualifiedCardinality>
                <owl:onClass rdf:resource="http://www.sisostds.org/ontologies/C2SIM#ActionTemporalAssociationCode"/>
            </owl:Restriction>
        </rdfs:subClassOf>
        <rdfs:subClassOf>
            <owl:Restriction>
                <owl:onProperty rdf:resource="http://www.sisostds.org/ontologies/C2SIM#hasDuration"/>
                <owl:maxQualifiedCardinality rdf:datatype="http://www.w3.org/2001/XMLSchema#nonNegativeInteger">1</owl:maxQualifiedCardinality>
                <owl:onClass rdf:resource="http://www.sisostds.org/ontologies/C2SIM#Duration"/>
            </owl:Restriction>
        </rdfs:subClassOf>
        <rdfs:subClassOf>
            <owl:Restriction>
                <owl:onProperty rdf:resource="http://www.sisostds.org/ontologies/C2SIM#hasTemporalAssociationWithAction"/>
                <owl:qualifiedCardinality rdf:datatype="http://www.w3.org/2001/XMLSchema#nonNegativeInteger">1</owl:qualifiedCardinality>
                <owl:onDataRange rdf:resource="http://www.sisostds.org/ontologies/C2SIM#UUIDBase"/>
            </owl:Restriction>
        </rdfs:subClassOf>
        <rdfs:comment>A temporal relationship between two actions. Some relationships involve a time duration.</rdfs:comment>
    </owl:Class>
    


    <!-- http://www.sisostds.org/ontologies/C2SIM#ActorEntity -->

    <owl:Class rdf:about="http://www.sisostds.org/ontologies/C2SIM#ActorEntity">
        <rdfs:subClassOf rdf:resource="http://www.sisostds.org/ontologies/C2SIM#Entity"/>
        <rdfs:subClassOf>
            <owl:Restriction>
                <owl:onProperty rdf:resource="http://www.sisostds.org/ontologies/C2SIM#hasResource"/>
                <owl:minQualifiedCardinality rdf:datatype="http://www.w3.org/2001/XMLSchema#nonNegativeInteger">0</owl:minQualifiedCardinality>
                <owl:onClass rdf:resource="http://www.sisostds.org/ontologies/C2SIM#Resource"/>
            </owl:Restriction>
        </rdfs:subClassOf>
        <rdfs:subClassOf>
            <owl:Restriction>
                <owl:onProperty rdf:resource="http://www.sisostds.org/ontologies/C2SIM#hasEntityDescriptor"/>
                <owl:qualifiedCardinality rdf:datatype="http://www.w3.org/2001/XMLSchema#nonNegativeInteger">1</owl:qualifiedCardinality>
                <owl:onClass rdf:resource="http://www.sisostds.org/ontologies/C2SIM#EntityDescriptor"/>
            </owl:Restriction>
        </rdfs:subClassOf>
        <rdfs:subClassOf>
            <owl:Restriction>
                <owl:onProperty rdf:resource="http://www.sisostds.org/ontologies/C2SIM#hasCurrentTask"/>
                <owl:minQualifiedCardinality rdf:datatype="http://www.w3.org/2001/XMLSchema#nonNegativeInteger">0</owl:minQualifiedCardinality>
                <owl:onDataRange rdf:resource="http://www.sisostds.org/ontologies/C2SIM#UUIDBase"/>
            </owl:Restriction>
        </rdfs:subClassOf>
        <rdfs:comment>An ActorEntity is an entity that can send/receive orders and reports and/or perform tasks.</rdfs:comment>
    </owl:Class>
    <owl:Axiom>
        <owl:annotatedSource rdf:resource="http://www.sisostds.org/ontologies/C2SIM#ActorEntity"/>
        <owl:annotatedProperty rdf:resource="http://www.w3.org/2000/01/rdf-schema#subClassOf"/>
        <owl:annotatedTarget>
            <owl:Restriction>
                <owl:onProperty rdf:resource="http://www.sisostds.org/ontologies/C2SIM#hasCurrentTask"/>
                <owl:minQualifiedCardinality rdf:datatype="http://www.w3.org/2001/XMLSchema#nonNegativeInteger">0</owl:minQualifiedCardinality>
                <owl:onDataRange rdf:resource="http://www.sisostds.org/ontologies/C2SIM#UUIDBase"/>
            </owl:Restriction>
        </owl:annotatedTarget>
        <rdfs:comment>This is the unique identifier of an individual of the Task class. The individual is defined elsewhere.</rdfs:comment>
    </owl:Axiom>
    


    <!-- http://www.sisostds.org/ontologies/C2SIM#AllegianceRelationship -->

    <owl:Class rdf:about="http://www.sisostds.org/ontologies/C2SIM#AllegianceRelationship">
        <rdfs:subClassOf rdf:resource="http://www.sisostds.org/ontologies/C2SIM#Relationship"/>
        <rdfs:subClassOf>
            <owl:Restriction>
                <owl:onProperty rdf:resource="http://www.sisostds.org/ontologies/C2SIM#hasAllegianceRelationshipCode"/>
                <owl:qualifiedCardinality rdf:datatype="http://www.w3.org/2001/XMLSchema#nonNegativeInteger">1</owl:qualifiedCardinality>
                <owl:onClass rdf:resource="http://www.sisostds.org/ontologies/C2SIM#AllegianceRelationshipCode"/>
            </owl:Restriction>
        </rdfs:subClassOf>
        <rdfs:subClassOf>
            <owl:Restriction>
                <owl:onProperty rdf:resource="http://www.sisostds.org/ontologies/C2SIM#hasActorReference"/>
                <owl:qualifiedCardinality rdf:datatype="http://www.w3.org/2001/XMLSchema#nonNegativeInteger">1</owl:qualifiedCardinality>
                <owl:onDataRange rdf:resource="http://www.sisostds.org/ontologies/C2SIM#UUIDBase"/>
            </owl:Restriction>
        </rdfs:subClassOf>
        <rdfs:comment>This is a relationship of friendly, hostile, or neutral toward an actor entity. It is part of the definition of the hasAllegianceTo property of an EntityDescriptor.</rdfs:comment>
    </owl:Class>
    <owl:Axiom>
        <owl:annotatedSource rdf:resource="http://www.sisostds.org/ontologies/C2SIM#AllegianceRelationship"/>
        <owl:annotatedProperty rdf:resource="http://www.w3.org/2000/01/rdf-schema#subClassOf"/>
        <owl:annotatedTarget>
            <owl:Restriction>
                <owl:onProperty rdf:resource="http://www.sisostds.org/ontologies/C2SIM#hasActorReference"/>
                <owl:qualifiedCardinality rdf:datatype="http://www.w3.org/2001/XMLSchema#nonNegativeInteger">1</owl:qualifiedCardinality>
                <owl:onDataRange rdf:resource="http://www.sisostds.org/ontologies/C2SIM#UUIDBase"/>
            </owl:Restriction>
        </owl:annotatedTarget>
        <rdfs:comment>The object of the relation.</rdfs:comment>
    </owl:Axiom>
    


    <!-- http://www.sisostds.org/ontologies/C2SIM#AllegianceRelationshipCode -->

    <owl:Class rdf:about="http://www.sisostds.org/ontologies/C2SIM#AllegianceRelationshipCode">
        <rdfs:subClassOf rdf:resource="http://www.sisostds.org/ontologies/C2SIM#Code"/>
        <rdfs:comment>This code defines the types of allegiance in an AllegianceRelationship.</rdfs:comment>
    </owl:Class>
    


    <!-- http://www.sisostds.org/ontologies/C2SIM#AuthorizationHeader -->

    <owl:Class rdf:about="http://www.sisostds.org/ontologies/C2SIM#AuthorizationHeader">
        <rdfs:subClassOf rdf:resource="http://www.sisostds.org/ontologies/C2SIM#C2SIMContent"/>
        <rdfs:subClassOf>
            <owl:Restriction>
                <owl:onProperty rdf:resource="http://www.sisostds.org/ontologies/C2SIM#hasAuthorizationCredentials"/>
                <owl:qualifiedCardinality rdf:datatype="http://www.w3.org/2001/XMLSchema#nonNegativeInteger">1</owl:qualifiedCardinality>
                <owl:onDataRange rdf:resource="http://www.sisostds.org/ontologies/C2SIM#angle"/>
            </owl:Restriction>
        </rdfs:subClassOf>
        <rdfs:subClassOf>
            <owl:Restriction>
                <owl:onProperty rdf:resource="http://www.sisostds.org/ontologies/C2SIM#hasAuthorizationType"/>
                <owl:qualifiedCardinality rdf:datatype="http://www.w3.org/2001/XMLSchema#nonNegativeInteger">1</owl:qualifiedCardinality>
                <owl:onDataRange rdf:resource="http://www.sisostds.org/ontologies/C2SIM#angle"/>
            </owl:Restriction>
        </rdfs:subClassOf>
        <rdfs:comment>The Authorization header is a part of the C2SIM headers used in client-server communications. Its primary function is to authenticate a user-agent with a server, typically by carrying credentials in the form of a token or a set of credentials like username and password. This header is fundamental in implementing security measures for web applications and APIs.</rdfs:comment>
    </owl:Class>
    


    <!-- http://www.sisostds.org/ontologies/C2SIM#C2SIMContent -->

    <owl:Class rdf:about="http://www.sisostds.org/ontologies/C2SIM#C2SIMContent">
        <rdfs:comment>Class of all concepts for the content of messages in the core C2SIM data model.</rdfs:comment>
    </owl:Class>
    


    <!-- http://www.sisostds.org/ontologies/C2SIM#C2SIMHeader -->

    <owl:Class rdf:about="http://www.sisostds.org/ontologies/C2SIM#C2SIMHeader">
        <rdfs:subClassOf rdf:resource="http://www.sisostds.org/ontologies/C2SIM#MessageConcept"/>
        <rdfs:subClassOf>
            <owl:Restriction>
                <owl:onProperty rdf:resource="http://www.sisostds.org/ontologies/C2SIM#hasCommunicativeActTypeCode"/>
                <owl:qualifiedCardinality rdf:datatype="http://www.w3.org/2001/XMLSchema#nonNegativeInteger">1</owl:qualifiedCardinality>
                <owl:onClass rdf:resource="http://www.sisostds.org/ontologies/C2SIM#CommunicativeActTypeCode"/>
            </owl:Restriction>
        </rdfs:subClassOf>
        <rdfs:subClassOf>
            <owl:Restriction>
                <owl:onProperty rdf:resource="http://www.sisostds.org/ontologies/C2SIM#hasAuthorizationHeader"/>
                <owl:maxQualifiedCardinality rdf:datatype="http://www.w3.org/2001/XMLSchema#nonNegativeInteger">1</owl:maxQualifiedCardinality>
                <owl:onClass rdf:resource="http://www.sisostds.org/ontologies/C2SIM#AuthorizationHeader"/>
            </owl:Restriction>
        </rdfs:subClassOf>
        <rdfs:subClassOf>
            <owl:Restriction>
                <owl:onProperty rdf:resource="http://www.sisostds.org/ontologies/C2SIM#hasSecurityClassificationCode"/>
                <owl:maxQualifiedCardinality rdf:datatype="http://www.w3.org/2001/XMLSchema#nonNegativeInteger">1</owl:maxQualifiedCardinality>
                <owl:onClass rdf:resource="http://www.sisostds.org/ontologies/C2SIM#SecurityClassificationCode"/>
            </owl:Restriction>
        </rdfs:subClassOf>
        <rdfs:subClassOf>
            <owl:Restriction>
                <owl:onProperty rdf:resource="http://www.sisostds.org/ontologies/C2SIM#hasSendingTime"/>
                <owl:maxQualifiedCardinality rdf:datatype="http://www.w3.org/2001/XMLSchema#nonNegativeInteger">1</owl:maxQualifiedCardinality>
                <owl:onClass rdf:resource="http://www.sisostds.org/ontologies/C2SIM#DateTime"/>
            </owl:Restriction>
        </rdfs:subClassOf>
        <rdfs:subClassOf>
            <owl:Restriction>
                <owl:onProperty rdf:resource="http://www.sisostds.org/ontologies/C2SIM#hasProtocol"/>
                <owl:hasValue>SISO-STD-C2SIM</owl:hasValue>
            </owl:Restriction>
        </rdfs:subClassOf>
        <rdfs:subClassOf>
            <owl:Restriction>
                <owl:onProperty rdf:resource="http://www.sisostds.org/ontologies/C2SIM#hasProtocolVersion"/>
                <owl:hasValue>1.0.0</owl:hasValue>
            </owl:Restriction>
        </rdfs:subClassOf>
        <rdfs:subClassOf>
            <owl:Restriction>
                <owl:onProperty rdf:resource="http://www.sisostds.org/ontologies/C2SIM#hasConversationID"/>
                <owl:qualifiedCardinality rdf:datatype="http://www.w3.org/2001/XMLSchema#nonNegativeInteger">1</owl:qualifiedCardinality>
                <owl:onDataRange rdf:resource="http://www.sisostds.org/ontologies/C2SIM#UUIDBase"/>
            </owl:Restriction>
        </rdfs:subClassOf>
        <rdfs:subClassOf>
            <owl:Restriction>
                <owl:onProperty rdf:resource="http://www.sisostds.org/ontologies/C2SIM#hasMessageID"/>
                <owl:qualifiedCardinality rdf:datatype="http://www.w3.org/2001/XMLSchema#nonNegativeInteger">1</owl:qualifiedCardinality>
                <owl:onDataRange rdf:resource="http://www.sisostds.org/ontologies/C2SIM#UUIDBase"/>
            </owl:Restriction>
        </rdfs:subClassOf>
        <rdfs:subClassOf>
            <owl:Restriction>
                <owl:onProperty rdf:resource="http://www.sisostds.org/ontologies/C2SIM#isFromSendingSystem"/>
                <owl:qualifiedCardinality rdf:datatype="http://www.w3.org/2001/XMLSchema#nonNegativeInteger">1</owl:qualifiedCardinality>
                <owl:onDataRange rdf:resource="http://www.w3.org/2001/XMLSchema#string"/>
            </owl:Restriction>
        </rdfs:subClassOf>
        <rdfs:subClassOf>
            <owl:Restriction>
                <owl:onProperty rdf:resource="http://www.sisostds.org/ontologies/C2SIM#isToReceivingSystem"/>
                <owl:qualifiedCardinality rdf:datatype="http://www.w3.org/2001/XMLSchema#nonNegativeInteger">1</owl:qualifiedCardinality>
                <owl:onDataRange rdf:resource="http://www.w3.org/2001/XMLSchema#string"/>
            </owl:Restriction>
        </rdfs:subClassOf>
        <rdfs:subClassOf>
            <owl:Restriction>
                <owl:onProperty rdf:resource="http://www.sisostds.org/ontologies/C2SIM#hasReplyToSystem"/>
                <owl:maxQualifiedCardinality rdf:datatype="http://www.w3.org/2001/XMLSchema#nonNegativeInteger">1</owl:maxQualifiedCardinality>
                <owl:onDataRange rdf:resource="http://www.w3.org/2001/XMLSchema#string"/>
            </owl:Restriction>
        </rdfs:subClassOf>
        <rdfs:subClassOf>
            <owl:Restriction>
                <owl:onProperty rdf:resource="http://www.sisostds.org/ontologies/C2SIM#isInReplyToMessageID"/>
                <owl:maxQualifiedCardinality rdf:datatype="http://www.w3.org/2001/XMLSchema#nonNegativeInteger">1</owl:maxQualifiedCardinality>
                <owl:onDataRange rdf:resource="http://www.sisostds.org/ontologies/C2SIM#UUIDBase"/>
            </owl:Restriction>
        </rdfs:subClassOf>
        <rdfs:comment>Indicates that the receiving system should submit its initialization data to the system identified in the</rdfs:comment>
    </owl:Class>
    <owl:Axiom>
        <owl:annotatedSource rdf:resource="http://www.sisostds.org/ontologies/C2SIM#C2SIMHeader"/>
        <owl:annotatedProperty rdf:resource="http://www.w3.org/2000/01/rdf-schema#subClassOf"/>
        <owl:annotatedTarget>
            <owl:Restriction>
                <owl:onProperty rdf:resource="http://www.sisostds.org/ontologies/C2SIM#hasConversationID"/>
                <owl:qualifiedCardinality rdf:datatype="http://www.w3.org/2001/XMLSchema#nonNegativeInteger">1</owl:qualifiedCardinality>
                <owl:onDataRange rdf:resource="http://www.sisostds.org/ontologies/C2SIM#UUIDBase"/>
            </owl:Restriction>
        </owl:annotatedTarget>
        <rdfs:comment>This is the unique identifier of a conversation. A conversation is a concept outside of the C2SIM data model.</rdfs:comment>
    </owl:Axiom>
    <owl:Axiom>
        <owl:annotatedSource rdf:resource="http://www.sisostds.org/ontologies/C2SIM#C2SIMHeader"/>
        <owl:annotatedProperty rdf:resource="http://www.w3.org/2000/01/rdf-schema#subClassOf"/>
        <owl:annotatedTarget>
            <owl:Restriction>
                <owl:onProperty rdf:resource="http://www.sisostds.org/ontologies/C2SIM#hasMessageID"/>
                <owl:qualifiedCardinality rdf:datatype="http://www.w3.org/2001/XMLSchema#nonNegativeInteger">1</owl:qualifiedCardinality>
                <owl:onDataRange rdf:resource="http://www.sisostds.org/ontologies/C2SIM#UUIDBase"/>
            </owl:Restriction>
        </owl:annotatedTarget>
        <rdfs:comment>This is the unique identifier of a message.</rdfs:comment>
    </owl:Axiom>
    <owl:Axiom>
        <owl:annotatedSource rdf:resource="http://www.sisostds.org/ontologies/C2SIM#C2SIMHeader"/>
        <owl:annotatedProperty rdf:resource="http://www.w3.org/2000/01/rdf-schema#subClassOf"/>
        <owl:annotatedTarget>
            <owl:Restriction>
                <owl:onProperty rdf:resource="http://www.sisostds.org/ontologies/C2SIM#isInReplyToMessageID"/>
                <owl:maxQualifiedCardinality rdf:datatype="http://www.w3.org/2001/XMLSchema#nonNegativeInteger">1</owl:maxQualifiedCardinality>
                <owl:onDataRange rdf:resource="http://www.sisostds.org/ontologies/C2SIM#UUIDBase"/>
            </owl:Restriction>
        </owl:annotatedTarget>
        <rdfs:comment>This is the unique identifier of a message.</rdfs:comment>
    </owl:Axiom>
    


    <!-- http://www.sisostds.org/ontologies/C2SIM#C2SIMInitializationBody -->

    <owl:Class rdf:about="http://www.sisostds.org/ontologies/C2SIM#C2SIMInitializationBody">
        <rdfs:subClassOf rdf:resource="http://www.sisostds.org/ontologies/C2SIM#MessageBody"/>
        <rdfs:subClassOf>
            <owl:Restriction>
                <owl:onProperty rdf:resource="http://www.sisostds.org/ontologies/C2SIM#hasInitializationDataFile"/>
                <owl:minQualifiedCardinality rdf:datatype="http://www.w3.org/2001/XMLSchema#nonNegativeInteger">0</owl:minQualifiedCardinality>
                <owl:onClass rdf:resource="http://www.sisostds.org/ontologies/C2SIM#InitializationDataFile"/>
            </owl:Restriction>
        </rdfs:subClassOf>
        <rdfs:subClassOf>
            <owl:Restriction>
                <owl:onProperty rdf:resource="http://www.sisostds.org/ontologies/C2SIM#hasObjectDefinitions"/>
                <owl:minQualifiedCardinality rdf:datatype="http://www.w3.org/2001/XMLSchema#nonNegativeInteger">1</owl:minQualifiedCardinality>
                <owl:onClass rdf:resource="http://www.sisostds.org/ontologies/C2SIM#ObjectDefinitions"/>
            </owl:Restriction>
        </rdfs:subClassOf>
        <rdfs:subClassOf>
            <owl:Restriction>
                <owl:onProperty rdf:resource="http://www.sisostds.org/ontologies/C2SIM#hasSystemEntityList"/>
                <owl:minQualifiedCardinality rdf:datatype="http://www.w3.org/2001/XMLSchema#nonNegativeInteger">1</owl:minQualifiedCardinality>
                <owl:onClass rdf:resource="http://www.sisostds.org/ontologies/C2SIM#SystemEntityList"/>
            </owl:Restriction>
        </rdfs:subClassOf>
        <rdfs:subClassOf>
            <owl:Restriction>
                <owl:onProperty rdf:resource="http://www.sisostds.org/ontologies/C2SIM#hasScenarioSetting"/>
                <owl:qualifiedCardinality rdf:datatype="http://www.w3.org/2001/XMLSchema#nonNegativeInteger">1</owl:qualifiedCardinality>
                <owl:onClass rdf:resource="http://www.sisostds.org/ontologies/C2SIM#ScenarioSetting"/>
            </owl:Restriction>
        </rdfs:subClassOf>
        <rdfs:comment>This message can initialize all of the objects in the scenario as well as the scenario setting.</rdfs:comment>
    </owl:Class>
    


    <!-- http://www.sisostds.org/ontologies/C2SIM#CartesianOffset -->

    <owl:Class rdf:about="http://www.sisostds.org/ontologies/C2SIM#CartesianOffset">
        <rdfs:subClassOf rdf:resource="http://www.sisostds.org/ontologies/C2SIM#SpatialOffset"/>
        <rdfs:subClassOf>
            <owl:Restriction>
                <owl:onProperty rdf:resource="http://www.sisostds.org/ontologies/C2SIM#hasEast"/>
                <owl:qualifiedCardinality rdf:datatype="http://www.w3.org/2001/XMLSchema#nonNegativeInteger">1</owl:qualifiedCardinality>
                <owl:onDataRange rdf:resource="http://www.w3.org/2001/XMLSchema#double"/>
            </owl:Restriction>
        </rdfs:subClassOf>
        <rdfs:subClassOf>
            <owl:Restriction>
                <owl:onProperty rdf:resource="http://www.sisostds.org/ontologies/C2SIM#hasNorth"/>
                <owl:qualifiedCardinality rdf:datatype="http://www.w3.org/2001/XMLSchema#nonNegativeInteger">1</owl:qualifiedCardinality>
                <owl:onDataRange rdf:resource="http://www.w3.org/2001/XMLSchema#double"/>
            </owl:Restriction>
        </rdfs:subClassOf>
        <rdfs:subClassOf>
            <owl:Restriction>
                <owl:onProperty rdf:resource="http://www.sisostds.org/ontologies/C2SIM#hasUp"/>
                <owl:qualifiedCardinality rdf:datatype="http://www.w3.org/2001/XMLSchema#nonNegativeInteger">1</owl:qualifiedCardinality>
                <owl:onDataRange rdf:resource="http://www.w3.org/2001/XMLSchema#double"/>
            </owl:Restriction>
        </rdfs:subClassOf>
        <rdfs:comment>A spatial offset expressed in local flat earth coordinates.</rdfs:comment>
    </owl:Class>
    <owl:Axiom>
        <owl:annotatedSource rdf:resource="http://www.sisostds.org/ontologies/C2SIM#CartesianOffset"/>
        <owl:annotatedProperty rdf:resource="http://www.w3.org/2000/01/rdf-schema#subClassOf"/>
        <owl:annotatedTarget>
            <owl:Restriction>
                <owl:onProperty rdf:resource="http://www.sisostds.org/ontologies/C2SIM#hasUp"/>
                <owl:qualifiedCardinality rdf:datatype="http://www.w3.org/2001/XMLSchema#nonNegativeInteger">1</owl:qualifiedCardinality>
                <owl:onDataRange rdf:resource="http://www.w3.org/2001/XMLSchema#double"/>
            </owl:Restriction>
        </owl:annotatedTarget>
        <rdfs:comment>In meters</rdfs:comment>
    </owl:Axiom>
    <owl:Axiom>
        <owl:annotatedSource rdf:resource="http://www.sisostds.org/ontologies/C2SIM#CartesianOffset"/>
        <owl:annotatedProperty rdf:resource="http://www.w3.org/2000/01/rdf-schema#subClassOf"/>
        <owl:annotatedTarget>
            <owl:Restriction>
                <owl:onProperty rdf:resource="http://www.sisostds.org/ontologies/C2SIM#hasEast"/>
                <owl:qualifiedCardinality rdf:datatype="http://www.w3.org/2001/XMLSchema#nonNegativeInteger">1</owl:qualifiedCardinality>
                <owl:onDataRange rdf:resource="http://www.w3.org/2001/XMLSchema#double"/>
            </owl:Restriction>
        </owl:annotatedTarget>
        <rdfs:comment>In meters</rdfs:comment>
    </owl:Axiom>
    <owl:Axiom>
        <owl:annotatedSource rdf:resource="http://www.sisostds.org/ontologies/C2SIM#CartesianOffset"/>
        <owl:annotatedProperty rdf:resource="http://www.w3.org/2000/01/rdf-schema#subClassOf"/>
        <owl:annotatedTarget>
            <owl:Restriction>
                <owl:onProperty rdf:resource="http://www.sisostds.org/ontologies/C2SIM#hasNorth"/>
                <owl:qualifiedCardinality rdf:datatype="http://www.w3.org/2001/XMLSchema#nonNegativeInteger">1</owl:qualifiedCardinality>
                <owl:onDataRange rdf:resource="http://www.w3.org/2001/XMLSchema#double"/>
            </owl:Restriction>
        </owl:annotatedTarget>
        <rdfs:comment>In meters</rdfs:comment>
    </owl:Axiom>
    


    <!-- http://www.sisostds.org/ontologies/C2SIM#CheckpointRestore -->

    <owl:Class rdf:about="http://www.sisostds.org/ontologies/C2SIM#CheckpointRestore">
        <rdfs:subClassOf rdf:resource="http://www.sisostds.org/ontologies/C2SIM#SystemMessageBody"/>
        <rdfs:subClassOf>
            <owl:Restriction>
                <owl:onProperty rdf:resource="http://www.sisostds.org/ontologies/C2SIM#hasName"/>
                <owl:qualifiedCardinality rdf:datatype="http://www.w3.org/2001/XMLSchema#nonNegativeInteger">1</owl:qualifiedCardinality>
                <owl:onDataRange rdf:resource="http://www.w3.org/2001/XMLSchema#string"/>
            </owl:Restriction>
        </rdfs:subClassOf>
        <rdfs:comment>The CheckpointRestore system command directs systems in a C2SIM coalition to restore their state to the saved data in the named checkpoint file.</rdfs:comment>
    </owl:Class>
    


    <!-- http://www.sisostds.org/ontologies/C2SIM#CheckpointSave -->

    <owl:Class rdf:about="http://www.sisostds.org/ontologies/C2SIM#CheckpointSave">
        <rdfs:subClassOf rdf:resource="http://www.sisostds.org/ontologies/C2SIM#SystemMessageBody"/>
        <rdfs:subClassOf>
            <owl:Restriction>
                <owl:onProperty rdf:resource="http://www.sisostds.org/ontologies/C2SIM#hasName"/>
                <owl:qualifiedCardinality rdf:datatype="http://www.w3.org/2001/XMLSchema#nonNegativeInteger">1</owl:qualifiedCardinality>
                <owl:onDataRange rdf:resource="http://www.w3.org/2001/XMLSchema#string"/>
            </owl:Restriction>
        </rdfs:subClassOf>
        <rdfs:comment>The CheckpointSave system command directs systems in a C2SIM coalition to save their current state. The name is used to distinguish the current set of saved data from other named checkpoints.</rdfs:comment>
    </owl:Class>
    


    <!-- http://www.sisostds.org/ontologies/C2SIM#Code -->

    <owl:Class rdf:about="http://www.sisostds.org/ontologies/C2SIM#Code">
        <rdfs:subClassOf rdf:resource="http://www.sisostds.org/ontologies/C2SIM#C2SIMContent"/>
        <rdfs:comment>A collection of enumerations used by various data types in C2SIM</rdfs:comment>
    </owl:Class>
    


    <!-- http://www.sisostds.org/ontologies/C2SIM#CollectiveEntity -->

    <owl:Class rdf:about="http://www.sisostds.org/ontologies/C2SIM#CollectiveEntity">
        <rdfs:subClassOf rdf:resource="http://www.sisostds.org/ontologies/C2SIM#ActorEntity"/>
        <rdfs:subClassOf>
            <owl:Restriction>
                <owl:onProperty rdf:resource="http://www.sisostds.org/ontologies/C2SIM#hasCurrentState"/>
                <owl:maxQualifiedCardinality rdf:datatype="http://www.w3.org/2001/XMLSchema#nonNegativeInteger">1</owl:maxQualifiedCardinality>
                <owl:onClass rdf:resource="http://www.sisostds.org/ontologies/C2SIM#PhysicalState"/>
            </owl:Restriction>
        </rdfs:subClassOf>
        <rdfs:subClassOf>
            <owl:Restriction>
                <owl:onProperty rdf:resource="http://www.sisostds.org/ontologies/C2SIM#hasSubordinate"/>
                <owl:minQualifiedCardinality rdf:datatype="http://www.w3.org/2001/XMLSchema#nonNegativeInteger">0</owl:minQualifiedCardinality>
                <owl:onDataRange rdf:resource="http://www.sisostds.org/ontologies/C2SIM#UUIDBase"/>
            </owl:Restriction>
        </rdfs:subClassOf>
        <rdfs:comment>This is an Entity that is normally thought of as having constituent entities, i.e. a Unit.

CollectiveEntities may or may not hve their subordinates explicitly represented in the exercise (i.e., it may always be aggregated, or it may have subordinates that are themselves entities).  If they are represented, then the hasSubordinate property will have at least one instance.

The CollectivEntity may be an abstract actor, or it may have physical properties; if the latter, then the hasCurrentState property is present with a PhysicalState.</rdfs:comment>
    </owl:Class>
    <owl:Axiom>
        <owl:annotatedSource rdf:resource="http://www.sisostds.org/ontologies/C2SIM#CollectiveEntity"/>
        <owl:annotatedProperty rdf:resource="http://www.w3.org/2000/01/rdf-schema#subClassOf"/>
        <owl:annotatedTarget>
            <owl:Restriction>
                <owl:onProperty rdf:resource="http://www.sisostds.org/ontologies/C2SIM#hasSubordinate"/>
                <owl:minQualifiedCardinality rdf:datatype="http://www.w3.org/2001/XMLSchema#nonNegativeInteger">0</owl:minQualifiedCardinality>
                <owl:onDataRange rdf:resource="http://www.sisostds.org/ontologies/C2SIM#UUIDBase"/>
            </owl:Restriction>
        </owl:annotatedTarget>
        <rdfs:comment>This is the unique identifier of an individual of the ActorEntity class. The individual is defined elsewhere.</rdfs:comment>
    </owl:Axiom>
    


    <!-- http://www.sisostds.org/ontologies/C2SIM#CommunicationNetwork -->

    <owl:Class rdf:about="http://www.sisostds.org/ontologies/C2SIM#CommunicationNetwork">
        <rdfs:subClassOf rdf:resource="http://www.sisostds.org/ontologies/C2SIM#AbstractObject"/>
        <rdfs:comment>An specific network over which an entity communicates. A logical entity. Will have data properties defining communication parameters.
Networks are part of an EntityDescriptor. If a message is sent to a CommunicationsNetwork, all ActorEntities that have this network will receive the message.</rdfs:comment>
    </owl:Class>
    


    <!-- http://www.sisostds.org/ontologies/C2SIM#CommunicativeActTypeCode -->

    <owl:Class rdf:about="http://www.sisostds.org/ontologies/C2SIM#CommunicativeActTypeCode">
        <rdfs:subClassOf rdf:resource="http://www.sisostds.org/ontologies/C2SIM#MessageCode"/>
        <rdfs:comment>Enumeration of different types of communications.</rdfs:comment>
    </owl:Class>
    


    <!-- http://www.sisostds.org/ontologies/C2SIM#CountryCode -->

    <owl:Class rdf:about="http://www.sisostds.org/ontologies/C2SIM#CountryCode">
        <rdfs:subClassOf rdf:resource="http://www.sisostds.org/ontologies/C2SIM#OrganizationCode"/>
        <rdfs:comment>A unique three-letter code for each nation on Earth, defined in ISO 3166-1 standard and also found in JC3IEDM AffiliationGeopoliticalCode.</rdfs:comment>
    </owl:Class>
    


    <!-- http://www.sisostds.org/ontologies/C2SIM#CulturalFeature -->

    <owl:Class rdf:about="http://www.sisostds.org/ontologies/C2SIM#CulturalFeature">
        <rdfs:subClassOf rdf:resource="http://www.sisostds.org/ontologies/C2SIM#PhysicalEntity"/>
        <rdfs:comment>Any man-made feature in the environment</rdfs:comment>
    </owl:Class>
    


    <!-- http://www.sisostds.org/ontologies/C2SIM#DateTime -->

    <owl:Class rdf:about="http://www.sisostds.org/ontologies/C2SIM#DateTime">
        <rdfs:subClassOf rdf:resource="http://www.sisostds.org/ontologies/C2SIM#TimeInstant"/>
        <rdfs:subClassOf>
            <owl:Restriction>
                <owl:onProperty rdf:resource="http://www.sisostds.org/ontologies/C2SIM#hasIsoDateTime"/>
                <owl:qualifiedCardinality rdf:datatype="http://www.w3.org/2001/XMLSchema#nonNegativeInteger">1</owl:qualifiedCardinality>
                <owl:onDataRange rdf:resource="http://www.sisostds.org/ontologies/C2SIM#IsoDateTimeBase"/>
            </owl:Restriction>
        </rdfs:subClassOf>
        <rdfs:comment>A date and time in ISO 8601:2000 DateTime Group format yyyy-mm-ddThh:mm:ssZ e.g. 1998-05-12T14:15:00Z. From MSDL simple types.</rdfs:comment>
    </owl:Class>
    


    <!-- http://www.sisostds.org/ontologies/C2SIM#DesiredEffectCode -->

    <owl:Class rdf:about="http://www.sisostds.org/ontologies/C2SIM#DesiredEffectCode">
        <rdfs:subClassOf rdf:resource="http://www.sisostds.org/ontologies/C2SIM#Code"/>
        <rdfs:comment>A code describing the intended effect of a task.</rdfs:comment>
    </owl:Class>
    


    <!-- http://www.sisostds.org/ontologies/C2SIM#DomainMessageBody -->

    <owl:Class rdf:about="http://www.sisostds.org/ontologies/C2SIM#DomainMessageBody">
        <rdfs:subClassOf rdf:resource="http://www.sisostds.org/ontologies/C2SIM#MessageBody"/>
        <rdfs:subClassOf>
            <owl:Restriction>
                <owl:onProperty rdf:resource="http://www.sisostds.org/ontologies/C2SIM#isFromSender"/>
                <owl:qualifiedCardinality rdf:datatype="http://www.w3.org/2001/XMLSchema#nonNegativeInteger">1</owl:qualifiedCardinality>
                <owl:onDataRange rdf:resource="http://www.sisostds.org/ontologies/C2SIM#UUIDBase"/>
            </owl:Restriction>
        </rdfs:subClassOf>
        <rdfs:subClassOf>
            <owl:Restriction>
                <owl:onProperty rdf:resource="http://www.sisostds.org/ontologies/C2SIM#isToReceiver"/>
                <owl:qualifiedCardinality rdf:datatype="http://www.w3.org/2001/XMLSchema#nonNegativeInteger">1</owl:qualifiedCardinality>
                <owl:onDataRange rdf:resource="http://www.sisostds.org/ontologies/C2SIM#UUIDBase"/>
            </owl:Restriction>
        </rdfs:subClassOf>
        <rdfs:comment>The body of a message that is sent between actors in the domain.
It is one subclass of MessageBody (other subclasses perform administrative functions in the C2SIM Coalition.)</rdfs:comment>
    </owl:Class>
    <owl:Axiom>
        <owl:annotatedSource rdf:resource="http://www.sisostds.org/ontologies/C2SIM#DomainMessageBody"/>
        <owl:annotatedProperty rdf:resource="http://www.w3.org/2000/01/rdf-schema#subClassOf"/>
        <owl:annotatedTarget>
            <owl:Restriction>
                <owl:onProperty rdf:resource="http://www.sisostds.org/ontologies/C2SIM#isFromSender"/>
                <owl:qualifiedCardinality rdf:datatype="http://www.w3.org/2001/XMLSchema#nonNegativeInteger">1</owl:qualifiedCardinality>
                <owl:onDataRange rdf:resource="http://www.sisostds.org/ontologies/C2SIM#UUIDBase"/>
            </owl:Restriction>
        </owl:annotatedTarget>
        <rdfs:comment>This is the unique indentifier of an individual of the ActorEntity class who is the sender of this message. The individual is defined elsewhere.</rdfs:comment>
    </owl:Axiom>
    <owl:Axiom>
        <owl:annotatedSource rdf:resource="http://www.sisostds.org/ontologies/C2SIM#DomainMessageBody"/>
        <owl:annotatedProperty rdf:resource="http://www.w3.org/2000/01/rdf-schema#subClassOf"/>
        <owl:annotatedTarget>
            <owl:Restriction>
                <owl:onProperty rdf:resource="http://www.sisostds.org/ontologies/C2SIM#isToReceiver"/>
                <owl:qualifiedCardinality rdf:datatype="http://www.w3.org/2001/XMLSchema#nonNegativeInteger">1</owl:qualifiedCardinality>
                <owl:onDataRange rdf:resource="http://www.sisostds.org/ontologies/C2SIM#UUIDBase"/>
            </owl:Restriction>
        </owl:annotatedTarget>
        <rdfs:comment>This is the unique identifier of an individual of the ActorEntity class OR an individual of the CommunicationNetwork class that is the intended recipient of this message. If the recipient is a CommunicationsNetwork, then all ActorEntities that have this network will receive the message.</rdfs:comment>
    </owl:Axiom>
    


    <!-- http://www.sisostds.org/ontologies/C2SIM#Duration -->

    <owl:Class rdf:about="http://www.sisostds.org/ontologies/C2SIM#Duration">
        <rdfs:subClassOf rdf:resource="http://www.sisostds.org/ontologies/C2SIM#TemporalConcept"/>
        <rdfs:subClassOf>
            <owl:Restriction>
                <owl:onProperty rdf:resource="http://www.sisostds.org/ontologies/C2SIM#hasIsoTimeDuration"/>
                <owl:qualifiedCardinality rdf:datatype="http://www.w3.org/2001/XMLSchema#nonNegativeInteger">1</owl:qualifiedCardinality>
                <owl:onDataRange rdf:resource="http://www.sisostds.org/ontologies/C2SIM#IsoTimeDurationBase"/>
            </owl:Restriction>
        </rdfs:subClassOf>
        <rdfs:comment>A time duration expressed in ISO 8601:2000 duration format PnYnMnDTnHnMnS e.g. P00Y00M00DT00H00M00S. Note that this does not support fractions of seconds. From MSDL simple types.</rdfs:comment>
    </owl:Class>
    


    <!-- http://www.sisostds.org/ontologies/C2SIM#Entity -->

    <owl:Class rdf:about="http://www.sisostds.org/ontologies/C2SIM#Entity">
        <rdfs:subClassOf rdf:resource="http://www.sisostds.org/ontologies/C2SIM#C2SIMContent"/>
        <rdfs:subClassOf>
            <owl:Restriction>
                <owl:onProperty rdf:resource="http://www.sisostds.org/ontologies/C2SIM#hasNamedEntityType"/>
                <owl:minQualifiedCardinality rdf:datatype="http://www.w3.org/2001/XMLSchema#nonNegativeInteger">0</owl:minQualifiedCardinality>
                <owl:onClass rdf:resource="http://www.sisostds.org/ontologies/C2SIM#NamedEntityType"/>
            </owl:Restriction>
        </rdfs:subClassOf>
        <rdfs:subClassOf>
            <owl:Restriction>
                <owl:onProperty rdf:resource="http://www.sisostds.org/ontologies/C2SIM#hasSISOEntityType"/>
                <owl:maxQualifiedCardinality rdf:datatype="http://www.w3.org/2001/XMLSchema#nonNegativeInteger">1</owl:maxQualifiedCardinality>
                <owl:onClass rdf:resource="http://www.sisostds.org/ontologies/C2SIM#SISOEntityType"/>
            </owl:Restriction>
        </rdfs:subClassOf>
        <rdfs:subClassOf>
            <owl:Restriction>
                <owl:onProperty rdf:resource="http://www.sisostds.org/ontologies/smx#hasAPP6CSymbol"/>
                <owl:maxQualifiedCardinality rdf:datatype="http://www.w3.org/2001/XMLSchema#nonNegativeInteger">1</owl:maxQualifiedCardinality>
                <owl:onClass rdf:resource="http://www.sisostds.org/ontologies/smx#APP6CSymbol"/>
            </owl:Restriction>
        </rdfs:subClassOf>
        <rdfs:subClassOf>
            <owl:Restriction>
                <owl:onProperty rdf:resource="http://www.sisostds.org/ontologies/C2SIM#hasUUID"/>
                <owl:qualifiedCardinality rdf:datatype="http://www.w3.org/2001/XMLSchema#nonNegativeInteger">1</owl:qualifiedCardinality>
                <owl:onDataRange rdf:resource="http://www.sisostds.org/ontologies/C2SIM#UUIDBase"/>
            </owl:Restriction>
        </rdfs:subClassOf>
        <rdfs:subClassOf>
            <owl:Restriction>
                <owl:onProperty rdf:resource="http://www.sisostds.org/ontologies/C2SIM#hasName"/>
                <owl:maxQualifiedCardinality rdf:datatype="http://www.w3.org/2001/XMLSchema#nonNegativeInteger">1</owl:maxQualifiedCardinality>
                <owl:onDataRange rdf:resource="http://www.w3.org/2001/XMLSchema#string"/>
            </owl:Restriction>
        </rdfs:subClassOf>
        <rdfs:comment>An individually identified object. Objects may have physical properties, in which case they belong to the subclass ConcreteEntity. Objects may be able to perform actions, in which case they belong in the subclass ActorEntity. If they have physical properties AND can perform actions, then they inherit from both subclasses.</rdfs:comment>
    </owl:Class>
    <owl:Axiom>
        <owl:annotatedSource rdf:resource="http://www.sisostds.org/ontologies/C2SIM#Entity"/>
        <owl:annotatedProperty rdf:resource="http://www.w3.org/2000/01/rdf-schema#subClassOf"/>
        <owl:annotatedTarget>
            <owl:Restriction>
                <owl:onProperty rdf:resource="http://www.sisostds.org/ontologies/C2SIM#hasUUID"/>
                <owl:qualifiedCardinality rdf:datatype="http://www.w3.org/2001/XMLSchema#nonNegativeInteger">1</owl:qualifiedCardinality>
                <owl:onDataRange rdf:resource="http://www.sisostds.org/ontologies/C2SIM#UUIDBase"/>
            </owl:Restriction>
        </owl:annotatedTarget>
        <rdfs:comment>This is the unique identifier of an individual of this class.</rdfs:comment>
    </owl:Axiom>
    


    <!-- http://www.sisostds.org/ontologies/C2SIM#EntityDescriptor -->

    <owl:Class rdf:about="http://www.sisostds.org/ontologies/C2SIM#EntityDescriptor">
        <rdfs:subClassOf rdf:resource="http://www.sisostds.org/ontologies/C2SIM#C2SIMContent"/>
        <rdfs:subClassOf>
            <owl:Restriction>
                <owl:onProperty rdf:resource="http://www.sisostds.org/ontologies/C2SIM#hasAllegianceRelationship"/>
                <owl:minQualifiedCardinality rdf:datatype="http://www.w3.org/2001/XMLSchema#nonNegativeInteger">0</owl:minQualifiedCardinality>
                <owl:onClass rdf:resource="http://www.sisostds.org/ontologies/C2SIM#AllegianceRelationship"/>
            </owl:Restriction>
        </rdfs:subClassOf>
        <rdfs:subClassOf>
            <owl:Restriction>
                <owl:onProperty rdf:resource="http://www.sisostds.org/ontologies/C2SIM#hasCommunicationsNetwork"/>
                <owl:minQualifiedCardinality rdf:datatype="http://www.w3.org/2001/XMLSchema#nonNegativeInteger">0</owl:minQualifiedCardinality>
                <owl:onDataRange rdf:resource="http://www.sisostds.org/ontologies/C2SIM#UUIDBase"/>
            </owl:Restriction>
        </rdfs:subClassOf>
        <rdfs:subClassOf>
            <owl:Restriction>
                <owl:onProperty rdf:resource="http://www.sisostds.org/ontologies/C2SIM#isAffiliatedWith"/>
                <owl:minQualifiedCardinality rdf:datatype="http://www.w3.org/2001/XMLSchema#nonNegativeInteger">0</owl:minQualifiedCardinality>
                <owl:onDataRange rdf:resource="http://www.sisostds.org/ontologies/C2SIM#UUIDBase"/>
            </owl:Restriction>
        </rdfs:subClassOf>
        <rdfs:subClassOf>
            <owl:Restriction>
                <owl:onProperty rdf:resource="http://www.sisostds.org/ontologies/C2SIM#hasSuperior"/>
                <owl:maxQualifiedCardinality rdf:datatype="http://www.w3.org/2001/XMLSchema#nonNegativeInteger">1</owl:maxQualifiedCardinality>
                <owl:onDataRange rdf:resource="http://www.sisostds.org/ontologies/C2SIM#UUIDBase"/>
            </owl:Restriction>
        </rdfs:subClassOf>
        <rdfs:subClassOf>
            <owl:Restriction>
                <owl:onProperty rdf:resource="http://www.sisostds.org/ontologies/smx#hasSide"/>
                <owl:maxQualifiedCardinality rdf:datatype="http://www.w3.org/2001/XMLSchema#nonNegativeInteger">1</owl:maxQualifiedCardinality>
                <owl:onDataRange rdf:resource="http://www.sisostds.org/ontologies/C2SIM#UUIDBase"/>
            </owl:Restriction>
        </rdfs:subClassOf>
        <rdfs:comment>The Descriptor defines static attributes of an entity, i.e. that do not change during the course of the simulation. This information is provided at initialization time.

The friend/hostile/... relationship of this entity with others can be specfied with hasAllegianceRelationship properties and/or the hasSide property. The hasSide property can define this entity as a member of a &quot;Force&quot; or &quot;Side,&quot; i.e. a team of entities that are friendly to each other and are all friendly, hostile or neutral to other defined teams. ForceSides are abstract objects.
The entity can also have friendly, hostile or neutral relationships with specific other objects as defined by its hasAllegianceRelationship properties. These can be used in place of ForceSide membership, or they can be used along with ForceSide memberships to define exceptions.

The isAffiliatedWith property defines organizations that this entity is affiliated with. These organizations are abstract; they are not actors.

C2 structures can be defined by using the hasSuperior property.</rdfs:comment>
    </owl:Class>
    <owl:Axiom>
        <owl:annotatedSource rdf:resource="http://www.sisostds.org/ontologies/C2SIM#EntityDescriptor"/>
        <owl:annotatedProperty rdf:resource="http://www.w3.org/2000/01/rdf-schema#subClassOf"/>
        <owl:annotatedTarget>
            <owl:Restriction>
                <owl:onProperty rdf:resource="http://www.sisostds.org/ontologies/C2SIM#hasCommunicationsNetwork"/>
                <owl:minQualifiedCardinality rdf:datatype="http://www.w3.org/2001/XMLSchema#nonNegativeInteger">0</owl:minQualifiedCardinality>
                <owl:onDataRange rdf:resource="http://www.sisostds.org/ontologies/C2SIM#UUIDBase"/>
            </owl:Restriction>
        </owl:annotatedTarget>
        <rdfs:comment>This is the unique identifier of an individual of the CommunicationNetwork class to which this entity belongs.</rdfs:comment>
    </owl:Axiom>
    <owl:Axiom>
        <owl:annotatedSource rdf:resource="http://www.sisostds.org/ontologies/C2SIM#EntityDescriptor"/>
        <owl:annotatedProperty rdf:resource="http://www.w3.org/2000/01/rdf-schema#subClassOf"/>
        <owl:annotatedTarget>
            <owl:Restriction>
                <owl:onProperty rdf:resource="http://www.sisostds.org/ontologies/C2SIM#isAffiliatedWith"/>
                <owl:minQualifiedCardinality rdf:datatype="http://www.w3.org/2001/XMLSchema#nonNegativeInteger">0</owl:minQualifiedCardinality>
                <owl:onDataRange rdf:resource="http://www.sisostds.org/ontologies/C2SIM#UUIDBase"/>
            </owl:Restriction>
        </owl:annotatedTarget>
        <rdfs:comment>This is the unique identifier of an individual of the AbstractOrganization class to which this entity is affiliated. Since AbstractOrganizations are not Actors, this is not a command relationship, but a descriptive attribute of the entity.</rdfs:comment>
    </owl:Axiom>
    <owl:Axiom>
        <owl:annotatedSource rdf:resource="http://www.sisostds.org/ontologies/C2SIM#EntityDescriptor"/>
        <owl:annotatedProperty rdf:resource="http://www.w3.org/2000/01/rdf-schema#subClassOf"/>
        <owl:annotatedTarget>
            <owl:Restriction>
                <owl:onProperty rdf:resource="http://www.sisostds.org/ontologies/C2SIM#hasSuperior"/>
                <owl:maxQualifiedCardinality rdf:datatype="http://www.w3.org/2001/XMLSchema#nonNegativeInteger">1</owl:maxQualifiedCardinality>
                <owl:onDataRange rdf:resource="http://www.sisostds.org/ontologies/C2SIM#UUIDBase"/>
            </owl:Restriction>
        </owl:annotatedTarget>
        <rdfs:comment>This is the unique identifier of an individual of the ActorEntity class who is this entity&apos;s superior in a command and control hierarchy.</rdfs:comment>
    </owl:Axiom>
    


    <!-- http://www.sisostds.org/ontologies/C2SIM#EntityHealthStatus -->

    <owl:Class rdf:about="http://www.sisostds.org/ontologies/C2SIM#EntityHealthStatus">
        <rdfs:subClassOf rdf:resource="http://www.sisostds.org/ontologies/C2SIM#PhysicalConcept"/>
        <rdfs:comment>A representation of the health status of an entity. Subclasses for representing health as Operational Status, a count of some salient resource, or a percentage of full strength.</rdfs:comment>
    </owl:Class>
    


    <!-- http://www.sisostds.org/ontologies/C2SIM#EntityState -->

    <owl:Class rdf:about="http://www.sisostds.org/ontologies/C2SIM#EntityState">
        <rdfs:subClassOf rdf:resource="http://www.sisostds.org/ontologies/C2SIM#C2SIMContent"/>
        <rdfs:subClassOf>
            <owl:Restriction>
                <owl:onProperty rdf:resource="http://www.sisostds.org/ontologies/C2SIM#hasDateTime"/>
                <owl:maxQualifiedCardinality rdf:datatype="http://www.w3.org/2001/XMLSchema#nonNegativeInteger">1</owl:maxQualifiedCardinality>
                <owl:onClass rdf:resource="http://www.sisostds.org/ontologies/C2SIM#TimeInstant"/>
            </owl:Restriction>
        </rdfs:subClassOf>
        <rdfs:comment>Dynamic state information for entities in the exercise.</rdfs:comment>
    </owl:Class>
    


    <!-- http://www.sisostds.org/ontologies/C2SIM#EnvironmentalObject -->

    <owl:Class rdf:about="http://www.sisostds.org/ontologies/C2SIM#EnvironmentalObject">
        <rdfs:subClassOf rdf:resource="http://www.sisostds.org/ontologies/C2SIM#PhysicalEntity"/>
        <rdfs:comment>A specified region in which the environment (e.g. weather, ocean state) is defined by a particular Environmental State.</rdfs:comment>
    </owl:Class>
    


    <!-- http://www.sisostds.org/ontologies/C2SIM#EthnicGroupCode -->

    <owl:Class rdf:about="http://www.sisostds.org/ontologies/C2SIM#EthnicGroupCode">
        <rdfs:subClassOf rdf:resource="http://www.sisostds.org/ontologies/C2SIM#OrganizationCode"/>
        <rdfs:comment>Alphabetic code up to six letters, describing an ethnic group, obtained from JC3IEDM AffiliationEthnicGroupCode-3.0.2</rdfs:comment>
    </owl:Class>
    


    <!-- http://www.sisostds.org/ontologies/C2SIM#EulerAngles -->

    <owl:Class rdf:about="http://www.sisostds.org/ontologies/C2SIM#EulerAngles">
        <rdfs:subClassOf rdf:resource="http://www.sisostds.org/ontologies/C2SIM#Orientation"/>
        <rdfs:subClassOf>
            <owl:Restriction>
                <owl:onProperty rdf:resource="http://www.sisostds.org/ontologies/C2SIM#hasPhi"/>
                <owl:qualifiedCardinality rdf:datatype="http://www.w3.org/2001/XMLSchema#nonNegativeInteger">1</owl:qualifiedCardinality>
                <owl:onDataRange rdf:resource="http://www.sisostds.org/ontologies/C2SIM#angle"/>
            </owl:Restriction>
        </rdfs:subClassOf>
        <rdfs:subClassOf>
            <owl:Restriction>
                <owl:onProperty rdf:resource="http://www.sisostds.org/ontologies/C2SIM#hasPsi"/>
                <owl:qualifiedCardinality rdf:datatype="http://www.w3.org/2001/XMLSchema#nonNegativeInteger">1</owl:qualifiedCardinality>
                <owl:onDataRange rdf:resource="http://www.sisostds.org/ontologies/C2SIM#angle"/>
            </owl:Restriction>
        </rdfs:subClassOf>
        <rdfs:subClassOf>
            <owl:Restriction>
                <owl:onProperty rdf:resource="http://www.sisostds.org/ontologies/C2SIM#hasTheta"/>
                <owl:qualifiedCardinality rdf:datatype="http://www.w3.org/2001/XMLSchema#nonNegativeInteger">1</owl:qualifiedCardinality>
                <owl:onDataRange rdf:resource="http://www.sisostds.org/ontologies/C2SIM#angle"/>
            </owl:Restriction>
        </rdfs:subClassOf>
        <rdfs:comment>Representation of the orientation of an entity in 3D space expressed as Euler angles (DIS). This orientation will be used primarily for initialization of simulation entities, especially those that are not clamped to the ground.
This orienation indicates rotations from a geocentric coordinate system.</rdfs:comment>
    </owl:Class>
    <owl:Axiom>
        <owl:annotatedSource rdf:resource="http://www.sisostds.org/ontologies/C2SIM#EulerAngles"/>
        <owl:annotatedProperty rdf:resource="http://www.w3.org/2000/01/rdf-schema#subClassOf"/>
        <owl:annotatedTarget>
            <owl:Restriction>
                <owl:onProperty rdf:resource="http://www.sisostds.org/ontologies/C2SIM#hasPhi"/>
                <owl:qualifiedCardinality rdf:datatype="http://www.w3.org/2001/XMLSchema#nonNegativeInteger">1</owl:qualifiedCardinality>
                <owl:onDataRange rdf:resource="http://www.sisostds.org/ontologies/C2SIM#angle"/>
            </owl:Restriction>
        </owl:annotatedTarget>
        <rdfs:comment>Angle in radians</rdfs:comment>
    </owl:Axiom>
    <owl:Axiom>
        <owl:annotatedSource rdf:resource="http://www.sisostds.org/ontologies/C2SIM#EulerAngles"/>
        <owl:annotatedProperty rdf:resource="http://www.w3.org/2000/01/rdf-schema#subClassOf"/>
        <owl:annotatedTarget>
            <owl:Restriction>
                <owl:onProperty rdf:resource="http://www.sisostds.org/ontologies/C2SIM#hasPsi"/>
                <owl:qualifiedCardinality rdf:datatype="http://www.w3.org/2001/XMLSchema#nonNegativeInteger">1</owl:qualifiedCardinality>
                <owl:onDataRange rdf:resource="http://www.sisostds.org/ontologies/C2SIM#angle"/>
            </owl:Restriction>
        </owl:annotatedTarget>
        <rdfs:comment>Angle in radians</rdfs:comment>
    </owl:Axiom>
    <owl:Axiom>
        <owl:annotatedSource rdf:resource="http://www.sisostds.org/ontologies/C2SIM#EulerAngles"/>
        <owl:annotatedProperty rdf:resource="http://www.w3.org/2000/01/rdf-schema#subClassOf"/>
        <owl:annotatedTarget>
            <owl:Restriction>
                <owl:onProperty rdf:resource="http://www.sisostds.org/ontologies/C2SIM#hasTheta"/>
                <owl:qualifiedCardinality rdf:datatype="http://www.w3.org/2001/XMLSchema#nonNegativeInteger">1</owl:qualifiedCardinality>
                <owl:onDataRange rdf:resource="http://www.sisostds.org/ontologies/C2SIM#angle"/>
            </owl:Restriction>
        </owl:annotatedTarget>
        <rdfs:comment>Angle in radians</rdfs:comment>
    </owl:Axiom>
    


    <!-- http://www.sisostds.org/ontologies/C2SIM#Event -->

    <owl:Class rdf:about="http://www.sisostds.org/ontologies/C2SIM#Event">
        <rdfs:subClassOf rdf:resource="http://www.sisostds.org/ontologies/C2SIM#Action"/>
        <rdfs:subClassOf>
            <owl:Restriction>
                <owl:onProperty rdf:resource="http://www.sisostds.org/ontologies/C2SIM#hasEventCode"/>
                <owl:qualifiedCardinality rdf:datatype="http://www.w3.org/2001/XMLSchema#nonNegativeInteger">1</owl:qualifiedCardinality>
                <owl:onClass rdf:resource="http://www.sisostds.org/ontologies/C2SIM#EventCode"/>
            </owl:Restriction>
        </rdfs:subClassOf>
        <rdfs:subClassOf>
            <owl:Restriction>
                <owl:onProperty rdf:resource="http://www.sisostds.org/ontologies/C2SIM#hasStartTime"/>
                <owl:qualifiedCardinality rdf:datatype="http://www.w3.org/2001/XMLSchema#nonNegativeInteger">1</owl:qualifiedCardinality>
                <owl:onClass rdf:resource="http://www.sisostds.org/ontologies/C2SIM#TimeInstant"/>
            </owl:Restriction>
        </rdfs:subClassOf>
        <rdfs:subClassOf>
            <owl:Restriction>
                <owl:onProperty rdf:resource="http://www.sisostds.org/ontologies/C2SIM#hasDuration"/>
                <owl:maxQualifiedCardinality rdf:datatype="http://www.w3.org/2001/XMLSchema#nonNegativeInteger">1</owl:maxQualifiedCardinality>
                <owl:onClass rdf:resource="http://www.sisostds.org/ontologies/C2SIM#Duration"/>
            </owl:Restriction>
        </rdfs:subClassOf>
        <rdfs:comment>An ACTION that is an incident, phenomenon, or occasion. May or may not be the result of an agent&apos;s action.</rdfs:comment>
    </owl:Class>
    


    <!-- http://www.sisostds.org/ontologies/C2SIM#EventCode -->

    <owl:Class rdf:about="http://www.sisostds.org/ontologies/C2SIM#EventCode">
        <rdfs:subClassOf rdf:resource="http://www.sisostds.org/ontologies/C2SIM#ActionCode"/>
        <rdfs:comment>The type of event.</rdfs:comment>
    </owl:Class>
    


    <!-- http://www.sisostds.org/ontologies/C2SIM#GeodeticCoordinate -->

    <owl:Class rdf:about="http://www.sisostds.org/ontologies/C2SIM#GeodeticCoordinate">
        <rdfs:subClassOf rdf:resource="http://www.sisostds.org/ontologies/C2SIM#Location"/>
        <rdfs:subClassOf>
            <owl:Restriction>
                <owl:onProperty rdf:resource="http://www.sisostds.org/ontologies/C2SIM#hasLatitude"/>
                <owl:qualifiedCardinality rdf:datatype="http://www.w3.org/2001/XMLSchema#nonNegativeInteger">1</owl:qualifiedCardinality>
                <owl:onDataRange rdf:resource="http://www.sisostds.org/ontologies/C2SIM#latitude"/>
            </owl:Restriction>
        </rdfs:subClassOf>
        <rdfs:subClassOf>
            <owl:Restriction>
                <owl:onProperty rdf:resource="http://www.sisostds.org/ontologies/C2SIM#hasLongitude"/>
                <owl:qualifiedCardinality rdf:datatype="http://www.w3.org/2001/XMLSchema#nonNegativeInteger">1</owl:qualifiedCardinality>
                <owl:onDataRange rdf:resource="http://www.sisostds.org/ontologies/C2SIM#longitude"/>
            </owl:Restriction>
        </rdfs:subClassOf>
        <rdfs:subClassOf>
            <owl:Restriction>
                <owl:onProperty rdf:resource="http://www.sisostds.org/ontologies/C2SIM#hasAltitudeAGL"/>
                <owl:maxQualifiedCardinality rdf:datatype="http://www.w3.org/2001/XMLSchema#nonNegativeInteger">1</owl:maxQualifiedCardinality>
                <owl:onDataRange rdf:resource="http://www.w3.org/2001/XMLSchema#double"/>
            </owl:Restriction>
        </rdfs:subClassOf>
        <rdfs:subClassOf>
            <owl:Restriction>
                <owl:onProperty rdf:resource="http://www.sisostds.org/ontologies/C2SIM#hasAltitudeMSL"/>
                <owl:maxQualifiedCardinality rdf:datatype="http://www.w3.org/2001/XMLSchema#nonNegativeInteger">1</owl:maxQualifiedCardinality>
                <owl:onDataRange rdf:resource="http://www.w3.org/2001/XMLSchema#double"/>
            </owl:Restriction>
        </rdfs:subClassOf>
        <rdfs:comment>A location defined by latitude, longitude, and altitude.</rdfs:comment>
    </owl:Class>
    


    <!-- http://www.sisostds.org/ontologies/C2SIM#GeographicFeature -->

    <owl:Class rdf:about="http://www.sisostds.org/ontologies/C2SIM#GeographicFeature">
        <rdfs:subClassOf rdf:resource="http://www.sisostds.org/ontologies/C2SIM#PhysicalEntity"/>
        <rdfs:comment>A geographic feature generally used for location reference. For example a hill, river, etc.</rdfs:comment>
    </owl:Class>
    


    <!-- http://www.sisostds.org/ontologies/C2SIM#Heading -->

    <owl:Class rdf:about="http://www.sisostds.org/ontologies/C2SIM#Heading">
        <rdfs:subClassOf rdf:resource="http://www.sisostds.org/ontologies/C2SIM#Orientation"/>
        <rdfs:comment>Heading is the rotation clockwise relative to local grid north. This is a rotation about one axis; other axis orientations are unspecified, and if a system needs values they can be assumed to be zero or appropriate angles to clamp the entity to the ground.</rdfs:comment>
    </owl:Class>
    


    <!-- http://www.sisostds.org/ontologies/C2SIM#InitializationComplete -->

    <owl:Class rdf:about="http://www.sisostds.org/ontologies/C2SIM#InitializationComplete">
        <rdfs:subClassOf rdf:resource="http://www.sisostds.org/ontologies/C2SIM#SystemMessageBody"/>
        <rdfs:comment>This C2SIM message is sent by each participating system in a C2SIM coalition of systems in response to the C2SIM initialization message, after that system has completed its initialization processing.</rdfs:comment>
    </owl:Class>
    


    <!-- http://www.sisostds.org/ontologies/C2SIM#InitializationConcept -->

    <owl:Class rdf:about="http://www.sisostds.org/ontologies/C2SIM#InitializationConcept">
        <rdfs:comment>This parent class collects together classes that are necessary for the initialization of a scenario.</rdfs:comment>
    </owl:Class>
    


    <!-- http://www.sisostds.org/ontologies/C2SIM#InitializationDataFile -->

    <owl:Class rdf:about="http://www.sisostds.org/ontologies/C2SIM#InitializationDataFile">
        <rdfs:subClassOf rdf:resource="http://www.sisostds.org/ontologies/C2SIM#InitializationConcept"/>
        <rdfs:subClassOf>
            <owl:Restriction>
                <owl:onProperty rdf:resource="http://www.sisostds.org/ontologies/C2SIM#hasName"/>
                <owl:qualifiedCardinality rdf:datatype="http://www.w3.org/2001/XMLSchema#nonNegativeInteger">1</owl:qualifiedCardinality>
                <owl:onDataRange rdf:resource="http://www.w3.org/2001/XMLSchema#string"/>
            </owl:Restriction>
        </rdfs:subClassOf>
        <rdfs:subClassOf>
            <owl:Restriction>
                <owl:onProperty rdf:resource="http://www.sisostds.org/ontologies/C2SIM#hasSystemName"/>
                <owl:qualifiedCardinality rdf:datatype="http://www.w3.org/2001/XMLSchema#nonNegativeInteger">1</owl:qualifiedCardinality>
                <owl:onDataRange rdf:resource="http://www.w3.org/2001/XMLSchema#string"/>
            </owl:Restriction>
        </rdfs:subClassOf>
        <rdfs:subClassOf>
            <owl:Restriction>
                <owl:onProperty rdf:resource="http://www.sisostds.org/ontologies/C2SIM#hasIntializationFileType"/>
                <owl:maxQualifiedCardinality rdf:datatype="http://www.w3.org/2001/XMLSchema#nonNegativeInteger">1</owl:maxQualifiedCardinality>
                <owl:onDataRange rdf:resource="http://www.w3.org/2001/XMLSchema#string"/>
            </owl:Restriction>
        </rdfs:subClassOf>
        <rdfs:comment>Defines a file of supplementary data that is used to initialize the scenario. This file is generally system-specific, for example a terrain database file or a mapping from C2SIM entity types to local entity type enumerations. It could apply to &quot;all&quot; systems.</rdfs:comment>
    </owl:Class>
    


    <!-- http://www.sisostds.org/ontologies/C2SIM#IntervalTime -->

    <owl:Class rdf:about="http://www.sisostds.org/ontologies/C2SIM#IntervalTime">
        <rdfs:subClassOf rdf:resource="http://www.sisostds.org/ontologies/C2SIM#TemporalConcept"/>
        <rdfs:subClassOf>
            <owl:Restriction>
                <owl:onProperty rdf:resource="http://www.sisostds.org/ontologies/C2SIM#hasDuration"/>
                <owl:maxQualifiedCardinality rdf:datatype="http://www.w3.org/2001/XMLSchema#nonNegativeInteger">1</owl:maxQualifiedCardinality>
                <owl:onClass rdf:resource="http://www.sisostds.org/ontologies/C2SIM#Duration"/>
            </owl:Restriction>
        </rdfs:subClassOf>
        <rdfs:subClassOf>
            <owl:Restriction>
                <owl:onProperty rdf:resource="http://www.sisostds.org/ontologies/C2SIM#hasEndTime"/>
                <owl:maxQualifiedCardinality rdf:datatype="http://www.w3.org/2001/XMLSchema#nonNegativeInteger">1</owl:maxQualifiedCardinality>
                <owl:onClass rdf:resource="http://www.sisostds.org/ontologies/C2SIM#TimeInstant"/>
            </owl:Restriction>
        </rdfs:subClassOf>
        <rdfs:subClassOf>
            <owl:Restriction>
                <owl:onProperty rdf:resource="http://www.sisostds.org/ontologies/C2SIM#hasStartTime"/>
                <owl:maxQualifiedCardinality rdf:datatype="http://www.w3.org/2001/XMLSchema#nonNegativeInteger">1</owl:maxQualifiedCardinality>
                <owl:onClass rdf:resource="http://www.sisostds.org/ontologies/C2SIM#TimeInstant"/>
            </owl:Restriction>
        </rdfs:subClassOf>
        <rdfs:comment>An interval defined by a start and end dateTime. Note that 2 of the 3 properties must be specified.</rdfs:comment>
    </owl:Class>
    


    <!-- http://www.sisostds.org/ontologies/C2SIM#Location -->

    <owl:Class rdf:about="http://www.sisostds.org/ontologies/C2SIM#Location">
        <rdfs:subClassOf rdf:resource="http://www.sisostds.org/ontologies/C2SIM#PhysicalConcept"/>
        <rdfs:comment>A representation of location in space. Can be a coordinate value, a reference to an entity location, or a location relative to another location.

An optional altitude representation code indicates whether this is a fully specified point in 3 dimensions, or whether the altitude encoded in the class should be ignored or set to some other reference. If the code is not present, then the location is assumed to be a fully specified 3D point.

The location of a CollectiveEntity may represent the center of mass or headquarters location in the case of an organization.</rdfs:comment>
    </owl:Class>
    


    <!-- http://www.sisostds.org/ontologies/C2SIM#MagicMove -->

    <owl:Class rdf:about="http://www.sisostds.org/ontologies/C2SIM#MagicMove">
        <rdfs:subClassOf rdf:resource="http://www.sisostds.org/ontologies/C2SIM#SystemMessageBody"/>
        <rdfs:subClassOf>
            <owl:Restriction>
                <owl:onProperty rdf:resource="http://www.sisostds.org/ontologies/C2SIM#hasLocation"/>
                <owl:qualifiedCardinality rdf:datatype="http://www.w3.org/2001/XMLSchema#nonNegativeInteger">1</owl:qualifiedCardinality>
                <owl:onClass rdf:resource="http://www.sisostds.org/ontologies/C2SIM#Location"/>
            </owl:Restriction>
        </rdfs:subClassOf>
        <rdfs:subClassOf>
            <owl:Restriction>
                <owl:onProperty rdf:resource="http://www.sisostds.org/ontologies/C2SIM#hasEntityReference"/>
                <owl:qualifiedCardinality rdf:datatype="http://www.w3.org/2001/XMLSchema#nonNegativeInteger">1</owl:qualifiedCardinality>
                <owl:onDataRange rdf:resource="http://www.sisostds.org/ontologies/C2SIM#UUIDBase"/>
            </owl:Restriction>
        </rdfs:subClassOf>
        <rdfs:subClassOf>
            <owl:Restriction>
                <owl:onProperty rdf:resource="http://www.sisostds.org/ontologies/C2SIM#hasTaskID"/>
                <owl:maxQualifiedCardinality rdf:datatype="http://www.w3.org/2001/XMLSchema#nonNegativeInteger">1</owl:maxQualifiedCardinality>
                <owl:onDataRange rdf:resource="http://www.sisostds.org/ontologies/C2SIM#UUIDBase"/>
            </owl:Restriction>
        </rdfs:subClassOf>
        <rdfs:subClassOf>
            <owl:Restriction>
                <owl:onProperty rdf:resource="http://www.sisostds.org/ontologies/C2SIM#hasTasker"/>
                <owl:maxQualifiedCardinality rdf:datatype="http://www.w3.org/2001/XMLSchema#nonNegativeInteger">1</owl:maxQualifiedCardinality>
                <owl:onDataRange rdf:resource="http://www.sisostds.org/ontologies/C2SIM#UUIDBase"/>
            </owl:Restriction>
        </rdfs:subClassOf>
        <rdfs:comment>System command used as an exercise control capabiliity to immediately reposition some entity (i.e., without going through a simulated movement). The hasEntityReference property provides the UUID of the entity being repositioned. The hasTasker property provides the UUID of the entity ordering the repositioning. The hasTaskID property gives the reference to a Task that the repositioning may be associated with.</rdfs:comment>
    </owl:Class>
    


    <!-- http://www.sisostds.org/ontologies/C2SIM#MapGraphic -->

    <owl:Class rdf:about="http://www.sisostds.org/ontologies/C2SIM#MapGraphic">
        <rdfs:subClassOf rdf:resource="http://www.sisostds.org/ontologies/C2SIM#PhysicalEntity"/>
        <rdfs:comment>Graphics on a map that define locations, lines, areas, actions, etc. The location of the graphic is the location in the real world represented on the map. The extent is the set of handle points or vertices that define its shape and size. This class includes task graphics, METOC graphics, and MOOTW graphics.</rdfs:comment>
    </owl:Class>
    


    <!-- http://www.sisostds.org/ontologies/C2SIM#Message -->

    <owl:Class rdf:about="http://www.sisostds.org/ontologies/C2SIM#Message">
        <rdfs:subClassOf rdf:resource="http://www.sisostds.org/ontologies/C2SIM#MessageConcept"/>
        <rdfs:subClassOf>
            <owl:Restriction>
                <owl:onProperty rdf:resource="http://www.sisostds.org/ontologies/C2SIM#hasC2SIMHeader"/>
                <owl:qualifiedCardinality rdf:datatype="http://www.w3.org/2001/XMLSchema#nonNegativeInteger">1</owl:qualifiedCardinality>
                <owl:onClass rdf:resource="http://www.sisostds.org/ontologies/C2SIM#C2SIMHeader"/>
            </owl:Restriction>
        </rdfs:subClassOf>
        <rdfs:subClassOf>
            <owl:Restriction>
                <owl:onProperty rdf:resource="http://www.sisostds.org/ontologies/C2SIM#hasMessageBody"/>
                <owl:qualifiedCardinality rdf:datatype="http://www.w3.org/2001/XMLSchema#nonNegativeInteger">1</owl:qualifiedCardinality>
                <owl:onClass rdf:resource="http://www.sisostds.org/ontologies/C2SIM#MessageBody"/>
            </owl:Restriction>
        </rdfs:subClassOf>
        <rdfs:comment>Any C2SIM message that is sent between host systems.</rdfs:comment>
    </owl:Class>
    


    <!-- http://www.sisostds.org/ontologies/C2SIM#MessageBody -->

    <owl:Class rdf:about="http://www.sisostds.org/ontologies/C2SIM#MessageBody">
        <rdfs:subClassOf rdf:resource="http://www.sisostds.org/ontologies/C2SIM#MessageConcept"/>
        <rdfs:comment>The structure for sending domain messages: orders, reports, and acknowledgements.</rdfs:comment>
    </owl:Class>
    


    <!-- http://www.sisostds.org/ontologies/C2SIM#MessageCode -->

    <owl:Class rdf:about="http://www.sisostds.org/ontologies/C2SIM#MessageCode">
        <rdfs:subClassOf rdf:resource="http://www.sisostds.org/ontologies/C2SIM#MessageConcept"/>
        <rdfs:comment>Enumerations used in messages.</rdfs:comment>
    </owl:Class>
    


    <!-- http://www.sisostds.org/ontologies/C2SIM#MessageConcept -->

    <owl:Class rdf:about="http://www.sisostds.org/ontologies/C2SIM#MessageConcept">
        <rdfs:comment>This parent class collects together classes that define the basic structure of messages used in C2SIM.</rdfs:comment>
    </owl:Class>
    


    <!-- http://www.sisostds.org/ontologies/C2SIM#MilitaryOrganization -->

    <owl:Class rdf:about="http://www.sisostds.org/ontologies/C2SIM#MilitaryOrganization">
        <rdfs:subClassOf rdf:resource="http://www.sisostds.org/ontologies/C2SIM#CollectiveEntity"/>
        <rdfs:comment>A collective entity that is a military organization (i.e., a unit).</rdfs:comment>
    </owl:Class>
    


    <!-- http://www.sisostds.org/ontologies/C2SIM#NamedEntityType -->

    <owl:Class rdf:about="http://www.sisostds.org/ontologies/C2SIM#NamedEntityType">
        <rdfs:subClassOf rdf:resource="http://www.sisostds.org/ontologies/C2SIM#C2SIMContent"/>
        <rdfs:subClassOf>
            <owl:Restriction>
                <owl:onProperty rdf:resource="http://www.sisostds.org/ontologies/C2SIM#hasEntityTypeName"/>
                <owl:qualifiedCardinality rdf:datatype="http://www.w3.org/2001/XMLSchema#nonNegativeInteger">1</owl:qualifiedCardinality>
                <owl:onDataRange rdf:resource="http://www.w3.org/2001/XMLSchema#string"/>
            </owl:Restriction>
        </rdfs:subClassOf>
        <rdfs:subClassOf>
            <owl:Restriction>
                <owl:onProperty rdf:resource="http://www.sisostds.org/ontologies/C2SIM#hasEntityTypeNamespace"/>
                <owl:qualifiedCardinality rdf:datatype="http://www.w3.org/2001/XMLSchema#nonNegativeInteger">1</owl:qualifiedCardinality>
                <owl:onDataRange rdf:resource="http://www.w3.org/2001/XMLSchema#string"/>
            </owl:Restriction>
        </rdfs:subClassOf>
        <rdfs:comment>The definition of an entity type with a unique identifier defined with a pair: namespace, name. 
The namespace and the name are free strings, and must be agreed in advance in the federation agreement template among the systems. For example the namespace could reference a standard, a format, or a simulation involved in the federation: openflight, app6d-sidc, sword, etc.</rdfs:comment>
    </owl:Class>
    


    <!-- http://www.sisostds.org/ontologies/C2SIM#NonMilitaryOrganization -->

    <owl:Class rdf:about="http://www.sisostds.org/ontologies/C2SIM#NonMilitaryOrganization">
        <rdfs:subClassOf rdf:resource="http://www.sisostds.org/ontologies/C2SIM#CollectiveEntity"/>
        <rdfs:comment>An organization operating external to military authority (e.g., law enforcement, non-governmental organizations).</rdfs:comment>
    </owl:Class>
    


    <!-- http://www.sisostds.org/ontologies/C2SIM#ObjectDefinitions -->

    <owl:Class rdf:about="http://www.sisostds.org/ontologies/C2SIM#ObjectDefinitions">
        <rdfs:subClassOf rdf:resource="http://www.sisostds.org/ontologies/C2SIM#InitializationConcept"/>
        <rdfs:subClassOf>
            <owl:Restriction>
                <owl:onProperty rdf:resource="http://www.sisostds.org/ontologies/C2SIM#hasAbstractObject"/>
                <owl:minQualifiedCardinality rdf:datatype="http://www.w3.org/2001/XMLSchema#nonNegativeInteger">0</owl:minQualifiedCardinality>
                <owl:onClass rdf:resource="http://www.sisostds.org/ontologies/C2SIM#AbstractObject"/>
            </owl:Restriction>
        </rdfs:subClassOf>
        <rdfs:subClassOf>
            <owl:Restriction>
                <owl:onProperty rdf:resource="http://www.sisostds.org/ontologies/C2SIM#hasAction"/>
                <owl:minQualifiedCardinality rdf:datatype="http://www.w3.org/2001/XMLSchema#nonNegativeInteger">0</owl:minQualifiedCardinality>
                <owl:onClass rdf:resource="http://www.sisostds.org/ontologies/C2SIM#Action"/>
            </owl:Restriction>
        </rdfs:subClassOf>
        <rdfs:subClassOf>
            <owl:Restriction>
                <owl:onProperty rdf:resource="http://www.sisostds.org/ontologies/C2SIM#hasEntity"/>
                <owl:minQualifiedCardinality rdf:datatype="http://www.w3.org/2001/XMLSchema#nonNegativeInteger">0</owl:minQualifiedCardinality>
                <owl:onClass rdf:resource="http://www.sisostds.org/ontologies/C2SIM#Entity"/>
            </owl:Restriction>
        </rdfs:subClassOf>
        <rdfs:subClassOf>
            <owl:Restriction>
                <owl:onProperty rdf:resource="http://www.sisostds.org/ontologies/lox#hasPlanPhaseReference"/>
                <owl:minQualifiedCardinality rdf:datatype="http://www.w3.org/2001/XMLSchema#nonNegativeInteger">0</owl:minQualifiedCardinality>
                <owl:onDataRange rdf:resource="http://www.sisostds.org/ontologies/C2SIM#UUIDBase"/>
            </owl:Restriction>
        </rdfs:subClassOf>
        <rdfs:comment>Information characterizing an object</rdfs:comment>
    </owl:Class>
    <owl:Axiom>
        <owl:annotatedSource rdf:resource="http://www.sisostds.org/ontologies/C2SIM#ObjectDefinitions"/>
        <owl:annotatedProperty rdf:resource="http://www.w3.org/2000/01/rdf-schema#subClassOf"/>
        <owl:annotatedTarget>
            <owl:Restriction>
                <owl:onProperty rdf:resource="http://www.sisostds.org/ontologies/C2SIM#hasEntity"/>
                <owl:minQualifiedCardinality rdf:datatype="http://www.w3.org/2001/XMLSchema#nonNegativeInteger">0</owl:minQualifiedCardinality>
                <owl:onClass rdf:resource="http://www.sisostds.org/ontologies/C2SIM#Entity"/>
            </owl:Restriction>
        </owl:annotatedTarget>
        <rdfs:comment>This element is optional to allow ObjectInitialization messages to define only AbstractObjects or Tasks. The usual case, however, will be for the ObjectDefinitions class to have Entity definitions.</rdfs:comment>
    </owl:Axiom>
    


    <!-- http://www.sisostds.org/ontologies/C2SIM#ObjectInitializationBody -->

    <owl:Class rdf:about="http://www.sisostds.org/ontologies/C2SIM#ObjectInitializationBody">
        <rdfs:subClassOf rdf:resource="http://www.sisostds.org/ontologies/C2SIM#MessageBody"/>
        <rdfs:subClassOf>
            <owl:Restriction>
                <owl:onProperty rdf:resource="http://www.sisostds.org/ontologies/C2SIM#hasInitializationDataFile"/>
                <owl:minQualifiedCardinality rdf:datatype="http://www.w3.org/2001/XMLSchema#nonNegativeInteger">0</owl:minQualifiedCardinality>
                <owl:onClass rdf:resource="http://www.sisostds.org/ontologies/C2SIM#InitializationDataFile"/>
            </owl:Restriction>
        </rdfs:subClassOf>
        <rdfs:subClassOf>
            <owl:Restriction>
                <owl:onProperty rdf:resource="http://www.sisostds.org/ontologies/C2SIM#hasObjectDefinitions"/>
                <owl:maxQualifiedCardinality rdf:datatype="http://www.w3.org/2001/XMLSchema#nonNegativeInteger">1</owl:maxQualifiedCardinality>
                <owl:onClass rdf:resource="http://www.sisostds.org/ontologies/C2SIM#ObjectDefinitions"/>
            </owl:Restriction>
        </rdfs:subClassOf>
        <rdfs:subClassOf>
            <owl:Restriction>
                <owl:onProperty rdf:resource="http://www.sisostds.org/ontologies/C2SIM#hasScenarioSetting"/>
                <owl:maxQualifiedCardinality rdf:datatype="http://www.w3.org/2001/XMLSchema#nonNegativeInteger">1</owl:maxQualifiedCardinality>
                <owl:onClass rdf:resource="http://www.sisostds.org/ontologies/C2SIM#ScenarioSetting"/>
            </owl:Restriction>
        </rdfs:subClassOf>
        <rdfs:subClassOf>
            <owl:Restriction>
                <owl:onProperty rdf:resource="http://www.sisostds.org/ontologies/C2SIM#hasSystemEntityList"/>
                <owl:maxQualifiedCardinality rdf:datatype="http://www.w3.org/2001/XMLSchema#nonNegativeInteger">1</owl:maxQualifiedCardinality>
                <owl:onClass rdf:resource="http://www.sisostds.org/ontologies/C2SIM#SystemEntityList"/>
            </owl:Restriction>
        </rdfs:subClassOf>
        <rdfs:comment>This message is sent by each system to a marshalling server upon receipt of a SubmitInitialization message.</rdfs:comment>
    </owl:Class>
    <owl:Axiom>
        <owl:annotatedSource rdf:resource="http://www.sisostds.org/ontologies/C2SIM#ObjectInitializationBody"/>
        <owl:annotatedProperty rdf:resource="http://www.w3.org/2000/01/rdf-schema#subClassOf"/>
        <owl:annotatedTarget>
            <owl:Restriction>
                <owl:onProperty rdf:resource="http://www.sisostds.org/ontologies/C2SIM#hasSystemEntityList"/>
                <owl:maxQualifiedCardinality rdf:datatype="http://www.w3.org/2001/XMLSchema#nonNegativeInteger">1</owl:maxQualifiedCardinality>
                <owl:onClass rdf:resource="http://www.sisostds.org/ontologies/C2SIM#SystemEntityList"/>
            </owl:Restriction>
        </owl:annotatedTarget>
        <rdfs:comment>A C2SIM system may provide to the marshalling server its own system entity list, which the server can use to compile a master list.</rdfs:comment>
    </owl:Axiom>
    


    <!-- http://www.sisostds.org/ontologies/C2SIM#OperationalStatus -->

    <owl:Class rdf:about="http://www.sisostds.org/ontologies/C2SIM#OperationalStatus">
        <rdfs:subClassOf rdf:resource="http://www.sisostds.org/ontologies/C2SIM#EntityHealthStatus"/>
        <rdfs:subClassOf>
            <owl:Restriction>
                <owl:onProperty rdf:resource="http://www.sisostds.org/ontologies/C2SIM#hasOperationalStatusCode"/>
                <owl:qualifiedCardinality rdf:datatype="http://www.w3.org/2001/XMLSchema#nonNegativeInteger">1</owl:qualifiedCardinality>
                <owl:onClass rdf:resource="http://www.sisostds.org/ontologies/C2SIM#OperationalStatusCode"/>
            </owl:Restriction>
        </rdfs:subClassOf>
        <rdfs:comment>An enumeration indicating degree of partial capability.</rdfs:comment>
    </owl:Class>
    


    <!-- http://www.sisostds.org/ontologies/C2SIM#OperationalStatusCode -->

    <owl:Class rdf:about="http://www.sisostds.org/ontologies/C2SIM#OperationalStatusCode">
        <rdfs:subClassOf rdf:resource="http://www.sisostds.org/ontologies/C2SIM#Code"/>
        <rdfs:comment>An enumeration indicating the general level of capability of an entity relative to its greatest expected capability.</rdfs:comment>
    </owl:Class>
    


    <!-- http://www.sisostds.org/ontologies/C2SIM#OrderBody -->

    <owl:Class rdf:about="http://www.sisostds.org/ontologies/C2SIM#OrderBody">
        <rdfs:subClassOf rdf:resource="http://www.sisostds.org/ontologies/C2SIM#DomainMessageBody"/>
        <rdfs:subClassOf>
            <owl:Restriction>
                <owl:onProperty rdf:resource="http://www.sisostds.org/ontologies/C2SIM#hasEntity"/>
                <owl:minQualifiedCardinality rdf:datatype="http://www.w3.org/2001/XMLSchema#nonNegativeInteger">0</owl:minQualifiedCardinality>
                <owl:onClass rdf:resource="http://www.sisostds.org/ontologies/C2SIM#MapGraphic"/>
            </owl:Restriction>
        </rdfs:subClassOf>
        <rdfs:subClassOf>
            <owl:Restriction>
                <owl:onProperty rdf:resource="http://www.sisostds.org/ontologies/C2SIM#hasTask"/>
                <owl:minQualifiedCardinality rdf:datatype="http://www.w3.org/2001/XMLSchema#nonNegativeInteger">0</owl:minQualifiedCardinality>
                <owl:onClass rdf:resource="http://www.sisostds.org/ontologies/C2SIM#Task"/>
            </owl:Restriction>
        </rdfs:subClassOf>
        <rdfs:subClassOf>
            <owl:Restriction>
                <owl:onProperty rdf:resource="http://www.sisostds.org/ontologies/C2SIM#hasIssuedTime"/>
                <owl:qualifiedCardinality rdf:datatype="http://www.w3.org/2001/XMLSchema#nonNegativeInteger">1</owl:qualifiedCardinality>
                <owl:onClass rdf:resource="http://www.sisostds.org/ontologies/C2SIM#DateTime"/>
            </owl:Restriction>
        </rdfs:subClassOf>
        <rdfs:subClassOf>
            <owl:Restriction>
                <owl:onProperty rdf:resource="http://www.sisostds.org/ontologies/C2SIM#hasTaskReference"/>
                <owl:minQualifiedCardinality rdf:datatype="http://www.w3.org/2001/XMLSchema#nonNegativeInteger">0</owl:minQualifiedCardinality>
                <owl:onDataRange rdf:resource="http://www.sisostds.org/ontologies/C2SIM#UUIDBase"/>
            </owl:Restriction>
        </rdfs:subClassOf>
        <rdfs:subClassOf>
            <owl:Restriction>
                <owl:onProperty rdf:resource="http://www.sisostds.org/ontologies/C2SIM#hasOrderID"/>
                <owl:qualifiedCardinality rdf:datatype="http://www.w3.org/2001/XMLSchema#nonNegativeInteger">1</owl:qualifiedCardinality>
                <owl:onDataRange rdf:resource="http://www.sisostds.org/ontologies/C2SIM#UUIDBase"/>
            </owl:Restriction>
        </rdfs:subClassOf>
        <rdfs:subClassOf>
            <owl:Restriction>
                <owl:onProperty rdf:resource="http://www.sisostds.org/ontologies/C2SIM#hasRequestingEntity"/>
                <owl:maxQualifiedCardinality rdf:datatype="http://www.w3.org/2001/XMLSchema#nonNegativeInteger">1</owl:maxQualifiedCardinality>
                <owl:onDataRange rdf:resource="http://www.sisostds.org/ontologies/C2SIM#UUIDBase"/>
            </owl:Restriction>
        </rdfs:subClassOf>
        <rdfs:comment>The structure for sending order messages.
This message may define tasks, or it may refer to tasks defined elsewhere (such as in an initialization message).
An order generally comes from an entity with command authority and thus is expected to be obeyed if it is physically possible to do so.</rdfs:comment>
    </owl:Class>
    <owl:Axiom>
        <owl:annotatedSource rdf:resource="http://www.sisostds.org/ontologies/C2SIM#OrderBody"/>
        <owl:annotatedProperty rdf:resource="http://www.w3.org/2000/01/rdf-schema#subClassOf"/>
        <owl:annotatedTarget>
            <owl:Restriction>
                <owl:onProperty rdf:resource="http://www.sisostds.org/ontologies/C2SIM#hasEntity"/>
                <owl:minQualifiedCardinality rdf:datatype="http://www.w3.org/2001/XMLSchema#nonNegativeInteger">0</owl:minQualifiedCardinality>
                <owl:onClass rdf:resource="http://www.sisostds.org/ontologies/C2SIM#MapGraphic"/>
            </owl:Restriction>
        </owl:annotatedTarget>
        <rdfs:comment>This optional property allows the order to define map graphics for use in the task.</rdfs:comment>
    </owl:Axiom>
    <owl:Axiom>
        <owl:annotatedSource rdf:resource="http://www.sisostds.org/ontologies/C2SIM#OrderBody"/>
        <owl:annotatedProperty rdf:resource="http://www.w3.org/2000/01/rdf-schema#subClassOf"/>
        <owl:annotatedTarget>
            <owl:Restriction>
                <owl:onProperty rdf:resource="http://www.sisostds.org/ontologies/C2SIM#hasTask"/>
                <owl:minQualifiedCardinality rdf:datatype="http://www.w3.org/2001/XMLSchema#nonNegativeInteger">0</owl:minQualifiedCardinality>
                <owl:onClass rdf:resource="http://www.sisostds.org/ontologies/C2SIM#Task"/>
            </owl:Restriction>
        </owl:annotatedTarget>
        <rdfs:comment>This is the definition of a task for this order. This property is optional, as the order may instead provide the unique identifier of a task defined elsewhere.</rdfs:comment>
    </owl:Axiom>
    <owl:Axiom>
        <owl:annotatedSource rdf:resource="http://www.sisostds.org/ontologies/C2SIM#OrderBody"/>
        <owl:annotatedProperty rdf:resource="http://www.w3.org/2000/01/rdf-schema#subClassOf"/>
        <owl:annotatedTarget>
            <owl:Restriction>
                <owl:onProperty rdf:resource="http://www.sisostds.org/ontologies/C2SIM#hasTaskReference"/>
                <owl:minQualifiedCardinality rdf:datatype="http://www.w3.org/2001/XMLSchema#nonNegativeInteger">0</owl:minQualifiedCardinality>
                <owl:onDataRange rdf:resource="http://www.sisostds.org/ontologies/C2SIM#UUIDBase"/>
            </owl:Restriction>
        </owl:annotatedTarget>
        <rdfs:comment>This is the unique identifier of an individual of Task class. This property is optional, as the individual may be defined in this message in the hasTask property.</rdfs:comment>
    </owl:Axiom>
    <owl:Axiom>
        <owl:annotatedSource rdf:resource="http://www.sisostds.org/ontologies/C2SIM#OrderBody"/>
        <owl:annotatedProperty rdf:resource="http://www.w3.org/2000/01/rdf-schema#subClassOf"/>
        <owl:annotatedTarget>
            <owl:Restriction>
                <owl:onProperty rdf:resource="http://www.sisostds.org/ontologies/C2SIM#hasOrderID"/>
                <owl:qualifiedCardinality rdf:datatype="http://www.w3.org/2001/XMLSchema#nonNegativeInteger">1</owl:qualifiedCardinality>
                <owl:onDataRange rdf:resource="http://www.sisostds.org/ontologies/C2SIM#UUIDBase"/>
            </owl:Restriction>
        </owl:annotatedTarget>
        <rdfs:comment>This is the unique identifier of an individual order.</rdfs:comment>
    </owl:Axiom>
    <owl:Axiom>
        <owl:annotatedSource rdf:resource="http://www.sisostds.org/ontologies/C2SIM#OrderBody"/>
        <owl:annotatedProperty rdf:resource="http://www.w3.org/2000/01/rdf-schema#subClassOf"/>
        <owl:annotatedTarget>
            <owl:Restriction>
                <owl:onProperty rdf:resource="http://www.sisostds.org/ontologies/C2SIM#hasRequestingEntity"/>
                <owl:maxQualifiedCardinality rdf:datatype="http://www.w3.org/2001/XMLSchema#nonNegativeInteger">1</owl:maxQualifiedCardinality>
                <owl:onDataRange rdf:resource="http://www.sisostds.org/ontologies/C2SIM#UUIDBase"/>
            </owl:Restriction>
        </owl:annotatedTarget>
        <rdfs:comment>The ID must refer to an Actor individual. 
The entity issuing the order might not  be the same as the Sender, if the order was relayed through another unit. This optional property supports this case.</rdfs:comment>
    </owl:Axiom>
    


    <!-- http://www.sisostds.org/ontologies/C2SIM#OrganizationCode -->

    <owl:Class rdf:about="http://www.sisostds.org/ontologies/C2SIM#OrganizationCode">
        <rdfs:subClassOf rdf:resource="http://www.sisostds.org/ontologies/C2SIM#Code"/>
        <rdfs:comment>These provide enumerations of alphabetic text codes identifying characteristics of organizations.</rdfs:comment>
    </owl:Class>
    


    <!-- http://www.sisostds.org/ontologies/C2SIM#OrganizationTypeCode -->

    <owl:Class rdf:about="http://www.sisostds.org/ontologies/C2SIM#OrganizationTypeCode">
        <rdfs:subClassOf rdf:resource="http://www.sisostds.org/ontologies/C2SIM#OrganizationCode"/>
        <rdfs:comment>Alphabetic code up to six letters describing the type of an organization, obtained from JC3IEDM-3.0.2 GroupOrganisationTypeCategoryCode</rdfs:comment>
    </owl:Class>
    


    <!-- http://www.sisostds.org/ontologies/C2SIM#Orientation -->

    <owl:Class rdf:about="http://www.sisostds.org/ontologies/C2SIM#Orientation">
        <rdfs:subClassOf rdf:resource="http://www.sisostds.org/ontologies/C2SIM#PhysicalConcept"/>
        <rdfs:subClassOf>
            <owl:Restriction>
                <owl:onProperty rdf:resource="http://www.sisostds.org/ontologies/C2SIM#hasHeadingAngle"/>
                <owl:qualifiedCardinality rdf:datatype="http://www.w3.org/2001/XMLSchema#nonNegativeInteger">1</owl:qualifiedCardinality>
                <owl:onDataRange rdf:resource="http://www.sisostds.org/ontologies/C2SIM#angle"/>
            </owl:Restriction>
        </rdfs:subClassOf>
        <rdfs:comment>Represents the direction in which an entity is oriented; typically the direction it is facing. Where this class is used, C2SIM Coalitions must state whether they require values for both EulerAngles, Heading, or both. In the absence of specification both are required.</rdfs:comment>
    </owl:Class>
    <owl:Axiom>
        <owl:annotatedSource rdf:resource="http://www.sisostds.org/ontologies/C2SIM#Orientation"/>
        <owl:annotatedProperty rdf:resource="http://www.w3.org/2000/01/rdf-schema#subClassOf"/>
        <owl:annotatedTarget>
            <owl:Restriction>
                <owl:onProperty rdf:resource="http://www.sisostds.org/ontologies/C2SIM#hasHeadingAngle"/>
                <owl:qualifiedCardinality rdf:datatype="http://www.w3.org/2001/XMLSchema#nonNegativeInteger">1</owl:qualifiedCardinality>
                <owl:onDataRange rdf:resource="http://www.sisostds.org/ontologies/C2SIM#angle"/>
            </owl:Restriction>
        </owl:annotatedTarget>
        <rdfs:comment>Angle in radians, clockwise from north.</rdfs:comment>
    </owl:Axiom>
    


    <!-- http://www.sisostds.org/ontologies/C2SIM#Overlay -->

    <owl:Class rdf:about="http://www.sisostds.org/ontologies/C2SIM#Overlay">
        <rdfs:subClassOf rdf:resource="http://www.sisostds.org/ontologies/C2SIM#AbstractObject"/>
        <rdfs:subClassOf>
            <owl:Restriction>
                <owl:onProperty rdf:resource="http://www.sisostds.org/ontologies/C2SIM#hasEntityReference"/>
                <owl:minQualifiedCardinality rdf:datatype="http://www.w3.org/2001/XMLSchema#nonNegativeInteger">1</owl:minQualifiedCardinality>
                <owl:onDataRange rdf:resource="http://www.sisostds.org/ontologies/C2SIM#UUIDBase"/>
            </owl:Restriction>
        </rdfs:subClassOf>
        <rdfs:comment>A logical grouping of Entities (units, graphics, etc.) for purposes of conveniently referring to them.</rdfs:comment>
    </owl:Class>
    <owl:Axiom>
        <owl:annotatedSource rdf:resource="http://www.sisostds.org/ontologies/C2SIM#Overlay"/>
        <owl:annotatedProperty rdf:resource="http://www.w3.org/2000/01/rdf-schema#subClassOf"/>
        <owl:annotatedTarget>
            <owl:Restriction>
                <owl:onProperty rdf:resource="http://www.sisostds.org/ontologies/C2SIM#hasEntityReference"/>
                <owl:minQualifiedCardinality rdf:datatype="http://www.w3.org/2001/XMLSchema#nonNegativeInteger">1</owl:minQualifiedCardinality>
                <owl:onDataRange rdf:resource="http://www.sisostds.org/ontologies/C2SIM#UUIDBase"/>
            </owl:Restriction>
        </owl:annotatedTarget>
        <rdfs:comment>This is the unique identifier of an individual of the Entity class that is in this overlay. The individual is defined elsewhere. The entity could be an actor or a graphic, for example.</rdfs:comment>
    </owl:Axiom>
    


    <!-- http://www.sisostds.org/ontologies/C2SIM#PausePlayback -->

    <owl:Class rdf:about="http://www.sisostds.org/ontologies/C2SIM#PausePlayback">
        <rdfs:subClassOf rdf:resource="http://www.sisostds.org/ontologies/C2SIM#SystemMessageBody"/>
        <rdfs:comment>System command for pausing the playback of recorded C2SIM messages in a C2SIM coalition of systems. The name of the recording being played back is not needed here since there can be only one playback in progress at a time.</rdfs:comment>
    </owl:Class>
    


    <!-- http://www.sisostds.org/ontologies/C2SIM#PauseRecording -->

    <owl:Class rdf:about="http://www.sisostds.org/ontologies/C2SIM#PauseRecording">
        <rdfs:subClassOf rdf:resource="http://www.sisostds.org/ontologies/C2SIM#SystemMessageBody"/>
        <rdfs:comment>System command for pausing the recording of C2SIM messages in a C2SIM coalition of systems. The name of the recording in progress is not needed here since there can be only one recording in progress at a time.</rdfs:comment>
    </owl:Class>
    


    <!-- http://www.sisostds.org/ontologies/C2SIM#PauseScenario -->

    <owl:Class rdf:about="http://www.sisostds.org/ontologies/C2SIM#PauseScenario">
        <rdfs:subClassOf rdf:resource="http://www.sisostds.org/ontologies/C2SIM#SystemMessageBody"/>
        <rdfs:comment>A system command to pause the execution of a scenario across a C2SIM coalition of systems.</rdfs:comment>
    </owl:Class>
    


    <!-- http://www.sisostds.org/ontologies/C2SIM#Person -->

    <owl:Class rdf:about="http://www.sisostds.org/ontologies/C2SIM#Person">
        <rdfs:subClassOf rdf:resource="http://www.sisostds.org/ontologies/C2SIM#ActorEntity"/>
        <rdfs:subClassOf>
            <owl:Restriction>
                <owl:onProperty rdf:resource="http://www.sisostds.org/ontologies/C2SIM#hasCurrentState"/>
                <owl:maxQualifiedCardinality rdf:datatype="http://www.w3.org/2001/XMLSchema#nonNegativeInteger">1</owl:maxQualifiedCardinality>
                <owl:onClass rdf:resource="http://www.sisostds.org/ontologies/C2SIM#PhysicalState"/>
            </owl:Restriction>
        </rdfs:subClassOf>
        <rdfs:subClassOf>
            <owl:Restriction>
                <owl:onProperty rdf:resource="http://www.sisostds.org/ontologies/C2SIM#hasMarking"/>
                <owl:maxQualifiedCardinality rdf:datatype="http://www.w3.org/2001/XMLSchema#nonNegativeInteger">1</owl:maxQualifiedCardinality>
                <owl:onDataRange rdf:resource="http://www.w3.org/2001/XMLSchema#string"/>
            </owl:Restriction>
        </rdfs:subClassOf>
        <rdfs:comment>An Entity that is an individual human being</rdfs:comment>
    </owl:Class>
    


    <!-- http://www.sisostds.org/ontologies/C2SIM#PhysicalConcept -->

    <owl:Class rdf:about="http://www.sisostds.org/ontologies/C2SIM#PhysicalConcept">
        <rdfs:subClassOf rdf:resource="http://www.sisostds.org/ontologies/C2SIM#C2SIMContent"/>
        <rdfs:comment>Concepts relating to the physical characteristics of an entity (e.g., location, health, orientation, size, etc.). The subclasses of this class have complex or alternative representations, and so are classes. Other physical properties such as mass that are simple scalars can be data type properties of (ConcreteEntity) objects.</rdfs:comment>
    </owl:Class>
    


    <!-- http://www.sisostds.org/ontologies/C2SIM#PhysicalEntity -->

    <owl:Class rdf:about="http://www.sisostds.org/ontologies/C2SIM#PhysicalEntity">
        <rdfs:subClassOf rdf:resource="http://www.sisostds.org/ontologies/C2SIM#Entity"/>
        <rdfs:subClassOf>
            <owl:Restriction>
                <owl:onProperty rdf:resource="http://www.sisostds.org/ontologies/C2SIM#hasCurrentState"/>
                <owl:qualifiedCardinality rdf:datatype="http://www.w3.org/2001/XMLSchema#nonNegativeInteger">1</owl:qualifiedCardinality>
                <owl:onClass rdf:resource="http://www.sisostds.org/ontologies/C2SIM#PhysicalState"/>
            </owl:Restriction>
        </rdfs:subClassOf>
        <rdfs:subClassOf>
            <owl:Restriction>
                <owl:onProperty rdf:resource="http://www.sisostds.org/ontologies/C2SIM#hasMarking"/>
                <owl:maxQualifiedCardinality rdf:datatype="http://www.w3.org/2001/XMLSchema#nonNegativeInteger">1</owl:maxQualifiedCardinality>
                <owl:onDataRange rdf:resource="http://www.w3.org/2001/XMLSchema#string"/>
            </owl:Restriction>
        </rdfs:subClassOf>
        <rdfs:comment>An Entity that has physical/kinematic properties.</rdfs:comment>
    </owl:Class>
    


    <!-- http://www.sisostds.org/ontologies/C2SIM#PhysicalState -->

    <owl:Class rdf:about="http://www.sisostds.org/ontologies/C2SIM#PhysicalState">
        <rdfs:subClassOf rdf:resource="http://www.sisostds.org/ontologies/C2SIM#EntityState"/>
        <rdfs:subClassOf>
            <owl:Restriction>
                <owl:onProperty rdf:resource="http://www.sisostds.org/ontologies/C2SIM#hasEntityHealthStatus"/>
                <owl:minQualifiedCardinality rdf:datatype="http://www.w3.org/2001/XMLSchema#nonNegativeInteger">0</owl:minQualifiedCardinality>
                <owl:onClass rdf:resource="http://www.sisostds.org/ontologies/C2SIM#EntityHealthStatus"/>
            </owl:Restriction>
        </rdfs:subClassOf>
        <rdfs:subClassOf>
            <owl:Restriction>
                <owl:onProperty rdf:resource="http://www.sisostds.org/ontologies/C2SIM#hasLocation"/>
                <owl:minQualifiedCardinality rdf:datatype="http://www.w3.org/2001/XMLSchema#nonNegativeInteger">1</owl:minQualifiedCardinality>
                <owl:onClass rdf:resource="http://www.sisostds.org/ontologies/C2SIM#Location"/>
            </owl:Restriction>
        </rdfs:subClassOf>
        <rdfs:subClassOf>
            <owl:Restriction>
                <owl:onProperty rdf:resource="http://www.sisostds.org/ontologies/C2SIM#hasDirectionOfMovement"/>
                <owl:maxQualifiedCardinality rdf:datatype="http://www.w3.org/2001/XMLSchema#nonNegativeInteger">1</owl:maxQualifiedCardinality>
                <owl:onClass rdf:resource="http://www.sisostds.org/ontologies/C2SIM#Orientation"/>
            </owl:Restriction>
        </rdfs:subClassOf>
        <rdfs:subClassOf>
            <owl:Restriction>
                <owl:onProperty rdf:resource="http://www.sisostds.org/ontologies/C2SIM#hasOrientation"/>
                <owl:maxQualifiedCardinality rdf:datatype="http://www.w3.org/2001/XMLSchema#nonNegativeInteger">1</owl:maxQualifiedCardinality>
                <owl:onClass rdf:resource="http://www.sisostds.org/ontologies/C2SIM#Orientation"/>
            </owl:Restriction>
        </rdfs:subClassOf>
        <rdfs:subClassOf>
            <owl:Restriction>
                <owl:onProperty rdf:resource="http://www.sisostds.org/ontologies/C2SIM#hasSpeed"/>
                <owl:maxQualifiedCardinality rdf:datatype="http://www.w3.org/2001/XMLSchema#nonNegativeInteger">1</owl:maxQualifiedCardinality>
                <owl:onDataRange rdf:resource="http://www.w3.org/2001/XMLSchema#double"/>
            </owl:Restriction>
        </rdfs:subClassOf>
        <rdfs:comment>Description of the physical state of an entity, including location, orientation, health, speed, etc.
Note that an EnvironmentalState class should be a subclass of PhysicalState. The EnvironmentalState could be the state of, for example, a smoke plume, which would have a location and could have direction, orientation, and speed.</rdfs:comment>
    </owl:Class>
    <owl:Axiom>
        <owl:annotatedSource rdf:resource="http://www.sisostds.org/ontologies/C2SIM#PhysicalState"/>
        <owl:annotatedProperty rdf:resource="http://www.w3.org/2000/01/rdf-schema#subClassOf"/>
        <owl:annotatedTarget>
            <owl:Restriction>
                <owl:onProperty rdf:resource="http://www.sisostds.org/ontologies/C2SIM#hasEntityHealthStatus"/>
                <owl:minQualifiedCardinality rdf:datatype="http://www.w3.org/2001/XMLSchema#nonNegativeInteger">0</owl:minQualifiedCardinality>
                <owl:onClass rdf:resource="http://www.sisostds.org/ontologies/C2SIM#EntityHealthStatus"/>
            </owl:Restriction>
        </owl:annotatedTarget>
        <rdfs:comment>This property has cardinality 0+ to allow for multiple health measures, e.g. operational status and a resource status.</rdfs:comment>
    </owl:Axiom>
    


    <!-- http://www.sisostds.org/ontologies/C2SIM#Platform -->

    <owl:Class rdf:about="http://www.sisostds.org/ontologies/C2SIM#Platform">
        <rdfs:subClassOf rdf:resource="http://www.sisostds.org/ontologies/C2SIM#ActorEntity"/>
        <rdfs:subClassOf>
            <owl:Restriction>
                <owl:onProperty rdf:resource="http://www.sisostds.org/ontologies/C2SIM#hasCurrentState"/>
                <owl:maxQualifiedCardinality rdf:datatype="http://www.w3.org/2001/XMLSchema#nonNegativeInteger">1</owl:maxQualifiedCardinality>
                <owl:onClass rdf:resource="http://www.sisostds.org/ontologies/C2SIM#PhysicalState"/>
            </owl:Restriction>
        </rdfs:subClassOf>
        <rdfs:subClassOf>
            <owl:Restriction>
                <owl:onProperty rdf:resource="http://www.sisostds.org/ontologies/C2SIM#hasMarking"/>
                <owl:maxQualifiedCardinality rdf:datatype="http://www.w3.org/2001/XMLSchema#nonNegativeInteger">1</owl:maxQualifiedCardinality>
                <owl:onDataRange rdf:resource="http://www.w3.org/2001/XMLSchema#string"/>
            </owl:Restriction>
        </rdfs:subClassOf>
        <rdfs:comment>An Entity that consists of an identifiable type physical equipment and/or software.</rdfs:comment>
    </owl:Class>
    


    <!-- http://www.sisostds.org/ontologies/C2SIM#PlaybackRealtimeMultipleReport -->

    <owl:Class rdf:about="http://www.sisostds.org/ontologies/C2SIM#PlaybackRealtimeMultipleReport">
        <rdfs:subClassOf rdf:resource="http://www.sisostds.org/ontologies/C2SIM#SystemMessageBody"/>
        <rdfs:comment>System command for reporting the current setting of the playbackRealtimeMultiple value indicating the multiple of simulation time to realtime currently set for the playback of recorded messages in the C2SIM coalition of systems.</rdfs:comment>
    </owl:Class>
    


    <!-- http://www.sisostds.org/ontologies/C2SIM#PlaybackStatusCode -->

    <owl:Class rdf:about="http://www.sisostds.org/ontologies/C2SIM#PlaybackStatusCode">
        <rdfs:subClassOf rdf:resource="http://www.sisostds.org/ontologies/C2SIM#MessageCode"/>
        <rdfs:comment>Enumeration of states of the playback of recorded messages.</rdfs:comment>
    </owl:Class>
    


    <!-- http://www.sisostds.org/ontologies/C2SIM#PlaybackStatusReport -->

    <owl:Class rdf:about="http://www.sisostds.org/ontologies/C2SIM#PlaybackStatusReport">
        <rdfs:subClassOf rdf:resource="http://www.sisostds.org/ontologies/C2SIM#SystemMessageBody"/>
        <rdfs:subClassOf>
            <owl:Restriction>
                <owl:onProperty rdf:resource="http://www.sisostds.org/ontologies/C2SIM#hasPlaybackStatusCode"/>
                <owl:qualifiedCardinality rdf:datatype="http://www.w3.org/2001/XMLSchema#nonNegativeInteger">1</owl:qualifiedCardinality>
                <owl:onClass rdf:resource="http://www.sisostds.org/ontologies/C2SIM#PlaybackStatusCode"/>
            </owl:Restriction>
        </rdfs:subClassOf>
        <rdfs:subClassOf>
            <owl:Restriction>
                <owl:onProperty rdf:resource="http://www.sisostds.org/ontologies/C2SIM#hasName"/>
                <owl:qualifiedCardinality rdf:datatype="http://www.w3.org/2001/XMLSchema#nonNegativeInteger">1</owl:qualifiedCardinality>
                <owl:onDataRange rdf:resource="http://www.w3.org/2001/XMLSchema#string"/>
            </owl:Restriction>
        </rdfs:subClassOf>
        <rdfs:subClassOf>
            <owl:Restriction>
                <owl:onProperty rdf:resource="http://www.sisostds.org/ontologies/C2SIM#hasPlaybackRealtimeMultiple"/>
                <owl:qualifiedCardinality rdf:datatype="http://www.w3.org/2001/XMLSchema#nonNegativeInteger">1</owl:qualifiedCardinality>
                <owl:onDataRange rdf:resource="http://www.w3.org/2001/XMLSchema#positiveInteger"/>
            </owl:Restriction>
        </rdfs:subClassOf>
        <rdfs:subClassOf>
            <owl:Restriction>
                <owl:onProperty rdf:resource="http://www.sisostds.org/ontologies/C2SIM#hasPlaybackPosition"/>
                <owl:maxQualifiedCardinality rdf:datatype="http://www.w3.org/2001/XMLSchema#nonNegativeInteger">1</owl:maxQualifiedCardinality>
                <owl:onDataRange rdf:resource="http://www.w3.org/2001/XMLSchema#string"/>
            </owl:Restriction>
        </rdfs:subClassOf>
        <rdfs:subClassOf>
            <owl:Restriction>
                <owl:onProperty rdf:resource="http://www.sisostds.org/ontologies/C2SIM#hasTimeSincePlaybackStart"/>
                <owl:maxQualifiedCardinality rdf:datatype="http://www.w3.org/2001/XMLSchema#nonNegativeInteger">1</owl:maxQualifiedCardinality>
                <owl:onDataRange rdf:resource="http://www.sisostds.org/ontologies/C2SIM#IsoTimeDurationBase"/>
            </owl:Restriction>
        </rdfs:subClassOf>
        <rdfs:comment>System command for reporting the status of the playback of recorded C2SIM messages in a C2SIM coalition of systems. The name refers to the name of the recording being played back at the time of this report. Playback position may be  something like sequence number in the recording file. The format and the meaning of the string value is out of the scope of the C2SIM standard, and should be defined at the Federation level (interoperability across different Federations is not guaranteed). The time since playback start gives the time duration (isoTimeDurationBase) since the start time of the current playback (i.e., the message timestamp that the playback has reached). The playbackRealtimeMultiple is the current setting of the rate at which recorded messages are being played back.</rdfs:comment>
    </owl:Class>
    


    <!-- http://www.sisostds.org/ontologies/C2SIM#PositionReportContent -->

    <owl:Class rdf:about="http://www.sisostds.org/ontologies/C2SIM#PositionReportContent">
        <rdfs:subClassOf rdf:resource="http://www.sisostds.org/ontologies/C2SIM#ReportContent"/>
        <rdfs:subClassOf>
            <owl:Restriction>
                <owl:onProperty rdf:resource="http://www.sisostds.org/ontologies/C2SIM#hasEntityHealthStatus"/>
                <owl:minQualifiedCardinality rdf:datatype="http://www.w3.org/2001/XMLSchema#nonNegativeInteger">0</owl:minQualifiedCardinality>
                <owl:onClass rdf:resource="http://www.sisostds.org/ontologies/C2SIM#EntityHealthStatus"/>
            </owl:Restriction>
        </rdfs:subClassOf>
        <rdfs:subClassOf>
            <owl:Restriction>
                <owl:onProperty rdf:resource="http://www.sisostds.org/ontologies/C2SIM#hasLocation"/>
                <owl:maxQualifiedCardinality rdf:datatype="http://www.w3.org/2001/XMLSchema#nonNegativeInteger">1</owl:maxQualifiedCardinality>
                <owl:onClass rdf:resource="http://www.sisostds.org/ontologies/C2SIM#Location"/>
            </owl:Restriction>
        </rdfs:subClassOf>
        <rdfs:subClassOf>
            <owl:Restriction>
                <owl:onProperty rdf:resource="http://www.sisostds.org/ontologies/C2SIM#hasHeadingAngle"/>
                <owl:maxQualifiedCardinality rdf:datatype="http://www.w3.org/2001/XMLSchema#nonNegativeInteger">1</owl:maxQualifiedCardinality>
                <owl:onDataRange rdf:resource="http://www.sisostds.org/ontologies/C2SIM#angle"/>
            </owl:Restriction>
        </rdfs:subClassOf>
        <rdfs:subClassOf>
            <owl:Restriction>
                <owl:onProperty rdf:resource="http://www.sisostds.org/ontologies/C2SIM#hasSpeed"/>
                <owl:maxQualifiedCardinality rdf:datatype="http://www.w3.org/2001/XMLSchema#nonNegativeInteger">1</owl:maxQualifiedCardinality>
                <owl:onDataRange rdf:resource="http://www.w3.org/2001/XMLSchema#double"/>
            </owl:Restriction>
        </rdfs:subClassOf>
        <rdfs:subClassOf>
            <owl:Restriction>
                <owl:onProperty rdf:resource="http://www.sisostds.org/ontologies/C2SIM#hasSubjectEntity"/>
                <owl:maxQualifiedCardinality rdf:datatype="http://www.w3.org/2001/XMLSchema#nonNegativeInteger">1</owl:maxQualifiedCardinality>
                <owl:onDataRange rdf:resource="http://www.sisostds.org/ontologies/C2SIM#UUIDBase"/>
            </owl:Restriction>
        </rdfs:subClassOf>
        <rdfs:comment>The content of a report that is used primarily to convey the position of an entity.</rdfs:comment>
    </owl:Class>
    <owl:Axiom>
        <owl:annotatedSource rdf:resource="http://www.sisostds.org/ontologies/C2SIM#PositionReportContent"/>
        <owl:annotatedProperty rdf:resource="http://www.w3.org/2000/01/rdf-schema#subClassOf"/>
        <owl:annotatedTarget>
            <owl:Restriction>
                <owl:onProperty rdf:resource="http://www.sisostds.org/ontologies/C2SIM#hasSubjectEntity"/>
                <owl:maxQualifiedCardinality rdf:datatype="http://www.w3.org/2001/XMLSchema#nonNegativeInteger">1</owl:maxQualifiedCardinality>
                <owl:onDataRange rdf:resource="http://www.sisostds.org/ontologies/C2SIM#UUIDBase"/>
            </owl:Restriction>
        </owl:annotatedTarget>
        <rdfs:comment>This is the unique identifier of an individual of the ActorEntity class. This property is omitted if the report is about the reporting entity. However, it must be included if the report is about, e.g., a subordinate.</rdfs:comment>
    </owl:Axiom>
    


    <!-- http://www.sisostds.org/ontologies/C2SIM#RecordingStatusCode -->

    <owl:Class rdf:about="http://www.sisostds.org/ontologies/C2SIM#RecordingStatusCode">
        <rdfs:subClassOf rdf:resource="http://www.sisostds.org/ontologies/C2SIM#MessageCode"/>
        <rdfs:comment>Enumeration of states of the recording of messages sent during execution of a C2SIM coalition of systems.</rdfs:comment>
    </owl:Class>
    


    <!-- http://www.sisostds.org/ontologies/C2SIM#RecordingStatusReport -->

    <owl:Class rdf:about="http://www.sisostds.org/ontologies/C2SIM#RecordingStatusReport">
        <rdfs:subClassOf rdf:resource="http://www.sisostds.org/ontologies/C2SIM#SystemMessageBody"/>
        <rdfs:subClassOf>
            <owl:Restriction>
                <owl:onProperty rdf:resource="http://www.sisostds.org/ontologies/C2SIM#hasRecordingStatusCode"/>
                <owl:qualifiedCardinality rdf:datatype="http://www.w3.org/2001/XMLSchema#nonNegativeInteger">1</owl:qualifiedCardinality>
                <owl:onClass rdf:resource="http://www.sisostds.org/ontologies/C2SIM#RecordingStatusCode"/>
            </owl:Restriction>
        </rdfs:subClassOf>
        <rdfs:subClassOf>
            <owl:Restriction>
                <owl:onProperty rdf:resource="http://www.sisostds.org/ontologies/C2SIM#hasFileSize"/>
                <owl:qualifiedCardinality rdf:datatype="http://www.w3.org/2001/XMLSchema#nonNegativeInteger">1</owl:qualifiedCardinality>
                <owl:onDataRange rdf:resource="http://www.w3.org/2001/XMLSchema#nonNegativeInteger"/>
            </owl:Restriction>
        </rdfs:subClassOf>
        <rdfs:subClassOf>
            <owl:Restriction>
                <owl:onProperty rdf:resource="http://www.sisostds.org/ontologies/C2SIM#hasName"/>
                <owl:qualifiedCardinality rdf:datatype="http://www.w3.org/2001/XMLSchema#nonNegativeInteger">1</owl:qualifiedCardinality>
                <owl:onDataRange rdf:resource="http://www.w3.org/2001/XMLSchema#string"/>
            </owl:Restriction>
        </rdfs:subClassOf>
        <rdfs:comment>System command for reporting the status of the recording of C2SIM messages in a C2SIM coalition of systems. The name refers to the name given to this recording. The file size is the size of the recording file in bytes (could be a &quot;current&quot; file size if a recording is in progress at the time of this report).</rdfs:comment>
    </owl:Class>
    


    <!-- http://www.sisostds.org/ontologies/C2SIM#RefreshInit -->

    <owl:Class rdf:about="http://www.sisostds.org/ontologies/C2SIM#RefreshInit">
        <rdfs:subClassOf rdf:resource="http://www.sisostds.org/ontologies/C2SIM#SystemMessageBody"/>
        <rdfs:subClassOf>
            <owl:Restriction>
                <owl:onProperty rdf:resource="http://www.sisostds.org/ontologies/C2SIM#hasRefreshInitSelection"/>
                <owl:qualifiedCardinality rdf:datatype="http://www.w3.org/2001/XMLSchema#nonNegativeInteger">1</owl:qualifiedCardinality>
                <owl:onClass rdf:resource="http://www.sisostds.org/ontologies/C2SIM#RefreshInitSelection"/>
            </owl:Restriction>
        </rdfs:subClassOf>
        <rdfs:comment>This system command supports late joiners to the C2SIM coalition of systems. It causes a fresh copy of the C2SIMInitialization message to be sent to the requesting system. Command parameters indicate that either a copy of the startup initialization (INITIALIZATION_ORIGINAL) or an updated version with latest reported positions of each ActorEntity (INITIALIZATION_LATEST_POSITIONS) be sent to the requesting system.</rdfs:comment>
    </owl:Class>
    


    <!-- http://www.sisostds.org/ontologies/C2SIM#RefreshInitSelection -->

    <owl:Class rdf:about="http://www.sisostds.org/ontologies/C2SIM#RefreshInitSelection">
        <rdfs:subClassOf rdf:resource="http://www.sisostds.org/ontologies/C2SIM#MessageCode"/>
        <rdfs:comment>Enumeration of initialization request options for a late joiner to a C2SIM coalition of systems.</rdfs:comment>
    </owl:Class>
    


    <!-- http://www.sisostds.org/ontologies/C2SIM#Relationship -->

    <owl:Class rdf:about="http://www.sisostds.org/ontologies/C2SIM#Relationship">
        <rdfs:subClassOf rdf:resource="http://www.sisostds.org/ontologies/C2SIM#C2SIMContent"/>
        <rdfs:comment>This class describes a relationship to some entity. The type of relationship is defined by a subclass, which has a code property that specifies what the relationship is.</rdfs:comment>
    </owl:Class>
    


    <!-- http://www.sisostds.org/ontologies/C2SIM#RelativeLocation -->

    <owl:Class rdf:about="http://www.sisostds.org/ontologies/C2SIM#RelativeLocation">
        <rdfs:subClassOf rdf:resource="http://www.sisostds.org/ontologies/C2SIM#Location"/>
        <rdfs:subClassOf>
            <owl:Restriction>
                <owl:onProperty rdf:resource="http://www.sisostds.org/ontologies/C2SIM#hasSpatialOffset"/>
                <owl:maxQualifiedCardinality rdf:datatype="http://www.w3.org/2001/XMLSchema#nonNegativeInteger">1</owl:maxQualifiedCardinality>
                <owl:onClass rdf:resource="http://www.sisostds.org/ontologies/C2SIM#SpatialOffset"/>
            </owl:Restriction>
        </rdfs:subClassOf>
        <rdfs:subClassOf>
            <owl:Restriction>
                <owl:onProperty rdf:resource="http://www.sisostds.org/ontologies/C2SIM#hasEntityReference"/>
                <owl:qualifiedCardinality rdf:datatype="http://www.w3.org/2001/XMLSchema#nonNegativeInteger">1</owl:qualifiedCardinality>
                <owl:onDataRange rdf:resource="http://www.sisostds.org/ontologies/C2SIM#UUIDBase"/>
            </owl:Restriction>
        </rdfs:subClassOf>
        <rdfs:comment>A location defined by an offset to some reference location.</rdfs:comment>
    </owl:Class>
    <owl:Axiom>
        <owl:annotatedSource rdf:resource="http://www.sisostds.org/ontologies/C2SIM#RelativeLocation"/>
        <owl:annotatedProperty rdf:resource="http://www.w3.org/2000/01/rdf-schema#subClassOf"/>
        <owl:annotatedTarget>
            <owl:Restriction>
                <owl:onProperty rdf:resource="http://www.sisostds.org/ontologies/C2SIM#hasEntityReference"/>
                <owl:qualifiedCardinality rdf:datatype="http://www.w3.org/2001/XMLSchema#nonNegativeInteger">1</owl:qualifiedCardinality>
                <owl:onDataRange rdf:resource="http://www.sisostds.org/ontologies/C2SIM#UUIDBase"/>
            </owl:Restriction>
        </owl:annotatedTarget>
        <rdfs:comment>This is the unique identifier of an individual of the Entity class whose location is the reference for this location. The individual is defined elsewhere.</rdfs:comment>
    </owl:Axiom>
    


    <!-- http://www.sisostds.org/ontologies/C2SIM#RelativeTime -->

    <owl:Class rdf:about="http://www.sisostds.org/ontologies/C2SIM#RelativeTime">
        <rdfs:subClassOf rdf:resource="http://www.sisostds.org/ontologies/C2SIM#TimeInstant"/>
        <rdfs:subClassOf>
            <owl:Restriction>
                <owl:onProperty rdf:resource="http://www.sisostds.org/ontologies/C2SIM#hasDelayTimeAmount"/>
                <owl:qualifiedCardinality rdf:datatype="http://www.w3.org/2001/XMLSchema#nonNegativeInteger">1</owl:qualifiedCardinality>
                <owl:onClass rdf:resource="http://www.sisostds.org/ontologies/C2SIM#Duration"/>
            </owl:Restriction>
        </rdfs:subClassOf>
        <rdfs:subClassOf>
            <owl:Restriction>
                <owl:onProperty rdf:resource="http://www.sisostds.org/ontologies/C2SIM#hasTimeReferenceCode"/>
                <owl:qualifiedCardinality rdf:datatype="http://www.w3.org/2001/XMLSchema#nonNegativeInteger">1</owl:qualifiedCardinality>
                <owl:onClass rdf:resource="http://www.sisostds.org/ontologies/C2SIM#TimeReferenceCode"/>
            </owl:Restriction>
        </rdfs:subClassOf>
        <rdfs:subClassOf>
            <owl:Restriction>
                <owl:onProperty rdf:resource="http://www.sisostds.org/ontologies/C2SIM#hasEventReference"/>
                <owl:qualifiedCardinality rdf:datatype="http://www.w3.org/2001/XMLSchema#nonNegativeInteger">1</owl:qualifiedCardinality>
                <owl:onDataRange rdf:resource="http://www.sisostds.org/ontologies/C2SIM#UUIDBase"/>
            </owl:Restriction>
        </rdfs:subClassOf>
        <rdfs:comment>Specifies an absolute time relative to the start or end time of an event.</rdfs:comment>
    </owl:Class>
    <owl:Axiom>
        <owl:annotatedSource rdf:resource="http://www.sisostds.org/ontologies/C2SIM#RelativeTime"/>
        <owl:annotatedProperty rdf:resource="http://www.w3.org/2000/01/rdf-schema#subClassOf"/>
        <owl:annotatedTarget>
            <owl:Restriction>
                <owl:onProperty rdf:resource="http://www.sisostds.org/ontologies/C2SIM#hasEventReference"/>
                <owl:qualifiedCardinality rdf:datatype="http://www.w3.org/2001/XMLSchema#nonNegativeInteger">1</owl:qualifiedCardinality>
                <owl:onDataRange rdf:resource="http://www.sisostds.org/ontologies/C2SIM#UUIDBase"/>
            </owl:Restriction>
        </owl:annotatedTarget>
        <rdfs:comment>This is the unique identifier of an individual of theh Event class that is the reference for this time instant. If the Event has a duration, then the time reference is the start time of the event.</rdfs:comment>
    </owl:Axiom>
    


    <!-- http://www.sisostds.org/ontologies/C2SIM#ReligionCode -->

    <owl:Class rdf:about="http://www.sisostds.org/ontologies/C2SIM#ReligionCode">
        <rdfs:subClassOf rdf:resource="http://www.sisostds.org/ontologies/C2SIM#OrganizationCode"/>
        <rdfs:comment>Alphabetic code, up to six letters, representing a religion, obtained from JC3IEDM-3.0.2 AffiliationReligionCode</rdfs:comment>
    </owl:Class>
    


    <!-- http://www.sisostds.org/ontologies/C2SIM#ReportBody -->

    <owl:Class rdf:about="http://www.sisostds.org/ontologies/C2SIM#ReportBody">
        <rdfs:subClassOf rdf:resource="http://www.sisostds.org/ontologies/C2SIM#DomainMessageBody"/>
        <rdfs:subClassOf>
            <owl:Restriction>
                <owl:onProperty rdf:resource="http://www.sisostds.org/ontologies/C2SIM#hasReportContent"/>
                <owl:minQualifiedCardinality rdf:datatype="http://www.w3.org/2001/XMLSchema#nonNegativeInteger">1</owl:minQualifiedCardinality>
                <owl:onClass rdf:resource="http://www.sisostds.org/ontologies/C2SIM#ReportContent"/>
            </owl:Restriction>
        </rdfs:subClassOf>
        <rdfs:subClassOf>
            <owl:Restriction>
                <owl:onProperty rdf:resource="http://www.sisostds.org/ontologies/C2SIM#hasReportID"/>
                <owl:qualifiedCardinality rdf:datatype="http://www.w3.org/2001/XMLSchema#nonNegativeInteger">1</owl:qualifiedCardinality>
                <owl:onDataRange rdf:resource="http://www.sisostds.org/ontologies/C2SIM#UUIDBase"/>
            </owl:Restriction>
        </rdfs:subClassOf>
        <rdfs:subClassOf>
            <owl:Restriction>
                <owl:onProperty rdf:resource="http://www.sisostds.org/ontologies/C2SIM#hasReportingEntity"/>
                <owl:qualifiedCardinality rdf:datatype="http://www.w3.org/2001/XMLSchema#nonNegativeInteger">1</owl:qualifiedCardinality>
                <owl:onDataRange rdf:resource="http://www.sisostds.org/ontologies/C2SIM#UUIDBase"/>
            </owl:Restriction>
        </rdfs:subClassOf>
        <rdfs:comment>The structure for sending report messages.</rdfs:comment>
    </owl:Class>
    <owl:Axiom>
        <owl:annotatedSource rdf:resource="http://www.sisostds.org/ontologies/C2SIM#ReportBody"/>
        <owl:annotatedProperty rdf:resource="http://www.w3.org/2000/01/rdf-schema#subClassOf"/>
        <owl:annotatedTarget>
            <owl:Restriction>
                <owl:onProperty rdf:resource="http://www.sisostds.org/ontologies/C2SIM#hasReportingEntity"/>
                <owl:qualifiedCardinality rdf:datatype="http://www.w3.org/2001/XMLSchema#nonNegativeInteger">1</owl:qualifiedCardinality>
                <owl:onDataRange rdf:resource="http://www.sisostds.org/ontologies/C2SIM#UUIDBase"/>
            </owl:Restriction>
        </owl:annotatedTarget>
        <rdfs:comment>This is the unique identifier of an individual of the ActorEntity class, that is making the report.</rdfs:comment>
    </owl:Axiom>
    


    <!-- http://www.sisostds.org/ontologies/C2SIM#ReportContent -->

    <owl:Class rdf:about="http://www.sisostds.org/ontologies/C2SIM#ReportContent">
        <rdfs:subClassOf rdf:resource="http://www.sisostds.org/ontologies/C2SIM#MessageConcept"/>
        <rdfs:subClassOf>
            <owl:Restriction>
                <owl:onProperty rdf:resource="http://www.sisostds.org/ontologies/C2SIM#hasTimeOfObservation"/>
                <owl:qualifiedCardinality rdf:datatype="http://www.w3.org/2001/XMLSchema#nonNegativeInteger">1</owl:qualifiedCardinality>
                <owl:onClass rdf:resource="http://www.sisostds.org/ontologies/C2SIM#DateTime"/>
            </owl:Restriction>
        </rdfs:subClassOf>
        <rdfs:subClassOf>
            <owl:Restriction>
                <owl:onProperty rdf:resource="http://www.sisostds.org/ontologies/C2SIM#hasDuration"/>
                <owl:maxQualifiedCardinality rdf:datatype="http://www.w3.org/2001/XMLSchema#nonNegativeInteger">1</owl:maxQualifiedCardinality>
                <owl:onClass rdf:resource="http://www.sisostds.org/ontologies/C2SIM#Duration"/>
            </owl:Restriction>
        </rdfs:subClassOf>
        <rdfs:comment>This is a collection class that may be used for different types of messages reporting information to other systems.</rdfs:comment>
    </owl:Class>
    <owl:Axiom>
        <owl:annotatedSource rdf:resource="http://www.sisostds.org/ontologies/C2SIM#ReportContent"/>
        <owl:annotatedProperty rdf:resource="http://www.w3.org/2000/01/rdf-schema#subClassOf"/>
        <owl:annotatedTarget>
            <owl:Restriction>
                <owl:onProperty rdf:resource="http://www.sisostds.org/ontologies/C2SIM#hasDuration"/>
                <owl:maxQualifiedCardinality rdf:datatype="http://www.w3.org/2001/XMLSchema#nonNegativeInteger">1</owl:maxQualifiedCardinality>
                <owl:onClass rdf:resource="http://www.sisostds.org/ontologies/C2SIM#Duration"/>
            </owl:Restriction>
        </owl:annotatedTarget>
        <rdfs:comment>Optional duration to specify the interval of time (a duration prior to the given observation time) over which the observation was made.</rdfs:comment>
    </owl:Axiom>
    


    <!-- http://www.sisostds.org/ontologies/C2SIM#RequestBody -->

    <owl:Class rdf:about="http://www.sisostds.org/ontologies/C2SIM#RequestBody">
        <rdfs:subClassOf rdf:resource="http://www.sisostds.org/ontologies/C2SIM#DomainMessageBody"/>
        <rdfs:subClassOf>
            <owl:Restriction>
                <owl:onProperty rdf:resource="http://www.sisostds.org/ontologies/C2SIM#hasRequestContent"/>
                <owl:minQualifiedCardinality rdf:datatype="http://www.w3.org/2001/XMLSchema#nonNegativeInteger">1</owl:minQualifiedCardinality>
                <owl:onClass rdf:resource="http://www.sisostds.org/ontologies/C2SIM#RequestContent"/>
            </owl:Restriction>
        </rdfs:subClassOf>
        <rdfs:subClassOf>
            <owl:Restriction>
                <owl:onProperty rdf:resource="http://www.sisostds.org/ontologies/C2SIM#hasRequestingEntity"/>
                <owl:qualifiedCardinality rdf:datatype="http://www.w3.org/2001/XMLSchema#nonNegativeInteger">1</owl:qualifiedCardinality>
                <owl:onDataRange rdf:resource="http://www.sisostds.org/ontologies/C2SIM#UUIDBase"/>
            </owl:Restriction>
        </rdfs:subClassOf>
        <rdfs:comment>The body of a message from an actor in the domain to another actor in the domain that requests something.
A request is fulfilled at the discretion of the entity to which it is directed.</rdfs:comment>
    </owl:Class>
    


    <!-- http://www.sisostds.org/ontologies/C2SIM#RequestContent -->

    <owl:Class rdf:about="http://www.sisostds.org/ontologies/C2SIM#RequestContent">
        <rdfs:subClassOf rdf:resource="http://www.sisostds.org/ontologies/C2SIM#MessageConcept"/>
        <rdfs:comment>The content of a request message in the domain. This is a parent class that has subclasses for different types of requests.</rdfs:comment>
    </owl:Class>
    


    <!-- http://www.sisostds.org/ontologies/C2SIM#RequestPlaybackRealtimeMultiple -->

    <owl:Class rdf:about="http://www.sisostds.org/ontologies/C2SIM#RequestPlaybackRealtimeMultiple">
        <rdfs:subClassOf rdf:resource="http://www.sisostds.org/ontologies/C2SIM#SystemMessageBody"/>
        <rdfs:comment>System command for requesting the current setting of the playbackRealtimeMultiple value indicating the multiple of simulation time to realtime currently set for recording playback in the C2SIM coalition of systems.</rdfs:comment>
    </owl:Class>
    


    <!-- http://www.sisostds.org/ontologies/C2SIM#RequestPlaybackStatus -->

    <owl:Class rdf:about="http://www.sisostds.org/ontologies/C2SIM#RequestPlaybackStatus">
        <rdfs:subClassOf rdf:resource="http://www.sisostds.org/ontologies/C2SIM#SystemMessageBody"/>
        <rdfs:comment>System command for requesting information about the current playback of recorded C2SIM messages in a C2SIM coalition of systems.</rdfs:comment>
    </owl:Class>
    


    <!-- http://www.sisostds.org/ontologies/C2SIM#RequestRecordingStatus -->

    <owl:Class rdf:about="http://www.sisostds.org/ontologies/C2SIM#RequestRecordingStatus">
        <rdfs:subClassOf rdf:resource="http://www.sisostds.org/ontologies/C2SIM#SystemMessageBody"/>
        <rdfs:comment>System command for requesting information about the current recording of C2SIM messages in a C2SIM coalition of systems.</rdfs:comment>
    </owl:Class>
    


    <!-- http://www.sisostds.org/ontologies/C2SIM#RequestSimulationRealtimeMultiple -->

    <owl:Class rdf:about="http://www.sisostds.org/ontologies/C2SIM#RequestSimulationRealtimeMultiple">
        <rdfs:subClassOf rdf:resource="http://www.sisostds.org/ontologies/C2SIM#SystemMessageBody"/>
        <rdfs:comment>System command for requesting the current setting of the simuationRealtimeMultiple value indicating the multiple of simulation time to realtime currently set for the simulation systems in the C2SIM coalition of systems.</rdfs:comment>
    </owl:Class>
    


    <!-- http://www.sisostds.org/ontologies/C2SIM#ResetScenario -->

    <owl:Class rdf:about="http://www.sisostds.org/ontologies/C2SIM#ResetScenario">
        <rdfs:subClassOf rdf:resource="http://www.sisostds.org/ontologies/C2SIM#SystemMessageBody"/>
    </owl:Class>
    


    <!-- http://www.sisostds.org/ontologies/C2SIM#Resource -->

    <owl:Class rdf:about="http://www.sisostds.org/ontologies/C2SIM#Resource">
        <rdfs:subClassOf rdf:resource="http://www.sisostds.org/ontologies/C2SIM#C2SIMContent"/>
        <rdfs:subClassOf>
            <owl:Restriction>
                <owl:onProperty rdf:resource="http://www.sisostds.org/ontologies/C2SIM#hasSISOEntityType"/>
                <owl:qualifiedCardinality rdf:datatype="http://www.w3.org/2001/XMLSchema#nonNegativeInteger">1</owl:qualifiedCardinality>
                <owl:onClass rdf:resource="http://www.sisostds.org/ontologies/C2SIM#SISOEntityType"/>
            </owl:Restriction>
        </rdfs:subClassOf>
        <rdfs:subClassOf>
            <owl:Restriction>
                <owl:onProperty rdf:resource="http://www.sisostds.org/ontologies/C2SIM#hasOperationalQuantity"/>
                <owl:qualifiedCardinality rdf:datatype="http://www.w3.org/2001/XMLSchema#nonNegativeInteger">1</owl:qualifiedCardinality>
                <owl:onDataRange rdf:resource="http://www.w3.org/2001/XMLSchema#double"/>
            </owl:Restriction>
        </rdfs:subClassOf>
        <rdfs:subClassOf>
            <owl:Restriction>
                <owl:onProperty rdf:resource="http://www.sisostds.org/ontologies/C2SIM#hasName"/>
                <owl:maxQualifiedCardinality rdf:datatype="http://www.w3.org/2001/XMLSchema#nonNegativeInteger">1</owl:maxQualifiedCardinality>
                <owl:onDataRange rdf:resource="http://www.w3.org/2001/XMLSchema#string"/>
            </owl:Restriction>
        </rdfs:subClassOf>
        <rdfs:subClassOf>
            <owl:Restriction>
                <owl:onProperty rdf:resource="http://www.sisostds.org/ontologies/C2SIM#hasOnHandQuantity"/>
                <owl:maxQualifiedCardinality rdf:datatype="http://www.w3.org/2001/XMLSchema#nonNegativeInteger">1</owl:maxQualifiedCardinality>
                <owl:onDataRange rdf:resource="http://www.w3.org/2001/XMLSchema#double"/>
            </owl:Restriction>
        </rdfs:subClassOf>
        <rdfs:subClassOf>
            <owl:Restriction>
                <owl:onProperty rdf:resource="http://www.sisostds.org/ontologies/C2SIM#hasRequiredOnHandQuantity"/>
                <owl:maxQualifiedCardinality rdf:datatype="http://www.w3.org/2001/XMLSchema#nonNegativeInteger">1</owl:maxQualifiedCardinality>
                <owl:onDataRange rdf:resource="http://www.w3.org/2001/XMLSchema#double"/>
            </owl:Restriction>
        </rdfs:subClassOf>
        <rdfs:comment>This is a resource that can be part of, transferred to, or removed from an object (Entity), but is not an entity itself; therefore it does not have a location, extent, or other physical attributes.
Resource can be used to manage (a) consumable material (such as ammunition and fuel); (b) equipment (such as weapons, vehicles, and communication devices); and (c) personnel.
A resource is defined by the SISO entity type of the resource, the operational quantity of the resource (available for operations), and optionnaly with required and &quot;on hand&quot; quantities.</rdfs:comment>
    </owl:Class>
    


    <!-- http://www.sisostds.org/ontologies/C2SIM#Resources -->

    <owl:Class rdf:about="http://www.sisostds.org/ontologies/C2SIM#Resources">
        <rdfs:subClassOf rdf:resource="http://www.sisostds.org/ontologies/C2SIM#EntityHealthStatus"/>
        <rdfs:subClassOf>
            <owl:Restriction>
                <owl:onProperty rdf:resource="http://www.sisostds.org/ontologies/C2SIM#hasResource"/>
                <owl:minQualifiedCardinality rdf:datatype="http://www.w3.org/2001/XMLSchema#nonNegativeInteger">1</owl:minQualifiedCardinality>
                <owl:onClass rdf:resource="http://www.sisostds.org/ontologies/C2SIM#Resource"/>
            </owl:Restriction>
        </rdfs:subClassOf>
        <rdfs:comment>A level of personnel, equipment, ammunition, fuel, etc. The user must compare this to the full strength of the unit.</rdfs:comment>
    </owl:Class>
    


    <!-- http://www.sisostds.org/ontologies/C2SIM#ResumePlayback -->

    <owl:Class rdf:about="http://www.sisostds.org/ontologies/C2SIM#ResumePlayback">
        <rdfs:subClassOf rdf:resource="http://www.sisostds.org/ontologies/C2SIM#SystemMessageBody"/>
        <rdfs:comment>System command for ordering resumption of the current playback of C2SIM messages in a C2SIM coalition of systems. The name of the recording being played back is not needed here since there can be only one playback in progress at a time.</rdfs:comment>
    </owl:Class>
    


    <!-- http://www.sisostds.org/ontologies/C2SIM#ResumeRecording -->

    <owl:Class rdf:about="http://www.sisostds.org/ontologies/C2SIM#ResumeRecording">
        <rdfs:subClassOf rdf:resource="http://www.sisostds.org/ontologies/C2SIM#SystemMessageBody"/>
        <rdfs:comment>System command for ordering resumption of recording of C2SIM messages in a C2SIM coalition of systems. The name of the recording in progress is not needed here since there can be only one recording in progress at a time.</rdfs:comment>
    </owl:Class>
    


    <!-- http://www.sisostds.org/ontologies/C2SIM#ResumeScenario -->

    <owl:Class rdf:about="http://www.sisostds.org/ontologies/C2SIM#ResumeScenario">
        <rdfs:subClassOf rdf:resource="http://www.sisostds.org/ontologies/C2SIM#SystemMessageBody"/>
        <rdfs:comment>A system command to resume the paused execution of a scenario across a C2SIM coalition of systems.</rdfs:comment>
    </owl:Class>
    


    <!-- http://www.sisostds.org/ontologies/C2SIM#SISOEntityType -->

    <owl:Class rdf:about="http://www.sisostds.org/ontologies/C2SIM#SISOEntityType">
        <rdfs:subClassOf rdf:resource="http://www.sisostds.org/ontologies/C2SIM#C2SIMContent"/>
        <rdfs:subClassOf>
            <owl:Restriction>
                <owl:onProperty rdf:resource="http://www.sisostds.org/ontologies/C2SIM#hasDISCategory"/>
                <owl:qualifiedCardinality rdf:datatype="http://www.w3.org/2001/XMLSchema#nonNegativeInteger">1</owl:qualifiedCardinality>
                <owl:onDataRange rdf:resource="http://www.w3.org/2001/XMLSchema#byte"/>
            </owl:Restriction>
        </rdfs:subClassOf>
        <rdfs:subClassOf>
            <owl:Restriction>
                <owl:onProperty rdf:resource="http://www.sisostds.org/ontologies/C2SIM#hasDISCountry"/>
                <owl:qualifiedCardinality rdf:datatype="http://www.w3.org/2001/XMLSchema#nonNegativeInteger">1</owl:qualifiedCardinality>
                <owl:onDataRange rdf:resource="http://www.w3.org/2001/XMLSchema#integer"/>
            </owl:Restriction>
        </rdfs:subClassOf>
        <rdfs:subClassOf>
            <owl:Restriction>
                <owl:onProperty rdf:resource="http://www.sisostds.org/ontologies/C2SIM#hasDISDomain"/>
                <owl:qualifiedCardinality rdf:datatype="http://www.w3.org/2001/XMLSchema#nonNegativeInteger">1</owl:qualifiedCardinality>
                <owl:onDataRange rdf:resource="http://www.w3.org/2001/XMLSchema#byte"/>
            </owl:Restriction>
        </rdfs:subClassOf>
        <rdfs:subClassOf>
            <owl:Restriction>
                <owl:onProperty rdf:resource="http://www.sisostds.org/ontologies/C2SIM#hasDISExtra"/>
                <owl:qualifiedCardinality rdf:datatype="http://www.w3.org/2001/XMLSchema#nonNegativeInteger">1</owl:qualifiedCardinality>
                <owl:onDataRange rdf:resource="http://www.w3.org/2001/XMLSchema#byte"/>
            </owl:Restriction>
        </rdfs:subClassOf>
        <rdfs:subClassOf>
            <owl:Restriction>
                <owl:onProperty rdf:resource="http://www.sisostds.org/ontologies/C2SIM#hasDISKind"/>
                <owl:qualifiedCardinality rdf:datatype="http://www.w3.org/2001/XMLSchema#nonNegativeInteger">1</owl:qualifiedCardinality>
                <owl:onDataRange rdf:resource="http://www.w3.org/2001/XMLSchema#byte"/>
            </owl:Restriction>
        </rdfs:subClassOf>
        <rdfs:subClassOf>
            <owl:Restriction>
                <owl:onProperty rdf:resource="http://www.sisostds.org/ontologies/C2SIM#hasDISSpecific"/>
                <owl:qualifiedCardinality rdf:datatype="http://www.w3.org/2001/XMLSchema#nonNegativeInteger">1</owl:qualifiedCardinality>
                <owl:onDataRange rdf:resource="http://www.w3.org/2001/XMLSchema#byte"/>
            </owl:Restriction>
        </rdfs:subClassOf>
        <rdfs:subClassOf>
            <owl:Restriction>
                <owl:onProperty rdf:resource="http://www.sisostds.org/ontologies/C2SIM#hasDISSubCategory"/>
                <owl:qualifiedCardinality rdf:datatype="http://www.w3.org/2001/XMLSchema#nonNegativeInteger">1</owl:qualifiedCardinality>
                <owl:onDataRange rdf:resource="http://www.w3.org/2001/XMLSchema#byte"/>
            </owl:Restriction>
        </rdfs:subClassOf>
        <rdfs:comment>Simulation Entity Type as specified by SISO-REF-010-2016, Reference for Enumerations for Simulation Interoperability, version 27 (2019). 
Used to define the type of an Entity for its representation and modeling in simulations.</rdfs:comment>
    </owl:Class>
    


    <!-- http://www.sisostds.org/ontologies/C2SIM#ScenarioSetting -->

    <owl:Class rdf:about="http://www.sisostds.org/ontologies/C2SIM#ScenarioSetting">
        <rdfs:subClassOf rdf:resource="http://www.sisostds.org/ontologies/C2SIM#InitializationConcept"/>
        <rdfs:subClassOf>
            <owl:Restriction>
                <owl:onProperty rdf:resource="http://www.sisostds.org/ontologies/C2SIM#hasDateTime"/>
                <owl:qualifiedCardinality rdf:datatype="http://www.w3.org/2001/XMLSchema#nonNegativeInteger">1</owl:qualifiedCardinality>
                <owl:onClass rdf:resource="http://www.sisostds.org/ontologies/C2SIM#DateTime"/>
            </owl:Restriction>
        </rdfs:subClassOf>
        <rdfs:subClassOf>
            <owl:Restriction>
                <owl:onProperty rdf:resource="http://www.sisostds.org/ontologies/C2SIM#hasVersion"/>
                <owl:qualifiedCardinality rdf:datatype="http://www.w3.org/2001/XMLSchema#nonNegativeInteger">1</owl:qualifiedCardinality>
                <owl:onDataRange rdf:resource="http://www.w3.org/2001/XMLSchema#string"/>
            </owl:Restriction>
        </rdfs:subClassOf>
        <rdfs:comment>Information describing the setting of the scenario, including the date, time, physical extent of the terrain, and a version string.</rdfs:comment>
    </owl:Class>
    


    <!-- http://www.sisostds.org/ontologies/C2SIM#SecurityClassificationCode -->

    <owl:Class rdf:about="http://www.sisostds.org/ontologies/C2SIM#SecurityClassificationCode">
        <rdfs:subClassOf rdf:resource="http://www.sisostds.org/ontologies/C2SIM#Code"/>
        <rdfs:comment>Alphabetic text descriptions used by the USA-Department of Defense to identify the level of sensitivity of information</rdfs:comment>
    </owl:Class>
    


    <!-- http://www.sisostds.org/ontologies/C2SIM#SetPlaybackRealtimeMultiple -->

    <owl:Class rdf:about="http://www.sisostds.org/ontologies/C2SIM#SetPlaybackRealtimeMultiple">
        <rdfs:subClassOf rdf:resource="http://www.sisostds.org/ontologies/C2SIM#SystemMessageBody"/>
        <rdfs:subClassOf>
            <owl:Restriction>
                <owl:onProperty rdf:resource="http://www.sisostds.org/ontologies/C2SIM#hasPlaybackRealtimeMultiple"/>
                <owl:qualifiedCardinality rdf:datatype="http://www.w3.org/2001/XMLSchema#nonNegativeInteger">1</owl:qualifiedCardinality>
                <owl:onDataRange rdf:resource="http://www.sisostds.org/ontologies/C2SIM#playbackRealtimeMultiple"/>
            </owl:Restriction>
        </rdfs:subClassOf>
        <rdfs:comment>System command for setting the playbackRealtimeMultiple value indicating the  multiple of simulation time to realtime for playback of recorded messages in the C2SIM coalition of systems.The SetPlaybackRealtimeMultiple enables a user in a C2SIM coalition to direct playback of recorded messages at a rate faster or slower than realtime. For example, a playbackRealtimeMultiple value of 2.0 directs recording playback at 2:1 simulation time to realtime (i.e., faster than realtime); a value of 0.5 directs recording playback at half realtime (i.e., slower than realtime).</rdfs:comment>
    </owl:Class>
    


    <!-- http://www.sisostds.org/ontologies/C2SIM#SetSimulationRealtimeMultiple -->

    <owl:Class rdf:about="http://www.sisostds.org/ontologies/C2SIM#SetSimulationRealtimeMultiple">
        <rdfs:subClassOf rdf:resource="http://www.sisostds.org/ontologies/C2SIM#SystemMessageBody"/>
        <rdfs:subClassOf>
            <owl:Restriction>
                <owl:onProperty rdf:resource="http://www.sisostds.org/ontologies/C2SIM#hasSimulationRealtimeMultiple"/>
                <owl:qualifiedCardinality rdf:datatype="http://www.w3.org/2001/XMLSchema#nonNegativeInteger">1</owl:qualifiedCardinality>
                <owl:onDataRange rdf:resource="http://www.sisostds.org/ontologies/C2SIM#simulationRealtimeMultiple"/>
            </owl:Restriction>
        </rdfs:subClassOf>
        <rdfs:comment>System command for setting the simuationRealtimeMultiple value indicating the  multiple of simulation time to realtime for the simulation systems in the C2SIM coalition of systems.The SetSimulationRealtimeMultiple enables a user in a C2SIM coalition to direct participating simulations to execute at a rate faster or slower than realtime. For example, a simulationRealtimeMultiple value of 2.0 directs participating simulations to operate at 2:1 simulation time to realtime (i.e., faster than realtime); a value of 0.5 directs participating simulations to operate at half realtime (i.e., slower than realtime).</rdfs:comment>
    </owl:Class>
    


    <!-- http://www.sisostds.org/ontologies/C2SIM#ShareScenario -->

    <owl:Class rdf:about="http://www.sisostds.org/ontologies/C2SIM#ShareScenario">
        <rdfs:subClassOf rdf:resource="http://www.sisostds.org/ontologies/C2SIM#SystemMessageBody"/>
        <rdfs:comment>Sent by a C2SIM controller to a marshalling server. When this C2SIM message is received, the marshalling server sends to all subscribed systems the C2SIM initialization message.</rdfs:comment>
    </owl:Class>
    


    <!-- http://www.sisostds.org/ontologies/C2SIM#SimulationRealtimeMultipleReport -->

    <owl:Class rdf:about="http://www.sisostds.org/ontologies/C2SIM#SimulationRealtimeMultipleReport">
        <rdfs:subClassOf rdf:resource="http://www.sisostds.org/ontologies/C2SIM#SystemMessageBody"/>
        <rdfs:subClassOf>
            <owl:Restriction>
                <owl:onProperty rdf:resource="http://www.sisostds.org/ontologies/C2SIM#hasSimulationRealtimeMultiple"/>
                <owl:qualifiedCardinality rdf:datatype="http://www.w3.org/2001/XMLSchema#nonNegativeInteger">1</owl:qualifiedCardinality>
                <owl:onDataRange rdf:resource="http://www.sisostds.org/ontologies/C2SIM#simulationRealtimeMultiple"/>
            </owl:Restriction>
        </rdfs:subClassOf>
        <rdfs:comment>System command for reporting the current setting of the simuationRealtimeMultiple value indicating the multiple of simulation time to realtime currently set for the simulation systems in the C2SIM coalition of systems.</rdfs:comment>
    </owl:Class>
    


    <!-- http://www.sisostds.org/ontologies/C2SIM#SimulationTime -->

    <owl:Class rdf:about="http://www.sisostds.org/ontologies/C2SIM#SimulationTime">
        <rdfs:subClassOf rdf:resource="http://www.sisostds.org/ontologies/C2SIM#TimeInstant"/>
        <rdfs:subClassOf>
            <owl:Restriction>
                <owl:onProperty rdf:resource="http://www.sisostds.org/ontologies/C2SIM#hasDelayTimeAmount"/>
                <owl:qualifiedCardinality rdf:datatype="http://www.w3.org/2001/XMLSchema#nonNegativeInteger">1</owl:qualifiedCardinality>
                <owl:onClass rdf:resource="http://www.sisostds.org/ontologies/C2SIM#Duration"/>
            </owl:Restriction>
        </rdfs:subClassOf>
        <rdfs:comment>A time measured as a time duration since the time instant of the scenario start.</rdfs:comment>
    </owl:Class>
    


    <!-- http://www.sisostds.org/ontologies/C2SIM#SpatialOffset -->

    <owl:Class rdf:about="http://www.sisostds.org/ontologies/C2SIM#SpatialOffset">
        <rdfs:subClassOf rdf:resource="http://www.sisostds.org/ontologies/C2SIM#PhysicalConcept"/>
        <rdfs:comment>Used in a relative location specification.</rdfs:comment>
    </owl:Class>
    


    <!-- http://www.sisostds.org/ontologies/C2SIM#StartPlayback -->

    <owl:Class rdf:about="http://www.sisostds.org/ontologies/C2SIM#StartPlayback">
        <rdfs:subClassOf rdf:resource="http://www.sisostds.org/ontologies/C2SIM#SystemMessageBody"/>
        <rdfs:subClassOf>
            <owl:Restriction>
                <owl:onProperty rdf:resource="http://www.sisostds.org/ontologies/C2SIM#hasStartTime"/>
                <owl:maxQualifiedCardinality rdf:datatype="http://www.w3.org/2001/XMLSchema#nonNegativeInteger">1</owl:maxQualifiedCardinality>
                <owl:onClass rdf:resource="http://www.sisostds.org/ontologies/C2SIM#SimulationTime"/>
            </owl:Restriction>
        </rdfs:subClassOf>
        <rdfs:subClassOf>
            <owl:Restriction>
                <owl:onProperty rdf:resource="http://www.sisostds.org/ontologies/C2SIM#hasName"/>
                <owl:qualifiedCardinality rdf:datatype="http://www.w3.org/2001/XMLSchema#nonNegativeInteger">1</owl:qualifiedCardinality>
                <owl:onDataRange rdf:resource="http://www.w3.org/2001/XMLSchema#string"/>
            </owl:Restriction>
        </rdfs:subClassOf>
        <rdfs:comment>System command ordering the initiation of playback of recorded C2SIM messages in a C2SIM coalition of systems. The name refers to the name given to a recording that was previously created for later playback. The start time refers to the position in the recording where the playback is to begin. Playback is controlled by the C2SIM server sending out C2SIM messages that were previously recorded.</rdfs:comment>
    </owl:Class>
    


    <!-- http://www.sisostds.org/ontologies/C2SIM#StartRecording -->

    <owl:Class rdf:about="http://www.sisostds.org/ontologies/C2SIM#StartRecording">
        <rdfs:subClassOf rdf:resource="http://www.sisostds.org/ontologies/C2SIM#SystemMessageBody"/>
        <rdfs:subClassOf>
            <owl:Restriction>
                <owl:onProperty rdf:resource="http://www.sisostds.org/ontologies/C2SIM#hasName"/>
                <owl:qualifiedCardinality rdf:datatype="http://www.w3.org/2001/XMLSchema#nonNegativeInteger">1</owl:qualifiedCardinality>
                <owl:onDataRange rdf:resource="http://www.w3.org/2001/XMLSchema#string"/>
            </owl:Restriction>
        </rdfs:subClassOf>
        <rdfs:comment>System command for ordering initiation of the recording of C2SIM messages in a C2SIM coalition of systems. The recording is given a name in order to distinguish this recording from others that may have been created and stored for later use. Note that there can be only one recording in progress at a time in the C2SIM coalition of systems. Recording is executed by the C2SIM server recording C2SIM messages that are exchanged across systems in a C2SIM coalition.</rdfs:comment>
    </owl:Class>
    


    <!-- http://www.sisostds.org/ontologies/C2SIM#StartScenario -->

    <owl:Class rdf:about="http://www.sisostds.org/ontologies/C2SIM#StartScenario">
        <rdfs:subClassOf rdf:resource="http://www.sisostds.org/ontologies/C2SIM#SystemMessageBody"/>
        <rdfs:comment>This C2SIM message is sent to all subscribed systems indicating that the simulation scenario is to begin.</rdfs:comment>
    </owl:Class>
    


    <!-- http://www.sisostds.org/ontologies/C2SIM#StopPlayback -->

    <owl:Class rdf:about="http://www.sisostds.org/ontologies/C2SIM#StopPlayback">
        <rdfs:subClassOf rdf:resource="http://www.sisostds.org/ontologies/C2SIM#SystemMessageBody"/>
        <rdfs:comment>System command used to terminate (no resumption allowed) the playback of recorded C2SIM messages in a C2SIM coalition of systems. The name of the recording being played back is not needed here since there can be only one playback in progress at a time.</rdfs:comment>
    </owl:Class>
    


    <!-- http://www.sisostds.org/ontologies/C2SIM#StopRecording -->

    <owl:Class rdf:about="http://www.sisostds.org/ontologies/C2SIM#StopRecording">
        <rdfs:subClassOf rdf:resource="http://www.sisostds.org/ontologies/C2SIM#SystemMessageBody"/>
        <rdfs:comment>System command used to terminate (no resumption allowed) the recording of C2SIM messages in a C2SIM coalition of systems. The name of the recording  is not needed here since there can be only one recording in progress at a time.</rdfs:comment>
    </owl:Class>
    


    <!-- http://www.sisostds.org/ontologies/C2SIM#StopScenario -->

    <owl:Class rdf:about="http://www.sisostds.org/ontologies/C2SIM#StopScenario">
        <rdfs:subClassOf rdf:resource="http://www.sisostds.org/ontologies/C2SIM#SystemMessageBody"/>
        <rdfs:comment>This C2SIM message is sent to all subscribed systems indicating that the simulation should be stopped and won’t be restarted. All initialization data should be discarded, and all systems should prepare to reinitialize.</rdfs:comment>
    </owl:Class>
    


    <!-- http://www.sisostds.org/ontologies/C2SIM#Strength -->

    <owl:Class rdf:about="http://www.sisostds.org/ontologies/C2SIM#Strength">
        <rdfs:subClassOf rdf:resource="http://www.sisostds.org/ontologies/C2SIM#EntityHealthStatus"/>
        <rdfs:subClassOf>
            <owl:Restriction>
                <owl:onProperty rdf:resource="http://www.sisostds.org/ontologies/C2SIM#hasStrengthPercentage"/>
                <owl:qualifiedCardinality rdf:datatype="http://www.w3.org/2001/XMLSchema#nonNegativeInteger">1</owl:qualifiedCardinality>
                <owl:onDataRange rdf:resource="http://www.sisostds.org/ontologies/C2SIM#percentage"/>
            </owl:Restriction>
        </rdfs:subClassOf>
        <rdfs:comment>Representation of the strength of an entity expressed as a percentage of some starting value.</rdfs:comment>
    </owl:Class>
    


    <!-- http://www.sisostds.org/ontologies/C2SIM#SubmitInitialization -->

    <owl:Class rdf:about="http://www.sisostds.org/ontologies/C2SIM#SubmitInitialization">
        <rdfs:subClassOf rdf:resource="http://www.sisostds.org/ontologies/C2SIM#SystemMessageBody"/>
        <rdfs:comment>Sent by a C2SIM controller. When C2SIM systems receive this C2SIM message, they should submit Object Initialization messages for object definitions they are configured to simulate. This message contains no data; it serves as a command and is not required if a preconfigured master initialization file is used.</rdfs:comment>
    </owl:Class>
    


    <!-- http://www.sisostds.org/ontologies/C2SIM#SystemAcknowledgementBody -->

    <owl:Class rdf:about="http://www.sisostds.org/ontologies/C2SIM#SystemAcknowledgementBody">
        <rdfs:subClassOf rdf:resource="http://www.sisostds.org/ontologies/C2SIM#MessageBody"/>
        <rdfs:subClassOf>
            <owl:Restriction>
                <owl:onProperty rdf:resource="http://www.sisostds.org/ontologies/C2SIM#hasAcknowledgeTypeCode"/>
                <owl:qualifiedCardinality rdf:datatype="http://www.w3.org/2001/XMLSchema#nonNegativeInteger">1</owl:qualifiedCardinality>
                <owl:onClass rdf:resource="http://www.sisostds.org/ontologies/C2SIM#AcknowledgeTypeCode"/>
            </owl:Restriction>
        </rdfs:subClassOf>
        <rdfs:comment>An acknowledgement from one C2SIM system to another that a message was received.</rdfs:comment>
    </owl:Class>
    


    <!-- http://www.sisostds.org/ontologies/C2SIM#SystemEntityList -->

    <owl:Class rdf:about="http://www.sisostds.org/ontologies/C2SIM#SystemEntityList">
        <rdfs:subClassOf rdf:resource="http://www.sisostds.org/ontologies/C2SIM#InitializationConcept"/>
        <rdfs:subClassOf>
            <owl:Restriction>
                <owl:onProperty rdf:resource="http://www.sisostds.org/ontologies/C2SIM#hasActorReference"/>
                <owl:minQualifiedCardinality rdf:datatype="http://www.w3.org/2001/XMLSchema#nonNegativeInteger">1</owl:minQualifiedCardinality>
                <owl:onDataRange rdf:resource="http://www.sisostds.org/ontologies/C2SIM#UUIDBase"/>
            </owl:Restriction>
        </rdfs:subClassOf>
        <rdfs:subClassOf>
            <owl:Restriction>
                <owl:onProperty rdf:resource="http://www.sisostds.org/ontologies/C2SIM#hasSystemName"/>
                <owl:qualifiedCardinality rdf:datatype="http://www.w3.org/2001/XMLSchema#nonNegativeInteger">1</owl:qualifiedCardinality>
                <owl:onDataRange rdf:resource="http://www.w3.org/2001/XMLSchema#string"/>
            </owl:Restriction>
        </rdfs:subClassOf>
        <rdfs:comment>This is a listing of entities that reside within a system. The list defines what system a message should be sent to in order to get it to a given actor.  Each entity can reside on only one system. This list does not define necessarily define the complete list of entities on the given system.
Systems can build a map from this and other lists to get the system from a given entity.</rdfs:comment>
    </owl:Class>
    <owl:Axiom>
        <owl:annotatedSource rdf:resource="http://www.sisostds.org/ontologies/C2SIM#SystemEntityList"/>
        <owl:annotatedProperty rdf:resource="http://www.w3.org/2000/01/rdf-schema#subClassOf"/>
        <owl:annotatedTarget>
            <owl:Restriction>
                <owl:onProperty rdf:resource="http://www.sisostds.org/ontologies/C2SIM#hasActorReference"/>
                <owl:minQualifiedCardinality rdf:datatype="http://www.w3.org/2001/XMLSchema#nonNegativeInteger">1</owl:minQualifiedCardinality>
                <owl:onDataRange rdf:resource="http://www.sisostds.org/ontologies/C2SIM#UUIDBase"/>
            </owl:Restriction>
        </owl:annotatedTarget>
        <rdfs:comment>This is the unique identifier of an individual of the ActorEntity class.</rdfs:comment>
    </owl:Axiom>
    


    <!-- http://www.sisostds.org/ontologies/C2SIM#SystemMessageBody -->

    <owl:Class rdf:about="http://www.sisostds.org/ontologies/C2SIM#SystemMessageBody">
        <rdfs:subClassOf rdf:resource="http://www.sisostds.org/ontologies/C2SIM#MessageBody"/>
        <rdfs:comment>The body of a message that is used to send coalition-level commands, requests, and reports between systems participating in the C2SIM coalition.</rdfs:comment>
    </owl:Class>
    


    <!-- http://www.sisostds.org/ontologies/C2SIM#Task -->

    <owl:Class rdf:about="http://www.sisostds.org/ontologies/C2SIM#Task">
        <rdfs:subClassOf rdf:resource="http://www.sisostds.org/ontologies/C2SIM#Action"/>
        <rdfs:subClassOf>
            <owl:Restriction>
                <owl:onProperty rdf:resource="http://www.sisostds.org/ontologies/C2SIM#hasDesiredEffectCode"/>
                <owl:minQualifiedCardinality rdf:datatype="http://www.w3.org/2001/XMLSchema#nonNegativeInteger">0</owl:minQualifiedCardinality>
                <owl:onClass rdf:resource="http://www.sisostds.org/ontologies/C2SIM#DesiredEffectCode"/>
            </owl:Restriction>
        </rdfs:subClassOf>
        <rdfs:subClassOf>
            <owl:Restriction>
                <owl:onProperty rdf:resource="http://www.sisostds.org/ontologies/C2SIM#hasTaskActionCode"/>
                <owl:qualifiedCardinality rdf:datatype="http://www.w3.org/2001/XMLSchema#nonNegativeInteger">1</owl:qualifiedCardinality>
                <owl:onClass rdf:resource="http://www.sisostds.org/ontologies/C2SIM#TaskActionCode"/>
            </owl:Restriction>
        </rdfs:subClassOf>
        <rdfs:subClassOf>
            <owl:Restriction>
                <owl:onProperty rdf:resource="http://www.sisostds.org/ontologies/C2SIM#hasDuration"/>
                <owl:maxQualifiedCardinality rdf:datatype="http://www.w3.org/2001/XMLSchema#nonNegativeInteger">1</owl:maxQualifiedCardinality>
                <owl:onClass rdf:resource="http://www.sisostds.org/ontologies/C2SIM#Duration"/>
            </owl:Restriction>
        </rdfs:subClassOf>
        <rdfs:subClassOf>
            <owl:Restriction>
                <owl:onProperty rdf:resource="http://www.sisostds.org/ontologies/C2SIM#hasEndTime"/>
                <owl:maxQualifiedCardinality rdf:datatype="http://www.w3.org/2001/XMLSchema#nonNegativeInteger">1</owl:maxQualifiedCardinality>
                <owl:onClass rdf:resource="http://www.sisostds.org/ontologies/C2SIM#TimeInstant"/>
            </owl:Restriction>
        </rdfs:subClassOf>
        <rdfs:subClassOf>
            <owl:Restriction>
                <owl:onProperty rdf:resource="http://www.sisostds.org/ontologies/C2SIM#hasStartTime"/>
                <owl:maxQualifiedCardinality rdf:datatype="http://www.w3.org/2001/XMLSchema#nonNegativeInteger">1</owl:maxQualifiedCardinality>
                <owl:onClass rdf:resource="http://www.sisostds.org/ontologies/C2SIM#TimeInstant"/>
            </owl:Restriction>
        </rdfs:subClassOf>
        <rdfs:subClassOf>
            <owl:Restriction>
                <owl:onProperty rdf:resource="http://www.sisostds.org/ontologies/C2SIM#hasAffectedEntity"/>
                <owl:minQualifiedCardinality rdf:datatype="http://www.w3.org/2001/XMLSchema#nonNegativeInteger">0</owl:minQualifiedCardinality>
                <owl:onDataRange rdf:resource="http://www.sisostds.org/ontologies/C2SIM#UUIDBase"/>
            </owl:Restriction>
        </rdfs:subClassOf>
        <rdfs:subClassOf>
            <owl:Restriction>
                <owl:onProperty rdf:resource="http://www.sisostds.org/ontologies/C2SIM#hasPerformingEntity"/>
                <owl:qualifiedCardinality rdf:datatype="http://www.w3.org/2001/XMLSchema#nonNegativeInteger">1</owl:qualifiedCardinality>
                <owl:onDataRange rdf:resource="http://www.sisostds.org/ontologies/C2SIM#UUIDBase"/>
            </owl:Restriction>
        </rdfs:subClassOf>
        <rdfs:comment>A request for an actor in the domain to perform a Task. The actor to perform the Task is indicated by the hasPerformingEntity property of the Task.</rdfs:comment>
        <rdfs:comment>An Action that takes place over time, and is performed by an Entity to change the state of the world.
Must identify WHO, WHAT, WHEN and WHERE.
WHO is represented by hasPerformingEntity (and hasAffectedEntity).
WHAT is represented by the hasTaskActionCode.
WHEN is represented by the start time/duration/end time (2 of 3)
WHERE is represented by hasLocation and/or hasMapGraphicID reference.
WHY may be represented by hasDesiredEffect.</rdfs:comment>
    </owl:Class>
    <owl:Axiom>
        <owl:annotatedSource rdf:resource="http://www.sisostds.org/ontologies/C2SIM#Task"/>
        <owl:annotatedProperty rdf:resource="http://www.w3.org/2000/01/rdf-schema#subClassOf"/>
        <owl:annotatedTarget>
            <owl:Restriction>
                <owl:onProperty rdf:resource="http://www.sisostds.org/ontologies/C2SIM#hasAffectedEntity"/>
                <owl:minQualifiedCardinality rdf:datatype="http://www.w3.org/2001/XMLSchema#nonNegativeInteger">0</owl:minQualifiedCardinality>
                <owl:onDataRange rdf:resource="http://www.sisostds.org/ontologies/C2SIM#UUIDBase"/>
            </owl:Restriction>
        </owl:annotatedTarget>
        <rdfs:comment>This is the unique identifier of an individual of the ActorEntity class.</rdfs:comment>
    </owl:Axiom>
    <owl:Axiom>
        <owl:annotatedSource rdf:resource="http://www.sisostds.org/ontologies/C2SIM#Task"/>
        <owl:annotatedProperty rdf:resource="http://www.w3.org/2000/01/rdf-schema#subClassOf"/>
        <owl:annotatedTarget>
            <owl:Restriction>
                <owl:onProperty rdf:resource="http://www.sisostds.org/ontologies/C2SIM#hasPerformingEntity"/>
                <owl:qualifiedCardinality rdf:datatype="http://www.w3.org/2001/XMLSchema#nonNegativeInteger">1</owl:qualifiedCardinality>
                <owl:onDataRange rdf:resource="http://www.sisostds.org/ontologies/C2SIM#UUIDBase"/>
            </owl:Restriction>
        </owl:annotatedTarget>
        <rdfs:comment>This is the unique identifier of an individual of the ActorEntity class.</rdfs:comment>
    </owl:Axiom>
    


    <!-- http://www.sisostds.org/ontologies/C2SIM#TaskActionCode -->

    <owl:Class rdf:about="http://www.sisostds.org/ontologies/C2SIM#TaskActionCode">
        <rdfs:subClassOf rdf:resource="http://www.sisostds.org/ontologies/C2SIM#ActionCode"/>
        <rdfs:comment>The activity to be performed in the task, e.g. Move, Observe, Assist.</rdfs:comment>
    </owl:Class>
    


    <!-- http://www.sisostds.org/ontologies/C2SIM#TaskRequestContent -->

    <owl:Class rdf:about="http://www.sisostds.org/ontologies/C2SIM#TaskRequestContent">
        <rdfs:subClassOf rdf:resource="http://www.sisostds.org/ontologies/C2SIM#RequestContent"/>
        <rdfs:subClassOf>
            <owl:Restriction>
                <owl:onProperty rdf:resource="http://www.sisostds.org/ontologies/C2SIM#hasTask"/>
                <owl:minQualifiedCardinality rdf:datatype="http://www.w3.org/2001/XMLSchema#nonNegativeInteger">1</owl:minQualifiedCardinality>
                <owl:onClass rdf:resource="http://www.sisostds.org/ontologies/C2SIM#Task"/>
            </owl:Restriction>
        </rdfs:subClassOf>
        <rdfs:comment>A request for an Actor to perform a Task. The Actor to perform the Task is identified by the hasPerformingEntity property of the Task.</rdfs:comment>
    </owl:Class>
    


    <!-- http://www.sisostds.org/ontologies/C2SIM#TaskStatus -->

    <owl:Class rdf:about="http://www.sisostds.org/ontologies/C2SIM#TaskStatus">
        <rdfs:subClassOf rdf:resource="http://www.sisostds.org/ontologies/C2SIM#ReportContent"/>
        <rdfs:subClassOf>
            <owl:Restriction>
                <owl:onProperty rdf:resource="http://www.sisostds.org/ontologies/C2SIM#hasTaskStatusCode"/>
                <owl:qualifiedCardinality rdf:datatype="http://www.w3.org/2001/XMLSchema#nonNegativeInteger">1</owl:qualifiedCardinality>
                <owl:onClass rdf:resource="http://www.sisostds.org/ontologies/C2SIM#TaskStatusCode"/>
            </owl:Restriction>
        </rdfs:subClassOf>
        <rdfs:subClassOf>
            <owl:Restriction>
                <owl:onProperty rdf:resource="http://www.sisostds.org/ontologies/C2SIM#hasCurrentTask"/>
                <owl:qualifiedCardinality rdf:datatype="http://www.w3.org/2001/XMLSchema#nonNegativeInteger">1</owl:qualifiedCardinality>
                <owl:onDataRange rdf:resource="http://www.sisostds.org/ontologies/C2SIM#UUIDBase"/>
            </owl:Restriction>
        </rdfs:subClassOf>
        <rdfs:comment>The status of a task, provided before, during or after a task is executed.</rdfs:comment>
    </owl:Class>
    <owl:Axiom>
        <owl:annotatedSource rdf:resource="http://www.sisostds.org/ontologies/C2SIM#TaskStatus"/>
        <owl:annotatedProperty rdf:resource="http://www.w3.org/2000/01/rdf-schema#subClassOf"/>
        <owl:annotatedTarget>
            <owl:Restriction>
                <owl:onProperty rdf:resource="http://www.sisostds.org/ontologies/C2SIM#hasCurrentTask"/>
                <owl:qualifiedCardinality rdf:datatype="http://www.w3.org/2001/XMLSchema#nonNegativeInteger">1</owl:qualifiedCardinality>
                <owl:onDataRange rdf:resource="http://www.sisostds.org/ontologies/C2SIM#UUIDBase"/>
            </owl:Restriction>
        </owl:annotatedTarget>
        <rdfs:comment>The task whose status is being reported.</rdfs:comment>
    </owl:Axiom>
    


    <!-- http://www.sisostds.org/ontologies/C2SIM#TaskStatusCode -->

    <owl:Class rdf:about="http://www.sisostds.org/ontologies/C2SIM#TaskStatusCode">
        <rdfs:subClassOf rdf:resource="http://www.sisostds.org/ontologies/C2SIM#MessageCode"/>
        <rdfs:comment>An enumeration of possible status values for a task.</rdfs:comment>
    </owl:Class>
    


    <!-- http://www.sisostds.org/ontologies/C2SIM#TemporalConcept -->

    <owl:Class rdf:about="http://www.sisostds.org/ontologies/C2SIM#TemporalConcept">
        <rdfs:subClassOf rdf:resource="http://www.sisostds.org/ontologies/C2SIM#PhysicalConcept"/>
        <rdfs:comment>Time concepts include instants in time, durations of time, and intervals between two times.</rdfs:comment>
    </owl:Class>
    


    <!-- http://www.sisostds.org/ontologies/C2SIM#TimeInstant -->

    <owl:Class rdf:about="http://www.sisostds.org/ontologies/C2SIM#TimeInstant">
        <rdfs:subClassOf rdf:resource="http://www.sisostds.org/ontologies/C2SIM#TemporalConcept"/>
        <rdfs:subClassOf>
            <owl:Restriction>
                <owl:onProperty rdf:resource="http://www.sisostds.org/ontologies/C2SIM#hasName"/>
                <owl:maxQualifiedCardinality rdf:datatype="http://www.w3.org/2001/XMLSchema#nonNegativeInteger">1</owl:maxQualifiedCardinality>
                <owl:onDataRange rdf:resource="http://www.w3.org/2001/XMLSchema#string"/>
            </owl:Restriction>
        </rdfs:subClassOf>
        <rdfs:comment>A specific time expressed in seconds, i.e. with no date. The generator and user of this time must understand a common reference point, for example the start of the scenario.</rdfs:comment>
    </owl:Class>
    


    <!-- http://www.sisostds.org/ontologies/C2SIM#TimeReferenceCode -->

    <owl:Class rdf:about="http://www.sisostds.org/ontologies/C2SIM#TimeReferenceCode">
        <rdfs:subClassOf rdf:resource="http://www.sisostds.org/ontologies/C2SIM#Code"/>
        <rdfs:comment>Indicates whether a relative time is referenced to the start or the end of an interval time.</rdfs:comment>
    </owl:Class>
    


    <!-- http://www.sisostds.org/ontologies/lox#EventTrigger -->

    <owl:Class rdf:about="http://www.sisostds.org/ontologies/lox#EventTrigger">
        <rdfs:subClassOf rdf:resource="http://www.sisostds.org/ontologies/lox#PlanPhaseTrigger"/>
        <rdfs:subClassOf>
            <owl:Restriction>
                <owl:onProperty rdf:resource="http://www.sisostds.org/ontologies/lox#hasEvent"/>
                <owl:qualifiedCardinality rdf:datatype="http://www.w3.org/2001/XMLSchema#nonNegativeInteger">1</owl:qualifiedCardinality>
                <owl:onClass rdf:resource="http://www.sisostds.org/ontologies/C2SIM#Event"/>
            </owl:Restriction>
        </rdfs:subClassOf>
        <rdfs:comment>A trigger to start a plan phase that is based on the time of an event.</rdfs:comment>
    </owl:Class>
    


    <!-- http://www.sisostds.org/ontologies/lox#ManeuverWarfareTask -->

    <owl:Class rdf:about="http://www.sisostds.org/ontologies/lox#ManeuverWarfareTask">
        <rdfs:subClassOf rdf:resource="http://www.sisostds.org/ontologies/C2SIM#Task"/>
        <rdfs:subClassOf>
            <owl:Restriction>
                <owl:onProperty rdf:resource="http://www.sisostds.org/ontologies/lox#hasRuleOfEngagement"/>
                <owl:minQualifiedCardinality rdf:datatype="http://www.w3.org/2001/XMLSchema#nonNegativeInteger">0</owl:minQualifiedCardinality>
                <owl:onClass rdf:resource="http://www.sisostds.org/ontologies/lox#RuleOfEngagement"/>
            </owl:Restriction>
        </rdfs:subClassOf>
        <rdfs:subClassOf>
            <owl:Restriction>
                <owl:onProperty rdf:resource="http://www.sisostds.org/ontologies/lox#hasTaskFunctionalRelation"/>
                <owl:minQualifiedCardinality rdf:datatype="http://www.w3.org/2001/XMLSchema#nonNegativeInteger">0</owl:minQualifiedCardinality>
                <owl:onClass rdf:resource="http://www.sisostds.org/ontologies/lox#TaskFunctionalRelation"/>
            </owl:Restriction>
        </rdfs:subClassOf>
        <rdfs:comment>A task with additional properties for a Maneuver Warfare Task, including a definition of rules of engagement, and a relationship to another task.

Note that the enumerated individuals in TaskActionCode have been expanded to include tasks defined by  the Joint Consultation Command Control Information Exchange Data Model (JC3IEDM) developed by the Multilateral Interoperability Programme (MIP).</rdfs:comment>
    </owl:Class>
    


    <!-- http://www.sisostds.org/ontologies/lox#MipWeaponUseROE -->

    <owl:Class rdf:about="http://www.sisostds.org/ontologies/lox#MipWeaponUseROE">
        <rdfs:subClassOf rdf:resource="http://www.sisostds.org/ontologies/lox#RuleOfEngagement"/>
        <rdfs:subClassOf>
            <owl:Restriction>
                <owl:onProperty rdf:resource="http://www.sisostds.org/ontologies/lox#hasWeaponROECode"/>
                <owl:qualifiedCardinality rdf:datatype="http://www.w3.org/2001/XMLSchema#nonNegativeInteger">1</owl:qualifiedCardinality>
                <owl:onClass rdf:resource="http://www.sisostds.org/ontologies/lox#WeaponRuleOfEngagementCode"/>
            </owl:Restriction>
        </rdfs:subClassOf>
        <rdfs:comment>A RuleofEngagement that is based on a standard code describing engagement conditions.</rdfs:comment>
    </owl:Class>
    


    <!-- http://www.sisostds.org/ontologies/lox#OnOrderTrigger -->

    <owl:Class rdf:about="http://www.sisostds.org/ontologies/lox#OnOrderTrigger">
        <rdfs:subClassOf rdf:resource="http://www.sisostds.org/ontologies/lox#PlanPhaseTrigger"/>
        <rdfs:subClassOf>
            <owl:Restriction>
                <owl:onProperty rdf:resource="http://www.sisostds.org/ontologies/C2SIM#hasTaskReference"/>
                <owl:qualifiedCardinality rdf:datatype="http://www.w3.org/2001/XMLSchema#nonNegativeInteger">1</owl:qualifiedCardinality>
                <owl:onDataRange rdf:resource="http://www.sisostds.org/ontologies/C2SIM#UUIDBase"/>
            </owl:Restriction>
        </rdfs:subClassOf>
        <rdfs:comment>A trigger for the execution of a plan phase that is based on the start time of a task. Typically this task will be defined in an order and will have a TaskActionCode of ExecutePlanPhase.</rdfs:comment>
    </owl:Class>
    


    <!-- http://www.sisostds.org/ontologies/lox#PlanBody -->

    <owl:Class rdf:about="http://www.sisostds.org/ontologies/lox#PlanBody">
        <rdfs:subClassOf rdf:resource="http://www.sisostds.org/ontologies/C2SIM#DomainMessageBody"/>
        <rdfs:subClassOf>
            <owl:Restriction>
                <owl:onProperty rdf:resource="http://www.sisostds.org/ontologies/lox#hasPlanPhase"/>
                <owl:minQualifiedCardinality rdf:datatype="http://www.w3.org/2001/XMLSchema#nonNegativeInteger">0</owl:minQualifiedCardinality>
                <owl:onClass rdf:resource="http://www.sisostds.org/ontologies/lox#PlanPhase"/>
            </owl:Restriction>
        </rdfs:subClassOf>
        <rdfs:subClassOf>
            <owl:Restriction>
                <owl:onProperty rdf:resource="http://www.sisostds.org/ontologies/lox#hasPlanPhaseReference"/>
                <owl:minQualifiedCardinality rdf:datatype="http://www.w3.org/2001/XMLSchema#nonNegativeInteger">0</owl:minQualifiedCardinality>
                <owl:onDataRange rdf:resource="http://www.sisostds.org/ontologies/C2SIM#UUIDBase"/>
            </owl:Restriction>
        </rdfs:subClassOf>
        <rdfs:subClassOf>
            <owl:Restriction>
                <owl:onProperty rdf:resource="http://www.sisostds.org/ontologies/lox#isToBeExecutedNow"/>
                <owl:qualifiedCardinality rdf:datatype="http://www.w3.org/2001/XMLSchema#nonNegativeInteger">1</owl:qualifiedCardinality>
                <owl:onDataRange rdf:resource="http://www.w3.org/2001/XMLSchema#boolean"/>
            </owl:Restriction>
        </rdfs:subClassOf>
        <rdfs:comment>This message orders the recipient unit to begin execution of the indicated plan.</rdfs:comment>
    </owl:Class>
    


    <!-- http://www.sisostds.org/ontologies/lox#PlanPhase -->

    <owl:Class rdf:about="http://www.sisostds.org/ontologies/lox#PlanPhase">
        <rdfs:subClassOf rdf:resource="http://www.sisostds.org/ontologies/C2SIM#C2SIMContent"/>
        <rdfs:subClassOf>
            <owl:Restriction>
                <owl:onProperty rdf:resource="http://www.sisostds.org/ontologies/lox#hasSubPhase"/>
                <owl:minQualifiedCardinality rdf:datatype="http://www.w3.org/2001/XMLSchema#nonNegativeInteger">0</owl:minQualifiedCardinality>
                <owl:onClass rdf:resource="http://www.sisostds.org/ontologies/lox#PlanPhase"/>
            </owl:Restriction>
        </rdfs:subClassOf>
        <rdfs:subClassOf>
            <owl:Restriction>
                <owl:onProperty rdf:resource="http://www.sisostds.org/ontologies/lox#hasPlanPhaseCompletionCondition"/>
                <owl:qualifiedCardinality rdf:datatype="http://www.w3.org/2001/XMLSchema#nonNegativeInteger">1</owl:qualifiedCardinality>
                <owl:onClass rdf:resource="http://www.sisostds.org/ontologies/lox#PlanPhaseCompletionCondition"/>
            </owl:Restriction>
        </rdfs:subClassOf>
        <rdfs:subClassOf>
            <owl:Restriction>
                <owl:onProperty rdf:resource="http://www.sisostds.org/ontologies/lox#hasPlanPhaseTrigger"/>
                <owl:qualifiedCardinality rdf:datatype="http://www.w3.org/2001/XMLSchema#nonNegativeInteger">1</owl:qualifiedCardinality>
                <owl:onClass rdf:resource="http://www.sisostds.org/ontologies/lox#PlanPhaseTrigger"/>
            </owl:Restriction>
        </rdfs:subClassOf>
        <rdfs:subClassOf>
            <owl:Restriction>
                <owl:onProperty rdf:resource="http://www.sisostds.org/ontologies/C2SIM#hasTaskReference"/>
                <owl:minQualifiedCardinality rdf:datatype="http://www.w3.org/2001/XMLSchema#nonNegativeInteger">0</owl:minQualifiedCardinality>
                <owl:onDataRange rdf:resource="http://www.sisostds.org/ontologies/C2SIM#UUIDBase"/>
            </owl:Restriction>
        </rdfs:subClassOf>
        <rdfs:comment>A plan for a unit. A PlanPhase may a single task for a unit, or tasks for multiple units (one each), or (recursively) multiple subphases.
Phases have completion conditions that indicate when they are complete, as well as Boolean flags that indicate whether the phase is active and whether it is complete.
Phases have trigger conditions that indicate when they start.  Phases may start on the completion of another phase--thus forming a task sequence--on receipt of an order, or at the time of an Event.
 A sequence of tasks for one unit is normally represented as a sequence of subphases in order to express the triggering conditions for each task; however a set of tasks for a unit may be included in a phase and executed with some implicit sequencing such as task time.</rdfs:comment>
    </owl:Class>
    <owl:Axiom>
        <owl:annotatedSource rdf:resource="http://www.sisostds.org/ontologies/lox#PlanPhase"/>
        <owl:annotatedProperty rdf:resource="http://www.w3.org/2000/01/rdf-schema#subClassOf"/>
        <owl:annotatedTarget>
            <owl:Restriction>
                <owl:onProperty rdf:resource="http://www.sisostds.org/ontologies/C2SIM#hasTaskReference"/>
                <owl:minQualifiedCardinality rdf:datatype="http://www.w3.org/2001/XMLSchema#nonNegativeInteger">0</owl:minQualifiedCardinality>
                <owl:onDataRange rdf:resource="http://www.sisostds.org/ontologies/C2SIM#UUIDBase"/>
            </owl:Restriction>
        </owl:annotatedTarget>
        <rdfs:comment>These are references to tasks to be performed in this plan phase. If the tasks have not been previously defined, this property should be omitted and the tasks defined in the hasTask property.</rdfs:comment>
    </owl:Axiom>
    


    <!-- http://www.sisostds.org/ontologies/lox#PlanPhaseCompletionCondition -->

    <owl:Class rdf:about="http://www.sisostds.org/ontologies/lox#PlanPhaseCompletionCondition">
        <rdfs:subClassOf rdf:resource="http://www.sisostds.org/ontologies/C2SIM#Code"/>
        <rdfs:comment>A code defining the condition to be used to test the tasks of a plan phase to determine whether the phase is considered to be complete.</rdfs:comment>
    </owl:Class>
    


    <!-- http://www.sisostds.org/ontologies/lox#PlanPhaseTrigger -->

    <owl:Class rdf:about="http://www.sisostds.org/ontologies/lox#PlanPhaseTrigger">
        <rdfs:subClassOf rdf:resource="http://www.sisostds.org/ontologies/C2SIM#C2SIMContent"/>
        <rdfs:comment>This is a condition that causes the start of execution of a PlanPhase.</rdfs:comment>
    </owl:Class>
    


    <!-- http://www.sisostds.org/ontologies/lox#PriorPhaseCompletionTrigger -->

    <owl:Class rdf:about="http://www.sisostds.org/ontologies/lox#PriorPhaseCompletionTrigger">
        <rdfs:subClassOf rdf:resource="http://www.sisostds.org/ontologies/lox#PlanPhaseTrigger"/>
        <rdfs:subClassOf>
            <owl:Restriction>
                <owl:onProperty rdf:resource="http://www.sisostds.org/ontologies/lox#hasTriggerPhase"/>
                <owl:qualifiedCardinality rdf:datatype="http://www.w3.org/2001/XMLSchema#nonNegativeInteger">1</owl:qualifiedCardinality>
                <owl:onDataRange rdf:resource="http://www.sisostds.org/ontologies/C2SIM#UUIDBase"/>
            </owl:Restriction>
        </rdfs:subClassOf>
        <rdfs:comment>A plan phase trigger that is based on the completion of another plan phase (typically, the phase immediately before this one in a plan).</rdfs:comment>
    </owl:Class>
    


    <!-- http://www.sisostds.org/ontologies/lox#RuleOfEngagement -->

    <owl:Class rdf:about="http://www.sisostds.org/ontologies/lox#RuleOfEngagement">
        <rdfs:subClassOf rdf:resource="http://www.sisostds.org/ontologies/C2SIM#C2SIMContent"/>
        <rdfs:comment>A rule that describes the conditions under which weapons can be used to engage other forces. This class is a collection class; different types of ROEs will be subclasses of this class.</rdfs:comment>
    </owl:Class>
    


    <!-- http://www.sisostds.org/ontologies/lox#TaskFunctionalAssociationCode -->

    <owl:Class rdf:about="http://www.sisostds.org/ontologies/lox#TaskFunctionalAssociationCode">
        <rdfs:subClassOf rdf:resource="http://www.sisostds.org/ontologies/C2SIM#Code"/>
        <rdfs:comment>Instances of this code will be taken from JC3IEDM 3.1.4, 	action-functional-association-category-code</rdfs:comment>
    </owl:Class>
    


    <!-- http://www.sisostds.org/ontologies/lox#TaskFunctionalRelation -->

    <owl:Class rdf:about="http://www.sisostds.org/ontologies/lox#TaskFunctionalRelation">
        <rdfs:subClassOf rdf:resource="http://www.sisostds.org/ontologies/C2SIM#Relationship"/>
        <rdfs:subClassOf>
            <owl:Restriction>
                <owl:onProperty rdf:resource="http://www.sisostds.org/ontologies/lox#hasTaskFunctionalAssociationCode"/>
                <owl:qualifiedCardinality rdf:datatype="http://www.w3.org/2001/XMLSchema#nonNegativeInteger">1</owl:qualifiedCardinality>
                <owl:onClass rdf:resource="http://www.sisostds.org/ontologies/lox#TaskFunctionalAssociationCode"/>
            </owl:Restriction>
        </rdfs:subClassOf>
        <rdfs:subClassOf>
            <owl:Restriction>
                <owl:onProperty rdf:resource="http://www.sisostds.org/ontologies/lox#hasFunctionalAssociationWithTask"/>
                <owl:qualifiedCardinality rdf:datatype="http://www.w3.org/2001/XMLSchema#nonNegativeInteger">1</owl:qualifiedCardinality>
                <owl:onDataRange rdf:resource="http://www.sisostds.org/ontologies/C2SIM#UUIDBase"/>
            </owl:Restriction>
        </rdfs:subClassOf>
        <rdfs:comment>A functional relationship between maneuver warfare tasks.</rdfs:comment>
    </owl:Class>
    


    <!-- http://www.sisostds.org/ontologies/lox#WeaponRuleOfEngagementCode -->

    <owl:Class rdf:about="http://www.sisostds.org/ontologies/lox#WeaponRuleOfEngagementCode">
        <rdfs:subClassOf rdf:resource="http://www.sisostds.org/ontologies/C2SIM#Code"/>
        <rdfs:comment>A code (enumerated value) describing a standard condition for using weapons to engage another force.</rdfs:comment>
    </owl:Class>
    


    <!-- http://www.sisostds.org/ontologies/smx#APP6CSymbol -->

    <owl:Class rdf:about="http://www.sisostds.org/ontologies/smx#APP6CSymbol">
        <rdfs:subClassOf rdf:resource="http://www.sisostds.org/ontologies/C2SIM#C2SIMContent"/>
        <rdfs:subClassOf>
            <owl:Restriction>
                <owl:onProperty rdf:resource="http://www.sisostds.org/ontologies/smx#hasAPP6C-SIDC"/>
                <owl:qualifiedCardinality rdf:datatype="http://www.w3.org/2001/XMLSchema#nonNegativeInteger">1</owl:qualifiedCardinality>
                <owl:onDataRange rdf:resource="http://www.w3.org/2001/XMLSchema#string"/>
            </owl:Restriction>
        </rdfs:subClassOf>
        <rdfs:comment>Tactical graphic symbol as specified by NATO APP-6-C.
Used to define the type of an Entity for its representation and depiction on C2 displays.</rdfs:comment>
    </owl:Class>
    <owl:Axiom>
        <owl:annotatedSource rdf:resource="http://www.sisostds.org/ontologies/smx#APP6CSymbol"/>
        <owl:annotatedProperty rdf:resource="http://www.w3.org/2000/01/rdf-schema#subClassOf"/>
        <owl:annotatedTarget>
            <owl:Restriction>
                <owl:onProperty rdf:resource="http://www.sisostds.org/ontologies/smx#hasAPP6C-SIDC"/>
                <owl:qualifiedCardinality rdf:datatype="http://www.w3.org/2001/XMLSchema#nonNegativeInteger">1</owl:qualifiedCardinality>
                <owl:onDataRange rdf:resource="http://www.w3.org/2001/XMLSchema#string"/>
            </owl:Restriction>
        </owl:annotatedTarget>
        <rdfs:comment>The string should have restrictions placed on it, e.g. 15 characters, etc.</rdfs:comment>
    </owl:Axiom>
    


    <!-- http://www.sisostds.org/ontologies/smx#ActivityObservation -->

    <owl:Class rdf:about="http://www.sisostds.org/ontologies/smx#ActivityObservation">
        <rdfs:subClassOf rdf:resource="http://www.sisostds.org/ontologies/smx#Observation"/>
        <rdfs:subClassOf>
            <owl:Restriction>
                <owl:onProperty rdf:resource="http://www.sisostds.org/ontologies/C2SIM#hasActionCode"/>
                <owl:qualifiedCardinality rdf:datatype="http://www.w3.org/2001/XMLSchema#nonNegativeInteger">1</owl:qualifiedCardinality>
                <owl:onClass rdf:resource="http://www.sisostds.org/ontologies/C2SIM#ActionCode"/>
            </owl:Restriction>
        </rdfs:subClassOf>
        <rdfs:comment>An observation of the activity of the subject.</rdfs:comment>
    </owl:Class>
    


    <!-- http://www.sisostds.org/ontologies/smx#Aircraft -->

    <owl:Class rdf:about="http://www.sisostds.org/ontologies/smx#Aircraft">
        <rdfs:subClassOf rdf:resource="http://www.sisostds.org/ontologies/C2SIM#Platform"/>
        <rdfs:comment>Air vehicle assembled for military use</rdfs:comment>
    </owl:Class>
    


    <!-- http://www.sisostds.org/ontologies/smx#Boundary -->

    <owl:Class rdf:about="http://www.sisostds.org/ontologies/smx#Boundary">
        <rdfs:subClassOf rdf:resource="http://www.sisostds.org/ontologies/smx#Line"/>
        <rdfs:comment>Specifies a NATO APP6-C-based tactical graphics symbol for a boundary line.</rdfs:comment>
    </owl:Class>
    


    <!-- http://www.sisostds.org/ontologies/smx#CommandRelation -->

    <owl:Class rdf:about="http://www.sisostds.org/ontologies/smx#CommandRelation">
        <rdfs:subClassOf rdf:resource="http://www.sisostds.org/ontologies/C2SIM#Relationship"/>
        <rdfs:subClassOf>
            <owl:Restriction>
                <owl:onProperty rdf:resource="http://www.sisostds.org/ontologies/smx#hasCommandRelationCode"/>
                <owl:qualifiedCardinality rdf:datatype="http://www.w3.org/2001/XMLSchema#nonNegativeInteger">1</owl:qualifiedCardinality>
                <owl:onClass rdf:resource="http://www.sisostds.org/ontologies/smx#CommandRelationCode"/>
            </owl:Restriction>
        </rdfs:subClassOf>
        <rdfs:subClassOf>
            <owl:Restriction>
                <owl:onProperty rdf:resource="http://www.sisostds.org/ontologies/C2SIM#hasActorReference"/>
                <owl:qualifiedCardinality rdf:datatype="http://www.w3.org/2001/XMLSchema#nonNegativeInteger">1</owl:qualifiedCardinality>
                <owl:onDataRange rdf:resource="http://www.sisostds.org/ontologies/C2SIM#UUIDBase"/>
            </owl:Restriction>
        </rdfs:subClassOf>
        <rdfs:comment>A relationship from some actor to an object actor, describing a relationship where one has some degree of command authority over the other</rdfs:comment>
    </owl:Class>
    <owl:Axiom>
        <owl:annotatedSource rdf:resource="http://www.sisostds.org/ontologies/smx#CommandRelation"/>
        <owl:annotatedProperty rdf:resource="http://www.w3.org/2000/01/rdf-schema#subClassOf"/>
        <owl:annotatedTarget>
            <owl:Restriction>
                <owl:onProperty rdf:resource="http://www.sisostds.org/ontologies/C2SIM#hasActorReference"/>
                <owl:qualifiedCardinality rdf:datatype="http://www.w3.org/2001/XMLSchema#nonNegativeInteger">1</owl:qualifiedCardinality>
                <owl:onDataRange rdf:resource="http://www.sisostds.org/ontologies/C2SIM#UUIDBase"/>
            </owl:Restriction>
        </owl:annotatedTarget>
        <rdfs:comment>The object of the command relation.</rdfs:comment>
    </owl:Axiom>
    


    <!-- http://www.sisostds.org/ontologies/smx#CommandRelationCode -->

    <owl:Class rdf:about="http://www.sisostds.org/ontologies/smx#CommandRelationCode">
        <rdfs:subClassOf rdf:resource="http://www.sisostds.org/ontologies/C2SIM#Code"/>
        <rdfs:comment>Enumerations of possible relationships between a unit and the unit that commands it. Obtained from JC3IEDM-v3.0.1.ObjectItemAssociationSubcategoryCode</rdfs:comment>
    </owl:Class>
    


    <!-- http://www.sisostds.org/ontologies/smx#EchelonCode -->

    <owl:Class rdf:about="http://www.sisostds.org/ontologies/smx#EchelonCode">
        <rdfs:subClassOf rdf:resource="http://www.sisostds.org/ontologies/C2SIM#Code"/>
        <rdfs:comment>Enumerations of possible echelons for a military organization from JC3IEDM-v3.0.1.EchelonSizeCode</rdfs:comment>
    </owl:Class>
    


    <!-- http://www.sisostds.org/ontologies/smx#ForceSide -->

    <owl:Class rdf:about="http://www.sisostds.org/ontologies/smx#ForceSide">
        <rdfs:subClassOf rdf:resource="http://www.sisostds.org/ontologies/C2SIM#AbstractObject"/>
        <rdfs:subClassOf>
            <owl:Restriction>
                <owl:onProperty rdf:resource="http://www.sisostds.org/ontologies/smx#hasForceSideRelation"/>
                <owl:minQualifiedCardinality rdf:datatype="http://www.w3.org/2001/XMLSchema#nonNegativeInteger">0</owl:minQualifiedCardinality>
                <owl:onClass rdf:resource="http://www.sisostds.org/ontologies/smx#ForceSideRelation"/>
            </owl:Restriction>
        </rdfs:subClassOf>
        <rdfs:comment>Class for a collection of Entities that have the same allegiance. I.e. they are all friendly to each other. For example, ForceSides could be defined for &quot;BLUFOR&quot;, &quot;OPFOR&quot;, and &quot;CIVILIAN.&quot; Entities could be associated with one of these ForceSides through the hasSide property of their EntityDescriptor object property.</rdfs:comment>
    </owl:Class>
    


    <!-- http://www.sisostds.org/ontologies/smx#ForceSideRelation -->

    <owl:Class rdf:about="http://www.sisostds.org/ontologies/smx#ForceSideRelation">
        <rdfs:subClassOf rdf:resource="http://www.sisostds.org/ontologies/C2SIM#Relationship"/>
        <rdfs:subClassOf>
            <owl:Restriction>
                <owl:onProperty rdf:resource="http://www.sisostds.org/ontologies/smx#hasHostilityStatusCode"/>
                <owl:qualifiedCardinality rdf:datatype="http://www.w3.org/2001/XMLSchema#nonNegativeInteger">1</owl:qualifiedCardinality>
                <owl:onClass rdf:resource="http://www.sisostds.org/ontologies/smx#HostilityStatusCode"/>
            </owl:Restriction>
        </rdfs:subClassOf>
        <rdfs:subClassOf>
            <owl:Restriction>
                <owl:onProperty rdf:resource="http://www.sisostds.org/ontologies/smx#hasOtherSide"/>
                <owl:qualifiedCardinality rdf:datatype="http://www.w3.org/2001/XMLSchema#nonNegativeInteger">1</owl:qualifiedCardinality>
                <owl:onDataRange rdf:resource="http://www.sisostds.org/ontologies/C2SIM#UUIDBase"/>
            </owl:Restriction>
        </rdfs:subClassOf>
        <rdfs:comment>This relation describes the hostility relationship of a military force toward another force. The force that has this relationship as its property is the &quot;military force&quot;, while the force named in the hasOtherSide property of this relationship is &quot;another force.&quot;</rdfs:comment>
    </owl:Class>
    <owl:Axiom>
        <owl:annotatedSource rdf:resource="http://www.sisostds.org/ontologies/smx#ForceSideRelation"/>
        <owl:annotatedProperty rdf:resource="http://www.w3.org/2000/01/rdf-schema#subClassOf"/>
        <owl:annotatedTarget>
            <owl:Restriction>
                <owl:onProperty rdf:resource="http://www.sisostds.org/ontologies/smx#hasOtherSide"/>
                <owl:qualifiedCardinality rdf:datatype="http://www.w3.org/2001/XMLSchema#nonNegativeInteger">1</owl:qualifiedCardinality>
                <owl:onDataRange rdf:resource="http://www.sisostds.org/ontologies/C2SIM#UUIDBase"/>
            </owl:Restriction>
        </owl:annotatedTarget>
        <rdfs:comment>The object of the relation--a ForceSide.</rdfs:comment>
    </owl:Axiom>
    


    <!-- http://www.sisostds.org/ontologies/smx#HealthObservation -->

    <owl:Class rdf:about="http://www.sisostds.org/ontologies/smx#HealthObservation">
        <rdfs:subClassOf rdf:resource="http://www.sisostds.org/ontologies/smx#Observation"/>
        <rdfs:subClassOf>
            <owl:Restriction>
                <owl:onProperty rdf:resource="http://www.sisostds.org/ontologies/C2SIM#hasEntityHealthStatus"/>
                <owl:minQualifiedCardinality rdf:datatype="http://www.w3.org/2001/XMLSchema#nonNegativeInteger">1</owl:minQualifiedCardinality>
                <owl:onClass rdf:resource="http://www.sisostds.org/ontologies/C2SIM#EntityHealthStatus"/>
            </owl:Restriction>
        </rdfs:subClassOf>
        <rdfs:comment>An observation of the health state of a subject; for example operational status or resource count.</rdfs:comment>
    </owl:Class>
    


    <!-- http://www.sisostds.org/ontologies/smx#HostilityStatusCode -->

    <owl:Class rdf:about="http://www.sisostds.org/ontologies/smx#HostilityStatusCode">
        <rdfs:subClassOf rdf:resource="http://www.sisostds.org/ontologies/C2SIM#Code"/>
        <rdfs:comment>Enumerations of possible hostility relationships in a military situation. Derived from JC3IEDM-v3.0.1.ObjectItemHostilityStatusCode</rdfs:comment>
    </owl:Class>
    


    <!-- http://www.sisostds.org/ontologies/smx#Line -->

    <owl:Class rdf:about="http://www.sisostds.org/ontologies/smx#Line">
        <rdfs:subClassOf rdf:resource="http://www.sisostds.org/ontologies/smx#TacticalGraphic"/>
        <rdfs:comment>Specifies a NATO APP6-C-based tactical graphics symbol for a line.</rdfs:comment>
    </owl:Class>
    


    <!-- http://www.sisostds.org/ontologies/smx#LocationObservation -->

    <owl:Class rdf:about="http://www.sisostds.org/ontologies/smx#LocationObservation">
        <rdfs:subClassOf rdf:resource="http://www.sisostds.org/ontologies/smx#Observation"/>
        <rdfs:subClassOf>
            <owl:Restriction>
                <owl:onProperty rdf:resource="http://www.sisostds.org/ontologies/C2SIM#hasLocation"/>
                <owl:qualifiedCardinality rdf:datatype="http://www.w3.org/2001/XMLSchema#nonNegativeInteger">1</owl:qualifiedCardinality>
                <owl:onClass rdf:resource="http://www.sisostds.org/ontologies/C2SIM#Location"/>
            </owl:Restriction>
        </rdfs:subClassOf>
        <rdfs:subClassOf>
            <owl:Restriction>
                <owl:onProperty rdf:resource="http://www.sisostds.org/ontologies/C2SIM#hasDirectionOfMovement"/>
                <owl:maxQualifiedCardinality rdf:datatype="http://www.w3.org/2001/XMLSchema#nonNegativeInteger">1</owl:maxQualifiedCardinality>
                <owl:onClass rdf:resource="http://www.sisostds.org/ontologies/C2SIM#Orientation"/>
            </owl:Restriction>
        </rdfs:subClassOf>
        <rdfs:subClassOf>
            <owl:Restriction>
                <owl:onProperty rdf:resource="http://www.sisostds.org/ontologies/C2SIM#hasSpeed"/>
                <owl:maxQualifiedCardinality rdf:datatype="http://www.w3.org/2001/XMLSchema#nonNegativeInteger">1</owl:maxQualifiedCardinality>
                <owl:onDataRange rdf:resource="http://www.w3.org/2001/XMLSchema#double"/>
            </owl:Restriction>
        </rdfs:subClassOf>
        <rdfs:comment>An observation of the location of a subject.</rdfs:comment>
    </owl:Class>
    


    <!-- http://www.sisostds.org/ontologies/smx#METOCGraphic -->

    <owl:Class rdf:about="http://www.sisostds.org/ontologies/smx#METOCGraphic">
        <rdfs:subClassOf rdf:resource="http://www.sisostds.org/ontologies/C2SIM#MapGraphic"/>
        <rdfs:comment>Specifies the NATO APP6-C-based meteorological conditions of the environment.</rdfs:comment>
    </owl:Class>
    


    <!-- http://www.sisostds.org/ontologies/smx#MIPRequestCategoryCode -->

    <owl:Class rdf:about="http://www.sisostds.org/ontologies/smx#MIPRequestCategoryCode">
        <rdfs:subClassOf rdf:resource="http://www.sisostds.org/ontologies/C2SIM#MessageCode"/>
        <rdfs:comment>A request category from the Joint Consultation Command Control Information Exchange Data Model (JC3IEDM) developed by the Multilateral Interoperability Programme (MIP).</rdfs:comment>
    </owl:Class>
    


    <!-- http://www.sisostds.org/ontologies/smx#MIPRequestContent -->

    <owl:Class rdf:about="http://www.sisostds.org/ontologies/smx#MIPRequestContent">
        <rdfs:subClassOf rdf:resource="http://www.sisostds.org/ontologies/C2SIM#RequestContent"/>
        <rdfs:subClassOf>
            <owl:Restriction>
                <owl:onProperty rdf:resource="http://www.sisostds.org/ontologies/smx#hasMIPRequestCategoryCode"/>
                <owl:qualifiedCardinality rdf:datatype="http://www.w3.org/2001/XMLSchema#nonNegativeInteger">1</owl:qualifiedCardinality>
                <owl:onClass rdf:resource="http://www.sisostds.org/ontologies/smx#MIPRequestCategoryCode"/>
            </owl:Restriction>
        </rdfs:subClassOf>
        <rdfs:comment>A request whose category is defined by the JC3IEDM request category code.</rdfs:comment>
    </owl:Class>
    


    <!-- http://www.sisostds.org/ontologies/smx#NBC_Event -->

    <owl:Class rdf:about="http://www.sisostds.org/ontologies/smx#NBC_Event">
        <rdfs:subClassOf rdf:resource="http://www.sisostds.org/ontologies/smx#TacticalGraphic"/>
        <rdfs:comment>Specifies a NATO APP6-C-based tactical graphics symbol for a Nuclear/Biological/Chemical event.</rdfs:comment>
    </owl:Class>
    


    <!-- http://www.sisostds.org/ontologies/smx#NameObservation -->

    <owl:Class rdf:about="http://www.sisostds.org/ontologies/smx#NameObservation">
        <rdfs:subClassOf rdf:resource="http://www.sisostds.org/ontologies/smx#Observation"/>
        <rdfs:subClassOf>
            <owl:Restriction>
                <owl:onProperty rdf:resource="http://www.sisostds.org/ontologies/smx#hasHostilityStatusCode"/>
                <owl:maxQualifiedCardinality rdf:datatype="http://www.w3.org/2001/XMLSchema#nonNegativeInteger">1</owl:maxQualifiedCardinality>
                <owl:onClass rdf:resource="http://www.sisostds.org/ontologies/smx#HostilityStatusCode"/>
            </owl:Restriction>
        </rdfs:subClassOf>
        <rdfs:subClassOf>
            <owl:Restriction>
                <owl:onProperty rdf:resource="http://www.sisostds.org/ontologies/C2SIM#hasName"/>
                <owl:qualifiedCardinality rdf:datatype="http://www.w3.org/2001/XMLSchema#nonNegativeInteger">1</owl:qualifiedCardinality>
                <owl:onDataRange rdf:resource="http://www.w3.org/2001/XMLSchema#string"/>
            </owl:Restriction>
        </rdfs:subClassOf>
        <rdfs:subClassOf>
            <owl:Restriction>
                <owl:onProperty rdf:resource="http://www.sisostds.org/ontologies/C2SIM#hasMarking"/>
                <owl:maxQualifiedCardinality rdf:datatype="http://www.w3.org/2001/XMLSchema#nonNegativeInteger">1</owl:maxQualifiedCardinality>
                <owl:onDataRange rdf:resource="http://www.w3.org/2001/XMLSchema#string"/>
            </owl:Restriction>
        </rdfs:subClassOf>
        <rdfs:subClassOf>
            <owl:Restriction>
                <owl:onProperty rdf:resource="http://www.sisostds.org/ontologies/smx#hasSide"/>
                <owl:maxQualifiedCardinality rdf:datatype="http://www.w3.org/2001/XMLSchema#nonNegativeInteger">1</owl:maxQualifiedCardinality>
                <owl:onDataRange rdf:resource="http://www.sisostds.org/ontologies/C2SIM#UUIDBase"/>
            </owl:Restriction>
        </rdfs:subClassOf>
        <rdfs:comment>An observation of the unit name, a vehicle marking, a force side, and/or a hostility status of the observed entity.</rdfs:comment>
    </owl:Class>
    <owl:Axiom>
        <owl:annotatedSource rdf:resource="http://www.sisostds.org/ontologies/smx#NameObservation"/>
        <owl:annotatedProperty rdf:resource="http://www.w3.org/2000/01/rdf-schema#subClassOf"/>
        <owl:annotatedTarget>
            <owl:Restriction>
                <owl:onProperty rdf:resource="http://www.sisostds.org/ontologies/smx#hasHostilityStatusCode"/>
                <owl:maxQualifiedCardinality rdf:datatype="http://www.w3.org/2001/XMLSchema#nonNegativeInteger">1</owl:maxQualifiedCardinality>
                <owl:onClass rdf:resource="http://www.sisostds.org/ontologies/smx#HostilityStatusCode"/>
            </owl:Restriction>
        </owl:annotatedTarget>
        <rdfs:comment>This code allows representation of temporary and dynamic hostility status to an observed entity.</rdfs:comment>
    </owl:Axiom>
    


    <!-- http://www.sisostds.org/ontologies/smx#Observation -->

    <owl:Class rdf:about="http://www.sisostds.org/ontologies/smx#Observation">
        <rdfs:subClassOf rdf:resource="http://www.sisostds.org/ontologies/C2SIM#C2SIMContent"/>
        <rdfs:subClassOf>
            <owl:Restriction>
                <owl:onProperty rdf:resource="http://www.sisostds.org/ontologies/C2SIM#hasActorReference"/>
                <owl:maxQualifiedCardinality rdf:datatype="http://www.w3.org/2001/XMLSchema#nonNegativeInteger">1</owl:maxQualifiedCardinality>
                <owl:onDataRange rdf:resource="http://www.w3.org/2001/XMLSchema#string"/>
            </owl:Restriction>
        </rdfs:subClassOf>
        <rdfs:subClassOf>
            <owl:Restriction>
                <owl:onProperty rdf:resource="http://www.sisostds.org/ontologies/smx#hasConfidenceLevel"/>
                <owl:maxQualifiedCardinality rdf:datatype="http://www.w3.org/2001/XMLSchema#nonNegativeInteger">1</owl:maxQualifiedCardinality>
                <owl:onDataRange rdf:resource="http://www.w3.org/2001/XMLSchema#double"/>
            </owl:Restriction>
        </rdfs:subClassOf>
        <rdfs:subClassOf>
            <owl:Restriction>
                <owl:onProperty rdf:resource="http://www.sisostds.org/ontologies/smx#hasUncertaintyInterval"/>
                <owl:maxQualifiedCardinality rdf:datatype="http://www.w3.org/2001/XMLSchema#nonNegativeInteger">1</owl:maxQualifiedCardinality>
                <owl:onDataRange rdf:resource="http://www.w3.org/2001/XMLSchema#double"/>
            </owl:Restriction>
        </rdfs:subClassOf>
        <rdfs:comment>This is an observation of the state of something in the world; generally an actor, but possibly anything that is an entity. Subclasses define specific observations that can be made.
The subclasses defined here are sufficient to create a report with Size, Activity, Location, Unit Identification, Time, and Equipment, or some subset of that.</rdfs:comment>
    </owl:Class>
    <owl:Axiom>
        <owl:annotatedSource rdf:resource="http://www.sisostds.org/ontologies/smx#Observation"/>
        <owl:annotatedProperty rdf:resource="http://www.w3.org/2000/01/rdf-schema#subClassOf"/>
        <owl:annotatedTarget>
            <owl:Restriction>
                <owl:onProperty rdf:resource="http://www.sisostds.org/ontologies/smx#hasConfidenceLevel"/>
                <owl:maxQualifiedCardinality rdf:datatype="http://www.w3.org/2001/XMLSchema#nonNegativeInteger">1</owl:maxQualifiedCardinality>
                <owl:onDataRange rdf:resource="http://www.w3.org/2001/XMLSchema#double"/>
            </owl:Restriction>
        </owl:annotatedTarget>
        <rdfs:comment>This is the probabilty that the reported value is correct.
A value between 0 and 1.</rdfs:comment>
    </owl:Axiom>
    <owl:Axiom>
        <owl:annotatedSource rdf:resource="http://www.sisostds.org/ontologies/smx#Observation"/>
        <owl:annotatedProperty rdf:resource="http://www.w3.org/2000/01/rdf-schema#subClassOf"/>
        <owl:annotatedTarget>
            <owl:Restriction>
                <owl:onProperty rdf:resource="http://www.sisostds.org/ontologies/smx#hasUncertaintyInterval"/>
                <owl:maxQualifiedCardinality rdf:datatype="http://www.w3.org/2001/XMLSchema#nonNegativeInteger">1</owl:maxQualifiedCardinality>
                <owl:onDataRange rdf:resource="http://www.w3.org/2001/XMLSchema#double"/>
            </owl:Restriction>
        </owl:annotatedTarget>
        <rdfs:comment>Uncertainty Interval is an optional qualification on an observation of a real-valued phenomenon. This is the size of the range of values (the reported value is the center) that the phenomenon could actually have. In two or three dimensions, this could be the diameter of a circle of uncertainty. The probability that the observation is in this range should be given by the ConfidenceLevel.</rdfs:comment>
    </owl:Axiom>
    


    <!-- http://www.sisostds.org/ontologies/smx#ObservationReportContent -->

    <owl:Class rdf:about="http://www.sisostds.org/ontologies/smx#ObservationReportContent">
        <rdfs:subClassOf rdf:resource="http://www.sisostds.org/ontologies/C2SIM#ReportContent"/>
        <rdfs:subClassOf>
            <owl:Restriction>
                <owl:onProperty rdf:resource="http://www.sisostds.org/ontologies/smx#hasObservation"/>
                <owl:minQualifiedCardinality rdf:datatype="http://www.w3.org/2001/XMLSchema#nonNegativeInteger">1</owl:minQualifiedCardinality>
                <owl:onClass rdf:resource="http://www.sisostds.org/ontologies/smx#Observation"/>
            </owl:Restriction>
        </rdfs:subClassOf>
        <rdfs:comment>This report contains an observation of some aspect of a subject--not necessarily including the location, health, or other facts that are in a position report.
Multiple observations all refer to the same observed actor.</rdfs:comment>
    </owl:Class>
    


    <!-- http://www.sisostds.org/ontologies/smx#Point -->

    <owl:Class rdf:about="http://www.sisostds.org/ontologies/smx#Point">
        <rdfs:subClassOf rdf:resource="http://www.sisostds.org/ontologies/smx#TacticalGraphic"/>
        <rdfs:comment>Specifies a NATO APP6-C-based tactical graphics symbol for a point location.</rdfs:comment>
    </owl:Class>
    


    <!-- http://www.sisostds.org/ontologies/smx#ReinforcedReducedType -->

    <owl:Class rdf:about="http://www.sisostds.org/ontologies/smx#ReinforcedReducedType">
        <rdfs:subClassOf rdf:resource="http://www.sisostds.org/ontologies/C2SIM#Code"/>
        <rdfs:comment>Enumerations of possible reinforcement relationships in a military situation. Dervived from JC3IEDM-v3.0.1.OrganisationStatusReinforcementCode</rdfs:comment>
    </owl:Class>
    


    <!-- http://www.sisostds.org/ontologies/smx#ResourceObservation -->

    <owl:Class rdf:about="http://www.sisostds.org/ontologies/smx#ResourceObservation">
        <rdfs:subClassOf rdf:resource="http://www.sisostds.org/ontologies/smx#Observation"/>
        <rdfs:subClassOf>
            <owl:Restriction>
                <owl:onProperty rdf:resource="http://www.sisostds.org/ontologies/C2SIM#hasResource"/>
                <owl:minQualifiedCardinality rdf:datatype="http://www.w3.org/2001/XMLSchema#nonNegativeInteger">1</owl:minQualifiedCardinality>
                <owl:onClass rdf:resource="http://www.sisostds.org/ontologies/C2SIM#Resource"/>
            </owl:Restriction>
        </rdfs:subClassOf>
        <rdfs:comment>Observations on resource availability, e.g. fuel, ammunition</rdfs:comment>
    </owl:Class>
    


    <!-- http://www.sisostds.org/ontologies/smx#Route -->

    <owl:Class rdf:about="http://www.sisostds.org/ontologies/smx#Route">
        <rdfs:subClassOf rdf:resource="http://www.sisostds.org/ontologies/smx#Line"/>
        <rdfs:comment>Specifies a NATO APP6-C-based tactical graphics symbol for a route line.</rdfs:comment>
    </owl:Class>
    


    <!-- http://www.sisostds.org/ontologies/smx#SubjectTypeObservation -->

    <owl:Class rdf:about="http://www.sisostds.org/ontologies/smx#SubjectTypeObservation">
        <rdfs:subClassOf rdf:resource="http://www.sisostds.org/ontologies/smx#Observation"/>
        <rdfs:subClassOf>
            <owl:Restriction>
                <owl:onProperty rdf:resource="http://www.sisostds.org/ontologies/smx#hasAPP6CSymbol"/>
                <owl:maxQualifiedCardinality rdf:datatype="http://www.w3.org/2001/XMLSchema#nonNegativeInteger">1</owl:maxQualifiedCardinality>
                <owl:onClass rdf:resource="http://www.sisostds.org/ontologies/smx#APP6CSymbol"/>
            </owl:Restriction>
        </rdfs:subClassOf>
        <rdfs:comment>Describes the type of the subject of an observation.</rdfs:comment>
    </owl:Class>
    <owl:Axiom>
        <owl:annotatedSource rdf:resource="http://www.sisostds.org/ontologies/smx#SubjectTypeObservation"/>
        <owl:annotatedProperty rdf:resource="http://www.w3.org/2000/01/rdf-schema#subClassOf"/>
        <owl:annotatedTarget>
            <owl:Restriction>
                <owl:onProperty rdf:resource="http://www.sisostds.org/ontologies/smx#hasAPP6CSymbol"/>
                <owl:maxQualifiedCardinality rdf:datatype="http://www.w3.org/2001/XMLSchema#nonNegativeInteger">1</owl:maxQualifiedCardinality>
                <owl:onClass rdf:resource="http://www.sisostds.org/ontologies/smx#APP6CSymbol"/>
            </owl:Restriction>
        </owl:annotatedTarget>
        <rdfs:comment>Note that the symbol SIDC allow for &quot;wildcards&quot; in some fields, i.e. for aspects of the type to be unspecified.</rdfs:comment>
    </owl:Axiom>
    


    <!-- http://www.sisostds.org/ontologies/smx#SubsurfaceVessel -->

    <owl:Class rdf:about="http://www.sisostds.org/ontologies/smx#SubsurfaceVessel">
        <rdfs:subClassOf rdf:resource="http://www.sisostds.org/ontologies/C2SIM#Platform"/>
        <rdfs:comment>Underwater vehicle assembled for military use</rdfs:comment>
    </owl:Class>
    


    <!-- http://www.sisostds.org/ontologies/smx#SurfaceVessel -->

    <owl:Class rdf:about="http://www.sisostds.org/ontologies/smx#SurfaceVessel">
        <rdfs:subClassOf rdf:resource="http://www.sisostds.org/ontologies/C2SIM#Platform"/>
        <rdfs:comment>Water surface vehicle assembled for military use</rdfs:comment>
    </owl:Class>
    


    <!-- http://www.sisostds.org/ontologies/smx#TacticalArea -->

    <owl:Class rdf:about="http://www.sisostds.org/ontologies/smx#TacticalArea">
        <rdfs:subClassOf rdf:resource="http://www.sisostds.org/ontologies/smx#TacticalGraphic"/>
        <rdfs:comment>Specifies a NATO APP6-C-based tactical graphics symbol for an area location.</rdfs:comment>
    </owl:Class>
    


    <!-- http://www.sisostds.org/ontologies/smx#TacticalGraphic -->

    <owl:Class rdf:about="http://www.sisostds.org/ontologies/smx#TacticalGraphic">
        <rdfs:subClassOf rdf:resource="http://www.sisostds.org/ontologies/C2SIM#MapGraphic"/>
        <rdfs:subClassOf>
            <owl:Restriction>
                <owl:onProperty rdf:resource="http://www.sisostds.org/ontologies/smx#hasOwner"/>
                <owl:maxQualifiedCardinality rdf:datatype="http://www.w3.org/2001/XMLSchema#nonNegativeInteger">1</owl:maxQualifiedCardinality>
                <owl:onDataRange rdf:resource="http://www.sisostds.org/ontologies/C2SIM#UUIDBase"/>
            </owl:Restriction>
        </rdfs:subClassOf>
        <rdfs:comment>Specifies a NATO APP6-C-based tactical graphics symbol.</rdfs:comment>
    </owl:Class>
    


    <!-- http://www.sisostds.org/ontologies/smx#TaskGraphic -->

    <owl:Class rdf:about="http://www.sisostds.org/ontologies/smx#TaskGraphic">
        <rdfs:subClassOf rdf:resource="http://www.sisostds.org/ontologies/smx#TacticalGraphic"/>
        <rdfs:comment>Specifies a NATO APP6-C-based tactical graphics symbol for a Task.</rdfs:comment>
    </owl:Class>
    


    <!-- http://www.sisostds.org/ontologies/smx#Unit -->

    <owl:Class rdf:about="http://www.sisostds.org/ontologies/smx#Unit">
        <rdfs:subClassOf rdf:resource="http://www.sisostds.org/ontologies/C2SIM#MilitaryOrganization"/>
        <rdfs:subClassOf>
            <owl:Restriction>
                <owl:onProperty rdf:resource="http://www.sisostds.org/ontologies/smx#hasCommandRelation"/>
                <owl:minQualifiedCardinality rdf:datatype="http://www.w3.org/2001/XMLSchema#nonNegativeInteger">0</owl:minQualifiedCardinality>
                <owl:onClass rdf:resource="http://www.sisostds.org/ontologies/smx#CommandRelation"/>
            </owl:Restriction>
        </rdfs:subClassOf>
        <rdfs:subClassOf>
            <owl:Restriction>
                <owl:onProperty rdf:resource="http://www.sisostds.org/ontologies/smx#hasEchelonCode"/>
                <owl:qualifiedCardinality rdf:datatype="http://www.w3.org/2001/XMLSchema#nonNegativeInteger">1</owl:qualifiedCardinality>
                <owl:onClass rdf:resource="http://www.sisostds.org/ontologies/smx#EchelonCode"/>
            </owl:Restriction>
        </rdfs:subClassOf>
        <rdfs:comment>An echelon of platforms, individuals, or other units.</rdfs:comment>
    </owl:Class>
    <owl:Axiom>
        <owl:annotatedSource rdf:resource="http://www.sisostds.org/ontologies/smx#Unit"/>
        <owl:annotatedProperty rdf:resource="http://www.w3.org/2000/01/rdf-schema#subClassOf"/>
        <owl:annotatedTarget>
            <owl:Restriction>
                <owl:onProperty rdf:resource="http://www.sisostds.org/ontologies/smx#hasCommandRelation"/>
                <owl:minQualifiedCardinality rdf:datatype="http://www.w3.org/2001/XMLSchema#nonNegativeInteger">0</owl:minQualifiedCardinality>
                <owl:onClass rdf:resource="http://www.sisostds.org/ontologies/smx#CommandRelation"/>
            </owl:Restriction>
        </owl:annotatedTarget>
        <rdfs:comment>An optional command relationship, which specifies an object (actor) of the relation and the relation type.</rdfs:comment>
    </owl:Axiom>
    


    <!-- http://www.sisostds.org/ontologies/smx#UnitOperationalStatusCode -->

    <owl:Class rdf:about="http://www.sisostds.org/ontologies/smx#UnitOperationalStatusCode">
        <rdfs:subClassOf rdf:resource="http://www.sisostds.org/ontologies/C2SIM#OperationalStatusCode"/>
        <rdfs:comment>Code indicating capability of unit to perform its mission, over a range of values.</rdfs:comment>
    </owl:Class>
    


    <!-- http://www.sisostds.org/ontologies/smx#UnitSymbol -->

    <owl:Class rdf:about="http://www.sisostds.org/ontologies/smx#UnitSymbol">
        <rdfs:subClassOf rdf:resource="http://www.sisostds.org/ontologies/C2SIM#MapGraphic"/>
        <rdfs:subClassOf>
            <owl:Restriction>
                <owl:onProperty rdf:resource="http://www.sisostds.org/ontologies/smx#hasOperationalStatus"/>
                <owl:maxQualifiedCardinality rdf:datatype="http://www.w3.org/2001/XMLSchema#nonNegativeInteger">1</owl:maxQualifiedCardinality>
                <owl:onClass rdf:resource="http://www.sisostds.org/ontologies/C2SIM#OperationalStatus"/>
            </owl:Restriction>
        </rdfs:subClassOf>
        <rdfs:subClassOf>
            <owl:Restriction>
                <owl:onProperty rdf:resource="http://www.sisostds.org/ontologies/smx#hasReinforcedReducedType"/>
                <owl:maxQualifiedCardinality rdf:datatype="http://www.w3.org/2001/XMLSchema#nonNegativeInteger">1</owl:maxQualifiedCardinality>
                <owl:onClass rdf:resource="http://www.sisostds.org/ontologies/smx#ReinforcedReducedType"/>
            </owl:Restriction>
        </rdfs:subClassOf>
        <rdfs:subClassOf>
            <owl:Restriction>
                <owl:onProperty rdf:resource="http://www.sisostds.org/ontologies/smx#hasHigherFormation"/>
                <owl:maxQualifiedCardinality rdf:datatype="http://www.w3.org/2001/XMLSchema#nonNegativeInteger">1</owl:maxQualifiedCardinality>
                <owl:onDataRange rdf:resource="http://www.w3.org/2001/XMLSchema#string"/>
            </owl:Restriction>
        </rdfs:subClassOf>
        <rdfs:subClassOf>
            <owl:Restriction>
                <owl:onProperty rdf:resource="http://www.sisostds.org/ontologies/smx#hasSpecialC2HQ"/>
                <owl:maxQualifiedCardinality rdf:datatype="http://www.w3.org/2001/XMLSchema#nonNegativeInteger">1</owl:maxQualifiedCardinality>
                <owl:onDataRange rdf:resource="http://www.w3.org/2001/XMLSchema#string"/>
            </owl:Restriction>
        </rdfs:subClassOf>
        <rdfs:comment>Specifies a NATO APP6-C-based tactical graphics symbol for a military unit, equipment, or installation.</rdfs:comment>
    </owl:Class>
    


    <!-- http://www.sisostds.org/ontologies/smx#Vehicle -->

    <owl:Class rdf:about="http://www.sisostds.org/ontologies/smx#Vehicle">
        <rdfs:subClassOf rdf:resource="http://www.sisostds.org/ontologies/C2SIM#Platform"/>
        <rdfs:comment>Vehicle assembled for military use; most often applies to ground vehicle</rdfs:comment>
    </owl:Class>
    


    <!-- 
    ///////////////////////////////////////////////////////////////////////////////////////
    //
    // Individuals
    //
    ///////////////////////////////////////////////////////////////////////////////////////
     -->

    


    <!-- http://www.sisostds.org/ontologies/C2SIM#ABKHAZ -->

    <owl:NamedIndividual rdf:about="http://www.sisostds.org/ontologies/C2SIM#ABKHAZ">
        <rdf:type rdf:resource="http://www.sisostds.org/ontologies/C2SIM#EthnicGroupCode"/>
        <rdfs:comment>Abkhaz: The ethnic group of Abkhaz people.</rdfs:comment>
    </owl:NamedIndividual>
    


    <!-- http://www.sisostds.org/ontologies/C2SIM#ABORGN -->

    <owl:NamedIndividual rdf:about="http://www.sisostds.org/ontologies/C2SIM#ABORGN">
        <rdf:type rdf:resource="http://www.sisostds.org/ontologies/C2SIM#EthnicGroupCode"/>
        <rdfs:comment>Aboriginal: The ethnic group of Aboriginal people.</rdfs:comment>
    </owl:NamedIndividual>
    


    <!-- http://www.sisostds.org/ontologies/C2SIM#ABW -->

    <owl:NamedIndividual rdf:about="http://www.sisostds.org/ontologies/C2SIM#ABW">
        <rdf:type rdf:resource="http://www.sisostds.org/ontologies/C2SIM#CountryCode"/>
        <rdfs:comment>Aruba: </rdfs:comment>
    </owl:NamedIndividual>
    


    <!-- http://www.sisostds.org/ontologies/C2SIM#ACKFAIL -->

    <owl:NamedIndividual rdf:about="http://www.sisostds.org/ontologies/C2SIM#ACKFAIL">
        <rdf:type rdf:resource="http://www.sisostds.org/ontologies/C2SIM#AcknowledgeTypeCode"/>
    </owl:NamedIndividual>
    


    <!-- http://www.sisostds.org/ontologies/C2SIM#ACKNOTEXEC -->

    <owl:NamedIndividual rdf:about="http://www.sisostds.org/ontologies/C2SIM#ACKNOTEXEC">
        <rdf:type rdf:resource="http://www.sisostds.org/ontologies/C2SIM#AcknowledgeTypeCode"/>
        <rdfs:comment>Not executable</rdfs:comment>
    </owl:NamedIndividual>
    


    <!-- http://www.sisostds.org/ontologies/C2SIM#ACKNOTRECGNZ -->

    <owl:NamedIndividual rdf:about="http://www.sisostds.org/ontologies/C2SIM#ACKNOTRECGNZ">
        <rdf:type rdf:resource="http://www.sisostds.org/ontologies/C2SIM#AcknowledgeTypeCode"/>
        <rdfs:comment>Not recognized</rdfs:comment>
    </owl:NamedIndividual>
    


    <!-- http://www.sisostds.org/ontologies/C2SIM#ACKNOTUNDSTD -->

    <owl:NamedIndividual rdf:about="http://www.sisostds.org/ontologies/C2SIM#ACKNOTUNDSTD">
        <rdf:type rdf:resource="http://www.sisostds.org/ontologies/C2SIM#AcknowledgeTypeCode"/>
    </owl:NamedIndividual>
    


    <!-- http://www.sisostds.org/ontologies/C2SIM#ACKRCVD -->

    <owl:NamedIndividual rdf:about="http://www.sisostds.org/ontologies/C2SIM#ACKRCVD">
        <rdf:type rdf:resource="http://www.sisostds.org/ontologies/C2SIM#AcknowledgeTypeCode"/>
    </owl:NamedIndividual>
    


    <!-- http://www.sisostds.org/ontologies/C2SIM#ACKREQDEN -->

    <owl:NamedIndividual rdf:about="http://www.sisostds.org/ontologies/C2SIM#ACKREQDEN">
        <rdf:type rdf:resource="http://www.sisostds.org/ontologies/C2SIM#AcknowledgeTypeCode"/>
        <rdfs:comment>Request denied</rdfs:comment>
    </owl:NamedIndividual>
    


    <!-- http://www.sisostds.org/ontologies/C2SIM#ACKREQGRT -->

    <owl:NamedIndividual rdf:about="http://www.sisostds.org/ontologies/C2SIM#ACKREQGRT">
        <rdf:type rdf:resource="http://www.sisostds.org/ontologies/C2SIM#AcknowledgeTypeCode"/>
        <rdfs:comment>Request granted</rdfs:comment>
    </owl:NamedIndividual>
    


    <!-- http://www.sisostds.org/ontologies/C2SIM#ACKSUCC -->

    <owl:NamedIndividual rdf:about="http://www.sisostds.org/ontologies/C2SIM#ACKSUCC">
        <rdf:type rdf:resource="http://www.sisostds.org/ontologies/C2SIM#AcknowledgeTypeCode"/>
    </owl:NamedIndividual>
    


    <!-- http://www.sisostds.org/ontologies/C2SIM#ADMISL -->

    <owl:NamedIndividual rdf:about="http://www.sisostds.org/ontologies/C2SIM#ADMISL">
        <rdf:type rdf:resource="http://www.sisostds.org/ontologies/C2SIM#EthnicGroupCode"/>
        <rdfs:comment>Admiralty Islander: The ethnic group of Admiralty Islander people.</rdfs:comment>
    </owl:NamedIndividual>
    


    <!-- http://www.sisostds.org/ontologies/C2SIM#AFAR -->

    <owl:NamedIndividual rdf:about="http://www.sisostds.org/ontologies/C2SIM#AFAR">
        <rdf:type rdf:resource="http://www.sisostds.org/ontologies/C2SIM#EthnicGroupCode"/>
        <rdfs:comment>Afar: The ethnic group of Afar people.</rdfs:comment>
    </owl:NamedIndividual>
    


    <!-- http://www.sisostds.org/ontologies/C2SIM#AFG -->

    <owl:NamedIndividual rdf:about="http://www.sisostds.org/ontologies/C2SIM#AFG">
        <rdf:type rdf:resource="http://www.sisostds.org/ontologies/C2SIM#CountryCode"/>
        <rdfs:comment>Afghanistan: </rdfs:comment>
    </owl:NamedIndividual>
    


    <!-- http://www.sisostds.org/ontologies/C2SIM#AFGHAN -->

    <owl:NamedIndividual rdf:about="http://www.sisostds.org/ontologies/C2SIM#AFGHAN">
        <rdf:type rdf:resource="http://www.sisostds.org/ontologies/C2SIM#EthnicGroupCode"/>
        <rdfs:comment>Afghani: The ethnic group of Afghani people.</rdfs:comment>
    </owl:NamedIndividual>
    


    <!-- http://www.sisostds.org/ontologies/C2SIM#AFRADJ -->

    <owl:NamedIndividual rdf:about="http://www.sisostds.org/ontologies/C2SIM#AFRADJ">
        <rdf:type rdf:resource="http://www.sisostds.org/ontologies/C2SIM#EthnicGroupCode"/>
        <rdfs:comment>African (Adja): The ethnic group of African (Adja) people.</rdfs:comment>
    </owl:NamedIndividual>
    


    <!-- http://www.sisostds.org/ontologies/C2SIM#AFRAMR -->

    <owl:NamedIndividual rdf:about="http://www.sisostds.org/ontologies/C2SIM#AFRAMR">
        <rdf:type rdf:resource="http://www.sisostds.org/ontologies/C2SIM#EthnicGroupCode"/>
        <rdfs:comment>African American: The ethnic group of African American people.</rdfs:comment>
    </owl:NamedIndividual>
    


    <!-- http://www.sisostds.org/ontologies/C2SIM#AFRBAL -->

    <owl:NamedIndividual rdf:about="http://www.sisostds.org/ontologies/C2SIM#AFRBAL">
        <rdf:type rdf:resource="http://www.sisostds.org/ontologies/C2SIM#EthnicGroupCode"/>
        <rdfs:comment>African (Balanta): The ethnic group of African (Balanta) people.</rdfs:comment>
    </owl:NamedIndividual>
    


    <!-- http://www.sisostds.org/ontologies/C2SIM#AFRBAR -->

    <owl:NamedIndividual rdf:about="http://www.sisostds.org/ontologies/C2SIM#AFRBAR">
        <rdf:type rdf:resource="http://www.sisostds.org/ontologies/C2SIM#EthnicGroupCode"/>
        <rdfs:comment>African (Bariba): The ethnic group of African (Bariba) people.</rdfs:comment>
    </owl:NamedIndividual>
    


    <!-- http://www.sisostds.org/ontologies/C2SIM#AFRBAS -->

    <owl:NamedIndividual rdf:about="http://www.sisostds.org/ontologies/C2SIM#AFRBAS">
        <rdf:type rdf:resource="http://www.sisostds.org/ontologies/C2SIM#EthnicGroupCode"/>
        <rdfs:comment>African (Bassa): The ethnic group of African (Bassa) people.</rdfs:comment>
    </owl:NamedIndividual>
    


    <!-- http://www.sisostds.org/ontologies/C2SIM#AFRBEL -->

    <owl:NamedIndividual rdf:about="http://www.sisostds.org/ontologies/C2SIM#AFRBEL">
        <rdf:type rdf:resource="http://www.sisostds.org/ontologies/C2SIM#EthnicGroupCode"/>
        <rdfs:comment>African (Bella): The ethnic group of African (Bella) people.</rdfs:comment>
    </owl:NamedIndividual>
    


    <!-- http://www.sisostds.org/ontologies/C2SIM#AFRBUR -->

    <owl:NamedIndividual rdf:about="http://www.sisostds.org/ontologies/C2SIM#AFRBUR">
        <rdf:type rdf:resource="http://www.sisostds.org/ontologies/C2SIM#EthnicGroupCode"/>
        <rdfs:comment>African (Burkinabe): The ethnic group of African (Burkinabe) people.</rdfs:comment>
    </owl:NamedIndividual>
    


    <!-- http://www.sisostds.org/ontologies/C2SIM#AFRFON -->

    <owl:NamedIndividual rdf:about="http://www.sisostds.org/ontologies/C2SIM#AFRFON">
        <rdf:type rdf:resource="http://www.sisostds.org/ontologies/C2SIM#EthnicGroupCode"/>
        <rdfs:comment>African (Fon): The ethnic group of African (Fon) people.</rdfs:comment>
    </owl:NamedIndividual>
    


    <!-- http://www.sisostds.org/ontologies/C2SIM#AFRFUL -->

    <owl:NamedIndividual rdf:about="http://www.sisostds.org/ontologies/C2SIM#AFRFUL">
        <rdf:type rdf:resource="http://www.sisostds.org/ontologies/C2SIM#EthnicGroupCode"/>
        <rdfs:comment>African (Fula): The ethnic group of African (Fula) people.</rdfs:comment>
    </owl:NamedIndividual>
    


    <!-- http://www.sisostds.org/ontologies/C2SIM#AFRGBA -->

    <owl:NamedIndividual rdf:about="http://www.sisostds.org/ontologies/C2SIM#AFRGBA">
        <rdf:type rdf:resource="http://www.sisostds.org/ontologies/C2SIM#EthnicGroupCode"/>
        <rdfs:comment>African (Gbandi): The ethnic group of African (Gbandi) people.</rdfs:comment>
    </owl:NamedIndividual>
    


    <!-- http://www.sisostds.org/ontologies/C2SIM#AFRGIO -->

    <owl:NamedIndividual rdf:about="http://www.sisostds.org/ontologies/C2SIM#AFRGIO">
        <rdf:type rdf:resource="http://www.sisostds.org/ontologies/C2SIM#EthnicGroupCode"/>
        <rdfs:comment>African (Gio): The ethnic group of African (Gio) people.</rdfs:comment>
    </owl:NamedIndividual>
    


    <!-- http://www.sisostds.org/ontologies/C2SIM#AFRGOL -->

    <owl:NamedIndividual rdf:about="http://www.sisostds.org/ontologies/C2SIM#AFRGOL">
        <rdf:type rdf:resource="http://www.sisostds.org/ontologies/C2SIM#EthnicGroupCode"/>
        <rdfs:comment>African (Gola): The ethnic group of African (Gola) people.</rdfs:comment>
    </owl:NamedIndividual>
    


    <!-- http://www.sisostds.org/ontologies/C2SIM#AFRGRE -->

    <owl:NamedIndividual rdf:about="http://www.sisostds.org/ontologies/C2SIM#AFRGRE">
        <rdf:type rdf:resource="http://www.sisostds.org/ontologies/C2SIM#EthnicGroupCode"/>
        <rdfs:comment>African (Grebo): The ethnic group of African (Grebo) people.</rdfs:comment>
    </owl:NamedIndividual>
    


    <!-- http://www.sisostds.org/ontologies/C2SIM#AFRJOL -->

    <owl:NamedIndividual rdf:about="http://www.sisostds.org/ontologies/C2SIM#AFRJOL">
        <rdf:type rdf:resource="http://www.sisostds.org/ontologies/C2SIM#EthnicGroupCode"/>
        <rdfs:comment>African (Jola): The ethnic group of African (Jola) people.</rdfs:comment>
    </owl:NamedIndividual>
    


    <!-- http://www.sisostds.org/ontologies/C2SIM#AFRKIS -->

    <owl:NamedIndividual rdf:about="http://www.sisostds.org/ontologies/C2SIM#AFRKIS">
        <rdf:type rdf:resource="http://www.sisostds.org/ontologies/C2SIM#EthnicGroupCode"/>
        <rdfs:comment>African (Kissi): The ethnic group of African (Kissi) people.</rdfs:comment>
    </owl:NamedIndividual>
    


    <!-- http://www.sisostds.org/ontologies/C2SIM#AFRKPE -->

    <owl:NamedIndividual rdf:about="http://www.sisostds.org/ontologies/C2SIM#AFRKPE">
        <rdf:type rdf:resource="http://www.sisostds.org/ontologies/C2SIM#EthnicGroupCode"/>
        <rdfs:comment>African (Kpelle): The ethnic group of African (Kpelle) people.</rdfs:comment>
    </owl:NamedIndividual>
    


    <!-- http://www.sisostds.org/ontologies/C2SIM#AFRKRA -->

    <owl:NamedIndividual rdf:about="http://www.sisostds.org/ontologies/C2SIM#AFRKRA">
        <rdf:type rdf:resource="http://www.sisostds.org/ontologies/C2SIM#EthnicGroupCode"/>
        <rdfs:comment>African (Krahn): The ethnic group of African (Krahn) people.</rdfs:comment>
    </owl:NamedIndividual>
    


    <!-- http://www.sisostds.org/ontologies/C2SIM#AFRKRU -->

    <owl:NamedIndividual rdf:about="http://www.sisostds.org/ontologies/C2SIM#AFRKRU">
        <rdf:type rdf:resource="http://www.sisostds.org/ontologies/C2SIM#EthnicGroupCode"/>
        <rdfs:comment>African (Kru): The ethnic group of African (Kru) people.</rdfs:comment>
    </owl:NamedIndividual>
    


    <!-- http://www.sisostds.org/ontologies/C2SIM#AFRLOM -->

    <owl:NamedIndividual rdf:about="http://www.sisostds.org/ontologies/C2SIM#AFRLOM">
        <rdf:type rdf:resource="http://www.sisostds.org/ontologies/C2SIM#EthnicGroupCode"/>
        <rdfs:comment>African (Loma): The ethnic group of African (Loma) people.</rdfs:comment>
    </owl:NamedIndividual>
    


    <!-- http://www.sisostds.org/ontologies/C2SIM#AFRMAN -->

    <owl:NamedIndividual rdf:about="http://www.sisostds.org/ontologies/C2SIM#AFRMAN">
        <rdf:type rdf:resource="http://www.sisostds.org/ontologies/C2SIM#EthnicGroupCode"/>
        <rdfs:comment>African (Mandinga): The ethnic group of African (Mandinga) people.</rdfs:comment>
    </owl:NamedIndividual>
    


    <!-- http://www.sisostds.org/ontologies/C2SIM#AFRMEN -->

    <owl:NamedIndividual rdf:about="http://www.sisostds.org/ontologies/C2SIM#AFRMEN">
        <rdf:type rdf:resource="http://www.sisostds.org/ontologies/C2SIM#EthnicGroupCode"/>
        <rdfs:comment>African (Mende): The ethnic group of African (Mende) people.</rdfs:comment>
    </owl:NamedIndividual>
    


    <!-- http://www.sisostds.org/ontologies/C2SIM#AFRMND -->

    <owl:NamedIndividual rdf:about="http://www.sisostds.org/ontologies/C2SIM#AFRMND">
        <rdf:type rdf:resource="http://www.sisostds.org/ontologies/C2SIM#EthnicGroupCode"/>
        <rdfs:comment>African (Mandinka): The ethnic group of African (Mandinka) people.</rdfs:comment>
    </owl:NamedIndividual>
    


    <!-- http://www.sisostds.org/ontologies/C2SIM#AFRMNJ -->

    <owl:NamedIndividual rdf:about="http://www.sisostds.org/ontologies/C2SIM#AFRMNJ">
        <rdf:type rdf:resource="http://www.sisostds.org/ontologies/C2SIM#EthnicGroupCode"/>
        <rdfs:comment>African (Manjaca): The ethnic group of African (Manjaca) people.</rdfs:comment>
    </owl:NamedIndividual>
    


    <!-- http://www.sisostds.org/ontologies/C2SIM#AFRMNO -->

    <owl:NamedIndividual rdf:about="http://www.sisostds.org/ontologies/C2SIM#AFRMNO">
        <rdf:type rdf:resource="http://www.sisostds.org/ontologies/C2SIM#EthnicGroupCode"/>
        <rdfs:comment>African (Mano): The ethnic group of African (Mano) people.</rdfs:comment>
    </owl:NamedIndividual>
    


    <!-- http://www.sisostds.org/ontologies/C2SIM#AFRMTH -->

    <owl:NamedIndividual rdf:about="http://www.sisostds.org/ontologies/C2SIM#AFRMTH">
        <rdf:type rdf:resource="http://www.sisostds.org/ontologies/C2SIM#ReligionCode"/>
        <rdfs:comment>African Methodist Episcopal (Zion): One who adheres to or identifies with the African Methodist Episcopal (Zion) doctrine.</rdfs:comment>
    </owl:NamedIndividual>
    


    <!-- http://www.sisostds.org/ontologies/C2SIM#AFRNDE -->

    <owl:NamedIndividual rdf:about="http://www.sisostds.org/ontologies/C2SIM#AFRNDE">
        <rdf:type rdf:resource="http://www.sisostds.org/ontologies/C2SIM#EthnicGroupCode"/>
        <rdfs:comment>African (Ndebele): The ethnic group of African (Ndebele) people.</rdfs:comment>
    </owl:NamedIndividual>
    


    <!-- http://www.sisostds.org/ontologies/C2SIM#AFRNFD -->

    <owl:NamedIndividual rdf:about="http://www.sisostds.org/ontologies/C2SIM#AFRNFD">
        <rdf:type rdf:resource="http://www.sisostds.org/ontologies/C2SIM#EthnicGroupCode"/>
        <rdfs:comment>African not further defined: The not further defined ethnic groups of African people.</rdfs:comment>
    </owl:NamedIndividual>
    


    <!-- http://www.sisostds.org/ontologies/C2SIM#AFROAR -->

    <owl:NamedIndividual rdf:about="http://www.sisostds.org/ontologies/C2SIM#AFROAR">
        <rdf:type rdf:resource="http://www.sisostds.org/ontologies/C2SIM#EthnicGroupCode"/>
        <rdfs:comment>Afro-Arab: The ethnic group of Afro-Arab people.</rdfs:comment>
    </owl:NamedIndividual>
    


    <!-- http://www.sisostds.org/ontologies/C2SIM#AFROAS -->

    <owl:NamedIndividual rdf:about="http://www.sisostds.org/ontologies/C2SIM#AFROAS">
        <rdf:type rdf:resource="http://www.sisostds.org/ontologies/C2SIM#EthnicGroupCode"/>
        <rdfs:comment>Afro-Asian: The ethnic group of Afro-Asian people.</rdfs:comment>
    </owl:NamedIndividual>
    


    <!-- http://www.sisostds.org/ontologies/C2SIM#AFROCH -->

    <owl:NamedIndividual rdf:about="http://www.sisostds.org/ontologies/C2SIM#AFROCH">
        <rdf:type rdf:resource="http://www.sisostds.org/ontologies/C2SIM#EthnicGroupCode"/>
        <rdfs:comment>Afro-Chinese: The ethnic group of Afro-Chinese people.</rdfs:comment>
    </owl:NamedIndividual>
    


    <!-- http://www.sisostds.org/ontologies/C2SIM#AFROEA -->

    <owl:NamedIndividual rdf:about="http://www.sisostds.org/ontologies/C2SIM#AFROEA">
        <rdf:type rdf:resource="http://www.sisostds.org/ontologies/C2SIM#EthnicGroupCode"/>
        <rdfs:comment>Afro-East Indian: The ethnic group of Afro-East Indian people.</rdfs:comment>
    </owl:NamedIndividual>
    


    <!-- http://www.sisostds.org/ontologies/C2SIM#AFROEU -->

    <owl:NamedIndividual rdf:about="http://www.sisostds.org/ontologies/C2SIM#AFROEU">
        <rdf:type rdf:resource="http://www.sisostds.org/ontologies/C2SIM#EthnicGroupCode"/>
        <rdfs:comment>Afro-European: The ethnic group of Afro-European people.</rdfs:comment>
    </owl:NamedIndividual>
    


    <!-- http://www.sisostds.org/ontologies/C2SIM#AFRPAP -->

    <owl:NamedIndividual rdf:about="http://www.sisostds.org/ontologies/C2SIM#AFRPAP">
        <rdf:type rdf:resource="http://www.sisostds.org/ontologies/C2SIM#EthnicGroupCode"/>
        <rdfs:comment>African (Papel): The ethnic group of African (Papel) people.</rdfs:comment>
    </owl:NamedIndividual>
    


    <!-- http://www.sisostds.org/ontologies/C2SIM#AFRSER -->

    <owl:NamedIndividual rdf:about="http://www.sisostds.org/ontologies/C2SIM#AFRSER">
        <rdf:type rdf:resource="http://www.sisostds.org/ontologies/C2SIM#EthnicGroupCode"/>
        <rdfs:comment>African (Serahuli): The ethnic group of African (Serahuli) people.</rdfs:comment>
    </owl:NamedIndividual>
    


    <!-- http://www.sisostds.org/ontologies/C2SIM#AFRSHO -->

    <owl:NamedIndividual rdf:about="http://www.sisostds.org/ontologies/C2SIM#AFRSHO">
        <rdf:type rdf:resource="http://www.sisostds.org/ontologies/C2SIM#EthnicGroupCode"/>
        <rdfs:comment>African (Shona): The ethnic group of African (Shona) people.</rdfs:comment>
    </owl:NamedIndividual>
    


    <!-- http://www.sisostds.org/ontologies/C2SIM#AFRTEM -->

    <owl:NamedIndividual rdf:about="http://www.sisostds.org/ontologies/C2SIM#AFRTEM">
        <rdf:type rdf:resource="http://www.sisostds.org/ontologies/C2SIM#EthnicGroupCode"/>
        <rdfs:comment>African (Temne): The ethnic group of African (Temne) people.</rdfs:comment>
    </owl:NamedIndividual>
    


    <!-- http://www.sisostds.org/ontologies/C2SIM#AFRVAI -->

    <owl:NamedIndividual rdf:about="http://www.sisostds.org/ontologies/C2SIM#AFRVAI">
        <rdf:type rdf:resource="http://www.sisostds.org/ontologies/C2SIM#EthnicGroupCode"/>
        <rdfs:comment>African (Vai): The ethnic group of African (Vai) people.</rdfs:comment>
    </owl:NamedIndividual>
    


    <!-- http://www.sisostds.org/ontologies/C2SIM#AFRWOL -->

    <owl:NamedIndividual rdf:about="http://www.sisostds.org/ontologies/C2SIM#AFRWOL">
        <rdf:type rdf:resource="http://www.sisostds.org/ontologies/C2SIM#EthnicGroupCode"/>
        <rdfs:comment>African (Wolof): The ethnic group of African (Wolof) people.</rdfs:comment>
    </owl:NamedIndividual>
    


    <!-- http://www.sisostds.org/ontologies/C2SIM#AFRYOR -->

    <owl:NamedIndividual rdf:about="http://www.sisostds.org/ontologies/C2SIM#AFRYOR">
        <rdf:type rdf:resource="http://www.sisostds.org/ontologies/C2SIM#EthnicGroupCode"/>
        <rdfs:comment>African (Yoruba): The ethnic group of African (Yoruba) people.</rdfs:comment>
    </owl:NamedIndividual>
    


    <!-- http://www.sisostds.org/ontologies/C2SIM#AGNI -->

    <owl:NamedIndividual rdf:about="http://www.sisostds.org/ontologies/C2SIM#AGNI">
        <rdf:type rdf:resource="http://www.sisostds.org/ontologies/C2SIM#EthnicGroupCode"/>
        <rdfs:comment>Agni: The ethnic group of Agni people.</rdfs:comment>
    </owl:NamedIndividual>
    


    <!-- http://www.sisostds.org/ontologies/C2SIM#AGO -->

    <owl:NamedIndividual rdf:about="http://www.sisostds.org/ontologies/C2SIM#AGO">
        <rdf:type rdf:resource="http://www.sisostds.org/ontologies/C2SIM#CountryCode"/>
        <rdfs:comment>Angola: </rdfs:comment>
    </owl:NamedIndividual>
    


    <!-- http://www.sisostds.org/ontologies/C2SIM#AIA -->

    <owl:NamedIndividual rdf:about="http://www.sisostds.org/ontologies/C2SIM#AIA">
        <rdf:type rdf:resource="http://www.sisostds.org/ontologies/C2SIM#CountryCode"/>
        <rdfs:comment>Anguilla: </rdfs:comment>
    </owl:NamedIndividual>
    


    <!-- http://www.sisostds.org/ontologies/C2SIM#AITISL -->

    <owl:NamedIndividual rdf:about="http://www.sisostds.org/ontologies/C2SIM#AITISL">
        <rdf:type rdf:resource="http://www.sisostds.org/ontologies/C2SIM#EthnicGroupCode"/>
        <rdfs:comment>Aitutaki Islander: The ethnic group of Aitutaki Islander people.</rdfs:comment>
    </owl:NamedIndividual>
    


    <!-- http://www.sisostds.org/ontologies/C2SIM#ALA -->

    <owl:NamedIndividual rdf:about="http://www.sisostds.org/ontologies/C2SIM#ALA">
        <rdf:type rdf:resource="http://www.sisostds.org/ontologies/C2SIM#CountryCode"/>
        <rdfs:comment>Åland Islands: Self governing part of Finland (added in 2004).</rdfs:comment>
    </owl:NamedIndividual>
    


    <!-- http://www.sisostds.org/ontologies/C2SIM#ALB -->

    <owl:NamedIndividual rdf:about="http://www.sisostds.org/ontologies/C2SIM#ALB">
        <rdf:type rdf:resource="http://www.sisostds.org/ontologies/C2SIM#CountryCode"/>
        <rdfs:comment>Albania: </rdfs:comment>
    </owl:NamedIndividual>
    


    <!-- http://www.sisostds.org/ontologies/C2SIM#ALBANN -->

    <owl:NamedIndividual rdf:about="http://www.sisostds.org/ontologies/C2SIM#ALBANN">
        <rdf:type rdf:resource="http://www.sisostds.org/ontologies/C2SIM#EthnicGroupCode"/>
        <rdfs:comment>Albanian-Italians: The ethnic group of Albanian-Italians people.</rdfs:comment>
    </owl:NamedIndividual>
    


    <!-- http://www.sisostds.org/ontologies/C2SIM#ALBNAN -->

    <owl:NamedIndividual rdf:about="http://www.sisostds.org/ontologies/C2SIM#ALBNAN">
        <rdf:type rdf:resource="http://www.sisostds.org/ontologies/C2SIM#EthnicGroupCode"/>
        <rdfs:comment>Albanian: The ethnic group of Albanian people.</rdfs:comment>
    </owl:NamedIndividual>
    


    <!-- http://www.sisostds.org/ontologies/C2SIM#ALEMAN -->

    <owl:NamedIndividual rdf:about="http://www.sisostds.org/ontologies/C2SIM#ALEMAN">
        <rdf:type rdf:resource="http://www.sisostds.org/ontologies/C2SIM#EthnicGroupCode"/>
        <rdfs:comment>Alemannic: The ethnic group of Alemannic people.</rdfs:comment>
    </owl:NamedIndividual>
    


    <!-- http://www.sisostds.org/ontologies/C2SIM#ALGRAN -->

    <owl:NamedIndividual rdf:about="http://www.sisostds.org/ontologies/C2SIM#ALGRAN">
        <rdf:type rdf:resource="http://www.sisostds.org/ontologies/C2SIM#EthnicGroupCode"/>
        <rdfs:comment>Algerian: The ethnic group of Algerian people.</rdfs:comment>
    </owl:NamedIndividual>
    


    <!-- http://www.sisostds.org/ontologies/C2SIM#AMERIC -->

    <owl:NamedIndividual rdf:about="http://www.sisostds.org/ontologies/C2SIM#AMERIC">
        <rdf:type rdf:resource="http://www.sisostds.org/ontologies/C2SIM#EthnicGroupCode"/>
        <rdfs:comment>Americo-Liberians: The ethnic group of Americo-Liberians people.</rdfs:comment>
    </owl:NamedIndividual>
    


    <!-- http://www.sisostds.org/ontologies/C2SIM#AMERIN -->

    <owl:NamedIndividual rdf:about="http://www.sisostds.org/ontologies/C2SIM#AMERIN">
        <rdf:type rdf:resource="http://www.sisostds.org/ontologies/C2SIM#EthnicGroupCode"/>
        <rdfs:comment>Amerindian: The ethnic group of Amerindian people.</rdfs:comment>
    </owl:NamedIndividual>
    


    <!-- http://www.sisostds.org/ontologies/C2SIM#AMERUS -->

    <owl:NamedIndividual rdf:about="http://www.sisostds.org/ontologies/C2SIM#AMERUS">
        <rdf:type rdf:resource="http://www.sisostds.org/ontologies/C2SIM#EthnicGroupCode"/>
        <rdfs:comment>American (US): The ethnic group of American (US) people.</rdfs:comment>
    </owl:NamedIndividual>
    


    <!-- http://www.sisostds.org/ontologies/C2SIM#AMHARA -->

    <owl:NamedIndividual rdf:about="http://www.sisostds.org/ontologies/C2SIM#AMHARA">
        <rdf:type rdf:resource="http://www.sisostds.org/ontologies/C2SIM#EthnicGroupCode"/>
        <rdfs:comment>Amhara: The ethnic group of Amhara people.</rdfs:comment>
    </owl:NamedIndividual>
    


    <!-- http://www.sisostds.org/ontologies/C2SIM#AND -->

    <owl:NamedIndividual rdf:about="http://www.sisostds.org/ontologies/C2SIM#AND">
        <rdf:type rdf:resource="http://www.sisostds.org/ontologies/C2SIM#CountryCode"/>
        <rdfs:comment>Andorra: </rdfs:comment>
    </owl:NamedIndividual>
    


    <!-- http://www.sisostds.org/ontologies/C2SIM#ANDORR -->

    <owl:NamedIndividual rdf:about="http://www.sisostds.org/ontologies/C2SIM#ANDORR">
        <rdf:type rdf:resource="http://www.sisostds.org/ontologies/C2SIM#EthnicGroupCode"/>
        <rdfs:comment>Andorran: The ethnic group of Andorran people.</rdfs:comment>
    </owl:NamedIndividual>
    


    <!-- http://www.sisostds.org/ontologies/C2SIM#ANGLCN -->

    <owl:NamedIndividual rdf:about="http://www.sisostds.org/ontologies/C2SIM#ANGLCN">
        <rdf:type rdf:resource="http://www.sisostds.org/ontologies/C2SIM#ReligionCode"/>
        <rdfs:comment>Anglican: One who adheres to or identifies with the Anglican doctrine.</rdfs:comment>
    </owl:NamedIndividual>
    


    <!-- http://www.sisostds.org/ontologies/C2SIM#ANGOLA -->

    <owl:NamedIndividual rdf:about="http://www.sisostds.org/ontologies/C2SIM#ANGOLA">
        <rdf:type rdf:resource="http://www.sisostds.org/ontologies/C2SIM#EthnicGroupCode"/>
        <rdfs:comment>Angolares: The ethnic group of Angolares people.</rdfs:comment>
    </owl:NamedIndividual>
    


    <!-- http://www.sisostds.org/ontologies/C2SIM#ANIMSM -->

    <owl:NamedIndividual rdf:about="http://www.sisostds.org/ontologies/C2SIM#ANIMSM">
        <rdf:type rdf:resource="http://www.sisostds.org/ontologies/C2SIM#ReligionCode"/>
        <rdfs:comment>Animism: One who adheres to or identifies with the Animism doctrine.</rdfs:comment>
    </owl:NamedIndividual>
    


    <!-- http://www.sisostds.org/ontologies/C2SIM#ANT -->

    <owl:NamedIndividual rdf:about="http://www.sisostds.org/ontologies/C2SIM#ANT">
        <rdf:type rdf:resource="http://www.sisostds.org/ontologies/C2SIM#CountryCode"/>
        <rdfs:comment>Netherlands Antilles: </rdfs:comment>
    </owl:NamedIndividual>
    


    <!-- http://www.sisostds.org/ontologies/C2SIM#ANTASA -->

    <owl:NamedIndividual rdf:about="http://www.sisostds.org/ontologies/C2SIM#ANTASA">
        <rdf:type rdf:resource="http://www.sisostds.org/ontologies/C2SIM#EthnicGroupCode"/>
        <rdfs:comment>Antaisaka: The ethnic group of Antaisaka people.</rdfs:comment>
    </owl:NamedIndividual>
    


    <!-- http://www.sisostds.org/ontologies/C2SIM#APSTLC -->

    <owl:NamedIndividual rdf:about="http://www.sisostds.org/ontologies/C2SIM#APSTLC">
        <rdf:type rdf:resource="http://www.sisostds.org/ontologies/C2SIM#ReligionCode"/>
        <rdfs:comment>Apostolic: One who adheres to or identifies with the Apostolic doctrine.</rdfs:comment>
    </owl:NamedIndividual>
    


    <!-- http://www.sisostds.org/ontologies/C2SIM#ARAB -->

    <owl:NamedIndividual rdf:about="http://www.sisostds.org/ontologies/C2SIM#ARAB">
        <rdf:type rdf:resource="http://www.sisostds.org/ontologies/C2SIM#EthnicGroupCode"/>
        <rdfs:comment>Arab: The ethnic group of Arab people.</rdfs:comment>
    </owl:NamedIndividual>
    


    <!-- http://www.sisostds.org/ontologies/C2SIM#ARABBE -->

    <owl:NamedIndividual rdf:about="http://www.sisostds.org/ontologies/C2SIM#ARABBE">
        <rdf:type rdf:resource="http://www.sisostds.org/ontologies/C2SIM#EthnicGroupCode"/>
        <rdfs:comment>Arab-Berber: The ethnic group of Arab-Berber people.</rdfs:comment>
    </owl:NamedIndividual>
    


    <!-- http://www.sisostds.org/ontologies/C2SIM#ARE -->

    <owl:NamedIndividual rdf:about="http://www.sisostds.org/ontologies/C2SIM#ARE">
        <rdf:type rdf:resource="http://www.sisostds.org/ontologies/C2SIM#CountryCode"/>
        <rdfs:comment>United Arab Emirates: </rdfs:comment>
    </owl:NamedIndividual>
    


    <!-- http://www.sisostds.org/ontologies/C2SIM#ARG -->

    <owl:NamedIndividual rdf:about="http://www.sisostds.org/ontologies/C2SIM#ARG">
        <rdf:type rdf:resource="http://www.sisostds.org/ontologies/C2SIM#CountryCode"/>
        <rdfs:comment>Argentina: </rdfs:comment>
    </owl:NamedIndividual>
    


    <!-- http://www.sisostds.org/ontologies/C2SIM#ARGNTN -->

    <owl:NamedIndividual rdf:about="http://www.sisostds.org/ontologies/C2SIM#ARGNTN">
        <rdf:type rdf:resource="http://www.sisostds.org/ontologies/C2SIM#EthnicGroupCode"/>
        <rdfs:comment>Argentinian: The ethnic group of Argentinian people.</rdfs:comment>
    </owl:NamedIndividual>
    


    <!-- http://www.sisostds.org/ontologies/C2SIM#ARM -->

    <owl:NamedIndividual rdf:about="http://www.sisostds.org/ontologies/C2SIM#ARM">
        <rdf:type rdf:resource="http://www.sisostds.org/ontologies/C2SIM#CountryCode"/>
        <rdfs:comment>Armenia: </rdfs:comment>
    </owl:NamedIndividual>
    


    <!-- http://www.sisostds.org/ontologies/C2SIM#ARMNAN -->

    <owl:NamedIndividual rdf:about="http://www.sisostds.org/ontologies/C2SIM#ARMNAN">
        <rdf:type rdf:resource="http://www.sisostds.org/ontologies/C2SIM#EthnicGroupCode"/>
        <rdf:type rdf:resource="http://www.sisostds.org/ontologies/C2SIM#ReligionCode"/>
        <rdfs:comment>Armenian: One who adheres to or identifies with the Armenian doctrine.</rdfs:comment>
        <rdfs:comment>Armenian: The ethnic group of Armenian people.</rdfs:comment>
    </owl:NamedIndividual>
    


    <!-- http://www.sisostds.org/ontologies/C2SIM#ARMORT -->

    <owl:NamedIndividual rdf:about="http://www.sisostds.org/ontologies/C2SIM#ARMORT">
        <rdf:type rdf:resource="http://www.sisostds.org/ontologies/C2SIM#ReligionCode"/>
        <rdfs:comment>Armenian Orthodox: One who adheres to or identifies with the Armenian Orthodox doctrine.</rdfs:comment>
    </owl:NamedIndividual>
    


    <!-- http://www.sisostds.org/ontologies/C2SIM#ASM -->

    <owl:NamedIndividual rdf:about="http://www.sisostds.org/ontologies/C2SIM#ASM">
        <rdf:type rdf:resource="http://www.sisostds.org/ontologies/C2SIM#CountryCode"/>
        <rdfs:comment>American Samoa: </rdfs:comment>
    </owl:NamedIndividual>
    


    <!-- http://www.sisostds.org/ontologies/C2SIM#ASMGOD -->

    <owl:NamedIndividual rdf:about="http://www.sisostds.org/ontologies/C2SIM#ASMGOD">
        <rdf:type rdf:resource="http://www.sisostds.org/ontologies/C2SIM#ReligionCode"/>
        <rdfs:comment>Assembly of God: One who adheres to or identifies with the Assembly of God doctrine.</rdfs:comment>
    </owl:NamedIndividual>
    


    <!-- http://www.sisostds.org/ontologies/C2SIM#ASNNFD -->

    <owl:NamedIndividual rdf:about="http://www.sisostds.org/ontologies/C2SIM#ASNNFD">
        <rdf:type rdf:resource="http://www.sisostds.org/ontologies/C2SIM#EthnicGroupCode"/>
        <rdfs:comment>Asian not further defined: The not further defined ethnic groups of Asian people.</rdfs:comment>
    </owl:NamedIndividual>
    


    <!-- http://www.sisostds.org/ontologies/C2SIM#ASSYRN -->

    <owl:NamedIndividual rdf:about="http://www.sisostds.org/ontologies/C2SIM#ASSYRN">
        <rdf:type rdf:resource="http://www.sisostds.org/ontologies/C2SIM#EthnicGroupCode"/>
        <rdfs:comment>Assyrian: The ethnic group of Assyrian people.</rdfs:comment>
    </owl:NamedIndividual>
    


    <!-- http://www.sisostds.org/ontologies/C2SIM#ATA -->

    <owl:NamedIndividual rdf:about="http://www.sisostds.org/ontologies/C2SIM#ATA">
        <rdf:type rdf:resource="http://www.sisostds.org/ontologies/C2SIM#CountryCode"/>
        <rdfs:comment>Antarctica: </rdfs:comment>
    </owl:NamedIndividual>
    


    <!-- http://www.sisostds.org/ontologies/C2SIM#ATF -->

    <owl:NamedIndividual rdf:about="http://www.sisostds.org/ontologies/C2SIM#ATF">
        <rdf:type rdf:resource="http://www.sisostds.org/ontologies/C2SIM#CountryCode"/>
        <rdfs:comment>French Southern Territories: </rdfs:comment>
    </owl:NamedIndividual>
    


    <!-- http://www.sisostds.org/ontologies/C2SIM#ATG -->

    <owl:NamedIndividual rdf:about="http://www.sisostds.org/ontologies/C2SIM#ATG">
        <rdf:type rdf:resource="http://www.sisostds.org/ontologies/C2SIM#CountryCode"/>
        <rdfs:comment>Antigua and Barbuda: </rdfs:comment>
    </owl:NamedIndividual>
    


    <!-- http://www.sisostds.org/ontologies/C2SIM#ATHEST -->

    <owl:NamedIndividual rdf:about="http://www.sisostds.org/ontologies/C2SIM#ATHEST">
        <rdf:type rdf:resource="http://www.sisostds.org/ontologies/C2SIM#ReligionCode"/>
        <rdfs:comment>Atheist: One who denies or disbelieves the existence of any deity.</rdfs:comment>
    </owl:NamedIndividual>
    


    <!-- http://www.sisostds.org/ontologies/C2SIM#ATUISL -->

    <owl:NamedIndividual rdf:about="http://www.sisostds.org/ontologies/C2SIM#ATUISL">
        <rdf:type rdf:resource="http://www.sisostds.org/ontologies/C2SIM#EthnicGroupCode"/>
        <rdfs:comment>Atiu Islander: The ethnic group of Atiu Islander people.</rdfs:comment>
    </owl:NamedIndividual>
    


    <!-- http://www.sisostds.org/ontologies/C2SIM#AUS -->

    <owl:NamedIndividual rdf:about="http://www.sisostds.org/ontologies/C2SIM#AUS">
        <rdf:type rdf:resource="http://www.sisostds.org/ontologies/C2SIM#CountryCode"/>
        <rdfs:comment>Australia: </rdfs:comment>
    </owl:NamedIndividual>
    


    <!-- http://www.sisostds.org/ontologies/C2SIM#AUSISL -->

    <owl:NamedIndividual rdf:about="http://www.sisostds.org/ontologies/C2SIM#AUSISL">
        <rdf:type rdf:resource="http://www.sisostds.org/ontologies/C2SIM#EthnicGroupCode"/>
        <rdfs:comment>Austral Islander: The ethnic group of Austral Islander people.</rdfs:comment>
    </owl:NamedIndividual>
    


    <!-- http://www.sisostds.org/ontologies/C2SIM#AUSTRA -->

    <owl:NamedIndividual rdf:about="http://www.sisostds.org/ontologies/C2SIM#AUSTRA">
        <rdf:type rdf:resource="http://www.sisostds.org/ontologies/C2SIM#EthnicGroupCode"/>
        <rdfs:comment>Australian Aboriginal: The ethnic group of Australian Aboriginal people.</rdfs:comment>
    </owl:NamedIndividual>
    


    <!-- http://www.sisostds.org/ontologies/C2SIM#AUSTRL -->

    <owl:NamedIndividual rdf:about="http://www.sisostds.org/ontologies/C2SIM#AUSTRL">
        <rdf:type rdf:resource="http://www.sisostds.org/ontologies/C2SIM#EthnicGroupCode"/>
        <rdfs:comment>Australian: The ethnic group of Australian people.</rdfs:comment>
    </owl:NamedIndividual>
    


    <!-- http://www.sisostds.org/ontologies/C2SIM#AUSTRN -->

    <owl:NamedIndividual rdf:about="http://www.sisostds.org/ontologies/C2SIM#AUSTRN">
        <rdf:type rdf:resource="http://www.sisostds.org/ontologies/C2SIM#EthnicGroupCode"/>
        <rdfs:comment>Austrian: The ethnic group of Austrian people.</rdfs:comment>
    </owl:NamedIndividual>
    


    <!-- http://www.sisostds.org/ontologies/C2SIM#AUT -->

    <owl:NamedIndividual rdf:about="http://www.sisostds.org/ontologies/C2SIM#AUT">
        <rdf:type rdf:resource="http://www.sisostds.org/ontologies/C2SIM#CountryCode"/>
        <rdfs:comment>Austria: </rdfs:comment>
    </owl:NamedIndividual>
    


    <!-- http://www.sisostds.org/ontologies/C2SIM#AYMARA -->

    <owl:NamedIndividual rdf:about="http://www.sisostds.org/ontologies/C2SIM#AYMARA">
        <rdf:type rdf:resource="http://www.sisostds.org/ontologies/C2SIM#EthnicGroupCode"/>
        <rdfs:comment>Aymara: The ethnic group of Aymara people.</rdfs:comment>
    </owl:NamedIndividual>
    


    <!-- http://www.sisostds.org/ontologies/C2SIM#AZE -->

    <owl:NamedIndividual rdf:about="http://www.sisostds.org/ontologies/C2SIM#AZE">
        <rdf:type rdf:resource="http://www.sisostds.org/ontologies/C2SIM#CountryCode"/>
        <rdfs:comment>Azerbaijan: </rdfs:comment>
    </owl:NamedIndividual>
    


    <!-- http://www.sisostds.org/ontologies/C2SIM#AZERBA -->

    <owl:NamedIndividual rdf:about="http://www.sisostds.org/ontologies/C2SIM#AZERBA">
        <rdf:type rdf:resource="http://www.sisostds.org/ontologies/C2SIM#EthnicGroupCode"/>
        <rdfs:comment>Azerbaijani: The ethnic group of Azerbaijani people.</rdfs:comment>
    </owl:NamedIndividual>
    


    <!-- http://www.sisostds.org/ontologies/C2SIM#AZERI -->

    <owl:NamedIndividual rdf:about="http://www.sisostds.org/ontologies/C2SIM#AZERI">
        <rdf:type rdf:resource="http://www.sisostds.org/ontologies/C2SIM#EthnicGroupCode"/>
        <rdfs:comment>Azeri: The ethnic group of Azeri people.</rdfs:comment>
    </owl:NamedIndividual>
    


    <!-- http://www.sisostds.org/ontologies/C2SIM#Accept -->

    <owl:NamedIndividual rdf:about="http://www.sisostds.org/ontologies/C2SIM#Accept">
        <rdf:type rdf:resource="http://www.sisostds.org/ontologies/C2SIM#CommunicativeActTypeCode"/>
    </owl:NamedIndividual>
    


    <!-- http://www.sisostds.org/ontologies/C2SIM#Agree -->

    <owl:NamedIndividual rdf:about="http://www.sisostds.org/ontologies/C2SIM#Agree">
        <rdf:type rdf:resource="http://www.sisostds.org/ontologies/C2SIM#CommunicativeActTypeCode"/>
    </owl:NamedIndividual>
    


    <!-- http://www.sisostds.org/ontologies/C2SIM#AssistOtherUnit -->

    <owl:NamedIndividual rdf:about="http://www.sisostds.org/ontologies/C2SIM#AssistOtherUnit">
        <rdf:type rdf:resource="http://www.sisostds.org/ontologies/C2SIM#TaskActionCode"/>
    </owl:NamedIndividual>
    <owl:Axiom>
        <owl:annotatedSource rdf:resource="http://www.sisostds.org/ontologies/C2SIM#AssistOtherUnit"/>
        <owl:annotatedProperty rdf:resource="http://www.w3.org/1999/02/22-rdf-syntax-ns#type"/>
        <owl:annotatedTarget rdf:resource="http://www.sisostds.org/ontologies/C2SIM#TaskActionCode"/>
        <rdfs:comment>Assist the AffectedUnit identified in the Task with the task it is performing.</rdfs:comment>
    </owl:Axiom>
    


    <!-- http://www.sisostds.org/ontologies/C2SIM#BABYLN -->

    <owl:NamedIndividual rdf:about="http://www.sisostds.org/ontologies/C2SIM#BABYLN">
        <rdf:type rdf:resource="http://www.sisostds.org/ontologies/C2SIM#ReligionCode"/>
        <rdfs:comment>Babylonian: One who adheres to or identifies with the Babylonian doctrine.</rdfs:comment>
    </owl:NamedIndividual>
    


    <!-- http://www.sisostds.org/ontologies/C2SIM#BAHAI -->

    <owl:NamedIndividual rdf:about="http://www.sisostds.org/ontologies/C2SIM#BAHAI">
        <rdf:type rdf:resource="http://www.sisostds.org/ontologies/C2SIM#ReligionCode"/>
        <rdfs:comment>Baha&apos;i: One who adheres to or identifies with the Baha&apos;i doctrine.</rdfs:comment>
    </owl:NamedIndividual>
    


    <!-- http://www.sisostds.org/ontologies/C2SIM#BAHRAN -->

    <owl:NamedIndividual rdf:about="http://www.sisostds.org/ontologies/C2SIM#BAHRAN">
        <rdf:type rdf:resource="http://www.sisostds.org/ontologies/C2SIM#EthnicGroupCode"/>
        <rdfs:comment>Bahraini: The ethnic group of Bahraini people.</rdfs:comment>
    </owl:NamedIndividual>
    


    <!-- http://www.sisostds.org/ontologies/C2SIM#BAKONG -->

    <owl:NamedIndividual rdf:about="http://www.sisostds.org/ontologies/C2SIM#BAKONG">
        <rdf:type rdf:resource="http://www.sisostds.org/ontologies/C2SIM#EthnicGroupCode"/>
        <rdfs:comment>Bakongo: The ethnic group of Bakongo people.</rdfs:comment>
    </owl:NamedIndividual>
    


    <!-- http://www.sisostds.org/ontologies/C2SIM#BALOCH -->

    <owl:NamedIndividual rdf:about="http://www.sisostds.org/ontologies/C2SIM#BALOCH">
        <rdf:type rdf:resource="http://www.sisostds.org/ontologies/C2SIM#EthnicGroupCode"/>
        <rdfs:comment>Baloch: The ethnic group of Baloch people.</rdfs:comment>
    </owl:NamedIndividual>
    


    <!-- http://www.sisostds.org/ontologies/C2SIM#BANDA -->

    <owl:NamedIndividual rdf:about="http://www.sisostds.org/ontologies/C2SIM#BANDA">
        <rdf:type rdf:resource="http://www.sisostds.org/ontologies/C2SIM#EthnicGroupCode"/>
        <rdfs:comment>Banda: The ethnic group of Banda people.</rdfs:comment>
    </owl:NamedIndividual>
    


    <!-- http://www.sisostds.org/ontologies/C2SIM#BANGLS -->

    <owl:NamedIndividual rdf:about="http://www.sisostds.org/ontologies/C2SIM#BANGLS">
        <rdf:type rdf:resource="http://www.sisostds.org/ontologies/C2SIM#EthnicGroupCode"/>
        <rdfs:comment>Bangladeshi: The ethnic group of Bangladeshi people.</rdfs:comment>
    </owl:NamedIndividual>
    


    <!-- http://www.sisostds.org/ontologies/C2SIM#BANTBA -->

    <owl:NamedIndividual rdf:about="http://www.sisostds.org/ontologies/C2SIM#BANTBA">
        <rdf:type rdf:resource="http://www.sisostds.org/ontologies/C2SIM#EthnicGroupCode"/>
        <rdfs:comment>Bantu (Bapounou): The ethnic group of Bantu (Bapounou) people.</rdfs:comment>
    </owl:NamedIndividual>
    


    <!-- http://www.sisostds.org/ontologies/C2SIM#BANTBT -->

    <owl:NamedIndividual rdf:about="http://www.sisostds.org/ontologies/C2SIM#BANTBT">
        <rdf:type rdf:resource="http://www.sisostds.org/ontologies/C2SIM#EthnicGroupCode"/>
        <rdfs:comment>Bantu (Bateke): The ethnic group of Bantu (Bateke) people.</rdfs:comment>
    </owl:NamedIndividual>
    


    <!-- http://www.sisostds.org/ontologies/C2SIM#BANTES -->

    <owl:NamedIndividual rdf:about="http://www.sisostds.org/ontologies/C2SIM#BANTES">
        <rdf:type rdf:resource="http://www.sisostds.org/ontologies/C2SIM#EthnicGroupCode"/>
        <rdfs:comment>Bantu (Eshira): The ethnic group of Bantu (Eshira) people.</rdfs:comment>
    </owl:NamedIndividual>
    


    <!-- http://www.sisostds.org/ontologies/C2SIM#BANTFA -->

    <owl:NamedIndividual rdf:about="http://www.sisostds.org/ontologies/C2SIM#BANTFA">
        <rdf:type rdf:resource="http://www.sisostds.org/ontologies/C2SIM#EthnicGroupCode"/>
        <rdfs:comment>Bantu (Fang): The ethnic group of Bantu (Fang) people.</rdfs:comment>
    </owl:NamedIndividual>
    


    <!-- http://www.sisostds.org/ontologies/C2SIM#BANTKO -->

    <owl:NamedIndividual rdf:about="http://www.sisostds.org/ontologies/C2SIM#BANTKO">
        <rdf:type rdf:resource="http://www.sisostds.org/ontologies/C2SIM#EthnicGroupCode"/>
        <rdfs:comment>Bantu (Kongo): The ethnic group of Bantu (Kongo) people.</rdfs:comment>
    </owl:NamedIndividual>
    


    <!-- http://www.sisostds.org/ontologies/C2SIM#BANTLU -->

    <owl:NamedIndividual rdf:about="http://www.sisostds.org/ontologies/C2SIM#BANTLU">
        <rdf:type rdf:resource="http://www.sisostds.org/ontologies/C2SIM#EthnicGroupCode"/>
        <rdfs:comment>Bantu (Luba): The ethnic group of Bantu (Luba) people.</rdfs:comment>
    </owl:NamedIndividual>
    


    <!-- http://www.sisostds.org/ontologies/C2SIM#BANTMO -->

    <owl:NamedIndividual rdf:about="http://www.sisostds.org/ontologies/C2SIM#BANTMO">
        <rdf:type rdf:resource="http://www.sisostds.org/ontologies/C2SIM#EthnicGroupCode"/>
        <rdfs:comment>Bantu (Mongo): The ethnic group of Bantu (Mongo) people.</rdfs:comment>
    </owl:NamedIndividual>
    


    <!-- http://www.sisostds.org/ontologies/C2SIM#BANTU -->

    <owl:NamedIndividual rdf:about="http://www.sisostds.org/ontologies/C2SIM#BANTU">
        <rdf:type rdf:resource="http://www.sisostds.org/ontologies/C2SIM#EthnicGroupCode"/>
        <rdfs:comment>Bantu: The ethnic group of Bantu people.</rdfs:comment>
    </owl:NamedIndividual>
    


    <!-- http://www.sisostds.org/ontologies/C2SIM#BAOULE -->

    <owl:NamedIndividual rdf:about="http://www.sisostds.org/ontologies/C2SIM#BAOULE">
        <rdf:type rdf:resource="http://www.sisostds.org/ontologies/C2SIM#EthnicGroupCode"/>
        <rdfs:comment>Baoule: The ethnic group of Baoule people.</rdfs:comment>
    </owl:NamedIndividual>
    


    <!-- http://www.sisostds.org/ontologies/C2SIM#BAPTST -->

    <owl:NamedIndividual rdf:about="http://www.sisostds.org/ontologies/C2SIM#BAPTST">
        <rdf:type rdf:resource="http://www.sisostds.org/ontologies/C2SIM#ReligionCode"/>
        <rdfs:comment>Baptist: One who adheres to or identifies with the Baptist doctrine.</rdfs:comment>
    </owl:NamedIndividual>
    


    <!-- http://www.sisostds.org/ontologies/C2SIM#BASARW -->

    <owl:NamedIndividual rdf:about="http://www.sisostds.org/ontologies/C2SIM#BASARW">
        <rdf:type rdf:resource="http://www.sisostds.org/ontologies/C2SIM#EthnicGroupCode"/>
        <rdfs:comment>Basarwa: The ethnic group of Basarwa people.</rdfs:comment>
    </owl:NamedIndividual>
    


    <!-- http://www.sisostds.org/ontologies/C2SIM#BASHKR -->

    <owl:NamedIndividual rdf:about="http://www.sisostds.org/ontologies/C2SIM#BASHKR">
        <rdf:type rdf:resource="http://www.sisostds.org/ontologies/C2SIM#EthnicGroupCode"/>
        <rdfs:comment>Bashkir: The ethnic group of Bashkir people.</rdfs:comment>
    </owl:NamedIndividual>
    


    <!-- http://www.sisostds.org/ontologies/C2SIM#BASQUE -->

    <owl:NamedIndividual rdf:about="http://www.sisostds.org/ontologies/C2SIM#BASQUE">
        <rdf:type rdf:resource="http://www.sisostds.org/ontologies/C2SIM#EthnicGroupCode"/>
        <rdfs:comment>Basque: The ethnic group of Basque people.</rdfs:comment>
    </owl:NamedIndividual>
    


    <!-- http://www.sisostds.org/ontologies/C2SIM#BATSWA -->

    <owl:NamedIndividual rdf:about="http://www.sisostds.org/ontologies/C2SIM#BATSWA">
        <rdf:type rdf:resource="http://www.sisostds.org/ontologies/C2SIM#EthnicGroupCode"/>
        <rdfs:comment>Batswana: The ethnic group of Batswana people.</rdfs:comment>
    </owl:NamedIndividual>
    


    <!-- http://www.sisostds.org/ontologies/C2SIM#BAYA -->

    <owl:NamedIndividual rdf:about="http://www.sisostds.org/ontologies/C2SIM#BAYA">
        <rdf:type rdf:resource="http://www.sisostds.org/ontologies/C2SIM#EthnicGroupCode"/>
        <rdfs:comment>Baya: The ethnic group of Baya people.</rdfs:comment>
    </owl:NamedIndividual>
    


    <!-- http://www.sisostds.org/ontologies/C2SIM#BDI -->

    <owl:NamedIndividual rdf:about="http://www.sisostds.org/ontologies/C2SIM#BDI">
        <rdf:type rdf:resource="http://www.sisostds.org/ontologies/C2SIM#CountryCode"/>
        <rdfs:comment>Burundi: </rdfs:comment>
    </owl:NamedIndividual>
    


    <!-- http://www.sisostds.org/ontologies/C2SIM#BEHAI -->

    <owl:NamedIndividual rdf:about="http://www.sisostds.org/ontologies/C2SIM#BEHAI">
        <rdf:type rdf:resource="http://www.sisostds.org/ontologies/C2SIM#ReligionCode"/>
        <rdfs:comment>Beha&apos;i: One who adheres to or identifies with the Beha&apos;i doctrine.</rdfs:comment>
    </owl:NamedIndividual>
    


    <!-- http://www.sisostds.org/ontologies/C2SIM#BEJA -->

    <owl:NamedIndividual rdf:about="http://www.sisostds.org/ontologies/C2SIM#BEJA">
        <rdf:type rdf:resource="http://www.sisostds.org/ontologies/C2SIM#EthnicGroupCode"/>
        <rdfs:comment>Beja: The ethnic group of Beja people.</rdfs:comment>
    </owl:NamedIndividual>
    


    <!-- http://www.sisostds.org/ontologies/C2SIM#BEL -->

    <owl:NamedIndividual rdf:about="http://www.sisostds.org/ontologies/C2SIM#BEL">
        <rdf:type rdf:resource="http://www.sisostds.org/ontologies/C2SIM#CountryCode"/>
        <rdfs:comment>Belgium: </rdfs:comment>
    </owl:NamedIndividual>
    


    <!-- http://www.sisostds.org/ontologies/C2SIM#BELAU -->

    <owl:NamedIndividual rdf:about="http://www.sisostds.org/ontologies/C2SIM#BELAU">
        <rdf:type rdf:resource="http://www.sisostds.org/ontologies/C2SIM#EthnicGroupCode"/>
        <rdfs:comment>Belau/Palau Islander: The ethnic group of Belau/Palau Islander people.</rdfs:comment>
    </owl:NamedIndividual>
    


    <!-- http://www.sisostds.org/ontologies/C2SIM#BELGAN -->

    <owl:NamedIndividual rdf:about="http://www.sisostds.org/ontologies/C2SIM#BELGAN">
        <rdf:type rdf:resource="http://www.sisostds.org/ontologies/C2SIM#EthnicGroupCode"/>
        <rdfs:comment>Belgian: The ethnic group of Belgian people.</rdfs:comment>
    </owl:NamedIndividual>
    


    <!-- http://www.sisostds.org/ontologies/C2SIM#BELORU -->

    <owl:NamedIndividual rdf:about="http://www.sisostds.org/ontologies/C2SIM#BELORU">
        <rdf:type rdf:resource="http://www.sisostds.org/ontologies/C2SIM#EthnicGroupCode"/>
        <rdfs:comment>Belorussian: The ethnic group of Belorussian people.</rdfs:comment>
    </owl:NamedIndividual>
    


    <!-- http://www.sisostds.org/ontologies/C2SIM#BEN -->

    <owl:NamedIndividual rdf:about="http://www.sisostds.org/ontologies/C2SIM#BEN">
        <rdf:type rdf:resource="http://www.sisostds.org/ontologies/C2SIM#CountryCode"/>
        <rdfs:comment>Benin: Formerly Dahomey (1977)</rdfs:comment>
    </owl:NamedIndividual>
    


    <!-- http://www.sisostds.org/ontologies/C2SIM#BENGLI -->

    <owl:NamedIndividual rdf:about="http://www.sisostds.org/ontologies/C2SIM#BENGLI">
        <rdf:type rdf:resource="http://www.sisostds.org/ontologies/C2SIM#EthnicGroupCode"/>
        <rdfs:comment>Bengali: The ethnic group of Bengali people.</rdfs:comment>
    </owl:NamedIndividual>
    


    <!-- http://www.sisostds.org/ontologies/C2SIM#BERBER -->

    <owl:NamedIndividual rdf:about="http://www.sisostds.org/ontologies/C2SIM#BERBER">
        <rdf:type rdf:resource="http://www.sisostds.org/ontologies/C2SIM#EthnicGroupCode"/>
        <rdfs:comment>Berber: The ethnic group of Berber people.</rdfs:comment>
    </owl:NamedIndividual>
    


    <!-- http://www.sisostds.org/ontologies/C2SIM#BERIKA -->

    <owl:NamedIndividual rdf:about="http://www.sisostds.org/ontologies/C2SIM#BERIKA">
        <rdf:type rdf:resource="http://www.sisostds.org/ontologies/C2SIM#EthnicGroupCode"/>
        <rdfs:comment>Beri (Kanouri): The ethnic group of Beri (Kanouri) people.</rdfs:comment>
    </owl:NamedIndividual>
    


    <!-- http://www.sisostds.org/ontologies/C2SIM#BETE -->

    <owl:NamedIndividual rdf:about="http://www.sisostds.org/ontologies/C2SIM#BETE">
        <rdf:type rdf:resource="http://www.sisostds.org/ontologies/C2SIM#EthnicGroupCode"/>
        <rdfs:comment>Bete: The ethnic group of Bete people.</rdfs:comment>
    </owl:NamedIndividual>
    


    <!-- http://www.sisostds.org/ontologies/C2SIM#BETSIM -->

    <owl:NamedIndividual rdf:about="http://www.sisostds.org/ontologies/C2SIM#BETSIM">
        <rdf:type rdf:resource="http://www.sisostds.org/ontologies/C2SIM#EthnicGroupCode"/>
        <rdfs:comment>Betsimisaraka: The ethnic group of Betsimisaraka people.</rdfs:comment>
    </owl:NamedIndividual>
    


    <!-- http://www.sisostds.org/ontologies/C2SIM#BFA -->

    <owl:NamedIndividual rdf:about="http://www.sisostds.org/ontologies/C2SIM#BFA">
        <rdf:type rdf:resource="http://www.sisostds.org/ontologies/C2SIM#CountryCode"/>
        <rdfs:comment>Burkina Faso: Formerly Upper Volta (1984)</rdfs:comment>
    </owl:NamedIndividual>
    


    <!-- http://www.sisostds.org/ontologies/C2SIM#BGD -->

    <owl:NamedIndividual rdf:about="http://www.sisostds.org/ontologies/C2SIM#BGD">
        <rdf:type rdf:resource="http://www.sisostds.org/ontologies/C2SIM#CountryCode"/>
        <rdfs:comment>Bangladesh: </rdfs:comment>
    </owl:NamedIndividual>
    


    <!-- http://www.sisostds.org/ontologies/C2SIM#BGR -->

    <owl:NamedIndividual rdf:about="http://www.sisostds.org/ontologies/C2SIM#BGR">
        <rdf:type rdf:resource="http://www.sisostds.org/ontologies/C2SIM#CountryCode"/>
        <rdfs:comment>Bulgaria: </rdfs:comment>
    </owl:NamedIndividual>
    


    <!-- http://www.sisostds.org/ontologies/C2SIM#BHOTE -->

    <owl:NamedIndividual rdf:about="http://www.sisostds.org/ontologies/C2SIM#BHOTE">
        <rdf:type rdf:resource="http://www.sisostds.org/ontologies/C2SIM#EthnicGroupCode"/>
        <rdfs:comment>Bhote: The ethnic group of Bhote people.</rdfs:comment>
    </owl:NamedIndividual>
    


    <!-- http://www.sisostds.org/ontologies/C2SIM#BHOTIA -->

    <owl:NamedIndividual rdf:about="http://www.sisostds.org/ontologies/C2SIM#BHOTIA">
        <rdf:type rdf:resource="http://www.sisostds.org/ontologies/C2SIM#EthnicGroupCode"/>
        <rdfs:comment>Bhotias: The ethnic group of Bhotias people.</rdfs:comment>
    </owl:NamedIndividual>
    


    <!-- http://www.sisostds.org/ontologies/C2SIM#BHR -->

    <owl:NamedIndividual rdf:about="http://www.sisostds.org/ontologies/C2SIM#BHR">
        <rdf:type rdf:resource="http://www.sisostds.org/ontologies/C2SIM#CountryCode"/>
        <rdfs:comment>Bahrain: </rdfs:comment>
    </owl:NamedIndividual>
    


    <!-- http://www.sisostds.org/ontologies/C2SIM#BHS -->

    <owl:NamedIndividual rdf:about="http://www.sisostds.org/ontologies/C2SIM#BHS">
        <rdf:type rdf:resource="http://www.sisostds.org/ontologies/C2SIM#CountryCode"/>
        <rdfs:comment>Bahamas: </rdfs:comment>
    </owl:NamedIndividual>
    


    <!-- http://www.sisostds.org/ontologies/C2SIM#BIH -->

    <owl:NamedIndividual rdf:about="http://www.sisostds.org/ontologies/C2SIM#BIH">
        <rdf:type rdf:resource="http://www.sisostds.org/ontologies/C2SIM#CountryCode"/>
        <rdfs:comment>Bosnia and Herzegovina: </rdfs:comment>
    </owl:NamedIndividual>
    


    <!-- http://www.sisostds.org/ontologies/C2SIM#BIHARS -->

    <owl:NamedIndividual rdf:about="http://www.sisostds.org/ontologies/C2SIM#BIHARS">
        <rdf:type rdf:resource="http://www.sisostds.org/ontologies/C2SIM#EthnicGroupCode"/>
        <rdfs:comment>Biharis: The ethnic group of Biharis people.</rdfs:comment>
    </owl:NamedIndividual>
    


    <!-- http://www.sisostds.org/ontologies/C2SIM#BIOKOB -->

    <owl:NamedIndividual rdf:about="http://www.sisostds.org/ontologies/C2SIM#BIOKOB">
        <rdf:type rdf:resource="http://www.sisostds.org/ontologies/C2SIM#EthnicGroupCode"/>
        <rdfs:comment>Bioko (Bubi): The ethnic group of Bioko (Bubi) people.</rdfs:comment>
    </owl:NamedIndividual>
    


    <!-- http://www.sisostds.org/ontologies/C2SIM#BIOKOF -->

    <owl:NamedIndividual rdf:about="http://www.sisostds.org/ontologies/C2SIM#BIOKOF">
        <rdf:type rdf:resource="http://www.sisostds.org/ontologies/C2SIM#EthnicGroupCode"/>
        <rdfs:comment>Bioko (Fernandinos): The ethnic group of Bioko (Fernandinos) people.</rdfs:comment>
    </owl:NamedIndividual>
    


    <!-- http://www.sisostds.org/ontologies/C2SIM#BISMAR -->

    <owl:NamedIndividual rdf:about="http://www.sisostds.org/ontologies/C2SIM#BISMAR">
        <rdf:type rdf:resource="http://www.sisostds.org/ontologies/C2SIM#EthnicGroupCode"/>
        <rdfs:comment>Bismark Archipelagoan: The ethnic group of Bismark Archipelagoan people.</rdfs:comment>
    </owl:NamedIndividual>
    


    <!-- http://www.sisostds.org/ontologies/C2SIM#BLACK -->

    <owl:NamedIndividual rdf:about="http://www.sisostds.org/ontologies/C2SIM#BLACK">
        <rdf:type rdf:resource="http://www.sisostds.org/ontologies/C2SIM#EthnicGroupCode"/>
        <rdfs:comment>Black: The ethnic group of Black people.</rdfs:comment>
    </owl:NamedIndividual>
    


    <!-- http://www.sisostds.org/ontologies/C2SIM#BLACKA -->

    <owl:NamedIndividual rdf:about="http://www.sisostds.org/ontologies/C2SIM#BLACKA">
        <rdf:type rdf:resource="http://www.sisostds.org/ontologies/C2SIM#EthnicGroupCode"/>
        <rdfs:comment>Black African: The ethnic group of Black African people.</rdfs:comment>
    </owl:NamedIndividual>
    


    <!-- http://www.sisostds.org/ontologies/C2SIM#BLGORT -->

    <owl:NamedIndividual rdf:about="http://www.sisostds.org/ontologies/C2SIM#BLGORT">
        <rdf:type rdf:resource="http://www.sisostds.org/ontologies/C2SIM#ReligionCode"/>
        <rdfs:comment>Bulgarian Orthodox: One who adheres to or identifies with the Bulgarian Orthodox doctrine.</rdfs:comment>
    </owl:NamedIndividual>
    


    <!-- http://www.sisostds.org/ontologies/C2SIM#BLR -->

    <owl:NamedIndividual rdf:about="http://www.sisostds.org/ontologies/C2SIM#BLR">
        <rdf:type rdf:resource="http://www.sisostds.org/ontologies/C2SIM#CountryCode"/>
        <rdfs:comment>Belarus: </rdfs:comment>
    </owl:NamedIndividual>
    


    <!-- http://www.sisostds.org/ontologies/C2SIM#BLZ -->

    <owl:NamedIndividual rdf:about="http://www.sisostds.org/ontologies/C2SIM#BLZ">
        <rdf:type rdf:resource="http://www.sisostds.org/ontologies/C2SIM#CountryCode"/>
        <rdfs:comment>Belize: </rdfs:comment>
    </owl:NamedIndividual>
    


    <!-- http://www.sisostds.org/ontologies/C2SIM#BMU -->

    <owl:NamedIndividual rdf:about="http://www.sisostds.org/ontologies/C2SIM#BMU">
        <rdf:type rdf:resource="http://www.sisostds.org/ontologies/C2SIM#CountryCode"/>
        <rdfs:comment>Bermuda: </rdfs:comment>
    </owl:NamedIndividual>
    


    <!-- http://www.sisostds.org/ontologies/C2SIM#BOBO -->

    <owl:NamedIndividual rdf:about="http://www.sisostds.org/ontologies/C2SIM#BOBO">
        <rdf:type rdf:resource="http://www.sisostds.org/ontologies/C2SIM#EthnicGroupCode"/>
        <rdfs:comment>Bobo: The ethnic group of Bobo people.</rdfs:comment>
    </owl:NamedIndividual>
    


    <!-- http://www.sisostds.org/ontologies/C2SIM#BOL -->

    <owl:NamedIndividual rdf:about="http://www.sisostds.org/ontologies/C2SIM#BOL">
        <rdf:type rdf:resource="http://www.sisostds.org/ontologies/C2SIM#CountryCode"/>
        <rdfs:comment>Bolivia: </rdfs:comment>
    </owl:NamedIndividual>
    


    <!-- http://www.sisostds.org/ontologies/C2SIM#BOLIVN -->

    <owl:NamedIndividual rdf:about="http://www.sisostds.org/ontologies/C2SIM#BOLIVN">
        <rdf:type rdf:resource="http://www.sisostds.org/ontologies/C2SIM#EthnicGroupCode"/>
        <rdfs:comment>Bolivian: The ethnic group of Bolivian people.</rdfs:comment>
    </owl:NamedIndividual>
    


    <!-- http://www.sisostds.org/ontologies/C2SIM#BOSCRO -->

    <owl:NamedIndividual rdf:about="http://www.sisostds.org/ontologies/C2SIM#BOSCRO">
        <rdf:type rdf:resource="http://www.sisostds.org/ontologies/C2SIM#EthnicGroupCode"/>
        <rdfs:comment>Bosnian Croat: The ethnic group of Bosnian Croat people.</rdfs:comment>
    </owl:NamedIndividual>
    


    <!-- http://www.sisostds.org/ontologies/C2SIM#BOSMUS -->

    <owl:NamedIndividual rdf:about="http://www.sisostds.org/ontologies/C2SIM#BOSMUS">
        <rdf:type rdf:resource="http://www.sisostds.org/ontologies/C2SIM#EthnicGroupCode"/>
        <rdfs:comment>Bosnian Muslim: The ethnic group of Bosnian Muslim people.</rdfs:comment>
    </owl:NamedIndividual>
    


    <!-- http://www.sisostds.org/ontologies/C2SIM#BOSSER -->

    <owl:NamedIndividual rdf:about="http://www.sisostds.org/ontologies/C2SIM#BOSSER">
        <rdf:type rdf:resource="http://www.sisostds.org/ontologies/C2SIM#EthnicGroupCode"/>
        <rdfs:comment>Bosnian Serb: The ethnic group of Bosnian Serb people.</rdfs:comment>
    </owl:NamedIndividual>
    


    <!-- http://www.sisostds.org/ontologies/C2SIM#BOUGNV -->

    <owl:NamedIndividual rdf:about="http://www.sisostds.org/ontologies/C2SIM#BOUGNV">
        <rdf:type rdf:resource="http://www.sisostds.org/ontologies/C2SIM#EthnicGroupCode"/>
        <rdfs:comment>Bougainvillean: The ethnic group of Bougainvillean people.</rdfs:comment>
    </owl:NamedIndividual>
    


    <!-- http://www.sisostds.org/ontologies/C2SIM#BRA -->

    <owl:NamedIndividual rdf:about="http://www.sisostds.org/ontologies/C2SIM#BRA">
        <rdf:type rdf:resource="http://www.sisostds.org/ontologies/C2SIM#CountryCode"/>
        <rdfs:comment>Brazil: </rdfs:comment>
    </owl:NamedIndividual>
    


    <!-- http://www.sisostds.org/ontologies/C2SIM#BRAZLN -->

    <owl:NamedIndividual rdf:about="http://www.sisostds.org/ontologies/C2SIM#BRAZLN">
        <rdf:type rdf:resource="http://www.sisostds.org/ontologies/C2SIM#EthnicGroupCode"/>
        <rdfs:comment>Brazilian: The ethnic group of Brazilian people.</rdfs:comment>
    </owl:NamedIndividual>
    


    <!-- http://www.sisostds.org/ontologies/C2SIM#BRB -->

    <owl:NamedIndividual rdf:about="http://www.sisostds.org/ontologies/C2SIM#BRB">
        <rdf:type rdf:resource="http://www.sisostds.org/ontologies/C2SIM#CountryCode"/>
        <rdfs:comment>Barbados: </rdfs:comment>
    </owl:NamedIndividual>
    


    <!-- http://www.sisostds.org/ontologies/C2SIM#BRETON -->

    <owl:NamedIndividual rdf:about="http://www.sisostds.org/ontologies/C2SIM#BRETON">
        <rdf:type rdf:resource="http://www.sisostds.org/ontologies/C2SIM#EthnicGroupCode"/>
        <rdfs:comment>Bretons: The ethnic group of Bretons people.</rdfs:comment>
    </owl:NamedIndividual>
    


    <!-- http://www.sisostds.org/ontologies/C2SIM#BRN -->

    <owl:NamedIndividual rdf:about="http://www.sisostds.org/ontologies/C2SIM#BRN">
        <rdf:type rdf:resource="http://www.sisostds.org/ontologies/C2SIM#CountryCode"/>
        <rdfs:comment>Brunei Darussalam: </rdfs:comment>
    </owl:NamedIndividual>
    


    <!-- http://www.sisostds.org/ontologies/C2SIM#BRTNEC -->

    <owl:NamedIndividual rdf:about="http://www.sisostds.org/ontologies/C2SIM#BRTNEC">
        <rdf:type rdf:resource="http://www.sisostds.org/ontologies/C2SIM#EthnicGroupCode"/>
        <rdfs:comment>British not elsewhere classified: The not elsewhere classified ethnic groups of British people.</rdfs:comment>
    </owl:NamedIndividual>
    


    <!-- http://www.sisostds.org/ontologies/C2SIM#BRTNFD -->

    <owl:NamedIndividual rdf:about="http://www.sisostds.org/ontologies/C2SIM#BRTNFD">
        <rdf:type rdf:resource="http://www.sisostds.org/ontologies/C2SIM#EthnicGroupCode"/>
        <rdfs:comment>British not further defined: The not further defined ethnic groups of British people.</rdfs:comment>
    </owl:NamedIndividual>
    


    <!-- http://www.sisostds.org/ontologies/C2SIM#BTN -->

    <owl:NamedIndividual rdf:about="http://www.sisostds.org/ontologies/C2SIM#BTN">
        <rdf:type rdf:resource="http://www.sisostds.org/ontologies/C2SIM#CountryCode"/>
        <rdfs:comment>Bhutan: </rdfs:comment>
    </owl:NamedIndividual>
    


    <!-- http://www.sisostds.org/ontologies/C2SIM#BUDHSM -->

    <owl:NamedIndividual rdf:about="http://www.sisostds.org/ontologies/C2SIM#BUDHSM">
        <rdf:type rdf:resource="http://www.sisostds.org/ontologies/C2SIM#ReligionCode"/>
        <rdfs:comment>Buddhism: One who adheres to or identifies with the Buddhism doctrine.</rdfs:comment>
    </owl:NamedIndividual>
    


    <!-- http://www.sisostds.org/ontologies/C2SIM#BULGRN -->

    <owl:NamedIndividual rdf:about="http://www.sisostds.org/ontologies/C2SIM#BULGRN">
        <rdf:type rdf:resource="http://www.sisostds.org/ontologies/C2SIM#EthnicGroupCode"/>
        <rdfs:comment>Bulgarian: The ethnic group of Bulgarian people.</rdfs:comment>
    </owl:NamedIndividual>
    


    <!-- http://www.sisostds.org/ontologies/C2SIM#BURGHR -->

    <owl:NamedIndividual rdf:about="http://www.sisostds.org/ontologies/C2SIM#BURGHR">
        <rdf:type rdf:resource="http://www.sisostds.org/ontologies/C2SIM#EthnicGroupCode"/>
        <rdfs:comment>Burgher: The ethnic group of Burgher people.</rdfs:comment>
    </owl:NamedIndividual>
    


    <!-- http://www.sisostds.org/ontologies/C2SIM#BURMAN -->

    <owl:NamedIndividual rdf:about="http://www.sisostds.org/ontologies/C2SIM#BURMAN">
        <rdf:type rdf:resource="http://www.sisostds.org/ontologies/C2SIM#EthnicGroupCode"/>
        <rdfs:comment>Burman: The ethnic group of Burman people.</rdfs:comment>
    </owl:NamedIndividual>
    


    <!-- http://www.sisostds.org/ontologies/C2SIM#BURMSE -->

    <owl:NamedIndividual rdf:about="http://www.sisostds.org/ontologies/C2SIM#BURMSE">
        <rdf:type rdf:resource="http://www.sisostds.org/ontologies/C2SIM#EthnicGroupCode"/>
        <rdfs:comment>Burmese: The ethnic group of Burmese people.</rdfs:comment>
    </owl:NamedIndividual>
    


    <!-- http://www.sisostds.org/ontologies/C2SIM#BUYI -->

    <owl:NamedIndividual rdf:about="http://www.sisostds.org/ontologies/C2SIM#BUYI">
        <rdf:type rdf:resource="http://www.sisostds.org/ontologies/C2SIM#EthnicGroupCode"/>
        <rdfs:comment>Buyi: The ethnic group of Buyi people.</rdfs:comment>
    </owl:NamedIndividual>
    


    <!-- http://www.sisostds.org/ontologies/C2SIM#BVT -->

    <owl:NamedIndividual rdf:about="http://www.sisostds.org/ontologies/C2SIM#BVT">
        <rdf:type rdf:resource="http://www.sisostds.org/ontologies/C2SIM#CountryCode"/>
        <rdfs:comment>Bouvet Island: </rdfs:comment>
    </owl:NamedIndividual>
    


    <!-- http://www.sisostds.org/ontologies/C2SIM#BWA -->

    <owl:NamedIndividual rdf:about="http://www.sisostds.org/ontologies/C2SIM#BWA">
        <rdf:type rdf:resource="http://www.sisostds.org/ontologies/C2SIM#CountryCode"/>
        <rdfs:comment>Botswana: </rdfs:comment>
    </owl:NamedIndividual>
    


    <!-- http://www.sisostds.org/ontologies/C2SIM#BYLRSN -->

    <owl:NamedIndividual rdf:about="http://www.sisostds.org/ontologies/C2SIM#BYLRSN">
        <rdf:type rdf:resource="http://www.sisostds.org/ontologies/C2SIM#EthnicGroupCode"/>
        <rdfs:comment>Byelorussian: The ethnic group of Byelorussian people.</rdfs:comment>
    </owl:NamedIndividual>
    


    <!-- http://www.sisostds.org/ontologies/C2SIM#CAF -->

    <owl:NamedIndividual rdf:about="http://www.sisostds.org/ontologies/C2SIM#CAF">
        <rdf:type rdf:resource="http://www.sisostds.org/ontologies/C2SIM#CountryCode"/>
        <rdfs:comment>Central African Republic: </rdfs:comment>
    </owl:NamedIndividual>
    


    <!-- http://www.sisostds.org/ontologies/C2SIM#CAFRE -->

    <owl:NamedIndividual rdf:about="http://www.sisostds.org/ontologies/C2SIM#CAFRE">
        <rdf:type rdf:resource="http://www.sisostds.org/ontologies/C2SIM#EthnicGroupCode"/>
        <rdfs:comment>Cafre: The ethnic group of Cafre people.</rdfs:comment>
    </owl:NamedIndividual>
    


    <!-- http://www.sisostds.org/ontologies/C2SIM#CALVNS -->

    <owl:NamedIndividual rdf:about="http://www.sisostds.org/ontologies/C2SIM#CALVNS">
        <rdf:type rdf:resource="http://www.sisostds.org/ontologies/C2SIM#ReligionCode"/>
        <rdfs:comment>Calvinist: One who adheres to or identifies with the Calvinist doctrine.</rdfs:comment>
    </owl:NamedIndividual>
    


    <!-- http://www.sisostds.org/ontologies/C2SIM#CAMERO -->

    <owl:NamedIndividual rdf:about="http://www.sisostds.org/ontologies/C2SIM#CAMERO">
        <rdf:type rdf:resource="http://www.sisostds.org/ontologies/C2SIM#EthnicGroupCode"/>
        <rdfs:comment>Cameroon Highlanders: The ethnic group of Cameroon Highlanders people.</rdfs:comment>
    </owl:NamedIndividual>
    


    <!-- http://www.sisostds.org/ontologies/C2SIM#CAN -->

    <owl:NamedIndividual rdf:about="http://www.sisostds.org/ontologies/C2SIM#CAN">
        <rdf:type rdf:resource="http://www.sisostds.org/ontologies/C2SIM#CountryCode"/>
        <rdfs:comment>Canada: </rdfs:comment>
    </owl:NamedIndividual>
    


    <!-- http://www.sisostds.org/ontologies/C2SIM#CANADN -->

    <owl:NamedIndividual rdf:about="http://www.sisostds.org/ontologies/C2SIM#CANADN">
        <rdf:type rdf:resource="http://www.sisostds.org/ontologies/C2SIM#EthnicGroupCode"/>
        <rdfs:comment>Canadian: The ethnic group of Canadian people.</rdfs:comment>
    </owl:NamedIndividual>
    


    <!-- http://www.sisostds.org/ontologies/C2SIM#CARIBN -->

    <owl:NamedIndividual rdf:about="http://www.sisostds.org/ontologies/C2SIM#CARIBN">
        <rdf:type rdf:resource="http://www.sisostds.org/ontologies/C2SIM#EthnicGroupCode"/>
        <rdfs:comment>Carib Indian: The ethnic group of Carib Indian people.</rdfs:comment>
    </owl:NamedIndividual>
    


    <!-- http://www.sisostds.org/ontologies/C2SIM#CARISL -->

    <owl:NamedIndividual rdf:about="http://www.sisostds.org/ontologies/C2SIM#CARISL">
        <rdf:type rdf:resource="http://www.sisostds.org/ontologies/C2SIM#EthnicGroupCode"/>
        <rdfs:comment>Caroline Islander: The ethnic group of Caroline Islander people.</rdfs:comment>
    </owl:NamedIndividual>
    


    <!-- http://www.sisostds.org/ontologies/C2SIM#CATHLC -->

    <owl:NamedIndividual rdf:about="http://www.sisostds.org/ontologies/C2SIM#CATHLC">
        <rdf:type rdf:resource="http://www.sisostds.org/ontologies/C2SIM#ReligionCode"/>
        <rdfs:comment>Catholic: One who adheres to or identifies with the Catholic doctrine.</rdfs:comment>
    </owl:NamedIndividual>
    


    <!-- http://www.sisostds.org/ontologies/C2SIM#CAUCAS -->

    <owl:NamedIndividual rdf:about="http://www.sisostds.org/ontologies/C2SIM#CAUCAS">
        <rdf:type rdf:resource="http://www.sisostds.org/ontologies/C2SIM#EthnicGroupCode"/>
        <rdfs:comment>Caucasian: The ethnic group of Caucasian people.</rdfs:comment>
    </owl:NamedIndividual>
    


    <!-- http://www.sisostds.org/ontologies/C2SIM#CCK -->

    <owl:NamedIndividual rdf:about="http://www.sisostds.org/ontologies/C2SIM#CCK">
        <rdf:type rdf:resource="http://www.sisostds.org/ontologies/C2SIM#CountryCode"/>
        <rdfs:comment>Cocos (Keeling) Islands: </rdfs:comment>
    </owl:NamedIndividual>
    


    <!-- http://www.sisostds.org/ontologies/C2SIM#CELTIC -->

    <owl:NamedIndividual rdf:about="http://www.sisostds.org/ontologies/C2SIM#CELTIC">
        <rdf:type rdf:resource="http://www.sisostds.org/ontologies/C2SIM#EthnicGroupCode"/>
        <rdfs:comment>Celtic: The ethnic group of Celtic people.</rdfs:comment>
    </owl:NamedIndividual>
    


    <!-- http://www.sisostds.org/ontologies/C2SIM#CENAMR -->

    <owl:NamedIndividual rdf:about="http://www.sisostds.org/ontologies/C2SIM#CENAMR">
        <rdf:type rdf:resource="http://www.sisostds.org/ontologies/C2SIM#EthnicGroupCode"/>
        <rdfs:comment>Central American Indian: The ethnic group of Central American Indian people.</rdfs:comment>
    </owl:NamedIndividual>
    


    <!-- http://www.sisostds.org/ontologies/C2SIM#CHAHAR -->

    <owl:NamedIndividual rdf:about="http://www.sisostds.org/ontologies/C2SIM#CHAHAR">
        <rdf:type rdf:resource="http://www.sisostds.org/ontologies/C2SIM#EthnicGroupCode"/>
        <rdfs:comment>Chahar Aimaks: The ethnic group of Chahar Aimaks people.</rdfs:comment>
    </owl:NamedIndividual>
    


    <!-- http://www.sisostds.org/ontologies/C2SIM#CHAM -->

    <owl:NamedIndividual rdf:about="http://www.sisostds.org/ontologies/C2SIM#CHAM">
        <rdf:type rdf:resource="http://www.sisostds.org/ontologies/C2SIM#EthnicGroupCode"/>
        <rdfs:comment>Cham: The ethnic group of Cham people.</rdfs:comment>
    </owl:NamedIndividual>
    


    <!-- http://www.sisostds.org/ontologies/C2SIM#CHAMOR -->

    <owl:NamedIndividual rdf:about="http://www.sisostds.org/ontologies/C2SIM#CHAMOR">
        <rdf:type rdf:resource="http://www.sisostds.org/ontologies/C2SIM#EthnicGroupCode"/>
        <rdfs:comment>Chamorro: The ethnic group of Chamorro people.</rdfs:comment>
    </owl:NamedIndividual>
    


    <!-- http://www.sisostds.org/ontologies/C2SIM#CHE -->

    <owl:NamedIndividual rdf:about="http://www.sisostds.org/ontologies/C2SIM#CHE">
        <rdf:type rdf:resource="http://www.sisostds.org/ontologies/C2SIM#CountryCode"/>
        <rdfs:comment>Switzerland: </rdfs:comment>
    </owl:NamedIndividual>
    


    <!-- http://www.sisostds.org/ontologies/C2SIM#CHEWA -->

    <owl:NamedIndividual rdf:about="http://www.sisostds.org/ontologies/C2SIM#CHEWA">
        <rdf:type rdf:resource="http://www.sisostds.org/ontologies/C2SIM#EthnicGroupCode"/>
        <rdfs:comment>Chewa: The ethnic group of Chewa people.</rdfs:comment>
    </owl:NamedIndividual>
    


    <!-- http://www.sisostds.org/ontologies/C2SIM#CHL -->

    <owl:NamedIndividual rdf:about="http://www.sisostds.org/ontologies/C2SIM#CHL">
        <rdf:type rdf:resource="http://www.sisostds.org/ontologies/C2SIM#CountryCode"/>
        <rdfs:comment>Chile: </rdfs:comment>
    </owl:NamedIndividual>
    


    <!-- http://www.sisostds.org/ontologies/C2SIM#CHLEAN -->

    <owl:NamedIndividual rdf:about="http://www.sisostds.org/ontologies/C2SIM#CHLEAN">
        <rdf:type rdf:resource="http://www.sisostds.org/ontologies/C2SIM#EthnicGroupCode"/>
        <rdfs:comment>Chilean: The ethnic group of Chilean people.</rdfs:comment>
    </owl:NamedIndividual>
    


    <!-- http://www.sisostds.org/ontologies/C2SIM#CHN -->

    <owl:NamedIndividual rdf:about="http://www.sisostds.org/ontologies/C2SIM#CHN">
        <rdf:type rdf:resource="http://www.sisostds.org/ontologies/C2SIM#CountryCode"/>
        <rdfs:comment>China: </rdfs:comment>
    </owl:NamedIndividual>
    


    <!-- http://www.sisostds.org/ontologies/C2SIM#CHNDGY -->

    <owl:NamedIndividual rdf:about="http://www.sisostds.org/ontologies/C2SIM#CHNDGY">
        <rdf:type rdf:resource="http://www.sisostds.org/ontologies/C2SIM#ReligionCode"/>
        <rdfs:comment>Chondogyo: One who adheres to or identifies with the Chondogyo doctrine.</rdfs:comment>
    </owl:NamedIndividual>
    


    <!-- http://www.sisostds.org/ontologies/C2SIM#CHNISL -->

    <owl:NamedIndividual rdf:about="http://www.sisostds.org/ontologies/C2SIM#CHNISL">
        <rdf:type rdf:resource="http://www.sisostds.org/ontologies/C2SIM#EthnicGroupCode"/>
        <rdfs:comment>Channel Islander: The ethnic group of Channel Islander people.</rdfs:comment>
    </owl:NamedIndividual>
    


    <!-- http://www.sisostds.org/ontologies/C2SIM#CHNNEC -->

    <owl:NamedIndividual rdf:about="http://www.sisostds.org/ontologies/C2SIM#CHNNEC">
        <rdf:type rdf:resource="http://www.sisostds.org/ontologies/C2SIM#EthnicGroupCode"/>
        <rdfs:comment>Chinese not elsewhere classified: The not elsewhere classified ethnic groups of Chinese people.</rdfs:comment>
    </owl:NamedIndividual>
    


    <!-- http://www.sisostds.org/ontologies/C2SIM#CHNNFD -->

    <owl:NamedIndividual rdf:about="http://www.sisostds.org/ontologies/C2SIM#CHNNFD">
        <rdf:type rdf:resource="http://www.sisostds.org/ontologies/C2SIM#EthnicGroupCode"/>
        <rdfs:comment>Chinese not further defined: The not further defined ethnic groups of Chinese people.</rdfs:comment>
    </owl:NamedIndividual>
    


    <!-- http://www.sisostds.org/ontologies/C2SIM#CHRENG -->

    <owl:NamedIndividual rdf:about="http://www.sisostds.org/ontologies/C2SIM#CHRENG">
        <rdf:type rdf:resource="http://www.sisostds.org/ontologies/C2SIM#ReligionCode"/>
        <rdfs:comment>Church of England: One who adheres to or identifies with the Church of England doctrine.</rdfs:comment>
    </owl:NamedIndividual>
    


    <!-- http://www.sisostds.org/ontologies/C2SIM#CHRFRW -->

    <owl:NamedIndividual rdf:about="http://www.sisostds.org/ontologies/C2SIM#CHRFRW">
        <rdf:type rdf:resource="http://www.sisostds.org/ontologies/C2SIM#ReligionCode"/>
        <rdfs:comment>Christian (Free Wesleyan Church): One who adheres to or identifies with the Christian (Free Wesleyan Church) doctrine.</rdfs:comment>
    </owl:NamedIndividual>
    


    <!-- http://www.sisostds.org/ontologies/C2SIM#CHRGOD -->

    <owl:NamedIndividual rdf:about="http://www.sisostds.org/ontologies/C2SIM#CHRGOD">
        <rdf:type rdf:resource="http://www.sisostds.org/ontologies/C2SIM#ReligionCode"/>
        <rdfs:comment>Church of God: One who adheres to or identifies with the Church of God doctrine.</rdfs:comment>
    </owl:NamedIndividual>
    


    <!-- http://www.sisostds.org/ontologies/C2SIM#CHRSLB -->

    <owl:NamedIndividual rdf:about="http://www.sisostds.org/ontologies/C2SIM#CHRSLB">
        <rdf:type rdf:resource="http://www.sisostds.org/ontologies/C2SIM#ReligionCode"/>
        <rdfs:comment>Christian (Liebenzell Mission): One who adheres to or identifies with the Christian (Liebenzell Mission) doctrine.</rdfs:comment>
    </owl:NamedIndividual>
    


    <!-- http://www.sisostds.org/ontologies/C2SIM#CHRSTN -->

    <owl:NamedIndividual rdf:about="http://www.sisostds.org/ontologies/C2SIM#CHRSTN">
        <rdf:type rdf:resource="http://www.sisostds.org/ontologies/C2SIM#EthnicGroupCode"/>
        <rdf:type rdf:resource="http://www.sisostds.org/ontologies/C2SIM#ReligionCode"/>
        <rdfs:comment>Christian Malay: The ethnic group of Christian Malay people.</rdfs:comment>
        <rdfs:comment>Christian: One who adheres to or identifies with the Christian doctrine.</rdfs:comment>
    </owl:NamedIndividual>
    


    <!-- http://www.sisostds.org/ontologies/C2SIM#CHRTVL -->

    <owl:NamedIndividual rdf:about="http://www.sisostds.org/ontologies/C2SIM#CHRTVL">
        <rdf:type rdf:resource="http://www.sisostds.org/ontologies/C2SIM#ReligionCode"/>
        <rdfs:comment>Church of Tuvalu: One who adheres to or identifies with the Church of Tuvalu doctrine.</rdfs:comment>
    </owl:NamedIndividual>
    


    <!-- http://www.sisostds.org/ontologies/C2SIM#CHUVAS -->

    <owl:NamedIndividual rdf:about="http://www.sisostds.org/ontologies/C2SIM#CHUVAS">
        <rdf:type rdf:resource="http://www.sisostds.org/ontologies/C2SIM#EthnicGroupCode"/>
        <rdfs:comment>Chuvash: The ethnic group of Chuvash people.</rdfs:comment>
    </owl:NamedIndividual>
    


    <!-- http://www.sisostds.org/ontologies/C2SIM#CIRCAS -->

    <owl:NamedIndividual rdf:about="http://www.sisostds.org/ontologies/C2SIM#CIRCAS">
        <rdf:type rdf:resource="http://www.sisostds.org/ontologies/C2SIM#EthnicGroupCode"/>
        <rdfs:comment>Circassian: The ethnic group of Circassian people.</rdfs:comment>
    </owl:NamedIndividual>
    


    <!-- http://www.sisostds.org/ontologies/C2SIM#CIV -->

    <owl:NamedIndividual rdf:about="http://www.sisostds.org/ontologies/C2SIM#CIV">
        <rdf:type rdf:resource="http://www.sisostds.org/ontologies/C2SIM#CountryCode"/>
        <rdfs:comment>Cote d&apos;Ivoire: Formerly Ivory Coast</rdfs:comment>
    </owl:NamedIndividual>
    


    <!-- http://www.sisostds.org/ontologies/C2SIM#CIVCON -->

    <owl:NamedIndividual rdf:about="http://www.sisostds.org/ontologies/C2SIM#CIVCON">
        <rdf:type rdf:resource="http://www.sisostds.org/ontologies/C2SIM#OrganizationTypeCode"/>
        <rdfs:comment>Civilian-convoy-type: A class of civilian convoys.</rdfs:comment>
    </owl:NamedIndividual>
    


    <!-- http://www.sisostds.org/ontologies/C2SIM#CMR -->

    <owl:NamedIndividual rdf:about="http://www.sisostds.org/ontologies/C2SIM#CMR">
        <rdf:type rdf:resource="http://www.sisostds.org/ontologies/C2SIM#CountryCode"/>
        <rdfs:comment>Cameroon: </rdfs:comment>
    </owl:NamedIndividual>
    


    <!-- http://www.sisostds.org/ontologies/C2SIM#CNFCNS -->

    <owl:NamedIndividual rdf:about="http://www.sisostds.org/ontologies/C2SIM#CNFCNS">
        <rdf:type rdf:resource="http://www.sisostds.org/ontologies/C2SIM#ReligionCode"/>
        <rdfs:comment>Confucianism: One who adheres to or identifies with the Confucianism doctrine.</rdfs:comment>
    </owl:NamedIndividual>
    


    <!-- http://www.sisostds.org/ontologies/C2SIM#CNG -->

    <owl:NamedIndividual rdf:about="http://www.sisostds.org/ontologies/C2SIM#CNG">
        <rdf:type rdf:resource="http://www.sisostds.org/ontologies/C2SIM#ReligionCode"/>
        <rdfs:comment>Congregational: One who adheres to or identifies with the Congregational doctrine.</rdfs:comment>
    </owl:NamedIndividual>
    


    <!-- http://www.sisostds.org/ontologies/C2SIM#CNGCCH -->

    <owl:NamedIndividual rdf:about="http://www.sisostds.org/ontologies/C2SIM#CNGCCH">
        <rdf:type rdf:resource="http://www.sisostds.org/ontologies/C2SIM#ReligionCode"/>
        <rdfs:comment>Congregational Christian Church: One who adheres to or identifies with the Congregational Christian Church doctrine.</rdfs:comment>
    </owl:NamedIndividual>
    


    <!-- http://www.sisostds.org/ontologies/C2SIM#CNGNCH -->

    <owl:NamedIndividual rdf:about="http://www.sisostds.org/ontologies/C2SIM#CNGNCH">
        <rdf:type rdf:resource="http://www.sisostds.org/ontologies/C2SIM#ReligionCode"/>
        <rdfs:comment>Congregational New Church: One who adheres to or identifies with the Congregational New Church doctrine.</rdfs:comment>
    </owl:NamedIndividual>
    


    <!-- http://www.sisostds.org/ontologies/C2SIM#CNTRCT -->

    <owl:NamedIndividual rdf:about="http://www.sisostds.org/ontologies/C2SIM#CNTRCT">
        <rdf:type rdf:resource="http://www.sisostds.org/ontologies/C2SIM#OrganizationTypeCode"/>
        <rdfs:comment>Contractor: A GROUP-ORGANISATION-TYPE who contracts or undertakes to supply certain articles, or to perform any work or service (esp.</rdfs:comment>
    </owl:NamedIndividual>
    


    <!-- http://www.sisostds.org/ontologies/C2SIM#COASTA -->

    <owl:NamedIndividual rdf:about="http://www.sisostds.org/ontologies/C2SIM#COASTA">
        <rdf:type rdf:resource="http://www.sisostds.org/ontologies/C2SIM#EthnicGroupCode"/>
        <rdfs:comment>Coastal Malays: The ethnic group of Coastal Malays people.</rdfs:comment>
    </owl:NamedIndividual>
    


    <!-- http://www.sisostds.org/ontologies/C2SIM#COCOSM -->

    <owl:NamedIndividual rdf:about="http://www.sisostds.org/ontologies/C2SIM#COCOSM">
        <rdf:type rdf:resource="http://www.sisostds.org/ontologies/C2SIM#EthnicGroupCode"/>
        <rdfs:comment>Cocos Malays: The ethnic group of Cocos Malays people.</rdfs:comment>
    </owl:NamedIndividual>
    


    <!-- http://www.sisostds.org/ontologies/C2SIM#COD -->

    <owl:NamedIndividual rdf:about="http://www.sisostds.org/ontologies/C2SIM#COD">
        <rdf:type rdf:resource="http://www.sisostds.org/ontologies/C2SIM#CountryCode"/>
        <rdfs:comment>Congo, Democratic Republic of the: </rdfs:comment>
    </owl:NamedIndividual>
    


    <!-- http://www.sisostds.org/ontologies/C2SIM#COG -->

    <owl:NamedIndividual rdf:about="http://www.sisostds.org/ontologies/C2SIM#COG">
        <rdf:type rdf:resource="http://www.sisostds.org/ontologies/C2SIM#CountryCode"/>
        <rdfs:comment>Congo: </rdfs:comment>
    </owl:NamedIndividual>
    


    <!-- http://www.sisostds.org/ontologies/C2SIM#COK -->

    <owl:NamedIndividual rdf:about="http://www.sisostds.org/ontologies/C2SIM#COK">
        <rdf:type rdf:resource="http://www.sisostds.org/ontologies/C2SIM#CountryCode"/>
        <rdfs:comment>Cook Islands: </rdfs:comment>
    </owl:NamedIndividual>
    


    <!-- http://www.sisostds.org/ontologies/C2SIM#COKNFD -->

    <owl:NamedIndividual rdf:about="http://www.sisostds.org/ontologies/C2SIM#COKNFD">
        <rdf:type rdf:resource="http://www.sisostds.org/ontologies/C2SIM#EthnicGroupCode"/>
        <rdfs:comment>Cook Island Maori not further defined: The not further defined ethnic groups of Cook Island Maori people.</rdfs:comment>
    </owl:NamedIndividual>
    


    <!-- http://www.sisostds.org/ontologies/C2SIM#COL -->

    <owl:NamedIndividual rdf:about="http://www.sisostds.org/ontologies/C2SIM#COL">
        <rdf:type rdf:resource="http://www.sisostds.org/ontologies/C2SIM#CountryCode"/>
        <rdfs:comment>Colombia: </rdfs:comment>
    </owl:NamedIndividual>
    


    <!-- http://www.sisostds.org/ontologies/C2SIM#COLMBN -->

    <owl:NamedIndividual rdf:about="http://www.sisostds.org/ontologies/C2SIM#COLMBN">
        <rdf:type rdf:resource="http://www.sisostds.org/ontologies/C2SIM#EthnicGroupCode"/>
        <rdfs:comment>Colombian: The ethnic group of Colombian people.</rdfs:comment>
    </owl:NamedIndividual>
    


    <!-- http://www.sisostds.org/ontologies/C2SIM#COM -->

    <owl:NamedIndividual rdf:about="http://www.sisostds.org/ontologies/C2SIM#COM">
        <rdf:type rdf:resource="http://www.sisostds.org/ontologies/C2SIM#CountryCode"/>
        <rdfs:comment>Comoros: </rdfs:comment>
    </owl:NamedIndividual>
    


    <!-- http://www.sisostds.org/ontologies/C2SIM#COMORA -->

    <owl:NamedIndividual rdf:about="http://www.sisostds.org/ontologies/C2SIM#COMORA">
        <rdf:type rdf:resource="http://www.sisostds.org/ontologies/C2SIM#EthnicGroupCode"/>
        <rdfs:comment>Comoran: The ethnic group of Comoran people.</rdfs:comment>
    </owl:NamedIndividual>
    


    <!-- http://www.sisostds.org/ontologies/C2SIM#CORNSH -->

    <owl:NamedIndividual rdf:about="http://www.sisostds.org/ontologies/C2SIM#CORNSH">
        <rdf:type rdf:resource="http://www.sisostds.org/ontologies/C2SIM#EthnicGroupCode"/>
        <rdfs:comment>Cornish: The ethnic group of Cornish people.</rdfs:comment>
    </owl:NamedIndividual>
    


    <!-- http://www.sisostds.org/ontologies/C2SIM#CORSCN -->

    <owl:NamedIndividual rdf:about="http://www.sisostds.org/ontologies/C2SIM#CORSCN">
        <rdf:type rdf:resource="http://www.sisostds.org/ontologies/C2SIM#EthnicGroupCode"/>
        <rdfs:comment>Corsican: The ethnic group of Corsican people.</rdfs:comment>
    </owl:NamedIndividual>
    


    <!-- http://www.sisostds.org/ontologies/C2SIM#COSTRN -->

    <owl:NamedIndividual rdf:about="http://www.sisostds.org/ontologies/C2SIM#COSTRN">
        <rdf:type rdf:resource="http://www.sisostds.org/ontologies/C2SIM#EthnicGroupCode"/>
        <rdfs:comment>Costa Rican: The ethnic group of Costa Rican people.</rdfs:comment>
    </owl:NamedIndividual>
    


    <!-- http://www.sisostds.org/ontologies/C2SIM#COTIER -->

    <owl:NamedIndividual rdf:about="http://www.sisostds.org/ontologies/C2SIM#COTIER">
        <rdf:type rdf:resource="http://www.sisostds.org/ontologies/C2SIM#EthnicGroupCode"/>
        <rdfs:comment>Cotiers: The ethnic group of Cotiers people.</rdfs:comment>
    </owl:NamedIndividual>
    


    <!-- http://www.sisostds.org/ontologies/C2SIM#CPTCHR -->

    <owl:NamedIndividual rdf:about="http://www.sisostds.org/ontologies/C2SIM#CPTCHR">
        <rdf:type rdf:resource="http://www.sisostds.org/ontologies/C2SIM#ReligionCode"/>
        <rdfs:comment>Coptic Christian: One who adheres to or identifies with the Coptic Christian doctrine.</rdfs:comment>
    </owl:NamedIndividual>
    


    <!-- http://www.sisostds.org/ontologies/C2SIM#CPV -->

    <owl:NamedIndividual rdf:about="http://www.sisostds.org/ontologies/C2SIM#CPV">
        <rdf:type rdf:resource="http://www.sisostds.org/ontologies/C2SIM#CountryCode"/>
        <rdfs:comment>Cape Verde: </rdfs:comment>
    </owl:NamedIndividual>
    


    <!-- http://www.sisostds.org/ontologies/C2SIM#CRELLA -->

    <owl:NamedIndividual rdf:about="http://www.sisostds.org/ontologies/C2SIM#CRELLA">
        <rdf:type rdf:resource="http://www.sisostds.org/ontologies/C2SIM#EthnicGroupCode"/>
        <rdfs:comment>Creole (Latin America): The ethnic group of Creole (Latin America) people.</rdfs:comment>
    </owl:NamedIndividual>
    


    <!-- http://www.sisostds.org/ontologies/C2SIM#CRELUS -->

    <owl:NamedIndividual rdf:about="http://www.sisostds.org/ontologies/C2SIM#CRELUS">
        <rdf:type rdf:resource="http://www.sisostds.org/ontologies/C2SIM#EthnicGroupCode"/>
        <rdfs:comment>Creole (US): The ethnic group of Creole (US) people.</rdfs:comment>
    </owl:NamedIndividual>
    


    <!-- http://www.sisostds.org/ontologies/C2SIM#CREOLE -->

    <owl:NamedIndividual rdf:about="http://www.sisostds.org/ontologies/C2SIM#CREOLE">
        <rdf:type rdf:resource="http://www.sisostds.org/ontologies/C2SIM#EthnicGroupCode"/>
        <rdfs:comment>Creole: The ethnic group of Creole people.</rdfs:comment>
    </owl:NamedIndividual>
    


    <!-- http://www.sisostds.org/ontologies/C2SIM#CREOLM -->

    <owl:NamedIndividual rdf:about="http://www.sisostds.org/ontologies/C2SIM#CREOLM">
        <rdf:type rdf:resource="http://www.sisostds.org/ontologies/C2SIM#EthnicGroupCode"/>
        <rdfs:comment>Creole (Mulatto): The ethnic group of Creole (Mulatto) people.</rdfs:comment>
    </owl:NamedIndividual>
    


    <!-- http://www.sisostds.org/ontologies/C2SIM#CRI -->

    <owl:NamedIndividual rdf:about="http://www.sisostds.org/ontologies/C2SIM#CRI">
        <rdf:type rdf:resource="http://www.sisostds.org/ontologies/C2SIM#CountryCode"/>
        <rdfs:comment>Costa Rica: </rdfs:comment>
    </owl:NamedIndividual>
    


    <!-- http://www.sisostds.org/ontologies/C2SIM#CRIMIN -->

    <owl:NamedIndividual rdf:about="http://www.sisostds.org/ontologies/C2SIM#CRIMIN">
        <rdf:type rdf:resource="http://www.sisostds.org/ontologies/C2SIM#OrganizationTypeCode"/>
        <rdfs:comment>Criminal: A GROUP-ORGANISATION-TYPE that comprises persons who attempt to profit by violating the law.</rdfs:comment>
    </owl:NamedIndividual>
    


    <!-- http://www.sisostds.org/ontologies/C2SIM#CROATN -->

    <owl:NamedIndividual rdf:about="http://www.sisostds.org/ontologies/C2SIM#CROATN">
        <rdf:type rdf:resource="http://www.sisostds.org/ontologies/C2SIM#EthnicGroupCode"/>
        <rdfs:comment>Croat/Croatian: The ethnic group of Croat/Croatian people.</rdfs:comment>
    </owl:NamedIndividual>
    


    <!-- http://www.sisostds.org/ontologies/C2SIM#CSHH -->

    <owl:NamedIndividual rdf:about="http://www.sisostds.org/ontologies/C2SIM#CSHH">
        <rdf:type rdf:resource="http://www.sisostds.org/ontologies/C2SIM#CountryCode"/>
        <rdfs:comment>Czech and Slovak Federative Republic (former): (1993)</rdfs:comment>
    </owl:NamedIndividual>
    


    <!-- http://www.sisostds.org/ontologies/C2SIM#CSXX -->

    <owl:NamedIndividual rdf:about="http://www.sisostds.org/ontologies/C2SIM#CSXX">
        <rdf:type rdf:resource="http://www.sisostds.org/ontologies/C2SIM#CountryCode"/>
        <rdfs:comment>Serbia and Montenegro (former): </rdfs:comment>
    </owl:NamedIndividual>
    


    <!-- http://www.sisostds.org/ontologies/C2SIM#CUB -->

    <owl:NamedIndividual rdf:about="http://www.sisostds.org/ontologies/C2SIM#CUB">
        <rdf:type rdf:resource="http://www.sisostds.org/ontologies/C2SIM#CountryCode"/>
        <rdfs:comment>Cuba: </rdfs:comment>
    </owl:NamedIndividual>
    


    <!-- http://www.sisostds.org/ontologies/C2SIM#CXR -->

    <owl:NamedIndividual rdf:about="http://www.sisostds.org/ontologies/C2SIM#CXR">
        <rdf:type rdf:resource="http://www.sisostds.org/ontologies/C2SIM#CountryCode"/>
        <rdfs:comment>Christmas Island: </rdfs:comment>
    </owl:NamedIndividual>
    


    <!-- http://www.sisostds.org/ontologies/C2SIM#CYM -->

    <owl:NamedIndividual rdf:about="http://www.sisostds.org/ontologies/C2SIM#CYM">
        <rdf:type rdf:resource="http://www.sisostds.org/ontologies/C2SIM#CountryCode"/>
        <rdfs:comment>Cayman Islands: </rdfs:comment>
    </owl:NamedIndividual>
    


    <!-- http://www.sisostds.org/ontologies/C2SIM#CYP -->

    <owl:NamedIndividual rdf:about="http://www.sisostds.org/ontologies/C2SIM#CYP">
        <rdf:type rdf:resource="http://www.sisostds.org/ontologies/C2SIM#CountryCode"/>
        <rdfs:comment>Cyprus: </rdfs:comment>
    </owl:NamedIndividual>
    


    <!-- http://www.sisostds.org/ontologies/C2SIM#CYRNFD -->

    <owl:NamedIndividual rdf:about="http://www.sisostds.org/ontologies/C2SIM#CYRNFD">
        <rdf:type rdf:resource="http://www.sisostds.org/ontologies/C2SIM#EthnicGroupCode"/>
        <rdfs:comment>Cypriot not further defined: The not further defined ethnic groups of Cypriot people.</rdfs:comment>
    </owl:NamedIndividual>
    


    <!-- http://www.sisostds.org/ontologies/C2SIM#CZE -->

    <owl:NamedIndividual rdf:about="http://www.sisostds.org/ontologies/C2SIM#CZE">
        <rdf:type rdf:resource="http://www.sisostds.org/ontologies/C2SIM#CountryCode"/>
        <rdfs:comment>Czech Republic: </rdfs:comment>
    </owl:NamedIndividual>
    


    <!-- http://www.sisostds.org/ontologies/C2SIM#CZECH -->

    <owl:NamedIndividual rdf:about="http://www.sisostds.org/ontologies/C2SIM#CZECH">
        <rdf:type rdf:resource="http://www.sisostds.org/ontologies/C2SIM#EthnicGroupCode"/>
        <rdfs:comment>Czech: The ethnic group of Czech people.</rdfs:comment>
    </owl:NamedIndividual>
    


    <!-- http://www.sisostds.org/ontologies/C2SIM#Confidential -->

    <owl:NamedIndividual rdf:about="http://www.sisostds.org/ontologies/C2SIM#Confidential">
        <rdf:type rdf:resource="http://www.sisostds.org/ontologies/C2SIM#SecurityClassificationCode"/>
    </owl:NamedIndividual>
    


    <!-- http://www.sisostds.org/ontologies/C2SIM#Confirm -->

    <owl:NamedIndividual rdf:about="http://www.sisostds.org/ontologies/C2SIM#Confirm">
        <rdf:type rdf:resource="http://www.sisostds.org/ontologies/C2SIM#CommunicativeActTypeCode"/>
    </owl:NamedIndividual>
    


    <!-- http://www.sisostds.org/ontologies/C2SIM#CurrentSimulationRate -->

    <owl:NamedIndividual rdf:about="http://www.sisostds.org/ontologies/C2SIM#CurrentSimulationRate"/>
    


    <!-- http://www.sisostds.org/ontologies/C2SIM#DAGHES -->

    <owl:NamedIndividual rdf:about="http://www.sisostds.org/ontologies/C2SIM#DAGHES">
        <rdf:type rdf:resource="http://www.sisostds.org/ontologies/C2SIM#EthnicGroupCode"/>
        <rdfs:comment>Daghestanis: The ethnic group of Daghestanis people.</rdfs:comment>
    </owl:NamedIndividual>
    


    <!-- http://www.sisostds.org/ontologies/C2SIM#DALMTN -->

    <owl:NamedIndividual rdf:about="http://www.sisostds.org/ontologies/C2SIM#DALMTN">
        <rdf:type rdf:resource="http://www.sisostds.org/ontologies/C2SIM#EthnicGroupCode"/>
        <rdfs:comment>Dalmatian: The ethnic group of Dalmatian people.</rdfs:comment>
    </owl:NamedIndividual>
    


    <!-- http://www.sisostds.org/ontologies/C2SIM#DANISH -->

    <owl:NamedIndividual rdf:about="http://www.sisostds.org/ontologies/C2SIM#DANISH">
        <rdf:type rdf:resource="http://www.sisostds.org/ontologies/C2SIM#EthnicGroupCode"/>
        <rdfs:comment>Danish: The ethnic group of Danish people.</rdfs:comment>
    </owl:NamedIndividual>
    


    <!-- http://www.sisostds.org/ontologies/C2SIM#DDDE -->

    <owl:NamedIndividual rdf:about="http://www.sisostds.org/ontologies/C2SIM#DDDE">
        <rdf:type rdf:resource="http://www.sisostds.org/ontologies/C2SIM#CountryCode"/>
        <rdfs:comment>German Democratic Republic (former): GDR (1990)</rdfs:comment>
    </owl:NamedIndividual>
    


    <!-- http://www.sisostds.org/ontologies/C2SIM#DEU -->

    <owl:NamedIndividual rdf:about="http://www.sisostds.org/ontologies/C2SIM#DEU">
        <rdf:type rdf:resource="http://www.sisostds.org/ontologies/C2SIM#CountryCode"/>
        <rdfs:comment>Germany: </rdfs:comment>
    </owl:NamedIndividual>
    


    <!-- http://www.sisostds.org/ontologies/C2SIM#DIOLA -->

    <owl:NamedIndividual rdf:about="http://www.sisostds.org/ontologies/C2SIM#DIOLA">
        <rdf:type rdf:resource="http://www.sisostds.org/ontologies/C2SIM#EthnicGroupCode"/>
        <rdfs:comment>Diola: The ethnic group of Diola people.</rdfs:comment>
    </owl:NamedIndividual>
    


    <!-- http://www.sisostds.org/ontologies/C2SIM#DJERMA -->

    <owl:NamedIndividual rdf:about="http://www.sisostds.org/ontologies/C2SIM#DJERMA">
        <rdf:type rdf:resource="http://www.sisostds.org/ontologies/C2SIM#EthnicGroupCode"/>
        <rdfs:comment>Djerma: The ethnic group of Djerma people.</rdfs:comment>
    </owl:NamedIndividual>
    


    <!-- http://www.sisostds.org/ontologies/C2SIM#DJI -->

    <owl:NamedIndividual rdf:about="http://www.sisostds.org/ontologies/C2SIM#DJI">
        <rdf:type rdf:resource="http://www.sisostds.org/ontologies/C2SIM#CountryCode"/>
        <rdfs:comment>Djibouti: </rdfs:comment>
    </owl:NamedIndividual>
    


    <!-- http://www.sisostds.org/ontologies/C2SIM#DMA -->

    <owl:NamedIndividual rdf:about="http://www.sisostds.org/ontologies/C2SIM#DMA">
        <rdf:type rdf:resource="http://www.sisostds.org/ontologies/C2SIM#CountryCode"/>
        <rdfs:comment>Dominica: </rdfs:comment>
    </owl:NamedIndividual>
    


    <!-- http://www.sisostds.org/ontologies/C2SIM#DNK -->

    <owl:NamedIndividual rdf:about="http://www.sisostds.org/ontologies/C2SIM#DNK">
        <rdf:type rdf:resource="http://www.sisostds.org/ontologies/C2SIM#CountryCode"/>
        <rdfs:comment>Denmark: </rdfs:comment>
    </owl:NamedIndividual>
    


    <!-- http://www.sisostds.org/ontologies/C2SIM#DOM -->

    <owl:NamedIndividual rdf:about="http://www.sisostds.org/ontologies/C2SIM#DOM">
        <rdf:type rdf:resource="http://www.sisostds.org/ontologies/C2SIM#CountryCode"/>
        <rdfs:comment>Dominican Republic: </rdfs:comment>
    </owl:NamedIndividual>
    


    <!-- http://www.sisostds.org/ontologies/C2SIM#DRAVID -->

    <owl:NamedIndividual rdf:about="http://www.sisostds.org/ontologies/C2SIM#DRAVID">
        <rdf:type rdf:resource="http://www.sisostds.org/ontologies/C2SIM#EthnicGroupCode"/>
        <rdfs:comment>Dravidian: The ethnic group of Dravidian people.</rdfs:comment>
    </owl:NamedIndividual>
    


    <!-- http://www.sisostds.org/ontologies/C2SIM#DRUZE -->

    <owl:NamedIndividual rdf:about="http://www.sisostds.org/ontologies/C2SIM#DRUZE">
        <rdf:type rdf:resource="http://www.sisostds.org/ontologies/C2SIM#ReligionCode"/>
        <rdfs:comment>Druze: One who adheres to or identifies with the Druze doctrine.</rdfs:comment>
    </owl:NamedIndividual>
    


    <!-- http://www.sisostds.org/ontologies/C2SIM#DSPLPR -->

    <owl:NamedIndividual rdf:about="http://www.sisostds.org/ontologies/C2SIM#DSPLPR">
        <rdf:type rdf:resource="http://www.sisostds.org/ontologies/C2SIM#OrganizationTypeCode"/>
        <rdfs:comment>Displaced person: A GROUP-ORGANISATION-TYPE that comprises persons removed from their home country by military or political pressure.</rdfs:comment>
    </owl:NamedIndividual>
    


    <!-- http://www.sisostds.org/ontologies/C2SIM#DUTCH -->

    <owl:NamedIndividual rdf:about="http://www.sisostds.org/ontologies/C2SIM#DUTCH">
        <rdf:type rdf:resource="http://www.sisostds.org/ontologies/C2SIM#EthnicGroupCode"/>
        <rdfs:comment>Dutch/Netherlands: The ethnic group of Dutch/Netherlands people.</rdfs:comment>
    </owl:NamedIndividual>
    


    <!-- http://www.sisostds.org/ontologies/C2SIM#DZA -->

    <owl:NamedIndividual rdf:about="http://www.sisostds.org/ontologies/C2SIM#DZA">
        <rdf:type rdf:resource="http://www.sisostds.org/ontologies/C2SIM#CountryCode"/>
        <rdfs:comment>Algeria: </rdfs:comment>
    </owl:NamedIndividual>
    


    <!-- http://www.sisostds.org/ontologies/C2SIM#EASISL -->

    <owl:NamedIndividual rdf:about="http://www.sisostds.org/ontologies/C2SIM#EASISL">
        <rdf:type rdf:resource="http://www.sisostds.org/ontologies/C2SIM#EthnicGroupCode"/>
        <rdfs:comment>Easter Islander: The ethnic group of Easter Islander people.</rdfs:comment>
    </owl:NamedIndividual>
    


    <!-- http://www.sisostds.org/ontologies/C2SIM#ECU -->

    <owl:NamedIndividual rdf:about="http://www.sisostds.org/ontologies/C2SIM#ECU">
        <rdf:type rdf:resource="http://www.sisostds.org/ontologies/C2SIM#CountryCode"/>
        <rdfs:comment>Ecuador: </rdfs:comment>
    </owl:NamedIndividual>
    


    <!-- http://www.sisostds.org/ontologies/C2SIM#ECUDRN -->

    <owl:NamedIndividual rdf:about="http://www.sisostds.org/ontologies/C2SIM#ECUDRN">
        <rdf:type rdf:resource="http://www.sisostds.org/ontologies/C2SIM#EthnicGroupCode"/>
        <rdfs:comment>Ecuadorian: The ethnic group of Ecuadorian people.</rdfs:comment>
    </owl:NamedIndividual>
    


    <!-- http://www.sisostds.org/ontologies/C2SIM#EDUCAL -->

    <owl:NamedIndividual rdf:about="http://www.sisostds.org/ontologies/C2SIM#EDUCAL">
        <rdf:type rdf:resource="http://www.sisostds.org/ontologies/C2SIM#OrganizationTypeCode"/>
        <rdfs:comment>Educational: A GROUP-ORGANISATION-TYPE that provides labour and material for the educational process.</rdfs:comment>
    </owl:NamedIndividual>
    


    <!-- http://www.sisostds.org/ontologies/C2SIM#EGY -->

    <owl:NamedIndividual rdf:about="http://www.sisostds.org/ontologies/C2SIM#EGY">
        <rdf:type rdf:resource="http://www.sisostds.org/ontologies/C2SIM#CountryCode"/>
        <rdfs:comment>Egypt: </rdfs:comment>
    </owl:NamedIndividual>
    


    <!-- http://www.sisostds.org/ontologies/C2SIM#EGYPTN -->

    <owl:NamedIndividual rdf:about="http://www.sisostds.org/ontologies/C2SIM#EGYPTN">
        <rdf:type rdf:resource="http://www.sisostds.org/ontologies/C2SIM#EthnicGroupCode"/>
        <rdfs:comment>Egyptian: The ethnic group of Egyptian people.</rdfs:comment>
    </owl:NamedIndividual>
    


    <!-- http://www.sisostds.org/ontologies/C2SIM#EKLNIE -->

    <owl:NamedIndividual rdf:about="http://www.sisostds.org/ontologies/C2SIM#EKLNIE">
        <rdf:type rdf:resource="http://www.sisostds.org/ontologies/C2SIM#ReligionCode"/>
        <rdfs:comment>Ekalesia Nieue: One who adheres to or identifies with the Ekalesia Nieue doctrine.</rdfs:comment>
    </owl:NamedIndividual>
    


    <!-- http://www.sisostds.org/ontologies/C2SIM#ENDEND -->

    <owl:NamedIndividual rdf:about="http://www.sisostds.org/ontologies/C2SIM#ENDEND">
        <rdf:type rdf:resource="http://www.sisostds.org/ontologies/C2SIM#ActionTemporalAssociationCode"/>
        <rdfs:comment>Ends after end of: The subject ACTION ends after the object ACTION ends.</rdfs:comment>
    </owl:NamedIndividual>
    


    <!-- http://www.sisostds.org/ontologies/C2SIM#ENDENE -->

    <owl:NamedIndividual rdf:about="http://www.sisostds.org/ontologies/C2SIM#ENDENE">
        <rdf:type rdf:resource="http://www.sisostds.org/ontologies/C2SIM#ActionTemporalAssociationCode"/>
        <rdfs:comment>Ends no earlier than after end of: The subject ACTION ends no earlier than the end of the object ACTION augmented by a fixed duration.</rdfs:comment>
    </owl:NamedIndividual>
    


    <!-- http://www.sisostds.org/ontologies/C2SIM#ENDENL -->

    <owl:NamedIndividual rdf:about="http://www.sisostds.org/ontologies/C2SIM#ENDENL">
        <rdf:type rdf:resource="http://www.sisostds.org/ontologies/C2SIM#ActionTemporalAssociationCode"/>
        <rdfs:comment>Ends no later than after end of: The subject ACTION ends no later than the end of object ACTION augmented by a fixed duration.</rdfs:comment>
    </owl:NamedIndividual>
    


    <!-- http://www.sisostds.org/ontologies/C2SIM#ENDSNE -->

    <owl:NamedIndividual rdf:about="http://www.sisostds.org/ontologies/C2SIM#ENDSNE">
        <rdf:type rdf:resource="http://www.sisostds.org/ontologies/C2SIM#ActionTemporalAssociationCode"/>
        <rdfs:comment>Ends no earlier than after start of: The subject ACTION ends no earlier than the start of the object ACTION augmented by a fixed duration.</rdfs:comment>
    </owl:NamedIndividual>
    


    <!-- http://www.sisostds.org/ontologies/C2SIM#ENDSNL -->

    <owl:NamedIndividual rdf:about="http://www.sisostds.org/ontologies/C2SIM#ENDSNL">
        <rdf:type rdf:resource="http://www.sisostds.org/ontologies/C2SIM#ActionTemporalAssociationCode"/>
        <rdfs:comment>Ends no later than after start of: The subject ACTION ends no later than the start of object ACTION augmented by a fixed duration.</rdfs:comment>
    </owl:NamedIndividual>
    


    <!-- http://www.sisostds.org/ontologies/C2SIM#ENDSTR -->

    <owl:NamedIndividual rdf:about="http://www.sisostds.org/ontologies/C2SIM#ENDSTR">
        <rdf:type rdf:resource="http://www.sisostds.org/ontologies/C2SIM#ActionTemporalAssociationCode"/>
        <rdfs:comment>Ends after start of: The subject ACTION ends after the object ACTION starts.</rdfs:comment>
    </owl:NamedIndividual>
    


    <!-- http://www.sisostds.org/ontologies/C2SIM#ENGLSH -->

    <owl:NamedIndividual rdf:about="http://www.sisostds.org/ontologies/C2SIM#ENGLSH">
        <rdf:type rdf:resource="http://www.sisostds.org/ontologies/C2SIM#EthnicGroupCode"/>
        <rdfs:comment>English: The ethnic group of English people.</rdfs:comment>
    </owl:NamedIndividual>
    


    <!-- http://www.sisostds.org/ontologies/C2SIM#EPSCPL -->

    <owl:NamedIndividual rdf:about="http://www.sisostds.org/ontologies/C2SIM#EPSCPL">
        <rdf:type rdf:resource="http://www.sisostds.org/ontologies/C2SIM#ReligionCode"/>
        <rdfs:comment>Episcopalian: One who adheres to or identifies with the Episcopalian doctrine.</rdfs:comment>
    </owl:NamedIndividual>
    


    <!-- http://www.sisostds.org/ontologies/C2SIM#EQUATO -->

    <owl:NamedIndividual rdf:about="http://www.sisostds.org/ontologies/C2SIM#EQUATO">
        <rdf:type rdf:resource="http://www.sisostds.org/ontologies/C2SIM#EthnicGroupCode"/>
        <rdfs:comment>Equatorial Bantu: The ethnic group of Equatorial Bantu people.</rdfs:comment>
    </owl:NamedIndividual>
    


    <!-- http://www.sisostds.org/ontologies/C2SIM#ERI -->

    <owl:NamedIndividual rdf:about="http://www.sisostds.org/ontologies/C2SIM#ERI">
        <rdf:type rdf:resource="http://www.sisostds.org/ontologies/C2SIM#CountryCode"/>
        <rdfs:comment>Eritrea: </rdfs:comment>
    </owl:NamedIndividual>
    


    <!-- http://www.sisostds.org/ontologies/C2SIM#ERIRIA -->

    <owl:NamedIndividual rdf:about="http://www.sisostds.org/ontologies/C2SIM#ERIRIA">
        <rdf:type rdf:resource="http://www.sisostds.org/ontologies/C2SIM#EthnicGroupCode"/>
        <rdfs:comment>Eririan: The ethnic group of Eririan people.</rdfs:comment>
    </owl:NamedIndividual>
    


    <!-- http://www.sisostds.org/ontologies/C2SIM#ESH -->

    <owl:NamedIndividual rdf:about="http://www.sisostds.org/ontologies/C2SIM#ESH">
        <rdf:type rdf:resource="http://www.sisostds.org/ontologies/C2SIM#CountryCode"/>
        <rdfs:comment>Western Sahara: </rdfs:comment>
    </owl:NamedIndividual>
    


    <!-- http://www.sisostds.org/ontologies/C2SIM#ESP -->

    <owl:NamedIndividual rdf:about="http://www.sisostds.org/ontologies/C2SIM#ESP">
        <rdf:type rdf:resource="http://www.sisostds.org/ontologies/C2SIM#CountryCode"/>
        <rdfs:comment>Spain: </rdfs:comment>
    </owl:NamedIndividual>
    


    <!-- http://www.sisostds.org/ontologies/C2SIM#EST -->

    <owl:NamedIndividual rdf:about="http://www.sisostds.org/ontologies/C2SIM#EST">
        <rdf:type rdf:resource="http://www.sisostds.org/ontologies/C2SIM#CountryCode"/>
        <rdfs:comment>Estonia: </rdfs:comment>
    </owl:NamedIndividual>
    


    <!-- http://www.sisostds.org/ontologies/C2SIM#ESTONN -->

    <owl:NamedIndividual rdf:about="http://www.sisostds.org/ontologies/C2SIM#ESTONN">
        <rdf:type rdf:resource="http://www.sisostds.org/ontologies/C2SIM#EthnicGroupCode"/>
        <rdfs:comment>Estonian: The ethnic group of Estonian people.</rdfs:comment>
    </owl:NamedIndividual>
    


    <!-- http://www.sisostds.org/ontologies/C2SIM#ESTORT -->

    <owl:NamedIndividual rdf:about="http://www.sisostds.org/ontologies/C2SIM#ESTORT">
        <rdf:type rdf:resource="http://www.sisostds.org/ontologies/C2SIM#ReligionCode"/>
        <rdfs:comment>Eastern Orthodox: One who adheres to or identifies with the Eastern Orthodox doctrine.</rdfs:comment>
    </owl:NamedIndividual>
    


    <!-- http://www.sisostds.org/ontologies/C2SIM#ETH -->

    <owl:NamedIndividual rdf:about="http://www.sisostds.org/ontologies/C2SIM#ETH">
        <rdf:type rdf:resource="http://www.sisostds.org/ontologies/C2SIM#CountryCode"/>
        <rdfs:comment>Ethiopia: </rdfs:comment>
    </owl:NamedIndividual>
    


    <!-- http://www.sisostds.org/ontologies/C2SIM#ETHNCN -->

    <owl:NamedIndividual rdf:about="http://www.sisostds.org/ontologies/C2SIM#ETHNCN">
        <rdf:type rdf:resource="http://www.sisostds.org/ontologies/C2SIM#EthnicGroupCode"/>
        <rdfs:comment>Ethnic Nepalese: The ethnic group of Ethnic Nepalese people.</rdfs:comment>
    </owl:NamedIndividual>
    


    <!-- http://www.sisostds.org/ontologies/C2SIM#ETHNCT -->

    <owl:NamedIndividual rdf:about="http://www.sisostds.org/ontologies/C2SIM#ETHNCT">
        <rdf:type rdf:resource="http://www.sisostds.org/ontologies/C2SIM#EthnicGroupCode"/>
        <rdfs:comment>Ethnic Tigrays: The ethnic group of Ethnic Tigrays people.</rdfs:comment>
    </owl:NamedIndividual>
    


    <!-- http://www.sisostds.org/ontologies/C2SIM#ETHORT -->

    <owl:NamedIndividual rdf:about="http://www.sisostds.org/ontologies/C2SIM#ETHORT">
        <rdf:type rdf:resource="http://www.sisostds.org/ontologies/C2SIM#ReligionCode"/>
        <rdfs:comment>Ethiopian Orthodox: One who adheres to or identifies with the Ethiopian Orthodox doctrine.</rdfs:comment>
    </owl:NamedIndividual>
    


    <!-- http://www.sisostds.org/ontologies/C2SIM#EURNEC -->

    <owl:NamedIndividual rdf:about="http://www.sisostds.org/ontologies/C2SIM#EURNEC">
        <rdf:type rdf:resource="http://www.sisostds.org/ontologies/C2SIM#EthnicGroupCode"/>
        <rdfs:comment>European not elsewhere classified: The not elsewhere classified ethnic groups of European people.</rdfs:comment>
    </owl:NamedIndividual>
    


    <!-- http://www.sisostds.org/ontologies/C2SIM#EURNFD -->

    <owl:NamedIndividual rdf:about="http://www.sisostds.org/ontologies/C2SIM#EURNFD">
        <rdf:type rdf:resource="http://www.sisostds.org/ontologies/C2SIM#EthnicGroupCode"/>
        <rdfs:comment>European not further defined: The not further defined ethnic groups of European people.</rdfs:comment>
    </owl:NamedIndividual>
    


    <!-- http://www.sisostds.org/ontologies/C2SIM#EUROAF -->

    <owl:NamedIndividual rdf:about="http://www.sisostds.org/ontologies/C2SIM#EUROAF">
        <rdf:type rdf:resource="http://www.sisostds.org/ontologies/C2SIM#EthnicGroupCode"/>
        <rdfs:comment>Euro-Africans: The ethnic group of Euro-Africans people.</rdfs:comment>
    </owl:NamedIndividual>
    


    <!-- http://www.sisostds.org/ontologies/C2SIM#EUROIN -->

    <owl:NamedIndividual rdf:about="http://www.sisostds.org/ontologies/C2SIM#EUROIN">
        <rdf:type rdf:resource="http://www.sisostds.org/ontologies/C2SIM#EthnicGroupCode"/>
        <rdfs:comment>Euronesians: The ethnic group of Euronesians people.</rdfs:comment>
    </owl:NamedIndividual>
    


    <!-- http://www.sisostds.org/ontologies/C2SIM#EUROPE -->

    <owl:NamedIndividual rdf:about="http://www.sisostds.org/ontologies/C2SIM#EUROPE">
        <rdf:type rdf:resource="http://www.sisostds.org/ontologies/C2SIM#EthnicGroupCode"/>
        <rdfs:comment>European-Indian: The ethnic group of European-Indian people.</rdfs:comment>
    </owl:NamedIndividual>
    


    <!-- http://www.sisostds.org/ontologies/C2SIM#EVNALL -->

    <owl:NamedIndividual rdf:about="http://www.sisostds.org/ontologies/C2SIM#EVNALL">
        <rdf:type rdf:resource="http://www.sisostds.org/ontologies/C2SIM#ReligionCode"/>
        <rdfs:comment>Evangelical Alliance: One who adheres to or identifies with the Evangelical Alliance doctrine.</rdfs:comment>
    </owl:NamedIndividual>
    


    <!-- http://www.sisostds.org/ontologies/C2SIM#EVNGCH -->

    <owl:NamedIndividual rdf:about="http://www.sisostds.org/ontologies/C2SIM#EVNGCH">
        <rdf:type rdf:resource="http://www.sisostds.org/ontologies/C2SIM#ReligionCode"/>
        <rdfs:comment>Evangelist Church: One who adheres to or identifies with the Evangelist Church doctrine.</rdfs:comment>
    </owl:NamedIndividual>
    


    <!-- http://www.sisostds.org/ontologies/C2SIM#EVNLUT -->

    <owl:NamedIndividual rdf:about="http://www.sisostds.org/ontologies/C2SIM#EVNLUT">
        <rdf:type rdf:resource="http://www.sisostds.org/ontologies/C2SIM#ReligionCode"/>
        <rdfs:comment>Evangelical Lutheran: One who adheres to or identifies with the Evangelical Lutheran doctrine.</rdfs:comment>
    </owl:NamedIndividual>
    


    <!-- http://www.sisostds.org/ontologies/C2SIM#EWE -->

    <owl:NamedIndividual rdf:about="http://www.sisostds.org/ontologies/C2SIM#EWE">
        <rdf:type rdf:resource="http://www.sisostds.org/ontologies/C2SIM#EthnicGroupCode"/>
        <rdfs:comment>Ewe: The ethnic group of Ewe people.</rdfs:comment>
    </owl:NamedIndividual>
    


    <!-- http://www.sisostds.org/ontologies/C2SIM#EnemySide -->

    <owl:NamedIndividual rdf:about="http://www.sisostds.org/ontologies/C2SIM#EnemySide"/>
    


    <!-- http://www.sisostds.org/ontologies/C2SIM#FAROES -->

    <owl:NamedIndividual rdf:about="http://www.sisostds.org/ontologies/C2SIM#FAROES">
        <rdf:type rdf:resource="http://www.sisostds.org/ontologies/C2SIM#EthnicGroupCode"/>
        <rdfs:comment>Faroese: The ethnic group of Faroese people.</rdfs:comment>
    </owl:NamedIndividual>
    


    <!-- http://www.sisostds.org/ontologies/C2SIM#FIJIAN -->

    <owl:NamedIndividual rdf:about="http://www.sisostds.org/ontologies/C2SIM#FIJIAN">
        <rdf:type rdf:resource="http://www.sisostds.org/ontologies/C2SIM#EthnicGroupCode"/>
        <rdfs:comment>Fijian (except Fiji Indian/Indo-Fijian): The ethnic group of Fijian (except Fiji Indian/Indo-Fijian) people.</rdfs:comment>
    </owl:NamedIndividual>
    


    <!-- http://www.sisostds.org/ontologies/C2SIM#FIJNIN -->

    <owl:NamedIndividual rdf:about="http://www.sisostds.org/ontologies/C2SIM#FIJNIN">
        <rdf:type rdf:resource="http://www.sisostds.org/ontologies/C2SIM#EthnicGroupCode"/>
        <rdfs:comment>Fijian Indian/Indo-Fijian: The ethnic group of Fijian Indian/Indo-Fijian people.</rdfs:comment>
    </owl:NamedIndividual>
    


    <!-- http://www.sisostds.org/ontologies/C2SIM#FILPNO -->

    <owl:NamedIndividual rdf:about="http://www.sisostds.org/ontologies/C2SIM#FILPNO">
        <rdf:type rdf:resource="http://www.sisostds.org/ontologies/C2SIM#EthnicGroupCode"/>
        <rdfs:comment>Filipino: The ethnic group of Filipino people.</rdfs:comment>
    </owl:NamedIndividual>
    


    <!-- http://www.sisostds.org/ontologies/C2SIM#FIN -->

    <owl:NamedIndividual rdf:about="http://www.sisostds.org/ontologies/C2SIM#FIN">
        <rdf:type rdf:resource="http://www.sisostds.org/ontologies/C2SIM#CountryCode"/>
        <rdfs:comment>Finland: </rdfs:comment>
    </owl:NamedIndividual>
    


    <!-- http://www.sisostds.org/ontologies/C2SIM#FINCAL -->

    <owl:NamedIndividual rdf:about="http://www.sisostds.org/ontologies/C2SIM#FINCAL">
        <rdf:type rdf:resource="http://www.sisostds.org/ontologies/C2SIM#OrganizationTypeCode"/>
        <rdfs:comment>Financial: A GROUP-ORGANISATION-TYPE that provides finance, financial advice and guidance, support for the procurement process, providing</rdfs:comment>
    </owl:NamedIndividual>
    


    <!-- http://www.sisostds.org/ontologies/C2SIM#FINNSH -->

    <owl:NamedIndividual rdf:about="http://www.sisostds.org/ontologies/C2SIM#FINNSH">
        <rdf:type rdf:resource="http://www.sisostds.org/ontologies/C2SIM#EthnicGroupCode"/>
        <rdfs:comment>Finnish: The ethnic group of Finnish people.</rdfs:comment>
    </owl:NamedIndividual>
    


    <!-- http://www.sisostds.org/ontologies/C2SIM#FJI -->

    <owl:NamedIndividual rdf:about="http://www.sisostds.org/ontologies/C2SIM#FJI">
        <rdf:type rdf:resource="http://www.sisostds.org/ontologies/C2SIM#CountryCode"/>
        <rdfs:comment>Fiji: </rdfs:comment>
    </owl:NamedIndividual>
    


    <!-- http://www.sisostds.org/ontologies/C2SIM#FLEMSH -->

    <owl:NamedIndividual rdf:about="http://www.sisostds.org/ontologies/C2SIM#FLEMSH">
        <rdf:type rdf:resource="http://www.sisostds.org/ontologies/C2SIM#EthnicGroupCode"/>
        <rdfs:comment>Flemish: The ethnic group of Flemish people.</rdfs:comment>
    </owl:NamedIndividual>
    


    <!-- http://www.sisostds.org/ontologies/C2SIM#FLK -->

    <owl:NamedIndividual rdf:about="http://www.sisostds.org/ontologies/C2SIM#FLK">
        <rdf:type rdf:resource="http://www.sisostds.org/ontologies/C2SIM#CountryCode"/>
        <rdfs:comment>Falkland Islands (Malvinas): </rdfs:comment>
    </owl:NamedIndividual>
    


    <!-- http://www.sisostds.org/ontologies/C2SIM#FLKISL -->

    <owl:NamedIndividual rdf:about="http://www.sisostds.org/ontologies/C2SIM#FLKISL">
        <rdf:type rdf:resource="http://www.sisostds.org/ontologies/C2SIM#EthnicGroupCode"/>
        <rdfs:comment>Falkland Islander/Kelper: The ethnic group of Falkland Islander/Kelper people.</rdfs:comment>
    </owl:NamedIndividual>
    


    <!-- http://www.sisostds.org/ontologies/C2SIM#FORROS -->

    <owl:NamedIndividual rdf:about="http://www.sisostds.org/ontologies/C2SIM#FORROS">
        <rdf:type rdf:resource="http://www.sisostds.org/ontologies/C2SIM#EthnicGroupCode"/>
        <rdfs:comment>Forros: The ethnic group of Forros people.</rdfs:comment>
    </owl:NamedIndividual>
    


    <!-- http://www.sisostds.org/ontologies/C2SIM#FRA -->

    <owl:NamedIndividual rdf:about="http://www.sisostds.org/ontologies/C2SIM#FRA">
        <rdf:type rdf:resource="http://www.sisostds.org/ontologies/C2SIM#CountryCode"/>
        <rdfs:comment>France: </rdfs:comment>
    </owl:NamedIndividual>
    


    <!-- http://www.sisostds.org/ontologies/C2SIM#FRANCO -->

    <owl:NamedIndividual rdf:about="http://www.sisostds.org/ontologies/C2SIM#FRANCO">
        <rdf:type rdf:resource="http://www.sisostds.org/ontologies/C2SIM#EthnicGroupCode"/>
        <rdfs:comment>Franco-Mauritian: The ethnic group of Franco-Mauritian people.</rdfs:comment>
    </owl:NamedIndividual>
    


    <!-- http://www.sisostds.org/ontologies/C2SIM#FRENCH -->

    <owl:NamedIndividual rdf:about="http://www.sisostds.org/ontologies/C2SIM#FRENCH">
        <rdf:type rdf:resource="http://www.sisostds.org/ontologies/C2SIM#EthnicGroupCode"/>
        <rdfs:comment>French: The ethnic group of French people.</rdfs:comment>
    </owl:NamedIndividual>
    


    <!-- http://www.sisostds.org/ontologies/C2SIM#FRNFGT -->

    <owl:NamedIndividual rdf:about="http://www.sisostds.org/ontologies/C2SIM#FRNFGT">
        <rdf:type rdf:resource="http://www.sisostds.org/ontologies/C2SIM#OrganizationTypeCode"/>
        <rdfs:comment>Foreign fighters: A GROUP-ORGANISATION-TYPE that consists of fighters who are not from the country in which the fighting is taking place supporting</rdfs:comment>
    </owl:NamedIndividual>
    


    <!-- http://www.sisostds.org/ontologies/C2SIM#FRO -->

    <owl:NamedIndividual rdf:about="http://www.sisostds.org/ontologies/C2SIM#FRO">
        <rdf:type rdf:resource="http://www.sisostds.org/ontologies/C2SIM#CountryCode"/>
        <rdfs:comment>Faroe Islands: </rdfs:comment>
    </owl:NamedIndividual>
    


    <!-- http://www.sisostds.org/ontologies/C2SIM#FSM -->

    <owl:NamedIndividual rdf:about="http://www.sisostds.org/ontologies/C2SIM#FSM">
        <rdf:type rdf:resource="http://www.sisostds.org/ontologies/C2SIM#CountryCode"/>
        <rdfs:comment>Micronesia Federated States of: </rdfs:comment>
    </owl:NamedIndividual>
    


    <!-- http://www.sisostds.org/ontologies/C2SIM#FULA -->

    <owl:NamedIndividual rdf:about="http://www.sisostds.org/ontologies/C2SIM#FULA">
        <rdf:type rdf:resource="http://www.sisostds.org/ontologies/C2SIM#EthnicGroupCode"/>
        <rdfs:comment>Fula: The ethnic group of Fula people.</rdfs:comment>
    </owl:NamedIndividual>
    


    <!-- http://www.sisostds.org/ontologies/C2SIM#FULANI -->

    <owl:NamedIndividual rdf:about="http://www.sisostds.org/ontologies/C2SIM#FULANI">
        <rdf:type rdf:resource="http://www.sisostds.org/ontologies/C2SIM#EthnicGroupCode"/>
        <rdfs:comment>Fulani: The ethnic group of Fulani people.</rdfs:comment>
    </owl:NamedIndividual>
    


    <!-- http://www.sisostds.org/ontologies/C2SIM#FXFR -->

    <owl:NamedIndividual rdf:about="http://www.sisostds.org/ontologies/C2SIM#FXFR">
        <rdf:type rdf:resource="http://www.sisostds.org/ontologies/C2SIM#CountryCode"/>
        <rdfs:comment>France, Metropolitan (former): </rdfs:comment>
    </owl:NamedIndividual>
    


    <!-- http://www.sisostds.org/ontologies/C2SIM#FriendlySide -->

    <owl:NamedIndividual rdf:about="http://www.sisostds.org/ontologies/C2SIM#FriendlySide"/>
    


    <!-- http://www.sisostds.org/ontologies/C2SIM#FriendlyTo -->

    <owl:NamedIndividual rdf:about="http://www.sisostds.org/ontologies/C2SIM#FriendlyTo">
        <rdf:type rdf:resource="http://www.sisostds.org/ontologies/C2SIM#AllegianceRelationshipCode"/>
    </owl:NamedIndividual>
    


    <!-- http://www.sisostds.org/ontologies/C2SIM#FullyOperational -->

    <owl:NamedIndividual rdf:about="http://www.sisostds.org/ontologies/C2SIM#FullyOperational">
        <rdf:type rdf:resource="http://www.sisostds.org/ontologies/C2SIM#OperationalStatusCode"/>
    </owl:NamedIndividual>
    


    <!-- http://www.sisostds.org/ontologies/C2SIM#GAB -->

    <owl:NamedIndividual rdf:about="http://www.sisostds.org/ontologies/C2SIM#GAB">
        <rdf:type rdf:resource="http://www.sisostds.org/ontologies/C2SIM#CountryCode"/>
        <rdfs:comment>Gabon: </rdfs:comment>
    </owl:NamedIndividual>
    


    <!-- http://www.sisostds.org/ontologies/C2SIM#GAELIC -->

    <owl:NamedIndividual rdf:about="http://www.sisostds.org/ontologies/C2SIM#GAELIC">
        <rdf:type rdf:resource="http://www.sisostds.org/ontologies/C2SIM#EthnicGroupCode"/>
        <rdfs:comment>Gaelic: The ethnic group of Gaelic people.</rdfs:comment>
    </owl:NamedIndividual>
    


    <!-- http://www.sisostds.org/ontologies/C2SIM#GAGAUZ -->

    <owl:NamedIndividual rdf:about="http://www.sisostds.org/ontologies/C2SIM#GAGAUZ">
        <rdf:type rdf:resource="http://www.sisostds.org/ontologies/C2SIM#EthnicGroupCode"/>
        <rdfs:comment>Gagauz: The ethnic group of Gagauz people.</rdfs:comment>
    </owl:NamedIndividual>
    


    <!-- http://www.sisostds.org/ontologies/C2SIM#GANG -->

    <owl:NamedIndividual rdf:about="http://www.sisostds.org/ontologies/C2SIM#GANG">
        <rdf:type rdf:resource="http://www.sisostds.org/ontologies/C2SIM#OrganizationTypeCode"/>
        <rdfs:comment>Gang: A GROUP-ORGANISATION-TYPE that comprises persons that go together or act in concert.</rdfs:comment>
    </owl:NamedIndividual>
    


    <!-- http://www.sisostds.org/ontologies/C2SIM#GARIFU -->

    <owl:NamedIndividual rdf:about="http://www.sisostds.org/ontologies/C2SIM#GARIFU">
        <rdf:type rdf:resource="http://www.sisostds.org/ontologies/C2SIM#EthnicGroupCode"/>
        <rdfs:comment>Garifuna: The ethnic group of Garifuna people.</rdfs:comment>
    </owl:NamedIndividual>
    


    <!-- http://www.sisostds.org/ontologies/C2SIM#GBR -->

    <owl:NamedIndividual rdf:about="http://www.sisostds.org/ontologies/C2SIM#GBR">
        <rdf:type rdf:resource="http://www.sisostds.org/ontologies/C2SIM#CountryCode"/>
        <rdfs:comment>United Kingdom: </rdfs:comment>
    </owl:NamedIndividual>
    


    <!-- http://www.sisostds.org/ontologies/C2SIM#GEO -->

    <owl:NamedIndividual rdf:about="http://www.sisostds.org/ontologies/C2SIM#GEO">
        <rdf:type rdf:resource="http://www.sisostds.org/ontologies/C2SIM#CountryCode"/>
        <rdfs:comment>Georgia: </rdfs:comment>
    </owl:NamedIndividual>
    


    <!-- http://www.sisostds.org/ontologies/C2SIM#GEOORT -->

    <owl:NamedIndividual rdf:about="http://www.sisostds.org/ontologies/C2SIM#GEOORT">
        <rdf:type rdf:resource="http://www.sisostds.org/ontologies/C2SIM#ReligionCode"/>
        <rdfs:comment>Georgian Orthodox: One who adheres to or identifies with the Georgian Orthodox doctrine.</rdfs:comment>
    </owl:NamedIndividual>
    


    <!-- http://www.sisostds.org/ontologies/C2SIM#GEORGN -->

    <owl:NamedIndividual rdf:about="http://www.sisostds.org/ontologies/C2SIM#GEORGN">
        <rdf:type rdf:resource="http://www.sisostds.org/ontologies/C2SIM#EthnicGroupCode"/>
        <rdfs:comment>Georgian: The ethnic group of Georgian people.</rdfs:comment>
    </owl:NamedIndividual>
    


    <!-- http://www.sisostds.org/ontologies/C2SIM#GERMAB -->

    <owl:NamedIndividual rdf:about="http://www.sisostds.org/ontologies/C2SIM#GERMAB">
        <rdf:type rdf:resource="http://www.sisostds.org/ontologies/C2SIM#EthnicGroupCode"/>
        <rdfs:comment>Germanic (Baltic): The ethnic group of Germanic (Baltic) people.</rdfs:comment>
    </owl:NamedIndividual>
    


    <!-- http://www.sisostds.org/ontologies/C2SIM#GERMAL -->

    <owl:NamedIndividual rdf:about="http://www.sisostds.org/ontologies/C2SIM#GERMAL">
        <rdf:type rdf:resource="http://www.sisostds.org/ontologies/C2SIM#EthnicGroupCode"/>
        <rdfs:comment>Germanic (Alpine): The ethnic group of Germanic (Alpine) people.</rdfs:comment>
    </owl:NamedIndividual>
    


    <!-- http://www.sisostds.org/ontologies/C2SIM#GERMAN -->

    <owl:NamedIndividual rdf:about="http://www.sisostds.org/ontologies/C2SIM#GERMAN">
        <rdf:type rdf:resource="http://www.sisostds.org/ontologies/C2SIM#EthnicGroupCode"/>
        <rdfs:comment>German: The ethnic group of German people.</rdfs:comment>
    </owl:NamedIndividual>
    


    <!-- http://www.sisostds.org/ontologies/C2SIM#GERMAR -->

    <owl:NamedIndividual rdf:about="http://www.sisostds.org/ontologies/C2SIM#GERMAR">
        <rdf:type rdf:resource="http://www.sisostds.org/ontologies/C2SIM#EthnicGroupCode"/>
        <rdfs:comment>Germanic (Nordic): The ethnic group of Germanic (Nordic) people.</rdfs:comment>
    </owl:NamedIndividual>
    


    <!-- http://www.sisostds.org/ontologies/C2SIM#GGY -->

    <owl:NamedIndividual rdf:about="http://www.sisostds.org/ontologies/C2SIM#GGY">
        <rdf:type rdf:resource="http://www.sisostds.org/ontologies/C2SIM#CountryCode"/>
        <rdfs:comment>Guernsey: No longer a subdivision of GBR (2006).</rdfs:comment>
    </owl:NamedIndividual>
    


    <!-- http://www.sisostds.org/ontologies/C2SIM#GHA -->

    <owl:NamedIndividual rdf:about="http://www.sisostds.org/ontologies/C2SIM#GHA">
        <rdf:type rdf:resource="http://www.sisostds.org/ontologies/C2SIM#CountryCode"/>
        <rdfs:comment>Ghana: </rdfs:comment>
    </owl:NamedIndividual>
    


    <!-- http://www.sisostds.org/ontologies/C2SIM#GIB -->

    <owl:NamedIndividual rdf:about="http://www.sisostds.org/ontologies/C2SIM#GIB">
        <rdf:type rdf:resource="http://www.sisostds.org/ontologies/C2SIM#CountryCode"/>
        <rdfs:comment>Gibraltar: </rdfs:comment>
    </owl:NamedIndividual>
    


    <!-- http://www.sisostds.org/ontologies/C2SIM#GILAKI -->

    <owl:NamedIndividual rdf:about="http://www.sisostds.org/ontologies/C2SIM#GILAKI">
        <rdf:type rdf:resource="http://www.sisostds.org/ontologies/C2SIM#EthnicGroupCode"/>
        <rdfs:comment>Gilaki: The ethnic group of Gilaki people.</rdfs:comment>
    </owl:NamedIndividual>
    


    <!-- http://www.sisostds.org/ontologies/C2SIM#GIN -->

    <owl:NamedIndividual rdf:about="http://www.sisostds.org/ontologies/C2SIM#GIN">
        <rdf:type rdf:resource="http://www.sisostds.org/ontologies/C2SIM#CountryCode"/>
        <rdfs:comment>Guinea: </rdfs:comment>
    </owl:NamedIndividual>
    


    <!-- http://www.sisostds.org/ontologies/C2SIM#GLP -->

    <owl:NamedIndividual rdf:about="http://www.sisostds.org/ontologies/C2SIM#GLP">
        <rdf:type rdf:resource="http://www.sisostds.org/ontologies/C2SIM#CountryCode"/>
        <rdfs:comment>Guadeloupe: </rdfs:comment>
    </owl:NamedIndividual>
    


    <!-- http://www.sisostds.org/ontologies/C2SIM#GMB -->

    <owl:NamedIndividual rdf:about="http://www.sisostds.org/ontologies/C2SIM#GMB">
        <rdf:type rdf:resource="http://www.sisostds.org/ontologies/C2SIM#CountryCode"/>
        <rdfs:comment>Gambia: </rdfs:comment>
    </owl:NamedIndividual>
    


    <!-- http://www.sisostds.org/ontologies/C2SIM#GMBISL -->

    <owl:NamedIndividual rdf:about="http://www.sisostds.org/ontologies/C2SIM#GMBISL">
        <rdf:type rdf:resource="http://www.sisostds.org/ontologies/C2SIM#EthnicGroupCode"/>
        <rdfs:comment>Gambier Islander: The ethnic group of Gambier Islander people.</rdfs:comment>
    </owl:NamedIndividual>
    


    <!-- http://www.sisostds.org/ontologies/C2SIM#GNB -->

    <owl:NamedIndividual rdf:about="http://www.sisostds.org/ontologies/C2SIM#GNB">
        <rdf:type rdf:resource="http://www.sisostds.org/ontologies/C2SIM#CountryCode"/>
        <rdfs:comment>Guinea-Bissau: </rdfs:comment>
    </owl:NamedIndividual>
    


    <!-- http://www.sisostds.org/ontologies/C2SIM#GNQ -->

    <owl:NamedIndividual rdf:about="http://www.sisostds.org/ontologies/C2SIM#GNQ">
        <rdf:type rdf:resource="http://www.sisostds.org/ontologies/C2SIM#CountryCode"/>
        <rdfs:comment>Equatorial Guinea: </rdfs:comment>
    </owl:NamedIndividual>
    


    <!-- http://www.sisostds.org/ontologies/C2SIM#GOULAY -->

    <owl:NamedIndividual rdf:about="http://www.sisostds.org/ontologies/C2SIM#GOULAY">
        <rdf:type rdf:resource="http://www.sisostds.org/ontologies/C2SIM#EthnicGroupCode"/>
        <rdfs:comment>Goulaye: The ethnic group of Goulaye people.</rdfs:comment>
    </owl:NamedIndividual>
    


    <!-- http://www.sisostds.org/ontologies/C2SIM#GOURMA -->

    <owl:NamedIndividual rdf:about="http://www.sisostds.org/ontologies/C2SIM#GOURMA">
        <rdf:type rdf:resource="http://www.sisostds.org/ontologies/C2SIM#EthnicGroupCode"/>
        <rdfs:comment>Gourmantche: The ethnic group of Gourmantche people.</rdfs:comment>
    </owl:NamedIndividual>
    


    <!-- http://www.sisostds.org/ontologies/C2SIM#GRC -->

    <owl:NamedIndividual rdf:about="http://www.sisostds.org/ontologies/C2SIM#GRC">
        <rdf:type rdf:resource="http://www.sisostds.org/ontologies/C2SIM#CountryCode"/>
        <rdfs:comment>Greece: </rdfs:comment>
    </owl:NamedIndividual>
    


    <!-- http://www.sisostds.org/ontologies/C2SIM#GRD -->

    <owl:NamedIndividual rdf:about="http://www.sisostds.org/ontologies/C2SIM#GRD">
        <rdf:type rdf:resource="http://www.sisostds.org/ontologies/C2SIM#CountryCode"/>
        <rdfs:comment>Grenada: </rdfs:comment>
    </owl:NamedIndividual>
    


    <!-- http://www.sisostds.org/ontologies/C2SIM#GREEK -->

    <owl:NamedIndividual rdf:about="http://www.sisostds.org/ontologies/C2SIM#GREEK">
        <rdf:type rdf:resource="http://www.sisostds.org/ontologies/C2SIM#EthnicGroupCode"/>
        <rdfs:comment>Greek (incl Greek Cypriot): The ethnic group of Greek (incl Greek Cypriot) people.</rdfs:comment>
    </owl:NamedIndividual>
    


    <!-- http://www.sisostds.org/ontologies/C2SIM#GREEKT -->

    <owl:NamedIndividual rdf:about="http://www.sisostds.org/ontologies/C2SIM#GREEKT">
        <rdf:type rdf:resource="http://www.sisostds.org/ontologies/C2SIM#EthnicGroupCode"/>
        <rdfs:comment>Greek-Italians: The ethnic group of Greek-Italians people.</rdfs:comment>
    </owl:NamedIndividual>
    


    <!-- http://www.sisostds.org/ontologies/C2SIM#GREENA -->

    <owl:NamedIndividual rdf:about="http://www.sisostds.org/ontologies/C2SIM#GREENA">
        <rdf:type rdf:resource="http://www.sisostds.org/ontologies/C2SIM#EthnicGroupCode"/>
        <rdfs:comment>Greenlander (Eskimo): The ethnic group of Greenlander (Eskimo) people.</rdfs:comment>
    </owl:NamedIndividual>
    


    <!-- http://www.sisostds.org/ontologies/C2SIM#GREENC -->

    <owl:NamedIndividual rdf:about="http://www.sisostds.org/ontologies/C2SIM#GREENC">
        <rdf:type rdf:resource="http://www.sisostds.org/ontologies/C2SIM#EthnicGroupCode"/>
        <rdfs:comment>Greenlander (Caucasian): The ethnic group of Greenlander (Caucasian) people.</rdfs:comment>
    </owl:NamedIndividual>
    


    <!-- http://www.sisostds.org/ontologies/C2SIM#GRGARM -->

    <owl:NamedIndividual rdf:about="http://www.sisostds.org/ontologies/C2SIM#GRGARM">
        <rdf:type rdf:resource="http://www.sisostds.org/ontologies/C2SIM#ReligionCode"/>
        <rdfs:comment>Gregorian-Armenian: One who adheres to or identifies with the Gregorian-Armenian doctrine.</rdfs:comment>
    </owl:NamedIndividual>
    


    <!-- http://www.sisostds.org/ontologies/C2SIM#GRKCTH -->

    <owl:NamedIndividual rdf:about="http://www.sisostds.org/ontologies/C2SIM#GRKCTH">
        <rdf:type rdf:resource="http://www.sisostds.org/ontologies/C2SIM#ReligionCode"/>
        <rdfs:comment>Greek Catholic: One who adheres to or identifies with the Greek Catholic doctrine.</rdfs:comment>
    </owl:NamedIndividual>
    


    <!-- http://www.sisostds.org/ontologies/C2SIM#GRKORT -->

    <owl:NamedIndividual rdf:about="http://www.sisostds.org/ontologies/C2SIM#GRKORT">
        <rdf:type rdf:resource="http://www.sisostds.org/ontologies/C2SIM#ReligionCode"/>
        <rdfs:comment>Greek Orthodox: One who adheres to or identifies with the Greek Orthodox doctrine.</rdfs:comment>
    </owl:NamedIndividual>
    


    <!-- http://www.sisostds.org/ontologies/C2SIM#GRL -->

    <owl:NamedIndividual rdf:about="http://www.sisostds.org/ontologies/C2SIM#GRL">
        <rdf:type rdf:resource="http://www.sisostds.org/ontologies/C2SIM#CountryCode"/>
        <rdfs:comment>Greenland: </rdfs:comment>
    </owl:NamedIndividual>
    


    <!-- http://www.sisostds.org/ontologies/C2SIM#GRNLND -->

    <owl:NamedIndividual rdf:about="http://www.sisostds.org/ontologies/C2SIM#GRNLND">
        <rdf:type rdf:resource="http://www.sisostds.org/ontologies/C2SIM#EthnicGroupCode"/>
        <rdfs:comment>Greenlander: The ethnic group of Greenlander people.</rdfs:comment>
    </owl:NamedIndividual>
    


    <!-- http://www.sisostds.org/ontologies/C2SIM#GTM -->

    <owl:NamedIndividual rdf:about="http://www.sisostds.org/ontologies/C2SIM#GTM">
        <rdf:type rdf:resource="http://www.sisostds.org/ontologies/C2SIM#CountryCode"/>
        <rdfs:comment>Guatemala: </rdfs:comment>
    </owl:NamedIndividual>
    


    <!-- http://www.sisostds.org/ontologies/C2SIM#GUADLN -->

    <owl:NamedIndividual rdf:about="http://www.sisostds.org/ontologies/C2SIM#GUADLN">
        <rdf:type rdf:resource="http://www.sisostds.org/ontologies/C2SIM#EthnicGroupCode"/>
        <rdfs:comment>Guadalcanalian: The ethnic group of Guadalcanalian people.</rdfs:comment>
    </owl:NamedIndividual>
    


    <!-- http://www.sisostds.org/ontologies/C2SIM#GUATLN -->

    <owl:NamedIndividual rdf:about="http://www.sisostds.org/ontologies/C2SIM#GUATLN">
        <rdf:type rdf:resource="http://www.sisostds.org/ontologies/C2SIM#EthnicGroupCode"/>
        <rdfs:comment>Guatemalan: The ethnic group of Guatemalan people.</rdfs:comment>
    </owl:NamedIndividual>
    


    <!-- http://www.sisostds.org/ontologies/C2SIM#GUF -->

    <owl:NamedIndividual rdf:about="http://www.sisostds.org/ontologies/C2SIM#GUF">
        <rdf:type rdf:resource="http://www.sisostds.org/ontologies/C2SIM#CountryCode"/>
        <rdfs:comment>French Guiana: </rdfs:comment>
    </owl:NamedIndividual>
    


    <!-- http://www.sisostds.org/ontologies/C2SIM#GUJART -->

    <owl:NamedIndividual rdf:about="http://www.sisostds.org/ontologies/C2SIM#GUJART">
        <rdf:type rdf:resource="http://www.sisostds.org/ontologies/C2SIM#EthnicGroupCode"/>
        <rdfs:comment>Gujarati: The ethnic group of Gujarati people.</rdfs:comment>
    </owl:NamedIndividual>
    


    <!-- http://www.sisostds.org/ontologies/C2SIM#GUM -->

    <owl:NamedIndividual rdf:about="http://www.sisostds.org/ontologies/C2SIM#GUM">
        <rdf:type rdf:resource="http://www.sisostds.org/ontologies/C2SIM#CountryCode"/>
        <rdfs:comment>Guam: </rdfs:comment>
    </owl:NamedIndividual>
    


    <!-- http://www.sisostds.org/ontologies/C2SIM#GUMISL -->

    <owl:NamedIndividual rdf:about="http://www.sisostds.org/ontologies/C2SIM#GUMISL">
        <rdf:type rdf:resource="http://www.sisostds.org/ontologies/C2SIM#EthnicGroupCode"/>
        <rdfs:comment>Guam Islander/Chamorro: The ethnic group of Guam Islander/Chamorro people.</rdfs:comment>
    </owl:NamedIndividual>
    


    <!-- http://www.sisostds.org/ontologies/C2SIM#GURAGE -->

    <owl:NamedIndividual rdf:about="http://www.sisostds.org/ontologies/C2SIM#GURAGE">
        <rdf:type rdf:resource="http://www.sisostds.org/ontologies/C2SIM#EthnicGroupCode"/>
        <rdfs:comment>Gurage: The ethnic group of Gurage people.</rdfs:comment>
    </owl:NamedIndividual>
    


    <!-- http://www.sisostds.org/ontologies/C2SIM#GURUNG -->

    <owl:NamedIndividual rdf:about="http://www.sisostds.org/ontologies/C2SIM#GURUNG">
        <rdf:type rdf:resource="http://www.sisostds.org/ontologies/C2SIM#EthnicGroupCode"/>
        <rdfs:comment>Gurungs: The ethnic group of Gurungs people.</rdfs:comment>
    </owl:NamedIndividual>
    


    <!-- http://www.sisostds.org/ontologies/C2SIM#GURUNS -->

    <owl:NamedIndividual rdf:about="http://www.sisostds.org/ontologies/C2SIM#GURUNS">
        <rdf:type rdf:resource="http://www.sisostds.org/ontologies/C2SIM#EthnicGroupCode"/>
        <rdfs:comment>Gurunsi: The ethnic group of Gurunsi people.</rdfs:comment>
    </owl:NamedIndividual>
    


    <!-- http://www.sisostds.org/ontologies/C2SIM#GUY -->

    <owl:NamedIndividual rdf:about="http://www.sisostds.org/ontologies/C2SIM#GUY">
        <rdf:type rdf:resource="http://www.sisostds.org/ontologies/C2SIM#CountryCode"/>
        <rdfs:comment>Guyana: </rdfs:comment>
    </owl:NamedIndividual>
    


    <!-- http://www.sisostds.org/ontologies/C2SIM#GUYANS -->

    <owl:NamedIndividual rdf:about="http://www.sisostds.org/ontologies/C2SIM#GUYANS">
        <rdf:type rdf:resource="http://www.sisostds.org/ontologies/C2SIM#EthnicGroupCode"/>
        <rdfs:comment>Guyanese: The ethnic group of Guyanese people.</rdfs:comment>
    </owl:NamedIndividual>
    


    <!-- http://www.sisostds.org/ontologies/C2SIM#GYPSY -->

    <owl:NamedIndividual rdf:about="http://www.sisostds.org/ontologies/C2SIM#GYPSY">
        <rdf:type rdf:resource="http://www.sisostds.org/ontologies/C2SIM#EthnicGroupCode"/>
        <rdfs:comment>Gypsy: The ethnic group of Gypsy people.</rdfs:comment>
    </owl:NamedIndividual>
    


    <!-- http://www.sisostds.org/ontologies/C2SIM#GenericEvent -->

    <owl:NamedIndividual rdf:about="http://www.sisostds.org/ontologies/C2SIM#GenericEvent">
        <rdf:type rdf:resource="http://www.sisostds.org/ontologies/C2SIM#EventCode"/>
    </owl:NamedIndividual>
    


    <!-- http://www.sisostds.org/ontologies/C2SIM#HAMTC -->

    <owl:NamedIndividual rdf:about="http://www.sisostds.org/ontologies/C2SIM#HAMTC">
        <rdf:type rdf:resource="http://www.sisostds.org/ontologies/C2SIM#EthnicGroupCode"/>
        <rdfs:comment>Hamitic: The ethnic group of Hamitic people.</rdfs:comment>
    </owl:NamedIndividual>
    


    <!-- http://www.sisostds.org/ontologies/C2SIM#HAMTCM -->

    <owl:NamedIndividual rdf:about="http://www.sisostds.org/ontologies/C2SIM#HAMTCM">
        <rdf:type rdf:resource="http://www.sisostds.org/ontologies/C2SIM#EthnicGroupCode"/>
        <rdfs:comment>Hamitic (Mangbetu-Azande): The ethnic group of Hamitic (Mangbetu-Azande) people.</rdfs:comment>
    </owl:NamedIndividual>
    


    <!-- http://www.sisostds.org/ontologies/C2SIM#HAN -->

    <owl:NamedIndividual rdf:about="http://www.sisostds.org/ontologies/C2SIM#HAN">
        <rdf:type rdf:resource="http://www.sisostds.org/ontologies/C2SIM#EthnicGroupCode"/>
        <rdfs:comment>Han Chinese: The ethnic group of Han Chinese people.</rdfs:comment>
    </owl:NamedIndividual>
    


    <!-- http://www.sisostds.org/ontologies/C2SIM#HAUSA -->

    <owl:NamedIndividual rdf:about="http://www.sisostds.org/ontologies/C2SIM#HAUSA">
        <rdf:type rdf:resource="http://www.sisostds.org/ontologies/C2SIM#EthnicGroupCode"/>
        <rdfs:comment>Hausa: The ethnic group of Hausa people.</rdfs:comment>
    </owl:NamedIndividual>
    


    <!-- http://www.sisostds.org/ontologies/C2SIM#HAWIAN -->

    <owl:NamedIndividual rdf:about="http://www.sisostds.org/ontologies/C2SIM#HAWIAN">
        <rdf:type rdf:resource="http://www.sisostds.org/ontologies/C2SIM#EthnicGroupCode"/>
        <rdfs:comment>Hawaiian: The ethnic group of Hawaiian people.</rdfs:comment>
    </owl:NamedIndividual>
    


    <!-- http://www.sisostds.org/ontologies/C2SIM#HAZARA -->

    <owl:NamedIndividual rdf:about="http://www.sisostds.org/ontologies/C2SIM#HAZARA">
        <rdf:type rdf:resource="http://www.sisostds.org/ontologies/C2SIM#EthnicGroupCode"/>
        <rdfs:comment>Hazara: The ethnic group of Hazara people.</rdfs:comment>
    </owl:NamedIndividual>
    


    <!-- http://www.sisostds.org/ontologies/C2SIM#HINDU -->

    <owl:NamedIndividual rdf:about="http://www.sisostds.org/ontologies/C2SIM#HINDU">
        <rdf:type rdf:resource="http://www.sisostds.org/ontologies/C2SIM#ReligionCode"/>
        <rdfs:comment>Hinduism: One who adheres to or identifies with the Hinduism doctrine.</rdfs:comment>
    </owl:NamedIndividual>
    


    <!-- http://www.sisostds.org/ontologies/C2SIM#HINDUS -->

    <owl:NamedIndividual rdf:about="http://www.sisostds.org/ontologies/C2SIM#HINDUS">
        <rdf:type rdf:resource="http://www.sisostds.org/ontologies/C2SIM#EthnicGroupCode"/>
        <rdfs:comment>Hindustani: The ethnic group of Hindustani people.</rdfs:comment>
    </owl:NamedIndividual>
    


    <!-- http://www.sisostds.org/ontologies/C2SIM#HISPAN -->

    <owl:NamedIndividual rdf:about="http://www.sisostds.org/ontologies/C2SIM#HISPAN">
        <rdf:type rdf:resource="http://www.sisostds.org/ontologies/C2SIM#EthnicGroupCode"/>
        <rdfs:comment>Hispanic: The ethnic group of Hispanic people.</rdfs:comment>
    </owl:NamedIndividual>
    


    <!-- http://www.sisostds.org/ontologies/C2SIM#HKCHNS -->

    <owl:NamedIndividual rdf:about="http://www.sisostds.org/ontologies/C2SIM#HKCHNS">
        <rdf:type rdf:resource="http://www.sisostds.org/ontologies/C2SIM#EthnicGroupCode"/>
        <rdfs:comment>Hong Kong Chinese: The ethnic group of Hong Kong Chinese people.</rdfs:comment>
    </owl:NamedIndividual>
    


    <!-- http://www.sisostds.org/ontologies/C2SIM#HKG -->

    <owl:NamedIndividual rdf:about="http://www.sisostds.org/ontologies/C2SIM#HKG">
        <rdf:type rdf:resource="http://www.sisostds.org/ontologies/C2SIM#CountryCode"/>
        <rdfs:comment>Hong Kong: </rdfs:comment>
    </owl:NamedIndividual>
    


    <!-- http://www.sisostds.org/ontologies/C2SIM#HMD -->

    <owl:NamedIndividual rdf:about="http://www.sisostds.org/ontologies/C2SIM#HMD">
        <rdf:type rdf:resource="http://www.sisostds.org/ontologies/C2SIM#CountryCode"/>
        <rdfs:comment>Heard and Mcdonald Islands: </rdfs:comment>
    </owl:NamedIndividual>
    


    <!-- http://www.sisostds.org/ontologies/C2SIM#HMONG -->

    <owl:NamedIndividual rdf:about="http://www.sisostds.org/ontologies/C2SIM#HMONG">
        <rdf:type rdf:resource="http://www.sisostds.org/ontologies/C2SIM#EthnicGroupCode"/>
        <rdfs:comment>Hmong: The ethnic group of Hmong people.</rdfs:comment>
    </owl:NamedIndividual>
    


    <!-- http://www.sisostds.org/ontologies/C2SIM#HND -->

    <owl:NamedIndividual rdf:about="http://www.sisostds.org/ontologies/C2SIM#HND">
        <rdf:type rdf:resource="http://www.sisostds.org/ontologies/C2SIM#CountryCode"/>
        <rdfs:comment>Honduras: </rdfs:comment>
    </owl:NamedIndividual>
    


    <!-- http://www.sisostds.org/ontologies/C2SIM#HONDRN -->

    <owl:NamedIndividual rdf:about="http://www.sisostds.org/ontologies/C2SIM#HONDRN">
        <rdf:type rdf:resource="http://www.sisostds.org/ontologies/C2SIM#EthnicGroupCode"/>
        <rdfs:comment>Honduran: The ethnic group of Honduran people.</rdfs:comment>
    </owl:NamedIndividual>
    


    <!-- http://www.sisostds.org/ontologies/C2SIM#HRV -->

    <owl:NamedIndividual rdf:about="http://www.sisostds.org/ontologies/C2SIM#HRV">
        <rdf:type rdf:resource="http://www.sisostds.org/ontologies/C2SIM#CountryCode"/>
        <rdfs:comment>Croatia: </rdfs:comment>
    </owl:NamedIndividual>
    


    <!-- http://www.sisostds.org/ontologies/C2SIM#HTI -->

    <owl:NamedIndividual rdf:about="http://www.sisostds.org/ontologies/C2SIM#HTI">
        <rdf:type rdf:resource="http://www.sisostds.org/ontologies/C2SIM#CountryCode"/>
        <rdfs:comment>Haiti: </rdfs:comment>
    </owl:NamedIndividual>
    


    <!-- http://www.sisostds.org/ontologies/C2SIM#HUI -->

    <owl:NamedIndividual rdf:about="http://www.sisostds.org/ontologies/C2SIM#HUI">
        <rdf:type rdf:resource="http://www.sisostds.org/ontologies/C2SIM#EthnicGroupCode"/>
        <rdfs:comment>Hui: The ethnic group of Hui people.</rdfs:comment>
    </owl:NamedIndividual>
    


    <!-- http://www.sisostds.org/ontologies/C2SIM#HUN -->

    <owl:NamedIndividual rdf:about="http://www.sisostds.org/ontologies/C2SIM#HUN">
        <rdf:type rdf:resource="http://www.sisostds.org/ontologies/C2SIM#CountryCode"/>
        <rdfs:comment>Hungary: </rdfs:comment>
    </owl:NamedIndividual>
    


    <!-- http://www.sisostds.org/ontologies/C2SIM#HUNGRN -->

    <owl:NamedIndividual rdf:about="http://www.sisostds.org/ontologies/C2SIM#HUNGRN">
        <rdf:type rdf:resource="http://www.sisostds.org/ontologies/C2SIM#EthnicGroupCode"/>
        <rdfs:comment>Hungarian: The ethnic group of Hungarian people.</rdfs:comment>
    </owl:NamedIndividual>
    


    <!-- http://www.sisostds.org/ontologies/C2SIM#HUTU -->

    <owl:NamedIndividual rdf:about="http://www.sisostds.org/ontologies/C2SIM#HUTU">
        <rdf:type rdf:resource="http://www.sisostds.org/ontologies/C2SIM#EthnicGroupCode"/>
        <rdfs:comment>Hutu: The ethnic group of Hutu people.</rdfs:comment>
    </owl:NamedIndividual>
    


    <!-- http://www.sisostds.org/ontologies/C2SIM#HUTUBA -->

    <owl:NamedIndividual rdf:about="http://www.sisostds.org/ontologies/C2SIM#HUTUBA">
        <rdf:type rdf:resource="http://www.sisostds.org/ontologies/C2SIM#EthnicGroupCode"/>
        <rdfs:comment>Hutu (Bantu): The ethnic group of Hutu (Bantu) people.</rdfs:comment>
    </owl:NamedIndividual>
    


    <!-- http://www.sisostds.org/ontologies/C2SIM#HoldInPlace -->

    <owl:NamedIndividual rdf:about="http://www.sisostds.org/ontologies/C2SIM#HoldInPlace">
        <rdf:type rdf:resource="http://www.sisostds.org/ontologies/C2SIM#TaskActionCode"/>
    </owl:NamedIndividual>
    <owl:Axiom>
        <owl:annotatedSource rdf:resource="http://www.sisostds.org/ontologies/C2SIM#HoldInPlace"/>
        <owl:annotatedProperty rdf:resource="http://www.w3.org/1999/02/22-rdf-syntax-ns#type"/>
        <owl:annotatedTarget rdf:resource="http://www.sisostds.org/ontologies/C2SIM#TaskActionCode"/>
        <rdfs:comment>Do not move.</rdfs:comment>
    </owl:Axiom>
    


    <!-- http://www.sisostds.org/ontologies/C2SIM#HostileTo -->

    <owl:NamedIndividual rdf:about="http://www.sisostds.org/ontologies/C2SIM#HostileTo">
        <rdf:type rdf:resource="http://www.sisostds.org/ontologies/C2SIM#AllegianceRelationshipCode"/>
    </owl:NamedIndividual>
    


    <!-- http://www.sisostds.org/ontologies/C2SIM#IBDMUS -->

    <owl:NamedIndividual rdf:about="http://www.sisostds.org/ontologies/C2SIM#IBDMUS">
        <rdf:type rdf:resource="http://www.sisostds.org/ontologies/C2SIM#ReligionCode"/>
        <rdfs:comment>Ibadhi Muslim: One who adheres to or identifies with the Ibadhi Muslim doctrine.</rdfs:comment>
    </owl:NamedIndividual>
    


    <!-- http://www.sisostds.org/ontologies/C2SIM#IBOS -->

    <owl:NamedIndividual rdf:about="http://www.sisostds.org/ontologies/C2SIM#IBOS">
        <rdf:type rdf:resource="http://www.sisostds.org/ontologies/C2SIM#EthnicGroupCode"/>
        <rdfs:comment>Ibos: The ethnic group of Ibos people.</rdfs:comment>
    </owl:NamedIndividual>
    


    <!-- http://www.sisostds.org/ontologies/C2SIM#ICLNDR -->

    <owl:NamedIndividual rdf:about="http://www.sisostds.org/ontologies/C2SIM#ICLNDR">
        <rdf:type rdf:resource="http://www.sisostds.org/ontologies/C2SIM#EthnicGroupCode"/>
        <rdfs:comment>Icelander: The ethnic group of Icelander people.</rdfs:comment>
    </owl:NamedIndividual>
    


    <!-- http://www.sisostds.org/ontologies/C2SIM#IDN -->

    <owl:NamedIndividual rdf:about="http://www.sisostds.org/ontologies/C2SIM#IDN">
        <rdf:type rdf:resource="http://www.sisostds.org/ontologies/C2SIM#CountryCode"/>
        <rdfs:comment>Indonesia: </rdfs:comment>
    </owl:NamedIndividual>
    


    <!-- http://www.sisostds.org/ontologies/C2SIM#IKRBAT -->

    <owl:NamedIndividual rdf:about="http://www.sisostds.org/ontologies/C2SIM#IKRBAT">
        <rdf:type rdf:resource="http://www.sisostds.org/ontologies/C2SIM#EthnicGroupCode"/>
        <rdfs:comment>I-Kiribati/Gilbertese: The ethnic group of I-Kiribati/Gilbertese people.</rdfs:comment>
    </owl:NamedIndividual>
    


    <!-- http://www.sisostds.org/ontologies/C2SIM#IMN -->

    <owl:NamedIndividual rdf:about="http://www.sisostds.org/ontologies/C2SIM#IMN">
        <rdf:type rdf:resource="http://www.sisostds.org/ontologies/C2SIM#CountryCode"/>
        <rdfs:comment>Isle of Man: No longer a subdivision of GBR (2006).</rdfs:comment>
    </owl:NamedIndividual>
    


    <!-- http://www.sisostds.org/ontologies/C2SIM#IND -->

    <owl:NamedIndividual rdf:about="http://www.sisostds.org/ontologies/C2SIM#IND">
        <rdf:type rdf:resource="http://www.sisostds.org/ontologies/C2SIM#CountryCode"/>
        <rdfs:comment>India: </rdfs:comment>
    </owl:NamedIndividual>
    


    <!-- http://www.sisostds.org/ontologies/C2SIM#INDGNS -->

    <owl:NamedIndividual rdf:about="http://www.sisostds.org/ontologies/C2SIM#INDGNS">
        <rdf:type rdf:resource="http://www.sisostds.org/ontologies/C2SIM#ReligionCode"/>
        <rdfs:comment>Indigenous: One who adheres to or identifies with the Indigenous doctrine.</rdfs:comment>
    </owl:NamedIndividual>
    


    <!-- http://www.sisostds.org/ontologies/C2SIM#INDIGE -->

    <owl:NamedIndividual rdf:about="http://www.sisostds.org/ontologies/C2SIM#INDIGE">
        <rdf:type rdf:resource="http://www.sisostds.org/ontologies/C2SIM#EthnicGroupCode"/>
        <rdfs:comment>Indigenous Eskimo: The ethnic group of Indigenous Eskimo people.</rdfs:comment>
    </owl:NamedIndividual>
    


    <!-- http://www.sisostds.org/ontologies/C2SIM#INDIGM -->

    <owl:NamedIndividual rdf:about="http://www.sisostds.org/ontologies/C2SIM#INDIGM">
        <rdf:type rdf:resource="http://www.sisostds.org/ontologies/C2SIM#EthnicGroupCode"/>
        <rdfs:comment>Indigenous Melanesian: The ethnic group of Indigenous Melanesian people.</rdfs:comment>
    </owl:NamedIndividual>
    


    <!-- http://www.sisostds.org/ontologies/C2SIM#INDIGN -->

    <owl:NamedIndividual rdf:about="http://www.sisostds.org/ontologies/C2SIM#INDIGN">
        <rdf:type rdf:resource="http://www.sisostds.org/ontologies/C2SIM#EthnicGroupCode"/>
        <rdfs:comment>Indigenous Indian: The ethnic group of Indigenous Indian people.</rdfs:comment>
    </owl:NamedIndividual>
    


    <!-- http://www.sisostds.org/ontologies/C2SIM#INDNEC -->

    <owl:NamedIndividual rdf:about="http://www.sisostds.org/ontologies/C2SIM#INDNEC">
        <rdf:type rdf:resource="http://www.sisostds.org/ontologies/C2SIM#EthnicGroupCode"/>
        <rdfs:comment>Indian not elsewhere classified: The not elsewhere classified ethnic groups of Indian people.</rdfs:comment>
    </owl:NamedIndividual>
    


    <!-- http://www.sisostds.org/ontologies/C2SIM#INDNFD -->

    <owl:NamedIndividual rdf:about="http://www.sisostds.org/ontologies/C2SIM#INDNFD">
        <rdf:type rdf:resource="http://www.sisostds.org/ontologies/C2SIM#EthnicGroupCode"/>
        <rdfs:comment>Indian not further defined: The not further defined ethnic groups of Indian people.</rdfs:comment>
    </owl:NamedIndividual>
    


    <!-- http://www.sisostds.org/ontologies/C2SIM#INDOAR -->

    <owl:NamedIndividual rdf:about="http://www.sisostds.org/ontologies/C2SIM#INDOAR">
        <rdf:type rdf:resource="http://www.sisostds.org/ontologies/C2SIM#EthnicGroupCode"/>
        <rdfs:comment>Indo-Aryan: The ethnic group of Indo-Aryan people.</rdfs:comment>
    </owl:NamedIndividual>
    


    <!-- http://www.sisostds.org/ontologies/C2SIM#INDOCH -->

    <owl:NamedIndividual rdf:about="http://www.sisostds.org/ontologies/C2SIM#INDOCH">
        <rdf:type rdf:resource="http://www.sisostds.org/ontologies/C2SIM#EthnicGroupCode"/>
        <rdfs:comment>Indochinese: The ethnic group of Indochinese people.</rdfs:comment>
    </owl:NamedIndividual>
    


    <!-- http://www.sisostds.org/ontologies/C2SIM#INDOMA -->

    <owl:NamedIndividual rdf:about="http://www.sisostds.org/ontologies/C2SIM#INDOMA">
        <rdf:type rdf:resource="http://www.sisostds.org/ontologies/C2SIM#EthnicGroupCode"/>
        <rdfs:comment>Indo-Mauritian: The ethnic group of Indo-Mauritian people.</rdfs:comment>
    </owl:NamedIndividual>
    


    <!-- http://www.sisostds.org/ontologies/C2SIM#INDOSN -->

    <owl:NamedIndividual rdf:about="http://www.sisostds.org/ontologies/C2SIM#INDOSN">
        <rdf:type rdf:resource="http://www.sisostds.org/ontologies/C2SIM#EthnicGroupCode"/>
        <rdfs:comment>Indonesian (incl Javanese/Sundanese/Sumatran): The ethnic group of Indonesian (incl Javanese/Sundanese/Sumatran) people.</rdfs:comment>
    </owl:NamedIndividual>
    


    <!-- http://www.sisostds.org/ontologies/C2SIM#INITIALIZATION_LATEST_POSITIONS -->

    <owl:NamedIndividual rdf:about="http://www.sisostds.org/ontologies/C2SIM#INITIALIZATION_LATEST_POSITIONS">
        <rdf:type rdf:resource="http://www.sisostds.org/ontologies/C2SIM#RefreshInitSelection"/>
        <rdfs:comment>Option for a late joiner to request initialization messages to include current positions of entities.</rdfs:comment>
    </owl:NamedIndividual>
    


    <!-- http://www.sisostds.org/ontologies/C2SIM#INITIALIZATION_ORIGINAL -->

    <owl:NamedIndividual rdf:about="http://www.sisostds.org/ontologies/C2SIM#INITIALIZATION_ORIGINAL">
        <rdf:type rdf:resource="http://www.sisostds.org/ontologies/C2SIM#RefreshInitSelection"/>
        <rdfs:comment>Option for a late joiner to request the oritinal initialization message used to initialize the C2SIM coalition of systems.</rdfs:comment>
    </owl:NamedIndividual>
    


    <!-- http://www.sisostds.org/ontologies/C2SIM#INSRGT -->

    <owl:NamedIndividual rdf:about="http://www.sisostds.org/ontologies/C2SIM#INSRGT">
        <rdf:type rdf:resource="http://www.sisostds.org/ontologies/C2SIM#OrganizationTypeCode"/>
        <rdfs:comment>Insurgent: A GROUP-ORGANISATION-TYPE that rises in revolt against authority.</rdfs:comment>
    </owl:NamedIndividual>
    


    <!-- http://www.sisostds.org/ontologies/C2SIM#INTEL -->

    <owl:NamedIndividual rdf:about="http://www.sisostds.org/ontologies/C2SIM#INTEL">
        <rdf:type rdf:resource="http://www.sisostds.org/ontologies/C2SIM#OrganizationTypeCode"/>
        <rdfs:comment>Intelligence: A GROUP-ORGANISATION-TYPE that is employed to gather information.</rdfs:comment>
    </owl:NamedIndividual>
    


    <!-- http://www.sisostds.org/ontologies/C2SIM#INTLCT -->

    <owl:NamedIndividual rdf:about="http://www.sisostds.org/ontologies/C2SIM#INTLCT">
        <rdf:type rdf:resource="http://www.sisostds.org/ontologies/C2SIM#OrganizationTypeCode"/>
        <rdfs:comment>Intellectual: A GROUP-ORGANISATION-TYPE that comprises intellectual beings possessing superior powers of intellect.</rdfs:comment>
    </owl:NamedIndividual>
    


    <!-- http://www.sisostds.org/ontologies/C2SIM#INUIT -->

    <owl:NamedIndividual rdf:about="http://www.sisostds.org/ontologies/C2SIM#INUIT">
        <rdf:type rdf:resource="http://www.sisostds.org/ontologies/C2SIM#EthnicGroupCode"/>
        <rdfs:comment>Inuit/Eskimo: The ethnic group of Inuit/Eskimo people.</rdfs:comment>
    </owl:NamedIndividual>
    


    <!-- http://www.sisostds.org/ontologies/C2SIM#IOT -->

    <owl:NamedIndividual rdf:about="http://www.sisostds.org/ontologies/C2SIM#IOT">
        <rdf:type rdf:resource="http://www.sisostds.org/ontologies/C2SIM#CountryCode"/>
        <rdfs:comment>British Indian Ocean Territory: </rdfs:comment>
    </owl:NamedIndividual>
    


    <!-- http://www.sisostds.org/ontologies/C2SIM#IRAQI -->

    <owl:NamedIndividual rdf:about="http://www.sisostds.org/ontologies/C2SIM#IRAQI">
        <rdf:type rdf:resource="http://www.sisostds.org/ontologies/C2SIM#EthnicGroupCode"/>
        <rdfs:comment>Iraqi: The ethnic group of Iraqi people.</rdfs:comment>
    </owl:NamedIndividual>
    


    <!-- http://www.sisostds.org/ontologies/C2SIM#IRISH -->

    <owl:NamedIndividual rdf:about="http://www.sisostds.org/ontologies/C2SIM#IRISH">
        <rdf:type rdf:resource="http://www.sisostds.org/ontologies/C2SIM#EthnicGroupCode"/>
        <rdfs:comment>Irish: The ethnic group of Irish people.</rdfs:comment>
    </owl:NamedIndividual>
    


    <!-- http://www.sisostds.org/ontologies/C2SIM#IRL -->

    <owl:NamedIndividual rdf:about="http://www.sisostds.org/ontologies/C2SIM#IRL">
        <rdf:type rdf:resource="http://www.sisostds.org/ontologies/C2SIM#CountryCode"/>
        <rdfs:comment>Ireland: </rdfs:comment>
    </owl:NamedIndividual>
    


    <!-- http://www.sisostds.org/ontologies/C2SIM#IRN -->

    <owl:NamedIndividual rdf:about="http://www.sisostds.org/ontologies/C2SIM#IRN">
        <rdf:type rdf:resource="http://www.sisostds.org/ontologies/C2SIM#CountryCode"/>
        <rdfs:comment>Iran, Islamic Republic of: </rdfs:comment>
    </owl:NamedIndividual>
    


    <!-- http://www.sisostds.org/ontologies/C2SIM#IRNPER -->

    <owl:NamedIndividual rdf:about="http://www.sisostds.org/ontologies/C2SIM#IRNPER">
        <rdf:type rdf:resource="http://www.sisostds.org/ontologies/C2SIM#EthnicGroupCode"/>
        <rdfs:comment>Iranian/Persian: The ethnic group of Iranian/Persian people.</rdfs:comment>
    </owl:NamedIndividual>
    


    <!-- http://www.sisostds.org/ontologies/C2SIM#IRQ -->

    <owl:NamedIndividual rdf:about="http://www.sisostds.org/ontologies/C2SIM#IRQ">
        <rdf:type rdf:resource="http://www.sisostds.org/ontologies/C2SIM#CountryCode"/>
        <rdfs:comment>Iraq: </rdfs:comment>
    </owl:NamedIndividual>
    


    <!-- http://www.sisostds.org/ontologies/C2SIM#ISL -->

    <owl:NamedIndividual rdf:about="http://www.sisostds.org/ontologies/C2SIM#ISL">
        <rdf:type rdf:resource="http://www.sisostds.org/ontologies/C2SIM#CountryCode"/>
        <rdfs:comment>Iceland: </rdfs:comment>
    </owl:NamedIndividual>
    


    <!-- http://www.sisostds.org/ontologies/C2SIM#ISLAMA -->

    <owl:NamedIndividual rdf:about="http://www.sisostds.org/ontologies/C2SIM#ISLAMA">
        <rdf:type rdf:resource="http://www.sisostds.org/ontologies/C2SIM#ReligionCode"/>
        <rdfs:comment>Islam (Alawite): One who adheres to or identifies with the Islam (Alawite) doctrine.</rdfs:comment>
    </owl:NamedIndividual>
    


    <!-- http://www.sisostds.org/ontologies/C2SIM#ISLAMC -->

    <owl:NamedIndividual rdf:about="http://www.sisostds.org/ontologies/C2SIM#ISLAMC">
        <rdf:type rdf:resource="http://www.sisostds.org/ontologies/C2SIM#ReligionCode"/>
        <rdfs:comment>Islamic: One who adheres to or identifies with the Islamic doctrine.</rdfs:comment>
    </owl:NamedIndividual>
    


    <!-- http://www.sisostds.org/ontologies/C2SIM#ISLAMI -->

    <owl:NamedIndividual rdf:about="http://www.sisostds.org/ontologies/C2SIM#ISLAMI">
        <rdf:type rdf:resource="http://www.sisostds.org/ontologies/C2SIM#ReligionCode"/>
        <rdfs:comment>Islam (Isma&apos;ilite): One who adheres to or identifies with the Islam (Isma&apos;ilite) doctrine.</rdfs:comment>
    </owl:NamedIndividual>
    


    <!-- http://www.sisostds.org/ontologies/C2SIM#ISLAMN -->

    <owl:NamedIndividual rdf:about="http://www.sisostds.org/ontologies/C2SIM#ISLAMN">
        <rdf:type rdf:resource="http://www.sisostds.org/ontologies/C2SIM#ReligionCode"/>
        <rdfs:comment>Islam (Nusayri): One who adheres to or identifies with the Islam (Nusayri) doctrine.</rdfs:comment>
    </owl:NamedIndividual>
    


    <!-- http://www.sisostds.org/ontologies/C2SIM#ISR -->

    <owl:NamedIndividual rdf:about="http://www.sisostds.org/ontologies/C2SIM#ISR">
        <rdf:type rdf:resource="http://www.sisostds.org/ontologies/C2SIM#CountryCode"/>
        <rdfs:comment>Israel: </rdfs:comment>
    </owl:NamedIndividual>
    


    <!-- http://www.sisostds.org/ontologies/C2SIM#ISRJEW -->

    <owl:NamedIndividual rdf:about="http://www.sisostds.org/ontologies/C2SIM#ISRJEW">
        <rdf:type rdf:resource="http://www.sisostds.org/ontologies/C2SIM#EthnicGroupCode"/>
        <rdfs:comment>Israeli/Jewish/Hebrew: The ethnic group of Israeli/Jewish/Hebrew people.</rdfs:comment>
    </owl:NamedIndividual>
    


    <!-- http://www.sisostds.org/ontologies/C2SIM#ITA -->

    <owl:NamedIndividual rdf:about="http://www.sisostds.org/ontologies/C2SIM#ITA">
        <rdf:type rdf:resource="http://www.sisostds.org/ontologies/C2SIM#CountryCode"/>
        <rdfs:comment>Italy: </rdfs:comment>
    </owl:NamedIndividual>
    


    <!-- http://www.sisostds.org/ontologies/C2SIM#ITALAN -->

    <owl:NamedIndividual rdf:about="http://www.sisostds.org/ontologies/C2SIM#ITALAN">
        <rdf:type rdf:resource="http://www.sisostds.org/ontologies/C2SIM#EthnicGroupCode"/>
        <rdfs:comment>Italian: The ethnic group of Italian people.</rdfs:comment>
    </owl:NamedIndividual>
    


    <!-- http://www.sisostds.org/ontologies/C2SIM#ITALFR -->

    <owl:NamedIndividual rdf:about="http://www.sisostds.org/ontologies/C2SIM#ITALFR">
        <rdf:type rdf:resource="http://www.sisostds.org/ontologies/C2SIM#EthnicGroupCode"/>
        <rdfs:comment>Italian-French: The ethnic group of Italian-French people.</rdfs:comment>
    </owl:NamedIndividual>
    


    <!-- http://www.sisostds.org/ontologies/C2SIM#ITALGE -->

    <owl:NamedIndividual rdf:about="http://www.sisostds.org/ontologies/C2SIM#ITALGE">
        <rdf:type rdf:resource="http://www.sisostds.org/ontologies/C2SIM#EthnicGroupCode"/>
        <rdfs:comment>Italian-German: The ethnic group of Italian-German people.</rdfs:comment>
    </owl:NamedIndividual>
    


    <!-- http://www.sisostds.org/ontologies/C2SIM#ITALSL -->

    <owl:NamedIndividual rdf:about="http://www.sisostds.org/ontologies/C2SIM#ITALSL">
        <rdf:type rdf:resource="http://www.sisostds.org/ontologies/C2SIM#EthnicGroupCode"/>
        <rdfs:comment>Italian-Slovene: The ethnic group of Italian-Slovene people.</rdfs:comment>
    </owl:NamedIndividual>
    


    <!-- http://www.sisostds.org/ontologies/C2SIM#Inform -->

    <owl:NamedIndividual rdf:about="http://www.sisostds.org/ontologies/C2SIM#Inform">
        <rdf:type rdf:resource="http://www.sisostds.org/ontologies/C2SIM#CommunicativeActTypeCode"/>
    </owl:NamedIndividual>
    


    <!-- http://www.sisostds.org/ontologies/C2SIM#IntervalEndTime -->

    <owl:NamedIndividual rdf:about="http://www.sisostds.org/ontologies/C2SIM#IntervalEndTime">
        <rdf:type rdf:resource="http://www.sisostds.org/ontologies/C2SIM#TimeReferenceCode"/>
    </owl:NamedIndividual>
    


    <!-- http://www.sisostds.org/ontologies/C2SIM#IntervalStartTime -->

    <owl:NamedIndividual rdf:about="http://www.sisostds.org/ontologies/C2SIM#IntervalStartTime">
        <rdf:type rdf:resource="http://www.sisostds.org/ontologies/C2SIM#TimeReferenceCode"/>
    </owl:NamedIndividual>
    


    <!-- http://www.sisostds.org/ontologies/C2SIM#JAINS -->

    <owl:NamedIndividual rdf:about="http://www.sisostds.org/ontologies/C2SIM#JAINS">
        <rdf:type rdf:resource="http://www.sisostds.org/ontologies/C2SIM#ReligionCode"/>
        <rdfs:comment>Jains: One who adheres to or identifies with the Jains doctrine.</rdfs:comment>
    </owl:NamedIndividual>
    


    <!-- http://www.sisostds.org/ontologies/C2SIM#JAM -->

    <owl:NamedIndividual rdf:about="http://www.sisostds.org/ontologies/C2SIM#JAM">
        <rdf:type rdf:resource="http://www.sisostds.org/ontologies/C2SIM#CountryCode"/>
        <rdfs:comment>Jamaica: </rdfs:comment>
    </owl:NamedIndividual>
    


    <!-- http://www.sisostds.org/ontologies/C2SIM#JAMACN -->

    <owl:NamedIndividual rdf:about="http://www.sisostds.org/ontologies/C2SIM#JAMACN">
        <rdf:type rdf:resource="http://www.sisostds.org/ontologies/C2SIM#EthnicGroupCode"/>
        <rdfs:comment>Jamaican: The ethnic group of Jamaican people.</rdfs:comment>
    </owl:NamedIndividual>
    


    <!-- http://www.sisostds.org/ontologies/C2SIM#JAPNES -->

    <owl:NamedIndividual rdf:about="http://www.sisostds.org/ontologies/C2SIM#JAPNES">
        <rdf:type rdf:resource="http://www.sisostds.org/ontologies/C2SIM#EthnicGroupCode"/>
        <rdfs:comment>Japanese: The ethnic group of Japanese people.</rdfs:comment>
    </owl:NamedIndividual>
    


    <!-- http://www.sisostds.org/ontologies/C2SIM#JAVANE -->

    <owl:NamedIndividual rdf:about="http://www.sisostds.org/ontologies/C2SIM#JAVANE">
        <rdf:type rdf:resource="http://www.sisostds.org/ontologies/C2SIM#EthnicGroupCode"/>
        <rdfs:comment>Javanese: The ethnic group of Javanese people.</rdfs:comment>
    </owl:NamedIndividual>
    


    <!-- http://www.sisostds.org/ontologies/C2SIM#JEWISH -->

    <owl:NamedIndividual rdf:about="http://www.sisostds.org/ontologies/C2SIM#JEWISH">
        <rdf:type rdf:resource="http://www.sisostds.org/ontologies/C2SIM#EthnicGroupCode"/>
        <rdfs:comment>Jewish: The ethnic group of Jewish people.</rdfs:comment>
    </owl:NamedIndividual>
    


    <!-- http://www.sisostds.org/ontologies/C2SIM#JEY -->

    <owl:NamedIndividual rdf:about="http://www.sisostds.org/ontologies/C2SIM#JEY">
        <rdf:type rdf:resource="http://www.sisostds.org/ontologies/C2SIM#CountryCode"/>
        <rdfs:comment>Jersey: No longer a subdivision of GBR (2006).</rdfs:comment>
    </owl:NamedIndividual>
    


    <!-- http://www.sisostds.org/ontologies/C2SIM#JHVWTN -->

    <owl:NamedIndividual rdf:about="http://www.sisostds.org/ontologies/C2SIM#JHVWTN">
        <rdf:type rdf:resource="http://www.sisostds.org/ontologies/C2SIM#ReligionCode"/>
        <rdfs:comment>Jehovah&apos;s Witness: One who adheres to or identifies with the Jehovah&apos;s Witness doctrine.</rdfs:comment>
    </owl:NamedIndividual>
    


    <!-- http://www.sisostds.org/ontologies/C2SIM#JOR -->

    <owl:NamedIndividual rdf:about="http://www.sisostds.org/ontologies/C2SIM#JOR">
        <rdf:type rdf:resource="http://www.sisostds.org/ontologies/C2SIM#CountryCode"/>
        <rdfs:comment>Jordan: </rdfs:comment>
    </owl:NamedIndividual>
    


    <!-- http://www.sisostds.org/ontologies/C2SIM#JORDNN -->

    <owl:NamedIndividual rdf:about="http://www.sisostds.org/ontologies/C2SIM#JORDNN">
        <rdf:type rdf:resource="http://www.sisostds.org/ontologies/C2SIM#EthnicGroupCode"/>
        <rdfs:comment>Jordanian: The ethnic group of Jordanian people.</rdfs:comment>
    </owl:NamedIndividual>
    


    <!-- http://www.sisostds.org/ontologies/C2SIM#JPN -->

    <owl:NamedIndividual rdf:about="http://www.sisostds.org/ontologies/C2SIM#JPN">
        <rdf:type rdf:resource="http://www.sisostds.org/ontologies/C2SIM#CountryCode"/>
        <rdfs:comment>Japan: </rdfs:comment>
    </owl:NamedIndividual>
    


    <!-- http://www.sisostds.org/ontologies/C2SIM#JRNLST -->

    <owl:NamedIndividual rdf:about="http://www.sisostds.org/ontologies/C2SIM#JRNLST">
        <rdf:type rdf:resource="http://www.sisostds.org/ontologies/C2SIM#OrganizationTypeCode"/>
        <rdfs:comment>Journalist: A GROUP-ORGANISATION-TYPE that comprises persons that earn their living by editing or writing for a public journal.</rdfs:comment>
    </owl:NamedIndividual>
    


    <!-- http://www.sisostds.org/ontologies/C2SIM#JUDASM -->

    <owl:NamedIndividual rdf:about="http://www.sisostds.org/ontologies/C2SIM#JUDASM">
        <rdf:type rdf:resource="http://www.sisostds.org/ontologies/C2SIM#ReligionCode"/>
        <rdfs:comment>Judaism: One who adheres to or identifies with the Judaism doctrine.</rdfs:comment>
    </owl:NamedIndividual>
    


    <!-- http://www.sisostds.org/ontologies/C2SIM#JUDCAL -->

    <owl:NamedIndividual rdf:about="http://www.sisostds.org/ontologies/C2SIM#JUDCAL">
        <rdf:type rdf:resource="http://www.sisostds.org/ontologies/C2SIM#OrganizationTypeCode"/>
        <rdfs:comment>Judicial: A GROUP-ORGANISATION-TYPE that is provides judgment in courts of justice or the administration of justice.</rdfs:comment>
    </owl:NamedIndividual>
    


    <!-- http://www.sisostds.org/ontologies/C2SIM#KABYE -->

    <owl:NamedIndividual rdf:about="http://www.sisostds.org/ontologies/C2SIM#KABYE">
        <rdf:type rdf:resource="http://www.sisostds.org/ontologies/C2SIM#EthnicGroupCode"/>
        <rdfs:comment>Kabye: The ethnic group of Kabye people.</rdfs:comment>
    </owl:NamedIndividual>
    


    <!-- http://www.sisostds.org/ontologies/C2SIM#KALANG -->

    <owl:NamedIndividual rdf:about="http://www.sisostds.org/ontologies/C2SIM#KALANG">
        <rdf:type rdf:resource="http://www.sisostds.org/ontologies/C2SIM#EthnicGroupCode"/>
        <rdfs:comment>Kalanga: The ethnic group of Kalanga people.</rdfs:comment>
    </owl:NamedIndividual>
    


    <!-- http://www.sisostds.org/ontologies/C2SIM#KALENJ -->

    <owl:NamedIndividual rdf:about="http://www.sisostds.org/ontologies/C2SIM#KALENJ">
        <rdf:type rdf:resource="http://www.sisostds.org/ontologies/C2SIM#EthnicGroupCode"/>
        <rdfs:comment>Kalenjin: The ethnic group of Kalenjin people.</rdfs:comment>
    </owl:NamedIndividual>
    


    <!-- http://www.sisostds.org/ontologies/C2SIM#KAMBA -->

    <owl:NamedIndividual rdf:about="http://www.sisostds.org/ontologies/C2SIM#KAMBA">
        <rdf:type rdf:resource="http://www.sisostds.org/ontologies/C2SIM#EthnicGroupCode"/>
        <rdfs:comment>Kamba: The ethnic group of Kamba people.</rdfs:comment>
    </owl:NamedIndividual>
    


    <!-- http://www.sisostds.org/ontologies/C2SIM#KAMCHN -->

    <owl:NamedIndividual rdf:about="http://www.sisostds.org/ontologies/C2SIM#KAMCHN">
        <rdf:type rdf:resource="http://www.sisostds.org/ontologies/C2SIM#EthnicGroupCode"/>
        <rdfs:comment>Kampuchean Chinese: The ethnic group of Kampuchean Chinese people.</rdfs:comment>
    </owl:NamedIndividual>
    


    <!-- http://www.sisostds.org/ontologies/C2SIM#KANAKA -->

    <owl:NamedIndividual rdf:about="http://www.sisostds.org/ontologies/C2SIM#KANAKA">
        <rdf:type rdf:resource="http://www.sisostds.org/ontologies/C2SIM#EthnicGroupCode"/>
        <rdfs:comment>Kanaka/Kanak: The ethnic group of Kanaka/Kanak people.</rdfs:comment>
    </owl:NamedIndividual>
    


    <!-- http://www.sisostds.org/ontologies/C2SIM#KARAKA -->

    <owl:NamedIndividual rdf:about="http://www.sisostds.org/ontologies/C2SIM#KARAKA">
        <rdf:type rdf:resource="http://www.sisostds.org/ontologies/C2SIM#EthnicGroupCode"/>
        <rdfs:comment>Karakalpaks: The ethnic group of Karakalpaks people.</rdfs:comment>
    </owl:NamedIndividual>
    


    <!-- http://www.sisostds.org/ontologies/C2SIM#KAREN -->

    <owl:NamedIndividual rdf:about="http://www.sisostds.org/ontologies/C2SIM#KAREN">
        <rdf:type rdf:resource="http://www.sisostds.org/ontologies/C2SIM#EthnicGroupCode"/>
        <rdfs:comment>Karen: The ethnic group of Karen people.</rdfs:comment>
    </owl:NamedIndividual>
    


    <!-- http://www.sisostds.org/ontologies/C2SIM#KAZ -->

    <owl:NamedIndividual rdf:about="http://www.sisostds.org/ontologies/C2SIM#KAZ">
        <rdf:type rdf:resource="http://www.sisostds.org/ontologies/C2SIM#CountryCode"/>
        <rdfs:comment>Kazakhstan: </rdfs:comment>
    </owl:NamedIndividual>
    


    <!-- http://www.sisostds.org/ontologies/C2SIM#KAZAKH -->

    <owl:NamedIndividual rdf:about="http://www.sisostds.org/ontologies/C2SIM#KAZAKH">
        <rdf:type rdf:resource="http://www.sisostds.org/ontologies/C2SIM#EthnicGroupCode"/>
        <rdfs:comment>Kazakh: The ethnic group of Kazakh people.</rdfs:comment>
    </owl:NamedIndividual>
    


    <!-- http://www.sisostds.org/ontologies/C2SIM#KAZAKQ -->

    <owl:NamedIndividual rdf:about="http://www.sisostds.org/ontologies/C2SIM#KAZAKQ">
        <rdf:type rdf:resource="http://www.sisostds.org/ontologies/C2SIM#EthnicGroupCode"/>
        <rdfs:comment>Kazakh (Qazaq): The ethnic group of Kazakh (Qazaq) people.</rdfs:comment>
    </owl:NamedIndividual>
    


    <!-- http://www.sisostds.org/ontologies/C2SIM#KEN -->

    <owl:NamedIndividual rdf:about="http://www.sisostds.org/ontologies/C2SIM#KEN">
        <rdf:type rdf:resource="http://www.sisostds.org/ontologies/C2SIM#CountryCode"/>
        <rdfs:comment>Kenya: </rdfs:comment>
    </owl:NamedIndividual>
    


    <!-- http://www.sisostds.org/ontologies/C2SIM#KENYAN -->

    <owl:NamedIndividual rdf:about="http://www.sisostds.org/ontologies/C2SIM#KENYAN">
        <rdf:type rdf:resource="http://www.sisostds.org/ontologies/C2SIM#EthnicGroupCode"/>
        <rdfs:comment>Kenyan: The ethnic group of Kenyan people.</rdfs:comment>
    </owl:NamedIndividual>
    


    <!-- http://www.sisostds.org/ontologies/C2SIM#KGALAG -->

    <owl:NamedIndividual rdf:about="http://www.sisostds.org/ontologies/C2SIM#KGALAG">
        <rdf:type rdf:resource="http://www.sisostds.org/ontologies/C2SIM#EthnicGroupCode"/>
        <rdfs:comment>Kgalagadi: The ethnic group of Kgalagadi people.</rdfs:comment>
    </owl:NamedIndividual>
    


    <!-- http://www.sisostds.org/ontologies/C2SIM#KGZ -->

    <owl:NamedIndividual rdf:about="http://www.sisostds.org/ontologies/C2SIM#KGZ">
        <rdf:type rdf:resource="http://www.sisostds.org/ontologies/C2SIM#CountryCode"/>
        <rdfs:comment>Kyrgyzstan: </rdfs:comment>
    </owl:NamedIndividual>
    


    <!-- http://www.sisostds.org/ontologies/C2SIM#KHM -->

    <owl:NamedIndividual rdf:about="http://www.sisostds.org/ontologies/C2SIM#KHM">
        <rdf:type rdf:resource="http://www.sisostds.org/ontologies/C2SIM#CountryCode"/>
        <rdfs:comment>Cambodia: Formerly Kampuchea</rdfs:comment>
    </owl:NamedIndividual>
    


    <!-- http://www.sisostds.org/ontologies/C2SIM#KHMER -->

    <owl:NamedIndividual rdf:about="http://www.sisostds.org/ontologies/C2SIM#KHMER">
        <rdf:type rdf:resource="http://www.sisostds.org/ontologies/C2SIM#EthnicGroupCode"/>
        <rdfs:comment>Khmer/Kampuchean/Cambodian: The ethnic group of Khmer/Kampuchean/Cambodian people.</rdfs:comment>
    </owl:NamedIndividual>
    


    <!-- http://www.sisostds.org/ontologies/C2SIM#KIEVPT -->

    <owl:NamedIndividual rdf:about="http://www.sisostds.org/ontologies/C2SIM#KIEVPT">
        <rdf:type rdf:resource="http://www.sisostds.org/ontologies/C2SIM#ReligionCode"/>
        <rdfs:comment>Kiev Patriarchate: One who adheres to or identifies with the Kiev Patriarchate doctrine.</rdfs:comment>
    </owl:NamedIndividual>
    


    <!-- http://www.sisostds.org/ontologies/C2SIM#KIKUYU -->

    <owl:NamedIndividual rdf:about="http://www.sisostds.org/ontologies/C2SIM#KIKUYU">
        <rdf:type rdf:resource="http://www.sisostds.org/ontologies/C2SIM#EthnicGroupCode"/>
        <rdfs:comment>Kikuyu: The ethnic group of Kikuyu people.</rdfs:comment>
    </owl:NamedIndividual>
    


    <!-- http://www.sisostds.org/ontologies/C2SIM#KIMBUN -->

    <owl:NamedIndividual rdf:about="http://www.sisostds.org/ontologies/C2SIM#KIMBUN">
        <rdf:type rdf:resource="http://www.sisostds.org/ontologies/C2SIM#EthnicGroupCode"/>
        <rdfs:comment>Kimbundu: The ethnic group of Kimbundu people.</rdfs:comment>
    </owl:NamedIndividual>
    


    <!-- http://www.sisostds.org/ontologies/C2SIM#KIR -->

    <owl:NamedIndividual rdf:about="http://www.sisostds.org/ontologies/C2SIM#KIR">
        <rdf:type rdf:resource="http://www.sisostds.org/ontologies/C2SIM#CountryCode"/>
        <rdfs:comment>Kiribati: </rdfs:comment>
    </owl:NamedIndividual>
    


    <!-- http://www.sisostds.org/ontologies/C2SIM#KIRDI -->

    <owl:NamedIndividual rdf:about="http://www.sisostds.org/ontologies/C2SIM#KIRDI">
        <rdf:type rdf:resource="http://www.sisostds.org/ontologies/C2SIM#EthnicGroupCode"/>
        <rdfs:comment>Kirdi: The ethnic group of Kirdi people.</rdfs:comment>
    </owl:NamedIndividual>
    


    <!-- http://www.sisostds.org/ontologies/C2SIM#KIRGHZ -->

    <owl:NamedIndividual rdf:about="http://www.sisostds.org/ontologies/C2SIM#KIRGHZ">
        <rdf:type rdf:resource="http://www.sisostds.org/ontologies/C2SIM#EthnicGroupCode"/>
        <rdfs:comment>Kirghiz: The ethnic group of Kirghiz people.</rdfs:comment>
    </owl:NamedIndividual>
    


    <!-- http://www.sisostds.org/ontologies/C2SIM#KISII -->

    <owl:NamedIndividual rdf:about="http://www.sisostds.org/ontologies/C2SIM#KISII">
        <rdf:type rdf:resource="http://www.sisostds.org/ontologies/C2SIM#EthnicGroupCode"/>
        <rdfs:comment>Kisii: The ethnic group of Kisii people.</rdfs:comment>
    </owl:NamedIndividual>
    


    <!-- http://www.sisostds.org/ontologies/C2SIM#KMBNGS -->

    <owl:NamedIndividual rdf:about="http://www.sisostds.org/ontologies/C2SIM#KMBNGS">
        <rdf:type rdf:resource="http://www.sisostds.org/ontologies/C2SIM#ReligionCode"/>
        <rdfs:comment>Kimbanguist: One who adheres to or identifies with the Kimbanguist doctrine.</rdfs:comment>
    </owl:NamedIndividual>
    


    <!-- http://www.sisostds.org/ontologies/C2SIM#KNA -->

    <owl:NamedIndividual rdf:about="http://www.sisostds.org/ontologies/C2SIM#KNA">
        <rdf:type rdf:resource="http://www.sisostds.org/ontologies/C2SIM#CountryCode"/>
        <rdfs:comment>Saint Kitts and Nevis: </rdfs:comment>
    </owl:NamedIndividual>
    


    <!-- http://www.sisostds.org/ontologies/C2SIM#KONGO -->

    <owl:NamedIndividual rdf:about="http://www.sisostds.org/ontologies/C2SIM#KONGO">
        <rdf:type rdf:resource="http://www.sisostds.org/ontologies/C2SIM#EthnicGroupCode"/>
        <rdfs:comment>Kongo: The ethnic group of Kongo people.</rdfs:comment>
    </owl:NamedIndividual>
    


    <!-- http://www.sisostds.org/ontologies/C2SIM#KOR -->

    <owl:NamedIndividual rdf:about="http://www.sisostds.org/ontologies/C2SIM#KOR">
        <rdf:type rdf:resource="http://www.sisostds.org/ontologies/C2SIM#CountryCode"/>
        <rdfs:comment>Korea, Republic of: </rdfs:comment>
    </owl:NamedIndividual>
    


    <!-- http://www.sisostds.org/ontologies/C2SIM#KOREAN -->

    <owl:NamedIndividual rdf:about="http://www.sisostds.org/ontologies/C2SIM#KOREAN">
        <rdf:type rdf:resource="http://www.sisostds.org/ontologies/C2SIM#EthnicGroupCode"/>
        <rdfs:comment>Korean: The ethnic group of Korean people.</rdfs:comment>
    </owl:NamedIndividual>
    


    <!-- http://www.sisostds.org/ontologies/C2SIM#KUNAMA -->

    <owl:NamedIndividual rdf:about="http://www.sisostds.org/ontologies/C2SIM#KUNAMA">
        <rdf:type rdf:resource="http://www.sisostds.org/ontologies/C2SIM#EthnicGroupCode"/>
        <rdfs:comment>Kunama: The ethnic group of Kunama people.</rdfs:comment>
    </owl:NamedIndividual>
    


    <!-- http://www.sisostds.org/ontologies/C2SIM#KURD -->

    <owl:NamedIndividual rdf:about="http://www.sisostds.org/ontologies/C2SIM#KURD">
        <rdf:type rdf:resource="http://www.sisostds.org/ontologies/C2SIM#EthnicGroupCode"/>
        <rdfs:comment>Kurd: The ethnic group of Kurd people.</rdfs:comment>
    </owl:NamedIndividual>
    


    <!-- http://www.sisostds.org/ontologies/C2SIM#KUWAIT -->

    <owl:NamedIndividual rdf:about="http://www.sisostds.org/ontologies/C2SIM#KUWAIT">
        <rdf:type rdf:resource="http://www.sisostds.org/ontologies/C2SIM#EthnicGroupCode"/>
        <rdfs:comment>Kuwaiti: The ethnic group of Kuwaiti people.</rdfs:comment>
    </owl:NamedIndividual>
    


    <!-- http://www.sisostds.org/ontologies/C2SIM#KWT -->

    <owl:NamedIndividual rdf:about="http://www.sisostds.org/ontologies/C2SIM#KWT">
        <rdf:type rdf:resource="http://www.sisostds.org/ontologies/C2SIM#CountryCode"/>
        <rdfs:comment>Kuwait: </rdfs:comment>
    </owl:NamedIndividual>
    


    <!-- http://www.sisostds.org/ontologies/C2SIM#LADINO -->

    <owl:NamedIndividual rdf:about="http://www.sisostds.org/ontologies/C2SIM#LADINO">
        <rdf:type rdf:resource="http://www.sisostds.org/ontologies/C2SIM#EthnicGroupCode"/>
        <rdfs:comment>Ladino (Indian/European): The ethnic group of Ladino (Indian/European) people.</rdfs:comment>
    </owl:NamedIndividual>
    


    <!-- http://www.sisostds.org/ontologies/C2SIM#LAMBUD -->

    <owl:NamedIndividual rdf:about="http://www.sisostds.org/ontologies/C2SIM#LAMBUD">
        <rdf:type rdf:resource="http://www.sisostds.org/ontologies/C2SIM#ReligionCode"/>
        <rdfs:comment>Lamaistic Buddhism: One who adheres to or identifies with the Lamaistic Buddhism doctrine.</rdfs:comment>
    </owl:NamedIndividual>
    


    <!-- http://www.sisostds.org/ontologies/C2SIM#LAO -->

    <owl:NamedIndividual rdf:about="http://www.sisostds.org/ontologies/C2SIM#LAO">
        <rdf:type rdf:resource="http://www.sisostds.org/ontologies/C2SIM#CountryCode"/>
        <rdfs:comment>Lao People&apos;s Democratic Republic: </rdfs:comment>
    </owl:NamedIndividual>
    


    <!-- http://www.sisostds.org/ontologies/C2SIM#LAOTAN -->

    <owl:NamedIndividual rdf:about="http://www.sisostds.org/ontologies/C2SIM#LAOTAN">
        <rdf:type rdf:resource="http://www.sisostds.org/ontologies/C2SIM#EthnicGroupCode"/>
        <rdfs:comment>Lao/Laotian: The ethnic group of Lao/Laotian people.</rdfs:comment>
    </owl:NamedIndividual>
    


    <!-- http://www.sisostds.org/ontologies/C2SIM#LAPP -->

    <owl:NamedIndividual rdf:about="http://www.sisostds.org/ontologies/C2SIM#LAPP">
        <rdf:type rdf:resource="http://www.sisostds.org/ontologies/C2SIM#EthnicGroupCode"/>
        <rdfs:comment>Lapp: The ethnic group of Lapp people.</rdfs:comment>
    </owl:NamedIndividual>
    


    <!-- http://www.sisostds.org/ontologies/C2SIM#LATIN -->

    <owl:NamedIndividual rdf:about="http://www.sisostds.org/ontologies/C2SIM#LATIN">
        <rdf:type rdf:resource="http://www.sisostds.org/ontologies/C2SIM#EthnicGroupCode"/>
        <rdfs:comment>Latin: The ethnic group of Latin people.</rdfs:comment>
    </owl:NamedIndividual>
    


    <!-- http://www.sisostds.org/ontologies/C2SIM#LATNEC -->

    <owl:NamedIndividual rdf:about="http://www.sisostds.org/ontologies/C2SIM#LATNEC">
        <rdf:type rdf:resource="http://www.sisostds.org/ontologies/C2SIM#EthnicGroupCode"/>
        <rdfs:comment>Latin American/Hispanic not elsewhere classified: The not elsewhere classified ethnic groups of Latin American/Hispanic people.</rdfs:comment>
    </owl:NamedIndividual>
    


    <!-- http://www.sisostds.org/ontologies/C2SIM#LATNFD -->

    <owl:NamedIndividual rdf:about="http://www.sisostds.org/ontologies/C2SIM#LATNFD">
        <rdf:type rdf:resource="http://www.sisostds.org/ontologies/C2SIM#EthnicGroupCode"/>
        <rdfs:comment>Latin American/Hispanic not further defined: The not further defined ethnic groups of Latin American/Hispanic people.</rdfs:comment>
    </owl:NamedIndividual>
    


    <!-- http://www.sisostds.org/ontologies/C2SIM#LATVAN -->

    <owl:NamedIndividual rdf:about="http://www.sisostds.org/ontologies/C2SIM#LATVAN">
        <rdf:type rdf:resource="http://www.sisostds.org/ontologies/C2SIM#EthnicGroupCode"/>
        <rdfs:comment>Latvian: The ethnic group of Latvian people.</rdfs:comment>
    </owl:NamedIndividual>
    


    <!-- http://www.sisostds.org/ontologies/C2SIM#LBN -->

    <owl:NamedIndividual rdf:about="http://www.sisostds.org/ontologies/C2SIM#LBN">
        <rdf:type rdf:resource="http://www.sisostds.org/ontologies/C2SIM#CountryCode"/>
        <rdfs:comment>Lebanon: </rdfs:comment>
    </owl:NamedIndividual>
    


    <!-- http://www.sisostds.org/ontologies/C2SIM#LBR -->

    <owl:NamedIndividual rdf:about="http://www.sisostds.org/ontologies/C2SIM#LBR">
        <rdf:type rdf:resource="http://www.sisostds.org/ontologies/C2SIM#CountryCode"/>
        <rdfs:comment>Liberia: </rdfs:comment>
    </owl:NamedIndividual>
    


    <!-- http://www.sisostds.org/ontologies/C2SIM#LBY -->

    <owl:NamedIndividual rdf:about="http://www.sisostds.org/ontologies/C2SIM#LBY">
        <rdf:type rdf:resource="http://www.sisostds.org/ontologies/C2SIM#CountryCode"/>
        <rdfs:comment>Libyan Arab Jamahiriya: </rdfs:comment>
    </owl:NamedIndividual>
    


    <!-- http://www.sisostds.org/ontologies/C2SIM#LCA -->

    <owl:NamedIndividual rdf:about="http://www.sisostds.org/ontologies/C2SIM#LCA">
        <rdf:type rdf:resource="http://www.sisostds.org/ontologies/C2SIM#CountryCode"/>
        <rdfs:comment>Saint Lucia: </rdfs:comment>
    </owl:NamedIndividual>
    


    <!-- http://www.sisostds.org/ontologies/C2SIM#LEBNSE -->

    <owl:NamedIndividual rdf:about="http://www.sisostds.org/ontologies/C2SIM#LEBNSE">
        <rdf:type rdf:resource="http://www.sisostds.org/ontologies/C2SIM#EthnicGroupCode"/>
        <rdfs:comment>Lebanese: The ethnic group of Lebanese people.</rdfs:comment>
    </owl:NamedIndividual>
    


    <!-- http://www.sisostds.org/ontologies/C2SIM#LIBYAN -->

    <owl:NamedIndividual rdf:about="http://www.sisostds.org/ontologies/C2SIM#LIBYAN">
        <rdf:type rdf:resource="http://www.sisostds.org/ontologies/C2SIM#EthnicGroupCode"/>
        <rdfs:comment>Libyan: The ethnic group of Libyan people.</rdfs:comment>
    </owl:NamedIndividual>
    


    <!-- http://www.sisostds.org/ontologies/C2SIM#LIE -->

    <owl:NamedIndividual rdf:about="http://www.sisostds.org/ontologies/C2SIM#LIE">
        <rdf:type rdf:resource="http://www.sisostds.org/ontologies/C2SIM#CountryCode"/>
        <rdfs:comment>Liechtenstein: </rdfs:comment>
    </owl:NamedIndividual>
    


    <!-- http://www.sisostds.org/ontologies/C2SIM#LIMBUS -->

    <owl:NamedIndividual rdf:about="http://www.sisostds.org/ontologies/C2SIM#LIMBUS">
        <rdf:type rdf:resource="http://www.sisostds.org/ontologies/C2SIM#EthnicGroupCode"/>
        <rdfs:comment>Limbus: The ethnic group of Limbus people.</rdfs:comment>
    </owl:NamedIndividual>
    


    <!-- http://www.sisostds.org/ontologies/C2SIM#LITHUN -->

    <owl:NamedIndividual rdf:about="http://www.sisostds.org/ontologies/C2SIM#LITHUN">
        <rdf:type rdf:resource="http://www.sisostds.org/ontologies/C2SIM#EthnicGroupCode"/>
        <rdfs:comment>Lithuanian: The ethnic group of Lithuanian people.</rdfs:comment>
    </owl:NamedIndividual>
    


    <!-- http://www.sisostds.org/ontologies/C2SIM#LKA -->

    <owl:NamedIndividual rdf:about="http://www.sisostds.org/ontologies/C2SIM#LKA">
        <rdf:type rdf:resource="http://www.sisostds.org/ontologies/C2SIM#CountryCode"/>
        <rdfs:comment>Sri Lanka: </rdfs:comment>
    </owl:NamedIndividual>
    


    <!-- http://www.sisostds.org/ontologies/C2SIM#LNDMSN -->

    <owl:NamedIndividual rdf:about="http://www.sisostds.org/ontologies/C2SIM#LNDMSN">
        <rdf:type rdf:resource="http://www.sisostds.org/ontologies/C2SIM#ReligionCode"/>
        <rdfs:comment>London Missionary Society: One who adheres to or identifies with the London Missionary Society doctrine.</rdfs:comment>
    </owl:NamedIndividual>
    


    <!-- http://www.sisostds.org/ontologies/C2SIM#LNDOWN -->

    <owl:NamedIndividual rdf:about="http://www.sisostds.org/ontologies/C2SIM#LNDOWN">
        <rdf:type rdf:resource="http://www.sisostds.org/ontologies/C2SIM#OrganizationTypeCode"/>
        <rdfs:comment>Landowner: A GROUP-ORGANISATION-TYPE that comprises persons that are owners or proprietors of land.</rdfs:comment>
    </owl:NamedIndividual>
    


    <!-- http://www.sisostds.org/ontologies/C2SIM#LOBI -->

    <owl:NamedIndividual rdf:about="http://www.sisostds.org/ontologies/C2SIM#LOBI">
        <rdf:type rdf:resource="http://www.sisostds.org/ontologies/C2SIM#EthnicGroupCode"/>
        <rdfs:comment>Lobi: The ethnic group of Lobi people.</rdfs:comment>
    </owl:NamedIndividual>
    


    <!-- http://www.sisostds.org/ontologies/C2SIM#LOCINH -->

    <owl:NamedIndividual rdf:about="http://www.sisostds.org/ontologies/C2SIM#LOCINH">
        <rdf:type rdf:resource="http://www.sisostds.org/ontologies/C2SIM#OrganizationTypeCode"/>
        <rdfs:comment>Local inhabitant: A GROUP-ORGANISATION-TYPE of a particular place regarded with reference to that place.</rdfs:comment>
    </owl:NamedIndividual>
    


    <!-- http://www.sisostds.org/ontologies/C2SIM#LOMWE -->

    <owl:NamedIndividual rdf:about="http://www.sisostds.org/ontologies/C2SIM#LOMWE">
        <rdf:type rdf:resource="http://www.sisostds.org/ontologies/C2SIM#EthnicGroupCode"/>
        <rdfs:comment>Lomwe: The ethnic group of Lomwe people.</rdfs:comment>
    </owl:NamedIndividual>
    


    <!-- http://www.sisostds.org/ontologies/C2SIM#LSO -->

    <owl:NamedIndividual rdf:about="http://www.sisostds.org/ontologies/C2SIM#LSO">
        <rdf:type rdf:resource="http://www.sisostds.org/ontologies/C2SIM#CountryCode"/>
        <rdfs:comment>Lesotho: </rdfs:comment>
    </owl:NamedIndividual>
    


    <!-- http://www.sisostds.org/ontologies/C2SIM#LTRSNT -->

    <owl:NamedIndividual rdf:about="http://www.sisostds.org/ontologies/C2SIM#LTRSNT">
        <rdf:type rdf:resource="http://www.sisostds.org/ontologies/C2SIM#ReligionCode"/>
        <rdfs:comment>Latter-day Saints: One who adheres to or identifies with the Latter-day Saints doctrine.</rdfs:comment>
    </owl:NamedIndividual>
    


    <!-- http://www.sisostds.org/ontologies/C2SIM#LTU -->

    <owl:NamedIndividual rdf:about="http://www.sisostds.org/ontologies/C2SIM#LTU">
        <rdf:type rdf:resource="http://www.sisostds.org/ontologies/C2SIM#CountryCode"/>
        <rdfs:comment>Lithuania: </rdfs:comment>
    </owl:NamedIndividual>
    


    <!-- http://www.sisostds.org/ontologies/C2SIM#LUHYA -->

    <owl:NamedIndividual rdf:about="http://www.sisostds.org/ontologies/C2SIM#LUHYA">
        <rdf:type rdf:resource="http://www.sisostds.org/ontologies/C2SIM#EthnicGroupCode"/>
        <rdfs:comment>Luhya: The ethnic group of Luhya people.</rdfs:comment>
    </owl:NamedIndividual>
    


    <!-- http://www.sisostds.org/ontologies/C2SIM#LUO -->

    <owl:NamedIndividual rdf:about="http://www.sisostds.org/ontologies/C2SIM#LUO">
        <rdf:type rdf:resource="http://www.sisostds.org/ontologies/C2SIM#EthnicGroupCode"/>
        <rdfs:comment>Luo: The ethnic group of Luo people.</rdfs:comment>
    </owl:NamedIndividual>
    


    <!-- http://www.sisostds.org/ontologies/C2SIM#LUR -->

    <owl:NamedIndividual rdf:about="http://www.sisostds.org/ontologies/C2SIM#LUR">
        <rdf:type rdf:resource="http://www.sisostds.org/ontologies/C2SIM#EthnicGroupCode"/>
        <rdfs:comment>Lur: The ethnic group of Lur people.</rdfs:comment>
    </owl:NamedIndividual>
    


    <!-- http://www.sisostds.org/ontologies/C2SIM#LUTHRN -->

    <owl:NamedIndividual rdf:about="http://www.sisostds.org/ontologies/C2SIM#LUTHRN">
        <rdf:type rdf:resource="http://www.sisostds.org/ontologies/C2SIM#ReligionCode"/>
        <rdfs:comment>Lutheran: One who adheres to or identifies with the Lutheran doctrine.</rdfs:comment>
    </owl:NamedIndividual>
    


    <!-- http://www.sisostds.org/ontologies/C2SIM#LUX -->

    <owl:NamedIndividual rdf:about="http://www.sisostds.org/ontologies/C2SIM#LUX">
        <rdf:type rdf:resource="http://www.sisostds.org/ontologies/C2SIM#CountryCode"/>
        <rdfs:comment>Luxembourg: </rdfs:comment>
    </owl:NamedIndividual>
    


    <!-- http://www.sisostds.org/ontologies/C2SIM#LVA -->

    <owl:NamedIndividual rdf:about="http://www.sisostds.org/ontologies/C2SIM#LVA">
        <rdf:type rdf:resource="http://www.sisostds.org/ontologies/C2SIM#CountryCode"/>
        <rdfs:comment>Latvia: </rdfs:comment>
    </owl:NamedIndividual>
    


    <!-- http://www.sisostds.org/ontologies/C2SIM#MAC -->

    <owl:NamedIndividual rdf:about="http://www.sisostds.org/ontologies/C2SIM#MAC">
        <rdf:type rdf:resource="http://www.sisostds.org/ontologies/C2SIM#CountryCode"/>
        <rdfs:comment>Macao: </rdfs:comment>
    </owl:NamedIndividual>
    


    <!-- http://www.sisostds.org/ontologies/C2SIM#MACDNN -->

    <owl:NamedIndividual rdf:about="http://www.sisostds.org/ontologies/C2SIM#MACDNN">
        <rdf:type rdf:resource="http://www.sisostds.org/ontologies/C2SIM#EthnicGroupCode"/>
        <rdfs:comment>Macedonian: The ethnic group of Macedonian people.</rdfs:comment>
    </owl:NamedIndividual>
    


    <!-- http://www.sisostds.org/ontologies/C2SIM#MADURE -->

    <owl:NamedIndividual rdf:about="http://www.sisostds.org/ontologies/C2SIM#MADURE">
        <rdf:type rdf:resource="http://www.sisostds.org/ontologies/C2SIM#EthnicGroupCode"/>
        <rdfs:comment>Madurese: The ethnic group of Madurese people.</rdfs:comment>
    </owl:NamedIndividual>
    


    <!-- http://www.sisostds.org/ontologies/C2SIM#MAGARS -->

    <owl:NamedIndividual rdf:about="http://www.sisostds.org/ontologies/C2SIM#MAGARS">
        <rdf:type rdf:resource="http://www.sisostds.org/ontologies/C2SIM#EthnicGroupCode"/>
        <rdfs:comment>Magars: The ethnic group of Magars people.</rdfs:comment>
    </owl:NamedIndividual>
    


    <!-- http://www.sisostds.org/ontologies/C2SIM#MAKOA -->

    <owl:NamedIndividual rdf:about="http://www.sisostds.org/ontologies/C2SIM#MAKOA">
        <rdf:type rdf:resource="http://www.sisostds.org/ontologies/C2SIM#EthnicGroupCode"/>
        <rdfs:comment>Makoa: The ethnic group of Makoa people.</rdfs:comment>
    </owl:NamedIndividual>
    


    <!-- http://www.sisostds.org/ontologies/C2SIM#MALAGA -->

    <owl:NamedIndividual rdf:about="http://www.sisostds.org/ontologies/C2SIM#MALAGA">
        <rdf:type rdf:resource="http://www.sisostds.org/ontologies/C2SIM#EthnicGroupCode"/>
        <rdfs:comment>Malagasy: The ethnic group of Malagasy people.</rdfs:comment>
    </owl:NamedIndividual>
    


    <!-- http://www.sisostds.org/ontologies/C2SIM#MALATN -->

    <owl:NamedIndividual rdf:about="http://www.sisostds.org/ontologies/C2SIM#MALATN">
        <rdf:type rdf:resource="http://www.sisostds.org/ontologies/C2SIM#EthnicGroupCode"/>
        <rdfs:comment>Malaitian: The ethnic group of Malaitian people.</rdfs:comment>
    </owl:NamedIndividual>
    


    <!-- http://www.sisostds.org/ontologies/C2SIM#MALAY -->

    <owl:NamedIndividual rdf:about="http://www.sisostds.org/ontologies/C2SIM#MALAY">
        <rdf:type rdf:resource="http://www.sisostds.org/ontologies/C2SIM#EthnicGroupCode"/>
        <rdfs:comment>Malay/Malayan: The ethnic group of Malay/Malayan people.</rdfs:comment>
    </owl:NamedIndividual>
    


    <!-- http://www.sisostds.org/ontologies/C2SIM#MALAYA -->

    <owl:NamedIndividual rdf:about="http://www.sisostds.org/ontologies/C2SIM#MALAYA">
        <rdf:type rdf:resource="http://www.sisostds.org/ontologies/C2SIM#EthnicGroupCode"/>
        <rdfs:comment>Malaya-Indonesian (Betwileo): The ethnic group of Malaya-Indonesian (Betwileo) people.</rdfs:comment>
    </owl:NamedIndividual>
    


    <!-- http://www.sisostds.org/ontologies/C2SIM#MALAYI -->

    <owl:NamedIndividual rdf:about="http://www.sisostds.org/ontologies/C2SIM#MALAYI">
        <rdf:type rdf:resource="http://www.sisostds.org/ontologies/C2SIM#EthnicGroupCode"/>
        <rdfs:comment>Malayo-Indonesian: The ethnic group of Malayo-Indonesian people.</rdfs:comment>
    </owl:NamedIndividual>
    


    <!-- http://www.sisostds.org/ontologies/C2SIM#MALAYM -->

    <owl:NamedIndividual rdf:about="http://www.sisostds.org/ontologies/C2SIM#MALAYM">
        <rdf:type rdf:resource="http://www.sisostds.org/ontologies/C2SIM#EthnicGroupCode"/>
        <rdfs:comment>Malayo-Indonesian (Merina): The ethnic group of Malayo-Indonesian (Merina) people.</rdfs:comment>
    </owl:NamedIndividual>
    


    <!-- http://www.sisostds.org/ontologies/C2SIM#MALCHN -->

    <owl:NamedIndividual rdf:about="http://www.sisostds.org/ontologies/C2SIM#MALCHN">
        <rdf:type rdf:resource="http://www.sisostds.org/ontologies/C2SIM#EthnicGroupCode"/>
        <rdfs:comment>Malaysian Chinese: The ethnic group of Malaysian Chinese people.</rdfs:comment>
    </owl:NamedIndividual>
    


    <!-- http://www.sisostds.org/ontologies/C2SIM#MALINK -->

    <owl:NamedIndividual rdf:about="http://www.sisostds.org/ontologies/C2SIM#MALINK">
        <rdf:type rdf:resource="http://www.sisostds.org/ontologies/C2SIM#EthnicGroupCode"/>
        <rdfs:comment>Malinke: The ethnic group of Malinke people.</rdfs:comment>
    </owl:NamedIndividual>
    


    <!-- http://www.sisostds.org/ontologies/C2SIM#MALTSE -->

    <owl:NamedIndividual rdf:about="http://www.sisostds.org/ontologies/C2SIM#MALTSE">
        <rdf:type rdf:resource="http://www.sisostds.org/ontologies/C2SIM#EthnicGroupCode"/>
        <rdfs:comment>Maltese: The ethnic group of Maltese people.</rdfs:comment>
    </owl:NamedIndividual>
    


    <!-- http://www.sisostds.org/ontologies/C2SIM#MALVAN -->

    <owl:NamedIndividual rdf:about="http://www.sisostds.org/ontologies/C2SIM#MALVAN">
        <rdf:type rdf:resource="http://www.sisostds.org/ontologies/C2SIM#EthnicGroupCode"/>
        <rdfs:comment>Malvinian (Spanish-speaking Falkland Islander): The ethnic group of Malvinian (Spanish-speaking Falkland Islander) people.</rdfs:comment>
    </owl:NamedIndividual>
    


    <!-- http://www.sisostds.org/ontologies/C2SIM#MAN -->

    <owl:NamedIndividual rdf:about="http://www.sisostds.org/ontologies/C2SIM#MAN">
        <rdf:type rdf:resource="http://www.sisostds.org/ontologies/C2SIM#EthnicGroupCode"/>
        <rdfs:comment>Man: The ethnic group of Man people.</rdfs:comment>
    </owl:NamedIndividual>
    


    <!-- http://www.sisostds.org/ontologies/C2SIM#MANCHU -->

    <owl:NamedIndividual rdf:about="http://www.sisostds.org/ontologies/C2SIM#MANCHU">
        <rdf:type rdf:resource="http://www.sisostds.org/ontologies/C2SIM#EthnicGroupCode"/>
        <rdfs:comment>Manchu: The ethnic group of Manchu people.</rdfs:comment>
    </owl:NamedIndividual>
    


    <!-- http://www.sisostds.org/ontologies/C2SIM#MANDE -->

    <owl:NamedIndividual rdf:about="http://www.sisostds.org/ontologies/C2SIM#MANDE">
        <rdf:type rdf:resource="http://www.sisostds.org/ontologies/C2SIM#EthnicGroupCode"/>
        <rdfs:comment>Mande: The ethnic group of Mande people.</rdfs:comment>
    </owl:NamedIndividual>
    


    <!-- http://www.sisostds.org/ontologies/C2SIM#MANDEA -->

    <owl:NamedIndividual rdf:about="http://www.sisostds.org/ontologies/C2SIM#MANDEA">
        <rdf:type rdf:resource="http://www.sisostds.org/ontologies/C2SIM#ReligionCode"/>
        <rdfs:comment>Mandeaen: One who adheres to or identifies with the Mandeaen doctrine.</rdfs:comment>
    </owl:NamedIndividual>
    


    <!-- http://www.sisostds.org/ontologies/C2SIM#MANDEB -->

    <owl:NamedIndividual rdf:about="http://www.sisostds.org/ontologies/C2SIM#MANDEB">
        <rdf:type rdf:resource="http://www.sisostds.org/ontologies/C2SIM#EthnicGroupCode"/>
        <rdfs:comment>Mande (Bambara): The ethnic group of Mande (Bambara) people.</rdfs:comment>
    </owl:NamedIndividual>
    


    <!-- http://www.sisostds.org/ontologies/C2SIM#MANDEM -->

    <owl:NamedIndividual rdf:about="http://www.sisostds.org/ontologies/C2SIM#MANDEM">
        <rdf:type rdf:resource="http://www.sisostds.org/ontologies/C2SIM#EthnicGroupCode"/>
        <rdfs:comment>Mande (Malinke): The ethnic group of Mande (Malinke) people.</rdfs:comment>
    </owl:NamedIndividual>
    


    <!-- http://www.sisostds.org/ontologies/C2SIM#MANDES -->

    <owl:NamedIndividual rdf:about="http://www.sisostds.org/ontologies/C2SIM#MANDES">
        <rdf:type rdf:resource="http://www.sisostds.org/ontologies/C2SIM#EthnicGroupCode"/>
        <rdfs:comment>Mande (Sarakole): The ethnic group of Mande (Sarakole) people.</rdfs:comment>
    </owl:NamedIndividual>
    


    <!-- http://www.sisostds.org/ontologies/C2SIM#MANDJI -->

    <owl:NamedIndividual rdf:about="http://www.sisostds.org/ontologies/C2SIM#MANDJI">
        <rdf:type rdf:resource="http://www.sisostds.org/ontologies/C2SIM#EthnicGroupCode"/>
        <rdfs:comment>Mandjia: The ethnic group of Mandjia people.</rdfs:comment>
    </owl:NamedIndividual>
    


    <!-- http://www.sisostds.org/ontologies/C2SIM#MANDNG -->

    <owl:NamedIndividual rdf:about="http://www.sisostds.org/ontologies/C2SIM#MANDNG">
        <rdf:type rdf:resource="http://www.sisostds.org/ontologies/C2SIM#EthnicGroupCode"/>
        <rdfs:comment>Mandingo: The ethnic group of Mandingo people.</rdfs:comment>
    </owl:NamedIndividual>
    


    <!-- http://www.sisostds.org/ontologies/C2SIM#MANGIS -->

    <owl:NamedIndividual rdf:about="http://www.sisostds.org/ontologies/C2SIM#MANGIS">
        <rdf:type rdf:resource="http://www.sisostds.org/ontologies/C2SIM#EthnicGroupCode"/>
        <rdfs:comment>Mangaia Islander: The ethnic group of Mangaia Islander people.</rdfs:comment>
    </owl:NamedIndividual>
    


    <!-- http://www.sisostds.org/ontologies/C2SIM#MANHIS -->

    <owl:NamedIndividual rdf:about="http://www.sisostds.org/ontologies/C2SIM#MANHIS">
        <rdf:type rdf:resource="http://www.sisostds.org/ontologies/C2SIM#EthnicGroupCode"/>
        <rdfs:comment>Manihiki Islander: The ethnic group of Manihiki Islander people.</rdfs:comment>
    </owl:NamedIndividual>
    


    <!-- http://www.sisostds.org/ontologies/C2SIM#MANUIS -->

    <owl:NamedIndividual rdf:about="http://www.sisostds.org/ontologies/C2SIM#MANUIS">
        <rdf:type rdf:resource="http://www.sisostds.org/ontologies/C2SIM#EthnicGroupCode"/>
        <rdfs:comment>Manus Islander: The ethnic group of Manus Islander people.</rdfs:comment>
    </owl:NamedIndividual>
    


    <!-- http://www.sisostds.org/ontologies/C2SIM#MANX -->

    <owl:NamedIndividual rdf:about="http://www.sisostds.org/ontologies/C2SIM#MANX">
        <rdf:type rdf:resource="http://www.sisostds.org/ontologies/C2SIM#EthnicGroupCode"/>
        <rdfs:comment>Manx: The ethnic group of Manx people.</rdfs:comment>
    </owl:NamedIndividual>
    


    <!-- http://www.sisostds.org/ontologies/C2SIM#MAORI -->

    <owl:NamedIndividual rdf:about="http://www.sisostds.org/ontologies/C2SIM#MAORI">
        <rdf:type rdf:resource="http://www.sisostds.org/ontologies/C2SIM#EthnicGroupCode"/>
        <rdfs:comment>Maori: The ethnic group of Maori people.</rdfs:comment>
    </owl:NamedIndividual>
    


    <!-- http://www.sisostds.org/ontologies/C2SIM#MAR -->

    <owl:NamedIndividual rdf:about="http://www.sisostds.org/ontologies/C2SIM#MAR">
        <rdf:type rdf:resource="http://www.sisostds.org/ontologies/C2SIM#CountryCode"/>
        <rdfs:comment>Morocco: </rdfs:comment>
    </owl:NamedIndividual>
    


    <!-- http://www.sisostds.org/ontologies/C2SIM#MARISL -->

    <owl:NamedIndividual rdf:about="http://www.sisostds.org/ontologies/C2SIM#MARISL">
        <rdf:type rdf:resource="http://www.sisostds.org/ontologies/C2SIM#EthnicGroupCode"/>
        <rdfs:comment>Marianas Islander: The ethnic group of Marianas Islander people.</rdfs:comment>
    </owl:NamedIndividual>
    


    <!-- http://www.sisostds.org/ontologies/C2SIM#MARONT -->

    <owl:NamedIndividual rdf:about="http://www.sisostds.org/ontologies/C2SIM#MARONT">
        <rdf:type rdf:resource="http://www.sisostds.org/ontologies/C2SIM#ReligionCode"/>
        <rdfs:comment>Maronite: One who adheres to or identifies with the Maronite doctrine.</rdfs:comment>
    </owl:NamedIndividual>
    


    <!-- http://www.sisostds.org/ontologies/C2SIM#MARQIS -->

    <owl:NamedIndividual rdf:about="http://www.sisostds.org/ontologies/C2SIM#MARQIS">
        <rdf:type rdf:resource="http://www.sisostds.org/ontologies/C2SIM#EthnicGroupCode"/>
        <rdfs:comment>Marquesas Islander: The ethnic group of Marquesas Islander people.</rdfs:comment>
    </owl:NamedIndividual>
    


    <!-- http://www.sisostds.org/ontologies/C2SIM#MARSIS -->

    <owl:NamedIndividual rdf:about="http://www.sisostds.org/ontologies/C2SIM#MARSIS">
        <rdf:type rdf:resource="http://www.sisostds.org/ontologies/C2SIM#EthnicGroupCode"/>
        <rdfs:comment>Marshall Islander: The ethnic group of Marshall Islander people.</rdfs:comment>
    </owl:NamedIndividual>
    


    <!-- http://www.sisostds.org/ontologies/C2SIM#MASSA -->

    <owl:NamedIndividual rdf:about="http://www.sisostds.org/ontologies/C2SIM#MASSA">
        <rdf:type rdf:resource="http://www.sisostds.org/ontologies/C2SIM#EthnicGroupCode"/>
        <rdfs:comment>Massa: The ethnic group of Massa people.</rdfs:comment>
    </owl:NamedIndividual>
    


    <!-- http://www.sisostds.org/ontologies/C2SIM#MAUKIS -->

    <owl:NamedIndividual rdf:about="http://www.sisostds.org/ontologies/C2SIM#MAUKIS">
        <rdf:type rdf:resource="http://www.sisostds.org/ontologies/C2SIM#EthnicGroupCode"/>
        <rdfs:comment>Mauke Islander: The ethnic group of Mauke Islander people.</rdfs:comment>
    </owl:NamedIndividual>
    


    <!-- http://www.sisostds.org/ontologies/C2SIM#MAUR -->

    <owl:NamedIndividual rdf:about="http://www.sisostds.org/ontologies/C2SIM#MAUR">
        <rdf:type rdf:resource="http://www.sisostds.org/ontologies/C2SIM#EthnicGroupCode"/>
        <rdfs:comment>Maur: The ethnic group of Maur people.</rdfs:comment>
    </owl:NamedIndividual>
    


    <!-- http://www.sisostds.org/ontologies/C2SIM#MAURTN -->

    <owl:NamedIndividual rdf:about="http://www.sisostds.org/ontologies/C2SIM#MAURTN">
        <rdf:type rdf:resource="http://www.sisostds.org/ontologies/C2SIM#EthnicGroupCode"/>
        <rdfs:comment>Mauritian: The ethnic group of Mauritian people.</rdfs:comment>
    </owl:NamedIndividual>
    


    <!-- http://www.sisostds.org/ontologies/C2SIM#MAYA -->

    <owl:NamedIndividual rdf:about="http://www.sisostds.org/ontologies/C2SIM#MAYA">
        <rdf:type rdf:resource="http://www.sisostds.org/ontologies/C2SIM#EthnicGroupCode"/>
        <rdfs:comment>Maya: The ethnic group of Maya people.</rdfs:comment>
    </owl:NamedIndividual>
    


    <!-- http://www.sisostds.org/ontologies/C2SIM#MAZAND -->

    <owl:NamedIndividual rdf:about="http://www.sisostds.org/ontologies/C2SIM#MAZAND">
        <rdf:type rdf:resource="http://www.sisostds.org/ontologies/C2SIM#EthnicGroupCode"/>
        <rdfs:comment>Mazandarani: The ethnic group of Mazandarani people.</rdfs:comment>
    </owl:NamedIndividual>
    


    <!-- http://www.sisostds.org/ontologies/C2SIM#MBAKA -->

    <owl:NamedIndividual rdf:about="http://www.sisostds.org/ontologies/C2SIM#MBAKA">
        <rdf:type rdf:resource="http://www.sisostds.org/ontologies/C2SIM#EthnicGroupCode"/>
        <rdfs:comment>Mbaka: The ethnic group of Mbaka people.</rdfs:comment>
    </owl:NamedIndividual>
    


    <!-- http://www.sisostds.org/ontologies/C2SIM#MBAYE -->

    <owl:NamedIndividual rdf:about="http://www.sisostds.org/ontologies/C2SIM#MBAYE">
        <rdf:type rdf:resource="http://www.sisostds.org/ontologies/C2SIM#EthnicGroupCode"/>
        <rdfs:comment>Mbaye: The ethnic group of Mbaye people.</rdfs:comment>
    </owl:NamedIndividual>
    


    <!-- http://www.sisostds.org/ontologies/C2SIM#MBOCHI -->

    <owl:NamedIndividual rdf:about="http://www.sisostds.org/ontologies/C2SIM#MBOCHI">
        <rdf:type rdf:resource="http://www.sisostds.org/ontologies/C2SIM#EthnicGroupCode"/>
        <rdfs:comment>Mbochi: The ethnic group of Mbochi people.</rdfs:comment>
    </owl:NamedIndividual>
    


    <!-- http://www.sisostds.org/ontologies/C2SIM#MBOUM -->

    <owl:NamedIndividual rdf:about="http://www.sisostds.org/ontologies/C2SIM#MBOUM">
        <rdf:type rdf:resource="http://www.sisostds.org/ontologies/C2SIM#EthnicGroupCode"/>
        <rdfs:comment>Mboum: The ethnic group of Mboum people.</rdfs:comment>
    </owl:NamedIndividual>
    


    <!-- http://www.sisostds.org/ontologies/C2SIM#MCO -->

    <owl:NamedIndividual rdf:about="http://www.sisostds.org/ontologies/C2SIM#MCO">
        <rdf:type rdf:resource="http://www.sisostds.org/ontologies/C2SIM#CountryCode"/>
        <rdfs:comment>Monaco: </rdfs:comment>
    </owl:NamedIndividual>
    


    <!-- http://www.sisostds.org/ontologies/C2SIM#MDA -->

    <owl:NamedIndividual rdf:about="http://www.sisostds.org/ontologies/C2SIM#MDA">
        <rdf:type rdf:resource="http://www.sisostds.org/ontologies/C2SIM#CountryCode"/>
        <rdfs:comment>Moldova, Republic of: </rdfs:comment>
    </owl:NamedIndividual>
    


    <!-- http://www.sisostds.org/ontologies/C2SIM#MDENEC -->

    <owl:NamedIndividual rdf:about="http://www.sisostds.org/ontologies/C2SIM#MDENEC">
        <rdf:type rdf:resource="http://www.sisostds.org/ontologies/C2SIM#EthnicGroupCode"/>
        <rdfs:comment>Middle Eastern not elsewhere classified: The not elsewhere classified ethnic groups of Middle Eastern people.</rdfs:comment>
    </owl:NamedIndividual>
    


    <!-- http://www.sisostds.org/ontologies/C2SIM#MDENFD -->

    <owl:NamedIndividual rdf:about="http://www.sisostds.org/ontologies/C2SIM#MDENFD">
        <rdf:type rdf:resource="http://www.sisostds.org/ontologies/C2SIM#EthnicGroupCode"/>
        <rdfs:comment>Middle Eastern not further defined: The not further defined ethnic groups of Middle Eastern people.</rdfs:comment>
    </owl:NamedIndividual>
    


    <!-- http://www.sisostds.org/ontologies/C2SIM#MDG -->

    <owl:NamedIndividual rdf:about="http://www.sisostds.org/ontologies/C2SIM#MDG">
        <rdf:type rdf:resource="http://www.sisostds.org/ontologies/C2SIM#CountryCode"/>
        <rdfs:comment>Madagascar: </rdfs:comment>
    </owl:NamedIndividual>
    


    <!-- http://www.sisostds.org/ontologies/C2SIM#MDV -->

    <owl:NamedIndividual rdf:about="http://www.sisostds.org/ontologies/C2SIM#MDV">
        <rdf:type rdf:resource="http://www.sisostds.org/ontologies/C2SIM#CountryCode"/>
        <rdfs:comment>Maldives: </rdfs:comment>
    </owl:NamedIndividual>
    


    <!-- http://www.sisostds.org/ontologies/C2SIM#MEDCAL -->

    <owl:NamedIndividual rdf:about="http://www.sisostds.org/ontologies/C2SIM#MEDCAL">
        <rdf:type rdf:resource="http://www.sisostds.org/ontologies/C2SIM#OrganizationTypeCode"/>
        <rdfs:comment>Medical: A GROUP-ORGANISATION-TYPE that provides a medical service.</rdfs:comment>
    </owl:NamedIndividual>
    


    <!-- http://www.sisostds.org/ontologies/C2SIM#MEDINT -->

    <owl:NamedIndividual rdf:about="http://www.sisostds.org/ontologies/C2SIM#MEDINT">
        <rdf:type rdf:resource="http://www.sisostds.org/ontologies/C2SIM#OrganizationTypeCode"/>
        <rdfs:comment>Media, international: A GROUP-ORGANISATION-TYPE that comprises persons that report for international mass communications, but do not take part in</rdfs:comment>
    </owl:NamedIndividual>
    


    <!-- http://www.sisostds.org/ontologies/C2SIM#MEDLCL -->

    <owl:NamedIndividual rdf:about="http://www.sisostds.org/ontologies/C2SIM#MEDLCL">
        <rdf:type rdf:resource="http://www.sisostds.org/ontologies/C2SIM#OrganizationTypeCode"/>
        <rdfs:comment>Media, local: A GROUP-ORGANISATION-TYPE that comprises persons that report for local mass communications, but do not take part in the actions.</rdfs:comment>
    </owl:NamedIndividual>
    


    <!-- http://www.sisostds.org/ontologies/C2SIM#MEDNAT -->

    <owl:NamedIndividual rdf:about="http://www.sisostds.org/ontologies/C2SIM#MEDNAT">
        <rdf:type rdf:resource="http://www.sisostds.org/ontologies/C2SIM#OrganizationTypeCode"/>
        <rdfs:comment>Media, national: A GROUP-ORGANISATION-TYPE that comprises persons that report for national mass communications, but do not take part in the</rdfs:comment>
    </owl:NamedIndividual>
    


    <!-- http://www.sisostds.org/ontologies/C2SIM#MEDNOS -->

    <owl:NamedIndividual rdf:about="http://www.sisostds.org/ontologies/C2SIM#MEDNOS">
        <rdf:type rdf:resource="http://www.sisostds.org/ontologies/C2SIM#OrganizationTypeCode"/>
        <rdfs:comment>Media, not otherwise specified: A GROUP-ORGANISATION-TYPE that comprises persons that report for mass communications (especially television, radio, and newspapers)</rdfs:comment>
    </owl:NamedIndividual>
    


    <!-- http://www.sisostds.org/ontologies/C2SIM#MELANE -->

    <owl:NamedIndividual rdf:about="http://www.sisostds.org/ontologies/C2SIM#MELANE">
        <rdf:type rdf:resource="http://www.sisostds.org/ontologies/C2SIM#EthnicGroupCode"/>
        <rdfs:comment>Melanesian: The ethnic group of Melanesian people.</rdfs:comment>
    </owl:NamedIndividual>
    


    <!-- http://www.sisostds.org/ontologies/C2SIM#MENNTE -->

    <owl:NamedIndividual rdf:about="http://www.sisostds.org/ontologies/C2SIM#MENNTE">
        <rdf:type rdf:resource="http://www.sisostds.org/ontologies/C2SIM#ReligionCode"/>
        <rdfs:comment>Mennonite: One who adheres to or identifies with the Mennonite doctrine.</rdfs:comment>
    </owl:NamedIndividual>
    


    <!-- http://www.sisostds.org/ontologies/C2SIM#MEO -->

    <owl:NamedIndividual rdf:about="http://www.sisostds.org/ontologies/C2SIM#MEO">
        <rdf:type rdf:resource="http://www.sisostds.org/ontologies/C2SIM#EthnicGroupCode"/>
        <rdfs:comment>Meo: The ethnic group of Meo people.</rdfs:comment>
    </owl:NamedIndividual>
    


    <!-- http://www.sisostds.org/ontologies/C2SIM#MERU -->

    <owl:NamedIndividual rdf:about="http://www.sisostds.org/ontologies/C2SIM#MERU">
        <rdf:type rdf:resource="http://www.sisostds.org/ontologies/C2SIM#EthnicGroupCode"/>
        <rdfs:comment>Meru: The ethnic group of Meru people.</rdfs:comment>
    </owl:NamedIndividual>
    


    <!-- http://www.sisostds.org/ontologies/C2SIM#MESTZE -->

    <owl:NamedIndividual rdf:about="http://www.sisostds.org/ontologies/C2SIM#MESTZE">
        <rdf:type rdf:resource="http://www.sisostds.org/ontologies/C2SIM#EthnicGroupCode"/>
        <rdfs:comment>Mestizo (Indian and European): The ethnic group of Mestizo (Indian and European) people.</rdfs:comment>
    </owl:NamedIndividual>
    


    <!-- http://www.sisostds.org/ontologies/C2SIM#MESTZS -->

    <owl:NamedIndividual rdf:about="http://www.sisostds.org/ontologies/C2SIM#MESTZS">
        <rdf:type rdf:resource="http://www.sisostds.org/ontologies/C2SIM#EthnicGroupCode"/>
        <rdfs:comment>Mestizo (Indian and Spanish): The ethnic group of Mestizo (Indian and Spanish) people.</rdfs:comment>
    </owl:NamedIndividual>
    


    <!-- http://www.sisostds.org/ontologies/C2SIM#METHDS -->

    <owl:NamedIndividual rdf:about="http://www.sisostds.org/ontologies/C2SIM#METHDS">
        <rdf:type rdf:resource="http://www.sisostds.org/ontologies/C2SIM#ReligionCode"/>
        <rdfs:comment>Methodist: One who adheres to or identifies with the Methodist doctrine.</rdfs:comment>
    </owl:NamedIndividual>
    


    <!-- http://www.sisostds.org/ontologies/C2SIM#MEX -->

    <owl:NamedIndividual rdf:about="http://www.sisostds.org/ontologies/C2SIM#MEX">
        <rdf:type rdf:resource="http://www.sisostds.org/ontologies/C2SIM#CountryCode"/>
        <rdfs:comment>Mexico: </rdfs:comment>
    </owl:NamedIndividual>
    


    <!-- http://www.sisostds.org/ontologies/C2SIM#MEXCAN -->

    <owl:NamedIndividual rdf:about="http://www.sisostds.org/ontologies/C2SIM#MEXCAN">
        <rdf:type rdf:resource="http://www.sisostds.org/ontologies/C2SIM#EthnicGroupCode"/>
        <rdfs:comment>Mexican: The ethnic group of Mexican people.</rdfs:comment>
    </owl:NamedIndividual>
    


    <!-- http://www.sisostds.org/ontologies/C2SIM#MHL -->

    <owl:NamedIndividual rdf:about="http://www.sisostds.org/ontologies/C2SIM#MHL">
        <rdf:type rdf:resource="http://www.sisostds.org/ontologies/C2SIM#CountryCode"/>
        <rdfs:comment>Marshall Islands: </rdfs:comment>
    </owl:NamedIndividual>
    


    <!-- http://www.sisostds.org/ontologies/C2SIM#MIAO -->

    <owl:NamedIndividual rdf:about="http://www.sisostds.org/ontologies/C2SIM#MIAO">
        <rdf:type rdf:resource="http://www.sisostds.org/ontologies/C2SIM#EthnicGroupCode"/>
        <rdfs:comment>Miao: The ethnic group of Miao people.</rdfs:comment>
    </owl:NamedIndividual>
    


    <!-- http://www.sisostds.org/ontologies/C2SIM#MICRON -->

    <owl:NamedIndividual rdf:about="http://www.sisostds.org/ontologies/C2SIM#MICRON">
        <rdf:type rdf:resource="http://www.sisostds.org/ontologies/C2SIM#EthnicGroupCode"/>
        <rdfs:comment>Micronesian: The ethnic group of Micronesian people.</rdfs:comment>
    </owl:NamedIndividual>
    


    <!-- http://www.sisostds.org/ontologies/C2SIM#MINA -->

    <owl:NamedIndividual rdf:about="http://www.sisostds.org/ontologies/C2SIM#MINA">
        <rdf:type rdf:resource="http://www.sisostds.org/ontologies/C2SIM#EthnicGroupCode"/>
        <rdfs:comment>Mina: The ethnic group of Mina people.</rdfs:comment>
    </owl:NamedIndividual>
    


    <!-- http://www.sisostds.org/ontologies/C2SIM#MITISL -->

    <owl:NamedIndividual rdf:about="http://www.sisostds.org/ontologies/C2SIM#MITISL">
        <rdf:type rdf:resource="http://www.sisostds.org/ontologies/C2SIM#EthnicGroupCode"/>
        <rdfs:comment>Mitiaro Islander: The ethnic group of Mitiaro Islander people.</rdfs:comment>
    </owl:NamedIndividual>
    


    <!-- http://www.sisostds.org/ontologies/C2SIM#MIXED -->

    <owl:NamedIndividual rdf:about="http://www.sisostds.org/ontologies/C2SIM#MIXED">
        <rdf:type rdf:resource="http://www.sisostds.org/ontologies/C2SIM#EthnicGroupCode"/>
        <rdfs:comment>Mixed: The ethnic group of Mixed people.</rdfs:comment>
    </owl:NamedIndividual>
    


    <!-- http://www.sisostds.org/ontologies/C2SIM#MKD -->

    <owl:NamedIndividual rdf:about="http://www.sisostds.org/ontologies/C2SIM#MKD">
        <rdf:type rdf:resource="http://www.sisostds.org/ontologies/C2SIM#CountryCode"/>
        <rdfs:comment>Macedonia, the former Yugoslav Republic of: </rdfs:comment>
    </owl:NamedIndividual>
    


    <!-- http://www.sisostds.org/ontologies/C2SIM#MLI -->

    <owl:NamedIndividual rdf:about="http://www.sisostds.org/ontologies/C2SIM#MLI">
        <rdf:type rdf:resource="http://www.sisostds.org/ontologies/C2SIM#CountryCode"/>
        <rdfs:comment>Mali: </rdfs:comment>
    </owl:NamedIndividual>
    


    <!-- http://www.sisostds.org/ontologies/C2SIM#MLT -->

    <owl:NamedIndividual rdf:about="http://www.sisostds.org/ontologies/C2SIM#MLT">
        <rdf:type rdf:resource="http://www.sisostds.org/ontologies/C2SIM#CountryCode"/>
        <rdfs:comment>Malta: </rdfs:comment>
    </owl:NamedIndividual>
    


    <!-- http://www.sisostds.org/ontologies/C2SIM#MMR -->

    <owl:NamedIndividual rdf:about="http://www.sisostds.org/ontologies/C2SIM#MMR">
        <rdf:type rdf:resource="http://www.sisostds.org/ontologies/C2SIM#CountryCode"/>
        <rdfs:comment>Myanmar: Formerly Burma (1989)</rdfs:comment>
    </owl:NamedIndividual>
    


    <!-- http://www.sisostds.org/ontologies/C2SIM#MNE -->

    <owl:NamedIndividual rdf:about="http://www.sisostds.org/ontologies/C2SIM#MNE">
        <rdf:type rdf:resource="http://www.sisostds.org/ontologies/C2SIM#CountryCode"/>
        <rdfs:comment>Montenegro: New entry after split of Serbia and Montenegro.</rdfs:comment>
    </owl:NamedIndividual>
    


    <!-- http://www.sisostds.org/ontologies/C2SIM#MNG -->

    <owl:NamedIndividual rdf:about="http://www.sisostds.org/ontologies/C2SIM#MNG">
        <rdf:type rdf:resource="http://www.sisostds.org/ontologies/C2SIM#CountryCode"/>
        <rdfs:comment>Mongolia: </rdfs:comment>
    </owl:NamedIndividual>
    


    <!-- http://www.sisostds.org/ontologies/C2SIM#MNP -->

    <owl:NamedIndividual rdf:about="http://www.sisostds.org/ontologies/C2SIM#MNP">
        <rdf:type rdf:resource="http://www.sisostds.org/ontologies/C2SIM#CountryCode"/>
        <rdfs:comment>Northern Mariana Islands: </rdfs:comment>
    </owl:NamedIndividual>
    


    <!-- http://www.sisostds.org/ontologies/C2SIM#MODKNG -->

    <owl:NamedIndividual rdf:about="http://www.sisostds.org/ontologies/C2SIM#MODKNG">
        <rdf:type rdf:resource="http://www.sisostds.org/ontologies/C2SIM#ReligionCode"/>
        <rdfs:comment>Modekngei: One who adheres to or identifies with the Modekngei doctrine.</rdfs:comment>
    </owl:NamedIndividual>
    


    <!-- http://www.sisostds.org/ontologies/C2SIM#MOLDOV -->

    <owl:NamedIndividual rdf:about="http://www.sisostds.org/ontologies/C2SIM#MOLDOV">
        <rdf:type rdf:resource="http://www.sisostds.org/ontologies/C2SIM#EthnicGroupCode"/>
        <rdfs:comment>Moldovan: The ethnic group of Moldovan people.</rdfs:comment>
    </owl:NamedIndividual>
    


    <!-- http://www.sisostds.org/ontologies/C2SIM#MON -->

    <owl:NamedIndividual rdf:about="http://www.sisostds.org/ontologies/C2SIM#MON">
        <rdf:type rdf:resource="http://www.sisostds.org/ontologies/C2SIM#EthnicGroupCode"/>
        <rdfs:comment>Mon: The ethnic group of Mon people.</rdfs:comment>
    </owl:NamedIndividual>
    


    <!-- http://www.sisostds.org/ontologies/C2SIM#MONEGA -->

    <owl:NamedIndividual rdf:about="http://www.sisostds.org/ontologies/C2SIM#MONEGA">
        <rdf:type rdf:resource="http://www.sisostds.org/ontologies/C2SIM#EthnicGroupCode"/>
        <rdfs:comment>Monegasque: The ethnic group of Monegasque people.</rdfs:comment>
    </owl:NamedIndividual>
    


    <!-- http://www.sisostds.org/ontologies/C2SIM#MONGOL -->

    <owl:NamedIndividual rdf:about="http://www.sisostds.org/ontologies/C2SIM#MONGOL">
        <rdf:type rdf:resource="http://www.sisostds.org/ontologies/C2SIM#EthnicGroupCode"/>
        <rdfs:comment>Mongol: The ethnic group of Mongol people.</rdfs:comment>
    </owl:NamedIndividual>
    


    <!-- http://www.sisostds.org/ontologies/C2SIM#MONTEN -->

    <owl:NamedIndividual rdf:about="http://www.sisostds.org/ontologies/C2SIM#MONTEN">
        <rdf:type rdf:resource="http://www.sisostds.org/ontologies/C2SIM#EthnicGroupCode"/>
        <rdfs:comment>Montenegrins: The ethnic group of Montenegrins people.</rdfs:comment>
    </owl:NamedIndividual>
    


    <!-- http://www.sisostds.org/ontologies/C2SIM#MOOR -->

    <owl:NamedIndividual rdf:about="http://www.sisostds.org/ontologies/C2SIM#MOOR">
        <rdf:type rdf:resource="http://www.sisostds.org/ontologies/C2SIM#EthnicGroupCode"/>
        <rdfs:comment>Moor: The ethnic group of Moor people.</rdfs:comment>
    </owl:NamedIndividual>
    


    <!-- http://www.sisostds.org/ontologies/C2SIM#MORAVI -->

    <owl:NamedIndividual rdf:about="http://www.sisostds.org/ontologies/C2SIM#MORAVI">
        <rdf:type rdf:resource="http://www.sisostds.org/ontologies/C2SIM#EthnicGroupCode"/>
        <rdfs:comment>Moravian: The ethnic group of Moravian people.</rdfs:comment>
    </owl:NamedIndividual>
    


    <!-- http://www.sisostds.org/ontologies/C2SIM#MORMON -->

    <owl:NamedIndividual rdf:about="http://www.sisostds.org/ontologies/C2SIM#MORMON">
        <rdf:type rdf:resource="http://www.sisostds.org/ontologies/C2SIM#ReligionCode"/>
        <rdfs:comment>Mormon: One who adheres to or identifies with the Mormon doctrine.</rdfs:comment>
    </owl:NamedIndividual>
    


    <!-- http://www.sisostds.org/ontologies/C2SIM#MOROCN -->

    <owl:NamedIndividual rdf:about="http://www.sisostds.org/ontologies/C2SIM#MOROCN">
        <rdf:type rdf:resource="http://www.sisostds.org/ontologies/C2SIM#EthnicGroupCode"/>
        <rdfs:comment>Moroccan: The ethnic group of Moroccan people.</rdfs:comment>
    </owl:NamedIndividual>
    


    <!-- http://www.sisostds.org/ontologies/C2SIM#MOSSI -->

    <owl:NamedIndividual rdf:about="http://www.sisostds.org/ontologies/C2SIM#MOSSI">
        <rdf:type rdf:resource="http://www.sisostds.org/ontologies/C2SIM#EthnicGroupCode"/>
        <rdfs:comment>Mossi: The ethnic group of Mossi people.</rdfs:comment>
    </owl:NamedIndividual>
    


    <!-- http://www.sisostds.org/ontologies/C2SIM#MOUND -->

    <owl:NamedIndividual rdf:about="http://www.sisostds.org/ontologies/C2SIM#MOUND">
        <rdf:type rdf:resource="http://www.sisostds.org/ontologies/C2SIM#EthnicGroupCode"/>
        <rdfs:comment>Moundang: The ethnic group of Moundang people.</rdfs:comment>
    </owl:NamedIndividual>
    


    <!-- http://www.sisostds.org/ontologies/C2SIM#MOUSSE -->

    <owl:NamedIndividual rdf:about="http://www.sisostds.org/ontologies/C2SIM#MOUSSE">
        <rdf:type rdf:resource="http://www.sisostds.org/ontologies/C2SIM#EthnicGroupCode"/>
        <rdfs:comment>Moussei: The ethnic group of Moussei people.</rdfs:comment>
    </owl:NamedIndividual>
    


    <!-- http://www.sisostds.org/ontologies/C2SIM#MOZ -->

    <owl:NamedIndividual rdf:about="http://www.sisostds.org/ontologies/C2SIM#MOZ">
        <rdf:type rdf:resource="http://www.sisostds.org/ontologies/C2SIM#CountryCode"/>
        <rdfs:comment>Mozambique: </rdfs:comment>
    </owl:NamedIndividual>
    


    <!-- http://www.sisostds.org/ontologies/C2SIM#MRCHNT -->

    <owl:NamedIndividual rdf:about="http://www.sisostds.org/ontologies/C2SIM#MRCHNT">
        <rdf:type rdf:resource="http://www.sisostds.org/ontologies/C2SIM#OrganizationTypeCode"/>
        <rdfs:comment>Merchant: A GROUP-ORGANISATION-TYPE that comprises persons whose occupation is the purchase and sale of marketable commodities for profit.</rdfs:comment>
    </owl:NamedIndividual>
    


    <!-- http://www.sisostds.org/ontologies/C2SIM#MRT -->

    <owl:NamedIndividual rdf:about="http://www.sisostds.org/ontologies/C2SIM#MRT">
        <rdf:type rdf:resource="http://www.sisostds.org/ontologies/C2SIM#CountryCode"/>
        <rdfs:comment>Mauritania: </rdfs:comment>
    </owl:NamedIndividual>
    


    <!-- http://www.sisostds.org/ontologies/C2SIM#MSCWPT -->

    <owl:NamedIndividual rdf:about="http://www.sisostds.org/ontologies/C2SIM#MSCWPT">
        <rdf:type rdf:resource="http://www.sisostds.org/ontologies/C2SIM#ReligionCode"/>
        <rdfs:comment>Moscow Patriarchate: One who adheres to or identifies with the Moscow Patriarchate doctrine.</rdfs:comment>
    </owl:NamedIndividual>
    


    <!-- http://www.sisostds.org/ontologies/C2SIM#MSR -->

    <owl:NamedIndividual rdf:about="http://www.sisostds.org/ontologies/C2SIM#MSR">
        <rdf:type rdf:resource="http://www.sisostds.org/ontologies/C2SIM#CountryCode"/>
        <rdfs:comment>Montserrat: </rdfs:comment>
    </owl:NamedIndividual>
    


    <!-- http://www.sisostds.org/ontologies/C2SIM#MTQ -->

    <owl:NamedIndividual rdf:about="http://www.sisostds.org/ontologies/C2SIM#MTQ">
        <rdf:type rdf:resource="http://www.sisostds.org/ontologies/C2SIM#CountryCode"/>
        <rdfs:comment>Martinique: </rdfs:comment>
    </owl:NamedIndividual>
    


    <!-- http://www.sisostds.org/ontologies/C2SIM#MUHAJR -->

    <owl:NamedIndividual rdf:about="http://www.sisostds.org/ontologies/C2SIM#MUHAJR">
        <rdf:type rdf:resource="http://www.sisostds.org/ontologies/C2SIM#EthnicGroupCode"/>
        <rdfs:comment>Muhajir: The ethnic group of Muhajir people.</rdfs:comment>
    </owl:NamedIndividual>
    


    <!-- http://www.sisostds.org/ontologies/C2SIM#MULATT -->

    <owl:NamedIndividual rdf:about="http://www.sisostds.org/ontologies/C2SIM#MULATT">
        <rdf:type rdf:resource="http://www.sisostds.org/ontologies/C2SIM#EthnicGroupCode"/>
        <rdfs:comment>Mulatto: The ethnic group of Mulatto people.</rdfs:comment>
    </owl:NamedIndividual>
    


    <!-- http://www.sisostds.org/ontologies/C2SIM#MUONG -->

    <owl:NamedIndividual rdf:about="http://www.sisostds.org/ontologies/C2SIM#MUONG">
        <rdf:type rdf:resource="http://www.sisostds.org/ontologies/C2SIM#EthnicGroupCode"/>
        <rdfs:comment>Muong: The ethnic group of Muong people.</rdfs:comment>
    </owl:NamedIndividual>
    


    <!-- http://www.sisostds.org/ontologies/C2SIM#MUS -->

    <owl:NamedIndividual rdf:about="http://www.sisostds.org/ontologies/C2SIM#MUS">
        <rdf:type rdf:resource="http://www.sisostds.org/ontologies/C2SIM#CountryCode"/>
        <rdfs:comment>Mauritius: </rdfs:comment>
    </owl:NamedIndividual>
    


    <!-- http://www.sisostds.org/ontologies/C2SIM#MUSIMO -->

    <owl:NamedIndividual rdf:about="http://www.sisostds.org/ontologies/C2SIM#MUSIMO">
        <rdf:type rdf:resource="http://www.sisostds.org/ontologies/C2SIM#EthnicGroupCode"/>
        <rdfs:comment>Muslim (Boulala): The ethnic group of Muslim (Boulala) people.</rdfs:comment>
    </owl:NamedIndividual>
    


    <!-- http://www.sisostds.org/ontologies/C2SIM#MUSLIM -->

    <owl:NamedIndividual rdf:about="http://www.sisostds.org/ontologies/C2SIM#MUSLIM">
        <rdf:type rdf:resource="http://www.sisostds.org/ontologies/C2SIM#EthnicGroupCode"/>
        <rdf:type rdf:resource="http://www.sisostds.org/ontologies/C2SIM#ReligionCode"/>
        <rdfs:comment>Muslim: One who adheres to or identifies with the Muslim doctrine.</rdfs:comment>
        <rdfs:comment>Muslim: The ethnic group of Muslim people.</rdfs:comment>
    </owl:NamedIndividual>
    


    <!-- http://www.sisostds.org/ontologies/C2SIM#MUSLMA -->

    <owl:NamedIndividual rdf:about="http://www.sisostds.org/ontologies/C2SIM#MUSLMA">
        <rdf:type rdf:resource="http://www.sisostds.org/ontologies/C2SIM#EthnicGroupCode"/>
        <rdfs:comment>Muslim (Arab): The ethnic group of Muslim (Arab) people.</rdfs:comment>
    </owl:NamedIndividual>
    


    <!-- http://www.sisostds.org/ontologies/C2SIM#MUSLMB -->

    <owl:NamedIndividual rdf:about="http://www.sisostds.org/ontologies/C2SIM#MUSLMB">
        <rdf:type rdf:resource="http://www.sisostds.org/ontologies/C2SIM#EthnicGroupCode"/>
        <rdfs:comment>Muslim (Baguirmi): The ethnic group of Muslim (Baguirmi) people.</rdfs:comment>
    </owl:NamedIndividual>
    


    <!-- http://www.sisostds.org/ontologies/C2SIM#MUSLMF -->

    <owl:NamedIndividual rdf:about="http://www.sisostds.org/ontologies/C2SIM#MUSLMF">
        <rdf:type rdf:resource="http://www.sisostds.org/ontologies/C2SIM#EthnicGroupCode"/>
        <rdfs:comment>Muslim (Fulbe): The ethnic group of Muslim (Fulbe) people.</rdfs:comment>
    </owl:NamedIndividual>
    


    <!-- http://www.sisostds.org/ontologies/C2SIM#MUSLMH -->

    <owl:NamedIndividual rdf:about="http://www.sisostds.org/ontologies/C2SIM#MUSLMH">
        <rdf:type rdf:resource="http://www.sisostds.org/ontologies/C2SIM#EthnicGroupCode"/>
        <rdfs:comment>Muslim (Hadjerai): The ethnic group of Muslim (Hadjerai) people.</rdfs:comment>
    </owl:NamedIndividual>
    


    <!-- http://www.sisostds.org/ontologies/C2SIM#MUSLMK -->

    <owl:NamedIndividual rdf:about="http://www.sisostds.org/ontologies/C2SIM#MUSLMK">
        <rdf:type rdf:resource="http://www.sisostds.org/ontologies/C2SIM#EthnicGroupCode"/>
        <rdfs:comment>Muslim (Kanembou): The ethnic group of Muslim (Kanembou) people.</rdfs:comment>
    </owl:NamedIndividual>
    


    <!-- http://www.sisostds.org/ontologies/C2SIM#MUSLMM -->

    <owl:NamedIndividual rdf:about="http://www.sisostds.org/ontologies/C2SIM#MUSLMM">
        <rdf:type rdf:resource="http://www.sisostds.org/ontologies/C2SIM#EthnicGroupCode"/>
        <rdfs:comment>Muslim (Maba): The ethnic group of Muslim (Maba) people.</rdfs:comment>
    </owl:NamedIndividual>
    


    <!-- http://www.sisostds.org/ontologies/C2SIM#MUSLMT -->

    <owl:NamedIndividual rdf:about="http://www.sisostds.org/ontologies/C2SIM#MUSLMT">
        <rdf:type rdf:resource="http://www.sisostds.org/ontologies/C2SIM#EthnicGroupCode"/>
        <rdfs:comment>Muslim (Kotoko): The ethnic group of Muslim (Kotoko) people.</rdfs:comment>
    </owl:NamedIndividual>
    


    <!-- http://www.sisostds.org/ontologies/C2SIM#MUSLMU -->

    <owl:NamedIndividual rdf:about="http://www.sisostds.org/ontologies/C2SIM#MUSLMU">
        <rdf:type rdf:resource="http://www.sisostds.org/ontologies/C2SIM#EthnicGroupCode"/>
        <rdfs:comment>Muslim (Toubou): The ethnic group of Muslim (Toubou) people.</rdfs:comment>
    </owl:NamedIndividual>
    


    <!-- http://www.sisostds.org/ontologies/C2SIM#MUSLMY -->

    <owl:NamedIndividual rdf:about="http://www.sisostds.org/ontologies/C2SIM#MUSLMY">
        <rdf:type rdf:resource="http://www.sisostds.org/ontologies/C2SIM#EthnicGroupCode"/>
        <rdfs:comment>Muslim (Malay): The ethnic group of Muslim (Malay) people.</rdfs:comment>
    </owl:NamedIndividual>
    


    <!-- http://www.sisostds.org/ontologies/C2SIM#MUSLMZ -->

    <owl:NamedIndividual rdf:about="http://www.sisostds.org/ontologies/C2SIM#MUSLMZ">
        <rdf:type rdf:resource="http://www.sisostds.org/ontologies/C2SIM#EthnicGroupCode"/>
        <rdfs:comment>Muslim (Zaghawa): The ethnic group of Muslim (Zaghawa) people.</rdfs:comment>
    </owl:NamedIndividual>
    


    <!-- http://www.sisostds.org/ontologies/C2SIM#MUSMLY -->

    <owl:NamedIndividual rdf:about="http://www.sisostds.org/ontologies/C2SIM#MUSMLY">
        <rdf:type rdf:resource="http://www.sisostds.org/ontologies/C2SIM#ReligionCode"/>
        <rdfs:comment>Muslim (Malays): One who adheres to or identifies with the Muslim (Malays) doctrine.</rdfs:comment>
    </owl:NamedIndividual>
    


    <!-- http://www.sisostds.org/ontologies/C2SIM#MUSSHF -->

    <owl:NamedIndividual rdf:about="http://www.sisostds.org/ontologies/C2SIM#MUSSHF">
        <rdf:type rdf:resource="http://www.sisostds.org/ontologies/C2SIM#ReligionCode"/>
        <rdfs:comment>Muslim (Sha&apos;fi): One who adheres to or identifies with the Muslim (Sha&apos;fi) doctrine.</rdfs:comment>
    </owl:NamedIndividual>
    


    <!-- http://www.sisostds.org/ontologies/C2SIM#MUSZYD -->

    <owl:NamedIndividual rdf:about="http://www.sisostds.org/ontologies/C2SIM#MUSZYD">
        <rdf:type rdf:resource="http://www.sisostds.org/ontologies/C2SIM#ReligionCode"/>
        <rdfs:comment>Muslim (Zaydi): One who adheres to or identifies with the Muslim (Zaydi) doctrine.</rdfs:comment>
    </owl:NamedIndividual>
    


    <!-- http://www.sisostds.org/ontologies/C2SIM#MWI -->

    <owl:NamedIndividual rdf:about="http://www.sisostds.org/ontologies/C2SIM#MWI">
        <rdf:type rdf:resource="http://www.sisostds.org/ontologies/C2SIM#CountryCode"/>
        <rdfs:comment>Malawi: </rdfs:comment>
    </owl:NamedIndividual>
    


    <!-- http://www.sisostds.org/ontologies/C2SIM#MYS -->

    <owl:NamedIndividual rdf:about="http://www.sisostds.org/ontologies/C2SIM#MYS">
        <rdf:type rdf:resource="http://www.sisostds.org/ontologies/C2SIM#CountryCode"/>
        <rdfs:comment>Malaysia: </rdfs:comment>
    </owl:NamedIndividual>
    


    <!-- http://www.sisostds.org/ontologies/C2SIM#MYT -->

    <owl:NamedIndividual rdf:about="http://www.sisostds.org/ontologies/C2SIM#MYT">
        <rdf:type rdf:resource="http://www.sisostds.org/ontologies/C2SIM#CountryCode"/>
        <rdfs:comment>Mayotte: </rdfs:comment>
    </owl:NamedIndividual>
    


    <!-- http://www.sisostds.org/ontologies/C2SIM#MostlyOperational -->

    <owl:NamedIndividual rdf:about="http://www.sisostds.org/ontologies/C2SIM#MostlyOperational">
        <rdf:type rdf:resource="http://www.sisostds.org/ontologies/C2SIM#OperationalStatusCode"/>
    </owl:NamedIndividual>
    


    <!-- http://www.sisostds.org/ontologies/C2SIM#MoveToLocation -->

    <owl:NamedIndividual rdf:about="http://www.sisostds.org/ontologies/C2SIM#MoveToLocation">
        <rdf:type rdf:resource="http://www.sisostds.org/ontologies/C2SIM#TaskActionCode"/>
    </owl:NamedIndividual>
    <owl:Axiom>
        <owl:annotatedSource rdf:resource="http://www.sisostds.org/ontologies/C2SIM#MoveToLocation"/>
        <owl:annotatedProperty rdf:resource="http://www.w3.org/1999/02/22-rdf-syntax-ns#type"/>
        <owl:annotatedTarget rdf:resource="http://www.sisostds.org/ontologies/C2SIM#TaskActionCode"/>
        <rdfs:comment>The destination of this Movement task is defined as follows: 
-Location property of the Task.  This is a choice of coordinate values, or an entity-defined reference (or entity-relative location); entity-defined can refer to a unit or a map graphic. This is an alternate way to specify location via a map graphic; see below.
- MagGraphicID of the Task. The destination is the Location of the map graphic.</rdfs:comment>
    </owl:Axiom>
    


    <!-- http://www.sisostds.org/ontologies/C2SIM#NAINDN -->

    <owl:NamedIndividual rdf:about="http://www.sisostds.org/ontologies/C2SIM#NAINDN">
        <rdf:type rdf:resource="http://www.sisostds.org/ontologies/C2SIM#EthnicGroupCode"/>
        <rdfs:comment>North American Indian: The ethnic group of North American Indian people.</rdfs:comment>
    </owl:NamedIndividual>
    


    <!-- http://www.sisostds.org/ontologies/C2SIM#NAM -->

    <owl:NamedIndividual rdf:about="http://www.sisostds.org/ontologies/C2SIM#NAM">
        <rdf:type rdf:resource="http://www.sisostds.org/ontologies/C2SIM#CountryCode"/>
        <rdfs:comment>Namibia: </rdfs:comment>
    </owl:NamedIndividual>
    


    <!-- http://www.sisostds.org/ontologies/C2SIM#NATVEF -->

    <owl:NamedIndividual rdf:about="http://www.sisostds.org/ontologies/C2SIM#NATVEF">
        <rdf:type rdf:resource="http://www.sisostds.org/ontologies/C2SIM#EthnicGroupCode"/>
        <rdfs:comment>Native African: The ethnic group of Native African people.</rdfs:comment>
    </owl:NamedIndividual>
    


    <!-- http://www.sisostds.org/ontologies/C2SIM#NATVEM -->

    <owl:NamedIndividual rdf:about="http://www.sisostds.org/ontologies/C2SIM#NATVEM">
        <rdf:type rdf:resource="http://www.sisostds.org/ontologies/C2SIM#EthnicGroupCode"/>
        <rdfs:comment>Native American: The ethnic group of Native American people.</rdfs:comment>
    </owl:NamedIndividual>
    


    <!-- http://www.sisostds.org/ontologies/C2SIM#NAUISL -->

    <owl:NamedIndividual rdf:about="http://www.sisostds.org/ontologies/C2SIM#NAUISL">
        <rdf:type rdf:resource="http://www.sisostds.org/ontologies/C2SIM#EthnicGroupCode"/>
        <rdfs:comment>Nauru Islander: The ethnic group of Nauru Islander people.</rdfs:comment>
    </owl:NamedIndividual>
    


    <!-- http://www.sisostds.org/ontologies/C2SIM#NCL -->

    <owl:NamedIndividual rdf:about="http://www.sisostds.org/ontologies/C2SIM#NCL">
        <rdf:type rdf:resource="http://www.sisostds.org/ontologies/C2SIM#CountryCode"/>
        <rdfs:comment>New Caledonia: </rdfs:comment>
    </owl:NamedIndividual>
    


    <!-- http://www.sisostds.org/ontologies/C2SIM#NEGRIT -->

    <owl:NamedIndividual rdf:about="http://www.sisostds.org/ontologies/C2SIM#NEGRIT">
        <rdf:type rdf:resource="http://www.sisostds.org/ontologies/C2SIM#EthnicGroupCode"/>
        <rdfs:comment>Negrito: The ethnic group of Negrito people.</rdfs:comment>
    </owl:NamedIndividual>
    


    <!-- http://www.sisostds.org/ontologies/C2SIM#NEPLSE -->

    <owl:NamedIndividual rdf:about="http://www.sisostds.org/ontologies/C2SIM#NEPLSE">
        <rdf:type rdf:resource="http://www.sisostds.org/ontologies/C2SIM#EthnicGroupCode"/>
        <rdfs:comment>Nepalese: The ethnic group of Nepalese people.</rdfs:comment>
    </owl:NamedIndividual>
    


    <!-- http://www.sisostds.org/ontologies/C2SIM#NER -->

    <owl:NamedIndividual rdf:about="http://www.sisostds.org/ontologies/C2SIM#NER">
        <rdf:type rdf:resource="http://www.sisostds.org/ontologies/C2SIM#CountryCode"/>
        <rdfs:comment>Niger: </rdfs:comment>
    </owl:NamedIndividual>
    


    <!-- http://www.sisostds.org/ontologies/C2SIM#NEWARS -->

    <owl:NamedIndividual rdf:about="http://www.sisostds.org/ontologies/C2SIM#NEWARS">
        <rdf:type rdf:resource="http://www.sisostds.org/ontologies/C2SIM#EthnicGroupCode"/>
        <rdfs:comment>Newars: The ethnic group of Newars people.</rdfs:comment>
    </owl:NamedIndividual>
    


    <!-- http://www.sisostds.org/ontologies/C2SIM#NEWBRT -->

    <owl:NamedIndividual rdf:about="http://www.sisostds.org/ontologies/C2SIM#NEWBRT">
        <rdf:type rdf:resource="http://www.sisostds.org/ontologies/C2SIM#EthnicGroupCode"/>
        <rdfs:comment>New Britain Islander: The ethnic group of New Britain Islander people.</rdfs:comment>
    </owl:NamedIndividual>
    


    <!-- http://www.sisostds.org/ontologies/C2SIM#NEWCAL -->

    <owl:NamedIndividual rdf:about="http://www.sisostds.org/ontologies/C2SIM#NEWCAL">
        <rdf:type rdf:resource="http://www.sisostds.org/ontologies/C2SIM#EthnicGroupCode"/>
        <rdfs:comment>New Caledonian: The ethnic group of New Caledonian people.</rdfs:comment>
    </owl:NamedIndividual>
    


    <!-- http://www.sisostds.org/ontologies/C2SIM#NEWGER -->

    <owl:NamedIndividual rdf:about="http://www.sisostds.org/ontologies/C2SIM#NEWGER">
        <rdf:type rdf:resource="http://www.sisostds.org/ontologies/C2SIM#EthnicGroupCode"/>
        <rdfs:comment>New Georgian: The ethnic group of New Georgian people.</rdfs:comment>
    </owl:NamedIndividual>
    


    <!-- http://www.sisostds.org/ontologies/C2SIM#NEWIRL -->

    <owl:NamedIndividual rdf:about="http://www.sisostds.org/ontologies/C2SIM#NEWIRL">
        <rdf:type rdf:resource="http://www.sisostds.org/ontologies/C2SIM#EthnicGroupCode"/>
        <rdfs:comment>New Irelander: The ethnic group of New Irelander people.</rdfs:comment>
    </owl:NamedIndividual>
    


    <!-- http://www.sisostds.org/ontologies/C2SIM#NEWZEA -->

    <owl:NamedIndividual rdf:about="http://www.sisostds.org/ontologies/C2SIM#NEWZEA">
        <rdf:type rdf:resource="http://www.sisostds.org/ontologies/C2SIM#EthnicGroupCode"/>
        <rdfs:comment>New Zealander: The ethnic group of New Zealander people.</rdfs:comment>
    </owl:NamedIndividual>
    


    <!-- http://www.sisostds.org/ontologies/C2SIM#NEWZLE -->

    <owl:NamedIndividual rdf:about="http://www.sisostds.org/ontologies/C2SIM#NEWZLE">
        <rdf:type rdf:resource="http://www.sisostds.org/ontologies/C2SIM#EthnicGroupCode"/>
        <rdfs:comment>New Zealand European/Pakeha: The ethnic group of New Zealand European/Pakeha people.</rdfs:comment>
    </owl:NamedIndividual>
    


    <!-- http://www.sisostds.org/ontologies/C2SIM#NEWZLM -->

    <owl:NamedIndividual rdf:about="http://www.sisostds.org/ontologies/C2SIM#NEWZLM">
        <rdf:type rdf:resource="http://www.sisostds.org/ontologies/C2SIM#EthnicGroupCode"/>
        <rdfs:comment>New Zealand Maori: The ethnic group of New Zealand Maori people.</rdfs:comment>
    </owl:NamedIndividual>
    


    <!-- http://www.sisostds.org/ontologies/C2SIM#NFK -->

    <owl:NamedIndividual rdf:about="http://www.sisostds.org/ontologies/C2SIM#NFK">
        <rdf:type rdf:resource="http://www.sisostds.org/ontologies/C2SIM#CountryCode"/>
        <rdfs:comment>Norfolk Island: </rdfs:comment>
    </owl:NamedIndividual>
    


    <!-- http://www.sisostds.org/ontologies/C2SIM#NGA -->

    <owl:NamedIndividual rdf:about="http://www.sisostds.org/ontologies/C2SIM#NGA">
        <rdf:type rdf:resource="http://www.sisostds.org/ontologies/C2SIM#CountryCode"/>
        <rdfs:comment>Nigeria: </rdfs:comment>
    </owl:NamedIndividual>
    


    <!-- http://www.sisostds.org/ontologies/C2SIM#NGAMBY -->

    <owl:NamedIndividual rdf:about="http://www.sisostds.org/ontologies/C2SIM#NGAMBY">
        <rdf:type rdf:resource="http://www.sisostds.org/ontologies/C2SIM#EthnicGroupCode"/>
        <rdfs:comment>Ngambye: The ethnic group of Ngambye people.</rdfs:comment>
    </owl:NamedIndividual>
    


    <!-- http://www.sisostds.org/ontologies/C2SIM#NGONDE -->

    <owl:NamedIndividual rdf:about="http://www.sisostds.org/ontologies/C2SIM#NGONDE">
        <rdf:type rdf:resource="http://www.sisostds.org/ontologies/C2SIM#EthnicGroupCode"/>
        <rdfs:comment>Ngonde: The ethnic group of Ngonde people.</rdfs:comment>
    </owl:NamedIndividual>
    


    <!-- http://www.sisostds.org/ontologies/C2SIM#NGONI -->

    <owl:NamedIndividual rdf:about="http://www.sisostds.org/ontologies/C2SIM#NGONI">
        <rdf:type rdf:resource="http://www.sisostds.org/ontologies/C2SIM#EthnicGroupCode"/>
        <rdfs:comment>Ngoni: The ethnic group of Ngoni people.</rdfs:comment>
    </owl:NamedIndividual>
    


    <!-- http://www.sisostds.org/ontologies/C2SIM#NIC -->

    <owl:NamedIndividual rdf:about="http://www.sisostds.org/ontologies/C2SIM#NIC">
        <rdf:type rdf:resource="http://www.sisostds.org/ontologies/C2SIM#CountryCode"/>
        <rdfs:comment>Nicaragua: </rdfs:comment>
    </owl:NamedIndividual>
    


    <!-- http://www.sisostds.org/ontologies/C2SIM#NICRGN -->

    <owl:NamedIndividual rdf:about="http://www.sisostds.org/ontologies/C2SIM#NICRGN">
        <rdf:type rdf:resource="http://www.sisostds.org/ontologies/C2SIM#EthnicGroupCode"/>
        <rdfs:comment>Nicaraguan: The ethnic group of Nicaraguan people.</rdfs:comment>
    </owl:NamedIndividual>
    


    <!-- http://www.sisostds.org/ontologies/C2SIM#NIGRAN -->

    <owl:NamedIndividual rdf:about="http://www.sisostds.org/ontologies/C2SIM#NIGRAN">
        <rdf:type rdf:resource="http://www.sisostds.org/ontologies/C2SIM#EthnicGroupCode"/>
        <rdfs:comment>Nigerian: The ethnic group of Nigerian people.</rdfs:comment>
    </owl:NamedIndividual>
    


    <!-- http://www.sisostds.org/ontologies/C2SIM#NIU -->

    <owl:NamedIndividual rdf:about="http://www.sisostds.org/ontologies/C2SIM#NIU">
        <rdf:type rdf:resource="http://www.sisostds.org/ontologies/C2SIM#CountryCode"/>
        <rdfs:comment>Niue: </rdfs:comment>
    </owl:NamedIndividual>
    


    <!-- http://www.sisostds.org/ontologies/C2SIM#NIUEAN -->

    <owl:NamedIndividual rdf:about="http://www.sisostds.org/ontologies/C2SIM#NIUEAN">
        <rdf:type rdf:resource="http://www.sisostds.org/ontologies/C2SIM#EthnicGroupCode"/>
        <rdfs:comment>Niuean: The ethnic group of Niuean people.</rdfs:comment>
    </owl:NamedIndividual>
    


    <!-- http://www.sisostds.org/ontologies/C2SIM#NIUNCH -->

    <owl:NamedIndividual rdf:about="http://www.sisostds.org/ontologies/C2SIM#NIUNCH">
        <rdf:type rdf:resource="http://www.sisostds.org/ontologies/C2SIM#ReligionCode"/>
        <rdfs:comment>Niuean Church: One who adheres to or identifies with the Niuean Church doctrine.</rdfs:comment>
    </owl:NamedIndividual>
    


    <!-- http://www.sisostds.org/ontologies/C2SIM#NKN -->

    <owl:NamedIndividual rdf:about="http://www.sisostds.org/ontologies/C2SIM#NKN">
        <rdf:type rdf:resource="http://www.sisostds.org/ontologies/C2SIM#EthnicGroupCode"/>
        <rdf:type rdf:resource="http://www.sisostds.org/ontologies/C2SIM#OrganizationTypeCode"/>
        <rdf:type rdf:resource="http://www.sisostds.org/ontologies/C2SIM#ReligionCode"/>
        <rdfs:comment>Not known: It is not possible to determine which value is most applicable.</rdfs:comment>
    </owl:NamedIndividual>
    


    <!-- http://www.sisostds.org/ontologies/C2SIM#NLD -->

    <owl:NamedIndividual rdf:about="http://www.sisostds.org/ontologies/C2SIM#NLD">
        <rdf:type rdf:resource="http://www.sisostds.org/ontologies/C2SIM#CountryCode"/>
        <rdfs:comment>Netherlands: </rdfs:comment>
    </owl:NamedIndividual>
    


    <!-- http://www.sisostds.org/ontologies/C2SIM#NONE -->

    <owl:NamedIndividual rdf:about="http://www.sisostds.org/ontologies/C2SIM#NONE">
        <rdf:type rdf:resource="http://www.sisostds.org/ontologies/C2SIM#ReligionCode"/>
        <rdfs:comment>None: One who does not adhere to a religion.</rdfs:comment>
    </owl:NamedIndividual>
    


    <!-- http://www.sisostds.org/ontologies/C2SIM#NOR -->

    <owl:NamedIndividual rdf:about="http://www.sisostds.org/ontologies/C2SIM#NOR">
        <rdf:type rdf:resource="http://www.sisostds.org/ontologies/C2SIM#CountryCode"/>
        <rdfs:comment>Norway: </rdfs:comment>
    </owl:NamedIndividual>
    


    <!-- http://www.sisostds.org/ontologies/C2SIM#NORDIC -->

    <owl:NamedIndividual rdf:about="http://www.sisostds.org/ontologies/C2SIM#NORDIC">
        <rdf:type rdf:resource="http://www.sisostds.org/ontologies/C2SIM#EthnicGroupCode"/>
        <rdfs:comment>Nordic: The ethnic group of Nordic people.</rdfs:comment>
    </owl:NamedIndividual>
    


    <!-- http://www.sisostds.org/ontologies/C2SIM#NORMAN -->

    <owl:NamedIndividual rdf:about="http://www.sisostds.org/ontologies/C2SIM#NORMAN">
        <rdf:type rdf:resource="http://www.sisostds.org/ontologies/C2SIM#EthnicGroupCode"/>
        <rdfs:comment>Norman: The ethnic group of Norman people.</rdfs:comment>
    </owl:NamedIndividual>
    


    <!-- http://www.sisostds.org/ontologies/C2SIM#NORMFR -->

    <owl:NamedIndividual rdf:about="http://www.sisostds.org/ontologies/C2SIM#NORMFR">
        <rdf:type rdf:resource="http://www.sisostds.org/ontologies/C2SIM#EthnicGroupCode"/>
        <rdfs:comment>Norman-French: The ethnic group of Norman-French people.</rdfs:comment>
    </owl:NamedIndividual>
    


    <!-- http://www.sisostds.org/ontologies/C2SIM#NORTAF -->

    <owl:NamedIndividual rdf:about="http://www.sisostds.org/ontologies/C2SIM#NORTAF">
        <rdf:type rdf:resource="http://www.sisostds.org/ontologies/C2SIM#EthnicGroupCode"/>
        <rdfs:comment>North African: The ethnic group of North African people.</rdfs:comment>
    </owl:NamedIndividual>
    


    <!-- http://www.sisostds.org/ontologies/C2SIM#NORWGN -->

    <owl:NamedIndividual rdf:about="http://www.sisostds.org/ontologies/C2SIM#NORWGN">
        <rdf:type rdf:resource="http://www.sisostds.org/ontologies/C2SIM#EthnicGroupCode"/>
        <rdfs:comment>Norwegian: The ethnic group of Norwegian people.</rdfs:comment>
    </owl:NamedIndividual>
    


    <!-- http://www.sisostds.org/ontologies/C2SIM#NOS -->

    <owl:NamedIndividual rdf:about="http://www.sisostds.org/ontologies/C2SIM#NOS">
        <rdf:type rdf:resource="http://www.sisostds.org/ontologies/C2SIM#CountryCode"/>
        <rdf:type rdf:resource="http://www.sisostds.org/ontologies/C2SIM#EthnicGroupCode"/>
        <rdf:type rdf:resource="http://www.sisostds.org/ontologies/C2SIM#OrganizationTypeCode"/>
        <rdf:type rdf:resource="http://www.sisostds.org/ontologies/C2SIM#ReligionCode"/>
        <rdfs:comment>Not otherwise specified: The appropriate value is not in the set of specified values.</rdfs:comment>
    </owl:NamedIndividual>
    


    <!-- http://www.sisostds.org/ontologies/C2SIM#NOT_RECORDING -->

    <owl:NamedIndividual rdf:about="http://www.sisostds.org/ontologies/C2SIM#NOT_RECORDING">
        <rdf:type rdf:resource="http://www.sisostds.org/ontologies/C2SIM#RecordingStatusCode"/>
    </owl:NamedIndividual>
    


    <!-- http://www.sisostds.org/ontologies/C2SIM#NO_PLAYBACK_IN_PROGRESS -->

    <owl:NamedIndividual rdf:about="http://www.sisostds.org/ontologies/C2SIM#NO_PLAYBACK_IN_PROGRESS">
        <rdf:type rdf:resource="http://www.sisostds.org/ontologies/C2SIM#PlaybackStatusCode"/>
    </owl:NamedIndividual>
    


    <!-- http://www.sisostds.org/ontologies/C2SIM#NPL -->

    <owl:NamedIndividual rdf:about="http://www.sisostds.org/ontologies/C2SIM#NPL">
        <rdf:type rdf:resource="http://www.sisostds.org/ontologies/C2SIM#CountryCode"/>
        <rdfs:comment>Nepal: </rdfs:comment>
    </owl:NamedIndividual>
    


    <!-- http://www.sisostds.org/ontologies/C2SIM#NRU -->

    <owl:NamedIndividual rdf:about="http://www.sisostds.org/ontologies/C2SIM#NRU">
        <rdf:type rdf:resource="http://www.sisostds.org/ontologies/C2SIM#CountryCode"/>
        <rdfs:comment>Nauru: </rdfs:comment>
    </owl:NamedIndividual>
    


    <!-- http://www.sisostds.org/ontologies/C2SIM#NYANJA -->

    <owl:NamedIndividual rdf:about="http://www.sisostds.org/ontologies/C2SIM#NYANJA">
        <rdf:type rdf:resource="http://www.sisostds.org/ontologies/C2SIM#EthnicGroupCode"/>
        <rdfs:comment>Nyanja: The ethnic group of Nyanja people.</rdfs:comment>
    </owl:NamedIndividual>
    


    <!-- http://www.sisostds.org/ontologies/C2SIM#NZL -->

    <owl:NamedIndividual rdf:about="http://www.sisostds.org/ontologies/C2SIM#NZL">
        <rdf:type rdf:resource="http://www.sisostds.org/ontologies/C2SIM#CountryCode"/>
        <rdfs:comment>New Zealand: </rdfs:comment>
    </owl:NamedIndividual>
    


    <!-- http://www.sisostds.org/ontologies/C2SIM#NeutralSide -->

    <owl:NamedIndividual rdf:about="http://www.sisostds.org/ontologies/C2SIM#NeutralSide"/>
    


    <!-- http://www.sisostds.org/ontologies/C2SIM#NeutralTo -->

    <owl:NamedIndividual rdf:about="http://www.sisostds.org/ontologies/C2SIM#NeutralTo">
        <rdf:type rdf:resource="http://www.sisostds.org/ontologies/C2SIM#AllegianceRelationshipCode"/>
    </owl:NamedIndividual>
    


    <!-- http://www.sisostds.org/ontologies/C2SIM#NotOperational -->

    <owl:NamedIndividual rdf:about="http://www.sisostds.org/ontologies/C2SIM#NotOperational">
        <rdf:type rdf:resource="http://www.sisostds.org/ontologies/C2SIM#OperationalStatusCode"/>
    </owl:NamedIndividual>
    


    <!-- http://www.sisostds.org/ontologies/C2SIM#OAFNEC -->

    <owl:NamedIndividual rdf:about="http://www.sisostds.org/ontologies/C2SIM#OAFNEC">
        <rdf:type rdf:resource="http://www.sisostds.org/ontologies/C2SIM#EthnicGroupCode"/>
        <rdfs:comment>Other African not elsewhere classified: The ethnic group of Other African not elsewhere classified people.</rdfs:comment>
    </owl:NamedIndividual>
    


    <!-- http://www.sisostds.org/ontologies/C2SIM#OASNEC -->

    <owl:NamedIndividual rdf:about="http://www.sisostds.org/ontologies/C2SIM#OASNEC">
        <rdf:type rdf:resource="http://www.sisostds.org/ontologies/C2SIM#EthnicGroupCode"/>
        <rdfs:comment>Other Asian not elsewhere classified: The ethnic group of Other Asian not elsewhere classified people.</rdfs:comment>
    </owl:NamedIndividual>
    


    <!-- http://www.sisostds.org/ontologies/C2SIM#OCNISL -->

    <owl:NamedIndividual rdf:about="http://www.sisostds.org/ontologies/C2SIM#OCNISL">
        <rdf:type rdf:resource="http://www.sisostds.org/ontologies/C2SIM#EthnicGroupCode"/>
        <rdfs:comment>Ocean Islander/Banaban: The ethnic group of Ocean Islander/Banaban people.</rdfs:comment>
    </owl:NamedIndividual>
    


    <!-- http://www.sisostds.org/ontologies/C2SIM#OEUNFD -->

    <owl:NamedIndividual rdf:about="http://www.sisostds.org/ontologies/C2SIM#OEUNFD">
        <rdf:type rdf:resource="http://www.sisostds.org/ontologies/C2SIM#EthnicGroupCode"/>
        <rdfs:comment>Other European not further defined: The ethnic group of Other European not further defined people.</rdfs:comment>
    </owl:NamedIndividual>
    


    <!-- http://www.sisostds.org/ontologies/C2SIM#OIMATS -->

    <owl:NamedIndividual rdf:about="http://www.sisostds.org/ontologies/C2SIM#OIMATS">
        <rdf:type rdf:resource="http://www.sisostds.org/ontologies/C2SIM#EthnicGroupCode"/>
        <rdfs:comment>Oimatsaha: The ethnic group of Oimatsaha people.</rdfs:comment>
    </owl:NamedIndividual>
    


    <!-- http://www.sisostds.org/ontologies/C2SIM#OMANI -->

    <owl:NamedIndividual rdf:about="http://www.sisostds.org/ontologies/C2SIM#OMANI">
        <rdf:type rdf:resource="http://www.sisostds.org/ontologies/C2SIM#EthnicGroupCode"/>
        <rdfs:comment>Omani: The ethnic group of Omani people.</rdfs:comment>
    </owl:NamedIndividual>
    


    <!-- http://www.sisostds.org/ontologies/C2SIM#OMN -->

    <owl:NamedIndividual rdf:about="http://www.sisostds.org/ontologies/C2SIM#OMN">
        <rdf:type rdf:resource="http://www.sisostds.org/ontologies/C2SIM#CountryCode"/>
        <rdfs:comment>Oman: </rdfs:comment>
    </owl:NamedIndividual>
    


    <!-- http://www.sisostds.org/ontologies/C2SIM#OPANEC -->

    <owl:NamedIndividual rdf:about="http://www.sisostds.org/ontologies/C2SIM#OPANEC">
        <rdf:type rdf:resource="http://www.sisostds.org/ontologies/C2SIM#EthnicGroupCode"/>
        <rdfs:comment>Other Pacific Island not elsewhere classified: The ethnic group of Other Pacific Island not elsewhere classified people.</rdfs:comment>
    </owl:NamedIndividual>
    


    <!-- http://www.sisostds.org/ontologies/C2SIM#OPANFD -->

    <owl:NamedIndividual rdf:about="http://www.sisostds.org/ontologies/C2SIM#OPANFD">
        <rdf:type rdf:resource="http://www.sisostds.org/ontologies/C2SIM#EthnicGroupCode"/>
        <rdfs:comment>Other Pacific Island Groups not further defined: The ethnic group of Other Pacific Island Groups not further defined people.</rdfs:comment>
    </owl:NamedIndividual>
    


    <!-- http://www.sisostds.org/ontologies/C2SIM#ORIENT -->

    <owl:NamedIndividual rdf:about="http://www.sisostds.org/ontologies/C2SIM#ORIENT">
        <rdf:type rdf:resource="http://www.sisostds.org/ontologies/C2SIM#EthnicGroupCode"/>
        <rdfs:comment>Oriental: The ethnic group of Oriental people.</rdfs:comment>
    </owl:NamedIndividual>
    


    <!-- http://www.sisostds.org/ontologies/C2SIM#ORKISL -->

    <owl:NamedIndividual rdf:about="http://www.sisostds.org/ontologies/C2SIM#ORKISL">
        <rdf:type rdf:resource="http://www.sisostds.org/ontologies/C2SIM#EthnicGroupCode"/>
        <rdfs:comment>Orkney Islander: The ethnic group of Orkney Islander people.</rdfs:comment>
    </owl:NamedIndividual>
    


    <!-- http://www.sisostds.org/ontologies/C2SIM#OROMO -->

    <owl:NamedIndividual rdf:about="http://www.sisostds.org/ontologies/C2SIM#OROMO">
        <rdf:type rdf:resource="http://www.sisostds.org/ontologies/C2SIM#EthnicGroupCode"/>
        <rdfs:comment>Oromo: The ethnic group of Oromo people.</rdfs:comment>
    </owl:NamedIndividual>
    


    <!-- http://www.sisostds.org/ontologies/C2SIM#ORTHDX -->

    <owl:NamedIndividual rdf:about="http://www.sisostds.org/ontologies/C2SIM#ORTHDX">
        <rdf:type rdf:resource="http://www.sisostds.org/ontologies/C2SIM#ReligionCode"/>
        <rdfs:comment>Orthodox: One who adheres to or identifies with the Orthodox doctrine.</rdfs:comment>
    </owl:NamedIndividual>
    


    <!-- http://www.sisostds.org/ontologies/C2SIM#OSANEC -->

    <owl:NamedIndividual rdf:about="http://www.sisostds.org/ontologies/C2SIM#OSANEC">
        <rdf:type rdf:resource="http://www.sisostds.org/ontologies/C2SIM#EthnicGroupCode"/>
        <rdfs:comment>Other Southeast Asian not elsewhere classified: The ethnic group of Other Southeast Asian not elsewhere classified people.</rdfs:comment>
    </owl:NamedIndividual>
    


    <!-- http://www.sisostds.org/ontologies/C2SIM#OSSET -->

    <owl:NamedIndividual rdf:about="http://www.sisostds.org/ontologies/C2SIM#OSSET">
        <rdf:type rdf:resource="http://www.sisostds.org/ontologies/C2SIM#EthnicGroupCode"/>
        <rdfs:comment>Ossetian: The ethnic group of Ossetian people.</rdfs:comment>
    </owl:NamedIndividual>
    


    <!-- http://www.sisostds.org/ontologies/C2SIM#OVIMBU -->

    <owl:NamedIndividual rdf:about="http://www.sisostds.org/ontologies/C2SIM#OVIMBU">
        <rdf:type rdf:resource="http://www.sisostds.org/ontologies/C2SIM#EthnicGroupCode"/>
        <rdfs:comment>Ovimbundu: The ethnic group of Ovimbundu people.</rdfs:comment>
    </owl:NamedIndividual>
    


    <!-- http://www.sisostds.org/ontologies/C2SIM#Observe -->

    <owl:NamedIndividual rdf:about="http://www.sisostds.org/ontologies/C2SIM#Observe">
        <rdf:type rdf:resource="http://www.sisostds.org/ontologies/C2SIM#TaskActionCode"/>
    </owl:NamedIndividual>
    <owl:Axiom>
        <owl:annotatedSource rdf:resource="http://www.sisostds.org/ontologies/C2SIM#Observe"/>
        <owl:annotatedProperty rdf:resource="http://www.w3.org/1999/02/22-rdf-syntax-ns#type"/>
        <owl:annotatedTarget rdf:resource="http://www.sisostds.org/ontologies/C2SIM#TaskActionCode"/>
        <rdfs:comment>Either generally observe, or observe the Location or AffectedEntity specified in the Task.</rdfs:comment>
    </owl:Axiom>
    


    <!-- http://www.sisostds.org/ontologies/C2SIM#OrientToLocation -->

    <owl:NamedIndividual rdf:about="http://www.sisostds.org/ontologies/C2SIM#OrientToLocation">
        <rdf:type rdf:resource="http://www.sisostds.org/ontologies/C2SIM#TaskActionCode"/>
    </owl:NamedIndividual>
    <owl:Axiom>
        <owl:annotatedSource rdf:resource="http://www.sisostds.org/ontologies/C2SIM#OrientToLocation"/>
        <owl:annotatedProperty rdf:resource="http://www.w3.org/1999/02/22-rdf-syntax-ns#type"/>
        <owl:annotatedTarget rdf:resource="http://www.sisostds.org/ontologies/C2SIM#TaskActionCode"/>
        <rdfs:comment>Orients (the heading of) an entity toward the Location or MapGraphic specified in the task.</rdfs:comment>
    </owl:Axiom>
    


    <!-- http://www.sisostds.org/ontologies/C2SIM#PACNFD -->

    <owl:NamedIndividual rdf:about="http://www.sisostds.org/ontologies/C2SIM#PACNFD">
        <rdf:type rdf:resource="http://www.sisostds.org/ontologies/C2SIM#EthnicGroupCode"/>
        <rdfs:comment>Pacific Island not further defined: The not further defined ethnic groups of Pacific Island people.</rdfs:comment>
    </owl:NamedIndividual>
    


    <!-- http://www.sisostds.org/ontologies/C2SIM#PAK -->

    <owl:NamedIndividual rdf:about="http://www.sisostds.org/ontologies/C2SIM#PAK">
        <rdf:type rdf:resource="http://www.sisostds.org/ontologies/C2SIM#CountryCode"/>
        <rdfs:comment>Pakistan: </rdfs:comment>
    </owl:NamedIndividual>
    


    <!-- http://www.sisostds.org/ontologies/C2SIM#PAKSTN -->

    <owl:NamedIndividual rdf:about="http://www.sisostds.org/ontologies/C2SIM#PAKSTN">
        <rdf:type rdf:resource="http://www.sisostds.org/ontologies/C2SIM#EthnicGroupCode"/>
        <rdfs:comment>Pakistani: The ethnic group of Pakistani people.</rdfs:comment>
    </owl:NamedIndividual>
    


    <!-- http://www.sisostds.org/ontologies/C2SIM#PALAUA -->

    <owl:NamedIndividual rdf:about="http://www.sisostds.org/ontologies/C2SIM#PALAUA">
        <rdf:type rdf:resource="http://www.sisostds.org/ontologies/C2SIM#EthnicGroupCode"/>
        <rdfs:comment>Palauans: The ethnic group of Palauans people.</rdfs:comment>
    </owl:NamedIndividual>
    


    <!-- http://www.sisostds.org/ontologies/C2SIM#PALMIS -->

    <owl:NamedIndividual rdf:about="http://www.sisostds.org/ontologies/C2SIM#PALMIS">
        <rdf:type rdf:resource="http://www.sisostds.org/ontologies/C2SIM#EthnicGroupCode"/>
        <rdfs:comment>Palmerston Islander: The ethnic group of Palmerston Islander people.</rdfs:comment>
    </owl:NamedIndividual>
    


    <!-- http://www.sisostds.org/ontologies/C2SIM#PALSTN -->

    <owl:NamedIndividual rdf:about="http://www.sisostds.org/ontologies/C2SIM#PALSTN">
        <rdf:type rdf:resource="http://www.sisostds.org/ontologies/C2SIM#EthnicGroupCode"/>
        <rdfs:comment>Palestinian: The ethnic group of Palestinian people.</rdfs:comment>
    </owl:NamedIndividual>
    


    <!-- http://www.sisostds.org/ontologies/C2SIM#PAN -->

    <owl:NamedIndividual rdf:about="http://www.sisostds.org/ontologies/C2SIM#PAN">
        <rdf:type rdf:resource="http://www.sisostds.org/ontologies/C2SIM#CountryCode"/>
        <rdfs:comment>Panama: </rdfs:comment>
    </owl:NamedIndividual>
    


    <!-- http://www.sisostds.org/ontologies/C2SIM#PANMAN -->

    <owl:NamedIndividual rdf:about="http://www.sisostds.org/ontologies/C2SIM#PANMAN">
        <rdf:type rdf:resource="http://www.sisostds.org/ontologies/C2SIM#EthnicGroupCode"/>
        <rdfs:comment>Panamanian: The ethnic group of Panamanian people.</rdfs:comment>
    </owl:NamedIndividual>
    


    <!-- http://www.sisostds.org/ontologies/C2SIM#PAPUAN -->

    <owl:NamedIndividual rdf:about="http://www.sisostds.org/ontologies/C2SIM#PAPUAN">
        <rdf:type rdf:resource="http://www.sisostds.org/ontologies/C2SIM#EthnicGroupCode"/>
        <rdfs:comment>Papuan/New Guinean/Irian Jayan: The ethnic group of Papuan/New Guinean/Irian Jayan people.</rdfs:comment>
    </owl:NamedIndividual>
    


    <!-- http://www.sisostds.org/ontologies/C2SIM#PARGYN -->

    <owl:NamedIndividual rdf:about="http://www.sisostds.org/ontologies/C2SIM#PARGYN">
        <rdf:type rdf:resource="http://www.sisostds.org/ontologies/C2SIM#EthnicGroupCode"/>
        <rdfs:comment>Paraguayan: The ethnic group of Paraguayan people.</rdfs:comment>
    </owl:NamedIndividual>
    


    <!-- http://www.sisostds.org/ontologies/C2SIM#PARSI -->

    <owl:NamedIndividual rdf:about="http://www.sisostds.org/ontologies/C2SIM#PARSI">
        <rdf:type rdf:resource="http://www.sisostds.org/ontologies/C2SIM#ReligionCode"/>
        <rdfs:comment>Parsi: One who adheres to or identifies with the Parsi doctrine.</rdfs:comment>
    </owl:NamedIndividual>
    


    <!-- http://www.sisostds.org/ontologies/C2SIM#PASHTP -->

    <owl:NamedIndividual rdf:about="http://www.sisostds.org/ontologies/C2SIM#PASHTP">
        <rdf:type rdf:resource="http://www.sisostds.org/ontologies/C2SIM#EthnicGroupCode"/>
        <rdfs:comment>Pashtun (Pathan): The ethnic group of Pashtun (Pathan) people.</rdfs:comment>
    </owl:NamedIndividual>
    


    <!-- http://www.sisostds.org/ontologies/C2SIM#PASHTU -->

    <owl:NamedIndividual rdf:about="http://www.sisostds.org/ontologies/C2SIM#PASHTU">
        <rdf:type rdf:resource="http://www.sisostds.org/ontologies/C2SIM#EthnicGroupCode"/>
        <rdfs:comment>Pashtun: The ethnic group of Pashtun people.</rdfs:comment>
    </owl:NamedIndividual>
    


    <!-- http://www.sisostds.org/ontologies/C2SIM#PCN -->

    <owl:NamedIndividual rdf:about="http://www.sisostds.org/ontologies/C2SIM#PCN">
        <rdf:type rdf:resource="http://www.sisostds.org/ontologies/C2SIM#CountryCode"/>
        <rdfs:comment>Pitcairn: </rdfs:comment>
    </owl:NamedIndividual>
    


    <!-- http://www.sisostds.org/ontologies/C2SIM#PENISL -->

    <owl:NamedIndividual rdf:about="http://www.sisostds.org/ontologies/C2SIM#PENISL">
        <rdf:type rdf:resource="http://www.sisostds.org/ontologies/C2SIM#EthnicGroupCode"/>
        <rdfs:comment>Penrhyn Islander: The ethnic group of Penrhyn Islander people.</rdfs:comment>
    </owl:NamedIndividual>
    


    <!-- http://www.sisostds.org/ontologies/C2SIM#PER -->

    <owl:NamedIndividual rdf:about="http://www.sisostds.org/ontologies/C2SIM#PER">
        <rdf:type rdf:resource="http://www.sisostds.org/ontologies/C2SIM#CountryCode"/>
        <rdfs:comment>Peru: </rdfs:comment>
    </owl:NamedIndividual>
    


    <!-- http://www.sisostds.org/ontologies/C2SIM#PERSAN -->

    <owl:NamedIndividual rdf:about="http://www.sisostds.org/ontologies/C2SIM#PERSAN">
        <rdf:type rdf:resource="http://www.sisostds.org/ontologies/C2SIM#EthnicGroupCode"/>
        <rdfs:comment>Persian: The ethnic group of Persian people.</rdfs:comment>
    </owl:NamedIndividual>
    


    <!-- http://www.sisostds.org/ontologies/C2SIM#PERUVN -->

    <owl:NamedIndividual rdf:about="http://www.sisostds.org/ontologies/C2SIM#PERUVN">
        <rdf:type rdf:resource="http://www.sisostds.org/ontologies/C2SIM#EthnicGroupCode"/>
        <rdfs:comment>Peruvian: The ethnic group of Peruvian people.</rdfs:comment>
    </owl:NamedIndividual>
    


    <!-- http://www.sisostds.org/ontologies/C2SIM#PEUL -->

    <owl:NamedIndividual rdf:about="http://www.sisostds.org/ontologies/C2SIM#PEUL">
        <rdf:type rdf:resource="http://www.sisostds.org/ontologies/C2SIM#EthnicGroupCode"/>
        <rdfs:comment>Peul: The ethnic group of Peul people.</rdfs:comment>
    </owl:NamedIndividual>
    


    <!-- http://www.sisostds.org/ontologies/C2SIM#PGNAFR -->

    <owl:NamedIndividual rdf:about="http://www.sisostds.org/ontologies/C2SIM#PGNAFR">
        <rdf:type rdf:resource="http://www.sisostds.org/ontologies/C2SIM#ReligionCode"/>
        <rdfs:comment>Pagan African: One who adheres to or identifies with the Pagan African doctrine.</rdfs:comment>
    </owl:NamedIndividual>
    


    <!-- http://www.sisostds.org/ontologies/C2SIM#PHL -->

    <owl:NamedIndividual rdf:about="http://www.sisostds.org/ontologies/C2SIM#PHL">
        <rdf:type rdf:resource="http://www.sisostds.org/ontologies/C2SIM#CountryCode"/>
        <rdfs:comment>Philippines: </rdfs:comment>
    </owl:NamedIndividual>
    


    <!-- http://www.sisostds.org/ontologies/C2SIM#PHNISL -->

    <owl:NamedIndividual rdf:about="http://www.sisostds.org/ontologies/C2SIM#PHNISL">
        <rdf:type rdf:resource="http://www.sisostds.org/ontologies/C2SIM#EthnicGroupCode"/>
        <rdfs:comment>Phoenix Islander: The ethnic group of Phoenix Islander people.</rdfs:comment>
    </owl:NamedIndividual>
    


    <!-- http://www.sisostds.org/ontologies/C2SIM#PHOUTH -->

    <owl:NamedIndividual rdf:about="http://www.sisostds.org/ontologies/C2SIM#PHOUTH">
        <rdf:type rdf:resource="http://www.sisostds.org/ontologies/C2SIM#EthnicGroupCode"/>
        <rdfs:comment>Phoutheung (Kya): The ethnic group of Phoutheung (Kya) people.</rdfs:comment>
    </owl:NamedIndividual>
    


    <!-- http://www.sisostds.org/ontologies/C2SIM#PITISL -->

    <owl:NamedIndividual rdf:about="http://www.sisostds.org/ontologies/C2SIM#PITISL">
        <rdf:type rdf:resource="http://www.sisostds.org/ontologies/C2SIM#EthnicGroupCode"/>
        <rdfs:comment>Pitcairn Islander: The ethnic group of Pitcairn Islander people.</rdfs:comment>
    </owl:NamedIndividual>
    


    <!-- http://www.sisostds.org/ontologies/C2SIM#PLAYBACK_PAUSED -->

    <owl:NamedIndividual rdf:about="http://www.sisostds.org/ontologies/C2SIM#PLAYBACK_PAUSED">
        <rdf:type rdf:resource="http://www.sisostds.org/ontologies/C2SIM#PlaybackStatusCode"/>
    </owl:NamedIndividual>
    


    <!-- http://www.sisostds.org/ontologies/C2SIM#PLAYBACK_RUNNING -->

    <owl:NamedIndividual rdf:about="http://www.sisostds.org/ontologies/C2SIM#PLAYBACK_RUNNING">
        <rdf:type rdf:resource="http://www.sisostds.org/ontologies/C2SIM#PlaybackStatusCode"/>
    </owl:NamedIndividual>
    


    <!-- http://www.sisostds.org/ontologies/C2SIM#PLW -->

    <owl:NamedIndividual rdf:about="http://www.sisostds.org/ontologies/C2SIM#PLW">
        <rdf:type rdf:resource="http://www.sisostds.org/ontologies/C2SIM#CountryCode"/>
        <rdfs:comment>Palau: </rdfs:comment>
    </owl:NamedIndividual>
    


    <!-- http://www.sisostds.org/ontologies/C2SIM#PNG -->

    <owl:NamedIndividual rdf:about="http://www.sisostds.org/ontologies/C2SIM#PNG">
        <rdf:type rdf:resource="http://www.sisostds.org/ontologies/C2SIM#CountryCode"/>
        <rdfs:comment>Papua New Guinea: </rdfs:comment>
    </owl:NamedIndividual>
    


    <!-- http://www.sisostds.org/ontologies/C2SIM#PNTCST -->

    <owl:NamedIndividual rdf:about="http://www.sisostds.org/ontologies/C2SIM#PNTCST">
        <rdf:type rdf:resource="http://www.sisostds.org/ontologies/C2SIM#ReligionCode"/>
        <rdfs:comment>Pentecostal: One who adheres to or identifies with the Pentecostal doctrine.</rdfs:comment>
    </owl:NamedIndividual>
    


    <!-- http://www.sisostds.org/ontologies/C2SIM#POL -->

    <owl:NamedIndividual rdf:about="http://www.sisostds.org/ontologies/C2SIM#POL">
        <rdf:type rdf:resource="http://www.sisostds.org/ontologies/C2SIM#CountryCode"/>
        <rdfs:comment>Poland: </rdfs:comment>
    </owl:NamedIndividual>
    


    <!-- http://www.sisostds.org/ontologies/C2SIM#POLCHF -->

    <owl:NamedIndividual rdf:about="http://www.sisostds.org/ontologies/C2SIM#POLCHF">
        <rdf:type rdf:resource="http://www.sisostds.org/ontologies/C2SIM#OrganizationTypeCode"/>
        <rdfs:comment>Police chief: A GROUP-ORGANISATION-TYPE that comprises persons that have the responsibility for the regulation, discipline, and control</rdfs:comment>
    </owl:NamedIndividual>
    


    <!-- http://www.sisostds.org/ontologies/C2SIM#POLICE -->

    <owl:NamedIndividual rdf:about="http://www.sisostds.org/ontologies/C2SIM#POLICE">
        <rdf:type rdf:resource="http://www.sisostds.org/ontologies/C2SIM#OrganizationTypeCode"/>
        <rdfs:comment>Police: A GROUP-ORGANISATION-TYPE that is responsible for the regulation, discipline and control of community, civil administration;</rdfs:comment>
    </owl:NamedIndividual>
    


    <!-- http://www.sisostds.org/ontologies/C2SIM#POLISH -->

    <owl:NamedIndividual rdf:about="http://www.sisostds.org/ontologies/C2SIM#POLISH">
        <rdf:type rdf:resource="http://www.sisostds.org/ontologies/C2SIM#EthnicGroupCode"/>
        <rdfs:comment>Polish: The ethnic group of Polish people.</rdfs:comment>
    </owl:NamedIndividual>
    


    <!-- http://www.sisostds.org/ontologies/C2SIM#POLTCL -->

    <owl:NamedIndividual rdf:about="http://www.sisostds.org/ontologies/C2SIM#POLTCL">
        <rdf:type rdf:resource="http://www.sisostds.org/ontologies/C2SIM#OrganizationTypeCode"/>
        <rdfs:comment>Political: A GROUP-ORGANISATION-TYPE that is identified as being involved within a political area of activity and concerned with politics</rdfs:comment>
    </owl:NamedIndividual>
    


    <!-- http://www.sisostds.org/ontologies/C2SIM#POLYNE -->

    <owl:NamedIndividual rdf:about="http://www.sisostds.org/ontologies/C2SIM#POLYNE">
        <rdf:type rdf:resource="http://www.sisostds.org/ontologies/C2SIM#EthnicGroupCode"/>
        <rdfs:comment>Polynesian: The ethnic group of Polynesian people.</rdfs:comment>
    </owl:NamedIndividual>
    


    <!-- http://www.sisostds.org/ontologies/C2SIM#POLYNS -->

    <owl:NamedIndividual rdf:about="http://www.sisostds.org/ontologies/C2SIM#POLYNS">
        <rdf:type rdf:resource="http://www.sisostds.org/ontologies/C2SIM#EthnicGroupCode"/>
        <rdfs:comment>Polynesian (Samoan): The ethnic group of Polynesian (Samoan) people.</rdfs:comment>
    </owl:NamedIndividual>
    


    <!-- http://www.sisostds.org/ontologies/C2SIM#POLYNT -->

    <owl:NamedIndividual rdf:about="http://www.sisostds.org/ontologies/C2SIM#POLYNT">
        <rdf:type rdf:resource="http://www.sisostds.org/ontologies/C2SIM#EthnicGroupCode"/>
        <rdfs:comment>Polynesian (Tongans): The ethnic group of Polynesian (Tongans) people.</rdfs:comment>
    </owl:NamedIndividual>
    


    <!-- http://www.sisostds.org/ontologies/C2SIM#PORTGS -->

    <owl:NamedIndividual rdf:about="http://www.sisostds.org/ontologies/C2SIM#PORTGS">
        <rdf:type rdf:resource="http://www.sisostds.org/ontologies/C2SIM#EthnicGroupCode"/>
        <rdfs:comment>Portuguese: The ethnic group of Portuguese people.</rdfs:comment>
    </owl:NamedIndividual>
    


    <!-- http://www.sisostds.org/ontologies/C2SIM#POW -->

    <owl:NamedIndividual rdf:about="http://www.sisostds.org/ontologies/C2SIM#POW">
        <rdf:type rdf:resource="http://www.sisostds.org/ontologies/C2SIM#OrganizationTypeCode"/>
        <rdfs:comment>Prisoner of war: A GROUP-ORGANISATION-TYPE that comprises persons that have fallen in the hands of or surrendered to an opponent.</rdfs:comment>
    </owl:NamedIndividual>
    


    <!-- http://www.sisostds.org/ontologies/C2SIM#PRI -->

    <owl:NamedIndividual rdf:about="http://www.sisostds.org/ontologies/C2SIM#PRI">
        <rdf:type rdf:resource="http://www.sisostds.org/ontologies/C2SIM#CountryCode"/>
        <rdfs:comment>Puerto Rico: </rdfs:comment>
    </owl:NamedIndividual>
    


    <!-- http://www.sisostds.org/ontologies/C2SIM#PRK -->

    <owl:NamedIndividual rdf:about="http://www.sisostds.org/ontologies/C2SIM#PRK">
        <rdf:type rdf:resource="http://www.sisostds.org/ontologies/C2SIM#CountryCode"/>
        <rdfs:comment>Korea, Democratic People&apos;s Republic of: </rdfs:comment>
    </owl:NamedIndividual>
    


    <!-- http://www.sisostds.org/ontologies/C2SIM#PRSBYT -->

    <owl:NamedIndividual rdf:about="http://www.sisostds.org/ontologies/C2SIM#PRSBYT">
        <rdf:type rdf:resource="http://www.sisostds.org/ontologies/C2SIM#ReligionCode"/>
        <rdfs:comment>Presbyterian: One who adheres to or identifies with the Presbyterian doctrine.</rdfs:comment>
    </owl:NamedIndividual>
    


    <!-- http://www.sisostds.org/ontologies/C2SIM#PRSNR -->

    <owl:NamedIndividual rdf:about="http://www.sisostds.org/ontologies/C2SIM#PRSNR">
        <rdf:type rdf:resource="http://www.sisostds.org/ontologies/C2SIM#OrganizationTypeCode"/>
        <rdfs:comment>Prisoner: A GROUP-ORGANISATION-TYPE in custody on a criminal charge and on trial.</rdfs:comment>
    </owl:NamedIndividual>
    


    <!-- http://www.sisostds.org/ontologies/C2SIM#PRT -->

    <owl:NamedIndividual rdf:about="http://www.sisostds.org/ontologies/C2SIM#PRT">
        <rdf:type rdf:resource="http://www.sisostds.org/ontologies/C2SIM#CountryCode"/>
        <rdf:type rdf:resource="http://www.sisostds.org/ontologies/C2SIM#ReligionCode"/>
        <rdfs:comment>Portugal: </rdfs:comment>
        <rdfs:comment>Protestant: One who adheres to or identifies with the Protestant doctrine.</rdfs:comment>
    </owl:NamedIndividual>
    


    <!-- http://www.sisostds.org/ontologies/C2SIM#PRTADV -->

    <owl:NamedIndividual rdf:about="http://www.sisostds.org/ontologies/C2SIM#PRTADV">
        <rdf:type rdf:resource="http://www.sisostds.org/ontologies/C2SIM#ReligionCode"/>
        <rdfs:comment>Protestant (Adventist): One who adheres to or identifies with the Protestant (Adventist) doctrine.</rdfs:comment>
    </owl:NamedIndividual>
    


    <!-- http://www.sisostds.org/ontologies/C2SIM#PRTEVN -->

    <owl:NamedIndividual rdf:about="http://www.sisostds.org/ontologies/C2SIM#PRTEVN">
        <rdf:type rdf:resource="http://www.sisostds.org/ontologies/C2SIM#ReligionCode"/>
        <rdfs:comment>Protestant (Evangelical Methodist): One who adheres to or identifies with the Protestant (Evangelical Methodist) doctrine.</rdfs:comment>
    </owl:NamedIndividual>
    


    <!-- http://www.sisostds.org/ontologies/C2SIM#PRTMRV -->

    <owl:NamedIndividual rdf:about="http://www.sisostds.org/ontologies/C2SIM#PRTMRV">
        <rdf:type rdf:resource="http://www.sisostds.org/ontologies/C2SIM#ReligionCode"/>
        <rdfs:comment>Protestant (Moravian): One who adheres to or identifies with the Protestant (Moravian) doctrine.</rdfs:comment>
    </owl:NamedIndividual>
    


    <!-- http://www.sisostds.org/ontologies/C2SIM#PRY -->

    <owl:NamedIndividual rdf:about="http://www.sisostds.org/ontologies/C2SIM#PRY">
        <rdf:type rdf:resource="http://www.sisostds.org/ontologies/C2SIM#CountryCode"/>
        <rdfs:comment>Paraguay: </rdfs:comment>
    </owl:NamedIndividual>
    


    <!-- http://www.sisostds.org/ontologies/C2SIM#PSE -->

    <owl:NamedIndividual rdf:about="http://www.sisostds.org/ontologies/C2SIM#PSE">
        <rdf:type rdf:resource="http://www.sisostds.org/ontologies/C2SIM#CountryCode"/>
        <rdfs:comment>Palestinian Territory, Occupied: </rdfs:comment>
    </owl:NamedIndividual>
    


    <!-- http://www.sisostds.org/ontologies/C2SIM#PUERTR -->

    <owl:NamedIndividual rdf:about="http://www.sisostds.org/ontologies/C2SIM#PUERTR">
        <rdf:type rdf:resource="http://www.sisostds.org/ontologies/C2SIM#EthnicGroupCode"/>
        <rdfs:comment>Puerto Rican: The ethnic group of Puerto Rican people.</rdfs:comment>
    </owl:NamedIndividual>
    


    <!-- http://www.sisostds.org/ontologies/C2SIM#PUKISL -->

    <owl:NamedIndividual rdf:about="http://www.sisostds.org/ontologies/C2SIM#PUKISL">
        <rdf:type rdf:resource="http://www.sisostds.org/ontologies/C2SIM#EthnicGroupCode"/>
        <rdfs:comment>Pukapuka Islander: The ethnic group of Pukapuka Islander people.</rdfs:comment>
    </owl:NamedIndividual>
    


    <!-- http://www.sisostds.org/ontologies/C2SIM#PUNJAB -->

    <owl:NamedIndividual rdf:about="http://www.sisostds.org/ontologies/C2SIM#PUNJAB">
        <rdf:type rdf:resource="http://www.sisostds.org/ontologies/C2SIM#EthnicGroupCode"/>
        <rdfs:comment>Punjabi: The ethnic group of Punjabi people.</rdfs:comment>
    </owl:NamedIndividual>
    


    <!-- http://www.sisostds.org/ontologies/C2SIM#PYF -->

    <owl:NamedIndividual rdf:about="http://www.sisostds.org/ontologies/C2SIM#PYF">
        <rdf:type rdf:resource="http://www.sisostds.org/ontologies/C2SIM#CountryCode"/>
        <rdfs:comment>French Polynesia: </rdfs:comment>
    </owl:NamedIndividual>
    


    <!-- http://www.sisostds.org/ontologies/C2SIM#PartlyOperational -->

    <owl:NamedIndividual rdf:about="http://www.sisostds.org/ontologies/C2SIM#PartlyOperational">
        <rdf:type rdf:resource="http://www.sisostds.org/ontologies/C2SIM#OperationalStatusCode"/>
    </owl:NamedIndividual>
    


    <!-- http://www.sisostds.org/ontologies/C2SIM#Propose -->

    <owl:NamedIndividual rdf:about="http://www.sisostds.org/ontologies/C2SIM#Propose">
        <rdf:type rdf:resource="http://www.sisostds.org/ontologies/C2SIM#CommunicativeActTypeCode"/>
    </owl:NamedIndividual>
    


    <!-- http://www.sisostds.org/ontologies/C2SIM#QAT -->

    <owl:NamedIndividual rdf:about="http://www.sisostds.org/ontologies/C2SIM#QAT">
        <rdf:type rdf:resource="http://www.sisostds.org/ontologies/C2SIM#CountryCode"/>
        <rdfs:comment>Qatar: </rdfs:comment>
    </owl:NamedIndividual>
    


    <!-- http://www.sisostds.org/ontologies/C2SIM#QUECHU -->

    <owl:NamedIndividual rdf:about="http://www.sisostds.org/ontologies/C2SIM#QUECHU">
        <rdf:type rdf:resource="http://www.sisostds.org/ontologies/C2SIM#EthnicGroupCode"/>
        <rdfs:comment>Quechua: The ethnic group of Quechua people.</rdfs:comment>
    </owl:NamedIndividual>
    


    <!-- http://www.sisostds.org/ontologies/C2SIM#RAIS -->

    <owl:NamedIndividual rdf:about="http://www.sisostds.org/ontologies/C2SIM#RAIS">
        <rdf:type rdf:resource="http://www.sisostds.org/ontologies/C2SIM#EthnicGroupCode"/>
        <rdfs:comment>Rais: The ethnic group of Rais people.</rdfs:comment>
    </owl:NamedIndividual>
    


    <!-- http://www.sisostds.org/ontologies/C2SIM#RAKHIN -->

    <owl:NamedIndividual rdf:about="http://www.sisostds.org/ontologies/C2SIM#RAKHIN">
        <rdf:type rdf:resource="http://www.sisostds.org/ontologies/C2SIM#EthnicGroupCode"/>
        <rdfs:comment>Rakhine: The ethnic group of Rakhine people.</rdfs:comment>
    </owl:NamedIndividual>
    


    <!-- http://www.sisostds.org/ontologies/C2SIM#RAKISL -->

    <owl:NamedIndividual rdf:about="http://www.sisostds.org/ontologies/C2SIM#RAKISL">
        <rdf:type rdf:resource="http://www.sisostds.org/ontologies/C2SIM#EthnicGroupCode"/>
        <rdfs:comment>Rakahanga Islander: The ethnic group of Rakahanga Islander people.</rdfs:comment>
    </owl:NamedIndividual>
    


    <!-- http://www.sisostds.org/ontologies/C2SIM#RARTGN -->

    <owl:NamedIndividual rdf:about="http://www.sisostds.org/ontologies/C2SIM#RARTGN">
        <rdf:type rdf:resource="http://www.sisostds.org/ontologies/C2SIM#EthnicGroupCode"/>
        <rdfs:comment>Rarotongan: The ethnic group of Rarotongan people.</rdfs:comment>
    </owl:NamedIndividual>
    


    <!-- http://www.sisostds.org/ontologies/C2SIM#RECORDING_IN_PROGRESS -->

    <owl:NamedIndividual rdf:about="http://www.sisostds.org/ontologies/C2SIM#RECORDING_IN_PROGRESS">
        <rdf:type rdf:resource="http://www.sisostds.org/ontologies/C2SIM#RecordingStatusCode"/>
    </owl:NamedIndividual>
    


    <!-- http://www.sisostds.org/ontologies/C2SIM#RECORDING_PAUSED -->

    <owl:NamedIndividual rdf:about="http://www.sisostds.org/ontologies/C2SIM#RECORDING_PAUSED">
        <rdf:type rdf:resource="http://www.sisostds.org/ontologies/C2SIM#RecordingStatusCode"/>
    </owl:NamedIndividual>
    


    <!-- http://www.sisostds.org/ontologies/C2SIM#REFUGE -->

    <owl:NamedIndividual rdf:about="http://www.sisostds.org/ontologies/C2SIM#REFUGE">
        <rdf:type rdf:resource="http://www.sisostds.org/ontologies/C2SIM#OrganizationTypeCode"/>
        <rdfs:comment>Refugee: A GROUP-ORGANISATION-TYPE that comprises persons who, owing to religious persecution or political troubles, seek refuge.</rdfs:comment>
    </owl:NamedIndividual>
    


    <!-- http://www.sisostds.org/ontologies/C2SIM#REU -->

    <owl:NamedIndividual rdf:about="http://www.sisostds.org/ontologies/C2SIM#REU">
        <rdf:type rdf:resource="http://www.sisostds.org/ontologies/C2SIM#CountryCode"/>
        <rdfs:comment>Reunion: </rdfs:comment>
    </owl:NamedIndividual>
    


    <!-- http://www.sisostds.org/ontologies/C2SIM#RIOMUN -->

    <owl:NamedIndividual rdf:about="http://www.sisostds.org/ontologies/C2SIM#RIOMUN">
        <rdf:type rdf:resource="http://www.sisostds.org/ontologies/C2SIM#EthnicGroupCode"/>
        <rdfs:comment>Rio Muni (Fang): The ethnic group of Rio Muni (Fang) people.</rdfs:comment>
    </owl:NamedIndividual>
    


    <!-- http://www.sisostds.org/ontologies/C2SIM#RMNCTH -->

    <owl:NamedIndividual rdf:about="http://www.sisostds.org/ontologies/C2SIM#RMNCTH">
        <rdf:type rdf:resource="http://www.sisostds.org/ontologies/C2SIM#ReligionCode"/>
        <rdfs:comment>Roman Catholic: One who adheres to or identifies with the Roman Catholic doctrine.</rdfs:comment>
    </owl:NamedIndividual>
    


    <!-- http://www.sisostds.org/ontologies/C2SIM#RMNCTU -->

    <owl:NamedIndividual rdf:about="http://www.sisostds.org/ontologies/C2SIM#RMNCTU">
        <rdf:type rdf:resource="http://www.sisostds.org/ontologies/C2SIM#ReligionCode"/>
        <rdfs:comment>Roman Catholic (Uniate): One who adheres to or identifies with the Roman Catholic (Uniate) doctrine.</rdfs:comment>
    </owl:NamedIndividual>
    


    <!-- http://www.sisostds.org/ontologies/C2SIM#ROMANN -->

    <owl:NamedIndividual rdf:about="http://www.sisostds.org/ontologies/C2SIM#ROMANN">
        <rdf:type rdf:resource="http://www.sisostds.org/ontologies/C2SIM#EthnicGroupCode"/>
        <rdfs:comment>Romanian/Rumanian: The ethnic group of Romanian/Rumanian people.</rdfs:comment>
    </owl:NamedIndividual>
    


    <!-- http://www.sisostds.org/ontologies/C2SIM#ROMANS -->

    <owl:NamedIndividual rdf:about="http://www.sisostds.org/ontologies/C2SIM#ROMANS">
        <rdf:type rdf:resource="http://www.sisostds.org/ontologies/C2SIM#EthnicGroupCode"/>
        <rdfs:comment>Romansch: The ethnic group of Romansch people.</rdfs:comment>
    </owl:NamedIndividual>
    


    <!-- http://www.sisostds.org/ontologies/C2SIM#ROMANY -->

    <owl:NamedIndividual rdf:about="http://www.sisostds.org/ontologies/C2SIM#ROMANY">
        <rdf:type rdf:resource="http://www.sisostds.org/ontologies/C2SIM#EthnicGroupCode"/>
        <rdfs:comment>Romany/Gypsy: The ethnic group of Romany/Gypsy people.</rdfs:comment>
    </owl:NamedIndividual>
    


    <!-- http://www.sisostds.org/ontologies/C2SIM#ROMORT -->

    <owl:NamedIndividual rdf:about="http://www.sisostds.org/ontologies/C2SIM#ROMORT">
        <rdf:type rdf:resource="http://www.sisostds.org/ontologies/C2SIM#ReligionCode"/>
        <rdfs:comment>Romanian Orthodox: One who adheres to or identifies with the Romanian Orthodox doctrine.</rdfs:comment>
    </owl:NamedIndividual>
    


    <!-- http://www.sisostds.org/ontologies/C2SIM#ROTUMN -->

    <owl:NamedIndividual rdf:about="http://www.sisostds.org/ontologies/C2SIM#ROTUMN">
        <rdf:type rdf:resource="http://www.sisostds.org/ontologies/C2SIM#EthnicGroupCode"/>
        <rdfs:comment>Rotuman/Rotuman Islander: The ethnic group of Rotuman/Rotuman Islander people.</rdfs:comment>
    </owl:NamedIndividual>
    


    <!-- http://www.sisostds.org/ontologies/C2SIM#ROU -->

    <owl:NamedIndividual rdf:about="http://www.sisostds.org/ontologies/C2SIM#ROU">
        <rdf:type rdf:resource="http://www.sisostds.org/ontologies/C2SIM#CountryCode"/>
        <rdfs:comment>Romania: </rdfs:comment>
    </owl:NamedIndividual>
    


    <!-- http://www.sisostds.org/ontologies/C2SIM#RUS -->

    <owl:NamedIndividual rdf:about="http://www.sisostds.org/ontologies/C2SIM#RUS">
        <rdf:type rdf:resource="http://www.sisostds.org/ontologies/C2SIM#CountryCode"/>
        <rdfs:comment>Russian Federation: </rdfs:comment>
    </owl:NamedIndividual>
    


    <!-- http://www.sisostds.org/ontologies/C2SIM#RUSORT -->

    <owl:NamedIndividual rdf:about="http://www.sisostds.org/ontologies/C2SIM#RUSORT">
        <rdf:type rdf:resource="http://www.sisostds.org/ontologies/C2SIM#ReligionCode"/>
        <rdfs:comment>Russian Orthodox: One who adheres to or identifies with the Russian Orthodox doctrine.</rdfs:comment>
    </owl:NamedIndividual>
    


    <!-- http://www.sisostds.org/ontologies/C2SIM#RUSSAN -->

    <owl:NamedIndividual rdf:about="http://www.sisostds.org/ontologies/C2SIM#RUSSAN">
        <rdf:type rdf:resource="http://www.sisostds.org/ontologies/C2SIM#EthnicGroupCode"/>
        <rdfs:comment>Russian: The ethnic group of Russian people.</rdfs:comment>
    </owl:NamedIndividual>
    


    <!-- http://www.sisostds.org/ontologies/C2SIM#RUTHEN -->

    <owl:NamedIndividual rdf:about="http://www.sisostds.org/ontologies/C2SIM#RUTHEN">
        <rdf:type rdf:resource="http://www.sisostds.org/ontologies/C2SIM#EthnicGroupCode"/>
        <rdfs:comment>Ruthenian: The ethnic group of Ruthenian people.</rdfs:comment>
    </owl:NamedIndividual>
    


    <!-- http://www.sisostds.org/ontologies/C2SIM#RWA -->

    <owl:NamedIndividual rdf:about="http://www.sisostds.org/ontologies/C2SIM#RWA">
        <rdf:type rdf:resource="http://www.sisostds.org/ontologies/C2SIM#CountryCode"/>
        <rdfs:comment>Rwanda: </rdfs:comment>
    </owl:NamedIndividual>
    


    <!-- http://www.sisostds.org/ontologies/C2SIM#RWANDA -->

    <owl:NamedIndividual rdf:about="http://www.sisostds.org/ontologies/C2SIM#RWANDA">
        <rdf:type rdf:resource="http://www.sisostds.org/ontologies/C2SIM#EthnicGroupCode"/>
        <rdfs:comment>Rwandans: The ethnic group of Rwandans people.</rdfs:comment>
    </owl:NamedIndividual>
    


    <!-- http://www.sisostds.org/ontologies/C2SIM#Refuse -->

    <owl:NamedIndividual rdf:about="http://www.sisostds.org/ontologies/C2SIM#Refuse">
        <rdf:type rdf:resource="http://www.sisostds.org/ontologies/C2SIM#CommunicativeActTypeCode"/>
    </owl:NamedIndividual>
    


    <!-- http://www.sisostds.org/ontologies/C2SIM#ReportPosition -->

    <owl:NamedIndividual rdf:about="http://www.sisostds.org/ontologies/C2SIM#ReportPosition">
        <rdf:type rdf:resource="http://www.sisostds.org/ontologies/C2SIM#TaskActionCode"/>
    </owl:NamedIndividual>
    <owl:Axiom>
        <owl:annotatedSource rdf:resource="http://www.sisostds.org/ontologies/C2SIM#ReportPosition"/>
        <owl:annotatedProperty rdf:resource="http://www.w3.org/1999/02/22-rdf-syntax-ns#type"/>
        <owl:annotatedTarget rdf:resource="http://www.sisostds.org/ontologies/C2SIM#TaskActionCode"/>
        <rdfs:comment>Requests the receiving entity to reply with a position report.</rdfs:comment>
    </owl:Axiom>
    


    <!-- http://www.sisostds.org/ontologies/C2SIM#Request -->

    <owl:NamedIndividual rdf:about="http://www.sisostds.org/ontologies/C2SIM#Request">
        <rdf:type rdf:resource="http://www.sisostds.org/ontologies/C2SIM#CommunicativeActTypeCode"/>
    </owl:NamedIndividual>
    


    <!-- http://www.sisostds.org/ontologies/C2SIM#SAEAST -->

    <owl:NamedIndividual rdf:about="http://www.sisostds.org/ontologies/C2SIM#SAEAST">
        <rdf:type rdf:resource="http://www.sisostds.org/ontologies/C2SIM#ActionTemporalAssociationCode"/>
        <rdfs:comment>Starts at and ends at the same time as: The two ACTIONs are concurrent.</rdfs:comment>
    </owl:NamedIndividual>
    


    <!-- http://www.sisostds.org/ontologies/C2SIM#SAENDO -->

    <owl:NamedIndividual rdf:about="http://www.sisostds.org/ontologies/C2SIM#SAENDO">
        <rdf:type rdf:resource="http://www.sisostds.org/ontologies/C2SIM#ActionTemporalAssociationCode"/>
        <rdfs:comment>Starts before and ends before end of: The subject ACTION begins before the object ACTION and ends before the object ACTION ends.</rdfs:comment>
    </owl:NamedIndividual>
    


    <!-- http://www.sisostds.org/ontologies/C2SIM#SAHO -->

    <owl:NamedIndividual rdf:about="http://www.sisostds.org/ontologies/C2SIM#SAHO">
        <rdf:type rdf:resource="http://www.sisostds.org/ontologies/C2SIM#EthnicGroupCode"/>
        <rdfs:comment>Saho: The ethnic group of Saho people.</rdfs:comment>
    </owl:NamedIndividual>
    


    <!-- http://www.sisostds.org/ontologies/C2SIM#SAKALA -->

    <owl:NamedIndividual rdf:about="http://www.sisostds.org/ontologies/C2SIM#SAKALA">
        <rdf:type rdf:resource="http://www.sisostds.org/ontologies/C2SIM#EthnicGroupCode"/>
        <rdfs:comment>Sakalava: The ethnic group of Sakalava people.</rdfs:comment>
    </owl:NamedIndividual>
    


    <!-- http://www.sisostds.org/ontologies/C2SIM#SAMMAR -->

    <owl:NamedIndividual rdf:about="http://www.sisostds.org/ontologies/C2SIM#SAMMAR">
        <rdf:type rdf:resource="http://www.sisostds.org/ontologies/C2SIM#EthnicGroupCode"/>
        <rdfs:comment>Sammarinese: The ethnic group of Sammarinese people.</rdfs:comment>
    </owl:NamedIndividual>
    


    <!-- http://www.sisostds.org/ontologies/C2SIM#SAMOAN -->

    <owl:NamedIndividual rdf:about="http://www.sisostds.org/ontologies/C2SIM#SAMOAN">
        <rdf:type rdf:resource="http://www.sisostds.org/ontologies/C2SIM#EthnicGroupCode"/>
        <rdfs:comment>Samoan: The ethnic group of Samoan people.</rdfs:comment>
    </owl:NamedIndividual>
    


    <!-- http://www.sisostds.org/ontologies/C2SIM#SAMOAP -->

    <owl:NamedIndividual rdf:about="http://www.sisostds.org/ontologies/C2SIM#SAMOAP">
        <rdf:type rdf:resource="http://www.sisostds.org/ontologies/C2SIM#EthnicGroupCode"/>
        <rdfs:comment>Samoan (Polynesian): The ethnic group of Samoan (Polynesian) people.</rdfs:comment>
    </owl:NamedIndividual>
    


    <!-- http://www.sisostds.org/ontologies/C2SIM#SANGHA -->

    <owl:NamedIndividual rdf:about="http://www.sisostds.org/ontologies/C2SIM#SANGHA">
        <rdf:type rdf:resource="http://www.sisostds.org/ontologies/C2SIM#EthnicGroupCode"/>
        <rdfs:comment>Sangha: The ethnic group of Sangha people.</rdfs:comment>
    </owl:NamedIndividual>
    


    <!-- http://www.sisostds.org/ontologies/C2SIM#SANISL -->

    <owl:NamedIndividual rdf:about="http://www.sisostds.org/ontologies/C2SIM#SANISL">
        <rdf:type rdf:resource="http://www.sisostds.org/ontologies/C2SIM#EthnicGroupCode"/>
        <rdfs:comment>Santa Cruz Islander: The ethnic group of Santa Cruz Islander people.</rdfs:comment>
    </owl:NamedIndividual>
    


    <!-- http://www.sisostds.org/ontologies/C2SIM#SARA -->

    <owl:NamedIndividual rdf:about="http://www.sisostds.org/ontologies/C2SIM#SARA">
        <rdf:type rdf:resource="http://www.sisostds.org/ontologies/C2SIM#EthnicGroupCode"/>
        <rdfs:comment>Sara: The ethnic group of Sara people.</rdfs:comment>
    </owl:NamedIndividual>
    


    <!-- http://www.sisostds.org/ontologies/C2SIM#SARDNN -->

    <owl:NamedIndividual rdf:about="http://www.sisostds.org/ontologies/C2SIM#SARDNN">
        <rdf:type rdf:resource="http://www.sisostds.org/ontologies/C2SIM#EthnicGroupCode"/>
        <rdfs:comment>Sardinian: The ethnic group of Sardinian people.</rdfs:comment>
    </owl:NamedIndividual>
    


    <!-- http://www.sisostds.org/ontologies/C2SIM#SASTEA -->

    <owl:NamedIndividual rdf:about="http://www.sisostds.org/ontologies/C2SIM#SASTEA">
        <rdf:type rdf:resource="http://www.sisostds.org/ontologies/C2SIM#ActionTemporalAssociationCode"/>
        <rdfs:comment>Starts at the same time and ends after: The subject ACTION begins concurrently with the object ACTION, but will extend beyond the object ACTION.</rdfs:comment>
    </owl:NamedIndividual>
    


    <!-- http://www.sisostds.org/ontologies/C2SIM#SAU -->

    <owl:NamedIndividual rdf:about="http://www.sisostds.org/ontologies/C2SIM#SAU">
        <rdf:type rdf:resource="http://www.sisostds.org/ontologies/C2SIM#CountryCode"/>
        <rdfs:comment>Saudi Arabia: </rdfs:comment>
    </owl:NamedIndividual>
    


    <!-- http://www.sisostds.org/ontologies/C2SIM#SBEAST -->

    <owl:NamedIndividual rdf:about="http://www.sisostds.org/ontologies/C2SIM#SBEAST">
        <rdf:type rdf:resource="http://www.sisostds.org/ontologies/C2SIM#ActionTemporalAssociationCode"/>
        <rdfs:comment>Starts during and ends at the same time as: The start of the object ACTION precedes that of the subject ACTION, but they will end concurrently.</rdfs:comment>
    </owl:NamedIndividual>
    


    <!-- http://www.sisostds.org/ontologies/C2SIM#SCANDN -->

    <owl:NamedIndividual rdf:about="http://www.sisostds.org/ontologies/C2SIM#SCANDN">
        <rdf:type rdf:resource="http://www.sisostds.org/ontologies/C2SIM#EthnicGroupCode"/>
        <rdfs:comment>Scandinavian: The ethnic group of Scandinavian people.</rdfs:comment>
    </owl:NamedIndividual>
    


    <!-- http://www.sisostds.org/ontologies/C2SIM#SCOTSH -->

    <owl:NamedIndividual rdf:about="http://www.sisostds.org/ontologies/C2SIM#SCOTSH">
        <rdf:type rdf:resource="http://www.sisostds.org/ontologies/C2SIM#EthnicGroupCode"/>
        <rdfs:comment>Scottish (Scots): The ethnic group of Scottish (Scots) people.</rdfs:comment>
    </owl:NamedIndividual>
    


    <!-- http://www.sisostds.org/ontologies/C2SIM#SDN -->

    <owl:NamedIndividual rdf:about="http://www.sisostds.org/ontologies/C2SIM#SDN">
        <rdf:type rdf:resource="http://www.sisostds.org/ontologies/C2SIM#CountryCode"/>
        <rdfs:comment>Sudan: </rdfs:comment>
    </owl:NamedIndividual>
    


    <!-- http://www.sisostds.org/ontologies/C2SIM#SDUREA -->

    <owl:NamedIndividual rdf:about="http://www.sisostds.org/ontologies/C2SIM#SDUREA">
        <rdf:type rdf:resource="http://www.sisostds.org/ontologies/C2SIM#ActionTemporalAssociationCode"/>
        <rdfs:comment>Starts during and ends after: The subject ACTION is sequential but overlapping with the object ACTION.</rdfs:comment>
    </owl:NamedIndividual>
    


    <!-- http://www.sisostds.org/ontologies/C2SIM#SDUREB -->

    <owl:NamedIndividual rdf:about="http://www.sisostds.org/ontologies/C2SIM#SDUREB">
        <rdf:type rdf:resource="http://www.sisostds.org/ontologies/C2SIM#ActionTemporalAssociationCode"/>
        <rdfs:comment>Starts and ends during: The subject ACTION starts after the start of object ACTION and ends before the end of object ACTION.</rdfs:comment>
    </owl:NamedIndividual>
    


    <!-- http://www.sisostds.org/ontologies/C2SIM#SEN -->

    <owl:NamedIndividual rdf:about="http://www.sisostds.org/ontologies/C2SIM#SEN">
        <rdf:type rdf:resource="http://www.sisostds.org/ontologies/C2SIM#CountryCode"/>
        <rdfs:comment>Senegal: </rdfs:comment>
    </owl:NamedIndividual>
    


    <!-- http://www.sisostds.org/ontologies/C2SIM#SENA -->

    <owl:NamedIndividual rdf:about="http://www.sisostds.org/ontologies/C2SIM#SENA">
        <rdf:type rdf:resource="http://www.sisostds.org/ontologies/C2SIM#EthnicGroupCode"/>
        <rdfs:comment>Sena: The ethnic group of Sena people.</rdfs:comment>
    </owl:NamedIndividual>
    


    <!-- http://www.sisostds.org/ontologies/C2SIM#SENOUF -->

    <owl:NamedIndividual rdf:about="http://www.sisostds.org/ontologies/C2SIM#SENOUF">
        <rdf:type rdf:resource="http://www.sisostds.org/ontologies/C2SIM#EthnicGroupCode"/>
        <rdfs:comment>Senoufou: The ethnic group of Senoufou people.</rdfs:comment>
    </owl:NamedIndividual>
    


    <!-- http://www.sisostds.org/ontologies/C2SIM#SENUFO -->

    <owl:NamedIndividual rdf:about="http://www.sisostds.org/ontologies/C2SIM#SENUFO">
        <rdf:type rdf:resource="http://www.sisostds.org/ontologies/C2SIM#EthnicGroupCode"/>
        <rdfs:comment>Senufo: The ethnic group of Senufo people.</rdfs:comment>
    </owl:NamedIndividual>
    


    <!-- http://www.sisostds.org/ontologies/C2SIM#SERBAN -->

    <owl:NamedIndividual rdf:about="http://www.sisostds.org/ontologies/C2SIM#SERBAN">
        <rdf:type rdf:resource="http://www.sisostds.org/ontologies/C2SIM#EthnicGroupCode"/>
        <rdfs:comment>Serb/Serbian: The ethnic group of Serb/Serbian people.</rdfs:comment>
    </owl:NamedIndividual>
    


    <!-- http://www.sisostds.org/ontologies/C2SIM#SERER -->

    <owl:NamedIndividual rdf:about="http://www.sisostds.org/ontologies/C2SIM#SERER">
        <rdf:type rdf:resource="http://www.sisostds.org/ontologies/C2SIM#EthnicGroupCode"/>
        <rdfs:comment>Serer: The ethnic group of Serer people.</rdfs:comment>
    </owl:NamedIndividual>
    


    <!-- http://www.sisostds.org/ontologies/C2SIM#SERVIC -->

    <owl:NamedIndividual rdf:about="http://www.sisostds.org/ontologies/C2SIM#SERVIC">
        <rdf:type rdf:resource="http://www.sisostds.org/ontologies/C2SIM#EthnicGroupCode"/>
        <rdfs:comment>Servicais: The ethnic group of Servicais people.</rdfs:comment>
    </owl:NamedIndividual>
    


    <!-- http://www.sisostds.org/ontologies/C2SIM#SEYISL -->

    <owl:NamedIndividual rdf:about="http://www.sisostds.org/ontologies/C2SIM#SEYISL">
        <rdf:type rdf:resource="http://www.sisostds.org/ontologies/C2SIM#EthnicGroupCode"/>
        <rdfs:comment>Seychelles Islander: The ethnic group of Seychelles Islander people.</rdfs:comment>
    </owl:NamedIndividual>
    


    <!-- http://www.sisostds.org/ontologies/C2SIM#SGP -->

    <owl:NamedIndividual rdf:about="http://www.sisostds.org/ontologies/C2SIM#SGP">
        <rdf:type rdf:resource="http://www.sisostds.org/ontologies/C2SIM#CountryCode"/>
        <rdfs:comment>Singapore: </rdfs:comment>
    </owl:NamedIndividual>
    


    <!-- http://www.sisostds.org/ontologies/C2SIM#SGS -->

    <owl:NamedIndividual rdf:about="http://www.sisostds.org/ontologies/C2SIM#SGS">
        <rdf:type rdf:resource="http://www.sisostds.org/ontologies/C2SIM#CountryCode"/>
        <rdfs:comment>South Georgia and the South Sandwich Islands: </rdfs:comment>
    </owl:NamedIndividual>
    


    <!-- http://www.sisostds.org/ontologies/C2SIM#SHAN -->

    <owl:NamedIndividual rdf:about="http://www.sisostds.org/ontologies/C2SIM#SHAN">
        <rdf:type rdf:resource="http://www.sisostds.org/ontologies/C2SIM#EthnicGroupCode"/>
        <rdfs:comment>Shan: The ethnic group of Shan people.</rdfs:comment>
    </owl:NamedIndividual>
    


    <!-- http://www.sisostds.org/ontologies/C2SIM#SHERPA -->

    <owl:NamedIndividual rdf:about="http://www.sisostds.org/ontologies/C2SIM#SHERPA">
        <rdf:type rdf:resource="http://www.sisostds.org/ontologies/C2SIM#EthnicGroupCode"/>
        <rdfs:comment>Sherpas: The ethnic group of Sherpas people.</rdfs:comment>
    </owl:NamedIndividual>
    


    <!-- http://www.sisostds.org/ontologies/C2SIM#SHIMUS -->

    <owl:NamedIndividual rdf:about="http://www.sisostds.org/ontologies/C2SIM#SHIMUS">
        <rdf:type rdf:resource="http://www.sisostds.org/ontologies/C2SIM#ReligionCode"/>
        <rdfs:comment>Shi&apos;a Muslim: One who adheres to or identifies with the Shi&apos;a Muslim doctrine.</rdfs:comment>
    </owl:NamedIndividual>
    


    <!-- http://www.sisostds.org/ontologies/C2SIM#SHINTO -->

    <owl:NamedIndividual rdf:about="http://www.sisostds.org/ontologies/C2SIM#SHINTO">
        <rdf:type rdf:resource="http://www.sisostds.org/ontologies/C2SIM#ReligionCode"/>
        <rdfs:comment>Shinto: One who adheres to or identifies with the Shinto doctrine.</rdfs:comment>
    </owl:NamedIndividual>
    


    <!-- http://www.sisostds.org/ontologies/C2SIM#SHMNSM -->

    <owl:NamedIndividual rdf:about="http://www.sisostds.org/ontologies/C2SIM#SHMNSM">
        <rdf:type rdf:resource="http://www.sisostds.org/ontologies/C2SIM#ReligionCode"/>
        <rdfs:comment>Shamanism: One who adheres to or identifies with the Shamanism doctrine.</rdfs:comment>
    </owl:NamedIndividual>
    


    <!-- http://www.sisostds.org/ontologies/C2SIM#SHN -->

    <owl:NamedIndividual rdf:about="http://www.sisostds.org/ontologies/C2SIM#SHN">
        <rdf:type rdf:resource="http://www.sisostds.org/ontologies/C2SIM#CountryCode"/>
        <rdfs:comment>Saint Helena: </rdfs:comment>
    </owl:NamedIndividual>
    


    <!-- http://www.sisostds.org/ontologies/C2SIM#SHTISL -->

    <owl:NamedIndividual rdf:about="http://www.sisostds.org/ontologies/C2SIM#SHTISL">
        <rdf:type rdf:resource="http://www.sisostds.org/ontologies/C2SIM#EthnicGroupCode"/>
        <rdfs:comment>Shetland Islander: The ethnic group of Shetland Islander people.</rdfs:comment>
    </owl:NamedIndividual>
    


    <!-- http://www.sisostds.org/ontologies/C2SIM#SHURA -->

    <owl:NamedIndividual rdf:about="http://www.sisostds.org/ontologies/C2SIM#SHURA">
        <rdf:type rdf:resource="http://www.sisostds.org/ontologies/C2SIM#OrganizationTypeCode"/>
        <rdfs:comment>Shura: A GROUP-ORGANISATION-TYPE that is an Islamic consultative council or similar advisory body.</rdfs:comment>
    </owl:NamedIndividual>
    


    <!-- http://www.sisostds.org/ontologies/C2SIM#SICLAN -->

    <owl:NamedIndividual rdf:about="http://www.sisostds.org/ontologies/C2SIM#SICLAN">
        <rdf:type rdf:resource="http://www.sisostds.org/ontologies/C2SIM#EthnicGroupCode"/>
        <rdfs:comment>Sicilian: The ethnic group of Sicilian people.</rdfs:comment>
    </owl:NamedIndividual>
    


    <!-- http://www.sisostds.org/ontologies/C2SIM#SIDAMO -->

    <owl:NamedIndividual rdf:about="http://www.sisostds.org/ontologies/C2SIM#SIDAMO">
        <rdf:type rdf:resource="http://www.sisostds.org/ontologies/C2SIM#EthnicGroupCode"/>
        <rdfs:comment>Sidamo: The ethnic group of Sidamo people.</rdfs:comment>
    </owl:NamedIndividual>
    


    <!-- http://www.sisostds.org/ontologies/C2SIM#SIKH -->

    <owl:NamedIndividual rdf:about="http://www.sisostds.org/ontologies/C2SIM#SIKH">
        <rdf:type rdf:resource="http://www.sisostds.org/ontologies/C2SIM#EthnicGroupCode"/>
        <rdf:type rdf:resource="http://www.sisostds.org/ontologies/C2SIM#ReligionCode"/>
        <rdfs:comment>Sikh: One who adheres to or identifies with the Sikh doctrine.</rdfs:comment>
        <rdfs:comment>Sikh: The ethnic group of Sikh people.</rdfs:comment>
    </owl:NamedIndividual>
    


    <!-- http://www.sisostds.org/ontologies/C2SIM#SINCHN -->

    <owl:NamedIndividual rdf:about="http://www.sisostds.org/ontologies/C2SIM#SINCHN">
        <rdf:type rdf:resource="http://www.sisostds.org/ontologies/C2SIM#EthnicGroupCode"/>
        <rdfs:comment>Singaporean Chinese: The ethnic group of Singaporean Chinese people.</rdfs:comment>
    </owl:NamedIndividual>
    


    <!-- http://www.sisostds.org/ontologies/C2SIM#SINDHI -->

    <owl:NamedIndividual rdf:about="http://www.sisostds.org/ontologies/C2SIM#SINDHI">
        <rdf:type rdf:resource="http://www.sisostds.org/ontologies/C2SIM#EthnicGroupCode"/>
        <rdfs:comment>Sindhi: The ethnic group of Sindhi people.</rdfs:comment>
    </owl:NamedIndividual>
    


    <!-- http://www.sisostds.org/ontologies/C2SIM#SINHLS -->

    <owl:NamedIndividual rdf:about="http://www.sisostds.org/ontologies/C2SIM#SINHLS">
        <rdf:type rdf:resource="http://www.sisostds.org/ontologies/C2SIM#EthnicGroupCode"/>
        <rdfs:comment>Sinhalese: The ethnic group of Sinhalese people.</rdfs:comment>
    </owl:NamedIndividual>
    


    <!-- http://www.sisostds.org/ontologies/C2SIM#SINOMA -->

    <owl:NamedIndividual rdf:about="http://www.sisostds.org/ontologies/C2SIM#SINOMA">
        <rdf:type rdf:resource="http://www.sisostds.org/ontologies/C2SIM#EthnicGroupCode"/>
        <rdfs:comment>Sino-Mauritian: The ethnic group of Sino-Mauritian people.</rdfs:comment>
    </owl:NamedIndividual>
    


    <!-- http://www.sisostds.org/ontologies/C2SIM#SJM -->

    <owl:NamedIndividual rdf:about="http://www.sisostds.org/ontologies/C2SIM#SJM">
        <rdf:type rdf:resource="http://www.sisostds.org/ontologies/C2SIM#CountryCode"/>
        <rdfs:comment>Svalbard and Jan Mayen Islands: </rdfs:comment>
    </owl:NamedIndividual>
    


    <!-- http://www.sisostds.org/ontologies/C2SIM#SLAVIC -->

    <owl:NamedIndividual rdf:about="http://www.sisostds.org/ontologies/C2SIM#SLAVIC">
        <rdf:type rdf:resource="http://www.sisostds.org/ontologies/C2SIM#EthnicGroupCode"/>
        <rdfs:comment>Slavic/Slav: The ethnic group of Slavic/Slav people.</rdfs:comment>
    </owl:NamedIndividual>
    


    <!-- http://www.sisostds.org/ontologies/C2SIM#SLB -->

    <owl:NamedIndividual rdf:about="http://www.sisostds.org/ontologies/C2SIM#SLB">
        <rdf:type rdf:resource="http://www.sisostds.org/ontologies/C2SIM#CountryCode"/>
        <rdfs:comment>Solomon Islands: </rdfs:comment>
    </owl:NamedIndividual>
    


    <!-- http://www.sisostds.org/ontologies/C2SIM#SLE -->

    <owl:NamedIndividual rdf:about="http://www.sisostds.org/ontologies/C2SIM#SLE">
        <rdf:type rdf:resource="http://www.sisostds.org/ontologies/C2SIM#CountryCode"/>
        <rdfs:comment>Sierra Leone: </rdfs:comment>
    </owl:NamedIndividual>
    


    <!-- http://www.sisostds.org/ontologies/C2SIM#SLOVAK -->

    <owl:NamedIndividual rdf:about="http://www.sisostds.org/ontologies/C2SIM#SLOVAK">
        <rdf:type rdf:resource="http://www.sisostds.org/ontologies/C2SIM#EthnicGroupCode"/>
        <rdfs:comment>Slovak: The ethnic group of Slovak people.</rdfs:comment>
    </owl:NamedIndividual>
    


    <!-- http://www.sisostds.org/ontologies/C2SIM#SLOVNE -->

    <owl:NamedIndividual rdf:about="http://www.sisostds.org/ontologies/C2SIM#SLOVNE">
        <rdf:type rdf:resource="http://www.sisostds.org/ontologies/C2SIM#EthnicGroupCode"/>
        <rdfs:comment>Slovene/Slovenian: The ethnic group of Slovene/Slovenian people.</rdfs:comment>
    </owl:NamedIndividual>
    


    <!-- http://www.sisostds.org/ontologies/C2SIM#SLV -->

    <owl:NamedIndividual rdf:about="http://www.sisostds.org/ontologies/C2SIM#SLV">
        <rdf:type rdf:resource="http://www.sisostds.org/ontologies/C2SIM#CountryCode"/>
        <rdfs:comment>El Salvador: </rdfs:comment>
    </owl:NamedIndividual>
    


    <!-- http://www.sisostds.org/ontologies/C2SIM#SLVMUS -->

    <owl:NamedIndividual rdf:about="http://www.sisostds.org/ontologies/C2SIM#SLVMUS">
        <rdf:type rdf:resource="http://www.sisostds.org/ontologies/C2SIM#ReligionCode"/>
        <rdfs:comment>Slavic Muslim: One who adheres to or identifies with the Slavic Muslim doctrine.</rdfs:comment>
    </owl:NamedIndividual>
    


    <!-- http://www.sisostds.org/ontologies/C2SIM#SLVNEC -->

    <owl:NamedIndividual rdf:about="http://www.sisostds.org/ontologies/C2SIM#SLVNEC">
        <rdf:type rdf:resource="http://www.sisostds.org/ontologies/C2SIM#EthnicGroupCode"/>
        <rdfs:comment>South Slav (formerly Yugoslav) not elsewhere classified: The not elsewhere classified ethnic groups of South Slav (formerly Yugoslav) people.</rdfs:comment>
    </owl:NamedIndividual>
    


    <!-- http://www.sisostds.org/ontologies/C2SIM#SLVNFD -->

    <owl:NamedIndividual rdf:about="http://www.sisostds.org/ontologies/C2SIM#SLVNFD">
        <rdf:type rdf:resource="http://www.sisostds.org/ontologies/C2SIM#EthnicGroupCode"/>
        <rdfs:comment>South Slav (formerly Yugoslav groups) not further defined: The not further defined ethnic groups of South Slav (formerly Yugoslav groups) people.</rdfs:comment>
    </owl:NamedIndividual>
    


    <!-- http://www.sisostds.org/ontologies/C2SIM#SMR -->

    <owl:NamedIndividual rdf:about="http://www.sisostds.org/ontologies/C2SIM#SMR">
        <rdf:type rdf:resource="http://www.sisostds.org/ontologies/C2SIM#CountryCode"/>
        <rdfs:comment>San Marino: </rdfs:comment>
    </owl:NamedIndividual>
    


    <!-- http://www.sisostds.org/ontologies/C2SIM#SOCFRD -->

    <owl:NamedIndividual rdf:about="http://www.sisostds.org/ontologies/C2SIM#SOCFRD">
        <rdf:type rdf:resource="http://www.sisostds.org/ontologies/C2SIM#ReligionCode"/>
        <rdfs:comment>Society of Friends: One who adheres to or identifies with the Society of Friends doctrine.</rdfs:comment>
    </owl:NamedIndividual>
    


    <!-- http://www.sisostds.org/ontologies/C2SIM#SOCIAL -->

    <owl:NamedIndividual rdf:about="http://www.sisostds.org/ontologies/C2SIM#SOCIAL">
        <rdf:type rdf:resource="http://www.sisostds.org/ontologies/C2SIM#OrganizationTypeCode"/>
        <rdfs:comment>Social: A GROUP-ORGANISATION-TYPE that seeks and enjoys companies of others, or characterized by friendly companionship or relations.</rdfs:comment>
    </owl:NamedIndividual>
    


    <!-- http://www.sisostds.org/ontologies/C2SIM#SOCISL -->

    <owl:NamedIndividual rdf:about="http://www.sisostds.org/ontologies/C2SIM#SOCISL">
        <rdf:type rdf:resource="http://www.sisostds.org/ontologies/C2SIM#EthnicGroupCode"/>
        <rdfs:comment>Society Islander (including Tahitian): The ethnic group of Society Islander (including Tahitian) people.</rdfs:comment>
    </owl:NamedIndividual>
    


    <!-- http://www.sisostds.org/ontologies/C2SIM#SOLISL -->

    <owl:NamedIndividual rdf:about="http://www.sisostds.org/ontologies/C2SIM#SOLISL">
        <rdf:type rdf:resource="http://www.sisostds.org/ontologies/C2SIM#EthnicGroupCode"/>
        <rdfs:comment>Solomon Islander: The ethnic group of Solomon Islander people.</rdfs:comment>
    </owl:NamedIndividual>
    


    <!-- http://www.sisostds.org/ontologies/C2SIM#SOLVEN -->

    <owl:NamedIndividual rdf:about="http://www.sisostds.org/ontologies/C2SIM#SOLVEN">
        <rdf:type rdf:resource="http://www.sisostds.org/ontologies/C2SIM#EthnicGroupCode"/>
        <rdfs:comment>Solvene: The ethnic group of Solvene people.</rdfs:comment>
    </owl:NamedIndividual>
    


    <!-- http://www.sisostds.org/ontologies/C2SIM#SOM -->

    <owl:NamedIndividual rdf:about="http://www.sisostds.org/ontologies/C2SIM#SOM">
        <rdf:type rdf:resource="http://www.sisostds.org/ontologies/C2SIM#CountryCode"/>
        <rdfs:comment>Somalia: </rdfs:comment>
    </owl:NamedIndividual>
    


    <!-- http://www.sisostds.org/ontologies/C2SIM#SOMALI -->

    <owl:NamedIndividual rdf:about="http://www.sisostds.org/ontologies/C2SIM#SOMALI">
        <rdf:type rdf:resource="http://www.sisostds.org/ontologies/C2SIM#EthnicGroupCode"/>
        <rdfs:comment>Somali: The ethnic group of Somali people.</rdfs:comment>
    </owl:NamedIndividual>
    


    <!-- http://www.sisostds.org/ontologies/C2SIM#SONGHA -->

    <owl:NamedIndividual rdf:about="http://www.sisostds.org/ontologies/C2SIM#SONGHA">
        <rdf:type rdf:resource="http://www.sisostds.org/ontologies/C2SIM#EthnicGroupCode"/>
        <rdfs:comment>Songhai: The ethnic group of Songhai people.</rdfs:comment>
    </owl:NamedIndividual>
    


    <!-- http://www.sisostds.org/ontologies/C2SIM#SOTHO -->

    <owl:NamedIndividual rdf:about="http://www.sisostds.org/ontologies/C2SIM#SOTHO">
        <rdf:type rdf:resource="http://www.sisostds.org/ontologies/C2SIM#EthnicGroupCode"/>
        <rdfs:comment>Sotho: The ethnic group of Sotho people.</rdfs:comment>
    </owl:NamedIndividual>
    


    <!-- http://www.sisostds.org/ontologies/C2SIM#SOUAFR -->

    <owl:NamedIndividual rdf:about="http://www.sisostds.org/ontologies/C2SIM#SOUAFR">
        <rdf:type rdf:resource="http://www.sisostds.org/ontologies/C2SIM#EthnicGroupCode"/>
        <rdfs:comment>South African: The ethnic group of South African people.</rdfs:comment>
    </owl:NamedIndividual>
    


    <!-- http://www.sisostds.org/ontologies/C2SIM#SOUAMR -->

    <owl:NamedIndividual rdf:about="http://www.sisostds.org/ontologies/C2SIM#SOUAMR">
        <rdf:type rdf:resource="http://www.sisostds.org/ontologies/C2SIM#EthnicGroupCode"/>
        <rdfs:comment>South American Indian: The ethnic group of South American Indian people.</rdfs:comment>
    </owl:NamedIndividual>
    


    <!-- http://www.sisostds.org/ontologies/C2SIM#SOUNFD -->

    <owl:NamedIndividual rdf:about="http://www.sisostds.org/ontologies/C2SIM#SOUNFD">
        <rdf:type rdf:resource="http://www.sisostds.org/ontologies/C2SIM#EthnicGroupCode"/>
        <rdfs:comment>Southeast Asian not further defined: The not further defined ethnic groups of Southeast Asian people.</rdfs:comment>
    </owl:NamedIndividual>
    


    <!-- http://www.sisostds.org/ontologies/C2SIM#SOUSSO -->

    <owl:NamedIndividual rdf:about="http://www.sisostds.org/ontologies/C2SIM#SOUSSO">
        <rdf:type rdf:resource="http://www.sisostds.org/ontologies/C2SIM#EthnicGroupCode"/>
        <rdfs:comment>Soussou: The ethnic group of Soussou people.</rdfs:comment>
    </owl:NamedIndividual>
    


    <!-- http://www.sisostds.org/ontologies/C2SIM#SOUTHA -->

    <owl:NamedIndividual rdf:about="http://www.sisostds.org/ontologies/C2SIM#SOUTHA">
        <rdf:type rdf:resource="http://www.sisostds.org/ontologies/C2SIM#EthnicGroupCode"/>
        <rdfs:comment>South Asian: The ethnic group of South Asian people.</rdfs:comment>
    </owl:NamedIndividual>
    


    <!-- http://www.sisostds.org/ontologies/C2SIM#SPANSH -->

    <owl:NamedIndividual rdf:about="http://www.sisostds.org/ontologies/C2SIM#SPANSH">
        <rdf:type rdf:resource="http://www.sisostds.org/ontologies/C2SIM#EthnicGroupCode"/>
        <rdfs:comment>Spanish: The ethnic group of Spanish people.</rdfs:comment>
    </owl:NamedIndividual>
    


    <!-- http://www.sisostds.org/ontologies/C2SIM#SPM -->

    <owl:NamedIndividual rdf:about="http://www.sisostds.org/ontologies/C2SIM#SPM">
        <rdf:type rdf:resource="http://www.sisostds.org/ontologies/C2SIM#CountryCode"/>
        <rdfs:comment>Saint Pierre and Miquelon: </rdfs:comment>
    </owl:NamedIndividual>
    


    <!-- http://www.sisostds.org/ontologies/C2SIM#SPRCLT -->

    <owl:NamedIndividual rdf:about="http://www.sisostds.org/ontologies/C2SIM#SPRCLT">
        <rdf:type rdf:resource="http://www.sisostds.org/ontologies/C2SIM#ReligionCode"/>
        <rdfs:comment>Spiritual Cults: One who adheres to or identifies with the Spiritual Cults doctrine.</rdfs:comment>
    </owl:NamedIndividual>
    


    <!-- http://www.sisostds.org/ontologies/C2SIM#SRB -->

    <owl:NamedIndividual rdf:about="http://www.sisostds.org/ontologies/C2SIM#SRB">
        <rdf:type rdf:resource="http://www.sisostds.org/ontologies/C2SIM#CountryCode"/>
        <rdfs:comment>Serbia: New entry after split of Serbia and Montenegro.</rdfs:comment>
    </owl:NamedIndividual>
    


    <!-- http://www.sisostds.org/ontologies/C2SIM#SRINEC -->

    <owl:NamedIndividual rdf:about="http://www.sisostds.org/ontologies/C2SIM#SRINEC">
        <rdf:type rdf:resource="http://www.sisostds.org/ontologies/C2SIM#EthnicGroupCode"/>
        <rdfs:comment>Sri Lankan not elsewhere classified: The not elsewhere classified ethnic groups of Sri Lankan people.</rdfs:comment>
    </owl:NamedIndividual>
    


    <!-- http://www.sisostds.org/ontologies/C2SIM#SRINFD -->

    <owl:NamedIndividual rdf:about="http://www.sisostds.org/ontologies/C2SIM#SRINFD">
        <rdf:type rdf:resource="http://www.sisostds.org/ontologies/C2SIM#EthnicGroupCode"/>
        <rdfs:comment>Sri Lankan not further defined: The not further defined ethnic groups of Sri Lankan people.</rdfs:comment>
    </owl:NamedIndividual>
    


    <!-- http://www.sisostds.org/ontologies/C2SIM#SRITML -->

    <owl:NamedIndividual rdf:about="http://www.sisostds.org/ontologies/C2SIM#SRITML">
        <rdf:type rdf:resource="http://www.sisostds.org/ontologies/C2SIM#EthnicGroupCode"/>
        <rdfs:comment>Sri Lankan Tamil: The ethnic group of Sri Lankan Tamil people.</rdfs:comment>
    </owl:NamedIndividual>
    


    <!-- http://www.sisostds.org/ontologies/C2SIM#STP -->

    <owl:NamedIndividual rdf:about="http://www.sisostds.org/ontologies/C2SIM#STP">
        <rdf:type rdf:resource="http://www.sisostds.org/ontologies/C2SIM#CountryCode"/>
        <rdfs:comment>Sao Tome and Principe: </rdfs:comment>
    </owl:NamedIndividual>
    


    <!-- http://www.sisostds.org/ontologies/C2SIM#STREND -->

    <owl:NamedIndividual rdf:about="http://www.sisostds.org/ontologies/C2SIM#STREND">
        <rdf:type rdf:resource="http://www.sisostds.org/ontologies/C2SIM#ActionTemporalAssociationCode"/>
        <rdfs:comment>Starts after end of: The subject ACTION starts after the object ACTION ends.</rdfs:comment>
    </owl:NamedIndividual>
    


    <!-- http://www.sisostds.org/ontologies/C2SIM#STRENE -->

    <owl:NamedIndividual rdf:about="http://www.sisostds.org/ontologies/C2SIM#STRENE">
        <rdf:type rdf:resource="http://www.sisostds.org/ontologies/C2SIM#ActionTemporalAssociationCode"/>
        <rdfs:comment>Starts no earlier than after end of: The subject ACTION starts no earlier than the end of the object ACTION augmented by a fixed duration.</rdfs:comment>
    </owl:NamedIndividual>
    


    <!-- http://www.sisostds.org/ontologies/C2SIM#STRENL -->

    <owl:NamedIndividual rdf:about="http://www.sisostds.org/ontologies/C2SIM#STRENL">
        <rdf:type rdf:resource="http://www.sisostds.org/ontologies/C2SIM#ActionTemporalAssociationCode"/>
        <rdfs:comment>Starts no later than after end of: The subject ACTION starts no later than the end of object ACTION augmented by a fixed duration.</rdfs:comment>
    </owl:NamedIndividual>
    


    <!-- http://www.sisostds.org/ontologies/C2SIM#STRSNE -->

    <owl:NamedIndividual rdf:about="http://www.sisostds.org/ontologies/C2SIM#STRSNE">
        <rdf:type rdf:resource="http://www.sisostds.org/ontologies/C2SIM#ActionTemporalAssociationCode"/>
        <rdfs:comment>Starts no earlier than after start of: The subject ACTION starts no earlier than the start of the object ACTION augmented by a fixed duration.</rdfs:comment>
    </owl:NamedIndividual>
    


    <!-- http://www.sisostds.org/ontologies/C2SIM#STRSNL -->

    <owl:NamedIndividual rdf:about="http://www.sisostds.org/ontologies/C2SIM#STRSNL">
        <rdf:type rdf:resource="http://www.sisostds.org/ontologies/C2SIM#ActionTemporalAssociationCode"/>
        <rdfs:comment>Starts no later than after start of: The subject ACTION starts no later than the start of object ACTION augmented by a fixed duration.</rdfs:comment>
    </owl:NamedIndividual>
    


    <!-- http://www.sisostds.org/ontologies/C2SIM#STRSTR -->

    <owl:NamedIndividual rdf:about="http://www.sisostds.org/ontologies/C2SIM#STRSTR">
        <rdf:type rdf:resource="http://www.sisostds.org/ontologies/C2SIM#ActionTemporalAssociationCode"/>
        <rdfs:comment>Starts after start of: The subject ACTION starts after the object ACTION starts.</rdfs:comment>
    </owl:NamedIndividual>
    


    <!-- http://www.sisostds.org/ontologies/C2SIM#SUHH -->

    <owl:NamedIndividual rdf:about="http://www.sisostds.org/ontologies/C2SIM#SUHH">
        <rdf:type rdf:resource="http://www.sisostds.org/ontologies/C2SIM#CountryCode"/>
        <rdfs:comment>Union of Soviet Socialist Republics (former): USSR (1992)</rdfs:comment>
    </owl:NamedIndividual>
    


    <!-- http://www.sisostds.org/ontologies/C2SIM#SUNDAN -->

    <owl:NamedIndividual rdf:about="http://www.sisostds.org/ontologies/C2SIM#SUNDAN">
        <rdf:type rdf:resource="http://www.sisostds.org/ontologies/C2SIM#EthnicGroupCode"/>
        <rdfs:comment>Sundanese: The ethnic group of Sundanese people.</rdfs:comment>
    </owl:NamedIndividual>
    


    <!-- http://www.sisostds.org/ontologies/C2SIM#SUNMUS -->

    <owl:NamedIndividual rdf:about="http://www.sisostds.org/ontologies/C2SIM#SUNMUS">
        <rdf:type rdf:resource="http://www.sisostds.org/ontologies/C2SIM#ReligionCode"/>
        <rdfs:comment>Sunni Muslim: One who adheres to or identifies with the Sunni Muslim doctrine.</rdfs:comment>
    </owl:NamedIndividual>
    


    <!-- http://www.sisostds.org/ontologies/C2SIM#SUR -->

    <owl:NamedIndividual rdf:about="http://www.sisostds.org/ontologies/C2SIM#SUR">
        <rdf:type rdf:resource="http://www.sisostds.org/ontologies/C2SIM#CountryCode"/>
        <rdfs:comment>Suriname: </rdfs:comment>
    </owl:NamedIndividual>
    


    <!-- http://www.sisostds.org/ontologies/C2SIM#SVK -->

    <owl:NamedIndividual rdf:about="http://www.sisostds.org/ontologies/C2SIM#SVK">
        <rdf:type rdf:resource="http://www.sisostds.org/ontologies/C2SIM#CountryCode"/>
        <rdfs:comment>Slovakia: </rdfs:comment>
    </owl:NamedIndividual>
    


    <!-- http://www.sisostds.org/ontologies/C2SIM#SVN -->

    <owl:NamedIndividual rdf:about="http://www.sisostds.org/ontologies/C2SIM#SVN">
        <rdf:type rdf:resource="http://www.sisostds.org/ontologies/C2SIM#CountryCode"/>
        <rdfs:comment>Slovenia: </rdfs:comment>
    </owl:NamedIndividual>
    


    <!-- http://www.sisostds.org/ontologies/C2SIM#SVNADV -->

    <owl:NamedIndividual rdf:about="http://www.sisostds.org/ontologies/C2SIM#SVNADV">
        <rdf:type rdf:resource="http://www.sisostds.org/ontologies/C2SIM#ReligionCode"/>
        <rdfs:comment>Seventh-day Adventist: One who adheres to or identifies with the Seventh-day Adventist doctrine.</rdfs:comment>
    </owl:NamedIndividual>
    


    <!-- http://www.sisostds.org/ontologies/C2SIM#SWE -->

    <owl:NamedIndividual rdf:about="http://www.sisostds.org/ontologies/C2SIM#SWE">
        <rdf:type rdf:resource="http://www.sisostds.org/ontologies/C2SIM#CountryCode"/>
        <rdfs:comment>Sweden: </rdfs:comment>
    </owl:NamedIndividual>
    


    <!-- http://www.sisostds.org/ontologies/C2SIM#SWEDSH -->

    <owl:NamedIndividual rdf:about="http://www.sisostds.org/ontologies/C2SIM#SWEDSH">
        <rdf:type rdf:resource="http://www.sisostds.org/ontologies/C2SIM#EthnicGroupCode"/>
        <rdfs:comment>Swedish: The ethnic group of Swedish people.</rdfs:comment>
    </owl:NamedIndividual>
    


    <!-- http://www.sisostds.org/ontologies/C2SIM#SWISS -->

    <owl:NamedIndividual rdf:about="http://www.sisostds.org/ontologies/C2SIM#SWISS">
        <rdf:type rdf:resource="http://www.sisostds.org/ontologies/C2SIM#EthnicGroupCode"/>
        <rdfs:comment>Swiss: The ethnic group of Swiss people.</rdfs:comment>
    </owl:NamedIndividual>
    


    <!-- http://www.sisostds.org/ontologies/C2SIM#SWZ -->

    <owl:NamedIndividual rdf:about="http://www.sisostds.org/ontologies/C2SIM#SWZ">
        <rdf:type rdf:resource="http://www.sisostds.org/ontologies/C2SIM#CountryCode"/>
        <rdfs:comment>Swaziland: </rdfs:comment>
    </owl:NamedIndividual>
    


    <!-- http://www.sisostds.org/ontologies/C2SIM#SYC -->

    <owl:NamedIndividual rdf:about="http://www.sisostds.org/ontologies/C2SIM#SYC">
        <rdf:type rdf:resource="http://www.sisostds.org/ontologies/C2SIM#CountryCode"/>
        <rdfs:comment>Seychelles: </rdfs:comment>
    </owl:NamedIndividual>
    


    <!-- http://www.sisostds.org/ontologies/C2SIM#SYNCHN -->

    <owl:NamedIndividual rdf:about="http://www.sisostds.org/ontologies/C2SIM#SYNCHN">
        <rdf:type rdf:resource="http://www.sisostds.org/ontologies/C2SIM#ReligionCode"/>
        <rdfs:comment>Syncretic Chondogyo: One who adheres to or identifies with the Syncretic Chondogyo doctrine.</rdfs:comment>
    </owl:NamedIndividual>
    


    <!-- http://www.sisostds.org/ontologies/C2SIM#SYR -->

    <owl:NamedIndividual rdf:about="http://www.sisostds.org/ontologies/C2SIM#SYR">
        <rdf:type rdf:resource="http://www.sisostds.org/ontologies/C2SIM#CountryCode"/>
        <rdfs:comment>Syrian Arab Republic: </rdfs:comment>
    </owl:NamedIndividual>
    


    <!-- http://www.sisostds.org/ontologies/C2SIM#SYRANL -->

    <owl:NamedIndividual rdf:about="http://www.sisostds.org/ontologies/C2SIM#SYRANL">
        <rdf:type rdf:resource="http://www.sisostds.org/ontologies/C2SIM#EthnicGroupCode"/>
        <rdfs:comment>Syrian-Lebanese: The ethnic group of Syrian-Lebanese people.</rdfs:comment>
    </owl:NamedIndividual>
    


    <!-- http://www.sisostds.org/ontologies/C2SIM#SYRIAN -->

    <owl:NamedIndividual rdf:about="http://www.sisostds.org/ontologies/C2SIM#SYRIAN">
        <rdf:type rdf:resource="http://www.sisostds.org/ontologies/C2SIM#EthnicGroupCode"/>
        <rdfs:comment>Syrian: The ethnic group of Syrian people.</rdfs:comment>
    </owl:NamedIndividual>
    


    <!-- http://www.sisostds.org/ontologies/C2SIM#SYROLE -->

    <owl:NamedIndividual rdf:about="http://www.sisostds.org/ontologies/C2SIM#SYROLE">
        <rdf:type rdf:resource="http://www.sisostds.org/ontologies/C2SIM#EthnicGroupCode"/>
        <rdfs:comment>Syro-Lebanese: The ethnic group of Syro-Lebanese people.</rdfs:comment>
    </owl:NamedIndividual>
    


    <!-- http://www.sisostds.org/ontologies/C2SIM#Secret -->

    <owl:NamedIndividual rdf:about="http://www.sisostds.org/ontologies/C2SIM#Secret">
        <rdf:type rdf:resource="http://www.sisostds.org/ontologies/C2SIM#SecurityClassificationCode"/>
    </owl:NamedIndividual>
    


    <!-- http://www.sisostds.org/ontologies/C2SIM#TAHITN -->

    <owl:NamedIndividual rdf:about="http://www.sisostds.org/ontologies/C2SIM#TAHITN">
        <rdf:type rdf:resource="http://www.sisostds.org/ontologies/C2SIM#EthnicGroupCode"/>
        <rdfs:comment>Tahitian (including Society Islander): The ethnic group of Tahitian (including Society Islander) people.</rdfs:comment>
    </owl:NamedIndividual>
    


    <!-- http://www.sisostds.org/ontologies/C2SIM#TAICHN -->

    <owl:NamedIndividual rdf:about="http://www.sisostds.org/ontologies/C2SIM#TAICHN">
        <rdf:type rdf:resource="http://www.sisostds.org/ontologies/C2SIM#EthnicGroupCode"/>
        <rdfs:comment>Taiwanese Chinese: The ethnic group of Taiwanese Chinese people.</rdfs:comment>
    </owl:NamedIndividual>
    


    <!-- http://www.sisostds.org/ontologies/C2SIM#TAJIK -->

    <owl:NamedIndividual rdf:about="http://www.sisostds.org/ontologies/C2SIM#TAJIK">
        <rdf:type rdf:resource="http://www.sisostds.org/ontologies/C2SIM#EthnicGroupCode"/>
        <rdfs:comment>Tajik: The ethnic group of Tajik people.</rdfs:comment>
    </owl:NamedIndividual>
    


    <!-- http://www.sisostds.org/ontologies/C2SIM#TAMANG -->

    <owl:NamedIndividual rdf:about="http://www.sisostds.org/ontologies/C2SIM#TAMANG">
        <rdf:type rdf:resource="http://www.sisostds.org/ontologies/C2SIM#EthnicGroupCode"/>
        <rdfs:comment>Tamangs: The ethnic group of Tamangs people.</rdfs:comment>
    </owl:NamedIndividual>
    


    <!-- http://www.sisostds.org/ontologies/C2SIM#TAMIL -->

    <owl:NamedIndividual rdf:about="http://www.sisostds.org/ontologies/C2SIM#TAMIL">
        <rdf:type rdf:resource="http://www.sisostds.org/ontologies/C2SIM#EthnicGroupCode"/>
        <rdfs:comment>Tamil: The ethnic group of Tamil people.</rdfs:comment>
    </owl:NamedIndividual>
    


    <!-- http://www.sisostds.org/ontologies/C2SIM#TAOISM -->

    <owl:NamedIndividual rdf:about="http://www.sisostds.org/ontologies/C2SIM#TAOISM">
        <rdf:type rdf:resource="http://www.sisostds.org/ontologies/C2SIM#ReligionCode"/>
        <rdfs:comment>Taoism: One who adheres to or identifies with the Taoism doctrine.</rdfs:comment>
    </owl:NamedIndividual>
    


    <!-- http://www.sisostds.org/ontologies/C2SIM#TASKABRT -->

    <owl:NamedIndividual rdf:about="http://www.sisostds.org/ontologies/C2SIM#TASKABRT">
        <rdf:type rdf:resource="http://www.sisostds.org/ontologies/C2SIM#TaskStatusCode"/>
        <rdfs:comment>Aborted.</rdfs:comment>
    </owl:NamedIndividual>
    


    <!-- http://www.sisostds.org/ontologies/C2SIM#TASKCMPLT -->

    <owl:NamedIndividual rdf:about="http://www.sisostds.org/ontologies/C2SIM#TASKCMPLT">
        <rdf:type rdf:resource="http://www.sisostds.org/ontologies/C2SIM#TaskStatusCode"/>
        <rdfs:comment>Completed</rdfs:comment>
    </owl:NamedIndividual>
    


    <!-- http://www.sisostds.org/ontologies/C2SIM#TASKINPRG -->

    <owl:NamedIndividual rdf:about="http://www.sisostds.org/ontologies/C2SIM#TASKINPRG">
        <rdf:type rdf:resource="http://www.sisostds.org/ontologies/C2SIM#TaskStatusCode"/>
        <rdfs:comment>Task in progress.</rdfs:comment>
    </owl:NamedIndividual>
    


    <!-- http://www.sisostds.org/ontologies/C2SIM#TASKPEND -->

    <owl:NamedIndividual rdf:about="http://www.sisostds.org/ontologies/C2SIM#TASKPEND">
        <rdf:type rdf:resource="http://www.sisostds.org/ontologies/C2SIM#TaskStatusCode"/>
        <rdfs:comment>Task pending (not yet started).</rdfs:comment>
    </owl:NamedIndividual>
    


    <!-- http://www.sisostds.org/ontologies/C2SIM#TASKSTRT -->

    <owl:NamedIndividual rdf:about="http://www.sisostds.org/ontologies/C2SIM#TASKSTRT">
        <rdf:type rdf:resource="http://www.sisostds.org/ontologies/C2SIM#TaskStatusCode"/>
        <rdfs:comment>Task started.</rdfs:comment>
    </owl:NamedIndividual>
    


    <!-- http://www.sisostds.org/ontologies/C2SIM#TATAR -->

    <owl:NamedIndividual rdf:about="http://www.sisostds.org/ontologies/C2SIM#TATAR">
        <rdf:type rdf:resource="http://www.sisostds.org/ontologies/C2SIM#EthnicGroupCode"/>
        <rdfs:comment>Tatar: The ethnic group of Tatar people.</rdfs:comment>
    </owl:NamedIndividual>
    


    <!-- http://www.sisostds.org/ontologies/C2SIM#TBTBUD -->

    <owl:NamedIndividual rdf:about="http://www.sisostds.org/ontologies/C2SIM#TBTBUD">
        <rdf:type rdf:resource="http://www.sisostds.org/ontologies/C2SIM#ReligionCode"/>
        <rdfs:comment>Tibetan Buddhist: One who adheres to or identifies with the Tibetan Buddhist doctrine.</rdfs:comment>
    </owl:NamedIndividual>
    


    <!-- http://www.sisostds.org/ontologies/C2SIM#TCA -->

    <owl:NamedIndividual rdf:about="http://www.sisostds.org/ontologies/C2SIM#TCA">
        <rdf:type rdf:resource="http://www.sisostds.org/ontologies/C2SIM#CountryCode"/>
        <rdfs:comment>Turks and Caicos Islands: </rdfs:comment>
    </owl:NamedIndividual>
    


    <!-- http://www.sisostds.org/ontologies/C2SIM#TCD -->

    <owl:NamedIndividual rdf:about="http://www.sisostds.org/ontologies/C2SIM#TCD">
        <rdf:type rdf:resource="http://www.sisostds.org/ontologies/C2SIM#CountryCode"/>
        <rdfs:comment>Chad: </rdfs:comment>
    </owl:NamedIndividual>
    


    <!-- http://www.sisostds.org/ontologies/C2SIM#TEKE -->

    <owl:NamedIndividual rdf:about="http://www.sisostds.org/ontologies/C2SIM#TEKE">
        <rdf:type rdf:resource="http://www.sisostds.org/ontologies/C2SIM#EthnicGroupCode"/>
        <rdfs:comment>Teke: The ethnic group of Teke people.</rdfs:comment>
    </owl:NamedIndividual>
    


    <!-- http://www.sisostds.org/ontologies/C2SIM#TERRST -->

    <owl:NamedIndividual rdf:about="http://www.sisostds.org/ontologies/C2SIM#TERRST">
        <rdf:type rdf:resource="http://www.sisostds.org/ontologies/C2SIM#OrganizationTypeCode"/>
        <rdfs:comment>Terrorist: A GROUP-ORGANISATION-TYPE that comprises persons that attempt to further their views by a system of coercive intimidation.</rdfs:comment>
    </owl:NamedIndividual>
    


    <!-- http://www.sisostds.org/ontologies/C2SIM#TEUTON -->

    <owl:NamedIndividual rdf:about="http://www.sisostds.org/ontologies/C2SIM#TEUTON">
        <rdf:type rdf:resource="http://www.sisostds.org/ontologies/C2SIM#EthnicGroupCode"/>
        <rdfs:comment>Teutonic: The ethnic group of Teutonic people.</rdfs:comment>
    </owl:NamedIndividual>
    


    <!-- http://www.sisostds.org/ontologies/C2SIM#TGO -->

    <owl:NamedIndividual rdf:about="http://www.sisostds.org/ontologies/C2SIM#TGO">
        <rdf:type rdf:resource="http://www.sisostds.org/ontologies/C2SIM#CountryCode"/>
        <rdfs:comment>Togo: </rdfs:comment>
    </owl:NamedIndividual>
    


    <!-- http://www.sisostds.org/ontologies/C2SIM#THA -->

    <owl:NamedIndividual rdf:about="http://www.sisostds.org/ontologies/C2SIM#THA">
        <rdf:type rdf:resource="http://www.sisostds.org/ontologies/C2SIM#CountryCode"/>
        <rdfs:comment>Thailand: </rdfs:comment>
    </owl:NamedIndividual>
    


    <!-- http://www.sisostds.org/ontologies/C2SIM#THAI -->

    <owl:NamedIndividual rdf:about="http://www.sisostds.org/ontologies/C2SIM#THAI">
        <rdf:type rdf:resource="http://www.sisostds.org/ontologies/C2SIM#EthnicGroupCode"/>
        <rdfs:comment>Thai/Tai/Siamese: The ethnic group of Thai/Tai/Siamese people.</rdfs:comment>
    </owl:NamedIndividual>
    


    <!-- http://www.sisostds.org/ontologies/C2SIM#THRVBD -->

    <owl:NamedIndividual rdf:about="http://www.sisostds.org/ontologies/C2SIM#THRVBD">
        <rdf:type rdf:resource="http://www.sisostds.org/ontologies/C2SIM#ReligionCode"/>
        <rdfs:comment>Theravada Buddhism: One who adheres to or identifies with the Theravada Buddhism doctrine.</rdfs:comment>
    </owl:NamedIndividual>
    


    <!-- http://www.sisostds.org/ontologies/C2SIM#TIBETN -->

    <owl:NamedIndividual rdf:about="http://www.sisostds.org/ontologies/C2SIM#TIBETN">
        <rdf:type rdf:resource="http://www.sisostds.org/ontologies/C2SIM#EthnicGroupCode"/>
        <rdfs:comment>Tibetan: The ethnic group of Tibetan people.</rdfs:comment>
    </owl:NamedIndividual>
    


    <!-- http://www.sisostds.org/ontologies/C2SIM#TIGREA -->

    <owl:NamedIndividual rdf:about="http://www.sisostds.org/ontologies/C2SIM#TIGREA">
        <rdf:type rdf:resource="http://www.sisostds.org/ontologies/C2SIM#EthnicGroupCode"/>
        <rdfs:comment>Tigrean: The ethnic group of Tigrean people.</rdfs:comment>
    </owl:NamedIndividual>
    


    <!-- http://www.sisostds.org/ontologies/C2SIM#TJK -->

    <owl:NamedIndividual rdf:about="http://www.sisostds.org/ontologies/C2SIM#TJK">
        <rdf:type rdf:resource="http://www.sisostds.org/ontologies/C2SIM#CountryCode"/>
        <rdfs:comment>Tajikistan: </rdfs:comment>
    </owl:NamedIndividual>
    


    <!-- http://www.sisostds.org/ontologies/C2SIM#TKL -->

    <owl:NamedIndividual rdf:about="http://www.sisostds.org/ontologies/C2SIM#TKL">
        <rdf:type rdf:resource="http://www.sisostds.org/ontologies/C2SIM#CountryCode"/>
        <rdfs:comment>Tokelau: </rdfs:comment>
    </owl:NamedIndividual>
    


    <!-- http://www.sisostds.org/ontologies/C2SIM#TKM -->

    <owl:NamedIndividual rdf:about="http://www.sisostds.org/ontologies/C2SIM#TKM">
        <rdf:type rdf:resource="http://www.sisostds.org/ontologies/C2SIM#CountryCode"/>
        <rdfs:comment>Turkmenistan: </rdfs:comment>
    </owl:NamedIndividual>
    


    <!-- http://www.sisostds.org/ontologies/C2SIM#TLS -->

    <owl:NamedIndividual rdf:about="http://www.sisostds.org/ontologies/C2SIM#TLS">
        <rdf:type rdf:resource="http://www.sisostds.org/ontologies/C2SIM#CountryCode"/>
        <rdfs:comment>Timor-Leste: Formerly East Timor (2002)</rdfs:comment>
    </owl:NamedIndividual>
    


    <!-- http://www.sisostds.org/ontologies/C2SIM#TOKELN -->

    <owl:NamedIndividual rdf:about="http://www.sisostds.org/ontologies/C2SIM#TOKELN">
        <rdf:type rdf:resource="http://www.sisostds.org/ontologies/C2SIM#EthnicGroupCode"/>
        <rdfs:comment>Tokelauan: The ethnic group of Tokelauan people.</rdfs:comment>
    </owl:NamedIndividual>
    


    <!-- http://www.sisostds.org/ontologies/C2SIM#TON -->

    <owl:NamedIndividual rdf:about="http://www.sisostds.org/ontologies/C2SIM#TON">
        <rdf:type rdf:resource="http://www.sisostds.org/ontologies/C2SIM#CountryCode"/>
        <rdfs:comment>Tonga: </rdfs:comment>
    </owl:NamedIndividual>
    


    <!-- http://www.sisostds.org/ontologies/C2SIM#TONGAN -->

    <owl:NamedIndividual rdf:about="http://www.sisostds.org/ontologies/C2SIM#TONGAN">
        <rdf:type rdf:resource="http://www.sisostds.org/ontologies/C2SIM#EthnicGroupCode"/>
        <rdfs:comment>Tongan: The ethnic group of Tongan people.</rdfs:comment>
    </owl:NamedIndividual>
    


    <!-- http://www.sisostds.org/ontologies/C2SIM#TONGAS -->

    <owl:NamedIndividual rdf:about="http://www.sisostds.org/ontologies/C2SIM#TONGAS">
        <rdf:type rdf:resource="http://www.sisostds.org/ontologies/C2SIM#EthnicGroupCode"/>
        <rdfs:comment>Tongas: The ethnic group of Tongas people.</rdfs:comment>
    </owl:NamedIndividual>
    


    <!-- http://www.sisostds.org/ontologies/C2SIM#TORISL -->

    <owl:NamedIndividual rdf:about="http://www.sisostds.org/ontologies/C2SIM#TORISL">
        <rdf:type rdf:resource="http://www.sisostds.org/ontologies/C2SIM#EthnicGroupCode"/>
        <rdfs:comment>Torres Strait Islander/Thursday Islander: The ethnic group of Torres Strait Islander/Thursday Islander people.</rdfs:comment>
    </owl:NamedIndividual>
    


    <!-- http://www.sisostds.org/ontologies/C2SIM#TOUBOU -->

    <owl:NamedIndividual rdf:about="http://www.sisostds.org/ontologies/C2SIM#TOUBOU">
        <rdf:type rdf:resource="http://www.sisostds.org/ontologies/C2SIM#EthnicGroupCode"/>
        <rdfs:comment>Toubou: The ethnic group of Toubou people.</rdfs:comment>
    </owl:NamedIndividual>
    


    <!-- http://www.sisostds.org/ontologies/C2SIM#TOUCOU -->

    <owl:NamedIndividual rdf:about="http://www.sisostds.org/ontologies/C2SIM#TOUCOU">
        <rdf:type rdf:resource="http://www.sisostds.org/ontologies/C2SIM#EthnicGroupCode"/>
        <rdfs:comment>Toucouleur: The ethnic group of Toucouleur people.</rdfs:comment>
    </owl:NamedIndividual>
    


    <!-- http://www.sisostds.org/ontologies/C2SIM#TRBREL -->

    <owl:NamedIndividual rdf:about="http://www.sisostds.org/ontologies/C2SIM#TRBREL">
        <rdf:type rdf:resource="http://www.sisostds.org/ontologies/C2SIM#ReligionCode"/>
        <rdfs:comment>Tribal Religion: One who adheres to or identifies with the Tribal Religion doctrine.</rdfs:comment>
    </owl:NamedIndividual>
    


    <!-- http://www.sisostds.org/ontologies/C2SIM#TRD -->

    <owl:NamedIndividual rdf:about="http://www.sisostds.org/ontologies/C2SIM#TRD">
        <rdf:type rdf:resource="http://www.sisostds.org/ontologies/C2SIM#ReligionCode"/>
        <rdfs:comment>Traditional: One who adheres to or identifies with the Traditional doctrine.</rdfs:comment>
    </owl:NamedIndividual>
    


    <!-- http://www.sisostds.org/ontologies/C2SIM#TRDMYN -->

    <owl:NamedIndividual rdf:about="http://www.sisostds.org/ontologies/C2SIM#TRDMYN">
        <rdf:type rdf:resource="http://www.sisostds.org/ontologies/C2SIM#ReligionCode"/>
        <rdfs:comment>Traditional Mayan: One who adheres to or identifies with the Traditional Mayan doctrine.</rdfs:comment>
    </owl:NamedIndividual>
    


    <!-- http://www.sisostds.org/ontologies/C2SIM#TRIBAL -->

    <owl:NamedIndividual rdf:about="http://www.sisostds.org/ontologies/C2SIM#TRIBAL">
        <rdf:type rdf:resource="http://www.sisostds.org/ontologies/C2SIM#OrganizationTypeCode"/>
        <rdfs:comment>Tribal: A GROUP-ORGANISATION-TYPE consisting of a number of families, clans, or other groups who share a common ancestry and culture.</rdfs:comment>
    </owl:NamedIndividual>
    


    <!-- http://www.sisostds.org/ontologies/C2SIM#TSIMHE -->

    <owl:NamedIndividual rdf:about="http://www.sisostds.org/ontologies/C2SIM#TSIMHE">
        <rdf:type rdf:resource="http://www.sisostds.org/ontologies/C2SIM#EthnicGroupCode"/>
        <rdfs:comment>Tsimihety: The ethnic group of Tsimihety people.</rdfs:comment>
    </owl:NamedIndividual>
    


    <!-- http://www.sisostds.org/ontologies/C2SIM#TTO -->

    <owl:NamedIndividual rdf:about="http://www.sisostds.org/ontologies/C2SIM#TTO">
        <rdf:type rdf:resource="http://www.sisostds.org/ontologies/C2SIM#CountryCode"/>
        <rdfs:comment>Trinidad and Tobago: </rdfs:comment>
    </owl:NamedIndividual>
    


    <!-- http://www.sisostds.org/ontologies/C2SIM#TUAISL -->

    <owl:NamedIndividual rdf:about="http://www.sisostds.org/ontologies/C2SIM#TUAISL">
        <rdf:type rdf:resource="http://www.sisostds.org/ontologies/C2SIM#EthnicGroupCode"/>
        <rdfs:comment>Tuamotu Islander: The ethnic group of Tuamotu Islander people.</rdfs:comment>
    </owl:NamedIndividual>
    


    <!-- http://www.sisostds.org/ontologies/C2SIM#TUAREG -->

    <owl:NamedIndividual rdf:about="http://www.sisostds.org/ontologies/C2SIM#TUAREG">
        <rdf:type rdf:resource="http://www.sisostds.org/ontologies/C2SIM#EthnicGroupCode"/>
        <rdfs:comment>Tuareg: The ethnic group of Tuareg people.</rdfs:comment>
    </owl:NamedIndividual>
    


    <!-- http://www.sisostds.org/ontologies/C2SIM#TUMBUK -->

    <owl:NamedIndividual rdf:about="http://www.sisostds.org/ontologies/C2SIM#TUMBUK">
        <rdf:type rdf:resource="http://www.sisostds.org/ontologies/C2SIM#EthnicGroupCode"/>
        <rdfs:comment>Tumbuko: The ethnic group of Tumbuko people.</rdfs:comment>
    </owl:NamedIndividual>
    


    <!-- http://www.sisostds.org/ontologies/C2SIM#TUN -->

    <owl:NamedIndividual rdf:about="http://www.sisostds.org/ontologies/C2SIM#TUN">
        <rdf:type rdf:resource="http://www.sisostds.org/ontologies/C2SIM#CountryCode"/>
        <rdfs:comment>Tunisia: </rdfs:comment>
    </owl:NamedIndividual>
    


    <!-- http://www.sisostds.org/ontologies/C2SIM#TUNISN -->

    <owl:NamedIndividual rdf:about="http://www.sisostds.org/ontologies/C2SIM#TUNISN">
        <rdf:type rdf:resource="http://www.sisostds.org/ontologies/C2SIM#EthnicGroupCode"/>
        <rdfs:comment>Tunisian: The ethnic group of Tunisian people.</rdfs:comment>
    </owl:NamedIndividual>
    


    <!-- http://www.sisostds.org/ontologies/C2SIM#TUR -->

    <owl:NamedIndividual rdf:about="http://www.sisostds.org/ontologies/C2SIM#TUR">
        <rdf:type rdf:resource="http://www.sisostds.org/ontologies/C2SIM#CountryCode"/>
        <rdfs:comment>Turkey: </rdfs:comment>
    </owl:NamedIndividual>
    


    <!-- http://www.sisostds.org/ontologies/C2SIM#TURKME -->

    <owl:NamedIndividual rdf:about="http://www.sisostds.org/ontologies/C2SIM#TURKME">
        <rdf:type rdf:resource="http://www.sisostds.org/ontologies/C2SIM#EthnicGroupCode"/>
        <rdfs:comment>Turkmen: The ethnic group of Turkmen people.</rdfs:comment>
    </owl:NamedIndividual>
    


    <!-- http://www.sisostds.org/ontologies/C2SIM#TURKOM -->

    <owl:NamedIndividual rdf:about="http://www.sisostds.org/ontologies/C2SIM#TURKOM">
        <rdf:type rdf:resource="http://www.sisostds.org/ontologies/C2SIM#EthnicGroupCode"/>
        <rdfs:comment>Turkoman: The ethnic group of Turkoman people.</rdfs:comment>
    </owl:NamedIndividual>
    


    <!-- http://www.sisostds.org/ontologies/C2SIM#TURKSH -->

    <owl:NamedIndividual rdf:about="http://www.sisostds.org/ontologies/C2SIM#TURKSH">
        <rdf:type rdf:resource="http://www.sisostds.org/ontologies/C2SIM#EthnicGroupCode"/>
        <rdfs:comment>Turkish (incl Turkish Cypriot): The ethnic group of Turkish (incl Turkish Cypriot) people.</rdfs:comment>
    </owl:NamedIndividual>
    


    <!-- http://www.sisostds.org/ontologies/C2SIM#TUTSI -->

    <owl:NamedIndividual rdf:about="http://www.sisostds.org/ontologies/C2SIM#TUTSI">
        <rdf:type rdf:resource="http://www.sisostds.org/ontologies/C2SIM#EthnicGroupCode"/>
        <rdfs:comment>Tutsi (Hamitic): The ethnic group of Tutsi (Hamitic) people.</rdfs:comment>
    </owl:NamedIndividual>
    


    <!-- http://www.sisostds.org/ontologies/C2SIM#TUV -->

    <owl:NamedIndividual rdf:about="http://www.sisostds.org/ontologies/C2SIM#TUV">
        <rdf:type rdf:resource="http://www.sisostds.org/ontologies/C2SIM#CountryCode"/>
        <rdfs:comment>Tuvalu: </rdfs:comment>
    </owl:NamedIndividual>
    


    <!-- http://www.sisostds.org/ontologies/C2SIM#TUVISL -->

    <owl:NamedIndividual rdf:about="http://www.sisostds.org/ontologies/C2SIM#TUVISL">
        <rdf:type rdf:resource="http://www.sisostds.org/ontologies/C2SIM#EthnicGroupCode"/>
        <rdfs:comment>Tuvalu Islander/Ellice Islander: The ethnic group of Tuvalu Islander/Ellice Islander people.</rdfs:comment>
    </owl:NamedIndividual>
    


    <!-- http://www.sisostds.org/ontologies/C2SIM#TWA -->

    <owl:NamedIndividual rdf:about="http://www.sisostds.org/ontologies/C2SIM#TWA">
        <rdf:type rdf:resource="http://www.sisostds.org/ontologies/C2SIM#EthnicGroupCode"/>
        <rdfs:comment>Twa (Pygmy): The ethnic group of Twa (Pygmy) people.</rdfs:comment>
    </owl:NamedIndividual>
    


    <!-- http://www.sisostds.org/ontologies/C2SIM#TWN -->

    <owl:NamedIndividual rdf:about="http://www.sisostds.org/ontologies/C2SIM#TWN">
        <rdf:type rdf:resource="http://www.sisostds.org/ontologies/C2SIM#CountryCode"/>
        <rdfs:comment>Taiwan, Province of China: </rdfs:comment>
    </owl:NamedIndividual>
    


    <!-- http://www.sisostds.org/ontologies/C2SIM#TZA -->

    <owl:NamedIndividual rdf:about="http://www.sisostds.org/ontologies/C2SIM#TZA">
        <rdf:type rdf:resource="http://www.sisostds.org/ontologies/C2SIM#CountryCode"/>
        <rdfs:comment>Tanzania, United Republic of: </rdfs:comment>
    </owl:NamedIndividual>
    


    <!-- http://www.sisostds.org/ontologies/C2SIM#TaskEnd -->

    <owl:NamedIndividual rdf:about="http://www.sisostds.org/ontologies/C2SIM#TaskEnd">
        <rdf:type rdf:resource="http://www.sisostds.org/ontologies/C2SIM#EventCode"/>
    </owl:NamedIndividual>
    


    <!-- http://www.sisostds.org/ontologies/C2SIM#TaskStart -->

    <owl:NamedIndividual rdf:about="http://www.sisostds.org/ontologies/C2SIM#TaskStart">
        <rdf:type rdf:resource="http://www.sisostds.org/ontologies/C2SIM#EventCode"/>
    </owl:NamedIndividual>
    


    <!-- http://www.sisostds.org/ontologies/C2SIM#TaskSuccess -->

    <owl:NamedIndividual rdf:about="http://www.sisostds.org/ontologies/C2SIM#TaskSuccess">
        <rdf:type rdf:resource="http://www.sisostds.org/ontologies/C2SIM#DesiredEffectCode"/>
    </owl:NamedIndividual>
    


    <!-- http://www.sisostds.org/ontologies/C2SIM#TopSecret -->

    <owl:NamedIndividual rdf:about="http://www.sisostds.org/ontologies/C2SIM#TopSecret">
        <rdf:type rdf:resource="http://www.sisostds.org/ontologies/C2SIM#SecurityClassificationCode"/>
    </owl:NamedIndividual>
    


    <!-- http://www.sisostds.org/ontologies/C2SIM#UGA -->

    <owl:NamedIndividual rdf:about="http://www.sisostds.org/ontologies/C2SIM#UGA">
        <rdf:type rdf:resource="http://www.sisostds.org/ontologies/C2SIM#CountryCode"/>
        <rdfs:comment>Uganda: </rdfs:comment>
    </owl:NamedIndividual>
    


    <!-- http://www.sisostds.org/ontologies/C2SIM#UGANDN -->

    <owl:NamedIndividual rdf:about="http://www.sisostds.org/ontologies/C2SIM#UGANDN">
        <rdf:type rdf:resource="http://www.sisostds.org/ontologies/C2SIM#EthnicGroupCode"/>
        <rdfs:comment>Ugandan: The ethnic group of Ugandan people.</rdfs:comment>
    </owl:NamedIndividual>
    


    <!-- http://www.sisostds.org/ontologies/C2SIM#UKR -->

    <owl:NamedIndividual rdf:about="http://www.sisostds.org/ontologies/C2SIM#UKR">
        <rdf:type rdf:resource="http://www.sisostds.org/ontologies/C2SIM#CountryCode"/>
        <rdfs:comment>Ukraine: </rdfs:comment>
    </owl:NamedIndividual>
    


    <!-- http://www.sisostds.org/ontologies/C2SIM#UKRANN -->

    <owl:NamedIndividual rdf:about="http://www.sisostds.org/ontologies/C2SIM#UKRANN">
        <rdf:type rdf:resource="http://www.sisostds.org/ontologies/C2SIM#EthnicGroupCode"/>
        <rdfs:comment>Ukrainian: The ethnic group of Ukrainian people.</rdfs:comment>
    </owl:NamedIndividual>
    


    <!-- http://www.sisostds.org/ontologies/C2SIM#UKRAUT -->

    <owl:NamedIndividual rdf:about="http://www.sisostds.org/ontologies/C2SIM#UKRAUT">
        <rdf:type rdf:resource="http://www.sisostds.org/ontologies/C2SIM#ReligionCode"/>
        <rdfs:comment>Ukrainian Autocephalous: One who adheres to or identifies with the Ukrainian Autocephalous doctrine.</rdfs:comment>
    </owl:NamedIndividual>
    


    <!-- http://www.sisostds.org/ontologies/C2SIM#UKRCTH -->

    <owl:NamedIndividual rdf:about="http://www.sisostds.org/ontologies/C2SIM#UKRCTH">
        <rdf:type rdf:resource="http://www.sisostds.org/ontologies/C2SIM#ReligionCode"/>
        <rdfs:comment>Ukrainian Catholic (Uniate): One who adheres to or identifies with the Ukrainian Catholic (Uniate) doctrine.</rdfs:comment>
    </owl:NamedIndividual>
    


    <!-- http://www.sisostds.org/ontologies/C2SIM#UKRORT -->

    <owl:NamedIndividual rdf:about="http://www.sisostds.org/ontologies/C2SIM#UKRORT">
        <rdf:type rdf:resource="http://www.sisostds.org/ontologies/C2SIM#ReligionCode"/>
        <rdfs:comment>Ukrainian Orthodox: One who adheres to or identifies with the Ukrainian Orthodox doctrine.</rdfs:comment>
    </owl:NamedIndividual>
    


    <!-- http://www.sisostds.org/ontologies/C2SIM#UMI -->

    <owl:NamedIndividual rdf:about="http://www.sisostds.org/ontologies/C2SIM#UMI">
        <rdf:type rdf:resource="http://www.sisostds.org/ontologies/C2SIM#CountryCode"/>
        <rdfs:comment>United States Minor Outlying Islands: </rdfs:comment>
    </owl:NamedIndividual>
    


    <!-- http://www.sisostds.org/ontologies/C2SIM#UNCH -->

    <owl:NamedIndividual rdf:about="http://www.sisostds.org/ontologies/C2SIM#UNCH">
        <rdf:type rdf:resource="http://www.sisostds.org/ontologies/C2SIM#ReligionCode"/>
        <rdfs:comment>United Church: One who adheres to or identifies with the United Church doctrine.</rdfs:comment>
    </owl:NamedIndividual>
    


    <!-- http://www.sisostds.org/ontologies/C2SIM#UNCHAU -->

    <owl:NamedIndividual rdf:about="http://www.sisostds.org/ontologies/C2SIM#UNCHAU">
        <rdf:type rdf:resource="http://www.sisostds.org/ontologies/C2SIM#ReligionCode"/>
        <rdfs:comment>Uniting Church in Australia: One who adheres to or identifies with the Uniting Church in Australia doctrine.</rdfs:comment>
    </owl:NamedIndividual>
    


    <!-- http://www.sisostds.org/ontologies/C2SIM#UNCHCN -->

    <owl:NamedIndividual rdf:about="http://www.sisostds.org/ontologies/C2SIM#UNCHCN">
        <rdf:type rdf:resource="http://www.sisostds.org/ontologies/C2SIM#ReligionCode"/>
        <rdfs:comment>United Church (Congregational): One who adheres to or identifies with the United Church (Congregational) doctrine.</rdfs:comment>
    </owl:NamedIndividual>
    


    <!-- http://www.sisostds.org/ontologies/C2SIM#UNCHPR -->

    <owl:NamedIndividual rdf:about="http://www.sisostds.org/ontologies/C2SIM#UNCHPR">
        <rdf:type rdf:resource="http://www.sisostds.org/ontologies/C2SIM#ReligionCode"/>
        <rdfs:comment>United Church (Presbyterian): One who adheres to or identifies with the United Church (Presbyterian) doctrine.</rdfs:comment>
    </owl:NamedIndividual>
    


    <!-- http://www.sisostds.org/ontologies/C2SIM#UNDMTH -->

    <owl:NamedIndividual rdf:about="http://www.sisostds.org/ontologies/C2SIM#UNDMTH">
        <rdf:type rdf:resource="http://www.sisostds.org/ontologies/C2SIM#ReligionCode"/>
        <rdfs:comment>United (Methodist): One who adheres to or identifies with the United (Methodist) doctrine.</rdfs:comment>
    </owl:NamedIndividual>
    


    <!-- http://www.sisostds.org/ontologies/C2SIM#UNDPRB -->

    <owl:NamedIndividual rdf:about="http://www.sisostds.org/ontologies/C2SIM#UNDPRB">
        <rdf:type rdf:resource="http://www.sisostds.org/ontologies/C2SIM#ReligionCode"/>
        <rdfs:comment>United (Presbyterian): One who adheres to or identifies with the United (Presbyterian) doctrine.</rdfs:comment>
    </owl:NamedIndividual>
    


    <!-- http://www.sisostds.org/ontologies/C2SIM#UNFRCH -->

    <owl:NamedIndividual rdf:about="http://www.sisostds.org/ontologies/C2SIM#UNFRCH">
        <rdf:type rdf:resource="http://www.sisostds.org/ontologies/C2SIM#ReligionCode"/>
        <rdfs:comment>United Free Church: One who adheres to or identifies with the United Free Church doctrine.</rdfs:comment>
    </owl:NamedIndividual>
    


    <!-- http://www.sisostds.org/ontologies/C2SIM#UNICTH -->

    <owl:NamedIndividual rdf:about="http://www.sisostds.org/ontologies/C2SIM#UNICTH">
        <rdf:type rdf:resource="http://www.sisostds.org/ontologies/C2SIM#ReligionCode"/>
        <rdfs:comment>Uniate Catholic: One who adheres to or identifies with the Uniate Catholic doctrine.</rdfs:comment>
    </owl:NamedIndividual>
    


    <!-- http://www.sisostds.org/ontologies/C2SIM#URUGYN -->

    <owl:NamedIndividual rdf:about="http://www.sisostds.org/ontologies/C2SIM#URUGYN">
        <rdf:type rdf:resource="http://www.sisostds.org/ontologies/C2SIM#EthnicGroupCode"/>
        <rdfs:comment>Uruguayan: The ethnic group of Uruguayan people.</rdfs:comment>
    </owl:NamedIndividual>
    


    <!-- http://www.sisostds.org/ontologies/C2SIM#URY -->

    <owl:NamedIndividual rdf:about="http://www.sisostds.org/ontologies/C2SIM#URY">
        <rdf:type rdf:resource="http://www.sisostds.org/ontologies/C2SIM#CountryCode"/>
        <rdfs:comment>Uruguay: </rdfs:comment>
    </owl:NamedIndividual>
    


    <!-- http://www.sisostds.org/ontologies/C2SIM#USA -->

    <owl:NamedIndividual rdf:about="http://www.sisostds.org/ontologies/C2SIM#USA">
        <rdf:type rdf:resource="http://www.sisostds.org/ontologies/C2SIM#CountryCode"/>
        <rdfs:comment>United States: </rdfs:comment>
    </owl:NamedIndividual>
    


    <!-- http://www.sisostds.org/ontologies/C2SIM#UYGUR -->

    <owl:NamedIndividual rdf:about="http://www.sisostds.org/ontologies/C2SIM#UYGUR">
        <rdf:type rdf:resource="http://www.sisostds.org/ontologies/C2SIM#EthnicGroupCode"/>
        <rdfs:comment>Uygur: The ethnic group of Uygur people.</rdfs:comment>
    </owl:NamedIndividual>
    


    <!-- http://www.sisostds.org/ontologies/C2SIM#UZB -->

    <owl:NamedIndividual rdf:about="http://www.sisostds.org/ontologies/C2SIM#UZB">
        <rdf:type rdf:resource="http://www.sisostds.org/ontologies/C2SIM#CountryCode"/>
        <rdfs:comment>Uzbekistan: </rdfs:comment>
    </owl:NamedIndividual>
    


    <!-- http://www.sisostds.org/ontologies/C2SIM#UZBEK -->

    <owl:NamedIndividual rdf:about="http://www.sisostds.org/ontologies/C2SIM#UZBEK">
        <rdf:type rdf:resource="http://www.sisostds.org/ontologies/C2SIM#EthnicGroupCode"/>
        <rdfs:comment>Uzbek: The ethnic group of Uzbek people.</rdfs:comment>
    </owl:NamedIndividual>
    


    <!-- http://www.sisostds.org/ontologies/C2SIM#Unclassified -->

    <owl:NamedIndividual rdf:about="http://www.sisostds.org/ontologies/C2SIM#Unclassified">
        <rdf:type rdf:resource="http://www.sisostds.org/ontologies/C2SIM#SecurityClassificationCode"/>
    </owl:NamedIndividual>
    


    <!-- http://www.sisostds.org/ontologies/C2SIM#UnkownAllegianceTo -->

    <owl:NamedIndividual rdf:about="http://www.sisostds.org/ontologies/C2SIM#UnkownAllegianceTo">
        <rdf:type rdf:resource="http://www.sisostds.org/ontologies/C2SIM#AllegianceRelationshipCode"/>
    </owl:NamedIndividual>
    


    <!-- http://www.sisostds.org/ontologies/C2SIM#UseCapability -->

    <owl:NamedIndividual rdf:about="http://www.sisostds.org/ontologies/C2SIM#UseCapability">
        <rdf:type rdf:resource="http://www.sisostds.org/ontologies/C2SIM#TaskActionCode"/>
    </owl:NamedIndividual>
    <owl:Axiom>
        <owl:annotatedSource rdf:resource="http://www.sisostds.org/ontologies/C2SIM#UseCapability"/>
        <owl:annotatedProperty rdf:resource="http://www.w3.org/1999/02/22-rdf-syntax-ns#type"/>
        <owl:annotatedTarget rdf:resource="http://www.sisostds.org/ontologies/C2SIM#TaskActionCode"/>
        <rdfs:comment>Use the main or default capability that the actor posseses.</rdfs:comment>
    </owl:Axiom>
    


    <!-- http://www.sisostds.org/ontologies/C2SIM#VANUAT -->

    <owl:NamedIndividual rdf:about="http://www.sisostds.org/ontologies/C2SIM#VANUAT">
        <rdf:type rdf:resource="http://www.sisostds.org/ontologies/C2SIM#EthnicGroupCode"/>
        <rdfs:comment>Vanuatu Islander/New Hebridean: The ethnic group of Vanuatu Islander/New Hebridean people.</rdfs:comment>
    </owl:NamedIndividual>
    


    <!-- http://www.sisostds.org/ontologies/C2SIM#VAT -->

    <owl:NamedIndividual rdf:about="http://www.sisostds.org/ontologies/C2SIM#VAT">
        <rdf:type rdf:resource="http://www.sisostds.org/ontologies/C2SIM#CountryCode"/>
        <rdfs:comment>Holy See (Vatican City State): </rdfs:comment>
    </owl:NamedIndividual>
    


    <!-- http://www.sisostds.org/ontologies/C2SIM#VCT -->

    <owl:NamedIndividual rdf:about="http://www.sisostds.org/ontologies/C2SIM#VCT">
        <rdf:type rdf:resource="http://www.sisostds.org/ontologies/C2SIM#CountryCode"/>
        <rdfs:comment>Saint Vincent and the Grenadines: </rdfs:comment>
    </owl:NamedIndividual>
    


    <!-- http://www.sisostds.org/ontologies/C2SIM#VEDDA -->

    <owl:NamedIndividual rdf:about="http://www.sisostds.org/ontologies/C2SIM#VEDDA">
        <rdf:type rdf:resource="http://www.sisostds.org/ontologies/C2SIM#EthnicGroupCode"/>
        <rdfs:comment>Vedda: The ethnic group of Vedda people.</rdfs:comment>
    </owl:NamedIndividual>
    


    <!-- http://www.sisostds.org/ontologies/C2SIM#VEN -->

    <owl:NamedIndividual rdf:about="http://www.sisostds.org/ontologies/C2SIM#VEN">
        <rdf:type rdf:resource="http://www.sisostds.org/ontologies/C2SIM#CountryCode"/>
        <rdfs:comment>Venezuela: </rdfs:comment>
    </owl:NamedIndividual>
    


    <!-- http://www.sisostds.org/ontologies/C2SIM#VENEZN -->

    <owl:NamedIndividual rdf:about="http://www.sisostds.org/ontologies/C2SIM#VENEZN">
        <rdf:type rdf:resource="http://www.sisostds.org/ontologies/C2SIM#EthnicGroupCode"/>
        <rdfs:comment>Venezuelan: The ethnic group of Venezuelan people.</rdfs:comment>
    </owl:NamedIndividual>
    


    <!-- http://www.sisostds.org/ontologies/C2SIM#VGB -->

    <owl:NamedIndividual rdf:about="http://www.sisostds.org/ontologies/C2SIM#VGB">
        <rdf:type rdf:resource="http://www.sisostds.org/ontologies/C2SIM#CountryCode"/>
        <rdfs:comment>Virgin Islands, British: </rdfs:comment>
    </owl:NamedIndividual>
    


    <!-- http://www.sisostds.org/ontologies/C2SIM#VIETNM -->

    <owl:NamedIndividual rdf:about="http://www.sisostds.org/ontologies/C2SIM#VIETNM">
        <rdf:type rdf:resource="http://www.sisostds.org/ontologies/C2SIM#EthnicGroupCode"/>
        <rdfs:comment>Vietnamese: The ethnic group of Vietnamese people.</rdfs:comment>
    </owl:NamedIndividual>
    


    <!-- http://www.sisostds.org/ontologies/C2SIM#VILELD -->

    <owl:NamedIndividual rdf:about="http://www.sisostds.org/ontologies/C2SIM#VILELD">
        <rdf:type rdf:resource="http://www.sisostds.org/ontologies/C2SIM#OrganizationTypeCode"/>
        <rdfs:comment>Village elder: A GROUP-ORGANISATION-TYPE that comprises persons that are of ripe years and experience whose counsel is therefore sought and</rdfs:comment>
    </owl:NamedIndividual>
    


    <!-- http://www.sisostds.org/ontologies/C2SIM#VIR -->

    <owl:NamedIndividual rdf:about="http://www.sisostds.org/ontologies/C2SIM#VIR">
        <rdf:type rdf:resource="http://www.sisostds.org/ontologies/C2SIM#CountryCode"/>
        <rdfs:comment>Virgin Islands, U.S.: </rdfs:comment>
    </owl:NamedIndividual>
    


    <!-- http://www.sisostds.org/ontologies/C2SIM#VITCHN -->

    <owl:NamedIndividual rdf:about="http://www.sisostds.org/ontologies/C2SIM#VITCHN">
        <rdf:type rdf:resource="http://www.sisostds.org/ontologies/C2SIM#EthnicGroupCode"/>
        <rdfs:comment>Vietnamese Chinese: The ethnic group of Vietnamese Chinese people.</rdfs:comment>
    </owl:NamedIndividual>
    


    <!-- http://www.sisostds.org/ontologies/C2SIM#VLACHS -->

    <owl:NamedIndividual rdf:about="http://www.sisostds.org/ontologies/C2SIM#VLACHS">
        <rdf:type rdf:resource="http://www.sisostds.org/ontologies/C2SIM#EthnicGroupCode"/>
        <rdfs:comment>Vlachs: The ethnic group of Vlachs people.</rdfs:comment>
    </owl:NamedIndividual>
    


    <!-- http://www.sisostds.org/ontologies/C2SIM#VNM -->

    <owl:NamedIndividual rdf:about="http://www.sisostds.org/ontologies/C2SIM#VNM">
        <rdf:type rdf:resource="http://www.sisostds.org/ontologies/C2SIM#CountryCode"/>
        <rdfs:comment>Viet Nam: </rdfs:comment>
    </owl:NamedIndividual>
    


    <!-- http://www.sisostds.org/ontologies/C2SIM#VOLTAC -->

    <owl:NamedIndividual rdf:about="http://www.sisostds.org/ontologies/C2SIM#VOLTAC">
        <rdf:type rdf:resource="http://www.sisostds.org/ontologies/C2SIM#EthnicGroupCode"/>
        <rdfs:comment>Voltaic: The ethnic group of Voltaic people.</rdfs:comment>
    </owl:NamedIndividual>
    


    <!-- http://www.sisostds.org/ontologies/C2SIM#VOODOO -->

    <owl:NamedIndividual rdf:about="http://www.sisostds.org/ontologies/C2SIM#VOODOO">
        <rdf:type rdf:resource="http://www.sisostds.org/ontologies/C2SIM#ReligionCode"/>
        <rdfs:comment>Voodoo: One who adheres to or identifies with the Voodoo doctrine.</rdfs:comment>
    </owl:NamedIndividual>
    


    <!-- http://www.sisostds.org/ontologies/C2SIM#VUT -->

    <owl:NamedIndividual rdf:about="http://www.sisostds.org/ontologies/C2SIM#VUT">
        <rdf:type rdf:resource="http://www.sisostds.org/ontologies/C2SIM#CountryCode"/>
        <rdfs:comment>Vanuatu: Formerly New Hebrides (1980)</rdfs:comment>
    </owl:NamedIndividual>
    


    <!-- http://www.sisostds.org/ontologies/C2SIM#WAKISL -->

    <owl:NamedIndividual rdf:about="http://www.sisostds.org/ontologies/C2SIM#WAKISL">
        <rdf:type rdf:resource="http://www.sisostds.org/ontologies/C2SIM#EthnicGroupCode"/>
        <rdfs:comment>Wake Islander: The ethnic group of Wake Islander people.</rdfs:comment>
    </owl:NamedIndividual>
    


    <!-- http://www.sisostds.org/ontologies/C2SIM#WALISL -->

    <owl:NamedIndividual rdf:about="http://www.sisostds.org/ontologies/C2SIM#WALISL">
        <rdf:type rdf:resource="http://www.sisostds.org/ontologies/C2SIM#EthnicGroupCode"/>
        <rdfs:comment>Wallis Islander: The ethnic group of Wallis Islander people.</rdfs:comment>
    </owl:NamedIndividual>
    


    <!-- http://www.sisostds.org/ontologies/C2SIM#WALLIS -->

    <owl:NamedIndividual rdf:about="http://www.sisostds.org/ontologies/C2SIM#WALLIS">
        <rdf:type rdf:resource="http://www.sisostds.org/ontologies/C2SIM#EthnicGroupCode"/>
        <rdfs:comment>Wallisian: The ethnic group of Wallisian people.</rdfs:comment>
    </owl:NamedIndividual>
    


    <!-- http://www.sisostds.org/ontologies/C2SIM#WALLOO -->

    <owl:NamedIndividual rdf:about="http://www.sisostds.org/ontologies/C2SIM#WALLOO">
        <rdf:type rdf:resource="http://www.sisostds.org/ontologies/C2SIM#EthnicGroupCode"/>
        <rdfs:comment>Walloon: The ethnic group of Walloon people.</rdfs:comment>
    </owl:NamedIndividual>
    


    <!-- http://www.sisostds.org/ontologies/C2SIM#WELSH -->

    <owl:NamedIndividual rdf:about="http://www.sisostds.org/ontologies/C2SIM#WELSH">
        <rdf:type rdf:resource="http://www.sisostds.org/ontologies/C2SIM#EthnicGroupCode"/>
        <rdfs:comment>Welsh: The ethnic group of Welsh people.</rdfs:comment>
    </owl:NamedIndividual>
    


    <!-- http://www.sisostds.org/ontologies/C2SIM#WHITE -->

    <owl:NamedIndividual rdf:about="http://www.sisostds.org/ontologies/C2SIM#WHITE">
        <rdf:type rdf:resource="http://www.sisostds.org/ontologies/C2SIM#EthnicGroupCode"/>
        <rdfs:comment>White: The ethnic group of White people.</rdfs:comment>
    </owl:NamedIndividual>
    


    <!-- http://www.sisostds.org/ontologies/C2SIM#WLF -->

    <owl:NamedIndividual rdf:about="http://www.sisostds.org/ontologies/C2SIM#WLF">
        <rdf:type rdf:resource="http://www.sisostds.org/ontologies/C2SIM#CountryCode"/>
        <rdfs:comment>Wallis and Futuna Islands: </rdfs:comment>
    </owl:NamedIndividual>
    


    <!-- http://www.sisostds.org/ontologies/C2SIM#WOLOF -->

    <owl:NamedIndividual rdf:about="http://www.sisostds.org/ontologies/C2SIM#WOLOF">
        <rdf:type rdf:resource="http://www.sisostds.org/ontologies/C2SIM#EthnicGroupCode"/>
        <rdfs:comment>Wolof: The ethnic group of Wolof people.</rdfs:comment>
    </owl:NamedIndividual>
    


    <!-- http://www.sisostds.org/ontologies/C2SIM#WRITER -->

    <owl:NamedIndividual rdf:about="http://www.sisostds.org/ontologies/C2SIM#WRITER">
        <rdf:type rdf:resource="http://www.sisostds.org/ontologies/C2SIM#OrganizationTypeCode"/>
        <rdfs:comment>Writer: A GROUP-ORGANISATION-TYPE that comprises persons that practice or perform writing.</rdfs:comment>
    </owl:NamedIndividual>
    


    <!-- http://www.sisostds.org/ontologies/C2SIM#WSM -->

    <owl:NamedIndividual rdf:about="http://www.sisostds.org/ontologies/C2SIM#WSM">
        <rdf:type rdf:resource="http://www.sisostds.org/ontologies/C2SIM#CountryCode"/>
        <rdfs:comment>Samoa: </rdfs:comment>
    </owl:NamedIndividual>
    


    <!-- http://www.sisostds.org/ontologies/C2SIM#WSTIND -->

    <owl:NamedIndividual rdf:about="http://www.sisostds.org/ontologies/C2SIM#WSTIND">
        <rdf:type rdf:resource="http://www.sisostds.org/ontologies/C2SIM#EthnicGroupCode"/>
        <rdfs:comment>West Indian/Caribbean: The ethnic group of West Indian/Caribbean people.</rdfs:comment>
    </owl:NamedIndividual>
    


    <!-- http://www.sisostds.org/ontologies/C2SIM#YAO -->

    <owl:NamedIndividual rdf:about="http://www.sisostds.org/ontologies/C2SIM#YAO">
        <rdf:type rdf:resource="http://www.sisostds.org/ontologies/C2SIM#EthnicGroupCode"/>
        <rdfs:comment>Yao: The ethnic group of Yao people.</rdfs:comment>
    </owl:NamedIndividual>
    


    <!-- http://www.sisostds.org/ontologies/C2SIM#YAPISL -->

    <owl:NamedIndividual rdf:about="http://www.sisostds.org/ontologies/C2SIM#YAPISL">
        <rdf:type rdf:resource="http://www.sisostds.org/ontologies/C2SIM#EthnicGroupCode"/>
        <rdfs:comment>Yap Islander: The ethnic group of Yap Islander people.</rdfs:comment>
    </owl:NamedIndividual>
    


    <!-- http://www.sisostds.org/ontologies/C2SIM#YEM -->

    <owl:NamedIndividual rdf:about="http://www.sisostds.org/ontologies/C2SIM#YEM">
        <rdf:type rdf:resource="http://www.sisostds.org/ontologies/C2SIM#CountryCode"/>
        <rdfs:comment>Yemen: </rdfs:comment>
    </owl:NamedIndividual>
    


    <!-- http://www.sisostds.org/ontologies/C2SIM#YEMENI -->

    <owl:NamedIndividual rdf:about="http://www.sisostds.org/ontologies/C2SIM#YEMENI">
        <rdf:type rdf:resource="http://www.sisostds.org/ontologies/C2SIM#EthnicGroupCode"/>
        <rdfs:comment>Yemeni: The ethnic group of Yemeni people.</rdfs:comment>
    </owl:NamedIndividual>
    


    <!-- http://www.sisostds.org/ontologies/C2SIM#YI -->

    <owl:NamedIndividual rdf:about="http://www.sisostds.org/ontologies/C2SIM#YI">
        <rdf:type rdf:resource="http://www.sisostds.org/ontologies/C2SIM#EthnicGroupCode"/>
        <rdfs:comment>Yi: The ethnic group of Yi people.</rdfs:comment>
    </owl:NamedIndividual>
    


    <!-- http://www.sisostds.org/ontologies/C2SIM#YORUBA -->

    <owl:NamedIndividual rdf:about="http://www.sisostds.org/ontologies/C2SIM#YORUBA">
        <rdf:type rdf:resource="http://www.sisostds.org/ontologies/C2SIM#EthnicGroupCode"/>
        <rdfs:comment>Yoruba: The ethnic group of Yoruba people.</rdfs:comment>
    </owl:NamedIndividual>
    


    <!-- http://www.sisostds.org/ontologies/C2SIM#YUCS -->

    <owl:NamedIndividual rdf:about="http://www.sisostds.org/ontologies/C2SIM#YUCS">
        <rdf:type rdf:resource="http://www.sisostds.org/ontologies/C2SIM#CountryCode"/>
        <rdfs:comment>Yugoslavia (former): (2003)</rdfs:comment>
    </owl:NamedIndividual>
    


    <!-- http://www.sisostds.org/ontologies/C2SIM#YUGOSL -->

    <owl:NamedIndividual rdf:about="http://www.sisostds.org/ontologies/C2SIM#YUGOSL">
        <rdf:type rdf:resource="http://www.sisostds.org/ontologies/C2SIM#EthnicGroupCode"/>
        <rdfs:comment>Yugoslavian: The ethnic group of Yugoslavian people.</rdfs:comment>
    </owl:NamedIndividual>
    


    <!-- http://www.sisostds.org/ontologies/C2SIM#ZAF -->

    <owl:NamedIndividual rdf:about="http://www.sisostds.org/ontologies/C2SIM#ZAF">
        <rdf:type rdf:resource="http://www.sisostds.org/ontologies/C2SIM#CountryCode"/>
        <rdfs:comment>South Africa: </rdfs:comment>
    </owl:NamedIndividual>
    


    <!-- http://www.sisostds.org/ontologies/C2SIM#ZAIRAN -->

    <owl:NamedIndividual rdf:about="http://www.sisostds.org/ontologies/C2SIM#ZAIRAN">
        <rdf:type rdf:resource="http://www.sisostds.org/ontologies/C2SIM#EthnicGroupCode"/>
        <rdfs:comment>Zairians: The ethnic group of Zairians people.</rdfs:comment>
    </owl:NamedIndividual>
    


    <!-- http://www.sisostds.org/ontologies/C2SIM#ZANZIB -->

    <owl:NamedIndividual rdf:about="http://www.sisostds.org/ontologies/C2SIM#ZANZIB">
        <rdf:type rdf:resource="http://www.sisostds.org/ontologies/C2SIM#EthnicGroupCode"/>
        <rdfs:comment>Zanzibari: The ethnic group of Zanzibari people.</rdfs:comment>
    </owl:NamedIndividual>
    


    <!-- http://www.sisostds.org/ontologies/C2SIM#ZHUANG -->

    <owl:NamedIndividual rdf:about="http://www.sisostds.org/ontologies/C2SIM#ZHUANG">
        <rdf:type rdf:resource="http://www.sisostds.org/ontologies/C2SIM#EthnicGroupCode"/>
        <rdfs:comment>Zhuang: The ethnic group of Zhuang people.</rdfs:comment>
    </owl:NamedIndividual>
    


    <!-- http://www.sisostds.org/ontologies/C2SIM#ZMB -->

    <owl:NamedIndividual rdf:about="http://www.sisostds.org/ontologies/C2SIM#ZMB">
        <rdf:type rdf:resource="http://www.sisostds.org/ontologies/C2SIM#CountryCode"/>
        <rdfs:comment>Zambia: </rdfs:comment>
    </owl:NamedIndividual>
    


    <!-- http://www.sisostds.org/ontologies/C2SIM#ZRSTRN -->

    <owl:NamedIndividual rdf:about="http://www.sisostds.org/ontologies/C2SIM#ZRSTRN">
        <rdf:type rdf:resource="http://www.sisostds.org/ontologies/C2SIM#ReligionCode"/>
        <rdfs:comment>Zoroastrian: One who adheres to or identifies with the Zoroastrian doctrine.</rdfs:comment>
    </owl:NamedIndividual>
    


    <!-- http://www.sisostds.org/ontologies/C2SIM#ZWE -->

    <owl:NamedIndividual rdf:about="http://www.sisostds.org/ontologies/C2SIM#ZWE">
        <rdf:type rdf:resource="http://www.sisostds.org/ontologies/C2SIM#CountryCode"/>
        <rdfs:comment>Zimbabwe: </rdfs:comment>
    </owl:NamedIndividual>
    


    <!-- http://www.sisostds.org/ontologies/lox#ACQUIR -->

    <owl:NamedIndividual rdf:about="http://www.sisostds.org/ontologies/lox#ACQUIR">
        <rdf:type rdf:resource="http://www.sisostds.org/ontologies/C2SIM#TaskActionCode"/>
        <rdfs:comment>Acquire: To detect the presence and location of a target in sufficient detail to permit identification.</rdfs:comment>
        <rdfs:comment>Documentation: 		
						To detect the presence and location of a target in sufficient detail to permit identification.	
					; Appinfo DisplayValue as &quot;Acquire&quot;</rdfs:comment>
    </owl:NamedIndividual>
    


    <!-- http://www.sisostds.org/ontologies/lox#ADVANC -->

    <owl:NamedIndividual rdf:about="http://www.sisostds.org/ontologies/lox#ADVANC">
        <rdf:type rdf:resource="http://www.sisostds.org/ontologies/C2SIM#TaskActionCode"/>
        <rdfs:comment>Advance: To move towards an objective in some form of tactical formation. This is a transitional phase between operations which may</rdfs:comment>
        <rdfs:comment>Documentation: 		
						To move towards an objective in some form of tactical formation. This is a transitional phase between operations which may or may not result in contact with the enemy.	
					; Appinfo DisplayValue as &quot;Advance&quot;</rdfs:comment>
    </owl:NamedIndividual>
    


    <!-- http://www.sisostds.org/ontologies/lox#AEREVA -->

    <owl:NamedIndividual rdf:about="http://www.sisostds.org/ontologies/lox#AEREVA">
        <rdf:type rdf:resource="http://www.sisostds.org/ontologies/C2SIM#TaskActionCode"/>
        <rdfs:comment>Aeromedical evacuation: To move patients under medical supervision to and between medical treatment facilities by air transportation.</rdfs:comment>
    </owl:NamedIndividual>
    


    <!-- http://www.sisostds.org/ontologies/lox#AERRFL -->

    <owl:NamedIndividual rdf:about="http://www.sisostds.org/ontologies/lox#AERRFL">
        <rdf:type rdf:resource="http://www.sisostds.org/ontologies/C2SIM#TaskActionCode"/>
        <rdfs:comment>Aerial refuelling: To refuel aircraft in flight, which extends presence, increases range, and serves as a force multiplier.</rdfs:comment>
    </owl:NamedIndividual>
    


    <!-- http://www.sisostds.org/ontologies/lox#AEW -->

    <owl:NamedIndividual rdf:about="http://www.sisostds.org/ontologies/lox#AEW">
        <rdf:type rdf:resource="http://www.sisostds.org/ontologies/C2SIM#TaskActionCode"/>
        <rdfs:comment>Airborne early warning: To provide airborne early warning and surveillance.</rdfs:comment>
    </owl:NamedIndividual>
    


    <!-- http://www.sisostds.org/ontologies/lox#AEWCON -->

    <owl:NamedIndividual rdf:about="http://www.sisostds.org/ontologies/lox#AEWCON">
        <rdf:type rdf:resource="http://www.sisostds.org/ontologies/C2SIM#TaskActionCode"/>
        <rdfs:comment>Airborne early warning and control: To provide airborne early warning, surveillance and the control of airborne weapon systems.</rdfs:comment>
    </owl:NamedIndividual>
    


    <!-- http://www.sisostds.org/ontologies/lox#AIRDEF -->

    <owl:NamedIndividual rdf:about="http://www.sisostds.org/ontologies/lox#AIRDEF">
        <rdf:type rdf:resource="http://www.sisostds.org/ontologies/C2SIM#TaskActionCode"/>
        <rdfs:comment>Air defence: To protect and defend an area, a strike attack, an installation or naval forces.</rdfs:comment>
        <rdfs:comment>Documentation: 		
						To protect and defend an area, a strike attack, an installation or naval forces.	
					; Appinfo DisplayValue as &quot;Air defence&quot;</rdfs:comment>
    </owl:NamedIndividual>
    


    <!-- http://www.sisostds.org/ontologies/lox#AIRLND -->

    <owl:NamedIndividual rdf:about="http://www.sisostds.org/ontologies/lox#AIRLND">
        <rdf:type rdf:resource="http://www.sisostds.org/ontologies/C2SIM#TaskActionCode"/>
        <rdfs:comment>Airland: To move a unit by air and disembark or unload it, after the aircraft has landed or while a helicopter is hovering.</rdfs:comment>
    </owl:NamedIndividual>
    


    <!-- http://www.sisostds.org/ontologies/lox#AIRSUP -->

    <owl:NamedIndividual rdf:about="http://www.sisostds.org/ontologies/lox#AIRSUP">
        <rdf:type rdf:resource="http://www.sisostds.org/ontologies/C2SIM#TaskActionCode"/>
        <rdfs:comment>Air superiority: To obtain a degree of dominance in the air battle of one force over another in order to permit the conduct of operations by</rdfs:comment>
    </owl:NamedIndividual>
    


    <!-- http://www.sisostds.org/ontologies/lox#AIRSWP -->

    <owl:NamedIndividual rdf:about="http://www.sisostds.org/ontologies/lox#AIRSWP">
        <rdf:type rdf:resource="http://www.sisostds.org/ontologies/C2SIM#TaskActionCode"/>
        <rdfs:comment>Air-to-air sweep: To conduct an offensive mission by fighter aircraft to seek out and destroy enemy aircraft or targets of opportunity in an</rdfs:comment>
    </owl:NamedIndividual>
    


    <!-- http://www.sisostds.org/ontologies/lox#ALT -->

    <owl:NamedIndividual rdf:about="http://www.sisostds.org/ontologies/lox#ALT">
        <rdf:type rdf:resource="http://www.sisostds.org/ontologies/lox#TaskFunctionalAssociationCode"/>
        <rdfs:comment>Is an alternative to: The subject ACTION may replace the object ACTION.</rdfs:comment>
    </owl:NamedIndividual>
    


    <!-- http://www.sisostds.org/ontologies/lox#AMBUSH -->

    <owl:NamedIndividual rdf:about="http://www.sisostds.org/ontologies/lox#AMBUSH">
        <rdf:type rdf:resource="http://www.sisostds.org/ontologies/C2SIM#TaskActionCode"/>
        <rdfs:comment>Ambush: To conduct a surprise attack by fire or other destructive means, from concealed positions on a moving or temporarily halted</rdfs:comment>
        <rdfs:comment>Documentation: 		
						To conduct a surprise attack by fire or other destructive means, from concealed positions on a moving or temporarily halted force or group of personnel.	
					; Appinfo DisplayValue as &quot;Ambush&quot;</rdfs:comment>
    </owl:NamedIndividual>
    


    <!-- http://www.sisostds.org/ontologies/lox#AMPH -->

    <owl:NamedIndividual rdf:about="http://www.sisostds.org/ontologies/lox#AMPH">
        <rdf:type rdf:resource="http://www.sisostds.org/ontologies/C2SIM#TaskActionCode"/>
        <rdfs:comment>Amphibious operation: To mount an operation launched from the sea by naval and land forces against a hostile, or potentially hostile shore.</rdfs:comment>
    </owl:NamedIndividual>
    


    <!-- http://www.sisostds.org/ontologies/lox#AMPHWF -->

    <owl:NamedIndividual rdf:about="http://www.sisostds.org/ontologies/lox#AMPHWF">
        <rdf:type rdf:resource="http://www.sisostds.org/ontologies/C2SIM#TaskActionCode"/>
        <rdfs:comment>Amphibious warfare: To conduct warfare that includes the launch of naval and land forces from sea against a hostile, or potentially hostile shore.</rdfs:comment>
    </owl:NamedIndividual>
    


    <!-- http://www.sisostds.org/ontologies/lox#ANALYS -->

    <owl:NamedIndividual rdf:about="http://www.sisostds.org/ontologies/lox#ANALYS">
        <rdf:type rdf:resource="http://www.sisostds.org/ontologies/C2SIM#TaskActionCode"/>
        <rdfs:comment>Analyse: To review in order to identify significant facts for subsequent interpretation.</rdfs:comment>
    </owl:NamedIndividual>
    


    <!-- http://www.sisostds.org/ontologies/lox#ANARWF -->

    <owl:NamedIndividual rdf:about="http://www.sisostds.org/ontologies/lox#ANARWF">
        <rdf:type rdf:resource="http://www.sisostds.org/ontologies/C2SIM#TaskActionCode"/>
        <rdfs:comment>Anti-air warfare: To conduct warfare with the purpose of defending friendly forces, against the threat aircraft and airborne weapons, whether</rdfs:comment>
    </owl:NamedIndividual>
    


    <!-- http://www.sisostds.org/ontologies/lox#ANSBWF -->

    <owl:NamedIndividual rdf:about="http://www.sisostds.org/ontologies/lox#ANSBWF">
        <rdf:type rdf:resource="http://www.sisostds.org/ontologies/C2SIM#TaskActionCode"/>
        <rdfs:comment>Anti-submarine warfare: To conduct warfare with the intention of denying the opponent the effective use of his submarines.</rdfs:comment>
    </owl:NamedIndividual>
    


    <!-- http://www.sisostds.org/ontologies/lox#ANSFWF -->

    <owl:NamedIndividual rdf:about="http://www.sisostds.org/ontologies/lox#ANSFWF">
        <rdf:type rdf:resource="http://www.sisostds.org/ontologies/C2SIM#TaskActionCode"/>
        <rdfs:comment>Anti-surface warfare: To conduct warfare against an adversary&apos;s surface forces or merchant ships to achieve sea control or sea denial, to disrupt</rdfs:comment>
    </owl:NamedIndividual>
    


    <!-- http://www.sisostds.org/ontologies/lox#ANTARM -->

    <owl:NamedIndividual rdf:about="http://www.sisostds.org/ontologies/lox#ANTARM">
        <rdf:type rdf:resource="http://www.sisostds.org/ontologies/C2SIM#TaskActionCode"/>
        <rdfs:comment>Anti-armour: To destroy armoured targets.</rdfs:comment>
    </owl:NamedIndividual>
    


    <!-- http://www.sisostds.org/ontologies/lox#ARASLT -->

    <owl:NamedIndividual rdf:about="http://www.sisostds.org/ontologies/lox#ARASLT">
        <rdf:type rdf:resource="http://www.sisostds.org/ontologies/C2SIM#TaskActionCode"/>
        <rdfs:comment>Air assault: To mount an operation in which assault forces (combat, combat service, and combat service support), using the firepower, mobility,</rdfs:comment>
        <rdfs:comment>Documentation: 		
						To mount an operation in which assault forces (combat, combat service, and combat service support), using the firepower, mobility, and total integration of helicopter assets, maneuver on the battlefield under the control of the ground or air manoeuvre commander to engage and destroy enemy forces or to seize and hold key terrain.	
					; Appinfo DisplayValue as &quot;Air assault&quot;</rdfs:comment>
    </owl:NamedIndividual>
    


    <!-- http://www.sisostds.org/ontologies/lox#ARBNAS -->

    <owl:NamedIndividual rdf:about="http://www.sisostds.org/ontologies/lox#ARBNAS">
        <rdf:type rdf:resource="http://www.sisostds.org/ontologies/C2SIM#TaskActionCode"/>
        <rdfs:comment>Airborne assault: In an airborne operation, a phase beginning with delivery by air of the assault echelon of the force into the objective area</rdfs:comment>
    </owl:NamedIndividual>
    


    <!-- http://www.sisostds.org/ontologies/lox#ARCCTL -->

    <owl:NamedIndividual rdf:about="http://www.sisostds.org/ontologies/lox#ARCCTL">
        <rdf:type rdf:resource="http://www.sisostds.org/ontologies/C2SIM#TaskActionCode"/>
        <rdfs:comment>Airborne command and control: To conduct battlespace command and control operations from an airborne platform.</rdfs:comment>
    </owl:NamedIndividual>
    


    <!-- http://www.sisostds.org/ontologies/lox#ARDREQ -->

    <owl:NamedIndividual rdf:about="http://www.sisostds.org/ontologies/lox#ARDREQ">
        <rdf:type rdf:resource="http://www.sisostds.org/ontologies/C2SIM#TaskActionCode"/>
        <rdfs:comment>Airdrop, heavy equipment: To unload heavy equipment from an aircraft in flight.</rdfs:comment>
    </owl:NamedIndividual>
    


    <!-- http://www.sisostds.org/ontologies/lox#ARDROP -->

    <owl:NamedIndividual rdf:about="http://www.sisostds.org/ontologies/lox#ARDROP">
        <rdf:type rdf:resource="http://www.sisostds.org/ontologies/C2SIM#TaskActionCode"/>
        <rdfs:comment>Airdrop: To deliver personnel or cargo from aircraft in flight.</rdfs:comment>
    </owl:NamedIndividual>
    


    <!-- http://www.sisostds.org/ontologies/lox#ARINTR -->

    <owl:NamedIndividual rdf:about="http://www.sisostds.org/ontologies/lox#ARINTR">
        <rdf:type rdf:resource="http://www.sisostds.org/ontologies/C2SIM#TaskActionCode"/>
        <rdfs:comment>Air interdiction, battlefield: To conduct air operations to destroy, neutralize, or delay the enemy&apos;s military potential on the battlefield before it can</rdfs:comment>
    </owl:NamedIndividual>
    


    <!-- http://www.sisostds.org/ontologies/lox#ARLFSA -->

    <owl:NamedIndividual rdf:about="http://www.sisostds.org/ontologies/lox#ARLFSA">
        <rdf:type rdf:resource="http://www.sisostds.org/ontologies/C2SIM#TaskActionCode"/>
        <rdfs:comment>Airlift, special assignment: To require a special airlift for which a need of special consideration due to the number of passengers involved or the weight</rdfs:comment>
    </owl:NamedIndividual>
    


    <!-- http://www.sisostds.org/ontologies/lox#ARLFTR -->

    <owl:NamedIndividual rdf:about="http://www.sisostds.org/ontologies/lox#ARLFTR">
        <rdf:type rdf:resource="http://www.sisostds.org/ontologies/C2SIM#TaskActionCode"/>
        <rdfs:comment>Airlift, theatre: To provide air movement and delivery of personnel and equipment directly into objective areas through air landing, airdrop,</rdfs:comment>
    </owl:NamedIndividual>
    


    <!-- http://www.sisostds.org/ontologies/lox#ARMAS -->

    <owl:NamedIndividual rdf:about="http://www.sisostds.org/ontologies/lox#ARMAS">
        <rdf:type rdf:resource="http://www.sisostds.org/ontologies/C2SIM#TaskActionCode"/>
        <rdfs:comment>Armed assault: To perform a short, violent, but well ordered, attack against a local objective such as a gun emplacement, a fort or a machine-gun</rdfs:comment>
    </owl:NamedIndividual>
    


    <!-- http://www.sisostds.org/ontologies/lox#ARRLGL -->

    <owl:NamedIndividual rdf:about="http://www.sisostds.org/ontologies/lox#ARRLGL">
        <rdf:type rdf:resource="http://www.sisostds.org/ontologies/C2SIM#TaskActionCode"/>
        <rdfs:comment>Arrest, legal: To seize and detain a person under authority of the law.</rdfs:comment>
    </owl:NamedIndividual>
    


    <!-- http://www.sisostds.org/ontologies/lox#ARROBS -->

    <owl:NamedIndividual rdf:about="http://www.sisostds.org/ontologies/lox#ARROBS">
        <rdf:type rdf:resource="http://www.sisostds.org/ontologies/C2SIM#TaskActionCode"/>
        <rdfs:comment>Arrest/obstruct: To stop or check the motion, progress, growth, or spread of something.</rdfs:comment>
    </owl:NamedIndividual>
    


    <!-- http://www.sisostds.org/ontologies/lox#ARTCTL -->

    <owl:NamedIndividual rdf:about="http://www.sisostds.org/ontologies/lox#ARTCTL">
        <rdf:type rdf:resource="http://www.sisostds.org/ontologies/C2SIM#TaskActionCode"/>
        <rdfs:comment>Air traffic control: To provide air traffic control service to flights in control areas.</rdfs:comment>
    </owl:NamedIndividual>
    


    <!-- http://www.sisostds.org/ontologies/lox#ASSMBL -->

    <owl:NamedIndividual rdf:about="http://www.sisostds.org/ontologies/lox#ASSMBL">
        <rdf:type rdf:resource="http://www.sisostds.org/ontologies/C2SIM#TaskActionCode"/>
        <rdfs:comment>Assemble: To join together multiple objects in the same area.</rdfs:comment>
        <rdfs:comment>Documentation: 		
						To join together multiple objects in the same area.	
					; Appinfo DisplayValue as &quot;Assemble&quot;</rdfs:comment>
    </owl:NamedIndividual>
    


    <!-- http://www.sisostds.org/ontologies/lox#ATTACK -->

    <owl:NamedIndividual rdf:about="http://www.sisostds.org/ontologies/lox#ATTACK">
        <rdf:type rdf:resource="http://www.sisostds.org/ontologies/C2SIM#TaskActionCode"/>
        <rdfs:comment>Attack, not otherwise specified: To conduct a type of offensive action characterised by coordinated employment of firepower and manoeuvre to close with and</rdfs:comment>
        <rdfs:comment>Documentation: 		
						To conduct a type of offensive action characterised by coordinated employment of firepower and manoeuvre to close with and destroy or capture the enemy.	
					; Appinfo DisplayValue as &quot;Attack, not otherwise specified&quot;</rdfs:comment>
    </owl:NamedIndividual>
    


    <!-- http://www.sisostds.org/ontologies/lox#ATTDVR -->

    <owl:NamedIndividual rdf:about="http://www.sisostds.org/ontologies/lox#ATTDVR">
        <rdf:type rdf:resource="http://www.sisostds.org/ontologies/C2SIM#TaskActionCode"/>
        <rdfs:comment>Attack, diversion: To conduct an attack wherein a force attacks, or threatens to attack, a target other than the main target for the purpose</rdfs:comment>
    </owl:NamedIndividual>
    


    <!-- http://www.sisostds.org/ontologies/lox#ATTEL -->

    <owl:NamedIndividual rdf:about="http://www.sisostds.org/ontologies/lox#ATTEL">
        <rdf:type rdf:resource="http://www.sisostds.org/ontologies/C2SIM#TaskActionCode"/>
        <rdfs:comment>Attack, electronic: To conduct electronic warfare involving the use of electromagnetic energy, directed energy or anti-radiation weapons to attack</rdfs:comment>
    </owl:NamedIndividual>
    


    <!-- http://www.sisostds.org/ontologies/lox#ATTMN -->

    <owl:NamedIndividual rdf:about="http://www.sisostds.org/ontologies/lox#ATTMN">
        <rdf:type rdf:resource="http://www.sisostds.org/ontologies/C2SIM#TaskActionCode"/>
        <rdfs:comment>Attack, main: To conduct the principal attack or effort into which the commander throws the full weight of the offensive power at his disposal.</rdfs:comment>
    </owl:NamedIndividual>
    


    <!-- http://www.sisostds.org/ontologies/lox#ATTRIT -->

    <owl:NamedIndividual rdf:about="http://www.sisostds.org/ontologies/lox#ATTRIT">
        <rdf:type rdf:resource="http://www.sisostds.org/ontologies/C2SIM#TaskActionCode"/>
        <rdfs:comment>Attrit: To reduce of the effectiveness of a force by causing loss of personnel and materiel.</rdfs:comment>
        <rdfs:comment>Documentation: 		
						To reduce of the effectiveness of a force by causing loss of personnel and materiel.	
					; Appinfo DisplayValue as &quot;Attrit&quot;</rdfs:comment>
    </owl:NamedIndividual>
    


    <!-- http://www.sisostds.org/ontologies/lox#ATTSPT -->

    <owl:NamedIndividual rdf:about="http://www.sisostds.org/ontologies/lox#ATTSPT">
        <rdf:type rdf:resource="http://www.sisostds.org/ontologies/C2SIM#TaskActionCode"/>
        <rdfs:comment>Attack, supporting: To conduct an offensive operation carried out in conjunction with a main attack and designed to achieve one or more of the</rdfs:comment>
        <rdfs:comment>Documentation: 		
						To conduct an offensive operation carried out in conjunction with a main attack and designed to achieve one or more of the following: a. deceive the enemy; b. destroy or pin down enemy forces which could interfere with the main attack; c. control ground whose occupation by the enemy will hinder the main attack; or d. force the enemy to commit reserves prematurely or in an indecisive area.	
					; Appinfo DisplayValue as &quot;Attack, supporting&quot;</rdfs:comment>
    </owl:NamedIndividual>
    


    <!-- http://www.sisostds.org/ontologies/lox#AVOID -->

    <owl:NamedIndividual rdf:about="http://www.sisostds.org/ontologies/lox#AVOID">
        <rdf:type rdf:resource="http://www.sisostds.org/ontologies/C2SIM#TaskActionCode"/>
        <rdfs:comment>Avoid: To miss or take evading action.</rdfs:comment>
        <rdfs:comment>Documentation: 		
						To miss or take evading action.	
					; Appinfo DisplayValue as &quot;Avoid&quot;</rdfs:comment>
    </owl:NamedIndividual>
    


    <!-- http://www.sisostds.org/ontologies/lox#AWACS -->

    <owl:NamedIndividual rdf:about="http://www.sisostds.org/ontologies/lox#AWACS">
        <rdf:type rdf:resource="http://www.sisostds.org/ontologies/C2SIM#TaskActionCode"/>
        <rdfs:comment>Air warning/air control: To provide information about enemy air activity that poses immediate threat to friendly forces and monitors and directs the</rdfs:comment>
    </owl:NamedIndividual>
    


    <!-- http://www.sisostds.org/ontologies/lox#AllTasksComplete -->

    <owl:NamedIndividual rdf:about="http://www.sisostds.org/ontologies/lox#AllTasksComplete">
        <rdf:type rdf:resource="http://www.sisostds.org/ontologies/lox#PlanPhaseCompletionCondition"/>
    </owl:NamedIndividual>
    


    <!-- http://www.sisostds.org/ontologies/lox#BIOSMP -->

    <owl:NamedIndividual rdf:about="http://www.sisostds.org/ontologies/lox#BIOSMP">
        <rdf:type rdf:resource="http://www.sisostds.org/ontologies/C2SIM#TaskActionCode"/>
        <rdfs:comment>Biological sampling: To collect samples for testing for biological hazards.</rdfs:comment>
    </owl:NamedIndividual>
    


    <!-- http://www.sisostds.org/ontologies/lox#BLDUP -->

    <owl:NamedIndividual rdf:about="http://www.sisostds.org/ontologies/lox#BLDUP">
        <rdf:type rdf:resource="http://www.sisostds.org/ontologies/C2SIM#TaskActionCode"/>
        <rdfs:comment>Build-up: To attain prescribed strength of units and prescribed levels of vehicles, equipment, stores and supplies.</rdfs:comment>
    </owl:NamedIndividual>
    


    <!-- http://www.sisostds.org/ontologies/lox#BLOCK -->

    <owl:NamedIndividual rdf:about="http://www.sisostds.org/ontologies/lox#BLOCK">
        <rdf:type rdf:resource="http://www.sisostds.org/ontologies/C2SIM#TaskActionCode"/>
        <rdfs:comment>Block: To deny the enemy access to an area or to prevent his advance in a direction or along an avenue of approach.</rdfs:comment>
        <rdfs:comment>Documentation: 		
						To deny the enemy access to an area or to prevent his advance in a direction or along an avenue of approach.	
					; Appinfo DisplayValue as &quot;Block&quot;</rdfs:comment>
    </owl:NamedIndividual>
    


    <!-- http://www.sisostds.org/ontologies/lox#BRAKUP -->

    <owl:NamedIndividual rdf:about="http://www.sisostds.org/ontologies/lox#BRAKUP">
        <rdf:type rdf:resource="http://www.sisostds.org/ontologies/C2SIM#TaskActionCode"/>
        <rdfs:comment>Breakup: No definition provided in ADatP-3 Baseline 13.1 FFIRN/FUD 1299/19.</rdfs:comment>
    </owl:NamedIndividual>
    


    <!-- http://www.sisostds.org/ontologies/lox#BREACH -->

    <owl:NamedIndividual rdf:about="http://www.sisostds.org/ontologies/lox#BREACH">
        <rdf:type rdf:resource="http://www.sisostds.org/ontologies/C2SIM#TaskActionCode"/>
        <rdfs:comment>Breach: To break through or secure a passage through an enemy defence, obstacle, minefield, or fortification.</rdfs:comment>
        <rdfs:comment>Documentation: 		
						To break through or secure a passage through an enemy defence, obstacle, minefield, or fortification.	
					; Appinfo DisplayValue as &quot;Breach&quot;</rdfs:comment>
    </owl:NamedIndividual>
    


    <!-- http://www.sisostds.org/ontologies/lox#BURN -->

    <owl:NamedIndividual rdf:about="http://www.sisostds.org/ontologies/lox#BURN">
        <rdfs:comment>Documentation: 		
						The ACTION objective is alight.	
					; Appinfo DisplayValue as &quot;Burning&quot;</rdfs:comment>
    </owl:NamedIndividual>
    


    <!-- http://www.sisostds.org/ontologies/lox#BYPASS -->

    <owl:NamedIndividual rdf:about="http://www.sisostds.org/ontologies/lox#BYPASS">
        <rdf:type rdf:resource="http://www.sisostds.org/ontologies/C2SIM#TaskActionCode"/>
        <rdfs:comment>Bypass: To manoeuvre around an obstacle, position, or enemy force in order to maintain the momentum of advance.</rdfs:comment>
        <rdfs:comment>Documentation: 		
						To manoeuvre around an obstacle, position, or enemy force in order to maintain the momentum of advance.	
					; Appinfo DisplayValue as &quot;Bypass&quot;</rdfs:comment>
    </owl:NamedIndividual>
    


    <!-- http://www.sisostds.org/ontologies/lox#CADVGD -->

    <owl:NamedIndividual rdf:about="http://www.sisostds.org/ontologies/lox#CADVGD">
        <rdf:type rdf:resource="http://www.sisostds.org/ontologies/C2SIM#TaskActionCode"/>
        <rdfs:comment>Constitute an advance guard: To provide a security element whose primary task is to move ahead of the main body and protect the main force by fighting</rdfs:comment>
    </owl:NamedIndividual>
    


    <!-- http://www.sisostds.org/ontologies/lox#CANDC -->

    <owl:NamedIndividual rdf:about="http://www.sisostds.org/ontologies/lox#CANDC">
        <rdf:type rdf:resource="http://www.sisostds.org/ontologies/C2SIM#TaskActionCode"/>
        <rdfs:comment>Command and control: To exercise authority and direction over assigned and attached forces in the accomplishment of the mission.</rdfs:comment>
    </owl:NamedIndividual>
    


    <!-- http://www.sisostds.org/ontologies/lox#CANLSE -->

    <owl:NamedIndividual rdf:about="http://www.sisostds.org/ontologies/lox#CANLSE">
        <rdf:type rdf:resource="http://www.sisostds.org/ontologies/C2SIM#TaskActionCode"/>
        <rdfs:comment>Canalise: To restrict operations to a narrow zone by use of existing or reinforcing obstacles or by fire or bombing. (Army)--A tactical</rdfs:comment>
    </owl:NamedIndividual>
    


    <!-- http://www.sisostds.org/ontologies/lox#CAPBAR -->

    <owl:NamedIndividual rdf:about="http://www.sisostds.org/ontologies/lox#CAPBAR">
        <rdf:type rdf:resource="http://www.sisostds.org/ontologies/C2SIM#TaskActionCode"/>
        <rdfs:comment>Combat air patrol, barrier: To conduct a patrol by fighter aircraft that is employed between a force and an objective area as a barrier across the probable</rdfs:comment>
    </owl:NamedIndividual>
    


    <!-- http://www.sisostds.org/ontologies/lox#CAPNGR -->

    <owl:NamedIndividual rdf:about="http://www.sisostds.org/ontologies/lox#CAPNGR">
        <rdf:type rdf:resource="http://www.sisostds.org/ontologies/C2SIM#TaskActionCode"/>
        <rdfs:comment>Combat air patrol, ingress: Combat air patrol flown in support of friendly aircraft as the aircraft ingress into enemy territory.</rdfs:comment>
    </owl:NamedIndividual>
    


    <!-- http://www.sisostds.org/ontologies/lox#CAPPRT -->

    <owl:NamedIndividual rdf:about="http://www.sisostds.org/ontologies/lox#CAPPRT">
        <rdf:type rdf:resource="http://www.sisostds.org/ontologies/C2SIM#TaskActionCode"/>
        <rdfs:comment>Combat air patrol, protect: An aircraft patrol flying over an objective area in order to protect friendly forces.</rdfs:comment>
    </owl:NamedIndividual>
    


    <!-- http://www.sisostds.org/ontologies/lox#CAPRES -->

    <owl:NamedIndividual rdf:about="http://www.sisostds.org/ontologies/lox#CAPRES">
        <rdf:type rdf:resource="http://www.sisostds.org/ontologies/C2SIM#TaskActionCode"/>
        <rdfs:comment>Combat air patrol, rescue: To protect the search and rescue task forces during recovery operations.</rdfs:comment>
    </owl:NamedIndividual>
    


    <!-- http://www.sisostds.org/ontologies/lox#CAPSRF -->

    <owl:NamedIndividual rdf:about="http://www.sisostds.org/ontologies/lox#CAPSRF">
        <rdf:type rdf:resource="http://www.sisostds.org/ontologies/C2SIM#TaskActionCode"/>
        <rdfs:comment>Combat air patrol, surface: Combat air patrol flown in support of surface vessels conducting maritime operations.</rdfs:comment>
    </owl:NamedIndividual>
    


    <!-- http://www.sisostds.org/ontologies/lox#CAPTRD -->

    <owl:NamedIndividual rdf:about="http://www.sisostds.org/ontologies/lox#CAPTRD">
        <rdfs:comment>Documentation: 		
						The ACTION objective has been captured or acquired and is available for use or interrogation/possession has been taken of an area, normally by force.	
					; Appinfo DisplayValue as &quot;Captured&quot;</rdfs:comment>
    </owl:NamedIndividual>
    


    <!-- http://www.sisostds.org/ontologies/lox#CAPTUR -->

    <owl:NamedIndividual rdf:about="http://www.sisostds.org/ontologies/lox#CAPTUR">
        <rdf:type rdf:resource="http://www.sisostds.org/ontologies/C2SIM#TaskActionCode"/>
        <rdfs:comment>Capture: To take possession of an object, normally by force; it frequently involves movement as a preliminary phase.</rdfs:comment>
        <rdfs:comment>Documentation: 		
						To take possession of an object, normally by force; it frequently involves movement as a preliminary phase.	
					; Appinfo DisplayValue as &quot;Capture&quot;</rdfs:comment>
    </owl:NamedIndividual>
    


    <!-- http://www.sisostds.org/ontologies/lox#CARLNC -->

    <owl:NamedIndividual rdf:about="http://www.sisostds.org/ontologies/lox#CARLNC">
        <rdf:type rdf:resource="http://www.sisostds.org/ontologies/C2SIM#TaskActionCode"/>
        <rdfs:comment>Carrier launch: To launch aircraft from a naval platform.</rdfs:comment>
    </owl:NamedIndividual>
    


    <!-- http://www.sisostds.org/ontologies/lox#CARREC -->

    <owl:NamedIndividual rdf:about="http://www.sisostds.org/ontologies/lox#CARREC">
        <rdf:type rdf:resource="http://www.sisostds.org/ontologies/C2SIM#TaskActionCode"/>
        <rdfs:comment>Carrier recovery: To recover aircraft on a naval platform.</rdfs:comment>
    </owl:NamedIndividual>
    


    <!-- http://www.sisostds.org/ontologies/lox#CBRHDF -->

    <owl:NamedIndividual rdf:about="http://www.sisostds.org/ontologies/lox#CBRHDF">
        <rdf:type rdf:resource="http://www.sisostds.org/ontologies/C2SIM#TaskActionCode"/>
        <rdfs:comment>Constitute bridgehead force: To form the force during an obstacle crossing which seizes or controls ground in order to permit the continuous embarkation,</rdfs:comment>
    </owl:NamedIndividual>
    


    <!-- http://www.sisostds.org/ontologies/lox#CBRKOF -->

    <owl:NamedIndividual rdf:about="http://www.sisostds.org/ontologies/lox#CBRKOF">
        <rdf:type rdf:resource="http://www.sisostds.org/ontologies/C2SIM#TaskActionCode"/>
        <rdfs:comment>Constitute breakout force: To form the force during an obstacle crossing which is tasked with the continuation of the operation.</rdfs:comment>
    </owl:NamedIndividual>
    


    <!-- http://www.sisostds.org/ontologies/lox#CDWDAC -->

    <owl:NamedIndividual rdf:about="http://www.sisostds.org/ontologies/lox#CDWDAC">
        <rdf:type rdf:resource="http://www.sisostds.org/ontologies/C2SIM#TaskActionCode"/>
        <rdfs:comment>Codeword activity: To conduct an activity described by the action-task-detail-text.</rdfs:comment>
    </owl:NamedIndividual>
    


    <!-- http://www.sisostds.org/ontologies/lox#CFLKGD -->

    <owl:NamedIndividual rdf:about="http://www.sisostds.org/ontologies/lox#CFLKGD">
        <rdf:type rdf:resource="http://www.sisostds.org/ontologies/C2SIM#TaskActionCode"/>
        <rdfs:comment>Constitute a flank guard: To provide a security element whose primary task is to protect the main force by fighting on the designated flank to gain</rdfs:comment>
    </owl:NamedIndividual>
    


    <!-- http://www.sisostds.org/ontologies/lox#CHAFF -->

    <owl:NamedIndividual rdf:about="http://www.sisostds.org/ontologies/lox#CHAFF">
        <rdf:type rdf:resource="http://www.sisostds.org/ontologies/C2SIM#TaskActionCode"/>
        <rdfs:comment>Release CHAFF: To deploy strips of frequency-cut metal foil, wire or metalized glass fibre to reflect electromagnetic energy, usually dropped</rdfs:comment>
    </owl:NamedIndividual>
    


    <!-- http://www.sisostds.org/ontologies/lox#CHMSMP -->

    <owl:NamedIndividual rdf:about="http://www.sisostds.org/ontologies/lox#CHMSMP">
        <rdf:type rdf:resource="http://www.sisostds.org/ontologies/C2SIM#TaskActionCode"/>
        <rdfs:comment>Chemical sampling: To collect samples for testing for chemical hazards.</rdfs:comment>
    </owl:NamedIndividual>
    


    <!-- http://www.sisostds.org/ontologies/lox#CINPLF -->

    <owl:NamedIndividual rdf:about="http://www.sisostds.org/ontologies/lox#CINPLF">
        <rdf:type rdf:resource="http://www.sisostds.org/ontologies/C2SIM#TaskActionCode"/>
        <rdfs:comment>Constitute in-place force: To form the force during an obstacle crossing which provides fire and other support to the bridgehead force.</rdfs:comment>
    </owl:NamedIndividual>
    


    <!-- http://www.sisostds.org/ontologies/lox#CLARSP -->

    <owl:NamedIndividual rdf:about="http://www.sisostds.org/ontologies/lox#CLARSP">
        <rdf:type rdf:resource="http://www.sisostds.org/ontologies/C2SIM#TaskActionCode"/>
        <rdfs:comment>Close air support: Air action against hostile targets which are in close proximity to friendly forces and which require detailed integration</rdfs:comment>
    </owl:NamedIndividual>
    


    <!-- http://www.sisostds.org/ontologies/lox#CLOSE -->

    <owl:NamedIndividual rdf:about="http://www.sisostds.org/ontologies/lox#CLOSE">
        <rdf:type rdf:resource="http://www.sisostds.org/ontologies/C2SIM#TaskActionCode"/>
        <rdfs:comment>Close: To prevent a FACILITY or FEATURE from performing its intended function.</rdfs:comment>
        <rdfs:comment>Documentation: 		
						To prevent a FACILITY or FEATURE from performing its intended function.	
					; Appinfo DisplayValue as &quot;Close&quot;</rdfs:comment>
    </owl:NamedIndividual>
    


    <!-- http://www.sisostds.org/ontologies/lox#CLRAIR -->

    <owl:NamedIndividual rdf:about="http://www.sisostds.org/ontologies/lox#CLRAIR">
        <rdf:type rdf:resource="http://www.sisostds.org/ontologies/C2SIM#TaskActionCode"/>
        <rdfs:comment>Clear, air: To clear the air to gain either temporary or permanent air superiority or control in a given sector.</rdfs:comment>
    </owl:NamedIndividual>
    


    <!-- http://www.sisostds.org/ontologies/lox#CLRLND -->

    <owl:NamedIndividual rdf:about="http://www.sisostds.org/ontologies/lox#CLRLND">
        <rdf:type rdf:resource="http://www.sisostds.org/ontologies/C2SIM#TaskActionCode"/>
        <rdfs:comment>Clear, land combat: To remove all enemy forces from a specific location, area, or zone.</rdfs:comment>
        <rdfs:comment>Documentation: 		
						To remove all enemy forces from a specific location, area, or zone.	
					; Appinfo DisplayValue as &quot;Clear, land combat&quot;</rdfs:comment>
    </owl:NamedIndividual>
    


    <!-- http://www.sisostds.org/ontologies/lox#CLROBS -->

    <owl:NamedIndividual rdf:about="http://www.sisostds.org/ontologies/lox#CLROBS">
        <rdf:type rdf:resource="http://www.sisostds.org/ontologies/C2SIM#TaskActionCode"/>
        <rdfs:comment>Clear, obstacle: To totally eliminate or neutralize an obstacle; a task that is usually performed by follow-on engineers and is not done under</rdfs:comment>
        <rdfs:comment>Documentation: 		
						To totally eliminate or neutralize an obstacle; a task that is usually performed by follow-on engineers and is not done under fire.	
					; Appinfo DisplayValue as &quot;Clear, obstacle&quot;</rdfs:comment>
    </owl:NamedIndividual>
    


    <!-- http://www.sisostds.org/ontologies/lox#CLRRAD -->

    <owl:NamedIndividual rdf:about="http://www.sisostds.org/ontologies/lox#CLRRAD">
        <rdf:type rdf:resource="http://www.sisostds.org/ontologies/C2SIM#TaskActionCode"/>
        <rdfs:comment>Clear, radio net: To eliminate transmissions on a tactical radio net in order to allow a higher precedence transmission to occur.</rdfs:comment>
    </owl:NamedIndividual>
    


    <!-- http://www.sisostds.org/ontologies/lox#CMAINB -->

    <owl:NamedIndividual rdf:about="http://www.sisostds.org/ontologies/lox#CMAINB">
        <rdf:type rdf:resource="http://www.sisostds.org/ontologies/C2SIM#TaskActionCode"/>
        <rdfs:comment>Constitute a main body: To constitute the main force for a specific operation.</rdfs:comment>
    </owl:NamedIndividual>
    


    <!-- http://www.sisostds.org/ontologies/lox#CNFPSL -->

    <owl:NamedIndividual rdf:about="http://www.sisostds.org/ontologies/lox#CNFPSL">
        <rdf:type rdf:resource="http://www.sisostds.org/ontologies/C2SIM#TaskActionCode"/>
        <rdfs:comment>Conduct forward passage of lines: An operation in which an incoming force attacks through a unit (outgoing force).that is in contact with the enemy.</rdfs:comment>
        <rdfs:comment>Documentation: 		
						An operation in which an incoming force attacks through a unit (outgoing force).that is in contact with the enemy.	
					; Appinfo DisplayValue as &quot;Conduct forward passage of lines&quot;</rdfs:comment>
    </owl:NamedIndividual>
    


    <!-- http://www.sisostds.org/ontologies/lox#CNFSTE -->

    <owl:NamedIndividual rdf:about="http://www.sisostds.org/ontologies/lox#CNFSTE">
        <rdf:type rdf:resource="http://www.sisostds.org/ontologies/C2SIM#TaskActionCode"/>
        <rdfs:comment>Confiscate: To deprive a person of his property as forfeited by public authority.</rdfs:comment>
    </owl:NamedIndividual>
    


    <!-- http://www.sisostds.org/ontologies/lox#CNRPSL -->

    <owl:NamedIndividual rdf:about="http://www.sisostds.org/ontologies/lox#CNRPSL">
        <rdf:type rdf:resource="http://www.sisostds.org/ontologies/C2SIM#TaskActionCode"/>
        <rdfs:comment>Conduct rearward passage of lines: An operation when a force (outgoing force) effecting a movement to the rear passes through the sector of a unit (incoming</rdfs:comment>
        <rdfs:comment>Documentation: 		
						An operation when a force (outgoing force) effecting a movement to the rear passes through the sector of a unit (incoming force).	
					; Appinfo DisplayValue as &quot;Conduct rearward passage of lines&quot;</rdfs:comment>
    </owl:NamedIndividual>
    


    <!-- http://www.sisostds.org/ontologies/lox#CNRSVC -->

    <owl:NamedIndividual rdf:about="http://www.sisostds.org/ontologies/lox#CNRSVC">
        <rdf:type rdf:resource="http://www.sisostds.org/ontologies/C2SIM#TaskActionCode"/>
        <rdfs:comment>Conduct road service: To enable the movement of a number of specific units.</rdfs:comment>
    </owl:NamedIndividual>
    


    <!-- http://www.sisostds.org/ontologies/lox#CNSLDT -->

    <owl:NamedIndividual rdf:about="http://www.sisostds.org/ontologies/lox#CNSLDT">
        <rdf:type rdf:resource="http://www.sisostds.org/ontologies/C2SIM#TaskActionCode"/>
        <rdfs:comment>Consolidate a position: To organise and strengthen a newly captured position so that it can be used against the enemy.</rdfs:comment>
    </owl:NamedIndividual>
    


    <!-- http://www.sisostds.org/ontologies/lox#COARPL -->

    <owl:NamedIndividual rdf:about="http://www.sisostds.org/ontologies/lox#COARPL">
        <rdf:type rdf:resource="http://www.sisostds.org/ontologies/C2SIM#TaskActionCode"/>
        <rdfs:comment>Combat air patrol: An aircraft patrol provided over an objective area, the force protected, the critical area of a combat zone, or in an air</rdfs:comment>
    </owl:NamedIndividual>
    


    <!-- http://www.sisostds.org/ontologies/lox#COMC3I -->

    <owl:NamedIndividual rdf:about="http://www.sisostds.org/ontologies/lox#COMC3I">
        <rdf:type rdf:resource="http://www.sisostds.org/ontologies/C2SIM#TaskActionCode"/>
        <rdfs:comment>Communications (C3I): To provide communication means such as data links or radio for the purpose of communication, command, control and intelligence.</rdfs:comment>
    </owl:NamedIndividual>
    


    <!-- http://www.sisostds.org/ontologies/lox#COMINC -->

    <owl:NamedIndividual rdf:about="http://www.sisostds.org/ontologies/lox#COMINC">
        <rdf:type rdf:resource="http://www.sisostds.org/ontologies/C2SIM#TaskActionCode"/>
        <rdfs:comment>Communication, intelligence collection: To gather communication intelligence in order to meet current operational requirements.</rdfs:comment>
    </owl:NamedIndividual>
    


    <!-- http://www.sisostds.org/ontologies/lox#COMREL -->

    <owl:NamedIndividual rdf:about="http://www.sisostds.org/ontologies/lox#COMREL">
        <rdf:type rdf:resource="http://www.sisostds.org/ontologies/C2SIM#TaskActionCode"/>
        <rdfs:comment>Communications relay: To employ an aircraft to serve as a communications relay.</rdfs:comment>
    </owl:NamedIndividual>
    


    <!-- http://www.sisostds.org/ontologies/lox#CONS -->

    <owl:NamedIndividual rdf:about="http://www.sisostds.org/ontologies/lox#CONS">
        <rdfs:comment>Documentation: 		
						The consumption of specified consumables or CONSUMABLE-MATERIEL-TYPEs.	
					; Appinfo DisplayValue as &quot;Consumed&quot;</rdfs:comment>
    </owl:NamedIndividual>
    


    <!-- http://www.sisostds.org/ontologies/lox#CONSTR -->

    <owl:NamedIndividual rdf:about="http://www.sisostds.org/ontologies/lox#CONSTR">
        <rdf:type rdf:resource="http://www.sisostds.org/ontologies/C2SIM#TaskActionCode"/>
        <rdfs:comment>Construct: To build, dig or create an object.</rdfs:comment>
    </owl:NamedIndividual>
    


    <!-- http://www.sisostds.org/ontologies/lox#CONTAN -->

    <owl:NamedIndividual rdf:about="http://www.sisostds.org/ontologies/lox#CONTAN">
        <rdf:type rdf:resource="http://www.sisostds.org/ontologies/C2SIM#TaskActionCode"/>
        <rdfs:comment>Contain: To stop, hold, or surround the forces of the enemy or to cause the enemy to centre activity on a given front and to prevent</rdfs:comment>
    </owl:NamedIndividual>
    


    <!-- http://www.sisostds.org/ontologies/lox#COOPER -->

    <owl:NamedIndividual rdf:about="http://www.sisostds.org/ontologies/lox#COOPER">
        <rdf:type rdf:resource="http://www.sisostds.org/ontologies/C2SIM#TaskActionCode"/>
        <rdfs:comment>Cooperate: To work or act together.</rdfs:comment>
    </owl:NamedIndividual>
    


    <!-- http://www.sisostds.org/ontologies/lox#COURER -->

    <owl:NamedIndividual rdf:about="http://www.sisostds.org/ontologies/lox#COURER">
        <rdf:type rdf:resource="http://www.sisostds.org/ontologies/C2SIM#TaskActionCode"/>
        <rdfs:comment>Courier: To travel as a courier.</rdfs:comment>
    </owl:NamedIndividual>
    


    <!-- http://www.sisostds.org/ontologies/lox#COVER -->

    <owl:NamedIndividual rdf:about="http://www.sisostds.org/ontologies/lox#COVER">
        <rdf:type rdf:resource="http://www.sisostds.org/ontologies/C2SIM#TaskActionCode"/>
        <rdfs:comment>Cover: To operate as a force apart to protect the main body by fighting to gain time while also observing and reporting information</rdfs:comment>
        <rdfs:comment>Documentation: 		
						To operate as a force apart to protect the main body by fighting to gain time while also observing and reporting information and preventing enemy ground observation of an direct fire against the main body.	
					; Appinfo DisplayValue as &quot;Cover&quot;</rdfs:comment>
    </owl:NamedIndividual>
    


    <!-- http://www.sisostds.org/ontologies/lox#CRESRV -->

    <owl:NamedIndividual rdf:about="http://www.sisostds.org/ontologies/lox#CRESRV">
        <rdf:type rdf:resource="http://www.sisostds.org/ontologies/C2SIM#TaskActionCode"/>
        <rdfs:comment>Constitute a reserve: To constitute a force which may be committed into combat only on the order of the commander of the ORGANISATION who so designated</rdfs:comment>
        <rdfs:comment>Documentation: 		
						To constitute a force which may be committed into combat only on the order of the commander of the ORGANISATION who so designated the reserve force.	
					; Appinfo DisplayValue as &quot;Constitute a reserve&quot;</rdfs:comment>
    </owl:NamedIndividual>
    


    <!-- http://www.sisostds.org/ontologies/lox#CROSS -->

    <owl:NamedIndividual rdf:about="http://www.sisostds.org/ontologies/lox#CROSS">
        <rdf:type rdf:resource="http://www.sisostds.org/ontologies/C2SIM#TaskActionCode"/>
        <rdfs:comment>Cross: To move over a FEATURE or FACILITY.</rdfs:comment>
    </owl:NamedIndividual>
    


    <!-- http://www.sisostds.org/ontologies/lox#CRRGD -->

    <owl:NamedIndividual rdf:about="http://www.sisostds.org/ontologies/lox#CRRGD">
        <rdf:type rdf:resource="http://www.sisostds.org/ontologies/C2SIM#TaskActionCode"/>
        <rdfs:comment>Constitute a rear guard: To provide a security element whose primary task is to move (or remain) at the rear of the main body and protect the main</rdfs:comment>
    </owl:NamedIndividual>
    


    <!-- http://www.sisostds.org/ontologies/lox#CTRATK -->

    <owl:NamedIndividual rdf:about="http://www.sisostds.org/ontologies/lox#CTRATK">
        <rdf:type rdf:resource="http://www.sisostds.org/ontologies/C2SIM#TaskActionCode"/>
        <rdfs:comment>Counter attack: To mount an offensive operation in which an attack by a part or all of a defending force is made against an enemy attacking</rdfs:comment>
        <rdfs:comment>Documentation: 		
						To mount an offensive operation in which an attack by a part or all of a defending force is made against an enemy attacking force, for such specific purposes as regaining ground lost, cutting off or destroying lead enemy units, and with the general objective of regaining the initiative and denying the enemy the attainment of his goal or purpose in attacking.	
					; Appinfo DisplayValue as &quot;Counter attack&quot;</rdfs:comment>
    </owl:NamedIndividual>
    


    <!-- http://www.sisostds.org/ontologies/lox#CTRBYF -->

    <owl:NamedIndividual rdf:about="http://www.sisostds.org/ontologies/lox#CTRBYF">
        <rdf:type rdf:resource="http://www.sisostds.org/ontologies/C2SIM#TaskActionCode"/>
        <rdfs:comment>Counter-battery fire: To deliver fire for the purpose of destroying or neutralizing indirect fire weapons systems.</rdfs:comment>
        <rdfs:comment>Documentation: 		
						To deliver fire for the purpose of destroying or neutralizing indirect fire weapons systems.	
					; Appinfo DisplayValue as &quot;Counter-battery fire&quot;</rdfs:comment>
    </owl:NamedIndividual>
    


    <!-- http://www.sisostds.org/ontologies/lox#CTRFIR -->

    <owl:NamedIndividual rdf:about="http://www.sisostds.org/ontologies/lox#CTRFIR">
        <rdf:type rdf:resource="http://www.sisostds.org/ontologies/C2SIM#TaskActionCode"/>
        <rdfs:comment>Counter attack by fire: To deny the enemy his goal in attacking through fire into an engagement area to defeat or destroy an enemy force.</rdfs:comment>
        <rdfs:comment>Documentation: 		
						To deny the enemy his goal in attacking through fire into an engagement area to defeat or destroy an enemy force.	
					; Appinfo DisplayValue as &quot;Counter attack by fire&quot;</rdfs:comment>
    </owl:NamedIndividual>
    


    <!-- http://www.sisostds.org/ontologies/lox#DAZZLE -->

    <owl:NamedIndividual rdf:about="http://www.sisostds.org/ontologies/lox#DAZZLE">
        <rdf:type rdf:resource="http://www.sisostds.org/ontologies/C2SIM#TaskActionCode"/>
        <rdfs:comment>Dazzle: To confuse the enemy by temporary loss of vision or a temporary reduction in visual acuity; may also be applied to effects</rdfs:comment>
    </owl:NamedIndividual>
    


    <!-- http://www.sisostds.org/ontologies/lox#DCPTEL -->

    <owl:NamedIndividual rdf:about="http://www.sisostds.org/ontologies/lox#DCPTEL">
        <rdf:type rdf:resource="http://www.sisostds.org/ontologies/C2SIM#TaskActionCode"/>
        <rdfs:comment>Deception, electronic: In electronic countermeasures, the deliberate radiation, re-radiation, alteration, absorption or reflection of electromagnetic</rdfs:comment>
    </owl:NamedIndividual>
    


    <!-- http://www.sisostds.org/ontologies/lox#DEBARK -->

    <owl:NamedIndividual rdf:about="http://www.sisostds.org/ontologies/lox#DEBARK">
        <rdf:type rdf:resource="http://www.sisostds.org/ontologies/C2SIM#TaskActionCode"/>
        <rdfs:comment>Debark: To unload troops with their supplies and equipment from a ship.</rdfs:comment>
    </owl:NamedIndividual>
    


    <!-- http://www.sisostds.org/ontologies/lox#DECEIV -->

    <owl:NamedIndividual rdf:about="http://www.sisostds.org/ontologies/lox#DECEIV">
        <rdf:type rdf:resource="http://www.sisostds.org/ontologies/C2SIM#TaskActionCode"/>
        <rdfs:comment>Deceive: To employ measures designed to mislead the enemy by manipulation, distortion, or falsification of evidence to induce him to</rdfs:comment>
        <rdfs:comment>Documentation: 		
						To employ measures designed to mislead the enemy by manipulation, distortion, or falsification of evidence to induce him to react in a manner prejudicial to his interests.	
					; Appinfo DisplayValue as &quot;Deceive&quot;</rdfs:comment>
    </owl:NamedIndividual>
    


    <!-- http://www.sisostds.org/ontologies/lox#DECSVC -->

    <owl:NamedIndividual rdf:about="http://www.sisostds.org/ontologies/lox#DECSVC">
        <rdf:type rdf:resource="http://www.sisostds.org/ontologies/C2SIM#TaskActionCode"/>
        <rdfs:comment>Decontamination services: To provide purification making any person, object, or area safe by absorbing, destroying, neutralizing, making harmless, or</rdfs:comment>
    </owl:NamedIndividual>
    


    <!-- http://www.sisostds.org/ontologies/lox#DEFCNT -->

    <owl:NamedIndividual rdf:about="http://www.sisostds.org/ontologies/lox#DEFCNT">
        <rdf:type rdf:resource="http://www.sisostds.org/ontologies/C2SIM#TaskActionCode"/>
        <rdfs:comment>Defensive counter air: To conduct air operations to attain and maintain a desired degree of air superiority by the destruction or neutralization</rdfs:comment>
    </owl:NamedIndividual>
    


    <!-- http://www.sisostds.org/ontologies/lox#DEFDST -->

    <owl:NamedIndividual rdf:about="http://www.sisostds.org/ontologies/lox#DEFDST">
        <rdf:type rdf:resource="http://www.sisostds.org/ontologies/C2SIM#TaskActionCode"/>
        <rdfs:comment>Defence destruction: To destroy enemy defences in a specific area by any means.</rdfs:comment>
    </owl:NamedIndividual>
    


    <!-- http://www.sisostds.org/ontologies/lox#DEFEAT -->

    <owl:NamedIndividual rdf:about="http://www.sisostds.org/ontologies/lox#DEFEAT">
        <rdf:type rdf:resource="http://www.sisostds.org/ontologies/C2SIM#TaskActionCode"/>
        <rdfs:comment>Defeat: To diminish the effectiveness of the enemy to the extent that he is unable to participate further in the battle or at least</rdfs:comment>
        <rdfs:comment>Documentation: 		
						To diminish the effectiveness of the enemy to the extent that he is unable to participate further in the battle or at least cannot fulfil his intention.	
					; Appinfo DisplayValue as &quot;Defeat&quot;</rdfs:comment>
    </owl:NamedIndividual>
    


    <!-- http://www.sisostds.org/ontologies/lox#DEFEND -->

    <owl:NamedIndividual rdf:about="http://www.sisostds.org/ontologies/lox#DEFEND">
        <rdf:type rdf:resource="http://www.sisostds.org/ontologies/C2SIM#TaskActionCode"/>
        <rdfs:comment>Defend: To hold a defined object against an enemy attack; to halt or ward off an attack in order to defeat or destroy the enemy.</rdfs:comment>
        <rdfs:comment>Documentation: 		
						To hold a defined object against an enemy attack; to halt or ward off an attack in order to defeat or destroy the enemy.	
					; Appinfo DisplayValue as &quot;Defend&quot;</rdfs:comment>
    </owl:NamedIndividual>
    


    <!-- http://www.sisostds.org/ontologies/lox#DEFLCT -->

    <owl:NamedIndividual rdf:about="http://www.sisostds.org/ontologies/lox#DEFLCT">
        <rdf:type rdf:resource="http://www.sisostds.org/ontologies/C2SIM#TaskActionCode"/>
        <rdfs:comment>Deflect: To prevent an enemy force from following the intended course.</rdfs:comment>
    </owl:NamedIndividual>
    


    <!-- http://www.sisostds.org/ontologies/lox#DEFSUP -->

    <owl:NamedIndividual rdf:about="http://www.sisostds.org/ontologies/lox#DEFSUP">
        <rdf:type rdf:resource="http://www.sisostds.org/ontologies/C2SIM#TaskActionCode"/>
        <rdfs:comment>Defence suppression: To neutralize, destroy or temporarily degrade enemy defences in a specific area by physical attack and/or electronic warfare.</rdfs:comment>
    </owl:NamedIndividual>
    


    <!-- http://www.sisostds.org/ontologies/lox#DELAY -->

    <owl:NamedIndividual rdf:about="http://www.sisostds.org/ontologies/lox#DELAY">
        <rdf:type rdf:resource="http://www.sisostds.org/ontologies/C2SIM#TaskActionCode"/>
        <rdfs:comment>Delay: To slow the momentum of the enemy by conducting an operation in which the force under pressure trades time for space. The</rdfs:comment>
        <rdfs:comment>Documentation: 		
						To slow the momentum of the enemy by conducting an operation in which the force under pressure trades time for space. The aim is to inflict the maximum damage on the enemy without becoming decisively engaged.	
					; Appinfo DisplayValue as &quot;Delay&quot;</rdfs:comment>
    </owl:NamedIndividual>
    


    <!-- http://www.sisostds.org/ontologies/lox#DEMFRP -->

    <owl:NamedIndividual rdf:about="http://www.sisostds.org/ontologies/lox#DEMFRP">
        <rdf:type rdf:resource="http://www.sisostds.org/ontologies/C2SIM#TaskActionCode"/>
        <rdfs:comment>Constitute a demolition firing party: To provide the party at the site which is technically responsible for the demolition.</rdfs:comment>
    </owl:NamedIndividual>
    


    <!-- http://www.sisostds.org/ontologies/lox#DEMGRD -->

    <owl:NamedIndividual rdf:about="http://www.sisostds.org/ontologies/lox#DEMGRD">
        <rdf:type rdf:resource="http://www.sisostds.org/ontologies/C2SIM#TaskActionCode"/>
        <rdfs:comment>Constitute a demolition guard: To provide a local force positioned to ensure that a target is not captured by an enemy before orders are given for its demolition</rdfs:comment>
    </owl:NamedIndividual>
    


    <!-- http://www.sisostds.org/ontologies/lox#DEMO -->

    <owl:NamedIndividual rdf:about="http://www.sisostds.org/ontologies/lox#DEMO">
        <rdf:type rdf:resource="http://www.sisostds.org/ontologies/C2SIM#TaskActionCode"/>
        <rdfs:comment>Demolish: To destroy structures, facilities, or materiel by use of fire, water, explosives, mechanical, or other means.</rdfs:comment>
    </owl:NamedIndividual>
    


    <!-- http://www.sisostds.org/ontologies/lox#DENY -->

    <owl:NamedIndividual rdf:about="http://www.sisostds.org/ontologies/lox#DENY">
        <rdf:type rdf:resource="http://www.sisostds.org/ontologies/C2SIM#TaskActionCode"/>
        <rdfs:comment>Deny: To prevent access by blocking, disrupting, dislocating and/or bringing fire to bear.</rdfs:comment>
        <rdfs:comment>Documentation: 		
						To prevent access by blocking, disrupting, dislocating and/or bringing fire to bear.	
					; Appinfo DisplayValue as &quot;Deny&quot;</rdfs:comment>
    </owl:NamedIndividual>
    


    <!-- http://www.sisostds.org/ontologies/lox#DEPLOY -->

    <owl:NamedIndividual rdf:about="http://www.sisostds.org/ontologies/lox#DEPLOY">
        <rdf:type rdf:resource="http://www.sisostds.org/ontologies/C2SIM#TaskActionCode"/>
        <rdfs:comment>Deploy: To move and adopt tactical formation or dispersal in a specific location.</rdfs:comment>
    </owl:NamedIndividual>
    


    <!-- http://www.sisostds.org/ontologies/lox#DESCRB -->

    <owl:NamedIndividual rdf:about="http://www.sisostds.org/ontologies/lox#DESCRB">
        <rdf:type rdf:resource="http://www.sisostds.org/ontologies/C2SIM#TaskActionCode"/>
        <rdfs:comment>Describe: To state the characteristics, appearance, etc. of an object.</rdfs:comment>
    </owl:NamedIndividual>
    


    <!-- http://www.sisostds.org/ontologies/lox#DESTRY -->

    <owl:NamedIndividual rdf:about="http://www.sisostds.org/ontologies/lox#DESTRY">
        <rdf:type rdf:resource="http://www.sisostds.org/ontologies/C2SIM#TaskActionCode"/>
        <rdfs:comment>Destroy: To physically render an enemy force combat-ineffective or damaging a target so that it cannot function as intended, nor be</rdfs:comment>
        <rdfs:comment>Documentation: 		
						To physically render an enemy force combat-ineffective or damaging a target so that it cannot function as intended, nor be restored to a usable condition without being entirely rebuilt.	
					; Appinfo DisplayValue as &quot;Destroy&quot;</rdfs:comment>
    </owl:NamedIndividual>
    


    <!-- http://www.sisostds.org/ontologies/lox#DETECT -->

    <owl:NamedIndividual rdf:about="http://www.sisostds.org/ontologies/lox#DETECT">
        <rdf:type rdf:resource="http://www.sisostds.org/ontologies/C2SIM#TaskActionCode"/>
        <rdfs:comment>Detect: To discover by any means of the presence of a person, object or phenomenon of potential military significance.</rdfs:comment>
    </owl:NamedIndividual>
    


    <!-- http://www.sisostds.org/ontologies/lox#DISENG -->

    <owl:NamedIndividual rdf:about="http://www.sisostds.org/ontologies/lox#DISENG">
        <rdf:type rdf:resource="http://www.sisostds.org/ontologies/C2SIM#TaskActionCode"/>
        <rdfs:comment>Disengage: To break off an action.</rdfs:comment>
        <rdfs:comment>Documentation: 		
						To break off an action.	
					; Appinfo DisplayValue as &quot;Disengage&quot;</rdfs:comment>
    </owl:NamedIndividual>
    


    <!-- http://www.sisostds.org/ontologies/lox#DISRPT -->

    <owl:NamedIndividual rdf:about="http://www.sisostds.org/ontologies/lox#DISRPT">
        <rdf:type rdf:resource="http://www.sisostds.org/ontologies/C2SIM#TaskActionCode"/>
        <rdfs:comment>Disrupt: To break apart an enemy&apos;s formation and tempo, to interrupt the enemy&apos;s timetable, to cause premature commitment of forces,</rdfs:comment>
        <rdfs:comment>Documentation: 		
						To break apart an enemy&apos;s formation and tempo, to interrupt the enemy&apos;s timetable, to cause premature commitment of forces, and/or splinter their attack using integrated fire planning and obstacle effect.	
					; Appinfo DisplayValue as &quot;Disrupt&quot;</rdfs:comment>
    </owl:NamedIndividual>
    


    <!-- http://www.sisostds.org/ontologies/lox#DIVE -->

    <owl:NamedIndividual rdf:about="http://www.sisostds.org/ontologies/lox#DIVE">
        <rdf:type rdf:resource="http://www.sisostds.org/ontologies/C2SIM#TaskActionCode"/>
        <rdfs:comment>Dive: To descend or plunge into or underwater or some other liquid.</rdfs:comment>
    </owl:NamedIndividual>
    


    <!-- http://www.sisostds.org/ontologies/lox#DIVERT -->

    <owl:NamedIndividual rdf:about="http://www.sisostds.org/ontologies/lox#DIVERT">
        <rdf:type rdf:resource="http://www.sisostds.org/ontologies/C2SIM#TaskActionCode"/>
        <rdfs:comment>Divert: To draw the attention and forces of an enemy from the point of the principal operation; an attack, alarm, or feint which diverts</rdfs:comment>
    </owl:NamedIndividual>
    


    <!-- http://www.sisostds.org/ontologies/lox#DLBATK -->

    <owl:NamedIndividual rdf:about="http://www.sisostds.org/ontologies/lox#DLBATK">
        <rdf:type rdf:resource="http://www.sisostds.org/ontologies/C2SIM#TaskActionCode"/>
        <rdfs:comment>Attack, deliberate: To conduct a type of offensive action characterised by pre-planned coordinated employment of firepower and manoeuvre to close</rdfs:comment>
        <rdfs:comment>Documentation: 		
						To conduct a type of offensive action characterised by pre-planned coordinated employment of firepower and manoeuvre to close with and destroy or capture the enemy.	
					; Appinfo DisplayValue as &quot;Attack, deliberate&quot;</rdfs:comment>
    </owl:NamedIndividual>
    


    <!-- http://www.sisostds.org/ontologies/lox#DRONL -->

    <owl:NamedIndividual rdf:about="http://www.sisostds.org/ontologies/lox#DRONL">
        <rdf:type rdf:resource="http://www.sisostds.org/ontologies/C2SIM#TaskActionCode"/>
        <rdfs:comment>Documentation: 		
						To perform the launching of drones.	
					; Appinfo DisplayValue as &quot;Drone launch&quot;</rdfs:comment>
        <rdfs:comment>Drone launch: To perform the launching of drones.</rdfs:comment>
    </owl:NamedIndividual>
    


    <!-- http://www.sisostds.org/ontologies/lox#DSTRBT -->

    <owl:NamedIndividual rdf:about="http://www.sisostds.org/ontologies/lox#DSTRBT">
        <rdf:type rdf:resource="http://www.sisostds.org/ontologies/C2SIM#TaskActionCode"/>
        <rdfs:comment>Distribute: To divide or dispense in portions.</rdfs:comment>
    </owl:NamedIndividual>
    


    <!-- http://www.sisostds.org/ontologies/lox#DSTRYK -->

    <owl:NamedIndividual rdf:about="http://www.sisostds.org/ontologies/lox#DSTRYK">
        <rdfs:comment>Documentation: 		
						Cannot function as intended nor be repaired or restored to an operational status.	
					; Appinfo DisplayValue as &quot;Destroyed (K-kill)&quot;</rdfs:comment>
    </owl:NamedIndividual>
    


    <!-- http://www.sisostds.org/ontologies/lox#DUMPNG -->

    <owl:NamedIndividual rdf:about="http://www.sisostds.org/ontologies/lox#DUMPNG">
        <rdf:type rdf:resource="http://www.sisostds.org/ontologies/C2SIM#TaskActionCode"/>
        <rdfs:comment>Dumping: To position stocks to meet future requirements.</rdfs:comment>
    </owl:NamedIndividual>
    


    <!-- http://www.sisostds.org/ontologies/lox#ELCCNM -->

    <owl:NamedIndividual rdf:about="http://www.sisostds.org/ontologies/lox#ELCCNM">
        <rdf:type rdf:resource="http://www.sisostds.org/ontologies/C2SIM#TaskActionCode"/>
        <rdfs:comment>Electronic counter measures: To perform electronic warfare actions to prevent or reduce an enemy&apos;s effective use of the electromagnetic spectrum through</rdfs:comment>
    </owl:NamedIndividual>
    


    <!-- http://www.sisostds.org/ontologies/lox#ELCWAR -->

    <owl:NamedIndividual rdf:about="http://www.sisostds.org/ontologies/lox#ELCWAR">
        <rdf:type rdf:resource="http://www.sisostds.org/ontologies/C2SIM#TaskActionCode"/>
        <rdfs:comment>Electronic warfare: To exploit the electromagnetic spectrum encompassing; the search for, interception of electromagnetic emissions, the employment</rdfs:comment>
    </owl:NamedIndividual>
    


    <!-- http://www.sisostds.org/ontologies/lox#ELCWRS -->

    <owl:NamedIndividual rdf:about="http://www.sisostds.org/ontologies/lox#ELCWRS">
        <rdf:type rdf:resource="http://www.sisostds.org/ontologies/C2SIM#TaskActionCode"/>
        <rdfs:comment>Electronic warfare support: To search for, intercept, locate, record measures and analyse radiated electromagnetic energy for the purpose of exploiting</rdfs:comment>
    </owl:NamedIndividual>
    


    <!-- http://www.sisostds.org/ontologies/lox#EMBARK -->

    <owl:NamedIndividual rdf:about="http://www.sisostds.org/ontologies/lox#EMBARK">
        <rdf:type rdf:resource="http://www.sisostds.org/ontologies/C2SIM#TaskActionCode"/>
        <rdfs:comment>Embark: To put personnel and/or vehicles and their associated stores and equipment into ships or aircraft.</rdfs:comment>
    </owl:NamedIndividual>
    


    <!-- http://www.sisostds.org/ontologies/lox#ENGAGE -->

    <owl:NamedIndividual rdf:about="http://www.sisostds.org/ontologies/lox#ENGAGE">
        <rdf:type rdf:resource="http://www.sisostds.org/ontologies/C2SIM#TaskActionCode"/>
        <rdfs:comment>Documentation: 		
						To bring the enemy under fire.	
					; Appinfo DisplayValue as &quot;Engage&quot;</rdfs:comment>
        <rdfs:comment>Engage: To bring the enemy under fire.</rdfs:comment>
    </owl:NamedIndividual>
    


    <!-- http://www.sisostds.org/ontologies/lox#ENVLP -->

    <owl:NamedIndividual rdf:about="http://www.sisostds.org/ontologies/lox#ENVLP">
        <rdf:type rdf:resource="http://www.sisostds.org/ontologies/C2SIM#TaskActionCode"/>
        <rdfs:comment>Documentation: 		
						To conduct an offensive manoeuvre in which the main attacking force passes around or over the enemy&apos;s principal defensive positions with the aim of securing objectives to the enemy&apos;s rear.	
					; Appinfo DisplayValue as &quot;Envelop&quot;</rdfs:comment>
        <rdfs:comment>Envelop: To conduct an offensive manoeuvre in which the main attacking force passes around or over the enemy&apos;s principal defensive</rdfs:comment>
    </owl:NamedIndividual>
    


    <!-- http://www.sisostds.org/ontologies/lox#ESCRT -->

    <owl:NamedIndividual rdf:about="http://www.sisostds.org/ontologies/lox#ESCRT">
        <rdf:type rdf:resource="http://www.sisostds.org/ontologies/C2SIM#TaskActionCode"/>
        <rdfs:comment>Escort: To accompany and protect another force or convoy.</rdfs:comment>
    </owl:NamedIndividual>
    


    <!-- http://www.sisostds.org/ontologies/lox#EVACT -->

    <owl:NamedIndividual rdf:about="http://www.sisostds.org/ontologies/lox#EVACT">
        <rdf:type rdf:resource="http://www.sisostds.org/ontologies/C2SIM#TaskActionCode"/>
        <rdfs:comment>Evacuate: To clear materiel and personnel from a given locality.</rdfs:comment>
    </owl:NamedIndividual>
    


    <!-- http://www.sisostds.org/ontologies/lox#EXFLTR -->

    <owl:NamedIndividual rdf:about="http://www.sisostds.org/ontologies/lox#EXFLTR">
        <rdf:type rdf:resource="http://www.sisostds.org/ontologies/C2SIM#TaskActionCode"/>
        <rdfs:comment>Exfiltrate: To withdraw from a dangerous position.</rdfs:comment>
    </owl:NamedIndividual>
    


    <!-- http://www.sisostds.org/ontologies/lox#EXPLT -->

    <owl:NamedIndividual rdf:about="http://www.sisostds.org/ontologies/lox#EXPLT">
        <rdf:type rdf:resource="http://www.sisostds.org/ontologies/C2SIM#TaskActionCode"/>
        <rdfs:comment>Documentation: 		
						To take advantage of a successful attack by mounting an offensive operation to follow-up and harass a dislocated enemy with the aim of further disorganising him in depth. This may provide the opportunity to capture ground which was not part of the objective of the original attack.	
					; Appinfo DisplayValue as &quot;Exploit&quot;</rdfs:comment>
        <rdfs:comment>Exploit: To take advantage of a successful attack by mounting an offensive operation to follow-up and harass a dislocated enemy with</rdfs:comment>
    </owl:NamedIndividual>
    


    <!-- http://www.sisostds.org/ontologies/lox#ExecutePlanPhase -->

    <owl:NamedIndividual rdf:about="http://www.sisostds.org/ontologies/lox#ExecutePlanPhase">
        <rdf:type rdf:resource="http://www.sisostds.org/ontologies/C2SIM#TaskActionCode"/>
    </owl:NamedIndividual>
    <owl:Axiom>
        <owl:annotatedSource rdf:resource="http://www.sisostds.org/ontologies/lox#ExecutePlanPhase"/>
        <owl:annotatedProperty rdf:resource="http://www.w3.org/1999/02/22-rdf-syntax-ns#type"/>
        <owl:annotatedTarget rdf:resource="http://www.sisostds.org/ontologies/C2SIM#TaskActionCode"/>
        <rdfs:comment>This code indicates that the task is to execute a previously provided plan phase.</rdfs:comment>
    </owl:Axiom>
    


    <!-- http://www.sisostds.org/ontologies/lox#FIX -->

    <owl:NamedIndividual rdf:about="http://www.sisostds.org/ontologies/lox#FIX">
        <rdf:type rdf:resource="http://www.sisostds.org/ontologies/C2SIM#TaskActionCode"/>
        <rdfs:comment>Documentation: 		
						To prevent the enemy from moving any part of his force from a specific location for a specific period of time.	
					; Appinfo DisplayValue as &quot;Fix&quot;</rdfs:comment>
        <rdfs:comment>Fix: To prevent the enemy from moving any part of his force from a specific location for a specific period of time.</rdfs:comment>
    </owl:NamedIndividual>
    


    <!-- http://www.sisostds.org/ontologies/lox#FIXACO -->

    <owl:NamedIndividual rdf:about="http://www.sisostds.org/ontologies/lox#FIXACO">
        <rdf:type rdf:resource="http://www.sisostds.org/ontologies/C2SIM#TaskActionCode"/>
        <rdfs:comment>Fix, acoustic: To determine a position using acoustic data.</rdfs:comment>
    </owl:NamedIndividual>
    


    <!-- http://www.sisostds.org/ontologies/lox#FIXELM -->

    <owl:NamedIndividual rdf:about="http://www.sisostds.org/ontologies/lox#FIXELM">
        <rdf:type rdf:resource="http://www.sisostds.org/ontologies/C2SIM#TaskActionCode"/>
        <rdfs:comment>Fix, electromagnetic: To determine a position using electromagnetic data.</rdfs:comment>
    </owl:NamedIndividual>
    


    <!-- http://www.sisostds.org/ontologies/lox#FIXELO -->

    <owl:NamedIndividual rdf:about="http://www.sisostds.org/ontologies/lox#FIXELO">
        <rdf:type rdf:resource="http://www.sisostds.org/ontologies/C2SIM#TaskActionCode"/>
        <rdfs:comment>Fix, electro-optical: To determine a position using electro-optical data.</rdfs:comment>
    </owl:NamedIndividual>
    


    <!-- http://www.sisostds.org/ontologies/lox#FKIL -->

    <owl:NamedIndividual rdf:about="http://www.sisostds.org/ontologies/lox#FKIL">
        <rdfs:comment>Documentation: 		
						The destruction of a vehicle (or system&apos;s) primary weapon system.	
					; Appinfo DisplayValue as &quot;Firepower kill (F-kill)&quot;</rdfs:comment>
    </owl:NamedIndividual>
    


    <!-- http://www.sisostds.org/ontologies/lox#FLIG -->

    <owl:NamedIndividual rdf:about="http://www.sisostds.org/ontologies/lox#FLIG">
        <rdfs:comment>Documentation: 		
						The setting to flight of a PERSON or PERSON-TYPEs from their present location.	
					; Appinfo DisplayValue as &quot;Forced to flee&quot;</rdfs:comment>
    </owl:NamedIndividual>
    


    <!-- http://www.sisostds.org/ontologies/lox#FNCHFL -->

    <owl:NamedIndividual rdf:about="http://www.sisostds.org/ontologies/lox#FNCHFL">
        <rdf:type rdf:resource="http://www.sisostds.org/ontologies/C2SIM#TaskActionCode"/>
        <rdfs:comment>Functional check flight: To conduct a test flight to ensure the general aircraft safety after maintenance/repair, and to ensure the aircraft is fully</rdfs:comment>
    </owl:NamedIndividual>
    


    <!-- http://www.sisostds.org/ontologies/lox#FOLASS -->

    <owl:NamedIndividual rdf:about="http://www.sisostds.org/ontologies/lox#FOLASS">
        <rdf:type rdf:resource="http://www.sisostds.org/ontologies/C2SIM#TaskActionCode"/>
        <rdfs:comment>Follow and assume: To operate as a committed force that follows a force conducting an offensive operation, and is prepared to continue the mission</rdfs:comment>
    </owl:NamedIndividual>
    


    <!-- http://www.sisostds.org/ontologies/lox#FOLSPT -->

    <owl:NamedIndividual rdf:about="http://www.sisostds.org/ontologies/lox#FOLSPT">
        <rdf:type rdf:resource="http://www.sisostds.org/ontologies/C2SIM#TaskActionCode"/>
        <rdfs:comment>Follow and support: To operate as a committed force that follows and supports the mission accomplishment of a force conducting an offensive operation.</rdfs:comment>
    </owl:NamedIndividual>
    


    <!-- http://www.sisostds.org/ontologies/lox#FRWDAC -->

    <owl:NamedIndividual rdf:about="http://www.sisostds.org/ontologies/lox#FRWDAC">
        <rdf:type rdf:resource="http://www.sisostds.org/ontologies/C2SIM#TaskActionCode"/>
        <rdfs:comment>Forward air control: To direct the action of combat aircraft engaged in close air support of land forces from a forward position on the ground</rdfs:comment>
    </owl:NamedIndividual>
    


    <!-- http://www.sisostds.org/ontologies/lox#GENCHS -->

    <owl:NamedIndividual rdf:about="http://www.sisostds.org/ontologies/lox#GENCHS">
        <rdf:type rdf:resource="http://www.sisostds.org/ontologies/C2SIM#TaskActionCode"/>
        <rdfs:comment>Generate chemical smoke: To produce chemical smoke to act as a form of cover to protect ongoing operations.</rdfs:comment>
    </owl:NamedIndividual>
    


    <!-- http://www.sisostds.org/ontologies/lox#GUARD -->

    <owl:NamedIndividual rdf:about="http://www.sisostds.org/ontologies/lox#GUARD">
        <rdf:type rdf:resource="http://www.sisostds.org/ontologies/C2SIM#TaskActionCode"/>
        <rdfs:comment>Documentation: 		
						To protect the main body by fighting to gain time while also observing and reporting information.	
					; Appinfo DisplayValue as &quot;Guard&quot;</rdfs:comment>
        <rdfs:comment>Guard: To protect the main body by fighting to gain time while also observing and reporting information.</rdfs:comment>
    </owl:NamedIndividual>
    


    <!-- http://www.sisostds.org/ontologies/lox#HARASS -->

    <owl:NamedIndividual rdf:about="http://www.sisostds.org/ontologies/lox#HARASS">
        <rdf:type rdf:resource="http://www.sisostds.org/ontologies/C2SIM#TaskActionCode"/>
        <rdfs:comment>Documentation: 		
						To mount an operation or fire plan designed to curtail movement and, by threat of losses, to lower the morale of enemy troops.	
					; Appinfo DisplayValue as &quot;Harass&quot;</rdfs:comment>
        <rdfs:comment>Harass: To mount an operation or fire plan designed to curtail movement and, by threat of losses, to lower the morale of enemy troops.</rdfs:comment>
    </owl:NamedIndividual>
    


    <!-- http://www.sisostds.org/ontologies/lox#HASPRV -->

    <owl:NamedIndividual rdf:about="http://www.sisostds.org/ontologies/lox#HASPRV">
        <rdf:type rdf:resource="http://www.sisostds.org/ontologies/lox#TaskFunctionalAssociationCode"/>
        <rdfs:comment>Has as a provisional sub-ACTION: The subject ACTION may be re-directed to an alternative object ACTION. Note: The need for object ACTION is foreseen in planning,</rdfs:comment>
    </owl:NamedIndividual>
    


    <!-- http://www.sisostds.org/ontologies/lox#HASSEC -->

    <owl:NamedIndividual rdf:about="http://www.sisostds.org/ontologies/lox#HASSEC">
        <rdf:type rdf:resource="http://www.sisostds.org/ontologies/lox#TaskFunctionalAssociationCode"/>
        <rdfs:comment>Has as secondary: The subject ACTION is designated as the primary activity and has the object ACTION as a secondary activity.</rdfs:comment>
    </owl:NamedIndividual>
    


    <!-- http://www.sisostds.org/ontologies/lox#HASTY -->

    <owl:NamedIndividual rdf:about="http://www.sisostds.org/ontologies/lox#HASTY">
        <rdf:type rdf:resource="http://www.sisostds.org/ontologies/C2SIM#TaskActionCode"/>
        <rdfs:comment>Attack, hasty: To conduct a type of offensive action using firepower and manoeuvre to close with and destroy or capture the enemy. Planning</rdfs:comment>
        <rdfs:comment>Documentation: 		
						To conduct a type of offensive action using firepower and manoeuvre to close with and destroy or capture the enemy. Planning and coordination will normally be limited, as the attack will be carried out at short notice.	
					; Appinfo DisplayValue as &quot;Attack, hasty&quot;</rdfs:comment>
    </owl:NamedIndividual>
    


    <!-- http://www.sisostds.org/ontologies/lox#HIDE -->

    <owl:NamedIndividual rdf:about="http://www.sisostds.org/ontologies/lox#HIDE">
        <rdf:type rdf:resource="http://www.sisostds.org/ontologies/C2SIM#TaskActionCode"/>
        <rdfs:comment>Hide: To occupy an area in which an ORGANISATION or FACILITY may conceal itself before operations or before moving into battle positions.</rdfs:comment>
    </owl:NamedIndividual>
    


    <!-- http://www.sisostds.org/ontologies/lox#HLDDEF -->

    <owl:NamedIndividual rdf:about="http://www.sisostds.org/ontologies/lox#HLDDEF">
        <rdf:type rdf:resource="http://www.sisostds.org/ontologies/C2SIM#TaskActionCode"/>
        <rdfs:comment>Hold, defensive: To maintain or retain possession by force, a position or area in defensive operations.</rdfs:comment>
    </owl:NamedIndividual>
    


    <!-- http://www.sisostds.org/ontologies/lox#HLDOFF -->

    <owl:NamedIndividual rdf:about="http://www.sisostds.org/ontologies/lox#HLDOFF">
        <rdf:type rdf:resource="http://www.sisostds.org/ontologies/C2SIM#TaskActionCode"/>
        <rdfs:comment>Hold, offensive: To exert sufficient pressure in an offensive operation by means of combat power, to prevent the movement or redeployment of</rdfs:comment>
    </owl:NamedIndividual>
    


    <!-- http://www.sisostds.org/ontologies/lox#HONASP -->

    <owl:NamedIndividual rdf:about="http://www.sisostds.org/ontologies/lox#HONASP">
        <rdf:type rdf:resource="http://www.sisostds.org/ontologies/C2SIM#TaskActionCode"/>
        <rdfs:comment>Documentation: 		
						Civil and military assistance rendered in peace, crisis and war by a host nation to Allied forces and NATO organisations which are located on or in transit through the host nation&apos;s territory. The basis of such assistance is commitments arising from the NATO Alliance or from bilateral or multilateral agreements concluded between the host nation, NATO organisations and (the) nation(s) having forces operating on the host nation&apos;s territory.	
					; Appinfo DisplayValue as &quot;Host nation support&quot;</rdfs:comment>
        <rdfs:comment>Host nation support: Civil and military assistance rendered in peace, crisis and war by a host nation to Allied forces and NATO organisations which</rdfs:comment>
    </owl:NamedIndividual>
    


    <!-- http://www.sisostds.org/ontologies/lox#HSA -->

    <owl:NamedIndividual rdf:about="http://www.sisostds.org/ontologies/lox#HSA">
        <rdf:type rdf:resource="http://www.sisostds.org/ontologies/lox#TaskFunctionalAssociationCode"/>
        <rdfs:comment>Has as a sub-ACTION: The value that links two activities such that the subject ACTION has as a sub-ACTION the object ACTION.</rdfs:comment>
    </owl:NamedIndividual>
    


    <!-- http://www.sisostds.org/ontologies/lox#IDENT -->

    <owl:NamedIndividual rdf:about="http://www.sisostds.org/ontologies/lox#IDENT">
        <rdf:type rdf:resource="http://www.sisostds.org/ontologies/C2SIM#TaskActionCode"/>
        <rdfs:comment>Identify: To determine the identification of a particular class of object, recognising the friendly or enemy character of an object,</rdfs:comment>
    </owl:NamedIndividual>
    


    <!-- http://www.sisostds.org/ontologies/lox#IDENTP -->

    <owl:NamedIndividual rdf:about="http://www.sisostds.org/ontologies/lox#IDENTP">
        <rdf:type rdf:resource="http://www.sisostds.org/ontologies/C2SIM#TaskActionCode"/>
        <rdfs:comment>Identify, precise: To determine by any act or means additional information of a detected person, object or phenomenon, in a detailed, accurate</rdfs:comment>
    </owl:NamedIndividual>
    


    <!-- http://www.sisostds.org/ontologies/lox#IDNT -->

    <owl:NamedIndividual rdf:about="http://www.sisostds.org/ontologies/lox#IDNT">
        <rdfs:comment>Documentation: 		
						The ACTION objective has been either identified (i.e., classified as friend/foe/neutral) or recognised (i.e., the unit designation of the ORGANISATION or object is known).	
					; Appinfo DisplayValue as &quot;Identified&quot;</rdfs:comment>
    </owl:NamedIndividual>
    


    <!-- http://www.sisostds.org/ontologies/lox#ILLUMN -->

    <owl:NamedIndividual rdf:about="http://www.sisostds.org/ontologies/lox#ILLUMN">
        <rdf:type rdf:resource="http://www.sisostds.org/ontologies/C2SIM#TaskActionCode"/>
        <rdfs:comment>Documentation: 		
						The temporary supply of IR or white-light illumination (usually in coordination with direct or indirect fire).	
					; Appinfo DisplayValue as &quot;Illuminated&quot;</rdfs:comment>
        <rdfs:comment>Illuminate: To provide battlespace lighting by employing searchlight or pyrotechnic illuminants using diffusion or reflection.</rdfs:comment>
    </owl:NamedIndividual>
    


    <!-- http://www.sisostds.org/ontologies/lox#IMINGT -->

    <owl:NamedIndividual rdf:about="http://www.sisostds.org/ontologies/lox#IMINGT">
        <rdf:type rdf:resource="http://www.sisostds.org/ontologies/C2SIM#TaskActionCode"/>
        <rdfs:comment>Imagery intelligence gathering: To gather imagery for intelligence purposes.</rdfs:comment>
    </owl:NamedIndividual>
    


    <!-- http://www.sisostds.org/ontologies/lox#IMO -->

    <owl:NamedIndividual rdf:about="http://www.sisostds.org/ontologies/lox#IMO">
        <rdf:type rdf:resource="http://www.sisostds.org/ontologies/lox#TaskFunctionalAssociationCode"/>
        <rdfs:comment>Is a modification of: The value denoting that the subject ACTION amends (or suggests an amendment to) an existing object ACTION (be it a plan, order,</rdfs:comment>
    </owl:NamedIndividual>
    


    <!-- http://www.sisostds.org/ontologies/lox#INFILT -->

    <owl:NamedIndividual rdf:about="http://www.sisostds.org/ontologies/lox#INFILT">
        <rdf:type rdf:resource="http://www.sisostds.org/ontologies/C2SIM#TaskActionCode"/>
        <rdfs:comment>Documentation: 		
						To move a force, broken down as individuals or small groups, over, through or around enemy positions with the aim of avoiding detection.	
					; Appinfo DisplayValue as &quot;Infiltrate&quot;</rdfs:comment>
        <rdfs:comment>Infiltrate: To move a force, broken down as individuals or small groups, over, through or around enemy positions with the aim of avoiding</rdfs:comment>
    </owl:NamedIndividual>
    


    <!-- http://www.sisostds.org/ontologies/lox#INFOOP -->

    <owl:NamedIndividual rdf:about="http://www.sisostds.org/ontologies/lox#INFOOP">
        <rdf:type rdf:resource="http://www.sisostds.org/ontologies/C2SIM#TaskActionCode"/>
        <rdfs:comment>Information operations: To conduct an operation that includes actions to influence decision makers in support of political and military objectives</rdfs:comment>
    </owl:NamedIndividual>
    


    <!-- http://www.sisostds.org/ontologies/lox#INRSTO -->

    <owl:NamedIndividual rdf:about="http://www.sisostds.org/ontologies/lox#INRSTO">
        <rdf:type rdf:resource="http://www.sisostds.org/ontologies/lox#TaskFunctionalAssociationCode"/>
        <rdfs:comment>In response to: The value that links two ACTIONs such that the subject ACTION is planned to be or may be expected to be carried out in reaction</rdfs:comment>
    </owl:NamedIndividual>
    


    <!-- http://www.sisostds.org/ontologies/lox#INTCEP -->

    <owl:NamedIndividual rdf:about="http://www.sisostds.org/ontologies/lox#INTCEP">
        <rdf:type rdf:resource="http://www.sisostds.org/ontologies/C2SIM#TaskActionCode"/>
        <rdfs:comment>Intercept: To conduct Electronic Warfare Support operations with a view to searching, locating, recording and analysing radiated electromagnetic</rdfs:comment>
    </owl:NamedIndividual>
    


    <!-- http://www.sisostds.org/ontologies/lox#INTCOL -->

    <owl:NamedIndividual rdf:about="http://www.sisostds.org/ontologies/lox#INTCOL">
        <rdf:type rdf:resource="http://www.sisostds.org/ontologies/C2SIM#TaskActionCode"/>
        <rdfs:comment>Intelligence collection: To gather information from all available sources to meet an intelligence requirement. Specifically, a logical plan for transforming</rdfs:comment>
    </owl:NamedIndividual>
    


    <!-- http://www.sisostds.org/ontologies/lox#INTDCT -->

    <owl:NamedIndividual rdf:about="http://www.sisostds.org/ontologies/lox#INTDCT">
        <rdf:type rdf:resource="http://www.sisostds.org/ontologies/C2SIM#TaskActionCode"/>
        <rdfs:comment>Documentation: 		
						To divert, disrupt, delay, or destroy the enemy&apos;s surface military potential before it can be used effectively against friendly forces.	
					; Appinfo DisplayValue as &quot;Interdict&quot;</rdfs:comment>
        <rdfs:comment>Interdict: To divert, disrupt, delay, or destroy the enemy&apos;s surface military potential before it can be used effectively against friendly</rdfs:comment>
    </owl:NamedIndividual>
    


    <!-- http://www.sisostds.org/ontologies/lox#INTREC -->

    <owl:NamedIndividual rdf:about="http://www.sisostds.org/ontologies/lox#INTREC">
        <rdfs:comment>Documentation: 		
						An equipment lost in an area unsuitable for recovery due to political, military or geographic/environmental considerations.	
					; Appinfo DisplayValue as &quot;Intact but unrecoverable&quot;</rdfs:comment>
    </owl:NamedIndividual>
    


    <!-- http://www.sisostds.org/ontologies/lox#IOT -->

    <owl:NamedIndividual rdf:about="http://www.sisostds.org/ontologies/lox#IOT">
        <rdf:type rdf:resource="http://www.sisostds.org/ontologies/lox#TaskFunctionalAssociationCode"/>
        <rdfs:comment>In order that: The subject ACTION is to be carried out so that the conditions are established for the completion of the object ACTION (e.g.,</rdfs:comment>
    </owl:NamedIndividual>
    


    <!-- http://www.sisostds.org/ontologies/lox#ISAPRQ -->

    <owl:NamedIndividual rdf:about="http://www.sisostds.org/ontologies/lox#ISAPRQ">
        <rdf:type rdf:resource="http://www.sisostds.org/ontologies/lox#TaskFunctionalAssociationCode"/>
        <rdfs:comment>Is a prerequisite for: The subject ACTION must be completed as planned before the object ACTION may commence.</rdfs:comment>
    </owl:NamedIndividual>
    


    <!-- http://www.sisostds.org/ontologies/lox#ISCAUS -->

    <owl:NamedIndividual rdf:about="http://www.sisostds.org/ontologies/lox#ISCAUS">
        <rdf:type rdf:resource="http://www.sisostds.org/ontologies/lox#TaskFunctionalAssociationCode"/>
        <rdfs:comment>Is the cause of: The value denoting that the subject ACTION is the cause for the object ACTION. (Note: This is intended to be used only when</rdfs:comment>
    </owl:NamedIndividual>
    


    <!-- http://www.sisostds.org/ontologies/lox#ISOLAT -->

    <owl:NamedIndividual rdf:about="http://www.sisostds.org/ontologies/lox#ISOLAT">
        <rdf:type rdf:resource="http://www.sisostds.org/ontologies/C2SIM#TaskActionCode"/>
        <rdfs:comment>Documentation: 		
						To seal off (both physically and psychologically) an enemy from its sources of support, to deny an enemy freedom of movement, and prevent an enemy unit from having contact with other enemy forces. An enemy must not be allowed sanctuary within its present position.	
					; Appinfo DisplayValue as &quot;Isolate&quot;</rdfs:comment>
        <rdfs:comment>Isolate: To seal off (both physically and psychologically) an enemy from its sources of support, to deny an enemy freedom of movement,</rdfs:comment>
    </owl:NamedIndividual>
    


    <!-- http://www.sisostds.org/ontologies/lox#ISSMDA -->

    <owl:NamedIndividual rdf:about="http://www.sisostds.org/ontologies/lox#ISSMDA">
        <rdf:type rdf:resource="http://www.sisostds.org/ontologies/C2SIM#TaskActionCode"/>
        <rdfs:comment>Issue media article: To send forth; publish; put into circulation a non-fictional essay, especially one included with others in a newspaper, magazine,</rdfs:comment>
    </owl:NamedIndividual>
    


    <!-- http://www.sisostds.org/ontologies/lox#ISSMDD -->

    <owl:NamedIndividual rdf:about="http://www.sisostds.org/ontologies/lox#ISSMDD">
        <rdf:type rdf:resource="http://www.sisostds.org/ontologies/C2SIM#TaskActionCode"/>
        <rdfs:comment>Issue media documentary: To send forth; publish; put into circulation any document published on a media that provides a factual record or report.</rdfs:comment>
    </owl:NamedIndividual>
    


    <!-- http://www.sisostds.org/ontologies/lox#ISSPRS -->

    <owl:NamedIndividual rdf:about="http://www.sisostds.org/ontologies/lox#ISSPRS">
        <rdf:type rdf:resource="http://www.sisostds.org/ontologies/C2SIM#TaskActionCode"/>
        <rdfs:comment>Issue press release: To send forth; publish; put into circulation an official statement issued to media for information.</rdfs:comment>
    </owl:NamedIndividual>
    


    <!-- http://www.sisostds.org/ontologies/lox#JAM -->

    <owl:NamedIndividual rdf:about="http://www.sisostds.org/ontologies/lox#JAM">
        <rdf:type rdf:resource="http://www.sisostds.org/ontologies/C2SIM#TaskActionCode"/>
        <rdfs:comment>Jam: To deliberately radiate, re-radiate or reflect electromagnetic energy with the object of impairing the use of electronic devices,</rdfs:comment>
    </owl:NamedIndividual>
    


    <!-- http://www.sisostds.org/ontologies/lox#KILL -->

    <owl:NamedIndividual rdf:about="http://www.sisostds.org/ontologies/lox#KILL">
        <rdfs:comment>Documentation: 		
						A casualty who is killed outright or dies as a result of wounds, disease or other injuries.	
					; Appinfo DisplayValue as &quot;Killed&quot;</rdfs:comment>
    </owl:NamedIndividual>
    


    <!-- http://www.sisostds.org/ontologies/lox#LAY -->

    <owl:NamedIndividual rdf:about="http://www.sisostds.org/ontologies/lox#LAY">
        <rdf:type rdf:resource="http://www.sisostds.org/ontologies/C2SIM#TaskActionCode"/>
        <rdfs:comment>Lay: To place on a surface, esp. horizontally or in the proper or specified place.</rdfs:comment>
    </owl:NamedIndividual>
    


    <!-- http://www.sisostds.org/ontologies/lox#LDAM -->

    <owl:NamedIndividual rdf:about="http://www.sisostds.org/ontologies/lox#LDAM">
        <rdfs:comment>Documentation: 		
						The subjective categorisation of the physical effect of an ACTION on buildings, infrastructure and/or equipment by a reporting ORGANISATION.	
					; Appinfo DisplayValue as &quot;Light damage&quot;</rdfs:comment>
    </owl:NamedIndividual>
    


    <!-- http://www.sisostds.org/ontologies/lox#LEAGR -->

    <owl:NamedIndividual rdf:about="http://www.sisostds.org/ontologies/lox#LEAGR">
        <rdf:type rdf:resource="http://www.sisostds.org/ontologies/C2SIM#TaskActionCode"/>
        <rdfs:comment>Leaguer: To adopt a defended formation as a temporary defensive measure in areas of low or moderate risk of combat (usually applied</rdfs:comment>
    </owl:NamedIndividual>
    


    <!-- http://www.sisostds.org/ontologies/lox#LGTRST -->

    <owl:NamedIndividual rdf:about="http://www.sisostds.org/ontologies/lox#LGTRST">
        <rdfs:comment>Documentation: 		
						The ACTION-OBJECTIVE reacted against the ACTION using light physical violence.	
					; Appinfo DisplayValue as &quot;Light resistance&quot;</rdfs:comment>
    </owl:NamedIndividual>
    


    <!-- http://www.sisostds.org/ontologies/lox#LIFT -->

    <owl:NamedIndividual rdf:about="http://www.sisostds.org/ontologies/lox#LIFT">
        <rdf:type rdf:resource="http://www.sisostds.org/ontologies/C2SIM#TaskActionCode"/>
        <rdfs:comment>Lift: To transport assets using non-organic means, by sea, land or air.</rdfs:comment>
    </owl:NamedIndividual>
    


    <!-- http://www.sisostds.org/ontologies/lox#LIFTAD -->

    <owl:NamedIndividual rdf:about="http://www.sisostds.org/ontologies/lox#LIFTAD">
        <rdf:type rdf:resource="http://www.sisostds.org/ontologies/C2SIM#TaskActionCode"/>
        <rdfs:comment>Lift, administrative: Airlift normally provided by specifically identifiable aircraft assigned to organisations or commands for internal administration.</rdfs:comment>
    </owl:NamedIndividual>
    


    <!-- http://www.sisostds.org/ontologies/lox#LOCATE -->

    <owl:NamedIndividual rdf:about="http://www.sisostds.org/ontologies/lox#LOCATE">
        <rdf:type rdf:resource="http://www.sisostds.org/ontologies/C2SIM#TaskActionCode"/>
        <rdfs:comment>Documentation: 		
						To establish the position or presence of an object.	
					; Appinfo DisplayValue as &quot;Locate&quot;</rdfs:comment>
        <rdfs:comment>Locate: To establish the position or presence of an object.</rdfs:comment>
    </owl:NamedIndividual>
    


    <!-- http://www.sisostds.org/ontologies/lox#LOST -->

    <owl:NamedIndividual rdf:about="http://www.sisostds.org/ontologies/lox#LOST">
        <rdfs:comment>Documentation: 		
						The object is no longer available for military operations.	
					; Appinfo DisplayValue as &quot;Lost&quot;</rdfs:comment>
    </owl:NamedIndividual>
    


    <!-- http://www.sisostds.org/ontologies/lox#MAINTN -->

    <owl:NamedIndividual rdf:about="http://www.sisostds.org/ontologies/lox#MAINTN">
        <rdf:type rdf:resource="http://www.sisostds.org/ontologies/C2SIM#TaskActionCode"/>
        <rdfs:comment>Maintain: To provide services to keep equipment in condition to carry out its function.</rdfs:comment>
    </owl:NamedIndividual>
    


    <!-- http://www.sisostds.org/ontologies/lox#MAP -->

    <owl:NamedIndividual rdf:about="http://www.sisostds.org/ontologies/lox#MAP">
        <rdf:type rdf:resource="http://www.sisostds.org/ontologies/C2SIM#TaskActionCode"/>
        <rdfs:comment>Map: To create a graphic representation, usually on a plane surface and at an established scale, of natural or artificial features</rdfs:comment>
    </owl:NamedIndividual>
    


    <!-- http://www.sisostds.org/ontologies/lox#MARK -->

    <owl:NamedIndividual rdf:about="http://www.sisostds.org/ontologies/lox#MARK">
        <rdf:type rdf:resource="http://www.sisostds.org/ontologies/C2SIM#TaskActionCode"/>
        <rdfs:comment>Mark: To make visible (by the use of light/IR/laser/arty) an object in order to allow its identification by another object (usually</rdfs:comment>
    </owl:NamedIndividual>
    


    <!-- http://www.sisostds.org/ontologies/lox#MASSFR -->

    <owl:NamedIndividual rdf:about="http://www.sisostds.org/ontologies/lox#MASSFR">
        <rdf:type rdf:resource="http://www.sisostds.org/ontologies/C2SIM#TaskActionCode"/>
        <rdfs:comment>Mass forces: To concentrate large quantities of military equipment and personnel.</rdfs:comment>
    </owl:NamedIndividual>
    


    <!-- http://www.sisostds.org/ontologies/lox#MCM11 -->

    <owl:NamedIndividual rdf:about="http://www.sisostds.org/ontologies/lox#MCM11">
        <rdf:type rdf:resource="http://www.sisostds.org/ontologies/C2SIM#TaskActionCode"/>
        <rdfs:comment>MCM operation stage 11: Mine Counter Measure operation stage 11.</rdfs:comment>
    </owl:NamedIndividual>
    


    <!-- http://www.sisostds.org/ontologies/lox#MCM12 -->

    <owl:NamedIndividual rdf:about="http://www.sisostds.org/ontologies/lox#MCM12">
        <rdf:type rdf:resource="http://www.sisostds.org/ontologies/C2SIM#TaskActionCode"/>
        <rdfs:comment>MCM operation stage 12: Mine Counter Measure operation stage 12.</rdfs:comment>
    </owl:NamedIndividual>
    


    <!-- http://www.sisostds.org/ontologies/lox#MCM13 -->

    <owl:NamedIndividual rdf:about="http://www.sisostds.org/ontologies/lox#MCM13">
        <rdf:type rdf:resource="http://www.sisostds.org/ontologies/C2SIM#TaskActionCode"/>
        <rdfs:comment>MCM operation stage 13: Mine Counter Measure operation stage 13.</rdfs:comment>
    </owl:NamedIndividual>
    


    <!-- http://www.sisostds.org/ontologies/lox#MCM14 -->

    <owl:NamedIndividual rdf:about="http://www.sisostds.org/ontologies/lox#MCM14">
        <rdf:type rdf:resource="http://www.sisostds.org/ontologies/C2SIM#TaskActionCode"/>
        <rdfs:comment>MCM operation stage 14: Mine Counter Measure operation stage 14.</rdfs:comment>
    </owl:NamedIndividual>
    


    <!-- http://www.sisostds.org/ontologies/lox#MCM31 -->

    <owl:NamedIndividual rdf:about="http://www.sisostds.org/ontologies/lox#MCM31">
        <rdf:type rdf:resource="http://www.sisostds.org/ontologies/C2SIM#TaskActionCode"/>
        <rdfs:comment>MCM operation stage 31: Mine Counter Measure operation stage 31.</rdfs:comment>
    </owl:NamedIndividual>
    


    <!-- http://www.sisostds.org/ontologies/lox#MCM32 -->

    <owl:NamedIndividual rdf:about="http://www.sisostds.org/ontologies/lox#MCM32">
        <rdf:type rdf:resource="http://www.sisostds.org/ontologies/C2SIM#TaskActionCode"/>
        <rdfs:comment>MCM operation stage 32: Mine Counter Measure operation stage 32.</rdfs:comment>
    </owl:NamedIndividual>
    


    <!-- http://www.sisostds.org/ontologies/lox#MCM33 -->

    <owl:NamedIndividual rdf:about="http://www.sisostds.org/ontologies/lox#MCM33">
        <rdf:type rdf:resource="http://www.sisostds.org/ontologies/C2SIM#TaskActionCode"/>
        <rdfs:comment>MCM operation stage 33: Mine Counter Measure operation stage 33.</rdfs:comment>
    </owl:NamedIndividual>
    


    <!-- http://www.sisostds.org/ontologies/lox#MCM34 -->

    <owl:NamedIndividual rdf:about="http://www.sisostds.org/ontologies/lox#MCM34">
        <rdf:type rdf:resource="http://www.sisostds.org/ontologies/C2SIM#TaskActionCode"/>
        <rdfs:comment>MCM operation stage 34: Mine Counter Measure operation stage 34.</rdfs:comment>
    </owl:NamedIndividual>
    


    <!-- http://www.sisostds.org/ontologies/lox#MCM35 -->

    <owl:NamedIndividual rdf:about="http://www.sisostds.org/ontologies/lox#MCM35">
        <rdf:type rdf:resource="http://www.sisostds.org/ontologies/C2SIM#TaskActionCode"/>
        <rdfs:comment>MCM operation stage 35: Mine Counter Measure operation stage 35.</rdfs:comment>
    </owl:NamedIndividual>
    


    <!-- http://www.sisostds.org/ontologies/lox#MCM36 -->

    <owl:NamedIndividual rdf:about="http://www.sisostds.org/ontologies/lox#MCM36">
        <rdf:type rdf:resource="http://www.sisostds.org/ontologies/C2SIM#TaskActionCode"/>
        <rdfs:comment>MCM operation stage 36: Mine Counter Measure operation stage 36.</rdfs:comment>
    </owl:NamedIndividual>
    


    <!-- http://www.sisostds.org/ontologies/lox#MCM37 -->

    <owl:NamedIndividual rdf:about="http://www.sisostds.org/ontologies/lox#MCM37">
        <rdf:type rdf:resource="http://www.sisostds.org/ontologies/C2SIM#TaskActionCode"/>
        <rdfs:comment>MCM operation stage 37: Mine Counter Measure operation stage 37.</rdfs:comment>
    </owl:NamedIndividual>
    


    <!-- http://www.sisostds.org/ontologies/lox#MCM38 -->

    <owl:NamedIndividual rdf:about="http://www.sisostds.org/ontologies/lox#MCM38">
        <rdf:type rdf:resource="http://www.sisostds.org/ontologies/C2SIM#TaskActionCode"/>
        <rdfs:comment>MCM operation stage 38: Mine Counter Measure operation stage 38.</rdfs:comment>
    </owl:NamedIndividual>
    


    <!-- http://www.sisostds.org/ontologies/lox#MCM39 -->

    <owl:NamedIndividual rdf:about="http://www.sisostds.org/ontologies/lox#MCM39">
        <rdf:type rdf:resource="http://www.sisostds.org/ontologies/C2SIM#TaskActionCode"/>
        <rdfs:comment>MCM operation stage 39: Mine Counter Measure operation stage 39.</rdfs:comment>
    </owl:NamedIndividual>
    


    <!-- http://www.sisostds.org/ontologies/lox#MCM41 -->

    <owl:NamedIndividual rdf:about="http://www.sisostds.org/ontologies/lox#MCM41">
        <rdf:type rdf:resource="http://www.sisostds.org/ontologies/C2SIM#TaskActionCode"/>
        <rdfs:comment>MCM operation stage 41: Mine Counter Measure operation stage 41.</rdfs:comment>
    </owl:NamedIndividual>
    


    <!-- http://www.sisostds.org/ontologies/lox#MCM42 -->

    <owl:NamedIndividual rdf:about="http://www.sisostds.org/ontologies/lox#MCM42">
        <rdf:type rdf:resource="http://www.sisostds.org/ontologies/C2SIM#TaskActionCode"/>
        <rdfs:comment>MCM operation stage 42: Mine Counter Measure operation stage 42.</rdfs:comment>
    </owl:NamedIndividual>
    


    <!-- http://www.sisostds.org/ontologies/lox#MCM43 -->

    <owl:NamedIndividual rdf:about="http://www.sisostds.org/ontologies/lox#MCM43">
        <rdf:type rdf:resource="http://www.sisostds.org/ontologies/C2SIM#TaskActionCode"/>
        <rdfs:comment>MCM operation stage 43: Mine Counter Measure operation stage 43.</rdfs:comment>
    </owl:NamedIndividual>
    


    <!-- http://www.sisostds.org/ontologies/lox#MCM44 -->

    <owl:NamedIndividual rdf:about="http://www.sisostds.org/ontologies/lox#MCM44">
        <rdf:type rdf:resource="http://www.sisostds.org/ontologies/C2SIM#TaskActionCode"/>
        <rdfs:comment>MCM operation stage 44: Mine Counter Measure operation stage 44.</rdfs:comment>
    </owl:NamedIndividual>
    


    <!-- http://www.sisostds.org/ontologies/lox#MCM45 -->

    <owl:NamedIndividual rdf:about="http://www.sisostds.org/ontologies/lox#MCM45">
        <rdf:type rdf:resource="http://www.sisostds.org/ontologies/C2SIM#TaskActionCode"/>
        <rdfs:comment>MCM operation stage 45: Mine Counter Measure operation stage 45.</rdfs:comment>
    </owl:NamedIndividual>
    


    <!-- http://www.sisostds.org/ontologies/lox#MCM46 -->

    <owl:NamedIndividual rdf:about="http://www.sisostds.org/ontologies/lox#MCM46">
        <rdf:type rdf:resource="http://www.sisostds.org/ontologies/C2SIM#TaskActionCode"/>
        <rdfs:comment>MCM operation stage 46: Mine Counter Measure operation stage 46.</rdfs:comment>
    </owl:NamedIndividual>
    


    <!-- http://www.sisostds.org/ontologies/lox#MCM47 -->

    <owl:NamedIndividual rdf:about="http://www.sisostds.org/ontologies/lox#MCM47">
        <rdf:type rdf:resource="http://www.sisostds.org/ontologies/C2SIM#TaskActionCode"/>
        <rdfs:comment>MCM operation stage 47: Mine Counter Measure operation stage 47.</rdfs:comment>
    </owl:NamedIndividual>
    


    <!-- http://www.sisostds.org/ontologies/lox#MCM48 -->

    <owl:NamedIndividual rdf:about="http://www.sisostds.org/ontologies/lox#MCM48">
        <rdf:type rdf:resource="http://www.sisostds.org/ontologies/C2SIM#TaskActionCode"/>
        <rdfs:comment>MCM operation stage 48: Mine Counter Measure operation stage 48.</rdfs:comment>
    </owl:NamedIndividual>
    


    <!-- http://www.sisostds.org/ontologies/lox#MCM50 -->

    <owl:NamedIndividual rdf:about="http://www.sisostds.org/ontologies/lox#MCM50">
        <rdf:type rdf:resource="http://www.sisostds.org/ontologies/C2SIM#TaskActionCode"/>
        <rdfs:comment>MCM operation stage 50: Mine Counter Measure operation stage 50.</rdfs:comment>
    </owl:NamedIndividual>
    


    <!-- http://www.sisostds.org/ontologies/lox#MCM51 -->

    <owl:NamedIndividual rdf:about="http://www.sisostds.org/ontologies/lox#MCM51">
        <rdf:type rdf:resource="http://www.sisostds.org/ontologies/C2SIM#TaskActionCode"/>
        <rdfs:comment>MCM operation stage 51: Mine Counter Measure operation stage 51.</rdfs:comment>
    </owl:NamedIndividual>
    


    <!-- http://www.sisostds.org/ontologies/lox#MCM52 -->

    <owl:NamedIndividual rdf:about="http://www.sisostds.org/ontologies/lox#MCM52">
        <rdf:type rdf:resource="http://www.sisostds.org/ontologies/C2SIM#TaskActionCode"/>
        <rdfs:comment>MCM operation stage 52: Mine Counter Measure operation stage 52.</rdfs:comment>
    </owl:NamedIndividual>
    


    <!-- http://www.sisostds.org/ontologies/lox#MCM53 -->

    <owl:NamedIndividual rdf:about="http://www.sisostds.org/ontologies/lox#MCM53">
        <rdf:type rdf:resource="http://www.sisostds.org/ontologies/C2SIM#TaskActionCode"/>
        <rdfs:comment>MCM operation stage 53: Mine Counter Measure operation stage 53.</rdfs:comment>
    </owl:NamedIndividual>
    


    <!-- http://www.sisostds.org/ontologies/lox#MCM54 -->

    <owl:NamedIndividual rdf:about="http://www.sisostds.org/ontologies/lox#MCM54">
        <rdf:type rdf:resource="http://www.sisostds.org/ontologies/C2SIM#TaskActionCode"/>
        <rdfs:comment>MCM operation stage 54: Mine Counter Measure operation stage 54.</rdfs:comment>
    </owl:NamedIndividual>
    


    <!-- http://www.sisostds.org/ontologies/lox#MCM55 -->

    <owl:NamedIndividual rdf:about="http://www.sisostds.org/ontologies/lox#MCM55">
        <rdf:type rdf:resource="http://www.sisostds.org/ontologies/C2SIM#TaskActionCode"/>
        <rdfs:comment>MCM operation stage 55: Mine Counter Measure operation stage 55.</rdfs:comment>
    </owl:NamedIndividual>
    


    <!-- http://www.sisostds.org/ontologies/lox#MCM56 -->

    <owl:NamedIndividual rdf:about="http://www.sisostds.org/ontologies/lox#MCM56">
        <rdf:type rdf:resource="http://www.sisostds.org/ontologies/C2SIM#TaskActionCode"/>
        <rdfs:comment>MCM operation stage 56: Mine Counter Measure operation stage 56.</rdfs:comment>
    </owl:NamedIndividual>
    


    <!-- http://www.sisostds.org/ontologies/lox#MCM57 -->

    <owl:NamedIndividual rdf:about="http://www.sisostds.org/ontologies/lox#MCM57">
        <rdf:type rdf:resource="http://www.sisostds.org/ontologies/C2SIM#TaskActionCode"/>
        <rdfs:comment>MCM operation stage 57: Mine Counter Measure operation stage 57.</rdfs:comment>
    </owl:NamedIndividual>
    


    <!-- http://www.sisostds.org/ontologies/lox#MCM58A -->

    <owl:NamedIndividual rdf:about="http://www.sisostds.org/ontologies/lox#MCM58A">
        <rdf:type rdf:resource="http://www.sisostds.org/ontologies/C2SIM#TaskActionCode"/>
        <rdfs:comment>MCM operation stage 58A: Mine Counter Measure operation stage 58A.</rdfs:comment>
    </owl:NamedIndividual>
    


    <!-- http://www.sisostds.org/ontologies/lox#MCM58B -->

    <owl:NamedIndividual rdf:about="http://www.sisostds.org/ontologies/lox#MCM58B">
        <rdf:type rdf:resource="http://www.sisostds.org/ontologies/C2SIM#TaskActionCode"/>
        <rdfs:comment>MCM operation stage 58B: Mine Counter Measure operation stage 58B.</rdfs:comment>
    </owl:NamedIndividual>
    


    <!-- http://www.sisostds.org/ontologies/lox#MCM58C -->

    <owl:NamedIndividual rdf:about="http://www.sisostds.org/ontologies/lox#MCM58C">
        <rdf:type rdf:resource="http://www.sisostds.org/ontologies/C2SIM#TaskActionCode"/>
        <rdfs:comment>MCM operation stage 58C: Mine Counter Measure operation stage 58C.</rdfs:comment>
    </owl:NamedIndividual>
    


    <!-- http://www.sisostds.org/ontologies/lox#MCM59 -->

    <owl:NamedIndividual rdf:about="http://www.sisostds.org/ontologies/lox#MCM59">
        <rdf:type rdf:resource="http://www.sisostds.org/ontologies/C2SIM#TaskActionCode"/>
        <rdfs:comment>MCM operation stage 59: Mine Counter Measure operation stage 59.</rdfs:comment>
    </owl:NamedIndividual>
    


    <!-- http://www.sisostds.org/ontologies/lox#MCM61 -->

    <owl:NamedIndividual rdf:about="http://www.sisostds.org/ontologies/lox#MCM61">
        <rdf:type rdf:resource="http://www.sisostds.org/ontologies/C2SIM#TaskActionCode"/>
        <rdfs:comment>MCM operation stage 61: Mine Counter Measure operation stage 61.</rdfs:comment>
    </owl:NamedIndividual>
    


    <!-- http://www.sisostds.org/ontologies/lox#MCM62 -->

    <owl:NamedIndividual rdf:about="http://www.sisostds.org/ontologies/lox#MCM62">
        <rdf:type rdf:resource="http://www.sisostds.org/ontologies/C2SIM#TaskActionCode"/>
        <rdfs:comment>MCM operation stage 62: Mine Counter Measure operation stage 62.</rdfs:comment>
    </owl:NamedIndividual>
    


    <!-- http://www.sisostds.org/ontologies/lox#MCM63 -->

    <owl:NamedIndividual rdf:about="http://www.sisostds.org/ontologies/lox#MCM63">
        <rdf:type rdf:resource="http://www.sisostds.org/ontologies/C2SIM#TaskActionCode"/>
        <rdfs:comment>MCM operation stage 63: Mine Counter Measure operation stage 63.</rdfs:comment>
    </owl:NamedIndividual>
    


    <!-- http://www.sisostds.org/ontologies/lox#MCM71 -->

    <owl:NamedIndividual rdf:about="http://www.sisostds.org/ontologies/lox#MCM71">
        <rdf:type rdf:resource="http://www.sisostds.org/ontologies/C2SIM#TaskActionCode"/>
        <rdfs:comment>MCM operation stage 71: Mine Counter Measure operation stage 71.</rdfs:comment>
    </owl:NamedIndividual>
    


    <!-- http://www.sisostds.org/ontologies/lox#MCM72 -->

    <owl:NamedIndividual rdf:about="http://www.sisostds.org/ontologies/lox#MCM72">
        <rdf:type rdf:resource="http://www.sisostds.org/ontologies/C2SIM#TaskActionCode"/>
        <rdfs:comment>MCM operation stage 72: Mine Counter Measure operation stage 72.</rdfs:comment>
    </owl:NamedIndividual>
    


    <!-- http://www.sisostds.org/ontologies/lox#MCM73 -->

    <owl:NamedIndividual rdf:about="http://www.sisostds.org/ontologies/lox#MCM73">
        <rdf:type rdf:resource="http://www.sisostds.org/ontologies/C2SIM#TaskActionCode"/>
        <rdfs:comment>MCM operation stage 73: Mine Counter Measure operation stage 73.</rdfs:comment>
    </owl:NamedIndividual>
    


    <!-- http://www.sisostds.org/ontologies/lox#MCM74 -->

    <owl:NamedIndividual rdf:about="http://www.sisostds.org/ontologies/lox#MCM74">
        <rdf:type rdf:resource="http://www.sisostds.org/ontologies/C2SIM#TaskActionCode"/>
        <rdfs:comment>MCM operation stage 74: Mine Counter Measure operation stage 74.</rdfs:comment>
    </owl:NamedIndividual>
    


    <!-- http://www.sisostds.org/ontologies/lox#MCM75 -->

    <owl:NamedIndividual rdf:about="http://www.sisostds.org/ontologies/lox#MCM75">
        <rdf:type rdf:resource="http://www.sisostds.org/ontologies/C2SIM#TaskActionCode"/>
        <rdfs:comment>MCM operation stage 75: Mine Counter Measure operation stage 75.</rdfs:comment>
    </owl:NamedIndividual>
    


    <!-- http://www.sisostds.org/ontologies/lox#MCM81 -->

    <owl:NamedIndividual rdf:about="http://www.sisostds.org/ontologies/lox#MCM81">
        <rdf:type rdf:resource="http://www.sisostds.org/ontologies/C2SIM#TaskActionCode"/>
        <rdfs:comment>MCM operation stage 81: Mine Counter Measure operation stage 81.</rdfs:comment>
    </owl:NamedIndividual>
    


    <!-- http://www.sisostds.org/ontologies/lox#MCM82 -->

    <owl:NamedIndividual rdf:about="http://www.sisostds.org/ontologies/lox#MCM82">
        <rdf:type rdf:resource="http://www.sisostds.org/ontologies/C2SIM#TaskActionCode"/>
        <rdfs:comment>MCM operation stage 82: Mine Counter Measure operation stage 82.</rdfs:comment>
    </owl:NamedIndividual>
    


    <!-- http://www.sisostds.org/ontologies/lox#MCM83 -->

    <owl:NamedIndividual rdf:about="http://www.sisostds.org/ontologies/lox#MCM83">
        <rdf:type rdf:resource="http://www.sisostds.org/ontologies/C2SIM#TaskActionCode"/>
        <rdfs:comment>MCM operation stage 83: Mine Counter Measure operation stage 83.</rdfs:comment>
    </owl:NamedIndividual>
    


    <!-- http://www.sisostds.org/ontologies/lox#MCM84 -->

    <owl:NamedIndividual rdf:about="http://www.sisostds.org/ontologies/lox#MCM84">
        <rdf:type rdf:resource="http://www.sisostds.org/ontologies/C2SIM#TaskActionCode"/>
        <rdfs:comment>MCM operation stage 84: Mine Counter Measure operation stage 84.</rdfs:comment>
    </owl:NamedIndividual>
    


    <!-- http://www.sisostds.org/ontologies/lox#MCM85 -->

    <owl:NamedIndividual rdf:about="http://www.sisostds.org/ontologies/lox#MCM85">
        <rdf:type rdf:resource="http://www.sisostds.org/ontologies/C2SIM#TaskActionCode"/>
        <rdfs:comment>MCM operation stage 85: Mine Counter Measure operation stage 85.</rdfs:comment>
    </owl:NamedIndividual>
    


    <!-- http://www.sisostds.org/ontologies/lox#MCM86 -->

    <owl:NamedIndividual rdf:about="http://www.sisostds.org/ontologies/lox#MCM86">
        <rdf:type rdf:resource="http://www.sisostds.org/ontologies/C2SIM#TaskActionCode"/>
        <rdfs:comment>MCM operation stage 86: Mine Counter Measure operation stage 86.</rdfs:comment>
    </owl:NamedIndividual>
    


    <!-- http://www.sisostds.org/ontologies/lox#MCM87 -->

    <owl:NamedIndividual rdf:about="http://www.sisostds.org/ontologies/lox#MCM87">
        <rdf:type rdf:resource="http://www.sisostds.org/ontologies/C2SIM#TaskActionCode"/>
        <rdfs:comment>MCM operation stage 87: Mine Counter Measure operation stage 87.</rdfs:comment>
    </owl:NamedIndividual>
    


    <!-- http://www.sisostds.org/ontologies/lox#MCM88 -->

    <owl:NamedIndividual rdf:about="http://www.sisostds.org/ontologies/lox#MCM88">
        <rdf:type rdf:resource="http://www.sisostds.org/ontologies/C2SIM#TaskActionCode"/>
        <rdfs:comment>MCM operation stage 88: Mine Counter Measure operation stage 88.</rdfs:comment>
    </owl:NamedIndividual>
    


    <!-- http://www.sisostds.org/ontologies/lox#MCM89 -->

    <owl:NamedIndividual rdf:about="http://www.sisostds.org/ontologies/lox#MCM89">
        <rdf:type rdf:resource="http://www.sisostds.org/ontologies/C2SIM#TaskActionCode"/>
        <rdfs:comment>MCM operation stage 89: Mine Counter Measure operation stage 89.</rdfs:comment>
    </owl:NamedIndividual>
    


    <!-- http://www.sisostds.org/ontologies/lox#MCM91 -->

    <owl:NamedIndividual rdf:about="http://www.sisostds.org/ontologies/lox#MCM91">
        <rdf:type rdf:resource="http://www.sisostds.org/ontologies/C2SIM#TaskActionCode"/>
        <rdfs:comment>MCM operation stage 91: Mine Counter Measure operation stage 91.</rdfs:comment>
    </owl:NamedIndividual>
    


    <!-- http://www.sisostds.org/ontologies/lox#MCM92 -->

    <owl:NamedIndividual rdf:about="http://www.sisostds.org/ontologies/lox#MCM92">
        <rdf:type rdf:resource="http://www.sisostds.org/ontologies/C2SIM#TaskActionCode"/>
        <rdfs:comment>MCM operation stage 92: Mine Counter Measure operation stage 92.</rdfs:comment>
    </owl:NamedIndividual>
    


    <!-- http://www.sisostds.org/ontologies/lox#MCM93 -->

    <owl:NamedIndividual rdf:about="http://www.sisostds.org/ontologies/lox#MCM93">
        <rdf:type rdf:resource="http://www.sisostds.org/ontologies/C2SIM#TaskActionCode"/>
        <rdfs:comment>MCM operation stage 93: Mine Counter Measure operation stage 93.</rdfs:comment>
    </owl:NamedIndividual>
    


    <!-- http://www.sisostds.org/ontologies/lox#MCMATT -->

    <owl:NamedIndividual rdf:about="http://www.sisostds.org/ontologies/lox#MCMATT">
        <rdf:type rdf:resource="http://www.sisostds.org/ontologies/C2SIM#TaskActionCode"/>
        <rdfs:comment>MCM, attrition: To conduct continuous application of Mine Countermeasures (MCM) to keep the risk from mines to all vessels as low as possible.</rdfs:comment>
    </owl:NamedIndividual>
    


    <!-- http://www.sisostds.org/ontologies/lox#MCMCHK -->

    <owl:NamedIndividual rdf:about="http://www.sisostds.org/ontologies/lox#MCMCHK">
        <rdf:type rdf:resource="http://www.sisostds.org/ontologies/C2SIM#TaskActionCode"/>
        <rdfs:comment>MCM, check: To conduct a Mine Countermeasures (MCM) operation to check that as far as possible no maritime mines are left after the previous</rdfs:comment>
    </owl:NamedIndividual>
    


    <!-- http://www.sisostds.org/ontologies/lox#MCMEXP -->

    <owl:NamedIndividual rdf:about="http://www.sisostds.org/ontologies/lox#MCMEXP">
        <rdf:type rdf:resource="http://www.sisostds.org/ontologies/C2SIM#TaskActionCode"/>
        <rdfs:comment>MCM, exploratory: To conduct a Mine Countermeasures (MCM) operation in which a sample of the route or area is subjected to MCM procedures to</rdfs:comment>
    </owl:NamedIndividual>
    


    <!-- http://www.sisostds.org/ontologies/lox#MCMLDT -->

    <owl:NamedIndividual rdf:about="http://www.sisostds.org/ontologies/lox#MCMLDT">
        <rdf:type rdf:resource="http://www.sisostds.org/ontologies/C2SIM#TaskActionCode"/>
        <rdfs:comment>MCM, lead through: To assist traffic in the transit of parts of a mined area which have previously been subject to Mine Countermeasures (MCM)</rdfs:comment>
    </owl:NamedIndividual>
    


    <!-- http://www.sisostds.org/ontologies/lox#MCMLMC -->

    <owl:NamedIndividual rdf:about="http://www.sisostds.org/ontologies/lox#MCMLMC">
        <rdf:type rdf:resource="http://www.sisostds.org/ontologies/C2SIM#TaskActionCode"/>
        <rdfs:comment>MCM, limited clearing: To clear particular types of mines from an area, channel or route.</rdfs:comment>
    </owl:NamedIndividual>
    


    <!-- http://www.sisostds.org/ontologies/lox#MCMPRE -->

    <owl:NamedIndividual rdf:about="http://www.sisostds.org/ontologies/lox#MCMPRE">
        <rdf:type rdf:resource="http://www.sisostds.org/ontologies/C2SIM#TaskActionCode"/>
        <rdfs:comment>MCM, precursor: To carry out operations in an area or channel using relatively safe methods and techniques in order to reduce the risk to</rdfs:comment>
    </owl:NamedIndividual>
    


    <!-- http://www.sisostds.org/ontologies/lox#MCMSA -->

    <owl:NamedIndividual rdf:about="http://www.sisostds.org/ontologies/lox#MCMSA">
        <rdf:type rdf:resource="http://www.sisostds.org/ontologies/C2SIM#TaskActionCode"/>
        <rdfs:comment>MCM-SLS-ALPHA: Mine Countermeasures Operation Standard Letter Suffixes ALPHA.</rdfs:comment>
    </owl:NamedIndividual>
    


    <!-- http://www.sisostds.org/ontologies/lox#MCMSAA -->

    <owl:NamedIndividual rdf:about="http://www.sisostds.org/ontologies/lox#MCMSAA">
        <rdf:type rdf:resource="http://www.sisostds.org/ontologies/C2SIM#TaskActionCode"/>
        <rdfs:comment>MCM-SLS-ALPHA-ALPHA: Mine Countermeasures Operation Standard Letter Suffixes ALPHA-ALPHA.</rdfs:comment>
    </owl:NamedIndividual>
    


    <!-- http://www.sisostds.org/ontologies/lox#MCMSAC -->

    <owl:NamedIndividual rdf:about="http://www.sisostds.org/ontologies/lox#MCMSAC">
        <rdf:type rdf:resource="http://www.sisostds.org/ontologies/C2SIM#TaskActionCode"/>
        <rdfs:comment>MCM-SLS-ALPHA-CHARLIE: Mine Countermeasures Operation Standard Letter Suffixes ALPHA-CHARLIE.</rdfs:comment>
    </owl:NamedIndividual>
    


    <!-- http://www.sisostds.org/ontologies/lox#MCMSAD -->

    <owl:NamedIndividual rdf:about="http://www.sisostds.org/ontologies/lox#MCMSAD">
        <rdf:type rdf:resource="http://www.sisostds.org/ontologies/C2SIM#TaskActionCode"/>
        <rdfs:comment>MCM-SLS-ALPHA-DELTA: Mine Countermeasures Operation Standard Letter Suffixes ALPHA-DELTA.</rdfs:comment>
    </owl:NamedIndividual>
    


    <!-- http://www.sisostds.org/ontologies/lox#MCMSAG -->

    <owl:NamedIndividual rdf:about="http://www.sisostds.org/ontologies/lox#MCMSAG">
        <rdf:type rdf:resource="http://www.sisostds.org/ontologies/C2SIM#TaskActionCode"/>
        <rdfs:comment>MCM-SLS-ALPHA-GOLF: Mine Countermeasures Operation Standard Letter Suffixes ALPHA-GOLF.</rdfs:comment>
    </owl:NamedIndividual>
    


    <!-- http://www.sisostds.org/ontologies/lox#MCMSAH -->

    <owl:NamedIndividual rdf:about="http://www.sisostds.org/ontologies/lox#MCMSAH">
        <rdf:type rdf:resource="http://www.sisostds.org/ontologies/C2SIM#TaskActionCode"/>
        <rdfs:comment>MCM-SLS-ALPHA-HOTEL: Mine Countermeasures Operation Standard Letter Suffixes ALPHA-HOTEL.</rdfs:comment>
    </owl:NamedIndividual>
    


    <!-- http://www.sisostds.org/ontologies/lox#MCMSAM -->

    <owl:NamedIndividual rdf:about="http://www.sisostds.org/ontologies/lox#MCMSAM">
        <rdf:type rdf:resource="http://www.sisostds.org/ontologies/C2SIM#TaskActionCode"/>
        <rdfs:comment>MCM-SLS-ALPHA-MIKE: Mine Countermeasures Operation Standard Letter Suffixes ALPHA-MIKE.</rdfs:comment>
    </owl:NamedIndividual>
    


    <!-- http://www.sisostds.org/ontologies/lox#MCMSAZ -->

    <owl:NamedIndividual rdf:about="http://www.sisostds.org/ontologies/lox#MCMSAZ">
        <rdf:type rdf:resource="http://www.sisostds.org/ontologies/C2SIM#TaskActionCode"/>
        <rdfs:comment>MCM-SLS-ALPHA-ZULU: Mine Countermeasures Operation Standard Letter Suffixes ALPHA-ZULU.</rdfs:comment>
    </owl:NamedIndividual>
    


    <!-- http://www.sisostds.org/ontologies/lox#MCMSB -->

    <owl:NamedIndividual rdf:about="http://www.sisostds.org/ontologies/lox#MCMSB">
        <rdf:type rdf:resource="http://www.sisostds.org/ontologies/C2SIM#TaskActionCode"/>
        <rdfs:comment>MCM-SLS-BRAVO: Mine Countermeasures Operation Standard Letter Suffixes BRAVO.</rdfs:comment>
    </owl:NamedIndividual>
    


    <!-- http://www.sisostds.org/ontologies/lox#MCMSBZ -->

    <owl:NamedIndividual rdf:about="http://www.sisostds.org/ontologies/lox#MCMSBZ">
        <rdf:type rdf:resource="http://www.sisostds.org/ontologies/C2SIM#TaskActionCode"/>
        <rdfs:comment>MCM-SLS-BRAVO-ZULU: Mine Countermeasures Operation Standard Letter Suffixes BRAVO-ZULU.</rdfs:comment>
    </owl:NamedIndividual>
    


    <!-- http://www.sisostds.org/ontologies/lox#MCMSC -->

    <owl:NamedIndividual rdf:about="http://www.sisostds.org/ontologies/lox#MCMSC">
        <rdf:type rdf:resource="http://www.sisostds.org/ontologies/C2SIM#TaskActionCode"/>
        <rdfs:comment>MCM-SLS-CHARLIE: Mine Countermeasures Operation Standard Letter Suffixes CHARLIE.</rdfs:comment>
    </owl:NamedIndividual>
    


    <!-- http://www.sisostds.org/ontologies/lox#MCMSCA -->

    <owl:NamedIndividual rdf:about="http://www.sisostds.org/ontologies/lox#MCMSCA">
        <rdf:type rdf:resource="http://www.sisostds.org/ontologies/C2SIM#TaskActionCode"/>
        <rdfs:comment>MCM-SLS-CHARLIE-ALPHA: Mine Countermeasures Operation Standard Letter Suffixes CHARLIE-ALPHA.</rdfs:comment>
    </owl:NamedIndividual>
    


    <!-- http://www.sisostds.org/ontologies/lox#MCMSCC -->

    <owl:NamedIndividual rdf:about="http://www.sisostds.org/ontologies/lox#MCMSCC">
        <rdf:type rdf:resource="http://www.sisostds.org/ontologies/C2SIM#TaskActionCode"/>
        <rdfs:comment>MCM-SLS-CHARLIE-CHARLIE: Mine Countermeasures Operation Standard Letter Suffixes CHARLIE-CHARLIE.</rdfs:comment>
    </owl:NamedIndividual>
    


    <!-- http://www.sisostds.org/ontologies/lox#MCMSCD -->

    <owl:NamedIndividual rdf:about="http://www.sisostds.org/ontologies/lox#MCMSCD">
        <rdf:type rdf:resource="http://www.sisostds.org/ontologies/C2SIM#TaskActionCode"/>
        <rdfs:comment>MCM-SLS-CHARLIE-DELTA: Mine Countermeasures Operation Standard Letter Suffixes CHARLIE-DELTA.</rdfs:comment>
    </owl:NamedIndividual>
    


    <!-- http://www.sisostds.org/ontologies/lox#MCMSCG -->

    <owl:NamedIndividual rdf:about="http://www.sisostds.org/ontologies/lox#MCMSCG">
        <rdf:type rdf:resource="http://www.sisostds.org/ontologies/C2SIM#TaskActionCode"/>
        <rdfs:comment>MCM-SLS-CHARLIE-GOLF: Mine Countermeasures Operation Standard Letter Suffixes CHARLIE-GOLF.</rdfs:comment>
    </owl:NamedIndividual>
    


    <!-- http://www.sisostds.org/ontologies/lox#MCMSCH -->

    <owl:NamedIndividual rdf:about="http://www.sisostds.org/ontologies/lox#MCMSCH">
        <rdf:type rdf:resource="http://www.sisostds.org/ontologies/C2SIM#TaskActionCode"/>
        <rdfs:comment>MCM-SLS-CHARLIE-HOTEL: Mine Countermeasures Operation Standard Letter Suffixes CHARLIE-HOTEL.</rdfs:comment>
    </owl:NamedIndividual>
    


    <!-- http://www.sisostds.org/ontologies/lox#MCMSCM -->

    <owl:NamedIndividual rdf:about="http://www.sisostds.org/ontologies/lox#MCMSCM">
        <rdf:type rdf:resource="http://www.sisostds.org/ontologies/C2SIM#TaskActionCode"/>
        <rdfs:comment>MCM-SLS-CHARLIE-MIKE: Mine Countermeasures Operation Standard Letter Suffixes CHARLIE-MIKE.</rdfs:comment>
    </owl:NamedIndividual>
    


    <!-- http://www.sisostds.org/ontologies/lox#MCMSCZ -->

    <owl:NamedIndividual rdf:about="http://www.sisostds.org/ontologies/lox#MCMSCZ">
        <rdf:type rdf:resource="http://www.sisostds.org/ontologies/C2SIM#TaskActionCode"/>
        <rdfs:comment>MCM-SLS-CHARLIE-ZULU: Mine Countermeasures Operation Standard Letter Suffixes CHARLIE-ZULU.</rdfs:comment>
    </owl:NamedIndividual>
    


    <!-- http://www.sisostds.org/ontologies/lox#MCMSE -->

    <owl:NamedIndividual rdf:about="http://www.sisostds.org/ontologies/lox#MCMSE">
        <rdf:type rdf:resource="http://www.sisostds.org/ontologies/C2SIM#TaskActionCode"/>
        <rdfs:comment>MCM-SLS-ECHO: Mine Countermeasures Operation Standard Letter Suffixes ECHO.</rdfs:comment>
    </owl:NamedIndividual>
    


    <!-- http://www.sisostds.org/ontologies/lox#MCMSEA -->

    <owl:NamedIndividual rdf:about="http://www.sisostds.org/ontologies/lox#MCMSEA">
        <rdf:type rdf:resource="http://www.sisostds.org/ontologies/C2SIM#TaskActionCode"/>
        <rdfs:comment>MCM-SLS-ECHO-ALPHA: Mine Countermeasures Operation Standard Letter Suffixes ECHO-ALPHA.</rdfs:comment>
    </owl:NamedIndividual>
    


    <!-- http://www.sisostds.org/ontologies/lox#MCMSEC -->

    <owl:NamedIndividual rdf:about="http://www.sisostds.org/ontologies/lox#MCMSEC">
        <rdf:type rdf:resource="http://www.sisostds.org/ontologies/C2SIM#TaskActionCode"/>
        <rdfs:comment>MCM-SLS-ECHO-CHARLIE: Mine Countermeasures Operation Standard Letter Suffixes ECHO-CHARLIE.</rdfs:comment>
    </owl:NamedIndividual>
    


    <!-- http://www.sisostds.org/ontologies/lox#MCMSED -->

    <owl:NamedIndividual rdf:about="http://www.sisostds.org/ontologies/lox#MCMSED">
        <rdf:type rdf:resource="http://www.sisostds.org/ontologies/C2SIM#TaskActionCode"/>
        <rdfs:comment>MCM-SLS-ECHO-DELTA: Mine Countermeasures Operation Standard Letter Suffixes ECHO-DELTA.</rdfs:comment>
    </owl:NamedIndividual>
    


    <!-- http://www.sisostds.org/ontologies/lox#MCMSEG -->

    <owl:NamedIndividual rdf:about="http://www.sisostds.org/ontologies/lox#MCMSEG">
        <rdf:type rdf:resource="http://www.sisostds.org/ontologies/C2SIM#TaskActionCode"/>
        <rdfs:comment>MCM-SLS-ECHO-GOLF: Mine Countermeasures Operation Standard Letter Suffixes ECHO-GOLF.</rdfs:comment>
    </owl:NamedIndividual>
    


    <!-- http://www.sisostds.org/ontologies/lox#MCMSEH -->

    <owl:NamedIndividual rdf:about="http://www.sisostds.org/ontologies/lox#MCMSEH">
        <rdf:type rdf:resource="http://www.sisostds.org/ontologies/C2SIM#TaskActionCode"/>
        <rdfs:comment>MCM-SLS-ECHO-HOTEL: Mine Countermeasures Operation Standard Letter Suffixes ECHO-HOTEL.</rdfs:comment>
    </owl:NamedIndividual>
    


    <!-- http://www.sisostds.org/ontologies/lox#MCMSEM -->

    <owl:NamedIndividual rdf:about="http://www.sisostds.org/ontologies/lox#MCMSEM">
        <rdf:type rdf:resource="http://www.sisostds.org/ontologies/C2SIM#TaskActionCode"/>
        <rdfs:comment>MCM-SLS-ECHO-MIKE: Mine Countermeasures Operation Standard Letter Suffixes ECHO-MIKE.</rdfs:comment>
    </owl:NamedIndividual>
    


    <!-- http://www.sisostds.org/ontologies/lox#MCMSEZ -->

    <owl:NamedIndividual rdf:about="http://www.sisostds.org/ontologies/lox#MCMSEZ">
        <rdf:type rdf:resource="http://www.sisostds.org/ontologies/C2SIM#TaskActionCode"/>
        <rdfs:comment>MCM-SLS-ECHO-ZULU: Mine Countermeasures Operation Standard Letter Suffixes ECHO-ZULU.</rdfs:comment>
    </owl:NamedIndividual>
    


    <!-- http://www.sisostds.org/ontologies/lox#MCMSL -->

    <owl:NamedIndividual rdf:about="http://www.sisostds.org/ontologies/lox#MCMSL">
        <rdf:type rdf:resource="http://www.sisostds.org/ontologies/C2SIM#TaskActionCode"/>
        <rdfs:comment>MCM-SLS-LIMA: Mine Countermeasures Operation Standard Letter Suffixes LIMA.</rdfs:comment>
    </owl:NamedIndividual>
    


    <!-- http://www.sisostds.org/ontologies/lox#MCMSLA -->

    <owl:NamedIndividual rdf:about="http://www.sisostds.org/ontologies/lox#MCMSLA">
        <rdf:type rdf:resource="http://www.sisostds.org/ontologies/C2SIM#TaskActionCode"/>
        <rdfs:comment>MCM-SLS-LIMA-ALPHA: Mine Countermeasures Operation Standard Letter Suffixes LIMA-ALPHA.</rdfs:comment>
    </owl:NamedIndividual>
    


    <!-- http://www.sisostds.org/ontologies/lox#MCMSLH -->

    <owl:NamedIndividual rdf:about="http://www.sisostds.org/ontologies/lox#MCMSLH">
        <rdf:type rdf:resource="http://www.sisostds.org/ontologies/C2SIM#TaskActionCode"/>
        <rdfs:comment>MCM-SLS-LIMA-HOTEL: Mine Countermeasures Operation Standard Letter Suffixes LIMA-HOTEL.</rdfs:comment>
    </owl:NamedIndividual>
    


    <!-- http://www.sisostds.org/ontologies/lox#MCMSLM -->

    <owl:NamedIndividual rdf:about="http://www.sisostds.org/ontologies/lox#MCMSLM">
        <rdf:type rdf:resource="http://www.sisostds.org/ontologies/C2SIM#TaskActionCode"/>
        <rdfs:comment>MCM-SLS-LIMA-MIKE: Mine Countermeasures Operation Standard Letter Suffixes LIMA-MIKE.</rdfs:comment>
    </owl:NamedIndividual>
    


    <!-- http://www.sisostds.org/ontologies/lox#MCMSLZ -->

    <owl:NamedIndividual rdf:about="http://www.sisostds.org/ontologies/lox#MCMSLZ">
        <rdf:type rdf:resource="http://www.sisostds.org/ontologies/C2SIM#TaskActionCode"/>
        <rdfs:comment>MCM-SLS-LIMA-ZULU: Mine Countermeasures Operation Standard Letter Suffixes LIMA-ZULU.</rdfs:comment>
    </owl:NamedIndividual>
    


    <!-- http://www.sisostds.org/ontologies/lox#MCMSP -->

    <owl:NamedIndividual rdf:about="http://www.sisostds.org/ontologies/lox#MCMSP">
        <rdf:type rdf:resource="http://www.sisostds.org/ontologies/C2SIM#TaskActionCode"/>
        <rdfs:comment>MCM-SLS-PAPA: Mine Countermeasures Operation Standard Letter Suffixes PAPA.</rdfs:comment>
    </owl:NamedIndividual>
    


    <!-- http://www.sisostds.org/ontologies/lox#MCMSPA -->

    <owl:NamedIndividual rdf:about="http://www.sisostds.org/ontologies/lox#MCMSPA">
        <rdf:type rdf:resource="http://www.sisostds.org/ontologies/C2SIM#TaskActionCode"/>
        <rdfs:comment>MCM-SLS-PAPA-ALPHA: Mine Countermeasures Operation Standard Letter Suffixes PAPA-ALPHA.</rdfs:comment>
    </owl:NamedIndividual>
    


    <!-- http://www.sisostds.org/ontologies/lox#MCMSPC -->

    <owl:NamedIndividual rdf:about="http://www.sisostds.org/ontologies/lox#MCMSPC">
        <rdf:type rdf:resource="http://www.sisostds.org/ontologies/C2SIM#TaskActionCode"/>
        <rdfs:comment>MCM-SLS-PAPA-CHARLIE: Mine Countermeasures Operation Standard Letter Suffixes PAPA-CHARLIE.</rdfs:comment>
    </owl:NamedIndividual>
    


    <!-- http://www.sisostds.org/ontologies/lox#MCMSPG -->

    <owl:NamedIndividual rdf:about="http://www.sisostds.org/ontologies/lox#MCMSPG">
        <rdf:type rdf:resource="http://www.sisostds.org/ontologies/C2SIM#TaskActionCode"/>
        <rdfs:comment>MCM-SLS-PAPA-GOLF: Mine Countermeasures Operation Standard Letter Suffixes PAPA-GOLF.</rdfs:comment>
    </owl:NamedIndividual>
    


    <!-- http://www.sisostds.org/ontologies/lox#MCMSPH -->

    <owl:NamedIndividual rdf:about="http://www.sisostds.org/ontologies/lox#MCMSPH">
        <rdf:type rdf:resource="http://www.sisostds.org/ontologies/C2SIM#TaskActionCode"/>
        <rdfs:comment>MCM-SLS-PAPA-HOTEL: Mine Countermeasures Operation Standard Letter Suffixes PAPA-HOTEL.</rdfs:comment>
    </owl:NamedIndividual>
    


    <!-- http://www.sisostds.org/ontologies/lox#MCMSPM -->

    <owl:NamedIndividual rdf:about="http://www.sisostds.org/ontologies/lox#MCMSPM">
        <rdf:type rdf:resource="http://www.sisostds.org/ontologies/C2SIM#TaskActionCode"/>
        <rdfs:comment>MCM-SLS-PAPA-MIKE: Mine Countermeasures Operation Standard Letter Suffixes PAPA-MIKE.</rdfs:comment>
    </owl:NamedIndividual>
    


    <!-- http://www.sisostds.org/ontologies/lox#MCMSPZ -->

    <owl:NamedIndividual rdf:about="http://www.sisostds.org/ontologies/lox#MCMSPZ">
        <rdf:type rdf:resource="http://www.sisostds.org/ontologies/C2SIM#TaskActionCode"/>
        <rdfs:comment>MCM-SLS-PAPA-ZULU: Mine Countermeasures Operation Standard Letter Suffixes PAPA-ZULU.</rdfs:comment>
    </owl:NamedIndividual>
    


    <!-- http://www.sisostds.org/ontologies/lox#MCMSR -->

    <owl:NamedIndividual rdf:about="http://www.sisostds.org/ontologies/lox#MCMSR">
        <rdf:type rdf:resource="http://www.sisostds.org/ontologies/C2SIM#TaskActionCode"/>
        <rdfs:comment>MCM-SLS-ROMEO: Mine Countermeasures Operation Standard Letter Suffixes ROMEO.</rdfs:comment>
    </owl:NamedIndividual>
    


    <!-- http://www.sisostds.org/ontologies/lox#MCMSRD -->

    <owl:NamedIndividual rdf:about="http://www.sisostds.org/ontologies/lox#MCMSRD">
        <rdf:type rdf:resource="http://www.sisostds.org/ontologies/C2SIM#TaskActionCode"/>
        <rdfs:comment>MCM-SLS-ROMEO-DELTA: Mine Countermeasures Operation Standard Letter Suffixes ROMEO-DELTA.</rdfs:comment>
    </owl:NamedIndividual>
    


    <!-- http://www.sisostds.org/ontologies/lox#MCMSRH -->

    <owl:NamedIndividual rdf:about="http://www.sisostds.org/ontologies/lox#MCMSRH">
        <rdf:type rdf:resource="http://www.sisostds.org/ontologies/C2SIM#TaskActionCode"/>
        <rdfs:comment>MCM-SLS-ROMEO-HOTEL: Mine Countermeasures Operation Standard Letter Suffixes ROMEO-HOTEL.</rdfs:comment>
    </owl:NamedIndividual>
    


    <!-- http://www.sisostds.org/ontologies/lox#MCMSRV -->

    <owl:NamedIndividual rdf:about="http://www.sisostds.org/ontologies/lox#MCMSRV">
        <rdf:type rdf:resource="http://www.sisostds.org/ontologies/C2SIM#TaskActionCode"/>
        <rdfs:comment>MCM, survey: To collect environmental data which may be used in support of current and future mine countermeasures (MCM) operations.</rdfs:comment>
    </owl:NamedIndividual>
    


    <!-- http://www.sisostds.org/ontologies/lox#MCMSS -->

    <owl:NamedIndividual rdf:about="http://www.sisostds.org/ontologies/lox#MCMSS">
        <rdf:type rdf:resource="http://www.sisostds.org/ontologies/C2SIM#TaskActionCode"/>
        <rdfs:comment>MCM-SLS-SIERRA: Mine Countermeasures Operation Standard Letter Suffixes SIERRA.</rdfs:comment>
    </owl:NamedIndividual>
    


    <!-- http://www.sisostds.org/ontologies/lox#MCMSSA -->

    <owl:NamedIndividual rdf:about="http://www.sisostds.org/ontologies/lox#MCMSSA">
        <rdf:type rdf:resource="http://www.sisostds.org/ontologies/C2SIM#TaskActionCode"/>
        <rdfs:comment>MCM-SLS-SIERRA-ALPHA: Mine Countermeasures Operation Standard Letter Suffixes SIERRA-ALPHA.</rdfs:comment>
    </owl:NamedIndividual>
    


    <!-- http://www.sisostds.org/ontologies/lox#MCMSSC -->

    <owl:NamedIndividual rdf:about="http://www.sisostds.org/ontologies/lox#MCMSSC">
        <rdf:type rdf:resource="http://www.sisostds.org/ontologies/C2SIM#TaskActionCode"/>
        <rdfs:comment>MCM-SLS-SIERRA-CHARLIE: Mine Countermeasures Operation Standard Letter Suffixes SIERRA-CHARLIE.</rdfs:comment>
    </owl:NamedIndividual>
    


    <!-- http://www.sisostds.org/ontologies/lox#MCMSSD -->

    <owl:NamedIndividual rdf:about="http://www.sisostds.org/ontologies/lox#MCMSSD">
        <rdf:type rdf:resource="http://www.sisostds.org/ontologies/C2SIM#TaskActionCode"/>
        <rdfs:comment>MCM-SLS-SIERRA-DELTA: Mine Countermeasures Operation Standard Letter Suffixes SIERRA-DELTA.</rdfs:comment>
    </owl:NamedIndividual>
    


    <!-- http://www.sisostds.org/ontologies/lox#MCMSSG -->

    <owl:NamedIndividual rdf:about="http://www.sisostds.org/ontologies/lox#MCMSSG">
        <rdf:type rdf:resource="http://www.sisostds.org/ontologies/C2SIM#TaskActionCode"/>
        <rdfs:comment>MCM-SLS-SIERRA-GOLF: Mine Countermeasures Operation Standard Letter Suffixes SIERRA-GOLF.</rdfs:comment>
    </owl:NamedIndividual>
    


    <!-- http://www.sisostds.org/ontologies/lox#MCMSSH -->

    <owl:NamedIndividual rdf:about="http://www.sisostds.org/ontologies/lox#MCMSSH">
        <rdf:type rdf:resource="http://www.sisostds.org/ontologies/C2SIM#TaskActionCode"/>
        <rdfs:comment>MCM-SLS-SIERRA-HOTEL: Mine Countermeasures Operation Standard Letter Suffixes SIERRA-HOTEL.</rdfs:comment>
    </owl:NamedIndividual>
    


    <!-- http://www.sisostds.org/ontologies/lox#MCMSSM -->

    <owl:NamedIndividual rdf:about="http://www.sisostds.org/ontologies/lox#MCMSSM">
        <rdf:type rdf:resource="http://www.sisostds.org/ontologies/C2SIM#TaskActionCode"/>
        <rdfs:comment>MCM-SLS-SIERRA-MIKE: Mine Countermeasures Operation Standard Letter Suffixes SIERRA-MIKE.</rdfs:comment>
    </owl:NamedIndividual>
    


    <!-- http://www.sisostds.org/ontologies/lox#MCMSSZ -->

    <owl:NamedIndividual rdf:about="http://www.sisostds.org/ontologies/lox#MCMSSZ">
        <rdf:type rdf:resource="http://www.sisostds.org/ontologies/C2SIM#TaskActionCode"/>
        <rdfs:comment>MCM-SLS-SIERRA-ZULU: Mine Countermeasures Operation Standard Letter Suffixes SIERRA-ZULU.</rdfs:comment>
    </owl:NamedIndividual>
    


    <!-- http://www.sisostds.org/ontologies/lox#MCMSU -->

    <owl:NamedIndividual rdf:about="http://www.sisostds.org/ontologies/lox#MCMSU">
        <rdf:type rdf:resource="http://www.sisostds.org/ontologies/C2SIM#TaskActionCode"/>
        <rdfs:comment>MCM-SLS-UNIFORM: Mine Countermeasures Operation Standard Letter Suffixes UNIFORM.</rdfs:comment>
    </owl:NamedIndividual>
    


    <!-- http://www.sisostds.org/ontologies/lox#MCMSUH -->

    <owl:NamedIndividual rdf:about="http://www.sisostds.org/ontologies/lox#MCMSUH">
        <rdf:type rdf:resource="http://www.sisostds.org/ontologies/C2SIM#TaskActionCode"/>
        <rdfs:comment>MCM-SLS-UNIFORM-HOTEL: Mine Countermeasures Operation Standard Letter Suffixes UNIFORM-HOTEL.</rdfs:comment>
    </owl:NamedIndividual>
    


    <!-- http://www.sisostds.org/ontologies/lox#MCMSUZ -->

    <owl:NamedIndividual rdf:about="http://www.sisostds.org/ontologies/lox#MCMSUZ">
        <rdf:type rdf:resource="http://www.sisostds.org/ontologies/C2SIM#TaskActionCode"/>
        <rdfs:comment>MCM-SLS-UNIFORM-ZULU: Mine Countermeasures Operation Standard Letter Suffixes UNIFORM-ZULU.</rdfs:comment>
    </owl:NamedIndividual>
    


    <!-- http://www.sisostds.org/ontologies/lox#MCMSV -->

    <owl:NamedIndividual rdf:about="http://www.sisostds.org/ontologies/lox#MCMSV">
        <rdf:type rdf:resource="http://www.sisostds.org/ontologies/C2SIM#TaskActionCode"/>
        <rdfs:comment>MCM-SLS-VICTOR: Mine Countermeasures Operation Standard Letter Suffixes VICTOR.</rdfs:comment>
    </owl:NamedIndividual>
    


    <!-- http://www.sisostds.org/ontologies/lox#MCMSVA -->

    <owl:NamedIndividual rdf:about="http://www.sisostds.org/ontologies/lox#MCMSVA">
        <rdf:type rdf:resource="http://www.sisostds.org/ontologies/C2SIM#TaskActionCode"/>
        <rdfs:comment>MCM-SLS-VICTOR-ALPHA: Mine Countermeasures Operation Standard Letter Suffixes VICTOR-ALPHA.</rdfs:comment>
    </owl:NamedIndividual>
    


    <!-- http://www.sisostds.org/ontologies/lox#MCMSVC -->

    <owl:NamedIndividual rdf:about="http://www.sisostds.org/ontologies/lox#MCMSVC">
        <rdf:type rdf:resource="http://www.sisostds.org/ontologies/C2SIM#TaskActionCode"/>
        <rdfs:comment>MCM-SLS-VICTOR-CHARLIE: Mine Countermeasures Operation Standard Letter Suffixes VICTOR-CHARLIE.</rdfs:comment>
    </owl:NamedIndividual>
    


    <!-- http://www.sisostds.org/ontologies/lox#MCMSVD -->

    <owl:NamedIndividual rdf:about="http://www.sisostds.org/ontologies/lox#MCMSVD">
        <rdf:type rdf:resource="http://www.sisostds.org/ontologies/C2SIM#TaskActionCode"/>
        <rdfs:comment>MCM-SLS-VICTOR-DELTA: Mine Countermeasures Operation Standard Letter Suffixes VICTOR-DELTA.</rdfs:comment>
    </owl:NamedIndividual>
    


    <!-- http://www.sisostds.org/ontologies/lox#MCMSVG -->

    <owl:NamedIndividual rdf:about="http://www.sisostds.org/ontologies/lox#MCMSVG">
        <rdf:type rdf:resource="http://www.sisostds.org/ontologies/C2SIM#TaskActionCode"/>
        <rdfs:comment>MCM-SLS-VICTOR-GOLF: Mine Countermeasures Operation Standard Letter Suffixes VICTOR-GOLF.</rdfs:comment>
    </owl:NamedIndividual>
    


    <!-- http://www.sisostds.org/ontologies/lox#MCMSVH -->

    <owl:NamedIndividual rdf:about="http://www.sisostds.org/ontologies/lox#MCMSVH">
        <rdf:type rdf:resource="http://www.sisostds.org/ontologies/C2SIM#TaskActionCode"/>
        <rdfs:comment>MCM-SLS-VICTOR-HOTEL: Mine Countermeasures Operation Standard Letter Suffixes VICTOR-HOTEL.</rdfs:comment>
    </owl:NamedIndividual>
    


    <!-- http://www.sisostds.org/ontologies/lox#MCMSVM -->

    <owl:NamedIndividual rdf:about="http://www.sisostds.org/ontologies/lox#MCMSVM">
        <rdf:type rdf:resource="http://www.sisostds.org/ontologies/C2SIM#TaskActionCode"/>
        <rdfs:comment>MCM-SLS-VICTOR-MIKE: Mine Countermeasures Operation Standard Letter Suffixes VICTOR-MIKE.</rdfs:comment>
    </owl:NamedIndividual>
    


    <!-- http://www.sisostds.org/ontologies/lox#MCMSVZ -->

    <owl:NamedIndividual rdf:about="http://www.sisostds.org/ontologies/lox#MCMSVZ">
        <rdf:type rdf:resource="http://www.sisostds.org/ontologies/C2SIM#TaskActionCode"/>
        <rdfs:comment>MCM-SLS-VICTOR-ZULU: Mine Countermeasures Operation Standard Letter Suffixes VICTOR-ZULU.</rdfs:comment>
    </owl:NamedIndividual>
    


    <!-- http://www.sisostds.org/ontologies/lox#MCMSW -->

    <owl:NamedIndividual rdf:about="http://www.sisostds.org/ontologies/lox#MCMSW">
        <rdf:type rdf:resource="http://www.sisostds.org/ontologies/C2SIM#TaskActionCode"/>
        <rdfs:comment>MCM-SLS-WHISKEY: Mine Countermeasures Operation Standard Letter Suffixes WHISKEY.</rdfs:comment>
    </owl:NamedIndividual>
    


    <!-- http://www.sisostds.org/ontologies/lox#MCMSWZ -->

    <owl:NamedIndividual rdf:about="http://www.sisostds.org/ontologies/lox#MCMSWZ">
        <rdf:type rdf:resource="http://www.sisostds.org/ontologies/C2SIM#TaskActionCode"/>
        <rdfs:comment>MCM-SLS-WHISKEY-ZULU: Mine Countermeasures Operation Standard Letter Suffixes WHISKEY-ZULU.</rdfs:comment>
    </owl:NamedIndividual>
    


    <!-- http://www.sisostds.org/ontologies/lox#MCMSZZ -->

    <owl:NamedIndividual rdf:about="http://www.sisostds.org/ontologies/lox#MCMSZZ">
        <rdf:type rdf:resource="http://www.sisostds.org/ontologies/C2SIM#TaskActionCode"/>
        <rdfs:comment>MCM-SLS-ZULU-ZULU: Mine Countermeasures Operation Standard Letter Suffixes ZULU-ZULU.</rdfs:comment>
    </owl:NamedIndividual>
    


    <!-- http://www.sisostds.org/ontologies/lox#MCMTML -->

    <owl:NamedIndividual rdf:about="http://www.sisostds.org/ontologies/lox#MCMTML">
        <rdf:type rdf:resource="http://www.sisostds.org/ontologies/C2SIM#TaskActionCode"/>
        <rdfs:comment>MCM, time limited: To conduct a minesweeping and/or minehunting carried out when time available before ships are passed through a mined area,</rdfs:comment>
    </owl:NamedIndividual>
    


    <!-- http://www.sisostds.org/ontologies/lox#MEDEVC -->

    <owl:NamedIndividual rdf:about="http://www.sisostds.org/ontologies/lox#MEDEVC">
        <rdf:type rdf:resource="http://www.sisostds.org/ontologies/C2SIM#TaskActionCode"/>
        <rdfs:comment>Documentation: 		
						To move any person who is wounded, injured or ill to/between medical treatment facilities.	
					; Appinfo DisplayValue as &quot;Medical evacuation&quot;</rdfs:comment>
        <rdfs:comment>Medical evacuation: To move any person who is wounded, injured or ill to/between medical treatment facilities.</rdfs:comment>
    </owl:NamedIndividual>
    


    <!-- http://www.sisostds.org/ontologies/lox#METBAL -->

    <owl:NamedIndividual rdf:about="http://www.sisostds.org/ontologies/lox#METBAL">
        <rdf:type rdf:resource="http://www.sisostds.org/ontologies/C2SIM#TaskActionCode"/>
        <rdfs:comment>Meteorological: To gather meteorological information such as humidity, pressure, and temperature characteristics of Earth&apos;s atmosphere.</rdfs:comment>
    </owl:NamedIndividual>
    


    <!-- http://www.sisostds.org/ontologies/lox#MINCM -->

    <owl:NamedIndividual rdf:about="http://www.sisostds.org/ontologies/lox#MINCM">
        <rdf:type rdf:resource="http://www.sisostds.org/ontologies/C2SIM#TaskActionCode"/>
        <rdfs:comment>Mine countermeasures: To perform mine countermeasures.</rdfs:comment>
    </owl:NamedIndividual>
    


    <!-- http://www.sisostds.org/ontologies/lox#MINEWF -->

    <owl:NamedIndividual rdf:about="http://www.sisostds.org/ontologies/lox#MINEWF">
        <rdf:type rdf:resource="http://www.sisostds.org/ontologies/C2SIM#TaskActionCode"/>
        <rdfs:comment>Mine warfare: To conduct warfare that includes the actions of laying mines and actions taken to counter the threat of an adversary (referred</rdfs:comment>
    </owl:NamedIndividual>
    


    <!-- http://www.sisostds.org/ontologies/lox#MINLAY -->

    <owl:NamedIndividual rdf:about="http://www.sisostds.org/ontologies/lox#MINLAY">
        <rdf:type rdf:resource="http://www.sisostds.org/ontologies/C2SIM#TaskActionCode"/>
        <rdfs:comment>Mine-laying: To emplace or deploy one or more mines.</rdfs:comment>
    </owl:NamedIndividual>
    


    <!-- http://www.sisostds.org/ontologies/lox#MINSWP -->

    <owl:NamedIndividual rdf:about="http://www.sisostds.org/ontologies/lox#MINSWP">
        <rdf:type rdf:resource="http://www.sisostds.org/ontologies/C2SIM#TaskActionCode"/>
        <rdfs:comment>Minesweeping, land: To search for or clear mines using mechanical or explosion gear, which physically removes or destroys the mine, or produces,</rdfs:comment>
    </owl:NamedIndividual>
    


    <!-- http://www.sisostds.org/ontologies/lox#MISSTG -->

    <owl:NamedIndividual rdf:about="http://www.sisostds.org/ontologies/lox#MISSTG">
        <rdf:type rdf:resource="http://www.sisostds.org/ontologies/C2SIM#TaskActionCode"/>
        <rdfs:comment>Mission staging: To perform the assembly of aircraft for the completion of a mission or other activity.</rdfs:comment>
    </owl:NamedIndividual>
    


    <!-- http://www.sisostds.org/ontologies/lox#MKIL -->

    <owl:NamedIndividual rdf:about="http://www.sisostds.org/ontologies/lox#MKIL">
        <rdfs:comment>Documentation: 		
						The rendering of a vehicle as being temporarily or permanently incapable of tactical movement.	
					; Appinfo DisplayValue as &quot;Mobility kill (M-kill)&quot;</rdfs:comment>
    </owl:NamedIndividual>
    


    <!-- http://www.sisostds.org/ontologies/lox#MNHUNT -->

    <owl:NamedIndividual rdf:about="http://www.sisostds.org/ontologies/lox#MNHUNT">
        <rdf:type rdf:resource="http://www.sisostds.org/ontologies/C2SIM#TaskActionCode"/>
        <rdfs:comment>Mine hunting, maritime: To locate and dispose of individual mines by means of detection equipment with the employment of ships, airborne equipment</rdfs:comment>
    </owl:NamedIndividual>
    


    <!-- http://www.sisostds.org/ontologies/lox#MNSWMA -->

    <owl:NamedIndividual rdf:about="http://www.sisostds.org/ontologies/lox#MNSWMA">
        <rdf:type rdf:resource="http://www.sisostds.org/ontologies/C2SIM#TaskActionCode"/>
        <rdfs:comment>Minesweeping, maritime: To search for or counter mines by maritime minesweepers using mechanical or explosive gear, which physically removes or destroys</rdfs:comment>
    </owl:NamedIndividual>
    


    <!-- http://www.sisostds.org/ontologies/lox#MNTAIR -->

    <owl:NamedIndividual rdf:about="http://www.sisostds.org/ontologies/lox#MNTAIR">
        <rdf:type rdf:resource="http://www.sisostds.org/ontologies/C2SIM#TaskActionCode"/>
        <rdfs:comment>Maintain on call airborne alert: To keep combat equipped aircraft airborne and prepared for immediate action. Airborne alert is designed to reduce reaction</rdfs:comment>
    </owl:NamedIndividual>
    


    <!-- http://www.sisostds.org/ontologies/lox#MNTGRD -->

    <owl:NamedIndividual rdf:about="http://www.sisostds.org/ontologies/lox#MNTGRD">
        <rdf:type rdf:resource="http://www.sisostds.org/ontologies/C2SIM#TaskActionCode"/>
        <rdfs:comment>Maintain on call ground alert: To keep aircraft on the ground/runway/deck fully serviced and armed, with combat crews in readiness to take off within a specified</rdfs:comment>
    </owl:NamedIndividual>
    


    <!-- http://www.sisostds.org/ontologies/lox#MODDAM -->

    <owl:NamedIndividual rdf:about="http://www.sisostds.org/ontologies/lox#MODDAM">
        <rdfs:comment>Documentation: 		
						The subjective categorisation of the physical effect of an ACTION on buildings, infrastructure and/or equipment by a reporting ORGANISATION.	
					; Appinfo DisplayValue as &quot;Moderate damage&quot;</rdfs:comment>
    </owl:NamedIndividual>
    


    <!-- http://www.sisostds.org/ontologies/lox#MOPUP -->

    <owl:NamedIndividual rdf:about="http://www.sisostds.org/ontologies/lox#MOPUP">
        <rdf:type rdf:resource="http://www.sisostds.org/ontologies/C2SIM#TaskActionCode"/>
        <rdfs:comment>Documentation: 		
						To liquidate the remnants of enemy resistance in an area that has been surrounded or isolated, or through which other units have passed without eliminating all active resistance.	
					; Appinfo DisplayValue as &quot;Mop up&quot;</rdfs:comment>
        <rdfs:comment>Mop up: To liquidate the remnants of enemy resistance in an area that has been surrounded or isolated, or through which other units</rdfs:comment>
    </owl:NamedIndividual>
    


    <!-- http://www.sisostds.org/ontologies/lox#MOVE -->

    <owl:NamedIndividual rdf:about="http://www.sisostds.org/ontologies/lox#MOVE">
        <rdf:type rdf:resource="http://www.sisostds.org/ontologies/C2SIM#TaskActionCode"/>
        <rdfs:comment>Documentation: 		
						To change position from one location to another.	
					; Appinfo DisplayValue as &quot;Move&quot;</rdfs:comment>
        <rdfs:comment>Move: To change position from one location to another.</rdfs:comment>
    </owl:NamedIndividual>
    


    <!-- http://www.sisostds.org/ontologies/lox#MPA -->

    <owl:NamedIndividual rdf:about="http://www.sisostds.org/ontologies/lox#MPA">
        <rdf:type rdf:resource="http://www.sisostds.org/ontologies/C2SIM#TaskActionCode"/>
        <rdfs:comment>Patrol, maritime: To fly over an area, monitor and, where necessary, destroy hostile aircraft, as well as protect friendly shipping in the vicinity</rdfs:comment>
    </owl:NamedIndividual>
    


    <!-- http://www.sisostds.org/ontologies/lox#MRITOP -->

    <owl:NamedIndividual rdf:about="http://www.sisostds.org/ontologies/lox#MRITOP">
        <rdf:type rdf:resource="http://www.sisostds.org/ontologies/C2SIM#TaskActionCode"/>
        <rdfs:comment>Maritime interdiction operations: To conduct an operation that encompasses seaborne enforcement measures to interdict the movement of certain types of designated</rdfs:comment>
    </owl:NamedIndividual>
    


    <!-- http://www.sisostds.org/ontologies/lox#NACLSP -->

    <owl:NamedIndividual rdf:about="http://www.sisostds.org/ontologies/lox#NACLSP">
        <rdf:type rdf:resource="http://www.sisostds.org/ontologies/C2SIM#TaskActionCode"/>
        <rdfs:comment>Naval control of shipping: Control exercised by naval authorities of movement, routing, reporting, convoy organisation and tactical diversion of Allied</rdfs:comment>
    </owl:NamedIndividual>
    


    <!-- http://www.sisostds.org/ontologies/lox#NBCAS -->

    <owl:NamedIndividual rdf:about="http://www.sisostds.org/ontologies/lox#NBCAS">
        <rdfs:comment>Documentation: 		
						A person who is not a battle casualty, but who is lost to his organisation by reason of disease or injury, including persons dying from disease or injury, or by reason of being missing where the absence does not appear to be voluntary or due to enemy action or to being interned.	
					; Appinfo DisplayValue as &quot;Non-battle casualty&quot;</rdfs:comment>
    </owl:NamedIndividual>
    


    <!-- http://www.sisostds.org/ontologies/lox#NKN -->

    <owl:NamedIndividual rdf:about="http://www.sisostds.org/ontologies/lox#NKN">
        <rdfs:comment>Documentation: 		
						It is not possible to determine which value is most applicable.	
					; Appinfo DisplayValue as &quot;Not known&quot;</rdfs:comment>
    </owl:NamedIndividual>
    


    <!-- http://www.sisostds.org/ontologies/lox#NORSTN -->

    <owl:NamedIndividual rdf:about="http://www.sisostds.org/ontologies/lox#NORSTN">
        <rdfs:comment>Documentation: 		
						The ACTION-OBJECTIVE did not react against the ACTION.	
					; Appinfo DisplayValue as &quot;No resistance&quot;</rdfs:comment>
    </owl:NamedIndividual>
    


    <!-- http://www.sisostds.org/ontologies/lox#NOS -->

    <owl:NamedIndividual rdf:about="http://www.sisostds.org/ontologies/lox#NOS">
        <rdfs:comment>Documentation: 		
						The appropriate value is not in the set of specified values.	
					; Appinfo DisplayValue as &quot;Not otherwise specified&quot;</rdfs:comment>
    </owl:NamedIndividual>
    


    <!-- http://www.sisostds.org/ontologies/lox#NTRCHM -->

    <owl:NamedIndividual rdf:about="http://www.sisostds.org/ontologies/lox#NTRCHM">
        <rdf:type rdf:resource="http://www.sisostds.org/ontologies/C2SIM#TaskActionCode"/>
        <rdfs:comment>Neutralize, chemical: To make safe or non-toxic an object contaminated with a chemical agent.</rdfs:comment>
    </owl:NamedIndividual>
    


    <!-- http://www.sisostds.org/ontologies/lox#NTRCOM -->

    <owl:NamedIndividual rdf:about="http://www.sisostds.org/ontologies/lox#NTRCOM">
        <rdf:type rdf:resource="http://www.sisostds.org/ontologies/C2SIM#TaskActionCode"/>
        <rdfs:comment>Neutralize, combat: To render ineffective or unusable in military operations.</rdfs:comment>
    </owl:NamedIndividual>
    


    <!-- http://www.sisostds.org/ontologies/lox#NTREXP -->

    <owl:NamedIndividual rdf:about="http://www.sisostds.org/ontologies/lox#NTREXP">
        <rdf:type rdf:resource="http://www.sisostds.org/ontologies/C2SIM#TaskActionCode"/>
        <rdfs:comment>Neutralize, explosive: To render bombs, mines, missiles and booby traps into a safe state.</rdfs:comment>
    </owl:NamedIndividual>
    


    <!-- http://www.sisostds.org/ontologies/lox#NUCSMP -->

    <owl:NamedIndividual rdf:about="http://www.sisostds.org/ontologies/lox#NUCSMP">
        <rdf:type rdf:resource="http://www.sisostds.org/ontologies/C2SIM#TaskActionCode"/>
        <rdfs:comment>Nuclear sampling: To collect samples for testing for nuclear hazards.</rdfs:comment>
    </owl:NamedIndividual>
    


    <!-- http://www.sisostds.org/ontologies/lox#NUTRLD -->

    <owl:NamedIndividual rdf:about="http://www.sisostds.org/ontologies/lox#NUTRLD">
        <rdfs:comment>Documentation: 		
						The rendering of the ACTION objective temporarily ineffective by the infliction of significant casualties (norm for indirect fire is 10 percent).	
					; Appinfo DisplayValue as &quot;Neutralized&quot;</rdfs:comment>
    </owl:NamedIndividual>
    


    <!-- http://www.sisostds.org/ontologies/lox#NVLPLF -->

    <owl:NamedIndividual rdf:about="http://www.sisostds.org/ontologies/lox#NVLPLF">
        <rdf:type rdf:resource="http://www.sisostds.org/ontologies/C2SIM#TaskActionCode"/>
        <rdfs:comment>Naval platform flight operations: To launch or recover aircraft by a naval platform.</rdfs:comment>
    </owl:NamedIndividual>
    


    <!-- http://www.sisostds.org/ontologies/lox#OBSCUR -->

    <owl:NamedIndividual rdf:about="http://www.sisostds.org/ontologies/lox#OBSCUR">
        <rdf:type rdf:resource="http://www.sisostds.org/ontologies/C2SIM#TaskActionCode"/>
        <rdfs:comment>Documentation: 		
						To cover something by a smoke screen.	
					; Appinfo DisplayValue as &quot;Obscure&quot;</rdfs:comment>
        <rdfs:comment>Obscure: To cover something by a smoke screen.</rdfs:comment>
    </owl:NamedIndividual>
    


    <!-- http://www.sisostds.org/ontologies/lox#OBSRV -->

    <owl:NamedIndividual rdf:about="http://www.sisostds.org/ontologies/lox#OBSRV">
        <rdf:type rdf:resource="http://www.sisostds.org/ontologies/C2SIM#TaskActionCode"/>
        <rdfs:comment>Documentation: 		
						To provide continuous view, and the potential for reports on the activity of an ACTION-OBJECTIVE.	
					; Appinfo DisplayValue as &quot;Observe&quot;</rdfs:comment>
        <rdfs:comment>Observe: To provide continuous view, and the potential for reports on the activity of an ACTION-OBJECTIVE.</rdfs:comment>
    </owl:NamedIndividual>
    


    <!-- http://www.sisostds.org/ontologies/lox#OCCUPY -->

    <owl:NamedIndividual rdf:about="http://www.sisostds.org/ontologies/lox#OCCUPY">
        <rdf:type rdf:resource="http://www.sisostds.org/ontologies/C2SIM#TaskActionCode"/>
        <rdfs:comment>Documentation: 		
						To move onto an objective, key terrain, or other manmade or natural terrain area without opposition and control that entire area.	
					; Appinfo DisplayValue as &quot;Occupy&quot;</rdfs:comment>
        <rdfs:comment>Occupy: To move onto an objective, key terrain, or other manmade or natural terrain area without opposition and control that entire</rdfs:comment>
    </owl:NamedIndividual>
    


    <!-- http://www.sisostds.org/ontologies/lox#OFFAIR -->

    <owl:NamedIndividual rdf:about="http://www.sisostds.org/ontologies/lox#OFFAIR">
        <rdf:type rdf:resource="http://www.sisostds.org/ontologies/C2SIM#TaskActionCode"/>
        <rdfs:comment>Offensive air support: To provide support by the air forces on land or sea in offensive operations.</rdfs:comment>
    </owl:NamedIndividual>
    


    <!-- http://www.sisostds.org/ontologies/lox#OFFCNA -->

    <owl:NamedIndividual rdf:about="http://www.sisostds.org/ontologies/lox#OFFCNA">
        <rdf:type rdf:resource="http://www.sisostds.org/ontologies/C2SIM#TaskActionCode"/>
        <rdfs:comment>Offensive counter air: To conduct an operation to destroy, disrupt or limit enemy air power as close to its source as possible.</rdfs:comment>
    </owl:NamedIndividual>
    


    <!-- http://www.sisostds.org/ontologies/lox#ORGCNF -->

    <owl:NamedIndividual rdf:about="http://www.sisostds.org/ontologies/lox#ORGCNF">
        <rdf:type rdf:resource="http://www.sisostds.org/ontologies/C2SIM#TaskActionCode"/>
        <rdfs:comment>Organise conference: To organise a meeting for discussion, esp. a regular one held by an association or organisation.</rdfs:comment>
    </owl:NamedIndividual>
    


    <!-- http://www.sisostds.org/ontologies/lox#ORGMED -->

    <owl:NamedIndividual rdf:about="http://www.sisostds.org/ontologies/lox#ORGMED">
        <rdf:type rdf:resource="http://www.sisostds.org/ontologies/C2SIM#TaskActionCode"/>
        <rdfs:comment>Organise media interview: To organise a conversation between a reporter etc. and a person of public interest, used as a basis of a broadcast or publication.</rdfs:comment>
    </owl:NamedIndividual>
    


    <!-- http://www.sisostds.org/ontologies/lox#ORGRCR -->

    <owl:NamedIndividual rdf:about="http://www.sisostds.org/ontologies/lox#ORGRCR">
        <rdf:type rdf:resource="http://www.sisostds.org/ontologies/C2SIM#TaskActionCode"/>
        <rdfs:comment>Organise recreational activities: To organise a refreshing or entertaining activity.</rdfs:comment>
    </owl:NamedIndividual>
    


    <!-- http://www.sisostds.org/ontologies/lox#ORGSCL -->

    <owl:NamedIndividual rdf:about="http://www.sisostds.org/ontologies/lox#ORGSCL">
        <rdf:type rdf:resource="http://www.sisostds.org/ontologies/C2SIM#TaskActionCode"/>
        <rdfs:comment>Organise social events: To organise any social gathering, esp. one organised by a club or congregation.</rdfs:comment>
    </owl:NamedIndividual>
    


    <!-- http://www.sisostds.org/ontologies/lox#ORGSPT -->

    <owl:NamedIndividual rdf:about="http://www.sisostds.org/ontologies/lox#ORGSPT">
        <rdf:type rdf:resource="http://www.sisostds.org/ontologies/C2SIM#TaskActionCode"/>
        <rdfs:comment>Organise sporting events: To organise any game or competitive activity, esp. an outdoor one involving physical exertion.</rdfs:comment>
    </owl:NamedIndividual>
    


    <!-- http://www.sisostds.org/ontologies/lox#OneTaskComplete -->

    <owl:NamedIndividual rdf:about="http://www.sisostds.org/ontologies/lox#OneTaskComplete">
        <rdf:type rdf:resource="http://www.sisostds.org/ontologies/lox#PlanPhaseCompletionCondition"/>
    </owl:NamedIndividual>
    


    <!-- http://www.sisostds.org/ontologies/lox#OtherOrderReceived -->

    <owl:NamedIndividual rdf:about="http://www.sisostds.org/ontologies/lox#OtherOrderReceived">
        <rdf:type rdf:resource="http://www.sisostds.org/ontologies/lox#PlanPhaseCompletionCondition"/>
    </owl:NamedIndividual>
    


    <!-- http://www.sisostds.org/ontologies/lox#PATROL -->

    <owl:NamedIndividual rdf:about="http://www.sisostds.org/ontologies/lox#PATROL">
        <rdf:type rdf:resource="http://www.sisostds.org/ontologies/C2SIM#TaskActionCode"/>
        <rdfs:comment>Documentation: 		
						To gather information or to carry out a destructive, harassing, mopping-up, or security mission.	
					; Appinfo DisplayValue as &quot;Patrol&quot;</rdfs:comment>
        <rdfs:comment>Patrol: To gather information or to carry out a destructive, harassing, mopping-up, or security mission.</rdfs:comment>
    </owl:NamedIndividual>
    


    <!-- http://www.sisostds.org/ontologies/lox#PENTRT -->

    <owl:NamedIndividual rdf:about="http://www.sisostds.org/ontologies/lox#PENTRT">
        <rdf:type rdf:resource="http://www.sisostds.org/ontologies/C2SIM#TaskActionCode"/>
        <rdfs:comment>Documentation: 		
						To break through the enemy&apos;s defence or to disrupt the enemy&apos;s defensive systems.	
					; Appinfo DisplayValue as &quot;Penetrate&quot;</rdfs:comment>
        <rdfs:comment>Penetrate: To break through the enemy&apos;s defence or to disrupt the enemy&apos;s defensive systems.</rdfs:comment>
    </owl:NamedIndividual>
    


    <!-- http://www.sisostds.org/ontologies/lox#PHOTO -->

    <owl:NamedIndividual rdf:about="http://www.sisostds.org/ontologies/lox#PHOTO">
        <rdf:type rdf:resource="http://www.sisostds.org/ontologies/C2SIM#TaskActionCode"/>
        <rdfs:comment>Photo mapping: To collect a series of photographs from which it is possible to create maps.</rdfs:comment>
    </owl:NamedIndividual>
    


    <!-- http://www.sisostds.org/ontologies/lox#PLAN -->

    <owl:NamedIndividual rdf:about="http://www.sisostds.org/ontologies/lox#PLAN">
        <rdf:type rdf:resource="http://www.sisostds.org/ontologies/C2SIM#TaskActionCode"/>
        <rdfs:comment>Documentation: 		
						To create a detailed formulation of a programme of action.	
					; Appinfo DisplayValue as &quot;Plan&quot;</rdfs:comment>
        <rdfs:comment>Plan: To create a detailed formulation of a programme of action.</rdfs:comment>
    </owl:NamedIndividual>
    


    <!-- http://www.sisostds.org/ontologies/lox#PREFIR -->

    <owl:NamedIndividual rdf:about="http://www.sisostds.org/ontologies/lox#PREFIR">
        <rdf:type rdf:resource="http://www.sisostds.org/ontologies/C2SIM#TaskActionCode"/>
        <rdfs:comment>Documentation: 		
						To deliver fire on a target preparatory to an assault.	
					; Appinfo DisplayValue as &quot;Preparatory fire&quot;</rdfs:comment>
        <rdfs:comment>Preparatory fire: To deliver fire on a target preparatory to an assault.</rdfs:comment>
    </owl:NamedIndividual>
    


    <!-- http://www.sisostds.org/ontologies/lox#PREPR -->

    <owl:NamedIndividual rdf:about="http://www.sisostds.org/ontologies/lox#PREPR">
        <rdf:type rdf:resource="http://www.sisostds.org/ontologies/C2SIM#TaskActionCode"/>
        <rdfs:comment>Prepare: To establish certain conditions.</rdfs:comment>
    </owl:NamedIndividual>
    


    <!-- http://www.sisostds.org/ontologies/lox#PROCUR -->

    <owl:NamedIndividual rdf:about="http://www.sisostds.org/ontologies/lox#PROCUR">
        <rdf:type rdf:resource="http://www.sisostds.org/ontologies/C2SIM#TaskActionCode"/>
        <rdfs:comment>Procure: To buy whatever is needed to fulfil a certain action.</rdfs:comment>
    </owl:NamedIndividual>
    


    <!-- http://www.sisostds.org/ontologies/lox#PROTEL -->

    <owl:NamedIndividual rdf:about="http://www.sisostds.org/ontologies/lox#PROTEL">
        <rdf:type rdf:resource="http://www.sisostds.org/ontologies/C2SIM#TaskActionCode"/>
        <rdfs:comment>Protection, electronic: That division of electronic warfare involving actions taken to ensure effective friendly use of the electromagnetic spectrum</rdfs:comment>
    </owl:NamedIndividual>
    


    <!-- http://www.sisostds.org/ontologies/lox#PRVACC -->

    <owl:NamedIndividual rdf:about="http://www.sisostds.org/ontologies/lox#PRVACC">
        <rdf:type rdf:resource="http://www.sisostds.org/ontologies/C2SIM#TaskActionCode"/>
        <rdfs:comment>Provide accommodation: To provide room for receiving people, esp. a place to live or lodgings.</rdfs:comment>
    </owl:NamedIndividual>
    


    <!-- http://www.sisostds.org/ontologies/lox#PRVAGR -->

    <owl:NamedIndividual rdf:about="http://www.sisostds.org/ontologies/lox#PRVAGR">
        <rdf:type rdf:resource="http://www.sisostds.org/ontologies/C2SIM#TaskActionCode"/>
        <rdfs:comment>Provide agricultural support: To provide advice or supplies for cultivating the soil and rearing animals.</rdfs:comment>
    </owl:NamedIndividual>
    


    <!-- http://www.sisostds.org/ontologies/lox#PRVBDD -->

    <owl:NamedIndividual rdf:about="http://www.sisostds.org/ontologies/lox#PRVBDD">
        <rdf:type rdf:resource="http://www.sisostds.org/ontologies/C2SIM#TaskActionCode"/>
        <rdfs:comment>Provide bedding: To provide (1) sleeping accommodation or (2) mattress and bedclothes.</rdfs:comment>
    </owl:NamedIndividual>
    


    <!-- http://www.sisostds.org/ontologies/lox#PRVCMP -->

    <owl:NamedIndividual rdf:about="http://www.sisostds.org/ontologies/lox#PRVCMP">
        <rdf:type rdf:resource="http://www.sisostds.org/ontologies/C2SIM#TaskActionCode"/>
        <rdfs:comment>Provide camps: To provide temporary accommodation of various kinds, usually consisting of huts or tents, for detainees, homeless persons,</rdfs:comment>
    </owl:NamedIndividual>
    


    <!-- http://www.sisostds.org/ontologies/lox#PRVCNS -->

    <owl:NamedIndividual rdf:about="http://www.sisostds.org/ontologies/lox#PRVCNS">
        <rdf:type rdf:resource="http://www.sisostds.org/ontologies/C2SIM#TaskActionCode"/>
        <rdfs:comment>Provide construction services: To provide labour and materiel for construction of facilities.</rdfs:comment>
    </owl:NamedIndividual>
    


    <!-- http://www.sisostds.org/ontologies/lox#PRVEDU -->

    <owl:NamedIndividual rdf:about="http://www.sisostds.org/ontologies/lox#PRVEDU">
        <rdf:type rdf:resource="http://www.sisostds.org/ontologies/C2SIM#TaskActionCode"/>
        <rdfs:comment>Provide education services: To provide labour and materiel for the educational process.</rdfs:comment>
    </owl:NamedIndividual>
    


    <!-- http://www.sisostds.org/ontologies/lox#PRVHLT -->

    <owl:NamedIndividual rdf:about="http://www.sisostds.org/ontologies/lox#PRVHLT">
        <rdf:type rdf:resource="http://www.sisostds.org/ontologies/C2SIM#TaskActionCode"/>
        <rdfs:comment>Provide healthcare services: To provide labour and materiel for maintaining the general health and welfare.</rdfs:comment>
    </owl:NamedIndividual>
    


    <!-- http://www.sisostds.org/ontologies/lox#PRVINF -->

    <owl:NamedIndividual rdf:about="http://www.sisostds.org/ontologies/lox#PRVINF">
        <rdf:type rdf:resource="http://www.sisostds.org/ontologies/C2SIM#TaskActionCode"/>
        <rdfs:comment>Provide infrastructure: To provide basic facilities such as roads, bridges, and sewers.</rdfs:comment>
    </owl:NamedIndividual>
    


    <!-- http://www.sisostds.org/ontologies/lox#PRVLND -->

    <owl:NamedIndividual rdf:about="http://www.sisostds.org/ontologies/lox#PRVLND">
        <rdf:type rdf:resource="http://www.sisostds.org/ontologies/C2SIM#TaskActionCode"/>
        <rdfs:comment>Provide laundry services: To provide labour and materiel for laundering of clothes or linens.</rdfs:comment>
    </owl:NamedIndividual>
    


    <!-- http://www.sisostds.org/ontologies/lox#PRVRPR -->

    <owl:NamedIndividual rdf:about="http://www.sisostds.org/ontologies/lox#PRVRPR">
        <rdf:type rdf:resource="http://www.sisostds.org/ontologies/C2SIM#TaskActionCode"/>
        <rdfs:comment>Provide repair services: To provide labour and materiel to restore objects to unimpaired condition.</rdfs:comment>
    </owl:NamedIndividual>
    


    <!-- http://www.sisostds.org/ontologies/lox#PRVSCY -->

    <owl:NamedIndividual rdf:about="http://www.sisostds.org/ontologies/lox#PRVSCY">
        <rdf:type rdf:resource="http://www.sisostds.org/ontologies/C2SIM#TaskActionCode"/>
        <rdfs:comment>Provide security services: To provide labour and materiel to assure safety of personnel and facilities.</rdfs:comment>
    </owl:NamedIndividual>
    


    <!-- http://www.sisostds.org/ontologies/lox#PRVSHL -->

    <owl:NamedIndividual rdf:about="http://www.sisostds.org/ontologies/lox#PRVSHL">
        <rdf:type rdf:resource="http://www.sisostds.org/ontologies/C2SIM#TaskActionCode"/>
        <rdfs:comment>Provide shelter: To provide housing.</rdfs:comment>
    </owl:NamedIndividual>
    


    <!-- http://www.sisostds.org/ontologies/lox#PRVSTG -->

    <owl:NamedIndividual rdf:about="http://www.sisostds.org/ontologies/lox#PRVSTG">
        <rdf:type rdf:resource="http://www.sisostds.org/ontologies/C2SIM#TaskActionCode"/>
        <rdfs:comment>Provide storage services: To provide services for storage.</rdfs:comment>
    </owl:NamedIndividual>
    


    <!-- http://www.sisostds.org/ontologies/lox#PRVTRS -->

    <owl:NamedIndividual rdf:about="http://www.sisostds.org/ontologies/lox#PRVTRS">
        <rdf:type rdf:resource="http://www.sisostds.org/ontologies/C2SIM#TaskActionCode"/>
        <rdfs:comment>Provide transhipment services: To provide movement of cargo from one ship or train or container to another for further shipment.</rdfs:comment>
    </owl:NamedIndividual>
    


    <!-- http://www.sisostds.org/ontologies/lox#PSYCHW -->

    <owl:NamedIndividual rdf:about="http://www.sisostds.org/ontologies/lox#PSYCHW">
        <rdf:type rdf:resource="http://www.sisostds.org/ontologies/C2SIM#TaskActionCode"/>
        <rdfs:comment>Psychological warfare: To use propaganda or other means designed to undermine the morale or allegiance of one&apos;s opponents.</rdfs:comment>
    </owl:NamedIndividual>
    


    <!-- http://www.sisostds.org/ontologies/lox#PUBMDA -->

    <owl:NamedIndividual rdf:about="http://www.sisostds.org/ontologies/lox#PUBMDA">
        <rdf:type rdf:resource="http://www.sisostds.org/ontologies/C2SIM#TaskActionCode"/>
        <rdfs:comment>Publish media article: To make generally known a non-fictional essay, esp. one included with others in a newspaper, magazine, journal, etc.</rdfs:comment>
    </owl:NamedIndividual>
    


    <!-- http://www.sisostds.org/ontologies/lox#PUBMDD -->

    <owl:NamedIndividual rdf:about="http://www.sisostds.org/ontologies/lox#PUBMDD">
        <rdf:type rdf:resource="http://www.sisostds.org/ontologies/C2SIM#TaskActionCode"/>
        <rdfs:comment>Publish media documentary: To make generally known any document published on a media that provides a factual record or report.</rdfs:comment>
    </owl:NamedIndividual>
    


    <!-- http://www.sisostds.org/ontologies/lox#PUBPRS -->

    <owl:NamedIndividual rdf:about="http://www.sisostds.org/ontologies/lox#PUBPRS">
        <rdf:type rdf:resource="http://www.sisostds.org/ontologies/C2SIM#TaskActionCode"/>
        <rdfs:comment>Publish press release: To make generally known an official statement issued to media for information.</rdfs:comment>
    </owl:NamedIndividual>
    


    <!-- http://www.sisostds.org/ontologies/lox#PURSUE -->

    <owl:NamedIndividual rdf:about="http://www.sisostds.org/ontologies/lox#PURSUE">
        <rdf:type rdf:resource="http://www.sisostds.org/ontologies/C2SIM#TaskActionCode"/>
        <rdfs:comment>Documentation: 		
						To continue offensive operations designed to catch or cut off a hostile force attempting to escape, with the aim of destroying it. Typically, contact is maintained and risk taken to harass relentlessly, thereby turning the pursuit into a rout.	
					; Appinfo DisplayValue as &quot;Pursue&quot;</rdfs:comment>
        <rdfs:comment>Pursue: To continue offensive operations designed to catch or cut off a hostile force attempting to escape, with the aim of destroying</rdfs:comment>
    </owl:NamedIndividual>
    


    <!-- http://www.sisostds.org/ontologies/lox#RCALIB -->

    <owl:NamedIndividual rdf:about="http://www.sisostds.org/ontologies/lox#RCALIB">
        <rdf:type rdf:resource="http://www.sisostds.org/ontologies/C2SIM#TaskActionCode"/>
        <rdfs:comment>Radio/radar calibration: To fly on a specific route in order to allow calibration of radars and radios.</rdfs:comment>
    </owl:NamedIndividual>
    


    <!-- http://www.sisostds.org/ontologies/lox#RECARM -->

    <owl:NamedIndividual rdf:about="http://www.sisostds.org/ontologies/lox#RECARM">
        <rdf:type rdf:resource="http://www.sisostds.org/ontologies/C2SIM#TaskActionCode"/>
        <rdfs:comment>Reconnaissance, armed: To locate and attack targets of opportunity, i.e. enemy material, personnel, and facilities in assigned surface communications</rdfs:comment>
    </owl:NamedIndividual>
    


    <!-- http://www.sisostds.org/ontologies/lox#RECCE -->

    <owl:NamedIndividual rdf:about="http://www.sisostds.org/ontologies/lox#RECCE">
        <rdf:type rdf:resource="http://www.sisostds.org/ontologies/C2SIM#TaskActionCode"/>
        <rdfs:comment>Documentation: 		
						To conduct a mission to obtain by visual operations or other detection methods information about the activities and resources of an enemy or potential enemy, or to secure data concerning the meteorological, hydrographic or geographic characteristics of a particular area.	
					; Appinfo DisplayValue as &quot;Reconnaissance&quot;</rdfs:comment>
        <rdfs:comment>Reconnaissance: To conduct a mission to obtain by visual operations or other detection methods information about the activities and resources</rdfs:comment>
    </owl:NamedIndividual>
    


    <!-- http://www.sisostds.org/ontologies/lox#RECCEF -->

    <owl:NamedIndividual rdf:about="http://www.sisostds.org/ontologies/lox#RECCEF">
        <rdf:type rdf:resource="http://www.sisostds.org/ontologies/C2SIM#TaskActionCode"/>
        <rdfs:comment>Reconnaissance in force: To conduct an offensive operation designed to discover and/or test the enemy&apos;s strength, or to obtain other information.</rdfs:comment>
    </owl:NamedIndividual>
    


    <!-- http://www.sisostds.org/ontologies/lox#RECCEL -->

    <owl:NamedIndividual rdf:about="http://www.sisostds.org/ontologies/lox#RECCEL">
        <rdf:type rdf:resource="http://www.sisostds.org/ontologies/C2SIM#TaskActionCode"/>
        <rdfs:comment>Reconnaissance, land: To obtain information concerning terrain, weather, and the disposition, composition, movement, installations, lines of communications,</rdfs:comment>
    </owl:NamedIndividual>
    


    <!-- http://www.sisostds.org/ontologies/lox#RECCES -->

    <owl:NamedIndividual rdf:about="http://www.sisostds.org/ontologies/lox#RECCES">
        <rdf:type rdf:resource="http://www.sisostds.org/ontologies/C2SIM#TaskActionCode"/>
        <rdfs:comment>Reconnaissance, shadow: To observe an enemy unit or force, usually as a sequel to surveillance or reconnaissance, for the purpose of reporting its</rdfs:comment>
    </owl:NamedIndividual>
    


    <!-- http://www.sisostds.org/ontologies/lox#RECECM -->

    <owl:NamedIndividual rdf:about="http://www.sisostds.org/ontologies/lox#RECECM">
        <rdf:type rdf:resource="http://www.sisostds.org/ontologies/C2SIM#TaskActionCode"/>
        <rdfs:comment>Reconnaissance, ECM: To detect ECM activities and resources of an enemy or potential enemy in a particular area.</rdfs:comment>
    </owl:NamedIndividual>
    


    <!-- http://www.sisostds.org/ontologies/lox#RECONS -->

    <owl:NamedIndividual rdf:about="http://www.sisostds.org/ontologies/lox#RECONS">
        <rdf:type rdf:resource="http://www.sisostds.org/ontologies/C2SIM#TaskActionCode"/>
        <rdfs:comment>Documentation: 		
						To attain prescribed strength of units and prescribed levels of vehicles, equipment, stores and supplies. The process will only take place after a unit/formation combat effectiveness has been reduced.	
					; Appinfo DisplayValue as &quot;Reconstitute&quot;</rdfs:comment>
        <rdfs:comment>Reconstitute: To attain prescribed strength of units and prescribed levels of vehicles, equipment, stores and supplies. The process will</rdfs:comment>
    </owl:NamedIndividual>
    


    <!-- http://www.sisostds.org/ontologies/lox#RECOVR -->

    <owl:NamedIndividual rdf:about="http://www.sisostds.org/ontologies/lox#RECOVR">
        <rdf:type rdf:resource="http://www.sisostds.org/ontologies/C2SIM#TaskActionCode"/>
        <rdfs:comment>Documentation: 		
						To retrieve any lost, incapacitated or captured object.	
					; Appinfo DisplayValue as &quot;Recover&quot;</rdfs:comment>
        <rdfs:comment>Recover: To retrieve any lost, incapacitated or captured object.</rdfs:comment>
    </owl:NamedIndividual>
    


    <!-- http://www.sisostds.org/ontologies/lox#RECPHO -->

    <owl:NamedIndividual rdf:about="http://www.sisostds.org/ontologies/lox#RECPHO">
        <rdf:type rdf:resource="http://www.sisostds.org/ontologies/C2SIM#TaskActionCode"/>
        <rdfs:comment>Reconnaissance, photographic: To obtain, by photographic means, information about the activities and resources of an enemy or potential enemy, or to secure</rdfs:comment>
    </owl:NamedIndividual>
    


    <!-- http://www.sisostds.org/ontologies/lox#RECRAD -->

    <owl:NamedIndividual rdf:about="http://www.sisostds.org/ontologies/lox#RECRAD">
        <rdf:type rdf:resource="http://www.sisostds.org/ontologies/C2SIM#TaskActionCode"/>
        <rdfs:comment>Reconnaissance, radar: To obtain, by radar detection methods, information about the activities and resources of an enemy or potential enemy, or to</rdfs:comment>
    </owl:NamedIndividual>
    


    <!-- http://www.sisostds.org/ontologies/lox#RECTGT -->

    <owl:NamedIndividual rdf:about="http://www.sisostds.org/ontologies/lox#RECTGT">
        <rdf:type rdf:resource="http://www.sisostds.org/ontologies/C2SIM#TaskActionCode"/>
        <rdfs:comment>Reconnaissance, target: To obtain information about the activities and resources of a target.</rdfs:comment>
    </owl:NamedIndividual>
    


    <!-- http://www.sisostds.org/ontologies/lox#RECUPR -->

    <owl:NamedIndividual rdf:about="http://www.sisostds.org/ontologies/lox#RECUPR">
        <rdf:type rdf:resource="http://www.sisostds.org/ontologies/C2SIM#TaskActionCode"/>
        <rdfs:comment>Recuperate: To rest a unit after it has been in action. Some reconstitution may take place as well.</rdfs:comment>
    </owl:NamedIndividual>
    


    <!-- http://www.sisostds.org/ontologies/lox#RECVIS -->

    <owl:NamedIndividual rdf:about="http://www.sisostds.org/ontologies/lox#RECVIS">
        <rdf:type rdf:resource="http://www.sisostds.org/ontologies/C2SIM#TaskActionCode"/>
        <rdfs:comment>Reconnaissance, visual: To obtain visual information about the activities and resources of an enemy or potential enemy, or to secure data concerning</rdfs:comment>
    </owl:NamedIndividual>
    


    <!-- http://www.sisostds.org/ontologies/lox#REDEPL -->

    <owl:NamedIndividual rdf:about="http://www.sisostds.org/ontologies/lox#REDEPL">
        <rdf:type rdf:resource="http://www.sisostds.org/ontologies/C2SIM#TaskActionCode"/>
        <rdfs:comment>Redeploy: To transfer a unit, an individual, or supplies deployed in one area to another area, or to another location within the area,</rdfs:comment>
    </owl:NamedIndividual>
    


    <!-- http://www.sisostds.org/ontologies/lox#REFILL -->

    <owl:NamedIndividual rdf:about="http://www.sisostds.org/ontologies/lox#REFILL">
        <rdf:type rdf:resource="http://www.sisostds.org/ontologies/C2SIM#TaskActionCode"/>
        <rdfs:comment>Refill: To fill again.</rdfs:comment>
    </owl:NamedIndividual>
    


    <!-- http://www.sisostds.org/ontologies/lox#REFORM -->

    <owl:NamedIndividual rdf:about="http://www.sisostds.org/ontologies/lox#REFORM">
        <rdf:type rdf:resource="http://www.sisostds.org/ontologies/C2SIM#TaskActionCode"/>
        <rdfs:comment>Reform: No definition provided in ADatP-3 Baseline 13.1 FFIRN/FUD 1299/19.</rdfs:comment>
    </owl:NamedIndividual>
    


    <!-- http://www.sisostds.org/ontologies/lox#REFUEL -->

    <owl:NamedIndividual rdf:about="http://www.sisostds.org/ontologies/lox#REFUEL">
        <rdf:type rdf:resource="http://www.sisostds.org/ontologies/C2SIM#TaskActionCode"/>
        <rdfs:comment>Documentation: 		
						To take on more fuel.	
					; Appinfo DisplayValue as &quot;Refuel&quot;</rdfs:comment>
        <rdfs:comment>Refuel: To take on more fuel.</rdfs:comment>
    </owl:NamedIndividual>
    


    <!-- http://www.sisostds.org/ontologies/lox#REINF -->

    <owl:NamedIndividual rdf:about="http://www.sisostds.org/ontologies/lox#REINF">
        <rdf:type rdf:resource="http://www.sisostds.org/ontologies/C2SIM#TaskActionCode"/>
        <rdfs:comment>Documentation: 		
						To move or make a force available to another commander for the purpose of supplementing the in-place forces.	
					; Appinfo DisplayValue as &quot;Reinforce&quot;</rdfs:comment>
        <rdfs:comment>Reinforce: To move or make a force available to another commander for the purpose of supplementing the in-place forces.</rdfs:comment>
    </owl:NamedIndividual>
    


    <!-- http://www.sisostds.org/ontologies/lox#REORG -->

    <owl:NamedIndividual rdf:about="http://www.sisostds.org/ontologies/lox#REORG">
        <rdf:type rdf:resource="http://www.sisostds.org/ontologies/C2SIM#TaskActionCode"/>
        <rdfs:comment>Reorganise: To change a task organisation for a particular operation. (Normally takes place before an operation). This includes the transfer</rdfs:comment>
    </owl:NamedIndividual>
    


    <!-- http://www.sisostds.org/ontologies/lox#REPAIR -->

    <owl:NamedIndividual rdf:about="http://www.sisostds.org/ontologies/lox#REPAIR">
        <rdf:type rdf:resource="http://www.sisostds.org/ontologies/C2SIM#TaskActionCode"/>
        <rdfs:comment>Repair: To restore an item to serviceable condition through correction of a specific failure or unserviceable condition.</rdfs:comment>
    </owl:NamedIndividual>
    


    <!-- http://www.sisostds.org/ontologies/lox#RESCUE -->

    <owl:NamedIndividual rdf:about="http://www.sisostds.org/ontologies/lox#RESCUE">
        <rdf:type rdf:resource="http://www.sisostds.org/ontologies/C2SIM#TaskActionCode"/>
        <rdfs:comment>Documentation: 		
						To use aircraft, surface craft (land or water), submarines, specialized rescue teams, and equipment to rescue personnel in distress on land or at sea.	
					; Appinfo DisplayValue as &quot;Rescue&quot;</rdfs:comment>
        <rdfs:comment>Rescue: To use aircraft, surface craft (land or water), submarines, specialized rescue teams, and equipment to rescue personnel in</rdfs:comment>
    </owl:NamedIndividual>
    


    <!-- http://www.sisostds.org/ontologies/lox#REST -->

    <owl:NamedIndividual rdf:about="http://www.sisostds.org/ontologies/lox#REST">
        <rdf:type rdf:resource="http://www.sisostds.org/ontologies/C2SIM#TaskActionCode"/>
        <rdfs:comment>Rest: To impose a specified period of inactivity on an ORGANISATION that is out of contact with the enemy.</rdfs:comment>
    </owl:NamedIndividual>
    


    <!-- http://www.sisostds.org/ontologies/lox#RESUPL -->

    <owl:NamedIndividual rdf:about="http://www.sisostds.org/ontologies/lox#RESUPL">
        <rdf:type rdf:resource="http://www.sisostds.org/ontologies/C2SIM#TaskActionCode"/>
        <rdfs:comment>Documentation: 		
						To replenish stocks in order to maintain the required levels of supply.	
					; Appinfo DisplayValue as &quot;Resupply&quot;</rdfs:comment>
        <rdfs:comment>Resupply: To replenish stocks in order to maintain the required levels of supply.</rdfs:comment>
    </owl:NamedIndividual>
    


    <!-- http://www.sisostds.org/ontologies/lox#RETAIN -->

    <owl:NamedIndividual rdf:about="http://www.sisostds.org/ontologies/lox#RETAIN">
        <rdf:type rdf:resource="http://www.sisostds.org/ontologies/C2SIM#TaskActionCode"/>
        <rdfs:comment>Documentation: 		
						To occupy and hold a terrain feature to ensure it is free of enemy occupation or use.	
					; Appinfo DisplayValue as &quot;Retain&quot;</rdfs:comment>
        <rdfs:comment>Retain: To occupy and hold a terrain feature to ensure it is free of enemy occupation or use.</rdfs:comment>
    </owl:NamedIndividual>
    


    <!-- http://www.sisostds.org/ontologies/lox#RETIRE -->

    <owl:NamedIndividual rdf:about="http://www.sisostds.org/ontologies/lox#RETIRE">
        <rdf:type rdf:resource="http://www.sisostds.org/ontologies/C2SIM#TaskActionCode"/>
        <rdfs:comment>Retire: To move a force out of contact with the enemy with the expectation of no further significant contact.</rdfs:comment>
    </owl:NamedIndividual>
    


    <!-- http://www.sisostds.org/ontologies/lox#RLFPLC -->

    <owl:NamedIndividual rdf:about="http://www.sisostds.org/ontologies/lox#RLFPLC">
        <rdf:type rdf:resource="http://www.sisostds.org/ontologies/C2SIM#TaskActionCode"/>
        <rdfs:comment>Documentation: 		
						To conduct an operation in which, by direction of higher authority, all or part of a unit is replaced in an area by the incoming unit. The responsibilities of the replaced elements for the mission and the assigned zone of operations are transferred to the incoming unit. The incoming unit continues the operation as ordered.	
					; Appinfo DisplayValue as &quot;Relief in place&quot;</rdfs:comment>
        <rdfs:comment>Relief in place: To conduct an operation in which, by direction of higher authority, all or part of a unit is replaced in an area by the incoming</rdfs:comment>
    </owl:NamedIndividual>
    


    <!-- http://www.sisostds.org/ontologies/lox#RNDZVA -->

    <owl:NamedIndividual rdf:about="http://www.sisostds.org/ontologies/lox#RNDZVA">
        <rdf:type rdf:resource="http://www.sisostds.org/ontologies/C2SIM#TaskActionCode"/>
        <rdfs:comment>Rendezvous procedure alpha: To rendezvous using a procedure directed by a radar control station, whether ground based, seaborne, or airborne (anchor rendezvous).</rdfs:comment>
    </owl:NamedIndividual>
    


    <!-- http://www.sisostds.org/ontologies/lox#RNDZVB -->

    <owl:NamedIndividual rdf:about="http://www.sisostds.org/ontologies/lox#RNDZVB">
        <rdf:type rdf:resource="http://www.sisostds.org/ontologies/C2SIM#TaskActionCode"/>
        <rdfs:comment>Rendezvous procedure bravo: To rendezvous using a heading based procedure which utilises air-to-air equipment of both tanker and receiver. The tanker</rdfs:comment>
    </owl:NamedIndividual>
    


    <!-- http://www.sisostds.org/ontologies/lox#RNDZVC -->

    <owl:NamedIndividual rdf:about="http://www.sisostds.org/ontologies/lox#RNDZVC">
        <rdf:type rdf:resource="http://www.sisostds.org/ontologies/C2SIM#TaskActionCode"/>
        <rdfs:comment>Rendezvous procedure charlie: To rendezvous using a heading based procedure which allows receivers with an airborne intercept (AI) radar to control the</rdfs:comment>
    </owl:NamedIndividual>
    


    <!-- http://www.sisostds.org/ontologies/lox#RNDZVD -->

    <owl:NamedIndividual rdf:about="http://www.sisostds.org/ontologies/lox#RNDZVD">
        <rdf:type rdf:resource="http://www.sisostds.org/ontologies/C2SIM#TaskActionCode"/>
        <rdfs:comment>Rendezvous procedure delta: To rendezvous using a procedure that requires the receiver to maintain an agreed track and the tanker to maintain the reciprocal</rdfs:comment>
    </owl:NamedIndividual>
    


    <!-- http://www.sisostds.org/ontologies/lox#RNDZVE -->

    <owl:NamedIndividual rdf:about="http://www.sisostds.org/ontologies/lox#RNDZVE">
        <rdf:type rdf:resource="http://www.sisostds.org/ontologies/C2SIM#TaskActionCode"/>
        <rdfs:comment>Rendezvous procedure echo: To rendezvous using a procedure for use in support of a combat air patrol (CAP). It is particularly useful during periods</rdfs:comment>
    </owl:NamedIndividual>
    


    <!-- http://www.sisostds.org/ontologies/lox#RNDZVF -->

    <owl:NamedIndividual rdf:about="http://www.sisostds.org/ontologies/lox#RNDZVF">
        <rdf:type rdf:resource="http://www.sisostds.org/ontologies/C2SIM#TaskActionCode"/>
        <rdfs:comment>Rendezvous procedure foxtrot: To rendezvous using a procedure where the tanker and receiver operate from the same base.</rdfs:comment>
    </owl:NamedIndividual>
    


    <!-- http://www.sisostds.org/ontologies/lox#RNDZVG -->

    <owl:NamedIndividual rdf:about="http://www.sisostds.org/ontologies/lox#RNDZVG">
        <rdf:type rdf:resource="http://www.sisostds.org/ontologies/C2SIM#TaskActionCode"/>
        <rdfs:comment>Rendezvous procedure golf: To rendezvous using a procedure that facilitates join-up on a common track; receivers may have departed either from the same</rdfs:comment>
    </owl:NamedIndividual>
    


    <!-- http://www.sisostds.org/ontologies/lox#RNDZVS -->

    <owl:NamedIndividual rdf:about="http://www.sisostds.org/ontologies/lox#RNDZVS">
        <rdf:type rdf:resource="http://www.sisostds.org/ontologies/C2SIM#TaskActionCode"/>
        <rdfs:comment>Rendezvous: To achieve a pre-arranged meeting at a given time and place.</rdfs:comment>
    </owl:NamedIndividual>
    


    <!-- http://www.sisostds.org/ontologies/lox#ROEFree -->

    <owl:NamedIndividual rdf:about="http://www.sisostds.org/ontologies/lox#ROEFree">
        <rdf:type rdf:resource="http://www.sisostds.org/ontologies/lox#WeaponRuleOfEngagementCode"/>
    </owl:NamedIndividual>
    


    <!-- http://www.sisostds.org/ontologies/lox#ROEHold -->

    <owl:NamedIndividual rdf:about="http://www.sisostds.org/ontologies/lox#ROEHold">
        <rdf:type rdf:resource="http://www.sisostds.org/ontologies/lox#WeaponRuleOfEngagementCode"/>
    </owl:NamedIndividual>
    


    <!-- http://www.sisostds.org/ontologies/lox#ROETight -->

    <owl:NamedIndividual rdf:about="http://www.sisostds.org/ontologies/lox#ROETight">
        <rdf:type rdf:resource="http://www.sisostds.org/ontologies/lox#WeaponRuleOfEngagementCode"/>
    </owl:NamedIndividual>
    


    <!-- http://www.sisostds.org/ontologies/lox#SAR -->

    <owl:NamedIndividual rdf:about="http://www.sisostds.org/ontologies/lox#SAR">
        <rdf:type rdf:resource="http://www.sisostds.org/ontologies/C2SIM#TaskActionCode"/>
        <rdfs:comment>Search and rescue: To use aircraft, surface craft, submarines, specialized rescue teams and equipment to search for and rescue personnel in distress</rdfs:comment>
    </owl:NamedIndividual>
    


    <!-- http://www.sisostds.org/ontologies/lox#SARCME -->

    <owl:NamedIndividual rdf:about="http://www.sisostds.org/ontologies/lox#SARCME">
        <rdf:type rdf:resource="http://www.sisostds.org/ontologies/C2SIM#TaskActionCode"/>
        <rdfs:comment>Search and rescue, combat, exfiltrate: To remove personnel from areas under enemy control by specially trained personnel qualified to penetrate to the site of an</rdfs:comment>
    </owl:NamedIndividual>
    


    <!-- http://www.sisostds.org/ontologies/lox#SARCMI -->

    <owl:NamedIndividual rdf:about="http://www.sisostds.org/ontologies/lox#SARCMI">
        <rdf:type rdf:resource="http://www.sisostds.org/ontologies/C2SIM#TaskActionCode"/>
        <rdfs:comment>Search and rescue, combat, infiltrate: To move through or into an area or territory occupied by either friendly or enemy troops or organisations specially trained</rdfs:comment>
    </owl:NamedIndividual>
    


    <!-- http://www.sisostds.org/ontologies/lox#SARPLG -->

    <owl:NamedIndividual rdf:about="http://www.sisostds.org/ontologies/lox#SARPLG">
        <rdf:type rdf:resource="http://www.sisostds.org/ontologies/C2SIM#TaskActionCode"/>
        <rdfs:comment>Search and rescue, plane guard: Helicopter maintains station in vicinity of carrier for potential SAR during flight operations.</rdfs:comment>
    </owl:NamedIndividual>
    


    <!-- http://www.sisostds.org/ontologies/lox#SCOUT -->

    <owl:NamedIndividual rdf:about="http://www.sisostds.org/ontologies/lox#SCOUT">
        <rdf:type rdf:resource="http://www.sisostds.org/ontologies/C2SIM#TaskActionCode"/>
        <rdfs:comment>Scout: To collect intelligence without engaging enemy forces.</rdfs:comment>
    </owl:NamedIndividual>
    


    <!-- http://www.sisostds.org/ontologies/lox#SCREEN -->

    <owl:NamedIndividual rdf:about="http://www.sisostds.org/ontologies/lox#SCREEN">
        <rdf:type rdf:resource="http://www.sisostds.org/ontologies/C2SIM#TaskActionCode"/>
        <rdfs:comment>Documentation: 		
						To operate as a security element whose primary task is to observe, identify and report information, and which only fights in self-protection.	
					; Appinfo DisplayValue as &quot;Screen&quot;</rdfs:comment>
        <rdfs:comment>Screen: To operate as a security element whose primary task is to observe, identify and report information, and which only fights</rdfs:comment>
    </owl:NamedIndividual>
    


    <!-- http://www.sisostds.org/ontologies/lox#SCRMBL -->

    <owl:NamedIndividual rdf:about="http://www.sisostds.org/ontologies/lox#SCRMBL">
        <rdf:type rdf:resource="http://www.sisostds.org/ontologies/C2SIM#TaskActionCode"/>
        <rdfs:comment>Scramble: To launch or take-off an aircraft as quickly as possible, usually followed by mission instructions.</rdfs:comment>
    </owl:NamedIndividual>
    


    <!-- http://www.sisostds.org/ontologies/lox#SDAM -->

    <owl:NamedIndividual rdf:about="http://www.sisostds.org/ontologies/lox#SDAM">
        <rdfs:comment>Documentation: 		
						The subjective categorisation of the physical effect of an ACTION on buildings, infrastructure and/or equipment by a reporting ORGANISATION.	
					; Appinfo DisplayValue as &quot;Severe damage&quot;</rdfs:comment>
    </owl:NamedIndividual>
    


    <!-- http://www.sisostds.org/ontologies/lox#SECURE -->

    <owl:NamedIndividual rdf:about="http://www.sisostds.org/ontologies/lox#SECURE">
        <rdf:type rdf:resource="http://www.sisostds.org/ontologies/C2SIM#TaskActionCode"/>
        <rdfs:comment>Documentation: 		
						To gain possession of a position or terrain feature, with or without force, and to make such disposition as will prevent, as far as possible, its destruction or loss by enemy action.	
					; Appinfo DisplayValue as &quot;Secure&quot;</rdfs:comment>
        <rdfs:comment>Secure: To gain possession of a position or terrain feature, with or without force, and to make such disposition as will prevent,</rdfs:comment>
    </owl:NamedIndividual>
    


    <!-- http://www.sisostds.org/ontologies/lox#SECURT -->

    <owl:NamedIndividual rdf:about="http://www.sisostds.org/ontologies/lox#SECURT">
        <rdf:type rdf:resource="http://www.sisostds.org/ontologies/C2SIM#TaskActionCode"/>
        <rdfs:comment>Security: To take measures necessary to achieve protection against espionage, sabotage, subversion and terrorism, as well as against</rdfs:comment>
    </owl:NamedIndividual>
    


    <!-- http://www.sisostds.org/ontologies/lox#SEIZE -->

    <owl:NamedIndividual rdf:about="http://www.sisostds.org/ontologies/lox#SEIZE">
        <rdf:type rdf:resource="http://www.sisostds.org/ontologies/C2SIM#TaskActionCode"/>
        <rdfs:comment>Documentation: 		
						To clear a designated area and obtain control of it.	
					; Appinfo DisplayValue as &quot;Seize&quot;</rdfs:comment>
        <rdfs:comment>Seize: To clear a designated area and obtain control of it.</rdfs:comment>
    </owl:NamedIndividual>
    


    <!-- http://www.sisostds.org/ontologies/lox#SENSIM -->

    <owl:NamedIndividual rdf:about="http://www.sisostds.org/ontologies/lox#SENSIM">
        <rdf:type rdf:resource="http://www.sisostds.org/ontologies/C2SIM#TaskActionCode"/>
        <rdfs:comment>Sensor implant: To insert a piece of equipment which detects, and may indicate, and/or record objects and activities by means of energy or</rdfs:comment>
    </owl:NamedIndividual>
    


    <!-- http://www.sisostds.org/ontologies/lox#SERASE -->

    <owl:NamedIndividual rdf:about="http://www.sisostds.org/ontologies/lox#SERASE">
        <rdf:type rdf:resource="http://www.sisostds.org/ontologies/C2SIM#TaskActionCode"/>
        <rdfs:comment>Serve as an assault echelon: To serve as an element of a force which is scheduled for initial assault on the objective area.</rdfs:comment>
    </owl:NamedIndividual>
    


    <!-- http://www.sisostds.org/ontologies/lox#SERATE -->

    <owl:NamedIndividual rdf:about="http://www.sisostds.org/ontologies/lox#SERATE">
        <rdf:type rdf:resource="http://www.sisostds.org/ontologies/C2SIM#TaskActionCode"/>
        <rdfs:comment>Serve as an attack echelon: To serve as a fraction of a command in the direction of depth, to which an attack mission is assigned.</rdfs:comment>
    </owl:NamedIndividual>
    


    <!-- http://www.sisostds.org/ontologies/lox#SERCH -->

    <owl:NamedIndividual rdf:about="http://www.sisostds.org/ontologies/lox#SERCH">
        <rdf:type rdf:resource="http://www.sisostds.org/ontologies/C2SIM#TaskActionCode"/>
        <rdfs:comment>Search: No definition provided in APP-6A.</rdfs:comment>
    </owl:NamedIndividual>
    


    <!-- http://www.sisostds.org/ontologies/lox#SERFLO -->

    <owl:NamedIndividual rdf:about="http://www.sisostds.org/ontologies/lox#SERFLO">
        <rdf:type rdf:resource="http://www.sisostds.org/ontologies/C2SIM#TaskActionCode"/>
        <rdfs:comment>Serve as the follow-on echelon: To serve as, in amphibious operations, that echelon of the assault troops, vehicles, aircraft equipment, and supplies which,</rdfs:comment>
    </owl:NamedIndividual>
    


    <!-- http://www.sisostds.org/ontologies/lox#SERFOE -->

    <owl:NamedIndividual rdf:about="http://www.sisostds.org/ontologies/lox#SERFOE">
        <rdf:type rdf:resource="http://www.sisostds.org/ontologies/C2SIM#TaskActionCode"/>
        <rdfs:comment>Serve as the first operational echelon: To serve as a fraction of a command, to which the first mission is assigned or which forms the forward line of own troops</rdfs:comment>
    </owl:NamedIndividual>
    


    <!-- http://www.sisostds.org/ontologies/lox#SERFRE -->

    <owl:NamedIndividual rdf:about="http://www.sisostds.org/ontologies/lox#SERFRE">
        <rdf:type rdf:resource="http://www.sisostds.org/ontologies/C2SIM#TaskActionCode"/>
        <rdfs:comment>Serve as the forward echelon: To serve as a forward subdivision of a headquarters.</rdfs:comment>
    </owl:NamedIndividual>
    


    <!-- http://www.sisostds.org/ontologies/lox#SERFTE -->

    <owl:NamedIndividual rdf:about="http://www.sisostds.org/ontologies/lox#SERFTE">
        <rdf:type rdf:resource="http://www.sisostds.org/ontologies/C2SIM#TaskActionCode"/>
        <rdfs:comment>Serve as the first tactical echelon: To serve as a fraction of a tactical command, to which a primary mission is assigned.</rdfs:comment>
    </owl:NamedIndividual>
    


    <!-- http://www.sisostds.org/ontologies/lox#SERFUE -->

    <owl:NamedIndividual rdf:about="http://www.sisostds.org/ontologies/lox#SERFUE">
        <rdf:type rdf:resource="http://www.sisostds.org/ontologies/C2SIM#TaskActionCode"/>
        <rdfs:comment>Serve as the follow-up echelon: To serve as, in air transport operations, an element moved into the objective area after the assault echelon.</rdfs:comment>
    </owl:NamedIndividual>
    


    <!-- http://www.sisostds.org/ontologies/lox#SERREE -->

    <owl:NamedIndividual rdf:about="http://www.sisostds.org/ontologies/lox#SERREE">
        <rdf:type rdf:resource="http://www.sisostds.org/ontologies/C2SIM#TaskActionCode"/>
        <rdfs:comment>Serve as the rear echelon: To serve as elements of a force which are not required in the objective area.</rdfs:comment>
    </owl:NamedIndividual>
    


    <!-- http://www.sisostds.org/ontologies/lox#SERRSE -->

    <owl:NamedIndividual rdf:about="http://www.sisostds.org/ontologies/lox#SERRSE">
        <rdf:type rdf:resource="http://www.sisostds.org/ontologies/C2SIM#TaskActionCode"/>
        <rdfs:comment>Serve as the reserve echelon: To serve as a fraction of a command in the direction of depth, which is an assigned reserve.</rdfs:comment>
    </owl:NamedIndividual>
    


    <!-- http://www.sisostds.org/ontologies/lox#SERSEA -->

    <owl:NamedIndividual rdf:about="http://www.sisostds.org/ontologies/lox#SERSEA">
        <rdf:type rdf:resource="http://www.sisostds.org/ontologies/C2SIM#TaskActionCode"/>
        <rdfs:comment>Serve as the sea echelon: To serve as a portion of the assault shipping which withdraws from, or remains out of, the transport area during an amphibious</rdfs:comment>
    </owl:NamedIndividual>
    


    <!-- http://www.sisostds.org/ontologies/lox#SERSOE -->

    <owl:NamedIndividual rdf:about="http://www.sisostds.org/ontologies/lox#SERSOE">
        <rdf:type rdf:resource="http://www.sisostds.org/ontologies/C2SIM#TaskActionCode"/>
        <rdfs:comment>Serve as the second operational echelon: To serve as a fraction of an operational command either in the direction of depth or as a follow up on the timeline, to which</rdfs:comment>
    </owl:NamedIndividual>
    


    <!-- http://www.sisostds.org/ontologies/lox#SERSPE -->

    <owl:NamedIndividual rdf:about="http://www.sisostds.org/ontologies/lox#SERSPE">
        <rdf:type rdf:resource="http://www.sisostds.org/ontologies/C2SIM#TaskActionCode"/>
        <rdfs:comment>Serve as a support echelon: To serve as a fraction of a command in the direction of depth, to which a support mission is assigned.</rdfs:comment>
    </owl:NamedIndividual>
    


    <!-- http://www.sisostds.org/ontologies/lox#SERSTE -->

    <owl:NamedIndividual rdf:about="http://www.sisostds.org/ontologies/lox#SERSTE">
        <rdf:type rdf:resource="http://www.sisostds.org/ontologies/C2SIM#TaskActionCode"/>
        <rdfs:comment>Serve as the second tactical echelon: To serve as a fraction of a tactical command either in the direction of depth or as a follow up on the timeline, to which</rdfs:comment>
    </owl:NamedIndividual>
    


    <!-- http://www.sisostds.org/ontologies/lox#SERSTR -->

    <owl:NamedIndividual rdf:about="http://www.sisostds.org/ontologies/lox#SERSTR">
        <rdf:type rdf:resource="http://www.sisostds.org/ontologies/C2SIM#TaskActionCode"/>
        <rdfs:comment>Serve as a strategic reserve: To serve as a fraction of a command in the direction of depth, which is an assigned strategic reserve.</rdfs:comment>
    </owl:NamedIndividual>
    


    <!-- http://www.sisostds.org/ontologies/lox#SERTHR -->

    <owl:NamedIndividual rdf:about="http://www.sisostds.org/ontologies/lox#SERTHR">
        <rdf:type rdf:resource="http://www.sisostds.org/ontologies/C2SIM#TaskActionCode"/>
        <rdfs:comment>Serve as the theatre reserve: To serve as a fraction of a command in the direction of depth, which is an assigned theatre reserve.</rdfs:comment>
    </owl:NamedIndividual>
    


    <!-- http://www.sisostds.org/ontologies/lox#SETUP -->

    <owl:NamedIndividual rdf:about="http://www.sisostds.org/ontologies/lox#SETUP">
        <rdf:type rdf:resource="http://www.sisostds.org/ontologies/C2SIM#TaskActionCode"/>
        <rdfs:comment>Set up: To prepare or establish a FACILITY, ORGANISATION or FEATURE.</rdfs:comment>
    </owl:NamedIndividual>
    


    <!-- http://www.sisostds.org/ontologies/lox#SINGA -->

    <owl:NamedIndividual rdf:about="http://www.sisostds.org/ontologies/lox#SINGA">
        <rdf:type rdf:resource="http://www.sisostds.org/ontologies/C2SIM#TaskActionCode"/>
        <rdfs:comment>Signals intelligence gathering: To intercept and gather electronic and communications transmissions for intelligence purposes.</rdfs:comment>
    </owl:NamedIndividual>
    


    <!-- http://www.sisostds.org/ontologies/lox#SPCOPS -->

    <owl:NamedIndividual rdf:about="http://www.sisostds.org/ontologies/lox#SPCOPS">
        <rdf:type rdf:resource="http://www.sisostds.org/ontologies/C2SIM#TaskActionCode"/>
        <rdfs:comment>Special operations: A mission conducted by specially designated, organised, trained and equipped forces using operational techniques and modes</rdfs:comment>
    </owl:NamedIndividual>
    


    <!-- http://www.sisostds.org/ontologies/lox#SPREAD -->

    <owl:NamedIndividual rdf:about="http://www.sisostds.org/ontologies/lox#SPREAD">
        <rdf:type rdf:resource="http://www.sisostds.org/ontologies/C2SIM#TaskActionCode"/>
        <rdfs:comment>Spread: No definition provided in ADatP-3 Baseline 13.1 FFIRN/FUD 1299/19.</rdfs:comment>
    </owl:NamedIndividual>
    


    <!-- http://www.sisostds.org/ontologies/lox#SPTCON -->

    <owl:NamedIndividual rdf:about="http://www.sisostds.org/ontologies/lox#SPTCON">
        <rdf:type rdf:resource="http://www.sisostds.org/ontologies/C2SIM#TaskActionCode"/>
        <rdfs:comment>Support, contingency: To involve in emergency, military forces due to natural disasters, terrorists, subversives, or by required military operations.</rdfs:comment>
    </owl:NamedIndividual>
    


    <!-- http://www.sisostds.org/ontologies/lox#SPTELC -->

    <owl:NamedIndividual rdf:about="http://www.sisostds.org/ontologies/lox#SPTELC">
        <rdf:type rdf:resource="http://www.sisostds.org/ontologies/C2SIM#TaskActionCode"/>
        <rdfs:comment>Support, electronic: To provide information required for decisions involving electronic warfare operations and other tactical actions such as threat</rdfs:comment>
    </owl:NamedIndividual>
    


    <!-- http://www.sisostds.org/ontologies/lox#SRCHFR -->

    <owl:NamedIndividual rdf:about="http://www.sisostds.org/ontologies/lox#SRCHFR">
        <rdf:type rdf:resource="http://www.sisostds.org/ontologies/C2SIM#TaskActionCode"/>
        <rdfs:comment>Search by fire: To distribute fire in depth by successive changes in the elevation of the gun.</rdfs:comment>
    </owl:NamedIndividual>
    


    <!-- http://www.sisostds.org/ontologies/lox#SRCRES -->

    <owl:NamedIndividual rdf:about="http://www.sisostds.org/ontologies/lox#SRCRES">
        <rdf:type rdf:resource="http://www.sisostds.org/ontologies/C2SIM#TaskActionCode"/>
        <rdfs:comment>Search and rescue, combat: To detect, locate, identify and rescue downed aircrew in hostile territory in crisis and wartime and, when appropriate, isolated</rdfs:comment>
    </owl:NamedIndividual>
    


    <!-- http://www.sisostds.org/ontologies/lox#STRCON -->

    <owl:NamedIndividual rdf:about="http://www.sisostds.org/ontologies/lox#STRCON">
        <rdf:type rdf:resource="http://www.sisostds.org/ontologies/C2SIM#TaskActionCode"/>
        <rdfs:comment>Strike control and reconnaissance: To conduct reconnaissance strike control and reconnaissance operations.</rdfs:comment>
    </owl:NamedIndividual>
    


    <!-- http://www.sisostds.org/ontologies/lox#STRWAF -->

    <owl:NamedIndividual rdf:about="http://www.sisostds.org/ontologies/lox#STRWAF">
        <rdf:type rdf:resource="http://www.sisostds.org/ontologies/C2SIM#TaskActionCode"/>
        <rdfs:comment>Strike warfare: To conduct warfare that includes strikes against targets ashore using carrier-based strike aircraft, sea-launched cruise missiles,</rdfs:comment>
    </owl:NamedIndividual>
    


    <!-- http://www.sisostds.org/ontologies/lox#SUBWAF -->

    <owl:NamedIndividual rdf:about="http://www.sisostds.org/ontologies/lox#SUBWAF">
        <rdf:type rdf:resource="http://www.sisostds.org/ontologies/C2SIM#TaskActionCode"/>
        <rdfs:comment>Submarine warfare: To conduct warfare that includes the use of submarines.</rdfs:comment>
    </owl:NamedIndividual>
    


    <!-- http://www.sisostds.org/ontologies/lox#SUPPRS -->

    <owl:NamedIndividual rdf:about="http://www.sisostds.org/ontologies/lox#SUPPRS">
        <rdf:type rdf:resource="http://www.sisostds.org/ontologies/C2SIM#TaskActionCode"/>
        <rdfs:comment>Documentation: 		
						To provide fire which neutralizes or temporarily degrades the capabilities of enemy forces within a specific area. This makes no assumptions as to enemy casualties; it may be a transitory effect.	
					; Appinfo DisplayValue as &quot;Suppress&quot;</rdfs:comment>
        <rdfs:comment>Suppress: To provide fire which neutralizes or temporarily degrades the capabilities of enemy forces within a specific area. This makes</rdfs:comment>
    </owl:NamedIndividual>
    


    <!-- http://www.sisostds.org/ontologies/lox#SUPPRT -->

    <owl:NamedIndividual rdf:about="http://www.sisostds.org/ontologies/lox#SUPPRT">
        <rdf:type rdf:resource="http://www.sisostds.org/ontologies/C2SIM#TaskActionCode"/>
        <rdfs:comment>Documentation: 		
						To aid, protect, complement or sustain any other object.	
					; Appinfo DisplayValue as &quot;Support&quot;</rdfs:comment>
        <rdfs:comment>Support: To aid, protect, complement or sustain any other object.</rdfs:comment>
    </owl:NamedIndividual>
    


    <!-- http://www.sisostds.org/ontologies/lox#SUPRSD -->

    <owl:NamedIndividual rdf:about="http://www.sisostds.org/ontologies/lox#SUPRSD">
        <rdfs:comment>Documentation: 		
						Reduction of the effectiveness of the ACTION objective for a specific period or purpose (normally to prevent an enemy from interfering with friendly ACTIONs); this effect may be entirely transitory and cause no casualties.	
					; Appinfo DisplayValue as &quot;Suppressed&quot;</rdfs:comment>
    </owl:NamedIndividual>
    


    <!-- http://www.sisostds.org/ontologies/lox#SURVEL -->

    <owl:NamedIndividual rdf:about="http://www.sisostds.org/ontologies/lox#SURVEL">
        <rdf:type rdf:resource="http://www.sisostds.org/ontologies/C2SIM#TaskActionCode"/>
        <rdfs:comment>Surveillance, electronic: The systematic observation of aerospace, surface or subsurface areas, places, persons, or things, by electronic means.</rdfs:comment>
    </owl:NamedIndividual>
    


    <!-- http://www.sisostds.org/ontologies/lox#SURVLE -->

    <owl:NamedIndividual rdf:about="http://www.sisostds.org/ontologies/lox#SURVLE">
        <rdf:type rdf:resource="http://www.sisostds.org/ontologies/C2SIM#TaskActionCode"/>
        <rdfs:comment>Surveillance: To observe aerospace, surface or subsurface areas, places, persons, or things, by visual, aural electronic, photographic,</rdfs:comment>
    </owl:NamedIndividual>
    


    <!-- http://www.sisostds.org/ontologies/lox#SUSOAA -->

    <owl:NamedIndividual rdf:about="http://www.sisostds.org/ontologies/lox#SUSOAA">
        <rdf:type rdf:resource="http://www.sisostds.org/ontologies/C2SIM#TaskActionCode"/>
        <rdfs:comment>Sustaining operations afloat and ashore: To conduct an operation in which maritime forces continue to provide direct and indirect support to combat operations ashore,</rdfs:comment>
    </owl:NamedIndividual>
    


    <!-- http://www.sisostds.org/ontologies/lox#SWEEP -->

    <owl:NamedIndividual rdf:about="http://www.sisostds.org/ontologies/lox#SWEEP">
        <rdf:type rdf:resource="http://www.sisostds.org/ontologies/C2SIM#TaskActionCode"/>
        <rdfs:comment>Sweep: An offensive mission by fighter aircraft to seek out and destroy enemy aircraft and other targets of opportunity in an allocated</rdfs:comment>
    </owl:NamedIndividual>
    


    <!-- http://www.sisostds.org/ontologies/lox#TCARRC -->

    <owl:NamedIndividual rdf:about="http://www.sisostds.org/ontologies/lox#TCARRC">
        <rdf:type rdf:resource="http://www.sisostds.org/ontologies/C2SIM#TaskActionCode"/>
        <rdfs:comment>Tactical air reconnaissance: Air action, which consist of the collection of information of intelligence from the air or through the use of airborne sensors.</rdfs:comment>
    </owl:NamedIndividual>
    


    <!-- http://www.sisostds.org/ontologies/lox#TGTDLT -->

    <owl:NamedIndividual rdf:about="http://www.sisostds.org/ontologies/lox#TGTDLT">
        <rdf:type rdf:resource="http://www.sisostds.org/ontologies/C2SIM#TaskActionCode"/>
        <rdfs:comment>Target dilution: To minimize the probability of acquisition of real targets by creating false targets in the vicinity of real targets by means</rdfs:comment>
    </owl:NamedIndividual>
    


    <!-- http://www.sisostds.org/ontologies/lox#THREAT -->

    <owl:NamedIndividual rdf:about="http://www.sisostds.org/ontologies/lox#THREAT">
        <rdf:type rdf:resource="http://www.sisostds.org/ontologies/C2SIM#TaskActionCode"/>
        <rdfs:comment>Documentation: 		
						To menace the enemy by manoeuvre or action.	
					; Appinfo DisplayValue as &quot;Threaten&quot;</rdfs:comment>
        <rdfs:comment>Threaten: To menace the enemy by manoeuvre or action.</rdfs:comment>
    </owl:NamedIndividual>
    


    <!-- http://www.sisostds.org/ontologies/lox#TOWTGT -->

    <owl:NamedIndividual rdf:about="http://www.sisostds.org/ontologies/lox#TOWTGT">
        <rdf:type rdf:resource="http://www.sisostds.org/ontologies/C2SIM#TaskActionCode"/>
        <rdfs:comment>Tow, target: To tow a target used for gunnery practice.</rdfs:comment>
    </owl:NamedIndividual>
    


    <!-- http://www.sisostds.org/ontologies/lox#TPL -->

    <owl:NamedIndividual rdf:about="http://www.sisostds.org/ontologies/lox#TPL">
        <rdf:type rdf:resource="http://www.sisostds.org/ontologies/lox#TaskFunctionalAssociationCode"/>
        <rdfs:comment>Is a template for: The subject ACTION constitutes an example that the object ACTION should conform to.</rdfs:comment>
    </owl:NamedIndividual>
    


    <!-- http://www.sisostds.org/ontologies/lox#TRAIN -->

    <owl:NamedIndividual rdf:about="http://www.sisostds.org/ontologies/lox#TRAIN">
        <rdf:type rdf:resource="http://www.sisostds.org/ontologies/C2SIM#TaskActionCode"/>
        <rdfs:comment>Train: To develop, maintain or improve the readiness of individuals or units.</rdfs:comment>
    </owl:NamedIndividual>
    


    <!-- http://www.sisostds.org/ontologies/lox#TRANOP -->

    <owl:NamedIndividual rdf:about="http://www.sisostds.org/ontologies/lox#TRANOP">
        <rdf:type rdf:resource="http://www.sisostds.org/ontologies/C2SIM#TaskActionCode"/>
        <rdfs:comment>Train, operations: Training operations or exercises. This training includes: a. delivery of personnel and equipment; b. Assault operations; c.</rdfs:comment>
    </owl:NamedIndividual>
    


    <!-- http://www.sisostds.org/ontologies/lox#TRANS -->

    <owl:NamedIndividual rdf:about="http://www.sisostds.org/ontologies/lox#TRANS">
        <rdf:type rdf:resource="http://www.sisostds.org/ontologies/C2SIM#TaskActionCode"/>
        <rdfs:comment>Transport: To move assets using any means by sea, land or air to a specified objective.</rdfs:comment>
    </owl:NamedIndividual>
    


    <!-- http://www.sisostds.org/ontologies/lox#TRNSAA -->

    <owl:NamedIndividual rdf:about="http://www.sisostds.org/ontologies/lox#TRNSAA">
        <rdf:type rdf:resource="http://www.sisostds.org/ontologies/C2SIM#TaskActionCode"/>
        <rdfs:comment>Transport, assault airland: To transport cargo and/or passengers delivered by air-landing the aircraft to a combat zone.</rdfs:comment>
    </owl:NamedIndividual>
    


    <!-- http://www.sisostds.org/ontologies/lox#TRVRS -->

    <owl:NamedIndividual rdf:about="http://www.sisostds.org/ontologies/lox#TRVRS">
        <rdf:type rdf:resource="http://www.sisostds.org/ontologies/C2SIM#TaskActionCode"/>
        <rdfs:comment>Traverse: To travel over a designated route.</rdfs:comment>
    </owl:NamedIndividual>
    


    <!-- http://www.sisostds.org/ontologies/lox#TURN -->

    <owl:NamedIndividual rdf:about="http://www.sisostds.org/ontologies/lox#TURN">
        <rdf:type rdf:resource="http://www.sisostds.org/ontologies/C2SIM#TaskActionCode"/>
        <rdfs:comment>Documentation: 		
						To compel an enemy force to move from an avenue of approach or movement corridor to another.	
					; Appinfo DisplayValue as &quot;Turn&quot;</rdfs:comment>
        <rdfs:comment>Turn: To compel an enemy force to move from an avenue of approach or movement corridor to another.</rdfs:comment>
    </owl:NamedIndividual>
    


    <!-- http://www.sisostds.org/ontologies/lox#UAR -->

    <owl:NamedIndividual rdf:about="http://www.sisostds.org/ontologies/lox#UAR">
        <rdf:type rdf:resource="http://www.sisostds.org/ontologies/lox#TaskFunctionalAssociationCode"/>
        <rdfs:comment>Uses as a reference: The value that establishes a link between existing ACTIONs and new ACTIONs, be they requests, plans, or orders. (Note: The</rdfs:comment>
    </owl:NamedIndividual>
    


    <!-- http://www.sisostds.org/ontologies/lox#UNCONW -->

    <owl:NamedIndividual rdf:about="http://www.sisostds.org/ontologies/lox#UNCONW">
        <rdf:type rdf:resource="http://www.sisostds.org/ontologies/C2SIM#TaskActionCode"/>
        <rdfs:comment>Unconventional warfare: To conduct operations for military, political or economic purposes within an area occupied by the enemy and making use of</rdfs:comment>
    </owl:NamedIndividual>
    


    <!-- http://www.sisostds.org/ontologies/lox#UTILTY -->

    <owl:NamedIndividual rdf:about="http://www.sisostds.org/ontologies/lox#UTILTY">
        <rdf:type rdf:resource="http://www.sisostds.org/ontologies/C2SIM#TaskActionCode"/>
        <rdfs:comment>Utility flight: To conduct a flight in which the aircraft has the capability of performing multiple missions.</rdfs:comment>
    </owl:NamedIndividual>
    


    <!-- http://www.sisostds.org/ontologies/lox#VERIFY -->

    <owl:NamedIndividual rdf:about="http://www.sisostds.org/ontologies/lox#VERIFY">
        <rdf:type rdf:resource="http://www.sisostds.org/ontologies/C2SIM#TaskActionCode"/>
        <rdfs:comment>Verify: To testify to, to assert, to affirm or confirm, as true or certain.</rdfs:comment>
    </owl:NamedIndividual>
    


    <!-- http://www.sisostds.org/ontologies/lox#WDRPRS -->

    <owl:NamedIndividual rdf:about="http://www.sisostds.org/ontologies/lox#WDRPRS">
        <rdf:type rdf:resource="http://www.sisostds.org/ontologies/C2SIM#TaskActionCode"/>
        <rdfs:comment>Withdraw under pressure: To disengage from the enemy when the enemy has sufficient contact with friendly forces to interfere with the withdrawal.</rdfs:comment>
    </owl:NamedIndividual>
    


    <!-- http://www.sisostds.org/ontologies/lox#WITHDR -->

    <owl:NamedIndividual rdf:about="http://www.sisostds.org/ontologies/lox#WITHDR">
        <rdf:type rdf:resource="http://www.sisostds.org/ontologies/C2SIM#TaskActionCode"/>
        <rdfs:comment>Withdraw: To disengage a force in contact from an enemy force.</rdfs:comment>
    </owl:NamedIndividual>
    


    <!-- http://www.sisostds.org/ontologies/lox#WITNES -->

    <owl:NamedIndividual rdf:about="http://www.sisostds.org/ontologies/lox#WITNES">
        <rdf:type rdf:resource="http://www.sisostds.org/ontologies/C2SIM#TaskActionCode"/>
        <rdfs:comment>Witness: To observe an activity in an official capacity with a view of providing evidence.</rdfs:comment>
    </owl:NamedIndividual>
    


    <!-- http://www.sisostds.org/ontologies/lox#WLDWSL -->

    <owl:NamedIndividual rdf:about="http://www.sisostds.org/ontologies/lox#WLDWSL">
        <rdf:type rdf:resource="http://www.sisostds.org/ontologies/C2SIM#TaskActionCode"/>
        <rdfs:comment>Wild weasel: To identify, locate, and physically suppress or destroy ground based enemy air defence systems that employ sensors radiating</rdfs:comment>
    </owl:NamedIndividual>
    


    <!-- http://www.sisostds.org/ontologies/lox#WNDD -->

    <owl:NamedIndividual rdf:about="http://www.sisostds.org/ontologies/lox#WNDD">
        <rdfs:comment>Documentation: 		
						A casualty other than &quot;killed&quot; who has incurred an injury due to an external agent or cause.	
					; Appinfo DisplayValue as &quot;Wounded&quot;</rdfs:comment>
    </owl:NamedIndividual>
    


    <!-- http://www.sisostds.org/ontologies/smx#ACTION -->

    <owl:NamedIndividual rdf:about="http://www.sisostds.org/ontologies/smx#ACTION">
        <rdf:type rdf:resource="http://www.sisostds.org/ontologies/smx#MIPRequestCategoryCode"/>
        <rdfs:comment>Action: To discover the actions of an ACTION-OBJECTIVE (OBJECT-ITEM) by any means.</rdfs:comment>
    </owl:NamedIndividual>
    


    <!-- http://www.sisostds.org/ontologies/smx#ADMCON -->

    <owl:NamedIndividual rdf:about="http://www.sisostds.org/ontologies/smx#ADMCON">
        <rdf:type rdf:resource="http://www.sisostds.org/ontologies/smx#CommandRelationCode"/>
        <rdfs:comment>Has administrative control of: Direction or exercise of authority over subordinate or other organizations in respect to administrative matters such as personnel</rdfs:comment>
    </owl:NamedIndividual>
    


    <!-- http://www.sisostds.org/ontologies/smx#AFR -->

    <owl:NamedIndividual rdf:about="http://www.sisostds.org/ontologies/smx#AFR">
        <rdf:type rdf:resource="http://www.sisostds.org/ontologies/smx#HostilityStatusCode"/>
        <rdfs:comment>Assumed friend: An OBJECT-ITEM that is assumed to be a friend because of its characteristics, behaviour or origin.</rdfs:comment>
    </owl:NamedIndividual>
    


    <!-- http://www.sisostds.org/ontologies/smx#AG -->

    <owl:NamedIndividual rdf:about="http://www.sisostds.org/ontologies/smx#AG">
        <rdf:type rdf:resource="http://www.sisostds.org/ontologies/smx#EchelonCode"/>
        <rdfs:comment>Army group: The largest formation of land forces, normally comprising two or more armies or army corps under a designated commander.</rdfs:comment>
    </owl:NamedIndividual>
    


    <!-- http://www.sisostds.org/ontologies/smx#AHO -->

    <owl:NamedIndividual rdf:about="http://www.sisostds.org/ontologies/smx#AHO">
        <rdf:type rdf:resource="http://www.sisostds.org/ontologies/smx#HostilityStatusCode"/>
        <rdfs:comment>Assumed hostile: An indication that the OBJECT-ITEM in question is likely to belong to enemy forces.</rdfs:comment>
    </owl:NamedIndividual>
    


    <!-- http://www.sisostds.org/ontologies/smx#AIV -->

    <owl:NamedIndividual rdf:about="http://www.sisostds.org/ontologies/smx#AIV">
        <rdf:type rdf:resource="http://www.sisostds.org/ontologies/smx#HostilityStatusCode"/>
        <rdfs:comment>Assumed involved: An indication that the OBJECT-ITEM in question is likely to belong to involved forces different from own, allied and enemy</rdfs:comment>
    </owl:NamedIndividual>
    


    <!-- http://www.sisostds.org/ontologies/smx#ALTFOR -->

    <owl:NamedIndividual rdf:about="http://www.sisostds.org/ontologies/smx#ALTFOR">
        <rdf:type rdf:resource="http://www.sisostds.org/ontologies/smx#CommandRelationCode"/>
        <rdfs:comment>Has as alternate: The subject ORGANISATION has the object ORGANISATION as able to execute its functions should the need arise.</rdfs:comment>
    </owl:NamedIndividual>
    


    <!-- http://www.sisostds.org/ontologies/smx#ANT -->

    <owl:NamedIndividual rdf:about="http://www.sisostds.org/ontologies/smx#ANT">
        <rdf:type rdf:resource="http://www.sisostds.org/ontologies/smx#HostilityStatusCode"/>
        <rdfs:comment>Assumed neutral: An indication that the OBJECT-ITEM in question is likely to belong to neither own, allied, enemy or otherwise involved forces.</rdfs:comment>
    </owl:NamedIndividual>
    


    <!-- http://www.sisostds.org/ontologies/smx#ARMY -->

    <owl:NamedIndividual rdf:about="http://www.sisostds.org/ontologies/smx#ARMY">
        <rdf:type rdf:resource="http://www.sisostds.org/ontologies/smx#EchelonCode"/>
        <rdfs:comment>Army: A formation larger than an army corps but smaller than an army group. It usually consists of two or more army corps.</rdfs:comment>
    </owl:NamedIndividual>
    


    <!-- http://www.sisostds.org/ontologies/smx#ASGND -->

    <owl:NamedIndividual rdf:about="http://www.sisostds.org/ontologies/smx#ASGND">
        <rdf:type rdf:resource="http://www.sisostds.org/ontologies/smx#CommandRelationCode"/>
        <rdfs:comment>Has assigned: An object ORGANISATION is placed in the subject ORGANISATION where such placement is relatively permanent, and/or where such</rdfs:comment>
    </owl:NamedIndividual>
    


    <!-- http://www.sisostds.org/ontologies/smx#ASSOC -->

    <owl:NamedIndividual rdf:about="http://www.sisostds.org/ontologies/smx#ASSOC">
        <rdf:type rdf:resource="http://www.sisostds.org/ontologies/smx#MIPRequestCategoryCode"/>
        <rdfs:comment>Association: To discover the relation between two ACTION-OBJECTIVEs (OBJECT-ITEMs) by any means.</rdfs:comment>
    </owl:NamedIndividual>
    


    <!-- http://www.sisostds.org/ontologies/smx#ATPRCL -->

    <owl:NamedIndividual rdf:about="http://www.sisostds.org/ontologies/smx#ATPRCL">
        <rdf:type rdf:resource="http://www.sisostds.org/ontologies/smx#CommandRelationCode"/>
        <rdfs:comment>Has at priority call: A precedence applied to the task of an artillery unit to provide fire to a formation/unit on a guaranteed basis.</rdfs:comment>
    </owl:NamedIndividual>
    


    <!-- http://www.sisostds.org/ontologies/smx#ATTACH -->

    <owl:NamedIndividual rdf:about="http://www.sisostds.org/ontologies/smx#ATTACH">
        <rdf:type rdf:resource="http://www.sisostds.org/ontologies/smx#CommandRelationCode"/>
        <rdfs:comment>Has attached: The placement of units in an organisation where such placement is relatively temporary.</rdfs:comment>
    </owl:NamedIndividual>
    


    <!-- http://www.sisostds.org/ontologies/smx#BATGRP -->

    <owl:NamedIndividual rdf:about="http://www.sisostds.org/ontologies/smx#BATGRP">
        <rdf:type rdf:resource="http://www.sisostds.org/ontologies/smx#EchelonCode"/>
        <rdfs:comment>Battle group: An operational grouping which is based on either an infantry battalion or a tank regiment, each with at least a squadron or</rdfs:comment>
    </owl:NamedIndividual>
    


    <!-- http://www.sisostds.org/ontologies/smx#BDE -->

    <owl:NamedIndividual rdf:about="http://www.sisostds.org/ontologies/smx#BDE">
        <rdf:type rdf:resource="http://www.sisostds.org/ontologies/smx#EchelonCode"/>
        <rdfs:comment>Brigade: Unit composed of a headquarters and two or more battalions. It may be part of an army and be charged with only tactical functions,</rdfs:comment>
    </owl:NamedIndividual>
    


    <!-- http://www.sisostds.org/ontologies/smx#BDEGRP -->

    <owl:NamedIndividual rdf:about="http://www.sisostds.org/ontologies/smx#BDEGRP">
        <rdf:type rdf:resource="http://www.sisostds.org/ontologies/smx#EchelonCode"/>
        <rdfs:comment>Brigade group: An operational grouping which is based on an infantry or armoured brigade and which has elements of other supporting arms</rdfs:comment>
    </owl:NamedIndividual>
    


    <!-- http://www.sisostds.org/ontologies/smx#BN -->

    <owl:NamedIndividual rdf:about="http://www.sisostds.org/ontologies/smx#BN">
        <rdf:type rdf:resource="http://www.sisostds.org/ontologies/smx#EchelonCode"/>
        <rdfs:comment>Battalion: Unit composed of a headquarters and two or more companies or batteries. It may be part of a regiment and be charged with only</rdfs:comment>
    </owl:NamedIndividual>
    


    <!-- http://www.sisostds.org/ontologies/smx#BNG -->

    <owl:NamedIndividual rdf:about="http://www.sisostds.org/ontologies/smx#BNG">
        <rdf:type rdf:resource="http://www.sisostds.org/ontologies/smx#EchelonCode"/>
        <rdfs:comment>Battalion group: An operational grouping which is based on an infantry battalion and which has elements of other supporting arms and services</rdfs:comment>
    </owl:NamedIndividual>
    


    <!-- http://www.sisostds.org/ontologies/smx#BURN -->

    <owl:NamedIndividual rdf:about="http://www.sisostds.org/ontologies/smx#BURN">
        <rdf:type rdf:resource="http://www.sisostds.org/ontologies/C2SIM#DesiredEffectCode"/>
        <rdfs:comment>Burning: The ACTION objective is alight.</rdfs:comment>
    </owl:NamedIndividual>
    


    <!-- http://www.sisostds.org/ontologies/smx#CAPAB -->

    <owl:NamedIndividual rdf:about="http://www.sisostds.org/ontologies/smx#CAPAB">
        <rdf:type rdf:resource="http://www.sisostds.org/ontologies/smx#MIPRequestCategoryCode"/>
        <rdfs:comment>Capability: To discover the capability of an ACTION-OBJECTIVE (OBJECT-ITEM) by any means.</rdfs:comment>
    </owl:NamedIndividual>
    


    <!-- http://www.sisostds.org/ontologies/smx#CAPTRD -->

    <owl:NamedIndividual rdf:about="http://www.sisostds.org/ontologies/smx#CAPTRD">
        <rdf:type rdf:resource="http://www.sisostds.org/ontologies/C2SIM#DesiredEffectCode"/>
        <rdfs:comment>Captured: The ACTION objective has been captured or acquired and is available for use or interrogation/possession has been taken of</rdfs:comment>
    </owl:NamedIndividual>
    


    <!-- http://www.sisostds.org/ontologies/smx#CASP1 -->

    <owl:NamedIndividual rdf:about="http://www.sisostds.org/ontologies/smx#CASP1">
        <rdf:type rdf:resource="http://www.sisostds.org/ontologies/smx#CommandRelationCode"/>
        <rdfs:comment>Coordinated air/sea procedure one: An air-defence capable warship ORGANISATION is under tactical control of the Air Defence Commander.</rdfs:comment>
    </owl:NamedIndividual>
    


    <!-- http://www.sisostds.org/ontologies/smx#CASP2 -->

    <owl:NamedIndividual rdf:about="http://www.sisostds.org/ontologies/smx#CASP2">
        <rdf:type rdf:resource="http://www.sisostds.org/ontologies/smx#CommandRelationCode"/>
        <rdfs:comment>Coordinated air/sea procedure two: An air-defence capable warship ORGANISATION is working closely with the shore based Air Defence Commander. Tactical control</rdfs:comment>
    </owl:NamedIndividual>
    


    <!-- http://www.sisostds.org/ontologies/smx#CASP3 -->

    <owl:NamedIndividual rdf:about="http://www.sisostds.org/ontologies/smx#CASP3">
        <rdf:type rdf:resource="http://www.sisostds.org/ontologies/smx#CommandRelationCode"/>
        <rdfs:comment>Coordinated air/sea procedure three: A warship ORGANISATION that is unable to contribute to the Recognized Air Picture but requires receiving it normally via the</rdfs:comment>
    </owl:NamedIndividual>
    


    <!-- http://www.sisostds.org/ontologies/smx#CASP4 -->

    <owl:NamedIndividual rdf:about="http://www.sisostds.org/ontologies/smx#CASP4">
        <rdf:type rdf:resource="http://www.sisostds.org/ontologies/smx#CommandRelationCode"/>
        <rdfs:comment>Coordinated air/sea procedure four: An air-defence capable warship ORGANISATION, entering or berthed in a port or anchorage, which is able to assist the SOC/CAOC</rdfs:comment>
    </owl:NamedIndividual>
    


    <!-- http://www.sisostds.org/ontologies/smx#CLSSUP -->

    <owl:NamedIndividual rdf:about="http://www.sisostds.org/ontologies/smx#CLSSUP">
        <rdf:type rdf:resource="http://www.sisostds.org/ontologies/smx#CommandRelationCode"/>
        <rdfs:comment>Has in close support: That action of the supporting force against targets or objectives that are sufficiently near the supported force as to require</rdfs:comment>
    </owl:NamedIndividual>
    


    <!-- http://www.sisostds.org/ontologies/smx#COAUTH -->

    <owl:NamedIndividual rdf:about="http://www.sisostds.org/ontologies/smx#COAUTH">
        <rdf:type rdf:resource="http://www.sisostds.org/ontologies/smx#CommandRelationCode"/>
        <rdfs:comment>Has coordination authority over: The authority granted to a commander or individual assigned responsibility for coordinating specific functions or activities</rdfs:comment>
    </owl:NamedIndividual>
    


    <!-- http://www.sisostds.org/ontologies/smx#COMD -->

    <owl:NamedIndividual rdf:about="http://www.sisostds.org/ontologies/smx#COMD">
        <rdf:type rdf:resource="http://www.sisostds.org/ontologies/smx#CommandRelationCode"/>
        <rdfs:comment>Has full command of: The military authority and responsibility of a superior officer to issue orders to subordinates.</rdfs:comment>
    </owl:NamedIndividual>
    


    <!-- http://www.sisostds.org/ontologies/smx#CONS -->

    <owl:NamedIndividual rdf:about="http://www.sisostds.org/ontologies/smx#CONS">
        <rdf:type rdf:resource="http://www.sisostds.org/ontologies/C2SIM#DesiredEffectCode"/>
        <rdfs:comment>Consumed: The consumption of specified consumables or CONSUMABLE-MATERIEL-TYPEs.</rdfs:comment>
    </owl:NamedIndividual>
    


    <!-- http://www.sisostds.org/ontologies/smx#CORPS -->

    <owl:NamedIndividual rdf:about="http://www.sisostds.org/ontologies/smx#CORPS">
        <rdf:type rdf:resource="http://www.sisostds.org/ontologies/smx#EchelonCode"/>
        <rdfs:comment>Corps: A formation larger than a division but smaller than an army or army group. It usually consists to two or more divisions together</rdfs:comment>
    </owl:NamedIndividual>
    


    <!-- http://www.sisostds.org/ontologies/smx#COY -->

    <owl:NamedIndividual rdf:about="http://www.sisostds.org/ontologies/smx#COY">
        <rdf:type rdf:resource="http://www.sisostds.org/ontologies/smx#EchelonCode"/>
        <rdfs:comment>Company: Basic administrative and tactical unit in most arms and services of the Army. A company is on a command level below a battalion</rdfs:comment>
    </owl:NamedIndividual>
    


    <!-- http://www.sisostds.org/ontologies/smx#COYG -->

    <owl:NamedIndividual rdf:about="http://www.sisostds.org/ontologies/smx#COYG">
        <rdf:type rdf:resource="http://www.sisostds.org/ontologies/smx#EchelonCode"/>
        <rdfs:comment>Company group: An operational grouping which is based on either an infantry company or a tank company, which has elements of other supporting</rdfs:comment>
    </owl:NamedIndividual>
    


    <!-- http://www.sisostds.org/ontologies/smx#DETACH -->

    <owl:NamedIndividual rdf:about="http://www.sisostds.org/ontologies/smx#DETACH">
        <rdf:type rdf:resource="http://www.sisostds.org/ontologies/smx#CommandRelationCode"/>
        <rdfs:comment>Has detached: The subject ORGANISATION has the object ORGANISATION separated from its main organisation for duty elsewhere.</rdfs:comment>
    </owl:NamedIndividual>
    


    <!-- http://www.sisostds.org/ontologies/smx#DETD -->

    <owl:NamedIndividual rdf:about="http://www.sisostds.org/ontologies/smx#DETD">
        <rdf:type rdf:resource="http://www.sisostds.org/ontologies/smx#ReinforcedReducedType"/>
    </owl:NamedIndividual>
    


    <!-- http://www.sisostds.org/ontologies/smx#DIRSUP -->

    <owl:NamedIndividual rdf:about="http://www.sisostds.org/ontologies/smx#DIRSUP">
        <rdf:type rdf:resource="http://www.sisostds.org/ontologies/smx#CommandRelationCode"/>
        <rdfs:comment>Has in direct support: The support provided by a unit not attached to or under command of the supported unit or formation, but required to give priority</rdfs:comment>
    </owl:NamedIndividual>
    


    <!-- http://www.sisostds.org/ontologies/smx#DIV -->

    <owl:NamedIndividual rdf:about="http://www.sisostds.org/ontologies/smx#DIV">
        <rdf:type rdf:resource="http://www.sisostds.org/ontologies/smx#EchelonCode"/>
        <rdfs:comment>Division: A tactical unit/formation that is a major administrative and tactical unit/formation that combines in itself the necessary</rdfs:comment>
    </owl:NamedIndividual>
    


    <!-- http://www.sisostds.org/ontologies/smx#DSTRYK -->

    <owl:NamedIndividual rdf:about="http://www.sisostds.org/ontologies/smx#DSTRYK">
        <rdf:type rdf:resource="http://www.sisostds.org/ontologies/C2SIM#DesiredEffectCode"/>
        <rdfs:comment>Destroyed (K-kill): Cannot function as intended nor be repaired or restored to an operational status.</rdfs:comment>
    </owl:NamedIndividual>
    


    <!-- http://www.sisostds.org/ontologies/smx#FAKER -->

    <owl:NamedIndividual rdf:about="http://www.sisostds.org/ontologies/smx#FAKER">
        <rdf:type rdf:resource="http://www.sisostds.org/ontologies/smx#HostilityStatusCode"/>
        <rdfs:comment>Faker: An OBJECT-ITEM that is a friendly aircraft simulating a hostile aircraft in an air defence exercise.</rdfs:comment>
    </owl:NamedIndividual>
    


    <!-- http://www.sisostds.org/ontologies/smx#FKIL -->

    <owl:NamedIndividual rdf:about="http://www.sisostds.org/ontologies/smx#FKIL">
        <rdf:type rdf:resource="http://www.sisostds.org/ontologies/C2SIM#DesiredEffectCode"/>
        <rdfs:comment>Firepower kill (F-kill): The destruction of a vehicle (or system&apos;s) primary weapon system.</rdfs:comment>
    </owl:NamedIndividual>
    


    <!-- http://www.sisostds.org/ontologies/smx#FLEET -->

    <owl:NamedIndividual rdf:about="http://www.sisostds.org/ontologies/smx#FLEET">
        <rdf:type rdf:resource="http://www.sisostds.org/ontologies/smx#EchelonCode"/>
        <rdfs:comment>Fleet: An organisation of ships, aircraft, Marine forces, and shore-based fleet activities all under the command of a commander or</rdfs:comment>
    </owl:NamedIndividual>
    


    <!-- http://www.sisostds.org/ontologies/smx#FLIG -->

    <owl:NamedIndividual rdf:about="http://www.sisostds.org/ontologies/smx#FLIG">
        <rdf:type rdf:resource="http://www.sisostds.org/ontologies/C2SIM#DesiredEffectCode"/>
        <rdfs:comment>Forced to flee: The setting to flight of a PERSON or PERSON-TYPEs from their present location.</rdfs:comment>
    </owl:NamedIndividual>
    


    <!-- http://www.sisostds.org/ontologies/smx#FLIGHT -->

    <owl:NamedIndividual rdf:about="http://www.sisostds.org/ontologies/smx#FLIGHT">
        <rdf:type rdf:resource="http://www.sisostds.org/ontologies/smx#EchelonCode"/>
        <rdfs:comment>Flight: A specified group of aircraft engaged in a common mission.</rdfs:comment>
    </owl:NamedIndividual>
    


    <!-- http://www.sisostds.org/ontologies/smx#FORCE -->

    <owl:NamedIndividual rdf:about="http://www.sisostds.org/ontologies/smx#FORCE">
        <rdf:type rdf:resource="http://www.sisostds.org/ontologies/smx#CommandRelationCode"/>
        <rdfs:comment>Reinforces: The subject ORGANISATION is made available to the object ORGANISATION commander for the purpose of supplementing an in-place</rdfs:comment>
    </owl:NamedIndividual>
    


    <!-- http://www.sisostds.org/ontologies/smx#FR -->

    <owl:NamedIndividual rdf:about="http://www.sisostds.org/ontologies/smx#FR">
        <rdf:type rdf:resource="http://www.sisostds.org/ontologies/smx#HostilityStatusCode"/>
        <rdfs:comment>Friend: An OBJECT-ITEM that belongs to a declared friendly nation.</rdfs:comment>
    </owl:NamedIndividual>
    


    <!-- http://www.sisostds.org/ontologies/smx#GENSRI -->

    <owl:NamedIndividual rdf:about="http://www.sisostds.org/ontologies/smx#GENSRI">
        <rdf:type rdf:resource="http://www.sisostds.org/ontologies/smx#CommandRelationCode"/>
        <rdfs:comment>Has in general support reinforcing: General Support Reinforcing artillery has the mission of supporting the forces as a whole and, on a secondary basis, of providing</rdfs:comment>
    </owl:NamedIndividual>
    


    <!-- http://www.sisostds.org/ontologies/smx#GENSUP -->

    <owl:NamedIndividual rdf:about="http://www.sisostds.org/ontologies/smx#GENSUP">
        <rdf:type rdf:resource="http://www.sisostds.org/ontologies/smx#CommandRelationCode"/>
        <rdfs:comment>Has in general support: The support that is given to the supported force as a whole and not to any particular subdivision thereof.</rdfs:comment>
    </owl:NamedIndividual>
    


    <!-- http://www.sisostds.org/ontologies/smx#HO -->

    <owl:NamedIndividual rdf:about="http://www.sisostds.org/ontologies/smx#HO">
        <rdf:type rdf:resource="http://www.sisostds.org/ontologies/smx#HostilityStatusCode"/>
        <rdfs:comment>Hostile: An OBJECT-ITEM that is positively identified as enemy.</rdfs:comment>
    </owl:NamedIndividual>
    


    <!-- http://www.sisostds.org/ontologies/smx#HOLDNG -->

    <owl:NamedIndividual rdf:about="http://www.sisostds.org/ontologies/smx#HOLDNG">
        <rdf:type rdf:resource="http://www.sisostds.org/ontologies/smx#MIPRequestCategoryCode"/>
        <rdfs:comment>Holding: To discover the holding of an ACTION-OBJECTIVE (OBJECT-ITEM) by any means.</rdfs:comment>
    </owl:NamedIndividual>
    


    <!-- http://www.sisostds.org/ontologies/smx#HOSTIL -->

    <owl:NamedIndividual rdf:about="http://www.sisostds.org/ontologies/smx#HOSTIL">
        <rdf:type rdf:resource="http://www.sisostds.org/ontologies/smx#MIPRequestCategoryCode"/>
        <rdfs:comment>Hostility: To recognise the friendly or enemy character of an ACTION-OBJECTIVE (OBJECT-ITEM) by any means.</rdfs:comment>
    </owl:NamedIndividual>
    


    <!-- http://www.sisostds.org/ontologies/smx#HSCPTD -->

    <owl:NamedIndividual rdf:about="http://www.sisostds.org/ontologies/smx#HSCPTD">
        <rdf:type rdf:resource="http://www.sisostds.org/ontologies/smx#CommandRelationCode"/>
        <rdfs:comment>Has captured: The subject ORGANISATION has taken possession, as a result of forceful means, of the object ORGANISATION.</rdfs:comment>
    </owl:NamedIndividual>
    


    <!-- http://www.sisostds.org/ontologies/smx#HSNSPT -->

    <owl:NamedIndividual rdf:about="http://www.sisostds.org/ontologies/smx#HSNSPT">
        <rdf:type rdf:resource="http://www.sisostds.org/ontologies/smx#CommandRelationCode"/>
        <rdfs:comment>Has in support of: Term designating the support provided to another unit, formation or organisation while remaining under the initial command.</rdfs:comment>
    </owl:NamedIndividual>
    


    <!-- http://www.sisostds.org/ontologies/smx#IDNT -->

    <owl:NamedIndividual rdf:about="http://www.sisostds.org/ontologies/smx#IDNT">
        <rdf:type rdf:resource="http://www.sisostds.org/ontologies/C2SIM#DesiredEffectCode"/>
        <rdfs:comment>Identified: The ACTION objective has been either identified (i.e., classified as friend/foe/neutral) or recognised (i.e., the unit designation</rdfs:comment>
    </owl:NamedIndividual>
    


    <!-- http://www.sisostds.org/ontologies/smx#ILLUMN -->

    <owl:NamedIndividual rdf:about="http://www.sisostds.org/ontologies/smx#ILLUMN">
        <rdf:type rdf:resource="http://www.sisostds.org/ontologies/C2SIM#DesiredEffectCode"/>
        <rdfs:comment>Illuminated: The temporary supply of IR or white-light illumination (usually in coordination with direct or indirect fire).</rdfs:comment>
    </owl:NamedIndividual>
    


    <!-- http://www.sisostds.org/ontologies/smx#INTREC -->

    <owl:NamedIndividual rdf:about="http://www.sisostds.org/ontologies/smx#INTREC">
        <rdf:type rdf:resource="http://www.sisostds.org/ontologies/C2SIM#DesiredEffectCode"/>
        <rdfs:comment>Intact but unrecoverable: An equipment lost in an area unsuitable for recovery due to political, military or geographic/environmental considerations.</rdfs:comment>
    </owl:NamedIndividual>
    


    <!-- http://www.sisostds.org/ontologies/smx#ISCPER -->

    <owl:NamedIndividual rdf:about="http://www.sisostds.org/ontologies/smx#ISCPER">
        <rdf:type rdf:resource="http://www.sisostds.org/ontologies/smx#CommandRelationCode"/>
        <rdfs:comment>Is co-operating with: Working or acting together.</rdfs:comment>
    </owl:NamedIndividual>
    


    <!-- http://www.sisostds.org/ontologies/smx#IV -->

    <owl:NamedIndividual rdf:about="http://www.sisostds.org/ontologies/smx#IV">
        <rdf:type rdf:resource="http://www.sisostds.org/ontologies/smx#HostilityStatusCode"/>
        <rdfs:comment>Involved: An indication that the OBJECT-ITEM in question belongs to involved forces different from own, allied and enemy forces.</rdfs:comment>
    </owl:NamedIndividual>
    


    <!-- http://www.sisostds.org/ontologies/smx#JOKER -->

    <owl:NamedIndividual rdf:about="http://www.sisostds.org/ontologies/smx#JOKER">
        <rdf:type rdf:resource="http://www.sisostds.org/ontologies/smx#HostilityStatusCode"/>
        <rdfs:comment>Joker: An OBJECT-ITEM that is acting as a suspect track for exercise purposes only.</rdfs:comment>
    </owl:NamedIndividual>
    


    <!-- http://www.sisostds.org/ontologies/smx#KILL -->

    <owl:NamedIndividual rdf:about="http://www.sisostds.org/ontologies/smx#KILL">
        <rdf:type rdf:resource="http://www.sisostds.org/ontologies/C2SIM#DesiredEffectCode"/>
        <rdfs:comment>Killed: A casualty who is killed outright or dies as a result of wounds, disease or other injuries.</rdfs:comment>
    </owl:NamedIndividual>
    


    <!-- http://www.sisostds.org/ontologies/smx#LDAM -->

    <owl:NamedIndividual rdf:about="http://www.sisostds.org/ontologies/smx#LDAM">
        <rdf:type rdf:resource="http://www.sisostds.org/ontologies/C2SIM#DesiredEffectCode"/>
        <rdfs:comment>Light damage: The subjective categorisation of the physical effect of an ACTION on buildings, infrastructure and/or equipment by a reporting</rdfs:comment>
    </owl:NamedIndividual>
    


    <!-- http://www.sisostds.org/ontologies/smx#LGTRST -->

    <owl:NamedIndividual rdf:about="http://www.sisostds.org/ontologies/smx#LGTRST">
        <rdf:type rdf:resource="http://www.sisostds.org/ontologies/C2SIM#DesiredEffectCode"/>
        <rdfs:comment>Light resistance: The ACTION-OBJECTIVE reacted against the ACTION using light physical violence.</rdfs:comment>
    </owl:NamedIndividual>
    


    <!-- http://www.sisostds.org/ontologies/smx#LOCATN -->

    <owl:NamedIndividual rdf:about="http://www.sisostds.org/ontologies/smx#LOCATN">
        <rdf:type rdf:resource="http://www.sisostds.org/ontologies/smx#MIPRequestCategoryCode"/>
        <rdfs:comment>Location: To discover the location of an ACTION-OBJECTIVE (OBJECT-ITEM) by any means.</rdfs:comment>
    </owl:NamedIndividual>
    


    <!-- http://www.sisostds.org/ontologies/smx#LOGCON -->

    <owl:NamedIndividual rdf:about="http://www.sisostds.org/ontologies/smx#LOGCON">
        <rdf:type rdf:resource="http://www.sisostds.org/ontologies/smx#CommandRelationCode"/>
        <rdfs:comment>Has logistical control of: Logistic Control (LOGCON) is that authority granted to a Commander over assigned logistics units and organizations in the</rdfs:comment>
    </owl:NamedIndividual>
    


    <!-- http://www.sisostds.org/ontologies/smx#LOST -->

    <owl:NamedIndividual rdf:about="http://www.sisostds.org/ontologies/smx#LOST">
        <rdf:type rdf:resource="http://www.sisostds.org/ontologies/C2SIM#DesiredEffectCode"/>
        <rdfs:comment>Lost: The object is no longer available for military operations.</rdfs:comment>
    </owl:NamedIndividual>
    


    <!-- http://www.sisostds.org/ontologies/smx#MKIL -->

    <owl:NamedIndividual rdf:about="http://www.sisostds.org/ontologies/smx#MKIL">
        <rdf:type rdf:resource="http://www.sisostds.org/ontologies/C2SIM#DesiredEffectCode"/>
        <rdfs:comment>Mobility kill (M-kill): The rendering of a vehicle as being temporarily or permanently incapable of tactical movement.</rdfs:comment>
    </owl:NamedIndividual>
    


    <!-- http://www.sisostds.org/ontologies/smx#MODDAM -->

    <owl:NamedIndividual rdf:about="http://www.sisostds.org/ontologies/smx#MODDAM">
        <rdf:type rdf:resource="http://www.sisostds.org/ontologies/C2SIM#DesiredEffectCode"/>
        <rdfs:comment>Moderate damage: The subjective categorisation of the physical effect of an ACTION on buildings, infrastructure and/or equipment by a reporting</rdfs:comment>
    </owl:NamedIndividual>
    


    <!-- http://www.sisostds.org/ontologies/smx#MOPS -->

    <owl:NamedIndividual rdf:about="http://www.sisostds.org/ontologies/smx#MOPS">
        <rdf:type rdf:resource="http://www.sisostds.org/ontologies/smx#UnitOperationalStatusCode"/>
    </owl:NamedIndividual>
    


    <!-- http://www.sisostds.org/ontologies/smx#MUTSUP -->

    <owl:NamedIndividual rdf:about="http://www.sisostds.org/ontologies/smx#MUTSUP">
        <rdf:type rdf:resource="http://www.sisostds.org/ontologies/smx#CommandRelationCode"/>
        <rdfs:comment>Has in mutual support: That support which units render each other against an enemy, because of their assigned tasks, their position relative to each</rdfs:comment>
    </owl:NamedIndividual>
    


    <!-- http://www.sisostds.org/ontologies/smx#NBCAS -->

    <owl:NamedIndividual rdf:about="http://www.sisostds.org/ontologies/smx#NBCAS">
        <rdf:type rdf:resource="http://www.sisostds.org/ontologies/C2SIM#DesiredEffectCode"/>
        <rdfs:comment>Non-battle casualty: A person who is not a battle casualty, but who is lost to his organisation by reason of disease or injury, including persons</rdfs:comment>
    </owl:NamedIndividual>
    


    <!-- http://www.sisostds.org/ontologies/smx#NEUTRL -->

    <owl:NamedIndividual rdf:about="http://www.sisostds.org/ontologies/smx#NEUTRL">
        <rdf:type rdf:resource="http://www.sisostds.org/ontologies/smx#HostilityStatusCode"/>
        <rdfs:comment>Neutral: An OBJECT-ITEM whose characteristics, behaviour, origin or nationality indicate that it is neither supporting friendly nor</rdfs:comment>
    </owl:NamedIndividual>
    


    <!-- http://www.sisostds.org/ontologies/smx#NKN -->

    <owl:NamedIndividual rdf:about="http://www.sisostds.org/ontologies/smx#NKN">
        <rdf:type rdf:resource="http://www.sisostds.org/ontologies/C2SIM#DesiredEffectCode"/>
        <rdf:type rdf:resource="http://www.sisostds.org/ontologies/smx#EchelonCode"/>
        <rdf:type rdf:resource="http://www.sisostds.org/ontologies/smx#UnitOperationalStatusCode"/>
        <rdfs:comment>Not known: It is not possible to determine which value is most applicable.</rdfs:comment>
    </owl:NamedIndividual>
    


    <!-- http://www.sisostds.org/ontologies/smx#NOP -->

    <owl:NamedIndividual rdf:about="http://www.sisostds.org/ontologies/smx#NOP">
        <rdf:type rdf:resource="http://www.sisostds.org/ontologies/smx#UnitOperationalStatusCode"/>
    </owl:NamedIndividual>
    


    <!-- http://www.sisostds.org/ontologies/smx#NORM -->

    <owl:NamedIndividual rdf:about="http://www.sisostds.org/ontologies/smx#NORM">
        <rdf:type rdf:resource="http://www.sisostds.org/ontologies/smx#ReinforcedReducedType"/>
    </owl:NamedIndividual>
    


    <!-- http://www.sisostds.org/ontologies/smx#NORSTN -->

    <owl:NamedIndividual rdf:about="http://www.sisostds.org/ontologies/smx#NORSTN">
        <rdf:type rdf:resource="http://www.sisostds.org/ontologies/C2SIM#DesiredEffectCode"/>
        <rdfs:comment>No resistance: The ACTION-OBJECTIVE did not react against the ACTION.</rdfs:comment>
    </owl:NamedIndividual>
    


    <!-- http://www.sisostds.org/ontologies/smx#NOS -->

    <owl:NamedIndividual rdf:about="http://www.sisostds.org/ontologies/smx#NOS">
        <rdf:type rdf:resource="http://www.sisostds.org/ontologies/C2SIM#DesiredEffectCode"/>
        <rdf:type rdf:resource="http://www.sisostds.org/ontologies/smx#EchelonCode"/>
        <rdfs:comment>Not otherwise specified: The appropriate value is not in the set of specified values.</rdfs:comment>
    </owl:NamedIndividual>
    


    <!-- http://www.sisostds.org/ontologies/smx#NTF -->

    <owl:NamedIndividual rdf:about="http://www.sisostds.org/ontologies/smx#NTF">
        <rdf:type rdf:resource="http://www.sisostds.org/ontologies/smx#EchelonCode"/>
        <rdfs:comment>Task force, Navy: A component of a fleet organized by the commander of a task fleet or higher authority for the accomplishment of a specific</rdfs:comment>
    </owl:NamedIndividual>
    


    <!-- http://www.sisostds.org/ontologies/smx#NTG -->

    <owl:NamedIndividual rdf:about="http://www.sisostds.org/ontologies/smx#NTG">
        <rdf:type rdf:resource="http://www.sisostds.org/ontologies/smx#EchelonCode"/>
        <rdfs:comment>Task group, Navy: A component of a task force organized by the commander of the task force or higher authority for accomplishing specific tasks.</rdfs:comment>
    </owl:NamedIndividual>
    


    <!-- http://www.sisostds.org/ontologies/smx#NTU -->

    <owl:NamedIndividual rdf:about="http://www.sisostds.org/ontologies/smx#NTU">
        <rdf:type rdf:resource="http://www.sisostds.org/ontologies/smx#EchelonCode"/>
        <rdfs:comment>Task unit, Navy: A component of a task group organized by the commander of a task group or higher authority for accomplishing specific tasks.</rdfs:comment>
    </owl:NamedIndividual>
    


    <!-- http://www.sisostds.org/ontologies/smx#NUTRLD -->

    <owl:NamedIndividual rdf:about="http://www.sisostds.org/ontologies/smx#NUTRLD">
        <rdf:type rdf:resource="http://www.sisostds.org/ontologies/C2SIM#DesiredEffectCode"/>
        <rdfs:comment>Neutralized: The rendering of the ACTION objective temporarily ineffective by the infliction of significant casualties (norm for indirect</rdfs:comment>
    </owl:NamedIndividual>
    


    <!-- http://www.sisostds.org/ontologies/smx#ONCALL -->

    <owl:NamedIndividual rdf:about="http://www.sisostds.org/ontologies/smx#ONCALL">
        <rdf:type rdf:resource="http://www.sisostds.org/ontologies/smx#CommandRelationCode"/>
        <rdfs:comment>Has on call: A term used to specify that a pre-arranged concentration, air strike or final protective fire may be called for.</rdfs:comment>
    </owl:NamedIndividual>
    


    <!-- http://www.sisostds.org/ontologies/smx#OPCOMD -->

    <owl:NamedIndividual rdf:about="http://www.sisostds.org/ontologies/smx#OPCOMD">
        <rdf:type rdf:resource="http://www.sisostds.org/ontologies/smx#CommandRelationCode"/>
        <rdfs:comment>Has operational command of: The authority granted to a commander to assign missions or tasks to subordinate commanders, to deploy units, to reassign forces,</rdfs:comment>
    </owl:NamedIndividual>
    


    <!-- http://www.sisostds.org/ontologies/smx#OPCON -->

    <owl:NamedIndividual rdf:about="http://www.sisostds.org/ontologies/smx#OPCON">
        <rdf:type rdf:resource="http://www.sisostds.org/ontologies/smx#CommandRelationCode"/>
        <rdfs:comment>Has operational control of: The authority delegated to a commander to direct forces assigned so that the commander may accomplish specific missions or</rdfs:comment>
    </owl:NamedIndividual>
    


    <!-- http://www.sisostds.org/ontologies/smx#OPR -->

    <owl:NamedIndividual rdf:about="http://www.sisostds.org/ontologies/smx#OPR">
        <rdf:type rdf:resource="http://www.sisostds.org/ontologies/smx#UnitOperationalStatusCode"/>
    </owl:NamedIndividual>
    


    <!-- http://www.sisostds.org/ontologies/smx#ORGANC -->

    <owl:NamedIndividual rdf:about="http://www.sisostds.org/ontologies/smx#ORGANC">
        <rdf:type rdf:resource="http://www.sisostds.org/ontologies/smx#CommandRelationCode"/>
        <rdfs:comment>Has organic: The subject ORGANISATION normally has the object ORGANISATION under command in garrison.</rdfs:comment>
    </owl:NamedIndividual>
    


    <!-- http://www.sisostds.org/ontologies/smx#PENDNG -->

    <owl:NamedIndividual rdf:about="http://www.sisostds.org/ontologies/smx#PENDNG">
        <rdf:type rdf:resource="http://www.sisostds.org/ontologies/smx#HostilityStatusCode"/>
        <rdfs:comment>Pending: An OBJECT-ITEM for which identification is to be determined.</rdfs:comment>
    </owl:NamedIndividual>
    


    <!-- http://www.sisostds.org/ontologies/smx#PLT -->

    <owl:NamedIndividual rdf:about="http://www.sisostds.org/ontologies/smx#PLT">
        <rdf:type rdf:resource="http://www.sisostds.org/ontologies/smx#EchelonCode"/>
        <rdfs:comment>Platoon: Basic administrative and tactical unit in most arms and services of the Army.</rdfs:comment>
    </owl:NamedIndividual>
    


    <!-- http://www.sisostds.org/ontologies/smx#PRESNC -->

    <owl:NamedIndividual rdf:about="http://www.sisostds.org/ontologies/smx#PRESNC">
        <rdf:type rdf:resource="http://www.sisostds.org/ontologies/smx#MIPRequestCategoryCode"/>
        <rdfs:comment>Presence: To discover the manifestation of an ACTION-OBJECTIVE in the area of operational interest specified through another ACTION-OBJECTIVE</rdfs:comment>
    </owl:NamedIndividual>
    


    <!-- http://www.sisostds.org/ontologies/smx#REGION -->

    <owl:NamedIndividual rdf:about="http://www.sisostds.org/ontologies/smx#REGION">
        <rdf:type rdf:resource="http://www.sisostds.org/ontologies/smx#EchelonCode"/>
        <rdfs:comment>Region: A grouping of two or more Army groups.</rdfs:comment>
    </owl:NamedIndividual>
    


    <!-- http://www.sisostds.org/ontologies/smx#REIN -->

    <owl:NamedIndividual rdf:about="http://www.sisostds.org/ontologies/smx#REIN">
        <rdf:type rdf:resource="http://www.sisostds.org/ontologies/smx#ReinforcedReducedType"/>
    </owl:NamedIndividual>
    


    <!-- http://www.sisostds.org/ontologies/smx#REINFC -->

    <owl:NamedIndividual rdf:about="http://www.sisostds.org/ontologies/smx#REINFC">
        <rdf:type rdf:resource="http://www.sisostds.org/ontologies/smx#CommandRelationCode"/>
        <rdfs:comment>Has reinforcing: In artillery usage, a tactical mission in which one artillery unit augments the fire of another artillery unit.</rdfs:comment>
    </owl:NamedIndividual>
    


    <!-- http://www.sisostds.org/ontologies/smx#RESERV -->

    <owl:NamedIndividual rdf:about="http://www.sisostds.org/ontologies/smx#RESERV">
        <rdf:type rdf:resource="http://www.sisostds.org/ontologies/smx#CommandRelationCode"/>
        <rdfs:comment>Has in reserve: The object ORGANISATION constitutes a force that may be committed into combat only on the order of the commander of the subject</rdfs:comment>
    </owl:NamedIndividual>
    


    <!-- http://www.sisostds.org/ontologies/smx#RGT -->

    <owl:NamedIndividual rdf:about="http://www.sisostds.org/ontologies/smx#RGT">
        <rdf:type rdf:resource="http://www.sisostds.org/ontologies/smx#EchelonCode"/>
        <rdfs:comment>Regiment: Administrative and tactical unit, on a command level below a division or brigade and above a battalion, the entire organisation</rdfs:comment>
    </owl:NamedIndividual>
    


    <!-- http://www.sisostds.org/ontologies/smx#RIDT -->

    <owl:NamedIndividual rdf:about="http://www.sisostds.org/ontologies/smx#RIDT">
        <rdf:type rdf:resource="http://www.sisostds.org/ontologies/smx#ReinforcedReducedType"/>
    </owl:NamedIndividual>
    


    <!-- http://www.sisostds.org/ontologies/smx#ROLE -->

    <owl:NamedIndividual rdf:about="http://www.sisostds.org/ontologies/smx#ROLE">
        <rdf:type rdf:resource="http://www.sisostds.org/ontologies/smx#CommandRelationCode"/>
        <rdfs:comment>Plays the role of: The subject ORGANISATION plays the role of an object ORGANISATION.</rdfs:comment>
    </owl:NamedIndividual>
    


    <!-- http://www.sisostds.org/ontologies/smx#ReinforcementNKN -->

    <owl:NamedIndividual rdf:about="http://www.sisostds.org/ontologies/smx#ReinforcementNKN">
        <rdf:type rdf:resource="http://www.sisostds.org/ontologies/smx#ReinforcedReducedType"/>
    </owl:NamedIndividual>
    


    <!-- http://www.sisostds.org/ontologies/smx#SAME -->

    <owl:NamedIndividual rdf:about="http://www.sisostds.org/ontologies/smx#SAME">
        <rdf:type rdf:resource="http://www.sisostds.org/ontologies/smx#CommandRelationCode"/>
        <rdfs:comment>Is the same as: The subject ORGANISATION is deemed to be the same as the object ORGANISATION.</rdfs:comment>
    </owl:NamedIndividual>
    


    <!-- http://www.sisostds.org/ontologies/smx#SDAM -->

    <owl:NamedIndividual rdf:about="http://www.sisostds.org/ontologies/smx#SDAM">
        <rdf:type rdf:resource="http://www.sisostds.org/ontologies/C2SIM#DesiredEffectCode"/>
        <rdfs:comment>Severe damage: The subjective categorisation of the physical effect of an ACTION on buildings, infrastructure and/or equipment by a reporting</rdfs:comment>
    </owl:NamedIndividual>
    


    <!-- http://www.sisostds.org/ontologies/smx#SECT -->

    <owl:NamedIndividual rdf:about="http://www.sisostds.org/ontologies/smx#SECT">
        <rdf:type rdf:resource="http://www.sisostds.org/ontologies/smx#EchelonCode"/>
        <rdfs:comment>Section: A small tactical unit.</rdfs:comment>
    </owl:NamedIndividual>
    


    <!-- http://www.sisostds.org/ontologies/smx#SOPS -->

    <owl:NamedIndividual rdf:about="http://www.sisostds.org/ontologies/smx#SOPS">
        <rdf:type rdf:resource="http://www.sisostds.org/ontologies/smx#UnitOperationalStatusCode"/>
    </owl:NamedIndividual>
    


    <!-- http://www.sisostds.org/ontologies/smx#SPTAMM -->

    <owl:NamedIndividual rdf:about="http://www.sisostds.org/ontologies/smx#SPTAMM">
        <rdf:type rdf:resource="http://www.sisostds.org/ontologies/smx#CommandRelationCode"/>
        <rdfs:comment>Support services - ammunition: Supporting unit satisfies all ammunition resupply requirements of the supported unit including crew-served weapons and artillery.</rdfs:comment>
    </owl:NamedIndividual>
    


    <!-- http://www.sisostds.org/ontologies/smx#SPTENG -->

    <owl:NamedIndividual rdf:about="http://www.sisostds.org/ontologies/smx#SPTENG">
        <rdf:type rdf:resource="http://www.sisostds.org/ontologies/smx#CommandRelationCode"/>
        <rdfs:comment>Support services - engineering: Supporting unit satisfies engineering support requirements of the supported unit.</rdfs:comment>
    </owl:NamedIndividual>
    


    <!-- http://www.sisostds.org/ontologies/smx#SPTMED -->

    <owl:NamedIndividual rdf:about="http://www.sisostds.org/ontologies/smx#SPTMED">
        <rdf:type rdf:resource="http://www.sisostds.org/ontologies/smx#CommandRelationCode"/>
        <rdfs:comment>Support services - medical: Supporting unit satisfies medical requirements of the supported unit.</rdfs:comment>
    </owl:NamedIndividual>
    


    <!-- http://www.sisostds.org/ontologies/smx#SPTMVT -->

    <owl:NamedIndividual rdf:about="http://www.sisostds.org/ontologies/smx#SPTMVT">
        <rdf:type rdf:resource="http://www.sisostds.org/ontologies/smx#CommandRelationCode"/>
        <rdfs:comment>Support services - movement: Supporting unit coordinates and provides road credits for the movement of the supported unit.</rdfs:comment>
    </owl:NamedIndividual>
    


    <!-- http://www.sisostds.org/ontologies/smx#SPTPAR -->

    <owl:NamedIndividual rdf:about="http://www.sisostds.org/ontologies/smx#SPTPAR">
        <rdf:type rdf:resource="http://www.sisostds.org/ontologies/smx#CommandRelationCode"/>
        <rdfs:comment>Support services - per adm rpl: Supporting unit satisfies all personnel administration and replacement requirements of the supported unit.</rdfs:comment>
    </owl:NamedIndividual>
    


    <!-- http://www.sisostds.org/ontologies/smx#SPTPOL -->

    <owl:NamedIndividual rdf:about="http://www.sisostds.org/ontologies/smx#SPTPOL">
        <rdf:type rdf:resource="http://www.sisostds.org/ontologies/smx#CommandRelationCode"/>
        <rdfs:comment>Support services - POL: Supporting unit satisfies fuel/POL supply requirements of the supported unit.</rdfs:comment>
    </owl:NamedIndividual>
    


    <!-- http://www.sisostds.org/ontologies/smx#SPTPST -->

    <owl:NamedIndividual rdf:about="http://www.sisostds.org/ontologies/smx#SPTPST">
        <rdf:type rdf:resource="http://www.sisostds.org/ontologies/smx#CommandRelationCode"/>
        <rdfs:comment>Support services - postal: Supporting unit satisfies postal requirements of the supported unit.</rdfs:comment>
    </owl:NamedIndividual>
    


    <!-- http://www.sisostds.org/ontologies/smx#SPTRAT -->

    <owl:NamedIndividual rdf:about="http://www.sisostds.org/ontologies/smx#SPTRAT">
        <rdf:type rdf:resource="http://www.sisostds.org/ontologies/smx#CommandRelationCode"/>
        <rdfs:comment>Support services - rations: Supporting unit satisfies food replenishment requirements of the supported unit.</rdfs:comment>
    </owl:NamedIndividual>
    


    <!-- http://www.sisostds.org/ontologies/smx#SPTRRE -->

    <owl:NamedIndividual rdf:about="http://www.sisostds.org/ontologies/smx#SPTRRE">
        <rdf:type rdf:resource="http://www.sisostds.org/ontologies/smx#CommandRelationCode"/>
        <rdfs:comment>Support services - rep, rec, evc: Supporting unit satisfies 2nd and 3rd line repair, recovery and evacuation requirements of the supported unit.</rdfs:comment>
    </owl:NamedIndividual>
    


    <!-- http://www.sisostds.org/ontologies/smx#SPTSPL -->

    <owl:NamedIndividual rdf:about="http://www.sisostds.org/ontologies/smx#SPTSPL">
        <rdf:type rdf:resource="http://www.sisostds.org/ontologies/smx#CommandRelationCode"/>
        <rdfs:comment>Support services - supply: Supporting unit satisfies supply requirements of the supported unit.</rdfs:comment>
    </owl:NamedIndividual>
    


    <!-- http://www.sisostds.org/ontologies/smx#SPTTRN -->

    <owl:NamedIndividual rdf:about="http://www.sisostds.org/ontologies/smx#SPTTRN">
        <rdf:type rdf:resource="http://www.sisostds.org/ontologies/smx#CommandRelationCode"/>
        <rdfs:comment>Support services - transport: Supporting unit satisfies 2nd and 3rd line transport requirements of the supported unit.</rdfs:comment>
    </owl:NamedIndividual>
    


    <!-- http://www.sisostds.org/ontologies/smx#SQDRNA -->

    <owl:NamedIndividual rdf:about="http://www.sisostds.org/ontologies/smx#SQDRNA">
        <rdf:type rdf:resource="http://www.sisostds.org/ontologies/smx#EchelonCode"/>
        <rdfs:comment>Squadron, air: An administrative or tactical organisation normally but not necessarily composed of aircraft of the same type.</rdfs:comment>
    </owl:NamedIndividual>
    


    <!-- http://www.sisostds.org/ontologies/smx#SQDRNM -->

    <owl:NamedIndividual rdf:about="http://www.sisostds.org/ontologies/smx#SQDRNM">
        <rdf:type rdf:resource="http://www.sisostds.org/ontologies/smx#EchelonCode"/>
        <rdfs:comment>Squadron, maritime: An administrative or tactical organisation consisting of two or more divisions of ships, plus such additional ships as may</rdfs:comment>
    </owl:NamedIndividual>
    


    <!-- http://www.sisostds.org/ontologies/smx#SQUAD -->

    <owl:NamedIndividual rdf:about="http://www.sisostds.org/ontologies/smx#SQUAD">
        <rdf:type rdf:resource="http://www.sisostds.org/ontologies/smx#EchelonCode"/>
        <rdfs:comment>Squad: A small number of men, a subdivision or section of a company, formed for drill.</rdfs:comment>
    </owl:NamedIndividual>
    


    <!-- http://www.sisostds.org/ontologies/smx#STATUS -->

    <owl:NamedIndividual rdf:about="http://www.sisostds.org/ontologies/smx#STATUS">
        <rdf:type rdf:resource="http://www.sisostds.org/ontologies/smx#MIPRequestCategoryCode"/>
        <rdfs:comment>Status: To recognise the status of an ACTION-OBJECTIVE (OBJECT-ITEM) by any means.</rdfs:comment>
    </owl:NamedIndividual>
    


    <!-- http://www.sisostds.org/ontologies/smx#SUPRSD -->

    <owl:NamedIndividual rdf:about="http://www.sisostds.org/ontologies/smx#SUPRSD">
        <rdf:type rdf:resource="http://www.sisostds.org/ontologies/C2SIM#DesiredEffectCode"/>
        <rdfs:comment>Suppressed: Reduction of the effectiveness of the ACTION objective for a specific period or purpose (normally to prevent an enemy from</rdfs:comment>
    </owl:NamedIndividual>
    


    <!-- http://www.sisostds.org/ontologies/smx#SUSPCT -->

    <owl:NamedIndividual rdf:about="http://www.sisostds.org/ontologies/smx#SUSPCT">
        <rdf:type rdf:resource="http://www.sisostds.org/ontologies/smx#HostilityStatusCode"/>
        <rdfs:comment>Suspect: An OBJECT-ITEM that is potentially hostile because of its characteristics, behaviour or origin.</rdfs:comment>
    </owl:NamedIndividual>
    


    <!-- http://www.sisostds.org/ontologies/smx#TACCNT -->

    <owl:NamedIndividual rdf:about="http://www.sisostds.org/ontologies/smx#TACCNT">
        <rdf:type rdf:resource="http://www.sisostds.org/ontologies/smx#CommandRelationCode"/>
        <rdfs:comment>Has tactical control of: The detailed, and, usually, local direction and control of movements or manoeuvres necessary to accomplish missions or tasks</rdfs:comment>
    </owl:NamedIndividual>
    


    <!-- http://www.sisostds.org/ontologies/smx#TACCOM -->

    <owl:NamedIndividual rdf:about="http://www.sisostds.org/ontologies/smx#TACCOM">
        <rdf:type rdf:resource="http://www.sisostds.org/ontologies/smx#CommandRelationCode"/>
        <rdfs:comment>Has tactical command of: The authority delegated to a commander to assign tasks to forces under his command for the accomplishment of the mission assigned</rdfs:comment>
    </owl:NamedIndividual>
    


    <!-- http://www.sisostds.org/ontologies/smx#TEAM -->

    <owl:NamedIndividual rdf:about="http://www.sisostds.org/ontologies/smx#TEAM">
        <rdf:type rdf:resource="http://www.sisostds.org/ontologies/smx#EchelonCode"/>
        <rdfs:comment>Team/fire team/crew: Any unit smaller than a squad that will be denoted by a vehicle or weapon symbol in a graphical representation.</rdfs:comment>
    </owl:NamedIndividual>
    


    <!-- http://www.sisostds.org/ontologies/smx#TNOPS -->

    <owl:NamedIndividual rdf:about="http://www.sisostds.org/ontologies/smx#TNOPS">
        <rdf:type rdf:resource="http://www.sisostds.org/ontologies/smx#UnitOperationalStatusCode"/>
    </owl:NamedIndividual>
    


    <!-- http://www.sisostds.org/ontologies/smx#TSKELN -->

    <owl:NamedIndividual rdf:about="http://www.sisostds.org/ontologies/smx#TSKELN">
        <rdf:type rdf:resource="http://www.sisostds.org/ontologies/smx#EchelonCode"/>
        <rdfs:comment>Task element, Navy: A component of a task unit organized by the commander of the task unit or higher authority for accomplishing a specific task.</rdfs:comment>
    </owl:NamedIndividual>
    


    <!-- http://www.sisostds.org/ontologies/smx#TYPE -->

    <owl:NamedIndividual rdf:about="http://www.sisostds.org/ontologies/smx#TYPE">
        <rdf:type rdf:resource="http://www.sisostds.org/ontologies/smx#MIPRequestCategoryCode"/>
        <rdfs:comment>Type: To recognise the type of an ACTION-OBJECTIVE (OBJECT-ITEM) by any means.</rdfs:comment>
    </owl:NamedIndividual>
    


    <!-- http://www.sisostds.org/ontologies/smx#UNK -->

    <owl:NamedIndividual rdf:about="http://www.sisostds.org/ontologies/smx#UNK">
        <rdf:type rdf:resource="http://www.sisostds.org/ontologies/smx#HostilityStatusCode"/>
        <rdfs:comment>Unknown: An OBJECT-ITEM for which its hostility status information is not available.</rdfs:comment>
    </owl:NamedIndividual>
    


    <!-- http://www.sisostds.org/ontologies/smx#VLNRST -->

    <owl:NamedIndividual rdf:about="http://www.sisostds.org/ontologies/smx#VLNRST">
        <rdf:type rdf:resource="http://www.sisostds.org/ontologies/C2SIM#DesiredEffectCode"/>
        <rdfs:comment>Violent resistance: The ACTION-OBJECTIVE reacted against the ACTION using heavy physical violence.</rdfs:comment>
    </owl:NamedIndividual>
    


    <!-- http://www.sisostds.org/ontologies/smx#VRBPRT -->

    <owl:NamedIndividual rdf:about="http://www.sisostds.org/ontologies/smx#VRBPRT">
        <rdf:type rdf:resource="http://www.sisostds.org/ontologies/C2SIM#DesiredEffectCode"/>
        <rdfs:comment>Verbal protest: The ACTION-OBJECTIVE reacted against the ACTION using verbal abuse.</rdfs:comment>
    </owl:NamedIndividual>
    


    <!-- http://www.sisostds.org/ontologies/smx#WING -->

    <owl:NamedIndividual rdf:about="http://www.sisostds.org/ontologies/smx#WING">
        <rdf:type rdf:resource="http://www.sisostds.org/ontologies/smx#EchelonCode"/>
        <rdfs:comment>Wing: An aviation unit composed normally of one primary mission group and the necessary supporting organisations.</rdfs:comment>
    </owl:NamedIndividual>
    


    <!-- http://www.sisostds.org/ontologies/smx#WNDD -->

    <owl:NamedIndividual rdf:about="http://www.sisostds.org/ontologies/smx#WNDD">
        <rdf:type rdf:resource="http://www.sisostds.org/ontologies/C2SIM#DesiredEffectCode"/>
        <rdfs:comment>Wounded: A casualty other than &quot;killed&quot; who has incurred an injury due to an external agent or cause.</rdfs:comment>
    </owl:NamedIndividual>
    <rdf:Description>
        <owl:qualifiedCardinality rdf:datatype="http://www.w3.org/2001/XMLSchema#nonNegativeInteger">1</owl:qualifiedCardinality>
    </rdf:Description>
    <rdf:Description>
        <owl:maxQualifiedCardinality rdf:datatype="http://www.w3.org/2001/XMLSchema#nonNegativeInteger">1</owl:maxQualifiedCardinality>
    </rdf:Description>
    <rdf:Description>
        <owl:qualifiedCardinality rdf:datatype="http://www.w3.org/2001/XMLSchema#nonNegativeInteger">1</owl:qualifiedCardinality>
    </rdf:Description>
    <rdf:Description>
        <owl:minQualifiedCardinality rdf:datatype="http://www.w3.org/2001/XMLSchema#nonNegativeInteger">1</owl:minQualifiedCardinality>
    </rdf:Description>
    <rdf:Description>
        <owl:qualifiedCardinality rdf:datatype="http://www.w3.org/2001/XMLSchema#nonNegativeInteger">1</owl:qualifiedCardinality>
    </rdf:Description>
    <rdf:Description>
        <owl:qualifiedCardinality rdf:datatype="http://www.w3.org/2001/XMLSchema#nonNegativeInteger">1</owl:qualifiedCardinality>
    </rdf:Description>
    <rdf:Description>
        <owl:minQualifiedCardinality rdf:datatype="http://www.w3.org/2001/XMLSchema#nonNegativeInteger">1</owl:minQualifiedCardinality>
    </rdf:Description>
    <rdf:Description>
        <owl:qualifiedCardinality rdf:datatype="http://www.w3.org/2001/XMLSchema#nonNegativeInteger">1</owl:qualifiedCardinality>
    </rdf:Description>
    <rdf:Description>
        <owl:qualifiedCardinality rdf:datatype="http://www.w3.org/2001/XMLSchema#nonNegativeInteger">1</owl:qualifiedCardinality>
    </rdf:Description>
    <rdf:Description>
        <owl:qualifiedCardinality rdf:datatype="http://www.w3.org/2001/XMLSchema#nonNegativeInteger">1</owl:qualifiedCardinality>
    </rdf:Description>
    <rdf:Description>
        <owl:qualifiedCardinality rdf:datatype="http://www.w3.org/2001/XMLSchema#nonNegativeInteger">1</owl:qualifiedCardinality>
    </rdf:Description>
    <rdf:Description>
        <owl:qualifiedCardinality rdf:datatype="http://www.w3.org/2001/XMLSchema#nonNegativeInteger">1</owl:qualifiedCardinality>
    </rdf:Description>
    <rdf:Description>
        <owl:qualifiedCardinality rdf:datatype="http://www.w3.org/2001/XMLSchema#nonNegativeInteger">1</owl:qualifiedCardinality>
    </rdf:Description>
    <rdf:Description>
        <owl:qualifiedCardinality rdf:datatype="http://www.w3.org/2001/XMLSchema#nonNegativeInteger">1</owl:qualifiedCardinality>
    </rdf:Description>
    <rdf:Description>
        <owl:qualifiedCardinality rdf:datatype="http://www.w3.org/2001/XMLSchema#nonNegativeInteger">1</owl:qualifiedCardinality>
    </rdf:Description>
    <rdf:Description>
        <owl:qualifiedCardinality rdf:datatype="http://www.w3.org/2001/XMLSchema#nonNegativeInteger">1</owl:qualifiedCardinality>
    </rdf:Description>
    <rdf:Description>
        <owl:qualifiedCardinality rdf:datatype="http://www.w3.org/2001/XMLSchema#nonNegativeInteger">1</owl:qualifiedCardinality>
    </rdf:Description>
    <rdf:Description>
        <owl:qualifiedCardinality rdf:datatype="http://www.w3.org/2001/XMLSchema#nonNegativeInteger">1</owl:qualifiedCardinality>
    </rdf:Description>
    <rdf:Description>
        <owl:minQualifiedCardinality rdf:datatype="http://www.w3.org/2001/XMLSchema#nonNegativeInteger">0</owl:minQualifiedCardinality>
    </rdf:Description>
    <rdf:Description>
        <owl:qualifiedCardinality rdf:datatype="http://www.w3.org/2001/XMLSchema#nonNegativeInteger">1</owl:qualifiedCardinality>
    </rdf:Description>
    <rdf:Description>
        <owl:qualifiedCardinality rdf:datatype="http://www.w3.org/2001/XMLSchema#nonNegativeInteger">1</owl:qualifiedCardinality>
    </rdf:Description>
    <rdf:Description>
        <owl:minQualifiedCardinality rdf:datatype="http://www.w3.org/2001/XMLSchema#nonNegativeInteger">0</owl:minQualifiedCardinality>
    </rdf:Description>
    <rdf:Description>
        <owl:qualifiedCardinality rdf:datatype="http://www.w3.org/2001/XMLSchema#nonNegativeInteger">1</owl:qualifiedCardinality>
    </rdf:Description>
    <rdf:Description>
        <owl:qualifiedCardinality rdf:datatype="http://www.w3.org/2001/XMLSchema#nonNegativeInteger">1</owl:qualifiedCardinality>
    </rdf:Description>
    <rdf:Description>
        <owl:minQualifiedCardinality rdf:datatype="http://www.w3.org/2001/XMLSchema#nonNegativeInteger">0</owl:minQualifiedCardinality>
    </rdf:Description>
    


    <!-- 
    ///////////////////////////////////////////////////////////////////////////////////////
    //
    // Annotations
    //
    ///////////////////////////////////////////////////////////////////////////////////////
     -->

    <rdf:Description rdf:about="http://www.w3.org/2002/07/owl#Thing">
        <rdfs:comment>Superclass of all classes in this ontology.</rdfs:comment>
    </rdf:Description>
    


    <!-- 
    ///////////////////////////////////////////////////////////////////////////////////////
    //
    // General axioms
    //
    ///////////////////////////////////////////////////////////////////////////////////////
     -->

    <rdf:Description>
        <rdf:type rdf:resource="http://www.w3.org/2002/07/owl#AllDisjointClasses"/>
        <owl:members rdf:parseType="Collection">
            <rdf:Description rdf:about="http://www.sisostds.org/ontologies/C2SIM#DateTime"/>
            <rdf:Description rdf:about="http://www.sisostds.org/ontologies/C2SIM#Duration"/>
            <rdf:Description rdf:about="http://www.sisostds.org/ontologies/C2SIM#IntervalTime"/>
        </owl:members>
    </rdf:Description>
    <rdf:Description>
        <rdf:type rdf:resource="http://www.w3.org/2002/07/owl#AllDisjointClasses"/>
        <owl:members rdf:parseType="Collection">
            <rdf:Description rdf:about="http://www.sisostds.org/ontologies/C2SIM#DateTime"/>
            <rdf:Description rdf:about="http://www.sisostds.org/ontologies/C2SIM#RelativeTime"/>
            <rdf:Description rdf:about="http://www.sisostds.org/ontologies/C2SIM#SimulationTime"/>
        </owl:members>
    </rdf:Description>
</rdf:RDF>



<!-- Generated by the OWL API (version 4.5.9.2019-02-01T07:24:44Z) https://github.com/owlcs/owlapi -->

