<?xml version="1.0"?>
<rdf:RDF xmlns="http://www.sisostds.org/ontologies/lox#"
     xml:base="http://www.sisostds.org/ontologies/lox"
     xmlns:owl="http://www.w3.org/2002/07/owl#"
     xmlns:rdf="http://www.w3.org/1999/02/22-rdf-syntax-ns#"
     xmlns:xml="http://www.w3.org/XML/1998/namespace"
     xmlns:xsd="http://www.w3.org/2001/XMLSchema#"
     xmlns:rdfs="http://www.w3.org/2000/01/rdf-schema#">
    <owl:Ontology rdf:about="http://www.sisostds.org/ontologies/lox">
        <owl:imports rdf:resource="http://www.sisostds.org/ontologies/smx"/>
        <rdfs:comment>Version 1.0.0 SISO Standard, May 2020</rdfs:comment>
        <owl:versionInfo>C2SIM Land Operations Extension v1.0.0</owl:versionInfo>
    </owl:Ontology>
    


    <!-- 
    ///////////////////////////////////////////////////////////////////////////////////////
    //
    // Annotation properties
    //
    ///////////////////////////////////////////////////////////////////////////////////////
     -->

    


    <!-- http://www.w3.org/2002/07/owl#minQualifiedCardinality -->

    <owl:AnnotationProperty rdf:about="http://www.w3.org/2002/07/owl#minQualifiedCardinality"/>
    


    <!-- http://www.w3.org/2002/07/owl#qualifiedCardinality -->

    <owl:AnnotationProperty rdf:about="http://www.w3.org/2002/07/owl#qualifiedCardinality"/>
    


    <!-- 
    ///////////////////////////////////////////////////////////////////////////////////////
    //
    // Datatypes
    //
    ///////////////////////////////////////////////////////////////////////////////////////
     -->

    


    <!-- http://www.sisostds.org/ontologies/C2SIM#UUIDBase -->

    <rdfs:Datatype rdf:about="http://www.sisostds.org/ontologies/C2SIM#UUIDBase"/>
    


    <!-- 
    ///////////////////////////////////////////////////////////////////////////////////////
    //
    // Object Properties
    //
    ///////////////////////////////////////////////////////////////////////////////////////
     -->

    


    <!-- http://www.sisostds.org/ontologies/C2SIM#hasAction -->

    <owl:ObjectProperty rdf:about="http://www.sisostds.org/ontologies/C2SIM#hasAction"/>
    


    <!-- http://www.sisostds.org/ontologies/lox#hasEvent -->

    <owl:ObjectProperty rdf:about="http://www.sisostds.org/ontologies/lox#hasEvent">
        <rdfs:subPropertyOf rdf:resource="http://www.sisostds.org/ontologies/C2SIM#hasAction"/>
        <rdfs:range rdf:resource="http://www.sisostds.org/ontologies/C2SIM#Event"/>
        <rdfs:comment>An event referenced to this class.</rdfs:comment>
    </owl:ObjectProperty>
    


    <!-- http://www.sisostds.org/ontologies/lox#hasPlanPhase -->

    <owl:ObjectProperty rdf:about="http://www.sisostds.org/ontologies/lox#hasPlanPhase">
        <rdfs:range rdf:resource="http://www.sisostds.org/ontologies/lox#PlanPhase"/>
        <rdfs:comment>Reference to a particular phase of an LOX Plan</rdfs:comment>
    </owl:ObjectProperty>
    


    <!-- http://www.sisostds.org/ontologies/lox#hasPlanPhaseCompletionCondition -->

    <owl:ObjectProperty rdf:about="http://www.sisostds.org/ontologies/lox#hasPlanPhaseCompletionCondition">
        <rdfs:range rdf:resource="http://www.sisostds.org/ontologies/lox#PlanPhaseCompletionCondition"/>
        <rdfs:comment>Provides a condition for completion of a LOX PlanPhase.</rdfs:comment>
    </owl:ObjectProperty>
    


    <!-- http://www.sisostds.org/ontologies/lox#hasPlanPhaseTrigger -->

    <owl:ObjectProperty rdf:about="http://www.sisostds.org/ontologies/lox#hasPlanPhaseTrigger">
        <rdfs:range rdf:resource="http://www.sisostds.org/ontologies/lox#PlanPhaseTrigger"/>
        <rdfs:comment>Provides the condition that will trigger an LOX PlanPhase</rdfs:comment>
    </owl:ObjectProperty>
    


    <!-- http://www.sisostds.org/ontologies/lox#hasRuleOfEngagement -->

    <owl:ObjectProperty rdf:about="http://www.sisostds.org/ontologies/lox#hasRuleOfEngagement">
        <rdfs:range rdf:resource="http://www.sisostds.org/ontologies/lox#RuleOfEngagement"/>
        <rdfs:comment>Provides RulesOfEngagement for an LOX Task or Activity.</rdfs:comment>
    </owl:ObjectProperty>
    


    <!-- http://www.sisostds.org/ontologies/lox#hasSubPhase -->

    <owl:ObjectProperty rdf:about="http://www.sisostds.org/ontologies/lox#hasSubPhase">
        <rdfs:range rdf:resource="http://www.sisostds.org/ontologies/lox#PlanPhase"/>
        <rdfs:comment>Reference to SubPhase of an LOX PlanPhase</rdfs:comment>
    </owl:ObjectProperty>
    


    <!-- http://www.sisostds.org/ontologies/lox#hasTaskFunctionalAssociationCode -->

    <owl:ObjectProperty rdf:about="http://www.sisostds.org/ontologies/lox#hasTaskFunctionalAssociationCode">
        <rdfs:range rdf:resource="http://www.sisostds.org/ontologies/lox#TaskFunctionalAssociationCode"/>
        <rdfs:comment>Provides a JC3IEDM ActionFunctionalAssociateCode forn LOX Task.</rdfs:comment>
    </owl:ObjectProperty>
    


    <!-- http://www.sisostds.org/ontologies/lox#hasTaskFunctionalRelation -->

    <owl:ObjectProperty rdf:about="http://www.sisostds.org/ontologies/lox#hasTaskFunctionalRelation">
        <rdfs:range rdf:resource="http://www.sisostds.org/ontologies/lox#TaskFunctionalRelation"/>
        <rdfs:comment>Provides a JC3IEDM FunctionalRelation code for an LOX Task.</rdfs:comment>
    </owl:ObjectProperty>
    


    <!-- http://www.sisostds.org/ontologies/lox#hasWeaponROECode -->

    <owl:ObjectProperty rdf:about="http://www.sisostds.org/ontologies/lox#hasWeaponROECode">
        <rdfs:subPropertyOf rdf:resource="http://www.sisostds.org/ontologies/C2SIM#hasCode"/>
    </owl:ObjectProperty>
    


    <!-- 
    ///////////////////////////////////////////////////////////////////////////////////////
    //
    // Data properties
    //
    ///////////////////////////////////////////////////////////////////////////////////////
     -->

    


    <!-- http://www.sisostds.org/ontologies/C2SIM#hasReference -->

    <owl:DatatypeProperty rdf:about="http://www.sisostds.org/ontologies/C2SIM#hasReference"/>
    


    <!-- http://www.sisostds.org/ontologies/C2SIM#hasTaskReference -->

    <owl:DatatypeProperty rdf:about="http://www.sisostds.org/ontologies/C2SIM#hasTaskReference"/>
    


    <!-- http://www.sisostds.org/ontologies/lox#hasFunctionalAssociationWithTask -->

    <owl:DatatypeProperty rdf:about="http://www.sisostds.org/ontologies/lox#hasFunctionalAssociationWithTask">
        <rdfs:subPropertyOf rdf:resource="http://www.sisostds.org/ontologies/C2SIM#hasTaskReference"/>
        <rdfs:range rdf:resource="http://www.sisostds.org/ontologies/C2SIM#UUIDBase"/>
        <rdfs:comment>This property identifies the UUID of a Maneuver Warfare Task that is the object of a JC3IEDM ActionFunctionalAssociation.</rdfs:comment>
    </owl:DatatypeProperty>
    


    <!-- http://www.sisostds.org/ontologies/lox#hasPlanPhaseReference -->

    <owl:DatatypeProperty rdf:about="http://www.sisostds.org/ontologies/lox#hasPlanPhaseReference">
        <rdfs:subPropertyOf rdf:resource="http://www.sisostds.org/ontologies/C2SIM#hasReference"/>
        <rdfs:range rdf:resource="http://www.sisostds.org/ontologies/C2SIM#UUIDBase"/>
        <rdfs:comment>A reference to a plan phase.</rdfs:comment>
    </owl:DatatypeProperty>
    


    <!-- http://www.sisostds.org/ontologies/lox#hasText -->

    <owl:DatatypeProperty rdf:about="http://www.sisostds.org/ontologies/lox#hasText">
        <rdfs:range rdf:resource="http://www.w3.org/2001/XMLSchema#string"/>
        <rdfs:comment>Provides a Text annotation as part on an Object.</rdfs:comment>
    </owl:DatatypeProperty>
    


    <!-- http://www.sisostds.org/ontologies/lox#hasTriggerPhase -->

    <owl:DatatypeProperty rdf:about="http://www.sisostds.org/ontologies/lox#hasTriggerPhase">
        <rdfs:range rdf:resource="http://www.sisostds.org/ontologies/C2SIM#UUIDBase"/>
        <rdfs:comment>Provides a phase to trigger another phase in an LOX Plan.</rdfs:comment>
    </owl:DatatypeProperty>
    


    <!-- http://www.sisostds.org/ontologies/lox#isToBeExecutedNow -->

    <owl:DatatypeProperty rdf:about="http://www.sisostds.org/ontologies/lox#isToBeExecutedNow">
        <rdfs:range rdf:resource="http://www.w3.org/2001/XMLSchema#boolean"/>
        <rdfs:comment>Indicates an LOX Task or Activity to be excuted at this time.</rdfs:comment>
    </owl:DatatypeProperty>
    


    <!-- 
    ///////////////////////////////////////////////////////////////////////////////////////
    //
    // Classes
    //
    ///////////////////////////////////////////////////////////////////////////////////////
     -->

    


    <!-- http://www.sisostds.org/ontologies/C2SIM#C2SIMContent -->

    <owl:Class rdf:about="http://www.sisostds.org/ontologies/C2SIM#C2SIMContent"/>
    


    <!-- http://www.sisostds.org/ontologies/C2SIM#Code -->

    <owl:Class rdf:about="http://www.sisostds.org/ontologies/C2SIM#Code"/>
    


    <!-- http://www.sisostds.org/ontologies/C2SIM#DesiredEffectCode -->

    <owl:Class rdf:about="http://www.sisostds.org/ontologies/C2SIM#DesiredEffectCode"/>
    


    <!-- http://www.sisostds.org/ontologies/C2SIM#DomainMessageBody -->

    <owl:Class rdf:about="http://www.sisostds.org/ontologies/C2SIM#DomainMessageBody"/>
    


    <!-- http://www.sisostds.org/ontologies/C2SIM#Event -->

    <owl:Class rdf:about="http://www.sisostds.org/ontologies/C2SIM#Event"/>
    


    <!-- http://www.sisostds.org/ontologies/C2SIM#ObjectDefinitions -->

    <owl:Class rdf:about="http://www.sisostds.org/ontologies/C2SIM#ObjectDefinitions">
        <rdfs:subClassOf>
            <owl:Restriction>
                <owl:onProperty rdf:resource="http://www.sisostds.org/ontologies/lox#hasPlanPhaseReference"/>
                <owl:minQualifiedCardinality rdf:datatype="http://www.w3.org/2001/XMLSchema#nonNegativeInteger">0</owl:minQualifiedCardinality>
                <owl:onDataRange rdf:resource="http://www.sisostds.org/ontologies/C2SIM#UUIDBase"/>
            </owl:Restriction>
        </rdfs:subClassOf>
    </owl:Class>
    


    <!-- http://www.sisostds.org/ontologies/C2SIM#Task -->

    <owl:Class rdf:about="http://www.sisostds.org/ontologies/C2SIM#Task"/>
    


    <!-- http://www.sisostds.org/ontologies/C2SIM#TaskActionCode -->

    <owl:Class rdf:about="http://www.sisostds.org/ontologies/C2SIM#TaskActionCode"/>
    


    <!-- http://www.sisostds.org/ontologies/lox#EventTrigger -->

    <owl:Class rdf:about="http://www.sisostds.org/ontologies/lox#EventTrigger">
        <rdfs:subClassOf rdf:resource="http://www.sisostds.org/ontologies/lox#PlanPhaseTrigger"/>
        <rdfs:subClassOf>
            <owl:Restriction>
                <owl:onProperty rdf:resource="http://www.sisostds.org/ontologies/lox#hasEvent"/>
                <owl:qualifiedCardinality rdf:datatype="http://www.w3.org/2001/XMLSchema#nonNegativeInteger">1</owl:qualifiedCardinality>
                <owl:onClass rdf:resource="http://www.sisostds.org/ontologies/C2SIM#Event"/>
            </owl:Restriction>
        </rdfs:subClassOf>
        <rdfs:comment>A trigger to start a plan phase that is based on the time of an event.</rdfs:comment>
    </owl:Class>
    


    <!-- http://www.sisostds.org/ontologies/lox#ManeuverWarfareTask -->

    <owl:Class rdf:about="http://www.sisostds.org/ontologies/lox#ManeuverWarfareTask">
        <rdfs:subClassOf rdf:resource="http://www.sisostds.org/ontologies/C2SIM#Task"/>
        <rdfs:subClassOf>
            <owl:Restriction>
                <owl:onProperty rdf:resource="http://www.sisostds.org/ontologies/lox#hasRuleOfEngagement"/>
                <owl:minQualifiedCardinality rdf:datatype="http://www.w3.org/2001/XMLSchema#nonNegativeInteger">0</owl:minQualifiedCardinality>
                <owl:onClass rdf:resource="http://www.sisostds.org/ontologies/lox#RuleOfEngagement"/>
            </owl:Restriction>
        </rdfs:subClassOf>
        <rdfs:subClassOf>
            <owl:Restriction>
                <owl:onProperty rdf:resource="http://www.sisostds.org/ontologies/lox#hasTaskFunctionalRelation"/>
                <owl:minQualifiedCardinality rdf:datatype="http://www.w3.org/2001/XMLSchema#nonNegativeInteger">0</owl:minQualifiedCardinality>
                <owl:onClass rdf:resource="http://www.sisostds.org/ontologies/lox#TaskFunctionalRelation"/>
            </owl:Restriction>
        </rdfs:subClassOf>
        <rdfs:comment>A task with additional properties for a Maneuver Warfare Task, including a definition of rules of engagement, and a relationship to another task.

Note that the enumerated individuals in TaskActionCode have been expanded to include tasks defined by  the Joint Consultation Command Control Information Exchange Data Model (JC3IEDM) developed by the Multilateral Interoperability Programme (MIP).</rdfs:comment>
    </owl:Class>
    


    <!-- http://www.sisostds.org/ontologies/lox#MipWeaponUseROE -->

    <owl:Class rdf:about="http://www.sisostds.org/ontologies/lox#MipWeaponUseROE">
        <rdfs:subClassOf rdf:resource="http://www.sisostds.org/ontologies/lox#RuleOfEngagement"/>
        <rdfs:subClassOf>
            <owl:Restriction>
                <owl:onProperty rdf:resource="http://www.sisostds.org/ontologies/lox#hasWeaponROECode"/>
                <owl:qualifiedCardinality rdf:datatype="http://www.w3.org/2001/XMLSchema#nonNegativeInteger">1</owl:qualifiedCardinality>
                <owl:onClass rdf:resource="http://www.sisostds.org/ontologies/lox#WeaponRuleOfEngagementCode"/>
            </owl:Restriction>
        </rdfs:subClassOf>
        <rdfs:comment>A RuleofEngagement that is based on a standard code describing engagement conditions.</rdfs:comment>
    </owl:Class>
    


    <!-- http://www.sisostds.org/ontologies/lox#OnOrderTrigger -->

    <owl:Class rdf:about="http://www.sisostds.org/ontologies/lox#OnOrderTrigger">
        <rdfs:subClassOf rdf:resource="http://www.sisostds.org/ontologies/lox#PlanPhaseTrigger"/>
        <rdfs:subClassOf>
            <owl:Restriction>
                <owl:onProperty rdf:resource="http://www.sisostds.org/ontologies/C2SIM#hasTaskReference"/>
                <owl:qualifiedCardinality rdf:datatype="http://www.w3.org/2001/XMLSchema#nonNegativeInteger">1</owl:qualifiedCardinality>
                <owl:onDataRange rdf:resource="http://www.sisostds.org/ontologies/C2SIM#UUIDBase"/>
            </owl:Restriction>
        </rdfs:subClassOf>
        <rdfs:comment>A trigger for the execution of a plan phase that is based on the start time of a task. Typically this task will be defined in an order and will have a TaskActionCode of ExecutePlanPhase.</rdfs:comment>
    </owl:Class>
    


    <!-- http://www.sisostds.org/ontologies/lox#PlanBody -->

    <owl:Class rdf:about="http://www.sisostds.org/ontologies/lox#PlanBody">
        <rdfs:subClassOf rdf:resource="http://www.sisostds.org/ontologies/C2SIM#DomainMessageBody"/>
        <rdfs:subClassOf>
            <owl:Restriction>
                <owl:onProperty rdf:resource="http://www.sisostds.org/ontologies/lox#hasPlanPhase"/>
                <owl:minQualifiedCardinality rdf:datatype="http://www.w3.org/2001/XMLSchema#nonNegativeInteger">0</owl:minQualifiedCardinality>
                <owl:onClass rdf:resource="http://www.sisostds.org/ontologies/lox#PlanPhase"/>
            </owl:Restriction>
        </rdfs:subClassOf>
        <rdfs:subClassOf>
            <owl:Restriction>
                <owl:onProperty rdf:resource="http://www.sisostds.org/ontologies/lox#hasPlanPhaseReference"/>
                <owl:minQualifiedCardinality rdf:datatype="http://www.w3.org/2001/XMLSchema#nonNegativeInteger">0</owl:minQualifiedCardinality>
                <owl:onDataRange rdf:resource="http://www.sisostds.org/ontologies/C2SIM#UUIDBase"/>
            </owl:Restriction>
        </rdfs:subClassOf>
        <rdfs:subClassOf>
            <owl:Restriction>
                <owl:onProperty rdf:resource="http://www.sisostds.org/ontologies/lox#isToBeExecutedNow"/>
                <owl:qualifiedCardinality rdf:datatype="http://www.w3.org/2001/XMLSchema#nonNegativeInteger">1</owl:qualifiedCardinality>
                <owl:onDataRange rdf:resource="http://www.w3.org/2001/XMLSchema#boolean"/>
            </owl:Restriction>
        </rdfs:subClassOf>
        <rdfs:comment>This message orders the recipient unit to begin execution of the indicated plan.</rdfs:comment>
    </owl:Class>
    


    <!-- http://www.sisostds.org/ontologies/lox#PlanPhase -->

    <owl:Class rdf:about="http://www.sisostds.org/ontologies/lox#PlanPhase">
        <rdfs:subClassOf rdf:resource="http://www.sisostds.org/ontologies/C2SIM#C2SIMContent"/>
        <rdfs:subClassOf>
            <owl:Restriction>
                <owl:onProperty rdf:resource="http://www.sisostds.org/ontologies/lox#hasSubPhase"/>
                <owl:minQualifiedCardinality rdf:datatype="http://www.w3.org/2001/XMLSchema#nonNegativeInteger">0</owl:minQualifiedCardinality>
                <owl:onClass rdf:resource="http://www.sisostds.org/ontologies/lox#PlanPhase"/>
            </owl:Restriction>
        </rdfs:subClassOf>
        <rdfs:subClassOf>
            <owl:Restriction>
                <owl:onProperty rdf:resource="http://www.sisostds.org/ontologies/lox#hasPlanPhaseCompletionCondition"/>
                <owl:qualifiedCardinality rdf:datatype="http://www.w3.org/2001/XMLSchema#nonNegativeInteger">1</owl:qualifiedCardinality>
                <owl:onClass rdf:resource="http://www.sisostds.org/ontologies/lox#PlanPhaseCompletionCondition"/>
            </owl:Restriction>
        </rdfs:subClassOf>
        <rdfs:subClassOf>
            <owl:Restriction>
                <owl:onProperty rdf:resource="http://www.sisostds.org/ontologies/lox#hasPlanPhaseTrigger"/>
                <owl:qualifiedCardinality rdf:datatype="http://www.w3.org/2001/XMLSchema#nonNegativeInteger">1</owl:qualifiedCardinality>
                <owl:onClass rdf:resource="http://www.sisostds.org/ontologies/lox#PlanPhaseTrigger"/>
            </owl:Restriction>
        </rdfs:subClassOf>
        <rdfs:subClassOf>
            <owl:Restriction>
                <owl:onProperty rdf:resource="http://www.sisostds.org/ontologies/C2SIM#hasTaskReference"/>
                <owl:minQualifiedCardinality rdf:datatype="http://www.w3.org/2001/XMLSchema#nonNegativeInteger">0</owl:minQualifiedCardinality>
                <owl:onDataRange rdf:resource="http://www.sisostds.org/ontologies/C2SIM#UUIDBase"/>
            </owl:Restriction>
        </rdfs:subClassOf>
        <rdfs:comment>A plan for a unit. A PlanPhase may a single task for a unit, or tasks for multiple units (one each), or (recursively) multiple subphases.
Phases have completion conditions that indicate when they are complete, as well as Boolean flags that indicate whether the phase is active and whether it is complete.
Phases have trigger conditions that indicate when they start.  Phases may start on the completion of another phase--thus forming a task sequence--on receipt of an order, or at the time of an Event.
 A sequence of tasks for one unit is normally represented as a sequence of subphases in order to express the triggering conditions for each task; however a set of tasks for a unit may be included in a phase and executed with some implicit sequencing such as task time.</rdfs:comment>
    </owl:Class>
    <owl:Axiom>
        <owl:annotatedSource rdf:resource="http://www.sisostds.org/ontologies/lox#PlanPhase"/>
        <owl:annotatedProperty rdf:resource="http://www.w3.org/2000/01/rdf-schema#subClassOf"/>
        <owl:annotatedTarget>
            <owl:Restriction>
                <owl:onProperty rdf:resource="http://www.sisostds.org/ontologies/C2SIM#hasTaskReference"/>
                <owl:minQualifiedCardinality rdf:datatype="http://www.w3.org/2001/XMLSchema#nonNegativeInteger">0</owl:minQualifiedCardinality>
                <owl:onDataRange rdf:resource="http://www.sisostds.org/ontologies/C2SIM#UUIDBase"/>
            </owl:Restriction>
        </owl:annotatedTarget>
        <rdfs:comment>These are references to tasks to be performed in this plan phase. If the tasks have not been previously defined, this property should be omitted and the tasks defined in the hasTask property.</rdfs:comment>
    </owl:Axiom>
    


    <!-- http://www.sisostds.org/ontologies/lox#PlanPhaseCompletionCondition -->

    <owl:Class rdf:about="http://www.sisostds.org/ontologies/lox#PlanPhaseCompletionCondition">
        <rdfs:subClassOf rdf:resource="http://www.sisostds.org/ontologies/C2SIM#Code"/>
        <rdfs:comment>A code defining the condition to be used to test the tasks of a plan phase to determine whether the phase is considered to be complete.</rdfs:comment>
    </owl:Class>
    


    <!-- http://www.sisostds.org/ontologies/lox#PlanPhaseTrigger -->

    <owl:Class rdf:about="http://www.sisostds.org/ontologies/lox#PlanPhaseTrigger">
        <rdfs:subClassOf rdf:resource="http://www.sisostds.org/ontologies/C2SIM#C2SIMContent"/>
        <rdfs:comment>This is a condition that causes the start of execution of a PlanPhase.</rdfs:comment>
    </owl:Class>
    


    <!-- http://www.sisostds.org/ontologies/lox#PriorPhaseCompletionTrigger -->

    <owl:Class rdf:about="http://www.sisostds.org/ontologies/lox#PriorPhaseCompletionTrigger">
        <rdfs:subClassOf rdf:resource="http://www.sisostds.org/ontologies/lox#PlanPhaseTrigger"/>
        <rdfs:subClassOf>
            <owl:Restriction>
                <owl:onProperty rdf:resource="http://www.sisostds.org/ontologies/lox#hasTriggerPhase"/>
                <owl:qualifiedCardinality rdf:datatype="http://www.w3.org/2001/XMLSchema#nonNegativeInteger">1</owl:qualifiedCardinality>
                <owl:onDataRange rdf:resource="http://www.sisostds.org/ontologies/C2SIM#UUIDBase"/>
            </owl:Restriction>
        </rdfs:subClassOf>
        <rdfs:comment>A plan phase trigger that is based on the completion of another plan phase (typically, the phase immediately before this one in a plan).</rdfs:comment>
    </owl:Class>
    


    <!-- http://www.sisostds.org/ontologies/lox#RuleOfEngagement -->

    <owl:Class rdf:about="http://www.sisostds.org/ontologies/lox#RuleOfEngagement">
        <rdfs:subClassOf rdf:resource="http://www.sisostds.org/ontologies/C2SIM#C2SIMContent"/>
        <rdfs:comment>A rule that describes the conditions under which weapons can be used to engage other forces. This class is a collection class; different types of ROEs will be subclasses of this class.</rdfs:comment>
    </owl:Class>
    


    <!-- http://www.sisostds.org/ontologies/lox#TaskFunctionalAssociationCode -->

    <owl:Class rdf:about="http://www.sisostds.org/ontologies/lox#TaskFunctionalAssociationCode">
        <rdfs:subClassOf rdf:resource="http://www.sisostds.org/ontologies/C2SIM#Code"/>
        <rdfs:comment>Instances of this code will be taken from JC3IEDM 3.1.4, 	action-functional-association-category-code</rdfs:comment>
    </owl:Class>
    


    <!-- http://www.sisostds.org/ontologies/lox#TaskFunctionalRelation -->

    <owl:Class rdf:about="http://www.sisostds.org/ontologies/lox#TaskFunctionalRelation">
        <rdfs:subClassOf rdf:resource="http://www.sisostds.org/ontologies/C2SIM#Relationship"/>
        <rdfs:subClassOf>
            <owl:Restriction>
                <owl:onProperty rdf:resource="http://www.sisostds.org/ontologies/lox#hasTaskFunctionalAssociationCode"/>
                <owl:qualifiedCardinality rdf:datatype="http://www.w3.org/2001/XMLSchema#nonNegativeInteger">1</owl:qualifiedCardinality>
                <owl:onClass rdf:resource="http://www.sisostds.org/ontologies/lox#TaskFunctionalAssociationCode"/>
            </owl:Restriction>
        </rdfs:subClassOf>
        <rdfs:subClassOf>
            <owl:Restriction>
                <owl:onProperty rdf:resource="http://www.sisostds.org/ontologies/lox#hasFunctionalAssociationWithTask"/>
                <owl:qualifiedCardinality rdf:datatype="http://www.w3.org/2001/XMLSchema#nonNegativeInteger">1</owl:qualifiedCardinality>
                <owl:onDataRange rdf:resource="http://www.sisostds.org/ontologies/C2SIM#UUIDBase"/>
            </owl:Restriction>
        </rdfs:subClassOf>
        <rdfs:comment>A functional relationship between maneuver warfare tasks.</rdfs:comment>
    </owl:Class>
    


    <!-- http://www.sisostds.org/ontologies/lox#WeaponRuleOfEngagementCode -->

    <owl:Class rdf:about="http://www.sisostds.org/ontologies/lox#WeaponRuleOfEngagementCode">
        <rdfs:subClassOf rdf:resource="http://www.sisostds.org/ontologies/C2SIM#Code"/>
        <rdfs:comment>A code (enumerated value) describing a standard condition for using weapons to engage another force.</rdfs:comment>
    </owl:Class>
    


    <!-- 
    ///////////////////////////////////////////////////////////////////////////////////////
    //
    // Individuals
    //
    ///////////////////////////////////////////////////////////////////////////////////////
     -->

    


    <!-- http://www.sisostds.org/ontologies/lox#ACQUIR -->

    <owl:NamedIndividual rdf:about="http://www.sisostds.org/ontologies/lox#ACQUIR">
        <rdf:type rdf:resource="http://www.sisostds.org/ontologies/C2SIM#TaskActionCode"/>
        <rdfs:comment>Acquire: To detect the presence and location of a target in sufficient detail to permit identification.</rdfs:comment>
        <rdfs:comment>Documentation: 		
						To detect the presence and location of a target in sufficient detail to permit identification.	
					; Appinfo DisplayValue as &quot;Acquire&quot;</rdfs:comment>
    </owl:NamedIndividual>
    


    <!-- http://www.sisostds.org/ontologies/lox#ADVANC -->

    <owl:NamedIndividual rdf:about="http://www.sisostds.org/ontologies/lox#ADVANC">
        <rdf:type rdf:resource="http://www.sisostds.org/ontologies/C2SIM#TaskActionCode"/>
        <rdfs:comment>Advance: To move towards an objective in some form of tactical formation. This is a transitional phase between operations which may</rdfs:comment>
        <rdfs:comment>Documentation: 		
						To move towards an objective in some form of tactical formation. This is a transitional phase between operations which may or may not result in contact with the enemy.	
					; Appinfo DisplayValue as &quot;Advance&quot;</rdfs:comment>
    </owl:NamedIndividual>
    


    <!-- http://www.sisostds.org/ontologies/lox#AEREVA -->

    <owl:NamedIndividual rdf:about="http://www.sisostds.org/ontologies/lox#AEREVA">
        <rdf:type rdf:resource="http://www.sisostds.org/ontologies/C2SIM#TaskActionCode"/>
        <rdfs:comment>Aeromedical evacuation: To move patients under medical supervision to and between medical treatment facilities by air transportation.</rdfs:comment>
    </owl:NamedIndividual>
    


    <!-- http://www.sisostds.org/ontologies/lox#AERRFL -->

    <owl:NamedIndividual rdf:about="http://www.sisostds.org/ontologies/lox#AERRFL">
        <rdf:type rdf:resource="http://www.sisostds.org/ontologies/C2SIM#TaskActionCode"/>
        <rdfs:comment>Aerial refuelling: To refuel aircraft in flight, which extends presence, increases range, and serves as a force multiplier.</rdfs:comment>
    </owl:NamedIndividual>
    


    <!-- http://www.sisostds.org/ontologies/lox#AEW -->

    <owl:NamedIndividual rdf:about="http://www.sisostds.org/ontologies/lox#AEW">
        <rdf:type rdf:resource="http://www.sisostds.org/ontologies/C2SIM#TaskActionCode"/>
        <rdfs:comment>Airborne early warning: To provide airborne early warning and surveillance.</rdfs:comment>
    </owl:NamedIndividual>
    


    <!-- http://www.sisostds.org/ontologies/lox#AEWCON -->

    <owl:NamedIndividual rdf:about="http://www.sisostds.org/ontologies/lox#AEWCON">
        <rdf:type rdf:resource="http://www.sisostds.org/ontologies/C2SIM#TaskActionCode"/>
        <rdfs:comment>Airborne early warning and control: To provide airborne early warning, surveillance and the control of airborne weapon systems.</rdfs:comment>
    </owl:NamedIndividual>
    


    <!-- http://www.sisostds.org/ontologies/lox#AIRDEF -->

    <owl:NamedIndividual rdf:about="http://www.sisostds.org/ontologies/lox#AIRDEF">
        <rdf:type rdf:resource="http://www.sisostds.org/ontologies/C2SIM#TaskActionCode"/>
        <rdfs:comment>Air defence: To protect and defend an area, a strike attack, an installation or naval forces.</rdfs:comment>
        <rdfs:comment>Documentation: 		
						To protect and defend an area, a strike attack, an installation or naval forces.	
					; Appinfo DisplayValue as &quot;Air defence&quot;</rdfs:comment>
    </owl:NamedIndividual>
    


    <!-- http://www.sisostds.org/ontologies/lox#AIRLND -->

    <owl:NamedIndividual rdf:about="http://www.sisostds.org/ontologies/lox#AIRLND">
        <rdf:type rdf:resource="http://www.sisostds.org/ontologies/C2SIM#TaskActionCode"/>
        <rdfs:comment>Airland: To move a unit by air and disembark or unload it, after the aircraft has landed or while a helicopter is hovering.</rdfs:comment>
    </owl:NamedIndividual>
    


    <!-- http://www.sisostds.org/ontologies/lox#AIRSUP -->

    <owl:NamedIndividual rdf:about="http://www.sisostds.org/ontologies/lox#AIRSUP">
        <rdf:type rdf:resource="http://www.sisostds.org/ontologies/C2SIM#TaskActionCode"/>
        <rdfs:comment>Air superiority: To obtain a degree of dominance in the air battle of one force over another in order to permit the conduct of operations by</rdfs:comment>
    </owl:NamedIndividual>
    


    <!-- http://www.sisostds.org/ontologies/lox#AIRSWP -->

    <owl:NamedIndividual rdf:about="http://www.sisostds.org/ontologies/lox#AIRSWP">
        <rdf:type rdf:resource="http://www.sisostds.org/ontologies/C2SIM#TaskActionCode"/>
        <rdfs:comment>Air-to-air sweep: To conduct an offensive mission by fighter aircraft to seek out and destroy enemy aircraft or targets of opportunity in an</rdfs:comment>
    </owl:NamedIndividual>
    


    <!-- http://www.sisostds.org/ontologies/lox#ALT -->

    <owl:NamedIndividual rdf:about="http://www.sisostds.org/ontologies/lox#ALT">
        <rdf:type rdf:resource="http://www.sisostds.org/ontologies/lox#TaskFunctionalAssociationCode"/>
        <rdfs:comment>Is an alternative to: The subject ACTION may replace the object ACTION.</rdfs:comment>
    </owl:NamedIndividual>
    


    <!-- http://www.sisostds.org/ontologies/lox#AMBUSH -->

    <owl:NamedIndividual rdf:about="http://www.sisostds.org/ontologies/lox#AMBUSH">
        <rdf:type rdf:resource="http://www.sisostds.org/ontologies/C2SIM#TaskActionCode"/>
        <rdfs:comment>Ambush: To conduct a surprise attack by fire or other destructive means, from concealed positions on a moving or temporarily halted</rdfs:comment>
        <rdfs:comment>Documentation: 		
						To conduct a surprise attack by fire or other destructive means, from concealed positions on a moving or temporarily halted force or group of personnel.	
					; Appinfo DisplayValue as &quot;Ambush&quot;</rdfs:comment>
    </owl:NamedIndividual>
    


    <!-- http://www.sisostds.org/ontologies/lox#AMPH -->

    <owl:NamedIndividual rdf:about="http://www.sisostds.org/ontologies/lox#AMPH">
        <rdf:type rdf:resource="http://www.sisostds.org/ontologies/C2SIM#TaskActionCode"/>
        <rdfs:comment>Amphibious operation: To mount an operation launched from the sea by naval and land forces against a hostile, or potentially hostile shore.</rdfs:comment>
    </owl:NamedIndividual>
    


    <!-- http://www.sisostds.org/ontologies/lox#AMPHWF -->

    <owl:NamedIndividual rdf:about="http://www.sisostds.org/ontologies/lox#AMPHWF">
        <rdf:type rdf:resource="http://www.sisostds.org/ontologies/C2SIM#TaskActionCode"/>
        <rdfs:comment>Amphibious warfare: To conduct warfare that includes the launch of naval and land forces from sea against a hostile, or potentially hostile shore.</rdfs:comment>
    </owl:NamedIndividual>
    


    <!-- http://www.sisostds.org/ontologies/lox#ANALYS -->

    <owl:NamedIndividual rdf:about="http://www.sisostds.org/ontologies/lox#ANALYS">
        <rdf:type rdf:resource="http://www.sisostds.org/ontologies/C2SIM#TaskActionCode"/>
        <rdfs:comment>Analyse: To review in order to identify significant facts for subsequent interpretation.</rdfs:comment>
    </owl:NamedIndividual>
    


    <!-- http://www.sisostds.org/ontologies/lox#ANARWF -->

    <owl:NamedIndividual rdf:about="http://www.sisostds.org/ontologies/lox#ANARWF">
        <rdf:type rdf:resource="http://www.sisostds.org/ontologies/C2SIM#TaskActionCode"/>
        <rdfs:comment>Anti-air warfare: To conduct warfare with the purpose of defending friendly forces, against the threat aircraft and airborne weapons, whether</rdfs:comment>
    </owl:NamedIndividual>
    


    <!-- http://www.sisostds.org/ontologies/lox#ANSBWF -->

    <owl:NamedIndividual rdf:about="http://www.sisostds.org/ontologies/lox#ANSBWF">
        <rdf:type rdf:resource="http://www.sisostds.org/ontologies/C2SIM#TaskActionCode"/>
        <rdfs:comment>Anti-submarine warfare: To conduct warfare with the intention of denying the opponent the effective use of his submarines.</rdfs:comment>
    </owl:NamedIndividual>
    


    <!-- http://www.sisostds.org/ontologies/lox#ANSFWF -->

    <owl:NamedIndividual rdf:about="http://www.sisostds.org/ontologies/lox#ANSFWF">
        <rdf:type rdf:resource="http://www.sisostds.org/ontologies/C2SIM#TaskActionCode"/>
        <rdfs:comment>Anti-surface warfare: To conduct warfare against an adversary&apos;s surface forces or merchant ships to achieve sea control or sea denial, to disrupt</rdfs:comment>
    </owl:NamedIndividual>
    


    <!-- http://www.sisostds.org/ontologies/lox#ANTARM -->

    <owl:NamedIndividual rdf:about="http://www.sisostds.org/ontologies/lox#ANTARM">
        <rdf:type rdf:resource="http://www.sisostds.org/ontologies/C2SIM#TaskActionCode"/>
        <rdfs:comment>Anti-armour: To destroy armoured targets.</rdfs:comment>
    </owl:NamedIndividual>
    


    <!-- http://www.sisostds.org/ontologies/lox#ARASLT -->

    <owl:NamedIndividual rdf:about="http://www.sisostds.org/ontologies/lox#ARASLT">
        <rdf:type rdf:resource="http://www.sisostds.org/ontologies/C2SIM#TaskActionCode"/>
        <rdfs:comment>Air assault: To mount an operation in which assault forces (combat, combat service, and combat service support), using the firepower, mobility,</rdfs:comment>
        <rdfs:comment>Documentation: 		
						To mount an operation in which assault forces (combat, combat service, and combat service support), using the firepower, mobility, and total integration of helicopter assets, maneuver on the battlefield under the control of the ground or air manoeuvre commander to engage and destroy enemy forces or to seize and hold key terrain.	
					; Appinfo DisplayValue as &quot;Air assault&quot;</rdfs:comment>
    </owl:NamedIndividual>
    


    <!-- http://www.sisostds.org/ontologies/lox#ARBNAS -->

    <owl:NamedIndividual rdf:about="http://www.sisostds.org/ontologies/lox#ARBNAS">
        <rdf:type rdf:resource="http://www.sisostds.org/ontologies/C2SIM#TaskActionCode"/>
        <rdfs:comment>Airborne assault: In an airborne operation, a phase beginning with delivery by air of the assault echelon of the force into the objective area</rdfs:comment>
    </owl:NamedIndividual>
    


    <!-- http://www.sisostds.org/ontologies/lox#ARCCTL -->

    <owl:NamedIndividual rdf:about="http://www.sisostds.org/ontologies/lox#ARCCTL">
        <rdf:type rdf:resource="http://www.sisostds.org/ontologies/C2SIM#TaskActionCode"/>
        <rdfs:comment>Airborne command and control: To conduct battlespace command and control operations from an airborne platform.</rdfs:comment>
    </owl:NamedIndividual>
    


    <!-- http://www.sisostds.org/ontologies/lox#ARDREQ -->

    <owl:NamedIndividual rdf:about="http://www.sisostds.org/ontologies/lox#ARDREQ">
        <rdf:type rdf:resource="http://www.sisostds.org/ontologies/C2SIM#TaskActionCode"/>
        <rdfs:comment>Airdrop, heavy equipment: To unload heavy equipment from an aircraft in flight.</rdfs:comment>
    </owl:NamedIndividual>
    


    <!-- http://www.sisostds.org/ontologies/lox#ARDROP -->

    <owl:NamedIndividual rdf:about="http://www.sisostds.org/ontologies/lox#ARDROP">
        <rdf:type rdf:resource="http://www.sisostds.org/ontologies/C2SIM#TaskActionCode"/>
        <rdfs:comment>Airdrop: To deliver personnel or cargo from aircraft in flight.</rdfs:comment>
    </owl:NamedIndividual>
    


    <!-- http://www.sisostds.org/ontologies/lox#ARINTR -->

    <owl:NamedIndividual rdf:about="http://www.sisostds.org/ontologies/lox#ARINTR">
        <rdf:type rdf:resource="http://www.sisostds.org/ontologies/C2SIM#TaskActionCode"/>
        <rdfs:comment>Air interdiction, battlefield: To conduct air operations to destroy, neutralize, or delay the enemy&apos;s military potential on the battlefield before it can</rdfs:comment>
    </owl:NamedIndividual>
    


    <!-- http://www.sisostds.org/ontologies/lox#ARLFSA -->

    <owl:NamedIndividual rdf:about="http://www.sisostds.org/ontologies/lox#ARLFSA">
        <rdf:type rdf:resource="http://www.sisostds.org/ontologies/C2SIM#TaskActionCode"/>
        <rdfs:comment>Airlift, special assignment: To require a special airlift for which a need of special consideration due to the number of passengers involved or the weight</rdfs:comment>
    </owl:NamedIndividual>
    


    <!-- http://www.sisostds.org/ontologies/lox#ARLFTR -->

    <owl:NamedIndividual rdf:about="http://www.sisostds.org/ontologies/lox#ARLFTR">
        <rdf:type rdf:resource="http://www.sisostds.org/ontologies/C2SIM#TaskActionCode"/>
        <rdfs:comment>Airlift, theatre: To provide air movement and delivery of personnel and equipment directly into objective areas through air landing, airdrop,</rdfs:comment>
    </owl:NamedIndividual>
    


    <!-- http://www.sisostds.org/ontologies/lox#ARMAS -->

    <owl:NamedIndividual rdf:about="http://www.sisostds.org/ontologies/lox#ARMAS">
        <rdf:type rdf:resource="http://www.sisostds.org/ontologies/C2SIM#TaskActionCode"/>
        <rdfs:comment>Armed assault: To perform a short, violent, but well ordered, attack against a local objective such as a gun emplacement, a fort or a machine-gun</rdfs:comment>
    </owl:NamedIndividual>
    


    <!-- http://www.sisostds.org/ontologies/lox#ARRLGL -->

    <owl:NamedIndividual rdf:about="http://www.sisostds.org/ontologies/lox#ARRLGL">
        <rdf:type rdf:resource="http://www.sisostds.org/ontologies/C2SIM#TaskActionCode"/>
        <rdfs:comment>Arrest, legal: To seize and detain a person under authority of the law.</rdfs:comment>
    </owl:NamedIndividual>
    


    <!-- http://www.sisostds.org/ontologies/lox#ARROBS -->

    <owl:NamedIndividual rdf:about="http://www.sisostds.org/ontologies/lox#ARROBS">
        <rdf:type rdf:resource="http://www.sisostds.org/ontologies/C2SIM#TaskActionCode"/>
        <rdfs:comment>Arrest/obstruct: To stop or check the motion, progress, growth, or spread of something.</rdfs:comment>
    </owl:NamedIndividual>
    


    <!-- http://www.sisostds.org/ontologies/lox#ARTCTL -->

    <owl:NamedIndividual rdf:about="http://www.sisostds.org/ontologies/lox#ARTCTL">
        <rdf:type rdf:resource="http://www.sisostds.org/ontologies/C2SIM#TaskActionCode"/>
        <rdfs:comment>Air traffic control: To provide air traffic control service to flights in control areas.</rdfs:comment>
    </owl:NamedIndividual>
    


    <!-- http://www.sisostds.org/ontologies/lox#ASSMBL -->

    <owl:NamedIndividual rdf:about="http://www.sisostds.org/ontologies/lox#ASSMBL">
        <rdf:type rdf:resource="http://www.sisostds.org/ontologies/C2SIM#TaskActionCode"/>
        <rdfs:comment>Assemble: To join together multiple objects in the same area.</rdfs:comment>
        <rdfs:comment>Documentation: 		
						To join together multiple objects in the same area.	
					; Appinfo DisplayValue as &quot;Assemble&quot;</rdfs:comment>
    </owl:NamedIndividual>
    


    <!-- http://www.sisostds.org/ontologies/lox#ATTACK -->

    <owl:NamedIndividual rdf:about="http://www.sisostds.org/ontologies/lox#ATTACK">
        <rdf:type rdf:resource="http://www.sisostds.org/ontologies/C2SIM#TaskActionCode"/>
        <rdfs:comment>Attack, not otherwise specified: To conduct a type of offensive action characterised by coordinated employment of firepower and manoeuvre to close with and</rdfs:comment>
        <rdfs:comment>Documentation: 		
						To conduct a type of offensive action characterised by coordinated employment of firepower and manoeuvre to close with and destroy or capture the enemy.	
					; Appinfo DisplayValue as &quot;Attack, not otherwise specified&quot;</rdfs:comment>
    </owl:NamedIndividual>
    


    <!-- http://www.sisostds.org/ontologies/lox#ATTDVR -->

    <owl:NamedIndividual rdf:about="http://www.sisostds.org/ontologies/lox#ATTDVR">
        <rdf:type rdf:resource="http://www.sisostds.org/ontologies/C2SIM#TaskActionCode"/>
        <rdfs:comment>Attack, diversion: To conduct an attack wherein a force attacks, or threatens to attack, a target other than the main target for the purpose</rdfs:comment>
    </owl:NamedIndividual>
    


    <!-- http://www.sisostds.org/ontologies/lox#ATTEL -->

    <owl:NamedIndividual rdf:about="http://www.sisostds.org/ontologies/lox#ATTEL">
        <rdf:type rdf:resource="http://www.sisostds.org/ontologies/C2SIM#TaskActionCode"/>
        <rdfs:comment>Attack, electronic: To conduct electronic warfare involving the use of electromagnetic energy, directed energy or anti-radiation weapons to attack</rdfs:comment>
    </owl:NamedIndividual>
    


    <!-- http://www.sisostds.org/ontologies/lox#ATTMN -->

    <owl:NamedIndividual rdf:about="http://www.sisostds.org/ontologies/lox#ATTMN">
        <rdf:type rdf:resource="http://www.sisostds.org/ontologies/C2SIM#TaskActionCode"/>
        <rdfs:comment>Attack, main: To conduct the principal attack or effort into which the commander throws the full weight of the offensive power at his disposal.</rdfs:comment>
    </owl:NamedIndividual>
    


    <!-- http://www.sisostds.org/ontologies/lox#ATTRIT -->

    <owl:NamedIndividual rdf:about="http://www.sisostds.org/ontologies/lox#ATTRIT">
        <rdf:type rdf:resource="http://www.sisostds.org/ontologies/C2SIM#TaskActionCode"/>
        <rdfs:comment>Attrit: To reduce of the effectiveness of a force by causing loss of personnel and materiel.</rdfs:comment>
        <rdfs:comment>Documentation: 		
						To reduce of the effectiveness of a force by causing loss of personnel and materiel.	
					; Appinfo DisplayValue as &quot;Attrit&quot;</rdfs:comment>
    </owl:NamedIndividual>
    


    <!-- http://www.sisostds.org/ontologies/lox#ATTSPT -->

    <owl:NamedIndividual rdf:about="http://www.sisostds.org/ontologies/lox#ATTSPT">
        <rdf:type rdf:resource="http://www.sisostds.org/ontologies/C2SIM#TaskActionCode"/>
        <rdfs:comment>Attack, supporting: To conduct an offensive operation carried out in conjunction with a main attack and designed to achieve one or more of the</rdfs:comment>
        <rdfs:comment>Documentation: 		
						To conduct an offensive operation carried out in conjunction with a main attack and designed to achieve one or more of the following: a. deceive the enemy; b. destroy or pin down enemy forces which could interfere with the main attack; c. control ground whose occupation by the enemy will hinder the main attack; or d. force the enemy to commit reserves prematurely or in an indecisive area.	
					; Appinfo DisplayValue as &quot;Attack, supporting&quot;</rdfs:comment>
    </owl:NamedIndividual>
    


    <!-- http://www.sisostds.org/ontologies/lox#AVOID -->

    <owl:NamedIndividual rdf:about="http://www.sisostds.org/ontologies/lox#AVOID">
        <rdf:type rdf:resource="http://www.sisostds.org/ontologies/C2SIM#TaskActionCode"/>
        <rdfs:comment>Avoid: To miss or take evading action.</rdfs:comment>
        <rdfs:comment>Documentation: 		
						To miss or take evading action.	
					; Appinfo DisplayValue as &quot;Avoid&quot;</rdfs:comment>
    </owl:NamedIndividual>
    


    <!-- http://www.sisostds.org/ontologies/lox#AWACS -->

    <owl:NamedIndividual rdf:about="http://www.sisostds.org/ontologies/lox#AWACS">
        <rdf:type rdf:resource="http://www.sisostds.org/ontologies/C2SIM#TaskActionCode"/>
        <rdfs:comment>Air warning/air control: To provide information about enemy air activity that poses immediate threat to friendly forces and monitors and directs the</rdfs:comment>
    </owl:NamedIndividual>
    


    <!-- http://www.sisostds.org/ontologies/lox#AllTasksComplete -->

    <owl:NamedIndividual rdf:about="http://www.sisostds.org/ontologies/lox#AllTasksComplete">
        <rdf:type rdf:resource="http://www.sisostds.org/ontologies/lox#PlanPhaseCompletionCondition"/>
    </owl:NamedIndividual>
    


    <!-- http://www.sisostds.org/ontologies/lox#BIOSMP -->

    <owl:NamedIndividual rdf:about="http://www.sisostds.org/ontologies/lox#BIOSMP">
        <rdf:type rdf:resource="http://www.sisostds.org/ontologies/C2SIM#TaskActionCode"/>
        <rdfs:comment>Biological sampling: To collect samples for testing for biological hazards.</rdfs:comment>
    </owl:NamedIndividual>
    


    <!-- http://www.sisostds.org/ontologies/lox#BLDUP -->

    <owl:NamedIndividual rdf:about="http://www.sisostds.org/ontologies/lox#BLDUP">
        <rdf:type rdf:resource="http://www.sisostds.org/ontologies/C2SIM#TaskActionCode"/>
        <rdfs:comment>Build-up: To attain prescribed strength of units and prescribed levels of vehicles, equipment, stores and supplies.</rdfs:comment>
    </owl:NamedIndividual>
    


    <!-- http://www.sisostds.org/ontologies/lox#BLOCK -->

    <owl:NamedIndividual rdf:about="http://www.sisostds.org/ontologies/lox#BLOCK">
        <rdf:type rdf:resource="http://www.sisostds.org/ontologies/C2SIM#TaskActionCode"/>
        <rdfs:comment>Block: To deny the enemy access to an area or to prevent his advance in a direction or along an avenue of approach.</rdfs:comment>
        <rdfs:comment>Documentation: 		
						To deny the enemy access to an area or to prevent his advance in a direction or along an avenue of approach.	
					; Appinfo DisplayValue as &quot;Block&quot;</rdfs:comment>
    </owl:NamedIndividual>
    


    <!-- http://www.sisostds.org/ontologies/lox#BRAKUP -->

    <owl:NamedIndividual rdf:about="http://www.sisostds.org/ontologies/lox#BRAKUP">
        <rdf:type rdf:resource="http://www.sisostds.org/ontologies/C2SIM#TaskActionCode"/>
        <rdfs:comment>Breakup: No definition provided in ADatP-3 Baseline 13.1 FFIRN/FUD 1299/19.</rdfs:comment>
    </owl:NamedIndividual>
    


    <!-- http://www.sisostds.org/ontologies/lox#BREACH -->

    <owl:NamedIndividual rdf:about="http://www.sisostds.org/ontologies/lox#BREACH">
        <rdf:type rdf:resource="http://www.sisostds.org/ontologies/C2SIM#TaskActionCode"/>
        <rdfs:comment>Breach: To break through or secure a passage through an enemy defence, obstacle, minefield, or fortification.</rdfs:comment>
        <rdfs:comment>Documentation: 		
						To break through or secure a passage through an enemy defence, obstacle, minefield, or fortification.	
					; Appinfo DisplayValue as &quot;Breach&quot;</rdfs:comment>
    </owl:NamedIndividual>
    


    <!-- http://www.sisostds.org/ontologies/lox#BURN -->

    <owl:NamedIndividual rdf:about="http://www.sisostds.org/ontologies/lox#BURN">
        <rdfs:comment>Documentation: 		
						The ACTION objective is alight.	
					; Appinfo DisplayValue as &quot;Burning&quot;</rdfs:comment>
    </owl:NamedIndividual>
    


    <!-- http://www.sisostds.org/ontologies/lox#BYPASS -->

    <owl:NamedIndividual rdf:about="http://www.sisostds.org/ontologies/lox#BYPASS">
        <rdf:type rdf:resource="http://www.sisostds.org/ontologies/C2SIM#TaskActionCode"/>
        <rdfs:comment>Bypass: To manoeuvre around an obstacle, position, or enemy force in order to maintain the momentum of advance.</rdfs:comment>
        <rdfs:comment>Documentation: 		
						To manoeuvre around an obstacle, position, or enemy force in order to maintain the momentum of advance.	
					; Appinfo DisplayValue as &quot;Bypass&quot;</rdfs:comment>
    </owl:NamedIndividual>
    


    <!-- http://www.sisostds.org/ontologies/lox#CADVGD -->

    <owl:NamedIndividual rdf:about="http://www.sisostds.org/ontologies/lox#CADVGD">
        <rdf:type rdf:resource="http://www.sisostds.org/ontologies/C2SIM#TaskActionCode"/>
        <rdfs:comment>Constitute an advance guard: To provide a security element whose primary task is to move ahead of the main body and protect the main force by fighting</rdfs:comment>
    </owl:NamedIndividual>
    


    <!-- http://www.sisostds.org/ontologies/lox#CANDC -->

    <owl:NamedIndividual rdf:about="http://www.sisostds.org/ontologies/lox#CANDC">
        <rdf:type rdf:resource="http://www.sisostds.org/ontologies/C2SIM#TaskActionCode"/>
        <rdfs:comment>Command and control: To exercise authority and direction over assigned and attached forces in the accomplishment of the mission.</rdfs:comment>
    </owl:NamedIndividual>
    


    <!-- http://www.sisostds.org/ontologies/lox#CANLSE -->

    <owl:NamedIndividual rdf:about="http://www.sisostds.org/ontologies/lox#CANLSE">
        <rdf:type rdf:resource="http://www.sisostds.org/ontologies/C2SIM#TaskActionCode"/>
        <rdfs:comment>Canalise: To restrict operations to a narrow zone by use of existing or reinforcing obstacles or by fire or bombing. (Army)--A tactical</rdfs:comment>
    </owl:NamedIndividual>
    


    <!-- http://www.sisostds.org/ontologies/lox#CAPBAR -->

    <owl:NamedIndividual rdf:about="http://www.sisostds.org/ontologies/lox#CAPBAR">
        <rdf:type rdf:resource="http://www.sisostds.org/ontologies/C2SIM#TaskActionCode"/>
        <rdfs:comment>Combat air patrol, barrier: To conduct a patrol by fighter aircraft that is employed between a force and an objective area as a barrier across the probable</rdfs:comment>
    </owl:NamedIndividual>
    


    <!-- http://www.sisostds.org/ontologies/lox#CAPNGR -->

    <owl:NamedIndividual rdf:about="http://www.sisostds.org/ontologies/lox#CAPNGR">
        <rdf:type rdf:resource="http://www.sisostds.org/ontologies/C2SIM#TaskActionCode"/>
        <rdfs:comment>Combat air patrol, ingress: Combat air patrol flown in support of friendly aircraft as the aircraft ingress into enemy territory.</rdfs:comment>
    </owl:NamedIndividual>
    


    <!-- http://www.sisostds.org/ontologies/lox#CAPPRT -->

    <owl:NamedIndividual rdf:about="http://www.sisostds.org/ontologies/lox#CAPPRT">
        <rdf:type rdf:resource="http://www.sisostds.org/ontologies/C2SIM#TaskActionCode"/>
        <rdfs:comment>Combat air patrol, protect: An aircraft patrol flying over an objective area in order to protect friendly forces.</rdfs:comment>
    </owl:NamedIndividual>
    


    <!-- http://www.sisostds.org/ontologies/lox#CAPRES -->

    <owl:NamedIndividual rdf:about="http://www.sisostds.org/ontologies/lox#CAPRES">
        <rdf:type rdf:resource="http://www.sisostds.org/ontologies/C2SIM#TaskActionCode"/>
        <rdfs:comment>Combat air patrol, rescue: To protect the search and rescue task forces during recovery operations.</rdfs:comment>
    </owl:NamedIndividual>
    


    <!-- http://www.sisostds.org/ontologies/lox#CAPSRF -->

    <owl:NamedIndividual rdf:about="http://www.sisostds.org/ontologies/lox#CAPSRF">
        <rdf:type rdf:resource="http://www.sisostds.org/ontologies/C2SIM#TaskActionCode"/>
        <rdfs:comment>Combat air patrol, surface: Combat air patrol flown in support of surface vessels conducting maritime operations.</rdfs:comment>
    </owl:NamedIndividual>
    


    <!-- http://www.sisostds.org/ontologies/lox#CAPTRD -->

    <owl:NamedIndividual rdf:about="http://www.sisostds.org/ontologies/lox#CAPTRD">
        <rdfs:comment>Documentation: 		
						The ACTION objective has been captured or acquired and is available for use or interrogation/possession has been taken of an area, normally by force.	
					; Appinfo DisplayValue as &quot;Captured&quot;</rdfs:comment>
    </owl:NamedIndividual>
    


    <!-- http://www.sisostds.org/ontologies/lox#CAPTUR -->

    <owl:NamedIndividual rdf:about="http://www.sisostds.org/ontologies/lox#CAPTUR">
        <rdf:type rdf:resource="http://www.sisostds.org/ontologies/C2SIM#TaskActionCode"/>
        <rdfs:comment>Capture: To take possession of an object, normally by force; it frequently involves movement as a preliminary phase.</rdfs:comment>
        <rdfs:comment>Documentation: 		
						To take possession of an object, normally by force; it frequently involves movement as a preliminary phase.	
					; Appinfo DisplayValue as &quot;Capture&quot;</rdfs:comment>
    </owl:NamedIndividual>
    


    <!-- http://www.sisostds.org/ontologies/lox#CARLNC -->

    <owl:NamedIndividual rdf:about="http://www.sisostds.org/ontologies/lox#CARLNC">
        <rdf:type rdf:resource="http://www.sisostds.org/ontologies/C2SIM#TaskActionCode"/>
        <rdfs:comment>Carrier launch: To launch aircraft from a naval platform.</rdfs:comment>
    </owl:NamedIndividual>
    


    <!-- http://www.sisostds.org/ontologies/lox#CARREC -->

    <owl:NamedIndividual rdf:about="http://www.sisostds.org/ontologies/lox#CARREC">
        <rdf:type rdf:resource="http://www.sisostds.org/ontologies/C2SIM#TaskActionCode"/>
        <rdfs:comment>Carrier recovery: To recover aircraft on a naval platform.</rdfs:comment>
    </owl:NamedIndividual>
    


    <!-- http://www.sisostds.org/ontologies/lox#CBRHDF -->

    <owl:NamedIndividual rdf:about="http://www.sisostds.org/ontologies/lox#CBRHDF">
        <rdf:type rdf:resource="http://www.sisostds.org/ontologies/C2SIM#TaskActionCode"/>
        <rdfs:comment>Constitute bridgehead force: To form the force during an obstacle crossing which seizes or controls ground in order to permit the continuous embarkation,</rdfs:comment>
    </owl:NamedIndividual>
    


    <!-- http://www.sisostds.org/ontologies/lox#CBRKOF -->

    <owl:NamedIndividual rdf:about="http://www.sisostds.org/ontologies/lox#CBRKOF">
        <rdf:type rdf:resource="http://www.sisostds.org/ontologies/C2SIM#TaskActionCode"/>
        <rdfs:comment>Constitute breakout force: To form the force during an obstacle crossing which is tasked with the continuation of the operation.</rdfs:comment>
    </owl:NamedIndividual>
    


    <!-- http://www.sisostds.org/ontologies/lox#CDWDAC -->

    <owl:NamedIndividual rdf:about="http://www.sisostds.org/ontologies/lox#CDWDAC">
        <rdf:type rdf:resource="http://www.sisostds.org/ontologies/C2SIM#TaskActionCode"/>
        <rdfs:comment>Codeword activity: To conduct an activity described by the action-task-detail-text.</rdfs:comment>
    </owl:NamedIndividual>
    


    <!-- http://www.sisostds.org/ontologies/lox#CFLKGD -->

    <owl:NamedIndividual rdf:about="http://www.sisostds.org/ontologies/lox#CFLKGD">
        <rdf:type rdf:resource="http://www.sisostds.org/ontologies/C2SIM#TaskActionCode"/>
        <rdfs:comment>Constitute a flank guard: To provide a security element whose primary task is to protect the main force by fighting on the designated flank to gain</rdfs:comment>
    </owl:NamedIndividual>
    


    <!-- http://www.sisostds.org/ontologies/lox#CHAFF -->

    <owl:NamedIndividual rdf:about="http://www.sisostds.org/ontologies/lox#CHAFF">
        <rdf:type rdf:resource="http://www.sisostds.org/ontologies/C2SIM#TaskActionCode"/>
        <rdfs:comment>Release CHAFF: To deploy strips of frequency-cut metal foil, wire or metalized glass fibre to reflect electromagnetic energy, usually dropped</rdfs:comment>
    </owl:NamedIndividual>
    


    <!-- http://www.sisostds.org/ontologies/lox#CHMSMP -->

    <owl:NamedIndividual rdf:about="http://www.sisostds.org/ontologies/lox#CHMSMP">
        <rdf:type rdf:resource="http://www.sisostds.org/ontologies/C2SIM#TaskActionCode"/>
        <rdfs:comment>Chemical sampling: To collect samples for testing for chemical hazards.</rdfs:comment>
    </owl:NamedIndividual>
    


    <!-- http://www.sisostds.org/ontologies/lox#CINPLF -->

    <owl:NamedIndividual rdf:about="http://www.sisostds.org/ontologies/lox#CINPLF">
        <rdf:type rdf:resource="http://www.sisostds.org/ontologies/C2SIM#TaskActionCode"/>
        <rdfs:comment>Constitute in-place force: To form the force during an obstacle crossing which provides fire and other support to the bridgehead force.</rdfs:comment>
    </owl:NamedIndividual>
    


    <!-- http://www.sisostds.org/ontologies/lox#CLARSP -->

    <owl:NamedIndividual rdf:about="http://www.sisostds.org/ontologies/lox#CLARSP">
        <rdf:type rdf:resource="http://www.sisostds.org/ontologies/C2SIM#TaskActionCode"/>
        <rdfs:comment>Close air support: Air action against hostile targets which are in close proximity to friendly forces and which require detailed integration</rdfs:comment>
    </owl:NamedIndividual>
    


    <!-- http://www.sisostds.org/ontologies/lox#CLOSE -->

    <owl:NamedIndividual rdf:about="http://www.sisostds.org/ontologies/lox#CLOSE">
        <rdf:type rdf:resource="http://www.sisostds.org/ontologies/C2SIM#TaskActionCode"/>
        <rdfs:comment>Close: To prevent a FACILITY or FEATURE from performing its intended function.</rdfs:comment>
        <rdfs:comment>Documentation: 		
						To prevent a FACILITY or FEATURE from performing its intended function.	
					; Appinfo DisplayValue as &quot;Close&quot;</rdfs:comment>
    </owl:NamedIndividual>
    


    <!-- http://www.sisostds.org/ontologies/lox#CLRAIR -->

    <owl:NamedIndividual rdf:about="http://www.sisostds.org/ontologies/lox#CLRAIR">
        <rdf:type rdf:resource="http://www.sisostds.org/ontologies/C2SIM#TaskActionCode"/>
        <rdfs:comment>Clear, air: To clear the air to gain either temporary or permanent air superiority or control in a given sector.</rdfs:comment>
    </owl:NamedIndividual>
    


    <!-- http://www.sisostds.org/ontologies/lox#CLRLND -->

    <owl:NamedIndividual rdf:about="http://www.sisostds.org/ontologies/lox#CLRLND">
        <rdf:type rdf:resource="http://www.sisostds.org/ontologies/C2SIM#TaskActionCode"/>
        <rdfs:comment>Clear, land combat: To remove all enemy forces from a specific location, area, or zone.</rdfs:comment>
        <rdfs:comment>Documentation: 		
						To remove all enemy forces from a specific location, area, or zone.	
					; Appinfo DisplayValue as &quot;Clear, land combat&quot;</rdfs:comment>
    </owl:NamedIndividual>
    


    <!-- http://www.sisostds.org/ontologies/lox#CLROBS -->

    <owl:NamedIndividual rdf:about="http://www.sisostds.org/ontologies/lox#CLROBS">
        <rdf:type rdf:resource="http://www.sisostds.org/ontologies/C2SIM#TaskActionCode"/>
        <rdfs:comment>Clear, obstacle: To totally eliminate or neutralize an obstacle; a task that is usually performed by follow-on engineers and is not done under</rdfs:comment>
        <rdfs:comment>Documentation: 		
						To totally eliminate or neutralize an obstacle; a task that is usually performed by follow-on engineers and is not done under fire.	
					; Appinfo DisplayValue as &quot;Clear, obstacle&quot;</rdfs:comment>
    </owl:NamedIndividual>
    


    <!-- http://www.sisostds.org/ontologies/lox#CLRRAD -->

    <owl:NamedIndividual rdf:about="http://www.sisostds.org/ontologies/lox#CLRRAD">
        <rdf:type rdf:resource="http://www.sisostds.org/ontologies/C2SIM#TaskActionCode"/>
        <rdfs:comment>Clear, radio net: To eliminate transmissions on a tactical radio net in order to allow a higher precedence transmission to occur.</rdfs:comment>
    </owl:NamedIndividual>
    


    <!-- http://www.sisostds.org/ontologies/lox#CMAINB -->

    <owl:NamedIndividual rdf:about="http://www.sisostds.org/ontologies/lox#CMAINB">
        <rdf:type rdf:resource="http://www.sisostds.org/ontologies/C2SIM#TaskActionCode"/>
        <rdfs:comment>Constitute a main body: To constitute the main force for a specific operation.</rdfs:comment>
    </owl:NamedIndividual>
    


    <!-- http://www.sisostds.org/ontologies/lox#CNFPSL -->

    <owl:NamedIndividual rdf:about="http://www.sisostds.org/ontologies/lox#CNFPSL">
        <rdf:type rdf:resource="http://www.sisostds.org/ontologies/C2SIM#TaskActionCode"/>
        <rdfs:comment>Conduct forward passage of lines: An operation in which an incoming force attacks through a unit (outgoing force).that is in contact with the enemy.</rdfs:comment>
        <rdfs:comment>Documentation: 		
						An operation in which an incoming force attacks through a unit (outgoing force).that is in contact with the enemy.	
					; Appinfo DisplayValue as &quot;Conduct forward passage of lines&quot;</rdfs:comment>
    </owl:NamedIndividual>
    


    <!-- http://www.sisostds.org/ontologies/lox#CNFSTE -->

    <owl:NamedIndividual rdf:about="http://www.sisostds.org/ontologies/lox#CNFSTE">
        <rdf:type rdf:resource="http://www.sisostds.org/ontologies/C2SIM#TaskActionCode"/>
        <rdfs:comment>Confiscate: To deprive a person of his property as forfeited by public authority.</rdfs:comment>
    </owl:NamedIndividual>
    


    <!-- http://www.sisostds.org/ontologies/lox#CNRPSL -->

    <owl:NamedIndividual rdf:about="http://www.sisostds.org/ontologies/lox#CNRPSL">
        <rdf:type rdf:resource="http://www.sisostds.org/ontologies/C2SIM#TaskActionCode"/>
        <rdfs:comment>Conduct rearward passage of lines: An operation when a force (outgoing force) effecting a movement to the rear passes through the sector of a unit (incoming</rdfs:comment>
        <rdfs:comment>Documentation: 		
						An operation when a force (outgoing force) effecting a movement to the rear passes through the sector of a unit (incoming force).	
					; Appinfo DisplayValue as &quot;Conduct rearward passage of lines&quot;</rdfs:comment>
    </owl:NamedIndividual>
    


    <!-- http://www.sisostds.org/ontologies/lox#CNRSVC -->

    <owl:NamedIndividual rdf:about="http://www.sisostds.org/ontologies/lox#CNRSVC">
        <rdf:type rdf:resource="http://www.sisostds.org/ontologies/C2SIM#TaskActionCode"/>
        <rdfs:comment>Conduct road service: To enable the movement of a number of specific units.</rdfs:comment>
    </owl:NamedIndividual>
    


    <!-- http://www.sisostds.org/ontologies/lox#CNSLDT -->

    <owl:NamedIndividual rdf:about="http://www.sisostds.org/ontologies/lox#CNSLDT">
        <rdf:type rdf:resource="http://www.sisostds.org/ontologies/C2SIM#TaskActionCode"/>
        <rdfs:comment>Consolidate a position: To organise and strengthen a newly captured position so that it can be used against the enemy.</rdfs:comment>
    </owl:NamedIndividual>
    


    <!-- http://www.sisostds.org/ontologies/lox#COARPL -->

    <owl:NamedIndividual rdf:about="http://www.sisostds.org/ontologies/lox#COARPL">
        <rdf:type rdf:resource="http://www.sisostds.org/ontologies/C2SIM#TaskActionCode"/>
        <rdfs:comment>Combat air patrol: An aircraft patrol provided over an objective area, the force protected, the critical area of a combat zone, or in an air</rdfs:comment>
    </owl:NamedIndividual>
    


    <!-- http://www.sisostds.org/ontologies/lox#COMC3I -->

    <owl:NamedIndividual rdf:about="http://www.sisostds.org/ontologies/lox#COMC3I">
        <rdf:type rdf:resource="http://www.sisostds.org/ontologies/C2SIM#TaskActionCode"/>
        <rdfs:comment>Communications (C3I): To provide communication means such as data links or radio for the purpose of communication, command, control and intelligence.</rdfs:comment>
    </owl:NamedIndividual>
    


    <!-- http://www.sisostds.org/ontologies/lox#COMINC -->

    <owl:NamedIndividual rdf:about="http://www.sisostds.org/ontologies/lox#COMINC">
        <rdf:type rdf:resource="http://www.sisostds.org/ontologies/C2SIM#TaskActionCode"/>
        <rdfs:comment>Communication, intelligence collection: To gather communication intelligence in order to meet current operational requirements.</rdfs:comment>
    </owl:NamedIndividual>
    


    <!-- http://www.sisostds.org/ontologies/lox#COMREL -->

    <owl:NamedIndividual rdf:about="http://www.sisostds.org/ontologies/lox#COMREL">
        <rdf:type rdf:resource="http://www.sisostds.org/ontologies/C2SIM#TaskActionCode"/>
        <rdfs:comment>Communications relay: To employ an aircraft to serve as a communications relay.</rdfs:comment>
    </owl:NamedIndividual>
    


    <!-- http://www.sisostds.org/ontologies/lox#CONS -->

    <owl:NamedIndividual rdf:about="http://www.sisostds.org/ontologies/lox#CONS">
        <rdfs:comment>Documentation: 		
						The consumption of specified consumables or CONSUMABLE-MATERIEL-TYPEs.	
					; Appinfo DisplayValue as &quot;Consumed&quot;</rdfs:comment>
    </owl:NamedIndividual>
    


    <!-- http://www.sisostds.org/ontologies/lox#CONSTR -->

    <owl:NamedIndividual rdf:about="http://www.sisostds.org/ontologies/lox#CONSTR">
        <rdf:type rdf:resource="http://www.sisostds.org/ontologies/C2SIM#TaskActionCode"/>
        <rdfs:comment>Construct: To build, dig or create an object.</rdfs:comment>
    </owl:NamedIndividual>
    


    <!-- http://www.sisostds.org/ontologies/lox#CONTAN -->

    <owl:NamedIndividual rdf:about="http://www.sisostds.org/ontologies/lox#CONTAN">
        <rdf:type rdf:resource="http://www.sisostds.org/ontologies/C2SIM#TaskActionCode"/>
        <rdfs:comment>Contain: To stop, hold, or surround the forces of the enemy or to cause the enemy to centre activity on a given front and to prevent</rdfs:comment>
    </owl:NamedIndividual>
    


    <!-- http://www.sisostds.org/ontologies/lox#COOPER -->

    <owl:NamedIndividual rdf:about="http://www.sisostds.org/ontologies/lox#COOPER">
        <rdf:type rdf:resource="http://www.sisostds.org/ontologies/C2SIM#TaskActionCode"/>
        <rdfs:comment>Cooperate: To work or act together.</rdfs:comment>
    </owl:NamedIndividual>
    


    <!-- http://www.sisostds.org/ontologies/lox#COURER -->

    <owl:NamedIndividual rdf:about="http://www.sisostds.org/ontologies/lox#COURER">
        <rdf:type rdf:resource="http://www.sisostds.org/ontologies/C2SIM#TaskActionCode"/>
        <rdfs:comment>Courier: To travel as a courier.</rdfs:comment>
    </owl:NamedIndividual>
    


    <!-- http://www.sisostds.org/ontologies/lox#COVER -->

    <owl:NamedIndividual rdf:about="http://www.sisostds.org/ontologies/lox#COVER">
        <rdf:type rdf:resource="http://www.sisostds.org/ontologies/C2SIM#TaskActionCode"/>
        <rdfs:comment>Cover: To operate as a force apart to protect the main body by fighting to gain time while also observing and reporting information</rdfs:comment>
        <rdfs:comment>Documentation: 		
						To operate as a force apart to protect the main body by fighting to gain time while also observing and reporting information and preventing enemy ground observation of an direct fire against the main body.	
					; Appinfo DisplayValue as &quot;Cover&quot;</rdfs:comment>
    </owl:NamedIndividual>
    


    <!-- http://www.sisostds.org/ontologies/lox#CRESRV -->

    <owl:NamedIndividual rdf:about="http://www.sisostds.org/ontologies/lox#CRESRV">
        <rdf:type rdf:resource="http://www.sisostds.org/ontologies/C2SIM#TaskActionCode"/>
        <rdfs:comment>Constitute a reserve: To constitute a force which may be committed into combat only on the order of the commander of the ORGANISATION who so designated</rdfs:comment>
        <rdfs:comment>Documentation: 		
						To constitute a force which may be committed into combat only on the order of the commander of the ORGANISATION who so designated the reserve force.	
					; Appinfo DisplayValue as &quot;Constitute a reserve&quot;</rdfs:comment>
    </owl:NamedIndividual>
    


    <!-- http://www.sisostds.org/ontologies/lox#CROSS -->

    <owl:NamedIndividual rdf:about="http://www.sisostds.org/ontologies/lox#CROSS">
        <rdf:type rdf:resource="http://www.sisostds.org/ontologies/C2SIM#TaskActionCode"/>
        <rdfs:comment>Cross: To move over a FEATURE or FACILITY.</rdfs:comment>
    </owl:NamedIndividual>
    


    <!-- http://www.sisostds.org/ontologies/lox#CRRGD -->

    <owl:NamedIndividual rdf:about="http://www.sisostds.org/ontologies/lox#CRRGD">
        <rdf:type rdf:resource="http://www.sisostds.org/ontologies/C2SIM#TaskActionCode"/>
        <rdfs:comment>Constitute a rear guard: To provide a security element whose primary task is to move (or remain) at the rear of the main body and protect the main</rdfs:comment>
    </owl:NamedIndividual>
    


    <!-- http://www.sisostds.org/ontologies/lox#CTRATK -->

    <owl:NamedIndividual rdf:about="http://www.sisostds.org/ontologies/lox#CTRATK">
        <rdf:type rdf:resource="http://www.sisostds.org/ontologies/C2SIM#TaskActionCode"/>
        <rdfs:comment>Counter attack: To mount an offensive operation in which an attack by a part or all of a defending force is made against an enemy attacking</rdfs:comment>
        <rdfs:comment>Documentation: 		
						To mount an offensive operation in which an attack by a part or all of a defending force is made against an enemy attacking force, for such specific purposes as regaining ground lost, cutting off or destroying lead enemy units, and with the general objective of regaining the initiative and denying the enemy the attainment of his goal or purpose in attacking.	
					; Appinfo DisplayValue as &quot;Counter attack&quot;</rdfs:comment>
    </owl:NamedIndividual>
    


    <!-- http://www.sisostds.org/ontologies/lox#CTRBYF -->

    <owl:NamedIndividual rdf:about="http://www.sisostds.org/ontologies/lox#CTRBYF">
        <rdf:type rdf:resource="http://www.sisostds.org/ontologies/C2SIM#TaskActionCode"/>
        <rdfs:comment>Counter-battery fire: To deliver fire for the purpose of destroying or neutralizing indirect fire weapons systems.</rdfs:comment>
        <rdfs:comment>Documentation: 		
						To deliver fire for the purpose of destroying or neutralizing indirect fire weapons systems.	
					; Appinfo DisplayValue as &quot;Counter-battery fire&quot;</rdfs:comment>
    </owl:NamedIndividual>
    


    <!-- http://www.sisostds.org/ontologies/lox#CTRFIR -->

    <owl:NamedIndividual rdf:about="http://www.sisostds.org/ontologies/lox#CTRFIR">
        <rdf:type rdf:resource="http://www.sisostds.org/ontologies/C2SIM#TaskActionCode"/>
        <rdfs:comment>Counter attack by fire: To deny the enemy his goal in attacking through fire into an engagement area to defeat or destroy an enemy force.</rdfs:comment>
        <rdfs:comment>Documentation: 		
						To deny the enemy his goal in attacking through fire into an engagement area to defeat or destroy an enemy force.	
					; Appinfo DisplayValue as &quot;Counter attack by fire&quot;</rdfs:comment>
    </owl:NamedIndividual>
    


    <!-- http://www.sisostds.org/ontologies/lox#DAZZLE -->

    <owl:NamedIndividual rdf:about="http://www.sisostds.org/ontologies/lox#DAZZLE">
        <rdf:type rdf:resource="http://www.sisostds.org/ontologies/C2SIM#TaskActionCode"/>
        <rdfs:comment>Dazzle: To confuse the enemy by temporary loss of vision or a temporary reduction in visual acuity; may also be applied to effects</rdfs:comment>
    </owl:NamedIndividual>
    


    <!-- http://www.sisostds.org/ontologies/lox#DCPTEL -->

    <owl:NamedIndividual rdf:about="http://www.sisostds.org/ontologies/lox#DCPTEL">
        <rdf:type rdf:resource="http://www.sisostds.org/ontologies/C2SIM#TaskActionCode"/>
        <rdfs:comment>Deception, electronic: In electronic countermeasures, the deliberate radiation, re-radiation, alteration, absorption or reflection of electromagnetic</rdfs:comment>
    </owl:NamedIndividual>
    


    <!-- http://www.sisostds.org/ontologies/lox#DEBARK -->

    <owl:NamedIndividual rdf:about="http://www.sisostds.org/ontologies/lox#DEBARK">
        <rdf:type rdf:resource="http://www.sisostds.org/ontologies/C2SIM#TaskActionCode"/>
        <rdfs:comment>Debark: To unload troops with their supplies and equipment from a ship.</rdfs:comment>
    </owl:NamedIndividual>
    


    <!-- http://www.sisostds.org/ontologies/lox#DECEIV -->

    <owl:NamedIndividual rdf:about="http://www.sisostds.org/ontologies/lox#DECEIV">
        <rdf:type rdf:resource="http://www.sisostds.org/ontologies/C2SIM#TaskActionCode"/>
        <rdfs:comment>Deceive: To employ measures designed to mislead the enemy by manipulation, distortion, or falsification of evidence to induce him to</rdfs:comment>
        <rdfs:comment>Documentation: 		
						To employ measures designed to mislead the enemy by manipulation, distortion, or falsification of evidence to induce him to react in a manner prejudicial to his interests.	
					; Appinfo DisplayValue as &quot;Deceive&quot;</rdfs:comment>
    </owl:NamedIndividual>
    


    <!-- http://www.sisostds.org/ontologies/lox#DECSVC -->

    <owl:NamedIndividual rdf:about="http://www.sisostds.org/ontologies/lox#DECSVC">
        <rdf:type rdf:resource="http://www.sisostds.org/ontologies/C2SIM#TaskActionCode"/>
        <rdfs:comment>Decontamination services: To provide purification making any person, object, or area safe by absorbing, destroying, neutralizing, making harmless, or</rdfs:comment>
    </owl:NamedIndividual>
    


    <!-- http://www.sisostds.org/ontologies/lox#DEFCNT -->

    <owl:NamedIndividual rdf:about="http://www.sisostds.org/ontologies/lox#DEFCNT">
        <rdf:type rdf:resource="http://www.sisostds.org/ontologies/C2SIM#TaskActionCode"/>
        <rdfs:comment>Defensive counter air: To conduct air operations to attain and maintain a desired degree of air superiority by the destruction or neutralization</rdfs:comment>
    </owl:NamedIndividual>
    


    <!-- http://www.sisostds.org/ontologies/lox#DEFDST -->

    <owl:NamedIndividual rdf:about="http://www.sisostds.org/ontologies/lox#DEFDST">
        <rdf:type rdf:resource="http://www.sisostds.org/ontologies/C2SIM#TaskActionCode"/>
        <rdfs:comment>Defence destruction: To destroy enemy defences in a specific area by any means.</rdfs:comment>
    </owl:NamedIndividual>
    


    <!-- http://www.sisostds.org/ontologies/lox#DEFEAT -->

    <owl:NamedIndividual rdf:about="http://www.sisostds.org/ontologies/lox#DEFEAT">
        <rdf:type rdf:resource="http://www.sisostds.org/ontologies/C2SIM#TaskActionCode"/>
        <rdfs:comment>Defeat: To diminish the effectiveness of the enemy to the extent that he is unable to participate further in the battle or at least</rdfs:comment>
        <rdfs:comment>Documentation: 		
						To diminish the effectiveness of the enemy to the extent that he is unable to participate further in the battle or at least cannot fulfil his intention.	
					; Appinfo DisplayValue as &quot;Defeat&quot;</rdfs:comment>
    </owl:NamedIndividual>
    


    <!-- http://www.sisostds.org/ontologies/lox#DEFEND -->

    <owl:NamedIndividual rdf:about="http://www.sisostds.org/ontologies/lox#DEFEND">
        <rdf:type rdf:resource="http://www.sisostds.org/ontologies/C2SIM#TaskActionCode"/>
        <rdfs:comment>Defend: To hold a defined object against an enemy attack; to halt or ward off an attack in order to defeat or destroy the enemy.</rdfs:comment>
        <rdfs:comment>Documentation: 		
						To hold a defined object against an enemy attack; to halt or ward off an attack in order to defeat or destroy the enemy.	
					; Appinfo DisplayValue as &quot;Defend&quot;</rdfs:comment>
    </owl:NamedIndividual>
    


    <!-- http://www.sisostds.org/ontologies/lox#DEFLCT -->

    <owl:NamedIndividual rdf:about="http://www.sisostds.org/ontologies/lox#DEFLCT">
        <rdf:type rdf:resource="http://www.sisostds.org/ontologies/C2SIM#TaskActionCode"/>
        <rdfs:comment>Deflect: To prevent an enemy force from following the intended course.</rdfs:comment>
    </owl:NamedIndividual>
    


    <!-- http://www.sisostds.org/ontologies/lox#DEFSUP -->

    <owl:NamedIndividual rdf:about="http://www.sisostds.org/ontologies/lox#DEFSUP">
        <rdf:type rdf:resource="http://www.sisostds.org/ontologies/C2SIM#TaskActionCode"/>
        <rdfs:comment>Defence suppression: To neutralize, destroy or temporarily degrade enemy defences in a specific area by physical attack and/or electronic warfare.</rdfs:comment>
    </owl:NamedIndividual>
    


    <!-- http://www.sisostds.org/ontologies/lox#DELAY -->

    <owl:NamedIndividual rdf:about="http://www.sisostds.org/ontologies/lox#DELAY">
        <rdf:type rdf:resource="http://www.sisostds.org/ontologies/C2SIM#TaskActionCode"/>
        <rdfs:comment>Delay: To slow the momentum of the enemy by conducting an operation in which the force under pressure trades time for space. The</rdfs:comment>
        <rdfs:comment>Documentation: 		
						To slow the momentum of the enemy by conducting an operation in which the force under pressure trades time for space. The aim is to inflict the maximum damage on the enemy without becoming decisively engaged.	
					; Appinfo DisplayValue as &quot;Delay&quot;</rdfs:comment>
    </owl:NamedIndividual>
    


    <!-- http://www.sisostds.org/ontologies/lox#DEMFRP -->

    <owl:NamedIndividual rdf:about="http://www.sisostds.org/ontologies/lox#DEMFRP">
        <rdf:type rdf:resource="http://www.sisostds.org/ontologies/C2SIM#TaskActionCode"/>
        <rdfs:comment>Constitute a demolition firing party: To provide the party at the site which is technically responsible for the demolition.</rdfs:comment>
    </owl:NamedIndividual>
    


    <!-- http://www.sisostds.org/ontologies/lox#DEMGRD -->

    <owl:NamedIndividual rdf:about="http://www.sisostds.org/ontologies/lox#DEMGRD">
        <rdf:type rdf:resource="http://www.sisostds.org/ontologies/C2SIM#TaskActionCode"/>
        <rdfs:comment>Constitute a demolition guard: To provide a local force positioned to ensure that a target is not captured by an enemy before orders are given for its demolition</rdfs:comment>
    </owl:NamedIndividual>
    


    <!-- http://www.sisostds.org/ontologies/lox#DEMO -->

    <owl:NamedIndividual rdf:about="http://www.sisostds.org/ontologies/lox#DEMO">
        <rdf:type rdf:resource="http://www.sisostds.org/ontologies/C2SIM#TaskActionCode"/>
        <rdfs:comment>Demolish: To destroy structures, facilities, or materiel by use of fire, water, explosives, mechanical, or other means.</rdfs:comment>
    </owl:NamedIndividual>
    


    <!-- http://www.sisostds.org/ontologies/lox#DENY -->

    <owl:NamedIndividual rdf:about="http://www.sisostds.org/ontologies/lox#DENY">
        <rdf:type rdf:resource="http://www.sisostds.org/ontologies/C2SIM#TaskActionCode"/>
        <rdfs:comment>Deny: To prevent access by blocking, disrupting, dislocating and/or bringing fire to bear.</rdfs:comment>
        <rdfs:comment>Documentation: 		
						To prevent access by blocking, disrupting, dislocating and/or bringing fire to bear.	
					; Appinfo DisplayValue as &quot;Deny&quot;</rdfs:comment>
    </owl:NamedIndividual>
    


    <!-- http://www.sisostds.org/ontologies/lox#DEPLOY -->

    <owl:NamedIndividual rdf:about="http://www.sisostds.org/ontologies/lox#DEPLOY">
        <rdf:type rdf:resource="http://www.sisostds.org/ontologies/C2SIM#TaskActionCode"/>
        <rdfs:comment>Deploy: To move and adopt tactical formation or dispersal in a specific location.</rdfs:comment>
    </owl:NamedIndividual>
    


    <!-- http://www.sisostds.org/ontologies/lox#DESCRB -->

    <owl:NamedIndividual rdf:about="http://www.sisostds.org/ontologies/lox#DESCRB">
        <rdf:type rdf:resource="http://www.sisostds.org/ontologies/C2SIM#TaskActionCode"/>
        <rdfs:comment>Describe: To state the characteristics, appearance, etc. of an object.</rdfs:comment>
    </owl:NamedIndividual>
    


    <!-- http://www.sisostds.org/ontologies/lox#DESTRY -->

    <owl:NamedIndividual rdf:about="http://www.sisostds.org/ontologies/lox#DESTRY">
        <rdf:type rdf:resource="http://www.sisostds.org/ontologies/C2SIM#TaskActionCode"/>
        <rdfs:comment>Destroy: To physically render an enemy force combat-ineffective or damaging a target so that it cannot function as intended, nor be</rdfs:comment>
        <rdfs:comment>Documentation: 		
						To physically render an enemy force combat-ineffective or damaging a target so that it cannot function as intended, nor be restored to a usable condition without being entirely rebuilt.	
					; Appinfo DisplayValue as &quot;Destroy&quot;</rdfs:comment>
    </owl:NamedIndividual>
    


    <!-- http://www.sisostds.org/ontologies/lox#DETECT -->

    <owl:NamedIndividual rdf:about="http://www.sisostds.org/ontologies/lox#DETECT">
        <rdf:type rdf:resource="http://www.sisostds.org/ontologies/C2SIM#TaskActionCode"/>
        <rdfs:comment>Detect: To discover by any means of the presence of a person, object or phenomenon of potential military significance.</rdfs:comment>
    </owl:NamedIndividual>
    


    <!-- http://www.sisostds.org/ontologies/lox#DISENG -->

    <owl:NamedIndividual rdf:about="http://www.sisostds.org/ontologies/lox#DISENG">
        <rdf:type rdf:resource="http://www.sisostds.org/ontologies/C2SIM#TaskActionCode"/>
        <rdfs:comment>Disengage: To break off an action.</rdfs:comment>
        <rdfs:comment>Documentation: 		
						To break off an action.	
					; Appinfo DisplayValue as &quot;Disengage&quot;</rdfs:comment>
    </owl:NamedIndividual>
    


    <!-- http://www.sisostds.org/ontologies/lox#DISRPT -->

    <owl:NamedIndividual rdf:about="http://www.sisostds.org/ontologies/lox#DISRPT">
        <rdf:type rdf:resource="http://www.sisostds.org/ontologies/C2SIM#TaskActionCode"/>
        <rdfs:comment>Disrupt: To break apart an enemy&apos;s formation and tempo, to interrupt the enemy&apos;s timetable, to cause premature commitment of forces,</rdfs:comment>
        <rdfs:comment>Documentation: 		
						To break apart an enemy&apos;s formation and tempo, to interrupt the enemy&apos;s timetable, to cause premature commitment of forces, and/or splinter their attack using integrated fire planning and obstacle effect.	
					; Appinfo DisplayValue as &quot;Disrupt&quot;</rdfs:comment>
    </owl:NamedIndividual>
    


    <!-- http://www.sisostds.org/ontologies/lox#DIVE -->

    <owl:NamedIndividual rdf:about="http://www.sisostds.org/ontologies/lox#DIVE">
        <rdf:type rdf:resource="http://www.sisostds.org/ontologies/C2SIM#TaskActionCode"/>
        <rdfs:comment>Dive: To descend or plunge into or underwater or some other liquid.</rdfs:comment>
    </owl:NamedIndividual>
    


    <!-- http://www.sisostds.org/ontologies/lox#DIVERT -->

    <owl:NamedIndividual rdf:about="http://www.sisostds.org/ontologies/lox#DIVERT">
        <rdf:type rdf:resource="http://www.sisostds.org/ontologies/C2SIM#TaskActionCode"/>
        <rdfs:comment>Divert: To draw the attention and forces of an enemy from the point of the principal operation; an attack, alarm, or feint which diverts</rdfs:comment>
    </owl:NamedIndividual>
    


    <!-- http://www.sisostds.org/ontologies/lox#DLBATK -->

    <owl:NamedIndividual rdf:about="http://www.sisostds.org/ontologies/lox#DLBATK">
        <rdf:type rdf:resource="http://www.sisostds.org/ontologies/C2SIM#TaskActionCode"/>
        <rdfs:comment>Attack, deliberate: To conduct a type of offensive action characterised by pre-planned coordinated employment of firepower and manoeuvre to close</rdfs:comment>
        <rdfs:comment>Documentation: 		
						To conduct a type of offensive action characterised by pre-planned coordinated employment of firepower and manoeuvre to close with and destroy or capture the enemy.	
					; Appinfo DisplayValue as &quot;Attack, deliberate&quot;</rdfs:comment>
    </owl:NamedIndividual>
    


    <!-- http://www.sisostds.org/ontologies/lox#DRONL -->

    <owl:NamedIndividual rdf:about="http://www.sisostds.org/ontologies/lox#DRONL">
        <rdf:type rdf:resource="http://www.sisostds.org/ontologies/C2SIM#TaskActionCode"/>
        <rdfs:comment>Documentation: 		
						To perform the launching of drones.	
					; Appinfo DisplayValue as &quot;Drone launch&quot;</rdfs:comment>
        <rdfs:comment>Drone launch: To perform the launching of drones.</rdfs:comment>
    </owl:NamedIndividual>
    


    <!-- http://www.sisostds.org/ontologies/lox#DSTRBT -->

    <owl:NamedIndividual rdf:about="http://www.sisostds.org/ontologies/lox#DSTRBT">
        <rdf:type rdf:resource="http://www.sisostds.org/ontologies/C2SIM#TaskActionCode"/>
        <rdfs:comment>Distribute: To divide or dispense in portions.</rdfs:comment>
    </owl:NamedIndividual>
    


    <!-- http://www.sisostds.org/ontologies/lox#DSTRYK -->

    <owl:NamedIndividual rdf:about="http://www.sisostds.org/ontologies/lox#DSTRYK">
        <rdfs:comment>Documentation: 		
						Cannot function as intended nor be repaired or restored to an operational status.	
					; Appinfo DisplayValue as &quot;Destroyed (K-kill)&quot;</rdfs:comment>
    </owl:NamedIndividual>
    


    <!-- http://www.sisostds.org/ontologies/lox#DUMPNG -->

    <owl:NamedIndividual rdf:about="http://www.sisostds.org/ontologies/lox#DUMPNG">
        <rdf:type rdf:resource="http://www.sisostds.org/ontologies/C2SIM#TaskActionCode"/>
        <rdfs:comment>Dumping: To position stocks to meet future requirements.</rdfs:comment>
    </owl:NamedIndividual>
    


    <!-- http://www.sisostds.org/ontologies/lox#ELCCNM -->

    <owl:NamedIndividual rdf:about="http://www.sisostds.org/ontologies/lox#ELCCNM">
        <rdf:type rdf:resource="http://www.sisostds.org/ontologies/C2SIM#TaskActionCode"/>
        <rdfs:comment>Electronic counter measures: To perform electronic warfare actions to prevent or reduce an enemy&apos;s effective use of the electromagnetic spectrum through</rdfs:comment>
    </owl:NamedIndividual>
    


    <!-- http://www.sisostds.org/ontologies/lox#ELCWAR -->

    <owl:NamedIndividual rdf:about="http://www.sisostds.org/ontologies/lox#ELCWAR">
        <rdf:type rdf:resource="http://www.sisostds.org/ontologies/C2SIM#TaskActionCode"/>
        <rdfs:comment>Electronic warfare: To exploit the electromagnetic spectrum encompassing; the search for, interception of electromagnetic emissions, the employment</rdfs:comment>
    </owl:NamedIndividual>
    


    <!-- http://www.sisostds.org/ontologies/lox#ELCWRS -->

    <owl:NamedIndividual rdf:about="http://www.sisostds.org/ontologies/lox#ELCWRS">
        <rdf:type rdf:resource="http://www.sisostds.org/ontologies/C2SIM#TaskActionCode"/>
        <rdfs:comment>Electronic warfare support: To search for, intercept, locate, record measures and analyse radiated electromagnetic energy for the purpose of exploiting</rdfs:comment>
    </owl:NamedIndividual>
    


    <!-- http://www.sisostds.org/ontologies/lox#EMBARK -->

    <owl:NamedIndividual rdf:about="http://www.sisostds.org/ontologies/lox#EMBARK">
        <rdf:type rdf:resource="http://www.sisostds.org/ontologies/C2SIM#TaskActionCode"/>
        <rdfs:comment>Embark: To put personnel and/or vehicles and their associated stores and equipment into ships or aircraft.</rdfs:comment>
    </owl:NamedIndividual>
    


    <!-- http://www.sisostds.org/ontologies/lox#ENGAGE -->

    <owl:NamedIndividual rdf:about="http://www.sisostds.org/ontologies/lox#ENGAGE">
        <rdf:type rdf:resource="http://www.sisostds.org/ontologies/C2SIM#TaskActionCode"/>
        <rdfs:comment>Documentation: 		
						To bring the enemy under fire.	
					; Appinfo DisplayValue as &quot;Engage&quot;</rdfs:comment>
        <rdfs:comment>Engage: To bring the enemy under fire.</rdfs:comment>
    </owl:NamedIndividual>
    


    <!-- http://www.sisostds.org/ontologies/lox#ENVLP -->

    <owl:NamedIndividual rdf:about="http://www.sisostds.org/ontologies/lox#ENVLP">
        <rdf:type rdf:resource="http://www.sisostds.org/ontologies/C2SIM#TaskActionCode"/>
        <rdfs:comment>Documentation: 		
						To conduct an offensive manoeuvre in which the main attacking force passes around or over the enemy&apos;s principal defensive positions with the aim of securing objectives to the enemy&apos;s rear.	
					; Appinfo DisplayValue as &quot;Envelop&quot;</rdfs:comment>
        <rdfs:comment>Envelop: To conduct an offensive manoeuvre in which the main attacking force passes around or over the enemy&apos;s principal defensive</rdfs:comment>
    </owl:NamedIndividual>
    


    <!-- http://www.sisostds.org/ontologies/lox#ESCRT -->

    <owl:NamedIndividual rdf:about="http://www.sisostds.org/ontologies/lox#ESCRT">
        <rdf:type rdf:resource="http://www.sisostds.org/ontologies/C2SIM#TaskActionCode"/>
        <rdfs:comment>Escort: To accompany and protect another force or convoy.</rdfs:comment>
    </owl:NamedIndividual>
    


    <!-- http://www.sisostds.org/ontologies/lox#EVACT -->

    <owl:NamedIndividual rdf:about="http://www.sisostds.org/ontologies/lox#EVACT">
        <rdf:type rdf:resource="http://www.sisostds.org/ontologies/C2SIM#TaskActionCode"/>
        <rdfs:comment>Evacuate: To clear materiel and personnel from a given locality.</rdfs:comment>
    </owl:NamedIndividual>
    


    <!-- http://www.sisostds.org/ontologies/lox#EXFLTR -->

    <owl:NamedIndividual rdf:about="http://www.sisostds.org/ontologies/lox#EXFLTR">
        <rdf:type rdf:resource="http://www.sisostds.org/ontologies/C2SIM#TaskActionCode"/>
        <rdfs:comment>Exfiltrate: To withdraw from a dangerous position.</rdfs:comment>
    </owl:NamedIndividual>
    


    <!-- http://www.sisostds.org/ontologies/lox#EXPLT -->

    <owl:NamedIndividual rdf:about="http://www.sisostds.org/ontologies/lox#EXPLT">
        <rdf:type rdf:resource="http://www.sisostds.org/ontologies/C2SIM#TaskActionCode"/>
        <rdfs:comment>Documentation: 		
						To take advantage of a successful attack by mounting an offensive operation to follow-up and harass a dislocated enemy with the aim of further disorganising him in depth. This may provide the opportunity to capture ground which was not part of the objective of the original attack.	
					; Appinfo DisplayValue as &quot;Exploit&quot;</rdfs:comment>
        <rdfs:comment>Exploit: To take advantage of a successful attack by mounting an offensive operation to follow-up and harass a dislocated enemy with</rdfs:comment>
    </owl:NamedIndividual>
    


    <!-- http://www.sisostds.org/ontologies/lox#ExecutePlanPhase -->

    <owl:NamedIndividual rdf:about="http://www.sisostds.org/ontologies/lox#ExecutePlanPhase">
        <rdf:type rdf:resource="http://www.sisostds.org/ontologies/C2SIM#TaskActionCode"/>
    </owl:NamedIndividual>
    <owl:Axiom>
        <owl:annotatedSource rdf:resource="http://www.sisostds.org/ontologies/lox#ExecutePlanPhase"/>
        <owl:annotatedProperty rdf:resource="http://www.w3.org/1999/02/22-rdf-syntax-ns#type"/>
        <owl:annotatedTarget rdf:resource="http://www.sisostds.org/ontologies/C2SIM#TaskActionCode"/>
        <rdfs:comment>This code indicates that the task is to execute a previously provided plan phase.</rdfs:comment>
    </owl:Axiom>
    


    <!-- http://www.sisostds.org/ontologies/lox#FIX -->

    <owl:NamedIndividual rdf:about="http://www.sisostds.org/ontologies/lox#FIX">
        <rdf:type rdf:resource="http://www.sisostds.org/ontologies/C2SIM#TaskActionCode"/>
        <rdfs:comment>Documentation: 		
						To prevent the enemy from moving any part of his force from a specific location for a specific period of time.	
					; Appinfo DisplayValue as &quot;Fix&quot;</rdfs:comment>
        <rdfs:comment>Fix: To prevent the enemy from moving any part of his force from a specific location for a specific period of time.</rdfs:comment>
    </owl:NamedIndividual>
    


    <!-- http://www.sisostds.org/ontologies/lox#FIXACO -->

    <owl:NamedIndividual rdf:about="http://www.sisostds.org/ontologies/lox#FIXACO">
        <rdf:type rdf:resource="http://www.sisostds.org/ontologies/C2SIM#TaskActionCode"/>
        <rdfs:comment>Fix, acoustic: To determine a position using acoustic data.</rdfs:comment>
    </owl:NamedIndividual>
    


    <!-- http://www.sisostds.org/ontologies/lox#FIXELM -->

    <owl:NamedIndividual rdf:about="http://www.sisostds.org/ontologies/lox#FIXELM">
        <rdf:type rdf:resource="http://www.sisostds.org/ontologies/C2SIM#TaskActionCode"/>
        <rdfs:comment>Fix, electromagnetic: To determine a position using electromagnetic data.</rdfs:comment>
    </owl:NamedIndividual>
    


    <!-- http://www.sisostds.org/ontologies/lox#FIXELO -->

    <owl:NamedIndividual rdf:about="http://www.sisostds.org/ontologies/lox#FIXELO">
        <rdf:type rdf:resource="http://www.sisostds.org/ontologies/C2SIM#TaskActionCode"/>
        <rdfs:comment>Fix, electro-optical: To determine a position using electro-optical data.</rdfs:comment>
    </owl:NamedIndividual>
    


    <!-- http://www.sisostds.org/ontologies/lox#FKIL -->

    <owl:NamedIndividual rdf:about="http://www.sisostds.org/ontologies/lox#FKIL">
        <rdfs:comment>Documentation: 		
						The destruction of a vehicle (or system&apos;s) primary weapon system.	
					; Appinfo DisplayValue as &quot;Firepower kill (F-kill)&quot;</rdfs:comment>
    </owl:NamedIndividual>
    


    <!-- http://www.sisostds.org/ontologies/lox#FLIG -->

    <owl:NamedIndividual rdf:about="http://www.sisostds.org/ontologies/lox#FLIG">
        <rdfs:comment>Documentation: 		
						The setting to flight of a PERSON or PERSON-TYPEs from their present location.	
					; Appinfo DisplayValue as &quot;Forced to flee&quot;</rdfs:comment>
    </owl:NamedIndividual>
    


    <!-- http://www.sisostds.org/ontologies/lox#FNCHFL -->

    <owl:NamedIndividual rdf:about="http://www.sisostds.org/ontologies/lox#FNCHFL">
        <rdf:type rdf:resource="http://www.sisostds.org/ontologies/C2SIM#TaskActionCode"/>
        <rdfs:comment>Functional check flight: To conduct a test flight to ensure the general aircraft safety after maintenance/repair, and to ensure the aircraft is fully</rdfs:comment>
    </owl:NamedIndividual>
    


    <!-- http://www.sisostds.org/ontologies/lox#FOLASS -->

    <owl:NamedIndividual rdf:about="http://www.sisostds.org/ontologies/lox#FOLASS">
        <rdf:type rdf:resource="http://www.sisostds.org/ontologies/C2SIM#TaskActionCode"/>
        <rdfs:comment>Follow and assume: To operate as a committed force that follows a force conducting an offensive operation, and is prepared to continue the mission</rdfs:comment>
    </owl:NamedIndividual>
    


    <!-- http://www.sisostds.org/ontologies/lox#FOLSPT -->

    <owl:NamedIndividual rdf:about="http://www.sisostds.org/ontologies/lox#FOLSPT">
        <rdf:type rdf:resource="http://www.sisostds.org/ontologies/C2SIM#TaskActionCode"/>
        <rdfs:comment>Follow and support: To operate as a committed force that follows and supports the mission accomplishment of a force conducting an offensive operation.</rdfs:comment>
    </owl:NamedIndividual>
    


    <!-- http://www.sisostds.org/ontologies/lox#FRWDAC -->

    <owl:NamedIndividual rdf:about="http://www.sisostds.org/ontologies/lox#FRWDAC">
        <rdf:type rdf:resource="http://www.sisostds.org/ontologies/C2SIM#TaskActionCode"/>
        <rdfs:comment>Forward air control: To direct the action of combat aircraft engaged in close air support of land forces from a forward position on the ground</rdfs:comment>
    </owl:NamedIndividual>
    


    <!-- http://www.sisostds.org/ontologies/lox#GENCHS -->

    <owl:NamedIndividual rdf:about="http://www.sisostds.org/ontologies/lox#GENCHS">
        <rdf:type rdf:resource="http://www.sisostds.org/ontologies/C2SIM#TaskActionCode"/>
        <rdfs:comment>Generate chemical smoke: To produce chemical smoke to act as a form of cover to protect ongoing operations.</rdfs:comment>
    </owl:NamedIndividual>
    


    <!-- http://www.sisostds.org/ontologies/lox#GUARD -->

    <owl:NamedIndividual rdf:about="http://www.sisostds.org/ontologies/lox#GUARD">
        <rdf:type rdf:resource="http://www.sisostds.org/ontologies/C2SIM#TaskActionCode"/>
        <rdfs:comment>Documentation: 		
						To protect the main body by fighting to gain time while also observing and reporting information.	
					; Appinfo DisplayValue as &quot;Guard&quot;</rdfs:comment>
        <rdfs:comment>Guard: To protect the main body by fighting to gain time while also observing and reporting information.</rdfs:comment>
    </owl:NamedIndividual>
    


    <!-- http://www.sisostds.org/ontologies/lox#HARASS -->

    <owl:NamedIndividual rdf:about="http://www.sisostds.org/ontologies/lox#HARASS">
        <rdf:type rdf:resource="http://www.sisostds.org/ontologies/C2SIM#TaskActionCode"/>
        <rdfs:comment>Documentation: 		
						To mount an operation or fire plan designed to curtail movement and, by threat of losses, to lower the morale of enemy troops.	
					; Appinfo DisplayValue as &quot;Harass&quot;</rdfs:comment>
        <rdfs:comment>Harass: To mount an operation or fire plan designed to curtail movement and, by threat of losses, to lower the morale of enemy troops.</rdfs:comment>
    </owl:NamedIndividual>
    


    <!-- http://www.sisostds.org/ontologies/lox#HASPRV -->

    <owl:NamedIndividual rdf:about="http://www.sisostds.org/ontologies/lox#HASPRV">
        <rdf:type rdf:resource="http://www.sisostds.org/ontologies/lox#TaskFunctionalAssociationCode"/>
        <rdfs:comment>Has as a provisional sub-ACTION: The subject ACTION may be re-directed to an alternative object ACTION. Note: The need for object ACTION is foreseen in planning,</rdfs:comment>
    </owl:NamedIndividual>
    


    <!-- http://www.sisostds.org/ontologies/lox#HASSEC -->

    <owl:NamedIndividual rdf:about="http://www.sisostds.org/ontologies/lox#HASSEC">
        <rdf:type rdf:resource="http://www.sisostds.org/ontologies/lox#TaskFunctionalAssociationCode"/>
        <rdfs:comment>Has as secondary: The subject ACTION is designated as the primary activity and has the object ACTION as a secondary activity.</rdfs:comment>
    </owl:NamedIndividual>
    


    <!-- http://www.sisostds.org/ontologies/lox#HASTY -->

    <owl:NamedIndividual rdf:about="http://www.sisostds.org/ontologies/lox#HASTY">
        <rdf:type rdf:resource="http://www.sisostds.org/ontologies/C2SIM#TaskActionCode"/>
        <rdfs:comment>Attack, hasty: To conduct a type of offensive action using firepower and manoeuvre to close with and destroy or capture the enemy. Planning</rdfs:comment>
        <rdfs:comment>Documentation: 		
						To conduct a type of offensive action using firepower and manoeuvre to close with and destroy or capture the enemy. Planning and coordination will normally be limited, as the attack will be carried out at short notice.	
					; Appinfo DisplayValue as &quot;Attack, hasty&quot;</rdfs:comment>
    </owl:NamedIndividual>
    


    <!-- http://www.sisostds.org/ontologies/lox#HIDE -->

    <owl:NamedIndividual rdf:about="http://www.sisostds.org/ontologies/lox#HIDE">
        <rdf:type rdf:resource="http://www.sisostds.org/ontologies/C2SIM#TaskActionCode"/>
        <rdfs:comment>Hide: To occupy an area in which an ORGANISATION or FACILITY may conceal itself before operations or before moving into battle positions.</rdfs:comment>
    </owl:NamedIndividual>
    


    <!-- http://www.sisostds.org/ontologies/lox#HLDDEF -->

    <owl:NamedIndividual rdf:about="http://www.sisostds.org/ontologies/lox#HLDDEF">
        <rdf:type rdf:resource="http://www.sisostds.org/ontologies/C2SIM#TaskActionCode"/>
        <rdfs:comment>Hold, defensive: To maintain or retain possession by force, a position or area in defensive operations.</rdfs:comment>
    </owl:NamedIndividual>
    


    <!-- http://www.sisostds.org/ontologies/lox#HLDOFF -->

    <owl:NamedIndividual rdf:about="http://www.sisostds.org/ontologies/lox#HLDOFF">
        <rdf:type rdf:resource="http://www.sisostds.org/ontologies/C2SIM#TaskActionCode"/>
        <rdfs:comment>Hold, offensive: To exert sufficient pressure in an offensive operation by means of combat power, to prevent the movement or redeployment of</rdfs:comment>
    </owl:NamedIndividual>
    


    <!-- http://www.sisostds.org/ontologies/lox#HONASP -->

    <owl:NamedIndividual rdf:about="http://www.sisostds.org/ontologies/lox#HONASP">
        <rdf:type rdf:resource="http://www.sisostds.org/ontologies/C2SIM#TaskActionCode"/>
        <rdfs:comment>Documentation: 		
						Civil and military assistance rendered in peace, crisis and war by a host nation to Allied forces and NATO organisations which are located on or in transit through the host nation&apos;s territory. The basis of such assistance is commitments arising from the NATO Alliance or from bilateral or multilateral agreements concluded between the host nation, NATO organisations and (the) nation(s) having forces operating on the host nation&apos;s territory.	
					; Appinfo DisplayValue as &quot;Host nation support&quot;</rdfs:comment>
        <rdfs:comment>Host nation support: Civil and military assistance rendered in peace, crisis and war by a host nation to Allied forces and NATO organisations which</rdfs:comment>
    </owl:NamedIndividual>
    


    <!-- http://www.sisostds.org/ontologies/lox#HSA -->

    <owl:NamedIndividual rdf:about="http://www.sisostds.org/ontologies/lox#HSA">
        <rdf:type rdf:resource="http://www.sisostds.org/ontologies/lox#TaskFunctionalAssociationCode"/>
        <rdfs:comment>Has as a sub-ACTION: The value that links two activities such that the subject ACTION has as a sub-ACTION the object ACTION.</rdfs:comment>
    </owl:NamedIndividual>
    


    <!-- http://www.sisostds.org/ontologies/lox#IDENT -->

    <owl:NamedIndividual rdf:about="http://www.sisostds.org/ontologies/lox#IDENT">
        <rdf:type rdf:resource="http://www.sisostds.org/ontologies/C2SIM#TaskActionCode"/>
        <rdfs:comment>Identify: To determine the identification of a particular class of object, recognising the friendly or enemy character of an object,</rdfs:comment>
    </owl:NamedIndividual>
    


    <!-- http://www.sisostds.org/ontologies/lox#IDENTP -->

    <owl:NamedIndividual rdf:about="http://www.sisostds.org/ontologies/lox#IDENTP">
        <rdf:type rdf:resource="http://www.sisostds.org/ontologies/C2SIM#TaskActionCode"/>
        <rdfs:comment>Identify, precise: To determine by any act or means additional information of a detected person, object or phenomenon, in a detailed, accurate</rdfs:comment>
    </owl:NamedIndividual>
    


    <!-- http://www.sisostds.org/ontologies/lox#IDNT -->

    <owl:NamedIndividual rdf:about="http://www.sisostds.org/ontologies/lox#IDNT">
        <rdfs:comment>Documentation: 		
						The ACTION objective has been either identified (i.e., classified as friend/foe/neutral) or recognised (i.e., the unit designation of the ORGANISATION or object is known).	
					; Appinfo DisplayValue as &quot;Identified&quot;</rdfs:comment>
    </owl:NamedIndividual>
    


    <!-- http://www.sisostds.org/ontologies/lox#ILLUMN -->

    <owl:NamedIndividual rdf:about="http://www.sisostds.org/ontologies/lox#ILLUMN">
        <rdf:type rdf:resource="http://www.sisostds.org/ontologies/C2SIM#TaskActionCode"/>
        <rdfs:comment>Documentation: 		
						The temporary supply of IR or white-light illumination (usually in coordination with direct or indirect fire).	
					; Appinfo DisplayValue as &quot;Illuminated&quot;</rdfs:comment>
        <rdfs:comment>Illuminate: To provide battlespace lighting by employing searchlight or pyrotechnic illuminants using diffusion or reflection.</rdfs:comment>
    </owl:NamedIndividual>
    


    <!-- http://www.sisostds.org/ontologies/lox#IMINGT -->

    <owl:NamedIndividual rdf:about="http://www.sisostds.org/ontologies/lox#IMINGT">
        <rdf:type rdf:resource="http://www.sisostds.org/ontologies/C2SIM#TaskActionCode"/>
        <rdfs:comment>Imagery intelligence gathering: To gather imagery for intelligence purposes.</rdfs:comment>
    </owl:NamedIndividual>
    


    <!-- http://www.sisostds.org/ontologies/lox#IMO -->

    <owl:NamedIndividual rdf:about="http://www.sisostds.org/ontologies/lox#IMO">
        <rdf:type rdf:resource="http://www.sisostds.org/ontologies/lox#TaskFunctionalAssociationCode"/>
        <rdfs:comment>Is a modification of: The value denoting that the subject ACTION amends (or suggests an amendment to) an existing object ACTION (be it a plan, order,</rdfs:comment>
    </owl:NamedIndividual>
    


    <!-- http://www.sisostds.org/ontologies/lox#INFILT -->

    <owl:NamedIndividual rdf:about="http://www.sisostds.org/ontologies/lox#INFILT">
        <rdf:type rdf:resource="http://www.sisostds.org/ontologies/C2SIM#TaskActionCode"/>
        <rdfs:comment>Documentation: 		
						To move a force, broken down as individuals or small groups, over, through or around enemy positions with the aim of avoiding detection.	
					; Appinfo DisplayValue as &quot;Infiltrate&quot;</rdfs:comment>
        <rdfs:comment>Infiltrate: To move a force, broken down as individuals or small groups, over, through or around enemy positions with the aim of avoiding</rdfs:comment>
    </owl:NamedIndividual>
    


    <!-- http://www.sisostds.org/ontologies/lox#INFOOP -->

    <owl:NamedIndividual rdf:about="http://www.sisostds.org/ontologies/lox#INFOOP">
        <rdf:type rdf:resource="http://www.sisostds.org/ontologies/C2SIM#TaskActionCode"/>
        <rdfs:comment>Information operations: To conduct an operation that includes actions to influence decision makers in support of political and military objectives</rdfs:comment>
    </owl:NamedIndividual>
    


    <!-- http://www.sisostds.org/ontologies/lox#INRSTO -->

    <owl:NamedIndividual rdf:about="http://www.sisostds.org/ontologies/lox#INRSTO">
        <rdf:type rdf:resource="http://www.sisostds.org/ontologies/lox#TaskFunctionalAssociationCode"/>
        <rdfs:comment>In response to: The value that links two ACTIONs such that the subject ACTION is planned to be or may be expected to be carried out in reaction</rdfs:comment>
    </owl:NamedIndividual>
    


    <!-- http://www.sisostds.org/ontologies/lox#INTCEP -->

    <owl:NamedIndividual rdf:about="http://www.sisostds.org/ontologies/lox#INTCEP">
        <rdf:type rdf:resource="http://www.sisostds.org/ontologies/C2SIM#TaskActionCode"/>
        <rdfs:comment>Intercept: To conduct Electronic Warfare Support operations with a view to searching, locating, recording and analysing radiated electromagnetic</rdfs:comment>
    </owl:NamedIndividual>
    


    <!-- http://www.sisostds.org/ontologies/lox#INTCOL -->

    <owl:NamedIndividual rdf:about="http://www.sisostds.org/ontologies/lox#INTCOL">
        <rdf:type rdf:resource="http://www.sisostds.org/ontologies/C2SIM#TaskActionCode"/>
        <rdfs:comment>Intelligence collection: To gather information from all available sources to meet an intelligence requirement. Specifically, a logical plan for transforming</rdfs:comment>
    </owl:NamedIndividual>
    


    <!-- http://www.sisostds.org/ontologies/lox#INTDCT -->

    <owl:NamedIndividual rdf:about="http://www.sisostds.org/ontologies/lox#INTDCT">
        <rdf:type rdf:resource="http://www.sisostds.org/ontologies/C2SIM#TaskActionCode"/>
        <rdfs:comment>Documentation: 		
						To divert, disrupt, delay, or destroy the enemy&apos;s surface military potential before it can be used effectively against friendly forces.	
					; Appinfo DisplayValue as &quot;Interdict&quot;</rdfs:comment>
        <rdfs:comment>Interdict: To divert, disrupt, delay, or destroy the enemy&apos;s surface military potential before it can be used effectively against friendly</rdfs:comment>
    </owl:NamedIndividual>
    


    <!-- http://www.sisostds.org/ontologies/lox#INTREC -->

    <owl:NamedIndividual rdf:about="http://www.sisostds.org/ontologies/lox#INTREC">
        <rdfs:comment>Documentation: 		
						An equipment lost in an area unsuitable for recovery due to political, military or geographic/environmental considerations.	
					; Appinfo DisplayValue as &quot;Intact but unrecoverable&quot;</rdfs:comment>
    </owl:NamedIndividual>
    


    <!-- http://www.sisostds.org/ontologies/lox#IOT -->

    <owl:NamedIndividual rdf:about="http://www.sisostds.org/ontologies/lox#IOT">
        <rdf:type rdf:resource="http://www.sisostds.org/ontologies/lox#TaskFunctionalAssociationCode"/>
        <rdfs:comment>In order that: The subject ACTION is to be carried out so that the conditions are established for the completion of the object ACTION (e.g.,</rdfs:comment>
    </owl:NamedIndividual>
    


    <!-- http://www.sisostds.org/ontologies/lox#ISAPRQ -->

    <owl:NamedIndividual rdf:about="http://www.sisostds.org/ontologies/lox#ISAPRQ">
        <rdf:type rdf:resource="http://www.sisostds.org/ontologies/lox#TaskFunctionalAssociationCode"/>
        <rdfs:comment>Is a prerequisite for: The subject ACTION must be completed as planned before the object ACTION may commence.</rdfs:comment>
    </owl:NamedIndividual>
    


    <!-- http://www.sisostds.org/ontologies/lox#ISCAUS -->

    <owl:NamedIndividual rdf:about="http://www.sisostds.org/ontologies/lox#ISCAUS">
        <rdf:type rdf:resource="http://www.sisostds.org/ontologies/lox#TaskFunctionalAssociationCode"/>
        <rdfs:comment>Is the cause of: The value denoting that the subject ACTION is the cause for the object ACTION. (Note: This is intended to be used only when</rdfs:comment>
    </owl:NamedIndividual>
    


    <!-- http://www.sisostds.org/ontologies/lox#ISOLAT -->

    <owl:NamedIndividual rdf:about="http://www.sisostds.org/ontologies/lox#ISOLAT">
        <rdf:type rdf:resource="http://www.sisostds.org/ontologies/C2SIM#TaskActionCode"/>
        <rdfs:comment>Documentation: 		
						To seal off (both physically and psychologically) an enemy from its sources of support, to deny an enemy freedom of movement, and prevent an enemy unit from having contact with other enemy forces. An enemy must not be allowed sanctuary within its present position.	
					; Appinfo DisplayValue as &quot;Isolate&quot;</rdfs:comment>
        <rdfs:comment>Isolate: To seal off (both physically and psychologically) an enemy from its sources of support, to deny an enemy freedom of movement,</rdfs:comment>
    </owl:NamedIndividual>
    


    <!-- http://www.sisostds.org/ontologies/lox#ISSMDA -->

    <owl:NamedIndividual rdf:about="http://www.sisostds.org/ontologies/lox#ISSMDA">
        <rdf:type rdf:resource="http://www.sisostds.org/ontologies/C2SIM#TaskActionCode"/>
        <rdfs:comment>Issue media article: To send forth; publish; put into circulation a non-fictional essay, especially one included with others in a newspaper, magazine,</rdfs:comment>
    </owl:NamedIndividual>
    


    <!-- http://www.sisostds.org/ontologies/lox#ISSMDD -->

    <owl:NamedIndividual rdf:about="http://www.sisostds.org/ontologies/lox#ISSMDD">
        <rdf:type rdf:resource="http://www.sisostds.org/ontologies/C2SIM#TaskActionCode"/>
        <rdfs:comment>Issue media documentary: To send forth; publish; put into circulation any document published on a media that provides a factual record or report.</rdfs:comment>
    </owl:NamedIndividual>
    


    <!-- http://www.sisostds.org/ontologies/lox#ISSPRS -->

    <owl:NamedIndividual rdf:about="http://www.sisostds.org/ontologies/lox#ISSPRS">
        <rdf:type rdf:resource="http://www.sisostds.org/ontologies/C2SIM#TaskActionCode"/>
        <rdfs:comment>Issue press release: To send forth; publish; put into circulation an official statement issued to media for information.</rdfs:comment>
    </owl:NamedIndividual>
    


    <!-- http://www.sisostds.org/ontologies/lox#JAM -->

    <owl:NamedIndividual rdf:about="http://www.sisostds.org/ontologies/lox#JAM">
        <rdf:type rdf:resource="http://www.sisostds.org/ontologies/C2SIM#TaskActionCode"/>
        <rdfs:comment>Jam: To deliberately radiate, re-radiate or reflect electromagnetic energy with the object of impairing the use of electronic devices,</rdfs:comment>
    </owl:NamedIndividual>
    


    <!-- http://www.sisostds.org/ontologies/lox#KILL -->

    <owl:NamedIndividual rdf:about="http://www.sisostds.org/ontologies/lox#KILL">
        <rdfs:comment>Documentation: 		
						A casualty who is killed outright or dies as a result of wounds, disease or other injuries.	
					; Appinfo DisplayValue as &quot;Killed&quot;</rdfs:comment>
    </owl:NamedIndividual>
    


    <!-- http://www.sisostds.org/ontologies/lox#LAY -->

    <owl:NamedIndividual rdf:about="http://www.sisostds.org/ontologies/lox#LAY">
        <rdf:type rdf:resource="http://www.sisostds.org/ontologies/C2SIM#TaskActionCode"/>
        <rdfs:comment>Lay: To place on a surface, esp. horizontally or in the proper or specified place.</rdfs:comment>
    </owl:NamedIndividual>
    


    <!-- http://www.sisostds.org/ontologies/lox#LDAM -->

    <owl:NamedIndividual rdf:about="http://www.sisostds.org/ontologies/lox#LDAM">
        <rdfs:comment>Documentation: 		
						The subjective categorisation of the physical effect of an ACTION on buildings, infrastructure and/or equipment by a reporting ORGANISATION.	
					; Appinfo DisplayValue as &quot;Light damage&quot;</rdfs:comment>
    </owl:NamedIndividual>
    


    <!-- http://www.sisostds.org/ontologies/lox#LEAGR -->

    <owl:NamedIndividual rdf:about="http://www.sisostds.org/ontologies/lox#LEAGR">
        <rdf:type rdf:resource="http://www.sisostds.org/ontologies/C2SIM#TaskActionCode"/>
        <rdfs:comment>Leaguer: To adopt a defended formation as a temporary defensive measure in areas of low or moderate risk of combat (usually applied</rdfs:comment>
    </owl:NamedIndividual>
    


    <!-- http://www.sisostds.org/ontologies/lox#LGTRST -->

    <owl:NamedIndividual rdf:about="http://www.sisostds.org/ontologies/lox#LGTRST">
        <rdfs:comment>Documentation: 		
						The ACTION-OBJECTIVE reacted against the ACTION using light physical violence.	
					; Appinfo DisplayValue as &quot;Light resistance&quot;</rdfs:comment>
    </owl:NamedIndividual>
    


    <!-- http://www.sisostds.org/ontologies/lox#LIFT -->

    <owl:NamedIndividual rdf:about="http://www.sisostds.org/ontologies/lox#LIFT">
        <rdf:type rdf:resource="http://www.sisostds.org/ontologies/C2SIM#TaskActionCode"/>
        <rdfs:comment>Lift: To transport assets using non-organic means, by sea, land or air.</rdfs:comment>
    </owl:NamedIndividual>
    


    <!-- http://www.sisostds.org/ontologies/lox#LIFTAD -->

    <owl:NamedIndividual rdf:about="http://www.sisostds.org/ontologies/lox#LIFTAD">
        <rdf:type rdf:resource="http://www.sisostds.org/ontologies/C2SIM#TaskActionCode"/>
        <rdfs:comment>Lift, administrative: Airlift normally provided by specifically identifiable aircraft assigned to organisations or commands for internal administration.</rdfs:comment>
    </owl:NamedIndividual>
    


    <!-- http://www.sisostds.org/ontologies/lox#LOCATE -->

    <owl:NamedIndividual rdf:about="http://www.sisostds.org/ontologies/lox#LOCATE">
        <rdf:type rdf:resource="http://www.sisostds.org/ontologies/C2SIM#TaskActionCode"/>
        <rdfs:comment>Documentation: 		
						To establish the position or presence of an object.	
					; Appinfo DisplayValue as &quot;Locate&quot;</rdfs:comment>
        <rdfs:comment>Locate: To establish the position or presence of an object.</rdfs:comment>
    </owl:NamedIndividual>
    


    <!-- http://www.sisostds.org/ontologies/lox#LOST -->

    <owl:NamedIndividual rdf:about="http://www.sisostds.org/ontologies/lox#LOST">
        <rdfs:comment>Documentation: 		
						The object is no longer available for military operations.	
					; Appinfo DisplayValue as &quot;Lost&quot;</rdfs:comment>
    </owl:NamedIndividual>
    


    <!-- http://www.sisostds.org/ontologies/lox#MAINTN -->

    <owl:NamedIndividual rdf:about="http://www.sisostds.org/ontologies/lox#MAINTN">
        <rdf:type rdf:resource="http://www.sisostds.org/ontologies/C2SIM#TaskActionCode"/>
        <rdfs:comment>Maintain: To provide services to keep equipment in condition to carry out its function.</rdfs:comment>
    </owl:NamedIndividual>
    


    <!-- http://www.sisostds.org/ontologies/lox#MAP -->

    <owl:NamedIndividual rdf:about="http://www.sisostds.org/ontologies/lox#MAP">
        <rdf:type rdf:resource="http://www.sisostds.org/ontologies/C2SIM#TaskActionCode"/>
        <rdfs:comment>Map: To create a graphic representation, usually on a plane surface and at an established scale, of natural or artificial features</rdfs:comment>
    </owl:NamedIndividual>
    


    <!-- http://www.sisostds.org/ontologies/lox#MARK -->

    <owl:NamedIndividual rdf:about="http://www.sisostds.org/ontologies/lox#MARK">
        <rdf:type rdf:resource="http://www.sisostds.org/ontologies/C2SIM#TaskActionCode"/>
        <rdfs:comment>Mark: To make visible (by the use of light/IR/laser/arty) an object in order to allow its identification by another object (usually</rdfs:comment>
    </owl:NamedIndividual>
    


    <!-- http://www.sisostds.org/ontologies/lox#MASSFR -->

    <owl:NamedIndividual rdf:about="http://www.sisostds.org/ontologies/lox#MASSFR">
        <rdf:type rdf:resource="http://www.sisostds.org/ontologies/C2SIM#TaskActionCode"/>
        <rdfs:comment>Mass forces: To concentrate large quantities of military equipment and personnel.</rdfs:comment>
    </owl:NamedIndividual>
    


    <!-- http://www.sisostds.org/ontologies/lox#MCM11 -->

    <owl:NamedIndividual rdf:about="http://www.sisostds.org/ontologies/lox#MCM11">
        <rdf:type rdf:resource="http://www.sisostds.org/ontologies/C2SIM#TaskActionCode"/>
        <rdfs:comment>MCM operation stage 11: Mine Counter Measure operation stage 11.</rdfs:comment>
    </owl:NamedIndividual>
    


    <!-- http://www.sisostds.org/ontologies/lox#MCM12 -->

    <owl:NamedIndividual rdf:about="http://www.sisostds.org/ontologies/lox#MCM12">
        <rdf:type rdf:resource="http://www.sisostds.org/ontologies/C2SIM#TaskActionCode"/>
        <rdfs:comment>MCM operation stage 12: Mine Counter Measure operation stage 12.</rdfs:comment>
    </owl:NamedIndividual>
    


    <!-- http://www.sisostds.org/ontologies/lox#MCM13 -->

    <owl:NamedIndividual rdf:about="http://www.sisostds.org/ontologies/lox#MCM13">
        <rdf:type rdf:resource="http://www.sisostds.org/ontologies/C2SIM#TaskActionCode"/>
        <rdfs:comment>MCM operation stage 13: Mine Counter Measure operation stage 13.</rdfs:comment>
    </owl:NamedIndividual>
    


    <!-- http://www.sisostds.org/ontologies/lox#MCM14 -->

    <owl:NamedIndividual rdf:about="http://www.sisostds.org/ontologies/lox#MCM14">
        <rdf:type rdf:resource="http://www.sisostds.org/ontologies/C2SIM#TaskActionCode"/>
        <rdfs:comment>MCM operation stage 14: Mine Counter Measure operation stage 14.</rdfs:comment>
    </owl:NamedIndividual>
    


    <!-- http://www.sisostds.org/ontologies/lox#MCM31 -->

    <owl:NamedIndividual rdf:about="http://www.sisostds.org/ontologies/lox#MCM31">
        <rdf:type rdf:resource="http://www.sisostds.org/ontologies/C2SIM#TaskActionCode"/>
        <rdfs:comment>MCM operation stage 31: Mine Counter Measure operation stage 31.</rdfs:comment>
    </owl:NamedIndividual>
    


    <!-- http://www.sisostds.org/ontologies/lox#MCM32 -->

    <owl:NamedIndividual rdf:about="http://www.sisostds.org/ontologies/lox#MCM32">
        <rdf:type rdf:resource="http://www.sisostds.org/ontologies/C2SIM#TaskActionCode"/>
        <rdfs:comment>MCM operation stage 32: Mine Counter Measure operation stage 32.</rdfs:comment>
    </owl:NamedIndividual>
    


    <!-- http://www.sisostds.org/ontologies/lox#MCM33 -->

    <owl:NamedIndividual rdf:about="http://www.sisostds.org/ontologies/lox#MCM33">
        <rdf:type rdf:resource="http://www.sisostds.org/ontologies/C2SIM#TaskActionCode"/>
        <rdfs:comment>MCM operation stage 33: Mine Counter Measure operation stage 33.</rdfs:comment>
    </owl:NamedIndividual>
    


    <!-- http://www.sisostds.org/ontologies/lox#MCM34 -->

    <owl:NamedIndividual rdf:about="http://www.sisostds.org/ontologies/lox#MCM34">
        <rdf:type rdf:resource="http://www.sisostds.org/ontologies/C2SIM#TaskActionCode"/>
        <rdfs:comment>MCM operation stage 34: Mine Counter Measure operation stage 34.</rdfs:comment>
    </owl:NamedIndividual>
    


    <!-- http://www.sisostds.org/ontologies/lox#MCM35 -->

    <owl:NamedIndividual rdf:about="http://www.sisostds.org/ontologies/lox#MCM35">
        <rdf:type rdf:resource="http://www.sisostds.org/ontologies/C2SIM#TaskActionCode"/>
        <rdfs:comment>MCM operation stage 35: Mine Counter Measure operation stage 35.</rdfs:comment>
    </owl:NamedIndividual>
    


    <!-- http://www.sisostds.org/ontologies/lox#MCM36 -->

    <owl:NamedIndividual rdf:about="http://www.sisostds.org/ontologies/lox#MCM36">
        <rdf:type rdf:resource="http://www.sisostds.org/ontologies/C2SIM#TaskActionCode"/>
        <rdfs:comment>MCM operation stage 36: Mine Counter Measure operation stage 36.</rdfs:comment>
    </owl:NamedIndividual>
    


    <!-- http://www.sisostds.org/ontologies/lox#MCM37 -->

    <owl:NamedIndividual rdf:about="http://www.sisostds.org/ontologies/lox#MCM37">
        <rdf:type rdf:resource="http://www.sisostds.org/ontologies/C2SIM#TaskActionCode"/>
        <rdfs:comment>MCM operation stage 37: Mine Counter Measure operation stage 37.</rdfs:comment>
    </owl:NamedIndividual>
    


    <!-- http://www.sisostds.org/ontologies/lox#MCM38 -->

    <owl:NamedIndividual rdf:about="http://www.sisostds.org/ontologies/lox#MCM38">
        <rdf:type rdf:resource="http://www.sisostds.org/ontologies/C2SIM#TaskActionCode"/>
        <rdfs:comment>MCM operation stage 38: Mine Counter Measure operation stage 38.</rdfs:comment>
    </owl:NamedIndividual>
    


    <!-- http://www.sisostds.org/ontologies/lox#MCM39 -->

    <owl:NamedIndividual rdf:about="http://www.sisostds.org/ontologies/lox#MCM39">
        <rdf:type rdf:resource="http://www.sisostds.org/ontologies/C2SIM#TaskActionCode"/>
        <rdfs:comment>MCM operation stage 39: Mine Counter Measure operation stage 39.</rdfs:comment>
    </owl:NamedIndividual>
    


    <!-- http://www.sisostds.org/ontologies/lox#MCM41 -->

    <owl:NamedIndividual rdf:about="http://www.sisostds.org/ontologies/lox#MCM41">
        <rdf:type rdf:resource="http://www.sisostds.org/ontologies/C2SIM#TaskActionCode"/>
        <rdfs:comment>MCM operation stage 41: Mine Counter Measure operation stage 41.</rdfs:comment>
    </owl:NamedIndividual>
    


    <!-- http://www.sisostds.org/ontologies/lox#MCM42 -->

    <owl:NamedIndividual rdf:about="http://www.sisostds.org/ontologies/lox#MCM42">
        <rdf:type rdf:resource="http://www.sisostds.org/ontologies/C2SIM#TaskActionCode"/>
        <rdfs:comment>MCM operation stage 42: Mine Counter Measure operation stage 42.</rdfs:comment>
    </owl:NamedIndividual>
    


    <!-- http://www.sisostds.org/ontologies/lox#MCM43 -->

    <owl:NamedIndividual rdf:about="http://www.sisostds.org/ontologies/lox#MCM43">
        <rdf:type rdf:resource="http://www.sisostds.org/ontologies/C2SIM#TaskActionCode"/>
        <rdfs:comment>MCM operation stage 43: Mine Counter Measure operation stage 43.</rdfs:comment>
    </owl:NamedIndividual>
    


    <!-- http://www.sisostds.org/ontologies/lox#MCM44 -->

    <owl:NamedIndividual rdf:about="http://www.sisostds.org/ontologies/lox#MCM44">
        <rdf:type rdf:resource="http://www.sisostds.org/ontologies/C2SIM#TaskActionCode"/>
        <rdfs:comment>MCM operation stage 44: Mine Counter Measure operation stage 44.</rdfs:comment>
    </owl:NamedIndividual>
    


    <!-- http://www.sisostds.org/ontologies/lox#MCM45 -->

    <owl:NamedIndividual rdf:about="http://www.sisostds.org/ontologies/lox#MCM45">
        <rdf:type rdf:resource="http://www.sisostds.org/ontologies/C2SIM#TaskActionCode"/>
        <rdfs:comment>MCM operation stage 45: Mine Counter Measure operation stage 45.</rdfs:comment>
    </owl:NamedIndividual>
    


    <!-- http://www.sisostds.org/ontologies/lox#MCM46 -->

    <owl:NamedIndividual rdf:about="http://www.sisostds.org/ontologies/lox#MCM46">
        <rdf:type rdf:resource="http://www.sisostds.org/ontologies/C2SIM#TaskActionCode"/>
        <rdfs:comment>MCM operation stage 46: Mine Counter Measure operation stage 46.</rdfs:comment>
    </owl:NamedIndividual>
    


    <!-- http://www.sisostds.org/ontologies/lox#MCM47 -->

    <owl:NamedIndividual rdf:about="http://www.sisostds.org/ontologies/lox#MCM47">
        <rdf:type rdf:resource="http://www.sisostds.org/ontologies/C2SIM#TaskActionCode"/>
        <rdfs:comment>MCM operation stage 47: Mine Counter Measure operation stage 47.</rdfs:comment>
    </owl:NamedIndividual>
    


    <!-- http://www.sisostds.org/ontologies/lox#MCM48 -->

    <owl:NamedIndividual rdf:about="http://www.sisostds.org/ontologies/lox#MCM48">
        <rdf:type rdf:resource="http://www.sisostds.org/ontologies/C2SIM#TaskActionCode"/>
        <rdfs:comment>MCM operation stage 48: Mine Counter Measure operation stage 48.</rdfs:comment>
    </owl:NamedIndividual>
    


    <!-- http://www.sisostds.org/ontologies/lox#MCM50 -->

    <owl:NamedIndividual rdf:about="http://www.sisostds.org/ontologies/lox#MCM50">
        <rdf:type rdf:resource="http://www.sisostds.org/ontologies/C2SIM#TaskActionCode"/>
        <rdfs:comment>MCM operation stage 50: Mine Counter Measure operation stage 50.</rdfs:comment>
    </owl:NamedIndividual>
    


    <!-- http://www.sisostds.org/ontologies/lox#MCM51 -->

    <owl:NamedIndividual rdf:about="http://www.sisostds.org/ontologies/lox#MCM51">
        <rdf:type rdf:resource="http://www.sisostds.org/ontologies/C2SIM#TaskActionCode"/>
        <rdfs:comment>MCM operation stage 51: Mine Counter Measure operation stage 51.</rdfs:comment>
    </owl:NamedIndividual>
    


    <!-- http://www.sisostds.org/ontologies/lox#MCM52 -->

    <owl:NamedIndividual rdf:about="http://www.sisostds.org/ontologies/lox#MCM52">
        <rdf:type rdf:resource="http://www.sisostds.org/ontologies/C2SIM#TaskActionCode"/>
        <rdfs:comment>MCM operation stage 52: Mine Counter Measure operation stage 52.</rdfs:comment>
    </owl:NamedIndividual>
    


    <!-- http://www.sisostds.org/ontologies/lox#MCM53 -->

    <owl:NamedIndividual rdf:about="http://www.sisostds.org/ontologies/lox#MCM53">
        <rdf:type rdf:resource="http://www.sisostds.org/ontologies/C2SIM#TaskActionCode"/>
        <rdfs:comment>MCM operation stage 53: Mine Counter Measure operation stage 53.</rdfs:comment>
    </owl:NamedIndividual>
    


    <!-- http://www.sisostds.org/ontologies/lox#MCM54 -->

    <owl:NamedIndividual rdf:about="http://www.sisostds.org/ontologies/lox#MCM54">
        <rdf:type rdf:resource="http://www.sisostds.org/ontologies/C2SIM#TaskActionCode"/>
        <rdfs:comment>MCM operation stage 54: Mine Counter Measure operation stage 54.</rdfs:comment>
    </owl:NamedIndividual>
    


    <!-- http://www.sisostds.org/ontologies/lox#MCM55 -->

    <owl:NamedIndividual rdf:about="http://www.sisostds.org/ontologies/lox#MCM55">
        <rdf:type rdf:resource="http://www.sisostds.org/ontologies/C2SIM#TaskActionCode"/>
        <rdfs:comment>MCM operation stage 55: Mine Counter Measure operation stage 55.</rdfs:comment>
    </owl:NamedIndividual>
    


    <!-- http://www.sisostds.org/ontologies/lox#MCM56 -->

    <owl:NamedIndividual rdf:about="http://www.sisostds.org/ontologies/lox#MCM56">
        <rdf:type rdf:resource="http://www.sisostds.org/ontologies/C2SIM#TaskActionCode"/>
        <rdfs:comment>MCM operation stage 56: Mine Counter Measure operation stage 56.</rdfs:comment>
    </owl:NamedIndividual>
    


    <!-- http://www.sisostds.org/ontologies/lox#MCM57 -->

    <owl:NamedIndividual rdf:about="http://www.sisostds.org/ontologies/lox#MCM57">
        <rdf:type rdf:resource="http://www.sisostds.org/ontologies/C2SIM#TaskActionCode"/>
        <rdfs:comment>MCM operation stage 57: Mine Counter Measure operation stage 57.</rdfs:comment>
    </owl:NamedIndividual>
    


    <!-- http://www.sisostds.org/ontologies/lox#MCM58A -->

    <owl:NamedIndividual rdf:about="http://www.sisostds.org/ontologies/lox#MCM58A">
        <rdf:type rdf:resource="http://www.sisostds.org/ontologies/C2SIM#TaskActionCode"/>
        <rdfs:comment>MCM operation stage 58A: Mine Counter Measure operation stage 58A.</rdfs:comment>
    </owl:NamedIndividual>
    


    <!-- http://www.sisostds.org/ontologies/lox#MCM58B -->

    <owl:NamedIndividual rdf:about="http://www.sisostds.org/ontologies/lox#MCM58B">
        <rdf:type rdf:resource="http://www.sisostds.org/ontologies/C2SIM#TaskActionCode"/>
        <rdfs:comment>MCM operation stage 58B: Mine Counter Measure operation stage 58B.</rdfs:comment>
    </owl:NamedIndividual>
    


    <!-- http://www.sisostds.org/ontologies/lox#MCM58C -->

    <owl:NamedIndividual rdf:about="http://www.sisostds.org/ontologies/lox#MCM58C">
        <rdf:type rdf:resource="http://www.sisostds.org/ontologies/C2SIM#TaskActionCode"/>
        <rdfs:comment>MCM operation stage 58C: Mine Counter Measure operation stage 58C.</rdfs:comment>
    </owl:NamedIndividual>
    


    <!-- http://www.sisostds.org/ontologies/lox#MCM59 -->

    <owl:NamedIndividual rdf:about="http://www.sisostds.org/ontologies/lox#MCM59">
        <rdf:type rdf:resource="http://www.sisostds.org/ontologies/C2SIM#TaskActionCode"/>
        <rdfs:comment>MCM operation stage 59: Mine Counter Measure operation stage 59.</rdfs:comment>
    </owl:NamedIndividual>
    


    <!-- http://www.sisostds.org/ontologies/lox#MCM61 -->

    <owl:NamedIndividual rdf:about="http://www.sisostds.org/ontologies/lox#MCM61">
        <rdf:type rdf:resource="http://www.sisostds.org/ontologies/C2SIM#TaskActionCode"/>
        <rdfs:comment>MCM operation stage 61: Mine Counter Measure operation stage 61.</rdfs:comment>
    </owl:NamedIndividual>
    


    <!-- http://www.sisostds.org/ontologies/lox#MCM62 -->

    <owl:NamedIndividual rdf:about="http://www.sisostds.org/ontologies/lox#MCM62">
        <rdf:type rdf:resource="http://www.sisostds.org/ontologies/C2SIM#TaskActionCode"/>
        <rdfs:comment>MCM operation stage 62: Mine Counter Measure operation stage 62.</rdfs:comment>
    </owl:NamedIndividual>
    


    <!-- http://www.sisostds.org/ontologies/lox#MCM63 -->

    <owl:NamedIndividual rdf:about="http://www.sisostds.org/ontologies/lox#MCM63">
        <rdf:type rdf:resource="http://www.sisostds.org/ontologies/C2SIM#TaskActionCode"/>
        <rdfs:comment>MCM operation stage 63: Mine Counter Measure operation stage 63.</rdfs:comment>
    </owl:NamedIndividual>
    


    <!-- http://www.sisostds.org/ontologies/lox#MCM71 -->

    <owl:NamedIndividual rdf:about="http://www.sisostds.org/ontologies/lox#MCM71">
        <rdf:type rdf:resource="http://www.sisostds.org/ontologies/C2SIM#TaskActionCode"/>
        <rdfs:comment>MCM operation stage 71: Mine Counter Measure operation stage 71.</rdfs:comment>
    </owl:NamedIndividual>
    


    <!-- http://www.sisostds.org/ontologies/lox#MCM72 -->

    <owl:NamedIndividual rdf:about="http://www.sisostds.org/ontologies/lox#MCM72">
        <rdf:type rdf:resource="http://www.sisostds.org/ontologies/C2SIM#TaskActionCode"/>
        <rdfs:comment>MCM operation stage 72: Mine Counter Measure operation stage 72.</rdfs:comment>
    </owl:NamedIndividual>
    


    <!-- http://www.sisostds.org/ontologies/lox#MCM73 -->

    <owl:NamedIndividual rdf:about="http://www.sisostds.org/ontologies/lox#MCM73">
        <rdf:type rdf:resource="http://www.sisostds.org/ontologies/C2SIM#TaskActionCode"/>
        <rdfs:comment>MCM operation stage 73: Mine Counter Measure operation stage 73.</rdfs:comment>
    </owl:NamedIndividual>
    


    <!-- http://www.sisostds.org/ontologies/lox#MCM74 -->

    <owl:NamedIndividual rdf:about="http://www.sisostds.org/ontologies/lox#MCM74">
        <rdf:type rdf:resource="http://www.sisostds.org/ontologies/C2SIM#TaskActionCode"/>
        <rdfs:comment>MCM operation stage 74: Mine Counter Measure operation stage 74.</rdfs:comment>
    </owl:NamedIndividual>
    


    <!-- http://www.sisostds.org/ontologies/lox#MCM75 -->

    <owl:NamedIndividual rdf:about="http://www.sisostds.org/ontologies/lox#MCM75">
        <rdf:type rdf:resource="http://www.sisostds.org/ontologies/C2SIM#TaskActionCode"/>
        <rdfs:comment>MCM operation stage 75: Mine Counter Measure operation stage 75.</rdfs:comment>
    </owl:NamedIndividual>
    


    <!-- http://www.sisostds.org/ontologies/lox#MCM81 -->

    <owl:NamedIndividual rdf:about="http://www.sisostds.org/ontologies/lox#MCM81">
        <rdf:type rdf:resource="http://www.sisostds.org/ontologies/C2SIM#TaskActionCode"/>
        <rdfs:comment>MCM operation stage 81: Mine Counter Measure operation stage 81.</rdfs:comment>
    </owl:NamedIndividual>
    


    <!-- http://www.sisostds.org/ontologies/lox#MCM82 -->

    <owl:NamedIndividual rdf:about="http://www.sisostds.org/ontologies/lox#MCM82">
        <rdf:type rdf:resource="http://www.sisostds.org/ontologies/C2SIM#TaskActionCode"/>
        <rdfs:comment>MCM operation stage 82: Mine Counter Measure operation stage 82.</rdfs:comment>
    </owl:NamedIndividual>
    


    <!-- http://www.sisostds.org/ontologies/lox#MCM83 -->

    <owl:NamedIndividual rdf:about="http://www.sisostds.org/ontologies/lox#MCM83">
        <rdf:type rdf:resource="http://www.sisostds.org/ontologies/C2SIM#TaskActionCode"/>
        <rdfs:comment>MCM operation stage 83: Mine Counter Measure operation stage 83.</rdfs:comment>
    </owl:NamedIndividual>
    


    <!-- http://www.sisostds.org/ontologies/lox#MCM84 -->

    <owl:NamedIndividual rdf:about="http://www.sisostds.org/ontologies/lox#MCM84">
        <rdf:type rdf:resource="http://www.sisostds.org/ontologies/C2SIM#TaskActionCode"/>
        <rdfs:comment>MCM operation stage 84: Mine Counter Measure operation stage 84.</rdfs:comment>
    </owl:NamedIndividual>
    


    <!-- http://www.sisostds.org/ontologies/lox#MCM85 -->

    <owl:NamedIndividual rdf:about="http://www.sisostds.org/ontologies/lox#MCM85">
        <rdf:type rdf:resource="http://www.sisostds.org/ontologies/C2SIM#TaskActionCode"/>
        <rdfs:comment>MCM operation stage 85: Mine Counter Measure operation stage 85.</rdfs:comment>
    </owl:NamedIndividual>
    


    <!-- http://www.sisostds.org/ontologies/lox#MCM86 -->

    <owl:NamedIndividual rdf:about="http://www.sisostds.org/ontologies/lox#MCM86">
        <rdf:type rdf:resource="http://www.sisostds.org/ontologies/C2SIM#TaskActionCode"/>
        <rdfs:comment>MCM operation stage 86: Mine Counter Measure operation stage 86.</rdfs:comment>
    </owl:NamedIndividual>
    


    <!-- http://www.sisostds.org/ontologies/lox#MCM87 -->

    <owl:NamedIndividual rdf:about="http://www.sisostds.org/ontologies/lox#MCM87">
        <rdf:type rdf:resource="http://www.sisostds.org/ontologies/C2SIM#TaskActionCode"/>
        <rdfs:comment>MCM operation stage 87: Mine Counter Measure operation stage 87.</rdfs:comment>
    </owl:NamedIndividual>
    


    <!-- http://www.sisostds.org/ontologies/lox#MCM88 -->

    <owl:NamedIndividual rdf:about="http://www.sisostds.org/ontologies/lox#MCM88">
        <rdf:type rdf:resource="http://www.sisostds.org/ontologies/C2SIM#TaskActionCode"/>
        <rdfs:comment>MCM operation stage 88: Mine Counter Measure operation stage 88.</rdfs:comment>
    </owl:NamedIndividual>
    


    <!-- http://www.sisostds.org/ontologies/lox#MCM89 -->

    <owl:NamedIndividual rdf:about="http://www.sisostds.org/ontologies/lox#MCM89">
        <rdf:type rdf:resource="http://www.sisostds.org/ontologies/C2SIM#TaskActionCode"/>
        <rdfs:comment>MCM operation stage 89: Mine Counter Measure operation stage 89.</rdfs:comment>
    </owl:NamedIndividual>
    


    <!-- http://www.sisostds.org/ontologies/lox#MCM91 -->

    <owl:NamedIndividual rdf:about="http://www.sisostds.org/ontologies/lox#MCM91">
        <rdf:type rdf:resource="http://www.sisostds.org/ontologies/C2SIM#TaskActionCode"/>
        <rdfs:comment>MCM operation stage 91: Mine Counter Measure operation stage 91.</rdfs:comment>
    </owl:NamedIndividual>
    


    <!-- http://www.sisostds.org/ontologies/lox#MCM92 -->

    <owl:NamedIndividual rdf:about="http://www.sisostds.org/ontologies/lox#MCM92">
        <rdf:type rdf:resource="http://www.sisostds.org/ontologies/C2SIM#TaskActionCode"/>
        <rdfs:comment>MCM operation stage 92: Mine Counter Measure operation stage 92.</rdfs:comment>
    </owl:NamedIndividual>
    


    <!-- http://www.sisostds.org/ontologies/lox#MCM93 -->

    <owl:NamedIndividual rdf:about="http://www.sisostds.org/ontologies/lox#MCM93">
        <rdf:type rdf:resource="http://www.sisostds.org/ontologies/C2SIM#TaskActionCode"/>
        <rdfs:comment>MCM operation stage 93: Mine Counter Measure operation stage 93.</rdfs:comment>
    </owl:NamedIndividual>
    


    <!-- http://www.sisostds.org/ontologies/lox#MCMATT -->

    <owl:NamedIndividual rdf:about="http://www.sisostds.org/ontologies/lox#MCMATT">
        <rdf:type rdf:resource="http://www.sisostds.org/ontologies/C2SIM#TaskActionCode"/>
        <rdfs:comment>MCM, attrition: To conduct continuous application of Mine Countermeasures (MCM) to keep the risk from mines to all vessels as low as possible.</rdfs:comment>
    </owl:NamedIndividual>
    


    <!-- http://www.sisostds.org/ontologies/lox#MCMCHK -->

    <owl:NamedIndividual rdf:about="http://www.sisostds.org/ontologies/lox#MCMCHK">
        <rdf:type rdf:resource="http://www.sisostds.org/ontologies/C2SIM#TaskActionCode"/>
        <rdfs:comment>MCM, check: To conduct a Mine Countermeasures (MCM) operation to check that as far as possible no maritime mines are left after the previous</rdfs:comment>
    </owl:NamedIndividual>
    


    <!-- http://www.sisostds.org/ontologies/lox#MCMEXP -->

    <owl:NamedIndividual rdf:about="http://www.sisostds.org/ontologies/lox#MCMEXP">
        <rdf:type rdf:resource="http://www.sisostds.org/ontologies/C2SIM#TaskActionCode"/>
        <rdfs:comment>MCM, exploratory: To conduct a Mine Countermeasures (MCM) operation in which a sample of the route or area is subjected to MCM procedures to</rdfs:comment>
    </owl:NamedIndividual>
    


    <!-- http://www.sisostds.org/ontologies/lox#MCMLDT -->

    <owl:NamedIndividual rdf:about="http://www.sisostds.org/ontologies/lox#MCMLDT">
        <rdf:type rdf:resource="http://www.sisostds.org/ontologies/C2SIM#TaskActionCode"/>
        <rdfs:comment>MCM, lead through: To assist traffic in the transit of parts of a mined area which have previously been subject to Mine Countermeasures (MCM)</rdfs:comment>
    </owl:NamedIndividual>
    


    <!-- http://www.sisostds.org/ontologies/lox#MCMLMC -->

    <owl:NamedIndividual rdf:about="http://www.sisostds.org/ontologies/lox#MCMLMC">
        <rdf:type rdf:resource="http://www.sisostds.org/ontologies/C2SIM#TaskActionCode"/>
        <rdfs:comment>MCM, limited clearing: To clear particular types of mines from an area, channel or route.</rdfs:comment>
    </owl:NamedIndividual>
    


    <!-- http://www.sisostds.org/ontologies/lox#MCMPRE -->

    <owl:NamedIndividual rdf:about="http://www.sisostds.org/ontologies/lox#MCMPRE">
        <rdf:type rdf:resource="http://www.sisostds.org/ontologies/C2SIM#TaskActionCode"/>
        <rdfs:comment>MCM, precursor: To carry out operations in an area or channel using relatively safe methods and techniques in order to reduce the risk to</rdfs:comment>
    </owl:NamedIndividual>
    


    <!-- http://www.sisostds.org/ontologies/lox#MCMSA -->

    <owl:NamedIndividual rdf:about="http://www.sisostds.org/ontologies/lox#MCMSA">
        <rdf:type rdf:resource="http://www.sisostds.org/ontologies/C2SIM#TaskActionCode"/>
        <rdfs:comment>MCM-SLS-ALPHA: Mine Countermeasures Operation Standard Letter Suffixes ALPHA.</rdfs:comment>
    </owl:NamedIndividual>
    


    <!-- http://www.sisostds.org/ontologies/lox#MCMSAA -->

    <owl:NamedIndividual rdf:about="http://www.sisostds.org/ontologies/lox#MCMSAA">
        <rdf:type rdf:resource="http://www.sisostds.org/ontologies/C2SIM#TaskActionCode"/>
        <rdfs:comment>MCM-SLS-ALPHA-ALPHA: Mine Countermeasures Operation Standard Letter Suffixes ALPHA-ALPHA.</rdfs:comment>
    </owl:NamedIndividual>
    


    <!-- http://www.sisostds.org/ontologies/lox#MCMSAC -->

    <owl:NamedIndividual rdf:about="http://www.sisostds.org/ontologies/lox#MCMSAC">
        <rdf:type rdf:resource="http://www.sisostds.org/ontologies/C2SIM#TaskActionCode"/>
        <rdfs:comment>MCM-SLS-ALPHA-CHARLIE: Mine Countermeasures Operation Standard Letter Suffixes ALPHA-CHARLIE.</rdfs:comment>
    </owl:NamedIndividual>
    


    <!-- http://www.sisostds.org/ontologies/lox#MCMSAD -->

    <owl:NamedIndividual rdf:about="http://www.sisostds.org/ontologies/lox#MCMSAD">
        <rdf:type rdf:resource="http://www.sisostds.org/ontologies/C2SIM#TaskActionCode"/>
        <rdfs:comment>MCM-SLS-ALPHA-DELTA: Mine Countermeasures Operation Standard Letter Suffixes ALPHA-DELTA.</rdfs:comment>
    </owl:NamedIndividual>
    


    <!-- http://www.sisostds.org/ontologies/lox#MCMSAG -->

    <owl:NamedIndividual rdf:about="http://www.sisostds.org/ontologies/lox#MCMSAG">
        <rdf:type rdf:resource="http://www.sisostds.org/ontologies/C2SIM#TaskActionCode"/>
        <rdfs:comment>MCM-SLS-ALPHA-GOLF: Mine Countermeasures Operation Standard Letter Suffixes ALPHA-GOLF.</rdfs:comment>
    </owl:NamedIndividual>
    


    <!-- http://www.sisostds.org/ontologies/lox#MCMSAH -->

    <owl:NamedIndividual rdf:about="http://www.sisostds.org/ontologies/lox#MCMSAH">
        <rdf:type rdf:resource="http://www.sisostds.org/ontologies/C2SIM#TaskActionCode"/>
        <rdfs:comment>MCM-SLS-ALPHA-HOTEL: Mine Countermeasures Operation Standard Letter Suffixes ALPHA-HOTEL.</rdfs:comment>
    </owl:NamedIndividual>
    


    <!-- http://www.sisostds.org/ontologies/lox#MCMSAM -->

    <owl:NamedIndividual rdf:about="http://www.sisostds.org/ontologies/lox#MCMSAM">
        <rdf:type rdf:resource="http://www.sisostds.org/ontologies/C2SIM#TaskActionCode"/>
        <rdfs:comment>MCM-SLS-ALPHA-MIKE: Mine Countermeasures Operation Standard Letter Suffixes ALPHA-MIKE.</rdfs:comment>
    </owl:NamedIndividual>
    


    <!-- http://www.sisostds.org/ontologies/lox#MCMSAZ -->

    <owl:NamedIndividual rdf:about="http://www.sisostds.org/ontologies/lox#MCMSAZ">
        <rdf:type rdf:resource="http://www.sisostds.org/ontologies/C2SIM#TaskActionCode"/>
        <rdfs:comment>MCM-SLS-ALPHA-ZULU: Mine Countermeasures Operation Standard Letter Suffixes ALPHA-ZULU.</rdfs:comment>
    </owl:NamedIndividual>
    


    <!-- http://www.sisostds.org/ontologies/lox#MCMSB -->

    <owl:NamedIndividual rdf:about="http://www.sisostds.org/ontologies/lox#MCMSB">
        <rdf:type rdf:resource="http://www.sisostds.org/ontologies/C2SIM#TaskActionCode"/>
        <rdfs:comment>MCM-SLS-BRAVO: Mine Countermeasures Operation Standard Letter Suffixes BRAVO.</rdfs:comment>
    </owl:NamedIndividual>
    


    <!-- http://www.sisostds.org/ontologies/lox#MCMSBZ -->

    <owl:NamedIndividual rdf:about="http://www.sisostds.org/ontologies/lox#MCMSBZ">
        <rdf:type rdf:resource="http://www.sisostds.org/ontologies/C2SIM#TaskActionCode"/>
        <rdfs:comment>MCM-SLS-BRAVO-ZULU: Mine Countermeasures Operation Standard Letter Suffixes BRAVO-ZULU.</rdfs:comment>
    </owl:NamedIndividual>
    


    <!-- http://www.sisostds.org/ontologies/lox#MCMSC -->

    <owl:NamedIndividual rdf:about="http://www.sisostds.org/ontologies/lox#MCMSC">
        <rdf:type rdf:resource="http://www.sisostds.org/ontologies/C2SIM#TaskActionCode"/>
        <rdfs:comment>MCM-SLS-CHARLIE: Mine Countermeasures Operation Standard Letter Suffixes CHARLIE.</rdfs:comment>
    </owl:NamedIndividual>
    


    <!-- http://www.sisostds.org/ontologies/lox#MCMSCA -->

    <owl:NamedIndividual rdf:about="http://www.sisostds.org/ontologies/lox#MCMSCA">
        <rdf:type rdf:resource="http://www.sisostds.org/ontologies/C2SIM#TaskActionCode"/>
        <rdfs:comment>MCM-SLS-CHARLIE-ALPHA: Mine Countermeasures Operation Standard Letter Suffixes CHARLIE-ALPHA.</rdfs:comment>
    </owl:NamedIndividual>
    


    <!-- http://www.sisostds.org/ontologies/lox#MCMSCC -->

    <owl:NamedIndividual rdf:about="http://www.sisostds.org/ontologies/lox#MCMSCC">
        <rdf:type rdf:resource="http://www.sisostds.org/ontologies/C2SIM#TaskActionCode"/>
        <rdfs:comment>MCM-SLS-CHARLIE-CHARLIE: Mine Countermeasures Operation Standard Letter Suffixes CHARLIE-CHARLIE.</rdfs:comment>
    </owl:NamedIndividual>
    


    <!-- http://www.sisostds.org/ontologies/lox#MCMSCD -->

    <owl:NamedIndividual rdf:about="http://www.sisostds.org/ontologies/lox#MCMSCD">
        <rdf:type rdf:resource="http://www.sisostds.org/ontologies/C2SIM#TaskActionCode"/>
        <rdfs:comment>MCM-SLS-CHARLIE-DELTA: Mine Countermeasures Operation Standard Letter Suffixes CHARLIE-DELTA.</rdfs:comment>
    </owl:NamedIndividual>
    


    <!-- http://www.sisostds.org/ontologies/lox#MCMSCG -->

    <owl:NamedIndividual rdf:about="http://www.sisostds.org/ontologies/lox#MCMSCG">
        <rdf:type rdf:resource="http://www.sisostds.org/ontologies/C2SIM#TaskActionCode"/>
        <rdfs:comment>MCM-SLS-CHARLIE-GOLF: Mine Countermeasures Operation Standard Letter Suffixes CHARLIE-GOLF.</rdfs:comment>
    </owl:NamedIndividual>
    


    <!-- http://www.sisostds.org/ontologies/lox#MCMSCH -->

    <owl:NamedIndividual rdf:about="http://www.sisostds.org/ontologies/lox#MCMSCH">
        <rdf:type rdf:resource="http://www.sisostds.org/ontologies/C2SIM#TaskActionCode"/>
        <rdfs:comment>MCM-SLS-CHARLIE-HOTEL: Mine Countermeasures Operation Standard Letter Suffixes CHARLIE-HOTEL.</rdfs:comment>
    </owl:NamedIndividual>
    


    <!-- http://www.sisostds.org/ontologies/lox#MCMSCM -->

    <owl:NamedIndividual rdf:about="http://www.sisostds.org/ontologies/lox#MCMSCM">
        <rdf:type rdf:resource="http://www.sisostds.org/ontologies/C2SIM#TaskActionCode"/>
        <rdfs:comment>MCM-SLS-CHARLIE-MIKE: Mine Countermeasures Operation Standard Letter Suffixes CHARLIE-MIKE.</rdfs:comment>
    </owl:NamedIndividual>
    


    <!-- http://www.sisostds.org/ontologies/lox#MCMSCZ -->

    <owl:NamedIndividual rdf:about="http://www.sisostds.org/ontologies/lox#MCMSCZ">
        <rdf:type rdf:resource="http://www.sisostds.org/ontologies/C2SIM#TaskActionCode"/>
        <rdfs:comment>MCM-SLS-CHARLIE-ZULU: Mine Countermeasures Operation Standard Letter Suffixes CHARLIE-ZULU.</rdfs:comment>
    </owl:NamedIndividual>
    


    <!-- http://www.sisostds.org/ontologies/lox#MCMSE -->

    <owl:NamedIndividual rdf:about="http://www.sisostds.org/ontologies/lox#MCMSE">
        <rdf:type rdf:resource="http://www.sisostds.org/ontologies/C2SIM#TaskActionCode"/>
        <rdfs:comment>MCM-SLS-ECHO: Mine Countermeasures Operation Standard Letter Suffixes ECHO.</rdfs:comment>
    </owl:NamedIndividual>
    


    <!-- http://www.sisostds.org/ontologies/lox#MCMSEA -->

    <owl:NamedIndividual rdf:about="http://www.sisostds.org/ontologies/lox#MCMSEA">
        <rdf:type rdf:resource="http://www.sisostds.org/ontologies/C2SIM#TaskActionCode"/>
        <rdfs:comment>MCM-SLS-ECHO-ALPHA: Mine Countermeasures Operation Standard Letter Suffixes ECHO-ALPHA.</rdfs:comment>
    </owl:NamedIndividual>
    


    <!-- http://www.sisostds.org/ontologies/lox#MCMSEC -->

    <owl:NamedIndividual rdf:about="http://www.sisostds.org/ontologies/lox#MCMSEC">
        <rdf:type rdf:resource="http://www.sisostds.org/ontologies/C2SIM#TaskActionCode"/>
        <rdfs:comment>MCM-SLS-ECHO-CHARLIE: Mine Countermeasures Operation Standard Letter Suffixes ECHO-CHARLIE.</rdfs:comment>
    </owl:NamedIndividual>
    


    <!-- http://www.sisostds.org/ontologies/lox#MCMSED -->

    <owl:NamedIndividual rdf:about="http://www.sisostds.org/ontologies/lox#MCMSED">
        <rdf:type rdf:resource="http://www.sisostds.org/ontologies/C2SIM#TaskActionCode"/>
        <rdfs:comment>MCM-SLS-ECHO-DELTA: Mine Countermeasures Operation Standard Letter Suffixes ECHO-DELTA.</rdfs:comment>
    </owl:NamedIndividual>
    


    <!-- http://www.sisostds.org/ontologies/lox#MCMSEG -->

    <owl:NamedIndividual rdf:about="http://www.sisostds.org/ontologies/lox#MCMSEG">
        <rdf:type rdf:resource="http://www.sisostds.org/ontologies/C2SIM#TaskActionCode"/>
        <rdfs:comment>MCM-SLS-ECHO-GOLF: Mine Countermeasures Operation Standard Letter Suffixes ECHO-GOLF.</rdfs:comment>
    </owl:NamedIndividual>
    


    <!-- http://www.sisostds.org/ontologies/lox#MCMSEH -->

    <owl:NamedIndividual rdf:about="http://www.sisostds.org/ontologies/lox#MCMSEH">
        <rdf:type rdf:resource="http://www.sisostds.org/ontologies/C2SIM#TaskActionCode"/>
        <rdfs:comment>MCM-SLS-ECHO-HOTEL: Mine Countermeasures Operation Standard Letter Suffixes ECHO-HOTEL.</rdfs:comment>
    </owl:NamedIndividual>
    


    <!-- http://www.sisostds.org/ontologies/lox#MCMSEM -->

    <owl:NamedIndividual rdf:about="http://www.sisostds.org/ontologies/lox#MCMSEM">
        <rdf:type rdf:resource="http://www.sisostds.org/ontologies/C2SIM#TaskActionCode"/>
        <rdfs:comment>MCM-SLS-ECHO-MIKE: Mine Countermeasures Operation Standard Letter Suffixes ECHO-MIKE.</rdfs:comment>
    </owl:NamedIndividual>
    


    <!-- http://www.sisostds.org/ontologies/lox#MCMSEZ -->

    <owl:NamedIndividual rdf:about="http://www.sisostds.org/ontologies/lox#MCMSEZ">
        <rdf:type rdf:resource="http://www.sisostds.org/ontologies/C2SIM#TaskActionCode"/>
        <rdfs:comment>MCM-SLS-ECHO-ZULU: Mine Countermeasures Operation Standard Letter Suffixes ECHO-ZULU.</rdfs:comment>
    </owl:NamedIndividual>
    


    <!-- http://www.sisostds.org/ontologies/lox#MCMSL -->

    <owl:NamedIndividual rdf:about="http://www.sisostds.org/ontologies/lox#MCMSL">
        <rdf:type rdf:resource="http://www.sisostds.org/ontologies/C2SIM#TaskActionCode"/>
        <rdfs:comment>MCM-SLS-LIMA: Mine Countermeasures Operation Standard Letter Suffixes LIMA.</rdfs:comment>
    </owl:NamedIndividual>
    


    <!-- http://www.sisostds.org/ontologies/lox#MCMSLA -->

    <owl:NamedIndividual rdf:about="http://www.sisostds.org/ontologies/lox#MCMSLA">
        <rdf:type rdf:resource="http://www.sisostds.org/ontologies/C2SIM#TaskActionCode"/>
        <rdfs:comment>MCM-SLS-LIMA-ALPHA: Mine Countermeasures Operation Standard Letter Suffixes LIMA-ALPHA.</rdfs:comment>
    </owl:NamedIndividual>
    


    <!-- http://www.sisostds.org/ontologies/lox#MCMSLH -->

    <owl:NamedIndividual rdf:about="http://www.sisostds.org/ontologies/lox#MCMSLH">
        <rdf:type rdf:resource="http://www.sisostds.org/ontologies/C2SIM#TaskActionCode"/>
        <rdfs:comment>MCM-SLS-LIMA-HOTEL: Mine Countermeasures Operation Standard Letter Suffixes LIMA-HOTEL.</rdfs:comment>
    </owl:NamedIndividual>
    


    <!-- http://www.sisostds.org/ontologies/lox#MCMSLM -->

    <owl:NamedIndividual rdf:about="http://www.sisostds.org/ontologies/lox#MCMSLM">
        <rdf:type rdf:resource="http://www.sisostds.org/ontologies/C2SIM#TaskActionCode"/>
        <rdfs:comment>MCM-SLS-LIMA-MIKE: Mine Countermeasures Operation Standard Letter Suffixes LIMA-MIKE.</rdfs:comment>
    </owl:NamedIndividual>
    


    <!-- http://www.sisostds.org/ontologies/lox#MCMSLZ -->

    <owl:NamedIndividual rdf:about="http://www.sisostds.org/ontologies/lox#MCMSLZ">
        <rdf:type rdf:resource="http://www.sisostds.org/ontologies/C2SIM#TaskActionCode"/>
        <rdfs:comment>MCM-SLS-LIMA-ZULU: Mine Countermeasures Operation Standard Letter Suffixes LIMA-ZULU.</rdfs:comment>
    </owl:NamedIndividual>
    


    <!-- http://www.sisostds.org/ontologies/lox#MCMSP -->

    <owl:NamedIndividual rdf:about="http://www.sisostds.org/ontologies/lox#MCMSP">
        <rdf:type rdf:resource="http://www.sisostds.org/ontologies/C2SIM#TaskActionCode"/>
        <rdfs:comment>MCM-SLS-PAPA: Mine Countermeasures Operation Standard Letter Suffixes PAPA.</rdfs:comment>
    </owl:NamedIndividual>
    


    <!-- http://www.sisostds.org/ontologies/lox#MCMSPA -->

    <owl:NamedIndividual rdf:about="http://www.sisostds.org/ontologies/lox#MCMSPA">
        <rdf:type rdf:resource="http://www.sisostds.org/ontologies/C2SIM#TaskActionCode"/>
        <rdfs:comment>MCM-SLS-PAPA-ALPHA: Mine Countermeasures Operation Standard Letter Suffixes PAPA-ALPHA.</rdfs:comment>
    </owl:NamedIndividual>
    


    <!-- http://www.sisostds.org/ontologies/lox#MCMSPC -->

    <owl:NamedIndividual rdf:about="http://www.sisostds.org/ontologies/lox#MCMSPC">
        <rdf:type rdf:resource="http://www.sisostds.org/ontologies/C2SIM#TaskActionCode"/>
        <rdfs:comment>MCM-SLS-PAPA-CHARLIE: Mine Countermeasures Operation Standard Letter Suffixes PAPA-CHARLIE.</rdfs:comment>
    </owl:NamedIndividual>
    


    <!-- http://www.sisostds.org/ontologies/lox#MCMSPG -->

    <owl:NamedIndividual rdf:about="http://www.sisostds.org/ontologies/lox#MCMSPG">
        <rdf:type rdf:resource="http://www.sisostds.org/ontologies/C2SIM#TaskActionCode"/>
        <rdfs:comment>MCM-SLS-PAPA-GOLF: Mine Countermeasures Operation Standard Letter Suffixes PAPA-GOLF.</rdfs:comment>
    </owl:NamedIndividual>
    


    <!-- http://www.sisostds.org/ontologies/lox#MCMSPH -->

    <owl:NamedIndividual rdf:about="http://www.sisostds.org/ontologies/lox#MCMSPH">
        <rdf:type rdf:resource="http://www.sisostds.org/ontologies/C2SIM#TaskActionCode"/>
        <rdfs:comment>MCM-SLS-PAPA-HOTEL: Mine Countermeasures Operation Standard Letter Suffixes PAPA-HOTEL.</rdfs:comment>
    </owl:NamedIndividual>
    


    <!-- http://www.sisostds.org/ontologies/lox#MCMSPM -->

    <owl:NamedIndividual rdf:about="http://www.sisostds.org/ontologies/lox#MCMSPM">
        <rdf:type rdf:resource="http://www.sisostds.org/ontologies/C2SIM#TaskActionCode"/>
        <rdfs:comment>MCM-SLS-PAPA-MIKE: Mine Countermeasures Operation Standard Letter Suffixes PAPA-MIKE.</rdfs:comment>
    </owl:NamedIndividual>
    


    <!-- http://www.sisostds.org/ontologies/lox#MCMSPZ -->

    <owl:NamedIndividual rdf:about="http://www.sisostds.org/ontologies/lox#MCMSPZ">
        <rdf:type rdf:resource="http://www.sisostds.org/ontologies/C2SIM#TaskActionCode"/>
        <rdfs:comment>MCM-SLS-PAPA-ZULU: Mine Countermeasures Operation Standard Letter Suffixes PAPA-ZULU.</rdfs:comment>
    </owl:NamedIndividual>
    


    <!-- http://www.sisostds.org/ontologies/lox#MCMSR -->

    <owl:NamedIndividual rdf:about="http://www.sisostds.org/ontologies/lox#MCMSR">
        <rdf:type rdf:resource="http://www.sisostds.org/ontologies/C2SIM#TaskActionCode"/>
        <rdfs:comment>MCM-SLS-ROMEO: Mine Countermeasures Operation Standard Letter Suffixes ROMEO.</rdfs:comment>
    </owl:NamedIndividual>
    


    <!-- http://www.sisostds.org/ontologies/lox#MCMSRD -->

    <owl:NamedIndividual rdf:about="http://www.sisostds.org/ontologies/lox#MCMSRD">
        <rdf:type rdf:resource="http://www.sisostds.org/ontologies/C2SIM#TaskActionCode"/>
        <rdfs:comment>MCM-SLS-ROMEO-DELTA: Mine Countermeasures Operation Standard Letter Suffixes ROMEO-DELTA.</rdfs:comment>
    </owl:NamedIndividual>
    


    <!-- http://www.sisostds.org/ontologies/lox#MCMSRH -->

    <owl:NamedIndividual rdf:about="http://www.sisostds.org/ontologies/lox#MCMSRH">
        <rdf:type rdf:resource="http://www.sisostds.org/ontologies/C2SIM#TaskActionCode"/>
        <rdfs:comment>MCM-SLS-ROMEO-HOTEL: Mine Countermeasures Operation Standard Letter Suffixes ROMEO-HOTEL.</rdfs:comment>
    </owl:NamedIndividual>
    


    <!-- http://www.sisostds.org/ontologies/lox#MCMSRV -->

    <owl:NamedIndividual rdf:about="http://www.sisostds.org/ontologies/lox#MCMSRV">
        <rdf:type rdf:resource="http://www.sisostds.org/ontologies/C2SIM#TaskActionCode"/>
        <rdfs:comment>MCM, survey: To collect environmental data which may be used in support of current and future mine countermeasures (MCM) operations.</rdfs:comment>
    </owl:NamedIndividual>
    


    <!-- http://www.sisostds.org/ontologies/lox#MCMSS -->

    <owl:NamedIndividual rdf:about="http://www.sisostds.org/ontologies/lox#MCMSS">
        <rdf:type rdf:resource="http://www.sisostds.org/ontologies/C2SIM#TaskActionCode"/>
        <rdfs:comment>MCM-SLS-SIERRA: Mine Countermeasures Operation Standard Letter Suffixes SIERRA.</rdfs:comment>
    </owl:NamedIndividual>
    


    <!-- http://www.sisostds.org/ontologies/lox#MCMSSA -->

    <owl:NamedIndividual rdf:about="http://www.sisostds.org/ontologies/lox#MCMSSA">
        <rdf:type rdf:resource="http://www.sisostds.org/ontologies/C2SIM#TaskActionCode"/>
        <rdfs:comment>MCM-SLS-SIERRA-ALPHA: Mine Countermeasures Operation Standard Letter Suffixes SIERRA-ALPHA.</rdfs:comment>
    </owl:NamedIndividual>
    


    <!-- http://www.sisostds.org/ontologies/lox#MCMSSC -->

    <owl:NamedIndividual rdf:about="http://www.sisostds.org/ontologies/lox#MCMSSC">
        <rdf:type rdf:resource="http://www.sisostds.org/ontologies/C2SIM#TaskActionCode"/>
        <rdfs:comment>MCM-SLS-SIERRA-CHARLIE: Mine Countermeasures Operation Standard Letter Suffixes SIERRA-CHARLIE.</rdfs:comment>
    </owl:NamedIndividual>
    


    <!-- http://www.sisostds.org/ontologies/lox#MCMSSD -->

    <owl:NamedIndividual rdf:about="http://www.sisostds.org/ontologies/lox#MCMSSD">
        <rdf:type rdf:resource="http://www.sisostds.org/ontologies/C2SIM#TaskActionCode"/>
        <rdfs:comment>MCM-SLS-SIERRA-DELTA: Mine Countermeasures Operation Standard Letter Suffixes SIERRA-DELTA.</rdfs:comment>
    </owl:NamedIndividual>
    


    <!-- http://www.sisostds.org/ontologies/lox#MCMSSG -->

    <owl:NamedIndividual rdf:about="http://www.sisostds.org/ontologies/lox#MCMSSG">
        <rdf:type rdf:resource="http://www.sisostds.org/ontologies/C2SIM#TaskActionCode"/>
        <rdfs:comment>MCM-SLS-SIERRA-GOLF: Mine Countermeasures Operation Standard Letter Suffixes SIERRA-GOLF.</rdfs:comment>
    </owl:NamedIndividual>
    


    <!-- http://www.sisostds.org/ontologies/lox#MCMSSH -->

    <owl:NamedIndividual rdf:about="http://www.sisostds.org/ontologies/lox#MCMSSH">
        <rdf:type rdf:resource="http://www.sisostds.org/ontologies/C2SIM#TaskActionCode"/>
        <rdfs:comment>MCM-SLS-SIERRA-HOTEL: Mine Countermeasures Operation Standard Letter Suffixes SIERRA-HOTEL.</rdfs:comment>
    </owl:NamedIndividual>
    


    <!-- http://www.sisostds.org/ontologies/lox#MCMSSM -->

    <owl:NamedIndividual rdf:about="http://www.sisostds.org/ontologies/lox#MCMSSM">
        <rdf:type rdf:resource="http://www.sisostds.org/ontologies/C2SIM#TaskActionCode"/>
        <rdfs:comment>MCM-SLS-SIERRA-MIKE: Mine Countermeasures Operation Standard Letter Suffixes SIERRA-MIKE.</rdfs:comment>
    </owl:NamedIndividual>
    


    <!-- http://www.sisostds.org/ontologies/lox#MCMSSZ -->

    <owl:NamedIndividual rdf:about="http://www.sisostds.org/ontologies/lox#MCMSSZ">
        <rdf:type rdf:resource="http://www.sisostds.org/ontologies/C2SIM#TaskActionCode"/>
        <rdfs:comment>MCM-SLS-SIERRA-ZULU: Mine Countermeasures Operation Standard Letter Suffixes SIERRA-ZULU.</rdfs:comment>
    </owl:NamedIndividual>
    


    <!-- http://www.sisostds.org/ontologies/lox#MCMSU -->

    <owl:NamedIndividual rdf:about="http://www.sisostds.org/ontologies/lox#MCMSU">
        <rdf:type rdf:resource="http://www.sisostds.org/ontologies/C2SIM#TaskActionCode"/>
        <rdfs:comment>MCM-SLS-UNIFORM: Mine Countermeasures Operation Standard Letter Suffixes UNIFORM.</rdfs:comment>
    </owl:NamedIndividual>
    


    <!-- http://www.sisostds.org/ontologies/lox#MCMSUH -->

    <owl:NamedIndividual rdf:about="http://www.sisostds.org/ontologies/lox#MCMSUH">
        <rdf:type rdf:resource="http://www.sisostds.org/ontologies/C2SIM#TaskActionCode"/>
        <rdfs:comment>MCM-SLS-UNIFORM-HOTEL: Mine Countermeasures Operation Standard Letter Suffixes UNIFORM-HOTEL.</rdfs:comment>
    </owl:NamedIndividual>
    


    <!-- http://www.sisostds.org/ontologies/lox#MCMSUZ -->

    <owl:NamedIndividual rdf:about="http://www.sisostds.org/ontologies/lox#MCMSUZ">
        <rdf:type rdf:resource="http://www.sisostds.org/ontologies/C2SIM#TaskActionCode"/>
        <rdfs:comment>MCM-SLS-UNIFORM-ZULU: Mine Countermeasures Operation Standard Letter Suffixes UNIFORM-ZULU.</rdfs:comment>
    </owl:NamedIndividual>
    


    <!-- http://www.sisostds.org/ontologies/lox#MCMSV -->

    <owl:NamedIndividual rdf:about="http://www.sisostds.org/ontologies/lox#MCMSV">
        <rdf:type rdf:resource="http://www.sisostds.org/ontologies/C2SIM#TaskActionCode"/>
        <rdfs:comment>MCM-SLS-VICTOR: Mine Countermeasures Operation Standard Letter Suffixes VICTOR.</rdfs:comment>
    </owl:NamedIndividual>
    


    <!-- http://www.sisostds.org/ontologies/lox#MCMSVA -->

    <owl:NamedIndividual rdf:about="http://www.sisostds.org/ontologies/lox#MCMSVA">
        <rdf:type rdf:resource="http://www.sisostds.org/ontologies/C2SIM#TaskActionCode"/>
        <rdfs:comment>MCM-SLS-VICTOR-ALPHA: Mine Countermeasures Operation Standard Letter Suffixes VICTOR-ALPHA.</rdfs:comment>
    </owl:NamedIndividual>
    


    <!-- http://www.sisostds.org/ontologies/lox#MCMSVC -->

    <owl:NamedIndividual rdf:about="http://www.sisostds.org/ontologies/lox#MCMSVC">
        <rdf:type rdf:resource="http://www.sisostds.org/ontologies/C2SIM#TaskActionCode"/>
        <rdfs:comment>MCM-SLS-VICTOR-CHARLIE: Mine Countermeasures Operation Standard Letter Suffixes VICTOR-CHARLIE.</rdfs:comment>
    </owl:NamedIndividual>
    


    <!-- http://www.sisostds.org/ontologies/lox#MCMSVD -->

    <owl:NamedIndividual rdf:about="http://www.sisostds.org/ontologies/lox#MCMSVD">
        <rdf:type rdf:resource="http://www.sisostds.org/ontologies/C2SIM#TaskActionCode"/>
        <rdfs:comment>MCM-SLS-VICTOR-DELTA: Mine Countermeasures Operation Standard Letter Suffixes VICTOR-DELTA.</rdfs:comment>
    </owl:NamedIndividual>
    


    <!-- http://www.sisostds.org/ontologies/lox#MCMSVG -->

    <owl:NamedIndividual rdf:about="http://www.sisostds.org/ontologies/lox#MCMSVG">
        <rdf:type rdf:resource="http://www.sisostds.org/ontologies/C2SIM#TaskActionCode"/>
        <rdfs:comment>MCM-SLS-VICTOR-GOLF: Mine Countermeasures Operation Standard Letter Suffixes VICTOR-GOLF.</rdfs:comment>
    </owl:NamedIndividual>
    


    <!-- http://www.sisostds.org/ontologies/lox#MCMSVH -->

    <owl:NamedIndividual rdf:about="http://www.sisostds.org/ontologies/lox#MCMSVH">
        <rdf:type rdf:resource="http://www.sisostds.org/ontologies/C2SIM#TaskActionCode"/>
        <rdfs:comment>MCM-SLS-VICTOR-HOTEL: Mine Countermeasures Operation Standard Letter Suffixes VICTOR-HOTEL.</rdfs:comment>
    </owl:NamedIndividual>
    


    <!-- http://www.sisostds.org/ontologies/lox#MCMSVM -->

    <owl:NamedIndividual rdf:about="http://www.sisostds.org/ontologies/lox#MCMSVM">
        <rdf:type rdf:resource="http://www.sisostds.org/ontologies/C2SIM#TaskActionCode"/>
        <rdfs:comment>MCM-SLS-VICTOR-MIKE: Mine Countermeasures Operation Standard Letter Suffixes VICTOR-MIKE.</rdfs:comment>
    </owl:NamedIndividual>
    


    <!-- http://www.sisostds.org/ontologies/lox#MCMSVZ -->

    <owl:NamedIndividual rdf:about="http://www.sisostds.org/ontologies/lox#MCMSVZ">
        <rdf:type rdf:resource="http://www.sisostds.org/ontologies/C2SIM#TaskActionCode"/>
        <rdfs:comment>MCM-SLS-VICTOR-ZULU: Mine Countermeasures Operation Standard Letter Suffixes VICTOR-ZULU.</rdfs:comment>
    </owl:NamedIndividual>
    


    <!-- http://www.sisostds.org/ontologies/lox#MCMSW -->

    <owl:NamedIndividual rdf:about="http://www.sisostds.org/ontologies/lox#MCMSW">
        <rdf:type rdf:resource="http://www.sisostds.org/ontologies/C2SIM#TaskActionCode"/>
        <rdfs:comment>MCM-SLS-WHISKEY: Mine Countermeasures Operation Standard Letter Suffixes WHISKEY.</rdfs:comment>
    </owl:NamedIndividual>
    


    <!-- http://www.sisostds.org/ontologies/lox#MCMSWZ -->

    <owl:NamedIndividual rdf:about="http://www.sisostds.org/ontologies/lox#MCMSWZ">
        <rdf:type rdf:resource="http://www.sisostds.org/ontologies/C2SIM#TaskActionCode"/>
        <rdfs:comment>MCM-SLS-WHISKEY-ZULU: Mine Countermeasures Operation Standard Letter Suffixes WHISKEY-ZULU.</rdfs:comment>
    </owl:NamedIndividual>
    


    <!-- http://www.sisostds.org/ontologies/lox#MCMSZZ -->

    <owl:NamedIndividual rdf:about="http://www.sisostds.org/ontologies/lox#MCMSZZ">
        <rdf:type rdf:resource="http://www.sisostds.org/ontologies/C2SIM#TaskActionCode"/>
        <rdfs:comment>MCM-SLS-ZULU-ZULU: Mine Countermeasures Operation Standard Letter Suffixes ZULU-ZULU.</rdfs:comment>
    </owl:NamedIndividual>
    


    <!-- http://www.sisostds.org/ontologies/lox#MCMTML -->

    <owl:NamedIndividual rdf:about="http://www.sisostds.org/ontologies/lox#MCMTML">
        <rdf:type rdf:resource="http://www.sisostds.org/ontologies/C2SIM#TaskActionCode"/>
        <rdfs:comment>MCM, time limited: To conduct a minesweeping and/or minehunting carried out when time available before ships are passed through a mined area,</rdfs:comment>
    </owl:NamedIndividual>
    


    <!-- http://www.sisostds.org/ontologies/lox#MEDEVC -->

    <owl:NamedIndividual rdf:about="http://www.sisostds.org/ontologies/lox#MEDEVC">
        <rdf:type rdf:resource="http://www.sisostds.org/ontologies/C2SIM#TaskActionCode"/>
        <rdfs:comment>Documentation: 		
						To move any person who is wounded, injured or ill to/between medical treatment facilities.	
					; Appinfo DisplayValue as &quot;Medical evacuation&quot;</rdfs:comment>
        <rdfs:comment>Medical evacuation: To move any person who is wounded, injured or ill to/between medical treatment facilities.</rdfs:comment>
    </owl:NamedIndividual>
    


    <!-- http://www.sisostds.org/ontologies/lox#METBAL -->

    <owl:NamedIndividual rdf:about="http://www.sisostds.org/ontologies/lox#METBAL">
        <rdf:type rdf:resource="http://www.sisostds.org/ontologies/C2SIM#TaskActionCode"/>
        <rdfs:comment>Meteorological: To gather meteorological information such as humidity, pressure, and temperature characteristics of Earth&apos;s atmosphere.</rdfs:comment>
    </owl:NamedIndividual>
    


    <!-- http://www.sisostds.org/ontologies/lox#MINCM -->

    <owl:NamedIndividual rdf:about="http://www.sisostds.org/ontologies/lox#MINCM">
        <rdf:type rdf:resource="http://www.sisostds.org/ontologies/C2SIM#TaskActionCode"/>
        <rdfs:comment>Mine countermeasures: To perform mine countermeasures.</rdfs:comment>
    </owl:NamedIndividual>
    


    <!-- http://www.sisostds.org/ontologies/lox#MINEWF -->

    <owl:NamedIndividual rdf:about="http://www.sisostds.org/ontologies/lox#MINEWF">
        <rdf:type rdf:resource="http://www.sisostds.org/ontologies/C2SIM#TaskActionCode"/>
        <rdfs:comment>Mine warfare: To conduct warfare that includes the actions of laying mines and actions taken to counter the threat of an adversary (referred</rdfs:comment>
    </owl:NamedIndividual>
    


    <!-- http://www.sisostds.org/ontologies/lox#MINLAY -->

    <owl:NamedIndividual rdf:about="http://www.sisostds.org/ontologies/lox#MINLAY">
        <rdf:type rdf:resource="http://www.sisostds.org/ontologies/C2SIM#TaskActionCode"/>
        <rdfs:comment>Mine-laying: To emplace or deploy one or more mines.</rdfs:comment>
    </owl:NamedIndividual>
    


    <!-- http://www.sisostds.org/ontologies/lox#MINSWP -->

    <owl:NamedIndividual rdf:about="http://www.sisostds.org/ontologies/lox#MINSWP">
        <rdf:type rdf:resource="http://www.sisostds.org/ontologies/C2SIM#TaskActionCode"/>
        <rdfs:comment>Minesweeping, land: To search for or clear mines using mechanical or explosion gear, which physically removes or destroys the mine, or produces,</rdfs:comment>
    </owl:NamedIndividual>
    


    <!-- http://www.sisostds.org/ontologies/lox#MISSTG -->

    <owl:NamedIndividual rdf:about="http://www.sisostds.org/ontologies/lox#MISSTG">
        <rdf:type rdf:resource="http://www.sisostds.org/ontologies/C2SIM#TaskActionCode"/>
        <rdfs:comment>Mission staging: To perform the assembly of aircraft for the completion of a mission or other activity.</rdfs:comment>
    </owl:NamedIndividual>
    


    <!-- http://www.sisostds.org/ontologies/lox#MKIL -->

    <owl:NamedIndividual rdf:about="http://www.sisostds.org/ontologies/lox#MKIL">
        <rdfs:comment>Documentation: 		
						The rendering of a vehicle as being temporarily or permanently incapable of tactical movement.	
					; Appinfo DisplayValue as &quot;Mobility kill (M-kill)&quot;</rdfs:comment>
    </owl:NamedIndividual>
    


    <!-- http://www.sisostds.org/ontologies/lox#MNHUNT -->

    <owl:NamedIndividual rdf:about="http://www.sisostds.org/ontologies/lox#MNHUNT">
        <rdf:type rdf:resource="http://www.sisostds.org/ontologies/C2SIM#TaskActionCode"/>
        <rdfs:comment>Mine hunting, maritime: To locate and dispose of individual mines by means of detection equipment with the employment of ships, airborne equipment</rdfs:comment>
    </owl:NamedIndividual>
    


    <!-- http://www.sisostds.org/ontologies/lox#MNSWMA -->

    <owl:NamedIndividual rdf:about="http://www.sisostds.org/ontologies/lox#MNSWMA">
        <rdf:type rdf:resource="http://www.sisostds.org/ontologies/C2SIM#TaskActionCode"/>
        <rdfs:comment>Minesweeping, maritime: To search for or counter mines by maritime minesweepers using mechanical or explosive gear, which physically removes or destroys</rdfs:comment>
    </owl:NamedIndividual>
    


    <!-- http://www.sisostds.org/ontologies/lox#MNTAIR -->

    <owl:NamedIndividual rdf:about="http://www.sisostds.org/ontologies/lox#MNTAIR">
        <rdf:type rdf:resource="http://www.sisostds.org/ontologies/C2SIM#TaskActionCode"/>
        <rdfs:comment>Maintain on call airborne alert: To keep combat equipped aircraft airborne and prepared for immediate action. Airborne alert is designed to reduce reaction</rdfs:comment>
    </owl:NamedIndividual>
    


    <!-- http://www.sisostds.org/ontologies/lox#MNTGRD -->

    <owl:NamedIndividual rdf:about="http://www.sisostds.org/ontologies/lox#MNTGRD">
        <rdf:type rdf:resource="http://www.sisostds.org/ontologies/C2SIM#TaskActionCode"/>
        <rdfs:comment>Maintain on call ground alert: To keep aircraft on the ground/runway/deck fully serviced and armed, with combat crews in readiness to take off within a specified</rdfs:comment>
    </owl:NamedIndividual>
    


    <!-- http://www.sisostds.org/ontologies/lox#MODDAM -->

    <owl:NamedIndividual rdf:about="http://www.sisostds.org/ontologies/lox#MODDAM">
        <rdfs:comment>Documentation: 		
						The subjective categorisation of the physical effect of an ACTION on buildings, infrastructure and/or equipment by a reporting ORGANISATION.	
					; Appinfo DisplayValue as &quot;Moderate damage&quot;</rdfs:comment>
    </owl:NamedIndividual>
    


    <!-- http://www.sisostds.org/ontologies/lox#MOPUP -->

    <owl:NamedIndividual rdf:about="http://www.sisostds.org/ontologies/lox#MOPUP">
        <rdf:type rdf:resource="http://www.sisostds.org/ontologies/C2SIM#TaskActionCode"/>
        <rdfs:comment>Documentation: 		
						To liquidate the remnants of enemy resistance in an area that has been surrounded or isolated, or through which other units have passed without eliminating all active resistance.	
					; Appinfo DisplayValue as &quot;Mop up&quot;</rdfs:comment>
        <rdfs:comment>Mop up: To liquidate the remnants of enemy resistance in an area that has been surrounded or isolated, or through which other units</rdfs:comment>
    </owl:NamedIndividual>
    


    <!-- http://www.sisostds.org/ontologies/lox#MOVE -->

    <owl:NamedIndividual rdf:about="http://www.sisostds.org/ontologies/lox#MOVE">
        <rdf:type rdf:resource="http://www.sisostds.org/ontologies/C2SIM#TaskActionCode"/>
        <rdfs:comment>Documentation: 		
						To change position from one location to another.	
					; Appinfo DisplayValue as &quot;Move&quot;</rdfs:comment>
        <rdfs:comment>Move: To change position from one location to another.</rdfs:comment>
    </owl:NamedIndividual>
    


    <!-- http://www.sisostds.org/ontologies/lox#MPA -->

    <owl:NamedIndividual rdf:about="http://www.sisostds.org/ontologies/lox#MPA">
        <rdf:type rdf:resource="http://www.sisostds.org/ontologies/C2SIM#TaskActionCode"/>
        <rdfs:comment>Patrol, maritime: To fly over an area, monitor and, where necessary, destroy hostile aircraft, as well as protect friendly shipping in the vicinity</rdfs:comment>
    </owl:NamedIndividual>
    


    <!-- http://www.sisostds.org/ontologies/lox#MRITOP -->

    <owl:NamedIndividual rdf:about="http://www.sisostds.org/ontologies/lox#MRITOP">
        <rdf:type rdf:resource="http://www.sisostds.org/ontologies/C2SIM#TaskActionCode"/>
        <rdfs:comment>Maritime interdiction operations: To conduct an operation that encompasses seaborne enforcement measures to interdict the movement of certain types of designated</rdfs:comment>
    </owl:NamedIndividual>
    


    <!-- http://www.sisostds.org/ontologies/lox#NACLSP -->

    <owl:NamedIndividual rdf:about="http://www.sisostds.org/ontologies/lox#NACLSP">
        <rdf:type rdf:resource="http://www.sisostds.org/ontologies/C2SIM#TaskActionCode"/>
        <rdfs:comment>Naval control of shipping: Control exercised by naval authorities of movement, routing, reporting, convoy organisation and tactical diversion of Allied</rdfs:comment>
    </owl:NamedIndividual>
    


    <!-- http://www.sisostds.org/ontologies/lox#NBCAS -->

    <owl:NamedIndividual rdf:about="http://www.sisostds.org/ontologies/lox#NBCAS">
        <rdfs:comment>Documentation: 		
						A person who is not a battle casualty, but who is lost to his organisation by reason of disease or injury, including persons dying from disease or injury, or by reason of being missing where the absence does not appear to be voluntary or due to enemy action or to being interned.	
					; Appinfo DisplayValue as &quot;Non-battle casualty&quot;</rdfs:comment>
    </owl:NamedIndividual>
    


    <!-- http://www.sisostds.org/ontologies/lox#NKN -->

    <owl:NamedIndividual rdf:about="http://www.sisostds.org/ontologies/lox#NKN">
        <rdfs:comment>Documentation: 		
						It is not possible to determine which value is most applicable.	
					; Appinfo DisplayValue as &quot;Not known&quot;</rdfs:comment>
    </owl:NamedIndividual>
    


    <!-- http://www.sisostds.org/ontologies/lox#NORSTN -->

    <owl:NamedIndividual rdf:about="http://www.sisostds.org/ontologies/lox#NORSTN">
        <rdfs:comment>Documentation: 		
						The ACTION-OBJECTIVE did not react against the ACTION.	
					; Appinfo DisplayValue as &quot;No resistance&quot;</rdfs:comment>
    </owl:NamedIndividual>
    


    <!-- http://www.sisostds.org/ontologies/lox#NOS -->

    <owl:NamedIndividual rdf:about="http://www.sisostds.org/ontologies/lox#NOS">
        <rdfs:comment>Documentation: 		
						The appropriate value is not in the set of specified values.	
					; Appinfo DisplayValue as &quot;Not otherwise specified&quot;</rdfs:comment>
    </owl:NamedIndividual>
    


    <!-- http://www.sisostds.org/ontologies/lox#NTRCHM -->

    <owl:NamedIndividual rdf:about="http://www.sisostds.org/ontologies/lox#NTRCHM">
        <rdf:type rdf:resource="http://www.sisostds.org/ontologies/C2SIM#TaskActionCode"/>
        <rdfs:comment>Neutralize, chemical: To make safe or non-toxic an object contaminated with a chemical agent.</rdfs:comment>
    </owl:NamedIndividual>
    


    <!-- http://www.sisostds.org/ontologies/lox#NTRCOM -->

    <owl:NamedIndividual rdf:about="http://www.sisostds.org/ontologies/lox#NTRCOM">
        <rdf:type rdf:resource="http://www.sisostds.org/ontologies/C2SIM#TaskActionCode"/>
        <rdfs:comment>Neutralize, combat: To render ineffective or unusable in military operations.</rdfs:comment>
    </owl:NamedIndividual>
    


    <!-- http://www.sisostds.org/ontologies/lox#NTREXP -->

    <owl:NamedIndividual rdf:about="http://www.sisostds.org/ontologies/lox#NTREXP">
        <rdf:type rdf:resource="http://www.sisostds.org/ontologies/C2SIM#TaskActionCode"/>
        <rdfs:comment>Neutralize, explosive: To render bombs, mines, missiles and booby traps into a safe state.</rdfs:comment>
    </owl:NamedIndividual>
    


    <!-- http://www.sisostds.org/ontologies/lox#NUCSMP -->

    <owl:NamedIndividual rdf:about="http://www.sisostds.org/ontologies/lox#NUCSMP">
        <rdf:type rdf:resource="http://www.sisostds.org/ontologies/C2SIM#TaskActionCode"/>
        <rdfs:comment>Nuclear sampling: To collect samples for testing for nuclear hazards.</rdfs:comment>
    </owl:NamedIndividual>
    


    <!-- http://www.sisostds.org/ontologies/lox#NUTRLD -->

    <owl:NamedIndividual rdf:about="http://www.sisostds.org/ontologies/lox#NUTRLD">
        <rdfs:comment>Documentation: 		
						The rendering of the ACTION objective temporarily ineffective by the infliction of significant casualties (norm for indirect fire is 10 percent).	
					; Appinfo DisplayValue as &quot;Neutralized&quot;</rdfs:comment>
    </owl:NamedIndividual>
    


    <!-- http://www.sisostds.org/ontologies/lox#NVLPLF -->

    <owl:NamedIndividual rdf:about="http://www.sisostds.org/ontologies/lox#NVLPLF">
        <rdf:type rdf:resource="http://www.sisostds.org/ontologies/C2SIM#TaskActionCode"/>
        <rdfs:comment>Naval platform flight operations: To launch or recover aircraft by a naval platform.</rdfs:comment>
    </owl:NamedIndividual>
    


    <!-- http://www.sisostds.org/ontologies/lox#OBSCUR -->

    <owl:NamedIndividual rdf:about="http://www.sisostds.org/ontologies/lox#OBSCUR">
        <rdf:type rdf:resource="http://www.sisostds.org/ontologies/C2SIM#TaskActionCode"/>
        <rdfs:comment>Documentation: 		
						To cover something by a smoke screen.	
					; Appinfo DisplayValue as &quot;Obscure&quot;</rdfs:comment>
        <rdfs:comment>Obscure: To cover something by a smoke screen.</rdfs:comment>
    </owl:NamedIndividual>
    


    <!-- http://www.sisostds.org/ontologies/lox#OBSRV -->

    <owl:NamedIndividual rdf:about="http://www.sisostds.org/ontologies/lox#OBSRV">
        <rdf:type rdf:resource="http://www.sisostds.org/ontologies/C2SIM#TaskActionCode"/>
        <rdfs:comment>Documentation: 		
						To provide continuous view, and the potential for reports on the activity of an ACTION-OBJECTIVE.	
					; Appinfo DisplayValue as &quot;Observe&quot;</rdfs:comment>
        <rdfs:comment>Observe: To provide continuous view, and the potential for reports on the activity of an ACTION-OBJECTIVE.</rdfs:comment>
    </owl:NamedIndividual>
    


    <!-- http://www.sisostds.org/ontologies/lox#OCCUPY -->

    <owl:NamedIndividual rdf:about="http://www.sisostds.org/ontologies/lox#OCCUPY">
        <rdf:type rdf:resource="http://www.sisostds.org/ontologies/C2SIM#TaskActionCode"/>
        <rdfs:comment>Documentation: 		
						To move onto an objective, key terrain, or other manmade or natural terrain area without opposition and control that entire area.	
					; Appinfo DisplayValue as &quot;Occupy&quot;</rdfs:comment>
        <rdfs:comment>Occupy: To move onto an objective, key terrain, or other manmade or natural terrain area without opposition and control that entire</rdfs:comment>
    </owl:NamedIndividual>
    


    <!-- http://www.sisostds.org/ontologies/lox#OFFAIR -->

    <owl:NamedIndividual rdf:about="http://www.sisostds.org/ontologies/lox#OFFAIR">
        <rdf:type rdf:resource="http://www.sisostds.org/ontologies/C2SIM#TaskActionCode"/>
        <rdfs:comment>Offensive air support: To provide support by the air forces on land or sea in offensive operations.</rdfs:comment>
    </owl:NamedIndividual>
    


    <!-- http://www.sisostds.org/ontologies/lox#OFFCNA -->

    <owl:NamedIndividual rdf:about="http://www.sisostds.org/ontologies/lox#OFFCNA">
        <rdf:type rdf:resource="http://www.sisostds.org/ontologies/C2SIM#TaskActionCode"/>
        <rdfs:comment>Offensive counter air: To conduct an operation to destroy, disrupt or limit enemy air power as close to its source as possible.</rdfs:comment>
    </owl:NamedIndividual>
    


    <!-- http://www.sisostds.org/ontologies/lox#ORGCNF -->

    <owl:NamedIndividual rdf:about="http://www.sisostds.org/ontologies/lox#ORGCNF">
        <rdf:type rdf:resource="http://www.sisostds.org/ontologies/C2SIM#TaskActionCode"/>
        <rdfs:comment>Organise conference: To organise a meeting for discussion, esp. a regular one held by an association or organisation.</rdfs:comment>
    </owl:NamedIndividual>
    


    <!-- http://www.sisostds.org/ontologies/lox#ORGMED -->

    <owl:NamedIndividual rdf:about="http://www.sisostds.org/ontologies/lox#ORGMED">
        <rdf:type rdf:resource="http://www.sisostds.org/ontologies/C2SIM#TaskActionCode"/>
        <rdfs:comment>Organise media interview: To organise a conversation between a reporter etc. and a person of public interest, used as a basis of a broadcast or publication.</rdfs:comment>
    </owl:NamedIndividual>
    


    <!-- http://www.sisostds.org/ontologies/lox#ORGRCR -->

    <owl:NamedIndividual rdf:about="http://www.sisostds.org/ontologies/lox#ORGRCR">
        <rdf:type rdf:resource="http://www.sisostds.org/ontologies/C2SIM#TaskActionCode"/>
        <rdfs:comment>Organise recreational activities: To organise a refreshing or entertaining activity.</rdfs:comment>
    </owl:NamedIndividual>
    


    <!-- http://www.sisostds.org/ontologies/lox#ORGSCL -->

    <owl:NamedIndividual rdf:about="http://www.sisostds.org/ontologies/lox#ORGSCL">
        <rdf:type rdf:resource="http://www.sisostds.org/ontologies/C2SIM#TaskActionCode"/>
        <rdfs:comment>Organise social events: To organise any social gathering, esp. one organised by a club or congregation.</rdfs:comment>
    </owl:NamedIndividual>
    


    <!-- http://www.sisostds.org/ontologies/lox#ORGSPT -->

    <owl:NamedIndividual rdf:about="http://www.sisostds.org/ontologies/lox#ORGSPT">
        <rdf:type rdf:resource="http://www.sisostds.org/ontologies/C2SIM#TaskActionCode"/>
        <rdfs:comment>Organise sporting events: To organise any game or competitive activity, esp. an outdoor one involving physical exertion.</rdfs:comment>
    </owl:NamedIndividual>
    


    <!-- http://www.sisostds.org/ontologies/lox#OneTaskComplete -->

    <owl:NamedIndividual rdf:about="http://www.sisostds.org/ontologies/lox#OneTaskComplete">
        <rdf:type rdf:resource="http://www.sisostds.org/ontologies/lox#PlanPhaseCompletionCondition"/>
    </owl:NamedIndividual>
    


    <!-- http://www.sisostds.org/ontologies/lox#OtherOrderReceived -->

    <owl:NamedIndividual rdf:about="http://www.sisostds.org/ontologies/lox#OtherOrderReceived">
        <rdf:type rdf:resource="http://www.sisostds.org/ontologies/lox#PlanPhaseCompletionCondition"/>
    </owl:NamedIndividual>
    


    <!-- http://www.sisostds.org/ontologies/lox#PATROL -->

    <owl:NamedIndividual rdf:about="http://www.sisostds.org/ontologies/lox#PATROL">
        <rdf:type rdf:resource="http://www.sisostds.org/ontologies/C2SIM#TaskActionCode"/>
        <rdfs:comment>Documentation: 		
						To gather information or to carry out a destructive, harassing, mopping-up, or security mission.	
					; Appinfo DisplayValue as &quot;Patrol&quot;</rdfs:comment>
        <rdfs:comment>Patrol: To gather information or to carry out a destructive, harassing, mopping-up, or security mission.</rdfs:comment>
    </owl:NamedIndividual>
    


    <!-- http://www.sisostds.org/ontologies/lox#PENTRT -->

    <owl:NamedIndividual rdf:about="http://www.sisostds.org/ontologies/lox#PENTRT">
        <rdf:type rdf:resource="http://www.sisostds.org/ontologies/C2SIM#TaskActionCode"/>
        <rdfs:comment>Documentation: 		
						To break through the enemy&apos;s defence or to disrupt the enemy&apos;s defensive systems.	
					; Appinfo DisplayValue as &quot;Penetrate&quot;</rdfs:comment>
        <rdfs:comment>Penetrate: To break through the enemy&apos;s defence or to disrupt the enemy&apos;s defensive systems.</rdfs:comment>
    </owl:NamedIndividual>
    


    <!-- http://www.sisostds.org/ontologies/lox#PHOTO -->

    <owl:NamedIndividual rdf:about="http://www.sisostds.org/ontologies/lox#PHOTO">
        <rdf:type rdf:resource="http://www.sisostds.org/ontologies/C2SIM#TaskActionCode"/>
        <rdfs:comment>Photo mapping: To collect a series of photographs from which it is possible to create maps.</rdfs:comment>
    </owl:NamedIndividual>
    


    <!-- http://www.sisostds.org/ontologies/lox#PLAN -->

    <owl:NamedIndividual rdf:about="http://www.sisostds.org/ontologies/lox#PLAN">
        <rdf:type rdf:resource="http://www.sisostds.org/ontologies/C2SIM#TaskActionCode"/>
        <rdfs:comment>Documentation: 		
						To create a detailed formulation of a programme of action.	
					; Appinfo DisplayValue as &quot;Plan&quot;</rdfs:comment>
        <rdfs:comment>Plan: To create a detailed formulation of a programme of action.</rdfs:comment>
    </owl:NamedIndividual>
    


    <!-- http://www.sisostds.org/ontologies/lox#PREFIR -->

    <owl:NamedIndividual rdf:about="http://www.sisostds.org/ontologies/lox#PREFIR">
        <rdf:type rdf:resource="http://www.sisostds.org/ontologies/C2SIM#TaskActionCode"/>
        <rdfs:comment>Documentation: 		
						To deliver fire on a target preparatory to an assault.	
					; Appinfo DisplayValue as &quot;Preparatory fire&quot;</rdfs:comment>
        <rdfs:comment>Preparatory fire: To deliver fire on a target preparatory to an assault.</rdfs:comment>
    </owl:NamedIndividual>
    


    <!-- http://www.sisostds.org/ontologies/lox#PREPR -->

    <owl:NamedIndividual rdf:about="http://www.sisostds.org/ontologies/lox#PREPR">
        <rdf:type rdf:resource="http://www.sisostds.org/ontologies/C2SIM#TaskActionCode"/>
        <rdfs:comment>Prepare: To establish certain conditions.</rdfs:comment>
    </owl:NamedIndividual>
    


    <!-- http://www.sisostds.org/ontologies/lox#PROCUR -->

    <owl:NamedIndividual rdf:about="http://www.sisostds.org/ontologies/lox#PROCUR">
        <rdf:type rdf:resource="http://www.sisostds.org/ontologies/C2SIM#TaskActionCode"/>
        <rdfs:comment>Procure: To buy whatever is needed to fulfil a certain action.</rdfs:comment>
    </owl:NamedIndividual>
    


    <!-- http://www.sisostds.org/ontologies/lox#PROTEL -->

    <owl:NamedIndividual rdf:about="http://www.sisostds.org/ontologies/lox#PROTEL">
        <rdf:type rdf:resource="http://www.sisostds.org/ontologies/C2SIM#TaskActionCode"/>
        <rdfs:comment>Protection, electronic: That division of electronic warfare involving actions taken to ensure effective friendly use of the electromagnetic spectrum</rdfs:comment>
    </owl:NamedIndividual>
    


    <!-- http://www.sisostds.org/ontologies/lox#PRVACC -->

    <owl:NamedIndividual rdf:about="http://www.sisostds.org/ontologies/lox#PRVACC">
        <rdf:type rdf:resource="http://www.sisostds.org/ontologies/C2SIM#TaskActionCode"/>
        <rdfs:comment>Provide accommodation: To provide room for receiving people, esp. a place to live or lodgings.</rdfs:comment>
    </owl:NamedIndividual>
    


    <!-- http://www.sisostds.org/ontologies/lox#PRVAGR -->

    <owl:NamedIndividual rdf:about="http://www.sisostds.org/ontologies/lox#PRVAGR">
        <rdf:type rdf:resource="http://www.sisostds.org/ontologies/C2SIM#TaskActionCode"/>
        <rdfs:comment>Provide agricultural support: To provide advice or supplies for cultivating the soil and rearing animals.</rdfs:comment>
    </owl:NamedIndividual>
    


    <!-- http://www.sisostds.org/ontologies/lox#PRVBDD -->

    <owl:NamedIndividual rdf:about="http://www.sisostds.org/ontologies/lox#PRVBDD">
        <rdf:type rdf:resource="http://www.sisostds.org/ontologies/C2SIM#TaskActionCode"/>
        <rdfs:comment>Provide bedding: To provide (1) sleeping accommodation or (2) mattress and bedclothes.</rdfs:comment>
    </owl:NamedIndividual>
    


    <!-- http://www.sisostds.org/ontologies/lox#PRVCMP -->

    <owl:NamedIndividual rdf:about="http://www.sisostds.org/ontologies/lox#PRVCMP">
        <rdf:type rdf:resource="http://www.sisostds.org/ontologies/C2SIM#TaskActionCode"/>
        <rdfs:comment>Provide camps: To provide temporary accommodation of various kinds, usually consisting of huts or tents, for detainees, homeless persons,</rdfs:comment>
    </owl:NamedIndividual>
    


    <!-- http://www.sisostds.org/ontologies/lox#PRVCNS -->

    <owl:NamedIndividual rdf:about="http://www.sisostds.org/ontologies/lox#PRVCNS">
        <rdf:type rdf:resource="http://www.sisostds.org/ontologies/C2SIM#TaskActionCode"/>
        <rdfs:comment>Provide construction services: To provide labour and materiel for construction of facilities.</rdfs:comment>
    </owl:NamedIndividual>
    


    <!-- http://www.sisostds.org/ontologies/lox#PRVEDU -->

    <owl:NamedIndividual rdf:about="http://www.sisostds.org/ontologies/lox#PRVEDU">
        <rdf:type rdf:resource="http://www.sisostds.org/ontologies/C2SIM#TaskActionCode"/>
        <rdfs:comment>Provide education services: To provide labour and materiel for the educational process.</rdfs:comment>
    </owl:NamedIndividual>
    


    <!-- http://www.sisostds.org/ontologies/lox#PRVHLT -->

    <owl:NamedIndividual rdf:about="http://www.sisostds.org/ontologies/lox#PRVHLT">
        <rdf:type rdf:resource="http://www.sisostds.org/ontologies/C2SIM#TaskActionCode"/>
        <rdfs:comment>Provide healthcare services: To provide labour and materiel for maintaining the general health and welfare.</rdfs:comment>
    </owl:NamedIndividual>
    


    <!-- http://www.sisostds.org/ontologies/lox#PRVINF -->

    <owl:NamedIndividual rdf:about="http://www.sisostds.org/ontologies/lox#PRVINF">
        <rdf:type rdf:resource="http://www.sisostds.org/ontologies/C2SIM#TaskActionCode"/>
        <rdfs:comment>Provide infrastructure: To provide basic facilities such as roads, bridges, and sewers.</rdfs:comment>
    </owl:NamedIndividual>
    


    <!-- http://www.sisostds.org/ontologies/lox#PRVLND -->

    <owl:NamedIndividual rdf:about="http://www.sisostds.org/ontologies/lox#PRVLND">
        <rdf:type rdf:resource="http://www.sisostds.org/ontologies/C2SIM#TaskActionCode"/>
        <rdfs:comment>Provide laundry services: To provide labour and materiel for laundering of clothes or linens.</rdfs:comment>
    </owl:NamedIndividual>
    


    <!-- http://www.sisostds.org/ontologies/lox#PRVRPR -->

    <owl:NamedIndividual rdf:about="http://www.sisostds.org/ontologies/lox#PRVRPR">
        <rdf:type rdf:resource="http://www.sisostds.org/ontologies/C2SIM#TaskActionCode"/>
        <rdfs:comment>Provide repair services: To provide labour and materiel to restore objects to unimpaired condition.</rdfs:comment>
    </owl:NamedIndividual>
    


    <!-- http://www.sisostds.org/ontologies/lox#PRVSCY -->

    <owl:NamedIndividual rdf:about="http://www.sisostds.org/ontologies/lox#PRVSCY">
        <rdf:type rdf:resource="http://www.sisostds.org/ontologies/C2SIM#TaskActionCode"/>
        <rdfs:comment>Provide security services: To provide labour and materiel to assure safety of personnel and facilities.</rdfs:comment>
    </owl:NamedIndividual>
    


    <!-- http://www.sisostds.org/ontologies/lox#PRVSHL -->

    <owl:NamedIndividual rdf:about="http://www.sisostds.org/ontologies/lox#PRVSHL">
        <rdf:type rdf:resource="http://www.sisostds.org/ontologies/C2SIM#TaskActionCode"/>
        <rdfs:comment>Provide shelter: To provide housing.</rdfs:comment>
    </owl:NamedIndividual>
    


    <!-- http://www.sisostds.org/ontologies/lox#PRVSTG -->

    <owl:NamedIndividual rdf:about="http://www.sisostds.org/ontologies/lox#PRVSTG">
        <rdf:type rdf:resource="http://www.sisostds.org/ontologies/C2SIM#TaskActionCode"/>
        <rdfs:comment>Provide storage services: To provide services for storage.</rdfs:comment>
    </owl:NamedIndividual>
    


    <!-- http://www.sisostds.org/ontologies/lox#PRVTRS -->

    <owl:NamedIndividual rdf:about="http://www.sisostds.org/ontologies/lox#PRVTRS">
        <rdf:type rdf:resource="http://www.sisostds.org/ontologies/C2SIM#TaskActionCode"/>
        <rdfs:comment>Provide transhipment services: To provide movement of cargo from one ship or train or container to another for further shipment.</rdfs:comment>
    </owl:NamedIndividual>
    


    <!-- http://www.sisostds.org/ontologies/lox#PSYCHW -->

    <owl:NamedIndividual rdf:about="http://www.sisostds.org/ontologies/lox#PSYCHW">
        <rdf:type rdf:resource="http://www.sisostds.org/ontologies/C2SIM#TaskActionCode"/>
        <rdfs:comment>Psychological warfare: To use propaganda or other means designed to undermine the morale or allegiance of one&apos;s opponents.</rdfs:comment>
    </owl:NamedIndividual>
    


    <!-- http://www.sisostds.org/ontologies/lox#PUBMDA -->

    <owl:NamedIndividual rdf:about="http://www.sisostds.org/ontologies/lox#PUBMDA">
        <rdf:type rdf:resource="http://www.sisostds.org/ontologies/C2SIM#TaskActionCode"/>
        <rdfs:comment>Publish media article: To make generally known a non-fictional essay, esp. one included with others in a newspaper, magazine, journal, etc.</rdfs:comment>
    </owl:NamedIndividual>
    


    <!-- http://www.sisostds.org/ontologies/lox#PUBMDD -->

    <owl:NamedIndividual rdf:about="http://www.sisostds.org/ontologies/lox#PUBMDD">
        <rdf:type rdf:resource="http://www.sisostds.org/ontologies/C2SIM#TaskActionCode"/>
        <rdfs:comment>Publish media documentary: To make generally known any document published on a media that provides a factual record or report.</rdfs:comment>
    </owl:NamedIndividual>
    


    <!-- http://www.sisostds.org/ontologies/lox#PUBPRS -->

    <owl:NamedIndividual rdf:about="http://www.sisostds.org/ontologies/lox#PUBPRS">
        <rdf:type rdf:resource="http://www.sisostds.org/ontologies/C2SIM#TaskActionCode"/>
        <rdfs:comment>Publish press release: To make generally known an official statement issued to media for information.</rdfs:comment>
    </owl:NamedIndividual>
    


    <!-- http://www.sisostds.org/ontologies/lox#PURSUE -->

    <owl:NamedIndividual rdf:about="http://www.sisostds.org/ontologies/lox#PURSUE">
        <rdf:type rdf:resource="http://www.sisostds.org/ontologies/C2SIM#TaskActionCode"/>
        <rdfs:comment>Documentation: 		
						To continue offensive operations designed to catch or cut off a hostile force attempting to escape, with the aim of destroying it. Typically, contact is maintained and risk taken to harass relentlessly, thereby turning the pursuit into a rout.	
					; Appinfo DisplayValue as &quot;Pursue&quot;</rdfs:comment>
        <rdfs:comment>Pursue: To continue offensive operations designed to catch or cut off a hostile force attempting to escape, with the aim of destroying</rdfs:comment>
    </owl:NamedIndividual>
    


    <!-- http://www.sisostds.org/ontologies/lox#RCALIB -->

    <owl:NamedIndividual rdf:about="http://www.sisostds.org/ontologies/lox#RCALIB">
        <rdf:type rdf:resource="http://www.sisostds.org/ontologies/C2SIM#TaskActionCode"/>
        <rdfs:comment>Radio/radar calibration: To fly on a specific route in order to allow calibration of radars and radios.</rdfs:comment>
    </owl:NamedIndividual>
    


    <!-- http://www.sisostds.org/ontologies/lox#RECARM -->

    <owl:NamedIndividual rdf:about="http://www.sisostds.org/ontologies/lox#RECARM">
        <rdf:type rdf:resource="http://www.sisostds.org/ontologies/C2SIM#TaskActionCode"/>
        <rdfs:comment>Reconnaissance, armed: To locate and attack targets of opportunity, i.e. enemy material, personnel, and facilities in assigned surface communications</rdfs:comment>
    </owl:NamedIndividual>
    


    <!-- http://www.sisostds.org/ontologies/lox#RECCE -->

    <owl:NamedIndividual rdf:about="http://www.sisostds.org/ontologies/lox#RECCE">
        <rdf:type rdf:resource="http://www.sisostds.org/ontologies/C2SIM#TaskActionCode"/>
        <rdfs:comment>Documentation: 		
						To conduct a mission to obtain by visual operations or other detection methods information about the activities and resources of an enemy or potential enemy, or to secure data concerning the meteorological, hydrographic or geographic characteristics of a particular area.	
					; Appinfo DisplayValue as &quot;Reconnaissance&quot;</rdfs:comment>
        <rdfs:comment>Reconnaissance: To conduct a mission to obtain by visual operations or other detection methods information about the activities and resources</rdfs:comment>
    </owl:NamedIndividual>
    


    <!-- http://www.sisostds.org/ontologies/lox#RECCEF -->

    <owl:NamedIndividual rdf:about="http://www.sisostds.org/ontologies/lox#RECCEF">
        <rdf:type rdf:resource="http://www.sisostds.org/ontologies/C2SIM#TaskActionCode"/>
        <rdfs:comment>Reconnaissance in force: To conduct an offensive operation designed to discover and/or test the enemy&apos;s strength, or to obtain other information.</rdfs:comment>
    </owl:NamedIndividual>
    


    <!-- http://www.sisostds.org/ontologies/lox#RECCEL -->

    <owl:NamedIndividual rdf:about="http://www.sisostds.org/ontologies/lox#RECCEL">
        <rdf:type rdf:resource="http://www.sisostds.org/ontologies/C2SIM#TaskActionCode"/>
        <rdfs:comment>Reconnaissance, land: To obtain information concerning terrain, weather, and the disposition, composition, movement, installations, lines of communications,</rdfs:comment>
    </owl:NamedIndividual>
    


    <!-- http://www.sisostds.org/ontologies/lox#RECCES -->

    <owl:NamedIndividual rdf:about="http://www.sisostds.org/ontologies/lox#RECCES">
        <rdf:type rdf:resource="http://www.sisostds.org/ontologies/C2SIM#TaskActionCode"/>
        <rdfs:comment>Reconnaissance, shadow: To observe an enemy unit or force, usually as a sequel to surveillance or reconnaissance, for the purpose of reporting its</rdfs:comment>
    </owl:NamedIndividual>
    


    <!-- http://www.sisostds.org/ontologies/lox#RECECM -->

    <owl:NamedIndividual rdf:about="http://www.sisostds.org/ontologies/lox#RECECM">
        <rdf:type rdf:resource="http://www.sisostds.org/ontologies/C2SIM#TaskActionCode"/>
        <rdfs:comment>Reconnaissance, ECM: To detect ECM activities and resources of an enemy or potential enemy in a particular area.</rdfs:comment>
    </owl:NamedIndividual>
    


    <!-- http://www.sisostds.org/ontologies/lox#RECONS -->

    <owl:NamedIndividual rdf:about="http://www.sisostds.org/ontologies/lox#RECONS">
        <rdf:type rdf:resource="http://www.sisostds.org/ontologies/C2SIM#TaskActionCode"/>
        <rdfs:comment>Documentation: 		
						To attain prescribed strength of units and prescribed levels of vehicles, equipment, stores and supplies. The process will only take place after a unit/formation combat effectiveness has been reduced.	
					; Appinfo DisplayValue as &quot;Reconstitute&quot;</rdfs:comment>
        <rdfs:comment>Reconstitute: To attain prescribed strength of units and prescribed levels of vehicles, equipment, stores and supplies. The process will</rdfs:comment>
    </owl:NamedIndividual>
    


    <!-- http://www.sisostds.org/ontologies/lox#RECOVR -->

    <owl:NamedIndividual rdf:about="http://www.sisostds.org/ontologies/lox#RECOVR">
        <rdf:type rdf:resource="http://www.sisostds.org/ontologies/C2SIM#TaskActionCode"/>
        <rdfs:comment>Documentation: 		
						To retrieve any lost, incapacitated or captured object.	
					; Appinfo DisplayValue as &quot;Recover&quot;</rdfs:comment>
        <rdfs:comment>Recover: To retrieve any lost, incapacitated or captured object.</rdfs:comment>
    </owl:NamedIndividual>
    


    <!-- http://www.sisostds.org/ontologies/lox#RECPHO -->

    <owl:NamedIndividual rdf:about="http://www.sisostds.org/ontologies/lox#RECPHO">
        <rdf:type rdf:resource="http://www.sisostds.org/ontologies/C2SIM#TaskActionCode"/>
        <rdfs:comment>Reconnaissance, photographic: To obtain, by photographic means, information about the activities and resources of an enemy or potential enemy, or to secure</rdfs:comment>
    </owl:NamedIndividual>
    


    <!-- http://www.sisostds.org/ontologies/lox#RECRAD -->

    <owl:NamedIndividual rdf:about="http://www.sisostds.org/ontologies/lox#RECRAD">
        <rdf:type rdf:resource="http://www.sisostds.org/ontologies/C2SIM#TaskActionCode"/>
        <rdfs:comment>Reconnaissance, radar: To obtain, by radar detection methods, information about the activities and resources of an enemy or potential enemy, or to</rdfs:comment>
    </owl:NamedIndividual>
    


    <!-- http://www.sisostds.org/ontologies/lox#RECTGT -->

    <owl:NamedIndividual rdf:about="http://www.sisostds.org/ontologies/lox#RECTGT">
        <rdf:type rdf:resource="http://www.sisostds.org/ontologies/C2SIM#TaskActionCode"/>
        <rdfs:comment>Reconnaissance, target: To obtain information about the activities and resources of a target.</rdfs:comment>
    </owl:NamedIndividual>
    


    <!-- http://www.sisostds.org/ontologies/lox#RECUPR -->

    <owl:NamedIndividual rdf:about="http://www.sisostds.org/ontologies/lox#RECUPR">
        <rdf:type rdf:resource="http://www.sisostds.org/ontologies/C2SIM#TaskActionCode"/>
        <rdfs:comment>Recuperate: To rest a unit after it has been in action. Some reconstitution may take place as well.</rdfs:comment>
    </owl:NamedIndividual>
    


    <!-- http://www.sisostds.org/ontologies/lox#RECVIS -->

    <owl:NamedIndividual rdf:about="http://www.sisostds.org/ontologies/lox#RECVIS">
        <rdf:type rdf:resource="http://www.sisostds.org/ontologies/C2SIM#TaskActionCode"/>
        <rdfs:comment>Reconnaissance, visual: To obtain visual information about the activities and resources of an enemy or potential enemy, or to secure data concerning</rdfs:comment>
    </owl:NamedIndividual>
    


    <!-- http://www.sisostds.org/ontologies/lox#REDEPL -->

    <owl:NamedIndividual rdf:about="http://www.sisostds.org/ontologies/lox#REDEPL">
        <rdf:type rdf:resource="http://www.sisostds.org/ontologies/C2SIM#TaskActionCode"/>
        <rdfs:comment>Redeploy: To transfer a unit, an individual, or supplies deployed in one area to another area, or to another location within the area,</rdfs:comment>
    </owl:NamedIndividual>
    


    <!-- http://www.sisostds.org/ontologies/lox#REFILL -->

    <owl:NamedIndividual rdf:about="http://www.sisostds.org/ontologies/lox#REFILL">
        <rdf:type rdf:resource="http://www.sisostds.org/ontologies/C2SIM#TaskActionCode"/>
        <rdfs:comment>Refill: To fill again.</rdfs:comment>
    </owl:NamedIndividual>
    


    <!-- http://www.sisostds.org/ontologies/lox#REFORM -->

    <owl:NamedIndividual rdf:about="http://www.sisostds.org/ontologies/lox#REFORM">
        <rdf:type rdf:resource="http://www.sisostds.org/ontologies/C2SIM#TaskActionCode"/>
        <rdfs:comment>Reform: No definition provided in ADatP-3 Baseline 13.1 FFIRN/FUD 1299/19.</rdfs:comment>
    </owl:NamedIndividual>
    


    <!-- http://www.sisostds.org/ontologies/lox#REFUEL -->

    <owl:NamedIndividual rdf:about="http://www.sisostds.org/ontologies/lox#REFUEL">
        <rdf:type rdf:resource="http://www.sisostds.org/ontologies/C2SIM#TaskActionCode"/>
        <rdfs:comment>Documentation: 		
						To take on more fuel.	
					; Appinfo DisplayValue as &quot;Refuel&quot;</rdfs:comment>
        <rdfs:comment>Refuel: To take on more fuel.</rdfs:comment>
    </owl:NamedIndividual>
    


    <!-- http://www.sisostds.org/ontologies/lox#REINF -->

    <owl:NamedIndividual rdf:about="http://www.sisostds.org/ontologies/lox#REINF">
        <rdf:type rdf:resource="http://www.sisostds.org/ontologies/C2SIM#TaskActionCode"/>
        <rdfs:comment>Documentation: 		
						To move or make a force available to another commander for the purpose of supplementing the in-place forces.	
					; Appinfo DisplayValue as &quot;Reinforce&quot;</rdfs:comment>
        <rdfs:comment>Reinforce: To move or make a force available to another commander for the purpose of supplementing the in-place forces.</rdfs:comment>
    </owl:NamedIndividual>
    


    <!-- http://www.sisostds.org/ontologies/lox#REORG -->

    <owl:NamedIndividual rdf:about="http://www.sisostds.org/ontologies/lox#REORG">
        <rdf:type rdf:resource="http://www.sisostds.org/ontologies/C2SIM#TaskActionCode"/>
        <rdfs:comment>Reorganise: To change a task organisation for a particular operation. (Normally takes place before an operation). This includes the transfer</rdfs:comment>
    </owl:NamedIndividual>
    


    <!-- http://www.sisostds.org/ontologies/lox#REPAIR -->

    <owl:NamedIndividual rdf:about="http://www.sisostds.org/ontologies/lox#REPAIR">
        <rdf:type rdf:resource="http://www.sisostds.org/ontologies/C2SIM#TaskActionCode"/>
        <rdfs:comment>Repair: To restore an item to serviceable condition through correction of a specific failure or unserviceable condition.</rdfs:comment>
    </owl:NamedIndividual>
    


    <!-- http://www.sisostds.org/ontologies/lox#RESCUE -->

    <owl:NamedIndividual rdf:about="http://www.sisostds.org/ontologies/lox#RESCUE">
        <rdf:type rdf:resource="http://www.sisostds.org/ontologies/C2SIM#TaskActionCode"/>
        <rdfs:comment>Documentation: 		
						To use aircraft, surface craft (land or water), submarines, specialized rescue teams, and equipment to rescue personnel in distress on land or at sea.	
					; Appinfo DisplayValue as &quot;Rescue&quot;</rdfs:comment>
        <rdfs:comment>Rescue: To use aircraft, surface craft (land or water), submarines, specialized rescue teams, and equipment to rescue personnel in</rdfs:comment>
    </owl:NamedIndividual>
    


    <!-- http://www.sisostds.org/ontologies/lox#REST -->

    <owl:NamedIndividual rdf:about="http://www.sisostds.org/ontologies/lox#REST">
        <rdf:type rdf:resource="http://www.sisostds.org/ontologies/C2SIM#TaskActionCode"/>
        <rdfs:comment>Rest: To impose a specified period of inactivity on an ORGANISATION that is out of contact with the enemy.</rdfs:comment>
    </owl:NamedIndividual>
    


    <!-- http://www.sisostds.org/ontologies/lox#RESUPL -->

    <owl:NamedIndividual rdf:about="http://www.sisostds.org/ontologies/lox#RESUPL">
        <rdf:type rdf:resource="http://www.sisostds.org/ontologies/C2SIM#TaskActionCode"/>
        <rdfs:comment>Documentation: 		
						To replenish stocks in order to maintain the required levels of supply.	
					; Appinfo DisplayValue as &quot;Resupply&quot;</rdfs:comment>
        <rdfs:comment>Resupply: To replenish stocks in order to maintain the required levels of supply.</rdfs:comment>
    </owl:NamedIndividual>
    


    <!-- http://www.sisostds.org/ontologies/lox#RETAIN -->

    <owl:NamedIndividual rdf:about="http://www.sisostds.org/ontologies/lox#RETAIN">
        <rdf:type rdf:resource="http://www.sisostds.org/ontologies/C2SIM#TaskActionCode"/>
        <rdfs:comment>Documentation: 		
						To occupy and hold a terrain feature to ensure it is free of enemy occupation or use.	
					; Appinfo DisplayValue as &quot;Retain&quot;</rdfs:comment>
        <rdfs:comment>Retain: To occupy and hold a terrain feature to ensure it is free of enemy occupation or use.</rdfs:comment>
    </owl:NamedIndividual>
    


    <!-- http://www.sisostds.org/ontologies/lox#RETIRE -->

    <owl:NamedIndividual rdf:about="http://www.sisostds.org/ontologies/lox#RETIRE">
        <rdf:type rdf:resource="http://www.sisostds.org/ontologies/C2SIM#TaskActionCode"/>
        <rdfs:comment>Retire: To move a force out of contact with the enemy with the expectation of no further significant contact.</rdfs:comment>
    </owl:NamedIndividual>
    


    <!-- http://www.sisostds.org/ontologies/lox#RLFPLC -->

    <owl:NamedIndividual rdf:about="http://www.sisostds.org/ontologies/lox#RLFPLC">
        <rdf:type rdf:resource="http://www.sisostds.org/ontologies/C2SIM#TaskActionCode"/>
        <rdfs:comment>Documentation: 		
						To conduct an operation in which, by direction of higher authority, all or part of a unit is replaced in an area by the incoming unit. The responsibilities of the replaced elements for the mission and the assigned zone of operations are transferred to the incoming unit. The incoming unit continues the operation as ordered.	
					; Appinfo DisplayValue as &quot;Relief in place&quot;</rdfs:comment>
        <rdfs:comment>Relief in place: To conduct an operation in which, by direction of higher authority, all or part of a unit is replaced in an area by the incoming</rdfs:comment>
    </owl:NamedIndividual>
    


    <!-- http://www.sisostds.org/ontologies/lox#RNDZVA -->

    <owl:NamedIndividual rdf:about="http://www.sisostds.org/ontologies/lox#RNDZVA">
        <rdf:type rdf:resource="http://www.sisostds.org/ontologies/C2SIM#TaskActionCode"/>
        <rdfs:comment>Rendezvous procedure alpha: To rendezvous using a procedure directed by a radar control station, whether ground based, seaborne, or airborne (anchor rendezvous).</rdfs:comment>
    </owl:NamedIndividual>
    


    <!-- http://www.sisostds.org/ontologies/lox#RNDZVB -->

    <owl:NamedIndividual rdf:about="http://www.sisostds.org/ontologies/lox#RNDZVB">
        <rdf:type rdf:resource="http://www.sisostds.org/ontologies/C2SIM#TaskActionCode"/>
        <rdfs:comment>Rendezvous procedure bravo: To rendezvous using a heading based procedure which utilises air-to-air equipment of both tanker and receiver. The tanker</rdfs:comment>
    </owl:NamedIndividual>
    


    <!-- http://www.sisostds.org/ontologies/lox#RNDZVC -->

    <owl:NamedIndividual rdf:about="http://www.sisostds.org/ontologies/lox#RNDZVC">
        <rdf:type rdf:resource="http://www.sisostds.org/ontologies/C2SIM#TaskActionCode"/>
        <rdfs:comment>Rendezvous procedure charlie: To rendezvous using a heading based procedure which allows receivers with an airborne intercept (AI) radar to control the</rdfs:comment>
    </owl:NamedIndividual>
    


    <!-- http://www.sisostds.org/ontologies/lox#RNDZVD -->

    <owl:NamedIndividual rdf:about="http://www.sisostds.org/ontologies/lox#RNDZVD">
        <rdf:type rdf:resource="http://www.sisostds.org/ontologies/C2SIM#TaskActionCode"/>
        <rdfs:comment>Rendezvous procedure delta: To rendezvous using a procedure that requires the receiver to maintain an agreed track and the tanker to maintain the reciprocal</rdfs:comment>
    </owl:NamedIndividual>
    


    <!-- http://www.sisostds.org/ontologies/lox#RNDZVE -->

    <owl:NamedIndividual rdf:about="http://www.sisostds.org/ontologies/lox#RNDZVE">
        <rdf:type rdf:resource="http://www.sisostds.org/ontologies/C2SIM#TaskActionCode"/>
        <rdfs:comment>Rendezvous procedure echo: To rendezvous using a procedure for use in support of a combat air patrol (CAP). It is particularly useful during periods</rdfs:comment>
    </owl:NamedIndividual>
    


    <!-- http://www.sisostds.org/ontologies/lox#RNDZVF -->

    <owl:NamedIndividual rdf:about="http://www.sisostds.org/ontologies/lox#RNDZVF">
        <rdf:type rdf:resource="http://www.sisostds.org/ontologies/C2SIM#TaskActionCode"/>
        <rdfs:comment>Rendezvous procedure foxtrot: To rendezvous using a procedure where the tanker and receiver operate from the same base.</rdfs:comment>
    </owl:NamedIndividual>
    


    <!-- http://www.sisostds.org/ontologies/lox#RNDZVG -->

    <owl:NamedIndividual rdf:about="http://www.sisostds.org/ontologies/lox#RNDZVG">
        <rdf:type rdf:resource="http://www.sisostds.org/ontologies/C2SIM#TaskActionCode"/>
        <rdfs:comment>Rendezvous procedure golf: To rendezvous using a procedure that facilitates join-up on a common track; receivers may have departed either from the same</rdfs:comment>
    </owl:NamedIndividual>
    


    <!-- http://www.sisostds.org/ontologies/lox#RNDZVS -->

    <owl:NamedIndividual rdf:about="http://www.sisostds.org/ontologies/lox#RNDZVS">
        <rdf:type rdf:resource="http://www.sisostds.org/ontologies/C2SIM#TaskActionCode"/>
        <rdfs:comment>Rendezvous: To achieve a pre-arranged meeting at a given time and place.</rdfs:comment>
    </owl:NamedIndividual>
    


    <!-- http://www.sisostds.org/ontologies/lox#ROEFree -->

    <owl:NamedIndividual rdf:about="http://www.sisostds.org/ontologies/lox#ROEFree">
        <rdf:type rdf:resource="http://www.sisostds.org/ontologies/lox#WeaponRuleOfEngagementCode"/>
    </owl:NamedIndividual>
    


    <!-- http://www.sisostds.org/ontologies/lox#ROEHold -->

    <owl:NamedIndividual rdf:about="http://www.sisostds.org/ontologies/lox#ROEHold">
        <rdf:type rdf:resource="http://www.sisostds.org/ontologies/lox#WeaponRuleOfEngagementCode"/>
    </owl:NamedIndividual>
    


    <!-- http://www.sisostds.org/ontologies/lox#ROETight -->

    <owl:NamedIndividual rdf:about="http://www.sisostds.org/ontologies/lox#ROETight">
        <rdf:type rdf:resource="http://www.sisostds.org/ontologies/lox#WeaponRuleOfEngagementCode"/>
    </owl:NamedIndividual>
    


    <!-- http://www.sisostds.org/ontologies/lox#SAR -->

    <owl:NamedIndividual rdf:about="http://www.sisostds.org/ontologies/lox#SAR">
        <rdf:type rdf:resource="http://www.sisostds.org/ontologies/C2SIM#TaskActionCode"/>
        <rdfs:comment>Search and rescue: To use aircraft, surface craft, submarines, specialized rescue teams and equipment to search for and rescue personnel in distress</rdfs:comment>
    </owl:NamedIndividual>
    


    <!-- http://www.sisostds.org/ontologies/lox#SARCME -->

    <owl:NamedIndividual rdf:about="http://www.sisostds.org/ontologies/lox#SARCME">
        <rdf:type rdf:resource="http://www.sisostds.org/ontologies/C2SIM#TaskActionCode"/>
        <rdfs:comment>Search and rescue, combat, exfiltrate: To remove personnel from areas under enemy control by specially trained personnel qualified to penetrate to the site of an</rdfs:comment>
    </owl:NamedIndividual>
    


    <!-- http://www.sisostds.org/ontologies/lox#SARCMI -->

    <owl:NamedIndividual rdf:about="http://www.sisostds.org/ontologies/lox#SARCMI">
        <rdf:type rdf:resource="http://www.sisostds.org/ontologies/C2SIM#TaskActionCode"/>
        <rdfs:comment>Search and rescue, combat, infiltrate: To move through or into an area or territory occupied by either friendly or enemy troops or organisations specially trained</rdfs:comment>
    </owl:NamedIndividual>
    


    <!-- http://www.sisostds.org/ontologies/lox#SARPLG -->

    <owl:NamedIndividual rdf:about="http://www.sisostds.org/ontologies/lox#SARPLG">
        <rdf:type rdf:resource="http://www.sisostds.org/ontologies/C2SIM#TaskActionCode"/>
        <rdfs:comment>Search and rescue, plane guard: Helicopter maintains station in vicinity of carrier for potential SAR during flight operations.</rdfs:comment>
    </owl:NamedIndividual>
    


    <!-- http://www.sisostds.org/ontologies/lox#SCOUT -->

    <owl:NamedIndividual rdf:about="http://www.sisostds.org/ontologies/lox#SCOUT">
        <rdf:type rdf:resource="http://www.sisostds.org/ontologies/C2SIM#TaskActionCode"/>
        <rdfs:comment>Scout: To collect intelligence without engaging enemy forces.</rdfs:comment>
    </owl:NamedIndividual>
    


    <!-- http://www.sisostds.org/ontologies/lox#SCREEN -->

    <owl:NamedIndividual rdf:about="http://www.sisostds.org/ontologies/lox#SCREEN">
        <rdf:type rdf:resource="http://www.sisostds.org/ontologies/C2SIM#TaskActionCode"/>
        <rdfs:comment>Documentation: 		
						To operate as a security element whose primary task is to observe, identify and report information, and which only fights in self-protection.	
					; Appinfo DisplayValue as &quot;Screen&quot;</rdfs:comment>
        <rdfs:comment>Screen: To operate as a security element whose primary task is to observe, identify and report information, and which only fights</rdfs:comment>
    </owl:NamedIndividual>
    


    <!-- http://www.sisostds.org/ontologies/lox#SCRMBL -->

    <owl:NamedIndividual rdf:about="http://www.sisostds.org/ontologies/lox#SCRMBL">
        <rdf:type rdf:resource="http://www.sisostds.org/ontologies/C2SIM#TaskActionCode"/>
        <rdfs:comment>Scramble: To launch or take-off an aircraft as quickly as possible, usually followed by mission instructions.</rdfs:comment>
    </owl:NamedIndividual>
    


    <!-- http://www.sisostds.org/ontologies/lox#SDAM -->

    <owl:NamedIndividual rdf:about="http://www.sisostds.org/ontologies/lox#SDAM">
        <rdfs:comment>Documentation: 		
						The subjective categorisation of the physical effect of an ACTION on buildings, infrastructure and/or equipment by a reporting ORGANISATION.	
					; Appinfo DisplayValue as &quot;Severe damage&quot;</rdfs:comment>
    </owl:NamedIndividual>
    


    <!-- http://www.sisostds.org/ontologies/lox#SECURE -->

    <owl:NamedIndividual rdf:about="http://www.sisostds.org/ontologies/lox#SECURE">
        <rdf:type rdf:resource="http://www.sisostds.org/ontologies/C2SIM#TaskActionCode"/>
        <rdfs:comment>Documentation: 		
						To gain possession of a position or terrain feature, with or without force, and to make such disposition as will prevent, as far as possible, its destruction or loss by enemy action.	
					; Appinfo DisplayValue as &quot;Secure&quot;</rdfs:comment>
        <rdfs:comment>Secure: To gain possession of a position or terrain feature, with or without force, and to make such disposition as will prevent,</rdfs:comment>
    </owl:NamedIndividual>
    


    <!-- http://www.sisostds.org/ontologies/lox#SECURT -->

    <owl:NamedIndividual rdf:about="http://www.sisostds.org/ontologies/lox#SECURT">
        <rdf:type rdf:resource="http://www.sisostds.org/ontologies/C2SIM#TaskActionCode"/>
        <rdfs:comment>Security: To take measures necessary to achieve protection against espionage, sabotage, subversion and terrorism, as well as against</rdfs:comment>
    </owl:NamedIndividual>
    


    <!-- http://www.sisostds.org/ontologies/lox#SEIZE -->

    <owl:NamedIndividual rdf:about="http://www.sisostds.org/ontologies/lox#SEIZE">
        <rdf:type rdf:resource="http://www.sisostds.org/ontologies/C2SIM#TaskActionCode"/>
        <rdfs:comment>Documentation: 		
						To clear a designated area and obtain control of it.	
					; Appinfo DisplayValue as &quot;Seize&quot;</rdfs:comment>
        <rdfs:comment>Seize: To clear a designated area and obtain control of it.</rdfs:comment>
    </owl:NamedIndividual>
    


    <!-- http://www.sisostds.org/ontologies/lox#SENSIM -->

    <owl:NamedIndividual rdf:about="http://www.sisostds.org/ontologies/lox#SENSIM">
        <rdf:type rdf:resource="http://www.sisostds.org/ontologies/C2SIM#TaskActionCode"/>
        <rdfs:comment>Sensor implant: To insert a piece of equipment which detects, and may indicate, and/or record objects and activities by means of energy or</rdfs:comment>
    </owl:NamedIndividual>
    


    <!-- http://www.sisostds.org/ontologies/lox#SERASE -->

    <owl:NamedIndividual rdf:about="http://www.sisostds.org/ontologies/lox#SERASE">
        <rdf:type rdf:resource="http://www.sisostds.org/ontologies/C2SIM#TaskActionCode"/>
        <rdfs:comment>Serve as an assault echelon: To serve as an element of a force which is scheduled for initial assault on the objective area.</rdfs:comment>
    </owl:NamedIndividual>
    


    <!-- http://www.sisostds.org/ontologies/lox#SERATE -->

    <owl:NamedIndividual rdf:about="http://www.sisostds.org/ontologies/lox#SERATE">
        <rdf:type rdf:resource="http://www.sisostds.org/ontologies/C2SIM#TaskActionCode"/>
        <rdfs:comment>Serve as an attack echelon: To serve as a fraction of a command in the direction of depth, to which an attack mission is assigned.</rdfs:comment>
    </owl:NamedIndividual>
    


    <!-- http://www.sisostds.org/ontologies/lox#SERCH -->

    <owl:NamedIndividual rdf:about="http://www.sisostds.org/ontologies/lox#SERCH">
        <rdf:type rdf:resource="http://www.sisostds.org/ontologies/C2SIM#TaskActionCode"/>
        <rdfs:comment>Search: No definition provided in APP-6A.</rdfs:comment>
    </owl:NamedIndividual>
    


    <!-- http://www.sisostds.org/ontologies/lox#SERFLO -->

    <owl:NamedIndividual rdf:about="http://www.sisostds.org/ontologies/lox#SERFLO">
        <rdf:type rdf:resource="http://www.sisostds.org/ontologies/C2SIM#TaskActionCode"/>
        <rdfs:comment>Serve as the follow-on echelon: To serve as, in amphibious operations, that echelon of the assault troops, vehicles, aircraft equipment, and supplies which,</rdfs:comment>
    </owl:NamedIndividual>
    


    <!-- http://www.sisostds.org/ontologies/lox#SERFOE -->

    <owl:NamedIndividual rdf:about="http://www.sisostds.org/ontologies/lox#SERFOE">
        <rdf:type rdf:resource="http://www.sisostds.org/ontologies/C2SIM#TaskActionCode"/>
        <rdfs:comment>Serve as the first operational echelon: To serve as a fraction of a command, to which the first mission is assigned or which forms the forward line of own troops</rdfs:comment>
    </owl:NamedIndividual>
    


    <!-- http://www.sisostds.org/ontologies/lox#SERFRE -->

    <owl:NamedIndividual rdf:about="http://www.sisostds.org/ontologies/lox#SERFRE">
        <rdf:type rdf:resource="http://www.sisostds.org/ontologies/C2SIM#TaskActionCode"/>
        <rdfs:comment>Serve as the forward echelon: To serve as a forward subdivision of a headquarters.</rdfs:comment>
    </owl:NamedIndividual>
    


    <!-- http://www.sisostds.org/ontologies/lox#SERFTE -->

    <owl:NamedIndividual rdf:about="http://www.sisostds.org/ontologies/lox#SERFTE">
        <rdf:type rdf:resource="http://www.sisostds.org/ontologies/C2SIM#TaskActionCode"/>
        <rdfs:comment>Serve as the first tactical echelon: To serve as a fraction of a tactical command, to which a primary mission is assigned.</rdfs:comment>
    </owl:NamedIndividual>
    


    <!-- http://www.sisostds.org/ontologies/lox#SERFUE -->

    <owl:NamedIndividual rdf:about="http://www.sisostds.org/ontologies/lox#SERFUE">
        <rdf:type rdf:resource="http://www.sisostds.org/ontologies/C2SIM#TaskActionCode"/>
        <rdfs:comment>Serve as the follow-up echelon: To serve as, in air transport operations, an element moved into the objective area after the assault echelon.</rdfs:comment>
    </owl:NamedIndividual>
    


    <!-- http://www.sisostds.org/ontologies/lox#SERREE -->

    <owl:NamedIndividual rdf:about="http://www.sisostds.org/ontologies/lox#SERREE">
        <rdf:type rdf:resource="http://www.sisostds.org/ontologies/C2SIM#TaskActionCode"/>
        <rdfs:comment>Serve as the rear echelon: To serve as elements of a force which are not required in the objective area.</rdfs:comment>
    </owl:NamedIndividual>
    


    <!-- http://www.sisostds.org/ontologies/lox#SERRSE -->

    <owl:NamedIndividual rdf:about="http://www.sisostds.org/ontologies/lox#SERRSE">
        <rdf:type rdf:resource="http://www.sisostds.org/ontologies/C2SIM#TaskActionCode"/>
        <rdfs:comment>Serve as the reserve echelon: To serve as a fraction of a command in the direction of depth, which is an assigned reserve.</rdfs:comment>
    </owl:NamedIndividual>
    


    <!-- http://www.sisostds.org/ontologies/lox#SERSEA -->

    <owl:NamedIndividual rdf:about="http://www.sisostds.org/ontologies/lox#SERSEA">
        <rdf:type rdf:resource="http://www.sisostds.org/ontologies/C2SIM#TaskActionCode"/>
        <rdfs:comment>Serve as the sea echelon: To serve as a portion of the assault shipping which withdraws from, or remains out of, the transport area during an amphibious</rdfs:comment>
    </owl:NamedIndividual>
    


    <!-- http://www.sisostds.org/ontologies/lox#SERSOE -->

    <owl:NamedIndividual rdf:about="http://www.sisostds.org/ontologies/lox#SERSOE">
        <rdf:type rdf:resource="http://www.sisostds.org/ontologies/C2SIM#TaskActionCode"/>
        <rdfs:comment>Serve as the second operational echelon: To serve as a fraction of an operational command either in the direction of depth or as a follow up on the timeline, to which</rdfs:comment>
    </owl:NamedIndividual>
    


    <!-- http://www.sisostds.org/ontologies/lox#SERSPE -->

    <owl:NamedIndividual rdf:about="http://www.sisostds.org/ontologies/lox#SERSPE">
        <rdf:type rdf:resource="http://www.sisostds.org/ontologies/C2SIM#TaskActionCode"/>
        <rdfs:comment>Serve as a support echelon: To serve as a fraction of a command in the direction of depth, to which a support mission is assigned.</rdfs:comment>
    </owl:NamedIndividual>
    


    <!-- http://www.sisostds.org/ontologies/lox#SERSTE -->

    <owl:NamedIndividual rdf:about="http://www.sisostds.org/ontologies/lox#SERSTE">
        <rdf:type rdf:resource="http://www.sisostds.org/ontologies/C2SIM#TaskActionCode"/>
        <rdfs:comment>Serve as the second tactical echelon: To serve as a fraction of a tactical command either in the direction of depth or as a follow up on the timeline, to which</rdfs:comment>
    </owl:NamedIndividual>
    


    <!-- http://www.sisostds.org/ontologies/lox#SERSTR -->

    <owl:NamedIndividual rdf:about="http://www.sisostds.org/ontologies/lox#SERSTR">
        <rdf:type rdf:resource="http://www.sisostds.org/ontologies/C2SIM#TaskActionCode"/>
        <rdfs:comment>Serve as a strategic reserve: To serve as a fraction of a command in the direction of depth, which is an assigned strategic reserve.</rdfs:comment>
    </owl:NamedIndividual>
    


    <!-- http://www.sisostds.org/ontologies/lox#SERTHR -->

    <owl:NamedIndividual rdf:about="http://www.sisostds.org/ontologies/lox#SERTHR">
        <rdf:type rdf:resource="http://www.sisostds.org/ontologies/C2SIM#TaskActionCode"/>
        <rdfs:comment>Serve as the theatre reserve: To serve as a fraction of a command in the direction of depth, which is an assigned theatre reserve.</rdfs:comment>
    </owl:NamedIndividual>
    


    <!-- http://www.sisostds.org/ontologies/lox#SETUP -->

    <owl:NamedIndividual rdf:about="http://www.sisostds.org/ontologies/lox#SETUP">
        <rdf:type rdf:resource="http://www.sisostds.org/ontologies/C2SIM#TaskActionCode"/>
        <rdfs:comment>Set up: To prepare or establish a FACILITY, ORGANISATION or FEATURE.</rdfs:comment>
    </owl:NamedIndividual>
    


    <!-- http://www.sisostds.org/ontologies/lox#SINGA -->

    <owl:NamedIndividual rdf:about="http://www.sisostds.org/ontologies/lox#SINGA">
        <rdf:type rdf:resource="http://www.sisostds.org/ontologies/C2SIM#TaskActionCode"/>
        <rdfs:comment>Signals intelligence gathering: To intercept and gather electronic and communications transmissions for intelligence purposes.</rdfs:comment>
    </owl:NamedIndividual>
    


    <!-- http://www.sisostds.org/ontologies/lox#SPCOPS -->

    <owl:NamedIndividual rdf:about="http://www.sisostds.org/ontologies/lox#SPCOPS">
        <rdf:type rdf:resource="http://www.sisostds.org/ontologies/C2SIM#TaskActionCode"/>
        <rdfs:comment>Special operations: A mission conducted by specially designated, organised, trained and equipped forces using operational techniques and modes</rdfs:comment>
    </owl:NamedIndividual>
    


    <!-- http://www.sisostds.org/ontologies/lox#SPREAD -->

    <owl:NamedIndividual rdf:about="http://www.sisostds.org/ontologies/lox#SPREAD">
        <rdf:type rdf:resource="http://www.sisostds.org/ontologies/C2SIM#TaskActionCode"/>
        <rdfs:comment>Spread: No definition provided in ADatP-3 Baseline 13.1 FFIRN/FUD 1299/19.</rdfs:comment>
    </owl:NamedIndividual>
    


    <!-- http://www.sisostds.org/ontologies/lox#SPTCON -->

    <owl:NamedIndividual rdf:about="http://www.sisostds.org/ontologies/lox#SPTCON">
        <rdf:type rdf:resource="http://www.sisostds.org/ontologies/C2SIM#TaskActionCode"/>
        <rdfs:comment>Support, contingency: To involve in emergency, military forces due to natural disasters, terrorists, subversives, or by required military operations.</rdfs:comment>
    </owl:NamedIndividual>
    


    <!-- http://www.sisostds.org/ontologies/lox#SPTELC -->

    <owl:NamedIndividual rdf:about="http://www.sisostds.org/ontologies/lox#SPTELC">
        <rdf:type rdf:resource="http://www.sisostds.org/ontologies/C2SIM#TaskActionCode"/>
        <rdfs:comment>Support, electronic: To provide information required for decisions involving electronic warfare operations and other tactical actions such as threat</rdfs:comment>
    </owl:NamedIndividual>
    


    <!-- http://www.sisostds.org/ontologies/lox#SRCHFR -->

    <owl:NamedIndividual rdf:about="http://www.sisostds.org/ontologies/lox#SRCHFR">
        <rdf:type rdf:resource="http://www.sisostds.org/ontologies/C2SIM#TaskActionCode"/>
        <rdfs:comment>Search by fire: To distribute fire in depth by successive changes in the elevation of the gun.</rdfs:comment>
    </owl:NamedIndividual>
    


    <!-- http://www.sisostds.org/ontologies/lox#SRCRES -->

    <owl:NamedIndividual rdf:about="http://www.sisostds.org/ontologies/lox#SRCRES">
        <rdf:type rdf:resource="http://www.sisostds.org/ontologies/C2SIM#TaskActionCode"/>
        <rdfs:comment>Search and rescue, combat: To detect, locate, identify and rescue downed aircrew in hostile territory in crisis and wartime and, when appropriate, isolated</rdfs:comment>
    </owl:NamedIndividual>
    


    <!-- http://www.sisostds.org/ontologies/lox#STRCON -->

    <owl:NamedIndividual rdf:about="http://www.sisostds.org/ontologies/lox#STRCON">
        <rdf:type rdf:resource="http://www.sisostds.org/ontologies/C2SIM#TaskActionCode"/>
        <rdfs:comment>Strike control and reconnaissance: To conduct reconnaissance strike control and reconnaissance operations.</rdfs:comment>
    </owl:NamedIndividual>
    


    <!-- http://www.sisostds.org/ontologies/lox#STRWAF -->

    <owl:NamedIndividual rdf:about="http://www.sisostds.org/ontologies/lox#STRWAF">
        <rdf:type rdf:resource="http://www.sisostds.org/ontologies/C2SIM#TaskActionCode"/>
        <rdfs:comment>Strike warfare: To conduct warfare that includes strikes against targets ashore using carrier-based strike aircraft, sea-launched cruise missiles,</rdfs:comment>
    </owl:NamedIndividual>
    


    <!-- http://www.sisostds.org/ontologies/lox#SUBWAF -->

    <owl:NamedIndividual rdf:about="http://www.sisostds.org/ontologies/lox#SUBWAF">
        <rdf:type rdf:resource="http://www.sisostds.org/ontologies/C2SIM#TaskActionCode"/>
        <rdfs:comment>Submarine warfare: To conduct warfare that includes the use of submarines.</rdfs:comment>
    </owl:NamedIndividual>
    


    <!-- http://www.sisostds.org/ontologies/lox#SUPPRS -->

    <owl:NamedIndividual rdf:about="http://www.sisostds.org/ontologies/lox#SUPPRS">
        <rdf:type rdf:resource="http://www.sisostds.org/ontologies/C2SIM#TaskActionCode"/>
        <rdfs:comment>Documentation: 		
						To provide fire which neutralizes or temporarily degrades the capabilities of enemy forces within a specific area. This makes no assumptions as to enemy casualties; it may be a transitory effect.	
					; Appinfo DisplayValue as &quot;Suppress&quot;</rdfs:comment>
        <rdfs:comment>Suppress: To provide fire which neutralizes or temporarily degrades the capabilities of enemy forces within a specific area. This makes</rdfs:comment>
    </owl:NamedIndividual>
    


    <!-- http://www.sisostds.org/ontologies/lox#SUPPRT -->

    <owl:NamedIndividual rdf:about="http://www.sisostds.org/ontologies/lox#SUPPRT">
        <rdf:type rdf:resource="http://www.sisostds.org/ontologies/C2SIM#TaskActionCode"/>
        <rdfs:comment>Documentation: 		
						To aid, protect, complement or sustain any other object.	
					; Appinfo DisplayValue as &quot;Support&quot;</rdfs:comment>
        <rdfs:comment>Support: To aid, protect, complement or sustain any other object.</rdfs:comment>
    </owl:NamedIndividual>
    


    <!-- http://www.sisostds.org/ontologies/lox#SUPRSD -->

    <owl:NamedIndividual rdf:about="http://www.sisostds.org/ontologies/lox#SUPRSD">
        <rdfs:comment>Documentation: 		
						Reduction of the effectiveness of the ACTION objective for a specific period or purpose (normally to prevent an enemy from interfering with friendly ACTIONs); this effect may be entirely transitory and cause no casualties.	
					; Appinfo DisplayValue as &quot;Suppressed&quot;</rdfs:comment>
    </owl:NamedIndividual>
    


    <!-- http://www.sisostds.org/ontologies/lox#SURVEL -->

    <owl:NamedIndividual rdf:about="http://www.sisostds.org/ontologies/lox#SURVEL">
        <rdf:type rdf:resource="http://www.sisostds.org/ontologies/C2SIM#TaskActionCode"/>
        <rdfs:comment>Surveillance, electronic: The systematic observation of aerospace, surface or subsurface areas, places, persons, or things, by electronic means.</rdfs:comment>
    </owl:NamedIndividual>
    


    <!-- http://www.sisostds.org/ontologies/lox#SURVLE -->

    <owl:NamedIndividual rdf:about="http://www.sisostds.org/ontologies/lox#SURVLE">
        <rdf:type rdf:resource="http://www.sisostds.org/ontologies/C2SIM#TaskActionCode"/>
        <rdfs:comment>Surveillance: To observe aerospace, surface or subsurface areas, places, persons, or things, by visual, aural electronic, photographic,</rdfs:comment>
    </owl:NamedIndividual>
    


    <!-- http://www.sisostds.org/ontologies/lox#SUSOAA -->

    <owl:NamedIndividual rdf:about="http://www.sisostds.org/ontologies/lox#SUSOAA">
        <rdf:type rdf:resource="http://www.sisostds.org/ontologies/C2SIM#TaskActionCode"/>
        <rdfs:comment>Sustaining operations afloat and ashore: To conduct an operation in which maritime forces continue to provide direct and indirect support to combat operations ashore,</rdfs:comment>
    </owl:NamedIndividual>
    


    <!-- http://www.sisostds.org/ontologies/lox#SWEEP -->

    <owl:NamedIndividual rdf:about="http://www.sisostds.org/ontologies/lox#SWEEP">
        <rdf:type rdf:resource="http://www.sisostds.org/ontologies/C2SIM#TaskActionCode"/>
        <rdfs:comment>Sweep: An offensive mission by fighter aircraft to seek out and destroy enemy aircraft and other targets of opportunity in an allocated</rdfs:comment>
    </owl:NamedIndividual>
    


    <!-- http://www.sisostds.org/ontologies/lox#TCARRC -->

    <owl:NamedIndividual rdf:about="http://www.sisostds.org/ontologies/lox#TCARRC">
        <rdf:type rdf:resource="http://www.sisostds.org/ontologies/C2SIM#TaskActionCode"/>
        <rdfs:comment>Tactical air reconnaissance: Air action, which consist of the collection of information of intelligence from the air or through the use of airborne sensors.</rdfs:comment>
    </owl:NamedIndividual>
    


    <!-- http://www.sisostds.org/ontologies/lox#TGTDLT -->

    <owl:NamedIndividual rdf:about="http://www.sisostds.org/ontologies/lox#TGTDLT">
        <rdf:type rdf:resource="http://www.sisostds.org/ontologies/C2SIM#TaskActionCode"/>
        <rdfs:comment>Target dilution: To minimize the probability of acquisition of real targets by creating false targets in the vicinity of real targets by means</rdfs:comment>
    </owl:NamedIndividual>
    


    <!-- http://www.sisostds.org/ontologies/lox#THREAT -->

    <owl:NamedIndividual rdf:about="http://www.sisostds.org/ontologies/lox#THREAT">
        <rdf:type rdf:resource="http://www.sisostds.org/ontologies/C2SIM#TaskActionCode"/>
        <rdfs:comment>Documentation: 		
						To menace the enemy by manoeuvre or action.	
					; Appinfo DisplayValue as &quot;Threaten&quot;</rdfs:comment>
        <rdfs:comment>Threaten: To menace the enemy by manoeuvre or action.</rdfs:comment>
    </owl:NamedIndividual>
    


    <!-- http://www.sisostds.org/ontologies/lox#TOWTGT -->

    <owl:NamedIndividual rdf:about="http://www.sisostds.org/ontologies/lox#TOWTGT">
        <rdf:type rdf:resource="http://www.sisostds.org/ontologies/C2SIM#TaskActionCode"/>
        <rdfs:comment>Tow, target: To tow a target used for gunnery practice.</rdfs:comment>
    </owl:NamedIndividual>
    


    <!-- http://www.sisostds.org/ontologies/lox#TPL -->

    <owl:NamedIndividual rdf:about="http://www.sisostds.org/ontologies/lox#TPL">
        <rdf:type rdf:resource="http://www.sisostds.org/ontologies/lox#TaskFunctionalAssociationCode"/>
        <rdfs:comment>Is a template for: The subject ACTION constitutes an example that the object ACTION should conform to.</rdfs:comment>
    </owl:NamedIndividual>
    


    <!-- http://www.sisostds.org/ontologies/lox#TRAIN -->

    <owl:NamedIndividual rdf:about="http://www.sisostds.org/ontologies/lox#TRAIN">
        <rdf:type rdf:resource="http://www.sisostds.org/ontologies/C2SIM#TaskActionCode"/>
        <rdfs:comment>Train: To develop, maintain or improve the readiness of individuals or units.</rdfs:comment>
    </owl:NamedIndividual>
    


    <!-- http://www.sisostds.org/ontologies/lox#TRANOP -->

    <owl:NamedIndividual rdf:about="http://www.sisostds.org/ontologies/lox#TRANOP">
        <rdf:type rdf:resource="http://www.sisostds.org/ontologies/C2SIM#TaskActionCode"/>
        <rdfs:comment>Train, operations: Training operations or exercises. This training includes: a. delivery of personnel and equipment; b. Assault operations; c.</rdfs:comment>
    </owl:NamedIndividual>
    


    <!-- http://www.sisostds.org/ontologies/lox#TRANS -->

    <owl:NamedIndividual rdf:about="http://www.sisostds.org/ontologies/lox#TRANS">
        <rdf:type rdf:resource="http://www.sisostds.org/ontologies/C2SIM#TaskActionCode"/>
        <rdfs:comment>Transport: To move assets using any means by sea, land or air to a specified objective.</rdfs:comment>
    </owl:NamedIndividual>
    


    <!-- http://www.sisostds.org/ontologies/lox#TRNSAA -->

    <owl:NamedIndividual rdf:about="http://www.sisostds.org/ontologies/lox#TRNSAA">
        <rdf:type rdf:resource="http://www.sisostds.org/ontologies/C2SIM#TaskActionCode"/>
        <rdfs:comment>Transport, assault airland: To transport cargo and/or passengers delivered by air-landing the aircraft to a combat zone.</rdfs:comment>
    </owl:NamedIndividual>
    


    <!-- http://www.sisostds.org/ontologies/lox#TRVRS -->

    <owl:NamedIndividual rdf:about="http://www.sisostds.org/ontologies/lox#TRVRS">
        <rdf:type rdf:resource="http://www.sisostds.org/ontologies/C2SIM#TaskActionCode"/>
        <rdfs:comment>Traverse: To travel over a designated route.</rdfs:comment>
    </owl:NamedIndividual>
    


    <!-- http://www.sisostds.org/ontologies/lox#TURN -->

    <owl:NamedIndividual rdf:about="http://www.sisostds.org/ontologies/lox#TURN">
        <rdf:type rdf:resource="http://www.sisostds.org/ontologies/C2SIM#TaskActionCode"/>
        <rdfs:comment>Documentation: 		
						To compel an enemy force to move from an avenue of approach or movement corridor to another.	
					; Appinfo DisplayValue as &quot;Turn&quot;</rdfs:comment>
        <rdfs:comment>Turn: To compel an enemy force to move from an avenue of approach or movement corridor to another.</rdfs:comment>
    </owl:NamedIndividual>
    


    <!-- http://www.sisostds.org/ontologies/lox#UAR -->

    <owl:NamedIndividual rdf:about="http://www.sisostds.org/ontologies/lox#UAR">
        <rdf:type rdf:resource="http://www.sisostds.org/ontologies/lox#TaskFunctionalAssociationCode"/>
        <rdfs:comment>Uses as a reference: The value that establishes a link between existing ACTIONs and new ACTIONs, be they requests, plans, or orders. (Note: The</rdfs:comment>
    </owl:NamedIndividual>
    


    <!-- http://www.sisostds.org/ontologies/lox#UNCONW -->

    <owl:NamedIndividual rdf:about="http://www.sisostds.org/ontologies/lox#UNCONW">
        <rdf:type rdf:resource="http://www.sisostds.org/ontologies/C2SIM#TaskActionCode"/>
        <rdfs:comment>Unconventional warfare: To conduct operations for military, political or economic purposes within an area occupied by the enemy and making use of</rdfs:comment>
    </owl:NamedIndividual>
    


    <!-- http://www.sisostds.org/ontologies/lox#UTILTY -->

    <owl:NamedIndividual rdf:about="http://www.sisostds.org/ontologies/lox#UTILTY">
        <rdf:type rdf:resource="http://www.sisostds.org/ontologies/C2SIM#TaskActionCode"/>
        <rdfs:comment>Utility flight: To conduct a flight in which the aircraft has the capability of performing multiple missions.</rdfs:comment>
    </owl:NamedIndividual>
    


    <!-- http://www.sisostds.org/ontologies/lox#VERIFY -->

    <owl:NamedIndividual rdf:about="http://www.sisostds.org/ontologies/lox#VERIFY">
        <rdf:type rdf:resource="http://www.sisostds.org/ontologies/C2SIM#TaskActionCode"/>
        <rdfs:comment>Verify: To testify to, to assert, to affirm or confirm, as true or certain.</rdfs:comment>
    </owl:NamedIndividual>
    


    <!-- http://www.sisostds.org/ontologies/lox#WDRPRS -->

    <owl:NamedIndividual rdf:about="http://www.sisostds.org/ontologies/lox#WDRPRS">
        <rdf:type rdf:resource="http://www.sisostds.org/ontologies/C2SIM#TaskActionCode"/>
        <rdfs:comment>Withdraw under pressure: To disengage from the enemy when the enemy has sufficient contact with friendly forces to interfere with the withdrawal.</rdfs:comment>
    </owl:NamedIndividual>
    


    <!-- http://www.sisostds.org/ontologies/lox#WITHDR -->

    <owl:NamedIndividual rdf:about="http://www.sisostds.org/ontologies/lox#WITHDR">
        <rdf:type rdf:resource="http://www.sisostds.org/ontologies/C2SIM#TaskActionCode"/>
        <rdfs:comment>Withdraw: To disengage a force in contact from an enemy force.</rdfs:comment>
    </owl:NamedIndividual>
    


    <!-- http://www.sisostds.org/ontologies/lox#WITNES -->

    <owl:NamedIndividual rdf:about="http://www.sisostds.org/ontologies/lox#WITNES">
        <rdf:type rdf:resource="http://www.sisostds.org/ontologies/C2SIM#TaskActionCode"/>
        <rdfs:comment>Witness: To observe an activity in an official capacity with a view of providing evidence.</rdfs:comment>
    </owl:NamedIndividual>
    


    <!-- http://www.sisostds.org/ontologies/lox#WLDWSL -->

    <owl:NamedIndividual rdf:about="http://www.sisostds.org/ontologies/lox#WLDWSL">
        <rdf:type rdf:resource="http://www.sisostds.org/ontologies/C2SIM#TaskActionCode"/>
        <rdfs:comment>Wild weasel: To identify, locate, and physically suppress or destroy ground based enemy air defence systems that employ sensors radiating</rdfs:comment>
    </owl:NamedIndividual>
    


    <!-- http://www.sisostds.org/ontologies/lox#WNDD -->

    <owl:NamedIndividual rdf:about="http://www.sisostds.org/ontologies/lox#WNDD">
        <rdfs:comment>Documentation: 		
						A casualty other than &quot;killed&quot; who has incurred an injury due to an external agent or cause.	
					; Appinfo DisplayValue as &quot;Wounded&quot;</rdfs:comment>
    </owl:NamedIndividual>
    <rdf:Description>
        <owl:minQualifiedCardinality rdf:datatype="http://www.w3.org/2001/XMLSchema#nonNegativeInteger">0</owl:minQualifiedCardinality>
    </rdf:Description>
    <rdf:Description>
        <owl:qualifiedCardinality rdf:datatype="http://www.w3.org/2001/XMLSchema#nonNegativeInteger">1</owl:qualifiedCardinality>
    </rdf:Description>
    <rdf:Description>
        <owl:qualifiedCardinality rdf:datatype="http://www.w3.org/2001/XMLSchema#nonNegativeInteger">1</owl:qualifiedCardinality>
    </rdf:Description>
    <rdf:Description>
        <owl:minQualifiedCardinality rdf:datatype="http://www.w3.org/2001/XMLSchema#nonNegativeInteger">0</owl:minQualifiedCardinality>
    </rdf:Description>
    <rdf:Description>
        <owl:minQualifiedCardinality rdf:datatype="http://www.w3.org/2001/XMLSchema#nonNegativeInteger">0</owl:minQualifiedCardinality>
    </rdf:Description>
    <rdf:Description>
        <owl:qualifiedCardinality rdf:datatype="http://www.w3.org/2001/XMLSchema#nonNegativeInteger">1</owl:qualifiedCardinality>
    </rdf:Description>
    <rdf:Description>
        <owl:qualifiedCardinality rdf:datatype="http://www.w3.org/2001/XMLSchema#nonNegativeInteger">1</owl:qualifiedCardinality>
    </rdf:Description>
    <rdf:Description>
        <owl:qualifiedCardinality rdf:datatype="http://www.w3.org/2001/XMLSchema#nonNegativeInteger">1</owl:qualifiedCardinality>
    </rdf:Description>
    <rdf:Description>
        <owl:qualifiedCardinality rdf:datatype="http://www.w3.org/2001/XMLSchema#nonNegativeInteger">1</owl:qualifiedCardinality>
    </rdf:Description>
</rdf:RDF>



<!-- Generated by the OWL API (version 4.5.9.2019-02-01T07:24:44Z) https://github.com/owlcs/owlapi -->

