<?xml version="1.0"?>
<rdf:RDF xmlns="http://www.sisostds.org/ontologies/C2SIM_SMX_LOX#"
     xml:base="http://www.sisostds.org/ontologies/C2SIM_SMX_LOX"
     xmlns:owl="http://www.w3.org/2002/07/owl#"
     xmlns:rdf="http://www.w3.org/1999/02/22-rdf-syntax-ns#"
     xmlns:xml="http://www.w3.org/XML/1998/namespace"
     xmlns:xsd="http://www.w3.org/2001/XMLSchema#"
     xmlns:rdfs="http://www.w3.org/2000/01/rdf-schema#">
    <owl:Ontology rdf:about="http://www.sisostds.org/ontologies/C2SIM_SMX_LOX">
        <rdfs:comment>C2SIM Standard Military Extension ontology.
v 1.0 First draft, matching v.9.3 of the Core ontology. Release Dec-18.

v 1.1 Imports Core v9.5

v 1.2 Must import Core v9.6; Replaced all occurrences of http://www.c2sim.com/mwx with http://www.sisostds.org/ontologies/smx; changed all subproperties of hasCode to reference the C2SIM namespace for the parent property; gave hasAPP6-SIDC a range of APP6-SIDC; gave hasObservation a range of Observation;  gave hasReinforcedReducedType a range of ReinforcedReducedType; renamed the Task subclass of MapGraphic to TaskGraphic; gave hasDISKindCode a range of DISKindCode; added datatype property axioms (hasX, hasY, hasZ each with exactly 1 xsd:double) to GeocentricCoordinateValue class; gave respective class ranges to object properties hasAircraftTypeCategoryCode, hasAmmunitionTypeCategoryCode, hasDISCountryCode, hasDISDomainCode, hasDISKindCode, hasEchelonCode, hasPersonTypeCategoryCode, hasSideHostilityCode, hasSubsurfaceVesselTypeCode, hasSurfaceVesselTypeCode, hasVehicleTypeCategoryCode, hasWeaponCategoryCode (also changed this property name to hasWeaponTypeCategoryCode); gave hasSupportingTaskCode a range of TaskNameCode; gave datatype property hasDISCodeType a range of xsd:string

v 1.3 Imports Core v9.7. Added the hasX, Y, Z properties to GeocentricCoordinate.
v 1.4 Imports Core v9.8. Remove hasDesiredEffectCode (duplicate of Core). Give hasDISKindCode a range restriction. Removed some unused individual definitions
v 1.5 Imports Core v9.9.
v 1.6 Imports Core v 9.11. Replaced SideHostilityCode individuals with FR, HO, NEUTRL to correspond with JC3IEDM.

v 1.7 Added &quot;hasLocation exactly 1 Coordinate&quot; propterty axiom to LocationObservation class</rdfs:comment>
        <rdfs:comment>This version of the LDM ontology is a result of the review process of Nov-Dec 2017 by Doug Reece, Samuel Singapogu, Magdalena Wolski, and Xavier Cuneo. 
After a number of discussions and review of the v.5 ontology by the group, Reece made significant edits to the ontology to reorganize it, producing v 6.4.
Reece made additional edits to change classes that were really &quot;attributes&quot; to data properties-- v 6.5.
v 6.6 -- additional tweaks; presented 25-Jan-2018 at the SIW PDG meeting.
v 6.7 -- cleanup by C. Blais: property name capitalization consistency, URLs
v 6.8 -- Reece small fixes based on discussion at SIW PDG.
v 6.9 -- Modified to incorporate comments received on 6.8, plus proposed improvements from 5/17 ontology group meeting
v 6.10-- Modified to align with CBML concepts in MWX better. Several data properties were converted to object properties, and enumerations turned into instances of classes, for better flexibility.
v 6.11-- Modified in partial response to comments from ontology group 5-7 June

v5 -- Released to PDG on about Jun 22, 2018
v5.1 Reece modifications based on ontology meeting Jul 5
v 5.2 Reece modifications based on ontology meeting Jul 20
v6, 6.1, 6.2 -- Modifications in Aug 2018 prior to SIW
v 7 SIW Fall 2018 release, Sept 2018
v 7.1 Changes to include perception, plans, more specific message info. Removed Peer.
v 7.2 Removed plans &amp; perceptions. 
v 7.3 Removed DIS type, Abstract State, Alias, LifeIntervalTime, PlannedState, has...Individuals, Actions and Entities from Scenario State, Geocentric Coordinates. Added Geodetic Coordinates, moved Equipment and Material under Resources under C2SIMConcept, made ResourceStatus refer to Resource. Changed InitializationConcept to ManagementConcept and added initial support for Management and Initialization messages there.  Change all Entity and Action class references in Object Properties to UUID references, EXCEPT in the initialization messages.
v 7.4 Start time cardinality in Action is changed to Max 1 (but Event retains Exactly 1). Order message has Task instead of UUID (for Task). Added ReportContent to the MessageConcepts moved the properties of ReportBody to it; ReportBody then has 1 or more ReportContent objects in it. Changed Message to BattleManagementMessage and ManagementMessage to SystemManagementMessage, and put them both under a new class Message. Removed PositionAltitudeCode; replace Altitude in GeodeticCoordinate with optional AltitudeAGL and AltitudeMSL.  5-Nov-2018

v 8. Release to PDG
v 8.1 BattleManagementMessage -&gt; DomainMessage. Added optional properties for AbstractObjects, Actions, and Entities in the ScenarioInitializationMessage. Removed unused class instances. Removed hasSide and hasAffiliation object properties (duplicate with those data properties).

provisional v9 -- for review prior to release
-&gt; Added datatype for percentage (nonNegative integer less than or equal to 100); added Range restrictions on data properties and object properties to aid in more precise schema generation; added classes and subclasses to make DomainMessage and SystemManagementMessage structures comparable; moved subclasses that were under DomainMessage to be subclasses under DomainMessageBody; added a SystemStateCode class with named individuals to generate an enumerated type in the schema; removed hasConstituentPart property and replaced with object properties having the precise ranges needed (e.g., DomainMessage hasDomainMessageHeader and hasDomainMessageBody); changed ScenarioInitializationMessage hasScenarioState property axiom to have exactly 1 ScenarioSetting; defined StrengthPercentage class as hasStrengthPercentage exactly 1 percentage; appended &quot;Base&quot; to datatypes IsoDateTime, IsoTimeDuration, and UUID to prevent duplicate type declarations in the generated schema when removing &quot;has&quot; from data properties; changed class names for CoordinateValue to Coordinate, GeodeticCoordinateValue to GeodeticCoordinate, Side to ForceSide, and StrengthPercentage to Strength to avoid duplicate type declarations in generated schema; renamed data property hasMapGraphic to hasMapGraphicID (also in annotation description of Task class)

provisional v9.1
-&gt; Added range restriction on object property hasSystemManagementMessageBody;  added generic named individuals (place-holders) for CountryCode, EthnicGroupCode; and ReligiousOrganizationCode; renamed hasAcknowledgeCode to hasAcknowledgeTypeCode (for consistency with other naming); give hasSystemManagementMessageHeader a range of class SystemManagementMessageHeader; set range of hasDateTime, hasEndTime, hasStartTime, and hasTimeOfDuration to class DateTime; give hasOrganizationCode range OrganizationCode class

provisional v9.2
-&gt; Add object property hasTimeInstant with range TimeInstant class; change hasDesiredEffect to hasDesiredEffectCode to match name of range class; change hasTimeReference to hasTimeReferenceCode (same reason); change hasScenarioState to hasScenarioSetting (same reason); changed hasHealth to hasEntityHealthStatus (same reason); changed name of LocationConcept class to Location so that the name of the property hasLocation matches the range class name; change hasTimeProperty to hasTemporalConcept to match name of range class

v9.3-&gt;v9.4
-&gt; Removed object property hasMessagingPropertyType since subproperties were not defined as restrictions on the parent property (retained the subproperties under the top-level property); removed subclasses IntializationCompleteBody, ShareScenarioBody, StartScenarioBody, and SubmitInitializationBody; added class SystemCommandBody under MessageBody with property axiom hasSystemCommandTypeCode exactly 1 SystemCommandTypeCode; added subclass SystemCommandTypeCode to MessageCode; created individuals InitializationComplete, ShareScenario, StartScenario, and SubmitInitialization as members of class SystemCommandTypeCode; added object property hasSystemCommandTypeCode with range SystemCommandTypeCode. 

9.5 Updated to make changes identified in telecon 27-11-2018. See notes in file schemaOntologyIssues_20181214.xlsx.
Added hasEntityDescriptor object property, and added this property to Actor entity.
Added data properties isFriendlyTo, isHostileTo, and isNeutralTo as sub properties of hasAllegiance.
Added Protocol and ProtocolVersion properties to C2SIM header.

9.6 Removed Person and Platform from PhysicalEntity; gave the Person and Platform classes properties hasConsumableMaterial min 0 ConsumableMaterial, hasCurrentState max 1 PhysicalState, and hasMarking max 1 xsd:string; gave hasEntityDescriptor a range of EntityDescriptor; gave hasEventCode a range of EventCode; removed UUID from datatypes; gave hasDesiredEffectCode a range of DesiredEffectCode and added property axiom hasDesiredEffectCode min 0 DesiredEffectCode to class Task

9.7 Removed property hasConsumableMaterial from Person and Platform.  Changed the location reference in RelativeLocation from a Location to an Entity reference.

9.8 Removed some unused definitions of individuals.

9.9 Added hasCode property; collected other has...Code properties under it.

9.10 Action property hasStartTime removed, and added to Task; it is already present in Event (with different cardinality). Changed Action property  hasLocation to be optional. Changed Action property hasUniqueIdentifier to hasUUID.

9.11 Added individuals to TaskNameCode. PositionReportContent now has hasStrength and hasOperationalStatus replacing hasEntityHealthStatus. Add hasName property to Action.

9.12 Gave hasOperationalStatus and hasStrength range restrictions.

9.13 In C2SIMHeader, changed the hasReplyToSystem property axiom from &quot;exactly 1&quot; (mandatory) to &quot;max 1&quot; (optional).</rdfs:comment>
        <rdfs:comment>v 1. First draft, matching v.7 of the Core ontology. Release 14-Sept-18

v 2. Adapted the extension to the changed Core v 8.1. Added initial plan support with PlanPhase and PlanPhaseTrigger. Added more report support with Observation and ObservationReport. Added a few things that were removed from the Core such as DISEntityType and GeocentricCoordinates.

v 2.1 Changed the IRI to www.sisostd.org/ontologies/lox.
Imports Core v.9.3

v 3.0 Moved type, graphics, observation classes and properties to the Standard Military Extension. Imports the SMX instead of the core.

v 3.1 Imports SMX v 1.1.  Added annotation for PlanPhase and ...Trigger that were not copied from 2.1 to 3.0. Added reference to PlanPhases in ObjectDefinitions.

v 3.2 Changed default and base namespaces to http://www.sisostds.org/ontologies/; removed occurrences of &quot;mwx&quot; (hasCode, hasTaskFunctionalAssociationCode); gave hasManeuverWarfareDesiredEffectCode a range of ManeuverWarfareDesiredEffectCode; on class OnOrderTrigger, added property axiom hasTaskReference exactly 1 UUIDBase; on class EventTrigger,  added property axiom hasEventReference exactly 1 UUIDBase; gave hasPlanPhaseCompletionCondition a range of PlanPhaseCompletionCondition; gave hasDISCodeType a range of xsd:string; added property hasPlanPhase with range of PlanPhase; gave hasSubPhase a range of PlanPhase; gave hasManeuverWarfareTaskCode a range of ManeuverWarfareTaskCode; gave hasPlanPhaseID a range of xsd:string; gave hasFunctionalAssociationWithTask and hasTriggerPhase a range of UUIDBase; gave isActive and isComplete a range of xsd:boolean.

v 3.3 Imports SMX v1.3

v 3.4 Imports SMX 1.4. Added hasEventTrigger property. Added a genericManeuverWarfareDesiredEffectCode individual.

v 3.5 Imports SMX v 1.5. Added property hasEvent to EventTrigger class.

v 3.6 Imports SMX v 1.6. Removes subclasses ManeuverWarfareTaskCode and ManeuverWarfareDesiredEffectCode and the related object properties. Added JC3IEDM codes for task names and desired effects as ...Code individuals.</rdfs:comment>
    </owl:Ontology>
    


    <!-- 
    ///////////////////////////////////////////////////////////////////////////////////////
    //
    // Annotation properties
    //
    ///////////////////////////////////////////////////////////////////////////////////////
     -->

    


    <!-- http://www.w3.org/2002/07/owl#minQualifiedCardinality -->

    <owl:AnnotationProperty rdf:about="http://www.w3.org/2002/07/owl#minQualifiedCardinality"/>
    


    <!-- http://www.w3.org/2002/07/owl#qualifiedCardinality -->

    <owl:AnnotationProperty rdf:about="http://www.w3.org/2002/07/owl#qualifiedCardinality"/>
    


    <!-- 
    ///////////////////////////////////////////////////////////////////////////////////////
    //
    // Datatypes
    //
    ///////////////////////////////////////////////////////////////////////////////////////
     -->

    


    <!-- http://www.sisostds.org/ontologies/C2SIM#IsoDateTimeBase -->

    <rdfs:Datatype rdf:about="http://www.sisostds.org/ontologies/C2SIM#IsoDateTimeBase">
        <owl:equivalentClass>
            <rdfs:Datatype>
                <owl:onDatatype rdf:resource="http://www.w3.org/2001/XMLSchema#string"/>
                <owl:withRestrictions rdf:parseType="Collection">
                    <rdf:Description>
                        <xsd:pattern>[0-9]{4}-[0-9]{2}-[0-9]{2}[T]{1}[0-9]{2}:[0-9]{2}:[0-9]{2}:[Z]{1}</xsd:pattern>
                    </rdf:Description>
                </owl:withRestrictions>
            </rdfs:Datatype>
        </owl:equivalentClass>
    </rdfs:Datatype>
    


    <!-- http://www.sisostds.org/ontologies/C2SIM#IsoTimeDurationBase -->

    <rdfs:Datatype rdf:about="http://www.sisostds.org/ontologies/C2SIM#IsoTimeDurationBase">
        <owl:equivalentClass>
            <rdfs:Datatype>
                <owl:onDatatype rdf:resource="http://www.w3.org/2001/XMLSchema#string"/>
                <owl:withRestrictions rdf:parseType="Collection">
                    <rdf:Description>
                        <xsd:pattern>[P]{1}[0-9]{2}[Y]{1}[0-9]{2}[M]{1}[0-9]{2}[D]{1}[0-9]{2}[H]{1}[0-9]{2}[M]{1}[0-9]{2}[S]{1}</xsd:pattern>
                    </rdf:Description>
                </owl:withRestrictions>
            </rdfs:Datatype>
        </owl:equivalentClass>
    </rdfs:Datatype>
    


    <!-- http://www.sisostds.org/ontologies/C2SIM#UUIDBase -->

    <rdfs:Datatype rdf:about="http://www.sisostds.org/ontologies/C2SIM#UUIDBase">
        <owl:equivalentClass>
            <rdfs:Datatype>
                <owl:onDatatype rdf:resource="http://www.w3.org/2001/XMLSchema#string"/>
                <owl:withRestrictions rdf:parseType="Collection">
                    <rdf:Description>
                        <xsd:pattern>[0-9a-z]{8}\-[0-9a-z]{4}\-[0-9a-z]{4}\-[0-9a-z]{4}\-[0-9a-z]{12}</xsd:pattern>
                    </rdf:Description>
                </owl:withRestrictions>
            </rdfs:Datatype>
        </owl:equivalentClass>
    </rdfs:Datatype>
    


    <!-- http://www.sisostds.org/ontologies/C2SIM#angle -->

    <rdfs:Datatype rdf:about="http://www.sisostds.org/ontologies/C2SIM#angle">
        <owl:equivalentClass>
            <rdfs:Datatype>
                <owl:onDatatype rdf:resource="http://www.w3.org/2001/XMLSchema#double"/>
                <owl:withRestrictions rdf:parseType="Collection">
                    <rdf:Description>
                        <xsd:minInclusive rdf:datatype="http://www.w3.org/2001/XMLSchema#double">-180.0</xsd:minInclusive>
                    </rdf:Description>
                    <rdf:Description>
                        <xsd:maxInclusive rdf:datatype="http://www.w3.org/2001/XMLSchema#double">180.0</xsd:maxInclusive>
                    </rdf:Description>
                </owl:withRestrictions>
            </rdfs:Datatype>
        </owl:equivalentClass>
    </rdfs:Datatype>
    


    <!-- http://www.sisostds.org/ontologies/C2SIM#entityTypeString -->

    <rdfs:Datatype rdf:about="http://www.sisostds.org/ontologies/C2SIM#entityTypeString">
        <rdfs:comment>A string, possibly with several separated fields that can each hold an enumeration, thus identifying a category at each level of a hierarchy.</rdfs:comment>
    </rdfs:Datatype>
    


    <!-- http://www.sisostds.org/ontologies/C2SIM#latitude -->

    <rdfs:Datatype rdf:about="http://www.sisostds.org/ontologies/C2SIM#latitude">
        <owl:equivalentClass>
            <rdfs:Datatype>
                <owl:onDatatype rdf:resource="http://www.w3.org/2001/XMLSchema#double"/>
                <owl:withRestrictions rdf:parseType="Collection">
                    <rdf:Description>
                        <xsd:minInclusive rdf:datatype="http://www.w3.org/2001/XMLSchema#double">-90.0</xsd:minInclusive>
                    </rdf:Description>
                    <rdf:Description>
                        <xsd:maxInclusive rdf:datatype="http://www.w3.org/2001/XMLSchema#double">90.0</xsd:maxInclusive>
                    </rdf:Description>
                </owl:withRestrictions>
            </rdfs:Datatype>
        </owl:equivalentClass>
    </rdfs:Datatype>
    


    <!-- http://www.sisostds.org/ontologies/C2SIM#longitude -->

    <rdfs:Datatype rdf:about="http://www.sisostds.org/ontologies/C2SIM#longitude">
        <owl:equivalentClass>
            <rdfs:Datatype>
                <owl:onDatatype rdf:resource="http://www.w3.org/2001/XMLSchema#double"/>
                <owl:withRestrictions rdf:parseType="Collection">
                    <rdf:Description>
                        <xsd:minInclusive rdf:datatype="http://www.w3.org/2001/XMLSchema#double">-180.0</xsd:minInclusive>
                    </rdf:Description>
                    <rdf:Description>
                        <xsd:maxInclusive rdf:datatype="http://www.w3.org/2001/XMLSchema#double">180.0</xsd:maxInclusive>
                    </rdf:Description>
                </owl:withRestrictions>
            </rdfs:Datatype>
        </owl:equivalentClass>
    </rdfs:Datatype>
    


    <!-- http://www.sisostds.org/ontologies/C2SIM#percentage -->

    <rdfs:Datatype rdf:about="http://www.sisostds.org/ontologies/C2SIM#percentage">
        <owl:equivalentClass>
            <rdfs:Datatype>
                <owl:onDatatype rdf:resource="http://www.w3.org/2001/XMLSchema#nonNegativeInteger"/>
                <owl:withRestrictions rdf:parseType="Collection">
                    <rdf:Description>
                        <xsd:maxInclusive rdf:datatype="http://www.w3.org/2001/XMLSchema#nonNegativeInteger">100</xsd:maxInclusive>
                    </rdf:Description>
                </owl:withRestrictions>
            </rdfs:Datatype>
        </owl:equivalentClass>
    </rdfs:Datatype>
    


    <!-- 
    ///////////////////////////////////////////////////////////////////////////////////////
    //
    // Object Properties
    //
    ///////////////////////////////////////////////////////////////////////////////////////
     -->

    


    <!-- http://www.sisostds.org/ontologies/C2SIM#hasAbstractObject -->

    <owl:ObjectProperty rdf:about="http://www.sisostds.org/ontologies/C2SIM#hasAbstractObject">
        <rdfs:range rdf:resource="http://www.sisostds.org/ontologies/C2SIM#AbstractObject"/>
    </owl:ObjectProperty>
    


    <!-- http://www.sisostds.org/ontologies/C2SIM#hasAcknowledgeTypeCode -->

    <owl:ObjectProperty rdf:about="http://www.sisostds.org/ontologies/C2SIM#hasAcknowledgeTypeCode">
        <rdfs:subPropertyOf rdf:resource="http://www.sisostds.org/ontologies/C2SIM#hasCode"/>
        <rdfs:range rdf:resource="http://www.sisostds.org/ontologies/C2SIM#AcknowledgeTypeCode"/>
    </owl:ObjectProperty>
    


    <!-- http://www.sisostds.org/ontologies/C2SIM#hasAction -->

    <owl:ObjectProperty rdf:about="http://www.sisostds.org/ontologies/C2SIM#hasAction">
        <rdfs:range rdf:resource="http://www.sisostds.org/ontologies/C2SIM#Action"/>
        <rdfs:comment>A reference to an Action (an Event or Task).</rdfs:comment>
    </owl:ObjectProperty>
    


    <!-- http://www.sisostds.org/ontologies/C2SIM#hasActionCode -->

    <owl:ObjectProperty rdf:about="http://www.sisostds.org/ontologies/C2SIM#hasActionCode">
        <rdfs:subPropertyOf rdf:resource="http://www.sisostds.org/ontologies/C2SIM#hasCode"/>
        <rdfs:range rdf:resource="http://www.sisostds.org/ontologies/C2SIM#ActionCode"/>
    </owl:ObjectProperty>
    


    <!-- http://www.sisostds.org/ontologies/C2SIM#hasC2SIMHeader -->

    <owl:ObjectProperty rdf:about="http://www.sisostds.org/ontologies/C2SIM#hasC2SIMHeader">
        <rdfs:subPropertyOf rdf:resource="http://www.sisostds.org/ontologies/C2SIM#hasMessageHeader"/>
        <rdfs:range rdf:resource="http://www.sisostds.org/ontologies/C2SIM#C2SIMHeader"/>
    </owl:ObjectProperty>
    


    <!-- http://www.sisostds.org/ontologies/C2SIM#hasCode -->

    <owl:ObjectProperty rdf:about="http://www.sisostds.org/ontologies/C2SIM#hasCode">
        <rdfs:range rdf:resource="http://www.sisostds.org/ontologies/C2SIM#Code"/>
    </owl:ObjectProperty>
    


    <!-- http://www.sisostds.org/ontologies/C2SIM#hasCommunicativeActTypeCode -->

    <owl:ObjectProperty rdf:about="http://www.sisostds.org/ontologies/C2SIM#hasCommunicativeActTypeCode">
        <rdfs:subPropertyOf rdf:resource="http://www.sisostds.org/ontologies/C2SIM#hasCode"/>
        <rdfs:range rdf:resource="http://www.sisostds.org/ontologies/C2SIM#CommunicativeActTypeCode"/>
    </owl:ObjectProperty>
    


    <!-- http://www.sisostds.org/ontologies/C2SIM#hasConsumableMaterial -->

    <owl:ObjectProperty rdf:about="http://www.sisostds.org/ontologies/C2SIM#hasConsumableMaterial">
        <rdfs:range rdf:resource="http://www.sisostds.org/ontologies/C2SIM#ConsumableMaterial"/>
    </owl:ObjectProperty>
    


    <!-- http://www.sisostds.org/ontologies/C2SIM#hasCountryCode -->

    <owl:ObjectProperty rdf:about="http://www.sisostds.org/ontologies/C2SIM#hasCountryCode">
        <rdfs:subPropertyOf rdf:resource="http://www.sisostds.org/ontologies/C2SIM#hasOrganizationCode"/>
        <rdfs:range rdf:resource="http://www.sisostds.org/ontologies/C2SIM#CountryCode"/>
    </owl:ObjectProperty>
    


    <!-- http://www.sisostds.org/ontologies/C2SIM#hasCurrentState -->

    <owl:ObjectProperty rdf:about="http://www.sisostds.org/ontologies/C2SIM#hasCurrentState">
        <rdfs:subPropertyOf rdf:resource="http://www.sisostds.org/ontologies/C2SIM#hasEntityState"/>
    </owl:ObjectProperty>
    


    <!-- http://www.sisostds.org/ontologies/C2SIM#hasDateTime -->

    <owl:ObjectProperty rdf:about="http://www.sisostds.org/ontologies/C2SIM#hasDateTime">
        <rdfs:subPropertyOf rdf:resource="http://www.sisostds.org/ontologies/C2SIM#hasTemporalConcept"/>
        <rdfs:range rdf:resource="http://www.sisostds.org/ontologies/C2SIM#DateTime"/>
    </owl:ObjectProperty>
    


    <!-- http://www.sisostds.org/ontologies/C2SIM#hasDelayTimeAmount -->

    <owl:ObjectProperty rdf:about="http://www.sisostds.org/ontologies/C2SIM#hasDelayTimeAmount">
        <rdfs:subPropertyOf rdf:resource="http://www.sisostds.org/ontologies/C2SIM#hasTemporalConcept"/>
        <rdfs:range rdf:resource="http://www.sisostds.org/ontologies/C2SIM#Duration"/>
    </owl:ObjectProperty>
    


    <!-- http://www.sisostds.org/ontologies/C2SIM#hasDesiredEffectCode -->

    <owl:ObjectProperty rdf:about="http://www.sisostds.org/ontologies/C2SIM#hasDesiredEffectCode">
        <rdfs:subPropertyOf rdf:resource="http://www.sisostds.org/ontologies/C2SIM#hasCode"/>
        <rdfs:range rdf:resource="http://www.sisostds.org/ontologies/C2SIM#DesiredEffectCode"/>
    </owl:ObjectProperty>
    


    <!-- http://www.sisostds.org/ontologies/C2SIM#hasDirectionOfMovement -->

    <owl:ObjectProperty rdf:about="http://www.sisostds.org/ontologies/C2SIM#hasDirectionOfMovement">
        <rdfs:range rdf:resource="http://www.sisostds.org/ontologies/C2SIM#Orientation"/>
    </owl:ObjectProperty>
    


    <!-- http://www.sisostds.org/ontologies/C2SIM#hasDuration -->

    <owl:ObjectProperty rdf:about="http://www.sisostds.org/ontologies/C2SIM#hasDuration">
        <rdfs:subPropertyOf rdf:resource="http://www.sisostds.org/ontologies/C2SIM#hasTemporalConcept"/>
        <rdfs:range rdf:resource="http://www.sisostds.org/ontologies/C2SIM#Duration"/>
    </owl:ObjectProperty>
    


    <!-- http://www.sisostds.org/ontologies/C2SIM#hasEndTime -->

    <owl:ObjectProperty rdf:about="http://www.sisostds.org/ontologies/C2SIM#hasEndTime">
        <rdfs:subPropertyOf rdf:resource="http://www.sisostds.org/ontologies/C2SIM#hasDateTime"/>
        <rdfs:range rdf:resource="http://www.sisostds.org/ontologies/C2SIM#DateTime"/>
        <rdfs:comment>ending date and time with respect to the period of effectiveness of an action/task (C-BML)</rdfs:comment>
    </owl:ObjectProperty>
    


    <!-- http://www.sisostds.org/ontologies/C2SIM#hasEntity -->

    <owl:ObjectProperty rdf:about="http://www.sisostds.org/ontologies/C2SIM#hasEntity">
        <rdfs:range rdf:resource="http://www.sisostds.org/ontologies/C2SIM#Entity"/>
        <rdfs:comment>A generic relation to an instance of an Entity.</rdfs:comment>
    </owl:ObjectProperty>
    


    <!-- http://www.sisostds.org/ontologies/C2SIM#hasEntityDescriptor -->

    <owl:ObjectProperty rdf:about="http://www.sisostds.org/ontologies/C2SIM#hasEntityDescriptor">
        <rdfs:range rdf:resource="http://www.sisostds.org/ontologies/C2SIM#EntityDescriptor"/>
    </owl:ObjectProperty>
    


    <!-- http://www.sisostds.org/ontologies/C2SIM#hasEntityHealthStatus -->

    <owl:ObjectProperty rdf:about="http://www.sisostds.org/ontologies/C2SIM#hasEntityHealthStatus">
        <rdfs:range rdf:resource="http://www.sisostds.org/ontologies/C2SIM#EntityHealthStatus"/>
    </owl:ObjectProperty>
    


    <!-- http://www.sisostds.org/ontologies/C2SIM#hasEntityState -->

    <owl:ObjectProperty rdf:about="http://www.sisostds.org/ontologies/C2SIM#hasEntityState">
        <rdfs:range rdf:resource="http://www.sisostds.org/ontologies/C2SIM#EntityState"/>
    </owl:ObjectProperty>
    


    <!-- http://www.sisostds.org/ontologies/C2SIM#hasEntityType -->

    <owl:ObjectProperty rdf:about="http://www.sisostds.org/ontologies/C2SIM#hasEntityType">
        <rdfs:range rdf:resource="http://www.sisostds.org/ontologies/C2SIM#EntityType"/>
    </owl:ObjectProperty>
    


    <!-- http://www.sisostds.org/ontologies/C2SIM#hasEnvironmentalState -->

    <owl:ObjectProperty rdf:about="http://www.sisostds.org/ontologies/C2SIM#hasEnvironmentalState"/>
    


    <!-- http://www.sisostds.org/ontologies/C2SIM#hasEthnicGroupCode -->

    <owl:ObjectProperty rdf:about="http://www.sisostds.org/ontologies/C2SIM#hasEthnicGroupCode">
        <rdfs:subPropertyOf rdf:resource="http://www.sisostds.org/ontologies/C2SIM#hasOrganizationCode"/>
        <rdfs:range rdf:resource="http://www.sisostds.org/ontologies/C2SIM#EthnicGroupCode"/>
    </owl:ObjectProperty>
    


    <!-- http://www.sisostds.org/ontologies/C2SIM#hasEventCode -->

    <owl:ObjectProperty rdf:about="http://www.sisostds.org/ontologies/C2SIM#hasEventCode">
        <rdfs:subPropertyOf rdf:resource="http://www.sisostds.org/ontologies/C2SIM#hasActionCode"/>
        <rdfs:range rdf:resource="http://www.sisostds.org/ontologies/C2SIM#EventCode"/>
    </owl:ObjectProperty>
    


    <!-- http://www.sisostds.org/ontologies/C2SIM#hasInitializationDataFile -->

    <owl:ObjectProperty rdf:about="http://www.sisostds.org/ontologies/C2SIM#hasInitializationDataFile">
        <rdfs:range rdf:resource="http://www.sisostds.org/ontologies/C2SIM#InitializationDataFile"/>
    </owl:ObjectProperty>
    


    <!-- http://www.sisostds.org/ontologies/C2SIM#hasIssuedTime -->

    <owl:ObjectProperty rdf:about="http://www.sisostds.org/ontologies/C2SIM#hasIssuedTime">
        <rdfs:range rdf:resource="http://www.sisostds.org/ontologies/C2SIM#TimeInstant"/>
    </owl:ObjectProperty>
    


    <!-- http://www.sisostds.org/ontologies/C2SIM#hasLocation -->

    <owl:ObjectProperty rdf:about="http://www.sisostds.org/ontologies/C2SIM#hasLocation">
        <rdfs:range rdf:resource="http://www.sisostds.org/ontologies/C2SIM#Location"/>
    </owl:ObjectProperty>
    


    <!-- http://www.sisostds.org/ontologies/C2SIM#hasMessageBody -->

    <owl:ObjectProperty rdf:about="http://www.sisostds.org/ontologies/C2SIM#hasMessageBody">
        <rdfs:range rdf:resource="http://www.sisostds.org/ontologies/C2SIM#MessageBody"/>
    </owl:ObjectProperty>
    


    <!-- http://www.sisostds.org/ontologies/C2SIM#hasMessageHeader -->

    <owl:ObjectProperty rdf:about="http://www.sisostds.org/ontologies/C2SIM#hasMessageHeader"/>
    


    <!-- http://www.sisostds.org/ontologies/C2SIM#hasObjectDefinitions -->

    <owl:ObjectProperty rdf:about="http://www.sisostds.org/ontologies/C2SIM#hasObjectDefinitions">
        <rdfs:range rdf:resource="http://www.sisostds.org/ontologies/C2SIM#ObjectDefinitions"/>
    </owl:ObjectProperty>
    


    <!-- http://www.sisostds.org/ontologies/C2SIM#hasOperationalStatus -->

    <owl:ObjectProperty rdf:about="http://www.sisostds.org/ontologies/C2SIM#hasOperationalStatus">
        <rdfs:subPropertyOf rdf:resource="http://www.sisostds.org/ontologies/C2SIM#hasEntityHealthStatus"/>
        <rdfs:range rdf:resource="http://www.sisostds.org/ontologies/C2SIM#OperationalStatus"/>
    </owl:ObjectProperty>
    


    <!-- http://www.sisostds.org/ontologies/C2SIM#hasOperationalStatusCode -->

    <owl:ObjectProperty rdf:about="http://www.sisostds.org/ontologies/C2SIM#hasOperationalStatusCode">
        <rdfs:subPropertyOf rdf:resource="http://www.sisostds.org/ontologies/C2SIM#hasCode"/>
        <rdfs:range rdf:resource="http://www.sisostds.org/ontologies/C2SIM#OperationalStatusCode"/>
    </owl:ObjectProperty>
    


    <!-- http://www.sisostds.org/ontologies/C2SIM#hasOrganizationCode -->

    <owl:ObjectProperty rdf:about="http://www.sisostds.org/ontologies/C2SIM#hasOrganizationCode">
        <rdfs:subPropertyOf rdf:resource="http://www.sisostds.org/ontologies/C2SIM#hasCode"/>
        <rdfs:range rdf:resource="http://www.sisostds.org/ontologies/C2SIM#OrganizationCode"/>
    </owl:ObjectProperty>
    


    <!-- http://www.sisostds.org/ontologies/C2SIM#hasOrientation -->

    <owl:ObjectProperty rdf:about="http://www.sisostds.org/ontologies/C2SIM#hasOrientation">
        <rdfs:range rdf:resource="http://www.sisostds.org/ontologies/C2SIM#Orientation"/>
    </owl:ObjectProperty>
    


    <!-- http://www.sisostds.org/ontologies/C2SIM#hasPhysicalExtent -->

    <owl:ObjectProperty rdf:about="http://www.sisostds.org/ontologies/C2SIM#hasPhysicalExtent">
        <rdfs:range rdf:resource="http://www.sisostds.org/ontologies/C2SIM#PhysicalExtent"/>
    </owl:ObjectProperty>
    


    <!-- http://www.sisostds.org/ontologies/C2SIM#hasReligiousOrganizationCode -->

    <owl:ObjectProperty rdf:about="http://www.sisostds.org/ontologies/C2SIM#hasReligiousOrganizationCode">
        <rdfs:subPropertyOf rdf:resource="http://www.sisostds.org/ontologies/C2SIM#hasOrganizationCode"/>
        <rdfs:range rdf:resource="http://www.sisostds.org/ontologies/C2SIM#ReligiousOrganizationCode"/>
    </owl:ObjectProperty>
    


    <!-- http://www.sisostds.org/ontologies/C2SIM#hasReportContent -->

    <owl:ObjectProperty rdf:about="http://www.sisostds.org/ontologies/C2SIM#hasReportContent">
        <rdfs:range rdf:resource="http://www.sisostds.org/ontologies/C2SIM#ReportContent"/>
    </owl:ObjectProperty>
    


    <!-- http://www.sisostds.org/ontologies/C2SIM#hasResource -->

    <owl:ObjectProperty rdf:about="http://www.sisostds.org/ontologies/C2SIM#hasResource">
        <rdfs:range rdf:resource="http://www.sisostds.org/ontologies/C2SIM#Resource"/>
    </owl:ObjectProperty>
    


    <!-- http://www.sisostds.org/ontologies/C2SIM#hasScenarioSetting -->

    <owl:ObjectProperty rdf:about="http://www.sisostds.org/ontologies/C2SIM#hasScenarioSetting">
        <rdfs:range rdf:resource="http://www.sisostds.org/ontologies/C2SIM#ScenarioSetting"/>
    </owl:ObjectProperty>
    


    <!-- http://www.sisostds.org/ontologies/C2SIM#hasSecurityClassificationCode -->

    <owl:ObjectProperty rdf:about="http://www.sisostds.org/ontologies/C2SIM#hasSecurityClassificationCode">
        <rdfs:subPropertyOf rdf:resource="http://www.sisostds.org/ontologies/C2SIM#hasCode"/>
        <rdfs:range rdf:resource="http://www.sisostds.org/ontologies/C2SIM#SecurityClassificationCode"/>
    </owl:ObjectProperty>
    


    <!-- http://www.sisostds.org/ontologies/C2SIM#hasSpatialOffset -->

    <owl:ObjectProperty rdf:about="http://www.sisostds.org/ontologies/C2SIM#hasSpatialOffset">
        <rdfs:range rdf:resource="http://www.sisostds.org/ontologies/C2SIM#SpatialOffset"/>
    </owl:ObjectProperty>
    


    <!-- http://www.sisostds.org/ontologies/C2SIM#hasStartTime -->

    <owl:ObjectProperty rdf:about="http://www.sisostds.org/ontologies/C2SIM#hasStartTime">
        <rdfs:subPropertyOf rdf:resource="http://www.sisostds.org/ontologies/C2SIM#hasDateTime"/>
        <rdfs:range rdf:resource="http://www.sisostds.org/ontologies/C2SIM#DateTime"/>
        <rdfs:comment>date/time at which an action/task is to begin (C-BML)</rdfs:comment>
    </owl:ObjectProperty>
    


    <!-- http://www.sisostds.org/ontologies/C2SIM#hasStrength -->

    <owl:ObjectProperty rdf:about="http://www.sisostds.org/ontologies/C2SIM#hasStrength">
        <rdfs:subPropertyOf rdf:resource="http://www.sisostds.org/ontologies/C2SIM#hasEntityHealthStatus"/>
        <rdfs:range rdf:resource="http://www.sisostds.org/ontologies/C2SIM#Strength"/>
    </owl:ObjectProperty>
    


    <!-- http://www.sisostds.org/ontologies/C2SIM#hasSystemCommandTypeCode -->

    <owl:ObjectProperty rdf:about="http://www.sisostds.org/ontologies/C2SIM#hasSystemCommandTypeCode">
        <rdfs:subPropertyOf rdf:resource="http://www.sisostds.org/ontologies/C2SIM#hasCode"/>
        <rdfs:range rdf:resource="http://www.sisostds.org/ontologies/C2SIM#SystemCommandTypeCode"/>
    </owl:ObjectProperty>
    


    <!-- http://www.sisostds.org/ontologies/C2SIM#hasSystemEntityList -->

    <owl:ObjectProperty rdf:about="http://www.sisostds.org/ontologies/C2SIM#hasSystemEntityList">
        <rdfs:range rdf:resource="http://www.sisostds.org/ontologies/C2SIM#SystemEntityList"/>
    </owl:ObjectProperty>
    


    <!-- http://www.sisostds.org/ontologies/C2SIM#hasSystemStateCode -->

    <owl:ObjectProperty rdf:about="http://www.sisostds.org/ontologies/C2SIM#hasSystemStateCode">
        <rdfs:subPropertyOf rdf:resource="http://www.sisostds.org/ontologies/C2SIM#hasCode"/>
        <rdfs:range rdf:resource="http://www.sisostds.org/ontologies/C2SIM#SystemStateCode"/>
    </owl:ObjectProperty>
    


    <!-- http://www.sisostds.org/ontologies/C2SIM#hasTask -->

    <owl:ObjectProperty rdf:about="http://www.sisostds.org/ontologies/C2SIM#hasTask">
        <rdfs:subPropertyOf rdf:resource="http://www.sisostds.org/ontologies/C2SIM#hasAction"/>
        <rdfs:range rdf:resource="http://www.sisostds.org/ontologies/C2SIM#Task"/>
    </owl:ObjectProperty>
    


    <!-- http://www.sisostds.org/ontologies/C2SIM#hasTaskNameCode -->

    <owl:ObjectProperty rdf:about="http://www.sisostds.org/ontologies/C2SIM#hasTaskNameCode">
        <rdfs:subPropertyOf rdf:resource="http://www.sisostds.org/ontologies/C2SIM#hasActionCode"/>
        <rdfs:range rdf:resource="http://www.sisostds.org/ontologies/C2SIM#TaskNameCode"/>
    </owl:ObjectProperty>
    


    <!-- http://www.sisostds.org/ontologies/C2SIM#hasTemporalConcept -->

    <owl:ObjectProperty rdf:about="http://www.sisostds.org/ontologies/C2SIM#hasTemporalConcept">
        <rdfs:range rdf:resource="http://www.sisostds.org/ontologies/C2SIM#TemporalConcept"/>
    </owl:ObjectProperty>
    


    <!-- http://www.sisostds.org/ontologies/C2SIM#hasTimeInstant -->

    <owl:ObjectProperty rdf:about="http://www.sisostds.org/ontologies/C2SIM#hasTimeInstant">
        <rdfs:subPropertyOf rdf:resource="http://www.sisostds.org/ontologies/C2SIM#hasTemporalConcept"/>
        <rdfs:range rdf:resource="http://www.sisostds.org/ontologies/C2SIM#TimeInstant"/>
    </owl:ObjectProperty>
    


    <!-- http://www.sisostds.org/ontologies/C2SIM#hasTimeOfObservation -->

    <owl:ObjectProperty rdf:about="http://www.sisostds.org/ontologies/C2SIM#hasTimeOfObservation">
        <rdfs:subPropertyOf rdf:resource="http://www.sisostds.org/ontologies/C2SIM#hasDateTime"/>
        <rdfs:range rdf:resource="http://www.sisostds.org/ontologies/C2SIM#DateTime"/>
    </owl:ObjectProperty>
    


    <!-- http://www.sisostds.org/ontologies/C2SIM#hasTimeReferenceCode -->

    <owl:ObjectProperty rdf:about="http://www.sisostds.org/ontologies/C2SIM#hasTimeReferenceCode">
        <rdfs:subPropertyOf rdf:resource="http://www.sisostds.org/ontologies/C2SIM#hasTemporalConcept"/>
        <rdfs:range rdf:resource="http://www.sisostds.org/ontologies/C2SIM#TimeReferenceCode"/>
    </owl:ObjectProperty>
    


    <!-- http://www.sisostds.org/ontologies/lox#hasEvent -->

    <owl:ObjectProperty rdf:about="http://www.sisostds.org/ontologies/lox#hasEvent">
        <rdfs:subPropertyOf rdf:resource="http://www.sisostds.org/ontologies/C2SIM#hasAction"/>
        <rdfs:range rdf:resource="http://www.sisostds.org/ontologies/C2SIM#Event"/>
    </owl:ObjectProperty>
    


    <!-- http://www.sisostds.org/ontologies/lox#hasPlanPhase -->

    <owl:ObjectProperty rdf:about="http://www.sisostds.org/ontologies/lox#hasPlanPhase">
        <rdfs:range rdf:resource="http://www.sisostds.org/ontologies/lox#PlanPhase"/>
    </owl:ObjectProperty>
    


    <!-- http://www.sisostds.org/ontologies/lox#hasPlanPhaseCompletionCondition -->

    <owl:ObjectProperty rdf:about="http://www.sisostds.org/ontologies/lox#hasPlanPhaseCompletionCondition">
        <rdfs:range rdf:resource="http://www.sisostds.org/ontologies/lox#PlanPhaseCompletionCondition"/>
    </owl:ObjectProperty>
    


    <!-- http://www.sisostds.org/ontologies/lox#hasPlanPhaseTrigger -->

    <owl:ObjectProperty rdf:about="http://www.sisostds.org/ontologies/lox#hasPlanPhaseTrigger">
        <rdfs:range rdf:resource="http://www.sisostds.org/ontologies/lox#PlanPhaseTrigger"/>
    </owl:ObjectProperty>
    


    <!-- http://www.sisostds.org/ontologies/lox#hasSubPhase -->

    <owl:ObjectProperty rdf:about="http://www.sisostds.org/ontologies/lox#hasSubPhase">
        <rdfs:range rdf:resource="http://www.sisostds.org/ontologies/lox#PlanPhase"/>
    </owl:ObjectProperty>
    


    <!-- http://www.sisostds.org/ontologies/lox#hasTaskFunctionalAssociationCode -->

    <owl:ObjectProperty rdf:about="http://www.sisostds.org/ontologies/lox#hasTaskFunctionalAssociationCode">
        <rdfs:range rdf:resource="http://www.sisostds.org/ontologies/lox#TaskFunctionalAssociationCode"/>
    </owl:ObjectProperty>
    


    <!-- http://www.sisostds.org/ontologies/smx#hasAPP6-SIDC -->

    <owl:ObjectProperty rdf:about="http://www.sisostds.org/ontologies/smx#hasAPP6-SIDC">
        <rdfs:subPropertyOf rdf:resource="http://www.sisostds.org/ontologies/C2SIM#hasEntityType"/>
        <rdfs:range rdf:resource="http://www.sisostds.org/ontologies/smx#APP6-SIDC"/>
    </owl:ObjectProperty>
    


    <!-- http://www.sisostds.org/ontologies/smx#hasAircraftTypeCategoryCode -->

    <owl:ObjectProperty rdf:about="http://www.sisostds.org/ontologies/smx#hasAircraftTypeCategoryCode">
        <rdfs:subPropertyOf rdf:resource="http://www.sisostds.org/ontologies/C2SIM#hasCode"/>
        <rdfs:range rdf:resource="http://www.sisostds.org/ontologies/smx#AircraftTypeCategoryCode"/>
    </owl:ObjectProperty>
    


    <!-- http://www.sisostds.org/ontologies/smx#hasAmmunitionTypeCategoryCode -->

    <owl:ObjectProperty rdf:about="http://www.sisostds.org/ontologies/smx#hasAmmunitionTypeCategoryCode">
        <rdfs:subPropertyOf rdf:resource="http://www.sisostds.org/ontologies/C2SIM#hasCode"/>
        <rdfs:range rdf:resource="http://www.sisostds.org/ontologies/smx#AmmunitionTypeCategoryCode"/>
    </owl:ObjectProperty>
    


    <!-- http://www.sisostds.org/ontologies/smx#hasCombatEffectiveness -->

    <owl:ObjectProperty rdf:about="http://www.sisostds.org/ontologies/smx#hasCombatEffectiveness">
        <rdfs:subPropertyOf rdf:resource="http://www.sisostds.org/ontologies/C2SIM#hasConsumableMaterial"/>
    </owl:ObjectProperty>
    


    <!-- http://www.sisostds.org/ontologies/smx#hasDISCountryCode -->

    <owl:ObjectProperty rdf:about="http://www.sisostds.org/ontologies/smx#hasDISCountryCode">
        <rdfs:subPropertyOf rdf:resource="http://www.sisostds.org/ontologies/smx#hasDISTypeCode"/>
        <rdfs:range rdf:resource="http://www.sisostds.org/ontologies/smx#DISCountryCode"/>
    </owl:ObjectProperty>
    


    <!-- http://www.sisostds.org/ontologies/smx#hasDISDomainCode -->

    <owl:ObjectProperty rdf:about="http://www.sisostds.org/ontologies/smx#hasDISDomainCode">
        <rdfs:subPropertyOf rdf:resource="http://www.sisostds.org/ontologies/smx#hasDISTypeCode"/>
        <rdfs:range rdf:resource="http://www.sisostds.org/ontologies/smx#DISDomainCode"/>
    </owl:ObjectProperty>
    


    <!-- http://www.sisostds.org/ontologies/smx#hasDISKindCode -->

    <owl:ObjectProperty rdf:about="http://www.sisostds.org/ontologies/smx#hasDISKindCode">
        <rdfs:subPropertyOf rdf:resource="http://www.sisostds.org/ontologies/smx#hasDISTypeCode"/>
        <rdfs:range rdf:resource="http://www.sisostds.org/ontologies/smx#DISKindCode"/>
    </owl:ObjectProperty>
    


    <!-- http://www.sisostds.org/ontologies/smx#hasDISTypeCode -->

    <owl:ObjectProperty rdf:about="http://www.sisostds.org/ontologies/smx#hasDISTypeCode">
        <rdfs:subPropertyOf rdf:resource="http://www.sisostds.org/ontologies/C2SIM#hasCode"/>
        <rdfs:range rdf:resource="http://www.sisostds.org/ontologies/smx#DISTypeCode"/>
    </owl:ObjectProperty>
    


    <!-- http://www.sisostds.org/ontologies/smx#hasEchelonCode -->

    <owl:ObjectProperty rdf:about="http://www.sisostds.org/ontologies/smx#hasEchelonCode">
        <rdfs:subPropertyOf rdf:resource="http://www.sisostds.org/ontologies/C2SIM#hasCode"/>
        <rdfs:range rdf:resource="http://www.sisostds.org/ontologies/smx#EchelonCode"/>
    </owl:ObjectProperty>
    


    <!-- http://www.sisostds.org/ontologies/smx#hasObservation -->

    <owl:ObjectProperty rdf:about="http://www.sisostds.org/ontologies/smx#hasObservation">
        <rdfs:range rdf:resource="http://www.sisostds.org/ontologies/smx#Observation"/>
    </owl:ObjectProperty>
    


    <!-- http://www.sisostds.org/ontologies/smx#hasPersonTypeCategoryCode -->

    <owl:ObjectProperty rdf:about="http://www.sisostds.org/ontologies/smx#hasPersonTypeCategoryCode">
        <rdfs:subPropertyOf rdf:resource="http://www.sisostds.org/ontologies/C2SIM#hasCode"/>
        <rdfs:range rdf:resource="http://www.sisostds.org/ontologies/smx#PersonTypeCategoryCode"/>
    </owl:ObjectProperty>
    


    <!-- http://www.sisostds.org/ontologies/smx#hasReinforcedReducedType -->

    <owl:ObjectProperty rdf:about="http://www.sisostds.org/ontologies/smx#hasReinforcedReducedType">
        <rdfs:range rdf:resource="http://www.sisostds.org/ontologies/smx#ReinforcedReducedType"/>
    </owl:ObjectProperty>
    


    <!-- http://www.sisostds.org/ontologies/smx#hasSideHostilityCode -->

    <owl:ObjectProperty rdf:about="http://www.sisostds.org/ontologies/smx#hasSideHostilityCode">
        <rdfs:subPropertyOf rdf:resource="http://www.sisostds.org/ontologies/C2SIM#hasCode"/>
        <rdfs:range rdf:resource="http://www.sisostds.org/ontologies/smx#SideHostilityCode"/>
    </owl:ObjectProperty>
    


    <!-- http://www.sisostds.org/ontologies/smx#hasSubsurfaceVesselTypeCode -->

    <owl:ObjectProperty rdf:about="http://www.sisostds.org/ontologies/smx#hasSubsurfaceVesselTypeCode">
        <rdfs:subPropertyOf rdf:resource="http://www.sisostds.org/ontologies/C2SIM#hasCode"/>
        <rdfs:range rdf:resource="http://www.sisostds.org/ontologies/smx#SurfaceVesselTypeCode"/>
    </owl:ObjectProperty>
    


    <!-- http://www.sisostds.org/ontologies/smx#hasSupportingTaskCode -->

    <owl:ObjectProperty rdf:about="http://www.sisostds.org/ontologies/smx#hasSupportingTaskCode">
        <rdfs:subPropertyOf rdf:resource="http://www.sisostds.org/ontologies/C2SIM#hasCode"/>
        <rdfs:range rdf:resource="http://www.sisostds.org/ontologies/C2SIM#TaskNameCode"/>
    </owl:ObjectProperty>
    


    <!-- http://www.sisostds.org/ontologies/smx#hasSurfaceVesselTypeCode -->

    <owl:ObjectProperty rdf:about="http://www.sisostds.org/ontologies/smx#hasSurfaceVesselTypeCode">
        <rdfs:subPropertyOf rdf:resource="http://www.sisostds.org/ontologies/C2SIM#hasCode"/>
        <rdfs:range rdf:resource="http://www.sisostds.org/ontologies/smx#SurfaceVesselTypeCode"/>
    </owl:ObjectProperty>
    


    <!-- http://www.sisostds.org/ontologies/smx#hasVehicleTypeCategoryCode -->

    <owl:ObjectProperty rdf:about="http://www.sisostds.org/ontologies/smx#hasVehicleTypeCategoryCode">
        <rdfs:subPropertyOf rdf:resource="http://www.sisostds.org/ontologies/C2SIM#hasCode"/>
        <rdfs:range rdf:resource="http://www.sisostds.org/ontologies/smx#VehicleTypeCategoryCode"/>
    </owl:ObjectProperty>
    


    <!-- http://www.sisostds.org/ontologies/smx#hasWeaponTypeCategoryCode -->

    <owl:ObjectProperty rdf:about="http://www.sisostds.org/ontologies/smx#hasWeaponTypeCategoryCode">
        <rdfs:subPropertyOf rdf:resource="http://www.sisostds.org/ontologies/C2SIM#hasCode"/>
        <rdfs:range rdf:resource="http://www.sisostds.org/ontologies/smx#WeaponTypeCategoryCode"/>
    </owl:ObjectProperty>
    


    <!-- 
    ///////////////////////////////////////////////////////////////////////////////////////
    //
    // Data properties
    //
    ///////////////////////////////////////////////////////////////////////////////////////
     -->

    


    <!-- http://www.sisostds.org/ontologies/C2SIM#hasAbstractObjectReference -->

    <owl:DatatypeProperty rdf:about="http://www.sisostds.org/ontologies/C2SIM#hasAbstractObjectReference">
        <rdfs:subPropertyOf rdf:resource="http://www.sisostds.org/ontologies/C2SIM#hasReference"/>
    </owl:DatatypeProperty>
    


    <!-- http://www.sisostds.org/ontologies/C2SIM#hasAbstractOrganizationReference -->

    <owl:DatatypeProperty rdf:about="http://www.sisostds.org/ontologies/C2SIM#hasAbstractOrganizationReference">
        <rdfs:subPropertyOf rdf:resource="http://www.sisostds.org/ontologies/C2SIM#hasAbstractObjectReference"/>
    </owl:DatatypeProperty>
    


    <!-- http://www.sisostds.org/ontologies/C2SIM#hasActionReference -->

    <owl:DatatypeProperty rdf:about="http://www.sisostds.org/ontologies/C2SIM#hasActionReference">
        <rdfs:subPropertyOf rdf:resource="http://www.sisostds.org/ontologies/C2SIM#hasReference"/>
    </owl:DatatypeProperty>
    


    <!-- http://www.sisostds.org/ontologies/C2SIM#hasActorReference -->

    <owl:DatatypeProperty rdf:about="http://www.sisostds.org/ontologies/C2SIM#hasActorReference">
        <rdfs:subPropertyOf rdf:resource="http://www.sisostds.org/ontologies/C2SIM#hasEntityReference"/>
        <rdfs:comment>These references should be to objects of class Actor, or subclasses.</rdfs:comment>
    </owl:DatatypeProperty>
    


    <!-- http://www.sisostds.org/ontologies/C2SIM#hasAffectedEntity -->

    <owl:DatatypeProperty rdf:about="http://www.sisostds.org/ontologies/C2SIM#hasAffectedEntity">
        <rdfs:subPropertyOf rdf:resource="http://www.sisostds.org/ontologies/C2SIM#hasActorReference"/>
    </owl:DatatypeProperty>
    


    <!-- http://www.sisostds.org/ontologies/C2SIM#hasAllegianceTo -->

    <owl:DatatypeProperty rdf:about="http://www.sisostds.org/ontologies/C2SIM#hasAllegianceTo">
        <rdfs:subPropertyOf rdf:resource="http://www.sisostds.org/ontologies/C2SIM#hasActorReference"/>
    </owl:DatatypeProperty>
    


    <!-- http://www.sisostds.org/ontologies/C2SIM#hasAltitude -->

    <owl:DatatypeProperty rdf:about="http://www.sisostds.org/ontologies/C2SIM#hasAltitude">
        <rdfs:subPropertyOf rdf:resource="http://www.sisostds.org/ontologies/C2SIM#spatialMeasures"/>
    </owl:DatatypeProperty>
    


    <!-- http://www.sisostds.org/ontologies/C2SIM#hasAltitudeAGL -->

    <owl:DatatypeProperty rdf:about="http://www.sisostds.org/ontologies/C2SIM#hasAltitudeAGL">
        <rdfs:subPropertyOf rdf:resource="http://www.sisostds.org/ontologies/C2SIM#hasAltitude"/>
        <rdfs:range rdf:resource="http://www.w3.org/2001/XMLSchema#double"/>
    </owl:DatatypeProperty>
    


    <!-- http://www.sisostds.org/ontologies/C2SIM#hasAltitudeMSL -->

    <owl:DatatypeProperty rdf:about="http://www.sisostds.org/ontologies/C2SIM#hasAltitudeMSL">
        <rdfs:subPropertyOf rdf:resource="http://www.sisostds.org/ontologies/C2SIM#hasAltitude"/>
        <rdfs:range rdf:resource="http://www.w3.org/2001/XMLSchema#double"/>
    </owl:DatatypeProperty>
    


    <!-- http://www.sisostds.org/ontologies/C2SIM#hasAngle -->

    <owl:DatatypeProperty rdf:about="http://www.sisostds.org/ontologies/C2SIM#hasAngle">
        <rdfs:subPropertyOf rdf:resource="http://www.sisostds.org/ontologies/C2SIM#spatialMeasures"/>
    </owl:DatatypeProperty>
    


    <!-- http://www.sisostds.org/ontologies/C2SIM#hasComment -->

    <owl:DatatypeProperty rdf:about="http://www.sisostds.org/ontologies/C2SIM#hasComment">
        <rdfs:range rdf:resource="http://www.w3.org/2001/XMLSchema#string"/>
    </owl:DatatypeProperty>
    


    <!-- http://www.sisostds.org/ontologies/C2SIM#hasCommunicationsNetwork -->

    <owl:DatatypeProperty rdf:about="http://www.sisostds.org/ontologies/C2SIM#hasCommunicationsNetwork">
        <rdfs:subPropertyOf rdf:resource="http://www.sisostds.org/ontologies/C2SIM#hasAbstractObjectReference"/>
    </owl:DatatypeProperty>
    


    <!-- http://www.sisostds.org/ontologies/C2SIM#hasConcreteEntityReference -->

    <owl:DatatypeProperty rdf:about="http://www.sisostds.org/ontologies/C2SIM#hasConcreteEntityReference">
        <rdfs:subPropertyOf rdf:resource="http://www.sisostds.org/ontologies/C2SIM#hasEntityReference"/>
    </owl:DatatypeProperty>
    


    <!-- http://www.sisostds.org/ontologies/C2SIM#hasConversationID -->

    <owl:DatatypeProperty rdf:about="http://www.sisostds.org/ontologies/C2SIM#hasConversationID">
        <rdfs:subPropertyOf rdf:resource="http://www.sisostds.org/ontologies/C2SIM#hasMessagingDataProperty"/>
        <rdfs:range rdf:resource="http://www.sisostds.org/ontologies/C2SIM#UUIDBase"/>
    </owl:DatatypeProperty>
    


    <!-- http://www.sisostds.org/ontologies/C2SIM#hasCoordinateValue -->

    <owl:DatatypeProperty rdf:about="http://www.sisostds.org/ontologies/C2SIM#hasCoordinateValue"/>
    


    <!-- http://www.sisostds.org/ontologies/C2SIM#hasCount -->

    <owl:DatatypeProperty rdf:about="http://www.sisostds.org/ontologies/C2SIM#hasCount">
        <rdfs:range rdf:resource="http://www.w3.org/2001/XMLSchema#nonNegativeInteger"/>
    </owl:DatatypeProperty>
    


    <!-- http://www.sisostds.org/ontologies/C2SIM#hasCurrentTask -->

    <owl:DatatypeProperty rdf:about="http://www.sisostds.org/ontologies/C2SIM#hasCurrentTask">
        <rdfs:subPropertyOf rdf:resource="http://www.sisostds.org/ontologies/C2SIM#hasTaskReference"/>
    </owl:DatatypeProperty>
    


    <!-- http://www.sisostds.org/ontologies/C2SIM#hasDepth -->

    <owl:DatatypeProperty rdf:about="http://www.sisostds.org/ontologies/C2SIM#hasDepth">
        <rdfs:subPropertyOf rdf:resource="http://www.sisostds.org/ontologies/C2SIM#hasDistance"/>
        <rdfs:range rdf:resource="http://www.w3.org/2001/XMLSchema#double"/>
        <rdfs:comment>This is a measure of distance below mean sea level, i.e. positive is down.</rdfs:comment>
    </owl:DatatypeProperty>
    


    <!-- http://www.sisostds.org/ontologies/C2SIM#hasDistance -->

    <owl:DatatypeProperty rdf:about="http://www.sisostds.org/ontologies/C2SIM#hasDistance">
        <rdfs:subPropertyOf rdf:resource="http://www.sisostds.org/ontologies/C2SIM#spatialMeasures"/>
    </owl:DatatypeProperty>
    


    <!-- http://www.sisostds.org/ontologies/C2SIM#hasEntityReference -->

    <owl:DatatypeProperty rdf:about="http://www.sisostds.org/ontologies/C2SIM#hasEntityReference">
        <rdfs:subPropertyOf rdf:resource="http://www.sisostds.org/ontologies/C2SIM#hasReference"/>
    </owl:DatatypeProperty>
    


    <!-- http://www.sisostds.org/ontologies/C2SIM#hasEntityTypeString -->

    <owl:DatatypeProperty rdf:about="http://www.sisostds.org/ontologies/C2SIM#hasEntityTypeString"/>
    


    <!-- http://www.sisostds.org/ontologies/C2SIM#hasEventReference -->

    <owl:DatatypeProperty rdf:about="http://www.sisostds.org/ontologies/C2SIM#hasEventReference">
        <rdfs:subPropertyOf rdf:resource="http://www.sisostds.org/ontologies/C2SIM#hasActionReference"/>
    </owl:DatatypeProperty>
    


    <!-- http://www.sisostds.org/ontologies/C2SIM#hasHealthStatus -->

    <owl:DatatypeProperty rdf:about="http://www.sisostds.org/ontologies/C2SIM#hasHealthStatus"/>
    


    <!-- http://www.sisostds.org/ontologies/C2SIM#hasHeight -->

    <owl:DatatypeProperty rdf:about="http://www.sisostds.org/ontologies/C2SIM#hasHeight">
        <rdfs:subPropertyOf rdf:resource="http://www.sisostds.org/ontologies/C2SIM#hasDistance"/>
        <rdfs:range rdf:resource="http://www.w3.org/2001/XMLSchema#double"/>
    </owl:DatatypeProperty>
    


    <!-- http://www.sisostds.org/ontologies/C2SIM#hasIntializationFileType -->

    <owl:DatatypeProperty rdf:about="http://www.sisostds.org/ontologies/C2SIM#hasIntializationFileType">
        <rdfs:range rdf:resource="http://www.w3.org/2001/XMLSchema#string"/>
    </owl:DatatypeProperty>
    


    <!-- http://www.sisostds.org/ontologies/C2SIM#hasIsoDateTime -->

    <owl:DatatypeProperty rdf:about="http://www.sisostds.org/ontologies/C2SIM#hasIsoDateTime">
        <rdfs:range rdf:resource="http://www.sisostds.org/ontologies/C2SIM#IsoDateTimeBase"/>
    </owl:DatatypeProperty>
    


    <!-- http://www.sisostds.org/ontologies/C2SIM#hasIsoTimeDuration -->

    <owl:DatatypeProperty rdf:about="http://www.sisostds.org/ontologies/C2SIM#hasIsoTimeDuration">
        <rdfs:range rdf:resource="http://www.sisostds.org/ontologies/C2SIM#IsoTimeDurationBase"/>
    </owl:DatatypeProperty>
    


    <!-- http://www.sisostds.org/ontologies/C2SIM#hasLatitude -->

    <owl:DatatypeProperty rdf:about="http://www.sisostds.org/ontologies/C2SIM#hasLatitude">
        <rdfs:subPropertyOf rdf:resource="http://www.sisostds.org/ontologies/C2SIM#spatialMeasures"/>
        <rdfs:range rdf:resource="http://www.sisostds.org/ontologies/C2SIM#latitude"/>
        <rdfs:comment>This should have a range specified of -90 to +90 (degrees)</rdfs:comment>
    </owl:DatatypeProperty>
    


    <!-- http://www.sisostds.org/ontologies/C2SIM#hasLength -->

    <owl:DatatypeProperty rdf:about="http://www.sisostds.org/ontologies/C2SIM#hasLength">
        <rdfs:subPropertyOf rdf:resource="http://www.sisostds.org/ontologies/C2SIM#hasDistance"/>
        <rdfs:range rdf:resource="http://www.w3.org/2001/XMLSchema#double"/>
    </owl:DatatypeProperty>
    


    <!-- http://www.sisostds.org/ontologies/C2SIM#hasLocationReferenceEntity -->

    <owl:DatatypeProperty rdf:about="http://www.sisostds.org/ontologies/C2SIM#hasLocationReferenceEntity">
        <rdfs:subPropertyOf rdf:resource="http://www.sisostds.org/ontologies/C2SIM#hasConcreteEntityReference"/>
    </owl:DatatypeProperty>
    


    <!-- http://www.sisostds.org/ontologies/C2SIM#hasLongitude -->

    <owl:DatatypeProperty rdf:about="http://www.sisostds.org/ontologies/C2SIM#hasLongitude">
        <rdfs:subPropertyOf rdf:resource="http://www.sisostds.org/ontologies/C2SIM#spatialMeasures"/>
        <rdfs:range rdf:resource="http://www.sisostds.org/ontologies/C2SIM#longitude"/>
        <rdfs:comment>This should have a range specified of -180 to +180 (degrees)</rdfs:comment>
    </owl:DatatypeProperty>
    


    <!-- http://www.sisostds.org/ontologies/C2SIM#hasMapGraphicID -->

    <owl:DatatypeProperty rdf:about="http://www.sisostds.org/ontologies/C2SIM#hasMapGraphicID">
        <rdfs:subPropertyOf rdf:resource="http://www.sisostds.org/ontologies/C2SIM#hasConcreteEntityReference"/>
    </owl:DatatypeProperty>
    


    <!-- http://www.sisostds.org/ontologies/C2SIM#hasMarking -->

    <owl:DatatypeProperty rdf:about="http://www.sisostds.org/ontologies/C2SIM#hasMarking">
        <rdfs:range rdf:resource="http://www.w3.org/2001/XMLSchema#string"/>
    </owl:DatatypeProperty>
    


    <!-- http://www.sisostds.org/ontologies/C2SIM#hasMessageID -->

    <owl:DatatypeProperty rdf:about="http://www.sisostds.org/ontologies/C2SIM#hasMessageID">
        <rdfs:subPropertyOf rdf:resource="http://www.sisostds.org/ontologies/C2SIM#hasMessagingDataProperty"/>
        <rdfs:range rdf:resource="http://www.sisostds.org/ontologies/C2SIM#UUIDBase"/>
    </owl:DatatypeProperty>
    


    <!-- http://www.sisostds.org/ontologies/C2SIM#hasMessagingDataProperty -->

    <owl:DatatypeProperty rdf:about="http://www.sisostds.org/ontologies/C2SIM#hasMessagingDataProperty"/>
    


    <!-- http://www.sisostds.org/ontologies/C2SIM#hasName -->

    <owl:DatatypeProperty rdf:about="http://www.sisostds.org/ontologies/C2SIM#hasName">
        <rdfs:range rdf:resource="http://www.w3.org/2001/XMLSchema#string"/>
    </owl:DatatypeProperty>
    


    <!-- http://www.sisostds.org/ontologies/C2SIM#hasNotificationType -->

    <owl:DatatypeProperty rdf:about="http://www.sisostds.org/ontologies/C2SIM#hasNotificationType"/>
    


    <!-- http://www.sisostds.org/ontologies/C2SIM#hasNumberOfOrganizations -->

    <owl:DatatypeProperty rdf:about="http://www.sisostds.org/ontologies/C2SIM#hasNumberOfOrganizations">
        <rdfs:range rdf:resource="http://www.w3.org/2001/XMLSchema#nonNegativeInteger"/>
    </owl:DatatypeProperty>
    


    <!-- http://www.sisostds.org/ontologies/C2SIM#hasOrderID -->

    <owl:DatatypeProperty rdf:about="http://www.sisostds.org/ontologies/C2SIM#hasOrderID">
        <rdfs:subPropertyOf rdf:resource="http://www.sisostds.org/ontologies/C2SIM#hasMessagingDataProperty"/>
        <rdfs:range rdf:resource="http://www.sisostds.org/ontologies/C2SIM#UUIDBase"/>
    </owl:DatatypeProperty>
    


    <!-- http://www.sisostds.org/ontologies/C2SIM#hasPerformingEntity -->

    <owl:DatatypeProperty rdf:about="http://www.sisostds.org/ontologies/C2SIM#hasPerformingEntity">
        <rdfs:subPropertyOf rdf:resource="http://www.sisostds.org/ontologies/C2SIM#hasActorReference"/>
    </owl:DatatypeProperty>
    


    <!-- http://www.sisostds.org/ontologies/C2SIM#hasPhi -->

    <owl:DatatypeProperty rdf:about="http://www.sisostds.org/ontologies/C2SIM#hasPhi">
        <rdfs:subPropertyOf rdf:resource="http://www.sisostds.org/ontologies/C2SIM#hasAngle"/>
        <rdfs:range rdf:resource="http://www.sisostds.org/ontologies/C2SIM#angle"/>
    </owl:DatatypeProperty>
    


    <!-- http://www.sisostds.org/ontologies/C2SIM#hasProtocol -->

    <owl:DatatypeProperty rdf:about="http://www.sisostds.org/ontologies/C2SIM#hasProtocol"/>
    


    <!-- http://www.sisostds.org/ontologies/C2SIM#hasProtocolVersion -->

    <owl:DatatypeProperty rdf:about="http://www.sisostds.org/ontologies/C2SIM#hasProtocolVersion"/>
    


    <!-- http://www.sisostds.org/ontologies/C2SIM#hasPsi -->

    <owl:DatatypeProperty rdf:about="http://www.sisostds.org/ontologies/C2SIM#hasPsi">
        <rdfs:subPropertyOf rdf:resource="http://www.sisostds.org/ontologies/C2SIM#hasAngle"/>
        <rdfs:range rdf:resource="http://www.sisostds.org/ontologies/C2SIM#angle"/>
    </owl:DatatypeProperty>
    


    <!-- http://www.sisostds.org/ontologies/C2SIM#hasReference -->

    <owl:DatatypeProperty rdf:about="http://www.sisostds.org/ontologies/C2SIM#hasReference">
        <rdfs:range rdf:resource="http://www.sisostds.org/ontologies/C2SIM#UUIDBase"/>
    </owl:DatatypeProperty>
    


    <!-- http://www.sisostds.org/ontologies/C2SIM#hasReplyToSystem -->

    <owl:DatatypeProperty rdf:about="http://www.sisostds.org/ontologies/C2SIM#hasReplyToSystem">
        <rdfs:subPropertyOf rdf:resource="http://www.sisostds.org/ontologies/C2SIM#hasMessagingDataProperty"/>
        <rdfs:range rdf:resource="http://www.w3.org/2001/XMLSchema#string"/>
    </owl:DatatypeProperty>
    


    <!-- http://www.sisostds.org/ontologies/C2SIM#hasReportingEntity -->

    <owl:DatatypeProperty rdf:about="http://www.sisostds.org/ontologies/C2SIM#hasReportingEntity">
        <rdfs:subPropertyOf rdf:resource="http://www.sisostds.org/ontologies/C2SIM#hasActorReference"/>
    </owl:DatatypeProperty>
    


    <!-- http://www.sisostds.org/ontologies/C2SIM#hasRequestingEntity -->

    <owl:DatatypeProperty rdf:about="http://www.sisostds.org/ontologies/C2SIM#hasRequestingEntity">
        <rdfs:subPropertyOf rdf:resource="http://www.sisostds.org/ontologies/C2SIM#hasActorReference"/>
    </owl:DatatypeProperty>
    


    <!-- http://www.sisostds.org/ontologies/C2SIM#hasSendingTime -->

    <owl:DatatypeProperty rdf:about="http://www.sisostds.org/ontologies/C2SIM#hasSendingTime">
        <rdfs:subPropertyOf rdf:resource="http://www.sisostds.org/ontologies/C2SIM#hasIsoDateTime"/>
        <rdfs:comment>The time that a message is sent.</rdfs:comment>
    </owl:DatatypeProperty>
    


    <!-- http://www.sisostds.org/ontologies/C2SIM#hasSpeed -->

    <owl:DatatypeProperty rdf:about="http://www.sisostds.org/ontologies/C2SIM#hasSpeed">
        <rdfs:subPropertyOf rdf:resource="http://www.sisostds.org/ontologies/C2SIM#spatialMeasures"/>
        <rdfs:range rdf:resource="http://www.w3.org/2001/XMLSchema#double"/>
        <rdfs:comment>Speed in meters/second.</rdfs:comment>
    </owl:DatatypeProperty>
    


    <!-- http://www.sisostds.org/ontologies/C2SIM#hasStrengthPercentage -->

    <owl:DatatypeProperty rdf:about="http://www.sisostds.org/ontologies/C2SIM#hasStrengthPercentage">
        <rdfs:subPropertyOf rdf:resource="http://www.sisostds.org/ontologies/C2SIM#hasHealthStatus"/>
        <rdfs:range rdf:resource="http://www.sisostds.org/ontologies/C2SIM#percentage"/>
    </owl:DatatypeProperty>
    


    <!-- http://www.sisostds.org/ontologies/C2SIM#hasSubjectEntity -->

    <owl:DatatypeProperty rdf:about="http://www.sisostds.org/ontologies/C2SIM#hasSubjectEntity">
        <rdfs:subPropertyOf rdf:resource="http://www.sisostds.org/ontologies/C2SIM#hasActorReference"/>
    </owl:DatatypeProperty>
    


    <!-- http://www.sisostds.org/ontologies/C2SIM#hasSubordinate -->

    <owl:DatatypeProperty rdf:about="http://www.sisostds.org/ontologies/C2SIM#hasSubordinate">
        <rdfs:subPropertyOf rdf:resource="http://www.sisostds.org/ontologies/C2SIM#hasActorReference"/>
    </owl:DatatypeProperty>
    


    <!-- http://www.sisostds.org/ontologies/C2SIM#hasSuperior -->

    <owl:DatatypeProperty rdf:about="http://www.sisostds.org/ontologies/C2SIM#hasSuperior">
        <rdfs:subPropertyOf rdf:resource="http://www.sisostds.org/ontologies/C2SIM#hasActorReference"/>
    </owl:DatatypeProperty>
    


    <!-- http://www.sisostds.org/ontologies/C2SIM#hasSystemName -->

    <owl:DatatypeProperty rdf:about="http://www.sisostds.org/ontologies/C2SIM#hasSystemName">
        <rdfs:subPropertyOf rdf:resource="http://www.sisostds.org/ontologies/C2SIM#hasName"/>
    </owl:DatatypeProperty>
    


    <!-- http://www.sisostds.org/ontologies/C2SIM#hasTaskReference -->

    <owl:DatatypeProperty rdf:about="http://www.sisostds.org/ontologies/C2SIM#hasTaskReference">
        <rdfs:subPropertyOf rdf:resource="http://www.sisostds.org/ontologies/C2SIM#hasActionReference"/>
    </owl:DatatypeProperty>
    


    <!-- http://www.sisostds.org/ontologies/C2SIM#hasTheta -->

    <owl:DatatypeProperty rdf:about="http://www.sisostds.org/ontologies/C2SIM#hasTheta">
        <rdfs:subPropertyOf rdf:resource="http://www.sisostds.org/ontologies/C2SIM#hasAngle"/>
        <rdfs:range rdf:resource="http://www.sisostds.org/ontologies/C2SIM#angle"/>
    </owl:DatatypeProperty>
    


    <!-- http://www.sisostds.org/ontologies/C2SIM#hasUUID -->

    <owl:DatatypeProperty rdf:about="http://www.sisostds.org/ontologies/C2SIM#hasUUID">
        <rdfs:subPropertyOf rdf:resource="http://www.sisostds.org/ontologies/C2SIM#hasUniqueIdentifier"/>
        <rdfs:range rdf:resource="http://www.sisostds.org/ontologies/C2SIM#UUIDBase"/>
    </owl:DatatypeProperty>
    


    <!-- http://www.sisostds.org/ontologies/C2SIM#hasUniqueIdentifier -->

    <owl:DatatypeProperty rdf:about="http://www.sisostds.org/ontologies/C2SIM#hasUniqueIdentifier"/>
    


    <!-- http://www.sisostds.org/ontologies/C2SIM#hasVersion -->

    <owl:DatatypeProperty rdf:about="http://www.sisostds.org/ontologies/C2SIM#hasVersion"/>
    


    <!-- http://www.sisostds.org/ontologies/C2SIM#hasWeatherProperty -->

    <owl:DatatypeProperty rdf:about="http://www.sisostds.org/ontologies/C2SIM#hasWeatherProperty">
        <rdfs:comment>Weather Property will have sub-properties for Atmosphere, Cloud Cover, Icing, Illumination, Precipitation, Visibility, Wind Speed and Direction, etc.</rdfs:comment>
    </owl:DatatypeProperty>
    


    <!-- http://www.sisostds.org/ontologies/C2SIM#hasWidth -->

    <owl:DatatypeProperty rdf:about="http://www.sisostds.org/ontologies/C2SIM#hasWidth">
        <rdfs:subPropertyOf rdf:resource="http://www.sisostds.org/ontologies/C2SIM#hasDistance"/>
        <rdfs:range rdf:resource="http://www.w3.org/2001/XMLSchema#double"/>
    </owl:DatatypeProperty>
    


    <!-- http://www.sisostds.org/ontologies/C2SIM#hasX -->

    <owl:DatatypeProperty rdf:about="http://www.sisostds.org/ontologies/C2SIM#hasX">
        <rdfs:subPropertyOf rdf:resource="http://www.sisostds.org/ontologies/C2SIM#hasCoordinateValue"/>
        <rdfs:range rdf:resource="http://www.w3.org/2001/XMLSchema#double"/>
    </owl:DatatypeProperty>
    


    <!-- http://www.sisostds.org/ontologies/C2SIM#hasY -->

    <owl:DatatypeProperty rdf:about="http://www.sisostds.org/ontologies/C2SIM#hasY">
        <rdfs:subPropertyOf rdf:resource="http://www.sisostds.org/ontologies/C2SIM#hasCoordinateValue"/>
        <rdfs:range rdf:resource="http://www.w3.org/2001/XMLSchema#double"/>
    </owl:DatatypeProperty>
    


    <!-- http://www.sisostds.org/ontologies/C2SIM#hasZ -->

    <owl:DatatypeProperty rdf:about="http://www.sisostds.org/ontologies/C2SIM#hasZ">
        <rdfs:subPropertyOf rdf:resource="http://www.sisostds.org/ontologies/C2SIM#hasCoordinateValue"/>
        <rdfs:range rdf:resource="http://www.w3.org/2001/XMLSchema#double"/>
    </owl:DatatypeProperty>
    


    <!-- http://www.sisostds.org/ontologies/C2SIM#isAffiliatedWith -->

    <owl:DatatypeProperty rdf:about="http://www.sisostds.org/ontologies/C2SIM#isAffiliatedWith">
        <rdfs:subPropertyOf rdf:resource="http://www.sisostds.org/ontologies/C2SIM#hasAbstractOrganizationReference"/>
    </owl:DatatypeProperty>
    


    <!-- http://www.sisostds.org/ontologies/C2SIM#isFriendlyTo -->

    <owl:DatatypeProperty rdf:about="http://www.sisostds.org/ontologies/C2SIM#isFriendlyTo">
        <rdfs:subPropertyOf rdf:resource="http://www.sisostds.org/ontologies/C2SIM#hasAllegianceTo"/>
    </owl:DatatypeProperty>
    


    <!-- http://www.sisostds.org/ontologies/C2SIM#isFromSender -->

    <owl:DatatypeProperty rdf:about="http://www.sisostds.org/ontologies/C2SIM#isFromSender">
        <rdfs:subPropertyOf rdf:resource="http://www.sisostds.org/ontologies/C2SIM#hasActorReference"/>
    </owl:DatatypeProperty>
    


    <!-- http://www.sisostds.org/ontologies/C2SIM#isFromSendingSystem -->

    <owl:DatatypeProperty rdf:about="http://www.sisostds.org/ontologies/C2SIM#isFromSendingSystem">
        <rdfs:subPropertyOf rdf:resource="http://www.sisostds.org/ontologies/C2SIM#hasMessagingDataProperty"/>
        <rdfs:range rdf:resource="http://www.w3.org/2001/XMLSchema#string"/>
    </owl:DatatypeProperty>
    


    <!-- http://www.sisostds.org/ontologies/C2SIM#isHostileTo -->

    <owl:DatatypeProperty rdf:about="http://www.sisostds.org/ontologies/C2SIM#isHostileTo">
        <rdfs:subPropertyOf rdf:resource="http://www.sisostds.org/ontologies/C2SIM#hasAllegianceTo"/>
    </owl:DatatypeProperty>
    


    <!-- http://www.sisostds.org/ontologies/C2SIM#isInReplyToMessageID -->

    <owl:DatatypeProperty rdf:about="http://www.sisostds.org/ontologies/C2SIM#isInReplyToMessageID">
        <rdfs:subPropertyOf rdf:resource="http://www.sisostds.org/ontologies/C2SIM#hasMessagingDataProperty"/>
        <rdfs:range rdf:resource="http://www.sisostds.org/ontologies/C2SIM#UUIDBase"/>
    </owl:DatatypeProperty>
    


    <!-- http://www.sisostds.org/ontologies/C2SIM#isNeutralTo -->

    <owl:DatatypeProperty rdf:about="http://www.sisostds.org/ontologies/C2SIM#isNeutralTo">
        <rdfs:subPropertyOf rdf:resource="http://www.sisostds.org/ontologies/C2SIM#hasAllegianceTo"/>
    </owl:DatatypeProperty>
    


    <!-- http://www.sisostds.org/ontologies/C2SIM#isToReceiver -->

    <owl:DatatypeProperty rdf:about="http://www.sisostds.org/ontologies/C2SIM#isToReceiver">
        <rdfs:subPropertyOf rdf:resource="http://www.sisostds.org/ontologies/C2SIM#hasActorReference"/>
    </owl:DatatypeProperty>
    


    <!-- http://www.sisostds.org/ontologies/C2SIM#isToReceivingSystem -->

    <owl:DatatypeProperty rdf:about="http://www.sisostds.org/ontologies/C2SIM#isToReceivingSystem">
        <rdfs:subPropertyOf rdf:resource="http://www.sisostds.org/ontologies/C2SIM#hasMessagingDataProperty"/>
        <rdfs:range rdf:resource="http://www.w3.org/2001/XMLSchema#string"/>
    </owl:DatatypeProperty>
    


    <!-- http://www.sisostds.org/ontologies/C2SIM#spatialMeasures -->

    <owl:DatatypeProperty rdf:about="http://www.sisostds.org/ontologies/C2SIM#spatialMeasures"/>
    


    <!-- http://www.sisostds.org/ontologies/C2SIM_SMX_LOX#hasAmount -->

    <owl:DatatypeProperty rdf:about="http://www.sisostds.org/ontologies/C2SIM_SMX_LOX#hasAmount">
        <rdfs:range rdf:resource="http://www.w3.org/2001/XMLSchema#nonNegativeInteger"/>
    </owl:DatatypeProperty>
    


    <!-- http://www.sisostds.org/ontologies/C2SIM_SMX_LOX#hasAmountOfAmmunition -->

    <owl:DatatypeProperty rdf:about="http://www.sisostds.org/ontologies/C2SIM_SMX_LOX#hasAmountOfAmmunition">
        <rdfs:subPropertyOf rdf:resource="http://www.sisostds.org/ontologies/C2SIM_SMX_LOX#hasAmount"/>
    </owl:DatatypeProperty>
    


    <!-- http://www.sisostds.org/ontologies/C2SIM_SMX_LOX#hasAmountOfDrones -->

    <owl:DatatypeProperty rdf:about="http://www.sisostds.org/ontologies/C2SIM_SMX_LOX#hasAmountOfDrones">
        <rdfs:subPropertyOf rdf:resource="http://www.sisostds.org/ontologies/C2SIM_SMX_LOX#hasAmount"/>
    </owl:DatatypeProperty>
    


    <!-- http://www.sisostds.org/ontologies/C2SIM_SMX_LOX#hasAmountOfMines -->

    <owl:DatatypeProperty rdf:about="http://www.sisostds.org/ontologies/C2SIM_SMX_LOX#hasAmountOfMines">
        <rdfs:subPropertyOf rdf:resource="http://www.sisostds.org/ontologies/C2SIM_SMX_LOX#hasAmount"/>
    </owl:DatatypeProperty>
    


    <!-- http://www.sisostds.org/ontologies/C2SIM_SMX_LOX#hasBoundaryProperty -->

    <owl:DatatypeProperty rdf:about="http://www.sisostds.org/ontologies/C2SIM_SMX_LOX#hasBoundaryProperty">
        <rdfs:subPropertyOf rdf:resource="http://www.w3.org/2002/07/owl#topDataProperty"/>
        <rdfs:range rdf:resource="http://www.sisostds.org/ontologies/C2SIM#UUIDBase"/>
    </owl:DatatypeProperty>
    


    <!-- http://www.sisostds.org/ontologies/C2SIM_SMX_LOX#hasDummyProperty -->

    <owl:DatatypeProperty rdf:about="http://www.sisostds.org/ontologies/C2SIM_SMX_LOX#hasDummyProperty">
        <rdfs:range rdf:resource="http://www.w3.org/2001/XMLSchema#string"/>
    </owl:DatatypeProperty>
    


    <!-- http://www.sisostds.org/ontologies/C2SIM_SMX_LOX#hasDummyProperty2 -->

    <owl:DatatypeProperty rdf:about="http://www.sisostds.org/ontologies/C2SIM_SMX_LOX#hasDummyProperty2">
        <rdfs:range rdf:resource="http://www.w3.org/2001/XMLSchema#boolean"/>
    </owl:DatatypeProperty>
    


    <!-- http://www.sisostds.org/ontologies/C2SIM_SMX_LOX#hasLeapFrogDistance -->

    <owl:DatatypeProperty rdf:about="http://www.sisostds.org/ontologies/C2SIM_SMX_LOX#hasLeapFrogDistance">
        <rdfs:subPropertyOf rdf:resource="http://www.sisostds.org/ontologies/C2SIM#hasDistance"/>
        <rdfs:range rdf:resource="http://www.w3.org/2001/XMLSchema#integer"/>
    </owl:DatatypeProperty>
    


    <!-- http://www.sisostds.org/ontologies/C2SIM_SMX_LOX#hasLeftBoundary -->

    <owl:DatatypeProperty rdf:about="http://www.sisostds.org/ontologies/C2SIM_SMX_LOX#hasLeftBoundary">
        <rdfs:subPropertyOf rdf:resource="http://www.sisostds.org/ontologies/C2SIM_SMX_LOX#hasBoundaryProperty"/>
    </owl:DatatypeProperty>
    


    <!-- http://www.sisostds.org/ontologies/C2SIM_SMX_LOX#hasRightBoundary -->

    <owl:DatatypeProperty rdf:about="http://www.sisostds.org/ontologies/C2SIM_SMX_LOX#hasRightBoundary">
        <rdfs:subPropertyOf rdf:resource="http://www.sisostds.org/ontologies/C2SIM_SMX_LOX#hasBoundaryProperty"/>
    </owl:DatatypeProperty>
    


    <!-- http://www.sisostds.org/ontologies/lox#hasFunctionalAssociationWithTask -->

    <owl:DatatypeProperty rdf:about="http://www.sisostds.org/ontologies/lox#hasFunctionalAssociationWithTask">
        <rdfs:subPropertyOf rdf:resource="http://www.sisostds.org/ontologies/C2SIM#hasTaskReference"/>
        <rdfs:range rdf:resource="http://www.sisostds.org/ontologies/C2SIM#UUIDBase"/>
    </owl:DatatypeProperty>
    


    <!-- http://www.sisostds.org/ontologies/lox#hasPlanPhaseId -->

    <owl:DatatypeProperty rdf:about="http://www.sisostds.org/ontologies/lox#hasPlanPhaseId">
        <rdfs:range rdf:resource="http://www.w3.org/2001/XMLSchema#string"/>
        <rdfs:comment>The unique ID of a PlanPhase.</rdfs:comment>
    </owl:DatatypeProperty>
    


    <!-- http://www.sisostds.org/ontologies/lox#hasPlanPhaseReference -->

    <owl:DatatypeProperty rdf:about="http://www.sisostds.org/ontologies/lox#hasPlanPhaseReference">
        <rdfs:subPropertyOf rdf:resource="http://www.sisostds.org/ontologies/C2SIM#hasReference"/>
        <rdfs:comment>A reference to a plan phase.</rdfs:comment>
    </owl:DatatypeProperty>
    


    <!-- http://www.sisostds.org/ontologies/lox#hasTriggerPhase -->

    <owl:DatatypeProperty rdf:about="http://www.sisostds.org/ontologies/lox#hasTriggerPhase">
        <rdfs:range rdf:resource="http://www.sisostds.org/ontologies/C2SIM#UUIDBase"/>
    </owl:DatatypeProperty>
    


    <!-- http://www.sisostds.org/ontologies/lox#isActive -->

    <owl:DatatypeProperty rdf:about="http://www.sisostds.org/ontologies/lox#isActive">
        <rdfs:range rdf:resource="http://www.w3.org/2001/XMLSchema#boolean"/>
    </owl:DatatypeProperty>
    


    <!-- http://www.sisostds.org/ontologies/lox#isComplete -->

    <owl:DatatypeProperty rdf:about="http://www.sisostds.org/ontologies/lox#isComplete">
        <rdfs:range rdf:resource="http://www.w3.org/2001/XMLSchema#boolean"/>
    </owl:DatatypeProperty>
    


    <!-- http://www.sisostds.org/ontologies/smx#hasConfidenceLevel -->

    <owl:DatatypeProperty rdf:about="http://www.sisostds.org/ontologies/smx#hasConfidenceLevel"/>
    


    <!-- http://www.sisostds.org/ontologies/smx#hasDISCategory -->

    <owl:DatatypeProperty rdf:about="http://www.sisostds.org/ontologies/smx#hasDISCategory">
        <rdfs:subPropertyOf rdf:resource="http://www.sisostds.org/ontologies/smx#hasDISCode"/>
        <rdfs:comment>Values for this property to be taken from the DIS standard, SISO-REF-010-2015</rdfs:comment>
    </owl:DatatypeProperty>
    


    <!-- http://www.sisostds.org/ontologies/smx#hasDISCode -->

    <owl:DatatypeProperty rdf:about="http://www.sisostds.org/ontologies/smx#hasDISCode">
        <rdfs:range rdf:resource="http://www.w3.org/2001/XMLSchema#string"/>
    </owl:DatatypeProperty>
    


    <!-- http://www.sisostds.org/ontologies/smx#hasDISExtra -->

    <owl:DatatypeProperty rdf:about="http://www.sisostds.org/ontologies/smx#hasDISExtra">
        <rdfs:subPropertyOf rdf:resource="http://www.sisostds.org/ontologies/smx#hasDISCode"/>
        <rdfs:comment>Values for this property to be taken from the DIS standard, SISO-REF-010-2015</rdfs:comment>
    </owl:DatatypeProperty>
    


    <!-- http://www.sisostds.org/ontologies/smx#hasDISSpecific -->

    <owl:DatatypeProperty rdf:about="http://www.sisostds.org/ontologies/smx#hasDISSpecific">
        <rdfs:subPropertyOf rdf:resource="http://www.sisostds.org/ontologies/smx#hasDISCode"/>
        <rdfs:comment>Values for this property to be taken from the DIS standard, SISO-REF-010-2015</rdfs:comment>
    </owl:DatatypeProperty>
    


    <!-- http://www.sisostds.org/ontologies/smx#hasDISSubCategory -->

    <owl:DatatypeProperty rdf:about="http://www.sisostds.org/ontologies/smx#hasDISSubCategory">
        <rdfs:subPropertyOf rdf:resource="http://www.sisostds.org/ontologies/smx#hasDISCode"/>
        <rdfs:comment>Values for this property to be taken from the DIS standard, SISO-REF-010-2015</rdfs:comment>
    </owl:DatatypeProperty>
    


    <!-- http://www.sisostds.org/ontologies/smx#hasEchelon -->

    <owl:DatatypeProperty rdf:about="http://www.sisostds.org/ontologies/smx#hasEchelon"/>
    


    <!-- http://www.sisostds.org/ontologies/smx#hasHigherFormation -->

    <owl:DatatypeProperty rdf:about="http://www.sisostds.org/ontologies/smx#hasHigherFormation"/>
    


    <!-- http://www.sisostds.org/ontologies/smx#hasObservationSubject -->

    <owl:DatatypeProperty rdf:about="http://www.sisostds.org/ontologies/smx#hasObservationSubject">
        <rdfs:subPropertyOf rdf:resource="http://www.sisostds.org/ontologies/C2SIM#hasActorReference"/>
    </owl:DatatypeProperty>
    


    <!-- http://www.sisostds.org/ontologies/smx#hasOwner -->

    <owl:DatatypeProperty rdf:about="http://www.sisostds.org/ontologies/smx#hasOwner">
        <rdfs:subPropertyOf rdf:resource="http://www.sisostds.org/ontologies/C2SIM#hasAbstractObjectReference"/>
        <rdfs:range rdf:resource="http://www.sisostds.org/ontologies/C2SIM#UUIDBase"/>
    </owl:DatatypeProperty>
    


    <!-- http://www.sisostds.org/ontologies/smx#hasSIDCString -->

    <owl:DatatypeProperty rdf:about="http://www.sisostds.org/ontologies/smx#hasSIDCString"/>
    


    <!-- http://www.sisostds.org/ontologies/smx#hasSide -->

    <owl:DatatypeProperty rdf:about="http://www.sisostds.org/ontologies/smx#hasSide">
        <rdfs:subPropertyOf rdf:resource="http://www.sisostds.org/ontologies/C2SIM#hasAbstractObjectReference"/>
        <rdfs:range rdf:resource="http://www.sisostds.org/ontologies/C2SIM#UUIDBase"/>
    </owl:DatatypeProperty>
    


    <!-- http://www.sisostds.org/ontologies/smx#hasSpecialC2HQ -->

    <owl:DatatypeProperty rdf:about="http://www.sisostds.org/ontologies/smx#hasSpecialC2HQ"/>
    


    <!-- http://www.sisostds.org/ontologies/smx#hasUncertaintyInterval -->

    <owl:DatatypeProperty rdf:about="http://www.sisostds.org/ontologies/smx#hasUncertaintyInterval"/>
    


    <!-- 
    ///////////////////////////////////////////////////////////////////////////////////////
    //
    // Classes
    //
    ///////////////////////////////////////////////////////////////////////////////////////
     -->

    


    <!-- http://www.co-ode.org/ontologies/ont.owl#Line -->

    <owl:Class rdf:about="http://www.co-ode.org/ontologies/ont.owl#Line">
        <rdfs:subClassOf rdf:resource="http://www.sisostds.org/ontologies/smx#TacticalGraphic"/>
        <rdfs:subClassOf>
            <owl:Restriction>
                <owl:onProperty rdf:resource="http://www.sisostds.org/ontologies/C2SIM_SMX_LOX#hasDummyProperty2"/>
                <owl:minQualifiedCardinality rdf:datatype="http://www.w3.org/2001/XMLSchema#nonNegativeInteger">0</owl:minQualifiedCardinality>
                <owl:onDataRange rdf:resource="http://www.w3.org/2001/XMLSchema#boolean"/>
            </owl:Restriction>
        </rdfs:subClassOf>
    </owl:Class>
    


    <!-- http://www.co-ode.org/ontologies/ont.owl#NBC_Event -->

    <owl:Class rdf:about="http://www.co-ode.org/ontologies/ont.owl#NBC_Event">
        <rdfs:subClassOf rdf:resource="http://www.sisostds.org/ontologies/smx#TacticalGraphic"/>
    </owl:Class>
    


    <!-- http://www.co-ode.org/ontologies/ont.owl#Point -->

    <owl:Class rdf:about="http://www.co-ode.org/ontologies/ont.owl#Point">
        <rdfs:subClassOf rdf:resource="http://www.sisostds.org/ontologies/smx#TacticalGraphic"/>
    </owl:Class>
    


    <!-- http://www.co-ode.org/ontologies/ont.owl#TacticalArea -->

    <owl:Class rdf:about="http://www.co-ode.org/ontologies/ont.owl#TacticalArea">
        <rdfs:subClassOf rdf:resource="http://www.sisostds.org/ontologies/smx#TacticalGraphic"/>
    </owl:Class>
    


    <!-- http://www.co-ode.org/ontologies/ont.owl#TaskGraphic -->

    <owl:Class rdf:about="http://www.co-ode.org/ontologies/ont.owl#TaskGraphic">
        <rdfs:subClassOf rdf:resource="http://www.sisostds.org/ontologies/smx#TacticalGraphic"/>
    </owl:Class>
    


    <!-- http://www.sisostds.org/ontologies/C2SIM#AbstractObject -->

    <owl:Class rdf:about="http://www.sisostds.org/ontologies/C2SIM#AbstractObject">
        <rdfs:subClassOf rdf:resource="http://www.sisostds.org/ontologies/C2SIM#C2SIMContent"/>
        <rdfs:subClassOf>
            <owl:Restriction>
                <owl:onProperty rdf:resource="http://www.sisostds.org/ontologies/C2SIM#hasName"/>
                <owl:minQualifiedCardinality rdf:datatype="http://www.w3.org/2001/XMLSchema#nonNegativeInteger">0</owl:minQualifiedCardinality>
                <owl:onDataRange rdf:resource="http://www.w3.org/2001/XMLSchema#string"/>
            </owl:Restriction>
        </rdfs:subClassOf>
        <rdfs:subClassOf>
            <owl:Restriction>
                <owl:onProperty rdf:resource="http://www.sisostds.org/ontologies/C2SIM#hasUUID"/>
                <owl:qualifiedCardinality rdf:datatype="http://www.w3.org/2001/XMLSchema#nonNegativeInteger">1</owl:qualifiedCardinality>
                <owl:onDataRange rdf:resource="http://www.sisostds.org/ontologies/C2SIM#UUIDBase"/>
            </owl:Restriction>
        </rdfs:subClassOf>
        <rdfs:comment>An AbstractObject is an object in the system that does not have the full characteristics of an entity. For example, it does not have a location or an extent. It does however have a unique identifier.</rdfs:comment>
    </owl:Class>
    


    <!-- http://www.sisostds.org/ontologies/C2SIM#AbstractOrganization -->

    <owl:Class rdf:about="http://www.sisostds.org/ontologies/C2SIM#AbstractOrganization">
        <rdfs:subClassOf rdf:resource="http://www.sisostds.org/ontologies/C2SIM#AbstractObject"/>
        <rdfs:subClassOf>
            <owl:Restriction>
                <owl:onProperty rdf:resource="http://www.sisostds.org/ontologies/C2SIM#hasCountryCode"/>
                <owl:maxQualifiedCardinality rdf:datatype="http://www.w3.org/2001/XMLSchema#nonNegativeInteger">1</owl:maxQualifiedCardinality>
                <owl:onClass rdf:resource="http://www.sisostds.org/ontologies/C2SIM#CountryCode"/>
            </owl:Restriction>
        </rdfs:subClassOf>
        <rdfs:subClassOf>
            <owl:Restriction>
                <owl:onProperty rdf:resource="http://www.sisostds.org/ontologies/C2SIM#hasEthnicGroupCode"/>
                <owl:maxQualifiedCardinality rdf:datatype="http://www.w3.org/2001/XMLSchema#nonNegativeInteger">1</owl:maxQualifiedCardinality>
                <owl:onClass rdf:resource="http://www.sisostds.org/ontologies/C2SIM#EthnicGroupCode"/>
            </owl:Restriction>
        </rdfs:subClassOf>
        <rdfs:subClassOf>
            <owl:Restriction>
                <owl:onProperty rdf:resource="http://www.sisostds.org/ontologies/C2SIM#hasReligiousOrganizationCode"/>
                <owl:maxQualifiedCardinality rdf:datatype="http://www.w3.org/2001/XMLSchema#nonNegativeInteger">1</owl:maxQualifiedCardinality>
                <owl:onClass rdf:resource="http://www.sisostds.org/ontologies/C2SIM#ReligiousOrganizationCode"/>
            </owl:Restriction>
        </rdfs:subClassOf>
        <rdfs:comment>A group that an actor can be affiliated with. Does not perform any actions and does not have a specific location.
Subclasses of this class can be created for country, religion, etc. Each of these will have defined instances (one for each country, etc.)</rdfs:comment>
    </owl:Class>
    


    <!-- http://www.sisostds.org/ontologies/C2SIM#AcknowledgeTypeCode -->

    <owl:Class rdf:about="http://www.sisostds.org/ontologies/C2SIM#AcknowledgeTypeCode">
        <rdfs:subClassOf rdf:resource="http://www.sisostds.org/ontologies/C2SIM#MessageCode"/>
        <rdfs:comment>Enumeration of different types of acknowledgements.</rdfs:comment>
    </owl:Class>
    


    <!-- http://www.sisostds.org/ontologies/C2SIM#AcknowledgementBody -->

    <owl:Class rdf:about="http://www.sisostds.org/ontologies/C2SIM#AcknowledgementBody">
        <rdfs:subClassOf rdf:resource="http://www.sisostds.org/ontologies/C2SIM#MessageBody"/>
        <rdfs:subClassOf>
            <owl:Restriction>
                <owl:onProperty rdf:resource="http://www.sisostds.org/ontologies/C2SIM#hasAcknowledgeTypeCode"/>
                <owl:qualifiedCardinality rdf:datatype="http://www.w3.org/2001/XMLSchema#nonNegativeInteger">1</owl:qualifiedCardinality>
                <owl:onClass rdf:resource="http://www.sisostds.org/ontologies/C2SIM#AcknowledgeTypeCode"/>
            </owl:Restriction>
        </rdfs:subClassOf>
        <rdfs:subClassOf>
            <owl:Restriction>
                <owl:onProperty rdf:resource="http://www.sisostds.org/ontologies/C2SIM#hasComment"/>
                <owl:maxQualifiedCardinality rdf:datatype="http://www.w3.org/2001/XMLSchema#nonNegativeInteger">1</owl:maxQualifiedCardinality>
                <owl:onDataRange rdf:resource="http://www.w3.org/2001/XMLSchema#string"/>
            </owl:Restriction>
        </rdfs:subClassOf>
        <rdfs:comment>The structure for sending acknowledgement messages.</rdfs:comment>
    </owl:Class>
    


    <!-- http://www.sisostds.org/ontologies/C2SIM#Action -->

    <owl:Class rdf:about="http://www.sisostds.org/ontologies/C2SIM#Action">
        <rdfs:subClassOf rdf:resource="http://www.sisostds.org/ontologies/C2SIM#C2SIMContent"/>
        <rdfs:subClassOf>
            <owl:Restriction>
                <owl:onProperty rdf:resource="http://www.sisostds.org/ontologies/C2SIM#hasLocation"/>
                <owl:minQualifiedCardinality rdf:datatype="http://www.w3.org/2001/XMLSchema#nonNegativeInteger">0</owl:minQualifiedCardinality>
                <owl:onClass rdf:resource="http://www.sisostds.org/ontologies/C2SIM#Location"/>
            </owl:Restriction>
        </rdfs:subClassOf>
        <rdfs:subClassOf>
            <owl:Restriction>
                <owl:onProperty rdf:resource="http://www.sisostds.org/ontologies/C2SIM#hasMapGraphicID"/>
                <owl:minQualifiedCardinality rdf:datatype="http://www.w3.org/2001/XMLSchema#nonNegativeInteger">0</owl:minQualifiedCardinality>
                <owl:onDataRange rdf:resource="http://www.sisostds.org/ontologies/C2SIM#UUIDBase"/>
            </owl:Restriction>
        </rdfs:subClassOf>
        <rdfs:subClassOf>
            <owl:Restriction>
                <owl:onProperty rdf:resource="http://www.sisostds.org/ontologies/C2SIM#hasUUID"/>
                <owl:qualifiedCardinality rdf:datatype="http://www.w3.org/2001/XMLSchema#nonNegativeInteger">1</owl:qualifiedCardinality>
                <owl:onDataRange rdf:resource="http://www.sisostds.org/ontologies/C2SIM#UUIDBase"/>
            </owl:Restriction>
        </rdfs:subClassOf>
        <rdfs:subClassOf>
            <owl:Restriction>
                <owl:onProperty rdf:resource="http://www.sisostds.org/ontologies/C2SIM#hasName"/>
                <owl:maxQualifiedCardinality rdf:datatype="http://www.w3.org/2001/XMLSchema#nonNegativeInteger">1</owl:maxQualifiedCardinality>
                <owl:onDataRange rdf:resource="http://www.w3.org/2001/XMLSchema#string"/>
            </owl:Restriction>
        </rdfs:subClassOf>
        <rdfs:comment>Any occurrence that occurs at a moment in time or over a period of time.</rdfs:comment>
    </owl:Class>
    <owl:Axiom>
        <owl:annotatedSource rdf:resource="http://www.sisostds.org/ontologies/C2SIM#Action"/>
        <owl:annotatedProperty rdf:resource="http://www.w3.org/2000/01/rdf-schema#subClassOf"/>
        <owl:annotatedTarget>
            <owl:Restriction>
                <owl:onProperty rdf:resource="http://www.sisostds.org/ontologies/C2SIM#hasLocation"/>
                <owl:minQualifiedCardinality rdf:datatype="http://www.w3.org/2001/XMLSchema#nonNegativeInteger">0</owl:minQualifiedCardinality>
                <owl:onClass rdf:resource="http://www.sisostds.org/ontologies/C2SIM#Location"/>
            </owl:Restriction>
        </owl:annotatedTarget>
        <rdfs:comment>The general location of the task, if that makes sense. Specification of multiple locations where events of the task take place is normally done with map graphics.</rdfs:comment>
    </owl:Axiom>
    


    <!-- http://www.sisostds.org/ontologies/C2SIM#ActionCode -->

    <owl:Class rdf:about="http://www.sisostds.org/ontologies/C2SIM#ActionCode">
        <rdfs:subClassOf rdf:resource="http://www.sisostds.org/ontologies/C2SIM#Code"/>
        <rdfs:comment>An enumeration describing what the action is.</rdfs:comment>
    </owl:Class>
    


    <!-- http://www.sisostds.org/ontologies/C2SIM#ActorEntity -->

    <owl:Class rdf:about="http://www.sisostds.org/ontologies/C2SIM#ActorEntity">
        <rdfs:subClassOf rdf:resource="http://www.sisostds.org/ontologies/C2SIM#Entity"/>
        <rdfs:subClassOf>
            <owl:Restriction>
                <owl:onProperty rdf:resource="http://www.sisostds.org/ontologies/C2SIM#hasResource"/>
                <owl:minQualifiedCardinality rdf:datatype="http://www.w3.org/2001/XMLSchema#nonNegativeInteger">0</owl:minQualifiedCardinality>
                <owl:onClass rdf:resource="http://www.sisostds.org/ontologies/C2SIM#Resource"/>
            </owl:Restriction>
        </rdfs:subClassOf>
        <rdfs:subClassOf>
            <owl:Restriction>
                <owl:onProperty rdf:resource="http://www.sisostds.org/ontologies/C2SIM#hasEntityDescriptor"/>
                <owl:qualifiedCardinality rdf:datatype="http://www.w3.org/2001/XMLSchema#nonNegativeInteger">1</owl:qualifiedCardinality>
                <owl:onClass rdf:resource="http://www.sisostds.org/ontologies/C2SIM#EntityDescriptor"/>
            </owl:Restriction>
        </rdfs:subClassOf>
        <rdfs:subClassOf>
            <owl:Restriction>
                <owl:onProperty rdf:resource="http://www.sisostds.org/ontologies/C2SIM#hasCurrentTask"/>
                <owl:minQualifiedCardinality rdf:datatype="http://www.w3.org/2001/XMLSchema#nonNegativeInteger">0</owl:minQualifiedCardinality>
                <owl:onDataRange rdf:resource="http://www.sisostds.org/ontologies/C2SIM#UUIDBase"/>
            </owl:Restriction>
        </rdfs:subClassOf>
        <rdfs:comment>An ActorEntity is an entity that can send/receive orders and reports and/or perform tasks.</rdfs:comment>
    </owl:Class>
    


    <!-- http://www.sisostds.org/ontologies/C2SIM#BoundingBox -->

    <owl:Class rdf:about="http://www.sisostds.org/ontologies/C2SIM#BoundingBox">
        <rdfs:subClassOf rdf:resource="http://www.sisostds.org/ontologies/C2SIM#PhysicalExtent"/>
        <rdfs:subClassOf>
            <owl:Restriction>
                <owl:onProperty rdf:resource="http://www.sisostds.org/ontologies/C2SIM#hasLength"/>
                <owl:qualifiedCardinality rdf:datatype="http://www.w3.org/2001/XMLSchema#nonNegativeInteger">1</owl:qualifiedCardinality>
                <owl:onDataRange rdf:resource="http://www.w3.org/2001/XMLSchema#double"/>
            </owl:Restriction>
        </rdfs:subClassOf>
        <rdfs:subClassOf>
            <owl:Restriction>
                <owl:onProperty rdf:resource="http://www.sisostds.org/ontologies/C2SIM#hasWidth"/>
                <owl:qualifiedCardinality rdf:datatype="http://www.w3.org/2001/XMLSchema#nonNegativeInteger">1</owl:qualifiedCardinality>
                <owl:onDataRange rdf:resource="http://www.w3.org/2001/XMLSchema#double"/>
            </owl:Restriction>
        </rdfs:subClassOf>
        <owl:disjointWith rdf:resource="http://www.sisostds.org/ontologies/C2SIM#BoundingVolume"/>
        <rdfs:comment>A rectangle in 2D space containing the two-dimensional extent of an entity.</rdfs:comment>
    </owl:Class>
    


    <!-- http://www.sisostds.org/ontologies/C2SIM#BoundingVolume -->

    <owl:Class rdf:about="http://www.sisostds.org/ontologies/C2SIM#BoundingVolume">
        <rdfs:subClassOf rdf:resource="http://www.sisostds.org/ontologies/C2SIM#PhysicalExtent"/>
        <rdfs:subClassOf>
            <owl:Restriction>
                <owl:onProperty rdf:resource="http://www.sisostds.org/ontologies/C2SIM#hasHeight"/>
                <owl:qualifiedCardinality rdf:datatype="http://www.w3.org/2001/XMLSchema#nonNegativeInteger">1</owl:qualifiedCardinality>
                <owl:onDataRange rdf:resource="http://www.w3.org/2001/XMLSchema#double"/>
            </owl:Restriction>
        </rdfs:subClassOf>
        <rdfs:subClassOf>
            <owl:Restriction>
                <owl:onProperty rdf:resource="http://www.sisostds.org/ontologies/C2SIM#hasLength"/>
                <owl:qualifiedCardinality rdf:datatype="http://www.w3.org/2001/XMLSchema#nonNegativeInteger">1</owl:qualifiedCardinality>
                <owl:onDataRange rdf:resource="http://www.w3.org/2001/XMLSchema#double"/>
            </owl:Restriction>
        </rdfs:subClassOf>
        <rdfs:subClassOf>
            <owl:Restriction>
                <owl:onProperty rdf:resource="http://www.sisostds.org/ontologies/C2SIM#hasWidth"/>
                <owl:qualifiedCardinality rdf:datatype="http://www.w3.org/2001/XMLSchema#nonNegativeInteger">1</owl:qualifiedCardinality>
                <owl:onDataRange rdf:resource="http://www.w3.org/2001/XMLSchema#double"/>
            </owl:Restriction>
        </rdfs:subClassOf>
        <rdfs:comment>A rectangular volume of 3D space containing the physical extend of an entity.</rdfs:comment>
    </owl:Class>
    


    <!-- http://www.sisostds.org/ontologies/C2SIM#C2SIMContent -->

    <owl:Class rdf:about="http://www.sisostds.org/ontologies/C2SIM#C2SIMContent">
        <rdfs:comment>Class of all concepts for the content of messages in the core C2SIM data model.</rdfs:comment>
    </owl:Class>
    


    <!-- http://www.sisostds.org/ontologies/C2SIM#C2SIMHeader -->

    <owl:Class rdf:about="http://www.sisostds.org/ontologies/C2SIM#C2SIMHeader">
        <rdfs:subClassOf rdf:resource="http://www.sisostds.org/ontologies/C2SIM#MessageConcept"/>
        <rdfs:subClassOf>
            <owl:Restriction>
                <owl:onProperty rdf:resource="http://www.sisostds.org/ontologies/C2SIM#hasCommunicativeActTypeCode"/>
                <owl:qualifiedCardinality rdf:datatype="http://www.w3.org/2001/XMLSchema#nonNegativeInteger">1</owl:qualifiedCardinality>
                <owl:onClass rdf:resource="http://www.sisostds.org/ontologies/C2SIM#CommunicativeActTypeCode"/>
            </owl:Restriction>
        </rdfs:subClassOf>
        <rdfs:subClassOf>
            <owl:Restriction>
                <owl:onProperty rdf:resource="http://www.sisostds.org/ontologies/C2SIM#hasSecurityClassificationCode"/>
                <owl:maxQualifiedCardinality rdf:datatype="http://www.w3.org/2001/XMLSchema#nonNegativeInteger">1</owl:maxQualifiedCardinality>
                <owl:onClass rdf:resource="http://www.sisostds.org/ontologies/C2SIM#SecurityClassificationCode"/>
            </owl:Restriction>
        </rdfs:subClassOf>
        <rdfs:subClassOf>
            <owl:Restriction>
                <owl:onProperty rdf:resource="http://www.sisostds.org/ontologies/C2SIM#hasConversationID"/>
                <owl:qualifiedCardinality rdf:datatype="http://www.w3.org/2001/XMLSchema#nonNegativeInteger">1</owl:qualifiedCardinality>
                <owl:onDataRange rdf:resource="http://www.sisostds.org/ontologies/C2SIM#UUIDBase"/>
            </owl:Restriction>
        </rdfs:subClassOf>
        <rdfs:subClassOf>
            <owl:Restriction>
                <owl:onProperty rdf:resource="http://www.sisostds.org/ontologies/C2SIM#hasMessageID"/>
                <owl:qualifiedCardinality rdf:datatype="http://www.w3.org/2001/XMLSchema#nonNegativeInteger">1</owl:qualifiedCardinality>
                <owl:onDataRange rdf:resource="http://www.sisostds.org/ontologies/C2SIM#UUIDBase"/>
            </owl:Restriction>
        </rdfs:subClassOf>
        <rdfs:subClassOf>
            <owl:Restriction>
                <owl:onProperty rdf:resource="http://www.sisostds.org/ontologies/C2SIM#hasProtocol"/>
                <owl:qualifiedCardinality rdf:datatype="http://www.w3.org/2001/XMLSchema#nonNegativeInteger">1</owl:qualifiedCardinality>
                <owl:onDataRange rdf:resource="http://www.w3.org/2001/XMLSchema#string"/>
            </owl:Restriction>
        </rdfs:subClassOf>
        <rdfs:subClassOf>
            <owl:Restriction>
                <owl:onProperty rdf:resource="http://www.sisostds.org/ontologies/C2SIM#hasProtocolVersion"/>
                <owl:qualifiedCardinality rdf:datatype="http://www.w3.org/2001/XMLSchema#nonNegativeInteger">1</owl:qualifiedCardinality>
                <owl:onDataRange rdf:resource="http://www.w3.org/2001/XMLSchema#string"/>
            </owl:Restriction>
        </rdfs:subClassOf>
        <rdfs:subClassOf>
            <owl:Restriction>
                <owl:onProperty rdf:resource="http://www.sisostds.org/ontologies/C2SIM#hasSendingTime"/>
                <owl:qualifiedCardinality rdf:datatype="http://www.w3.org/2001/XMLSchema#nonNegativeInteger">1</owl:qualifiedCardinality>
                <owl:onDataRange rdf:resource="http://www.sisostds.org/ontologies/C2SIM#IsoDateTimeBase"/>
            </owl:Restriction>
        </rdfs:subClassOf>
        <rdfs:subClassOf>
            <owl:Restriction>
                <owl:onProperty rdf:resource="http://www.sisostds.org/ontologies/C2SIM#isFromSendingSystem"/>
                <owl:qualifiedCardinality rdf:datatype="http://www.w3.org/2001/XMLSchema#nonNegativeInteger">1</owl:qualifiedCardinality>
                <owl:onDataRange rdf:resource="http://www.w3.org/2001/XMLSchema#string"/>
            </owl:Restriction>
        </rdfs:subClassOf>
        <rdfs:subClassOf>
            <owl:Restriction>
                <owl:onProperty rdf:resource="http://www.sisostds.org/ontologies/C2SIM#isToReceivingSystem"/>
                <owl:qualifiedCardinality rdf:datatype="http://www.w3.org/2001/XMLSchema#nonNegativeInteger">1</owl:qualifiedCardinality>
                <owl:onDataRange rdf:resource="http://www.w3.org/2001/XMLSchema#string"/>
            </owl:Restriction>
        </rdfs:subClassOf>
        <rdfs:subClassOf>
            <owl:Restriction>
                <owl:onProperty rdf:resource="http://www.sisostds.org/ontologies/C2SIM#hasReplyToSystem"/>
                <owl:maxQualifiedCardinality rdf:datatype="http://www.w3.org/2001/XMLSchema#nonNegativeInteger">1</owl:maxQualifiedCardinality>
                <owl:onDataRange rdf:resource="http://www.w3.org/2001/XMLSchema#string"/>
            </owl:Restriction>
        </rdfs:subClassOf>
        <rdfs:subClassOf>
            <owl:Restriction>
                <owl:onProperty rdf:resource="http://www.sisostds.org/ontologies/C2SIM#isInReplyToMessageID"/>
                <owl:maxQualifiedCardinality rdf:datatype="http://www.w3.org/2001/XMLSchema#nonNegativeInteger">1</owl:maxQualifiedCardinality>
                <owl:onDataRange rdf:resource="http://www.sisostds.org/ontologies/C2SIM#UUIDBase"/>
            </owl:Restriction>
        </rdfs:subClassOf>
        <rdfs:comment>Indicates that the receiving system should submit its initialization data to the system identified in the</rdfs:comment>
    </owl:Class>
    


    <!-- http://www.sisostds.org/ontologies/C2SIM#C2SIMInitializationBody -->

    <owl:Class rdf:about="http://www.sisostds.org/ontologies/C2SIM#C2SIMInitializationBody">
        <rdfs:subClassOf rdf:resource="http://www.sisostds.org/ontologies/C2SIM#MessageBody"/>
        <rdfs:subClassOf>
            <owl:Restriction>
                <owl:onProperty rdf:resource="http://www.sisostds.org/ontologies/C2SIM#hasInitializationDataFile"/>
                <owl:minQualifiedCardinality rdf:datatype="http://www.w3.org/2001/XMLSchema#nonNegativeInteger">0</owl:minQualifiedCardinality>
                <owl:onClass rdf:resource="http://www.sisostds.org/ontologies/C2SIM#InitializationDataFile"/>
            </owl:Restriction>
        </rdfs:subClassOf>
        <rdfs:subClassOf>
            <owl:Restriction>
                <owl:onProperty rdf:resource="http://www.sisostds.org/ontologies/C2SIM#hasObjectDefinitions"/>
                <owl:minQualifiedCardinality rdf:datatype="http://www.w3.org/2001/XMLSchema#nonNegativeInteger">1</owl:minQualifiedCardinality>
                <owl:onClass rdf:resource="http://www.sisostds.org/ontologies/C2SIM#ObjectDefinitions"/>
            </owl:Restriction>
        </rdfs:subClassOf>
        <rdfs:subClassOf>
            <owl:Restriction>
                <owl:onProperty rdf:resource="http://www.sisostds.org/ontologies/C2SIM#hasSystemEntityList"/>
                <owl:minQualifiedCardinality rdf:datatype="http://www.w3.org/2001/XMLSchema#nonNegativeInteger">1</owl:minQualifiedCardinality>
                <owl:onClass rdf:resource="http://www.sisostds.org/ontologies/C2SIM#SystemEntityList"/>
            </owl:Restriction>
        </rdfs:subClassOf>
        <rdfs:subClassOf>
            <owl:Restriction>
                <owl:onProperty rdf:resource="http://www.sisostds.org/ontologies/C2SIM#hasScenarioSetting"/>
                <owl:qualifiedCardinality rdf:datatype="http://www.w3.org/2001/XMLSchema#nonNegativeInteger">1</owl:qualifiedCardinality>
                <owl:onClass rdf:resource="http://www.sisostds.org/ontologies/C2SIM#ScenarioSetting"/>
            </owl:Restriction>
        </rdfs:subClassOf>
        <rdfs:comment>This message can initialize all of the objects in the scenario as well as the scenario setting.</rdfs:comment>
    </owl:Class>
    


    <!-- http://www.sisostds.org/ontologies/C2SIM#CartesianOffset -->

    <owl:Class rdf:about="http://www.sisostds.org/ontologies/C2SIM#CartesianOffset">
        <rdfs:subClassOf rdf:resource="http://www.sisostds.org/ontologies/C2SIM#SpatialOffset"/>
        <rdfs:subClassOf>
            <owl:Restriction>
                <owl:onProperty rdf:resource="http://www.sisostds.org/ontologies/C2SIM#hasX"/>
                <owl:qualifiedCardinality rdf:datatype="http://www.w3.org/2001/XMLSchema#nonNegativeInteger">1</owl:qualifiedCardinality>
                <owl:onDataRange rdf:resource="http://www.w3.org/2001/XMLSchema#double"/>
            </owl:Restriction>
        </rdfs:subClassOf>
        <rdfs:subClassOf>
            <owl:Restriction>
                <owl:onProperty rdf:resource="http://www.sisostds.org/ontologies/C2SIM#hasY"/>
                <owl:qualifiedCardinality rdf:datatype="http://www.w3.org/2001/XMLSchema#nonNegativeInteger">1</owl:qualifiedCardinality>
                <owl:onDataRange rdf:resource="http://www.w3.org/2001/XMLSchema#double"/>
            </owl:Restriction>
        </rdfs:subClassOf>
        <rdfs:subClassOf>
            <owl:Restriction>
                <owl:onProperty rdf:resource="http://www.sisostds.org/ontologies/C2SIM#hasZ"/>
                <owl:qualifiedCardinality rdf:datatype="http://www.w3.org/2001/XMLSchema#nonNegativeInteger">1</owl:qualifiedCardinality>
                <owl:onDataRange rdf:resource="http://www.w3.org/2001/XMLSchema#double"/>
            </owl:Restriction>
        </rdfs:subClassOf>
        <rdfs:comment>A spatial offset expressed in geocentric coordinates.</rdfs:comment>
    </owl:Class>
    


    <!-- http://www.sisostds.org/ontologies/C2SIM#Code -->

    <owl:Class rdf:about="http://www.sisostds.org/ontologies/C2SIM#Code">
        <rdfs:subClassOf rdf:resource="http://www.sisostds.org/ontologies/C2SIM#C2SIMContent"/>
        <rdfs:comment>A collection of enumerations used by various data types in C2SIM</rdfs:comment>
    </owl:Class>
    


    <!-- http://www.sisostds.org/ontologies/C2SIM#CollectiveEntity -->

    <owl:Class rdf:about="http://www.sisostds.org/ontologies/C2SIM#CollectiveEntity">
        <rdfs:subClassOf rdf:resource="http://www.sisostds.org/ontologies/C2SIM#ActorEntity"/>
        <rdfs:subClassOf>
            <owl:Restriction>
                <owl:onProperty rdf:resource="http://www.sisostds.org/ontologies/C2SIM#hasCurrentState"/>
                <owl:maxQualifiedCardinality rdf:datatype="http://www.w3.org/2001/XMLSchema#nonNegativeInteger">1</owl:maxQualifiedCardinality>
                <owl:onClass rdf:resource="http://www.sisostds.org/ontologies/C2SIM#PhysicalState"/>
            </owl:Restriction>
        </rdfs:subClassOf>
        <rdfs:subClassOf>
            <owl:Restriction>
                <owl:onProperty rdf:resource="http://www.sisostds.org/ontologies/C2SIM#hasSubordinate"/>
                <owl:minQualifiedCardinality rdf:datatype="http://www.w3.org/2001/XMLSchema#nonNegativeInteger">0</owl:minQualifiedCardinality>
                <owl:onDataRange rdf:resource="http://www.sisostds.org/ontologies/C2SIM#UUIDBase"/>
            </owl:Restriction>
        </rdfs:subClassOf>
        <rdfs:comment>This is an Entity that is normally thought of as having constituent entities, i.e. a Unit.

CollectiveEntities may or may not hve their subordinates explicitly represented in the exercise (i.e., it may always be aggregated, or it may have subordinates that are themselves entities).  If they are represented, then the hasSubordinate property will have at least one instance.

The CollectivEntity may be an abstract actor, or it may have physical properties; if the latter, then the hasCurrentState property is present with a PhysicalState.</rdfs:comment>
    </owl:Class>
    


    <!-- http://www.sisostds.org/ontologies/C2SIM#CommunicationDevice -->

    <owl:Class rdf:about="http://www.sisostds.org/ontologies/C2SIM#CommunicationDevice">
        <rdfs:subClassOf rdf:resource="http://www.sisostds.org/ontologies/C2SIM#Equipment"/>
        <rdfs:comment>For example, radios.</rdfs:comment>
    </owl:Class>
    


    <!-- http://www.sisostds.org/ontologies/C2SIM#CommunicationNetwork -->

    <owl:Class rdf:about="http://www.sisostds.org/ontologies/C2SIM#CommunicationNetwork">
        <rdfs:subClassOf rdf:resource="http://www.sisostds.org/ontologies/C2SIM#AbstractObject"/>
        <rdfs:comment>An specific network over which an entity communicates. A logical entity. Will have data properties defining communication parameters.</rdfs:comment>
    </owl:Class>
    


    <!-- http://www.sisostds.org/ontologies/C2SIM#CommunicativeActTypeCode -->

    <owl:Class rdf:about="http://www.sisostds.org/ontologies/C2SIM#CommunicativeActTypeCode">
        <rdfs:subClassOf rdf:resource="http://www.sisostds.org/ontologies/C2SIM#MessageCode"/>
        <rdfs:comment>Enumeration of different types of communications.</rdfs:comment>
    </owl:Class>
    


    <!-- http://www.sisostds.org/ontologies/C2SIM#ConsumableMaterial -->

    <owl:Class rdf:about="http://www.sisostds.org/ontologies/C2SIM#ConsumableMaterial">
        <rdfs:subClassOf rdf:resource="http://www.sisostds.org/ontologies/C2SIM#Resource"/>
        <rdfs:comment>Physical assets that are significant to the exercise but that are inanimate and do not perform actions by themselves. They are consumable resources, such as food or ammunition.</rdfs:comment>
    </owl:Class>
    


    <!-- http://www.sisostds.org/ontologies/C2SIM#Coordinate -->

    <owl:Class rdf:about="http://www.sisostds.org/ontologies/C2SIM#Coordinate">
        <rdfs:subClassOf rdf:resource="http://www.sisostds.org/ontologies/C2SIM#Location"/>
    </owl:Class>
    


    <!-- http://www.sisostds.org/ontologies/C2SIM#CountryCode -->

    <owl:Class rdf:about="http://www.sisostds.org/ontologies/C2SIM#CountryCode">
        <rdfs:subClassOf rdf:resource="http://www.sisostds.org/ontologies/C2SIM#OrganizationCode"/>
    </owl:Class>
    


    <!-- http://www.sisostds.org/ontologies/C2SIM#CulturalFeature -->

    <owl:Class rdf:about="http://www.sisostds.org/ontologies/C2SIM#CulturalFeature">
        <rdfs:subClassOf rdf:resource="http://www.sisostds.org/ontologies/C2SIM#PhysicalEntity"/>
        <rdfs:subClassOf>
            <owl:Restriction>
                <owl:onProperty rdf:resource="http://www.sisostds.org/ontologies/C2SIM#hasConsumableMaterial"/>
                <owl:minQualifiedCardinality rdf:datatype="http://www.w3.org/2001/XMLSchema#nonNegativeInteger">0</owl:minQualifiedCardinality>
                <owl:onClass rdf:resource="http://www.sisostds.org/ontologies/C2SIM#ConsumableMaterial"/>
            </owl:Restriction>
        </rdfs:subClassOf>
        <rdfs:comment>Any man-made feature in the environment</rdfs:comment>
    </owl:Class>
    


    <!-- http://www.sisostds.org/ontologies/C2SIM#DateTime -->

    <owl:Class rdf:about="http://www.sisostds.org/ontologies/C2SIM#DateTime">
        <rdfs:subClassOf rdf:resource="http://www.sisostds.org/ontologies/C2SIM#TimeInstant"/>
        <rdfs:subClassOf>
            <owl:Restriction>
                <owl:onProperty rdf:resource="http://www.sisostds.org/ontologies/C2SIM#hasIsoDateTime"/>
                <owl:qualifiedCardinality rdf:datatype="http://www.w3.org/2001/XMLSchema#nonNegativeInteger">1</owl:qualifiedCardinality>
                <owl:onDataRange rdf:resource="http://www.sisostds.org/ontologies/C2SIM#IsoDateTimeBase"/>
            </owl:Restriction>
        </rdfs:subClassOf>
        <rdfs:comment>A date and time in ISO 8601:2000 DateTime Group format yyyy-mm-ddThh:mm:ssZ e.g. 1998-05-12T14:15:00Z. From MSDL simple types.</rdfs:comment>
    </owl:Class>
    


    <!-- http://www.sisostds.org/ontologies/C2SIM#DesiredEffectCode -->

    <owl:Class rdf:about="http://www.sisostds.org/ontologies/C2SIM#DesiredEffectCode">
        <rdfs:subClassOf rdf:resource="http://www.sisostds.org/ontologies/C2SIM#Code"/>
        <rdfs:comment>A code describing the intended effect of a task.</rdfs:comment>
    </owl:Class>
    


    <!-- http://www.sisostds.org/ontologies/C2SIM#DomainMessageBody -->

    <owl:Class rdf:about="http://www.sisostds.org/ontologies/C2SIM#DomainMessageBody">
        <rdfs:subClassOf rdf:resource="http://www.sisostds.org/ontologies/C2SIM#MessageBody"/>
        <rdfs:subClassOf>
            <owl:Restriction>
                <owl:onProperty rdf:resource="http://www.sisostds.org/ontologies/C2SIM#isFromSender"/>
                <owl:qualifiedCardinality rdf:datatype="http://www.w3.org/2001/XMLSchema#nonNegativeInteger">1</owl:qualifiedCardinality>
                <owl:onDataRange rdf:resource="http://www.sisostds.org/ontologies/C2SIM#UUIDBase"/>
            </owl:Restriction>
        </rdfs:subClassOf>
        <rdfs:subClassOf>
            <owl:Restriction>
                <owl:onProperty rdf:resource="http://www.sisostds.org/ontologies/C2SIM#isToReceiver"/>
                <owl:qualifiedCardinality rdf:datatype="http://www.w3.org/2001/XMLSchema#nonNegativeInteger">1</owl:qualifiedCardinality>
                <owl:onDataRange rdf:resource="http://www.sisostds.org/ontologies/C2SIM#UUIDBase"/>
            </owl:Restriction>
        </rdfs:subClassOf>
    </owl:Class>
    


    <!-- http://www.sisostds.org/ontologies/C2SIM#Duration -->

    <owl:Class rdf:about="http://www.sisostds.org/ontologies/C2SIM#Duration">
        <rdfs:subClassOf rdf:resource="http://www.sisostds.org/ontologies/C2SIM#TemporalConcept"/>
        <rdfs:subClassOf>
            <owl:Restriction>
                <owl:onProperty rdf:resource="http://www.sisostds.org/ontologies/C2SIM#hasIsoTimeDuration"/>
                <owl:qualifiedCardinality rdf:datatype="http://www.w3.org/2001/XMLSchema#nonNegativeInteger">1</owl:qualifiedCardinality>
                <owl:onDataRange rdf:resource="http://www.sisostds.org/ontologies/C2SIM#IsoTimeDurationBase"/>
            </owl:Restriction>
        </rdfs:subClassOf>
        <rdfs:comment>A time duration expressed in ISO 8601:2000 duration format PnYnMnDTnHnMnS e.g. P00Y00M00DT00H00M00S. Note that this does not support fractions of seconds. From MSDL simple types.</rdfs:comment>
    </owl:Class>
    


    <!-- http://www.sisostds.org/ontologies/C2SIM#Entity -->

    <owl:Class rdf:about="http://www.sisostds.org/ontologies/C2SIM#Entity">
        <rdfs:subClassOf rdf:resource="http://www.sisostds.org/ontologies/C2SIM#C2SIMContent"/>
        <rdfs:subClassOf>
            <owl:Restriction>
                <owl:onProperty rdf:resource="http://www.sisostds.org/ontologies/C2SIM#hasEntityType"/>
                <owl:someValuesFrom rdf:resource="http://www.sisostds.org/ontologies/C2SIM#EntityType"/>
            </owl:Restriction>
        </rdfs:subClassOf>
        <rdfs:subClassOf>
            <owl:Restriction>
                <owl:onProperty rdf:resource="http://www.sisostds.org/ontologies/C2SIM#hasUUID"/>
                <owl:qualifiedCardinality rdf:datatype="http://www.w3.org/2001/XMLSchema#nonNegativeInteger">1</owl:qualifiedCardinality>
                <owl:onDataRange rdf:resource="http://www.sisostds.org/ontologies/C2SIM#UUIDBase"/>
            </owl:Restriction>
        </rdfs:subClassOf>
        <rdfs:subClassOf>
            <owl:Restriction>
                <owl:onProperty rdf:resource="http://www.sisostds.org/ontologies/C2SIM#hasName"/>
                <owl:maxQualifiedCardinality rdf:datatype="http://www.w3.org/2001/XMLSchema#nonNegativeInteger">1</owl:maxQualifiedCardinality>
                <owl:onDataRange rdf:resource="http://www.w3.org/2001/XMLSchema#string"/>
            </owl:Restriction>
        </rdfs:subClassOf>
        <rdfs:comment>An individually identified object. Objects may have physical properties, in which case they belong to the subclass ConcreteEntity. Objects may be able to perform actions, in which case they belong in the subclass ActorEntity. If they have physical properties AND can perform actions, then they inherit from both subclasses.</rdfs:comment>
    </owl:Class>
    


    <!-- http://www.sisostds.org/ontologies/C2SIM#EntityDefinedLocation -->

    <owl:Class rdf:about="http://www.sisostds.org/ontologies/C2SIM#EntityDefinedLocation">
        <rdfs:subClassOf rdf:resource="http://www.sisostds.org/ontologies/C2SIM#Location"/>
        <rdfs:subClassOf>
            <owl:Restriction>
                <owl:onProperty rdf:resource="http://www.sisostds.org/ontologies/C2SIM#hasLocationReferenceEntity"/>
                <owl:qualifiedCardinality rdf:datatype="http://www.w3.org/2001/XMLSchema#nonNegativeInteger">1</owl:qualifiedCardinality>
                <owl:onDataRange rdf:resource="http://www.sisostds.org/ontologies/C2SIM#UUIDBase"/>
            </owl:Restriction>
        </rdfs:subClassOf>
        <rdfs:comment>A location defined by the location of a ConcreteEntity.</rdfs:comment>
    </owl:Class>
    


    <!-- http://www.sisostds.org/ontologies/C2SIM#EntityDescriptor -->

    <owl:Class rdf:about="http://www.sisostds.org/ontologies/C2SIM#EntityDescriptor">
        <rdfs:subClassOf rdf:resource="http://www.sisostds.org/ontologies/C2SIM#C2SIMContent"/>
        <rdfs:subClassOf>
            <owl:Restriction>
                <owl:onProperty rdf:resource="http://www.sisostds.org/ontologies/C2SIM#hasAllegianceTo"/>
                <owl:minQualifiedCardinality rdf:datatype="http://www.w3.org/2001/XMLSchema#nonNegativeInteger">0</owl:minQualifiedCardinality>
                <owl:onDataRange rdf:resource="http://www.sisostds.org/ontologies/C2SIM#UUIDBase"/>
            </owl:Restriction>
        </rdfs:subClassOf>
        <rdfs:subClassOf>
            <owl:Restriction>
                <owl:onProperty rdf:resource="http://www.sisostds.org/ontologies/C2SIM#hasCommunicationsNetwork"/>
                <owl:minQualifiedCardinality rdf:datatype="http://www.w3.org/2001/XMLSchema#nonNegativeInteger">0</owl:minQualifiedCardinality>
                <owl:onDataRange rdf:resource="http://www.sisostds.org/ontologies/C2SIM#UUIDBase"/>
            </owl:Restriction>
        </rdfs:subClassOf>
        <rdfs:subClassOf>
            <owl:Restriction>
                <owl:onProperty rdf:resource="http://www.sisostds.org/ontologies/C2SIM#isAffiliatedWith"/>
                <owl:minQualifiedCardinality rdf:datatype="http://www.w3.org/2001/XMLSchema#nonNegativeInteger">0</owl:minQualifiedCardinality>
                <owl:onDataRange rdf:resource="http://www.sisostds.org/ontologies/C2SIM#UUIDBase"/>
            </owl:Restriction>
        </rdfs:subClassOf>
        <rdfs:subClassOf>
            <owl:Restriction>
                <owl:onProperty rdf:resource="http://www.sisostds.org/ontologies/C2SIM#hasSuperior"/>
                <owl:maxQualifiedCardinality rdf:datatype="http://www.w3.org/2001/XMLSchema#nonNegativeInteger">1</owl:maxQualifiedCardinality>
                <owl:onDataRange rdf:resource="http://www.sisostds.org/ontologies/C2SIM#UUIDBase"/>
            </owl:Restriction>
        </rdfs:subClassOf>
        <rdfs:subClassOf>
            <owl:Restriction>
                <owl:onProperty rdf:resource="http://www.sisostds.org/ontologies/smx#hasSide"/>
                <owl:maxQualifiedCardinality rdf:datatype="http://www.w3.org/2001/XMLSchema#nonNegativeInteger">1</owl:maxQualifiedCardinality>
                <owl:onDataRange rdf:resource="http://www.sisostds.org/ontologies/C2SIM#UUIDBase"/>
            </owl:Restriction>
        </rdfs:subClassOf>
        <rdfs:comment>The Descriptor defines static attributes of an entity, i.e. that do not change during the course of the simulation. This information is provided at initialization time.

The friend/hostile/... relationship of this entity with others can be specfied with hasAllegianceRelationship properties, to define specific and possibly asymmetric relations with other enitities.

The isAffiliatedWith property defines organizations that this entity is affiliated with. These organizations are abstract; they are not actors.

C2 structures can be defined by using the hasSuperior property.</rdfs:comment>
    </owl:Class>
    


    <!-- http://www.sisostds.org/ontologies/C2SIM#EntityHealthStatus -->

    <owl:Class rdf:about="http://www.sisostds.org/ontologies/C2SIM#EntityHealthStatus">
        <rdfs:subClassOf rdf:resource="http://www.sisostds.org/ontologies/C2SIM#PhysicalConcept"/>
        <rdfs:comment>A representation of the health status of an entity. Subclasses for representing health as Operational Status, a count of some salient resource, or a percentage of full strength.</rdfs:comment>
    </owl:Class>
    


    <!-- http://www.sisostds.org/ontologies/C2SIM#EntityState -->

    <owl:Class rdf:about="http://www.sisostds.org/ontologies/C2SIM#EntityState">
        <rdfs:subClassOf rdf:resource="http://www.sisostds.org/ontologies/C2SIM#C2SIMContent"/>
        <rdfs:subClassOf>
            <owl:Restriction>
                <owl:onProperty rdf:resource="http://www.sisostds.org/ontologies/C2SIM#hasDateTime"/>
                <owl:maxQualifiedCardinality rdf:datatype="http://www.w3.org/2001/XMLSchema#nonNegativeInteger">1</owl:maxQualifiedCardinality>
                <owl:onClass rdf:resource="http://www.sisostds.org/ontologies/C2SIM#TimeInstant"/>
            </owl:Restriction>
        </rdfs:subClassOf>
        <rdfs:comment>Dynamic state information for entities in the exercise.</rdfs:comment>
    </owl:Class>
    


    <!-- http://www.sisostds.org/ontologies/C2SIM#EntityType -->

    <owl:Class rdf:about="http://www.sisostds.org/ontologies/C2SIM#EntityType">
        <rdfs:subClassOf rdf:resource="http://www.sisostds.org/ontologies/C2SIM#C2SIMContent"/>
        <rdfs:subClassOf>
            <owl:Restriction>
                <owl:onProperty rdf:resource="http://www.sisostds.org/ontologies/C2SIM#hasEntityTypeString"/>
                <owl:qualifiedCardinality rdf:datatype="http://www.w3.org/2001/XMLSchema#nonNegativeInteger">1</owl:qualifiedCardinality>
                <owl:onDataRange rdf:resource="http://www.w3.org/2001/XMLSchema#string"/>
            </owl:Restriction>
        </rdfs:subClassOf>
        <rdfs:comment>This is a set of category enumerations, e.g. a DIS type specification, or other set of unique values defining the type of an Entity for representation in simulations and depiction on C2 displays.</rdfs:comment>
    </owl:Class>
    


    <!-- http://www.sisostds.org/ontologies/C2SIM#EnvironmentalObject -->

    <owl:Class rdf:about="http://www.sisostds.org/ontologies/C2SIM#EnvironmentalObject">
        <rdfs:subClassOf rdf:resource="http://www.sisostds.org/ontologies/C2SIM#PhysicalEntity"/>
        <rdfs:comment>A specified region in which the environment (e.g. weather, ocean state) is defined by a particular Environmental State.</rdfs:comment>
    </owl:Class>
    


    <!-- http://www.sisostds.org/ontologies/C2SIM#Equipment -->

    <owl:Class rdf:about="http://www.sisostds.org/ontologies/C2SIM#Equipment">
        <rdfs:subClassOf rdf:resource="http://www.sisostds.org/ontologies/C2SIM#Resource"/>
        <rdfs:comment>A physical object that is normally part of an entity. For example an uncrewed gun.</rdfs:comment>
    </owl:Class>
    


    <!-- http://www.sisostds.org/ontologies/C2SIM#EthnicGroupCode -->

    <owl:Class rdf:about="http://www.sisostds.org/ontologies/C2SIM#EthnicGroupCode">
        <rdfs:subClassOf rdf:resource="http://www.sisostds.org/ontologies/C2SIM#OrganizationCode"/>
    </owl:Class>
    


    <!-- http://www.sisostds.org/ontologies/C2SIM#EulerAngles -->

    <owl:Class rdf:about="http://www.sisostds.org/ontologies/C2SIM#EulerAngles">
        <rdfs:subClassOf rdf:resource="http://www.sisostds.org/ontologies/C2SIM#Orientation"/>
        <rdfs:subClassOf>
            <owl:Restriction>
                <owl:onProperty rdf:resource="http://www.sisostds.org/ontologies/C2SIM#hasPhi"/>
                <owl:qualifiedCardinality rdf:datatype="http://www.w3.org/2001/XMLSchema#nonNegativeInteger">1</owl:qualifiedCardinality>
                <owl:onDataRange rdf:resource="http://www.sisostds.org/ontologies/C2SIM#angle"/>
            </owl:Restriction>
        </rdfs:subClassOf>
        <rdfs:subClassOf>
            <owl:Restriction>
                <owl:onProperty rdf:resource="http://www.sisostds.org/ontologies/C2SIM#hasPsi"/>
                <owl:qualifiedCardinality rdf:datatype="http://www.w3.org/2001/XMLSchema#nonNegativeInteger">1</owl:qualifiedCardinality>
                <owl:onDataRange rdf:resource="http://www.sisostds.org/ontologies/C2SIM#angle"/>
            </owl:Restriction>
        </rdfs:subClassOf>
        <rdfs:subClassOf>
            <owl:Restriction>
                <owl:onProperty rdf:resource="http://www.sisostds.org/ontologies/C2SIM#hasTheta"/>
                <owl:qualifiedCardinality rdf:datatype="http://www.w3.org/2001/XMLSchema#nonNegativeInteger">1</owl:qualifiedCardinality>
                <owl:onDataRange rdf:resource="http://www.sisostds.org/ontologies/C2SIM#angle"/>
            </owl:Restriction>
        </rdfs:subClassOf>
        <rdfs:comment>Representation of the orientation of an entity in 3D space expressed as Euler angles (DIS).</rdfs:comment>
    </owl:Class>
    


    <!-- http://www.sisostds.org/ontologies/C2SIM#Event -->

    <owl:Class rdf:about="http://www.sisostds.org/ontologies/C2SIM#Event">
        <rdfs:subClassOf rdf:resource="http://www.sisostds.org/ontologies/C2SIM#Action"/>
        <rdfs:subClassOf>
            <owl:Restriction>
                <owl:onProperty rdf:resource="http://www.sisostds.org/ontologies/C2SIM#hasEventCode"/>
                <owl:qualifiedCardinality rdf:datatype="http://www.w3.org/2001/XMLSchema#nonNegativeInteger">1</owl:qualifiedCardinality>
                <owl:onClass rdf:resource="http://www.sisostds.org/ontologies/C2SIM#EventCode"/>
            </owl:Restriction>
        </rdfs:subClassOf>
        <rdfs:subClassOf>
            <owl:Restriction>
                <owl:onProperty rdf:resource="http://www.sisostds.org/ontologies/C2SIM#hasStartTime"/>
                <owl:qualifiedCardinality rdf:datatype="http://www.w3.org/2001/XMLSchema#nonNegativeInteger">1</owl:qualifiedCardinality>
                <owl:onClass rdf:resource="http://www.sisostds.org/ontologies/C2SIM#TimeInstant"/>
            </owl:Restriction>
        </rdfs:subClassOf>
        <rdfs:comment>An ACTION that is an incident, phenomenon, or occasion. May or may not be the result of an agent&apos;s action.</rdfs:comment>
    </owl:Class>
    


    <!-- http://www.sisostds.org/ontologies/C2SIM#EventCode -->

    <owl:Class rdf:about="http://www.sisostds.org/ontologies/C2SIM#EventCode">
        <rdfs:subClassOf rdf:resource="http://www.sisostds.org/ontologies/C2SIM#ActionCode"/>
        <rdfs:comment>The type of event.</rdfs:comment>
    </owl:Class>
    


    <!-- http://www.sisostds.org/ontologies/C2SIM#ExtentVertices -->

    <owl:Class rdf:about="http://www.sisostds.org/ontologies/C2SIM#ExtentVertices">
        <rdfs:subClassOf rdf:resource="http://www.sisostds.org/ontologies/C2SIM#PhysicalExtent"/>
        <rdfs:subClassOf>
            <owl:Restriction>
                <owl:onProperty rdf:resource="http://www.sisostds.org/ontologies/C2SIM#hasLocation"/>
                <owl:minQualifiedCardinality rdf:datatype="http://www.w3.org/2001/XMLSchema#nonNegativeInteger">1</owl:minQualifiedCardinality>
                <owl:onClass rdf:resource="http://www.sisostds.org/ontologies/C2SIM#Location"/>
            </owl:Restriction>
        </rdfs:subClassOf>
        <rdfs:comment>The locations of multiple vertices defining the space occupied by an entity. For example, points on a multi-point line or a convex hull. These vertices are in a specific order.</rdfs:comment>
    </owl:Class>
    <owl:Axiom>
        <owl:annotatedSource rdf:resource="http://www.sisostds.org/ontologies/C2SIM#ExtentVertices"/>
        <owl:annotatedProperty rdf:resource="http://www.w3.org/2000/01/rdf-schema#subClassOf"/>
        <owl:annotatedTarget>
            <owl:Restriction>
                <owl:onProperty rdf:resource="http://www.sisostds.org/ontologies/C2SIM#hasLocation"/>
                <owl:minQualifiedCardinality rdf:datatype="http://www.w3.org/2001/XMLSchema#nonNegativeInteger">1</owl:minQualifiedCardinality>
                <owl:onClass rdf:resource="http://www.sisostds.org/ontologies/C2SIM#Location"/>
            </owl:Restriction>
        </owl:annotatedTarget>
        <rdfs:comment>These vertices must be given in a specific order.</rdfs:comment>
    </owl:Axiom>
    


    <!-- http://www.sisostds.org/ontologies/C2SIM#GeodeticCoordinate -->

    <owl:Class rdf:about="http://www.sisostds.org/ontologies/C2SIM#GeodeticCoordinate">
        <rdfs:subClassOf rdf:resource="http://www.sisostds.org/ontologies/C2SIM#Coordinate"/>
        <rdfs:subClassOf>
            <owl:Restriction>
                <owl:onProperty rdf:resource="http://www.sisostds.org/ontologies/C2SIM#hasLatitude"/>
                <owl:qualifiedCardinality rdf:datatype="http://www.w3.org/2001/XMLSchema#nonNegativeInteger">1</owl:qualifiedCardinality>
                <owl:onDataRange rdf:resource="http://www.sisostds.org/ontologies/C2SIM#latitude"/>
            </owl:Restriction>
        </rdfs:subClassOf>
        <rdfs:subClassOf>
            <owl:Restriction>
                <owl:onProperty rdf:resource="http://www.sisostds.org/ontologies/C2SIM#hasLongitude"/>
                <owl:qualifiedCardinality rdf:datatype="http://www.w3.org/2001/XMLSchema#nonNegativeInteger">1</owl:qualifiedCardinality>
                <owl:onDataRange rdf:resource="http://www.sisostds.org/ontologies/C2SIM#longitude"/>
            </owl:Restriction>
        </rdfs:subClassOf>
        <rdfs:subClassOf>
            <owl:Restriction>
                <owl:onProperty rdf:resource="http://www.sisostds.org/ontologies/C2SIM#hasAltitudeAGL"/>
                <owl:maxQualifiedCardinality rdf:datatype="http://www.w3.org/2001/XMLSchema#nonNegativeInteger">1</owl:maxQualifiedCardinality>
                <owl:onDataRange rdf:resource="http://www.w3.org/2001/XMLSchema#double"/>
            </owl:Restriction>
        </rdfs:subClassOf>
        <rdfs:subClassOf>
            <owl:Restriction>
                <owl:onProperty rdf:resource="http://www.sisostds.org/ontologies/C2SIM#hasAltitudeMSL"/>
                <owl:maxQualifiedCardinality rdf:datatype="http://www.w3.org/2001/XMLSchema#nonNegativeInteger">1</owl:maxQualifiedCardinality>
                <owl:onDataRange rdf:resource="http://www.w3.org/2001/XMLSchema#double"/>
            </owl:Restriction>
        </rdfs:subClassOf>
    </owl:Class>
    


    <!-- http://www.sisostds.org/ontologies/C2SIM#GeographicFeature -->

    <owl:Class rdf:about="http://www.sisostds.org/ontologies/C2SIM#GeographicFeature">
        <rdfs:subClassOf rdf:resource="http://www.sisostds.org/ontologies/C2SIM#PhysicalEntity"/>
        <rdfs:comment>A geographic feature generally used for location reference. For example a hill, river, etc.</rdfs:comment>
    </owl:Class>
    


    <!-- http://www.sisostds.org/ontologies/C2SIM#Handles -->

    <owl:Class rdf:about="http://www.sisostds.org/ontologies/C2SIM#Handles">
        <rdfs:subClassOf rdf:resource="http://www.sisostds.org/ontologies/C2SIM#PhysicalExtent"/>
        <rdfs:subClassOf>
            <owl:Restriction>
                <owl:onProperty rdf:resource="http://www.sisostds.org/ontologies/C2SIM#hasLocation"/>
                <owl:minQualifiedCardinality rdf:datatype="http://www.w3.org/2001/XMLSchema#nonNegativeInteger">1</owl:minQualifiedCardinality>
                <owl:onClass rdf:resource="http://www.sisostds.org/ontologies/C2SIM#Location"/>
            </owl:Restriction>
        </rdfs:subClassOf>
        <rdfs:comment>The locations of the special locations that define the shape of a physical object. For example, the tip of an arrow head graphic, a side point defining the arrow head width, and a bottom point defining its length.</rdfs:comment>
    </owl:Class>
    


    <!-- http://www.sisostds.org/ontologies/C2SIM#InitializationConcept -->

    <owl:Class rdf:about="http://www.sisostds.org/ontologies/C2SIM#InitializationConcept">
        <rdfs:comment>This parent class collects together classes that are necessary for the initialization of a scenario.</rdfs:comment>
    </owl:Class>
    


    <!-- http://www.sisostds.org/ontologies/C2SIM#InitializationDataFile -->

    <owl:Class rdf:about="http://www.sisostds.org/ontologies/C2SIM#InitializationDataFile">
        <rdfs:subClassOf rdf:resource="http://www.sisostds.org/ontologies/C2SIM#InitializationConcept"/>
        <rdfs:subClassOf>
            <owl:Restriction>
                <owl:onProperty rdf:resource="http://www.sisostds.org/ontologies/C2SIM#hasName"/>
                <owl:qualifiedCardinality rdf:datatype="http://www.w3.org/2001/XMLSchema#nonNegativeInteger">1</owl:qualifiedCardinality>
                <owl:onDataRange rdf:resource="http://www.w3.org/2001/XMLSchema#string"/>
            </owl:Restriction>
        </rdfs:subClassOf>
        <rdfs:subClassOf>
            <owl:Restriction>
                <owl:onProperty rdf:resource="http://www.sisostds.org/ontologies/C2SIM#hasSystemName"/>
                <owl:qualifiedCardinality rdf:datatype="http://www.w3.org/2001/XMLSchema#nonNegativeInteger">1</owl:qualifiedCardinality>
                <owl:onDataRange rdf:resource="http://www.w3.org/2001/XMLSchema#string"/>
            </owl:Restriction>
        </rdfs:subClassOf>
        <rdfs:subClassOf>
            <owl:Restriction>
                <owl:onProperty rdf:resource="http://www.sisostds.org/ontologies/C2SIM#hasIntializationFileType"/>
                <owl:maxQualifiedCardinality rdf:datatype="http://www.w3.org/2001/XMLSchema#nonNegativeInteger">1</owl:maxQualifiedCardinality>
                <owl:onDataRange rdf:resource="http://www.w3.org/2001/XMLSchema#string"/>
            </owl:Restriction>
        </rdfs:subClassOf>
        <rdfs:comment>Defines a file of supplementary data that is used to initialize the scenario. This file is generally system-specific, for example a terrain database file or a mapping from C2SIM entity types to local entity type enumerations. It could apply to &quot;all&quot; systems.</rdfs:comment>
    </owl:Class>
    


    <!-- http://www.sisostds.org/ontologies/C2SIM#IntervalTime -->

    <owl:Class rdf:about="http://www.sisostds.org/ontologies/C2SIM#IntervalTime">
        <rdfs:subClassOf rdf:resource="http://www.sisostds.org/ontologies/C2SIM#TemporalConcept"/>
        <rdfs:subClassOf>
            <owl:Restriction>
                <owl:onProperty rdf:resource="http://www.sisostds.org/ontologies/C2SIM#hasDuration"/>
                <owl:maxQualifiedCardinality rdf:datatype="http://www.w3.org/2001/XMLSchema#nonNegativeInteger">1</owl:maxQualifiedCardinality>
                <owl:onClass rdf:resource="http://www.sisostds.org/ontologies/C2SIM#Duration"/>
            </owl:Restriction>
        </rdfs:subClassOf>
        <rdfs:subClassOf>
            <owl:Restriction>
                <owl:onProperty rdf:resource="http://www.sisostds.org/ontologies/C2SIM#hasEndTime"/>
                <owl:maxQualifiedCardinality rdf:datatype="http://www.w3.org/2001/XMLSchema#nonNegativeInteger">1</owl:maxQualifiedCardinality>
                <owl:onClass rdf:resource="http://www.sisostds.org/ontologies/C2SIM#TimeInstant"/>
            </owl:Restriction>
        </rdfs:subClassOf>
        <rdfs:subClassOf>
            <owl:Restriction>
                <owl:onProperty rdf:resource="http://www.sisostds.org/ontologies/C2SIM#hasStartTime"/>
                <owl:maxQualifiedCardinality rdf:datatype="http://www.w3.org/2001/XMLSchema#nonNegativeInteger">1</owl:maxQualifiedCardinality>
                <owl:onClass rdf:resource="http://www.sisostds.org/ontologies/C2SIM#TimeInstant"/>
            </owl:Restriction>
        </rdfs:subClassOf>
        <rdfs:comment>An interval defined by a start and end dateTime. Note that 2 of the 3 properties must be specified.</rdfs:comment>
    </owl:Class>
    


    <!-- http://www.sisostds.org/ontologies/C2SIM#Location -->

    <owl:Class rdf:about="http://www.sisostds.org/ontologies/C2SIM#Location">
        <rdfs:subClassOf rdf:resource="http://www.sisostds.org/ontologies/C2SIM#PhysicalConcept"/>
        <rdfs:comment>A representation of location in space. Can be a coordinate value, a reference to an entity location, or a location relative to another location.

An optional altitude representation code indicates whether this is a fully specified point in 3 dimensions, or whether the altitude encoded in the class should be ignored or set to some other reference. If the code is not present, then the location is assumed to be a fully specified 3D point.

The location of a CollectiveEntity may represent the center of mass or headquarters location in the case of an organization.</rdfs:comment>
    </owl:Class>
    


    <!-- http://www.sisostds.org/ontologies/C2SIM#MapGraphic -->

    <owl:Class rdf:about="http://www.sisostds.org/ontologies/C2SIM#MapGraphic">
        <rdfs:subClassOf rdf:resource="http://www.sisostds.org/ontologies/C2SIM#PhysicalEntity"/>
        <rdfs:subClassOf>
            <owl:Restriction>
                <owl:onProperty rdf:resource="http://www.sisostds.org/ontologies/C2SIM_SMX_LOX#hasDummyProperty"/>
                <owl:minQualifiedCardinality rdf:datatype="http://www.w3.org/2001/XMLSchema#nonNegativeInteger">0</owl:minQualifiedCardinality>
                <owl:onDataRange rdf:resource="http://www.w3.org/2001/XMLSchema#string"/>
            </owl:Restriction>
        </rdfs:subClassOf>
        <rdfs:comment>Graphics on a map that define locations, lines, areas, actions, etc. The location of the graphic is the location in the real world represented on the map. The extent is the set of handle points or vertices that define its shape and size. This class includes task graphics, METOC graphics, and MOOTW graphics.</rdfs:comment>
    </owl:Class>
    


    <!-- http://www.sisostds.org/ontologies/C2SIM#Message -->

    <owl:Class rdf:about="http://www.sisostds.org/ontologies/C2SIM#Message">
        <rdfs:subClassOf rdf:resource="http://www.sisostds.org/ontologies/C2SIM#MessageConcept"/>
        <rdfs:subClassOf>
            <owl:Restriction>
                <owl:onProperty rdf:resource="http://www.sisostds.org/ontologies/C2SIM#hasC2SIMHeader"/>
                <owl:qualifiedCardinality rdf:datatype="http://www.w3.org/2001/XMLSchema#nonNegativeInteger">1</owl:qualifiedCardinality>
                <owl:onClass rdf:resource="http://www.sisostds.org/ontologies/C2SIM#C2SIMHeader"/>
            </owl:Restriction>
        </rdfs:subClassOf>
        <rdfs:subClassOf>
            <owl:Restriction>
                <owl:onProperty rdf:resource="http://www.sisostds.org/ontologies/C2SIM#hasMessageBody"/>
                <owl:qualifiedCardinality rdf:datatype="http://www.w3.org/2001/XMLSchema#nonNegativeInteger">1</owl:qualifiedCardinality>
                <owl:onClass rdf:resource="http://www.sisostds.org/ontologies/C2SIM#MessageBody"/>
            </owl:Restriction>
        </rdfs:subClassOf>
        <rdfs:comment>Any C2SIM message that is sent between host systems.</rdfs:comment>
    </owl:Class>
    


    <!-- http://www.sisostds.org/ontologies/C2SIM#MessageBody -->

    <owl:Class rdf:about="http://www.sisostds.org/ontologies/C2SIM#MessageBody">
        <rdfs:subClassOf rdf:resource="http://www.sisostds.org/ontologies/C2SIM#MessageConcept"/>
        <rdfs:comment>The structure for sending domain messages: orders, reports, and acknowledgements.</rdfs:comment>
    </owl:Class>
    


    <!-- http://www.sisostds.org/ontologies/C2SIM#MessageCode -->

    <owl:Class rdf:about="http://www.sisostds.org/ontologies/C2SIM#MessageCode">
        <rdfs:subClassOf rdf:resource="http://www.sisostds.org/ontologies/C2SIM#MessageConcept"/>
        <rdfs:comment>Enumerations used in messages.</rdfs:comment>
    </owl:Class>
    


    <!-- http://www.sisostds.org/ontologies/C2SIM#MessageConcept -->

    <owl:Class rdf:about="http://www.sisostds.org/ontologies/C2SIM#MessageConcept">
        <rdfs:comment>This parent class collects together classes that define the basic structure of messages used in C2SIM.</rdfs:comment>
    </owl:Class>
    


    <!-- http://www.sisostds.org/ontologies/C2SIM#MilitaryOrganization -->

    <owl:Class rdf:about="http://www.sisostds.org/ontologies/C2SIM#MilitaryOrganization">
        <rdfs:subClassOf rdf:resource="http://www.sisostds.org/ontologies/C2SIM#CollectiveEntity"/>
        <rdfs:subClassOf>
            <owl:Restriction>
                <owl:onProperty rdf:resource="http://www.sisostds.org/ontologies/C2SIM_SMX_LOX#hasDummyProperty"/>
                <owl:minQualifiedCardinality rdf:datatype="http://www.w3.org/2001/XMLSchema#nonNegativeInteger">0</owl:minQualifiedCardinality>
                <owl:onDataRange rdf:resource="http://www.w3.org/2001/XMLSchema#string"/>
            </owl:Restriction>
        </rdfs:subClassOf>
    </owl:Class>
    


    <!-- http://www.sisostds.org/ontologies/C2SIM#NonMilitaryOrganization -->

    <owl:Class rdf:about="http://www.sisostds.org/ontologies/C2SIM#NonMilitaryOrganization">
        <rdfs:subClassOf rdf:resource="http://www.sisostds.org/ontologies/C2SIM#CollectiveEntity"/>
        <rdfs:comment>An organization operating external to military authority (e.g., law enforcement, non-governmental organizations).</rdfs:comment>
    </owl:Class>
    


    <!-- http://www.sisostds.org/ontologies/C2SIM#ObjectDefinitions -->

    <owl:Class rdf:about="http://www.sisostds.org/ontologies/C2SIM#ObjectDefinitions">
        <rdfs:subClassOf rdf:resource="http://www.sisostds.org/ontologies/C2SIM#InitializationConcept"/>
        <rdfs:subClassOf>
            <owl:Restriction>
                <owl:onProperty rdf:resource="http://www.sisostds.org/ontologies/C2SIM#hasAbstractObject"/>
                <owl:minQualifiedCardinality rdf:datatype="http://www.w3.org/2001/XMLSchema#nonNegativeInteger">0</owl:minQualifiedCardinality>
                <owl:onClass rdf:resource="http://www.sisostds.org/ontologies/C2SIM#AbstractObject"/>
            </owl:Restriction>
        </rdfs:subClassOf>
        <rdfs:subClassOf>
            <owl:Restriction>
                <owl:onProperty rdf:resource="http://www.sisostds.org/ontologies/C2SIM#hasAction"/>
                <owl:minQualifiedCardinality rdf:datatype="http://www.w3.org/2001/XMLSchema#nonNegativeInteger">0</owl:minQualifiedCardinality>
                <owl:onClass rdf:resource="http://www.sisostds.org/ontologies/C2SIM#Action"/>
            </owl:Restriction>
        </rdfs:subClassOf>
        <rdfs:subClassOf>
            <owl:Restriction>
                <owl:onProperty rdf:resource="http://www.sisostds.org/ontologies/C2SIM#hasEntity"/>
                <owl:minQualifiedCardinality rdf:datatype="http://www.w3.org/2001/XMLSchema#nonNegativeInteger">0</owl:minQualifiedCardinality>
                <owl:onClass rdf:resource="http://www.sisostds.org/ontologies/C2SIM#Entity"/>
            </owl:Restriction>
        </rdfs:subClassOf>
        <rdfs:subClassOf>
            <owl:Restriction>
                <owl:onProperty rdf:resource="http://www.sisostds.org/ontologies/lox#hasPlanPhaseReference"/>
                <owl:minQualifiedCardinality rdf:datatype="http://www.w3.org/2001/XMLSchema#nonNegativeInteger">0</owl:minQualifiedCardinality>
                <owl:onDataRange rdf:resource="http://www.sisostds.org/ontologies/C2SIM#UUIDBase"/>
            </owl:Restriction>
        </rdfs:subClassOf>
    </owl:Class>
    <owl:Axiom>
        <owl:annotatedSource rdf:resource="http://www.sisostds.org/ontologies/C2SIM#ObjectDefinitions"/>
        <owl:annotatedProperty rdf:resource="http://www.w3.org/2000/01/rdf-schema#subClassOf"/>
        <owl:annotatedTarget>
            <owl:Restriction>
                <owl:onProperty rdf:resource="http://www.sisostds.org/ontologies/C2SIM#hasEntity"/>
                <owl:minQualifiedCardinality rdf:datatype="http://www.w3.org/2001/XMLSchema#nonNegativeInteger">0</owl:minQualifiedCardinality>
                <owl:onClass rdf:resource="http://www.sisostds.org/ontologies/C2SIM#Entity"/>
            </owl:Restriction>
        </owl:annotatedTarget>
        <rdfs:comment>This element is optional to allow ObjectInitialization messages to define only AbstractObjects or Tasks. The usual case, however, will be for the ObjectDefinitions class to have Entity definitions.</rdfs:comment>
    </owl:Axiom>
    


    <!-- http://www.sisostds.org/ontologies/C2SIM#ObjectInitialization -->

    <owl:Class rdf:about="http://www.sisostds.org/ontologies/C2SIM#ObjectInitialization">
        <rdfs:subClassOf rdf:resource="http://www.sisostds.org/ontologies/C2SIM#MessageBody"/>
        <rdfs:subClassOf>
            <owl:Restriction>
                <owl:onProperty rdf:resource="http://www.sisostds.org/ontologies/C2SIM#hasInitializationDataFile"/>
                <owl:minQualifiedCardinality rdf:datatype="http://www.w3.org/2001/XMLSchema#nonNegativeInteger">0</owl:minQualifiedCardinality>
                <owl:onClass rdf:resource="http://www.sisostds.org/ontologies/C2SIM#InitializationDataFile"/>
            </owl:Restriction>
        </rdfs:subClassOf>
        <rdfs:subClassOf>
            <owl:Restriction>
                <owl:onProperty rdf:resource="http://www.sisostds.org/ontologies/C2SIM#hasObjectDefinitions"/>
                <owl:maxQualifiedCardinality rdf:datatype="http://www.w3.org/2001/XMLSchema#nonNegativeInteger">1</owl:maxQualifiedCardinality>
                <owl:onClass rdf:resource="http://www.sisostds.org/ontologies/C2SIM#ObjectDefinitions"/>
            </owl:Restriction>
        </rdfs:subClassOf>
        <rdfs:subClassOf>
            <owl:Restriction>
                <owl:onProperty rdf:resource="http://www.sisostds.org/ontologies/C2SIM#hasScenarioSetting"/>
                <owl:maxQualifiedCardinality rdf:datatype="http://www.w3.org/2001/XMLSchema#nonNegativeInteger">1</owl:maxQualifiedCardinality>
                <owl:onClass rdf:resource="http://www.sisostds.org/ontologies/C2SIM#ScenarioSetting"/>
            </owl:Restriction>
        </rdfs:subClassOf>
        <rdfs:comment>This message is sent by each system to a marshalling server upon receipt of a SubmitInitialization message.</rdfs:comment>
    </owl:Class>
    


    <!-- http://www.sisostds.org/ontologies/C2SIM#OperationalStatus -->

    <owl:Class rdf:about="http://www.sisostds.org/ontologies/C2SIM#OperationalStatus">
        <rdfs:subClassOf rdf:resource="http://www.sisostds.org/ontologies/C2SIM#EntityHealthStatus"/>
        <rdfs:subClassOf>
            <owl:Restriction>
                <owl:onProperty rdf:resource="http://www.sisostds.org/ontologies/C2SIM#hasOperationalStatusCode"/>
                <owl:qualifiedCardinality rdf:datatype="http://www.w3.org/2001/XMLSchema#nonNegativeInteger">1</owl:qualifiedCardinality>
                <owl:onClass rdf:resource="http://www.sisostds.org/ontologies/C2SIM#OperationalStatusCode"/>
            </owl:Restriction>
        </rdfs:subClassOf>
        <rdfs:comment>An enumeration indicating degree of partial capability.</rdfs:comment>
    </owl:Class>
    


    <!-- http://www.sisostds.org/ontologies/C2SIM#OperationalStatusCode -->

    <owl:Class rdf:about="http://www.sisostds.org/ontologies/C2SIM#OperationalStatusCode">
        <rdfs:subClassOf rdf:resource="http://www.sisostds.org/ontologies/C2SIM#Code"/>
        <rdfs:comment>An enumeration indicating the general level of capability of an entity.</rdfs:comment>
    </owl:Class>
    


    <!-- http://www.sisostds.org/ontologies/C2SIM#OrderBody -->

    <owl:Class rdf:about="http://www.sisostds.org/ontologies/C2SIM#OrderBody">
        <rdfs:subClassOf rdf:resource="http://www.sisostds.org/ontologies/C2SIM#DomainMessageBody"/>
        <rdfs:subClassOf>
            <owl:Restriction>
                <owl:onProperty rdf:resource="http://www.sisostds.org/ontologies/C2SIM#hasTask"/>
                <owl:minQualifiedCardinality rdf:datatype="http://www.w3.org/2001/XMLSchema#nonNegativeInteger">1</owl:minQualifiedCardinality>
                <owl:onClass rdf:resource="http://www.sisostds.org/ontologies/C2SIM#Task"/>
            </owl:Restriction>
        </rdfs:subClassOf>
        <rdfs:subClassOf>
            <owl:Restriction>
                <owl:onProperty rdf:resource="http://www.sisostds.org/ontologies/C2SIM#hasIssuedTime"/>
                <owl:qualifiedCardinality rdf:datatype="http://www.w3.org/2001/XMLSchema#nonNegativeInteger">1</owl:qualifiedCardinality>
                <owl:onClass rdf:resource="http://www.sisostds.org/ontologies/C2SIM#TimeInstant"/>
            </owl:Restriction>
        </rdfs:subClassOf>
        <rdfs:subClassOf>
            <owl:Restriction>
                <owl:onProperty rdf:resource="http://www.sisostds.org/ontologies/C2SIM#hasOrderID"/>
                <owl:qualifiedCardinality rdf:datatype="http://www.w3.org/2001/XMLSchema#nonNegativeInteger">1</owl:qualifiedCardinality>
                <owl:onDataRange rdf:resource="http://www.sisostds.org/ontologies/C2SIM#UUIDBase"/>
            </owl:Restriction>
        </rdfs:subClassOf>
        <rdfs:subClassOf>
            <owl:Restriction>
                <owl:onProperty rdf:resource="http://www.sisostds.org/ontologies/C2SIM#hasRequestingEntity"/>
                <owl:maxQualifiedCardinality rdf:datatype="http://www.w3.org/2001/XMLSchema#nonNegativeInteger">1</owl:maxQualifiedCardinality>
                <owl:onDataRange rdf:resource="http://www.sisostds.org/ontologies/C2SIM#UUIDBase"/>
            </owl:Restriction>
        </rdfs:subClassOf>
        <rdfs:comment>The structure for sending order messages.</rdfs:comment>
    </owl:Class>
    <owl:Axiom>
        <owl:annotatedSource rdf:resource="http://www.sisostds.org/ontologies/C2SIM#OrderBody"/>
        <owl:annotatedProperty rdf:resource="http://www.w3.org/2000/01/rdf-schema#subClassOf"/>
        <owl:annotatedTarget>
            <owl:Restriction>
                <owl:onProperty rdf:resource="http://www.sisostds.org/ontologies/C2SIM#hasRequestingEntity"/>
                <owl:maxQualifiedCardinality rdf:datatype="http://www.w3.org/2001/XMLSchema#nonNegativeInteger">1</owl:maxQualifiedCardinality>
                <owl:onDataRange rdf:resource="http://www.sisostds.org/ontologies/C2SIM#UUIDBase"/>
            </owl:Restriction>
        </owl:annotatedTarget>
        <rdfs:comment>The entity issuing the order may not  be the same as the Sender, if the order was relayed through another unit. This optional property supports this case.</rdfs:comment>
    </owl:Axiom>
    


    <!-- http://www.sisostds.org/ontologies/C2SIM#OrganizationCode -->

    <owl:Class rdf:about="http://www.sisostds.org/ontologies/C2SIM#OrganizationCode">
        <rdfs:subClassOf rdf:resource="http://www.sisostds.org/ontologies/C2SIM#Code"/>
    </owl:Class>
    


    <!-- http://www.sisostds.org/ontologies/C2SIM#Orientation -->

    <owl:Class rdf:about="http://www.sisostds.org/ontologies/C2SIM#Orientation">
        <rdfs:subClassOf rdf:resource="http://www.sisostds.org/ontologies/C2SIM#PhysicalConcept"/>
        <rdfs:comment>Orientation is a set of rotations relative to the geocentric coordinate axes (DIS).</rdfs:comment>
    </owl:Class>
    


    <!-- http://www.sisostds.org/ontologies/C2SIM#Overlay -->

    <owl:Class rdf:about="http://www.sisostds.org/ontologies/C2SIM#Overlay">
        <rdfs:subClassOf rdf:resource="http://www.sisostds.org/ontologies/C2SIM#AbstractObject"/>
        <rdfs:subClassOf>
            <owl:Restriction>
                <owl:onProperty rdf:resource="http://www.sisostds.org/ontologies/C2SIM#hasReference"/>
                <owl:minQualifiedCardinality rdf:datatype="http://www.w3.org/2001/XMLSchema#nonNegativeInteger">1</owl:minQualifiedCardinality>
                <owl:onDataRange rdf:resource="http://www.sisostds.org/ontologies/C2SIM#UUIDBase"/>
            </owl:Restriction>
        </rdfs:subClassOf>
        <rdfs:comment>A logical grouping of Entities (units, graphics, etc.) for purposes of conveniently referring to them.</rdfs:comment>
    </owl:Class>
    


    <!-- http://www.sisostds.org/ontologies/C2SIM#Person -->

    <owl:Class rdf:about="http://www.sisostds.org/ontologies/C2SIM#Person">
        <rdfs:subClassOf rdf:resource="http://www.sisostds.org/ontologies/C2SIM#ActorEntity"/>
        <rdfs:subClassOf>
            <owl:Restriction>
                <owl:onProperty rdf:resource="http://www.sisostds.org/ontologies/C2SIM#hasCurrentState"/>
                <owl:maxQualifiedCardinality rdf:datatype="http://www.w3.org/2001/XMLSchema#nonNegativeInteger">1</owl:maxQualifiedCardinality>
                <owl:onClass rdf:resource="http://www.sisostds.org/ontologies/C2SIM#PhysicalState"/>
            </owl:Restriction>
        </rdfs:subClassOf>
        <rdfs:subClassOf>
            <owl:Restriction>
                <owl:onProperty rdf:resource="http://www.sisostds.org/ontologies/smx#hasPersonTypeCategoryCode"/>
                <owl:maxQualifiedCardinality rdf:datatype="http://www.w3.org/2001/XMLSchema#nonNegativeInteger">1</owl:maxQualifiedCardinality>
                <owl:onClass rdf:resource="http://www.sisostds.org/ontologies/smx#PersonTypeCategoryCode"/>
            </owl:Restriction>
        </rdfs:subClassOf>
        <rdfs:subClassOf>
            <owl:Restriction>
                <owl:onProperty rdf:resource="http://www.sisostds.org/ontologies/C2SIM#hasMarking"/>
                <owl:maxQualifiedCardinality rdf:datatype="http://www.w3.org/2001/XMLSchema#nonNegativeInteger">1</owl:maxQualifiedCardinality>
                <owl:onDataRange rdf:resource="http://www.w3.org/2001/XMLSchema#string"/>
            </owl:Restriction>
        </rdfs:subClassOf>
    </owl:Class>
    


    <!-- http://www.sisostds.org/ontologies/C2SIM#PhysicalConcept -->

    <owl:Class rdf:about="http://www.sisostds.org/ontologies/C2SIM#PhysicalConcept">
        <rdfs:subClassOf rdf:resource="http://www.sisostds.org/ontologies/C2SIM#C2SIMContent"/>
        <rdfs:comment>Concepts relating to the physical characteristics of an entity (e.g., location, health, orientation, size, etc.). The subclasses of this class have complex or alternative representations, and so are classes. Other physical properties such as mass that are simple scalars can be data type properties of (ConcreteEntity) objects.</rdfs:comment>
    </owl:Class>
    


    <!-- http://www.sisostds.org/ontologies/C2SIM#PhysicalEntity -->

    <owl:Class rdf:about="http://www.sisostds.org/ontologies/C2SIM#PhysicalEntity">
        <rdfs:subClassOf rdf:resource="http://www.sisostds.org/ontologies/C2SIM#Entity"/>
        <rdfs:subClassOf>
            <owl:Restriction>
                <owl:onProperty rdf:resource="http://www.sisostds.org/ontologies/C2SIM#hasCurrentState"/>
                <owl:qualifiedCardinality rdf:datatype="http://www.w3.org/2001/XMLSchema#nonNegativeInteger">1</owl:qualifiedCardinality>
                <owl:onClass rdf:resource="http://www.sisostds.org/ontologies/C2SIM#PhysicalState"/>
            </owl:Restriction>
        </rdfs:subClassOf>
        <rdfs:subClassOf>
            <owl:Restriction>
                <owl:onProperty rdf:resource="http://www.sisostds.org/ontologies/C2SIM#hasMarking"/>
                <owl:maxQualifiedCardinality rdf:datatype="http://www.w3.org/2001/XMLSchema#nonNegativeInteger">1</owl:maxQualifiedCardinality>
                <owl:onDataRange rdf:resource="http://www.w3.org/2001/XMLSchema#string"/>
            </owl:Restriction>
        </rdfs:subClassOf>
        <rdfs:comment>An Entity that has physical/kinematic properties.</rdfs:comment>
    </owl:Class>
    


    <!-- http://www.sisostds.org/ontologies/C2SIM#PhysicalExtent -->

    <owl:Class rdf:about="http://www.sisostds.org/ontologies/C2SIM#PhysicalExtent">
        <rdfs:subClassOf rdf:resource="http://www.sisostds.org/ontologies/C2SIM#PhysicalConcept"/>
        <rdfs:comment>A description of the space occupied by a physical object.  Can be described as a bounding box (2D), a bounding volume (3D), by a set of vertices, or by a set of handle points.</rdfs:comment>
    </owl:Class>
    


    <!-- http://www.sisostds.org/ontologies/C2SIM#PhysicalState -->

    <owl:Class rdf:about="http://www.sisostds.org/ontologies/C2SIM#PhysicalState">
        <rdfs:subClassOf rdf:resource="http://www.sisostds.org/ontologies/C2SIM#EntityState"/>
        <rdfs:subClassOf>
            <owl:Restriction>
                <owl:onProperty rdf:resource="http://www.sisostds.org/ontologies/C2SIM#hasLocation"/>
                <owl:qualifiedCardinality rdf:datatype="http://www.w3.org/2001/XMLSchema#nonNegativeInteger">1</owl:qualifiedCardinality>
                <owl:onClass rdf:resource="http://www.sisostds.org/ontologies/C2SIM#Location"/>
            </owl:Restriction>
        </rdfs:subClassOf>
        <rdfs:subClassOf>
            <owl:Restriction>
                <owl:onProperty rdf:resource="http://www.sisostds.org/ontologies/C2SIM#hasPhysicalExtent"/>
                <owl:qualifiedCardinality rdf:datatype="http://www.w3.org/2001/XMLSchema#nonNegativeInteger">1</owl:qualifiedCardinality>
                <owl:onClass rdf:resource="http://www.sisostds.org/ontologies/C2SIM#PhysicalExtent"/>
            </owl:Restriction>
        </rdfs:subClassOf>
        <rdfs:subClassOf>
            <owl:Restriction>
                <owl:onProperty rdf:resource="http://www.sisostds.org/ontologies/C2SIM#hasDirectionOfMovement"/>
                <owl:maxQualifiedCardinality rdf:datatype="http://www.w3.org/2001/XMLSchema#nonNegativeInteger">1</owl:maxQualifiedCardinality>
                <owl:onClass rdf:resource="http://www.sisostds.org/ontologies/C2SIM#Orientation"/>
            </owl:Restriction>
        </rdfs:subClassOf>
        <rdfs:subClassOf>
            <owl:Restriction>
                <owl:onProperty rdf:resource="http://www.sisostds.org/ontologies/C2SIM#hasEntityHealthStatus"/>
                <owl:maxQualifiedCardinality rdf:datatype="http://www.w3.org/2001/XMLSchema#nonNegativeInteger">1</owl:maxQualifiedCardinality>
                <owl:onClass rdf:resource="http://www.sisostds.org/ontologies/C2SIM#EntityHealthStatus"/>
            </owl:Restriction>
        </rdfs:subClassOf>
        <rdfs:subClassOf>
            <owl:Restriction>
                <owl:onProperty rdf:resource="http://www.sisostds.org/ontologies/C2SIM#hasOrientation"/>
                <owl:maxQualifiedCardinality rdf:datatype="http://www.w3.org/2001/XMLSchema#nonNegativeInteger">1</owl:maxQualifiedCardinality>
                <owl:onClass rdf:resource="http://www.sisostds.org/ontologies/C2SIM#Orientation"/>
            </owl:Restriction>
        </rdfs:subClassOf>
        <rdfs:subClassOf>
            <owl:Restriction>
                <owl:onProperty rdf:resource="http://www.sisostds.org/ontologies/C2SIM#hasSpeed"/>
                <owl:maxQualifiedCardinality rdf:datatype="http://www.w3.org/2001/XMLSchema#nonNegativeInteger">1</owl:maxQualifiedCardinality>
                <owl:onDataRange rdf:resource="http://www.w3.org/2001/XMLSchema#float"/>
            </owl:Restriction>
        </rdfs:subClassOf>
        <rdfs:comment>Description of the physical state of an entity, including location, orientation, health, speed, etc.
Note that an EnvironmentalState class should be a subclass of PhysicalState. The EnvironmentalState could be the state of, for example, a smoke plume, which would have a location and could have direction, orientation, and speed.</rdfs:comment>
    </owl:Class>
    


    <!-- http://www.sisostds.org/ontologies/C2SIM#Platform -->

    <owl:Class rdf:about="http://www.sisostds.org/ontologies/C2SIM#Platform">
        <rdfs:subClassOf rdf:resource="http://www.sisostds.org/ontologies/C2SIM#ActorEntity"/>
        <rdfs:subClassOf>
            <owl:Restriction>
                <owl:onProperty rdf:resource="http://www.sisostds.org/ontologies/C2SIM#hasCurrentState"/>
                <owl:maxQualifiedCardinality rdf:datatype="http://www.w3.org/2001/XMLSchema#nonNegativeInteger">1</owl:maxQualifiedCardinality>
                <owl:onClass rdf:resource="http://www.sisostds.org/ontologies/C2SIM#PhysicalState"/>
            </owl:Restriction>
        </rdfs:subClassOf>
        <rdfs:subClassOf>
            <owl:Restriction>
                <owl:onProperty rdf:resource="http://www.sisostds.org/ontologies/C2SIM#hasMarking"/>
                <owl:maxQualifiedCardinality rdf:datatype="http://www.w3.org/2001/XMLSchema#nonNegativeInteger">1</owl:maxQualifiedCardinality>
                <owl:onDataRange rdf:resource="http://www.w3.org/2001/XMLSchema#string"/>
            </owl:Restriction>
        </rdfs:subClassOf>
    </owl:Class>
    


    <!-- http://www.sisostds.org/ontologies/C2SIM#PositionReportContent -->

    <owl:Class rdf:about="http://www.sisostds.org/ontologies/C2SIM#PositionReportContent">
        <rdfs:subClassOf rdf:resource="http://www.sisostds.org/ontologies/C2SIM#ReportContent"/>
        <rdfs:subClassOf>
            <owl:Restriction>
                <owl:onProperty rdf:resource="http://www.sisostds.org/ontologies/C2SIM#hasLocation"/>
                <owl:qualifiedCardinality rdf:datatype="http://www.w3.org/2001/XMLSchema#nonNegativeInteger">1</owl:qualifiedCardinality>
                <owl:onClass rdf:resource="http://www.sisostds.org/ontologies/C2SIM#Coordinate"/>
            </owl:Restriction>
        </rdfs:subClassOf>
        <rdfs:subClassOf>
            <owl:Restriction>
                <owl:onProperty rdf:resource="http://www.sisostds.org/ontologies/C2SIM#hasOperationalStatus"/>
                <owl:maxQualifiedCardinality rdf:datatype="http://www.w3.org/2001/XMLSchema#nonNegativeInteger">1</owl:maxQualifiedCardinality>
                <owl:onClass rdf:resource="http://www.sisostds.org/ontologies/C2SIM#OperationalStatus"/>
            </owl:Restriction>
        </rdfs:subClassOf>
        <rdfs:subClassOf>
            <owl:Restriction>
                <owl:onProperty rdf:resource="http://www.sisostds.org/ontologies/C2SIM#hasStrength"/>
                <owl:maxQualifiedCardinality rdf:datatype="http://www.w3.org/2001/XMLSchema#nonNegativeInteger">1</owl:maxQualifiedCardinality>
                <owl:onClass rdf:resource="http://www.sisostds.org/ontologies/C2SIM#Strength"/>
            </owl:Restriction>
        </rdfs:subClassOf>
        <rdfs:subClassOf>
            <owl:Restriction>
                <owl:onProperty rdf:resource="http://www.sisostds.org/ontologies/C2SIM#hasSubjectEntity"/>
                <owl:qualifiedCardinality rdf:datatype="http://www.w3.org/2001/XMLSchema#nonNegativeInteger">1</owl:qualifiedCardinality>
                <owl:onDataRange rdf:resource="http://www.sisostds.org/ontologies/C2SIM#UUIDBase"/>
            </owl:Restriction>
        </rdfs:subClassOf>
    </owl:Class>
    


    <!-- http://www.sisostds.org/ontologies/C2SIM#RelativeLocation -->

    <owl:Class rdf:about="http://www.sisostds.org/ontologies/C2SIM#RelativeLocation">
        <rdfs:subClassOf rdf:resource="http://www.sisostds.org/ontologies/C2SIM#Location"/>
        <rdfs:subClassOf>
            <owl:Restriction>
                <owl:onProperty rdf:resource="http://www.sisostds.org/ontologies/C2SIM#hasSpatialOffset"/>
                <owl:qualifiedCardinality rdf:datatype="http://www.w3.org/2001/XMLSchema#nonNegativeInteger">1</owl:qualifiedCardinality>
                <owl:onClass rdf:resource="http://www.sisostds.org/ontologies/C2SIM#SpatialOffset"/>
            </owl:Restriction>
        </rdfs:subClassOf>
        <rdfs:subClassOf>
            <owl:Restriction>
                <owl:onProperty rdf:resource="http://www.sisostds.org/ontologies/C2SIM#hasEntityReference"/>
                <owl:qualifiedCardinality rdf:datatype="http://www.w3.org/2001/XMLSchema#nonNegativeInteger">1</owl:qualifiedCardinality>
                <owl:onDataRange rdf:resource="http://www.sisostds.org/ontologies/C2SIM#UUIDBase"/>
            </owl:Restriction>
        </rdfs:subClassOf>
        <rdfs:comment>A location defined by an offset to some reference location.</rdfs:comment>
    </owl:Class>
    


    <!-- http://www.sisostds.org/ontologies/C2SIM#RelativeTime -->

    <owl:Class rdf:about="http://www.sisostds.org/ontologies/C2SIM#RelativeTime">
        <rdfs:subClassOf rdf:resource="http://www.sisostds.org/ontologies/C2SIM#TimeInstant"/>
        <rdfs:subClassOf>
            <owl:Restriction>
                <owl:onProperty rdf:resource="http://www.sisostds.org/ontologies/C2SIM#hasDelayTimeAmount"/>
                <owl:qualifiedCardinality rdf:datatype="http://www.w3.org/2001/XMLSchema#nonNegativeInteger">1</owl:qualifiedCardinality>
                <owl:onClass rdf:resource="http://www.sisostds.org/ontologies/C2SIM#Duration"/>
            </owl:Restriction>
        </rdfs:subClassOf>
        <rdfs:subClassOf>
            <owl:Restriction>
                <owl:onProperty rdf:resource="http://www.sisostds.org/ontologies/C2SIM#hasTimeReferenceCode"/>
                <owl:qualifiedCardinality rdf:datatype="http://www.w3.org/2001/XMLSchema#nonNegativeInteger">1</owl:qualifiedCardinality>
                <owl:onClass rdf:resource="http://www.sisostds.org/ontologies/C2SIM#TimeReferenceCode"/>
            </owl:Restriction>
        </rdfs:subClassOf>
        <rdfs:subClassOf>
            <owl:Restriction>
                <owl:onProperty rdf:resource="http://www.sisostds.org/ontologies/C2SIM#hasEventReference"/>
                <owl:qualifiedCardinality rdf:datatype="http://www.w3.org/2001/XMLSchema#nonNegativeInteger">1</owl:qualifiedCardinality>
                <owl:onDataRange rdf:resource="http://www.sisostds.org/ontologies/C2SIM#UUIDBase"/>
            </owl:Restriction>
        </rdfs:subClassOf>
        <rdfs:comment>Specifies an absolute time relative to the start or end time of an event.</rdfs:comment>
    </owl:Class>
    


    <!-- http://www.sisostds.org/ontologies/C2SIM#ReligiousOrganizationCode -->

    <owl:Class rdf:about="http://www.sisostds.org/ontologies/C2SIM#ReligiousOrganizationCode">
        <rdfs:subClassOf rdf:resource="http://www.sisostds.org/ontologies/C2SIM#OrganizationCode"/>
    </owl:Class>
    


    <!-- http://www.sisostds.org/ontologies/C2SIM#ReportBody -->

    <owl:Class rdf:about="http://www.sisostds.org/ontologies/C2SIM#ReportBody">
        <rdfs:subClassOf rdf:resource="http://www.sisostds.org/ontologies/C2SIM#DomainMessageBody"/>
        <rdfs:subClassOf>
            <owl:Restriction>
                <owl:onProperty rdf:resource="http://www.sisostds.org/ontologies/C2SIM#hasReportContent"/>
                <owl:minQualifiedCardinality rdf:datatype="http://www.w3.org/2001/XMLSchema#nonNegativeInteger">1</owl:minQualifiedCardinality>
                <owl:onClass rdf:resource="http://www.sisostds.org/ontologies/C2SIM#ReportContent"/>
            </owl:Restriction>
        </rdfs:subClassOf>
        <rdfs:subClassOf>
            <owl:Restriction>
                <owl:onProperty rdf:resource="http://www.sisostds.org/ontologies/C2SIM#hasReportingEntity"/>
                <owl:qualifiedCardinality rdf:datatype="http://www.w3.org/2001/XMLSchema#nonNegativeInteger">1</owl:qualifiedCardinality>
                <owl:onDataRange rdf:resource="http://www.sisostds.org/ontologies/C2SIM#UUIDBase"/>
            </owl:Restriction>
        </rdfs:subClassOf>
        <rdfs:comment>The structure for sending report messages.</rdfs:comment>
    </owl:Class>
    


    <!-- http://www.sisostds.org/ontologies/C2SIM#ReportContent -->

    <owl:Class rdf:about="http://www.sisostds.org/ontologies/C2SIM#ReportContent">
        <rdfs:subClassOf rdf:resource="http://www.sisostds.org/ontologies/C2SIM#MessageConcept"/>
        <rdfs:subClassOf>
            <owl:Restriction>
                <owl:onProperty rdf:resource="http://www.sisostds.org/ontologies/C2SIM#hasTimeOfObservation"/>
                <owl:qualifiedCardinality rdf:datatype="http://www.w3.org/2001/XMLSchema#nonNegativeInteger">1</owl:qualifiedCardinality>
                <owl:onClass rdf:resource="http://www.sisostds.org/ontologies/C2SIM#DateTime"/>
            </owl:Restriction>
        </rdfs:subClassOf>
        <rdfs:comment>This is a collection class that may be used for different types of reports.</rdfs:comment>
    </owl:Class>
    


    <!-- http://www.sisostds.org/ontologies/C2SIM#Resource -->

    <owl:Class rdf:about="http://www.sisostds.org/ontologies/C2SIM#Resource">
        <rdfs:subClassOf rdf:resource="http://www.sisostds.org/ontologies/C2SIM#C2SIMContent"/>
        <rdfs:subClassOf>
            <owl:Restriction>
                <owl:onProperty rdf:resource="http://www.sisostds.org/ontologies/C2SIM#hasEntityType"/>
                <owl:maxQualifiedCardinality rdf:datatype="http://www.w3.org/2001/XMLSchema#nonNegativeInteger">1</owl:maxQualifiedCardinality>
                <owl:onClass rdf:resource="http://www.sisostds.org/ontologies/C2SIM#EntityType"/>
            </owl:Restriction>
        </rdfs:subClassOf>
        <rdfs:subClassOf>
            <owl:Restriction>
                <owl:onProperty rdf:resource="http://www.sisostds.org/ontologies/C2SIM#hasCount"/>
                <owl:maxQualifiedCardinality rdf:datatype="http://www.w3.org/2001/XMLSchema#nonNegativeInteger">1</owl:maxQualifiedCardinality>
                <owl:onDataRange rdf:resource="http://www.w3.org/2001/XMLSchema#integer"/>
            </owl:Restriction>
        </rdfs:subClassOf>
        <rdfs:subClassOf>
            <owl:Restriction>
                <owl:onProperty rdf:resource="http://www.sisostds.org/ontologies/C2SIM#hasName"/>
                <owl:maxQualifiedCardinality rdf:datatype="http://www.w3.org/2001/XMLSchema#nonNegativeInteger">1</owl:maxQualifiedCardinality>
                <owl:onDataRange rdf:resource="http://www.w3.org/2001/XMLSchema#string"/>
            </owl:Restriction>
        </rdfs:subClassOf>
        <rdfs:comment>This is a resource that can be part of, transferred to, or removed from an object (Entity), but is not an entity itself; therefore it does not have a location, extent, or other physical attributes.</rdfs:comment>
    </owl:Class>
    


    <!-- http://www.sisostds.org/ontologies/C2SIM#Resources -->

    <owl:Class rdf:about="http://www.sisostds.org/ontologies/C2SIM#Resources">
        <rdfs:subClassOf rdf:resource="http://www.sisostds.org/ontologies/C2SIM#EntityHealthStatus"/>
        <rdfs:subClassOf>
            <owl:Restriction>
                <owl:onProperty rdf:resource="http://www.sisostds.org/ontologies/C2SIM#hasResource"/>
                <owl:minQualifiedCardinality rdf:datatype="http://www.w3.org/2001/XMLSchema#nonNegativeInteger">1</owl:minQualifiedCardinality>
                <owl:onClass rdf:resource="http://www.sisostds.org/ontologies/C2SIM#Resource"/>
            </owl:Restriction>
        </rdfs:subClassOf>
        <rdfs:comment>A level of personnel, equipment, ammunition, fuel, etc. The user must compare this to the full strength of the unit.</rdfs:comment>
    </owl:Class>
    


    <!-- http://www.sisostds.org/ontologies/C2SIM#ScenarioSetting -->

    <owl:Class rdf:about="http://www.sisostds.org/ontologies/C2SIM#ScenarioSetting">
        <rdfs:subClassOf rdf:resource="http://www.sisostds.org/ontologies/C2SIM#InitializationConcept"/>
        <rdfs:subClassOf>
            <owl:Restriction>
                <owl:onProperty rdf:resource="http://www.sisostds.org/ontologies/C2SIM#hasDateTime"/>
                <owl:qualifiedCardinality rdf:datatype="http://www.w3.org/2001/XMLSchema#nonNegativeInteger">1</owl:qualifiedCardinality>
                <owl:onClass rdf:resource="http://www.sisostds.org/ontologies/C2SIM#DateTime"/>
            </owl:Restriction>
        </rdfs:subClassOf>
        <rdfs:subClassOf>
            <owl:Restriction>
                <owl:onProperty rdf:resource="http://www.sisostds.org/ontologies/C2SIM#hasPhysicalExtent"/>
                <owl:qualifiedCardinality rdf:datatype="http://www.w3.org/2001/XMLSchema#nonNegativeInteger">1</owl:qualifiedCardinality>
                <owl:onClass rdf:resource="http://www.sisostds.org/ontologies/C2SIM#PhysicalExtent"/>
            </owl:Restriction>
        </rdfs:subClassOf>
        <rdfs:subClassOf>
            <owl:Restriction>
                <owl:onProperty rdf:resource="http://www.sisostds.org/ontologies/C2SIM#hasVersion"/>
                <owl:qualifiedCardinality rdf:datatype="http://www.w3.org/2001/XMLSchema#nonNegativeInteger">1</owl:qualifiedCardinality>
                <owl:onDataRange rdf:resource="http://www.w3.org/2001/XMLSchema#string"/>
            </owl:Restriction>
        </rdfs:subClassOf>
        <rdfs:comment>Information describing the setting of the scenario, including the date, time, physical extent of the terrain, and a version string.</rdfs:comment>
    </owl:Class>
    


    <!-- http://www.sisostds.org/ontologies/C2SIM#SecurityClassificationCode -->

    <owl:Class rdf:about="http://www.sisostds.org/ontologies/C2SIM#SecurityClassificationCode">
        <rdfs:subClassOf rdf:resource="http://www.sisostds.org/ontologies/C2SIM#Code"/>
    </owl:Class>
    


    <!-- http://www.sisostds.org/ontologies/C2SIM#SimulationTime -->

    <owl:Class rdf:about="http://www.sisostds.org/ontologies/C2SIM#SimulationTime">
        <rdfs:subClassOf rdf:resource="http://www.sisostds.org/ontologies/C2SIM#TimeInstant"/>
        <rdfs:subClassOf>
            <owl:Restriction>
                <owl:onProperty rdf:resource="http://www.sisostds.org/ontologies/C2SIM#hasDelayTimeAmount"/>
                <owl:qualifiedCardinality rdf:datatype="http://www.w3.org/2001/XMLSchema#nonNegativeInteger">1</owl:qualifiedCardinality>
                <owl:onClass rdf:resource="http://www.sisostds.org/ontologies/C2SIM#Duration"/>
            </owl:Restriction>
        </rdfs:subClassOf>
        <rdfs:comment>A time measured as a time duration since the time instant of the scenario start.</rdfs:comment>
    </owl:Class>
    


    <!-- http://www.sisostds.org/ontologies/C2SIM#SpatialOffset -->

    <owl:Class rdf:about="http://www.sisostds.org/ontologies/C2SIM#SpatialOffset">
        <rdfs:subClassOf rdf:resource="http://www.sisostds.org/ontologies/C2SIM#PhysicalConcept"/>
        <rdfs:comment>Used in a relative location specification.</rdfs:comment>
    </owl:Class>
    


    <!-- http://www.sisostds.org/ontologies/C2SIM#Strength -->

    <owl:Class rdf:about="http://www.sisostds.org/ontologies/C2SIM#Strength">
        <rdfs:subClassOf rdf:resource="http://www.sisostds.org/ontologies/C2SIM#EntityHealthStatus"/>
        <rdfs:subClassOf>
            <owl:Restriction>
                <owl:onProperty rdf:resource="http://www.sisostds.org/ontologies/C2SIM#hasStrengthPercentage"/>
                <owl:qualifiedCardinality rdf:datatype="http://www.w3.org/2001/XMLSchema#nonNegativeInteger">1</owl:qualifiedCardinality>
                <owl:onDataRange rdf:resource="http://www.sisostds.org/ontologies/C2SIM#percentage"/>
            </owl:Restriction>
        </rdfs:subClassOf>
        <rdfs:comment>Representation of the strength of an entity expressed as a percentage of some starting value.</rdfs:comment>
    </owl:Class>
    


    <!-- http://www.sisostds.org/ontologies/C2SIM#SystemCommandBody -->

    <owl:Class rdf:about="http://www.sisostds.org/ontologies/C2SIM#SystemCommandBody">
        <rdfs:subClassOf rdf:resource="http://www.sisostds.org/ontologies/C2SIM#MessageBody"/>
        <rdfs:subClassOf>
            <owl:Restriction>
                <owl:onProperty rdf:resource="http://www.sisostds.org/ontologies/C2SIM#hasSystemCommandTypeCode"/>
                <owl:qualifiedCardinality rdf:datatype="http://www.w3.org/2001/XMLSchema#nonNegativeInteger">1</owl:qualifiedCardinality>
                <owl:onClass rdf:resource="http://www.sisostds.org/ontologies/C2SIM#SystemCommandTypeCode"/>
            </owl:Restriction>
        </rdfs:subClassOf>
    </owl:Class>
    


    <!-- http://www.sisostds.org/ontologies/C2SIM#SystemCommandTypeCode -->

    <owl:Class rdf:about="http://www.sisostds.org/ontologies/C2SIM#SystemCommandTypeCode">
        <rdfs:subClassOf rdf:resource="http://www.sisostds.org/ontologies/C2SIM#MessageCode"/>
    </owl:Class>
    


    <!-- http://www.sisostds.org/ontologies/C2SIM#SystemEntityList -->

    <owl:Class rdf:about="http://www.sisostds.org/ontologies/C2SIM#SystemEntityList">
        <rdfs:subClassOf rdf:resource="http://www.sisostds.org/ontologies/C2SIM#InitializationConcept"/>
        <rdfs:subClassOf>
            <owl:Restriction>
                <owl:onProperty rdf:resource="http://www.sisostds.org/ontologies/C2SIM#hasActorReference"/>
                <owl:minQualifiedCardinality rdf:datatype="http://www.w3.org/2001/XMLSchema#nonNegativeInteger">1</owl:minQualifiedCardinality>
                <owl:onDataRange rdf:resource="http://www.sisostds.org/ontologies/C2SIM#UUIDBase"/>
            </owl:Restriction>
        </rdfs:subClassOf>
        <rdfs:subClassOf>
            <owl:Restriction>
                <owl:onProperty rdf:resource="http://www.sisostds.org/ontologies/C2SIM#hasSystemName"/>
                <owl:qualifiedCardinality rdf:datatype="http://www.w3.org/2001/XMLSchema#nonNegativeInteger">1</owl:qualifiedCardinality>
                <owl:onDataRange rdf:resource="http://www.w3.org/2001/XMLSchema#string"/>
            </owl:Restriction>
        </rdfs:subClassOf>
        <rdfs:comment>This is a listing of entities that reside of a system. The list defines what system a message should be sent to in order to get it to a given actor.  Each entity can reside on only one system. This list does not define necessarily define the complete list of entities on the given system.
Systems can build a map from this and other lists to get the system from a given entity.</rdfs:comment>
    </owl:Class>
    


    <!-- http://www.sisostds.org/ontologies/C2SIM#SystemStateCode -->

    <owl:Class rdf:about="http://www.sisostds.org/ontologies/C2SIM#SystemStateCode">
        <rdfs:subClassOf rdf:resource="http://www.sisostds.org/ontologies/C2SIM#Code"/>
    </owl:Class>
    


    <!-- http://www.sisostds.org/ontologies/C2SIM#Task -->

    <owl:Class rdf:about="http://www.sisostds.org/ontologies/C2SIM#Task">
        <rdfs:subClassOf rdf:resource="http://www.sisostds.org/ontologies/C2SIM#Action"/>
        <rdfs:subClassOf>
            <owl:Restriction>
                <owl:onProperty rdf:resource="http://www.sisostds.org/ontologies/C2SIM#hasDesiredEffectCode"/>
                <owl:minQualifiedCardinality rdf:datatype="http://www.w3.org/2001/XMLSchema#nonNegativeInteger">0</owl:minQualifiedCardinality>
                <owl:onClass rdf:resource="http://www.sisostds.org/ontologies/C2SIM#DesiredEffectCode"/>
            </owl:Restriction>
        </rdfs:subClassOf>
        <rdfs:subClassOf>
            <owl:Restriction>
                <owl:onProperty rdf:resource="http://www.sisostds.org/ontologies/C2SIM#hasTaskNameCode"/>
                <owl:qualifiedCardinality rdf:datatype="http://www.w3.org/2001/XMLSchema#nonNegativeInteger">1</owl:qualifiedCardinality>
                <owl:onClass rdf:resource="http://www.sisostds.org/ontologies/C2SIM#TaskNameCode"/>
            </owl:Restriction>
        </rdfs:subClassOf>
        <rdfs:subClassOf>
            <owl:Restriction>
                <owl:onProperty rdf:resource="http://www.sisostds.org/ontologies/C2SIM#hasDuration"/>
                <owl:maxQualifiedCardinality rdf:datatype="http://www.w3.org/2001/XMLSchema#nonNegativeInteger">1</owl:maxQualifiedCardinality>
                <owl:onClass rdf:resource="http://www.sisostds.org/ontologies/C2SIM#Duration"/>
            </owl:Restriction>
        </rdfs:subClassOf>
        <rdfs:subClassOf>
            <owl:Restriction>
                <owl:onProperty rdf:resource="http://www.sisostds.org/ontologies/C2SIM#hasEndTime"/>
                <owl:maxQualifiedCardinality rdf:datatype="http://www.w3.org/2001/XMLSchema#nonNegativeInteger">1</owl:maxQualifiedCardinality>
                <owl:onClass rdf:resource="http://www.sisostds.org/ontologies/C2SIM#TimeInstant"/>
            </owl:Restriction>
        </rdfs:subClassOf>
        <rdfs:subClassOf>
            <owl:Restriction>
                <owl:onProperty rdf:resource="http://www.sisostds.org/ontologies/C2SIM#hasStartTime"/>
                <owl:maxQualifiedCardinality rdf:datatype="http://www.w3.org/2001/XMLSchema#nonNegativeInteger">1</owl:maxQualifiedCardinality>
                <owl:onClass rdf:resource="http://www.sisostds.org/ontologies/C2SIM#TimeInstant"/>
            </owl:Restriction>
        </rdfs:subClassOf>
        <rdfs:subClassOf>
            <owl:Restriction>
                <owl:onProperty rdf:resource="http://www.sisostds.org/ontologies/C2SIM#hasAffectedEntity"/>
                <owl:minQualifiedCardinality rdf:datatype="http://www.w3.org/2001/XMLSchema#nonNegativeInteger">0</owl:minQualifiedCardinality>
                <owl:onDataRange rdf:resource="http://www.sisostds.org/ontologies/C2SIM#UUIDBase"/>
            </owl:Restriction>
        </rdfs:subClassOf>
        <rdfs:subClassOf>
            <owl:Restriction>
                <owl:onProperty rdf:resource="http://www.sisostds.org/ontologies/C2SIM#hasPerformingEntity"/>
                <owl:qualifiedCardinality rdf:datatype="http://www.w3.org/2001/XMLSchema#nonNegativeInteger">1</owl:qualifiedCardinality>
                <owl:onDataRange rdf:resource="http://www.sisostds.org/ontologies/C2SIM#UUIDBase"/>
            </owl:Restriction>
        </rdfs:subClassOf>
        <rdfs:comment>A Action that takes place over time, and is performed by an Entity to change the state of the world.
WHO is represented by hasPerformingEntity (and hasEntity, which can be an affected entity, a supporting entity, etc. depending on the context of WHAT).
WHAT is represented by the hasActionCode.
WHEN is represented by the start time/duration/end time (2 of 3)
WHERE is represented by hasLocation and/or hasMapGraphicID reference.
WHY may be represented by hasDesiredEffect.</rdfs:comment>
    </owl:Class>
    


    <!-- http://www.sisostds.org/ontologies/C2SIM#TaskNameCode -->

    <owl:Class rdf:about="http://www.sisostds.org/ontologies/C2SIM#TaskNameCode">
        <rdfs:subClassOf rdf:resource="http://www.sisostds.org/ontologies/C2SIM#ActionCode"/>
        <rdfs:comment>The activity to be performed in the task, e.g. Move, Observe, Assist.</rdfs:comment>
    </owl:Class>
    


    <!-- http://www.sisostds.org/ontologies/C2SIM#TemporalConcept -->

    <owl:Class rdf:about="http://www.sisostds.org/ontologies/C2SIM#TemporalConcept">
        <rdfs:subClassOf rdf:resource="http://www.sisostds.org/ontologies/C2SIM#PhysicalConcept"/>
        <rdfs:comment>Time concepts include instants in time, durations of time, and intervals between two times.</rdfs:comment>
    </owl:Class>
    


    <!-- http://www.sisostds.org/ontologies/C2SIM#TimeInstant -->

    <owl:Class rdf:about="http://www.sisostds.org/ontologies/C2SIM#TimeInstant">
        <rdfs:subClassOf rdf:resource="http://www.sisostds.org/ontologies/C2SIM#TemporalConcept"/>
        <rdfs:subClassOf>
            <owl:Restriction>
                <owl:onProperty rdf:resource="http://www.sisostds.org/ontologies/C2SIM#hasName"/>
                <owl:maxQualifiedCardinality rdf:datatype="http://www.w3.org/2001/XMLSchema#nonNegativeInteger">1</owl:maxQualifiedCardinality>
                <owl:onDataRange rdf:resource="http://www.w3.org/2001/XMLSchema#string"/>
            </owl:Restriction>
        </rdfs:subClassOf>
        <rdfs:comment>A specific time expressed in seconds, i.e. with no date. The generator and user of this time must understand a common reference point, for example the start of the scenario.</rdfs:comment>
    </owl:Class>
    


    <!-- http://www.sisostds.org/ontologies/C2SIM#TimeReferenceCode -->

    <owl:Class rdf:about="http://www.sisostds.org/ontologies/C2SIM#TimeReferenceCode">
        <rdfs:subClassOf rdf:resource="http://www.sisostds.org/ontologies/C2SIM#Code"/>
        <rdfs:comment>Indicates whether a relative time is referenced to the start or the end of an interval time.</rdfs:comment>
    </owl:Class>
    


    <!-- http://www.sisostds.org/ontologies/C2SIM_SMX_LOX#CheckPoint -->

    <owl:Class rdf:about="http://www.sisostds.org/ontologies/C2SIM_SMX_LOX#CheckPoint">
        <rdfs:subClassOf rdf:resource="http://www.co-ode.org/ontologies/ont.owl#Point"/>
    </owl:Class>
    


    <!-- http://www.sisostds.org/ontologies/C2SIM_SMX_LOX#FireTask -->

    <owl:Class rdf:about="http://www.sisostds.org/ontologies/C2SIM_SMX_LOX#FireTask">
        <rdfs:subClassOf rdf:resource="http://www.sisostds.org/ontologies/C2SIM_SMX_LOX#UAVTask"/>
        <rdfs:subClassOf>
            <owl:Restriction>
                <owl:onProperty rdf:resource="http://www.sisostds.org/ontologies/C2SIM_SMX_LOX#hasAmountOfAmmunition"/>
                <owl:someValuesFrom rdf:resource="http://www.w3.org/2001/XMLSchema#nonNegativeInteger"/>
            </owl:Restriction>
        </rdfs:subClassOf>
    </owl:Class>
    


    <!-- http://www.sisostds.org/ontologies/C2SIM_SMX_LOX#RecceUAVTask -->

    <owl:Class rdf:about="http://www.sisostds.org/ontologies/C2SIM_SMX_LOX#RecceUAVTask">
        <rdfs:subClassOf rdf:resource="http://www.sisostds.org/ontologies/C2SIM_SMX_LOX#UAVTask"/>
        <rdfs:subClassOf>
            <owl:Restriction>
                <owl:onProperty rdf:resource="http://www.sisostds.org/ontologies/C2SIM_SMX_LOX#hasLeapFrogDistance"/>
                <owl:someValuesFrom rdf:resource="http://www.w3.org/2001/XMLSchema#integer"/>
            </owl:Restriction>
        </rdfs:subClassOf>
        <rdfs:subClassOf>
            <owl:Restriction>
                <owl:onProperty rdf:resource="http://www.sisostds.org/ontologies/C2SIM_SMX_LOX#hasAmountOfDrones"/>
                <owl:qualifiedCardinality rdf:datatype="http://www.w3.org/2001/XMLSchema#nonNegativeInteger">1</owl:qualifiedCardinality>
                <owl:onDataRange rdf:resource="http://www.w3.org/2001/XMLSchema#nonNegativeInteger"/>
            </owl:Restriction>
        </rdfs:subClassOf>
    </owl:Class>
    


    <!-- http://www.sisostds.org/ontologies/C2SIM_SMX_LOX#UAVTask -->

    <owl:Class rdf:about="http://www.sisostds.org/ontologies/C2SIM_SMX_LOX#UAVTask">
        <rdfs:subClassOf rdf:resource="http://www.sisostds.org/ontologies/C2SIM#Task"/>
        <rdfs:subClassOf>
            <owl:Restriction>
                <owl:onProperty rdf:resource="http://www.sisostds.org/ontologies/C2SIM_SMX_LOX#hasDummyProperty"/>
                <owl:minQualifiedCardinality rdf:datatype="http://www.w3.org/2001/XMLSchema#nonNegativeInteger">0</owl:minQualifiedCardinality>
                <owl:onDataRange rdf:resource="http://www.w3.org/2001/XMLSchema#string"/>
            </owl:Restriction>
        </rdfs:subClassOf>
    </owl:Class>
    


    <!-- http://www.sisostds.org/ontologies/C2SIM_SMX_LOX#WayPoint -->

    <owl:Class rdf:about="http://www.sisostds.org/ontologies/C2SIM_SMX_LOX#WayPoint">
        <rdfs:subClassOf rdf:resource="http://www.co-ode.org/ontologies/ont.owl#Point"/>
    </owl:Class>
    


    <!-- http://www.sisostds.org/ontologies/lox#EventTrigger -->

    <owl:Class rdf:about="http://www.sisostds.org/ontologies/lox#EventTrigger">
        <rdfs:subClassOf rdf:resource="http://www.sisostds.org/ontologies/lox#PlanPhaseTrigger"/>
        <rdfs:subClassOf>
            <owl:Restriction>
                <owl:onProperty rdf:resource="http://www.sisostds.org/ontologies/lox#hasEvent"/>
                <owl:qualifiedCardinality rdf:datatype="http://www.w3.org/2001/XMLSchema#nonNegativeInteger">1</owl:qualifiedCardinality>
                <owl:onClass rdf:resource="http://www.sisostds.org/ontologies/C2SIM#Event"/>
            </owl:Restriction>
        </rdfs:subClassOf>
    </owl:Class>
    


    <!-- http://www.sisostds.org/ontologies/lox#ExecutePlanBody -->

    <owl:Class rdf:about="http://www.sisostds.org/ontologies/lox#ExecutePlanBody">
        <rdfs:subClassOf rdf:resource="http://www.sisostds.org/ontologies/C2SIM#DomainMessageBody"/>
        <rdfs:subClassOf>
            <owl:Restriction>
                <owl:onProperty rdf:resource="http://www.sisostds.org/ontologies/lox#hasPlanPhaseReference"/>
                <owl:minQualifiedCardinality rdf:datatype="http://www.w3.org/2001/XMLSchema#nonNegativeInteger">1</owl:minQualifiedCardinality>
                <owl:onDataRange rdf:resource="http://www.sisostds.org/ontologies/C2SIM#UUIDBase"/>
            </owl:Restriction>
        </rdfs:subClassOf>
        <rdfs:comment>This message orders the recipient unit to begin execution of the indicated plan.</rdfs:comment>
    </owl:Class>
    


    <!-- http://www.sisostds.org/ontologies/lox#ManeuverWarfareTask -->

    <owl:Class rdf:about="http://www.sisostds.org/ontologies/lox#ManeuverWarfareTask">
        <rdfs:subClassOf rdf:resource="http://www.sisostds.org/ontologies/C2SIM#Task"/>
        <rdfs:subClassOf>
            <owl:Restriction>
                <owl:onProperty rdf:resource="http://www.sisostds.org/ontologies/lox#hasTaskFunctionalAssociationCode"/>
                <owl:maxQualifiedCardinality rdf:datatype="http://www.w3.org/2001/XMLSchema#nonNegativeInteger">1</owl:maxQualifiedCardinality>
                <owl:onClass rdf:resource="http://www.sisostds.org/ontologies/lox#TaskFunctionalAssociationCode"/>
            </owl:Restriction>
        </rdfs:subClassOf>
        <rdfs:subClassOf>
            <owl:Restriction>
                <owl:onProperty rdf:resource="http://www.sisostds.org/ontologies/lox#hasFunctionalAssociationWithTask"/>
                <owl:maxQualifiedCardinality rdf:datatype="http://www.w3.org/2001/XMLSchema#nonNegativeInteger">1</owl:maxQualifiedCardinality>
                <owl:onDataRange rdf:resource="http://www.sisostds.org/ontologies/C2SIM#UUIDBase"/>
            </owl:Restriction>
        </rdfs:subClassOf>
        <rdfs:comment>A task containing the who, what, where, when, why of a ground maneuver task.</rdfs:comment>
        <rdfs:comment>Advance, Attack, Block, CounterAttack, Destroy, Engage, HoldDefensive, March, Observe, Patrol, Reccon</rdfs:comment>
    </owl:Class>
    


    <!-- http://www.sisostds.org/ontologies/lox#OnOrderTrigger -->

    <owl:Class rdf:about="http://www.sisostds.org/ontologies/lox#OnOrderTrigger">
        <rdfs:subClassOf rdf:resource="http://www.sisostds.org/ontologies/lox#PlanPhaseTrigger"/>
        <rdfs:subClassOf>
            <owl:Restriction>
                <owl:onProperty rdf:resource="http://www.sisostds.org/ontologies/C2SIM#hasTaskReference"/>
                <owl:qualifiedCardinality rdf:datatype="http://www.w3.org/2001/XMLSchema#nonNegativeInteger">1</owl:qualifiedCardinality>
                <owl:onDataRange rdf:resource="http://www.sisostds.org/ontologies/C2SIM#UUIDBase"/>
            </owl:Restriction>
        </rdfs:subClassOf>
    </owl:Class>
    


    <!-- http://www.sisostds.org/ontologies/lox#PlanPhase -->

    <owl:Class rdf:about="http://www.sisostds.org/ontologies/lox#PlanPhase">
        <rdfs:subClassOf rdf:resource="http://www.sisostds.org/ontologies/C2SIM#C2SIMContent"/>
        <rdfs:subClassOf>
            <owl:Restriction>
                <owl:onProperty rdf:resource="http://www.sisostds.org/ontologies/lox#hasSubPhase"/>
                <owl:minQualifiedCardinality rdf:datatype="http://www.w3.org/2001/XMLSchema#nonNegativeInteger">0</owl:minQualifiedCardinality>
                <owl:onClass rdf:resource="http://www.sisostds.org/ontologies/lox#PlanPhase"/>
            </owl:Restriction>
        </rdfs:subClassOf>
        <rdfs:subClassOf>
            <owl:Restriction>
                <owl:onProperty rdf:resource="http://www.sisostds.org/ontologies/lox#hasPlanPhaseCompletionCondition"/>
                <owl:qualifiedCardinality rdf:datatype="http://www.w3.org/2001/XMLSchema#nonNegativeInteger">1</owl:qualifiedCardinality>
                <owl:onClass rdf:resource="http://www.sisostds.org/ontologies/lox#PlanPhaseCompletionCondition"/>
            </owl:Restriction>
        </rdfs:subClassOf>
        <rdfs:subClassOf>
            <owl:Restriction>
                <owl:onProperty rdf:resource="http://www.sisostds.org/ontologies/lox#hasPlanPhaseTrigger"/>
                <owl:qualifiedCardinality rdf:datatype="http://www.w3.org/2001/XMLSchema#nonNegativeInteger">1</owl:qualifiedCardinality>
                <owl:onClass rdf:resource="http://www.sisostds.org/ontologies/lox#PlanPhaseTrigger"/>
            </owl:Restriction>
        </rdfs:subClassOf>
        <rdfs:subClassOf>
            <owl:Restriction>
                <owl:onProperty rdf:resource="http://www.sisostds.org/ontologies/lox#hasPlanPhaseId"/>
                <owl:qualifiedCardinality rdf:datatype="http://www.w3.org/2001/XMLSchema#nonNegativeInteger">1</owl:qualifiedCardinality>
                <owl:onDataRange rdf:resource="http://www.sisostds.org/ontologies/C2SIM#UUIDBase"/>
            </owl:Restriction>
        </rdfs:subClassOf>
        <rdfs:subClassOf>
            <owl:Restriction>
                <owl:onProperty rdf:resource="http://www.sisostds.org/ontologies/lox#isActive"/>
                <owl:qualifiedCardinality rdf:datatype="http://www.w3.org/2001/XMLSchema#nonNegativeInteger">1</owl:qualifiedCardinality>
                <owl:onDataRange rdf:resource="http://www.w3.org/2001/XMLSchema#boolean"/>
            </owl:Restriction>
        </rdfs:subClassOf>
        <rdfs:subClassOf>
            <owl:Restriction>
                <owl:onProperty rdf:resource="http://www.sisostds.org/ontologies/lox#isComplete"/>
                <owl:qualifiedCardinality rdf:datatype="http://www.w3.org/2001/XMLSchema#nonNegativeInteger">1</owl:qualifiedCardinality>
                <owl:onDataRange rdf:resource="http://www.w3.org/2001/XMLSchema#boolean"/>
            </owl:Restriction>
        </rdfs:subClassOf>
        <rdfs:comment>A plan for a unit. A PlanPhase may a single task for a unit, or tasks for multiple units (one each), or (recursively) multiple subphases.
Phases have completion conditions that indicate when they are complete, as well as Boolean flags that indicate whether the phase is active and whether it is complete.
Phases have trigger conditions that indicate when they start.  Phases may start on the completion of another phase--thus forming a task sequence--on receipt of an order, or at the time of an Event.
 A sequence of tasks for one unit is normally represented as a sequence of subphases in order to express the triggering conditions for each task; however a set of tasks for a unit may be included in a phase and executed with some implicit sequencing such as task time.</rdfs:comment>
    </owl:Class>
    


    <!-- http://www.sisostds.org/ontologies/lox#PlanPhaseCompletionCondition -->

    <owl:Class rdf:about="http://www.sisostds.org/ontologies/lox#PlanPhaseCompletionCondition">
        <rdfs:subClassOf rdf:resource="http://www.sisostds.org/ontologies/C2SIM#Code"/>
    </owl:Class>
    


    <!-- http://www.sisostds.org/ontologies/lox#PlanPhaseTrigger -->

    <owl:Class rdf:about="http://www.sisostds.org/ontologies/lox#PlanPhaseTrigger">
        <rdfs:subClassOf rdf:resource="http://www.sisostds.org/ontologies/C2SIM#C2SIMContent"/>
        <rdfs:comment>This is a condition that causes the start of execution of a PlanPhase.</rdfs:comment>
    </owl:Class>
    


    <!-- http://www.sisostds.org/ontologies/lox#PriorPhaseCompletionTrigger -->

    <owl:Class rdf:about="http://www.sisostds.org/ontologies/lox#PriorPhaseCompletionTrigger">
        <rdfs:subClassOf rdf:resource="http://www.sisostds.org/ontologies/lox#PlanPhaseTrigger"/>
        <rdfs:subClassOf>
            <owl:Restriction>
                <owl:onProperty rdf:resource="http://www.sisostds.org/ontologies/lox#hasTriggerPhase"/>
                <owl:qualifiedCardinality rdf:datatype="http://www.w3.org/2001/XMLSchema#nonNegativeInteger">1</owl:qualifiedCardinality>
                <owl:onDataRange rdf:resource="http://www.sisostds.org/ontologies/C2SIM#UUIDBase"/>
            </owl:Restriction>
        </rdfs:subClassOf>
    </owl:Class>
    


    <!-- http://www.sisostds.org/ontologies/lox#TaskFunctionalAssociationCode -->

    <owl:Class rdf:about="http://www.sisostds.org/ontologies/lox#TaskFunctionalAssociationCode">
        <rdfs:subClassOf rdf:resource="http://www.sisostds.org/ontologies/C2SIM#Code"/>
        <rdfs:comment>Instances of this code will be taken from JC3IEDM 3.1.4, 	action-functional-association-category-code</rdfs:comment>
    </owl:Class>
    


    <!-- http://www.sisostds.org/ontologies/smx#APP6-SIDC -->

    <owl:Class rdf:about="http://www.sisostds.org/ontologies/smx#APP6-SIDC">
        <rdfs:subClassOf rdf:resource="http://www.sisostds.org/ontologies/C2SIM#EntityType"/>
        <rdfs:subClassOf>
            <owl:Restriction>
                <owl:onProperty rdf:resource="http://www.sisostds.org/ontologies/smx#hasSIDCString"/>
                <owl:qualifiedCardinality rdf:datatype="http://www.w3.org/2001/XMLSchema#nonNegativeInteger">1</owl:qualifiedCardinality>
                <owl:onDataRange rdf:resource="http://www.w3.org/2001/XMLSchema#string"/>
            </owl:Restriction>
        </rdfs:subClassOf>
    </owl:Class>
    <owl:Axiom>
        <owl:annotatedSource rdf:resource="http://www.sisostds.org/ontologies/smx#APP6-SIDC"/>
        <owl:annotatedProperty rdf:resource="http://www.w3.org/2000/01/rdf-schema#subClassOf"/>
        <owl:annotatedTarget>
            <owl:Restriction>
                <owl:onProperty rdf:resource="http://www.sisostds.org/ontologies/smx#hasSIDCString"/>
                <owl:qualifiedCardinality rdf:datatype="http://www.w3.org/2001/XMLSchema#nonNegativeInteger">1</owl:qualifiedCardinality>
                <owl:onDataRange rdf:resource="http://www.w3.org/2001/XMLSchema#string"/>
            </owl:Restriction>
        </owl:annotatedTarget>
        <rdfs:comment>The string should have restrictions placed on it, e.g. 15 characters, etc.</rdfs:comment>
    </owl:Axiom>
    


    <!-- http://www.sisostds.org/ontologies/smx#ActivityObservation -->

    <owl:Class rdf:about="http://www.sisostds.org/ontologies/smx#ActivityObservation">
        <rdfs:subClassOf rdf:resource="http://www.sisostds.org/ontologies/smx#Observation"/>
        <rdfs:comment>An observation of the activity of the subject.</rdfs:comment>
    </owl:Class>
    


    <!-- http://www.sisostds.org/ontologies/smx#Aircraft -->

    <owl:Class rdf:about="http://www.sisostds.org/ontologies/smx#Aircraft">
        <rdfs:subClassOf rdf:resource="http://www.sisostds.org/ontologies/C2SIM#Platform"/>
        <rdfs:subClassOf>
            <owl:Restriction>
                <owl:onProperty rdf:resource="http://www.sisostds.org/ontologies/smx#hasAircraftTypeCategoryCode"/>
                <owl:maxQualifiedCardinality rdf:datatype="http://www.w3.org/2001/XMLSchema#nonNegativeInteger">1</owl:maxQualifiedCardinality>
                <owl:onClass rdf:resource="http://www.sisostds.org/ontologies/smx#AircraftTypeCategoryCode"/>
            </owl:Restriction>
        </rdfs:subClassOf>
    </owl:Class>
    


    <!-- http://www.sisostds.org/ontologies/smx#AircraftTypeCategoryCode -->

    <owl:Class rdf:about="http://www.sisostds.org/ontologies/smx#AircraftTypeCategoryCode">
        <rdfs:subClassOf rdf:resource="http://www.sisostds.org/ontologies/smx#MIPCategoryCode"/>
        <rdfs:comment>Instances of this class (code values) to be taken from JC3IEDM 3.1.4 AircraftTypeCategoryCode</rdfs:comment>
    </owl:Class>
    


    <!-- http://www.sisostds.org/ontologies/smx#Ammunition -->

    <owl:Class rdf:about="http://www.sisostds.org/ontologies/smx#Ammunition">
        <rdfs:subClassOf rdf:resource="http://www.sisostds.org/ontologies/C2SIM#ConsumableMaterial"/>
        <rdfs:subClassOf>
            <owl:Restriction>
                <owl:onProperty rdf:resource="http://www.sisostds.org/ontologies/smx#hasAmmunitionTypeCategoryCode"/>
                <owl:qualifiedCardinality rdf:datatype="http://www.w3.org/2001/XMLSchema#nonNegativeInteger">1</owl:qualifiedCardinality>
                <owl:onClass rdf:resource="http://www.sisostds.org/ontologies/smx#AmmunitionTypeCategoryCode"/>
            </owl:Restriction>
        </rdfs:subClassOf>
        <rdfs:comment>A CONSUMABLE-MATERIEL-TYPE that is a complete device charged with explosives, propellants, pyrotechnics, initiating composition, or nuclear, biological, or chemical material for use in military operations.</rdfs:comment>
    </owl:Class>
    


    <!-- http://www.sisostds.org/ontologies/smx#AmmunitionTypeCategoryCode -->

    <owl:Class rdf:about="http://www.sisostds.org/ontologies/smx#AmmunitionTypeCategoryCode">
        <rdfs:subClassOf rdf:resource="http://www.sisostds.org/ontologies/smx#MIPCategoryCode"/>
        <rdfs:comment>Instances of this class (code values) to be taken from JC3IEDM 3.1.4 AmmunitionTypeCategoryCode</rdfs:comment>
    </owl:Class>
    


    <!-- http://www.sisostds.org/ontologies/smx#Boundary -->

    <owl:Class rdf:about="http://www.sisostds.org/ontologies/smx#Boundary">
        <rdfs:subClassOf rdf:resource="http://www.co-ode.org/ontologies/ont.owl#Line"/>
        <rdfs:subClassOf>
            <owl:Restriction>
                <owl:onProperty rdf:resource="http://www.sisostds.org/ontologies/C2SIM#hasLocation"/>
                <owl:qualifiedCardinality rdf:datatype="http://www.w3.org/2001/XMLSchema#nonNegativeInteger">2</owl:qualifiedCardinality>
                <owl:onClass rdf:resource="http://www.sisostds.org/ontologies/C2SIM#GeodeticCoordinate"/>
            </owl:Restriction>
        </rdfs:subClassOf>
        <rdfs:comment>Does this have any properties that are not also properties of a line? If so this should be promoted to be under TacticalGraphic.</rdfs:comment>
    </owl:Class>
    


    <!-- http://www.sisostds.org/ontologies/smx#DISCountryCode -->

    <owl:Class rdf:about="http://www.sisostds.org/ontologies/smx#DISCountryCode">
        <rdfs:subClassOf rdf:resource="http://www.sisostds.org/ontologies/smx#DISTypeCode"/>
        <rdfs:comment>Instances of this class (code values) to be taken from the DIS standard, SISO-REF-010-2015</rdfs:comment>
    </owl:Class>
    


    <!-- http://www.sisostds.org/ontologies/smx#DISDomainCode -->

    <owl:Class rdf:about="http://www.sisostds.org/ontologies/smx#DISDomainCode">
        <rdfs:subClassOf rdf:resource="http://www.sisostds.org/ontologies/smx#DISTypeCode"/>
    </owl:Class>
    


    <!-- http://www.sisostds.org/ontologies/smx#DISEntityType -->

    <owl:Class rdf:about="http://www.sisostds.org/ontologies/smx#DISEntityType">
        <rdfs:subClassOf rdf:resource="http://www.sisostds.org/ontologies/C2SIM#EntityType"/>
        <rdfs:subClassOf>
            <owl:Restriction>
                <owl:onProperty rdf:resource="http://www.sisostds.org/ontologies/smx#hasDISCountryCode"/>
                <owl:qualifiedCardinality rdf:datatype="http://www.w3.org/2001/XMLSchema#nonNegativeInteger">1</owl:qualifiedCardinality>
                <owl:onClass rdf:resource="http://www.sisostds.org/ontologies/smx#DISCountryCode"/>
            </owl:Restriction>
        </rdfs:subClassOf>
        <rdfs:subClassOf>
            <owl:Restriction>
                <owl:onProperty rdf:resource="http://www.sisostds.org/ontologies/smx#hasDISDomainCode"/>
                <owl:qualifiedCardinality rdf:datatype="http://www.w3.org/2001/XMLSchema#nonNegativeInteger">1</owl:qualifiedCardinality>
                <owl:onClass rdf:resource="http://www.sisostds.org/ontologies/smx#DISDomainCode"/>
            </owl:Restriction>
        </rdfs:subClassOf>
        <rdfs:subClassOf>
            <owl:Restriction>
                <owl:onProperty rdf:resource="http://www.sisostds.org/ontologies/smx#hasDISKindCode"/>
                <owl:qualifiedCardinality rdf:datatype="http://www.w3.org/2001/XMLSchema#nonNegativeInteger">1</owl:qualifiedCardinality>
                <owl:onClass rdf:resource="http://www.sisostds.org/ontologies/smx#DISKindCode"/>
            </owl:Restriction>
        </rdfs:subClassOf>
        <rdfs:subClassOf>
            <owl:Restriction>
                <owl:onProperty rdf:resource="http://www.sisostds.org/ontologies/smx#hasDISCategory"/>
                <owl:qualifiedCardinality rdf:datatype="http://www.w3.org/2001/XMLSchema#nonNegativeInteger">1</owl:qualifiedCardinality>
                <owl:onDataRange rdf:resource="http://www.w3.org/2001/XMLSchema#byte"/>
            </owl:Restriction>
        </rdfs:subClassOf>
        <rdfs:subClassOf>
            <owl:Restriction>
                <owl:onProperty rdf:resource="http://www.sisostds.org/ontologies/smx#hasDISExtra"/>
                <owl:qualifiedCardinality rdf:datatype="http://www.w3.org/2001/XMLSchema#nonNegativeInteger">1</owl:qualifiedCardinality>
                <owl:onDataRange rdf:resource="http://www.w3.org/2001/XMLSchema#byte"/>
            </owl:Restriction>
        </rdfs:subClassOf>
        <rdfs:subClassOf>
            <owl:Restriction>
                <owl:onProperty rdf:resource="http://www.sisostds.org/ontologies/smx#hasDISSpecific"/>
                <owl:qualifiedCardinality rdf:datatype="http://www.w3.org/2001/XMLSchema#nonNegativeInteger">1</owl:qualifiedCardinality>
                <owl:onDataRange rdf:resource="http://www.w3.org/2001/XMLSchema#byte"/>
            </owl:Restriction>
        </rdfs:subClassOf>
        <rdfs:subClassOf>
            <owl:Restriction>
                <owl:onProperty rdf:resource="http://www.sisostds.org/ontologies/smx#hasDISSubCategory"/>
                <owl:qualifiedCardinality rdf:datatype="http://www.w3.org/2001/XMLSchema#nonNegativeInteger">1</owl:qualifiedCardinality>
                <owl:onDataRange rdf:resource="http://www.w3.org/2001/XMLSchema#byte"/>
            </owl:Restriction>
        </rdfs:subClassOf>
    </owl:Class>
    


    <!-- http://www.sisostds.org/ontologies/smx#DISKindCode -->

    <owl:Class rdf:about="http://www.sisostds.org/ontologies/smx#DISKindCode">
        <rdfs:subClassOf rdf:resource="http://www.sisostds.org/ontologies/smx#DISTypeCode"/>
    </owl:Class>
    


    <!-- http://www.sisostds.org/ontologies/smx#DISTypeCode -->

    <owl:Class rdf:about="http://www.sisostds.org/ontologies/smx#DISTypeCode">
        <rdfs:subClassOf rdf:resource="http://www.sisostds.org/ontologies/C2SIM#Code"/>
    </owl:Class>
    


    <!-- http://www.sisostds.org/ontologies/smx#EchelonCode -->

    <owl:Class rdf:about="http://www.sisostds.org/ontologies/smx#EchelonCode">
        <rdfs:subClassOf rdf:resource="http://www.sisostds.org/ontologies/C2SIM#Code"/>
    </owl:Class>
    


    <!-- http://www.sisostds.org/ontologies/smx#Force -->

    <owl:Class rdf:about="http://www.sisostds.org/ontologies/smx#Force">
        <rdfs:subClassOf rdf:resource="http://www.sisostds.org/ontologies/C2SIM#MilitaryOrganization"/>
    </owl:Class>
    


    <!-- http://www.sisostds.org/ontologies/smx#ForceSide -->

    <owl:Class rdf:about="http://www.sisostds.org/ontologies/smx#ForceSide">
        <rdfs:subClassOf rdf:resource="http://www.sisostds.org/ontologies/C2SIM#AbstractObject"/>
        <rdfs:subClassOf>
            <owl:Restriction>
                <owl:onProperty rdf:resource="http://www.sisostds.org/ontologies/smx#hasSideHostilityCode"/>
                <owl:qualifiedCardinality rdf:datatype="http://www.w3.org/2001/XMLSchema#nonNegativeInteger">1</owl:qualifiedCardinality>
                <owl:onClass rdf:resource="http://www.sisostds.org/ontologies/smx#SideHostilityCode"/>
            </owl:Restriction>
        </rdfs:subClassOf>
    </owl:Class>
    


    <!-- http://www.sisostds.org/ontologies/smx#GeocentricCoordinateValue -->

    <owl:Class rdf:about="http://www.sisostds.org/ontologies/smx#GeocentricCoordinateValue">
        <rdfs:subClassOf rdf:resource="http://www.sisostds.org/ontologies/C2SIM#Coordinate"/>
        <rdfs:subClassOf>
            <owl:Restriction>
                <owl:onProperty rdf:resource="http://www.sisostds.org/ontologies/C2SIM#hasX"/>
                <owl:qualifiedCardinality rdf:datatype="http://www.w3.org/2001/XMLSchema#nonNegativeInteger">1</owl:qualifiedCardinality>
                <owl:onDataRange rdf:resource="http://www.w3.org/2001/XMLSchema#double"/>
            </owl:Restriction>
        </rdfs:subClassOf>
        <rdfs:subClassOf>
            <owl:Restriction>
                <owl:onProperty rdf:resource="http://www.sisostds.org/ontologies/C2SIM#hasY"/>
                <owl:qualifiedCardinality rdf:datatype="http://www.w3.org/2001/XMLSchema#nonNegativeInteger">1</owl:qualifiedCardinality>
                <owl:onDataRange rdf:resource="http://www.w3.org/2001/XMLSchema#double"/>
            </owl:Restriction>
        </rdfs:subClassOf>
        <rdfs:subClassOf>
            <owl:Restriction>
                <owl:onProperty rdf:resource="http://www.sisostds.org/ontologies/C2SIM#hasZ"/>
                <owl:qualifiedCardinality rdf:datatype="http://www.w3.org/2001/XMLSchema#nonNegativeInteger">1</owl:qualifiedCardinality>
                <owl:onDataRange rdf:resource="http://www.w3.org/2001/XMLSchema#double"/>
            </owl:Restriction>
        </rdfs:subClassOf>
    </owl:Class>
    


    <!-- http://www.sisostds.org/ontologies/smx#HealthObservation -->

    <owl:Class rdf:about="http://www.sisostds.org/ontologies/smx#HealthObservation">
        <rdfs:subClassOf rdf:resource="http://www.sisostds.org/ontologies/smx#Observation"/>
        <rdfs:comment>An observation of the health state of a subject; for example operational status or resource count.</rdfs:comment>
    </owl:Class>
    


    <!-- http://www.sisostds.org/ontologies/smx#LocationObservation -->

    <owl:Class rdf:about="http://www.sisostds.org/ontologies/smx#LocationObservation">
        <rdfs:subClassOf rdf:resource="http://www.sisostds.org/ontologies/smx#Observation"/>
        <rdfs:subClassOf>
            <owl:Restriction>
                <owl:onProperty rdf:resource="http://www.sisostds.org/ontologies/C2SIM#hasLocation"/>
                <owl:qualifiedCardinality rdf:datatype="http://www.w3.org/2001/XMLSchema#nonNegativeInteger">1</owl:qualifiedCardinality>
                <owl:onClass rdf:resource="http://www.sisostds.org/ontologies/C2SIM#Coordinate"/>
            </owl:Restriction>
        </rdfs:subClassOf>
        <rdfs:comment>An observation of the location of a subject.</rdfs:comment>
    </owl:Class>
    


    <!-- http://www.sisostds.org/ontologies/smx#METOCGraphic -->

    <owl:Class rdf:about="http://www.sisostds.org/ontologies/smx#METOCGraphic">
        <rdfs:subClassOf rdf:resource="http://www.sisostds.org/ontologies/C2SIM#MapGraphic"/>
        <rdfs:comment>Specifies the MIL-STD-2525B-based meteorological conditions of the environment.</rdfs:comment>
    </owl:Class>
    


    <!-- http://www.sisostds.org/ontologies/smx#MIPCategoryCode -->

    <owl:Class rdf:about="http://www.sisostds.org/ontologies/smx#MIPCategoryCode">
        <rdfs:subClassOf rdf:resource="http://www.sisostds.org/ontologies/C2SIM#Code"/>
    </owl:Class>
    


    <!-- http://www.sisostds.org/ontologies/smx#NameObservation -->

    <owl:Class rdf:about="http://www.sisostds.org/ontologies/smx#NameObservation">
        <rdfs:subClassOf rdf:resource="http://www.sisostds.org/ontologies/smx#Observation"/>
        <rdfs:comment>An observation of the unit name of the subject.</rdfs:comment>
    </owl:Class>
    


    <!-- http://www.sisostds.org/ontologies/smx#Observation -->

    <owl:Class rdf:about="http://www.sisostds.org/ontologies/smx#Observation">
        <rdfs:subClassOf rdf:resource="http://www.sisostds.org/ontologies/C2SIM#C2SIMContent"/>
        <rdfs:subClassOf>
            <owl:Restriction>
                <owl:onProperty rdf:resource="http://www.sisostds.org/ontologies/smx#hasConfidenceLevel"/>
                <owl:qualifiedCardinality rdf:datatype="http://www.w3.org/2001/XMLSchema#nonNegativeInteger">1</owl:qualifiedCardinality>
                <owl:onDataRange rdf:resource="http://www.w3.org/2001/XMLSchema#double"/>
            </owl:Restriction>
        </rdfs:subClassOf>
        <rdfs:subClassOf>
            <owl:Restriction>
                <owl:onProperty rdf:resource="http://www.sisostds.org/ontologies/smx#hasUncertaintyInterval"/>
                <owl:qualifiedCardinality rdf:datatype="http://www.w3.org/2001/XMLSchema#nonNegativeInteger">1</owl:qualifiedCardinality>
                <owl:onDataRange rdf:resource="http://www.w3.org/2001/XMLSchema#double"/>
            </owl:Restriction>
        </rdfs:subClassOf>
        <rdfs:comment>This is an observation of the state of something in the world; generally an actor, but possibly anything that is an entity. Subclasses define specific observations that can be made.
The subclasses defined here are sufficient to create a report with Size, Activity, Location, Unit Identification, Time, and Equipment, or some subset of that.</rdfs:comment>
    </owl:Class>
    <owl:Axiom>
        <owl:annotatedSource rdf:resource="http://www.sisostds.org/ontologies/smx#Observation"/>
        <owl:annotatedProperty rdf:resource="http://www.w3.org/2000/01/rdf-schema#subClassOf"/>
        <owl:annotatedTarget>
            <owl:Restriction>
                <owl:onProperty rdf:resource="http://www.sisostds.org/ontologies/smx#hasConfidenceLevel"/>
                <owl:qualifiedCardinality rdf:datatype="http://www.w3.org/2001/XMLSchema#nonNegativeInteger">1</owl:qualifiedCardinality>
                <owl:onDataRange rdf:resource="http://www.w3.org/2001/XMLSchema#double"/>
            </owl:Restriction>
        </owl:annotatedTarget>
        <rdfs:comment>This is the probabilty that the reported value is correct.
A value between 0 and 1.</rdfs:comment>
    </owl:Axiom>
    <owl:Axiom>
        <owl:annotatedSource rdf:resource="http://www.sisostds.org/ontologies/smx#Observation"/>
        <owl:annotatedProperty rdf:resource="http://www.w3.org/2000/01/rdf-schema#subClassOf"/>
        <owl:annotatedTarget>
            <owl:Restriction>
                <owl:onProperty rdf:resource="http://www.sisostds.org/ontologies/smx#hasUncertaintyInterval"/>
                <owl:qualifiedCardinality rdf:datatype="http://www.w3.org/2001/XMLSchema#nonNegativeInteger">1</owl:qualifiedCardinality>
                <owl:onDataRange rdf:resource="http://www.w3.org/2001/XMLSchema#double"/>
            </owl:Restriction>
        </owl:annotatedTarget>
        <rdfs:comment>Uncertainty Interval is an optional qualification on an observation of a real-valued phenomenon. This is the size of the range of values (the reported value is the center) that the phenomenon could actually have. In two or three dimensions, this could be the diameter of a circle of uncertainty. The probability that the observation is in this range should be given by the ConfidenceLevel.</rdfs:comment>
    </owl:Axiom>
    


    <!-- http://www.sisostds.org/ontologies/smx#ObservationReportContent -->

    <owl:Class rdf:about="http://www.sisostds.org/ontologies/smx#ObservationReportContent">
        <rdfs:subClassOf rdf:resource="http://www.sisostds.org/ontologies/C2SIM#ReportContent"/>
        <rdfs:subClassOf>
            <owl:Restriction>
                <owl:onProperty rdf:resource="http://www.sisostds.org/ontologies/smx#hasObservation"/>
                <owl:qualifiedCardinality rdf:datatype="http://www.w3.org/2001/XMLSchema#nonNegativeInteger">1</owl:qualifiedCardinality>
                <owl:onClass rdf:resource="http://www.sisostds.org/ontologies/smx#Observation"/>
            </owl:Restriction>
        </rdfs:subClassOf>
        <rdfs:comment>This report contains an observation of some aspect of a subject--not necessarily including the location, health, or other facts that are in a position report.</rdfs:comment>
    </owl:Class>
    


    <!-- http://www.sisostds.org/ontologies/smx#PersonTypeCategoryCode -->

    <owl:Class rdf:about="http://www.sisostds.org/ontologies/smx#PersonTypeCategoryCode">
        <rdfs:subClassOf rdf:resource="http://www.sisostds.org/ontologies/smx#MIPCategoryCode"/>
        <rdfs:comment>Instances of this class (code values) to be taken from JC3IEDM 3.1.4 PersonTypeCategoryCode</rdfs:comment>
    </owl:Class>
    


    <!-- http://www.sisostds.org/ontologies/smx#ReinforcedReducedType -->

    <owl:Class rdf:about="http://www.sisostds.org/ontologies/smx#ReinforcedReducedType">
        <rdfs:subClassOf rdf:resource="http://www.sisostds.org/ontologies/C2SIM#Code"/>
    </owl:Class>
    


    <!-- http://www.sisostds.org/ontologies/smx#RouteWhere -->

    <owl:Class rdf:about="http://www.sisostds.org/ontologies/smx#RouteWhere">
        <rdfs:subClassOf rdf:resource="http://www.co-ode.org/ontologies/ont.owl#Line"/>
    </owl:Class>
    


    <!-- http://www.sisostds.org/ontologies/smx#SideHostilityCode -->

    <owl:Class rdf:about="http://www.sisostds.org/ontologies/smx#SideHostilityCode">
        <rdfs:subClassOf rdf:resource="http://www.sisostds.org/ontologies/C2SIM#Code"/>
    </owl:Class>
    


    <!-- http://www.sisostds.org/ontologies/smx#SubjectTypeObservation -->

    <owl:Class rdf:about="http://www.sisostds.org/ontologies/smx#SubjectTypeObservation">
        <rdfs:subClassOf rdf:resource="http://www.sisostds.org/ontologies/smx#Observation"/>
        <rdfs:subClassOf>
            <owl:Restriction>
                <owl:onProperty rdf:resource="http://www.sisostds.org/ontologies/C2SIM#hasEntityType"/>
                <owl:maxQualifiedCardinality rdf:datatype="http://www.w3.org/2001/XMLSchema#nonNegativeInteger">1</owl:maxQualifiedCardinality>
                <owl:onClass rdf:resource="http://www.sisostds.org/ontologies/C2SIM#EntityType"/>
            </owl:Restriction>
        </rdfs:subClassOf>
        <rdfs:comment>An observation of the type of the subject.</rdfs:comment>
    </owl:Class>
    <owl:Axiom>
        <owl:annotatedSource rdf:resource="http://www.sisostds.org/ontologies/smx#SubjectTypeObservation"/>
        <owl:annotatedProperty rdf:resource="http://www.w3.org/2000/01/rdf-schema#subClassOf"/>
        <owl:annotatedTarget>
            <owl:Restriction>
                <owl:onProperty rdf:resource="http://www.sisostds.org/ontologies/C2SIM#hasEntityType"/>
                <owl:maxQualifiedCardinality rdf:datatype="http://www.w3.org/2001/XMLSchema#nonNegativeInteger">1</owl:maxQualifiedCardinality>
                <owl:onClass rdf:resource="http://www.sisostds.org/ontologies/C2SIM#EntityType"/>
            </owl:Restriction>
        </owl:annotatedTarget>
        <rdfs:comment>The cardinality here is max 1, i.e. the data is optional. This permits future ontology extensions to make subclasses where only part of the type information is observed. For example, observing that the subject is a vehicle but not identifying it.</rdfs:comment>
    </owl:Axiom>
    


    <!-- http://www.sisostds.org/ontologies/smx#SubsurfaceVessel -->

    <owl:Class rdf:about="http://www.sisostds.org/ontologies/smx#SubsurfaceVessel">
        <rdfs:subClassOf rdf:resource="http://www.sisostds.org/ontologies/C2SIM#Platform"/>
        <rdfs:subClassOf>
            <owl:Restriction>
                <owl:onProperty rdf:resource="http://www.sisostds.org/ontologies/smx#hasSubsurfaceVesselTypeCode"/>
                <owl:maxQualifiedCardinality rdf:datatype="http://www.w3.org/2001/XMLSchema#nonNegativeInteger">1</owl:maxQualifiedCardinality>
                <owl:onClass rdf:resource="http://www.sisostds.org/ontologies/smx#SubsurfaceVesselTypeCode"/>
            </owl:Restriction>
        </rdfs:subClassOf>
    </owl:Class>
    


    <!-- http://www.sisostds.org/ontologies/smx#SubsurfaceVesselTypeCode -->

    <owl:Class rdf:about="http://www.sisostds.org/ontologies/smx#SubsurfaceVesselTypeCode">
        <rdfs:subClassOf rdf:resource="http://www.sisostds.org/ontologies/smx#VesselTypeCategoryCode"/>
        <rdfs:comment>Instances of this class (code values) to be taken from JC3IEDM 3.1.4 SubsurfaceVesselTypeCategoryCode</rdfs:comment>
    </owl:Class>
    


    <!-- http://www.sisostds.org/ontologies/smx#SurfaceVessel -->

    <owl:Class rdf:about="http://www.sisostds.org/ontologies/smx#SurfaceVessel">
        <rdfs:subClassOf rdf:resource="http://www.sisostds.org/ontologies/C2SIM#Platform"/>
        <rdfs:subClassOf>
            <owl:Restriction>
                <owl:onProperty rdf:resource="http://www.sisostds.org/ontologies/smx#hasSurfaceVesselTypeCode"/>
                <owl:maxQualifiedCardinality rdf:datatype="http://www.w3.org/2001/XMLSchema#nonNegativeInteger">1</owl:maxQualifiedCardinality>
                <owl:onClass rdf:resource="http://www.sisostds.org/ontologies/smx#SurfaceVesselTypeCode"/>
            </owl:Restriction>
        </rdfs:subClassOf>
    </owl:Class>
    


    <!-- http://www.sisostds.org/ontologies/smx#SurfaceVesselTypeCode -->

    <owl:Class rdf:about="http://www.sisostds.org/ontologies/smx#SurfaceVesselTypeCode">
        <rdfs:subClassOf rdf:resource="http://www.sisostds.org/ontologies/smx#VesselTypeCategoryCode"/>
        <rdfs:comment>Instances of this class (code values) to be taken from JC3IEDM 3.1.4 SurfaceVesselTypeCategoryCode</rdfs:comment>
    </owl:Class>
    


    <!-- http://www.sisostds.org/ontologies/smx#TacticalGraphic -->

    <owl:Class rdf:about="http://www.sisostds.org/ontologies/smx#TacticalGraphic">
        <rdfs:subClassOf rdf:resource="http://www.sisostds.org/ontologies/C2SIM#MapGraphic"/>
        <rdfs:subClassOf>
            <owl:Restriction>
                <owl:onProperty rdf:resource="http://www.sisostds.org/ontologies/smx#hasAPP6-SIDC"/>
                <owl:qualifiedCardinality rdf:datatype="http://www.w3.org/2001/XMLSchema#nonNegativeInteger">1</owl:qualifiedCardinality>
                <owl:onClass rdf:resource="http://www.sisostds.org/ontologies/smx#APP6-SIDC"/>
            </owl:Restriction>
        </rdfs:subClassOf>
        <rdfs:subClassOf>
            <owl:Restriction>
                <owl:onProperty rdf:resource="http://www.sisostds.org/ontologies/smx#hasOwner"/>
                <owl:maxQualifiedCardinality rdf:datatype="http://www.w3.org/2001/XMLSchema#nonNegativeInteger">1</owl:maxQualifiedCardinality>
                <owl:onDataRange rdf:resource="http://www.sisostds.org/ontologies/C2SIM#UUIDBase"/>
            </owl:Restriction>
        </rdfs:subClassOf>
    </owl:Class>
    


    <!-- http://www.sisostds.org/ontologies/smx#Unit -->

    <owl:Class rdf:about="http://www.sisostds.org/ontologies/smx#Unit">
        <rdfs:subClassOf rdf:resource="http://www.sisostds.org/ontologies/C2SIM#MilitaryOrganization"/>
        <rdfs:subClassOf>
            <owl:Restriction>
                <owl:onProperty rdf:resource="http://www.sisostds.org/ontologies/C2SIM_SMX_LOX#hasLeftBoundary"/>
                <owl:maxQualifiedCardinality rdf:datatype="http://www.w3.org/2001/XMLSchema#nonNegativeInteger">1</owl:maxQualifiedCardinality>
                <owl:onDataRange rdf:resource="http://www.sisostds.org/ontologies/C2SIM#UUIDBase"/>
            </owl:Restriction>
        </rdfs:subClassOf>
        <rdfs:subClassOf>
            <owl:Restriction>
                <owl:onProperty rdf:resource="http://www.sisostds.org/ontologies/C2SIM_SMX_LOX#hasRightBoundary"/>
                <owl:maxQualifiedCardinality rdf:datatype="http://www.w3.org/2001/XMLSchema#nonNegativeInteger">1</owl:maxQualifiedCardinality>
                <owl:onDataRange rdf:resource="http://www.sisostds.org/ontologies/C2SIM#UUIDBase"/>
            </owl:Restriction>
        </rdfs:subClassOf>
    </owl:Class>
    


    <!-- http://www.sisostds.org/ontologies/smx#UnitOperationalStatusCode -->

    <owl:Class rdf:about="http://www.sisostds.org/ontologies/smx#UnitOperationalStatusCode">
        <rdfs:subClassOf rdf:resource="http://www.sisostds.org/ontologies/C2SIM#OperationalStatusCode"/>
    </owl:Class>
    


    <!-- http://www.sisostds.org/ontologies/smx#UnitSymbol -->

    <owl:Class rdf:about="http://www.sisostds.org/ontologies/smx#UnitSymbol">
        <rdfs:subClassOf rdf:resource="http://www.sisostds.org/ontologies/smx#TacticalGraphic"/>
        <rdfs:subClassOf>
            <owl:Restriction>
                <owl:onProperty rdf:resource="http://www.sisostds.org/ontologies/smx#hasCombatEffectiveness"/>
                <owl:maxQualifiedCardinality rdf:datatype="http://www.w3.org/2001/XMLSchema#nonNegativeInteger">1</owl:maxQualifiedCardinality>
                <owl:onClass rdf:resource="http://www.sisostds.org/ontologies/C2SIM#OperationalStatus"/>
            </owl:Restriction>
        </rdfs:subClassOf>
        <rdfs:subClassOf>
            <owl:Restriction>
                <owl:onProperty rdf:resource="http://www.sisostds.org/ontologies/smx#hasReinforcedReducedType"/>
                <owl:maxQualifiedCardinality rdf:datatype="http://www.w3.org/2001/XMLSchema#nonNegativeInteger">1</owl:maxQualifiedCardinality>
                <owl:onClass rdf:resource="http://www.sisostds.org/ontologies/smx#ReinforcedReducedType"/>
            </owl:Restriction>
        </rdfs:subClassOf>
        <rdfs:subClassOf>
            <owl:Restriction>
                <owl:onProperty rdf:resource="http://www.sisostds.org/ontologies/smx#hasHigherFormation"/>
                <owl:maxQualifiedCardinality rdf:datatype="http://www.w3.org/2001/XMLSchema#nonNegativeInteger">1</owl:maxQualifiedCardinality>
                <owl:onDataRange rdf:resource="http://www.w3.org/2001/XMLSchema#string"/>
            </owl:Restriction>
        </rdfs:subClassOf>
        <rdfs:subClassOf>
            <owl:Restriction>
                <owl:onProperty rdf:resource="http://www.sisostds.org/ontologies/smx#hasSpecialC2HQ"/>
                <owl:maxQualifiedCardinality rdf:datatype="http://www.w3.org/2001/XMLSchema#nonNegativeInteger">1</owl:maxQualifiedCardinality>
                <owl:onDataRange rdf:resource="http://www.w3.org/2001/XMLSchema#string"/>
            </owl:Restriction>
        </rdfs:subClassOf>
    </owl:Class>
    


    <!-- http://www.sisostds.org/ontologies/smx#Vehicle -->

    <owl:Class rdf:about="http://www.sisostds.org/ontologies/smx#Vehicle">
        <rdfs:subClassOf rdf:resource="http://www.sisostds.org/ontologies/C2SIM#Platform"/>
        <rdfs:subClassOf>
            <owl:Restriction>
                <owl:onProperty rdf:resource="http://www.sisostds.org/ontologies/smx#hasVehicleTypeCategoryCode"/>
                <owl:maxQualifiedCardinality rdf:datatype="http://www.w3.org/2001/XMLSchema#nonNegativeInteger">1</owl:maxQualifiedCardinality>
                <owl:onClass rdf:resource="http://www.sisostds.org/ontologies/smx#VehicleTypeCategoryCode"/>
            </owl:Restriction>
        </rdfs:subClassOf>
    </owl:Class>
    


    <!-- http://www.sisostds.org/ontologies/smx#VehicleTypeCategoryCode -->

    <owl:Class rdf:about="http://www.sisostds.org/ontologies/smx#VehicleTypeCategoryCode">
        <rdfs:subClassOf rdf:resource="http://www.sisostds.org/ontologies/smx#MIPCategoryCode"/>
        <rdfs:comment>Instances of this class (code values) to be taken from JC3IEDM 3.1.4 VehicleTypeCategoryCode</rdfs:comment>
    </owl:Class>
    


    <!-- http://www.sisostds.org/ontologies/smx#VesselTypeCategoryCode -->

    <owl:Class rdf:about="http://www.sisostds.org/ontologies/smx#VesselTypeCategoryCode">
        <rdfs:subClassOf rdf:resource="http://www.sisostds.org/ontologies/smx#MIPCategoryCode"/>
    </owl:Class>
    


    <!-- http://www.sisostds.org/ontologies/smx#Weapon -->

    <owl:Class rdf:about="http://www.sisostds.org/ontologies/smx#Weapon">
        <rdfs:subClassOf rdf:resource="http://www.sisostds.org/ontologies/C2SIM#Equipment"/>
        <rdfs:subClassOf>
            <owl:Restriction>
                <owl:onProperty rdf:resource="http://www.sisostds.org/ontologies/smx#hasWeaponTypeCategoryCode"/>
                <owl:qualifiedCardinality rdf:datatype="http://www.w3.org/2001/XMLSchema#nonNegativeInteger">1</owl:qualifiedCardinality>
                <owl:onClass rdf:resource="http://www.sisostds.org/ontologies/smx#WeaponTypeCategoryCode"/>
            </owl:Restriction>
        </rdfs:subClassOf>
        <rdfs:comment>An EQUIPMENT-TYPE of any kind used in warfare or combat to attack and overcome an enemy.
Assumed here that Equipment is used by an Actor, and is not an actor itself. If Equipment can take actions, then it should be a Platform or other Actor Entity.</rdfs:comment>
    </owl:Class>
    


    <!-- http://www.sisostds.org/ontologies/smx#WeaponTypeCategoryCode -->

    <owl:Class rdf:about="http://www.sisostds.org/ontologies/smx#WeaponTypeCategoryCode">
        <rdfs:subClassOf rdf:resource="http://www.sisostds.org/ontologies/smx#MIPCategoryCode"/>
        <rdfs:comment>Instances of this class (code values) to be taken from JC3IEDM 3.1.4 WeaponTypeCategoryCode</rdfs:comment>
    </owl:Class>
    


    <!-- 
    ///////////////////////////////////////////////////////////////////////////////////////
    //
    // Individuals
    //
    ///////////////////////////////////////////////////////////////////////////////////////
     -->

    


    <!-- http://www.sisostds.org/ontologies/C2SIM#ACKFAIL -->

    <owl:NamedIndividual rdf:about="http://www.sisostds.org/ontologies/C2SIM#ACKFAIL">
        <rdf:type rdf:resource="http://www.sisostds.org/ontologies/C2SIM#AcknowledgeTypeCode"/>
    </owl:NamedIndividual>
    


    <!-- http://www.sisostds.org/ontologies/C2SIM#ACKNOTEX -->

    <owl:NamedIndividual rdf:about="http://www.sisostds.org/ontologies/C2SIM#ACKNOTEX">
        <rdf:type rdf:resource="http://www.sisostds.org/ontologies/C2SIM#AcknowledgeTypeCode"/>
    </owl:NamedIndividual>
    


    <!-- http://www.sisostds.org/ontologies/C2SIM#ACKNOTREC -->

    <owl:NamedIndividual rdf:about="http://www.sisostds.org/ontologies/C2SIM#ACKNOTREC">
        <rdf:type rdf:resource="http://www.sisostds.org/ontologies/C2SIM#AcknowledgeTypeCode"/>
    </owl:NamedIndividual>
    


    <!-- http://www.sisostds.org/ontologies/C2SIM#ACKNOTUNDSTD -->

    <owl:NamedIndividual rdf:about="http://www.sisostds.org/ontologies/C2SIM#ACKNOTUNDSTD">
        <rdf:type rdf:resource="http://www.sisostds.org/ontologies/C2SIM#AcknowledgeTypeCode"/>
    </owl:NamedIndividual>
    


    <!-- http://www.sisostds.org/ontologies/C2SIM#ACKRCVD -->

    <owl:NamedIndividual rdf:about="http://www.sisostds.org/ontologies/C2SIM#ACKRCVD">
        <rdf:type rdf:resource="http://www.sisostds.org/ontologies/C2SIM#AcknowledgeTypeCode"/>
    </owl:NamedIndividual>
    


    <!-- http://www.sisostds.org/ontologies/C2SIM#ACKSUCC -->

    <owl:NamedIndividual rdf:about="http://www.sisostds.org/ontologies/C2SIM#ACKSUCC">
        <rdf:type rdf:resource="http://www.sisostds.org/ontologies/C2SIM#AcknowledgeTypeCode"/>
    </owl:NamedIndividual>
    


    <!-- http://www.sisostds.org/ontologies/C2SIM#ACQUIR -->

    <owl:NamedIndividual rdf:about="http://www.sisostds.org/ontologies/C2SIM#ACQUIR">
        <rdf:type rdf:resource="http://www.sisostds.org/ontologies/C2SIM#TaskNameCode"/>
        <rdfs:comment>Documentation: 		
						To detect the presence and location of a target in sufficient detail to permit identification.	
					; Appinfo DisplayValue as &quot;Acquire&quot;</rdfs:comment>
    </owl:NamedIndividual>
    


    <!-- http://www.sisostds.org/ontologies/C2SIM#ADVANC -->

    <owl:NamedIndividual rdf:about="http://www.sisostds.org/ontologies/C2SIM#ADVANC">
        <rdf:type rdf:resource="http://www.sisostds.org/ontologies/C2SIM#TaskNameCode"/>
        <rdfs:comment>Documentation: 		
						To move towards an objective in some form of tactical formation. This is a transitional phase between operations which may or may not result in contact with the enemy.	
					; Appinfo DisplayValue as &quot;Advance&quot;</rdfs:comment>
    </owl:NamedIndividual>
    


    <!-- http://www.sisostds.org/ontologies/C2SIM#AIRDEF -->

    <owl:NamedIndividual rdf:about="http://www.sisostds.org/ontologies/C2SIM#AIRDEF">
        <rdf:type rdf:resource="http://www.sisostds.org/ontologies/C2SIM#TaskNameCode"/>
        <rdfs:comment>Documentation: 		
						To protect and defend an area, a strike attack, an installation or naval forces.	
					; Appinfo DisplayValue as &quot;Air defence&quot;</rdfs:comment>
    </owl:NamedIndividual>
    


    <!-- http://www.sisostds.org/ontologies/C2SIM#AMBUSH -->

    <owl:NamedIndividual rdf:about="http://www.sisostds.org/ontologies/C2SIM#AMBUSH">
        <rdf:type rdf:resource="http://www.sisostds.org/ontologies/C2SIM#TaskNameCode"/>
        <rdfs:comment>Documentation: 		
						To conduct a surprise attack by fire or other destructive means, from concealed positions on a moving or temporarily halted force or group of personnel.	
					; Appinfo DisplayValue as &quot;Ambush&quot;</rdfs:comment>
    </owl:NamedIndividual>
    


    <!-- http://www.sisostds.org/ontologies/C2SIM#ARASLT -->

    <owl:NamedIndividual rdf:about="http://www.sisostds.org/ontologies/C2SIM#ARASLT">
        <rdf:type rdf:resource="http://www.sisostds.org/ontologies/C2SIM#TaskNameCode"/>
        <rdfs:comment>Documentation: 		
						To mount an operation in which assault forces (combat, combat service, and combat service support), using the firepower, mobility, and total integration of helicopter assets, maneuver on the battlefield under the control of the ground or air manoeuvre commander to engage and destroy enemy forces or to seize and hold key terrain.	
					; Appinfo DisplayValue as &quot;Air assault&quot;</rdfs:comment>
    </owl:NamedIndividual>
    


    <!-- http://www.sisostds.org/ontologies/C2SIM#ASSMBL -->

    <owl:NamedIndividual rdf:about="http://www.sisostds.org/ontologies/C2SIM#ASSMBL">
        <rdf:type rdf:resource="http://www.sisostds.org/ontologies/C2SIM#TaskNameCode"/>
        <rdfs:comment>Documentation: 		
						To join together multiple objects in the same area.	
					; Appinfo DisplayValue as &quot;Assemble&quot;</rdfs:comment>
    </owl:NamedIndividual>
    


    <!-- http://www.sisostds.org/ontologies/C2SIM#ATTACK -->

    <owl:NamedIndividual rdf:about="http://www.sisostds.org/ontologies/C2SIM#ATTACK">
        <rdf:type rdf:resource="http://www.sisostds.org/ontologies/C2SIM#TaskNameCode"/>
        <rdfs:comment>Documentation: 		
						To conduct a type of offensive action characterised by coordinated employment of firepower and manoeuvre to close with and destroy or capture the enemy.	
					; Appinfo DisplayValue as &quot;Attack, not otherwise specified&quot;</rdfs:comment>
    </owl:NamedIndividual>
    


    <!-- http://www.sisostds.org/ontologies/C2SIM#ATTRIT -->

    <owl:NamedIndividual rdf:about="http://www.sisostds.org/ontologies/C2SIM#ATTRIT">
        <rdf:type rdf:resource="http://www.sisostds.org/ontologies/C2SIM#TaskNameCode"/>
        <rdfs:comment>Documentation: 		
						To reduce of the effectiveness of a force by causing loss of personnel and materiel.	
					; Appinfo DisplayValue as &quot;Attrit&quot;</rdfs:comment>
    </owl:NamedIndividual>
    


    <!-- http://www.sisostds.org/ontologies/C2SIM#ATTSPT -->

    <owl:NamedIndividual rdf:about="http://www.sisostds.org/ontologies/C2SIM#ATTSPT">
        <rdf:type rdf:resource="http://www.sisostds.org/ontologies/C2SIM#TaskNameCode"/>
        <rdfs:comment>Documentation: 		
						To conduct an offensive operation carried out in conjunction with a main attack and designed to achieve one or more of the following: a. deceive the enemy; b. destroy or pin down enemy forces which could interfere with the main attack; c. control ground whose occupation by the enemy will hinder the main attack; or d. force the enemy to commit reserves prematurely or in an indecisive area.	
					; Appinfo DisplayValue as &quot;Attack, supporting&quot;</rdfs:comment>
    </owl:NamedIndividual>
    


    <!-- http://www.sisostds.org/ontologies/C2SIM#AVOID -->

    <owl:NamedIndividual rdf:about="http://www.sisostds.org/ontologies/C2SIM#AVOID">
        <rdf:type rdf:resource="http://www.sisostds.org/ontologies/C2SIM#TaskNameCode"/>
        <rdfs:comment>Documentation: 		
						To miss or take evading action.	
					; Appinfo DisplayValue as &quot;Avoid&quot;</rdfs:comment>
    </owl:NamedIndividual>
    


    <!-- http://www.sisostds.org/ontologies/C2SIM#Accept -->

    <owl:NamedIndividual rdf:about="http://www.sisostds.org/ontologies/C2SIM#Accept">
        <rdf:type rdf:resource="http://www.sisostds.org/ontologies/C2SIM#CommunicativeActTypeCode"/>
    </owl:NamedIndividual>
    


    <!-- http://www.sisostds.org/ontologies/C2SIM#Agree -->

    <owl:NamedIndividual rdf:about="http://www.sisostds.org/ontologies/C2SIM#Agree">
        <rdf:type rdf:resource="http://www.sisostds.org/ontologies/C2SIM#CommunicativeActTypeCode"/>
    </owl:NamedIndividual>
    


    <!-- http://www.sisostds.org/ontologies/C2SIM#AssistOtherUnit -->

    <owl:NamedIndividual rdf:about="http://www.sisostds.org/ontologies/C2SIM#AssistOtherUnit">
        <rdf:type rdf:resource="http://www.sisostds.org/ontologies/C2SIM#TaskNameCode"/>
    </owl:NamedIndividual>
    <owl:Axiom>
        <owl:annotatedSource rdf:resource="http://www.sisostds.org/ontologies/C2SIM#AssistOtherUnit"/>
        <owl:annotatedProperty rdf:resource="http://www.w3.org/1999/02/22-rdf-syntax-ns#type"/>
        <owl:annotatedTarget rdf:resource="http://www.sisostds.org/ontologies/C2SIM#TaskNameCode"/>
        <rdfs:comment>Assist the AffectedUnit identified in the Task with the task it is performing.</rdfs:comment>
    </owl:Axiom>
    


    <!-- http://www.sisostds.org/ontologies/C2SIM#BLOCK -->

    <owl:NamedIndividual rdf:about="http://www.sisostds.org/ontologies/C2SIM#BLOCK">
        <rdf:type rdf:resource="http://www.sisostds.org/ontologies/C2SIM#TaskNameCode"/>
        <rdfs:comment>Documentation: 		
						To deny the enemy access to an area or to prevent his advance in a direction or along an avenue of approach.	
					; Appinfo DisplayValue as &quot;Block&quot;</rdfs:comment>
    </owl:NamedIndividual>
    


    <!-- http://www.sisostds.org/ontologies/C2SIM#BREACH -->

    <owl:NamedIndividual rdf:about="http://www.sisostds.org/ontologies/C2SIM#BREACH">
        <rdf:type rdf:resource="http://www.sisostds.org/ontologies/C2SIM#TaskNameCode"/>
        <rdfs:comment>Documentation: 		
						To break through or secure a passage through an enemy defence, obstacle, minefield, or fortification.	
					; Appinfo DisplayValue as &quot;Breach&quot;</rdfs:comment>
    </owl:NamedIndividual>
    


    <!-- http://www.sisostds.org/ontologies/C2SIM#BURN -->

    <owl:NamedIndividual rdf:about="http://www.sisostds.org/ontologies/C2SIM#BURN">
        <rdf:type rdf:resource="http://www.sisostds.org/ontologies/C2SIM#DesiredEffectCode"/>
        <rdfs:comment>Documentation: 		
						The ACTION objective is alight.	
					; Appinfo DisplayValue as &quot;Burning&quot;</rdfs:comment>
    </owl:NamedIndividual>
    


    <!-- http://www.sisostds.org/ontologies/C2SIM#BYPASS -->

    <owl:NamedIndividual rdf:about="http://www.sisostds.org/ontologies/C2SIM#BYPASS">
        <rdf:type rdf:resource="http://www.sisostds.org/ontologies/C2SIM#TaskNameCode"/>
        <rdfs:comment>Documentation: 		
						To manoeuvre around an obstacle, position, or enemy force in order to maintain the momentum of advance.	
					; Appinfo DisplayValue as &quot;Bypass&quot;</rdfs:comment>
    </owl:NamedIndividual>
    


    <!-- http://www.sisostds.org/ontologies/C2SIM#CAPTRD -->

    <owl:NamedIndividual rdf:about="http://www.sisostds.org/ontologies/C2SIM#CAPTRD">
        <rdf:type rdf:resource="http://www.sisostds.org/ontologies/C2SIM#DesiredEffectCode"/>
        <rdfs:comment>Documentation: 		
						The ACTION objective has been captured or acquired and is available for use or interrogation/possession has been taken of an area, normally by force.	
					; Appinfo DisplayValue as &quot;Captured&quot;</rdfs:comment>
    </owl:NamedIndividual>
    


    <!-- http://www.sisostds.org/ontologies/C2SIM#CAPTUR -->

    <owl:NamedIndividual rdf:about="http://www.sisostds.org/ontologies/C2SIM#CAPTUR">
        <rdf:type rdf:resource="http://www.sisostds.org/ontologies/C2SIM#TaskNameCode"/>
        <rdfs:comment>Documentation: 		
						To take possession of an object, normally by force; it frequently involves movement as a preliminary phase.	
					; Appinfo DisplayValue as &quot;Capture&quot;</rdfs:comment>
    </owl:NamedIndividual>
    


    <!-- http://www.sisostds.org/ontologies/C2SIM#CLOSE -->

    <owl:NamedIndividual rdf:about="http://www.sisostds.org/ontologies/C2SIM#CLOSE">
        <rdf:type rdf:resource="http://www.sisostds.org/ontologies/C2SIM#TaskNameCode"/>
        <rdfs:comment>Documentation: 		
						To prevent a FACILITY or FEATURE from performing its intended function.	
					; Appinfo DisplayValue as &quot;Close&quot;</rdfs:comment>
    </owl:NamedIndividual>
    


    <!-- http://www.sisostds.org/ontologies/C2SIM#CLRLND -->

    <owl:NamedIndividual rdf:about="http://www.sisostds.org/ontologies/C2SIM#CLRLND">
        <rdf:type rdf:resource="http://www.sisostds.org/ontologies/C2SIM#TaskNameCode"/>
        <rdfs:comment>Documentation: 		
						To remove all enemy forces from a specific location, area, or zone.	
					; Appinfo DisplayValue as &quot;Clear, land combat&quot;</rdfs:comment>
    </owl:NamedIndividual>
    


    <!-- http://www.sisostds.org/ontologies/C2SIM#CLROBS -->

    <owl:NamedIndividual rdf:about="http://www.sisostds.org/ontologies/C2SIM#CLROBS">
        <rdf:type rdf:resource="http://www.sisostds.org/ontologies/C2SIM#TaskNameCode"/>
        <rdfs:comment>Documentation: 		
						To totally eliminate or neutralize an obstacle; a task that is usually performed by follow-on engineers and is not done under fire.	
					; Appinfo DisplayValue as &quot;Clear, obstacle&quot;</rdfs:comment>
    </owl:NamedIndividual>
    


    <!-- http://www.sisostds.org/ontologies/C2SIM#CNFPSL -->

    <owl:NamedIndividual rdf:about="http://www.sisostds.org/ontologies/C2SIM#CNFPSL">
        <rdf:type rdf:resource="http://www.sisostds.org/ontologies/C2SIM#TaskNameCode"/>
        <rdfs:comment>Documentation: 		
						An operation in which an incoming force attacks through a unit (outgoing force).that is in contact with the enemy.	
					; Appinfo DisplayValue as &quot;Conduct forward passage of lines&quot;</rdfs:comment>
    </owl:NamedIndividual>
    


    <!-- http://www.sisostds.org/ontologies/C2SIM#CNRPSL -->

    <owl:NamedIndividual rdf:about="http://www.sisostds.org/ontologies/C2SIM#CNRPSL">
        <rdf:type rdf:resource="http://www.sisostds.org/ontologies/C2SIM#TaskNameCode"/>
        <rdfs:comment>Documentation: 		
						An operation when a force (outgoing force) effecting a movement to the rear passes through the sector of a unit (incoming force).	
					; Appinfo DisplayValue as &quot;Conduct rearward passage of lines&quot;</rdfs:comment>
    </owl:NamedIndividual>
    


    <!-- http://www.sisostds.org/ontologies/C2SIM#CONS -->

    <owl:NamedIndividual rdf:about="http://www.sisostds.org/ontologies/C2SIM#CONS">
        <rdf:type rdf:resource="http://www.sisostds.org/ontologies/C2SIM#DesiredEffectCode"/>
        <rdfs:comment>Documentation: 		
						The consumption of specified consumables or CONSUMABLE-MATERIEL-TYPEs.	
					; Appinfo DisplayValue as &quot;Consumed&quot;</rdfs:comment>
    </owl:NamedIndividual>
    


    <!-- http://www.sisostds.org/ontologies/C2SIM#COVER -->

    <owl:NamedIndividual rdf:about="http://www.sisostds.org/ontologies/C2SIM#COVER">
        <rdf:type rdf:resource="http://www.sisostds.org/ontologies/C2SIM#TaskNameCode"/>
        <rdfs:comment>Documentation: 		
						To operate as a force apart to protect the main body by fighting to gain time while also observing and reporting information and preventing enemy ground observation of an direct fire against the main body.	
					; Appinfo DisplayValue as &quot;Cover&quot;</rdfs:comment>
    </owl:NamedIndividual>
    


    <!-- http://www.sisostds.org/ontologies/C2SIM#CRESRV -->

    <owl:NamedIndividual rdf:about="http://www.sisostds.org/ontologies/C2SIM#CRESRV">
        <rdf:type rdf:resource="http://www.sisostds.org/ontologies/C2SIM#TaskNameCode"/>
        <rdfs:comment>Documentation: 		
						To constitute a force which may be committed into combat only on the order of the commander of the ORGANISATION who so designated the reserve force.	
					; Appinfo DisplayValue as &quot;Constitute a reserve&quot;</rdfs:comment>
    </owl:NamedIndividual>
    


    <!-- http://www.sisostds.org/ontologies/C2SIM#CTRATK -->

    <owl:NamedIndividual rdf:about="http://www.sisostds.org/ontologies/C2SIM#CTRATK">
        <rdf:type rdf:resource="http://www.sisostds.org/ontologies/C2SIM#TaskNameCode"/>
        <rdfs:comment>Documentation: 		
						To mount an offensive operation in which an attack by a part or all of a defending force is made against an enemy attacking force, for such specific purposes as regaining ground lost, cutting off or destroying lead enemy units, and with the general objective of regaining the initiative and denying the enemy the attainment of his goal or purpose in attacking.	
					; Appinfo DisplayValue as &quot;Counter attack&quot;</rdfs:comment>
    </owl:NamedIndividual>
    


    <!-- http://www.sisostds.org/ontologies/C2SIM#CTRBYF -->

    <owl:NamedIndividual rdf:about="http://www.sisostds.org/ontologies/C2SIM#CTRBYF">
        <rdf:type rdf:resource="http://www.sisostds.org/ontologies/C2SIM#TaskNameCode"/>
        <rdfs:comment>Documentation: 		
						To deliver fire for the purpose of destroying or neutralizing indirect fire weapons systems.	
					; Appinfo DisplayValue as &quot;Counter-battery fire&quot;</rdfs:comment>
    </owl:NamedIndividual>
    


    <!-- http://www.sisostds.org/ontologies/C2SIM#CTRFIR -->

    <owl:NamedIndividual rdf:about="http://www.sisostds.org/ontologies/C2SIM#CTRFIR">
        <rdf:type rdf:resource="http://www.sisostds.org/ontologies/C2SIM#TaskNameCode"/>
        <rdfs:comment>Documentation: 		
						To deny the enemy his goal in attacking through fire into an engagement area to defeat or destroy an enemy force.	
					; Appinfo DisplayValue as &quot;Counter attack by fire&quot;</rdfs:comment>
    </owl:NamedIndividual>
    


    <!-- http://www.sisostds.org/ontologies/C2SIM#Confidential -->

    <owl:NamedIndividual rdf:about="http://www.sisostds.org/ontologies/C2SIM#Confidential">
        <rdf:type rdf:resource="http://www.sisostds.org/ontologies/C2SIM#SecurityClassificationCode"/>
    </owl:NamedIndividual>
    


    <!-- http://www.sisostds.org/ontologies/C2SIM#Confirm -->

    <owl:NamedIndividual rdf:about="http://www.sisostds.org/ontologies/C2SIM#Confirm">
        <rdf:type rdf:resource="http://www.sisostds.org/ontologies/C2SIM#CommunicativeActTypeCode"/>
    </owl:NamedIndividual>
    


    <!-- http://www.sisostds.org/ontologies/C2SIM#DECEIV -->

    <owl:NamedIndividual rdf:about="http://www.sisostds.org/ontologies/C2SIM#DECEIV">
        <rdf:type rdf:resource="http://www.sisostds.org/ontologies/C2SIM#TaskNameCode"/>
        <rdfs:comment>Documentation: 		
						To employ measures designed to mislead the enemy by manipulation, distortion, or falsification of evidence to induce him to react in a manner prejudicial to his interests.	
					; Appinfo DisplayValue as &quot;Deceive&quot;</rdfs:comment>
    </owl:NamedIndividual>
    


    <!-- http://www.sisostds.org/ontologies/C2SIM#DEFEAT -->

    <owl:NamedIndividual rdf:about="http://www.sisostds.org/ontologies/C2SIM#DEFEAT">
        <rdf:type rdf:resource="http://www.sisostds.org/ontologies/C2SIM#TaskNameCode"/>
        <rdfs:comment>Documentation: 		
						To diminish the effectiveness of the enemy to the extent that he is unable to participate further in the battle or at least cannot fulfil his intention.	
					; Appinfo DisplayValue as &quot;Defeat&quot;</rdfs:comment>
    </owl:NamedIndividual>
    


    <!-- http://www.sisostds.org/ontologies/C2SIM#DEFEND -->

    <owl:NamedIndividual rdf:about="http://www.sisostds.org/ontologies/C2SIM#DEFEND">
        <rdf:type rdf:resource="http://www.sisostds.org/ontologies/C2SIM#TaskNameCode"/>
        <rdfs:comment>Documentation: 		
						To hold a defined object against an enemy attack; to halt or ward off an attack in order to defeat or destroy the enemy.	
					; Appinfo DisplayValue as &quot;Defend&quot;</rdfs:comment>
    </owl:NamedIndividual>
    


    <!-- http://www.sisostds.org/ontologies/C2SIM#DELAY -->

    <owl:NamedIndividual rdf:about="http://www.sisostds.org/ontologies/C2SIM#DELAY">
        <rdf:type rdf:resource="http://www.sisostds.org/ontologies/C2SIM#TaskNameCode"/>
        <rdfs:comment>Documentation: 		
						To slow the momentum of the enemy by conducting an operation in which the force under pressure trades time for space. The aim is to inflict the maximum damage on the enemy without becoming decisively engaged.	
					; Appinfo DisplayValue as &quot;Delay&quot;</rdfs:comment>
    </owl:NamedIndividual>
    


    <!-- http://www.sisostds.org/ontologies/C2SIM#DENY -->

    <owl:NamedIndividual rdf:about="http://www.sisostds.org/ontologies/C2SIM#DENY">
        <rdf:type rdf:resource="http://www.sisostds.org/ontologies/C2SIM#TaskNameCode"/>
        <rdfs:comment>Documentation: 		
						To prevent access by blocking, disrupting, dislocating and/or bringing fire to bear.	
					; Appinfo DisplayValue as &quot;Deny&quot;</rdfs:comment>
    </owl:NamedIndividual>
    


    <!-- http://www.sisostds.org/ontologies/C2SIM#DESTRY -->

    <owl:NamedIndividual rdf:about="http://www.sisostds.org/ontologies/C2SIM#DESTRY">
        <rdf:type rdf:resource="http://www.sisostds.org/ontologies/C2SIM#TaskNameCode"/>
        <rdfs:comment>Documentation: 		
						To physically render an enemy force combat-ineffective or damaging a target so that it cannot function as intended, nor be restored to a usable condition without being entirely rebuilt.	
					; Appinfo DisplayValue as &quot;Destroy&quot;</rdfs:comment>
    </owl:NamedIndividual>
    


    <!-- http://www.sisostds.org/ontologies/C2SIM#DISENG -->

    <owl:NamedIndividual rdf:about="http://www.sisostds.org/ontologies/C2SIM#DISENG">
        <rdf:type rdf:resource="http://www.sisostds.org/ontologies/C2SIM#TaskNameCode"/>
        <rdfs:comment>Documentation: 		
						To break off an action.	
					; Appinfo DisplayValue as &quot;Disengage&quot;</rdfs:comment>
    </owl:NamedIndividual>
    


    <!-- http://www.sisostds.org/ontologies/C2SIM#DISRPT -->

    <owl:NamedIndividual rdf:about="http://www.sisostds.org/ontologies/C2SIM#DISRPT">
        <rdf:type rdf:resource="http://www.sisostds.org/ontologies/C2SIM#TaskNameCode"/>
        <rdfs:comment>Documentation: 		
						To break apart an enemy&apos;s formation and tempo, to interrupt the enemy&apos;s timetable, to cause premature commitment of forces, and/or splinter their attack using integrated fire planning and obstacle effect.	
					; Appinfo DisplayValue as &quot;Disrupt&quot;</rdfs:comment>
    </owl:NamedIndividual>
    


    <!-- http://www.sisostds.org/ontologies/C2SIM#DLBATK -->

    <owl:NamedIndividual rdf:about="http://www.sisostds.org/ontologies/C2SIM#DLBATK">
        <rdf:type rdf:resource="http://www.sisostds.org/ontologies/C2SIM#TaskNameCode"/>
        <rdfs:comment>Documentation: 		
						To conduct a type of offensive action characterised by pre-planned coordinated employment of firepower and manoeuvre to close with and destroy or capture the enemy.	
					; Appinfo DisplayValue as &quot;Attack, deliberate&quot;</rdfs:comment>
    </owl:NamedIndividual>
    


    <!-- http://www.sisostds.org/ontologies/C2SIM#DRONL -->

    <owl:NamedIndividual rdf:about="http://www.sisostds.org/ontologies/C2SIM#DRONL">
        <rdf:type rdf:resource="http://www.sisostds.org/ontologies/C2SIM#TaskNameCode"/>
        <rdfs:comment>Documentation: 		
						To perform the launching of drones.	
					; Appinfo DisplayValue as &quot;Drone launch&quot;</rdfs:comment>
    </owl:NamedIndividual>
    


    <!-- http://www.sisostds.org/ontologies/C2SIM#DSTRYK -->

    <owl:NamedIndividual rdf:about="http://www.sisostds.org/ontologies/C2SIM#DSTRYK">
        <rdf:type rdf:resource="http://www.sisostds.org/ontologies/C2SIM#DesiredEffectCode"/>
        <rdfs:comment>Documentation: 		
						Cannot function as intended nor be repaired or restored to an operational status.	
					; Appinfo DisplayValue as &quot;Destroyed (K-kill)&quot;</rdfs:comment>
    </owl:NamedIndividual>
    


    <!-- http://www.sisostds.org/ontologies/C2SIM#ENGAGE -->

    <owl:NamedIndividual rdf:about="http://www.sisostds.org/ontologies/C2SIM#ENGAGE">
        <rdf:type rdf:resource="http://www.sisostds.org/ontologies/C2SIM#TaskNameCode"/>
        <rdfs:comment>Documentation: 		
						To bring the enemy under fire.	
					; Appinfo DisplayValue as &quot;Engage&quot;</rdfs:comment>
    </owl:NamedIndividual>
    


    <!-- http://www.sisostds.org/ontologies/C2SIM#ENVLP -->

    <owl:NamedIndividual rdf:about="http://www.sisostds.org/ontologies/C2SIM#ENVLP">
        <rdf:type rdf:resource="http://www.sisostds.org/ontologies/C2SIM#TaskNameCode"/>
        <rdfs:comment>Documentation: 		
						To conduct an offensive manoeuvre in which the main attacking force passes around or over the enemy&apos;s principal defensive positions with the aim of securing objectives to the enemy&apos;s rear.	
					; Appinfo DisplayValue as &quot;Envelop&quot;</rdfs:comment>
    </owl:NamedIndividual>
    


    <!-- http://www.sisostds.org/ontologies/C2SIM#EXPLT -->

    <owl:NamedIndividual rdf:about="http://www.sisostds.org/ontologies/C2SIM#EXPLT">
        <rdf:type rdf:resource="http://www.sisostds.org/ontologies/C2SIM#TaskNameCode"/>
        <rdfs:comment>Documentation: 		
						To take advantage of a successful attack by mounting an offensive operation to follow-up and harass a dislocated enemy with the aim of further disorganising him in depth. This may provide the opportunity to capture ground which was not part of the objective of the original attack.	
					; Appinfo DisplayValue as &quot;Exploit&quot;</rdfs:comment>
    </owl:NamedIndividual>
    


    <!-- http://www.sisostds.org/ontologies/C2SIM#EnemySide -->

    <owl:NamedIndividual rdf:about="http://www.sisostds.org/ontologies/C2SIM#EnemySide"/>
    


    <!-- http://www.sisostds.org/ontologies/C2SIM#FIX -->

    <owl:NamedIndividual rdf:about="http://www.sisostds.org/ontologies/C2SIM#FIX">
        <rdf:type rdf:resource="http://www.sisostds.org/ontologies/C2SIM#TaskNameCode"/>
        <rdfs:comment>Documentation: 		
						To prevent the enemy from moving any part of his force from a specific location for a specific period of time.	
					; Appinfo DisplayValue as &quot;Fix&quot;</rdfs:comment>
    </owl:NamedIndividual>
    


    <!-- http://www.sisostds.org/ontologies/C2SIM#FKIL -->

    <owl:NamedIndividual rdf:about="http://www.sisostds.org/ontologies/C2SIM#FKIL">
        <rdf:type rdf:resource="http://www.sisostds.org/ontologies/C2SIM#DesiredEffectCode"/>
        <rdfs:comment>Documentation: 		
						The destruction of a vehicle (or system&apos;s) primary weapon system.	
					; Appinfo DisplayValue as &quot;Firepower kill (F-kill)&quot;</rdfs:comment>
    </owl:NamedIndividual>
    


    <!-- http://www.sisostds.org/ontologies/C2SIM#FLIG -->

    <owl:NamedIndividual rdf:about="http://www.sisostds.org/ontologies/C2SIM#FLIG">
        <rdf:type rdf:resource="http://www.sisostds.org/ontologies/C2SIM#DesiredEffectCode"/>
        <rdfs:comment>Documentation: 		
						The setting to flight of a PERSON or PERSON-TYPEs from their present location.	
					; Appinfo DisplayValue as &quot;Forced to flee&quot;</rdfs:comment>
    </owl:NamedIndividual>
    


    <!-- http://www.sisostds.org/ontologies/C2SIM#FriendlySide -->

    <owl:NamedIndividual rdf:about="http://www.sisostds.org/ontologies/C2SIM#FriendlySide"/>
    


    <!-- http://www.sisostds.org/ontologies/C2SIM#FullyOperational -->

    <owl:NamedIndividual rdf:about="http://www.sisostds.org/ontologies/C2SIM#FullyOperational">
        <rdf:type rdf:resource="http://www.sisostds.org/ontologies/C2SIM#OperationalStatusCode"/>
    </owl:NamedIndividual>
    


    <!-- http://www.sisostds.org/ontologies/C2SIM#GUARD -->

    <owl:NamedIndividual rdf:about="http://www.sisostds.org/ontologies/C2SIM#GUARD">
        <rdf:type rdf:resource="http://www.sisostds.org/ontologies/C2SIM#TaskNameCode"/>
        <rdfs:comment>Documentation: 		
						To protect the main body by fighting to gain time while also observing and reporting information.	
					; Appinfo DisplayValue as &quot;Guard&quot;</rdfs:comment>
    </owl:NamedIndividual>
    


    <!-- http://www.sisostds.org/ontologies/C2SIM#GenericAction -->

    <owl:NamedIndividual rdf:about="http://www.sisostds.org/ontologies/C2SIM#GenericAction">
        <rdf:type rdf:resource="http://www.sisostds.org/ontologies/C2SIM#EventCode"/>
    </owl:NamedIndividual>
    


    <!-- http://www.sisostds.org/ontologies/C2SIM#GenericCountry -->

    <owl:NamedIndividual rdf:about="http://www.sisostds.org/ontologies/C2SIM#GenericCountry">
        <rdf:type rdf:resource="http://www.sisostds.org/ontologies/C2SIM#CountryCode"/>
    </owl:NamedIndividual>
    


    <!-- http://www.sisostds.org/ontologies/C2SIM#GenericEffect -->

    <owl:NamedIndividual rdf:about="http://www.sisostds.org/ontologies/C2SIM#GenericEffect">
        <rdf:type rdf:resource="http://www.sisostds.org/ontologies/C2SIM#DesiredEffectCode"/>
    </owl:NamedIndividual>
    


    <!-- http://www.sisostds.org/ontologies/C2SIM#GenericEthnicGroup -->

    <owl:NamedIndividual rdf:about="http://www.sisostds.org/ontologies/C2SIM#GenericEthnicGroup">
        <rdf:type rdf:resource="http://www.sisostds.org/ontologies/C2SIM#EthnicGroupCode"/>
    </owl:NamedIndividual>
    


    <!-- http://www.sisostds.org/ontologies/C2SIM#GenericReligiousOrganization -->

    <owl:NamedIndividual rdf:about="http://www.sisostds.org/ontologies/C2SIM#GenericReligiousOrganization">
        <rdf:type rdf:resource="http://www.sisostds.org/ontologies/C2SIM#ReligiousOrganizationCode"/>
    </owl:NamedIndividual>
    


    <!-- http://www.sisostds.org/ontologies/C2SIM#HARASS -->

    <owl:NamedIndividual rdf:about="http://www.sisostds.org/ontologies/C2SIM#HARASS">
        <rdf:type rdf:resource="http://www.sisostds.org/ontologies/C2SIM#TaskNameCode"/>
        <rdfs:comment>Documentation: 		
						To mount an operation or fire plan designed to curtail movement and, by threat of losses, to lower the morale of enemy troops.	
					; Appinfo DisplayValue as &quot;Harass&quot;</rdfs:comment>
    </owl:NamedIndividual>
    


    <!-- http://www.sisostds.org/ontologies/C2SIM#HASTY -->

    <owl:NamedIndividual rdf:about="http://www.sisostds.org/ontologies/C2SIM#HASTY">
        <rdf:type rdf:resource="http://www.sisostds.org/ontologies/C2SIM#TaskNameCode"/>
        <rdfs:comment>Documentation: 		
						To conduct a type of offensive action using firepower and manoeuvre to close with and destroy or capture the enemy. Planning and coordination will normally be limited, as the attack will be carried out at short notice.	
					; Appinfo DisplayValue as &quot;Attack, hasty&quot;</rdfs:comment>
    </owl:NamedIndividual>
    


    <!-- http://www.sisostds.org/ontologies/C2SIM#HONASP -->

    <owl:NamedIndividual rdf:about="http://www.sisostds.org/ontologies/C2SIM#HONASP">
        <rdf:type rdf:resource="http://www.sisostds.org/ontologies/C2SIM#TaskNameCode"/>
        <rdfs:comment>Documentation: 		
						Civil and military assistance rendered in peace, crisis and war by a host nation to Allied forces and NATO organisations which are located on or in transit through the host nation&apos;s territory. The basis of such assistance is commitments arising from the NATO Alliance or from bilateral or multilateral agreements concluded between the host nation, NATO organisations and (the) nation(s) having forces operating on the host nation&apos;s territory.	
					; Appinfo DisplayValue as &quot;Host nation support&quot;</rdfs:comment>
    </owl:NamedIndividual>
    


    <!-- http://www.sisostds.org/ontologies/C2SIM#HoldInPlace -->

    <owl:NamedIndividual rdf:about="http://www.sisostds.org/ontologies/C2SIM#HoldInPlace">
        <rdf:type rdf:resource="http://www.sisostds.org/ontologies/C2SIM#TaskNameCode"/>
    </owl:NamedIndividual>
    <owl:Axiom>
        <owl:annotatedSource rdf:resource="http://www.sisostds.org/ontologies/C2SIM#HoldInPlace"/>
        <owl:annotatedProperty rdf:resource="http://www.w3.org/1999/02/22-rdf-syntax-ns#type"/>
        <owl:annotatedTarget rdf:resource="http://www.sisostds.org/ontologies/C2SIM#TaskNameCode"/>
        <rdfs:comment>Do not move.</rdfs:comment>
    </owl:Axiom>
    


    <!-- http://www.sisostds.org/ontologies/C2SIM#IDNT -->

    <owl:NamedIndividual rdf:about="http://www.sisostds.org/ontologies/C2SIM#IDNT">
        <rdf:type rdf:resource="http://www.sisostds.org/ontologies/C2SIM#DesiredEffectCode"/>
        <rdfs:comment>Documentation: 		
						The ACTION objective has been either identified (i.e., classified as friend/foe/neutral) or recognised (i.e., the unit designation of the ORGANISATION or object is known).	
					; Appinfo DisplayValue as &quot;Identified&quot;</rdfs:comment>
    </owl:NamedIndividual>
    


    <!-- http://www.sisostds.org/ontologies/C2SIM#ILLUMN -->

    <owl:NamedIndividual rdf:about="http://www.sisostds.org/ontologies/C2SIM#ILLUMN">
        <rdf:type rdf:resource="http://www.sisostds.org/ontologies/C2SIM#DesiredEffectCode"/>
        <rdfs:comment>Documentation: 		
						The temporary supply of IR or white-light illumination (usually in coordination with direct or indirect fire).	
					; Appinfo DisplayValue as &quot;Illuminated&quot;</rdfs:comment>
    </owl:NamedIndividual>
    


    <!-- http://www.sisostds.org/ontologies/C2SIM#INFILT -->

    <owl:NamedIndividual rdf:about="http://www.sisostds.org/ontologies/C2SIM#INFILT">
        <rdf:type rdf:resource="http://www.sisostds.org/ontologies/C2SIM#TaskNameCode"/>
        <rdfs:comment>Documentation: 		
						To move a force, broken down as individuals or small groups, over, through or around enemy positions with the aim of avoiding detection.	
					; Appinfo DisplayValue as &quot;Infiltrate&quot;</rdfs:comment>
    </owl:NamedIndividual>
    


    <!-- http://www.sisostds.org/ontologies/C2SIM#INITIALIZED -->

    <owl:NamedIndividual rdf:about="http://www.sisostds.org/ontologies/C2SIM#INITIALIZED">
        <rdf:type rdf:resource="http://www.sisostds.org/ontologies/C2SIM#SystemStateCode"/>
    </owl:NamedIndividual>
    


    <!-- http://www.sisostds.org/ontologies/C2SIM#INTDCT -->

    <owl:NamedIndividual rdf:about="http://www.sisostds.org/ontologies/C2SIM#INTDCT">
        <rdf:type rdf:resource="http://www.sisostds.org/ontologies/C2SIM#TaskNameCode"/>
        <rdfs:comment>Documentation: 		
						To divert, disrupt, delay, or destroy the enemy&apos;s surface military potential before it can be used effectively against friendly forces.	
					; Appinfo DisplayValue as &quot;Interdict&quot;</rdfs:comment>
    </owl:NamedIndividual>
    


    <!-- http://www.sisostds.org/ontologies/C2SIM#INTREC -->

    <owl:NamedIndividual rdf:about="http://www.sisostds.org/ontologies/C2SIM#INTREC">
        <rdf:type rdf:resource="http://www.sisostds.org/ontologies/C2SIM#DesiredEffectCode"/>
        <rdfs:comment>Documentation: 		
						An equipment lost in an area unsuitable for recovery due to political, military or geographic/environmental considerations.	
					; Appinfo DisplayValue as &quot;Intact but unrecoverable&quot;</rdfs:comment>
    </owl:NamedIndividual>
    


    <!-- http://www.sisostds.org/ontologies/C2SIM#ISOLAT -->

    <owl:NamedIndividual rdf:about="http://www.sisostds.org/ontologies/C2SIM#ISOLAT">
        <rdf:type rdf:resource="http://www.sisostds.org/ontologies/C2SIM#TaskNameCode"/>
        <rdfs:comment>Documentation: 		
						To seal off (both physically and psychologically) an enemy from its sources of support, to deny an enemy freedom of movement, and prevent an enemy unit from having contact with other enemy forces. An enemy must not be allowed sanctuary within its present position.	
					; Appinfo DisplayValue as &quot;Isolate&quot;</rdfs:comment>
    </owl:NamedIndividual>
    


    <!-- http://www.sisostds.org/ontologies/C2SIM#Inform -->

    <owl:NamedIndividual rdf:about="http://www.sisostds.org/ontologies/C2SIM#Inform">
        <rdf:type rdf:resource="http://www.sisostds.org/ontologies/C2SIM#CommunicativeActTypeCode"/>
    </owl:NamedIndividual>
    


    <!-- http://www.sisostds.org/ontologies/C2SIM#InitializationComplete -->

    <owl:NamedIndividual rdf:about="http://www.sisostds.org/ontologies/C2SIM#InitializationComplete">
        <rdf:type rdf:resource="http://www.sisostds.org/ontologies/C2SIM#SystemCommandTypeCode"/>
        <rdfs:comment>This command is emitted by a system after it has received a C2SIMInitialization message, has completed its initialization procedures, and is ready for scenario start.</rdfs:comment>
    </owl:NamedIndividual>
    


    <!-- http://www.sisostds.org/ontologies/C2SIM#IntervalEndTime -->

    <owl:NamedIndividual rdf:about="http://www.sisostds.org/ontologies/C2SIM#IntervalEndTime">
        <rdf:type rdf:resource="http://www.sisostds.org/ontologies/C2SIM#TimeReferenceCode"/>
    </owl:NamedIndividual>
    


    <!-- http://www.sisostds.org/ontologies/C2SIM#IntervalStartTime -->

    <owl:NamedIndividual rdf:about="http://www.sisostds.org/ontologies/C2SIM#IntervalStartTime">
        <rdf:type rdf:resource="http://www.sisostds.org/ontologies/C2SIM#TimeReferenceCode"/>
    </owl:NamedIndividual>
    


    <!-- http://www.sisostds.org/ontologies/C2SIM#KILL -->

    <owl:NamedIndividual rdf:about="http://www.sisostds.org/ontologies/C2SIM#KILL">
        <rdf:type rdf:resource="http://www.sisostds.org/ontologies/C2SIM#DesiredEffectCode"/>
        <rdfs:comment>Documentation: 		
						A casualty who is killed outright or dies as a result of wounds, disease or other injuries.	
					; Appinfo DisplayValue as &quot;Killed&quot;</rdfs:comment>
    </owl:NamedIndividual>
    


    <!-- http://www.sisostds.org/ontologies/C2SIM#LDAM -->

    <owl:NamedIndividual rdf:about="http://www.sisostds.org/ontologies/C2SIM#LDAM">
        <rdf:type rdf:resource="http://www.sisostds.org/ontologies/C2SIM#DesiredEffectCode"/>
        <rdfs:comment>Documentation: 		
						The subjective categorisation of the physical effect of an ACTION on buildings, infrastructure and/or equipment by a reporting ORGANISATION.	
					; Appinfo DisplayValue as &quot;Light damage&quot;</rdfs:comment>
    </owl:NamedIndividual>
    


    <!-- http://www.sisostds.org/ontologies/C2SIM#LGTRST -->

    <owl:NamedIndividual rdf:about="http://www.sisostds.org/ontologies/C2SIM#LGTRST">
        <rdf:type rdf:resource="http://www.sisostds.org/ontologies/C2SIM#DesiredEffectCode"/>
        <rdfs:comment>Documentation: 		
						The ACTION-OBJECTIVE reacted against the ACTION using light physical violence.	
					; Appinfo DisplayValue as &quot;Light resistance&quot;</rdfs:comment>
    </owl:NamedIndividual>
    


    <!-- http://www.sisostds.org/ontologies/C2SIM#LOCATE -->

    <owl:NamedIndividual rdf:about="http://www.sisostds.org/ontologies/C2SIM#LOCATE">
        <rdf:type rdf:resource="http://www.sisostds.org/ontologies/C2SIM#TaskNameCode"/>
        <rdfs:comment>Documentation: 		
						To establish the position or presence of an object.	
					; Appinfo DisplayValue as &quot;Locate&quot;</rdfs:comment>
    </owl:NamedIndividual>
    


    <!-- http://www.sisostds.org/ontologies/C2SIM#LOST -->

    <owl:NamedIndividual rdf:about="http://www.sisostds.org/ontologies/C2SIM#LOST">
        <rdf:type rdf:resource="http://www.sisostds.org/ontologies/C2SIM#DesiredEffectCode"/>
        <rdfs:comment>Documentation: 		
						The object is no longer available for military operations.	
					; Appinfo DisplayValue as &quot;Lost&quot;</rdfs:comment>
    </owl:NamedIndividual>
    


    <!-- http://www.sisostds.org/ontologies/C2SIM#MEDEVC -->

    <owl:NamedIndividual rdf:about="http://www.sisostds.org/ontologies/C2SIM#MEDEVC">
        <rdf:type rdf:resource="http://www.sisostds.org/ontologies/C2SIM#TaskNameCode"/>
        <rdfs:comment>Documentation: 		
						To move any person who is wounded, injured or ill to/between medical treatment facilities.	
					; Appinfo DisplayValue as &quot;Medical evacuation&quot;</rdfs:comment>
    </owl:NamedIndividual>
    


    <!-- http://www.sisostds.org/ontologies/C2SIM#MKIL -->

    <owl:NamedIndividual rdf:about="http://www.sisostds.org/ontologies/C2SIM#MKIL">
        <rdf:type rdf:resource="http://www.sisostds.org/ontologies/C2SIM#DesiredEffectCode"/>
        <rdfs:comment>Documentation: 		
						The rendering of a vehicle as being temporarily or permanently incapable of tactical movement.	
					; Appinfo DisplayValue as &quot;Mobility kill (M-kill)&quot;</rdfs:comment>
    </owl:NamedIndividual>
    


    <!-- http://www.sisostds.org/ontologies/C2SIM#MODDAM -->

    <owl:NamedIndividual rdf:about="http://www.sisostds.org/ontologies/C2SIM#MODDAM">
        <rdf:type rdf:resource="http://www.sisostds.org/ontologies/C2SIM#DesiredEffectCode"/>
        <rdfs:comment>Documentation: 		
						The subjective categorisation of the physical effect of an ACTION on buildings, infrastructure and/or equipment by a reporting ORGANISATION.	
					; Appinfo DisplayValue as &quot;Moderate damage&quot;</rdfs:comment>
    </owl:NamedIndividual>
    


    <!-- http://www.sisostds.org/ontologies/C2SIM#MOPUP -->

    <owl:NamedIndividual rdf:about="http://www.sisostds.org/ontologies/C2SIM#MOPUP">
        <rdf:type rdf:resource="http://www.sisostds.org/ontologies/C2SIM#TaskNameCode"/>
        <rdfs:comment>Documentation: 		
						To liquidate the remnants of enemy resistance in an area that has been surrounded or isolated, or through which other units have passed without eliminating all active resistance.	
					; Appinfo DisplayValue as &quot;Mop up&quot;</rdfs:comment>
    </owl:NamedIndividual>
    


    <!-- http://www.sisostds.org/ontologies/C2SIM#MOVE -->

    <owl:NamedIndividual rdf:about="http://www.sisostds.org/ontologies/C2SIM#MOVE">
        <rdf:type rdf:resource="http://www.sisostds.org/ontologies/C2SIM#TaskNameCode"/>
        <rdfs:comment>Documentation: 		
						To change position from one location to another.	
					; Appinfo DisplayValue as &quot;Move&quot;</rdfs:comment>
    </owl:NamedIndividual>
    


    <!-- http://www.sisostds.org/ontologies/C2SIM#MostlyOperational -->

    <owl:NamedIndividual rdf:about="http://www.sisostds.org/ontologies/C2SIM#MostlyOperational">
        <rdf:type rdf:resource="http://www.sisostds.org/ontologies/C2SIM#OperationalStatusCode"/>
    </owl:NamedIndividual>
    


    <!-- http://www.sisostds.org/ontologies/C2SIM#MoveToLocation -->

    <owl:NamedIndividual rdf:about="http://www.sisostds.org/ontologies/C2SIM#MoveToLocation">
        <rdf:type rdf:resource="http://www.sisostds.org/ontologies/C2SIM#TaskNameCode"/>
    </owl:NamedIndividual>
    <owl:Axiom>
        <owl:annotatedSource rdf:resource="http://www.sisostds.org/ontologies/C2SIM#MoveToLocation"/>
        <owl:annotatedProperty rdf:resource="http://www.w3.org/1999/02/22-rdf-syntax-ns#type"/>
        <owl:annotatedTarget rdf:resource="http://www.sisostds.org/ontologies/C2SIM#TaskNameCode"/>
        <rdfs:comment>The destination of this Movement task is defined as follows: 
-Location property of the Task.  This is a choice of coordinate values, or an entity-defined reference (or entity-relative location); entity-defined can refer to a unit or a map graphic. This is an alternate way to specify location via a map graphic; see below.
- MagGraphicID of the Task. The destination is the Location of the map graphic.</rdfs:comment>
    </owl:Axiom>
    


    <!-- http://www.sisostds.org/ontologies/C2SIM#NBCAS -->

    <owl:NamedIndividual rdf:about="http://www.sisostds.org/ontologies/C2SIM#NBCAS">
        <rdf:type rdf:resource="http://www.sisostds.org/ontologies/C2SIM#DesiredEffectCode"/>
        <rdfs:comment>Documentation: 		
						A person who is not a battle casualty, but who is lost to his organisation by reason of disease or injury, including persons dying from disease or injury, or by reason of being missing where the absence does not appear to be voluntary or due to enemy action or to being interned.	
					; Appinfo DisplayValue as &quot;Non-battle casualty&quot;</rdfs:comment>
    </owl:NamedIndividual>
    


    <!-- http://www.sisostds.org/ontologies/C2SIM#NKN -->

    <owl:NamedIndividual rdf:about="http://www.sisostds.org/ontologies/C2SIM#NKN">
        <rdf:type rdf:resource="http://www.sisostds.org/ontologies/C2SIM#DesiredEffectCode"/>
        <rdfs:comment>Documentation: 		
						It is not possible to determine which value is most applicable.	
					; Appinfo DisplayValue as &quot;Not known&quot;</rdfs:comment>
    </owl:NamedIndividual>
    


    <!-- http://www.sisostds.org/ontologies/C2SIM#NORSTN -->

    <owl:NamedIndividual rdf:about="http://www.sisostds.org/ontologies/C2SIM#NORSTN">
        <rdf:type rdf:resource="http://www.sisostds.org/ontologies/C2SIM#DesiredEffectCode"/>
        <rdfs:comment>Documentation: 		
						The ACTION-OBJECTIVE did not react against the ACTION.	
					; Appinfo DisplayValue as &quot;No resistance&quot;</rdfs:comment>
    </owl:NamedIndividual>
    


    <!-- http://www.sisostds.org/ontologies/C2SIM#NOS -->

    <owl:NamedIndividual rdf:about="http://www.sisostds.org/ontologies/C2SIM#NOS">
        <rdf:type rdf:resource="http://www.sisostds.org/ontologies/C2SIM#DesiredEffectCode"/>
        <rdfs:comment>Documentation: 		
						The appropriate value is not in the set of specified values.	
					; Appinfo DisplayValue as &quot;Not otherwise specified&quot;</rdfs:comment>
    </owl:NamedIndividual>
    


    <!-- http://www.sisostds.org/ontologies/C2SIM#NUTRLD -->

    <owl:NamedIndividual rdf:about="http://www.sisostds.org/ontologies/C2SIM#NUTRLD">
        <rdf:type rdf:resource="http://www.sisostds.org/ontologies/C2SIM#DesiredEffectCode"/>
        <rdfs:comment>Documentation: 		
						The rendering of the ACTION objective temporarily ineffective by the infliction of significant casualties (norm for indirect fire is 10 percent).	
					; Appinfo DisplayValue as &quot;Neutralized&quot;</rdfs:comment>
    </owl:NamedIndividual>
    


    <!-- http://www.sisostds.org/ontologies/C2SIM#NeutralSide -->

    <owl:NamedIndividual rdf:about="http://www.sisostds.org/ontologies/C2SIM#NeutralSide"/>
    


    <!-- http://www.sisostds.org/ontologies/C2SIM#NotOperational -->

    <owl:NamedIndividual rdf:about="http://www.sisostds.org/ontologies/C2SIM#NotOperational">
        <rdf:type rdf:resource="http://www.sisostds.org/ontologies/C2SIM#OperationalStatusCode"/>
    </owl:NamedIndividual>
    


    <!-- http://www.sisostds.org/ontologies/C2SIM#OBSCUR -->

    <owl:NamedIndividual rdf:about="http://www.sisostds.org/ontologies/C2SIM#OBSCUR">
        <rdf:type rdf:resource="http://www.sisostds.org/ontologies/C2SIM#TaskNameCode"/>
        <rdfs:comment>Documentation: 		
						To cover something by a smoke screen.	
					; Appinfo DisplayValue as &quot;Obscure&quot;</rdfs:comment>
    </owl:NamedIndividual>
    


    <!-- http://www.sisostds.org/ontologies/C2SIM#OBSRV -->

    <owl:NamedIndividual rdf:about="http://www.sisostds.org/ontologies/C2SIM#OBSRV">
        <rdf:type rdf:resource="http://www.sisostds.org/ontologies/C2SIM#TaskNameCode"/>
        <rdfs:comment>Documentation: 		
						To provide continuous view, and the potential for reports on the activity of an ACTION-OBJECTIVE.	
					; Appinfo DisplayValue as &quot;Observe&quot;</rdfs:comment>
    </owl:NamedIndividual>
    


    <!-- http://www.sisostds.org/ontologies/C2SIM#OCCUPY -->

    <owl:NamedIndividual rdf:about="http://www.sisostds.org/ontologies/C2SIM#OCCUPY">
        <rdf:type rdf:resource="http://www.sisostds.org/ontologies/C2SIM#TaskNameCode"/>
        <rdfs:comment>Documentation: 		
						To move onto an objective, key terrain, or other manmade or natural terrain area without opposition and control that entire area.	
					; Appinfo DisplayValue as &quot;Occupy&quot;</rdfs:comment>
    </owl:NamedIndividual>
    


    <!-- http://www.sisostds.org/ontologies/C2SIM#Observe -->

    <owl:NamedIndividual rdf:about="http://www.sisostds.org/ontologies/C2SIM#Observe">
        <rdf:type rdf:resource="http://www.sisostds.org/ontologies/C2SIM#TaskNameCode"/>
    </owl:NamedIndividual>
    <owl:Axiom>
        <owl:annotatedSource rdf:resource="http://www.sisostds.org/ontologies/C2SIM#Observe"/>
        <owl:annotatedProperty rdf:resource="http://www.w3.org/1999/02/22-rdf-syntax-ns#type"/>
        <owl:annotatedTarget rdf:resource="http://www.sisostds.org/ontologies/C2SIM#TaskNameCode"/>
        <rdfs:comment>Either generally observe, or observe the Location or AffectedEntity specified in the Task.</rdfs:comment>
    </owl:Axiom>
    


    <!-- http://www.sisostds.org/ontologies/C2SIM#OrientToLocation -->

    <owl:NamedIndividual rdf:about="http://www.sisostds.org/ontologies/C2SIM#OrientToLocation">
        <rdf:type rdf:resource="http://www.sisostds.org/ontologies/C2SIM#TaskNameCode"/>
    </owl:NamedIndividual>
    <owl:Axiom>
        <owl:annotatedSource rdf:resource="http://www.sisostds.org/ontologies/C2SIM#OrientToLocation"/>
        <owl:annotatedProperty rdf:resource="http://www.w3.org/1999/02/22-rdf-syntax-ns#type"/>
        <owl:annotatedTarget rdf:resource="http://www.sisostds.org/ontologies/C2SIM#TaskNameCode"/>
        <rdfs:comment>Orients (the heading of) an entity toward the Location or MapGraphic specified in the task.</rdfs:comment>
    </owl:Axiom>
    


    <!-- http://www.sisostds.org/ontologies/C2SIM#PATROL -->

    <owl:NamedIndividual rdf:about="http://www.sisostds.org/ontologies/C2SIM#PATROL">
        <rdf:type rdf:resource="http://www.sisostds.org/ontologies/C2SIM#TaskNameCode"/>
        <rdfs:comment>Documentation: 		
						To gather information or to carry out a destructive, harassing, mopping-up, or security mission.	
					; Appinfo DisplayValue as &quot;Patrol&quot;</rdfs:comment>
    </owl:NamedIndividual>
    


    <!-- http://www.sisostds.org/ontologies/C2SIM#PAUSED -->

    <owl:NamedIndividual rdf:about="http://www.sisostds.org/ontologies/C2SIM#PAUSED">
        <rdf:type rdf:resource="http://www.sisostds.org/ontologies/C2SIM#SystemStateCode"/>
    </owl:NamedIndividual>
    


    <!-- http://www.sisostds.org/ontologies/C2SIM#PENTRT -->

    <owl:NamedIndividual rdf:about="http://www.sisostds.org/ontologies/C2SIM#PENTRT">
        <rdf:type rdf:resource="http://www.sisostds.org/ontologies/C2SIM#TaskNameCode"/>
        <rdfs:comment>Documentation: 		
						To break through the enemy&apos;s defence or to disrupt the enemy&apos;s defensive systems.	
					; Appinfo DisplayValue as &quot;Penetrate&quot;</rdfs:comment>
    </owl:NamedIndividual>
    


    <!-- http://www.sisostds.org/ontologies/C2SIM#PLAN -->

    <owl:NamedIndividual rdf:about="http://www.sisostds.org/ontologies/C2SIM#PLAN">
        <rdf:type rdf:resource="http://www.sisostds.org/ontologies/C2SIM#TaskNameCode"/>
        <rdfs:comment>Documentation: 		
						To create a detailed formulation of a programme of action.	
					; Appinfo DisplayValue as &quot;Plan&quot;</rdfs:comment>
    </owl:NamedIndividual>
    


    <!-- http://www.sisostds.org/ontologies/C2SIM#PREFIR -->

    <owl:NamedIndividual rdf:about="http://www.sisostds.org/ontologies/C2SIM#PREFIR">
        <rdf:type rdf:resource="http://www.sisostds.org/ontologies/C2SIM#TaskNameCode"/>
        <rdfs:comment>Documentation: 		
						To deliver fire on a target preparatory to an assault.	
					; Appinfo DisplayValue as &quot;Preparatory fire&quot;</rdfs:comment>
    </owl:NamedIndividual>
    


    <!-- http://www.sisostds.org/ontologies/C2SIM#PURSUE -->

    <owl:NamedIndividual rdf:about="http://www.sisostds.org/ontologies/C2SIM#PURSUE">
        <rdf:type rdf:resource="http://www.sisostds.org/ontologies/C2SIM#TaskNameCode"/>
        <rdfs:comment>Documentation: 		
						To continue offensive operations designed to catch or cut off a hostile force attempting to escape, with the aim of destroying it. Typically, contact is maintained and risk taken to harass relentlessly, thereby turning the pursuit into a rout.	
					; Appinfo DisplayValue as &quot;Pursue&quot;</rdfs:comment>
    </owl:NamedIndividual>
    


    <!-- http://www.sisostds.org/ontologies/C2SIM#PartlyOperational -->

    <owl:NamedIndividual rdf:about="http://www.sisostds.org/ontologies/C2SIM#PartlyOperational">
        <rdf:type rdf:resource="http://www.sisostds.org/ontologies/C2SIM#OperationalStatusCode"/>
    </owl:NamedIndividual>
    


    <!-- http://www.sisostds.org/ontologies/C2SIM#RECCE -->

    <owl:NamedIndividual rdf:about="http://www.sisostds.org/ontologies/C2SIM#RECCE">
        <rdf:type rdf:resource="http://www.sisostds.org/ontologies/C2SIM#TaskNameCode"/>
        <rdfs:comment>Documentation: 		
						To conduct a mission to obtain by visual operations or other detection methods information about the activities and resources of an enemy or potential enemy, or to secure data concerning the meteorological, hydrographic or geographic characteristics of a particular area.	
					; Appinfo DisplayValue as &quot;Reconnaissance&quot;</rdfs:comment>
    </owl:NamedIndividual>
    


    <!-- http://www.sisostds.org/ontologies/C2SIM#RECONS -->

    <owl:NamedIndividual rdf:about="http://www.sisostds.org/ontologies/C2SIM#RECONS">
        <rdf:type rdf:resource="http://www.sisostds.org/ontologies/C2SIM#TaskNameCode"/>
        <rdfs:comment>Documentation: 		
						To attain prescribed strength of units and prescribed levels of vehicles, equipment, stores and supplies. The process will only take place after a unit/formation combat effectiveness has been reduced.	
					; Appinfo DisplayValue as &quot;Reconstitute&quot;</rdfs:comment>
    </owl:NamedIndividual>
    


    <!-- http://www.sisostds.org/ontologies/C2SIM#RECOVR -->

    <owl:NamedIndividual rdf:about="http://www.sisostds.org/ontologies/C2SIM#RECOVR">
        <rdf:type rdf:resource="http://www.sisostds.org/ontologies/C2SIM#TaskNameCode"/>
        <rdfs:comment>Documentation: 		
						To retrieve any lost, incapacitated or captured object.	
					; Appinfo DisplayValue as &quot;Recover&quot;</rdfs:comment>
    </owl:NamedIndividual>
    


    <!-- http://www.sisostds.org/ontologies/C2SIM#REFUEL -->

    <owl:NamedIndividual rdf:about="http://www.sisostds.org/ontologies/C2SIM#REFUEL">
        <rdf:type rdf:resource="http://www.sisostds.org/ontologies/C2SIM#TaskNameCode"/>
        <rdfs:comment>Documentation: 		
						To take on more fuel.	
					; Appinfo DisplayValue as &quot;Refuel&quot;</rdfs:comment>
    </owl:NamedIndividual>
    


    <!-- http://www.sisostds.org/ontologies/C2SIM#REINF -->

    <owl:NamedIndividual rdf:about="http://www.sisostds.org/ontologies/C2SIM#REINF">
        <rdf:type rdf:resource="http://www.sisostds.org/ontologies/C2SIM#TaskNameCode"/>
        <rdfs:comment>Documentation: 		
						To move or make a force available to another commander for the purpose of supplementing the in-place forces.	
					; Appinfo DisplayValue as &quot;Reinforce&quot;</rdfs:comment>
    </owl:NamedIndividual>
    


    <!-- http://www.sisostds.org/ontologies/C2SIM#RESCUE -->

    <owl:NamedIndividual rdf:about="http://www.sisostds.org/ontologies/C2SIM#RESCUE">
        <rdf:type rdf:resource="http://www.sisostds.org/ontologies/C2SIM#TaskNameCode"/>
        <rdfs:comment>Documentation: 		
						To use aircraft, surface craft (land or water), submarines, specialized rescue teams, and equipment to rescue personnel in distress on land or at sea.	
					; Appinfo DisplayValue as &quot;Rescue&quot;</rdfs:comment>
    </owl:NamedIndividual>
    


    <!-- http://www.sisostds.org/ontologies/C2SIM#RESUPL -->

    <owl:NamedIndividual rdf:about="http://www.sisostds.org/ontologies/C2SIM#RESUPL">
        <rdf:type rdf:resource="http://www.sisostds.org/ontologies/C2SIM#TaskNameCode"/>
        <rdfs:comment>Documentation: 		
						To replenish stocks in order to maintain the required levels of supply.	
					; Appinfo DisplayValue as &quot;Resupply&quot;</rdfs:comment>
    </owl:NamedIndividual>
    


    <!-- http://www.sisostds.org/ontologies/C2SIM#RETAIN -->

    <owl:NamedIndividual rdf:about="http://www.sisostds.org/ontologies/C2SIM#RETAIN">
        <rdf:type rdf:resource="http://www.sisostds.org/ontologies/C2SIM#TaskNameCode"/>
        <rdfs:comment>Documentation: 		
						To occupy and hold a terrain feature to ensure it is free of enemy occupation or use.	
					; Appinfo DisplayValue as &quot;Retain&quot;</rdfs:comment>
    </owl:NamedIndividual>
    


    <!-- http://www.sisostds.org/ontologies/C2SIM#RLFPLC -->

    <owl:NamedIndividual rdf:about="http://www.sisostds.org/ontologies/C2SIM#RLFPLC">
        <rdf:type rdf:resource="http://www.sisostds.org/ontologies/C2SIM#TaskNameCode"/>
        <rdfs:comment>Documentation: 		
						To conduct an operation in which, by direction of higher authority, all or part of a unit is replaced in an area by the incoming unit. The responsibilities of the replaced elements for the mission and the assigned zone of operations are transferred to the incoming unit. The incoming unit continues the operation as ordered.	
					; Appinfo DisplayValue as &quot;Relief in place&quot;</rdfs:comment>
    </owl:NamedIndividual>
    


    <!-- http://www.sisostds.org/ontologies/C2SIM#RUNNING -->

    <owl:NamedIndividual rdf:about="http://www.sisostds.org/ontologies/C2SIM#RUNNING">
        <rdf:type rdf:resource="http://www.sisostds.org/ontologies/C2SIM#SystemStateCode"/>
    </owl:NamedIndividual>
    


    <!-- http://www.sisostds.org/ontologies/C2SIM#Refuse -->

    <owl:NamedIndividual rdf:about="http://www.sisostds.org/ontologies/C2SIM#Refuse">
        <rdf:type rdf:resource="http://www.sisostds.org/ontologies/C2SIM#CommunicativeActTypeCode"/>
    </owl:NamedIndividual>
    


    <!-- http://www.sisostds.org/ontologies/C2SIM#ReportPosition -->

    <owl:NamedIndividual rdf:about="http://www.sisostds.org/ontologies/C2SIM#ReportPosition">
        <rdf:type rdf:resource="http://www.sisostds.org/ontologies/C2SIM#TaskNameCode"/>
    </owl:NamedIndividual>
    <owl:Axiom>
        <owl:annotatedSource rdf:resource="http://www.sisostds.org/ontologies/C2SIM#ReportPosition"/>
        <owl:annotatedProperty rdf:resource="http://www.w3.org/1999/02/22-rdf-syntax-ns#type"/>
        <owl:annotatedTarget rdf:resource="http://www.sisostds.org/ontologies/C2SIM#TaskNameCode"/>
        <rdfs:comment>Requests the receiving entity to reply with a position report.</rdfs:comment>
    </owl:Axiom>
    


    <!-- http://www.sisostds.org/ontologies/C2SIM#Request -->

    <owl:NamedIndividual rdf:about="http://www.sisostds.org/ontologies/C2SIM#Request">
        <rdf:type rdf:resource="http://www.sisostds.org/ontologies/C2SIM#CommunicativeActTypeCode"/>
    </owl:NamedIndividual>
    


    <!-- http://www.sisostds.org/ontologies/C2SIM#SCREEN -->

    <owl:NamedIndividual rdf:about="http://www.sisostds.org/ontologies/C2SIM#SCREEN">
        <rdf:type rdf:resource="http://www.sisostds.org/ontologies/C2SIM#TaskNameCode"/>
        <rdfs:comment>Documentation: 		
						To operate as a security element whose primary task is to observe, identify and report information, and which only fights in self-protection.	
					; Appinfo DisplayValue as &quot;Screen&quot;</rdfs:comment>
    </owl:NamedIndividual>
    


    <!-- http://www.sisostds.org/ontologies/C2SIM#SDAM -->

    <owl:NamedIndividual rdf:about="http://www.sisostds.org/ontologies/C2SIM#SDAM">
        <rdf:type rdf:resource="http://www.sisostds.org/ontologies/C2SIM#DesiredEffectCode"/>
        <rdfs:comment>Documentation: 		
						The subjective categorisation of the physical effect of an ACTION on buildings, infrastructure and/or equipment by a reporting ORGANISATION.	
					; Appinfo DisplayValue as &quot;Severe damage&quot;</rdfs:comment>
    </owl:NamedIndividual>
    


    <!-- http://www.sisostds.org/ontologies/C2SIM#SECURE -->

    <owl:NamedIndividual rdf:about="http://www.sisostds.org/ontologies/C2SIM#SECURE">
        <rdf:type rdf:resource="http://www.sisostds.org/ontologies/C2SIM#TaskNameCode"/>
        <rdfs:comment>Documentation: 		
						To gain possession of a position or terrain feature, with or without force, and to make such disposition as will prevent, as far as possible, its destruction or loss by enemy action.	
					; Appinfo DisplayValue as &quot;Secure&quot;</rdfs:comment>
    </owl:NamedIndividual>
    


    <!-- http://www.sisostds.org/ontologies/C2SIM#SEIZE -->

    <owl:NamedIndividual rdf:about="http://www.sisostds.org/ontologies/C2SIM#SEIZE">
        <rdf:type rdf:resource="http://www.sisostds.org/ontologies/C2SIM#TaskNameCode"/>
        <rdfs:comment>Documentation: 		
						To clear a designated area and obtain control of it.	
					; Appinfo DisplayValue as &quot;Seize&quot;</rdfs:comment>
    </owl:NamedIndividual>
    


    <!-- http://www.sisostds.org/ontologies/C2SIM#SUPPRS -->

    <owl:NamedIndividual rdf:about="http://www.sisostds.org/ontologies/C2SIM#SUPPRS">
        <rdf:type rdf:resource="http://www.sisostds.org/ontologies/C2SIM#TaskNameCode"/>
        <rdfs:comment>Documentation: 		
						To provide fire which neutralizes or temporarily degrades the capabilities of enemy forces within a specific area. This makes no assumptions as to enemy casualties; it may be a transitory effect.	
					; Appinfo DisplayValue as &quot;Suppress&quot;</rdfs:comment>
    </owl:NamedIndividual>
    


    <!-- http://www.sisostds.org/ontologies/C2SIM#SUPPRT -->

    <owl:NamedIndividual rdf:about="http://www.sisostds.org/ontologies/C2SIM#SUPPRT">
        <rdf:type rdf:resource="http://www.sisostds.org/ontologies/C2SIM#TaskNameCode"/>
        <rdfs:comment>Documentation: 		
						To aid, protect, complement or sustain any other object.	
					; Appinfo DisplayValue as &quot;Support&quot;</rdfs:comment>
    </owl:NamedIndividual>
    


    <!-- http://www.sisostds.org/ontologies/C2SIM#SUPRSD -->

    <owl:NamedIndividual rdf:about="http://www.sisostds.org/ontologies/C2SIM#SUPRSD">
        <rdf:type rdf:resource="http://www.sisostds.org/ontologies/C2SIM#DesiredEffectCode"/>
        <rdfs:comment>Documentation: 		
						Reduction of the effectiveness of the ACTION objective for a specific period or purpose (normally to prevent an enemy from interfering with friendly ACTIONs); this effect may be entirely transitory and cause no casualties.	
					; Appinfo DisplayValue as &quot;Suppressed&quot;</rdfs:comment>
    </owl:NamedIndividual>
    


    <!-- http://www.sisostds.org/ontologies/C2SIM#Secret -->

    <owl:NamedIndividual rdf:about="http://www.sisostds.org/ontologies/C2SIM#Secret">
        <rdf:type rdf:resource="http://www.sisostds.org/ontologies/C2SIM#SecurityClassificationCode"/>
    </owl:NamedIndividual>
    


    <!-- http://www.sisostds.org/ontologies/C2SIM#ShareScenario -->

    <owl:NamedIndividual rdf:about="http://www.sisostds.org/ontologies/C2SIM#ShareScenario">
        <rdf:type rdf:resource="http://www.sisostds.org/ontologies/C2SIM#SystemCommandTypeCode"/>
        <rdfs:comment>When thiscommand is received by the marshalling system, in other words the system to whom ObjectInitialization messages were sent, the marshalling system should emit a C2SIM Initialization message.</rdfs:comment>
    </owl:NamedIndividual>
    


    <!-- http://www.sisostds.org/ontologies/C2SIM#StartScenario -->

    <owl:NamedIndividual rdf:about="http://www.sisostds.org/ontologies/C2SIM#StartScenario">
        <rdf:type rdf:resource="http://www.sisostds.org/ontologies/C2SIM#SystemCommandTypeCode"/>
        <rdfs:comment>This command indicates that the scenario has started.</rdfs:comment>
    </owl:NamedIndividual>
    


    <!-- http://www.sisostds.org/ontologies/C2SIM#SubmitInitialization -->

    <owl:NamedIndividual rdf:about="http://www.sisostds.org/ontologies/C2SIM#SubmitInitialization">
        <rdf:type rdf:resource="http://www.sisostds.org/ontologies/C2SIM#SystemCommandTypeCode"/>
        <rdfs:comment>This command indicates that the receiving system should submit its scenario initialization data (and ObjectInitialzation message) to the system indicated in the ReplyTo field of the header.</rdfs:comment>
    </owl:NamedIndividual>
    


    <!-- http://www.sisostds.org/ontologies/C2SIM#THREAT -->

    <owl:NamedIndividual rdf:about="http://www.sisostds.org/ontologies/C2SIM#THREAT">
        <rdf:type rdf:resource="http://www.sisostds.org/ontologies/C2SIM#TaskNameCode"/>
        <rdfs:comment>Documentation: 		
						To menace the enemy by manoeuvre or action.	
					; Appinfo DisplayValue as &quot;Threaten&quot;</rdfs:comment>
    </owl:NamedIndividual>
    


    <!-- http://www.sisostds.org/ontologies/C2SIM#TURN -->

    <owl:NamedIndividual rdf:about="http://www.sisostds.org/ontologies/C2SIM#TURN">
        <rdf:type rdf:resource="http://www.sisostds.org/ontologies/C2SIM#TaskNameCode"/>
        <rdfs:comment>Documentation: 		
						To compel an enemy force to move from an avenue of approach or movement corridor to another.	
					; Appinfo DisplayValue as &quot;Turn&quot;</rdfs:comment>
    </owl:NamedIndividual>
    


    <!-- http://www.sisostds.org/ontologies/C2SIM#TaskEnd -->

    <owl:NamedIndividual rdf:about="http://www.sisostds.org/ontologies/C2SIM#TaskEnd">
        <rdf:type rdf:resource="http://www.sisostds.org/ontologies/C2SIM#EventCode"/>
    </owl:NamedIndividual>
    


    <!-- http://www.sisostds.org/ontologies/C2SIM#TaskStart -->

    <owl:NamedIndividual rdf:about="http://www.sisostds.org/ontologies/C2SIM#TaskStart">
        <rdf:type rdf:resource="http://www.sisostds.org/ontologies/C2SIM#EventCode"/>
    </owl:NamedIndividual>
    


    <!-- http://www.sisostds.org/ontologies/C2SIM#TopSecret -->

    <owl:NamedIndividual rdf:about="http://www.sisostds.org/ontologies/C2SIM#TopSecret">
        <rdf:type rdf:resource="http://www.sisostds.org/ontologies/C2SIM#SecurityClassificationCode"/>
    </owl:NamedIndividual>
    


    <!-- http://www.sisostds.org/ontologies/C2SIM#UNINITIALIZED -->

    <owl:NamedIndividual rdf:about="http://www.sisostds.org/ontologies/C2SIM#UNINITIALIZED">
        <rdf:type rdf:resource="http://www.sisostds.org/ontologies/C2SIM#SystemStateCode"/>
    </owl:NamedIndividual>
    


    <!-- http://www.sisostds.org/ontologies/C2SIM#Unclassified -->

    <owl:NamedIndividual rdf:about="http://www.sisostds.org/ontologies/C2SIM#Unclassified">
        <rdf:type rdf:resource="http://www.sisostds.org/ontologies/C2SIM#SecurityClassificationCode"/>
    </owl:NamedIndividual>
    


    <!-- http://www.sisostds.org/ontologies/C2SIM#UseCapability -->

    <owl:NamedIndividual rdf:about="http://www.sisostds.org/ontologies/C2SIM#UseCapability">
        <rdf:type rdf:resource="http://www.sisostds.org/ontologies/C2SIM#TaskNameCode"/>
    </owl:NamedIndividual>
    <owl:Axiom>
        <owl:annotatedSource rdf:resource="http://www.sisostds.org/ontologies/C2SIM#UseCapability"/>
        <owl:annotatedProperty rdf:resource="http://www.w3.org/1999/02/22-rdf-syntax-ns#type"/>
        <owl:annotatedTarget rdf:resource="http://www.sisostds.org/ontologies/C2SIM#TaskNameCode"/>
        <rdfs:comment>Use the main or default capability that the actor posseses.</rdfs:comment>
    </owl:Axiom>
    


    <!-- http://www.sisostds.org/ontologies/C2SIM#WNDD -->

    <owl:NamedIndividual rdf:about="http://www.sisostds.org/ontologies/C2SIM#WNDD">
        <rdf:type rdf:resource="http://www.sisostds.org/ontologies/C2SIM#DesiredEffectCode"/>
        <rdfs:comment>Documentation: 		
						A casualty other than &quot;killed&quot; who has incurred an injury due to an external agent or cause.	
					; Appinfo DisplayValue as &quot;Wounded&quot;</rdfs:comment>
    </owl:NamedIndividual>
    


    <!-- http://www.sisostds.org/ontologies/C2SIM_SMX_LOX#Fire -->

    <owl:NamedIndividual rdf:about="http://www.sisostds.org/ontologies/C2SIM_SMX_LOX#Fire">
        <rdf:type rdf:resource="http://www.sisostds.org/ontologies/C2SIM#TaskNameCode"/>
    </owl:NamedIndividual>
    


    <!-- http://www.sisostds.org/ontologies/MGCS#HLDDEF -->

    <owl:NamedIndividual rdf:about="http://www.sisostds.org/ontologies/MGCS#HLDDEF">
        <rdf:type rdf:resource="http://www.sisostds.org/ontologies/C2SIM#TaskNameCode"/>
    </owl:NamedIndividual>
    


    <!-- http://www.sisostds.org/ontologies/MGCS#March -->

    <owl:NamedIndividual rdf:about="http://www.sisostds.org/ontologies/MGCS#March">
        <rdf:type rdf:resource="http://www.sisostds.org/ontologies/C2SIM#TaskNameCode"/>
    </owl:NamedIndividual>
    


    <!-- http://www.sisostds.org/ontologies/lox#AllTasksComplete -->

    <owl:NamedIndividual rdf:about="http://www.sisostds.org/ontologies/lox#AllTasksComplete">
        <rdf:type rdf:resource="http://www.sisostds.org/ontologies/lox#PlanPhaseCompletionCondition"/>
    </owl:NamedIndividual>
    


    <!-- http://www.sisostds.org/ontologies/lox#OneTaskComplete -->

    <owl:NamedIndividual rdf:about="http://www.sisostds.org/ontologies/lox#OneTaskComplete">
        <rdf:type rdf:resource="http://www.sisostds.org/ontologies/lox#PlanPhaseCompletionCondition"/>
    </owl:NamedIndividual>
    


    <!-- http://www.sisostds.org/ontologies/lox#OtherOrderReceived -->

    <owl:NamedIndividual rdf:about="http://www.sisostds.org/ontologies/lox#OtherOrderReceived">
        <rdf:type rdf:resource="http://www.sisostds.org/ontologies/lox#PlanPhaseCompletionCondition"/>
    </owl:NamedIndividual>
    


    <!-- http://www.sisostds.org/ontologies/lox#genericManeuverWarfareDesiredEffectCode -->

    <owl:NamedIndividual rdf:about="http://www.sisostds.org/ontologies/lox#genericManeuverWarfareDesiredEffectCode"/>
    


    <!-- http://www.sisostds.org/ontologies/smx#ARMY -->

    <owl:NamedIndividual rdf:about="http://www.sisostds.org/ontologies/smx#ARMY">
        <rdf:type rdf:resource="http://www.sisostds.org/ontologies/smx#EchelonCode"/>
    </owl:NamedIndividual>
    


    <!-- http://www.sisostds.org/ontologies/smx#ARMYGROUP -->

    <owl:NamedIndividual rdf:about="http://www.sisostds.org/ontologies/smx#ARMYGROUP">
        <rdf:type rdf:resource="http://www.sisostds.org/ontologies/smx#EchelonCode"/>
    </owl:NamedIndividual>
    


    <!-- http://www.sisostds.org/ontologies/smx#BATTALION -->

    <owl:NamedIndividual rdf:about="http://www.sisostds.org/ontologies/smx#BATTALION">
        <rdf:type rdf:resource="http://www.sisostds.org/ontologies/smx#EchelonCode"/>
    </owl:NamedIndividual>
    


    <!-- http://www.sisostds.org/ontologies/smx#BATTERY -->

    <owl:NamedIndividual rdf:about="http://www.sisostds.org/ontologies/smx#BATTERY">
        <rdf:type rdf:resource="http://www.sisostds.org/ontologies/smx#EchelonCode"/>
    </owl:NamedIndividual>
    


    <!-- http://www.sisostds.org/ontologies/smx#BRIGADE -->

    <owl:NamedIndividual rdf:about="http://www.sisostds.org/ontologies/smx#BRIGADE">
        <rdf:type rdf:resource="http://www.sisostds.org/ontologies/smx#EchelonCode"/>
    </owl:NamedIndividual>
    


    <!-- http://www.sisostds.org/ontologies/smx#COMPANY -->

    <owl:NamedIndividual rdf:about="http://www.sisostds.org/ontologies/smx#COMPANY">
        <rdf:type rdf:resource="http://www.sisostds.org/ontologies/smx#EchelonCode"/>
    </owl:NamedIndividual>
    


    <!-- http://www.sisostds.org/ontologies/smx#CORPS -->

    <owl:NamedIndividual rdf:about="http://www.sisostds.org/ontologies/smx#CORPS">
        <rdf:type rdf:resource="http://www.sisostds.org/ontologies/smx#EchelonCode"/>
    </owl:NamedIndividual>
    


    <!-- http://www.sisostds.org/ontologies/smx#CREW -->

    <owl:NamedIndividual rdf:about="http://www.sisostds.org/ontologies/smx#CREW">
        <rdf:type rdf:resource="http://www.sisostds.org/ontologies/smx#EchelonCode"/>
    </owl:NamedIndividual>
    


    <!-- http://www.sisostds.org/ontologies/smx#D -->

    <owl:NamedIndividual rdf:about="http://www.sisostds.org/ontologies/smx#D">
        <rdf:type rdf:resource="http://www.sisostds.org/ontologies/smx#ReinforcedReducedType"/>
    </owl:NamedIndividual>
    


    <!-- http://www.sisostds.org/ontologies/smx#DETACHMENT -->

    <owl:NamedIndividual rdf:about="http://www.sisostds.org/ontologies/smx#DETACHMENT">
        <rdf:type rdf:resource="http://www.sisostds.org/ontologies/smx#EchelonCode"/>
    </owl:NamedIndividual>
    


    <!-- http://www.sisostds.org/ontologies/smx#DIVISION -->

    <owl:NamedIndividual rdf:about="http://www.sisostds.org/ontologies/smx#DIVISION">
        <rdf:type rdf:resource="http://www.sisostds.org/ontologies/smx#EchelonCode"/>
    </owl:NamedIndividual>
    


    <!-- http://www.sisostds.org/ontologies/smx#DomainAir -->

    <owl:NamedIndividual rdf:about="http://www.sisostds.org/ontologies/smx#DomainAir">
        <rdf:type rdf:resource="http://www.sisostds.org/ontologies/smx#DISDomainCode"/>
    </owl:NamedIndividual>
    


    <!-- http://www.sisostds.org/ontologies/smx#DomainLand -->

    <owl:NamedIndividual rdf:about="http://www.sisostds.org/ontologies/smx#DomainLand">
        <rdf:type rdf:resource="http://www.sisostds.org/ontologies/smx#DISDomainCode"/>
    </owl:NamedIndividual>
    


    <!-- http://www.sisostds.org/ontologies/smx#DomainOther -->

    <owl:NamedIndividual rdf:about="http://www.sisostds.org/ontologies/smx#DomainOther">
        <rdf:type rdf:resource="http://www.sisostds.org/ontologies/smx#DISDomainCode"/>
    </owl:NamedIndividual>
    


    <!-- http://www.sisostds.org/ontologies/smx#DomainSpace -->

    <owl:NamedIndividual rdf:about="http://www.sisostds.org/ontologies/smx#DomainSpace">
        <rdf:type rdf:resource="http://www.sisostds.org/ontologies/smx#DISDomainCode"/>
    </owl:NamedIndividual>
    


    <!-- http://www.sisostds.org/ontologies/smx#DomainSubsurface -->

    <owl:NamedIndividual rdf:about="http://www.sisostds.org/ontologies/smx#DomainSubsurface">
        <rdf:type rdf:resource="http://www.sisostds.org/ontologies/smx#DISDomainCode"/>
    </owl:NamedIndividual>
    


    <!-- http://www.sisostds.org/ontologies/smx#DomainSurface -->

    <owl:NamedIndividual rdf:about="http://www.sisostds.org/ontologies/smx#DomainSurface">
        <rdf:type rdf:resource="http://www.sisostds.org/ontologies/smx#DISDomainCode"/>
    </owl:NamedIndividual>
    


    <!-- http://www.sisostds.org/ontologies/smx#FR -->

    <owl:NamedIndividual rdf:about="http://www.sisostds.org/ontologies/smx#FR">
        <rdf:type rdf:resource="http://www.sisostds.org/ontologies/smx#SideHostilityCode"/>
        <rdfs:comment>Friendly</rdfs:comment>
    </owl:NamedIndividual>
    


    <!-- http://www.sisostds.org/ontologies/smx#FRONT -->

    <owl:NamedIndividual rdf:about="http://www.sisostds.org/ontologies/smx#FRONT">
        <rdf:type rdf:resource="http://www.sisostds.org/ontologies/smx#EchelonCode"/>
    </owl:NamedIndividual>
    


    <!-- http://www.sisostds.org/ontologies/smx#GROUP -->

    <owl:NamedIndividual rdf:about="http://www.sisostds.org/ontologies/smx#GROUP">
        <rdf:type rdf:resource="http://www.sisostds.org/ontologies/smx#EchelonCode"/>
    </owl:NamedIndividual>
    


    <!-- http://www.sisostds.org/ontologies/smx#GenericInstance -->

    <owl:NamedIndividual rdf:about="http://www.sisostds.org/ontologies/smx#GenericInstance">
        <rdf:type rdf:resource="http://www.sisostds.org/ontologies/smx#AircraftTypeCategoryCode"/>
        <rdf:type rdf:resource="http://www.sisostds.org/ontologies/smx#PersonTypeCategoryCode"/>
        <rdf:type rdf:resource="http://www.sisostds.org/ontologies/smx#VehicleTypeCategoryCode"/>
    </owl:NamedIndividual>
    


    <!-- http://www.sisostds.org/ontologies/smx#HO -->

    <owl:NamedIndividual rdf:about="http://www.sisostds.org/ontologies/smx#HO">
        <rdf:type rdf:resource="http://www.sisostds.org/ontologies/smx#SideHostilityCode"/>
        <rdfs:comment>Hostile</rdfs:comment>
    </owl:NamedIndividual>
    


    <!-- http://www.sisostds.org/ontologies/smx#KindCulturalFeature -->

    <owl:NamedIndividual rdf:about="http://www.sisostds.org/ontologies/smx#KindCulturalFeature">
        <rdf:type rdf:resource="http://www.sisostds.org/ontologies/smx#DISKindCode"/>
    </owl:NamedIndividual>
    


    <!-- http://www.sisostds.org/ontologies/smx#KindEnvironmental -->

    <owl:NamedIndividual rdf:about="http://www.sisostds.org/ontologies/smx#KindEnvironmental">
        <rdf:type rdf:resource="http://www.sisostds.org/ontologies/smx#DISKindCode"/>
    </owl:NamedIndividual>
    


    <!-- http://www.sisostds.org/ontologies/smx#KindExpendable -->

    <owl:NamedIndividual rdf:about="http://www.sisostds.org/ontologies/smx#KindExpendable">
        <rdf:type rdf:resource="http://www.sisostds.org/ontologies/smx#DISKindCode"/>
    </owl:NamedIndividual>
    


    <!-- http://www.sisostds.org/ontologies/smx#KindLifeForm -->

    <owl:NamedIndividual rdf:about="http://www.sisostds.org/ontologies/smx#KindLifeForm">
        <rdf:type rdf:resource="http://www.sisostds.org/ontologies/smx#DISKindCode"/>
    </owl:NamedIndividual>
    


    <!-- http://www.sisostds.org/ontologies/smx#KindMunition -->

    <owl:NamedIndividual rdf:about="http://www.sisostds.org/ontologies/smx#KindMunition">
        <rdf:type rdf:resource="http://www.sisostds.org/ontologies/smx#DISKindCode"/>
    </owl:NamedIndividual>
    


    <!-- http://www.sisostds.org/ontologies/smx#KindOther -->

    <owl:NamedIndividual rdf:about="http://www.sisostds.org/ontologies/smx#KindOther">
        <rdf:type rdf:resource="http://www.sisostds.org/ontologies/smx#DISKindCode"/>
    </owl:NamedIndividual>
    


    <!-- http://www.sisostds.org/ontologies/smx#KindPlatform -->

    <owl:NamedIndividual rdf:about="http://www.sisostds.org/ontologies/smx#KindPlatform">
        <rdf:type rdf:resource="http://www.sisostds.org/ontologies/smx#DISKindCode"/>
    </owl:NamedIndividual>
    


    <!-- http://www.sisostds.org/ontologies/smx#KindRadio -->

    <owl:NamedIndividual rdf:about="http://www.sisostds.org/ontologies/smx#KindRadio">
        <rdf:type rdf:resource="http://www.sisostds.org/ontologies/smx#DISKindCode"/>
    </owl:NamedIndividual>
    


    <!-- http://www.sisostds.org/ontologies/smx#KindSensorEmitter -->

    <owl:NamedIndividual rdf:about="http://www.sisostds.org/ontologies/smx#KindSensorEmitter">
        <rdf:type rdf:resource="http://www.sisostds.org/ontologies/smx#DISKindCode"/>
    </owl:NamedIndividual>
    


    <!-- http://www.sisostds.org/ontologies/smx#KindSupply -->

    <owl:NamedIndividual rdf:about="http://www.sisostds.org/ontologies/smx#KindSupply">
        <rdf:type rdf:resource="http://www.sisostds.org/ontologies/smx#DISKindCode"/>
    </owl:NamedIndividual>
    


    <!-- http://www.sisostds.org/ontologies/smx#MOPS -->

    <owl:NamedIndividual rdf:about="http://www.sisostds.org/ontologies/smx#MOPS">
        <rdf:type rdf:resource="http://www.sisostds.org/ontologies/smx#UnitOperationalStatusCode"/>
    </owl:NamedIndividual>
    


    <!-- http://www.sisostds.org/ontologies/smx#NEUTRL -->

    <owl:NamedIndividual rdf:about="http://www.sisostds.org/ontologies/smx#NEUTRL">
        <rdf:type rdf:resource="http://www.sisostds.org/ontologies/smx#SideHostilityCode"/>
        <rdfs:comment>Neutral</rdfs:comment>
    </owl:NamedIndividual>
    


    <!-- http://www.sisostds.org/ontologies/smx#NONE -->

    <owl:NamedIndividual rdf:about="http://www.sisostds.org/ontologies/smx#NONE">
        <rdf:type rdf:resource="http://www.sisostds.org/ontologies/smx#EchelonCode"/>
    </owl:NamedIndividual>
    


    <!-- http://www.sisostds.org/ontologies/smx#NOP -->

    <owl:NamedIndividual rdf:about="http://www.sisostds.org/ontologies/smx#NOP">
        <rdf:type rdf:resource="http://www.sisostds.org/ontologies/smx#UnitOperationalStatusCode"/>
    </owl:NamedIndividual>
    


    <!-- http://www.sisostds.org/ontologies/smx#OPR -->

    <owl:NamedIndividual rdf:about="http://www.sisostds.org/ontologies/smx#OPR">
        <rdf:type rdf:resource="http://www.sisostds.org/ontologies/smx#UnitOperationalStatusCode"/>
    </owl:NamedIndividual>
    


    <!-- http://www.sisostds.org/ontologies/smx#PLATOON -->

    <owl:NamedIndividual rdf:about="http://www.sisostds.org/ontologies/smx#PLATOON">
        <rdf:type rdf:resource="http://www.sisostds.org/ontologies/smx#EchelonCode"/>
    </owl:NamedIndividual>
    


    <!-- http://www.sisostds.org/ontologies/smx#R -->

    <owl:NamedIndividual rdf:about="http://www.sisostds.org/ontologies/smx#R">
        <rdf:type rdf:resource="http://www.sisostds.org/ontologies/smx#ReinforcedReducedType"/>
    </owl:NamedIndividual>
    


    <!-- http://www.sisostds.org/ontologies/smx#RD -->

    <owl:NamedIndividual rdf:about="http://www.sisostds.org/ontologies/smx#RD">
        <rdf:type rdf:resource="http://www.sisostds.org/ontologies/smx#ReinforcedReducedType"/>
    </owl:NamedIndividual>
    


    <!-- http://www.sisostds.org/ontologies/smx#REGIMENT -->

    <owl:NamedIndividual rdf:about="http://www.sisostds.org/ontologies/smx#REGIMENT">
        <rdf:type rdf:resource="http://www.sisostds.org/ontologies/smx#EchelonCode"/>
    </owl:NamedIndividual>
    


    <!-- http://www.sisostds.org/ontologies/smx#REGION -->

    <owl:NamedIndividual rdf:about="http://www.sisostds.org/ontologies/smx#REGION">
        <rdf:type rdf:resource="http://www.sisostds.org/ontologies/smx#EchelonCode"/>
    </owl:NamedIndividual>
    


    <!-- http://www.sisostds.org/ontologies/smx#SECTION -->

    <owl:NamedIndividual rdf:about="http://www.sisostds.org/ontologies/smx#SECTION">
        <rdf:type rdf:resource="http://www.sisostds.org/ontologies/smx#EchelonCode"/>
    </owl:NamedIndividual>
    


    <!-- http://www.sisostds.org/ontologies/smx#SOPS -->

    <owl:NamedIndividual rdf:about="http://www.sisostds.org/ontologies/smx#SOPS">
        <rdf:type rdf:resource="http://www.sisostds.org/ontologies/smx#UnitOperationalStatusCode"/>
    </owl:NamedIndividual>
    


    <!-- http://www.sisostds.org/ontologies/smx#SQUAD -->

    <owl:NamedIndividual rdf:about="http://www.sisostds.org/ontologies/smx#SQUAD">
        <rdf:type rdf:resource="http://www.sisostds.org/ontologies/smx#EchelonCode"/>
    </owl:NamedIndividual>
    


    <!-- http://www.sisostds.org/ontologies/smx#SQUADRON -->

    <owl:NamedIndividual rdf:about="http://www.sisostds.org/ontologies/smx#SQUADRON">
        <rdf:type rdf:resource="http://www.sisostds.org/ontologies/smx#EchelonCode"/>
    </owl:NamedIndividual>
    


    <!-- http://www.sisostds.org/ontologies/smx#TEAM -->

    <owl:NamedIndividual rdf:about="http://www.sisostds.org/ontologies/smx#TEAM">
        <rdf:type rdf:resource="http://www.sisostds.org/ontologies/smx#EchelonCode"/>
    </owl:NamedIndividual>
    


    <!-- http://www.sisostds.org/ontologies/smx#TNOPS -->

    <owl:NamedIndividual rdf:about="http://www.sisostds.org/ontologies/smx#TNOPS">
        <rdf:type rdf:resource="http://www.sisostds.org/ontologies/smx#UnitOperationalStatusCode"/>
    </owl:NamedIndividual>
    


    <!-- http://www.sisostds.org/ontologies/smx#TROOP -->

    <owl:NamedIndividual rdf:about="http://www.sisostds.org/ontologies/smx#TROOP">
        <rdf:type rdf:resource="http://www.sisostds.org/ontologies/smx#EchelonCode"/>
    </owl:NamedIndividual>
    


    <!-- http://www.sisostds.org/ontologies/smx#WING -->

    <owl:NamedIndividual rdf:about="http://www.sisostds.org/ontologies/smx#WING">
        <rdf:type rdf:resource="http://www.sisostds.org/ontologies/smx#EchelonCode"/>
    </owl:NamedIndividual>
    <rdf:Description>
        <owl:minQualifiedCardinality rdf:datatype="http://www.w3.org/2001/XMLSchema#nonNegativeInteger">0</owl:minQualifiedCardinality>
    </rdf:Description>
    <rdf:Description>
        <owl:qualifiedCardinality rdf:datatype="http://www.w3.org/2001/XMLSchema#nonNegativeInteger">1</owl:qualifiedCardinality>
    </rdf:Description>
    <rdf:Description>
        <owl:qualifiedCardinality rdf:datatype="http://www.w3.org/2001/XMLSchema#nonNegativeInteger">1</owl:qualifiedCardinality>
    </rdf:Description>
    <rdf:Description>
        <owl:qualifiedCardinality rdf:datatype="http://www.w3.org/2001/XMLSchema#nonNegativeInteger">1</owl:qualifiedCardinality>
    </rdf:Description>
    <rdf:Description>
        <owl:qualifiedCardinality rdf:datatype="http://www.w3.org/2001/XMLSchema#nonNegativeInteger">1</owl:qualifiedCardinality>
    </rdf:Description>
    <rdf:Description>
        <owl:qualifiedCardinality rdf:datatype="http://www.w3.org/2001/XMLSchema#nonNegativeInteger">1</owl:qualifiedCardinality>
    </rdf:Description>
    <rdf:Description>
        <owl:qualifiedCardinality rdf:datatype="http://www.w3.org/2001/XMLSchema#nonNegativeInteger">1</owl:qualifiedCardinality>
    </rdf:Description>
    <rdf:Description>
        <owl:qualifiedCardinality rdf:datatype="http://www.w3.org/2001/XMLSchema#nonNegativeInteger">1</owl:qualifiedCardinality>
    </rdf:Description>
    <rdf:Description>
        <owl:qualifiedCardinality rdf:datatype="http://www.w3.org/2001/XMLSchema#nonNegativeInteger">1</owl:qualifiedCardinality>
    </rdf:Description>
    <rdf:Description>
        <owl:qualifiedCardinality rdf:datatype="http://www.w3.org/2001/XMLSchema#nonNegativeInteger">1</owl:qualifiedCardinality>
    </rdf:Description>
    <rdf:Description>
        <owl:qualifiedCardinality rdf:datatype="http://www.w3.org/2001/XMLSchema#nonNegativeInteger">1</owl:qualifiedCardinality>
    </rdf:Description>
    <rdf:Description>
        <owl:qualifiedCardinality rdf:datatype="http://www.w3.org/2001/XMLSchema#nonNegativeInteger">1</owl:qualifiedCardinality>
    </rdf:Description>
    <rdf:Description>
        <owl:qualifiedCardinality rdf:datatype="http://www.w3.org/2001/XMLSchema#nonNegativeInteger">1</owl:qualifiedCardinality>
    </rdf:Description>
    


    <!-- 
    ///////////////////////////////////////////////////////////////////////////////////////
    //
    // General axioms
    //
    ///////////////////////////////////////////////////////////////////////////////////////
     -->

    <rdf:Description>
        <rdf:type rdf:resource="http://www.w3.org/2002/07/owl#AllDisjointClasses"/>
        <owl:members rdf:parseType="Collection">
            <rdf:Description rdf:about="http://www.sisostds.org/ontologies/C2SIM#BoundingBox"/>
            <rdf:Description rdf:about="http://www.sisostds.org/ontologies/C2SIM#BoundingVolume"/>
            <rdf:Description rdf:about="http://www.sisostds.org/ontologies/C2SIM#ExtentVertices"/>
            <rdf:Description rdf:about="http://www.sisostds.org/ontologies/C2SIM#Handles"/>
        </owl:members>
    </rdf:Description>
    <rdf:Description>
        <rdf:type rdf:resource="http://www.w3.org/2002/07/owl#AllDisjointClasses"/>
        <owl:members rdf:parseType="Collection">
            <rdf:Description rdf:about="http://www.sisostds.org/ontologies/C2SIM#DateTime"/>
            <rdf:Description rdf:about="http://www.sisostds.org/ontologies/C2SIM#Duration"/>
            <rdf:Description rdf:about="http://www.sisostds.org/ontologies/C2SIM#IntervalTime"/>
        </owl:members>
    </rdf:Description>
    <rdf:Description>
        <rdf:type rdf:resource="http://www.w3.org/2002/07/owl#AllDisjointClasses"/>
        <owl:members rdf:parseType="Collection">
            <rdf:Description rdf:about="http://www.sisostds.org/ontologies/C2SIM#DateTime"/>
            <rdf:Description rdf:about="http://www.sisostds.org/ontologies/C2SIM#RelativeTime"/>
            <rdf:Description rdf:about="http://www.sisostds.org/ontologies/C2SIM#SimulationTime"/>
        </owl:members>
    </rdf:Description>
</rdf:RDF>



<!-- Generated by the OWL API (version 4.5.7.2018-12-02T02:23:35Z) https://github.com/owlcs/owlapi -->

